<subsection xmlns:xi="http://www.w3.org/2001/XInclude"><title> 1st-Order Equations </title>
	
	<p>
		In the previous section, we learned that solutions to Linear Homogeneous Constant Coefficient (LHCC) equations often involve terms of the form <m>e^{rx}</m>. However, not every value of <m>r</m> will work. The correct values of <m>r</m> arise from solving an important algebraic equation, obtained by substituting <m>y = e^{rx}</m> into the differential equation. In this section, we will focus on this process for first-order equations before building up to higher-order cases.
	</p>
	
	<p>
		Let's start with a simple first-order equation:
		<me> y' - 5y = 0 </me>
		We want to find the value of <m>r</m> such that <m>y = e^{rx}</m> is a solution. Substituting <m>y = e^{rx}</m> into the differential equation gives:
		<md>
			<mrow> \left[e^{rx}\right]' - 5 \left[e^{rx}\right] =\amp 0 </mrow>
			<mrow> r e^{rx} - 5 e^{rx} 							=\amp 0 </mrow>
			<mrow> (r - 5) e^{rx} 								=\amp 0 </mrow>
		</md>
		Since <m>e^{rx}</m> is never zero, we must have:
		<md>
			<mrow> r - 5 = 0 \quad \Rightarrow \quad r = 5 </mrow>
		</md>
		This tells us that <m>y = e^{5x}</m> is a solution. Therefore, the general solution is:
		<me> y = C e^{5x} </me>
	</p>
	
	<p>
		The equation <m>r - 5 = 0</m>, which gave us the value of <m>r</m>, is called the <term>characteristic equation</term>. Every LHCC equation has one. The characteristic equation gives us the values of <m>r</m> that we need to construct the general solution.
	</p>
	
	<p>
		Applying the same approach to the general first-order LHCC equation gives us:
		<md>
			<mrow> 
				y=e^{rx} \quad\rightarrow\quad
				ay' + by = 0 \quad\Rightarrow\quad a \left[e^{rx}\right]' + b \left[e^{rx}\right] 
											=\amp 0 
			</mrow>
			<mrow> a r e^{rx} + b e^{rx}	=\amp 0 </mrow>
			<mrow> (ar + b) e^{rx} 			=\amp 0 </mrow>
		</md>
		This results in the characteristic equation and general solution:
		<me> ar + b = 0 \quad \Rightarrow \quad r = -\frac{b}{a} \quad \Rightarrow \quad y = C e^{-\frac{b}{a}x} </me>
	</p>
	
	<p>
		Now, let's apply this method to a couple of examples.
	</p>
	
	<example>
		<p>
			Find the general solution for each LHCC equation.
			<me> 3y' - 9y = 0 \hspace{5em} 5y' = \pi y </me>
		</p>
	
		<solution><title> Solution </title>
			<p>
				First, rewrite the equations in standard form:
				<me> y' - 3y = 0 \hspace{5em} 5y' - \pi y = 0 </me>
			</p>
			
			<p>
				Now solve the characteristic equations:
				<me> 3r - 9 = 0 \quad \Rightarrow \quad r = 3 \hspace{5em} 5r - \pi = 0 \quad \Rightarrow \quad r = \frac{\pi}{5} </me>
				Thus, the general solutions are:
				<me> y = C e^{3x} \hspace{5em} y = C e^{\frac{\pi}{5}x} </me>
			</p>
		</solution>
	</example>
	
	<p>
		This straightforward method works for any first-order LHCC equation by using the characteristic equation. In the next sections, we'll extend this technique to higher-order equations.
	</p>

	<xi:include href="./p3-c1-s3-interactives.ptx" />

</subsection>