<section><title> SOV - Orphaned Content </title>

	<introduction>
		<p>
			This is just a place to put content that was written and may or not be used.
		</p>
	</introduction>

	<paragraphs><title> Additional Examples </title>
		
		<example>

			<p>
				Determine if the following DE is separable.
				<me> \frac{dz}{dt} = \cos^2 z </me>
			</p>
	
			<solution>
	
				<p>
					This differential equation is first order. Since the derivative is already isolated, we need to determine if we can express the right-hand side as a product of functions where one function does not contain the dependent variable <m>z</m>, and the other does not contain the independent variable <m>t</m>. Consider the equivalent equation:
					<me> \frac{dz}{dt} = \big( 1 \big) \cdot \big( \cos^2 z \big) </me>
					It may seem trivial, but this satisfies the definition of separable. The first factor is a function that does not contain <m>z</m>, and the second factor is a function that does not contain <m>t</m>. The first factor is a constant function, which is perfectly acceptable. Therefore, this differential equation <em>is separable</em>.
				</p>
	
			</solution>
	
		</example>

		<example><title> Verify our solution </title>

			<p>
				Verify that 
				<me>z = \tan(t+C)</me>
				is the particular solution to the initial value problem
				<me>z' - 1 = z^2, \quad z(4) = 9</me>
			</p>

			<solution>
				<p>
					As in the previous example, we don't have to check our answer, but one of the best parts about DEs is that we always can check, which means we can really know if we have the right solution. Let's check this one. We will substitute our solution back into the DE and verify that when we do, we get the same thing on both sides of the equation.
		
					<md>
						<mrow> LHS	=\amp\ z' -1</mrow>
						<mrow> =\amp\ \frac{d}{dt}\Big( \tan(t+C) \Big) - 1</mrow>
						<mrow> =\amp\ \sec^2(t+C)\cdot \frac{d}{dt}(t+C) - 1</mrow>
						<mrow> =\amp\ \sec^2(t+C)\cdot (1+0) - 1</mrow>
						<mrow> =\amp\ \sec^2(t+C) - 1</mrow>
					</md>
		
					<md>
						<mrow> RHS	=\amp\ z^2</mrow>
						<mrow> =\amp\ \Big( \tan(t+C) \Big)^2</mrow>
						<mrow> =\amp\ \tan^2(t+C)</mrow>
					</md>
		
				</p>
		
				<p>
					At first glance, it looks like we have different expressions on the left and right hand sides of the equation. However, if we recall the trigonometric identity
		
						<me>\tan^2 x = \sec^2 x - 1,</me>
		
					then we can see that these expressions are, in fact equivalent. Thus, we have verified that <m>z = \tan(t+C)</m>, where <m>C</m> is any constant, is a solution to the DE <m>z' -1 = z^2</m>.
				</p>
		
				<p>
					Now that we've practiced this solution technique a couple of times, let's summarize.
				</p>
			</solution>
	
		</example>

		<example>

			<p>
				Solve the following initial value problem.
				<me>\frac{dz}{dy} - yz = y, \hspace{1cm} z(0) = 5</me>
			</p>
	
			<solution>
	
				<p>
					It's always worth it when you first start solving DEs to step back and make sure you identify independent and dependent variables. Here <m>z</m> is dependent and <m>y</m> is independent. That means when we're done we hope to have a function
					<me>
					z = \underbrace{\hspace{4.0cm}}_{\text{some function of } y}
					</me>
				</p>
	
				<p>
					Also, even though the terminology we use is <em>initial</em> condition, we typically won't use that piece of information until the very end.
	
					<aside>
						<p>
							* Until we get to Laplace Transforms...
						</p>
					</aside>
				</p>
	
				<p>
					First let's verify that the DE is first order (it is!), and then we go about solving for the derivative.
					<md>
						<mrow> \frac{dz}{dy} - yz	=\amp\ y</mrow>
						<mrow> \frac{dz}{dy} 	=\amp\ y + yz</mrow>
					</md>
				</p>
	
				<p>
					Now that we have solved for the derivative, is it possible write the right hand side of the equation as a product of functions where one of the functions does not contain the dependent variable, <m>z</m> and the other function does not contain the independent variable, <m>y</m>?  That is, we'd like to write the DE in the form suggested below.
					<me>
						\frac{dz}{dy} = \Big( \underbrace{\hspace{2.0cm}}_{\mbox{no z's}} \Big) \cdot
						\Big( \underbrace{\hspace{2.0cm}}_{\mbox{no x's}} \Big)
					</me>
					Hopefully you can see that there is a way, by factoring <m>y</m> out of each term on the right hand side, as below.
					<me>\frac{dz}{dy} = y(1 + z)</me>
				</p>
	
				<p>
					Now we need to completely separate variables.
					<me>\frac{1}{1+z}dz = ydy</me>
				</p>
	
				<p>
					The next step will be to integrate both sides of the equation. (If the integral on the right hand side is at all questionable to you, you should do take an extra step and actually do the substitution <m>u = 1+z.</m>)
					<md>
						<mrow> \int \frac{1}{1+z}dz	=\amp\ \int ydy</mrow>
						<mrow> \ln|1+z|	=\amp\ \frac{1}{2}y^2 + c</mrow>
					</md>
				</p>
	
				<p>
					As before, we write only one constant of integration (recall that we're skipping a couple of steps here; details provided in Example 6).
				</p>
	
				<p>
					Remember that our goal is to solve for the unknown function <m>z</m>. Since it's currently inside of a logarithm, we exponentiate both sides of the equation.
					<md>
						<mrow> \ln|1+z|	=\amp\ \frac{1}{2}y^2 + c</mrow>
						<mrow> e^{\ln|1+z|}	=\amp\ e^{\frac{1}{2}y^2 + c}</mrow>
						<mrow> |1+z|	=\amp\ e^{\frac{1}{2}y^2}\cdot e^c</mrow>
					</md>
				</p>
	
				<p>
					We continue solving for <m>z</m>.
					<md>
						<mrow> 1+z	=\amp\ \underbrace{\pm e^c}_{\text{rename } A} \cdot e^{\frac{1}{2}y^2}</mrow>
						<mrow> 1+z	=\amp\ Ae^{\frac{1}{2}y^2}		</mrow>
						<mrow> z	=\amp\ Ae^{\frac{1}{2}y^2} - 1	</mrow>
					</md>
				</p>
	
				<p>
					Now we can use that initial condition, <m>z(0) = 5</m>, to solve for <m>A</m>. The initial condition can be read,
					"when <m>y</m> is zero, <m>z</m> is 5."  We substitute into our solution accordingly.
					<md>
						<mrow> z	=\amp\ Ae^{\frac{1}{2}y^2} - 1</mrow>
						<mrow> 5	=\amp\ Ae^{\frac{1}{2}\cdot 0^2} - 1</mrow>
						<mrow> 5	=\amp\ Ae^0 - 1</mrow>
						<mrow> 6	=\amp\ A\cdot 1</mrow>
						<mrow> 6	=\amp\ A</mrow>
					</md>
					<aside>
						<p>
							* mention that we can't call <m>A = 6</m> our solution!
						</p>
					</aside>
				</p>
	
				<p>
					Therefore, the solution to the IVP is
					<me>z = 6e^{\frac{1}{2}y^2} - 1.</me>
				</p>
	
			</solution>
	
		</example>

	</paragraphs>
	
	<reading-questions><title> Additional Practice </title>
	
		<exercise label="p2-c1-s2-e1"><title> <em>Multiple-Choice</em> </title>
			<statement>
				<em>What is the method used to solve the differential equation <me>\frac{d}{dx}[g(x,y)] = f(x)</me>?</em>
			</statement>
			<choices>
				<choice correct="yes">
					<statement>Direct integration.</statement>
					<feedback>Correct! The equation is solved by integrating both sides with respect to <m>x</m>.</feedback>
				</choice>
				<choice>
					<statement>Separation of variables.</statement>
					<feedback>Incorrect. Separation of variables is used when the variables can be separated, but here the equation is solved by direct integration.</feedback>
				</choice>
				<choice>
					<statement>Substitution.</statement>
					<feedback>Incorrect. Substitution is a different method. The correct method here is direct integration.</feedback>
				</choice>
				<choice>
					<statement>Partial fractions.</statement>
					<feedback>Incorrect. Partial fractions are used to simplify the integration process, but the primary method here is direct integration.</feedback>
				</choice>
			</choices>
		</exercise>

		<exercise label="sov-question-5"><title> <em>The general solution to a differential equation represents a family of solutions, while a <var width="10"/> solution is a specific solution obtained by assigning particular values to the constants</em> </title>
			<statement>
				<em>The general solution to a differential equation represents a family of solutions, while a <var width="10"/> solution is a specific solution obtained by assigning particular values to the constants.</em>
			</statement>
			<setup>
				<var case="insensitive">
					<condition string="particular"> 
						<feedback> <p>Good job! The correct term is "particular."</p> </feedback> 
					</condition>
					<condition string=".*"> 
						<feedback> <p>Incorrect. The correct answer starts with a "p".</p> </feedback>
					</condition>
				</var>
			</setup>
		</exercise>
		
		<exercise label="sov-question-1"><title> <em>Is the equation <m>\ds\frac{dy}{dx} = \frac{\cos x}{y}</m> separable?</em> </title>
			<statement>
				<p><em>Is the equation <m>\frac{dy}{dx} = \frac{\cos x}{y}</m> separable?</em></p>
			</statement>
			<choices>
				<choice correct="yes">
					<statement><p>Yes</p></statement>
					<feedback>Correct! This equation can be separated into <m>y\ dy = \cos(x)\ dx</m>.</feedback>
				</choice>
				<choice>
					<statement><p>No</p></statement>
					<feedback>Incorrect. The equation is separable because we can write it as <m>y\ dy = \cos(x)\ dx</m>.</feedback>
				</choice>
			</choices>
		</exercise>
		
		<exercise><title> <em>True/False</em> </title>
			<statement correct="yes">
			<p>
				The differential equation, <m>\displaystyle \frac{dy}{dx} = y^2</m>, is <xref ref="separable" text="custom">separable</xref>.
			</p>
			</statement>
			<feedback>
			<p>
				Even though no <m>x</m> terms are present, we still can group the terms like so: 
				<me>
				\frac{dy}{dx} = y^2 = (1)(y^2) = \underset{f(x)}{\left(\boxed{1}\right)}\underset{g(y)}{\left(\boxed{y^2}\right)}.
				</me>
			</p>
			</feedback>
		</exercise>
			
		<exercise><title> <em>True/False</em> </title>
			<statement correct="yes">
			<p>
				The differential equation, <m>\displaystyle \frac{dy}{dx} = x - 1</m>, is <xref ref="separable" text="custom">separable</xref>.
			</p>
			</statement>
			<feedback>
			<p>
				As in the previous problem, we can group the terms like so: 
				<me>
				\frac{dy}{dx} = x - 1 = (x - 1)(1) = \underset{f(x)}{\left(\boxed{x - 1}\right)}\underset{g(y)}{\left(\boxed{1}\right)}.
				</me>
			</p>
			</feedback>
		</exercise>
	
		<exercise><title> <em>True/False</em> </title>
			<statement correct="yes">
			<p>
				The differential equation, <m>\displaystyle \frac{dy}{dx} = 15</m>, is <xref ref="separable" text="custom">separable</xref>.
			</p>
			</statement>
			<feedback>
			<p>
				Despite not having any <m>x</m> nor <m>y</m> terms, it is still technically separable since 
				<me>
				\frac{dy}{dx} = 15 = (15)(1) = \underset{f(x)}{\left(\boxed{15}\right)}\underset{g(y)}{\left(\boxed{1}\right)}.
				</me>
			</p>
			</feedback>
		</exercise>

		<exercise><title> <em>True/False</em> </title>
			<statement correct="no">
				<p>
					The differential equation <m>x+\frac{dy}{dx}=y</m> can be solved using separation.
				</p>
			</statement>
			<feedback>
				<p>
					The differential equation is first order and can be written as <m>\frac{dy}{dx}=y-x</m>, which is not separable.
				</p>
			</feedback>
			<hint>
				<p>
					Check to see that the differential equation is first order and separable.
				</p>
			</hint>
		</exercise>

		<exercise><title> <em>True/False</em> </title>
			<statement correct="no">
				<p>
					The differential equation <m>\frac{dz^2}{d^2t}=\cos^2(z)</m> can be solved using separation.
				</p>
			</statement>
			<feedback>
				<p>
					The differential equation is separable, but not first order.
				</p>
			</feedback>
			<hint>
				<p>
					Check to see that the differential equation is first order and separable.
				</p>
			</hint>
		</exercise>

		<exercise><title> <em>Multiple Choice</em> </title>
			<statement>Write the differential equation <m>x\frac{dy}{dx}+10x^2y=6x^2</m> in separable form.</statement>
			<choices>
				<choice>
					<statement><m>\frac{dy}{dx}=6x-10xy</m></statement>
				<feedback>
					<p>
						This is not written in separable form.
					</p>
				</feedback>
				</choice>
				<choice correct="yes">
					<statement><m>\frac{dy}{dx}=x(6-10y)</m></statement>
				<feedback>
					<p>
						This is written in separable form.
					</p>
				</feedback>
				</choice>
				<choice>
					<statement><m>\frac{dy}{dx}=x(6+10y)</m></statement>
				<feedback>
					<p>
						This is written in separable form, but is not equivalent to the original differential equation.
					</p>
				</feedback>
				</choice>
			</choices>
			<hint>
				<p>
					Try writing <m>\frac{dy}{dx}</m> as the product of the independent and dependent variables.
				</p>
			</hint>
		</exercise>

		<exercise label="p2-c2-s3-rq3"><title> <em>Which of the following is the correct sequence of steps in the separation of variables method?</em> </title>
			<statement>
				<p><em>Which of the following is the correct sequence of steps in the separation of variables method?</em></p>
			</statement>
			<choices>
				<choice>
					<statement>Integrate, Separate, Isolate and Combine Constants</statement>
					<feedback>Incorrect. Integration comes after separating the variables, not before.</feedback>
				</choice>
				<choice>
					<statement>Isolate, Integrate, Separate, and Combine Constants</statement>
					<feedback>Incorrect. Isolation is typically the final step, not the first.</feedback>
				</choice>
				<choice>
					<statement>Separate, Differentiate, Isolate and Combine Constants</statement>
					<feedback>Incorrect. Differentiation is not part of the separation of variables method; integration is the key step.</feedback>
				</choice>
				<choice correct="yes">
					<statement>Separate, Integrate, Isolate and Combine Constants</statement>
					<feedback>Correct! The correct sequence is to first separate the variables, then integrate, and finally isolate the dependent variable and combine constants.</feedback>
				</choice>
			</choices>
		</exercise>

		<exercise label="p2-c2-s3-rq5"><title> <em>When solving a separable differential equation, why is it important to combine constants?</em> </title>
			<statement>
				<p><em>When solving a separable differential equation, why is it important to combine constants?</em></p>
			</statement>
			<choices>
			   <choice>
					<statement>To ensure the solution is exact and matches initial conditions.</statement>
					<feedback>Incorrect. While combining constants simplifies the solution, it doesn't directly relate to matching initial conditions.</feedback>
				</choice>
				<choice>
					<statement>To eliminate any arbitrary constants from the solution.</statement>
					<feedback>Incorrect. Combining constants doesn't eliminate them but rather simplifies them into one term.</feedback>
				</choice>
				<choice correct="yes">
					<statement>To simplify the solution by reducing multiple constants into a single constant.</statement>
					<feedback>Correct! Combining constants simplifies the final solution and avoids unnecessary complexity.</feedback>
				</choice>
				<choice>
					<statement>To convert the solution into a standard form for easier interpretation.</statement>
					<feedback>Incorrect. While combining constants can lead to a simpler form, the main purpose is to avoid having multiple constants when one will suffice.</feedback>
				</choice>
			</choices>
		</exercise>
		
		<exercise label="sov-method-steps-parson2" adaptive="yes"><title>Separation of Variables Method Steps</title>
		
			<statement>List the steps of the separation of variables method by dragging task on the left to the step on the right?</statement>
			<blocks>
				<block>
					<line>Check that the DE</line>
					<line>is first order.</line>
				</block>
				<block>
					<line>Write the DE in</line>
					<line>separable form.</line>
				</block>
				<block>
					<m>\frac{1}{g(y)} dy = f(x) dx</m>
				</block>
				<block>
					<line>Integrate both sides</line>
					<line>of the equation.</line>   
				</block>
				<block>
					<line>Solve for <m>y</m></line>
					<line>(if possible).</line>   
				</block>
			</blocks>
		</exercise>

		<exercise label="sov-method-steps-matching" randomize="true" adaptive="yes"><title>Separation of Variables Method Steps</title>
			
			<statement>List the steps of the separation of variables method by dragging each task on the left to the corresponding step on the right?</statement>

			<feedback>
			<p>
				Review
			</p>
			</feedback>

			<matches>
				<match>
					<premise>Check that the DE is first order</premise>
					<response>Step 1</response>
				</match>
				<match>
					<premise>
						Write DE in separable form, if possible: <me>\frac{dy}{dx} = f(x) \cdot g(y)</me>
					</premise>
					<response>Step 2</response>
				</match>
				<match>
					<premise>
						Separate <m>x</m> &amp; <m>y</m>: <me>\frac{1}{g(y)} dy = f(x) dx</me>
					</premise>
					<response>Step 3</response>
				</match>
				<match>
					<premise>Integrate both sides of the DE</premise>
					<response>Step 4</response>
				</match>
				<match>
					<premise>Solve for <m>y</m>, if possible</premise>
					<response>Step 5</response>
				</match>
			</matches>
		</exercise>
		
		<exercise><title> <em>Solve the Differential Equation</em> </title>

			<introduction>
				<p>
					Complete each step below to solve the differential equation
					<me> y'= e^{2x} - 5x. </me>
				</p>
			</introduction>
				
			<webwork xml:id="ww_5"> 

				<pg-code>
					Context()->variables->add(y => 'Real');
					$ans2a =Formula("e^{2 x} - 4 x");
					$ans2b = 1;
					$ans3a = 1;
					$ans3b = Formula("e^{2 x} - 4 x");
					$ans4a = Formula("y");
					$ans4b = FormulaUpToConstant("1/2 e^(2x) - 2 x^2");
					$ans = FormulaUpToConstant("1/2 e^{2x} - 2 x^2");
				</pg-code>

				<statement>
					<ol marker="1.">
						<li>
							Verify that the DE has first order. 
						</li>

						<li>
							<p>
								Write the DE into the separable form, <m> y'= f(x) \cdot g(y).</m>
							</p>
							<p>
								<m>f(x) =</m> <var name="$ans2a" width="15" /> , 
								<m>g(y) =</m> <var name="$ans2b" width="15" />
							</p>
						</li>

						<li>
							<p>
								Use algebra to move the <m>y</m> terms to the left
								<me> \frac{1}{g(y)} \cdot y'= f(x).</me>
								<var name="$ans3a" width="15" /> <m> \cdot y' = </m> <var name="$ans3b" width="15" />
							</p>
						</li>

						<li>
							<p>
								Integrate both sides with respect to <m>x</m>. Don't forget the integration constant, <m>+C</m>. 
								<me> y'= e^{2 x} - 4 x.</me>
								<var name="$ans4a" width="25" /> <m> = </m> <var name="$ans4b" width="25" />
							</p>
						</li>

						<li>
							<p>
								After working out the integrals on each side of the equation, you will be left with <m>y</m>'s on the left and <m>x</m>'s on the right. Finish the problem by using algebra to solve for <m>y</m>.
							</p>
							<p>
								<m>y(x) = </m> <var name="$ans" width="25" />
							</p>
						</li>
						
					</ol>

				</statement>

			</webwork>

		</exercise>

		<exercise><title> <em>Solve the Differential Equation</em> </title>
			<introduction>
				<p>
					Use algebra to show the differential equation is separable. Give the <m>x</m> terms in the left blank and the <m>y</m> terms in the right blank.
					<me> \frac{dy}{dx} - y\cos(x) = y.</me>
				</p>
			</introduction>
				
			<webwork xml:id="ww_6_2"> 
				<description>
					Solve a separable DE using separation of variables.
				</description>

				<pg-code>
					Context()->variables->add(y => 'Real');
					Context()->variables->add(t => 'Real');
					Context()->variables->add(C => 'Real');
					$a = random(2,8,1);
					$ans1 = 1;
					$ans2a = Formula("t^{$a}");
					$ans2b = Formula("1-y");
					$ans3a = Formula("1/(1-y)");
					$ans3b = Formula("t^{$a}");
					$ans4a = Formula("-ln(1-y)");
					$ans4b = FormulaUpToConstant("1/($a + 1)* t^{$a + 1}");
					$ans = Formula("1 - C*exp(-t^{$a+1}/($a + 1)) "); 
				</pg-code>

				<statement>
					<ol marker="1.">
						<li>
							Verify that the DE has first order. 
							<me> \frac{dy}{dt}= t^{<var name="$a" /> }-yt^{<var name="$a" /> } .</me>
							Order <m>=</m> <var name="$ans1"  width="15" />
						</li>

						<li>
							<p>
								Attempt to re-write the DE into the separable form
								<me> y'= f(t) \cdot g(y).</me>
								<m>f(t) =</m> <var name="$ans2a" width="15" /> , 
								<m>g(y) =</m> <var name="$ans2b" width="15" />
							</p>
						</li>

						<li>
							<p>
								Use algebra to move the <m>y</m> terms to the left
								<me> \frac{1}{g(y)} \cdot y'= f(t).</me>
								<var name="$ans3a" width="15" /> <m> \cdot y' = </m> <var name="$ans3b" width="15" />
							</p>
						</li>

						<li>
							<p>
								Integrate both sides with respect to <m>t</m>. Hint: Don't forget the +C after doing the indefinite integral. 
								<var name="$ans4a" width="25" /> <m> = </m> <var name="$ans4b" width="25" />
							</p>
						</li>

						<li>
							<p>
								After working out the integrals on each side of the equation, you will be left with <m>y</m>'s on the left and <m>t</m>'s on the right. Finish the problem by using algebra to solve for <m>y</m>.
							</p>
							<p>
								<m>y(t) = </m> <var name="$ans" width="25" />
							</p>
						</li>
						
					</ol>

				</statement>

			</webwork>
		</exercise>

		<exercise><title> <em>Solve the Differential Equation</em> </title>
			<introduction>
				<p>
				Find the general solution of the differential equation
					<me> y'= e^{<var name="$a" /> x}- <var name="$b" /> x.</me>
				</p>
			</introduction>
				
			<webwork xml:id="ww_7_2">
				<description>
					Solve a separable DE using separation of variables.
				</description>

				<pg-code>
					$a = random(4,9,1);
					$b = random(2,9,1);
					$ans = FormulaUpToConstant("1/$a e^{$a x}- $b/2 x^2");
				</pg-code>

				<statement><m>y(x) =</m> <var name="$ans" width="25" /></statement>

				<solution>
					<m></m>.
				</solution>
			</webwork>
		</exercise>

		<!-- <figure>
			<caption>Drag-and-Drop Task Ordering</caption>
			<interactive xml:id="interactive-drag-drop" iframe="http://127.0.0.1:8128/output/custom_html/task_ordering.html" width="95%" aspect="15:10" />
			<instructions>
				<p>
					Drag the tasks from the left column to the correct order on the right column. 
					Once all tasks are placed in the correct order, you will receive feedback.
				</p>
			</instructions>
		</figure> -->
		
	</reading-questions>
	
	<paragraphs><title> Additional Narrative </title>

		
	</paragraphs>

	<paragraphs><title>Methods Summary</title>
		
		<outcomes>
			<dl width="narrow">
				<li xml:id="di-summary"><title> Direct Integration </title>
					<p>
						Solving a differential equation by integrating both sides of the equation.
					</p>
				</li>
				<li xml:id="sov-summary"><title> Separation of Variables </title>
					<p>
						Solving a differential equation by separating the variables on opposite sides of the equation followed by direct integration.
					</p>
				</li>
				<li xml:id="if-summary"><title> Integrating Factor </title>
					<p>
						Solving a differential equation by multiplying both sides by a factor followed by direct integration.
					</p>
				</li>
				<li xml:id="lhcc-summary"><title> Characteristic Equation </title>
					<p>
						Solving a differential equation by finding the roots of the characteristic equation.
					</p>
				</li>
				<li xml:id="lhm-summary"><title> Undetermined Coefficients </title>
					<p>
						Solving a differential equation by assuming a form of the solution and then solving for the unknown parts of this form.
					</p>
				</li>
				<li xml:id="lt-summary"><title> Laplace Transforms </title>
					<p>
						Solving a differential equation by transforming it into an algebraic equation, solving it, then converting the result back into the solution of our differential equation.
					</p>
				</li>
			</dl>
		</outcomes>

	</paragraphs>
	
</section>