<subsection xmlns:xi="http://www.w3.org/2001/XInclude"><title> Linear Homogeneous Constant Coefficients </title>

	<paragraphs xml:id="nth-derivative-of-exp"><title> N-th Derivative of <m>e^{rx}</m> </title>

		Each derivative of <m>e^{rx}</m> adds a multiple of <m>r</m>, so
		<me>
			\us{\ \text{ rule}}{\text{chain}} \rightarrow \ \ \left[e^{rx}\right]' = r e^{rx}, \quad \left[e^{rx}\right]'' = r^2 e^{rx}, \quad \ldots, \quad \left[e^{rx}\right]^{(n)} = r^n e^{rx}
		</me>.
	</paragraphs>


	<paragraphs xml:id="second-order-lhcc-complex-case"><title> 2nd Order LHCC Complex Case 3 </title>

		<p>
			The following explains how <xref ref="lhcc-case-3" text="title"/> comes directly from <xref ref="lhcc-case-1" text="title"/>.
		</p>

		<p>
			Since <m>r_1</m> and <m>r_2</m> are complex, they can be written as
			<me>
				r_1 = \alpha + \beta i \quad \text{and} \quad r_2 = \alpha - \beta i
			</me>.
			Substituting these into <xref ref="second-order-lhcc-solution-r1-notequalto-r2"/>, using <xref ref="eulers-formula" text="title"/>, the <xref ref="evenodd-cos" text="custom"> even property of cosine </xref> and <xref ref="evenodd-sin" text="custom"> odd property of sine </xref>, we can rewrite the general solution as
			<md>
				<mrow> y\  &amp;= C_1 e^{(\alpha + \beta i) x} + C_2 e^{(\alpha - \beta i) x} </mrow>
				<mrow> &amp;= C_1 e^{\alpha x} e^{i \beta x} + C_2 e^{\alpha x} e^{-i \beta x} </mrow>
				<mrow> &amp;= e^{\alpha x} \Big{[}C_1 e^{i \beta x} + C_2 e^{-i \beta x}\Big{]} </mrow>
				<mrow> &amp;= e^{\alpha x} \Big{[}C_1 (\cos(\beta x) + i\sin(\beta x)) + C_2 (\cos(-\beta x) + i\sin(-\beta x))\Big{]} </mrow>
				<mrow> &amp;= e^{\alpha x} \Big{[}C_1 \cos(\beta x) + i C_1 \sin(\beta x) + C_2 \cos(-\beta x) + i C_2 \sin(-\beta x)\Big{]} </mrow>
				<mrow> &amp;= e^{\alpha x} \Big{[}C_1 \cos(\beta x) + i C_1 \sin(\beta x) + C_2 \cos(\beta x) - i C_2 \sin(\beta x)\Big{]} </mrow>
				<mrow> &amp;= e^{\alpha x} \Big{[}(\us{C_1}{\ub{C_1 + C_2}}) \cos(\beta x) + \us{C_2}{\ub{i (C_1 - C_2)}} \sin(\beta x)\Big{]} </mrow>
				<mrow> &amp;= e^{\alpha x} (C_1 \cos(\beta x) + C_2 \sin(\beta x)) </mrow>
			</md>.
		</p>
	</paragraphs>

	<paragraphs xml:id="like-terms"><title> like-terms </title>

		<p>
			Terms are called <term>like-terms</term> if they have identical variable parts. That is, they differ only by a coefficient. like-terms can be combined via addition and subtraction. For example, the <m>x^2</m> and <m>e^{-3x}</m> terms below are pairs of like-terms, which can be combined as follows:
			<md>
				<mrow> \underline{3x^2} + \underline{\underline{5e^{-3x}}} - 2 + \underline{7x^2} - \underline{\underline{4e^{-3x}}}</mrow>
				<mrow> \underline{10x^2} + \underline{\underline{e^{-3x}}} - 2 </mrow>
			</md>.
		</p>

	</paragraphs>

	<paragraphs xml:id="poly-factor-p"><title> Polynomial Factoring Calculator </title>
		<figure xml:id="figure-pp">
			<caption>Type in any polynomial of <m>r</m>. Use <q><m>*</m></q> for multiplication. If the polynomial has rational roots, it will show the factors.</caption>
			<interactive xml:id="poly-factor" platform="sage" width="86%" aspect="3.2:1">
				<slate surface="sage">
					r = var('r')
					r = PolynomialRing(RationalField(), 'r').gen()
					F = 'r^2 - 2*r - 8'
					P = r^2 - 2*r - 8
					@interact
					def _(ce = input_box(P, label="	Polynomial:", type=str, width=30)):
						ce_poly = sage_eval('lambda r: ' + ce)
						pretty_print( html( r'Polynomial: $ %s $'%latex(ce_poly(r) ) ) )
						pretty_print( html( r'Factored Polynomial: $ %s $'%latex(ce_poly(r).factor()) ) )
				</slate>
			</interactive>
		</figure>
	</paragraphs>

	<paragraphs xml:id="characteristic-eqn-details"><title/>
		<p>
			To find the characteristic equation, we substitute <m>y = e^{rx}</m> into the <m>n</m>-th order <xref ref="lhcc-equation" text="custom">LHCC equation</xref> and solve for <m>r</m>. Doing this gives us
			<md>
				<mrow>	
					a_n\ \left[e^{rx}\right]^{(n)} + \cdots + a_2\ \left[e^{rx}\right]'' + a_1\ \left[e^{rx}\right]' + a_0\ e^{rx} =\amp\ 0
				</mrow>
				<mrow>	a_n\ r^n e^{rx} + \cdots + a_2\ r^2 e^{rx} + a_1\ r e^{rx} + a_0\ e^{rx} =\amp\ 0 </mrow>
				<mrow>	\left(a_n\ r^n + \cdots + a_2\ r^2 + a_1\ r + a_0\right)e^{rx}  =\amp\ 0 </mrow>
			</md>.
			Since <m>e^{rx}</m> is never zero, we must have
			<me>
				a_n\ r^n + \cdots + a_2\ r^2 + a_1\ r + a_0 = 0
			</me>
			which is an <m>n</m>-th order polynomial in <m>r</m>.
		</p>
	</paragraphs>

</subsection>