<section><title> Orphaned Content </title>

	<introduction>
		<p>
			This is just a place to put content that was written and may or not be used.
		</p>
	</introduction>

	<paragraphs><title> Additional Narrative </title>
		
		<theorem><title> N-th Derivative of <m>e^{rx}</m> </title>
			<statement>
				<p>
					Each derivative of <m>e^{rx}</m> adds a multiple of <m>r</m>, so
					<me>
						\us{\ \text{ rule}}{\text{chain}} \rightarrow \ \ \left[e^{rx}\right]' = r e^{rx}, \quad \left[e^{rx}\right]'' = r^2 e^{rx}, \quad \ldots, \quad \left[e^{rx}\right]^{(n)} = r^n e^{rx}
					</me>.
				</p>
			</statement>
		</theorem>

				<table xml:id="multiplying-yp-forms-table">
			<title> Common Forms for Products in <m>y_p</m> </title>
			<tabular top="medium" left="medium" right="medium" bottom="minor">
			<col halign="center" right="medium"/>
			<col halign="center"/>
			<row bottom="medium">
				<cell><term>Forcing Function, </term><m>f(x)</m></cell>
				<cell><term>Particular Solution Form, </term><m>y_p</m></cell>
			</row>
			<row>
				<cell><m>(ax^2+bx+c)e^{\alpha x}</m></cell>
				<cell><m>(Ax^2+Bx+C)e^{\alpha x}</m></cell>
			</row>
			<row>
				<cell><m>(ax^2+bx+c)\cos(\beta x)</m></cell>
				<cell><m>(Ax^2+Bx+C)\cos(\beta x)</m></cell>
			</row>
			<row>
				<cell><m>(ax^2+bx+c)\sin(\beta x)</m></cell>
				<cell><m>+ (Dx^2+Ex+F)\sin(\beta x)</m></cell>
			</row>
			<row>
				<cell>
				<line><m>e^{\alpha x}\cos(\beta x)</m></line>
				<line><m>e^{\alpha x}\sin(\beta x)</m></line>
				</cell>
				<cell><m>e^{\alpha x}(A\cos(\beta x) + B\sin(\beta x))</m></cell>
			</row>
			<row>
				<cell><m>(ax^2+bx+c)e^{\alpha x}\cos(\beta x)</m></cell>
				<cell><m>(Ax^2+Bx+C)e^{\alpha x}\cos(\beta x)</m></cell>
			</row>
			<row bottom="medium">
				<cell><m>(ax^2+bx+c)e^{\alpha x}\sin(\beta x)</m></cell>
				<cell><m>+ (Dx^2+Ex+F)e^{\alpha x}\sin(\beta x)</m></cell>
			</row>
			</tabular>
		</table>

		<tabular>
			<row>
				<cell colspan="2"><m>\ds a_n\ r^ne^{rx} + \cdots + a_2\ r^2e^{rx} + a_1\ re^{rx} + a_0\ e^{rx} = 0 </m></cell>
				<cell/>
			</row>
			<row>
				<cell colspan="2"><m>\ds (a_n\ r^n + \cdots + a_2\ r^2 + a_1\ r + a_0)\ e^{rx} = 0</m></cell>
				<cell><em>(factor out <m>e^{rx}</m>)</em></cell>
			</row>
			<row halign="center">
				<cell><m>\ds a_n\ r^n + \cdots + a_2\ r^2 + a_1\ r + a_0 = 0,</m></cell>
				<cell><m>\ds e^{rx} = 0</m></cell>
				<cell><em>(set each factor to 0)</em></cell>
			</row>
			<row halign="center">
				<cell><m>\uparrow</m></cell>
				<cell><m>\uparrow</m></cell>
				<cell/>
			</row>
			<row halign="center">
				<cell><em>characteristic equation!</em></cell>
				<cell><em>no solution</em></cell>
				<cell/>
			</row>
		</tabular>

		<theorem><title> How <m>c_1 e^{(\alpha + i\beta)x} + c_2 e^{(\alpha - i\beta)x} \rightarrow e^{\alpha x}(c_1 \cos(\beta x) + c_2 \sin(\beta x))</m>? </title>
			<statement>
				<p>
					Since <m>r_1</m> and <m>r_2</m> are complex, they can be written as
					<me>
						r_1 = \alpha + \beta i \quad \text{and} \quad r_2 = \alpha - \beta i
					</me>.
					Substituting these into  even property of cosine  and  odd property of sine , we can rewrite the general solution as
					<md>
						<mrow> y\  &amp;= c_1 e^{(\alpha + \beta i) x} + c_2 e^{(\alpha - \beta i) x} </mrow>
						<mrow> &amp;= c_1 e^{\alpha x} e^{i \beta x} + c_2 e^{\alpha x} e^{-i \beta x} </mrow>
						<mrow> &amp;= e^{\alpha x} \Big{[}c_1 e^{i \beta x} + c_2 e^{-i \beta x}\Big{]} </mrow>
						<mrow> &amp;= e^{\alpha x} \Big{[}c_1 (\cos(\beta x) + i\sin(\beta x)) + c_2 (\cos(-\beta x) + i\sin(-\beta x))\Big{]} </mrow>
						<mrow> &amp;= e^{\alpha x} \Big{[}c_1 \cos(\beta x) + i c_1 \sin(\beta x) + c_2 \cos(\beta x) - i c_2 \sin(\beta x)\Big{]} </mrow>
						<mrow> &amp;= e^{\alpha x} \Big{[}(\us{c_1}{\ub{c_1 + c_2}}) \cos(\beta x) + \us{c_2}{\ub{i (c_1 - c_2)}} \sin(\beta x)\Big{]} </mrow>
						<mrow> &amp;= e^{\alpha x} (c_1 \cos(\beta x) + c_2 \sin(\beta x)) </mrow>
					</md>.
				</p>
			</statement>
		</theorem>
		
		

	</paragraphs>



</section>