<!-- LICENSING
  This file is part of the textbook "Exploring Differential Equations, An Interactive, Student-Centered Approach" by Geoffrey Cox.
  License: Creative Commons Attribution-ShareAlike 4.0 International (CC BY-SA 4.0)
  You are free to:
    ‚Ä¢ Share ‚Äî copy and redistribute the material in any medium or format.
    ‚Ä¢ Adapt ‚Äî remix, transform, and build upon the material for any purpose, even commercially.
  Under the following terms:
    ‚Ä¢ Attribution ‚Äî You must give appropriate credit, provide a link to the license, and indicate if changes were made.
    ‚Ä¢ ShareAlike ‚Äî If you remix, transform, or build upon the material, you must distribute your contributions under the same license.
  Full license text: https://creativecommons.org/licenses/by-sa/4.0/legalcode
  Recommended attribution: "Exploring Differential Equations" by Geoffrey Cox, licensed CC BY-SA 4.0"
-->
<section xml:id="solving-linear-systems">
	<title>Solving Linear Systems</title>

	<xref provisional="WORK-IN-PROGRESS"/>

	<introduction>
		<p>
			We've explored what linear systems are, how to visualize their behavior, and how to write them in compact matrix form. 
			Now it's time to actually <em>solve</em> them.
		</p>
		<p>
			We'll start with a method that mirrors how we solved single constant-coefficient equations: 
			we guess exponential solutions. This guess transforms the differential system into an algebra problem ‚Äî 
			one that will lead naturally to eigenvalues and eigenvectors.
		</p>
	</introduction>

	<paragraphs xml:id="guessing-exponentials">
		<title>Guessing Exponential Solutions</title>

		<p>
			Recall how we solved single first-order linear equations like <m>y' = ky</m> by 
			guessing solutions of the form <m>y(t) = Ce^{kt}</m>.  
			We'll try the same idea for systems.
		</p>

		<p>
			Consider the system:
		</p>

		<men xml:id="guess-exponential-system">
			\begin{array}{l}
			\dfrac{dx}{dt} = 3x + 4y\\
			\dfrac{dy}{dt} = -4x + 3y
			\end{array}
		</men>

		<p>
			Let's guess that <m>x(t)</m> and <m>y(t)</m> share the same exponential rate <m>r</m>:
		</p>

		<me>
			x(t) = Ce^{rt}, \qquad y(t) = De^{rt}.
		</me>

		<aside>
			<p>
				Clearly, if <m>C = D = 0</m>, then we would have the trivial solution, so let's assume <m>C</m> and <m>D</m> are not both zero.
			</p>
		</aside>

		<p>
			Differentiating gives:
		</p>

		<me>
			x' = Cr e^{rt}, \qquad y' = Dr e^{rt}.
		</me>

		<p>
			Substituting into the system:
		</p>

		<md alignment="alignat">
			<mrow>Cr e^{rt} \amp {}={} \amp 3Ce^{rt} \amp {}+{} \amp 4De^{rt}</mrow>
			<mrow>Dr e^{rt} \amp {}={} \amp -4Ce^{rt} \amp {}+{} \amp 3De^{rt}</mrow>
		</md>

		<p>
			Divide through by <m>e^{rt}</m> (which is never zero):
		</p>

		<md alignment="alignat">
			<mrow>Cr \amp {}={} \amp 3C \amp {}+{} \amp 4D</mrow>
			<mrow>Dr \amp {}={} \amp -4C \amp {}+{} \amp 3D</mrow>
		</md>

		<p>
			This leaves an algebraic system involving the unknowns: <m>C</m>, <m>D</m>, and <m>r</m>. It turns out that these unknowns have a very special relationship. To see this, flip the system around:
		</p>

		<md alignment="alignat">
			<mrow>3{\DLBb C} \amp {}+{} \amp 4{\DLGb D} \amp {}={} \amp r{\DLBb C}   </mrow>
			<mrow>-4{\DLBb C} \amp {}+{} \amp 3{\DLGb D} \amp {}={} \amp r{\DLGb D} </mrow>.
		</md>

		<p>
			Now, convert this into a <m>2 \times 2</m> matrix system:
		</p>

		<me>
			\begin{bmatrix}
				3 \amp 4\\
				-4 \amp 3
			\end{bmatrix}
			\begin{bmatrix}
				{\DLBb C}\\
				{\DLGb D}
			\end{bmatrix}
			= r
			\begin{bmatrix}
				{\DLBb C}\\
				{\DLGb D}
			\end{bmatrix}
		</me>

		<p>
			This is the <em>eigenvalue equation</em> <m>A \vec{v} = r \vec{v}</m> for the coefficient matrix
		</p>

		<me>
			A = \begin{bmatrix} 3 \amp 4 \\ -4 \amp 3 \end{bmatrix}.
		</me>

		
		<p>
			This tells us something powerful:  
			<ul marker="disc">
				<li>Linear systems often have solutions made of exponentials.</li>
				<li>The allowed exponential rates <m>r</m> are the <em>eigenvalues</em> of <m>A</m>.</li>
				<li>The corresponding coefficients <m>C</m> and <m>D</m> form the <em>eigenvectors</em>.</li>
			</ul>
		</p>

		<example xml:id="ex-worked-linear-system">
			<title>Solving a Simple Linear System</title>
			<statement>
				<p>
					Solve the system:
				</p>
				<md>
					<mrow>\frac{dx}{dt} \amp = x + y</mrow>
					<mrow>\frac{dy}{dt} \amp = 4x + y</mrow>
				</md>
			</statement>
			<solution>
				<p>
					Write in matrix form <m>\frac{dY}{dt} = AY</m> with 
					<m>A = \begin{bmatrix}1 \amp 1 \\ 4 \amp 1\end{bmatrix}</m>.
				</p>

				<p>
					Guess <m>Y(t) = \vec{v}e^{rt}</m>.  
					Substituting gives <m>A\vec{v} = r\vec{v}</m>.
				</p>

				<p>
					Find eigenvalues of <m>A</m> by solving <m>\det(A - rI) = 0</m>.
				</p>

				<me>
					\det \begin{bmatrix} 1-r \amp 1 \\ 4 \amp 1-r \end{bmatrix} = (1-r)^2 - 4 = r^2 - 2r - 3.
				</me>

				<p>
					Set equal to zero: <m>r^2 - 2r - 3 = 0</m>. Factor:
				</p>

				<me>
					(r - 3)(r + 1) = 0 \quad \Rightarrow \quad r_1 = 3, \ r_2 = -1.
				</me>

				<p>
					Find eigenvectors for each eigenvalue.
				</p>

				<ul>
					<li><term>For r = 3:</term> Solve <m>(A - 3I)\vec{v} = 0</m>.
						<me>
							\begin{bmatrix} -2 \amp 1 \\ 4 \amp -2 \end{bmatrix} \begin{bmatrix} v_1 \\ v_2 \end{bmatrix} = \begin{bmatrix} 0 \\ 0 \end{bmatrix}.
						</me>
						From the first row: <m>-2v_1 + v_2 = 0 \Rightarrow v_2 = 2v_1</m>.  
						Choose <m>v_1 = 1</m>, giving eigenvector <m>\vec{v}_1 = \begin{bmatrix}1 \\ 2\end{bmatrix}</m>.
					</li>

					<li><term>For r = -1:</term> Solve <m>(A + I)\vec{v} = 0</m>.
						<me>
							\begin{bmatrix} 2 \amp 1 \\ 4 \amp 2 \end{bmatrix} \begin{bmatrix} v_1 \\ v_2 \end{bmatrix} = \begin{bmatrix} 0 \\ 0 \end{bmatrix}.
						</me>
						From the first row: <m>2v_1 + v_2 = 0 \Rightarrow v_2 = -2v_1</m>.  
						Choose <m>v_1 = 1</m>, giving eigenvector <m>\vec{v}_2 = \begin{bmatrix}1 \\ -2\end{bmatrix}</m>.
					</li>
				</ul>

				<p>
					Write the general solution.
				</p>

				<me>
					Y(t) = C_1 \vec{v}_1 e^{3t} + C_2 \vec{v}_2 e^{-t}.
				</me>

				<p>
					Substitute the eigenvectors:
				</p>

				<me>
					\begin{bmatrix} x(t) \\ y(t) \end{bmatrix} =
					C_1 \begin{bmatrix} 1 \\ 2 \end{bmatrix} e^{3t} +
					C_2 \begin{bmatrix} 1 \\ -2 \end{bmatrix} e^{-t}.
				</me>

				<p>
					Or written componentwise:
				</p>

				<me>
					x(t) = C_1 e^{3t} + C_2 e^{-t}, \qquad
					y(t) = 2C_1 e^{3t} - 2C_2 e^{-t}.
				</me>

				<p>
					The constants <m>C_1</m> and <m>C_2</m> will be found from initial conditions.
				</p>
			</solution>
		</example>

		<example xml:id="ex-complex-eigenvalues">
			<title>Complex Eigenvalues and Spirals</title>
			<statement>
				<p>
					Consider the system:
				</p>
				<md>
					<mrow>\frac{dx}{dt} \amp = 2x - 5y</mrow>
					<mrow>\frac{dy}{dt} \amp = 5x + 2y</mrow>
				</md>
				<p>
					Solve the system and describe the behavior of solutions.
				</p>
			</statement>
			<solution>
				<p>
					Write <m>A = \begin{bmatrix}2 \amp -5 \\ 5 \amp 2\end{bmatrix}</m>.
				</p>

				<p>
					Find eigenvalues by solving <m>\det(A - rI) = 0</m>.
				</p>

				<me>
					\det \begin{bmatrix} 2-r \amp -5 \\ 5 \amp 2-r \end{bmatrix} = (2-r)^2 + 25 = r^2 - 4r + 29.
				</me>

				<p>
					Set equal to zero: <m>r^2 - 4r + 29 = 0</m>.  
					Using the quadratic formula:
				</p>

				<me>
					r = \frac{4 \pm \sqrt{(-4)^2 - 4(29)}}{2} = \frac{4 \pm \sqrt{-100}}{2} = 2 \pm 5i.
				</me>

				<p>
					The eigenvalues are <m>2 \pm 5i</m> ‚Äî complex conjugates.  
					The real part (<m>2</m>) means solutions grow exponentially;  
					the imaginary part (<m>5i</m>) means they also rotate: the system's trajectories spiral outward.
				</p>

				<p>
					Find an eigenvector for <m>r = 2 + 5i</m> (the other is its conjugate).  
					Solving <m>(A - rI)\vec{v} = 0</m> gives an eigenvector <m>\vec{v} = \begin{bmatrix} 1 \\ -i \end{bmatrix}</m>.
				</p>

				<p>
					Write the solution.
				</p>

				<p>
					We form the real solution by taking the real and imaginary parts:
				</p>

				<me>
					\begin{aligned}
					x(t) \amp = e^{2t}\left( C_1 \cos(5t) + C_2 \sin(5t) \right) \\
					y(t) \amp = e^{2t}\left( -C_1 \sin(5t) + C_2 \cos(5t) \right)
					\end{aligned}
				</me>

				<p>
					The exponential factor <m>e^{2t}</m> causes growth; the sine and cosine produce rotation.
					The system's phase portrait shows spirals moving outward from the origin.
				</p>
			</solution>
		</example>
	</paragraphs>

	<exercise label="solving-linear-systems-cyu-bundle">
		<title><e component="emoji">ü§îüí≠</e> Solving Linear Systems Reading Questions</title>

		<task label="solving-linear-systems-cyu-1">
			<title><e component="emoji">üìñ‚ùì</e> Eigenvalues and Behavior</title>
			<statement>
				<p>
					Suppose the eigenvalues of a system are <m>r = -2 \pm 3i</m>. What does this tell you about the solutions?
				</p>
			</statement>
			<choices randomize="yes">
				<choice correct="yes">
					<statement><p>They spiral inward toward the origin.</p></statement>
				</choice>
				<choice correct="no">
					<statement><p>They spiral outward away from the origin.</p></statement>
					<feedback><p>The negative real part means decay, not growth.</p></feedback>
				</choice>
				<choice correct="no">
					<statement><p>They move straight toward the origin with no oscillation.</p></statement>
					<feedback><p>The imaginary part implies rotation (spiraling).</p></feedback>
				</choice>
			</choices>
		</task>
	</exercise>

</section>