<subsection xmlns:xi="http://www.w3.org/2001/XInclude"><title>Common Transforms</title>

	<p>
		In this section, we will explore some of the most commonly encountered Laplace transforms. These functions frequently appear in differential equations, making their transforms especially valuable tools for solving such equations. Let's start with the Laplace transform of the exponential function, <m>e^{at}</m>, and gradually build up to more complex functions like power functions, sine, and cosine.
	</p>

	<paragraphs><title>Laplace Transform of the Exponential Function, <m>e^{at}</m></title>
		
		The exponential function <m>e^{at}</m> is one of the most important functions in mathematics, especially in the context of differential equations. Let's explore how this works with a specific example. 

	</paragraphs>

	<example>

		<m>\quad</m> Compute <m> \lap \{ e^{7t} \} </m>.

		<solution>
			<p>
				We begin by applying the definition of the Laplace transform:
				<md>
					<mrow> 
						\lap\{ e^{7t} \} 
						\amp= \int_0^{\infty} e^{-st} \cdot e^{7t}\ dt
					</mrow>
					<mrow> 
						\amp= \lim_{b \to \infty}\int_0^b e^{(-s+7)t}\ dt
					</mrow>
				</md>
				For this improper integral to converge, the exponent <m>-s+7</m> must be negative, meaning:
				<me> 
					-s+7 \lt 0 \hspace{0.5cm}\Rightarrow \hspace{0.5cm} -s \lt -7 \hspace{0.5cm}\Rightarrow \hspace{0.5cm} s \gt 7
				</me>.
				Thus, we proceed under the assumption that <m>s \gt 7</m>.
				<md>
					<mrow> 
						\lap\{ e^{7t} \} 
							\amp= \lim_{b \to \infty}\int_0^b e^{(-s+7)t}\, dt
					</mrow>
					<mrow> 
							\amp= \lim_{b \to \infty} \frac{1}{7-s} e^{(-s+7)t} \Bigg|_0^b
					</mrow>
					<mrow> 
							\amp= \frac{1}{-s+7} \left[ \lim_{b \to \infty} \left( e^{(-s+7)b} - e^{0} \right) \right]
					</mrow>
					<mrow> 
							\amp= \frac{1}{-s+7} \left[ \lim_{b \to \infty} e^{(-s+7)b} - 1 \right]
					</mrow>
					<mrow>
							\amp= \frac{1}{-s+7} \left[ 0 - 1 \right] \qquad \Big(e^{(\text{negative})b} \to 0\Big)
					</mrow>
					<mrow>
							\amp= -\frac{1}{-s+7} = \frac{1}{s-7}. \quad \text{for } s \gt 7
					</mrow>
				</md>
				Thus, the Laplace transform of <m>e^{7t}</m> is:
				<me>\ds \lap\{e^{7t}\} = \frac{1}{s - 7}, \quad s \gt 7.</me>
			</p>
		</solution>

	</example>

	<p>
		This result can be generalized for any constant <m>a</m>, giving us the Laplace transform of <m>e^{at}</m>. <xref ref="laplace-transform-of-exponential" text="custom">Here are the details.</xref>
	</p>

	<assemblage xml:id="lt-table-L2"><title>Common Laplace Transform (Exponential)</title>
		<p>
			<dl width="narrow">
				<li xml:id="L2"><title><m>L_2.</m></title>
					<m>\ds \lap\{ e^{at} \} = \frac{1}{s - a}, \quad s \gt a, \quad <xref ref="laplace-transform-of-exponential" text="custom">\text{details}</xref></m>
				</li>
			</dl>
		</p>
	</assemblage>

	<xi:include href="./c4-s1-ss3-1-interactives.ptx" />

	<paragraphs><title>Laplace Transform of the Power Function, <m>t^{n}</m></title>

		The power function <m>t^n</m> appears frequently in differential equations, particularly in polynomial solutions. We've already encountered the case when <m>n = 0</m>, since <m>t^0 = 1</m>. Now, let's explore the transform for the first and second powers.

	</paragraphs>

	<example>

		<m>\quad</m> The Laplace transforms for <m>t</m> and <m>t^2</m> are as follows:

		<p>
			<ul marker="square">
				<li>	
					<m> \ds \lap\{t\} 	= \frac{1}{s^2}, \quad s \gt 0 \quad </m> <xref ref="laplace-transform-of-t-power-1" text="custom">Details</xref>
				</li>
				<li>	
					<m> \ds \lap\{t^2\} = \frac{2}{s^3}, \quad s \gt 0 \quad </m> <xref ref="laplace-transform-of-t-power-2" text="custom">Details</xref>
				</li>
			</ul>
		</p>
	</example>

	<p>
		If you look in each solution, before computing <m>L = 0</m>, you'll notice a relationship between the Laplace transforms of powers that differ by one. Namely,
		<me>
			\lap\{t\} = \frac{1}{s}\lap\{1\} \quad \text{and} \quad \lap\{t^2\} = \frac{2}{s}\lap\{t\}
		</me>,
		and if you compute the Laplace transform of <m>t^3</m>, you'll find that
		<me>
			\lap\{t^3\} = \frac{3}{s}\lap\{t^2\}
		</me>.
		In general, this recursive pattern continues for any power <m>n</m> as
		<me>
			\lap\{t^n\} = \frac{n}{s}\lap\{t^{n-1}\}
		</me>.
		So if we wanted the Laplace transform of <m>t^4</m>, we could find it like so
		<md>
			<mrow> 
				\lap\{t^4\}
					=\amp\ \frac{4}{s}\lap\{t^3\}
			</mrow>
			<mrow> 				
					=\amp\ \frac{4}{s}\left[\frac{3}{s}\lap\{t^2\}\right] 
					= \frac{4\cdot 3}{s^2}\left[\frac{2}{s}\lap\{t\}\right] 
					= \frac{4\cdot 3\cdot 2}{s^3}\cdot\frac{1}{s^2} 
					= \ob{\frac{4\cdot 3\cdot 2\cdot 1}{s^5}}^{\text{factorial}}
			</mrow>
		</md>.
		This pattern is true for higher powers of <m>t</m>, leading to the next laplace transform rule which makes use of the <xref ref="factorial" text="title"/>.
	</p>

	<assemblage xml:id="lt-table-L3"><title>Common Laplace Transform (Power)</title>
		<p>
			<dl width="narrow">
				<li xml:id="L3"><title><m>{\LARGE \vphantom{\int}}L_3</m></title>
					<m>\ds \lap\{ t^n \} = \frac{n!}{s^{n+1}}, \quad s >0, \quad n = 1, 2, 3, \ldots </m>
				</li>
			</dl>
		</p>
	</assemblage>

	<xi:include href="./c4-s1-ss3-2-interactives.ptx" />

	<paragraphs><title>Laplace Transform of Sine and Cosine, <m>\sin(bt),\ \cos(bt)</m></title>
	
		Finally, let's consider the Laplace transforms of the famous sine and cosine functions.

	</paragraphs>

	<example>
	
		<m>\quad</m>Compute <m>\lap\{\cos(3t)\}</m>.
		
		<solution>
			<p>
				We start by applying the definition of the Laplace transform:
				<me>
					\lap \{ \cos(3t) \} = \int_0^{\infty} e^{-st} \cdot \cos(3t)\ dt 
				</me>.
				Rather than directly integrating, we will use a modified <xref ref="eulers-formula" text="title"></xref> to express cosine in terms of <m>e</m>
				<me>
					\cos(3t) = \frac12\left(e^{3it} + e^{-3it}\right).
				</me>
				Substituting this into the integral gives:
				<md>
					<mrow> 
						\lap \{ \cos(3t) \} 
						=\amp\ \frac12 \int_0^{\infty} e^{-st} \frac12\left(e^{3it} + e^{-3it}\right)\ dt 
					</mrow>
					<mrow>
						=\amp\ \frac12\left[\int_0^{\infty} e^{-st}\cdot e^{3it}\ dt + \int_0^{\infty} e^{-st}\cdot e^{-3it}\ dt\right]
					</mrow>
					<mrow>
						=\amp\ \frac{1}{2} \left[\lap\{e^{3it}\} + \lap\{e^{-3it}\}\right]
					</mrow>
					<mrow>
						=\amp\ \frac{1}{2} \left[\frac{1}{s - 3i} + \frac{1}{s + 3i}\right] \qquad (\text{by } <xref ref="L2" text="title"/>)
					</mrow>
					<mrow>
						=\amp\ \frac{1}{2} \left[\frac{s + 3i + s - 3i}{(s - 3i)(s + 3i)}\right]
					</mrow>
					<mrow>
						=\amp\ \frac{s}{s^2 + 9}.
					</mrow>
				</md>
				Therefore, the Laplace transform of <m>\cos(3t)</m> is:
				<me>
					\lap \{\cos(3t)\} = \frac{s}{s^2 + 9}.
				</me>
			</p>
		</solution>
	</example>

	<example>

		<m>\quad</m>Compute <m>\lap\{\sin(-4t)\}</m>.
	
		<solution>
			<p>
				As with cosine, we begin with the definition of the Laplace transform,
				<me>
					\lap \{ \sin(-4t) \} = \int_0^{\infty} e^{-st} \cdot \sin(-4t)\ dt
				</me>
				and rewrite sine using Euler's formula,
				<me>
					\sin(-4t) = \frac{e^{-4it} - e^{4it}}{2i}.
				</me>
				Substituting this into the integral, we get:
				<md>
					<mrow> 
						\lap \{ \sin(-4t) \} 
						=\amp \frac{1}{2i} \int_0^{\infty} e^{-st} \left(e^{-4it} - e^{4it}\right)\, dt 
					</mrow>
					<mrow>
						=\amp \frac{1}{2i} \left[\int_0^{\infty} e^{-(s + 4i)t}\, dt - \int_0^{\infty} e^{-(s - 4i)t}\, dt\right]
					</mrow>
					<mrow>
						=\amp \frac{1}{2i} \left[\lap\{e^{-4it}\} - \lap\{e^{4it}\}\right].
					</mrow>
					<mrow>
						=\amp \frac{1}{2i} \left[\frac{1}{s + 4i} - \frac{1}{s - 4i}\right] \qquad (\text{by } <xref ref="L2" text="title"/>)
					</mrow>
					<mrow>
						=\amp \frac{1}{2i} \left[\frac{s - 4i - (s + 4i)}{(s + 4i)(s - 4i)}\right]
					</mrow>
					<mrow>
						=\amp \frac{4}{s^2 + 16}.
					</mrow>
				</md>
				Thus, the Laplace transform of <m>\sin(-4t)</m> is:
				<me>
					\lap \{\sin(-4t)\} = \frac{4}{s^2 + 16}.
				</me>
			</p>
		</solution>
	</example>

	<p>
		A similar approach can be used to show the general formula for the Laplace transforms of sine and cosine are given as follows
	</p>

	<assemblage xml:id="lt-table-L4-L5"><title>Common Laplace Transform (Sine, Cosine)</title>
		<p>
			<dl width="narrow">
				<li xml:id="L4"><title><m>{\LARGE \vphantom{\int}}L_4</m></title>
					<m>\ds \lap\{\sin(bt)\} = \frac{b}{s^2+b^2}, \quad s \gt 0 </m>
				</li>
				<li xml:id="L5"><title><m>{\LARGE \vphantom{\int}}L_5</m></title>
					<m>\ds \lap\{\cos(bt)\} = \frac{s}{s^2+b^2}, \quad s \gt 0 </m>
				</li>
			</dl>
		</p>
	</assemblage>

	<xi:include href="./c4-s1-ss3-3-interactives.ptx" />
	
</subsection>