<subsection xmlns:xi="http://www.w3.org/2001/XInclude"><title>Common Transforms</title>

	<p>
		The exponential function is commonly encountered in differential equations, making its Laplace transform especially important. Let's explore the Laplace transform of the exponential function <m>e^{at}</m>, where <m>a</m> is a constant. We'll start with a specific example, setting <m>a = 7</m>, and then generalize the result.
	</p>

	<example>

		<m>\quad</m> Compute <m> \lap \{ e^{7t} \} </m>.

		<solution>
			<p>
				We begin by applying the definition of the Laplace transform:
				<md>
					<mrow> 
						\lap\{ e^{7t} \} 
						\amp= \int_0^{\infty} e^{-st} \cdot e^{7t}\ dt
					</mrow>
					<mrow> 
						\amp= \lim_{b \to \infty}\int_0^b e^{(-s+7)t}\ dt
					</mrow>
				</md>
				For this improper integral to converge, the exponent <m>-s+7</m> must be negative, meaning:
				<me> 
					-s+7 \lt 0 \hspace{0.5cm}\Rightarrow \hspace{0.5cm} -s \lt -7 \hspace{0.5cm}\Rightarrow \hspace{0.5cm} s \gt 7
				</me>.
				Thus, we proceed under the assumption that <m>s \gt 7</m>.
				<md>
					<mrow> 
						\lap\{ e^{7t} \} 
							\amp= \lim_{b \to \infty}\int_0^b e^{(-s+7)t}\, dt
					</mrow>
					<mrow> 
							\amp= \lim_{b \to \infty} \frac{1}{7-s} e^{(-s+7)t} \Bigg|_0^b
					</mrow>
					<mrow> 
							\amp= \frac{1}{-s+7} \left[ \lim_{b \to \infty} \left( e^{(-s+7)b} - e^{0} \right) \right]
					</mrow>
					<mrow> 
							\amp= \frac{1}{-s+7} \left[ \lim_{b \to \infty} e^{(-s+7)b} - 1 \right]
					</mrow>
					<mrow>
							\amp= \frac{1}{-s+7} \left[ 0 - 1 \right] \qquad \Big(e^{(\text{negative})b} \to 0\Big)
					</mrow>
					<mrow>
							\amp= -\frac{1}{-s+7} = \frac{1}{s-7}. \quad \text{for } s \gt 7
					</mrow>
				</md>
				Thus, the Laplace transform of <m>e^{7t}</m> is:
				<me>\ds \lap\{e^{7t}\} = \frac{1}{s - 7}, \quad s \gt 7.</me>
			</p>
		</solution>

	</example>

	<p>
		To generalize this result, let's replace <m>7</m> with a constant <m>a</m>.
	</p>

	<example>

		<m>\quad</m> Show that <m>\ds \lap \{ e^{at} \} = \frac{1}{s - a} </m>.

		<solution>
			<p>
				We follow a similar process, starting with the definition of the Laplace transform:
				<md>
					<mrow> 
						\lap\{ e^{at} \} 
						\amp= \int_0^{\infty} e^{-st} \cdot e^{at}\ dt
					</mrow>
					<mrow> 
						\amp= \lim_{b \to \infty}\int_0^b e^{(-s+a)t}\ dt
					</mrow>
				</md>
				For the integral to converge, the exponent <m>-s+a</m> must be negative, which requires <m>\ -s+a \lt 0\ </m> or <m>\ s \gt a</m> to proceed
				<md>
					<mrow> 
						\lap\{ e^{at} \} 
						\amp= \lim_{b \to \infty}\int_0^b e^{(-s+a)t}\ dt
					</mrow>
					<mrow> 
						\amp= \lim_{b \to \infty} \frac{1}{-s+a} e^{(-s+a)t} \Bigg|_0^b
					</mrow>
					<mrow> 
						\amp= \frac{1}{-s+a} \left[ \lim_{b \to \infty} \left( e^{(-s+a)b} - e^{0} \right) \right]
					</mrow>
					<mrow> 
						\amp= \frac{1}{-s+a} \left[ \lim_{b \to \infty} e^{(-s+a)b} - 1 \right]
					</mrow>
					<mrow>
						\amp= \frac{1}{-s+a} \left[ 0 - 1 \right]
					</mrow>
					<mrow>
						\amp= -\frac{1}{-s+a} = \frac{1}{s-a}. \quad \text{for } s \gt a
					</mrow>
				</md>
				Thus, the Laplace transform of <m>e^{at}</m> is:
				<me>\ds \lap\{e^{at}\} = \frac{1}{s - a}, \quad s \gt a.</me>
			</p>
		</solution>

	</example>

	<p>
		With this result, we can now add the Laplace transform of <m>e^{at}</m> to our list of common Laplace transforms.
	</p>

	<p>
		Next, we'll explore the Laplace transform of the power function <m>t^n</m>, where <m>n</m> is a non-negative integer. We've already encountered the case where <m>n = 0</m>, since <m>t^0 = 1</m> and its transform is given by <xref ref="L1" text="custom"><m>L_1</m></xref>. Now, let's start with <m>n = 1</m> and work our way up to find a general formula for the Laplace transform of <m>t^n</m>.
	</p>

	<example>
		<p>
			Compute <m>\lap\{t\}</m>.
		</p>
	
		<solution>
			<p>
				We'll begin by applying the definition of the Laplace transform:
				<md>
					<mrow> 
						\lap\{ t \}
							\amp= \int_0^{\infty} e^{-st} \cdot t\ dt 
					</mrow>
					<mrow> 				
							\amp= \lim_{b \to \infty} \int_0^b t e^{-st}\, dt \quad (s \ne 0) \quad <xref text="custom" ref="LT-s-ne-0-t">Why is <m>s \ne 0</m>?</xref>
					</mrow>
				</md>
				Using integration by parts, we have:
				<md>
					<mrow> 
						\phantom{\lap\{t\}}
							\amp= \lim_{b \to \infty} \left[-\frac{b}{s}e^{-sb} + \frac{1}{s^2}\right] \quad <xref text="custom" ref="reason-int-by-parts-texpt">Integration by parts</xref>
					</mrow>
				</md>
				As <m>b</m> approaches infinity:
				<md>
					<mrow> 
						\phantom{\lap\{t\}}
							\amp= \left[-\frac{1}{s}\lim_{b \to \infty}\frac{b}{e^{sb}} + \frac{1}{s^2}\right] \quad (s &gt; 0) \quad <xref text="custom" ref="LT-s-gt-0-t">\text{Why is } s &gt; 0?</xref>
					</mrow>
					<mrow> 
						\phantom{\lap\{t\}}
							\amp= \left[0 + \frac{1}{s^2}\right] \quad <xref text="custom" ref="reason-limit-to-zero-t">Why is the limit 0?</xref>
					</mrow>
					<mrow> 		
							\amp= \frac{1}{s^2}, \quad s \gt 0
					</mrow>
				</md>
				Therefore, <m>\ds \lap\{ t \} = \frac{1}{s^2}</m>, valid for <m>s &gt; 0</m>.
			</p>
		</solution>
	</example>
	
	<p>
		Using similar steps, we can derive the following results:
	</p>

	<example>
		<p>
			<ul marker="square">
				<li>	
					<m> \ds \lap\{t^2\} = \frac{2}{s^3}, \quad s \gt 0 \quad </m> <xref ref="std_LT_01" text="custom">Solution</xref>
				</li>
				<li>	
					<m> \ds \lap\{t^3\} = \frac{6}{s^4}, \quad s \gt 0 \quad </m> <xref ref="std_LT_02" text="custom">Solution</xref> 
				</li>
				<li>
					<m> \ds \lap\{t^4\} = \frac{24}{s^5}, \quad s \gt 0 \quad </m> <xref ref="std_LT_03" text="custom">Solution</xref> 
				</li>
			</ul>
		</p>
	</example>

	<p>
		Do you notice the emerging pattern? Let's rewrite the numerators:
		<ul marker="">
			<li>	
				<m> \ds \lap\{t^2\} = \frac{2}{s^3} = \frac{2 \cdot 1}{s^3} = \frac{2!}{s^3} </m>
			</li>
			<li>	
				<m> \ds \lap\{t^3\} = \frac{6}{s^4} = \frac{3 \cdot 2 \cdot 1}{s^4} = \frac{3!}{s^4} </m>
			</li>
			<li>
				<m> \ds \lap\{t^4\} = \frac{24}{s^5} = \frac{4 \cdot 3 \cdot 2 \cdot 1}{s^5} = \frac{4!}{s^5} </m>
			</li>
			<li>
				<m> \hspace{6em} \vdots </m>
			</li>
			<li>
				<m> \ds \lap\{t^n\} = \frac{n!}{s^{n+1}} </m>
			</li>
		</ul>
		Thus, the general formula for the Laplace transform of <m>t^n</m> is:
		<me>\ds \lap\{t^n\} = \frac{n!}{s^{n+1}}, \quad s &gt; 0.</me>
	</p>
	
	<p>
		In this section, we will explore the Laplace transforms of the sine and cosine functions. These transforms are particularly important because sine and cosine frequently appear in the solutions of differential equations.
	</p>

	<example>
	
		<m>\quad</m>Compute <m>\lap\{\cos(3t)\}</m>.
		
		<solution>
			<p>
				We start by applying the definition of the Laplace transform:
				<me>
					\lap \{ \cos(3t) \} = \int_0^{\infty} e^{-st} \cdot \cos(3t)\ dt 
				</me>.
				While we could proceed with integration by parts, a more efficient approach is to use the Euler's formula representation of cosine:
				<me>
					\cos(3t) = \frac{e^{3it} + e^{-3it}}{2}.
				</me>
				Substituting this into the integral gives:
				<md>
					<mrow> 
						\lap \{ \cos(3t) \} 
							=\amp \frac{1}{2} \int_0^{\infty} e^{-st} \left(e^{3it} + e^{-3it}\right)\, dt 
					</mrow>
					<mrow>
						=\amp \frac{1}{2} \left[\int_0^{\infty} e^{-(s - 3i)t}\, dt + \int_0^{\infty} e^{-(s + 3i)t}\, dt\right]
					</mrow>
					<mrow>
						=\amp \frac{1}{2} \left[\lap\{e^{3it}\} + \lap\{e^{-3it}\}\right].
					</mrow>
				</md>
				Using the known Laplace transforms for exponential functions, we have:
				<md>
					<mrow>
						\lap \{ \cos(3t) \} 
							=\amp \frac{1}{2} \left[\frac{1}{s - 3i} + \frac{1}{s + 3i}\right]
					</mrow>
					<mrow>
						=\amp \frac{1}{2} \left[\frac{s + 3i + s - 3i}{(s - 3i)(s + 3i)}\right]
					</mrow>
					<mrow>
						=\amp \frac{s}{s^2 + 9}.
					</mrow>
				</md>
				Therefore, the Laplace transform of <m>\cos(3t)</m> is:
				<me>
					\lap \{\cos(3t)\} = \frac{s}{s^2 + 9}.
				</me>
			</p>
		</solution>
	</example>

	<example>
	
		<m>\quad</m>Compute <m>\lap\{\sin(-4t)\}</m>.
	
		<solution>
			<p>
				Again, we begin with the definition of the Laplace transform:
				<me>
					\lap \{ \sin(-4t) \} = \int_0^{\infty} e^{-st} \cdot \sin(-4t)\ dt.
				</me>
				As with the cosine, we can use the Euler's formula for sine:
				<me>
					\sin(-4t) = \frac{e^{-4it} - e^{4it}}{2i}.
				</me>
				Substituting this into the integral, we get:
				<md>
					<mrow> 
						\lap \{ \sin(-4t) \} 
							=\amp \frac{1}{2i} \int_0^{\infty} e^{-st} \left(e^{-4it} - e^{4it}\right)\, dt 
					</mrow>
					<mrow>
						=\amp \frac{1}{2i} \left[\int_0^{\infty} e^{-(s + 4i)t}\, dt - \int_0^{\infty} e^{-(s - 4i)t}\, dt\right]
					</mrow>
					<mrow>
						=\amp \frac{1}{2i} \left[\lap\{e^{-4it}\} - \lap\{e^{4it}\}\right].
					</mrow>
				</md>
				Substituting the known Laplace transforms, we have:
				<md>
					<mrow>
						\lap \{ \sin(-4t) \} 
							=\amp \frac{1}{2i} \left[\frac{1}{s + 4i} - \frac{1}{s - 4i}\right]
					</mrow>
					<mrow>
						=\amp \frac{1}{2i} \left[\frac{s - 4i - (s + 4i)}{(s + 4i)(s - 4i)}\right]
					</mrow>
					<mrow>
						=\amp \frac{4}{s^2 + 16}.
					</mrow>
				</md>
				Thus, the Laplace transform of <m>\sin(-4t)</m> is:
				<me>
					\lap \{\sin(-4t)\} = \frac{4}{s^2 + 16}.
				</me>
			</p>
		</solution>
	</example>

	<p>
		We can generalize these results by replacing <m>3</m> and <m>4</m> with <m>b</m> in the above examples. The updated common transforms are as follows:
	</p>

	<assemblage xml:id="lt-table-L4-L5"><title>Common Laplace Transforms <m>L_3</m>, <m>L_4</m></title>
		<p>
			<dl width="narrow">
				<li xml:id="L2"><title><m>{\LARGE \vphantom{\int}}L_2</m></title>
					<m>\ds \lap\{ e^{at} \} = \frac{1}{s - a}, \quad s \gt a, \quad a \text{ is a constant} </m>
				</li>
				<li xml:id="L3"><title><m>{\LARGE \vphantom{\int}}L_3</m></title>
					<m>\ds \lap\{ t^n \} = \frac{n!}{s^{n+1}}, \quad s &gt;0, \quad n = 1, 2, 3, \ldots </m>
				</li>
				<li xml:id="L4"><title><m>{\LARGE \vphantom{\int}}L_4</m></title>
					<m>\ds \lap\{ \sin(bt) \} = \frac{b}{s^2+b^2}, \quad s &gt;0, \quad b \text{ is a constant} </m>
				</li>
				<li xml:id="L5"><title><m>{\LARGE \vphantom{\int}}L_5</m></title>
					<m>\ds \lap\{ \cos(bt) \} = \frac{s}{s^2+b^2}, \quad s &gt;0, \quad b \text{ is a constant} </m>
				</li>
			</dl>
		</p>
	</assemblage>

	<xi:include href="./c4-s1-ss3-interactives.ptx" />

</subsection>