<section xmlns:xi="http://www.w3.org/2001/XInclude"><title> Higher-Order LHCC </title>

	<p>
		As in the previous section, the approach to solving higher-order linear homogeneous constant coefficient (LHCC) equations is fairly straightforward. Find the solutions to the characteristic equation and use them to write down each term of the general solution. The key difference lies in the fact that you must solve a high-degree polynomial equation, which can be challenging since you no longer have a simple formula to give you the solutions.
	</p>
	
	<p>
		To see this, consider the <m>n</m>-th order LHCC equation,
		<me>
			a_n y^{(n)} + a_{n-1} y^{(n-1)} + \cdots + a_1 y' + a_0 y = 0
		</me>,
		which has an <m>n</m>-th degree characteristic equation
		<me>
			a_n r^n + a_{n-1} r^{n-1} + \cdots + a_1 r + a_0 = 0
		</me>.
		
	</p>
	
	<xref provisional="Maybe ask the department the preferred approach here and come back."/>

	<example>
		<statement>
			<p>
				Completely factor and solve the following characteristic equations
				<ol>
					<li> <m> 4\ r^2 - 9 = 0 </m> </li>
					<li> <m> r^2 - 3 = 0 </m> </li>
					<li> <m> r^3 + 3\ r^2 - 4\ r = 0 </m> </li>
					<li> <m> r^5 + 10\ r^4 = 0 </m> </li>
					<li> <m> r^4 - 100\ r^2 = 0 </m> </li>
					<li> <m> r^5 - 4\ r^3 = 0 </m> </li>
					<li> <m> r^4 - 32 = 0 </m> </li>
				</ol>
			</p>
		</statement>
		<solution>
			<p>
				The degree of each equation tells you how many factors you should have.
				<ol>
					<li>
						<p>
							<tabular>
								<row>
									<cell><m> 4\ r^2 - 9 = 0 </m></cell>
									<cell/>
								</row>
								<row>
									<cell><m> (2\ r + 3)(2\ r - 3) = 0 </m></cell>
									<cell> <m>\leftarrow</m> difference of squares </cell>
								</row>
								<row>
									<cell><m> 2\ r + 3 = 0, \quad 2\ r - 3 = 0 </m></cell>
									<cell><m>\leftarrow</m> set each factor to 0 </cell>
								</row>
								<row>
									<cell><m> \displaystyle r_1 = -\frac32, \quad r_2 = \frac32 </m></cell>
									<cell><m>\leftarrow</m> solutions </cell>
								</row>
							</tabular>
						</p>
					</li>

					<li>
						<p>
							<tabular>
								<row>
									<cell><m> r^2 - 3 = 0 </m></cell>
									<cell/>
								</row>
								<row>
									<cell><m> (r + \sqrt{3})(r - \sqrt{3}) = 0 </m></cell>
									<cell> <m>\leftarrow</m> difference of squares </cell>
								</row>
								<row>
									<cell><m> \displaystyle r_1 = -\sqrt{3}, \quad r_2 = \sqrt{3} </m></cell>
									<cell><m>\leftarrow</m> solutions </cell>
								</row>
							</tabular>
						</p>
					</li>

					<li>
						<p>
							<tabular>
								<row>
									<cell><m> r^3 + 3\ r^2 - 4\ r = 0 </m></cell>
									<cell/>
								</row>
								<row>
									<cell><m> r\ (r^2 + 3\ r - 4) = 0 </m></cell>
									<cell> <m>\leftarrow</m> common factor </cell>
								</row>
								<row>
									<cell><m> r\ (r + 4)(r - 1) = 0 </m></cell>
									<cell> <m>\leftarrow</m> standard quadratic factoring </cell>
								</row>
								<row>
									<cell><m> \displaystyle r_1 = 0, \quad r_2 = -4, \quad r_3 = 1 </m></cell>
									<cell><m>\leftarrow</m> solutions </cell>
								</row>
							</tabular>
						</p>
					</li>
					
					<li>
						<p>
							<tabular>
								<row>
									<cell><m> r^5 + 10\ r^4 = 0 </m></cell>
									<cell/>
								</row>
								<row>
									<cell><m> r^4\ (r + 10) = 0 </m></cell>
									<cell> <m>\leftarrow</m> common factor </cell>
								</row>
								<row>
									<cell><m> \displaystyle r_1 = 0\ (\text{4 repeats}), \quad r_2 = -10 </m></cell>
									<cell><m>\leftarrow</m> solutions </cell>
								</row>
							</tabular>
						</p>
						<p>
							<em> Technically, <m>r^4 = (r-0)^4</m> and represents 4 repeated factors. </em>
						</p>
					</li>


					<li>
						<p>
							<tabular>
								<row>
									<cell><m> r^4 - 100\ r^2 = 0 </m></cell>
									<cell/>
								</row>
								<row>
									<cell><m> r^2\ (r^2 - 100) = 0 </m></cell>
									<cell> <m>\leftarrow</m> common factor </cell>
								</row>
								<row>
									<cell><m> r^2\ (r + 10)(r - 10) = 0 </m></cell>
									<cell> <m>\leftarrow</m> difference of squares </cell>
								</row>
								<row>
									<cell><m> \displaystyle r_1 = 0\ (\text{2 repeats}), \quad r_2 = -10, \quad r_3 = 10 </m></cell>
									<cell><m>\leftarrow</m> solutions </cell>
								</row>
							</tabular>
						</p>
					</li>

					<li>
						<p>
							<tabular>
								<row>
									<cell><m> r^5 - 4\ r^3 = 0 </m></cell>
									<cell/>
								</row>
								<row>
									<cell><m> r^3\ (r^2  - 4) = 0 </m></cell>
									<cell> <m>\leftarrow</m> common factor </cell>
								</row>
								<row>
									<cell><m> r^3\ (r + 2)(r - 2) = 0 </m></cell>
									<cell> <m>\leftarrow</m> difference of squares </cell>
								</row>
								<row>
									<cell><m> \displaystyle r_1 = 0\ (\text{3 repeats}), \quad r_2 = -2, \quad r_3 = 2 </m></cell>
									<cell><m>\leftarrow</m> solutions </cell>
								</row>
							</tabular>
						</p>
					</li>

					<li>
						<p>
							<tabular>
								<row>
									<cell><m> r^4 - 25 = 0 </m></cell>
									<cell/>
								</row>
								<row>
									<cell><m> (r^2 + 5)(r^2  - 5) = 0 </m></cell>
									<cell> <m>\leftarrow</m> difference of squares </cell>
								</row>
								<row>
									<cell><m> (r^2 + 5)(r - \sqrt{5})(r + \sqrt{5}) = 0 </m></cell>
									<cell> <m>\leftarrow</m> difference of squares </cell>
								</row>
								<row>
									<cell><m> r^2 + 5 = 0, \quad r - \sqrt{5} = 0, \quad r + \sqrt{5} = 0 </m></cell>
									<cell><m>\leftarrow</m> set each factor to 0 </cell>
								</row>
								<row>
									<cell><m> \displaystyle r_1 = -i\sqrt{5}, \quad r_2 = i\sqrt{5}, \quad r_3 = -\sqrt{5}, \quad r_4 = \sqrt{5} </m></cell>
									<cell><m>\leftarrow</m> solutions </cell>
								</row>
							</tabular>
						</p>
					</li>

				</ol>
			</p>
		</solution>
	</example>

	<example>
		<m>\ \ </m> Let's solve a third-order LHCC equation:
		<statement>
		<me> y''' - 6y'' + 11y' - 6y = 0 </me>.
	</statement>
	<solution>
		<p>
		First, write down the characteristic equation:
		</p>
		<md>
		<mrow> r^3 - 6r^2 + 11r - 6 = 0 </mrow>
		</md>.
		<p>
		Solving for <m>r</m>, we get three distinct real roots:
		</p>
		<md>
		<mrow> r = 1, \quad r = 2, \quad r = 3 </mrow>
		</md>.
		<p>
		Therefore, the general solution is:
		</p>
		<me> y = C_1 e^{x} + C_2 e^{2x} + C_3 e^{3x} </me>.
	</solution>
	</example>
	
	<example>
		<m>\ \ </m> Consider another example, a fourth-order LHCC equation:
		<statement>
		<me> y^{(4)} - 5y'' + 4y = 0 </me>.
	</statement>
	<solution>
		<p>
		The characteristic equation is:
		</p>
		<md>
		<mrow> r^4 - 5r^2 + 4 = 0 </mrow>
		</md>.
		<p>
		Let <m>u = r^2</m>, then we can rewrite the equation as:
		</p>
		<md>
		<mrow> u^2 - 5u + 4 = 0 </mrow>
		</md>.
		<p>
		Solving for <m>u</m>, we get:
		</p>
		<md>
		<mrow> u = 1, \quad u = 4 </mrow>
		</md>.
		<p>
		Thus, <m>r^2 = 1</m> gives <m>r = \pm 1</m>, and <m>r^2 = 4</m> gives <m>r = \pm 2</m>. The general solution is:
		</p>
		<me> y = C_1 e^{x} + C_2 e^{-x} + C_3 e^{2x} + C_4 e^{-2x} </me>.
	</solution>
	</example>
	
	<p>
		As seen in these examples, solving the characteristic equation for higher-order LHCC equations follows the same principles as for lower-order equations. However, as the degree of the polynomial increases, solving the characteristic equation analytically can become impractical due to the complexity of the roots.
	</p>
	
	<p>
		For higher-degree characteristic equations, numerical methods and computer algebra systems are typically employed to find the roots. Software tools like MATLAB, Mathematica, and even graphing calculators can assist in solving these polynomial equations, allowing us to focus on interpreting and utilizing the solutions.
	</p>
	
	<example>
		<m>\ \ </m> Consider the fifth-order LHCC equation:
		<statement>
			<me> y^{(5)} - 4y''' + 3y'' - y = 0 </me>.
		</statement>
		<solution>
			<p>
			The characteristic equation is:
			</p>
			<md>
			<mrow> r^5 - 4r^3 + 3r^2 - 1 = 0 </mrow>
			</md>.
			<p>
			Solving this polynomial equation analytically is challenging, so we use a numerical solver. The roots are found to be approximately:
			</p>
			<md>
			<mrow> r_1 = 1, \quad r_2 \approx 1.5, \quad r_3 \approx -1, \quad r_4 \approx 0.5 + 0.5i, \quad r_5 \approx 0.5 - 0.5i </mrow>
			</md>.
			<p>
			The general solution, incorporating these roots, is:
			</p>
			<me> y = C_1 e^{x} + C_2 e^{1.5x} + C_3 e^{-x} + e^{0.5x} (C_4 \cos(0.5x) + C_5 \sin(0.5x)) </me>.
		</solution>
	</example>
	
	<p>
		By recognizing the type of roots and using technology to solve higher-degree polynomials, we can extend our approach to solve any higher-order LHCC equation effectively.
	</p>

	<paragraphs xml:id="poly-factor-p"><title>Polynomial Factoring Calculator</title>
		<interactive xml:id="poly-factor" platform="sage" width="95%" aspect="3.25:1">
			<slate surface="sage">
				r = var('r')
				r = PolynomialRing(RationalField(), 'r').gen()
				F = 'r^2 - 2*r - 8'
				P = r^2 - 2*r - 8
				@interact
				def _(ce = input_box(P, label="	Polynomial:", type=str, width=30)):
					ce_poly = sage_eval('lambda r: ' + ce)
					pretty_print( html( r'Polynomial: $ %s = 0 $'%latex(ce_poly(r) ) ) )
					pretty_print( html( r'Factored Polynomial: $ %s = 0 $'%latex(ce_poly(r).factor()) ) )
			</slate>
		</interactive>
	</paragraphs>

	<xi:include href="./p3-c2-s3-interactives.ptx" />

</section>