<section xmlns:xi="http://www.w3.org/2001/XInclude"><title> Solutions </title>

	<p>
		Before diving into how to solve <xref ref="def-lhcc" text="custom">LHCC equations</xref>, let's develop some intuition about what the solutions should look like. For this discussion we will assume that the equations contain a <m>y</m> term. If they didn't, then you could repeatedly integrate both sides of the equation until you are left with a <m>y</m> term and a nonhomogeneous equation.
		<fn>
			For example, the following shows how an LHCC equation with no <m>y</m> term can be reduced to a nonhomogeneous equation with a <m>y</m> term.
			<md>
				<mrow> y''' - 2y'' = 0 \ \ \rightarrow \ \ (y' - 2y)''	=\amp\ 0 \quad \text{(direct integration x2)}	</mrow>
				<mrow> (y' - 2y)'										=\amp\ c_1										</mrow>
				<mrow> y' - 2y											=\amp\ c_1x + c_2								</mrow>
			</md>.
		</fn>
	</p>

	<p>
		We begin with the simple first-order LHCC equation,
		<men xml:id="lhcc-intro-de"> 
			y' - 2 y = 0
		</men>
		and note that this equation requires <m>y' - 2y</m> to sum to zero. Recall from algebra that only <xref ref="like-terms" text="custom">like terms</xref> can combine to simplify to zero. 
		So, for the equation to hold, <m>y'</m> and <m>y</m> must be like terms.
	</p>

	<p>
		Let's test a few guesses for <m>y</m>: 
		<m>y = x^2</m>, <m>y = 2 \ln x</m>, and <m>y = e^{2x}</m>.
	</p>

	<sidebyside widths="30% 40% 30%">
		<p>
			<md>
				<mrow> \left[x^2\right]' - 2 \left[x^2\right] = 0 </mrow>
				<mrow> \ub{2x - 2x^2}_{\text{not like terms}} = 0 </mrow>
			</md>
		</p>
		<p>
			<md>
				<mrow> \left[2\ln x\right]' - 4\ln x = 0 </mrow>
				<mrow> \ub{\frac{2}{x} - 4\ln x}_{\text{not like terms}} = 0 </mrow>
			</md>
		</p>
		<p>
			<md>
				<mrow> \left[e^{2x}\right]' - 2 \left[e^{2x}\right] = 0 </mrow>
				<mrow> \ub{2e^{2x} - 2e^{2x}}_{\text{like terms}\, =\, 0} = 0 </mrow>
			</md>
		</p>
	</sidebyside>

	<p>
		As you can see, only <m>y = e^{2x}</m> produces like terms that simplify to zero. This is why exponential functions often work well in LHCC equations. Let's now examine a more complex example to expand on this idea.
	</p>

	<example>
		<m>\ \ </m> Consider the LHCC equation:
		<me>
			y'' - 3y' - 4y = 0.
		</me>
		<p>
			Verify that <m>y = e^{4x}</m> is a solution, but <m>y = x^4</m> is not.
		</p>
		<solution>
			<p>
				Let's check each function:
			</p>
			<sidebyside>
				<p>
					<md>
						<mrow> 	[e^{4x}]'' - 3\left[e^{4x}\right]' - 4\left[e^{4x}\right]	=\amp\ 0	</mrow>
						<mrow> 	
							\us{\text{like terms simplify to }0}{\ub{
								16e^{4x} - 12e^{4x} - 4e^{4x}	
							}}
							=\amp\ 0	
						</mrow>
						<mrow> 	0	=\amp\ 0	\ \ ✅ </mrow>
					</md>
				</p>
				<p>
					<md>
						<mrow> 	[x^4]'' - 3\left[x^4\right]' - 4\left[x^4\right]	=\amp\ 0	</mrow>
						<mrow> 	
							\us{\text{not like terms, do not combine}}{\ub{
								12x^2 - 12x^3 - 4x^4	
							}}
							=\amp\ 0	\ \ ❌
						</mrow>
					</md>
				</p>
			</sidebyside>
			<p>
				Therefore, only <m>y = e^{-4x}</m> is a solution.
			</p>
		</solution>
	</example>

	<p>
		This example further supports the claim that exponential functions, like <m>e^{rx}</m>, are well-suited for LHCC equations because they produce like terms when differentiated. Later, we will see that if <m>e^{rx}</m> is a solution then, in some cases, it is possible for <m>xe^{rx}</m> to be a solution as well.
	</p>

	<p>
		We conclude this section with an important concept that will guide us in the sections to follow.
		<assemblage><title> Terms of the Solution to an LHCC Equation </title>
			<p>
				The general solution to an LHCC equation involves terms of the form:
				<me> e^{rx}, \quad \ub{xe^{rx}, \quad x^2e^{rx}, \quad x^3e^{rx},\  \ldots}_{\text{For Special Cases}} </me> 
				where <m>r</m> is a constant. Note, if <m>r</m> is complex, then <m>r=a+\theta i</m>, and by <xref ref="eulers-formula" text="custom">Euler's formula</xref>, 
				<me> e^{rx} = e^{(a+\theta i)x} = e^{ax}\cdot e^{\theta i x} = e^{ax}(\cos(bx) + i\sin(bx)) </me>.
				In this case, it is common to see a solution written with sine and cosine terms.
			</p>
			<!-- <p>
				When <m>r</m> is complex, then <m>r=a+\theta i</m>, and by <xref ref="eulers-formula" text="custom">Euler's formula</xref>, <m> e^{rx} = e^{(a+\theta i)x} = e^{ax}\cdot e^{\theta i x} = e^{ax}(\cos(bx) + i\sin(bx)) </m>.
				In this case, the general solution may also contain sine and cosine terms.
			</p> -->
		</assemblage>
	</p>

	<xi:include href="./p3-c1-s2-interactives.ptx" />

</section>