<subsection><title> Additional Examples </title>

	<subsubsection><title> Order &amp; Linearity </title>
		
		<example><title>Classify Terms</title>
			<p>
				<statement>
					<p>
						Consider the following differential equation:
						<me>
							e^{t}y^{(7)} + (t+1)y'y''' - t \ln y'' - y' \sin t - \tan y + \frac{4}{y} = \frac{3}{t}.
						</me>
						Let's determine the linearity of each term.
					</p>
				</statement>
			</p>

			<p>
				<solution>
					<p>
						To classify terms, focus on the dependent variable <m>y</m> and its derivatives. The table below summarizes the linearity of each term:
					</p>
					<tabular>
						<col width="25%" halign="center" />
						<col width="25%" halign="center" />
						<col width="25%" halign="center" />
						<col width="25%" halign="center" />
						<row>
							<cell>Term</cell>
							<cell>Coefficient</cell>
							<cell>Dependent Variable</cell>
							<cell>Linearity</cell>
						</row>
						<row>
							<cell><m>e^t y^{(7)}</m></cell>
							<cell><m>e^t</m></cell>
							<cell><m>y^{(7)}</m></cell>
							<cell>Linear</cell>
						</row>
						<row>
							<cell><m>(t+1)y'y'''</m></cell>
							<cell><m>(t+1)</m></cell>
							<cell><m>y'y'''</m></cell>
							<cell>Nonlinear</cell>
						</row>
						<row>
							<cell><m>t \ln y''</m></cell>
							<cell><m>t</m></cell>
							<cell><m>\ln y''</m></cell>
							<cell>Nonlinear</cell>
						</row>
						<row>
							<cell><m>y' \sin t</m></cell>
							<cell><m>\sin t</m></cell>
							<cell><m>y'</m></cell>
							<cell>Linear</cell>
						</row>
						<row>
							<cell><m>\tan y</m></cell>
							<cell><m>1</m></cell>
							<cell><m>\tan y</m></cell>
							<cell>Nonlinear</cell>
						</row>
						<row>
							<cell><m>\frac{4}{y}</m></cell>
							<cell><m>4</m></cell>
							<cell><m>\frac{1}{y}</m></cell>
							<cell>Nonlinear</cell>
						</row>
						<row>
							<cell><m>\frac{3}{t}</m></cell>
							<cell><m>-</m></cell>
							<cell><m>-</m></cell>
							<cell>Linear</cell>
						</row>
					</tabular>
					<p>
						Note the last term, <m>\frac{3}{t}</m>, is a constant term since it does not involve the dependent variable <m>y</m> or its derivatives. These terms are always linear in the context of differential equations.
					</p>
				</solution>
			</p>
		</example>

	</subsubsection>

	<subsubsection><title> Solutions &amp; Initial Conditions </title>

		<example xml:id="de-two-solutions">

			<statement>
				<p>
					Verify if both <m>y= 2e^{-3t}</m> and <m>y= e^{4t}</m> are solutions to 
					<me>y'' - y' - 12y = 0</me>.
				</p>
			</statement>

			<solution>
				<p>
					Find <m>y'</m> and <m>y''</m> since they appear in the equation.
					<md>
						<mrow>	y	=\amp\  2e^{-3t}								</mrow>
						<mrow>	y' 	=\amp\  2e^{-3t}\left(-3\right)	=	-6e^{-3t}	</mrow>
						<mrow>	y'' =\amp\ -6e^{-3t}\left(-3\right)	=	18e^{-3t}	</mrow>
					</md>
				</p>

				<p>
					Plug <m>y, y',</m> and <m>y''</m> into the DE and simplify.
					<md>
						<mrow> 													y'' - y' - 12y	=\amp\ 0									</mrow>
						<mrow> 18e^{-3t} - \left( -6e^{-3t} \right) - 12\left( 2e^{-3t} \right)	=\amp\ 0									</mrow>
						<mrow> 								18e^{-3t} + 6e^{-3t} - 24e^{-3t}	=\amp\ 0									</mrow>
						<mrow> 																0	=\amp\ 0	\quad✅	</mrow>
					</md>
					Therefore, <m>y= 2e^{-3t}</m> is a solution to <m>y'' - y' - 12y = 0.</m>
				</p>
			
				<p>
					Find <m>y'</m> and <m>y''</m> since they appear in the DE.
					<md>
						<mrow>	y	=\amp\  e^{4t}								</mrow>
						<mrow>	y' 	=\amp\  e^{4t}\left(4\right)	=	4e^{4t}	</mrow>
						<mrow>	y'' =\amp\ 4e^{4t}\left(4\right)	=	16e^{4t}</mrow>
					</md>
				</p>

				<p>
					Plug <m>y, y',</m> and <m>y''</m> into the DE and simplify.
					<md>
						<mrow> 								y'' - y' - 12y	=\amp\ 0									</mrow>
						<mrow> 16e^{4t} - 4e^{4t} - 12\left( e^{4t} \right)	=\amp\ 0									</mrow>
						<mrow> 				16e^{4t} - 4e^{4t} - 12e^{4t}	=\amp\ 0									</mrow>
						<mrow> 											0	=\amp\ 0	\quad✅	</mrow>
					</md>
					Therefore, <m>y= e^{4t}</m> is a solution to <m>y'' - y' - 12y = 0.</m>
				</p>
			</solution>

		</example>

		<example>

			<statement>
				<p>
					Verify if <m>\ds\ y = 3\sin(x^2) </m> is a solution to 
					<me>y' - xy'' = 12x^2\sin(x^2)</me>.
				</p>
			</statement>

			<solution>
				<p>
					Find <m>y'</m> and <m>y''</m> since they appear in the equation and move all terms to the left-side.
					<md>
						<mrow>	y	=\amp\  3\sin(x^2)									</mrow>
						<mrow>	y' 	=\amp\  3\cos(x^2) \cdot 2x	=	6x\cos(x^2)	</mrow>
						<mrow>	y'' =\amp\ 6\cos(x^2) - 12x\sin(x^2)	=	6\cos(x^2) - 12x\sin(x^2)	</mrow>
					</md>
				</p>

				<p>
					Plug in <m>y, y',</m> and <m>y''</m> and simplify.
					<md>
						<mrow> 												
							y' - xy'' - 12x^2\sin(x^2) 	
								=\amp\ 0	
						</mrow>
						<mrow> 
							6x\cos(x^2) - x\left( 6\cos(x^2) - 12x\sin(x^2) \right) - 12x^2\sin(x^2)
								=\amp\ 0																
						</mrow>
						<mrow> 
							\cancel{6x\cos(x^2)} - \cancel{6x\cos(x^2)} - \cancel{12x^2\sin(x^2)} - \cancel{12x^2\sin(x^2)}	
								=\amp\ 0
							</mrow>
						<mrow> 
							0	=\amp\ 0
						</mrow>
					</md>
					Therefore, <m>y= 3\sin(x^2)</m> is a solution to <m>y' - 12x^2\sin(x^2) = xy''.</m>
				</p>
			</solution>

		</example>

		<example>
		
			<statement>
				<p>
					Verify that <m>y = Ce^{-5x^2} + \frac{3}{5}</m> is a solution to the DE
					<me>\frac{dy}{dx} = \big( 2x \big) \big( 3 - 5y \big)</me>
				</p>
			</statement>
		
			<solution>
				<p>
					Working out the left and right hand sides of this DE, we have:
		
					<sidebyside widths="45% 55%" margins="auto" valign="top" halign="center">
						<p>
							<md>
								<mrow> LHS: </mrow>
								<mrow> \frac{dy}{dx}
										=\amp\ \frac{d}{dx}\left( Ce^{-5x^2} + \frac{3}{5} \right)</mrow>
								<mrow> 	=\amp\ Ce^{-5x^2} \cdot \frac{d}{dx}(-5x^2) + 0</mrow>
								<mrow> 	=\amp\ Ce^{-5x^2} \cdot -10x</mrow>
								<mrow> 	=\amp\ -10Cxe^{-5x^2}</mrow>
							</md>
						</p>
						<p>
							<md>
								<mrow> RHS: </mrow>
								<mrow> 	\big(2x\big)\amp\big(3 - 5y\big)</mrow>
								<mrow> 	=\amp\ 2x \left[3 - 5\left(Ce^{-5x^2} + \frac{3}{5}\right) \right]</mrow>
								<mrow> 	=\amp\ 2x \left[ 3 - 5Ce^{-5x^2} - 3 \right]</mrow>
								<mrow> 	=\amp\ 2x \left[-5Ce^{-5x^2}\right]</mrow>
								<mrow> 	=\amp\ -10Cxe^{-5x^2}</mrow>
							</md>
						</p>
					</sidebyside>
				</p>
		
				<p>
					Since <m>LHS = RHS</m>, we have verified that
					<m>y = Ce^{-5x^2} + \frac{3}{5}</m> is a solution to
					<me>\frac{dy}{dx} = \big( 2x \big) \big( 3 - 5y \big)</me>
				</p>
			</solution>
		
		</example>
		
	</subsubsection>

</subsection>