<subsection xmlns:xi="http://www.w3.org/2001/XInclude" xml:id="subsec-if-int-factor"><title> The Integrating Factor </title>

	<introduction>
		<p>
			As mentioned at the end of the previous section, the integrating factor (IF) aims to rewrite the differential equation
			<md>
				<mrow> \frac{dy}{dx} - 2y \amp = 5 </mrow>
			</md>
			into the form
			<md>
				<mrow> \frac{d}{dx}\left[ y \cdot e^{-2x} \right] \amp = 5 e^{-2x} \quad \leftarrow \text{Easy to solve!} </mrow>
			</md>
			and then we integrate both sides with respect to <m>x</m> to free the unknown <m>y</m> from inside the <m>\frac{d}{dx}</m>, so that we can solve for it. However, we have not talked about how the integrating factor gets the differential equation into this form. Luckily, the product rule for deriviatives holds the answer. Therefore, let's start this discussing by reminding ourselves that the product rule is given by
			<me> \frac{d}{dx}[\ f \cdot g\ ] = \frac{d}{dx}[\ f\ ] \cdot g + f \cdot \frac{d}{dx}[\ g\ ]. </me>
		</p>

		<p>
			Ok, the claim is that after a some math the differential equation
			<men xml:id="if_prod_rule_eq1"> \frac{dy}{dx} - 2y = 5 </men>
			can be rewritten as 
			<men xml:id="if_prod_rule_eq2"> \frac{d}{dx}\left[ y \cdot e^{-2x} \right] = 5 e^{-2x}. </men>
			To explain this, it may be easier to work backwards. That is, let's start with <xref ref="if_prod_rule_eq2" /> and see how it may connect back to <xref ref="if_prod_rule_eq1" />. We start by applying the product rule on the left side,
			<mdn>
				<mrow> \frac{d}{dx}[\ y \cdot e^{-2x}\ ] \amp = 5 e^{-2x} </mrow>
				<mrow> \frac{d}{dx}[\ y\ ] \cdot e^{-2x} + y \cdot \frac{d}{dx}[\ e^{-2x}\ ] \amp = 5 e^{-2x} </mrow>
				<mrow> \frac{dy}{dx} \cdot e^{-2x} + y \cdot \left(-2 e^{-2x}\right) \amp = 5 e^{-2x} </mrow>
				<mrow xml:id="if_prod_rule_eq3"> \frac{dy}{dx} \cdot e^{-2x} - 2 y \cdot e^{-2x} \amp = 5 e^{-2x}. </mrow>
			</mdn>
			At this point stop and compare equation <xref ref="if_prod_rule_eq1" /> with the last equation <xref ref="if_prod_rule_eq3" />. Do you see how the two equations are connected?
		</p>
	
		<p>
			You should see that multiplying both sides of <xref ref="if_prod_rule_eq1" /> by <m>e^{-2x}</m> gives you <xref ref="if_prod_rule_eq3" />.
	
		</p>
	
		<p>
			In a nutshell, the integrating factor technique attempts to solve
			<me>y' + P(x)y = Q(x)</me>
			by multiplying both sides by an unknown function, <m>\mu</m>
			<me>\mu y' + \mu P(x)y = \mu Q(x)</me>
			then find a <m>\mu</m> so that the left-hand side can be written as the product rule of <m>\mu</m> and <m>y</m>.
			<me>\US{\large \text{product rule}}{\UB{\mu y' + \mu P(x)y}} = \mu Q(x)</me>
		</p>
	
		<p>
			To clarify, let's look at an example where we know <m>\mu</m>.
		</p>

	</introduction>

	<example xml:id="if-intro-exercise">
		<p> 
			Solve the differential equation, 
			<me>y' + 6y = 1,</me>
			for <m>y</m> by completing the following steps:
			<ol>
				<li>Multiply both sides of the equation by <m>\mu = e^{6x}</m>.</li>
				<li>Rewrite the left-hand side as a product rule of <m>e^{6x}</m> and <m>y</m>.</li>
				<li>Integrate both sides of the equation with respect to <m>x</m>.</li>
				<li>Solve for <m>y</m> as a function of <m>x</m>.</li>
			</ol>
		</p>
	  
		<solution>
			<p>
				1. In this example, we are told that <m>\mu = e^{6x}</m>. We also note that <m>\mu' = 6e^{6x}</m>. Multiplying both sides of the original equation by <m>\mu</m> gives
				<md>
				<mrow>e^{6x} \cdot (y' + 6y) \amp= e^{6x} \cdot 1</mrow>
				<mrow>e^{6x} \cdot y' + e^{6x} \cdot 6y \amp= e^{6x}</mrow>
				<mrow>e^{6x} y' + (6e^{6x}) y \amp= e^{6x}</mrow>
				</md>
				2. Do you see that the left-hand side is the result of using the product rule to find the derivative of the product of <m>\mu = e^{6x}</m> and <m>y</m>?
			<!--
			<sidebyside>
				<tabular halign="center">
				<row>
					<cell><m>\mu</m></cell>
					<cell><m>y'</m></cell>
					<cell></cell>
					<cell><m>\mu'</m></cell>
					<cell><m>y</m></cell>
					<cell></cell>
				</row>
				<row>
					<cell><m>\downarrow</m></cell>
					<cell><m>\downarrow</m></cell>
					<cell></cell>
					<cell><m>\downarrow</m></cell>
					<cell><m>\downarrow</m></cell>
					<cell></cell>
				</row>
				<row>
					<cell><m>e^{6x}</m></cell>
					<cell><m>\!\!y'\!\!</m></cell>
					<cell><m>\!\!+\!\!</m></cell>
					<cell><m>(6e^{6x})</m></cell>
					<cell><m>\!\!y\!\!</m></cell>
					<cell><m>\!\! = e^{6x}</m></cell>
				</row>
				</tabular>
			</sidebyside>
			<me>\frac{d}{dx}\left[e^{6x} y\right] = e^{6x}</me>
			-->
				<md>
				<mrow>\OS{\large \mu\ \cdot\ y' \,+\, \mu'\ \cdot\ y}{\OB{e^{6x} y' + (6e^{6x}) y}} \amp= e^{6x}</mrow>
				</md>
				So this equation can be re-written as
				<md>
				<mrow>\frac{d}{dx}\left[e^{6x} y\right] \amp= e^{6x}.</mrow>
				</md>
				3. Now, integrating both sides (with respect to <m>x</m>) gives
				<md>
				<mrow>\int\frac{d}{dx}\left[e^{6x} y\right] \ dx \amp= \int e^{6x}\ dx</mrow>
				<mrow>e^{6x} y \amp= \frac{1}{6}e^{6x} + C.</mrow>
				</md>
				4. Finally, we get our solution by solving for <m>y</m> (multiply by <m>e^{-6x}</m>), as follows
				<md>
				<mrow>y \amp= \left(\frac{1}{6}e^{6x} + C\right)e^{-6x}</mrow>
				<mrow>y \amp= \frac{1}{6} + Ce^{-6x}.</mrow>
				</md>
			</p>
		</solution>
	</example>
	  
	<p>
		The previous example shows how to solve the equation when you know what <m>\mu</m> is. However, in a real problem, you will have to find <m>\mu</m> first!
	</p>
	  
	<p>
		Let's build on the previous example to try and understand why <m>\mu = e^{6x}</m> worked. It is important to try and think of <m>\mu(x)</m> as the missing part needed to to be consistent with the product rule. That is, the left-side of the equation
	  
		<me>\US{\large \text{product rule}}{\US{\large \text{incomplete}}{\UB{y' + 6y}}} = 1</me>
	  
		is missing a second function needed to be consistent with the product rule. So let's fill-in this missing function by multiplying both sides by <m>\mu</m>,
	  
		<men xml:id="complete-product-rule-eqn">\mu y' + 6 \mu y = \mu.</men>
	  
		Is the left-side, <m>\mu y' + 6 \mu y</m>, equal to <m>\left[\mu y\right]'</m>? Well, not exactly, since taking this derivative shows the difference between these two, namely
	  
		<sidebyside>
			<tabular halign="center">
				<row>
					<cell></cell>
					<cell></cell>
					<cell></cell>
					<cell></cell>
					<cell bottom="minor"></cell>
					<cell></cell>
					<cell></cell>
				</row>
		
				<row>
					<cell halign="right"><m>\DS\left[\mu y\right]'</m></cell>
					<cell><m>=</m></cell>
					<cell><m>\mu y'</m></cell>
					<cell right="minor"><m>+</m></cell>
					<cell bottom="minor" right="minor"><m>\mu'</m></cell>
					<cell><m>y</m></cell>
					<cell></cell>
				</row>
		
				<row>
					<cell></cell>
					<cell></cell>
					<cell></cell>
					<cell></cell>
					<cell><m>\uparrow</m></cell>
					<cell></cell>
					<cell></cell>
				</row>
		
				<row>
					<cell></cell>
					<cell></cell>
					<cell></cell>
					<cell colspan="4"><em>difference</em></cell>
				</row>
		
				<row>
					<cell></cell>
					<cell></cell>
					<cell></cell>
					<cell></cell>
					<cell bottom="minor"><m>\downarrow</m></cell>
					<cell></cell>
					<cell></cell>
				</row>
		
				<row>
					<cell>left-side</cell>
					<cell><m>\rightarrow</m></cell>
					<cell><m>\mu y'</m></cell>
					<cell right="minor"><m>+</m></cell>
					<cell bottom="minor" right="minor"><m>6\mu</m></cell>
					<cell><m>y</m></cell>
				</row>
			</tabular>
		</sidebyside>
	</p>
	  
	<p>
		However, what if <m>\mu</m> was chosen so that <m>\mu' = 6\mu</m>? It turns out that this is exactly how we chose <m>\mu</m>. Finding <m>\mu</m> such that <m>\mu' = 6\mu</m> is itself a differential equation which can be solved using separation of variables. (You may try it yourself first for practice, then look below to see how to solve this DE.)
	</p>
	  
	<p>
		Using separation of variables, solve
		<md>
		  <mrow>\mu' \amp= 6\mu.</mrow>
		</md>
		to get the solution
		  <fn>
			<md>
			  <mrow>\frac{d\mu}{dx} \amp= 6\mu</mrow>
			  <mrow>\frac{1}{\mu}d\mu \amp= 6\ dx</mrow>
			  <mrow>\int\frac{1}{\mu}d\mu \amp= \int 6\ dx</mrow>
			  <mrow>\ln|\mu| \amp= 6x + C</mrow>
			  <mrow>|\mu| \amp= e^{6x + C}</mrow>
			  <mrow>\mu \amp= \pm e^C e^{6x}</mrow>
			  <mrow>\mu \amp= A e^{6x}</mrow>
			</md>
		  </fn>
		<me>\mu = A e^{6x}.</me>
	  
		Since, we only need one <m>\mu</m> to work, we choose <m>A=1</m> for convenience, hence
	  
		<me>\mu = e^{6x}.</me>
	  
		Now you see where the <m>\mu</m> came from in part 1 of <xref ref="if-intro-exercise"/>.  In fact, this example outlines how <m>\mu</m> is found for any first order linear differential equation of the form 
		<men xml:id="EQ-1st-order-de-pre">y' + P(x)y = Q(x).</men>
	</p>

</subsection>