<section xmlns:xi="http://www.w3.org/2001/XInclude"><title> Solving LHCC Equations </title>

	<introduction>
		<p>
			
		</p>
	</introduction>

	<subsection><title> 1st-Order Equations </title>
		
		<p>
			In the previous section, we learned that solutions to Linear Homogeneous Constant Coefficient (LHCC) equations often involve terms of the form <m>e^{rx}</m>. However, not every value of <m>r</m> will work. The correct values of <m>r</m> arise from solving an important algebraic equation, obtained by substituting <m>y = e^{rx}</m> into the differential equation. In this section, we will focus on this process for first-order equations before building up to higher-order cases.
		</p>
		
		<p>
			Let's start with a simple first-order equation:
			<me> y' - 5y = 0 </me>
			We want to find the value of <m>r</m> such that <m>y = e^{rx}</m> is a solution. Substituting <m>y = e^{rx}</m> into the differential equation gives:
			<md>
				<mrow> \left[e^{rx}\right]' - 5 \left[e^{rx}\right] =\amp 0 </mrow>
				<mrow> r e^{rx} - 5 e^{rx} 							=\amp 0 </mrow>
				<mrow> (r - 5) e^{rx} 								=\amp 0 </mrow>
			</md>
			Since <m>e^{rx}</m> is never zero, we must have:
			<md>
				<mrow> r - 5 = 0 \quad \Rightarrow \quad r = 5 </mrow>
			</md>
			This tells us that <m>y = e^{5x}</m> is a solution. Therefore, the general solution is:
			<me> y = c e^{5x} </me>
		</p>
		
		<p>
			The equation <m>r - 5 = 0</m>, which gave us the value of <m>r</m>, is called the <term>characteristic equation</term>. Every LHCC equation has one. The characteristic equation gives us the values of <m>r</m> that we need to construct the general solution.
		</p>
		
		<p>
			Applying the same approach to the general first-order LHCC equation gives us:
			<md>
				<mrow>
					y=e^{rx} \quad\rightarrow\quad
					ay' + by = 0 \quad\Rightarrow\quad a \left[e^{rx}\right]' + b \left[e^{rx}\right]
												=\amp 0
				</mrow>
				<mrow> a r e^{rx} + b e^{rx}	=\amp 0 </mrow>
				<mrow> (ar + b) e^{rx} 			=\amp 0 </mrow>
			</md>
			This results in the characteristic equation and general solution:
			<me> ar + b = 0 \quad \Rightarrow \quad r = -\frac{b}{a} \quad \Rightarrow \quad y = c e^{-\frac{b}{a}x} </me>
		</p>
		
		<p>
			Now, let's apply this method to a couple of examples.
		</p>
		
		<example>
			<p>
				Find the general solution for each LHCC equation.
				<me> 3y' - 9y = 0 \hspace{5em} 5y' = \pi y </me>
			</p>
		
			<solution>
				<p>
					First, rewrite the equations in standard form:
					<me> y' - 3y = 0 \hspace{5em} 5y' - \pi y = 0 </me>
				</p>
				
				<p>
					Now solve the characteristic equations:
					<me> 3r - 9 = 0 \quad \Rightarrow \quad r = 3 \hspace{5em} 5r - \pi = 0 \quad \Rightarrow \quad r = \frac{\pi}{5} </me>
					Thus, the general solutions are:
					<me> y = c e^{3x} \hspace{5em} y = c e^{\frac{\pi}{5}x} </me>
				</p>
			</solution>
		</example>
		
		<p>
			This straightforward method works for any first-order LHCC equation by using the characteristic equation. In the next sections, we'll extend this technique to higher-order equations.
		</p>

		<!-- <xi:include href="./p3-c1-s3-interactives.ptx" /> -->

	</subsection>

	<subsection><title> 2nd-Order Equations </title>

		<p>
			Now that we've mastered first-order LHCC equations, it's time to explore second-order LHCC equations. These are slightly more complex but follow a similar approach. We'll see how the characteristic equation helps us find solutions and look at the different cases that arise depending on the nature of the roots.
		</p>

		<p>
			Consider the following second-order equation:
			<men xml:id="second-order-lhcc-intro-de"> y'' - 5y' + 6y = 0 </men>
			Substituting <m>y = e^{rx}</m> into this equation, we get:
			<md>
				<mrow> \left[e^{rx}\right]'' - 5 \left[e^{rx}\right]' + 6 \left[e^{rx}\right] =	\amp\ 0							</mrow>
				<mrow> r^2 e^{rx} - 5r e^{rx} + 6 e^{rx} =										\amp\ 0							</mrow>
				<mrow> (r^2 - 5r + 6) e^{rx} =													\amp\ 0 \qquad (e^{rx} \ne 0)	</mrow>
				<mrow> \text{characteristic equation} \rightarrow \qquad r^2 - 5r + 6 =			\amp\ 0							</mrow>
				<mrow> r_1 = 2, \quad  r_2 =													\amp\ 3							</mrow>
			</md>.
			Therefore, <m>y = e^{2x}</m> and <m>y = e^{3x}</m> are solutions, and the general solution is the combination of these two:
			<me> y = c_1 e^{2x} + c_2 e^{3x} </me>.
		</p>

		<p>
			In general, for any second-order LHCC equation of the form:
			<men xml:id="second-order-lhcc-de"> a y'' + b y' + c y = 0 </men>
			The characteristic equation is:
			<men xml:id="second-order-lhcc-characteristic-equation"> a r^2 + b r + c = 0 </men>
			This quadratic equation will have two solutions, which could be either real or complex. The general solution depends on the nature of these solutions, and we will now explore the different  cases. Before moving on, we highly recommend taking a minute to review some <xref ref="solving-the-quadratic-equation" text="custom">concepts related to solving quadratic equations</xref>.
		</p>

		<p>
			Let <m>r_1</m> and <m>r_2</m> be the solutions to the characteristic equation. When <m>r_1 \ne r_2</m>, the general solution is:
			<men xml:id="second-order-lhcc-solution-r1-notequalto-r2"> y = c_1\, e^{r_1 x} + c_2\, e^{r_2 x} </men>
			However, if <m>r_1 = r_2</m>, the terms combine into like terms,
			<me>
				y = c_1\, e^{r_1 x} + c_2\, e^{r_2 x} = \color{blue}\us{ \large \text{like terms}}{\us{\nwarrow}{\ul{c_1\, e^{r_1 x}}} + \us{\nearrow}{\ul{c_2\, e^{r_1 x}}}} = (\us{C}{\ub{c_1 + c_2}})\, e^{r_1 x}
			</me>,
			which is an incomplete solution. To fix this, we multiply the second term by <m>x</m>, resulting in the correct general solution:
			<fn>
				<p>
					See <xref ref="tba"/> for an outline of why the extra <m>x</m> is required in the general solution of a second order LHCC equation when <m>r_1=r_2</m>.
				</p>
			</fn>
			<me> y = c_1\, e^{r_1 x} + c_2\, x e^{r_1 x} </me>
		</p>

		<theorem xml:id="tba"><title> Why do add <m>x</m> to Some Solutions? </title>
			<statement>
				<p>
					<exercise>
						<statement>
							<p> Show why <m>x</m> is needed in the general solution for repeated roots of the CE </p>
						</statement>
						<solution>
							<p>
								
							</p>
						</solution>
						<answer>
							<p>
								
							</p>
						</answer>
					</exercise>
				</p>
			</statement>
		</theorem>

		<p>
			Although, the above explanation covers the situation when <m>r_1</m> and <m>r_2</m> are equal or not, we will split the <m>r_1 \ne r_2</m> case into <xref ref="second-order-lhcc-complex-case" text="custom">two cases that treat real or complex values separately</xref>. The three cases are summarized below.
		</p>

		<theorem xml:id="second-order-lhcc-complex-case"><title> 2nd Order LHCC Complex Case 3 </title>

			<p>
				The following explains how <xref ref="lhcc-case-3" text="title"/> comes directly from <xref ref="lhcc-case-1" text="title"/>.
			</p>

			<p>
				Since <m>r_1</m> and <m>r_2</m> are complex, they can be written as
				<me>
					r_1 = \alpha + \beta i \quad \text{and} \quad r_2 = \alpha - \beta i
				</me>.
				Substituting these into <xref ref="second-order-lhcc-solution-r1-notequalto-r2"/>, using <xref ref="eulers-formula" text="title"/>, the <xref ref="evenodd-cos" text="custom"> even property of cosine </xref> and <xref ref="evenodd-sin" text="custom"> odd property of sine </xref>, we can rewrite the general solution as
				<md>
					<mrow> y\  &amp;= c_1 e^{(\alpha + \beta i) x} + c_2 e^{(\alpha - \beta i) x} </mrow>
					<mrow> &amp;= c_1 e^{\alpha x} e^{i \beta x} + c_2 e^{\alpha x} e^{-i \beta x} </mrow>
					<mrow> &amp;= e^{\alpha x} \Big{[}c_1 e^{i \beta x} + c_2 e^{-i \beta x}\Big{]} </mrow>
					<mrow> &amp;= e^{\alpha x} \Big{[}c_1 (\cos(\beta x) + i\sin(\beta x)) + c_2 (\cos(-\beta x) + i\sin(-\beta x))\Big{]} </mrow>
					<mrow> &amp;= e^{\alpha x} \Big{[}c_1 \cos(\beta x) + i c_1 \sin(\beta x) + c_2 \cos(-\beta x) + i c_2 \sin(-\beta x)\Big{]} </mrow>
					<mrow> &amp;= e^{\alpha x} \Big{[}c_1 \cos(\beta x) + i c_1 \sin(\beta x) + c_2 \cos(\beta x) - i c_2 \sin(\beta x)\Big{]} </mrow>
					<mrow> &amp;= e^{\alpha x} \Big{[}(\us{c_1}{\ub{c_1 + c_2}}) \cos(\beta x) + \us{c_2}{\ub{i (c_1 - c_2)}} \sin(\beta x)\Big{]} </mrow>
					<mrow> &amp;= e^{\alpha x} (c_1 \cos(\beta x) + c_2 \sin(\beta x)) </mrow>
				</md>.
			</p>
		</theorem>

		<assemblage><title> Summary of Cases </title>
			<p>
				Let <m>r_1</m> and <m>r_2</m> be the solutions of the characteristic equation associated with the second-order LHCC equation. The general solution is:
				<dl width="wide">
					<li xml:id="lhcc-case-1"><title>Case 1 (real &amp; <m>\ne</m>)</title>
						<m>
							\ds y = c_1 e^{r_1 x} + c_2 e^{r_2 x} \quad (r_1 \ne r_2)
						</m>
					</li>
					<li xml:id="lhcc-case-2"><title>Case 2 (real &amp; <m>=</m>)</title>
						<m>
							\ds y = (c_1 + c_2 x) e^{r_1 x} \quad (r_1 = r_2)
						</m>
					</li>
					<li xml:id="lhcc-case-3"><title>Case 3 (complex)</title>
						<line>
							<m>
								\ds y = e^{\alpha x} (c_1 \cos(\beta x) + c_2 \sin(\beta x))
							</m>
						</line>
						<line>
							<m>
								\ds (r = \alpha \pm i\beta \implies r_1 = \alpha + i\beta, \ r_2 = \alpha - i\beta)
							</m>
						</line>
					</li>
				</dl>
			</p>
		</assemblage>

		<p>
			Let's now practice solving some second-order LHCC equations.
		</p>

		<example>


			<p>
				Find the general solutions for each LHCC equation.
				<sidebyside widths="30% 70%">
					<p>
						<m> y'' - 5y' + 6y = 0 </m>
					</p>
					<p>
						<solution>
							<p>
								First, write down and solve the characteristic equation:
								<md>
									<mrow> r^2 - 5r + 6 =\amp\ 0 </mrow>
									<mrow> (r-2)(r-3) =\amp\ 0 </mrow>
									<mrow> r_1 = 2 \quad \text{and} \quad r_2 =\amp\ 3 </mrow>
								</md>.
								Since <m>r_1</m> and <m>r_2</m> are real and <m>r_1 \ne r_2</m>, we are in <xref ref="lhcc-case-1" text="custom">Case 1</xref>. Therefore, the general solution is:
								<me> y = c_1 e^{2x} + c_2 e^{3x} </me>.
							</p>
						</solution>
					</p>
				</sidebyside>
			</p>
			
			<p>
				<sidebyside widths="30% 70%">
					<p>
						<m> y'' + 4y' + 4y = 0 </m>
					</p>

					<p>
						<solution>
							<p>
								The characteristic equation is:
								<md>
									<mrow> r^2 + 4r + 4 =\amp\ 0 </mrow>
									<mrow> (r+2)(r+2) =\amp\ 0 </mrow>
									<mrow> r_1 = -2 \quad \text{and} \quad r_2 =\amp\ -2 \quad \leftarrow <xref ref="lhcc-case-2" text="custom">Case 2</xref> </mrow>
								</md>.
								Therefore, the general solution is:
								<me> y = (c_1 + c_2 x) e^{-2x} </me>.
							</p>
						</solution>
					</p>
				</sidebyside>
			</p>

			<p>
				<sidebyside widths="30% 70%">
					<p>
						<m> y'' + 2y' + 5y = 0 </m>
					</p>
			
					<p>
						<solution>
							<p>
								The characteristic equation in this problem is:
								<md>
									<mrow> r^2 + 2r + 5 = 0\amp </mrow>
									<mrow> r = \us{\alpha}{\boxed{-1}} \pm \us{\beta}{\boxed{2}}i \amp\ \quad \leftarrow <xref ref="lhcc-case-3" text="custom">Case 3</xref> </mrow>
								</md>.
								Here, <m>\alpha = -1</m> and <m>\beta = 2</m>. So the general solution is:
								<me> y = e^{-x} (c_1 \cos(2x) + c_2 \sin(2x)) </me>.
							</p>
						</solution>
					</p>
				</sidebyside>
			</p>
		</example>

		<!-- <xi:include href="./p3-c1-s4-interactives.ptx" /> -->

	</subsection>

	<subsection><title> Higher-Order Equations </title>

		<p>
			Solving higher-order linear homogeneous constant coefficient (LHCC) equations is an extension of the methods used for second-order equations. The basic strategy remains the same: solve the characteristic equation, then construct the general solution. However, for higher-order equations, the characteristic equation is a higher-degree polynomial, which can make finding the solutions more challenging.
		</p>

		<definition xml:id="def-characteristic-equation">
			<title><em>LHCC Characteristic Equation</em></title>
			<statement>
				<p>
					The <term>characteristic equation</term> of an <m>n</m>-th order LHCC equation
					<me>a_n\ y^{(n)} + a_{n-1}\ y^{(n-1)} + \cdots + a_1\ y' + a_0\ y = 0</me>
					is the <m>n</m>-th degree polynomial
					<fn>
						<xref ref="characteristic-eqn-details" text="custom">Click here for an explanation.</xref>
					</fn>
					<me>a_n\ r^n + a_{n-1}\ r^{n-1} + \cdots + a_1 r + a_0 = 0</me>.
					The solutions to this polynomial, <m>r_1, r_2, \dots r_n</m>, correspond to the roots that determine the form of the general solution.
				</p>
			</statement>
		</definition>

		<theorem xml:id="characteristic-eqn-details"><title/>
			<p>
				To find the characteristic equation, we substitute <m>y = e^{rx}</m> into the <m>n</m>-th order <xref ref="lhcc-equation" text="custom">LHCC equation</xref> and solve for <m>r</m>. Doing this gives us
				<md>
					<mrow>	
						a_n\ \left[e^{rx}\right]^{(n)} + \cdots + a_2\ \left[e^{rx}\right]'' + a_1\ \left[e^{rx}\right]' + a_0\ e^{rx} =\amp\ 0
					</mrow>
					<mrow>	a_n\ r^n e^{rx} + \cdots + a_2\ r^2 e^{rx} + a_1\ r e^{rx} + a_0\ e^{rx} =\amp\ 0 </mrow>
					<mrow>	\left(a_n\ r^n + \cdots + a_2\ r^2 + a_1\ r + a_0\right)e^{rx}  =\amp\ 0 </mrow>
				</md>.
				Since <m>e^{rx}</m> is never zero, we must have
				<me>
					a_n\ r^n + \cdots + a_2\ r^2 + a_1\ r + a_0 = 0
				</me>
				which is an <m>n</m>-th order polynomial in <m>r</m>.
			</p>
		</theorem>
		
		<p>
			In general, the characteristic equation will have <m>n</m> roots, which may be real or complex and may also include repeated roots. Each root of the characteristic equation leads to a term in the general solution of the LHCC. Examples in the table below illustrate the process of constructing these general solutions based on the different types of roots.
		</p>

		<table xml:id="higher-order-lhcc-general-solution-examples"><title>Examples of LHCC General Solutions</title>
			<tabular left="minor" right="minor" top="minor" bottom="minor" halign="center">
				<row>
					<cell>
						<line>Characteristic Equation</line>
						<line>Solutions</line>
					</cell>
					<cell>General Solution</cell>
				</row>
				<row>
					<cell>
						<line><m>r = 3, -3, 5.3</m></line>
						<line><em>(3rd order)</em></line>
					</cell>
					<cell><me>c_1e^{3t} + c_2e^{-3t} + c_3e^{5.3t}</me></cell>
				</row>
				<row>
					<cell>
						<line><m>r = 6 \pm i\sqrt{7.7}, 0</m></line>
						<line><em>(3rd order)</em></line>
					</cell>
					<cell><me>e^{6t}\left(c_1\sin(\sqrt{7.7}t) + c_2\cos(\sqrt{7.7}t)\right) + c_3</me></cell>
				</row>
				<row>
					<cell>
						<line><m>r = -4 \text{ (triple)}, 5.3</m></line>
						<line><em>(4th order)</em></line>
					</cell>
					<cell><me>(c_1t^2 + c_2t + c_3)e^{-4t} + c_4e^{5.3t}</me></cell>
				</row>
				<row>
					<cell>
						<line><m>r = \pm \frac{i}{2}, 2 \pm i</m></line>
						<line><em>(4th order)</em></line>
					</cell>
					<cell><me>c_1\sin\left(\frac{t}{2}\right) + c_2\cos\left(\frac{t}{2}\right) + e^{2t}(c_3\sin t + c_4\cos t)</me></cell>
				</row>
				<row>
					<cell>
						<line><m>r = 0 \text{ (double)}, 3 \text{ (5-repeats)}</m></line>
						<line><em>(7th order)</em></line>
					</cell>
					<cell><me>c_1t + c_2 + (c_3t^4 + c_4t^3 + c_5t^2 + c_6t + c_7)e^{3t}</me></cell>
				</row>
				<row>
					<cell>
						<line><m>r = \pm i, \pi \text{ (double)}, 5</m></line>
						<line><em>(5th order)</em></line>
					</cell>
					<cell><me>c_1\sin t + c_2\cos t + (c_3t + c_4)e^{\pi t} + c_5e^{5t}</me></cell>
				</row>
			</tabular>
		</table>

		<p>
			As the table demonstrates, constructing the general solution of an LHCC equation is systematic once you have the roots of the characteristic equation. However, solving higher-order polynomial equations by hand can be difficult. The next example shows a few algebra techniques you can use to handle higher degree equations.
		</p>

		<example>

			<p>
				Solve the following characteristic equations.
				<ol>
					<li> <m> 4 r^2 - 9 = 0 </m> </li>
					<li> <m> r^3 + 3 r^2 - 4 r = 0 </m> </li>
					<li> <m> r^5 + 10 r^4 = 0 </m> </li>
					<li> <m> r^5 - 4 r^3 = 0 </m> </li>
					<li> <m> r^4 - 25 = 0 </m> </li>
					<li> <m> r^4 - 5r^2 + 4 = 0 </m> </li>
				</ol>
			</p>

			<solution>
				<p>
					Note: DoS = Difference of Squares.
					<ol>
						<li>
							<p>
								<tabular>
									<row>
										<cell><m> 4 r^2 - 9 = 0 </m></cell>
										<cell> <m>\leftarrow</m> DoS </cell>
									</row>
									<row>
										<cell><m> (2 r + 3)(2 r - 3) = 0 </m></cell>
										<cell/>
									</row>
									<row>
										<cell><m> 2 r + 3 = 0, \quad 2 r - 3 = 0 </m></cell>
										<cell></cell>
									</row>
									<row>
										<cell><m> \ds r_1 = -\frac32, \quad r_2 = \frac32 </m></cell>
										<cell></cell>
									</row>
								</tabular>
							</p>
						</li>

						<li>
							<p>
								<tabular>
									<row>
										<cell><m> r^3 + 3 r^2 - 4 r = 0 </m></cell>
										<cell> <m>\leftarrow r </m> common </cell>
									</row>
									<row>
										<cell><m> r\ (r^2 + 3 r - 4) = 0 </m></cell>
										<cell/>
									</row>
									<row>
										<cell><m> r\ (r + 4)(r - 1) = 0 </m></cell>
										<cell></cell>
									</row>
									<row>
										<cell><m> \ds r_1 = 0, \quad r_2 = -4, \quad r_3 = 1 </m></cell>
										<cell></cell>
									</row>
								</tabular>
							</p>
						</li>
						
						<li>
							<p>
								<tabular>
									<row>
										<cell><m> r^5 + 10 r^4 = 0 </m></cell>
										<cell> <m>\leftarrow r^4 </m> common </cell>
									</row>
									<row>
										<cell><m> r^4\ (r + 10) = 0 </m></cell>
										<cell/>
									</row>
									<row>
										<cell><m> \ds r_1 = 0\ (\text{4 repeats}), \quad r_2 = -10 </m></cell>
										<cell></cell>
									</row>
								</tabular>
							</p>
							<p>
								<em> Technically, <m>r^4 = (r-0)^4</m> and represents 4 repeated factors. </em>
							</p>
						</li>

						<li>
							<p>
								<tabular>
									<row>
										<cell><m> r^5 - 4 r^3 = 0 </m></cell>
										<cell> <m>\leftarrow</m> common </cell>
									</row>
									<row>
										<cell><m> r^3\ (r^2  - 4) = 0 </m></cell>
										<cell> <m>\leftarrow</m> DoS </cell>
									</row>
									<row>
										<cell><m> r^3\ (r + 2)(r - 2) = 0 </m></cell>
										<cell/>
									</row>
									<row>
										<cell><m> \ds r_1 = 0\ (\text{3 repeats}), \quad r_2 = -2, \quad r_3 = 2 </m></cell>
										<cell></cell>
									</row>
								</tabular>
							</p>
						</li>

						<li>
							<p>
								<tabular>
									<row>
										<cell><m> r^4 - 25 = 0 </m></cell>
										<cell> <m>\leftarrow</m> DoS </cell>
									</row>
									<row>
										<cell><m> (r^2 + 5)(r^2  - 5) = 0 </m></cell>
										<cell> <m>\leftarrow</m> DoS </cell>
									</row>
									<row>
										<cell><m> (r^2 + 5)(r - \sqrt{5})(r + \sqrt{5}) = 0 </m></cell>
										<cell/>
									</row>
									<row>
										<cell><m> r^2 + 5 = 0, \quad r - \sqrt{5} = 0, \quad r + \sqrt{5} = 0 </m></cell>
										<cell></cell>
									</row>
									<row>
										<cell><m> \ds r_1 = -i\sqrt{5}, \quad r_2 = i\sqrt{5}, \quad r_3 = -\sqrt{5}, \quad r_4 = \sqrt{5} </m></cell>
										<cell></cell>
									</row>
								</tabular>
							</p>
						</li>

						<li>
							<p>
								<md>
									<mrow> r^4 - 5r^2 + 4 = 0 </mrow>
								</md>.
								Let <m>u = r^2</m>, then we can rewrite the equation as:
								<md>
									<mrow> u^2 - 5u + 4 = 0 </mrow>
								</md>.
								Solving for <m>u</m>, we get:
								<md>
									<mrow> u = 1, \quad u = 4 </mrow>
								</md>.
								Thus, <m>r^2 = 1</m> gives <m>r = \pm 1</m>, and <m>r^2 = 4</m> gives <m>r = \pm 2</m>. The general solution is:
								<me> y = c_1 e^{x} + c_2 e^{-x} + c_3 e^{2x} + c_4 e^{-2x} </me>.
							</p>
						</li>
					</ol>
				</p>
			</solution>
		</example>

		<p>
			These factoring techniques useful, but they only apply to specific forms of polynomials and it is unlikely that you will be lucky enough to encounter such forms in practice. Therefore, it is reasonable to use technology to aid you with these tyes of problems. Many software tools are available and you are encouraged to use any that you are familiar with.
		</p>

		<example>

			<p>
				Find the general solution to the LHCC equations
				<ol>
					<li> <m> y''' - 6y'' + 11y' - 6y = 0 </m> </li>
					<li> <m> 2 y^{(4)} + 9 y''' + y'' - 21 y' + 9 y  = 0 </m> </li>
				</ol>
				using the <xref ref="poly-factor-p" text="title"/>.
			</p>

			<theorem xml:id="poly-factor-p"><title>Polynomial Factoring Calculator</title>
				<figure xml:id="figure-pp">
					<caption>Type in any polynomial of <m>r</m>. Use <q><m>*</m></q> for multiplication. If the polynomial has rational roots, it will show the factors.</caption>
					<interactive xml:id="poly-factor" platform="sage" width="86%" aspect="3.2:1">
						<slate surface="sage">
							r = var('r')
							r = PolynomialRing(RationalField(), 'r').gen()
							F = 'r^2 - 2*r - 8'
							P = r^2 - 2*r - 8
							@interact
							def _(ce = input_box(P, label="	Polynomial:", type=str, width=30)):
								ce_poly = sage_eval('lambda r: ' + ce)
								pretty_print( html( r'Polynomial: $ %s $'%latex(ce_poly(r) ) ) )
								pretty_print( html( r'Factored Polynomial: $ %s $'%latex(ce_poly(r).factor()) ) )
						</slate>
					</interactive>
				</figure>
			</theorem>

			<solution>
				<p>
			<ol>
					<li>
						<p>
							First, write down the characteristic equation:
							<md>
								<mrow> r^3 - 6r^2 + 11r - 6 = 0 </mrow>
							</md>.
							Plugging this into to the factoring tool shows that it factors as <m> (r-3)(r-2)(r-1) </m>.	Solving for <m>r</m>, we get
							<md>
								<mrow> r = 1, \quad r = 2, \quad r = 3 </mrow>
							</md>.
							Therefore, the general solution is:
							<me> y = c_1 e^{x} + c_2 e^{2x} + c_3 e^{3x} </me>.
						</p>
					</li>
					<li>
						<p>
							The characteristic equation is:
							<me>
								9 r^5 - 4 r^4 + r + 10 = 0
							</me>
							which is challenging to solve by hand. However, typing it into factoring tool above shows that it can be factored as
							<me>
								2\left(r+3\right)^2 \left(r-1\right) \left(r-\frac12\right) = 0
							</me>,
							which gives the solutions
							<me>
								r = -3, \quad r = -3, \quad r = 1, \quad r = \frac12
							</me>.
							Therefore, the general solution is:
							<me>
								y = (c_1x + c_2) e^{-3x} + c_3 e^{x} + c_4 e^{\frac12 x}
							</me>.
						</p>
					</li>
				</ol>
				
				</p>
			</solution>
		</example>
		
		<p>
			Besides factoring software, another options is to use numerical solvers. The next example illustrates this.
		</p>
		
		<example>
			<p>
				Consider the fifth-order LHCC equation:
				<me> y^{(5)} - 4y''' + 3y'' - y = 0 </me>.
			</p>
			<solution>
				<p>
					The characteristic equation is:
					<me> r^5 - 4r^3 + 3r^2 - 1 = 0 </me>.
					Solving this polynomial equation analytically is challenging, so we use a numerical solver (<url href="https://www.wolframalpha.com/input?i=r%5E5-4*r%5E3%2B3*r%5E2-1">Wolfram Alpha</url>). This equation has five roots. Three are real:
					<me> r_1 \approx -2.29, \quad r_2 \approx -0.46, \quad r_3 \approx 1.52, </me>
					and two are complex:
					<me> r_4 \approx 0.61 + 0.5i, \quad r_5 \approx 0.61 - 0.5i </me>.
					The general solution, incorporating these roots, is:
					<md>
						<mrow> y = c_1 e^{-2.29x} + c_2 e^{-0.46x}	+\amp\ c_3 e^{1.52x}								</mrow>
						<mrow> 										+\amp\ e^{0.61x} (c_4 \cos(0.5x) + c_5 \sin(0.5x))	</mrow>
					</md>.
					<me>y = c_1e^{-2.29t} + c_2e^{-0.46t} + c_3e^{1.52t} + e^{0.61t}(c_4\cos(0.5t) + c_5\sin(0.5t))</me>.
				</p>
			</solution>
		</example>
		
		<p>
			By recognizing the nature of the roots and utilizing appropriate technology for solving polynomial equations, we can tackle higher-order LHCC equations with confidence.
		</p>

		<!-- <xi:include href="./p3-c1-s5-interactives.ptx" /> -->

	</subsection>

	<conclusion>
		<p>
			
		</p>
	</conclusion>

</section>