<exercises><title> Warm-ups &amp; Drills </title>

	<exercise label="drill-identifying-lhcc-all"><title> Identifying LHCC Equations </title>

		<task label="drill-identifying-lhcc-1"><title> <term>Identify the Linear Equations</term> </title>
			<statement>
				<p>
					Click on the equations that are linear.
				</p>
			</statement>

			<areas>
				<tabular>
					<row>
						<cell correct="yes"><area>	<m>y'' + 3y' - 2y = 0</m>		</area></cell><cell/>
						<cell correct="no"><area>	<m>y' + y^2 = 5</m>				</area></cell><cell/>
						<cell correct="yes"><area>	<m>x^2 y'' - 4x y' + 6y = 0</m>	</area></cell>
					</row>
					<row><cell/></row>
					<row>
						<cell correct="no"><area>	<m>y'' + y y' = \sin x</m>	</area></cell><cell/>
						<cell correct="yes"><area>	<m>y' + 4xy = 0</m>			</area></cell><cell/>
						<cell correct="no"><area>	<m>y'' + \cos(y) = x</m>	</area></cell>
					</row>
					<row><cell/></row>
					<row>
						<cell correct="yes"><area>	<m>y''' - 2y' + y = e^x</m>	</area></cell><cell/>
						<cell correct="yes"><area>	<m>y' + x = 0</m>			</area></cell><cell/>
						<cell correct="yes"><area>	<m>3y''' + y' - 3y = 0</m>	</area></cell>
					</row>
					<row><cell/></row>
				</tabular>
			</areas>

			<feedback>
				<p>
					Remember, a linear equation cannot contain products or compositions of <m> y </m> and its derivatives.
				</p>
			</feedback>
		</task>

		<task label="drill-identifying-lhcc-2"><title> <term>Identify the Linear Homogeneous Equations</term> </title>
			<statement>
				<p>
					Click on the linear and homogeneous equations.
				</p>
			</statement>
			<areas>
				<tabular>
					<row>
						<cell correct="yes"><area>	<m>y'' + 3y' - 2y = 0</m>		</area></cell><cell/>
						<cell correct="no"><area>	<m>y' + y^2 = 5</m>				</area></cell><cell/>
						<cell correct="yes"><area>	<m>x^2 y'' - 4x y' + 6y = 0</m>	</area></cell>
					</row>
					<row><cell/></row>
					<row>
						<cell correct="no"><area>	<m>y'' + y y' = \sin x</m>	</area></cell><cell/>
						<cell correct="yes"><area>	<m>y' + 4xy = 0</m>			</area></cell><cell/>
						<cell correct="no"><area>	<m>y'' + \cos(y) = x</m>	</area></cell>
					</row>
					<row><cell/></row>
					<row>
						<cell correct="no"><area>	<m>y''' - 2y' + y = e^x</m>	</area></cell><cell/>
						<cell correct="no"><area>	<m>y' + x = 0</m>			</area></cell><cell/>
						<cell correct="yes"><area>	<m>3y''' + y' - 3y = 0</m>	</area></cell>
					</row>
					<row><cell/></row>
				</tabular>
			</areas>
			<feedback>
				<p>
					Remember, a linear equation cannot contain products or compositions of <m> y </m> and its derivatives.
				</p>
			</feedback>
		</task>

		<task label="drill-identifying-lhcc-3"><title> <term>Identify the Linear Constant Coefficient Equations</term> </title>
			<statement>
				<p>
					Click on the linear equations with constant coefficients.
				</p>
			</statement>
			<areas>
				<tabular>
					<row>
						<cell correct="yes"><area>	<m>y'' + 3y' - 2y = 0</m>		</area></cell><cell/>
						<cell correct="no"><area>	<m>y' + y^2 = 5</m>				</area></cell><cell/>
						<cell correct="no"><area>	<m>x^2 y'' - 4x y' + 6y = 0</m>	</area></cell>
					</row>
					<row><cell/></row>
					<row>
						<cell correct="no"><area>	<m>y'' + y y' = \sin x</m>	</area></cell><cell/>
						<cell correct="no"><area>	<m>y' + 4xy = 0</m>			</area></cell><cell/>
						<cell correct="no"><area>	<m>y'' + \cos(y) = x</m>	</area></cell>
					</row>
					<row><cell/></row>
					<row>
						<cell correct="yes"><area>	<m>y''' - 2y' + y = e^x</m>	</area></cell><cell/>
						<cell correct="yes"><area>	<m>y' + x = 0</m>			</area></cell><cell/>
						<cell correct="yes"><area>	<m>3y''' + y' - 3y = 0</m>	</area></cell>
					</row>
					<row><cell/></row>
				</tabular>
			</areas>
			<feedback>
				<p>
					Remember, a linear equation cannot contain products or compositions of <m> y </m> and its derivatives.
				</p>
			</feedback>
		</task>

		<task label="drill-identifying-lhcc-4"><title> <term>Identify the LHCC Equations</term> </title>
			<statement>
				<p>
					Click on the LHCC equations.
				</p>
			</statement>
			<areas>
				<tabular>
					<row>
						<cell correct="yes"><area>	<m>y'' + 3y' - 2y = 0</m>		</area></cell><cell/>
						<cell correct="no"><area>	<m>y' + y^2 = 5</m>				</area></cell><cell/>
						<cell correct="no"><area>	<m>x^2 y'' - 4x y' + 6y = 0</m>	</area></cell>
					</row>
					<row><cell/></row>
					<row>
						<cell correct="no"><area>	<m>y'' + y y' = \sin x</m>	</area></cell><cell/>
						<cell correct="no"><area>	<m>y' + 4xy = 0</m>			</area></cell><cell/>
						<cell correct="no"><area>	<m>y'' + \cos(y) = x</m>	</area></cell>
					</row>
					<row><cell/></row>
					<row>
						<cell correct="no"><area>	<m>y''' - 2y' + y = e^x</m>	</area></cell><cell/>
						<cell correct="no"><area>	<m>y' + x = 0</m>			</area></cell><cell/>
						<cell correct="yes"><area>	<m>3y''' + y' - 3y = 0</m>	</area></cell>
					</row>
					<row><cell/></row>
				</tabular>
			</areas>
			<feedback>
				<p>
					Remember, a linear equation cannot contain products or compositions of <m> y </m> and its derivatives.
				</p>
			</feedback>
		</task>

	</exercise>

	<exercise label="drill-characteristic-equation-all"><title> Characteristic Equations </title>
		<task label="drill-characteristic-equation-1"><title> <term>Differential Equation <m>\to</m> Characteristic Equation</term> </title>
			<introduction>
				<p>
					Give the characteristic equation corresponding to each differential equation below.
				</p>
			</introduction>

			<webwork>
				<pg-code>
					Context('ImplicitEquation');
					Context()->{error}{msg}{"Can't find any solutions to your equation"} = ' ';
					Context()->{error}{msg}{"Can't generate enough valid points for comparison"} =
						' ';
					Context()->variables->add(r=>'Real');
					$diff_eqn_A = "y'' + 5y' - y = 0";
					$char_eqn_A = ImplicitEquation("r^2 + 5*r - 1 = 0");

					$diff_eqn_B = "w''' - 7.1w'' + 0.1w = 0";
					$char_eqn_B = ImplicitEquation("r^3 - 7.1*r^2 + 0.1 = 0");

					$diff_eqn_C = "2 p'' + 5p' = 0";
					$char_eqn_C = ImplicitEquation("2*r^2 + 5*r = 0");
				</pg-code>

				<statement>
					<p>
						<m>\displaystyle <var name="$diff_eqn_A" /> \hspace{4.2em}\to\quad </m> <var name="$char_eqn_A" width="30" />
					</p>
					<p>
						<m>\displaystyle <var name="$diff_eqn_B" /> \quad\to\quad </m> <var name="$char_eqn_B" width="30" />
					</p>
					<p>
						<m>\displaystyle <var name="$diff_eqn_C" /> \hspace{5.3em}\to\quad </m> <var name="$char_eqn_C" width="30" />
					</p>
					<p>
						<em>Use <m>r</m> for the variable in your answer. Don't forget the <q><m>=</m></q> sign.</em>
					</p>
				</statement>
			</webwork>
		</task>

		<task label="drill-characteristic-equation-2"><title> <term>Factor the Characteristic Equation</term> </title>
			<introduction>
				<p>
					Give the characteristic equation corresponding to each differential equation below.
				</p>
			</introduction>

			<webwork>
				<pg-code>
					#  Vertex form
					Context("Numeric");
					Context()->variables->add(r=>'Real');

					$r1_A = random(-1, 1, 2) * random(1, 4, 1);
					$r2_A = random(-1, 1, 2) * random(5, 9, 1);
					$expanded_A = Compute("r^2 - ($r1_A + $r2_A) r + ($r1_A * $r2_A)")->reduce;
					$factored_A_str = "(r - $r1_A)(r - $r2_A)";

# (r+2)(r-8) = r^2 - 6r - 16
					$r1_B = random(-1, 1, 2) * random(1, 4, 1);
					$r2_B = random(-1, 1, 2) * random(5, 9, 1);
					$expanded_B = Compute("r^3 - ($r1_B + $r2_B) r^2 + ($r1_B * $r2_B) r")->reduce;
					$factored_B_str = "r(r - $r1_B)(r - $r2_B)";

# r(r-6)(r-4) = r^3 - 10r^2 + 24r
					$r1_C = random(1, 2, 1);
					$r2_C = random(3, 3, 1);
					$expanded_C = Compute("r^4 - ($r1_C**2 + $r2_C**2) r^2 + ($r1_C * $r2_C)**2")->reduce;
					$factored_C_str = "(r - $r1_C)(r + $r1_C)(r - $r2_C)(r + $r2_C)";

# (r-1)(r+1)(r-3)(r+3) = (r^2-1)(r^2-9) = r^4 - 10r^2 + 9
					$r1_D = random(-1, 1, 2) * random(4, 6, 1);
					$r2_D = random(1, 3, 1);
					$expanded_D = Compute("r^3 - $r1_D r^2 - $r2_D**2 r + $r1_D * $r2_D**2")->reduce;
					$factored_D_str = "(r - $r1_D)(r - $r2_D)(r + $r2_D)";

# (r-4)(r+1)(r-1) = (r-4)(r^2-1) = r^3 - 4r^2 - r + 4
					Context("PolynomialFactors-Strict");
					Context()->flags->set(singleFactors => 0);
					LimitedPowers::OnlyIntegers(
						minPower => 0,
						maxPower => 1,
						message  => "either 0 or 1 for each factor",
					);
					Context()->variables->add(r=>'Real');

					$factored_A = Compute($factored_A_str)->reduce;
					$factored_B = Compute($factored_B_str)->reduce;
					$factored_C = Compute($factored_C_str)->reduce;
					$factored_D = Compute($factored_D_str)->reduce;

				</pg-code>

				<statement>
					<p>
						<m>\displaystyle <var name="$expanded_A" />\ =\ </m> <var name="$factored_A" width="35" />
					</p>
					<p>
						<m>\displaystyle <var name="$expanded_B" />\ =\ </m> <var name="$factored_B" width="35" />
					</p>
					<p>
						<m>\displaystyle <var name="$expanded_C" />\ =\ </m> <var name="$factored_C" width="35" />
					</p>
					<p>
						<m>\displaystyle <var name="$expanded_D" />\ =\ </m> <var name="$factored_D" width="35" />
					</p>
					<p>
						<em>Fully factor each as far as possible.</em>
					</p>
				</statement>
			</webwork>
		</task>

		<task label="drill-characteristic-equation-3"><title> <term>Characteristic Equation <m>\to</m> Characteristic Solutions</term> </title>
			
		</task>

		<task label="drill-characteristic-equation-4"><title> <term>Characteristic Equation <m>\to</m> Differential Equation</term> </title>
			
		</task>
	</exercise>

	<!-- <example xml:id="lhcc-roots-to-general-solution">
		<title> From Charateristic Roots to General Solution </title>
		<p>
			<statement>
				<p>
					Suppose the solutions to a characteristic equation for an LHCC equation are given below. In each case, find the corresponding general solution.
					<ol>
						<li><m>	r_1 = 3,\quad				r_2 = -3,\quad				r_3 = 5.3													</m></li>
						<li><m>	r_1 = 6 - i\sqrt{7.7},\quad	r_2 = 6 + i\sqrt{7.7},\quad	r_3 = 0														</m></li>
						<li><m>	r_1 =						r_2 =						r_3 = -4,\quad		r_4 = 5.3								</m></li>
						<li><m>	r_1 = -\frac{i}{2},\quad	r_2 = \frac{i}{2},\quad		r_3 = 2 + i,\quad	r_4 = 2 - i								</m></li>
						<li><m>	r_1 =						r_2 = 0,\quad				r_3 =				r_4 =			r_5 =	r_6 =	r_7 = 3	</m></li>
						<li><m>	r_1 = i,\quad				r_2 = -i,\quad				r_3 =				r_4 = \pi,\quad	r_5 = 5					</m></li>
					</ol>
				</p>
			</statement>

			<solution>
				<ol>
					<li>
						<p>
							Since we have three different real numbers, we use the <em>standard case</em> to get the general solution as
						</p>
						<me>
							y = c_1 e^{3x} + c_2 e^{-3x} + c_3 e^{5.3x}
						</me>
					</li>
					<li>
						<p>
							A complex conjugate pair and a single <m>0</m> solutions, means we use a combination of the <em>complex</em> and <em>standard cases</em>.
						</p>
						<me>
							y = e^{6x} (c_1 \sin(\sqrt{7.7}x) + c_2 \cos(\sqrt{7.7}x)) + c_3
						</me>
					</li>
					<li>
						<p>
							The solution <m>-4</m> repeats three times and the single <m>5.3</m> gives the general solution
						</p>
						<me>
							y = c_1 e^{-4x} + c_2 x e^{-4x} + c_3 x^2 e^{-4x} + c_4 e^{5.3x}
						</me>
					</li>
					<li>
						<p>
							The two separate complex conjugate pairs implies we use the <em>complex case</em> for both to get
						</p>
						<me>
							y = c_1 \sin\left(\frac{x}{2}\right) + c_2 \cos\left(\frac{x}{2}\right) + e^{2x} (c_3 \sin x + c_4 \cos x)
						</me>
					</li>
					<li>
						<p>
							Two <m>0</m>'s and five <m>3</m>'s means the general solution is
						</p>
						<me>
							y = c_1 x + c_2 + c_3 e^{3x} + c_4 x e^{3x} + c_5 x^2 e^{3x} + c_6 x^3 e^{3x} + c_7 x^4 e^{3x}
						</me>
					</li>
					<li>
						<p>
							One complex pair, two <m>\pi</m>'s, and a single <m>5</m>, gives us
						</p>
						<me>
							y = c_1 \sin x + c_2 \cos x + (c_3 x + c_4) e^{\pi x} + c_5 e^{5x}
						</me>
					</li>
				</ol>
			</solution>
		</p>
	</example> -->
</exercises>