<section><title> Orphaned Content </title>

	<introduction>
		<p>
			This is just a place to put content that was written and may or not be used.
		</p>
	</introduction>

	<paragraphs><title> Additional Narrative </title>
		
		<theorem xml:id="nth-derivative-of-exp"><title> N-th Derivative of <m>e^{rx}</m> </title>

			Each derivative of <m>e^{rx}</m> adds a multiple of <m>r</m>, so
			<me>
				\us{\ \text{ rule}}{\text{chain}} \rightarrow \ \ \left[e^{rx}\right]' = r e^{rx}, \quad \left[e^{rx}\right]'' = r^2 e^{rx}, \quad \ldots, \quad \left[e^{rx}\right]^{(n)} = r^n e^{rx}
			</me>.
		</theorem>

		<p>
			Before diving into how to solve <xref ref="def-lhcc" text="custom">LHCC equations</xref>, let's develop some intuition about what the solutions should look like. For this discussion we will assume that the equations contain a <m>y</m> term. If they didn't, then you could integrate both sides of the equation leaving you with a reduced order nonhomogeneous equation, which is a topic for the next chapter.
			<fn>
				For example, the following shows how an LHCC equation with no <m>y</m> term can be reduced to a nonhomogeneous equation with a <m>y</m> term.
				<md>
					<mrow> y''' - 2y'' = 0 \ \ \rightarrow \ \ (y' - 2y)''	=\amp\ 0 \quad \text{(direct integration x2)}	</mrow>
					<mrow> (y' - 2y)'										=\amp\ c_1										</mrow>
					<mrow> y' - 2y											=\amp\ c_1x + c_2								</mrow>
				</md>.
			</fn>
		</p>

		<tabular>
			<row>
				<cell colspan="2"><m>\ds a_n\ r^ne^{rx} + \cdots + a_2\ r^2e^{rx} + a_1\ re^{rx} + a_0\ e^{rx} = 0 </m></cell>
				<cell/>
			</row>
			<row>
				<cell colspan="2"><m>\ds (a_n\ r^n + \cdots + a_2\ r^2 + a_1\ r + a_0)\ e^{rx} = 0</m></cell>
				<cell><em>(factor out <m>e^{rx}</m>)</em></cell>
			</row>
			<row halign="center">
				<cell><m>\ds a_n\ r^n + \cdots + a_2\ r^2 + a_1\ r + a_0 = 0,</m></cell>
				<cell><m>\ds e^{rx} = 0</m></cell>
				<cell><em>(set each factor to 0)</em></cell>
			</row>
			<row halign="center">
				<cell><m>\uparrow</m></cell>
				<cell><m>\uparrow</m></cell>
				<cell/>
			</row>
			<row halign="center">
				<cell><em>characteristic equation!</em></cell>
				<cell><em>no solution</em></cell>
				<cell/>
			</row>
		</tabular>
		
		<p>
			The previous section showed us that solutions to LHCC equations involve <m>e^{rx}</m> terms. We will now build on this idea by showing that every LHCC equation is associated with another equation that allows us to find the specific <m>r</m>-values that give us our solutions. Let's explore this by looking at a few concrete examples, starting the equation
			<me>y' - 5y = 0</me>,
			Now, imagine we wanted verify that <m>y = e^{rx}</m> is a solution to this equation. To do this, we plug it into the equation and see if it leads to <m>0=0</m>. In this case, we get
			<md>
				<mrow>	\left[e^{rx}\right]' - 5 \left[e^{rx}\right] =\amp\ 0 </mrow>
				<mrow>	r e^{rx} - 5 e^{rx} =\amp\ 0 </mrow>
				<mrow>	\us{\text{must be 0}}{\ub{(r - 5) e^{rx}}} =\amp\ 0 </mrow>
			</md>,
			which shows that the left-side must also be <m>0</m>, but this only happens for specific <m>r</m>-values. To find them, we note that <m>e^{rx}</m> is never zero, and solve
			<md>
				<mrow>	(r - 5) e^{rx}	=\amp \ 0 \qquad (\text{divide by } e^{rx})</mrow>
				<mrow>			r - 5	=\amp \ 0 \quad \rightarrow \quad r = 5</mrow>
			</md>,
			showing that <m>e^{5x}</m> is a solution.
		</p>
	
		<p>
			Now, let's consider a second order equation, say
			<me>y'' - 5y' + 6y = 0</me>.
			Plugging <m>y = e^{rx}</m> into this equation, we have
			<md>
				<mrow>	\left[e^{rx}\right]'' - 5 \left[e^{rx}\right]' + 6 \left[e^{rx}\right] =\amp\ 0 </mrow>
				<mrow>	r^2 e^{rx} - 5 r e^{rx} + 6 e^{rx} =\amp\ 0 </mrow>
				<mrow>	(r^2 - 5r + 6) e^{rx} =\amp\ 0 </mrow>
			</md>
			Again, <m>e^{rx}</m> is never zero, so we must have <m>r^2 - 5r + 6 = 0</m>. Solving this quadratic equation gives <m>r = 2</m> and <m>r = 3</m>, yielding the solutions <m>e^{2x}</m> and <m>e^{3x}</m>.
		</p>
		
		<p>
			Regardless of the order, every LHCC equation can be approached in a similar way. To help us with the general equation, observe how each derivative of <m>e^{rx}</m> adds a multiple of <m>r</m> (by the chain rule). In particular,
			<me>
				y = e^{rx} \ \ \os{\text{chain rule}}{\rightarrow} \ \
				y' = re^{rx} \ \ \os{\text{chain rule}}{\rightarrow} \ \
				y'' = r^2e^{rx} \quad \os{\text{chain rule}}{\rightarrow \, \dots \, \rightarrow} \quad
				y^{(n)} = r^ne^{rx}
			</me>.
			We are now ready to plug <m>y = e^{rx}</m> into the general <xref ref="lhcc-equation" text="custom">LHCC equation</xref>:
			<md>
				<mrow>	
					a_n\ \left[e^{rx}\right]^{(n)} + \cdots + a_2\ \left[e^{rx}\right]'' + a_1\ \left[e^{rx}\right]' + a_0\ e^{rx} =\amp\ 0
				</mrow>
				<mrow>	a_n\ r^n e^{rx} + \cdots + a_2\ r^2 e^{rx} + a_1\ r e^{rx} + a_0\ e^{rx} =\amp\ 0 </mrow>
				<mrow>	\left(a_n\ r^n + \cdots + a_2\ r^2 + a_1\ r + a_0\right)e^{rx}  =\amp\ 0 </mrow>
			</md>.
			Following the same pattern as before, we get the <m>r</m>-values we need by solving
			<me>
				a_n\ r^n + \cdots + a_2\ r^2 + a_1\ r + a_0 = 0
			</me>.
			This polynomial equation that gives us the <m>r</m>-values we need to write down our solutions is referred to as the <em>characteristic equation</em>.
		</p>

		<p>
			We conclude this section with an important concept that will guide us in the sections to follow.
		</p>

		<assemblage><title> Terms of the Solution to an LHCC Equation </title>
			<p>
				The general solution to an LHCC equation involves terms of the form:
				<me> e^{rx}, \quad \ub{xe^{rx}, \quad x^2e^{rx}, \quad x^3e^{rx},\  \ldots}_{\text{For Special Cases}} </me>
				where <m>r</m> is a constant. Note, if <m>r</m> is complex, then <m>r=a+b i</m>, and by <xref ref="eulers-formula" text="custom">Euler's formula</xref>,
				<me> e^{rx} = e^{(a+b i)x} = e^{ax}\cdot e^{b i x} = e^{ax}(\cos(bx) + i\sin(bx)) </me>.
				In this case, it is common to see a solution written with sine and cosine terms.
			</p>
			<p>
				When <m>r</m> is complex, then <m>r=a+b i</m>, and by <xref ref="eulers-formula" text="custom">Euler's formula</xref>, <m> e^{rx} = e^{(a+b i)x} = e^{ax}\cdot e^{b i x} = e^{ax}(\cos(bx) + i\sin(bx)) </m>.
				In this case, the general solution may also contain sine and cosine terms.
			</p>
		</assemblage>
		
		<definition xml:id="def-char-eqn"><title> <em>LHCC Characteristic Equation</em> </title>
		
			<statement>
				<p>
					The <term>characteristic equation</term> of a <xref ref="lhcc-equation" text="custom">linear homogeneous differential equations with constant coefficients</xref> is given by the <m>n</m>-th degree polynomial equation
				</p>
				<men xml:id="characteristic-equation">
					a_n\ r^n + \cdots + a_2\ r^2 + a_1\ r + a_0 = 0	
				</men>.
			</statement>
		</definition>

		<p>
			The key takeaways from this subsection are:
		</p>

		<ul>
			<li> <em>Exponential functions</em> naturally emerge as solutions to LHCC equations due to their unique differentiation properties.</li>
			<li> The <em>characteristic equation</em> provides a systematic way to determine the fundamental solutions.</li>
			<li> The <em>general solution</em> consists of all independent exponential solutions, each multiplied by an arbitrary constant.</li>
			<li> The number of solutions matches the <em>order</em> of the differential equation.</li>
		</ul>

		<p>
			In summary, a differential equation is classified as an <xref ref="lhcc-equation">LHCC equation</xref> if it satisfies three criteria:
		</p>
		
		<ul>
			<li>It is <em>linear</em>: each term involves <m>y</m> or its derivatives to the first power only.</li>
			<li>It is <em>homogeneous</em>: the right-hand side is zero.</li>
			<li>It has <em>constant coefficients</em>: the coefficients of <m>y</m> and its derivatives do not depend on <m>x</m>.</li>
		</ul>

		<p>
			The following explains how <xref ref="lhcc-case-3" text="title"/> comes directly from <xref ref="lhcc-case-1" text="title"/>.
		</p>

		<p>
			Since <m>r_1</m> and <m>r_2</m> are complex, they can be written as
			<me>
				r_1 = \alpha + \beta i \quad \text{and} \quad r_2 = \alpha - \beta i
			</me>.
			Substituting these into <xref ref="lhcc-order-2-case-1-general-solution"/>, using <xref ref="eulers-formula" text="title"/>, the <xref ref="evenodd-cos" text="custom"> even property of cosine </xref> and <xref ref="evenodd-sin" text="custom"> odd property of sine </xref>, we can rewrite the general solution as
			<md>
				<mrow> y\  &amp;= c_1 e^{(\alpha + \beta i) x} + c_2 e^{(\alpha - \beta i) x} </mrow>
				<mrow> &amp;= c_1 e^{\alpha x} e^{i \beta x} + c_2 e^{\alpha x} e^{-i \beta x} </mrow>
				<mrow> &amp;= e^{\alpha x} \Big{[}c_1 e^{i \beta x} + c_2 e^{-i \beta x}\Big{]} </mrow>
				<mrow> &amp;= e^{\alpha x} \Big{[}c_1 (\cos(\beta x) + i\sin(\beta x)) + c_2 (\cos(-\beta x) + i\sin(-\beta x))\Big{]} </mrow>
				<mrow> &amp;= e^{\alpha x} \Big{[}c_1 \cos(\beta x) + i c_1 \sin(\beta x) + c_2 \cos(-\beta x) + i c_2 \sin(-\beta x)\Big{]} </mrow>
				<mrow> &amp;= e^{\alpha x} \Big{[}c_1 \cos(\beta x) + i c_1 \sin(\beta x) + c_2 \cos(\beta x) - i c_2 \sin(\beta x)\Big{]} </mrow>
				<mrow> &amp;= e^{\alpha x} \Big{[}(\us{c_1}{\ub{c_1 + c_2}}) \cos(\beta x) + \us{c_2}{\ub{i (c_1 - c_2)}} \sin(\beta x)\Big{]} </mrow>
				<mrow> &amp;= e^{\alpha x} (c_1 \cos(\beta x) + c_2 \sin(\beta x)) </mrow>
			</md>.
		</p>

	</paragraphs>



</section>