
<!-- LICENSING
  This file is part of the textbook "Exploring Differential Equations, An Interactive, Student-Centered Approach" by Geoffrey Cox.
  License: Creative Commons Attribution-ShareAlike 4.0 International (CC BY-SA 4.0)
  You are free to:
    ‚Ä¢ Share ‚Äî copy and redistribute the material in any medium or format.
    ‚Ä¢ Adapt ‚Äî remix, transform, and build upon the material for any purpose, even commercially.
  Under the following terms:
    ‚Ä¢ Attribution ‚Äî You must give appropriate credit, provide a link to the license, and indicate if changes were made.
    ‚Ä¢ ShareAlike ‚Äî If you remix, transform, or build upon the material, you must distribute your contributions under the same license.
  Full license text: https://creativecommons.org/licenses/by-sa/4.0/legalcode
  Recommended attribution: "Exploring Differential Equations" by Geoffrey Cox, licensed CC BY-SA 4.0.
-->
<section label="em-exercises">
	<title>Exercises</title>

	<!-- <exercises label="em-concept-quiz">
		<title><e component="emoji">üí°</e> Conceptual Quiz</title>
		
		<aside>
			<title>Abbreviations</title>
			<tabular>
				<col width="10%" />
				<col width="90%" />
				<row>
					<cell><p><em>DE</em></p></cell>
					<cell><em>Differential Equation</em></cell>
				</row>
				<row>
					<cell><p><em>IVP</em></p></cell>
					<cell><em>Initial Value Problem</em></cell>
				</row>
			</tabular>
		</aside>

	</exercises> -->

	<exercises label="em-problems">
		<title><e component="emoji">‚úçüèª</e> Problems </title>

		<exercise label="em-problem-01">

			<statement>
				Approximate the solution to the differential equation
				<p><me> y' = y^2 - x, \quad y(0) = -1 </me></p>
				<p>over the interval <m>[0, 1]</m> with a step size of <m>h = 0.5</m>.</p>
			</statement>

			<solution>
				<p>
					Solution omitted.
				</p>
			</solution>
		</exercise>

		<exercise label="em-problem-02">
			<statement>
				Use Euler's Method to approximate the solution to the initial-value problem,
				<p>
					<mdn>
						<mrow xml:id="euler-ex-01-de">	y'(x) - 2x y(x) = 0	\amp </mrow>
						<mrow xml:id="euler-ex-01-ic">	y(0) = 2, \amp </mrow>
					</mdn>
					at the <m>x</m>-values <m>0,\ 0.5,\ 1,\ 1.5,\ 2</m> (spaced 0.5 apart).
				</p>
			</statement>
			<solution>
				<p>
					Euler's method works by replacing <m>y'(x)</m> in <xref ref="euler-ex-01-de"/> with its forward-difference approximation, giving us
					<me>
						\frac{1}{h}\Big(y(x+h) - y(x)\Big) - 2x y(x) = 0
					</me>
					and if we let <m>h</m> be the space between the <m>x</m>-values (0.5), then we have
					<me>
						\frac{1}{0.5}\Big(y(x+0.5) - y(x)\Big) - 2x y(x) = 0.
					</me>
				</p>

				<p>
					To see how this is helpful, we isolate <m>y(x+h)</m> as follows:
					<md>
						<mrow>	\frac{1}{0.5}\Big(y(x+0.5) - y(x)\Big) 	=\ \amp 2x y(x)	</mrow>
						<mrow>							y(x+0.5) - y(x)	=\ \amp x y(x)	</mrow>
					</md>
					and the final step gives the approximation formula:
					<men xml:id="euler-ex-01-approx">
						y(x+0.5) = y(x) + x y(x).
					</men>
				</p>

				<p>
					Note that we already know <m>y(0) = 2</m> from <xref ref="euler-ex-01-ic"/>, so to find the rest of the approximation points, we plug <m>x = 0, 0.5, 1, 1.5</m> into <xref ref="euler-ex-01-approx"/>, as shown below.
				</p>

				<p>
					<tabular top="major" valign="top">
						<col width="0%" />
						<col width="45%" />
						<col width="20%" />
						<row bottom="minor">
							<cell> <m>x</m> </cell>
							<cell halign="center"> Approximation Formula <xref ref="euler-ex-01-approx"/> </cell>
							<cell> Approximation </cell>
						</row>
						<row bottom="minor">
							<cell> <m>0</m> </cell>
							<cell halign="left">
								<line><m>y(0+0.5) = y(0) + (0)y(0)</m></line>
								<line><m>\phantom{y(0+0.5)} = 2 + (0)(2) </m></line>
								<line><m>\phantom{y(0+0.5)} = 2 </m></line>
							</cell>
							<cell> <m>y(0.5) = 2</m> </cell>
						</row>

						<row bottom="minor">
							<cell> <m>0.5</m> </cell>
							<cell halign="left">
								<line><m>y(0.5+0.5) = y(0.5) + (0.5)y(0.5)</m></line>
								<line><m>\phantom{y(0.5+0.5)} = 2 + (0.5)(2) </m></line>
								<line><m>\phantom{y(0.5+0.5)} = 3 </m></line>
							</cell>
							<cell> <m>y(1) = 3</m> </cell>
						</row>

						<row bottom="minor">
							<cell> <m>1</m> </cell>
							<cell halign="left">
								<line><m>y(1+0.5) = y(1) + (1)y(1)</m></line>
								<line><m>\phantom{y(1+0.5)} = 3 + (1)(3) </m></line>
								<line><m>\phantom{y(1+0.5)} = 6 </m></line>
							</cell>
							<cell> <m>y(1.5) = 6</m> </cell>
						</row>

						<row bottom="major">
							<cell> <m>1.5</m> </cell>
							<cell halign="left">
								<line><m>y(1.5+0.5) = y(1.5) + (1.5)y(1.5)</m></line>
								<line><m>\phantom{y(1.5+0.5)} = 6 + (1.5)(6) </m></line>
								<line><m>\phantom{y(1.5+0.5)} = 15 </m></line>
							</cell>
							<cell> <m>y(2) = 15</m> </cell>
						</row>
					</tabular>

				</p>
			</solution>
		</exercise>

		<exercise label="em-problem-03">
			<title>Basic Euler's Method</title>

			<introduction>
				<p>
					Consider the initial-value problem
					<me>
						y'	= 2x - 3y + 1,\quad y(1) = 5
					</me>
					and answer the following:
				</p>
			</introduction>

			<p>
				<ol>
					<li>
						Compute 2 iterations of Euler's method using step size <m>h = 0.1</m>.
						<solution>
							<p>
						<md>
								<mrow>  \mbox{Preliminaries:	}	\amp \amp	f(x,y)	 \amp =  2x - 3y + 1 </mrow>
								<mrow>  \amp \amp	h	 \amp =  0.1 </mrow>
								<mrow>  \amp \amp	x_0	 \amp =  1 </mrow>
								<mrow>  \amp \amp	y_0	 \amp =  5 </mrow>
								<mrow>  \amp \amp		 \amp \mbox{Iteration 1:}		\amp \amp	x_1	 \amp =  x_0 + h </mrow>
								<mrow>  \amp \amp		 \amp =  1 + 0.1 </mrow>
								<mrow>  \amp \amp		 \amp =  1.1 </mrow>
								<mrow>  \amp \amp	y_1	 \amp =  y_0 + h\cdot f(x_0,y_0) </mrow>
								<mrow>  \amp \amp		 \amp =  5 + 0.1 \cdot f(1,5) </mrow>
								<mrow>  \amp \amp		 \amp =  5 + 0.1 \cdot [2(1) - 3(5) + 1] </mrow>
								<mrow>  \amp \amp		 \amp =  3.8 </mrow>
								<mrow>  \amp \amp		 \amp \mbox{Iteration 2:}		\amp \amp	x_2	 \amp =  x_1 + h </mrow>
								<mrow>  \amp \amp		 \amp =  1.1 + 0.1 </mrow>
								<mrow>  \amp \amp		 \amp =  1.2 </mrow>
								<mrow>  \amp \amp	y_2	 \amp =  y_1 + h\cdot f(x_1,y_1) </mrow>
								<mrow>  \amp \amp		 \amp =  3.8 + 0.1 \cdot f(1.1,3.8) </mrow>
								<mrow>  \amp \amp		 \amp =  3.8 + 0.1 \cdot [2(1.1) - 3(3.8) + 1] </mrow>
								<mrow>  \amp \amp		 \amp =  2.98  </mrow>
							</md>
							%
							</p>
						</solution>
						<answer>
							<p>
								<m> \ds x_1 = 1.1 \hspace{0.5cm} \ds x_2 = 1.2, \hspace{0.5cm} \ds y_1 = 3.8, \hspace{0.5cm} \ds y_2 = 2.98 </m>
							</p>
						</answer>
					</li>
					<li>
						What is the meaning of your answer in part (a)?
					</li>
					<li>
						Compute 2 iterations of Euler's method using step size <m> \ds h = 0.05</m>.
						<solution>
							<p>
								<md>
									<mrow>  \mbox{Preliminaries:	}	\amp \amp	f(x,y)	 \amp =  2x - 3y + 1 </mrow>
									<mrow>  \amp \amp	h	 \amp =  0.05 </mrow>
									<mrow>  \amp \amp	x_0	 \amp =  1 </mrow>
									<mrow>  \amp \amp	y_0	 \amp =  5 </mrow>
									<mrow>  \amp \amp		 \amp \mbox{Iteration 1:}		\amp \amp	x_1	 \amp =  x_0 + h </mrow>
									<mrow>  \amp \amp		 \amp =  1 + 0.05 </mrow>
									<mrow>  \amp \amp		 \amp =  1.05 </mrow>
									<mrow>  \amp \amp	y_1	 \amp =  y_0 + h\cdot f(x_0,y_0) </mrow>
									<mrow>  \amp \amp		 \amp =  5 + 0.05 \cdot f(1,5) </mrow>
									<mrow>  \amp \amp		 \amp =  5 + 0.05 \cdot [2(1) - 3(5) + 1] </mrow>
									<mrow>  \amp \amp		 \amp =  4.4 </mrow>
									<mrow>  \amp \amp		 \amp \mbox{Iteration 2:}		\amp \amp	x_2	 \amp =  x_1 + h </mrow>
									<mrow>  \amp \amp		 \amp =  1.05 + 0.05 </mrow>
									<mrow>  \amp \amp		 \amp =  1.1 </mrow>
									<mrow>  \amp \amp	y_2	 \amp =  y_1 + h\cdot f(x_1,y_1) </mrow>
									<mrow>  \amp \amp		 \amp =  4.4 + 0.05 \cdot f(1.05,4.4) </mrow>
									<mrow>  \amp \amp		 \amp =  4.4 + 0.05 \cdot [2(1.05) - 3(4.4) + 1] </mrow>
									<mrow>  \amp \amp		 \amp =  3.895  </mrow>
								</md>
							</p>
						</solution>
						<answer>
							<p>
								<m> x_1 = 1.05 \hspace{0.5cm} x_2 = 1.1, \hspace{0.5cm} y_1 = 4.4, \hspace{0.5cm} y_2 = 3.895 </m>
							</p>
						</answer>
					</li>
					<li>
						What is the meaning of your answer in part (b)?
					</li>
					<li>
						Find the analytic solution to the IVP. Use your solution to compare the exact value of <m>y(1.1)</m> with your answers from parts (a) and (b).
						<solution>
							<p>
							This DE is first-order and linear, so we can solve it using an integrating factor. (There are other solution techniques, as well.)
							</p>

							<p>
								We begin by putting the DE in the standard form for a first-order linear DE so that we can identify <m> \ds P(x) </m>.
								<md>
									<mrow>  y'	 \amp =  2x - 3y + 1 </mrow>
									<mrow>  y' + 3y	 \amp =  2x + 1 </mrow>
								</md>
								We can see that <m> \ds P(x) = 3.</m> Then we can find the integrating factor <m> \ds z </m>
								<md>
									<mrow> z	\amp = e^{\mbox{an antiderivative of P(x)}} </mrow>
									<mrow>		\amp = e^{\mbox{an antiderivative of 3}} </mrow>
									<mrow>		\amp = e^{3x} </mrow>
								</md>
								Now we multiply both sides of the DE by the integrating factor.
								<md>
									<mrow>  e^{3x}\cdot y' + 3e^{3x}y	 \amp =  (2x+1)e^{3x} \nonumber </mrow>
									<mrow>  \underbrace{e^{3x}}_{f}\cdot\underbrace{y'}_{g'} + \underbrace{3e^{3x}}_{f'}\cdot\underbrace{y}_{g}  \amp =  (2x+1)e^{3x}</mrow>
								</md>
								Now we recall the product rule for derivatives: <m>\dfrac{d}{dx}\Big( f \cdot g \Big) = f\cdot g' + f' \cdot g</m>. We note that the two terms on the left-hand side of the equation are the result of taking the derivative of the product. Hence we can undo the product rule as follows: <m>\dfrac{d}{dx}\Big(e^{3x}\cdot y \Big) = (2x+1)e^{3x}.</m> We would like to integrate both sides of the equation so we can isolate <m>y</m>. On the right-hand side, we will need to use integration by parts. We choose <m>u</m> and <m>dv</m> as follows: <m>u = 2x+1 \hspace{2cm} dv = e^{3x}\ dx \hspace{2cm} du</m> by taking the derivative of <m>u</m> and <m>v</m> by taking the antiderivative of <m>dv</m> : <m>du = 2dx  \hspace{2cm} v = \frac{1}{3}e^{3x}</m>. Now we proceed by integrating as follows:
								<md>
									<mrow> \int \frac{d}{dx}\Big(e^{3x}\cdot y \Big)dx
																				\amp =  \int (2x+1)e^{3x} dx </mrow>
									<mrow> e^{3x}\cdot y	\amp =  (2x+1)\cdot\frac{1}{3}e^{3x} - \int \frac{1}{3}e^{3x} \cdot 2dx </mrow>
									<mrow>								\amp =  \frac{1}{3}(2x+1)e^{3x} - \frac{2}{3}\int e^{3x}dx </mrow>
									<mrow>								\amp =  \frac{1}{3}(2x+1)e^{3x} - \frac{2}{3}\cdot \frac{1}{3}e^{3x} + C </mrow>
									<mrow>								\amp =  \frac{2}{3}xe^{3x} + \frac{1}{3}e^{3x} - \frac{2}{9}e^{3x} + C </mrow>
									<mrow>								\amp =  \frac{2}{3}xe^{3x} + \frac{1}{9}e^{3x} + C </mrow>
									<mrow> y							\amp =  \frac{2}{3}x + \frac{1}{9} + \frac{C}{e^{3x}} </mrow>
									<mrow>								\amp =  \frac{2}{3}x + \frac{1}{9} + Ce^{-3x}  </mrow>
								</md>
								Now we use the initial condition to find the value of <m> \ds C </m>.
								<md>
									<mrow>  y(1)	 \amp =  5 </mrow>
									<mrow>  \frac{2}{3}\cdot 1 + \frac{1}{9} + Ce^{-3\cdot 1}	 \amp =  5 </mrow>
									<mrow>  \frac{7}{9} + Ce^{-3}	 \amp =  5 </mrow>
									<mrow>  Ce^{-3}	 \amp =  \frac{38}{9} </mrow>
									<mrow>  C	 \amp =  \frac{38}{9e^{-3}} </mrow>
									<mrow>   \amp =  \frac{38e^3}{9} </mrow>
								</md>
								Hence, the solution is <m> \ds y = \frac{2}{3}x + \frac{1}{9} + \frac{38e^3}{9}e^{-3x}. </m> We can use this to find <m> \ds y(1.1)</m>:
								<md>
									<mrow> y(1.1)	\amp =  \frac{2}{3}\cdot 1.1 + \frac{1}{9} + \frac{38e^3}{9}e^{-3\cdot 1.1} </mrow>
									<mrow>				\amp =  3.9723  </mrow>
								</md>
								Note that the two numerical approximations were <m> \ds y(1.1) \approx 3.8 </m> (found using <m>h = 0.1 </m>) and <m>y(1.1) \approx 3.895 </m> (found using <m> \ds h = 0.05 </m>). Both are reasonable approximations, but the approximation using the smaller step size is closer to the exact answer.
							</p>
						</solution>
						<answer>
							<p>
								<m> \ds y = \frac{2}{3}x + \frac{1}{9} + \frac{38e^3}{9}e^{-3x},\quad y(1.1) \approx 3.9723 </m>
							</p>
						</answer>
					</li>
				</ol>
			</p>
		</exercise>

		<exercise label="em-problem-04">
			<title>Basic Euler's Method</title>

			<introduction>
				<p>
					Consider the initial-value problem
					<me>y' = y,\quad y(0) = 1</me>
					and answer the following:
				</p>
			</introduction>

			<p>
				<ol>
					<li>
						Use Euler's method to approximate <m>y(0.5)</m> using step size <m> \ds h = 0.5</m>.
						<solution>
							<p>
							<md>
									<mrow>  \mbox{Preliminaries:	}	\amp \amp	f(x,y)	 \amp =  y </mrow>
									<mrow>  \amp \amp	h	 \amp =  0.5 </mrow>
									<mrow>  \amp \amp	x_0	 \amp =  0 </mrow>
									<mrow>  \amp \amp	y_0	 \amp =  1 </mrow>
									<mrow>  \amp \amp		 \amp \mbox{Iteration 1:}		\amp \amp	x_1	 \amp =  x_0 + h </mrow>
									<mrow>  \amp \amp		 \amp =  0 + 0.5 </mrow>
									<mrow>  \amp \amp		 \amp =  0.5 </mrow>
									<mrow>  \amp \amp	y_1	 \amp =  y_0 + h\cdot f(x_0,y_0) </mrow>
									<mrow>  \amp \amp		 \amp =  1 + 0.5 \cdot f(0,1) </mrow>
									<mrow>  \amp \amp		 \amp =  1 + 0.5 \cdot [1] </mrow>
									<mrow>  \amp \amp		 \amp =  1.5 </mrow>
		
								</md>
								Hence <m> \ds y(0.5) \approx 1.5. </m>
							</p>
						</solution>
						<answer><p><m> y(0.5) \approx 1.5 </m></p></answer>
					</li>
					<li>
						Use Euler's method to approximate <m>y(0.5)</m> using step size <m>h = 0.25</m>.
						<solution>
							<p>
							<md>
									<mrow>  \mbox{Preliminaries:	}	\amp \amp	f(x,y)	 \amp =  y </mrow>
									<mrow>  \amp \amp	h	 \amp =  0.25 </mrow>
									<mrow>  \amp \amp	x_0	 \amp =  0 </mrow>
									<mrow>  \amp \amp	y_0	 \amp =  1 </mrow>
									<mrow>  \amp \amp		 \amp \mbox{Iteration 1:}		\amp \amp	x_1	 \amp =  x_0 + h </mrow>
									<mrow>  \amp \amp		 \amp =  0 + 0.25 </mrow>
									<mrow>  \amp \amp		 \amp =  0.25 </mrow>
									<mrow>  \amp \amp	y_1	 \amp =  y_0 + h\cdot f(x_0,y_0) </mrow>
									<mrow>  \amp \amp		 \amp =  1 + 0.25 \cdot f(0,1) </mrow>
									<mrow>  \amp \amp		 \amp =  1 + 0.25 \cdot [1] </mrow>
									<mrow>  \amp \amp		 \amp =  1.25 </mrow>
									<mrow>  \amp \amp		 \amp \mbox{Iteration 2:}		\amp \amp	x_2	 \amp =  x_1 + h </mrow>
									<mrow>  \amp \amp		 \amp =  0.25 + 0.25 </mrow>
									<mrow>  \amp \amp		 \amp =  0.5 </mrow>
									<mrow>  \amp \amp	y_2	 \amp =  y_1 + h\cdot f(x_1,y_1) </mrow>
									<mrow>  \amp \amp		 \amp =  1.25 + 0.25 \cdot f(0.25,1.25) </mrow>
									<mrow>  \amp \amp		 \amp =  1.25 + 0.25 \cdot [1.25] </mrow>
									<mrow>  \amp \amp		 \amp =  1.5625 </mrow>
								</md>
								Hence <m> \ds y(0.5) \approx 1.5625. </m>
							</p>
						</solution>
						<answer><p><m> y(0.5) \approx 1.5625 </m></p></answer>
					</li>
					<li>
						Which of the approximations above do you trust more?
					</li>
					<li>
						Find the analytic solution to the IVP. Use it to compute the exact value of <m>y(0.5)</m> and compare with your answers from parts (a) and (b).
						<solution>
							<p>
							There are multiple solution techniques that will work to solve this DE. We will separate variables here.
									<md>
										<mrow>  y'	 \amp =  y </mrow>
										<mrow>  \frac{dy}{dx}	 \amp =  y </mrow>
										<mrow>  \frac{1}{y}dy	 \amp =  dx </mrow>
										<mrow>  \int \frac{1}{y}dy	 \amp =  \int dx </mrow>
										<mrow>  \ln|y|	 \amp =  x+C </mrow>
										<mrow>  |y|	 \amp =  e^{x+C} </mrow>
										<mrow>  y	 \amp =  \pm e^C e^x </mrow>
										<mrow>   \amp =  Ae^x </mrow>
									</md>
									Now we can apply the initial condition to find the value of the constant <m> \ds A </m>.
									<md>
										<mrow>  y(0)	 \amp =  1 </mrow>
										<mrow>  Ae^{0}	 \amp =  1 </mrow>
										<mrow>  A	 \amp =  1  </mrow>
									</md>.
									Therefore, the solution is <m>y = e^x. </m> We can use this to find <m>y(0.5): y(0.5)	= e^{0.5} = 1.6487</m>. Note that the two numerical approximations were <m>y(0.5) \approx 1.5 </m> (found using <m>h = 0.5</m>) and <m>y(0.5) \approx 1.5625 </m> (found using <m>h = 0.25 </m>). Both are reasonable approximations, but the approximation using the smaller step size is closer to the exact answer.
							</p>
						</solution>
						<answer><p><m>y = e^x,\quad y(0.5) \approx e^{0.5} \approx 1.6487</m></p></answer>
					</li>
				</ol>
			</p>
		</exercise>

	</exercises>

</section>
