<subsection xmlns:xi="http://www.w3.org/2001/XInclude"><title>Finding Inverse Laplace Transforms by Completing the Square</title>

    <p>
        As you progress through the Laplace Transform Method, you will often encounter <xref ref="rational-function" text="custom">rational functions</xref> that do not immediately match any known form in the table of Laplace transforms. For example, the <m>s</m>-function 
        <me>\frac{s-6}{s^2 + 5s + 1}</me> 
        does not align with the forms in the <xref ref="common-lt-table" text="custom">common forward transform table</xref>. One common way to address this is by rewriting the denominator in the form <m>(s-a)^2 + b^2</m> to match known transforms like <m>L_7</m> or <m>L_8</m>. This technique, called completing the square, is essential in transforming quadratic expressions to forms that are easier to work with in inverse Laplace computations.
    </p>

    <p>
        This approach is appropriate when the roots of the quadratic expression in the denominator are complex. Recall from <xref ref="solving-the-quadratic-equation" text="custom">solving quadratic equations</xref>, if the discriminant 
        <me>b^2 - 4ac</me> 
        is negative, then the quadratic function has complex roots. Therefore, a quick compuation of this value provides a good signal that completing the square is the correct approach as the following examples demonstrate.
    </p>

    <example>
        <m>\quad</m>Compute the inverse Laplace transforms of the following functions:
        <me>H(s) = \frac{s-1}{s^2 - 2s + 5}, \quad K(s) = \frac{11}{s^2 - 6s + 14}, \quad P(s) = \frac{s+3}{s^2 + 2s + 10}.</me>
        
        <solution><title><m>\ilap{H(s)}</m></title>
            <p>
                The discriminant of the denominator <m>s^2 - 2s + 5</m> is 
                <me>b^2 - 4ac = (-2)^2 - 4(1)(5) = 4 - 20 = -16</me>, 
                which is negative. Therefore, completing the square is necessary:
                <md>
                    <mrow> s^2 - 2s + 5 = (s^2 - 2s) + 5    =\amp\ (\ob{s^2 - 2s + 1}^{(s - 1)^2} - 1) + 5   </mrow>
                    <mrow>                                  =\amp\ (s - 1)^2 + 4                             </mrow>
                </md>.
                Rewriting <m>H(s)</m> gives:
                <me>\frac{s-1}{s^2 - 2s + 5} = \frac{s-1}{(s - 1)^2 + 4},</me>
                which matches <xref ref="L8" text="title"/> (<m>a=1, b=2</m>). Therefore,
                <me>h(t) = \ilap{H(s)} = e^{t}\cos(2t).</me>
            </p>
        </solution>

        <solution><title><m>\ilap{K(s)}</m></title>
            <p>
                The discriminant of the denominator <m>s^2 - 6s + 14</m> is 
                <me>b^2 - 4ac = (-6)^2 - 4(1)(14) = 36 - 56 = -20</me>, 
                which is negative. Completing the square gives:
                <md>
                    <mrow> s^2 - 6s + 14 = (s^2 - 6s) + 14  =\amp (\ob{s^2 - 6s + 9}^{(s - 3)^2} - 9) + 14  </mrow>
                    <mrow>                                  =\amp (s - 3)^2 + 5                             </mrow>
                </md>.
                Rewriting <m>K(s)</m> as:
                <me>
                    \frac{11}{s^2 - 6s + 14} 
                        = \ub{\frac{11}{(s - 3)^2 + 5}}_{\large \text{Match with } L_7} 
                        = \frac{11}{\sqrt{5}}\ub{\frac{\sqrt{5}}{(s - 3)^2 + 5}}_{\large <xref ref="L7" text="custom">L_7</xref> (a\,=\,3,\ b\,=\,\sqrt{5})}
                </me>. 
                Therefore,
                <md>
                    <mrow>
                        k(t) = \ilap{K(s)}  =\amp\ \frac{11}{\sqrt{5}}e^{3t}\sin(\sqrt{5}t)
                    </mrow>
                </md>.
            </p>
        </solution>

        <solution><title><m>\ilap{P(s)}</m></title>
            <p>
                Completing the square for the denominator of <m>P(s)</m> gives:
                <me>
                    \frac{s+3}{s^2 + 2s + 10} = \frac{s+3}{(s + 1)^2 + 9}
                </me>,
                and leaves us in a tricky situation where the numerator is not <m>s+1</m>. This situation is addressed by rewriting <m>3</m> as <m>1 + 2</m> and grouping the <m>1</m> with the <m>s</m>. We then split the fraction. Here are all the details:
                <md>
                    <mrow>  
                        \frac{s+3}{s^2 + 2s + 10}
                            =\amp\ \frac{s + 1 + 2}{(s + 1)^2 + 9}
                    </mrow>
                    <mrow>
                            =\amp\ \frac{s+1}{(s + 1)^2 + 9} + \frac{2}{(s + 1)^2 + 9}
                    </mrow>
                    <mrow>
                            =\amp\ \ub{\frac{s+1}{(s + 1)^2 + 9}}_{\large <xref ref="L8" text="title"/>\ (a=-1, b=3)} 
                                + \frac{2}{3}\ub{\frac{3}{(s + 1)^2 + 9}}_{\large <xref ref="L7" text="title"/>\ (a=-1, b=3)}
                    </mrow>    
                </md>,
                Therefore,
                <md>
                    <mrow>  
                        p(t) =\amp\ \ilap{P(s)}
                    </mrow>
                    <mrow>
                            =\amp\ \ilap{ \frac{s+1}{(s + 1)^2 + 9} } + \frac{2}{3}\ilap{ \frac{3}{(s + 1)^2 + 9} }
                    </mrow>
                    <mrow>
                            =\amp\ e^{-t}\cos(3t) + \frac{2}{3}e^{-t}\sin(3t)
                    </mrow>    
                </md>
            </p>
        </solution>
    </example>

    <p>
        Completing the square is a crucial technique when working with quadratic expressions in the denominator of Laplace transforms. It allows the backward transformations to be found by rewriting the <m>s</m>-function in a form that aligns with known inverse Laplace transforms. In the next subsection, we will explore another technique: partial fraction decomposition, which helps break down even more complex rational functions into simpler parts that can be easily matched to common inverse transforms.
    </p>

    <xi:include href="./c4-s2-ss3-interactives.ptx" />

</subsection>
