
<subsection xmlns:xi="http://www.w3.org/2001/XInclude"><title> Summary &amp; Exercises </title>

	<introduction>
		
		<p>
			<assemblage color="green"><title>Summary of the Key Ideas</title>
				<p>
					<term> <em> Method</em> </term>
					<p>
						
					</p>
				</p>
			</assemblage>
		</p>
		
	</introduction>

	<exercises>

		<!--========== Exercise Group 1 ==========--> 
<exercisegroup>
	<title>
	<p>
	
	</p>
	<p/> <!-- added for vertical space -->
	</title>
		<exercise> <!--== Problem 1 ==-->
			<statement>
				 Use Laplace transforms to find the solutio <m> \ds y(t) </m> of the following initial value problem.<m> \ds x'' + 6x' + 9x = 64e^{5t}, \hspace{0.5cm}x(0) = 3, \hspace{0.5cm} x'(0) = 0 </m>
			</statement>
			<solution>
				 We begin by taking the Laplace transform and substituting in the initial conditions.
				<md>
					<mrow>  \Big[ s^2X(s) - sx(0) - x'(0) \Big] +6\Big[ sX(s) - x(0) \Big] + 9X(s)  \amp =  \frac{64}{s-5} \mbox{ (by L12, L11 and L2)} </mrow>
					<mrow>  \Big[ s^2X(s) - s\cdot 3 - 0 \Big] +6\Big[ sX(s) - 3 \Big] + 9X(s)	 \amp =  \frac{64}{s-5} </mrow>
					<mrow>  s^2X(s) - 3s + 6sX(s) - 18 + 9X(s)	 \amp =  \frac{64}{s-5} </mrow>
					<mrow>  s^2X(s) + 6sX(s)+9X(s) -3s - 18	 \amp =  \frac{64}{s-5} </mrow>
	 
				</md>
				 Now we aim to solve fo <m> \ds X(s), </m> so we use algebra to rearrange as follows.
				<md>
					<mrow>  s^2X(s) + 6sX(s)+9X(s)	 \amp =  \frac{64}{s-5} + 3s + 18 </mrow>
					<mrow>  X(s)	 \amp =  \frac{64}{s-5} + (3s + 18)\cdot \frac{s-5}{s-5} </mrow>
					<mrow>   \amp =  \frac{64}{s-5} + \frac{(3s+18)(s-5)}{s-5} </mrow>
					<mrow>   \amp =  \frac{64}{s-5} + \frac{3s^2 +3s- 90}{s-5} </mrow>
					<mrow>   \amp =  \frac{64 + 3s^2 +3s- 90}{s-5} </mrow>
					<mrow>   \amp =  \frac{3s^2 +3s- 26}{s-5} </mrow>
					<mrow>  X(s)	 \amp =  \frac{3s^2 +3s- 26}{(s-5)(s^2 + 6s + 9)} </mrow>
					<mrow>   \amp =  \frac{3s^2 +3s- 26}{(s-5)(s+3)^2} </mrow>
	 
				</md>
				 We need to do a partial fraction decomposition before we can take the inverse LT.
				<md>
					<mrow>  \frac{3s^2 +3s- 26}{(s-5)(s+3)^2}	 \amp =  \frac{A}{s-5} + \frac{B}{s+3} + \frac{C}{(s+3)^2} </mrow>
					<mrow>  3s^2 +3s - 26	 \amp =  A(s+3)^2 + B(s-5)(s+3) + C(s-5) </mrow>
					<mrow> \  \amp =  A(s^2 + 6s + 9) + B(s^2 - 2s - 15) + Cs - 5C </mrow>
					<mrow>   \amp =  As^2 + 6As + 9A + Bs^2 - 2Bs - 15B + Cs - 5C </mrow>
					<mrow>   \amp =  (A + B)s^2 + (6A - 2B + C)s + (9A - 15B - 5C) </mrow>
	 
				</md>
				 Equating the coefficients of like terms yields, we can solve fo <m> \ds A </m> <m> \ds B </m> , an <m> \ds C </m> .
				<md>
					<mrow>  A+B	 \amp =  3		\amp 6A - 2B + C	\amp= 3		\amp 			9A - 15B - 5C	\amp= -26 </mrow>
					<mrow>  B	 \amp =  3-A	\amp			\amp		\amp						\amp </mrow>
					<mrow>  \amp		\amp6A - 2(3-A)+C	 \amp =  3		\amp						\amp </mrow>
					<mrow>  \amp		\amp 6A-6+2A+C	 \amp =  3		\amp						\amp </mrow>
					<mrow>  \amp		\amp 	8A + C	 \amp =  9		\amp						\amp </mrow>
					<mrow>  \amp		\amp		C	 \amp =  9 - 8A	\amp						\amp </mrow>
					<mrow>  \amp		\amp			\amp		\amp 	9A - 15(3-A) - 5(9-8A)	 \amp =  -26 </mrow>
					<mrow>  \amp		\amp			\amp		\amp 9A - 45 + 15A - 45 + 40A	 \amp =  -26 </mrow>
					<mrow>  \amp		\amp			\amp		\amp 					64A	 \amp =  64 </mrow>
					<mrow>  \amp		\amp			\amp		\amp					A	 \amp =  1 </mrow>
					<mrow>  \amp		\amp		C	 \amp =  9-8(1)	\amp						\amp </mrow>
					<mrow>  \amp		\amp			 \amp =  1		\amp						\amp </mrow>
					<mrow>  B	 \amp =  3 - 1	\amp			\amp		\amp						\amp </mrow>
					<mrow>   \amp =  2		\amp			\amp		\amp						\amp </mrow>
	 
				</md>
				 Hence we have <m> \ds X(s) = \frac{1}{s-5} + \frac{2}{s+3} + \frac{1}{(s+3)^2}. </m> Now we need only take the inverse LT to find the solution.
				<md>
					<mrow>  x(t)	 \amp =  \lap^{-1}\left\{ \frac{1}{s-5} + \frac{2}{s+3} + \frac{1}{(s+3)^2} \right\} </mrow>
					<mrow>   \amp =  \lap^{-1}\left\{ \frac{1}{s-5} \right\} + 2\cdot \lap^{-1}\left\{\frac{1}{s+3} \right\} + \lap^{-1}\left\{\frac{1}{(s+3)^2} \right\}  </mrow>
					<mrow>   \amp =  e^{5t} + 2e^{-3t} + te^{-3t} </mrow>
	 
				</md>
				
			</solution>
			<answer>
				<m> \ds x = e^{5t} + 2e^{-3t} + te^{-3t} </m>
			</answer>
		</exercise>
	
	</exercisegroup>
	
	<!--========== Exercise Group 2 ==========--> 
	<exercisegroup>
	<title>
	<p>
	
	</p>
	<p/> <!-- added for vertical space -->
	</title>
		<exercise> <!--== Problem 2 ==-->
			<statement>
				 Use Laplace transforms to find the solutio <m> \ds y(t) </m> of the following initial value problem.<m> \ds y''-2y'+5y = -8e^{-t}, \hspace{0.5cm}y(0) = 2, \hspace{0.5cm} y'(0) = 12 </m>
			</statement>
			<solution>
				 We begin by taking the Laplace transform and substituting in the initial conditions.
				<md>
					<mrow>  \Big[ s^2Y(s) - sy(0) - y'(0) \Big] - 2\Big[ sY(s) - y(0) \Big] + 5Y(s)  \amp =  \frac{-8}{s+1} \mbox{ (by L12, L11 and L2)} </mrow>
					<mrow>  \Big[ s^2Y(s) - s\cdot 2 - 12) \Big] - 2\Big[ sY(s) - 2 \Big] + 5Y(s)	 \amp =  \frac{-8}{s+1} </mrow>
					<mrow>  s^2Y(s) - 2s - 12 - 2sY(s) +4 + 5Y(s)	 \amp =  \frac{-8}{s+1} </mrow>
					<mrow>  s^2Y(s) - 2sY(s) + 5Y(s)- 2s - 8	 \amp =  \frac{-8}{s+1} </mrow>
	 
				</md>
				 Now we aim to solve fo <m> \ds Y(s), </m> so we use algebra to rearrange as follows.
				<md>
					<mrow>  s^2Y(s) - 2sY(s) + 5Y(s)	 \amp =  \frac{-8}{s+1} + 2s - 8 </mrow>
					<mrow>  (s^2 - 2s + 5)Y(s)	 \amp =  \frac{-8}{s+1} + (2s - 8)\cdot \frac{s+1}{s+1} </mrow>
					<mrow>  (s^2 - 2s + 5)Y(s)	 \amp =  \frac{-8}{s+1} + \frac{2s^2+10s+8}{s+1} </mrow>
					<mrow>  (s^2 - 2s + 5)Y(s)	 \amp =  \frac{-8 + 2s^2+10s+8}{s+1} </mrow>
					<mrow>  (s^2 - 2s + 5)Y(s)	 \amp =  \frac{2s^2+10s}{s+1} </mrow>
					<mrow>  Y(s)	 \amp =  \frac{2s^2+10s}{(s+1)(s^2 - 2s + 5)} </mrow>
	 
				</md>
				 We need to do a partial fraction decomposition before we can take the inverse LT.
				<md>
					<mrow>  \frac{2s^2+10s}{(s+1)(s^2 - 2s + 5)}	 \amp =  \frac{A}{s+1} + \frac{Bs+C}{s^2 - 2s + 5} </mrow>
					<mrow>  2s^2 + 10s	 \amp =  A(s^2 - 2s + 5) + (Bs+ C)(s+1) </mrow>
					<mrow>   \amp =  As^2 - 2As + 5A + Bs^2 + Bs + Cs + C </mrow>
					<mrow>   \amp =  (A + B)s^2 + (-2A + B + C)s + (5A + C) </mrow>
	 
				</md>
				 Equating the coefficients of like terms yields, we can solve fo <m> \ds A </m> <m> \ds B </m> , an <m> \ds C </m> .
				<md>
					<mrow>  A+B	 \amp =  2	\amp		-2A+B+C	\amp= 10	\amp 5A + C	\amp= 0 </mrow>
					<mrow>  \amp	\amp				\amp		\amp	C	 \amp =  -5A </mrow>
					<mrow>  \amp	\amp				\amp		\amp		\amp	\amp	-2A + B + (-5A)	 \amp =  10	\amp		\amp </mrow>
					<mrow>  \amp	\amp		-7A + B	 \amp =  10	\amp		\amp </mrow>
					<mrow>  \amp	\amp			B	 \amp =  10+7A	\amp		\amp </mrow>
					<mrow>  \amp	\amp				\amp		\amp		A + (10+7A)	 \amp =  2	\amp				\amp		\amp		\amp </mrow>
					<mrow>  8A+10	 \amp =  2	\amp				\amp		\amp		\amp </mrow>
					<mrow>  8A	 \amp = -8	\amp				\amp		\amp		\amp </mrow>
					<mrow>  A	 \amp = -1	\amp				\amp		\amp		\amp </mrow>
					<mrow>  \amp	\amp			B	 \amp =  3		\amp		\amp </mrow>
					<mrow>  \amp	\amp				\amp		\amp	C	 \amp =  5 </mrow>
	 
				</md>
				 Hence, we have \begin{equation} Y(s) = \frac{-1}{s+1} + \frac{3s+5}{s^2 - 2s + 5}. \label{Y_of_s} \end{equation} We need to take the inverse Laplace Transform to fin <m> \ds y(t). </m>  We need to complete the square on the irreducible quadratic term as follows.
				<md>
					<mrow>  s^2 - 2s + 5	 \amp =  (s^2 - 2s) + 5 </mrow>
					<mrow>   \amp =  (s^2 - 2s + 1) - 1 + 5 </mrow>
					<mrow>   \amp =  (s - 1)^2 + 4 </mrow>
	 
				</md>
				 We need to transform the second term, as follows, so we can use L8 and L7 on the Laplace transform table.
				<md>
					<mrow>  \frac{3s+5}{s^2 - 2s + 5}	 \amp =  \frac{3s+5}{(s - 1)^2 + 2^2} </mrow>
					<mrow>   \amp =  \frac{3(s-1)+3+5}{(s - 1)^2 + 2^2} </mrow>
					<mrow>   \amp =  \frac{3(s-1)+8}{(s - 1)^2 + 2^2} </mrow>
					<mrow>   \amp =  \frac{3(s-1)}{(s - 1)^2 + 2^2} + \frac{8}{(s - 1)^2 + 2^2} </mrow>
					<mrow>   \amp =  3\cdot\frac{s-1}{(s - 1)^2 + 2^2} + \frac{4\cdot 2}{(s - 1)^2 + 2^2} </mrow>
					<mrow>   \amp =  3\cdot\frac{s-1}{(s - 1)^2 + 2^2} + 4\cdot\frac{2}{(s - 1)^2 + 2^2} </mrow>
	 
				</md>
				 We are now prepared to take the inverse LT of equation \ref{Y_of_s} to get the solution to the IVP.
				<md>
					<mrow>  y(t)	 \amp =  \lap^{-1}\left\{ Y(s) \right\} </mrow>
					<mrow>   \amp =  \lap^{-1}\left\{ \frac{-1}{s+1} + \frac{3s+5}{s^2 - 2s + 5} \right\} </mrow>
					<mrow>   \amp =  \lap^{-1}\left\{ -1\cdot \frac{1}{s+1} + 3\cdot\frac{s-1}{(s - 1)^2 + 2^2} + 4\cdot\frac{2}{(s - 1)^2 + 2^2} \right\} </mrow>
					<mrow>   \amp =  -1\cdot \lap^{-1}\left\{ \frac{1}{s+1}\right\} + 3\cdot\lap^{-1}\left\{\frac{s-1}{(s - 1)^2 + 2^2} \right\} + 4\cdot\lap^{-1}\left\{\frac{2}{(s - 1)^2 + 2^2} \right\} </mrow>
					<mrow>   \amp =  -e^{-t} + 3e^t\cos(2t) + 4e^t\sin(2t) </mrow>
	 
				</md>
				
			</solution>
			<answer>
				<m> \ds y(t) = -e^{-t} + 3e^t \cos(2t) + 4e^t \sin(2t) </m>
			</answer>
		</exercise>
	
	</exercisegroup>
	
	</exercises>

</subsection>