<subsection><title> Orphaned Content </title>

	<introduction>
		<p>
			This is just a place to put content that was written and may or not be used.
		</p>
	</introduction>

	<subsubsection><title> Direct Integration </title>

	</subsubsection>

	<subsubsection><title> Separation of Variables </title>

		<men xml:id="separable-form-for-integration">
			y' = f(x) \cdot g(y) \qquad \text{or} \qquad 
			\us{\text{variables}}{\ub{\frac{1}{g(y)} \cdot y'}_{\text{dependent}}} = 
			\us{\text{variables}}{\ub{\vphantom{\frac{1}{()}}\ \ f(x)\ \ \vphantom{\frac{1}{()}}}_{\text{independent}}}
		</men>

		<p>
			Writing a differential equation in separable form is the first key step in applying the separation of variables method and will be the focus of this section.
		</p>

		<note>
			<p>
				Be aware that it is not enough to put the dependent and independent variables on opposite sides of the equation. Separable form requires that <m>\frac{1}{g(y)}</m> be multiplied by the derivative term. Thus, we recommend writing the equation in the first form to avoid this oversight.
			</p>
		</note>
		
	</subsubsection>

	<subsubsection><title> Integrating Factor </title>

		<p>
			Suppose <m>f</m> and <m>g</m> are differentiable functions. The product rule states that
			<men xml:id="if-product-rule">
				\underset{\xrightarrow[\LARGE\text{forward}]{} }{\ds [f \cdot g ]'} = 
				\underset{\xleftarrow[\LARGE\text{backward}]{} }{\ds f \cdot g' + f' \cdot g}.
			</men>
			The <q>forward</q> version goes from left to right, while the <q>backward</q> version, which we'll focus on, goes from right to left. Let's practice applying both versions with a few examples.
		</p>

		<theorem><title>Solving <xref ref="if-sov-eqn"/></title>
			<statement>
				<p>
					The <term>integrating factor</term> for the first-order linear differential equation
					<me xml:id="standard-first-order-linear-de">y' + P(x)y = Q(x)</me>
					is <m>\mu = e^{\int P(x) dx}</m>. Multiplying both sides by <m>\mu</m> transforms the equation into:
					<me>\frac{d}{dx}\left[\mu(x) \cdot y\right] = \mu(x)Q(x)</me>.
				</p>
			</statement>
			
			<proof><title>Derivation of the Integrating Factor</title>
				<p>
					Note, all first-order linear differential equations can be written in the form
					<men xml:id="if-general-eqn"> 
						\frac{dy}{dx} + P(x) y = Q(x)
					</men>,
					where <m>P(x)</m> and <m>Q(x)</m> are functions of <m>x</m>. The goal is to write the left-side as a single derivative. However, backward product rule is missing a piece, <m>\mu(x)</m>, that we still need to find. We find <m>\mu(x)</m> by multiplying it onto <xref ref="if-general-eqn"/>, like so
					<sidebyside widths="50% 50%">
						<p>
							<md>
								<mrow> \frac{dy}{dx} + P(x)\amp\ y = Q(x) </mrow>
								<mrow> \mu \frac{dy}{dx} + {\color{blue} \mu P(} \amp\ {\color{blue}\! x)} y = \mu Q(x) </mrow>
								<mrow> {\color{blue} \updownarrow}\ \ \amp \ {\color{blue} \text{match &amp; solve}}</mrow>
								<mrow> \mu \frac{dy}{dx} + {\color{blue} \frac{d\mu}{dx}}\amp\ y = \mu Q(x) </mrow>
								<mrow> \frac{d}{dx}\big[\mu \cdot \amp\ y\big] = \mu Q(x) </mrow>
							</md>
						</p>
						
						<p>
							<md>
								<mrow> {\color{blue} \frac{d\mu}{dx} =}\amp\ {\color{blue} \mu P(x)} </mrow>
								<mrow> {\color{blue} \frac{1}{\mu}d\mu =}\amp\ {\color{blue} P(x) dx} </mrow>
								<mrow> {\color{blue} \int \frac{1}{\mu}d\mu =}\amp\ {\color{blue} \int P(x) dx} </mrow>
								<mrow> {\color{blue} \ln|\mu| =}\amp\ {\color{blue} \int P(x) dx} </mrow>
								<mrow> {\color{blue} \mu =}\amp\ {\color{blue} e^{\int P(x) dx}} </mrow>
							</md>
						</p>
					</sidebyside>
						
				</p>
			</proof>
		</theorem>
		
		<paragraphs><title> Another Approach to the IF Method.. </title>

			<p>
				The integrating factor method uses a three-step strategy to solve first-order linear differential equations in the <em>standard form</em>:
				<fn>
					<p>
						Every linear differential equation looks like
						<me> 
							a_n(x)y^{(n)} + \cdots + a_2(x)y'' + a_1(x)y' + a_0(x)y = f(x)
						</me>.
						The first-order version of this is
						<me> 
							a_1(x)y' + a_0(x)y = f(x)
						</me>,
						but we can divide both sides of this equation by <m>a_1(x)</m>:
						<me>
							y' + \us{P(x)}{\ub{\frac{a_0(x)}{a_1(x)}}}y = \us{Q(x)}{\ub{\frac{f(x)}{a_1(x)}}}
						</me>.
						Since every first-order linear differential equation can always be written as
						<me> 
							y' + P(x)y = Q(x) 
						</me>,
						we call this the first-order linear <em>standard form</em>.
					</p>
				</fn>
				<men xml:id="if-standard-form"> 
					y' + P(x)y = Q(x)
				</men>.
				The heart of this method is the first step: finding the correct integrating factor. The second step uses this factor to write the left side as a single derivative. Finally, the last step finds the solution by <xref ref="direct-integration" text="custom">direct integration</xref>.
			</p>
		
			<paragraphs><title> Step 1: Finding the Integrating Factor </title>
			
				<p>
					Understanding how to find the integrating factor is crucial. Let's carefully walk through this important process.
				</p>
				<p>
					Consider the differential equations (specific on the left, general on the right):
					<sidebyside>
						<p>
							<me> 
								\us{\text{product rule?}}{\ub{y' + x^2 y}} = 5x^2 
							</me>,
						</p>
						<p>
							<me> 
								\us{\text{product rule?}}{\ub{y' + P(x)y}} = Q(x) 
							</me>.
						</p>
					</sidebyside>
					We would like to rewrite the left side as a single derivative using the <xref ref="if-product-rule" text="custom">backward product rule</xref>. However, the <m>y'</m> alone suggests there is a missing second function that the product rule needs. Maybe there is a function that we can multiply both sides of the equation by to get the desired product rule. Let's call it <m>\mu</m> for now and see if we can find it. We start by multiplying both sides by <m>\mu</m>:
					<sidebyside>
						<p>
							<me> 
								\mu y' + 3x^2 \mu y = 5x^2\mu 
							</me>.
						</p>
						<p>
							<me> 
								\mu y' + P(x)\mu y = Q(x)\mu 
							</me>.
						</p>
					</sidebyside>
		
					Notice that the left side almost looks like the product rule <m>\left[ \mu y \right]' = \mu y' + \mu' y</m>, except for the boxed value where <m>\mu'</m> should be (see below).
		
					<sidebyside>
						<p>
							<me> 
								\overset{\ds \mu}	{\overset{\downarrow}{\vphantom{\Big[}\ds \mu}} 	\cdot 
								\overset{\ds y'}	{\overset{\downarrow}{\vphantom{\Big[}\ds y'}} 		+ 
								\overset{\ds \color{blue}{\mu'}}	{\overset{\downarrow}{\vphantom{\Big[}\ds \color{blue}{\boxed{3x^2 \mu}}}}	\cdot 
								\overset{\ds y}		{\overset{\downarrow}{\vphantom{\Big[}\ds y}} 		= 
								5x^2\mu 
							</me>,
						</p>
						<p>
							<me> 
								\overset{\ds \mu}	{\overset{\downarrow}{\vphantom{\Big[}\ds \mu}} 	\cdot 
								\overset{\ds y'}	{\overset{\downarrow}{\vphantom{\Big[}\ds y'}} 		+ 
								\overset{\ds \color{blue}{\mu'}}	{\overset{\downarrow}{\vphantom{\Big[}\ds \color{blue}{\boxed{P(x) \mu}}}}	\cdot 
								\overset{\ds y}		{\overset{\downarrow}{\vphantom{\Big[}\ds y}} 		= 
								Q(x)\mu 
							</me>.
						</p>
					</sidebyside>
		
					This shows that the <m>\mu</m> that works is the one that satisfies
					<sidebyside>
						<p>
							<me> 
								\mu' = 3x^2 \mu
							</me>
						</p>
						<p>
							<me> 
								\mu' = P(x) \mu
							</me>.
						</p>
					</sidebyside>
		
					Careful inspection shows that these are separable differential equations where the unknown <m>\mu</m> can be found using separation of variables!
		
					<sidebyside>
						<p>
							<md>
								<mrow>	\int \frac{1}{\mu}d\mu	\amp = \int 3x^2\ dx										</mrow>
								<mrow>				\ln|\mu|	\amp = x^3 + C												</mrow>
								<mrow>						\mu	\amp = \pm e^{x^3 + C}										</mrow>
								<mrow>						\mu	\amp = {\color{green} \us{C}{\boxed{\pm e^C}}} e^{x^3}	</mrow>
								<mrow>						\mu	\amp = Ce^{x^3}												</mrow>
							</md>
						</p>
						<p>
							<md>
								<mrow>	\int \frac{1}{\mu}d\mu	\amp = \int P(x)\ dx	</mrow>
								<mrow>				\ln|\mu|	\amp = \int P(x)\ dx		</mrow>
								<mrow>						\mu	\amp = e^{\int P(x)\ dx}	</mrow>
							</md>
						</p>
					</sidebyside>
		
					Although the solution conatains a constant, we only need one function that works, so we set <m>C = 1</m>. The function <m>\mu</m> is called the <em>integrating factor</em> and finding it is the first step toward solving a first order differential equation.
				</p>
		
			</paragraphs>
		
			<paragraphs><title> Step 2: Rewriting the Equation </title>
			
				With the integrating factor in hand, we are ready to write the left side as a derivative using the <xref ref="if-product-rule" text="custom">backward product rule</xref>.
				<sidebyside>
					<p>
						Integrating Factor: <m>\mu = e^{x^3}</m>
						<md>
							<mrow>					y' + x^2 y	=\ \amp 5x^2		</mrow>
							<mrow>	e^{x^3}y' + x^2 e^{x^3}y	=\ \amp 5x^2e^{x^3}	</mrow>
							<mrow>	\left[ e^{x^3}y \right]'	=\ \amp 5x^2e^{x^3}	</mrow>
						</md>
					</p>
					<p>
						Integrating Factor: <m>\mu = e^{\int P(x)\ dx}</m>
						<md>
							<mrow>				y' + P(x)y	=\ \amp Q(x)		</mrow>
							<mrow>		\mu y' + P(x) \mu y	=\ \amp Q(x) \mu	</mrow>
							<mrow>	\left[ \mu y \right]'	=\ \amp Q(x) \mu	</mrow>
						</md>.
					</p>
				</sidebyside>
			</paragraphs>
		
			<paragraphs><title> Step 3: Solving the Equation </title>
			
				<p>
					The final step is to apply <xref ref="direct-integration" text="custom">direct integration</xref>. This was covered in a previous section, so we will skip some of the details here.
				</p>
		
				<sidebyside widths="50% 38%">
					<p>
						<md>
							<mrow>	\int \left[ e^{x^3}y \right]' \ dx	=\ \amp \int 5x^2e^{x^3} \ dx	</mrow>
							<mrow>							e^{x^3}y	=\ \amp \frac{5}{3} e^{x^3} + C	</mrow>
							<mrow>									y	=\ \amp \frac{5}{3} + Ce^{-x^3}	</mrow>
						</md>
					</p>
					<p>
						<md>
							<mrow>	\int \left[ \mu y \right]' \ dx	=\ \amp \int Q(x) \mu \ dx					</mrow>
							<mrow>							\mu y	=\ \amp \int Q(x) \mu \ dx					</mrow>
							<mrow>								y	=\ \amp \frac{1}{\mu} \int Q(x) \mu \ dx	</mrow>
						</md>
						where <m>\mu = e^{\int P(x)\ dx}</m>.
					</p>
				</sidebyside>
		
				<p>
					<assemblage xml:id="integrating-factor-general-solution"><title> General Solution </title>
						<p>
							The general solution for the first-order linear differential equation
						</p>
						<p>
							<me> 
								y' + P(x)y = Q(x) 
							</me>
							is given by	
							<me>
								y = \frac{1}{\mu} \int Q(x) \mu \ dx 
							</me> where <m>\mu = e^{\int P(x)\ dx}</m> is the integrating factor.
						</p>
					</assemblage>
				</p>
			</paragraphs>
		
			<p>
				In summary, the integrating factor method is a three-step process that utilizes the integrating factor to rewrite the left side of the equation, enabling direct integration and leading to the general solution.
			</p>

		</paragraphs>

		<paragraphs><title> Another Approach to the IF Method.. </title>
			
			<p>
				<md>
					<mrow> \frac{d}{dx}\left[ y \cdot e^{-2x} \right] \amp = 5 e^{-2x} \quad \leftarrow \text{Easy to solve!} </mrow>
				</md>
				and then we integrate both sides with respect to <m>x</m> to free the unknown <m>y</m> from inside the <m>\ds\frac{d}{dx}</m>, so that we can solve for it. However, we have not talked about how the integrating factor gets the differential equation into this form. Luckily, the product rule for deriviatives holds the answer. Therefore, let's start this discussing by reminding ourselves that the product rule is given by
				<me> \frac{d}{dx}[\ f \cdot g\ ] = \frac{d}{dx}[\ f\ ] \cdot g + f \cdot \frac{d}{dx}[\ g\ ]. </me>
			</p>
		
			<p>
				Ok, the claim is that after a some math the differential equation
				<men xml:id="if_prod_rule_eq1"> \frac{dy}{dx} - 2y = 5 </men>
				can be rewritten as 
				<men xml:id="if_prod_rule_eq2"> \frac{d}{dx}\left[ y \cdot e^{-2x} \right] = 5 e^{-2x}. </men>
				To explain this, it may be easier to work backwards. That is, let's start with <xref ref="if_prod_rule_eq2" /> and see how it may connect back to <xref ref="if_prod_rule_eq1" />. We start by applying the product rule on the left side,
				<mdn>
					<mrow> \frac{d}{dx}[\ y \cdot e^{-2x}\ ] \amp = 5 e^{-2x} </mrow>
					<mrow> \frac{d}{dx}[\ y\ ] \cdot e^{-2x} + y \cdot \frac{d}{dx}[\ e^{-2x}\ ] \amp = 5 e^{-2x} </mrow>
					<mrow> \frac{dy}{dx} \cdot e^{-2x} + y \cdot \left(-2 e^{-2x}\right) \amp = 5 e^{-2x} </mrow>
					<mrow xml:id="if_prod_rule_eq3"> \frac{dy}{dx} \cdot e^{-2x} - 2 y \cdot e^{-2x} \amp = 5 e^{-2x}. </mrow>
				</mdn>
				At this point stop and compare equation <xref ref="if_prod_rule_eq1" /> with the last equation <xref ref="if_prod_rule_eq3" />. Do you see how the two equations are connected?
			</p>
		
			<p>
				You should see that multiplying both sides of <xref ref="if_prod_rule_eq1" /> by <m>e^{-2x}</m> gives you <xref ref="if_prod_rule_eq3" />.
		
			</p>
		
			<p>
				In a nutshell, the integrating factor technique attempts to solve
				<me>y' + P(x)y = Q(x)</me>
				by multiplying both sides by an unknown function, <m>\mu</m>
				<me>\mu y' + \mu P(x)y = \mu Q(x)</me>
				then find a <m>\mu</m> so that the left-hand side can be written as the product rule of <m>\mu</m> and <m>y</m>.
				<me>\us{\large \text{product rule}}{\ub{\mu y' + \mu P(x)y}} = \mu Q(x)</me>
			</p>
		
			<p>
				To clarify, let's look at an example where we know <m>\mu</m>.
			</p>
			
			<p>
				The previous example shows how to solve the equation when you know what <m>\mu</m> is. However, in a real problem, you will have to find <m>\mu</m> first!
			</p>
			
			<p>
				Let's build on the previous example to try and understand why <m>\mu = e^{6x}</m> worked. It is important to try and think of <m>\mu(x)</m> as the missing part needed to to be consistent with the product rule. That is, the left-side of the equation
			
				<me>\us{\large \text{product rule}}{\us{\large \text{incomplete}}{\ub{y' + 6y}}} = 1</me>
			
				is missing a second function needed to be consistent with the product rule. So let's fill-in this missing function by multiplying both sides by <m>\mu</m>,
			
				<men xml:id="complete-product-rule-eqn">\mu y' + 6 \mu y = \mu.</men>
			
				Is the left-side, <m>\mu y' + 6 \mu y</m>, equal to <m>\left[\mu y\right]'</m>? Well, not exactly, since taking this derivative shows the difference between these two, namely
			
				<sidebyside>
					<tabular halign="center">
						<row>
							<cell></cell>
							<cell></cell>
							<cell></cell>
							<cell></cell>
							<cell bottom="minor"></cell>
							<cell></cell>
							<cell></cell>
						</row>
				
						<row>
							<cell halign="right"><m>\ds\left[\mu y\right]'</m></cell>
							<cell><m>=</m></cell>
							<cell><m>\mu y'</m></cell>
							<cell right="minor"><m>+</m></cell>
							<cell bottom="minor" right="minor"><m>\mu'</m></cell>
							<cell><m>y</m></cell>
							<cell></cell>
						</row>
				
						<row>
							<cell></cell>
							<cell></cell>
							<cell></cell>
							<cell></cell>
							<cell><m>\uparrow</m></cell>
							<cell></cell>
							<cell></cell>
						</row>
				
						<row>
							<cell></cell>
							<cell></cell>
							<cell></cell>
							<cell colspan="4"><em>difference</em></cell>
						</row>
				
						<row>
							<cell></cell>
							<cell></cell>
							<cell></cell>
							<cell></cell>
							<cell bottom="minor"><m>\downarrow</m></cell>
							<cell></cell>
							<cell></cell>
						</row>
				
						<row>
							<cell>left-side</cell>
							<cell><m>\rightarrow</m></cell>
							<cell><m>\mu y'</m></cell>
							<cell right="minor"><m>+</m></cell>
							<cell bottom="minor" right="minor"><m>6\mu</m></cell>
							<cell><m>y</m></cell>
						</row>
					</tabular>
				</sidebyside>
			</p>
			
			<p>
				However, what if <m>\mu</m> was chosen so that <m>\mu' = 6\mu</m>? It turns out that this is exactly how we chose <m>\mu</m>. Finding <m>\mu</m> such that <m>\mu' = 6\mu</m> is itself a differential equation which can be solved using separation of variables. (You may try it yourself first for practice, then look below to see how to solve this DE.)
			</p>
			
			<p>
				Using separation of variables, solve
				<md>
				<mrow>\mu' =\amp\ 6\mu.</mrow>
				</md>
				to get the solution
				<fn>
					<md>
					<mrow>\frac{d\mu}{dx} =\amp\ 6\mu</mrow>
					<mrow>\frac{1}{\mu}d\mu =\amp\ 6\ dx</mrow>
					<mrow>\int\frac{1}{\mu}d\mu =\amp\ \int 6\ dx</mrow>
					<mrow>\ln|\mu| =\amp\ 6x + C</mrow>
					<mrow>|\mu| =\amp\ e^{6x + C}</mrow>
					<mrow>\mu =\amp\ \pm e^C e^{6x}</mrow>
					<mrow>\mu =\amp\ A e^{6x}</mrow>
					</md>
				</fn>
				<me>\mu = A e^{6x}.</me>
			
				Since, we only need one <m>\mu</m> to work, we choose <m>A=1</m> for convenience, hence
			
				<me>\mu = e^{6x}.</me>
			
				Now you see where the <m>\mu</m> came from in part 1 of <xref ref="if-intro-exercise"/>.  In fact, this example outlines how <m>\mu</m> is found for any first order linear differential equation of the form 
				<men xml:id="EQ-1st-order-de-pre">y' + P(x)y = Q(x).</men>
			</p>

			<figure>
				<caption> 
					Matching the terms of the top and middle expressions in order to reverse the product rule. Notice the <m>y</m> terms are already equal, so we only need to find <m>\mu</m>.
				</caption>
				<image width="40%">

					<latex-image>
						\begin{tikzpicture}[relative]
							\node[anchor=south, inner sep=-1pt] (E1T1) 	at (-1.44,2.8)	{\underline{$\ds\frac{dy}{dx}$}};
							\node[anchor=south, inner sep=-1pt] (E1D1) 	at (-1.1,3.1) 	{$\cdot$};
							\node[anchor=south, inner sep=-1pt] (E1T2) 	at (-0.6,3) {\underline{$\ds e^{5x^2}$}};
							\node[anchor=south, inner sep=-1pt] (E1C) 	at (0,3.1) 	{$+$};
							\node[anchor=south, inner sep=-1pt] (E1T3) 	at (0.9,3) 	{\underline{$\ds10xe^{5x^2}$}};
							\node[anchor=south, inner sep=-1pt] (E1D2) 	at (1.6,3.1) 	{$\cdot$};
							\node[anchor=south, inner sep=-1pt] (E1T4) 	at (1.9,3) 	{\underline{$\ds y$}};
							\node[anchor=center, inner sep=0pt] (E2T1) at (-1,2) 	{$\ds\frac{dy}{dx}$};
							\node[anchor=center] (E2D1) at (-0.7,2) 	{$\cdot$};
							\node[anchor=center] (E2T2) at (-0.4,2) 	{$\ds\mu$};
							\node[anchor=center, inner sep=6pt] (E2C) 	at (0,2) 	{$+$};
							\node[anchor=center] (E2T3) at (0.5,2) 	{$\ds\frac{d\mu}{dx}$};
							\node[anchor=center] (E2D2) at (0.8,2) 	{$\cdot$};
							\node[anchor=center] (E2T4) at (1,2) 	{$\ds y$};
							\node[anchor=center] (E3C) 	at (0,0.8) 	{$\ds\frac{d}{dx}\left[y \cdot \mu\right]$};
							
							\path[&lt;->] (E1T1.south) edge [bend right=30] (E2T1.north west);
							\path[&lt;->] (E1T2.south) edge (E2T2.north);
							\path[&lt;->] (E1T3.south) edge (E2T3.north);
							\path[&lt;->] (E1T4.south) edge [bend left=40] (E2T4.east);

							\draw (-0.06,1.47) to (-0.06,1.23);
							\draw (0.06,1.47) to (0.06,1.23);
						\end{tikzpicture}
					</latex-image>

				</image>
			</figure>
			
		</paragraphs>

	</subsubsection>

</subsection>