<subsubsection xml:id="quick-ref-lt"><title> Laplace Transforms </title>

	<worksheet><title> Key Terms &amp; Concepts </title>

		<p>
			In this section, we introduced the concept of the forward Laplace transform and derived some common Laplace transforms that we will use throughtout this chapter. The following points summarize the essential concepts from the forward Laplace transform section:
		</p>

		<p>
			<assemblage><title> ✳️ Summary of the Key Ideas </title>
				<p>
					<ul>
						<li>
							<term>Differential <m>\to</m> Algebraic Equations</term>. The Laplace transform converts a differential equation into an algebraic equation, simplifying the solution process by eliminating derivatives.
						</li>
						<li>
							<term>Laplace Transform Concept</term>. Applying the Laplace transform to a differential equation involves transforming each term by multiplying by <m>e^{-st}</m> and integrating with respect to <m>t</m> from <m>0</m> to <m>\infty</m>, but is often simplified by directly applying the Laplace operator, <m>\laplacesym</m>.
						</li>
						<li>
							<term>Linearity Property</term>. The Laplace transform is linear, meaning it distributes across addition and subtraction, and allows for constants to be factored out. This property is essential for transforming complex equations.
						</li>
						<li>
							<term>Transforming Initial Conditions</term>. Initial conditions are incorporated directly into the Laplace-transformed equation, modifying the transformed terms to include initial values, making it easier to solve the resulting algebraic equation.
						</li>
						<li>
							<term>Common Function Transforms</term>. The Laplace transforms of common functions, such as exponentials, sines, cosines, and polynomials, are essential tools in transforming differential equations and are summarized in the provided table.
						</li>
						<li>
							<term>Transforming Derivatives</term>. The Laplace transform of a derivative, <m>y'(t)</m> or higher, transfers the derivative onto the Laplace variable <m>s</m>, reducing the order of the equation while introducing initial condition terms.
						</li>
						<li>
							<term>Multiplication by <m>e^{at}</m> and <m>t^n</m></term>. When multiplying a function by an exponential <m>e^{at}</m>, the Laplace transform shifts by <m>a</m> in the <m>s</m>-domain, and multiplying by <m>t^n</m> corresponds to differentiating the transform <m>n</m> times with respect to <m>s</m>, introducing a sign change.
						</li>
						<li>
							<term>Transforming the Entire Equation</term>. The process of applying the Laplace transform to an entire differential equation with initial conditions involves systematically transforming each term and leads to a simplified algebraic equation in the <m>s</m>-domain, ready for solving.
						</li>
					</ul>
				</p>
			</assemblage>
			
		</p>

		<p>
			The table below summarizes the common Laplace transforms that we derived in this section.
		</p>

		<assemblage xml:id="lt-table-L1-L8"><title> ✳️ Common Laplace Transforms <m>L_1-L_8</m> </title>
			<p>
				Let <m>a</m> and <m>b</m> be constant.
				<dl width="narrow">
					<li><title> <m>{\LARGE \vphantom{\int}}L_1</m> </title>
						<m>\ds \lap{ 1 } = \frac{1}{s}, \quad s &gt;0 </m>
					</li>
					<li><title> <m>{\LARGE \vphantom{\int}}L_2</m> </title>
						<m>\ds \lap{ e^{at} } = \frac{1}{s - a}, \quad s &gt;a </m>
					</li>
					<li><title> <m>{\LARGE \vphantom{\int}}L_3</m> </title>
						<m>\ds \lap{ t^n } = \frac{n!}{s^{n+1}}, \quad s &gt;0, \quad n = 1, 2, 3, \ldots </m>
					</li>
					<li><title> <m>{\LARGE \vphantom{\int}}L_4</m> </title>
						<m>\ds \lap{ \sin(bt) } = \frac{b}{s^2+b^2}, \quad s &gt;0</m>
					</li>
					<li><title> <m>{\LARGE \vphantom{\int}}L_5</m> </title>
						<m>\ds \lap{ \cos(bt) } = \frac{s}{s^2+b^2}, \quad s &gt;0 </m>
					</li>
					<li><title> <m>{\LARGE \vphantom{\int}}L_6</m> </title>
						<m>\lap{ t^n e^{at} } = \ds\frac{n!}{(s-a)^{n+1}}, \quad s &gt;a </m>
					</li>
					<li><title> <m>{\LARGE \vphantom{\int}}L_7.</m> </title>
						<m>\ds \lap{ e^{at}\sin(bt) } = \frac{b}{(s-a)^2+b^2}, \quad s &gt;a </m>
					</li>
					<li><title> <m>{\LARGE \vphantom{\int}}L_8.</m> </title>
						<m>\ds \lap{ e^{at}\cos(bt) } = \frac{s-a}{(s-a)^2+b^2}, \quad s &gt;a</m>
					</li>
				</dl>
			</p>
		</assemblage>

		<table halign="center" xml:id="common-lt-table-copy"><title> <em>Common Laplace Transforms. <m>a, b</m> are constant, <m>n = 1, 2, \ldots</m></em> </title>
			<tabular halign="center">
				<row>
					<cell/>
					<cell><m>t</m>-functions</cell>
					<cell colspan="2"><m>s</m>-functions</cell>
				</row>
				<row>
					<cell/>
					<cell><m>\downarrow</m></cell>
					<cell colspan="2"><m>\downarrow</m></cell>
				</row>
				<row bottom="minor">
					<cell right="minor"/>
					<cell right="minor"><m>f(t)</m></cell>
					<cell colspan="2"><m>\lap{ f(t) }</m></cell>
				</row>
				<row bottom="minor">
					<cell right="minor"><m>L_1</m></cell>
					<cell right="minor"><m>1</m></cell>
					<cell><m>\ds \frac{1}{s}</m></cell>
					<cell><m>s \gt 0</m></cell>
				</row>
				<row bottom="minor">
					<cell right="minor"><m>L_2</m></cell>
					<cell right="minor"><m>e^{at}</m></cell>
					<cell><m>\ds \frac{1}{s-a}</m></cell>
					<cell><m>s \gt a</m></cell>
				</row>
				<row bottom="minor">
					<cell right="minor"><m>L_3</m></cell>
					<cell right="minor"><m>t^n</m></cell>
					<cell><m>\ds \frac{n!}{s^{n+1}}</m></cell>
					<cell><m>s \gt 0</m></cell>
				</row>
				<row bottom="minor">
					<cell right="minor"><m>L_4</m></cell>
					<cell right="minor"><m>\sin (bt)</m></cell>
					<cell><m>\ds \frac{b}{s^2 + b^2}</m></cell>
					<cell><m>s \gt 0</m></cell>
				</row>
				<row bottom="minor">
					<cell right="minor"><m>L_5</m></cell>
					<cell right="minor"><m>\cos(bt)</m></cell>
					<cell><m>\ds \frac{s}{s^2 + b^2}</m></cell>
					<cell><m>s \gt 0</m></cell>
				</row>
				<row bottom="minor">
					<cell right="minor"><m>L_6</m></cell>
					<cell right="minor"><m>t^n e^{at}</m></cell>
					<cell><m>\ds \frac{n!}{(s-a)^{n+1}}</m></cell>
					<cell><m>s \gt a</m></cell>
				</row>
				<row bottom="minor">
					<cell right="minor"><m>L_7</m></cell>
					<cell right="minor"><m>e^{at} \sin(bt)</m></cell>
					<cell><m>\ds \frac{b}{(s-a)^2 + b^2}</m></cell>
					<cell><m>s \gt a</m></cell>
				</row>
				<row>
					<cell right="minor"><m>L_8</m></cell>
					<cell right="minor"><m>e^{at} \cos(bt)</m></cell>
					<cell><m>\ds \frac{s-a}{(s-a)^2 + b^2}</m></cell>
					<cell><m>s \gt a</m></cell>
				</row>
				<!-- <row>
					<cell/>
					<cell><m>\uparrow</m></cell>
					<cell><m>\uparrow</m></cell>
					<cell></cell>
				</row>
				<row>
					<cell/>
					<cell><m>t</m>-function</cell>
					<cell><m>s</m>-function</cell>
					<cell></cell>
				</row> -->
			</tabular>
		</table>

		<table halign="center" xml:id="lt-properties-table"><title> <em>Laplace Transforms Properties, <m>{\small \lap{ y(t) } = Y(t), \ \lap{ z(t) } = Z(t)}</m></em> </title>
			<tabular halign="center">
				<row bottom="minor">
					<cell right="minor"/>
					<cell><term>Properties</term></cell>
				</row>
				<row bottom="minor">
					<cell right="minor"><m>P_1</m></cell>
					<cell><m>\ds \lap{ a y(t) \pm b z(t) } = a Y(s) \pm b Z(s) \vphantom{\frac{d}{d}}</m></cell>
				</row>
				<row bottom="minor">
					<cell right="minor"><m>P_2</m></cell>
					<cell><m>\ds \lap{ e^{at} y(t) } = Y(s-a) \vphantom{\frac{d}{d}}</m></cell>
				</row>
				<row bottom="minor">
					<cell right="minor"><m>P_3</m></cell>
					<cell><m>\ds \lap{ y'(t) } = s\,Y(s) - y(0) \vphantom{\frac{d}{d}}</m></cell>
				</row>
				<row bottom="minor">
					<cell right="minor"><m>P_4</m></cell>
					<cell><m>\ds \lap{ y''(t) } = s^2\,Y(s) - s\,y(0) - y'(0) \vphantom{\frac{d}{d}}</m></cell>
				</row>
				<row bottom="minor">
					<cell right="minor"><m>P_5</m></cell>
					<cell><m>\ds \lap{ y'''(t) } = s^3\,Y(s) - s^2\,y(0) - s\,y'(0) - y''(0) \vphantom{\frac{d}{d}}</m></cell>
				</row>
				<row>
					<cell right="minor"><m>P_6</m></cell>
					<cell><m>\ds \lap{ t^n y(t) } = (-1)^n \frac{d^{(n)}}{ds^{(n)}}Y(s) \vphantom{\frac{d}{d}}</m></cell>
				</row>
			</tabular>
		</table>

		<assemblage xml:id="lt-table-L1-L12"><title> ✳️ Common Laplace Transform and Properties </title>
			<p>
				Assume <m>F(s) = \lap{f(t)}</m>, <m>a</m>, <m>b</m> are constant, and <m>n=0,1,2,3,\ldots</m>
			</p>

			<p>
				<tabular top="minor"><row bottom="minor"><cell/></row><row><cell><me>\hphantom{------------HLINE HACK------------}</me></cell></row></tabular>
				<sidebyside widths="5% 30% 50% 15%" valign="middle">
					<p> <me> \text{ID} </me> </p>
					<p> <me> f(t) </me> </p>
					<p> <me> \lap{f(t)} = F(s) </me> </p>
					<p> <me> \text{Condition} </me> </p>
				</sidebyside>
				<tabular top="minor"><row bottom="minor"><cell top="minor"/></row><row><cell><me>\hphantom{------------HLINE HACK------------}</me></cell></row></tabular>
				<sidebyside widths="5% 30% 50% 15%" valign="middle">
					<p> <me>L_{1}</me> </p>
					<p> <me> 1 </me> </p>
					<p> <me>\frac{1}{s}</me> </p>
					<p> <me>\vphantom{\int}s &gt; 0</me> </p>
				</sidebyside>
				<tabular><row bottom="minor"><cell/></row><row><cell><me>\hphantom{------------HLINE HACK------------}</me></cell></row></tabular>
				<sidebyside widths="5% 30% 50% 15%" valign="middle">
					<p> <me>L_{2}</me> </p>
					<p> <me> e^{at} </me> </p>
					<p> <me>\frac{1}{s - a}</me> </p>
					<p> <me>\vphantom{\int}s &gt; 0</me> </p>
				</sidebyside>
				<tabular><row bottom="minor"><cell/></row><row><cell><me>\hphantom{------------HLINE HACK------------}</me></cell></row></tabular>
				<sidebyside widths="5% 30% 50% 15%" valign="middle">
					<p> <me>L_{3}</me> </p>
					<p> <me> t^n </me> </p>
					<p> <me>\frac{n!}{s^{n+1}}</me> </p>
					<p> <me>\vphantom{\int}s &gt; 0</me> </p>
				</sidebyside>
				<tabular><row bottom="minor"><cell/></row><row><cell><me>\hphantom{------------HLINE HACK------------}</me></cell></row></tabular>
				<sidebyside widths="5% 30% 50% 15%" valign="middle">
					<p> <me>L_{4}</me> </p>
					<p> <me>\sin(bt)</me> </p>
					<p> <me>\frac{b}{s^2+b^2}</me> </p>
					<p> <me>\vphantom{\int}s &gt; 0</me> </p>
				</sidebyside>
				<tabular><row bottom="minor"><cell/></row><row><cell><me>\hphantom{------------HLINE HACK------------}</me></cell></row></tabular>
				<sidebyside widths="5% 30% 50% 15%" valign="middle">
					<p> <me>L_{5}</me> </p>
					<p> <me>\cos(bt)</me> </p>
					<p> <me>\frac{s}{s^2+b^2}</me> </p>
					<p> <me>\vphantom{\int}s &gt; 0</me> </p>
				</sidebyside>
				<tabular><row bottom="minor"><cell/></row><row><cell><me>\hphantom{------------HLINE HACK------------}</me></cell></row></tabular>
				<sidebyside widths="5% 30% 50% 15%" valign="middle">
					<p> <me>L_{6}</me> </p>
					<p> <me> e^{at}\ t^n </me> </p>
					<p> <me>\ds\frac{n!}{(s-a)^{n+1}}</me> </p>
					<p> <me>\vphantom{\int}s &gt; a</me> </p>
				</sidebyside>
				<tabular><row bottom="minor"><cell/></row><row><cell><me>\hphantom{------------HLINE HACK------------}</me></cell></row></tabular>
				<sidebyside widths="5% 30% 50% 15%" valign="middle">
					<p> <me>L_{7}</me> </p>
					<p> <me> e^{at}\sin(bt) </me> </p>
					<p> <me>\frac{b}{(s-a)^2+b^2}</me> </p>
					<p> <me>\vphantom{\int}s &gt; a</me> </p>
				</sidebyside>
				<tabular><row bottom="minor"><cell/></row><row><cell><me>\hphantom{------------HLINE HACK------------}</me></cell></row></tabular>
				<sidebyside widths="5% 30% 50% 15%" valign="middle">
					<p> <me>L_{8}</me> </p>
					<p> <me> e^{at}\cos(bt) </me> </p>
					<p> <me>\frac{s-a}{(s-a)^2+b^2}</me> </p>
					<p> <me>\vphantom{\int}s &gt; a</me> </p>
				</sidebyside>
				<tabular><row bottom="minor"><cell/></row><row><cell><me>\hphantom{------------HLINE HACK------------}</me></cell></row></tabular>
				<sidebyside widths="5% 30% 50% 15%" valign="middle">
					<p> <me>L_{9}</me> </p>
					<p> <me> f'(t) </me> </p>
					<p> <me>sF(s) - f(0) </me> </p>
					<p> <me>\vphantom{\int}s &gt; 0</me> </p>
				</sidebyside>
				<tabular><row bottom="minor"><cell/></row><row><cell><me>\hphantom{------------HLINE HACK------------}</me></cell></row></tabular>
				<sidebyside widths="5% 30% 50% 15%" valign="middle">
					<p> <me>L_{10}</me> </p>
					<p> <me> f''(t) </me> </p>
					<p> <me>s^2F(s) - sf(0) - f'(0) </me> </p>
					<p> <me>\vphantom{\int}s &gt; 0</me> </p>
				</sidebyside>
				<tabular><row bottom="minor"><cell/></row><row><cell><me>\hphantom{------------HLINE HACK------------}</me></cell></row></tabular>
				<sidebyside widths="5% 30% 50% 15%" valign="middle">
					<p> <me>L_{11}</me> </p>
					<p> <me> f'''(t) </me> </p>
					<p> <me>s^3F(s) - s^2f(0) - sf'(0) - f''(0) </me> </p>
					<p> <me>\vphantom{\int}s &gt; 0</me> </p>
				</sidebyside>
				<tabular><row bottom="minor"><cell/></row><row><cell><me>\hphantom{------------HLINE HACK------------}</me></cell></row></tabular>
				<sidebyside widths="5% 30% 50% 15%" valign="middle">
					<p> <me>L_{12}</me> </p>
					<p> <me> t^n f(t) </me> </p>
					<p> <me>(-1)^n \frac{d^{(n)}}{ds^{(n)}}F(s)</me> </p>
					<p> <me>\vphantom{\int}s &gt; 0</me> </p>
				</sidebyside>
			</p>

		</assemblage>

		<assemblage xml:id="lt-table-L1"><title> ✳️ Common Laplace Transform and Properties </title>
			<p>
				Assume <m>F(s) = \lap{f(t)}</m>, <m>a</m>, <m>b</m> are constant, and <m>n=0,1,2,3,\ldots</m>.
			</p>

			<p>
				<sidebyside widths="5% 80% 15%" valign="middle">
					<p> <me> \text{ID} </me> </p>
					<p> <me> \lap{f(t)} = F(s) </me> </p>
					<p> <me> \text{Condition} </me> </p>
				</sidebyside>
				<tabular><row bottom="minor"><cell/></row><row><cell><me>\hphantom{------------HLINE HACK------------}</me></cell></row></tabular>
				<sidebyside widths="5% 80% 15%" valign="middle">
					<p> <me>L_1</me> </p>
					<p> <me>\lap{ 1 } = \frac{1}{s}</me> </p>
					<p> <me>\vphantom{\int}s &gt; 0</me> </p>
				</sidebyside>
				<sidebyside widths="5% 80% 15%" valign="middle">
					<p> <me>L_2</me> </p>
					<p> <me>\lap{ e^{at} } = \frac{1}{s - a}</me> </p>
					<p> <me>\vphantom{\int}s &gt; 0</me> </p>
				</sidebyside>
				<sidebyside widths="5% 80% 15%" valign="middle">
					<p> <me>L_3</me> </p>
					<p> <me>\lap{ t^n } = \frac{n!}{s^{n+1}}</me> </p>
					<p> <me>\vphantom{\int}s &gt; 0</me> </p>
				</sidebyside>
				<sidebyside widths="5% 80% 15%" valign="middle">
					<p> <me>L_4</me> </p>
					<p> <me>\lap{\sin(bt)} = \frac{b}{s^2+b^2}</me> </p>
					<p> <me>\vphantom{\int}s &gt; 0</me> </p>
				</sidebyside>
				<sidebyside widths="5% 80% 15%" valign="middle">
					<p> <me>L_5</me> </p>
					<p> <me>\lap{\cos(bt)} = \frac{s}{s^2+b^2}</me> </p>
					<p> <me>\vphantom{\int}s &gt; 0</me> </p>
				</sidebyside>
				<sidebyside widths="5% 80% 15%" valign="middle">
					<p> <me>L_6</me> </p>
					<p> <me>\lap{ e^{at}\ t^n } = \ds\frac{n!}{(s-a)^{n+1}}</me> </p>
					<p> <me>\vphantom{\int}s &gt; a</me> </p>
				</sidebyside>
				<sidebyside widths="5% 80% 15%" valign="middle">
					<p> <me>L_7</me> </p>
					<p> <me>\lap{ e^{at}\sin(bt) } = \frac{b}{(s-a)^2+b^2}</me> </p>
					<p> <me>\vphantom{\int}s &gt; a</me> </p>
				</sidebyside>
				<sidebyside widths="5% 80% 15%" valign="middle">
					<p> <me>L_8</me> </p>
					<p> <me>\lap{ e^{at}\cos(bt) } = \frac{s-a}{(s-a)^2+b^2}</me> </p>
					<p> <me>\vphantom{\int}s &gt; a</me> </p>
				</sidebyside>
				<sidebyside widths="5% 80% 15%" valign="middle">
					<p> <me>L_9</me> </p>
					<p> <me>\lap{ f'(t) } = sF(s) - f(0) </me> </p>
					<p> <me>\vphantom{\int}s &gt; 0</me> </p>
				</sidebyside>
				<sidebyside widths="5% 80% 15%" valign="middle">
					<p> <me>L_{10}</me> </p>
					<p> <me>\lap{ f''(t) } = s^2F(s) - sf(0) - f'(0) </me> </p>
					<p> <me>\vphantom{\int}s &gt; 0</me> </p>
				</sidebyside>
				<sidebyside widths="5% 80% 15%" valign="middle">
					<p> <me>L_{11}</me> </p>
					<p> <me>\lap{ f'''(t) } = s^3F(s) - s^2f(0) - sf'(0) - f''(0) </me> </p>
					<p> <me>\vphantom{\int}s &gt; 0</me> </p>
				</sidebyside>
				<sidebyside widths="5% 80% 15%" valign="middle">
					<p> <me>L_{12}</me> </p>
					<p> <me>\lap{ t^n f(t) } = (-1)^n \frac{d^{(n)}}{ds^{(n)}}F(s)</me> </p>
					<p> <me>\vphantom{\int}s &gt; 0</me> </p>
				</sidebyside>
			</p>

		</assemblage>

		<assemblage xml:id="lt-linearity-property-P6"><title> ✳️ Laplace Transform Property <m>P_1</m> </title>
			<p>
				Let <m>F(s) = \lap{f(t)}</m> and <m>G(s) = \lap{g(t)}</m>.
				<dl width="narrow">
					<li><title> <m>P_1</m> </title>
						<m>\ds \lap{ a f(t) \pm b g(t) } = a F(s) \pm b G(s), \quad a, b </m> are constants
					</li>
					<li><title> <m>P_2.</m> </title>
						<m>\ds \lap{ e^{at} f(t) } = F(s-a), \quad a </m> is a constant
					</li>
					<li><title> <m>P_3.</m> </title>
						<m>\ds \lap{ f'(t) } = sF(s) - f(0) </m>
					</li>
					<li><title> <m>P_4.</m> </title>
						<m>\ds \lap{ f''(t) } = s^2F(s) - sf(0) - f'(0) </m>
					</li>
					<li><title> <m>P_5.</m> </title>
						<m>\ds \lap{ f'''(t) } = s^3F(s) - s^2f(0) - sf'(0) - f''(0) </m>
					</li>
					<li><title> <m>{\LARGE \vphantom{\int}}P_6.</m> </title>
						<m>\ds \lap{ t^n f(t) } = (-1)^n \frac{d^{(n)}}{ds^{(n)}}F(s), \quad n = 1, 2, 3, \ldots </m>
					</li>
				</dl>
			</p>
		</assemblage>

		<p>
			This section covers the final step in solving differential equations using the Laplace Transform Method: finding the inverse Laplace transform. The focus is on converting the algebraic equation with unknown function <m>Y(s)</m> back to the original function <m>y(t)</m>. Several methods and techniques are introduced to handle different cases where direct computation isn't possible.
		</p>
		
		<p>
			<assemblage><title> ✳️ Summary of the Key Ideas </title>
				<p>
						<term>Common Forms:</term> A table of common Laplace transforms is provided, which doubles as a reference for inverse transforms. The focus is on recognizing forms that match the table entries for functions like <m>\sin(bt), \cos(bt)</m>, and others.
					</p>

					<p>
						<term>Direct Computation:</term> When the function of <m>s</m> directly matches a form in the common Laplace transform table, the inverse Laplace transform can be easily computed.
					</p>
					
					<p>
						<term>Modifying Functions:</term> When a function doesn't match a known form, minor modifications, such as multiplying by missing constants or splitting fractions, can help.
					</p>
					
					<p>
						<term>Completing the Square:</term> When dealing with quadratic expressions in the denominator, especially when the discriminant is negative, completing the square can transform the expression into a form that matches known inverse Laplace transforms. Several examples demonstrate this technique.
					</p>

					<p>
						<term>Partial Fraction Decomposition:</term> For more complex rational functions, partial fraction decomposition breaks down the function into simpler fractions that match the common transform forms.
					</p>
			</assemblage>
		</p>

		<p>
			Completing the square is an essential technique for transforming quadratic expressions that don't directly match a form in the table of common Laplace transforms. However, it's not the only strategy available. In this section, we'll explore another important technique: partial fraction decomposition. This method is useful for breaking down complex fractions into simpler components that can each be matched with forms in the Laplace transform table.
		</p>
	
		<p>
			Two other forms we may wish to match when we study Laplace transforms are 
			<me>
				\frac{b}{(s-a)^2 + b^2} \mbox{ and } \frac{s-a}{(s-a)^2 + b^2}.
			</me>
			As before, we work toward <em> making the denominator match first</em>, and then we sort out the numerator second.
		</p>

		<p>
			When we want to take the inverse Laplace transform of a rational function with a second-degree polynomial in the denominator, we may complete the square or we may do a partial fraction decomposition. How will we know which is appropriate?	Here are a few guidelines for you to consider.
			<ul>
				<li>
					Does the denominator factor in an obvious way?  If so, factor the denominator and do a partial fraction decomposition if necessary.
				</li>
				<li>
					If the denominator does not factor in an obvious way, try completing the square.
				</li>
				<li>
					If you end up with addition outside of the parentheses, as in <m>(s - a)^2 + b^2,</m> then you should aim to match <xref ref="LT-Table-L7" text="custom"><m>L7</m></xref> and/or <xref ref="LT-Table-L8" text="custom"><m>L8</m></xref>.
				</li>
				<li>
					If instead you end up with subtraction outside the parentheses, as in <m>(s - a)^2 - b^2,</m> then you should factor and do a partial fraction decomposition. You may consider using the quadratic formula if the factorization is not obvious to you.
				</li>
				<li>
					If you end up with no terms outside the parentheses, as in <m>(s - a)^2,</m> then use <xref ref="LT-Table-L6" text="custom"><m>L6</m></xref>.
				</li>
			</ul>
		</p>

		<p>
			<assemblage><title> ✳️ Summary of the Key Ideas </title>
				<p>
					<term> <em> Laplace Transform Method</em> </term>
						
					</p>
			</assemblage>
		</p>

		<p>
			<assemblage><title> ✳️ Summary of the Key Ideas </title>
				<p>
					<term> <em> PIECEWISE SHIT </em> </term>
						
					</p>
			</assemblage>
		</p>

	</worksheet>

</subsubsection>