<subsection><title> Standard Exercises </title>
<exercises><title> Standard Exercises </title>

	<exercise>

		<p>
			Determine if <m>y = c_1 \sin x + c_2 \cos x</m> is a solution to the differential equation 
			<men xml:id="diff_eqn_soln">
				\frac{d^2y}{dx^2} + y = 0
			</men>.
		</p>

		<p>
			<answer>
				<p>
					<me> y = c_1 \sin x + c_2 \cos x </me> is a solution to the differential equation <xref ref="diff_eqn_soln"/>.
				</p>
			</answer>
			
			<solution>
				<p>
					We need to substitute into the differential equation. In order to substitute into the left hand side, we need to know the second derivative. So we begin by finding that.
				
					<md>
						<mrow>						y	=\amp\ c_1 \sin x + c_2 \cos x			</mrow>
						<mrow>	\Rightarrow \quad   y'	=\amp\ c_1 \cos x - c_2 \sin x			</mrow>
						<mrow>	\Rightarrow \quad   y''	=\amp\ -c_1 \sin x - c_2 \cos x			</mrow>	
					</md>
					
					Now we can substitute into the differential equation:

					<md>
						<mrow>	\frac{d^2y}{dx^2} + y	=\amp\ 0							</mrow>
						<mrow>	\Big[ -c_1 \sin x - c_2 \cos x \Big] + \Big[ c_1 \sin x + c_2 \cos x \Big]	=\amp\ 0	</mrow>
						<mrow>	-c_1 \sin x - c_2 \cos x + c_1 \sin x + c_2 \cos x	=\amp\ 0	</mrow>
						<mrow>	0	=\amp\ 0	\quad✅	</mrow>
					</md>
					
					Since when we substitute in to the differential equation, we find that the LHS is equal to the RHS, we have verified that <m>y = c_1 \sin x + c_2 \cos x</m> is a solution to the differential equation <m>\ds \frac{d^2y}{dx^2} + y = 0.</m>
				</p>
			</solution>
		</p>

	</exercise>

	<exercise><title> Verifying Solutions to Initial-Valued Problems </title>

		<statement>
			<p>
				To verify that the function <m>y = -3e^{x^2} + 3</m> is a particular solution to the initial-value problem
				<me>
					\frac{dy}{dx} = 2xy - 6x, \qquad y(0) = 0
				</me>,
				you must show two things. Explain what you must show and show them.
			</p>
		</statement>
		
		<solution>
			<p>
				To verify that the function <m>y = -3e^{x^2} + 3</m> is a particular solution to the initial-value problem
				<me>
					\frac{dy}{dx} = 2xy - 6x, \qquad y(0) = 0
				</me>,
				we must show the following two things:
			</p>

			<ul>
				<li>
					<p>
						<m>y = -3e^{x^2} + 3</m> satisfies the differential equation.
					</p>
				</li>
				<li>
					<p>
						<m>y = -3e^{x^2} + 3</m> satisfies the initial condition.
					</p>
				</li>
			</ul>

			<p>
				Let's start by showing that the function <m>y = -3e^{x^2} + 3</m> satisfies the differential equation.
			</p>

			<p>
				<md>
					<mrow>							\frac{dy}{dx}	=\amp\ 2xy - 6x					</mrow>
					<mrow>	\frac{d}{dx}\left[-3e^{x^2} + 3\right]	=\amp\ 2x(-3e^{x^2} + 3) - 6x	</mrow>
					<mrow>	-3\frac{d}{dx}\left[e^{x^2}\right]+ 0	=\amp\ -6xe^{x^2} + 6x - 6x		</mrow>
					<mrow>			-3\left(e^{x^2} \cdot 2x\right)	=\amp\ -6xe^{x^2}				</mrow>
					<mrow>								-6xe^{x^2}	=\amp\ -6xe^{x^2}\quad✅		  </mrow>
				</md>
			</p>
			
			<p>
				Now, let's show that the function satisfies the initial condition <m>y(0) = 0</m>.
			</p>

			<p>
				<md>
					<mrow>	y(0)	=\amp\ -3e^{0^2} + 3	</mrow>
					<mrow>		0	=\amp\ -3e^0 + 3		</mrow>
					<mrow>		0	=\amp\ -3 + 3			</mrow>
					<mrow>		0	=\amp\ 0\quad✅		  </mrow>
				</md>
			</p>

		</solution>

	</exercise>
	
	<exercise>
		<p>
			Determine if <m>\ds y = c_{1}e^{2x} + c_{2}xe^{2x}</m> a solution of the differential equation
			<me>
				\frac{d^{2}y}{dx^{2}} - 4\frac{dy}{dx} + 4y = 0
			</me>.
		</p>

		<p>
			<answer>
				<p>
					It is a solution.
				</p>
			</answer>
		
			<solution>
				<p>
					The function <m>\ds y = c_{1}e^{2x} + c_{2}xe^{2x}</m> is a solution to the differential equation
					<me>
						\frac{d^{2}y}{dx^{2}} - 4\frac{dy}{dx} + 4y = 0
					</me> 
					since plugging it in gives
					<me>
						4c_{1}e^{2x} + 4c_{2}xe^{2x} - 4(2c_{1}e^{2x} + c_{2}e^{2x}) + 4(c_{1}e^{2x} + c_{2}xe^{2x}) = 0
					</me>
					<me>
						0 = 0 \quad ✅
					</me>
				</p>
			</solution>
		</p>
	</exercise>

	<exercise>
		<p>
			Consider the differential equation
			<me>
				x^2y' + xy = 1
			</me>
			<ol>
				<li>
					Verify that the function
					<me>
						y = \frac{\ln x + c}{x}
					</me>
					a solution to this differential equation.
				</li>
				<li>
					Find the particular solution that corresponds to the condition <m>y(9)=8</m>.
				</li>
			</ol>
		</p>

		<p>
			<answer>
				<p>
					<ol>
						<li>
							Yes
						</li>
						<li>
							<m>c = 72-\ln(9)</m>, so
							<m>\ds y = \frac{\ln x + 72-\ln(9)}{x} </m> is the particular solution
						</li>
					</ol>
				</p>
			</answer>

			<solution>
				<p>
					<ol>
						<li>
							<p>
								To show this, let's first move all terms to one side of the equation, so
							</p>

							<p>
								<me>
									\os{\large{\text{LHS}}}{\overline{x^2y^\prime + xy - 1}} = 0
								</me>
							</p>

							<p>
								Now, we will compute <m>y^\prime</m> and plug it and <m>y</m> into the left hand side (LHS) of the equation to see if it simplifies to zero.
							</p>

							<p>
								<md>
									<mrow>
										\os{\large{\text{LHS}}}{\overline{x^2y^\prime + xy - 1}}
											=\amp\ x^2\left(\frac{1 - \ln x - c}{x^2}\right) + x\left(\frac{\ln x + c}{x}\right) - 1
									</mrow>
									<mrow>	=\amp\ 1 - \ln x - c + \ln x + c - 1	</mrow>
									<mrow>	=\amp\ 0	\quad ✅					  </mrow>
								</md>
							</p>

							<p>
								Applying <m>8=y(9)</m> gives
								<me>
									8 = \frac{\ln 9 + c}{9} \quad \implies \quad c = 72-\ln(9)
								</me>
								and so the particular solution is
								<me>
									\ds y = \frac{\ln x + 72-\ln(9)}{x}
								</me>
							</p>
						</li>
					</ol>
				</p>
			</solution>
		</p>
	</exercise>

	<exercise>
		<p>
			Consider the differential equation
			<me>
				y^\prime = y-y^2
			</me>
			<ol>
				<li>
					<p>
						Verify if any of the following functions are a solution to this differential equation.
						<ol type="i.">
							<li> <m>\quad\ds y=c\sin(-x)</m></li>
							<li> <m>\quad\ds y=\frac{1}{1+ce^{-x}}</m></li>
							<li> <m>\quad\ds y=\frac{1}{c+x^2}</m></li>
						</ol>
					</p>
				</li>
				<li>
					<p>
						For all solutions found in (a), find <m>c</m> that corresponds to <m>y(0) = 7</m>.
					</p>
				</li>
			</ol>
		</p>

		<p>
			<answer>
				<p>
					<line>b. <m>\ds y=\frac{1}{1+ce^{-x}}</m></line>
					<line>
						<m>c = \frac{1}{7}-1 \approx -0.857</m>, so
						<m>\ds y = \frac{1}{1+(-0.857)e^{-x}} </m> is the particular solution
					</line>
				</p>
			</answer>

			<solution>

				<ol>
					<li>
						<p>
							To show this, let's first move all terms to one side of the equation, so
						</p>

						<p>
							<me>
								\os{\large{\text{LHS}}}{\overline{y^{\prime}-y+y^2}} = 0
							</me>
						</p>

						<p>
							For each of the functions above, we will compute <m>y^\prime</m> and plug it and <m>y</m> into the left hand side (LHS) of the equation to see if it simplifies to zero.
						</p>

						<ol type="i.">
							<li>
								<p>
									<me>
										y=c\sin(-x) \quad \implies \quad y^\prime = -c\cos(-x)
									</me>
								</p>

								<p>
									<md>
										<mrow>
											\os{\large{\text{LHS}}}{\overline{y^{\prime}-y+y^2}}
												=\amp\ -c\cos(-x) - c\sin(-x) + c^2\sin^2(-x)
										</mrow>
										<mrow>	=\amp\ -c\cos(x) + c\sin(x) + c^2\sin^2(x)	</mrow>
									</md>
									It can be difficult to see why this doesn't simplify to zero. However, if we assume it does, then plugging any <m>x</m> into this expression must also give you zero. So, if you can find one <m>x</m> value where this doesn't happen, then this function cannot be a solution. 
								</p>

								<p>
									Letting <m>x=0</m> gives <m>-c</m>, but <m>c</m> can be any constant, so <m>y = c\sin(-x)</m> is not a solution.
								</p>
							</li>
							<li>
								<p>
									<me>
										y = \frac{1}{c+x^2} \quad \implies \quad y^\prime = \frac{-2x}{(c+x^2)^2}
									</me>
								</p>

								<p>
									<md>
										<mrow>
											\os{\large{\text{LHS}}}{\overline{y^{\prime}-y+y^2}}
												=\amp\ \frac{-2x}{(c+x^2)^2} - \frac{1}{c+x^2} - \frac{1}{(c+x^2)^2}
										</mrow>
										<mrow>	
												=\amp\ \frac{-2x}{(c+x^2)^2} - \frac{1}{c+x^2}\cdot \frac{c+x^2}{c+x^2} - \frac{1}{(c+x^2)^2}
										</mrow>
										<mrow>	=\amp\ \frac{-2x}{(c+x^2)^2} - \frac{c+x^2}{(c+x^2)^2} - \frac{1}{(c+x^2)^2}	</mrow>
										<mrow>	=\amp\ \frac{-2x-c-x^2-1}{(c+x^2)^2}	\ne 0 \quad ❌						  </mrow>
									</md>
								</p>

								<p>
									Letting <m>x=0</m> gives <m>-1/c</m>, but since <m>c</m> can be any constant, <m>\ds y = \frac{1}{c+x^2}</m> is not a solution. 
								</p>
							</li>
							<li>
								<p>
									<me>
										y = \frac{1}{1+ce^{-x}} \quad \implies \quad y^\prime = \frac{ce^{-x}}{(1+ce^{-x})^2}
									</me>
								</p>

								<p>
									<md>
										<mrow>
											\os{\large{\text{LHS}}}{\overline{y^{\prime}-y+y^2}}
												=\amp\ \frac{ce^{-x}}{(1+ce^{-x})^2} - \frac{1}{1+ce^{-x}} - \frac{1}{(1+ce^{-x})^2}
										</mrow>
										<mrow>	
												=\amp\ \frac{ce^{-x}}{(1+ce^{-x})^2} - \frac{1+ce^{-x}}{(1+ce^{-x})^2} - \frac{1}{(1+ce^{-x})^2}
										</mrow>
										<mrow>	=\amp\ \frac{ce^{-x}-1-ce^{-x}-1}{(1+ce^{-x})^2}	</mrow>
										<mrow>	=\amp\ \frac{0}{(1+ce^{-x})^2}	= 0 \quad ✅						  </mrow>
									</md>
								</p>

								<p>
									So <m>\ds y = \frac{1}{1+ce^{-x}}</m> is a solution.
								</p>
							</li>
						</ol>
					</li>
					<li>
						<p>
							Setting <m>y(0)=7</m> we get
						</p>

						<p>
							<me>
								7 = \frac{1}{1+c} \quad \implies \quad c = \frac{1}{7}-1 = -\frac{6}{7}
							</me>
						</p>

						<p>
							So the particular solution for this initial condition is 
							<me>
								y = \frac{1}{1-\frac{6}{7}e^{-x}}
							</me>
						</p>
					</li>
				</ol>

			</solution>
		</p>
	</exercise>

	<exercisegroup cols="2"><title> General Solution </title>

		<introduction>
			<p>
				Find the general solution for each of the following differential equations. Combine constants where appropriate.
			</p>
		</introduction>

		<exercise>
			<statement>
				<m> \ds \frac{dy}{dx} = 2x - 5 </m>
			</statement>
			<answer>
				<p>
					<m> \ds y = x^2 - 5x + C </m>
				</p>
			</answer>
		</exercise>

		<exercise>
			<statement>
				<m> \ds \frac{d}{dx}[y] = e^{2x} </m>
			</statement>
			<answer>
				<p>
					<m> \ds y = \frac{1}{2}e^{2x} + C </m>
				</p>
			</answer>
		</exercise>

		<exercise>
			<statement>
				<m> \ds \frac{d}{dx}[x \cdot y] = \cos(x) </m>
			</statement>
			<answer>
				<p>
					<m> \ds y = \frac{\sin(x)}{x} + \frac{C}{x} </m>
				</p>
			</answer>
		</exercise>

		<exercise>
			<statement>
				<m> \ds \frac{dy}{dt} = \frac{1}{t^2} + t </m>
			</statement>
			<answer>
				<p>
					<m> \ds y = -\frac{1}{t} + \frac{1}{2}t^2 + C </m>
				</p>
			</answer>
		</exercise>

		<exercise>
			<statement>
				<m> \ds \frac{dy}{dx} = x e^x </m>
			</statement>
			<answer>
				<p>
					<m> \ds y = (x - 1)e^x + C </m>
				</p>
			</answer>
		</exercise>

		<exercise>
			<statement>
				<m> \ds \left[\sin(x) \cdot y\right]^\prime = \cos^2(x) </m>
			</statement>
			<answer>
				<p>
					<m> \ds y = \frac{\sin(x)}{2} + \frac{C}{\sin(x)} </m>
				</p>
			</answer>
		</exercise>

		<exercise>
			<statement>
				<m> \ds y' = \ln(x) + x^2 </m>
			</statement>
			<answer>
				<p>
					<m> \ds y = x \ln(x) - x + \frac{1}{3}x^3 + C </m>
				</p>
			</answer>
		</exercise>

		<exercise>
			<statement>
				<m> \ds \frac{d}{dP}\left[e^P \cdot Q\right] = P </m>
			</statement>
			<answer>
				<p>
					<m> \ds Q = e^{-P} \left(\frac{P}{e^P} + C \right) </m>
				</p>
			</answer>
		</exercise>

	</exercisegroup>

	<exercisegroup cols="2"><title> Particular Solution </title>

		<introduction>
			<p>
				Find the particular solution for each of the following differential equations with the given initial condition.
			</p>
		</introduction>

		<exercise>
			<statement>
				<m> \ds \frac{dy}{dx} = 3x^2 + 2, \ \ y(1) = 4 </m>
			</statement>
			<answer>
				<p>
					<m> \ds y = x^3 + 2x + 1 </m>
				</p>
			</answer>
		</exercise>

		<exercise>
			<statement>
				<m> \ds \frac{d}{dt}[y] = \sin(t), \ \ y(0) = 2 </m>
			</statement>
			<answer>
				<p>
					<m> \ds y = -\cos(t) + 3 </m>
				</p>
			</answer>
		</exercise>

		<exercise>
			<statement>
				<m> \ds \frac{d}{dx}[x \cdot y] = e^x, \ \ y(1) = 0 </m>
			</statement>
			<answer>
				<p>
					<m> \ds y = \frac{e^x}{x} - \frac{e}{x} </m>
				</p>
			</answer>
		</exercise>

		<exercise>
			<statement>
				<m> \ds \frac{dy}{dx} = x^3 - 4, \ \ y(2) = 1 </m>
			</statement>
			<answer>
				<p>
					<m> \ds y = \frac{x^4}{4} - 4x + 5 </m>
				</p>
			</answer>
		</exercise>

		<exercise>
			<statement>
				<m> \ds \frac{dR}{dh} = \frac{1}{h} + h, \ \ R(1) = 3 </m>
			</statement>
			<answer>
				<p>
					<m> \ds R = \ln|h| + \frac{h^2}{2} + \frac{5}{2} </m>
				</p>
			</answer>
		</exercise>

		<exercise>
			<statement>
				<m> \ds \frac{d}{dx}\left[e^x \cdot y\right] = \sin(x), \ \ y(0) = 2 </m>
			</statement>
			<answer>
				<p>
					<m> \ds y = e^{-x} \left(-\cos(x) + 3 \right) </m>
				</p>
			</answer>
		</exercise>

		<exercise>
			<statement>
				<m> \ds y' = \cos(x) + x^2, \ \ y(0) = -2 </m>
			</statement>
			<answer>
				<p>
					<m> \ds y = \sin(x) + \frac{x^3}{3} - 2 </m>
				</p>
			</answer>
		</exercise>

		<exercise>
			<statement>
				<m> \ds \frac{d}{dx}\left[\tan(x) \cdot y\right] = \sec^2(x), \quad y\left(\frac{\pi}{4}\right) = 1 </m>
			</statement>
			<answer>
				<p>
					<m> \ds y = \frac{x \sec^2(x)}{\tan(x)} + \frac{\pi/4 - 1}{\tan(x)} </m>
				</p>
			</answer>
		</exercise>

	</exercisegroup>

	<exercise>
		<statement>
			<p>
				Attempt to apply direct integration to the differential equation
				<me> \frac{dy}{dx} = x + y</me>.
				Get to the point where it becomes clear that you cannot solve for <m>y</m> directly. What is the obstacle?
			</p>
		</statement>
		<answer>
			<p>
				<p>
				Integrating both sides gives
				<md>
					<mrow> \int \frac{dy}{dx}\ dx	\amp = \int\left(x + y\right)\ dx 		</mrow>
					<mrow> 					y + C_1	\amp = \int x\ dx + \int y\ dx 			</mrow>
					<mrow> 					y + C_1	\amp = \frac12 x^2 + C_2 + \int y\ dx	</mrow>
					<mrow> 			y - \int y\ dx	\amp = \frac12 x^2 + C_2 - C_1  		</mrow>
				</md>
				Without knowing <m>y</m>, we cannot simplify <m>\int y\ dx</m>. So the obstacle is that we are unable to combine the these <m>y</m> variables into a single <m>y</m> on the left side. 
			</p>
			</p>
		</answer>
	</exercise>

	<exercisegroup>
	
		<introduction>
			<p>
				Convert this idea from the integrating factor into some exercises for the direct integration method.
			</p>
		</introduction>
	
		<exercise>
			<statement>
				<note>
					To Readers: This is not an exercise (yet).  Ignore it.
				</note>
				<p>
					In this chapter, we will study a solution technique that will help us solve differential equations that are first order and linear. Consider this (carefully selected) example.
					<men xml:id="original_de">
						x^7 \cdot \frac{dy}{dx} + 7x^{6}\cdot y = e^x
					</men>
					Notice that the dependent variable is <m>y</m> and the independent variable is <m>x</m>, so we seek to find a formula for <m>y</m> in terms of <m>x</m>. The DE is also first order and linear.
				</p>
			</statement>
			<solution>
				<p>
					What makes this DE special is that the left hand side can be rewritten as follows.
					<men xml:id="rewritten_de">
						\frac{d}{dx}\Big(x^7 \cdot y \Big) = e^x
					</men>
					We can verify this by actually using the product rule to take the derivative on the left hand side:
					<md>
						<mrow>\frac{d}{dx}\Big(x^7 \cdot y \Big)</mrow>
						<mrow>   =\amp\  \frac{d}{dx}\Big(\underbrace{x^7}_{f(x)} \cdot \underbrace{y}_{g(x)} \Big)</mrow>
						<mrow>   =\amp\ f(x) \cdot g'(x) + f'(x) \cdot g(x)</mrow>
						<mrow>   =\amp\ x^7 \cdot \frac{dy}{dx} + 7x^{6}\cdot y</mrow>
					</md>
				</p>
						
				<p>
					Now that we have confirmed that Equation <xref ref="rewritten_de"/> is equivalent to Equation <xref ref="original_de"/>, we can proceed in solving the DE. 
				</p>
						
				<p>
					The unknown function we want to solve for is <m>y</m>, and it is part of the product we are taking the derivative of in Equation <xref ref="rewritten_de"/>. So we begin by undoing that differentiation by integrating both sides of Equation <xref ref="rewritten_de"/> with respect to <m>x</m>:
					
					<md>
						<mrow>
							\int \frac{d}{dx}\Big(x^7 \cdot y \Big) dx =\amp\ \int e^x dx
						</mrow>
						<mrow>
							x^7 \cdot y	  =\amp\ e^x + C
						</mrow>
					</md>
				</p>
						
				<p>
					We can now just divide both sides of Equation by the coefficient on <m>y</m> to obtain the general solution.
					<me>y = \frac{e^x}{x^7} + \frac{C}{x^7}</me>
				</p>
						
				<p>
					Recall that we said this was a carefully selected DE. This very special DE had the property that we could undo the product rule on its left hand side. This is not, in general, the case when we encounter a first order linear DE. For example, consider this DE.
				</p>
			</solution>
		</exercise>
	
	</exercisegroup>

</exercises>
</subsection>