<?xml version="1.0" encoding="UTF-8" ?>

<!--********************************************************************-->

<exercises>
<title>Exercises</title>

<!--========== Exercise Group 1 ==========--> 
<exercisegroup>
<title>
<p>

</p>
<p/> <!-- added for vertical space -->
</title>
	<exercise> <!--== Problem 1 ==-->
		<statement>
			
		</statement>
		<solution>
			<m> \DS g(t) = t^3 e^{-9t} </m>
		</solution>
		<answer>
			
		</answer>
	</exercise>

</exercisegroup>

<!--========== Exercise Group 2 ==========--> 
<exercisegroup>
<title>
<p>

</p>
<p/> <!-- added for vertical space -->
</title>
	<exercise> <!--== Problem 2 ==-->
		<statement>
			<m> \DS g(t) = t^3 e^{-9t} </m>
		</statement>
		<solution>
			
			<md>
				<mrow>  G(s)	 \amp =  \LAP\{ g(t) \} </mrow>
				<mrow>   \amp =  \LAP\{ t^3 e^{-9t} \} </mrow>
				<mrow>   \amp =  \frac{3!}{\big(s-(-9)\big)^{3+1}} \mbox{ (by L6)} </mrow>
				<mrow>   \amp =  \frac{6}{(s+9)^4} </mrow>
 
			</md>
			
		</solution>
		<answer>
			<m> \DS G(s) = \frac{6}{(s+9)^4} </m>
		</answer>
	</exercise>

</exercisegroup>

<!--========== Exercise Group 3 ==========--> 
<exercisegroup>
<title>
<p>

</p>
<p/> <!-- added for vertical space -->
</title>
	<exercise> <!--== Problem 3 ==-->
		<statement>
			<m> \DS h(t) = e^{2t} - t^3 + t^2 - \sin (5t) </m>
		</statement>
		<solution>
			
			<md>
				<mrow>  H(s)	 \amp =  \LAP\{ h(t) \} </mrow>
				<mrow>   \amp =  \LAP\{ e^{2t} - t^3 + t^2 - \sin (5t) \} </mrow>
				<mrow>   \amp =  \LAP\{ e^{2t} \} - \LAP\{ t^3 \} + \LAP\{ t^2 \} - \LAP\{ \sin(5t) \} \mbox{ (by L9)} </mrow>
				<mrow>   \amp =  \frac{1}{s-2} - \frac{3!}{s^{3+1}} + \frac{2!}{s^{2+1}} - \frac{5}{s^2 + 5^2} \mbox{ (by L2, L3 and L4)} </mrow>
				<mrow>   \amp =  \frac{1}{s-2} - \frac{6}{s^4} + \frac{2}{s^3} - \frac{5}{s^2 + 25} </mrow>
 
			</md>
			
		</solution>
		<answer>
			<m> \DS H(s) = \frac{1}{s-2} - \frac{5}{s^4} + \frac{2}{s^3} - \frac{5}{s^2 + 25} </m>
		</answer>
	</exercise>

</exercisegroup>

<!--========== Exercise Group 4 ==========--> 
<exercisegroup>
<title>
<p>

</p>
<p/> <!-- added for vertical space -->
</title>
	<exercise> <!--== Problem 4 ==-->
		<statement>
			<m> \DS f(t) = e^{-2t}\sin(2t) + t^2 e^{3t} </m>
		</statement>
		<solution>
			
			<md>
				<mrow>  F(s)	 \amp =  \LAP\{ f(t) \} </mrow>
				<mrow>   \amp =  \LAP\{ e^{-2t}\sin(2t) + t^2 e^{3t} \} </mrow>
				<mrow>   \amp =  \LAP\{ e^{-2t}\sin(2t)\} + \LAP\{t^2 e^{3t} \} \mbox{ (by L9)} </mrow>
				<mrow>   \amp =  \frac{2}{\big(s- (-2) \big)^2 + 2^2} + \frac{2!}{(s-3)^{2+1}} \mbox{ (by L7 and L6)} </mrow>
				<mrow>   \amp =  \frac{2}{(s+2)^2 + 4} + \frac{2}{(s-3)^3} </mrow>
 
			</md>
			
		</solution>
		<answer>
			<m> \DS F(s) = \frac{2}{(s+2)^2 + 4} + \frac{2}{(s-3)^3} </m>
		</answer>
	</exercise>

</exercisegroup>

<!--========== Exercise Group 5 ==========--> 
<exercisegroup>
<title>
<p>

</p>
<p/> <!-- added for vertical space -->
</title>
	<exercise> <!--== Problem 5 ==-->
		<statement>
			<m> \DS q(t) = 8t\cos(6t) + e^{3t}\sin(4t) </m>
		</statement>
		<solution>
			 For this solution, we will need to use property L14 wit <m> \DS f(t) = \cos(6t). </m>  We will need to know the Laplace transform for this function, so let's do that now.
			<md>
				<mrow>  F(s)	 \amp =  \LAP\{ f(t) \} </mrow>
				<mrow>   \amp =  \LAP\{ \cos(6t) \} </mrow>
				<mrow>   \amp =  \frac{s}{s^2 + 6^2} \mbox{ (by L5)} </mrow>
				<mrow>   \amp =  \frac{s}{s^2 + 36} </mrow>
 
			</md>
			 Then we have the following.  Note that when we use the quotient rule to take the derivative o <m> \DS F(s) </m> .
			<md>
				<mrow>  Q(s)	 \amp =  \LAP\{ q(t) \} </mrow>
				<mrow>   \amp =  \LAP\{ 8t\cos(6t) + e^{3t}\sin(4t) \} </mrow>
				<mrow>   \amp =  8\LAP\{ t\cos(6t) \} + \LAP\{ e^{3t}\sin(4t) \} \mbox{ (by L9)} </mrow>
				<mrow>   \amp =  8\LAP\{ t\cos(6t) \} + \frac{4}{(s-3)^2 + 4^2} \mbox{ (by L7)} </mrow>
				<mrow>   \amp =  8\LAP\{ t\cos(6t) \} + \frac{4}{(s-3)^2 + 16} </mrow>
				<mrow>   \amp =  8\LAP\{ t\cdot f(t) \} + \frac{4}{(s-3)^2 + 16} </mrow>
				<mrow>   \amp =  8\cdot (-1)^1 \cdot \frac{d}{ds}F(s) + \frac{4}{(s-3)^2 + 16} \mbox{ (by L14)} </mrow>
				<mrow>   \amp =  -8 \cdot \frac{d}{ds}\left( \frac{s}{s^2 + 36} \right) + \frac{4}{(s-3)^2 + 16} </mrow>
				<mrow>   \amp =  -8 \cdot  \frac{(s^2 + 36)\cdot 1 - s\cdot (2s + 0)}{(s^2 + 36)^2} + \frac{4}{(s-3)^2 + 16} </mrow>
				<mrow>   \amp =  -8 \cdot  \frac{s^2 + 36 - 2s^2}{(s^2 + 36)^2} + \frac{4}{(s-3)^2 + 16} </mrow>
				<mrow>   \amp =  -\frac{8(36 - s^2)}{(s^2 + 36)^2} + \frac{4}{(s-3)^2 + 16} </mrow>
 
			</md>
			
		</solution>
		<answer>
			<m> \DS Q(s) = -\frac{8(36 - s^2)}{(s^2 + 36)^2} + \frac{4}{(s-3)^2 + 16} </m>
		</answer>
	</exercise>

</exercisegroup>

<!--========== Exercise Group 6 ==========--> 
<exercisegroup>
<title>
<p>

</p>
<p/> <!-- added for vertical space -->
</title>
	<exercise> <!--== Problem 6 ==-->
		<statement>
			<m> \DS p(t) = t^2 \sin(3t) </m>
		</statement>
		<solution>
			 For this solution, we will need to use property L14 wit <m> \DS f(t) = \sin(3t). </m>  We will need to know the Laplace transform for this function, so let's do that now.
			<md>
				<mrow>  F(s)	 \amp =  \LAP\{ f(t) \} </mrow>
				<mrow>   \amp =  \LAP\{ \sin(3t) \} </mrow>
				<mrow>   \amp =  \frac{3}{s^2 + 3^2} \mbox{ (by L5)} </mrow>
				<mrow>   \amp =  \frac{3}{s^2 + 9}  </mrow>
			</md>
			 In using L14, we will also need the second derivative o <m> \DS F(s), </m> so we work to compute that now.  Note that we will use the chain rule when we take the derivative o <m> \DS (s^2 + 9)^2 </m> .
			<md>
				<mrow>  F'(s)	 \amp =  \frac{d}{ds}\left( \frac{3}{s^2 + 9} \right) </mrow>
				<mrow>   \amp =  \frac{(s^2 + 9) \cdot 0 - 3 \cdot (2s+0)}{(s^2 + 9)^2} </mrow>
				<mrow>   \amp =  \frac{-6s}{(s^2 + 9)^2} </mrow>
				<mrow>  F''(s)	 \amp =  \frac{(s^2 + 9)^2 \cdot (-6) - (-6s) \cdot 2(s^2 + 9)(2s)}{(s^2 + 9)^4} </mrow>
				<mrow>   \amp =  \frac{-6(s^2 + 9)^2 + 24s^2(s^2 +9)}{(s^2 + 9)^4} </mrow>
				<mrow>   \amp =  \frac{6(s^2 + 9)\left[-(s^2 + 9) + 4s^2\right]}{(s^2 + 9)^4} </mrow>
				<mrow>   \amp =  \frac{6\left[-s^2 - 9 + 4s^2\right]}{(s^2 + 9)^3} </mrow>
				<mrow>   \amp =  \frac{6\left[3s^2 - 9\right]}{(s^2 + 9)^3} </mrow>
				<mrow>   \amp =  \frac{18\left[s^2 - 3\right]}{(s^2 + 9)^3}  </mrow>
			</md>
			 Then we have the following.
			<md>
				<mrow>  P(s)	 \amp =  \LAP\{ t^2 \sin(3t) \} </mrow>
				<mrow>   \amp =  \LAP\{ t^2 f(t) \} </mrow>
				<mrow>   \amp =  (-1)^2 \cdot F''(s) \mbox{ (by L14)} </mrow>
				<mrow>   \amp =  1 \cdot \frac{18\left[s^2 - 3\right]}{(s^2 + 9)^3} </mrow>
				<mrow>   \amp =  \frac{18\left[s^2 - 3\right]}{(s^2 + 9)^3} </mrow>
 
			</md>
			
		</solution>
		<answer>
			<m> \DS P(s) = \frac{18\left[s^2 - 3\right]}{(s^2 + 9)^3} </m>
		</answer>
	</exercise>

</exercisegroup>

</exercises>
