<?xml version="1.0" encoding="UTF-8" ?>

<!--********************************************************************-->

<exercises>
<title>Exercises</title>

<!--========== Exercise Group 1 ==========--> 
<exercisegroup>
<title>
<p>
 Express each function below in terms of unit step functions andthen compute its Laplace transform.
</p>
<p/> <!-- added for vertical space -->
</title>
	<exercise> <!--== Problem 1 ==-->
		<statement>
			<m> \DS g(t) = \left\{ \begin{array}{ll} 0,	\amp t \le 1\\ 2,	\amp 1 \le t \le 2\\ 1,	\amp 2 \le t \le 3\\ 3,	\amp t \ge 3\\\end{array} \right. </m> 	\showto{student}{\vspace{1cm}}
		</statement>
		<solution>
			
		</solution>
		<answer>
			
		</answer>
	</exercise>

	<exercise> <!--== Problem 2 ==-->
		<statement>
			  \includegraphics[scale = 0.35,trim = 0 3in 0 0]{figs/12_LTs_unit_step/fig1.png}\\\vspace{0.8in}
		</statement>
		<solution>
			
		</solution>
		<answer>
			
		</answer>
	</exercise>

</exercisegroup>

<!--========== Exercise Group 2 ==========--> 
<exercisegroup>
<title>
<p>
 Sketch the graph of the given function and determine its Laplacetransform.
</p>
<p/> <!-- added for vertical space -->
</title>
	<exercise> <!--== Problem 3 ==-->
		<statement>
			<m> \DS w(t) = U(t-1) - U(t-4) </m>
		</statement>
		<solution>
			<m> \DS w(t) = U(t-1) - U(t-4) </m>
		</solution>
		<answer>
			
		</answer>
	</exercise>

	<exercise> <!--== Problem 4 ==-->
		<statement>
			<m> \DS y(t) = (t-1)^2U(t-3) </m>
		</statement>
		<solution>
			<m> \DS y(t) = (t-1)^2U(t-3) </m>
		</solution>
		<answer>
			
		</answer>
	</exercise>

	<exercise> <!--== Problem 5 ==-->
		<statement>
			<m> \DS x(t) = te^{3t}U(t+\pi/4) </m> 
		</statement>
		<solution>
			<m> \DS x(t) = te^{3t}U(t+\pi/4) </m> 
		</solution>
		<answer>
			
		</answer>
	</exercise>

</exercisegroup>

<!--========== Exercise Group 3 ==========--> 
<exercisegroup>
<title>
<p>
Find the inverse Laplace transform of each function.
</p>
<p/> <!-- added for vertical space -->
</title>
	<exercise> <!--== Problem 6 ==-->
		<statement>
			<m> \DS Y(s) = \frac{e^{-2s}}{s-1} </m>
		</statement>
		<solution>
			<m> \DS Y(s) = \frac{e^{-2s}}{s-1} </m>
		</solution>
		<answer>
			
		</answer>
	</exercise>

	<exercise> <!--== Problem 7 ==-->
		<statement>
			<m> \DS H(s) = \frac{e^{-2s} - 3e^{-4s}}{s+2} </m>
		</statement>
		<solution>
			<m> \DS H(s) = \frac{e^{-2s} - 3e^{-4s}}{s+2} </m>
		</solution>
		<answer>
			
		</answer>
	</exercise>

	<exercise> <!--== Problem 8 ==-->
		<statement>
			<m> \DS M(s) = \frac{e^{-3s}}{s^2+9} </m>
		</statement>
		<solution>
			<m> \DS M(s) = \frac{e^{-3s}}{s^2+9} </m>
		</solution>
		<answer>
			
		</answer>
	</exercise>

	<exercise> <!--== Problem 9 ==-->
		<statement>
			<m> \DS X(s) = \frac{e^{-s}(s-5)}{(s+1)(s+2)} </m> vspace{1cm}
		</statement>
		<solution>
			<m> \DS X(s) = \frac{e^{-s}(s-5)}{(s+1)(s+2)} </m> vspace{1cm}
		</solution>
		<answer>
			
		</answer>
	</exercise>

</exercisegroup>

<!--========== Exercise Group 4 ==========--> 
<exercisegroup>
<title>
<p>
Solve each initial value problem.
</p>
<p/> <!-- added for vertical space -->
</title>
	<exercise> <!--== Problem 10 ==-->
		<statement>
			<m> \DS z'' + 3z' + 2z = e^{-3t}U(t-2), \hspace{0.5cm}z(0) = 2,\hspace{0.5cm}z'(0) = -3 </m>
		</statement>
		<solution>
			
		</solution>
		<answer>
			
		</answer>
	</exercise>

	<exercise> <!--== Problem 11 ==-->
		<statement>
			<m> \DS w'' + w = U(t-2) - U(t-4), \hspace{0.5cm}w(0) = 1,\hspace{0.5cm}w'(0) = 0 </m>
		</statement>
		<solution>
			
		</solution>
		<answer>
			
		</answer>
	</exercise>

</exercisegroup>

</exercises>
