<exercises><title>Exercises</title>

<exercisegroup>
<title></title>
	<exercise>
		<statement>
			<alert>Use the definition of Laplace Transform</alert> (above) to find the Laplace Transform of <m> \ds h(t) = 7t. </m>
		</statement>
		<solution>
			 \\ In order to evaluate this integral, we will need to compute an integration by parts. When that time comes, we will choose <m> \ds u = t </m> an <m> \ds dv = e^{-st}. </m>  Then we take the derivative o <m> \ds u </m> to fin <m> \ds du </m> and the antiderivative o <m> \ds dv </m> to fin <m> \ds v </m> , as follows.
			<md>
				<mrow>  u	 \amp =  t 						\amp dv	\amp= e^{-st}dt </mrow>
				<mrow>  \Rightarrow du	 \amp =  dt\hspace{1cm}\mbox{}	\amp \Rightarrow v	\amp= -\frac{1}{s}e^{-st}  </mrow>
			</md>
			 Note also that we will use L'Hospital's Rule when we have a limit of for <m> \ds \frac{\infty}{\infty}. </m>
			<md>
				<mrow>  H(s)	 \amp =  \lap\{ h(t) \} </mrow>
				<mrow>   \amp =  \int_0^{\infty}e^{-st}h(t) dt </mrow>
				<mrow>   \amp =  \int_0^{\infty}e^{-st}\cdot 7t dt </mrow>
				<mrow>   \amp =  \lim_{b \to \infty} \int_0^b e^{-st}\cdot 7t dt </mrow>
				<mrow>   \amp =   7\cdot \lim_{b \to \infty} \int_0^b te^{-st} dt </mrow>
				<mrow>   \amp =   7\cdot \lim_{b \to \infty} \left[t\cdot\left(-\frac{1}{s}e^{-st}\right)\Bigg|_0^b - \int_0^b -\frac{1}{s}e^{-st} dt\right] </mrow>
				<mrow>   \amp =   7\cdot \lim_{b \to \infty} \left[-\frac{t}{se^{st}}\Bigg|_0^b + \frac{1}{s}\int_0^b e^{-st} dt\right] </mrow>
				<mrow>   \amp =   7\cdot \lim_{b \to \infty} \left[-\frac{t}{se^{st}} + \frac{1}{s} \cdot -\frac{1}{s}e^{-st} \right]_0^b </mrow>
				<mrow>   \amp =   7\cdot \lim_{b \to \infty} \left[-\frac{t}{se^{st}} - \frac{1}{s^2 e^{st}} \right]_0^b </mrow>
			</md>

			<md>
				<mrow>   \amp =   7\cdot \lim_{b \to \infty} \left[\left( -\frac{b}{se^{sb}} - \frac{1}{s^2 e^{sb}} \right) - \left( -\frac{0}{se^{s\cdot 0}} - \frac{1}{s^2 e^{s\cdot 0}} \right) \right] </mrow>
				<mrow>   \amp =   7\cdot \lim_{b \to \infty} \left[\left( -\frac{b}{se^{sb}} - \frac{1}{s^2 e^{sb}} \right) - \left( 0 - \frac{1}{s^2} \right) \right] </mrow>
				<mrow>   \amp =   7\cdot \lim_{b \to \infty} \left[-\frac{b}{se^{sb}} - \frac{1}{s^2 e^{sb}}+ \frac{1}{s^2} \right] </mrow>
				<mrow>   \amp =   7\cdot \lim_{b \to \infty} \left[-\frac{b}{se^{sb}} \right] - 7\cdot \lim_{b \to \infty} \left[\frac{1}{s^2 e^{sb}} \right] + 7\cdot \lim_{b \to \infty} \left[\frac{1}{s^2} \right] </mrow>
				<mrow>   \amp =   -7\cdot \frac{1}{s} \cdot \lim_{b \to \infty} \left[\frac{b}{e^{sb}} \right] - 7\cdot \frac{1}{s^2}\cdot \lim_{b \to \infty} \left[\frac{1}{e^{sb}} \right] + 7\cdot \frac{1}{s^2} </mrow>
				<mrow>   \amp =   -\frac{7}{s} \cdot  \lim_{b \to \infty} \left[\frac{1}{se^{sb}} \right] - \frac{7}{s^2}\cdot \lim_{b \to \infty} \left[\frac{1}{e^{sb}} \right] + \frac{7}{s^2} \mbox{ (using L'H Rule)} </mrow>
				<mrow>   \amp =   -\frac{7}{s^2} \cdot  \lim_{b \to \infty} \left[\frac{1}{e^{sb}} \right] - \frac{7}{s^2}\cdot \lim_{b \to \infty} \left[\frac{1}{e^{sb}} \right] + \frac{7}{s^2} </mrow>
				<mrow>   \amp =   -\frac{7}{s^2} \cdot  0 - \frac{7}{s^2}\cdot 0 + \frac{7}{s^2} </mrow>
				<mrow>   \amp =   \frac{7}{s^2} </mrow>
			</md>

		</solution>
		<answer>
			<m> \ds H(s) = \frac{7}{s^2} </m>
		</answer>
	</exercise>

</exercisegroup>

<!--	-->

<exercisegroup>
<title></title>
	<exercise>

		<statement>
			<alert>Use the definition of Laplace Transform</alert> (above) to find the Laplace Transform of <m>\ds h(t) = e^{at}</m> where <m>a</m> is some constant.
		</statement>

		<solution>
			 \\
			<md>
				<mrow>  W(s)	 \amp =  \lap\{ w(t) \} </mrow>
				<mrow>   \amp =  \int_0^{\infty}e^{-st}w(t) dt </mrow>
				<mrow>   \amp =  \int_0^{\infty}e^{-st}\cdot e^{at} dt </mrow>
				<mrow>   \amp =  \lim_{b \to \infty} \int_0^b e^{-st}\cdot e^{at} dt </mrow>
				<mrow>   \amp =  \lim_{b \to \infty} \int_0^b e^{-st + at}dt </mrow>
				<mrow>   \amp =  \lim_{b \to \infty} \int_0^b e^{(-s + a)t}dt </mrow>
				<mrow>   \amp =  \lim_{b \to \infty} \left[ \frac{1}{-s+a} \cdot e^{(-s + a)t} \right]_0^b </mrow>
				<mrow>   \amp =  \lim_{b \to \infty} \left[ \left(\frac{1}{-s+a} \cdot e^{(-s + a)\cdot b}\right) - \left(\frac{1}{-s+a} \cdot e^{(-s + a)\cdot 0}\right) \right] </mrow>
				<mrow>   \amp =  \lim_{b \to \infty} \left[ \left(\frac{1}{-s+a} \cdot e^{(-s + a)\cdot b}\right) - \left(\frac{1}{-s+a} \cdot 1\right) \right] </mrow>
				<mrow>   \amp =  \lim_{b \to \infty} \left[ \frac{1}{-s+a} \cdot e^{(-s + a)\cdot b} - \frac{1}{-s+a} \right] </mrow>
				<mrow>   \amp =  \lim_{b \to \infty} \left[ \frac{1}{-s+a} \cdot e^{(-s + a)\cdot b} \right] - \lim_{b \to \infty} \left[ \frac{1}{-s+a} \right] </mrow>
				<mrow>   \amp =  \frac{1}{-s+a} \cdot \lim_{b \to \infty} \left[ e^{(-s + a)\cdot b} \right] - \frac{1}{-s+a} </mrow>
				<mrow>   \amp =  \frac{1}{-s+a} \cdot 0 - \frac{1}{-s+a} \mbox{ (assumin <m> \ds -s+a </m> is negative)} </mrow>
				<mrow>   \amp =  - \frac{1}{-s+a} </mrow>
				<mrow>   \amp =  \frac{1}{s-a}  </mrow>
			</md>

		</solution>

		<answer>
			<m> \ds W(s) = \frac{1}{s-a} </m>
		</answer>

	</exercise>

</exercisegroup>

<exercisegroup>
<title></title>
	<exercise>
		<statement>
			<alert>Use the definition of Laplace Transform</alert> (above) to find the Laplace Transform of <m>\ds y(t) = 7t + e^{5t}</m>.
		</statement>
		<solution>
			 \\ We will use the results from the previous two questions.
			<md>
				<mrow>  Y(s)	 \amp =  \lap\{ y(t) \} </mrow>
				<mrow>   \amp =  \int_0^{\infty}e^{-st}y(t) dt </mrow>
				<mrow>   \amp =  \int_0^{\infty}e^{-st}\cdot (7t + e^{5t}) dt </mrow>
				<mrow>   \amp =  \int_0^{\infty}(e^{-st}\cdot 7t + e^{-st}\cdot e^{5t}) dt </mrow>
				<mrow>   \amp =  \int_0^{\infty}e^{-st}\cdot 7t dt + \int_0^{\infty}(e^{-st}\cdot e^{5t} dt </mrow>
				<mrow>   \amp =  \lap\{ 7t \} + \lap\{ e^{5t} \} </mrow>
				<mrow>   \amp= \frac{7}{s^2} + \frac{1}{s-5} </mrow>
			</md>
			 Notice that what we showed in the middle of all this is that <m> \ds \lap\{ 7t + e^{5t} \} = \lap\{ 7t \} + \lap\{ e^{5t} \}. </m> This is an example of the linearity property of Laplace Transforms.
		</solution>
		<answer>
			<m> \ds Y(s) = \frac{7}{s^2} + \frac{1}{s-5} </m>
		</answer>
	</exercise>

</exercisegroup>

<exercisegroup>
<title></title>
	<exercise>
		<statement>
			<alert>Use the definition of Laplace Transform</alert> (above) to find the Laplace Transform of the function
				<m>\ds
					d(t) = \left\{
					\begin{array}{ll}
					0,	\amp t \lt 0\\
					7,	\amp 0 \le t \lt 3\\
					0,	\amp t \ge 3\\
					\end{array} \right.
				</m>
		</statement>
		<solution>

			<md>
				<mrow>  D(s)	 \amp =  \lap\{ d(t) \} </mrow>
				<mrow>   \amp =  \int_0^{\infty}e^{-st}d(t) dt </mrow>
				<mrow>   \amp =  \int_0^3 e^{-st}\cdot 7 dt + \int_3^{\infty} e^{-st}\cdot 0 dt </mrow>
				<mrow>   \amp =  7\int_0^3 e^{-st}dt + 0 </mrow>
				<mrow>   \amp =  7 \cdot \left[\frac{1}{-s}e^{-st}\right]_0^3 </mrow>
				<mrow>   \amp =  7 \cdot \left[\left(\frac{1}{-s}e^{-s\cdot 3}\right) - \left(\frac{1}{-s}e^{-s\cdot 0}\right)\right] </mrow>
				<mrow>   \amp =  7 \cdot \left[\left(\frac{1}{-s}e^{-s\cdot 3}\right) - \left(\frac{1}{-s}\cdot 1\right)\right] </mrow>
				<mrow>   \amp =  7 \cdot \left[-\frac{1}{s}e^{-3s} +\frac{1}{s}\cdot 1\right] </mrow>
				<mrow>   \amp =  7 \cdot \left[-\frac{1}{s}e^{-3s} +\frac{1}{s}\right] </mrow>
				<mrow>   \amp =  \frac{7}{s} - \frac{7}{s}e^{-3s} </mrow>

			</md>

		</solution>
		<answer>
			<m> \ds D(s) = \frac{7}{s} - \frac{7}{s}e^{-3s} </m>
		</answer>
	</exercise>

</exercisegroup>

</exercises>
