<subsection xmlns:xi="http://www.w3.org/2001/XInclude"><title> Direct Integration Method </title>

	<p>
		The previous section showed us that if we can isolate the derivative of the dependent variable, <m>y</m>, in the form
		<me>
			\frac{d}{dx}[y] = f(x)
		</me>, 
		then the solution can be found by integrating both sides. This principle extends to more complex equations of the form:
		<me>
			\frac{d}{dx}\left[g(x,y)\right] = f(x)
		</me>.
	</p>

	<p>
		Here, <m>f(x)</m> is a placeholder that indicates that <em>only</em> <m>x</m> variables can appear on the right-hand side of this equation. Similarly, <m>g(x,y)</m> indicates that <em>only</em> <m>x</m> or <m>y</m> variables can appear inside the derivative. This leads us to our first method for solving first-order differential equations—<em>direct integration</em>.
	</p>

	<exploration xml:id="direct-integration"><title> Direct Integration </title>
		<p>
			The general solution of a differential equation in the form
			<men xml:id="direct-integration-equation">
				\frac{d}{dx}\left[g(x,y)\right] = f(x)
			</men>,
			can be determined by through the following steps:
			<dl>
				<li xml:id="di-step-1"><title> Integrate both Sides </title>
					<p>
						Integrate both sides with respect to the independent variable, <m>x</m>, to eliminate the derivative containing <m>y</m>.
					</p>
				</li>
				<li xml:id="di-step-2"><title> Isolate the Solution </title>
					<p>
						Now, isolate the dependent variable, <m>y</m>, to find the general solution.
					</p>
				</li>
			</dl>
		</p>
	</exploration> 

	<p>
		Consider the following examples to see how this approach applies to some more interesting problems.
	</p>

	<example xml:id="direct-integration-example-1"><title> Integrate both sides to Recover <m>y</m> </title>
	
		<p>
			<statement>
				<p>
					Find the particular solution to the differential equation
					<me>
						\frac{d}{dx}\left[5x \cdot y\right] = \frac{1}{x^2} , \quad y\left(1\right) = -4
					</me>.
				</p>
			</statement>
		</p>
		<solution>

			<p>
				First, observe that this problem is in the form
				<me>
					\frac{d}{dx}\left[g(x,y)\right] = f(x)
				</me>
				where
				<me>
					g(x,y) = 5x \cdot y \quad \text{ and } \quad f(x) = \frac{1}{x^2}
				</me>.
			</p>
			<p>
				So, we can solve for <m>y</m> using direct integration:
			</p>

			<p>
				<term> <xref ref="di-step-1" text="custom">Step 1: Integrate both Sides</xref> </term>
			</p>

			<p>
				Integrating both sides with respect to <m>x</m>, we get
				<md>
					<mrow> \int \frac{d}{dx}\left[5x \cdot y\right]\ dx \amp = \int x^{-2}\ dx </mrow>
					<mrow> 5x \cdot y + c_1 \amp = -x^{-1} + c_2 </mrow>
				</md>
			</p>

			<p>
				<term> <xref ref="di-step-2" text="custom">Step 2: Isolate the Solution</xref> </term>
			</p>

			<p>
				Now that the dependent variable <m>y</m> is free from the derivative, we can isolate it to find the general solution, as follows
				<md>
					<mrow>  y \amp = \frac{1}{5x}\Big(-\frac{1}{x} + \overset{=\ c}{\overbrace{c_2 - c_1}}\Big) </mrow>
					<mrow>  y \amp = \frac{1}{5x}\left(-\frac{1}{x} + c\right) \quad \leftarrow \ \text{general solution}</mrow>
				</md>
			</p>

			<p>
				Since we are given the condition <m>y\left(1\right) = -4</m>, we need to find <m>c</m>.
				<md>
					<mrow>  -4	\amp = \frac{1}{5}\left(-1 + c\right)\qquad \leftarrow \small\text{ multiply both sides by } 5	</mrow>
					<mrow>  -20	\amp = -1 + c \quad \implies \quad c = -19	</mrow>
				</md>
				Therefore, the particular solution (for <m>c=-19</m>) is
				<me>
					y = \frac{1}{5x}\left(-\frac{1}{x} - 19\right)
				</me>.
			</p>

		</solution>

	</example>

	<example xml:id="direct-integration-example-2"><title> Isolate the Derivative before Integrating </title>
		<p>
			<statement>
				<p>
					Compute the general solution of the differential equation
					<me>
						\frac{1}{\cos x}\frac{d}{dx}\Big[y\sin(2x)\Big] - 1 = \sec x
					</me>
				</p>
			</statement>
		</p>
		<solution>
			<p>
				First, we get the derivative by itself on the left-hand side
				<aside><title>☝️ Recall the Identity </title>
					<p>
						<me>
							\sec x = \frac{1}{\cos x}
						</me>
					</p>
				</aside>
				<md>
					<mrow> 
						\frac{d}{dx}\Big[ y \sin(2x) \Big] =\amp\ \cos x\left( 1 + \frac{1}{\cos x} \right)
					 </mrow>
					 <mrow> 
						\frac{d}{dx}\Big[
							\us{\textcolor{BurntOrange}{g(x,y)}}{\us{\textcolor{BurntOrange}{\uparrow}}{\ul{y\sin(2x)}}}
						\Big] =\amp\ \us{\textcolor{BurntOrange}{f(x)}}{\us{\textcolor{BurntOrange}{\uparrow}}{\ul{\cos x + 1}}}
					 </mrow>
				</md>
				Now, we integrate by sides with respect to <m>x</m>, releasing <m>y</m> from the derivative and allowing us to isolate the general solution.
				<md>
					<mrow>	\int \frac{d}{dx}\Big[y\sin(2x)\Big]dx	\amp = \int \left(\cos x + 1\right) \ dx	</mrow>
					<mrow>							y\sin(2x) + c_1	\amp = \sin x + x + c_2						</mrow>
					<mrow>										y	\amp = \frac{\sin x + x + c}{\sin(2x)} 
																				\qquad (c = c_2 - c_1)
					</mrow>
				</md>.
			</p>
		</solution>

	</example>

	<xi:include href="./chkpts-1-6-2-direct-integration.ptx" />

	<p>
		The direct integration method is one of the simplest ways to solve a differential equation when the derivative of the dependent variable or an expression involving it is isolated. By integrating both sides and solving for <m>y</m>, you can find either the general solution or a particular solution if initial conditions are provided. This method highlights the close relationship between differentiation and integration, making it a natural starting point for understanding how to solve differential equations.
	</p>

</subsection>