
<subsection><title> Summary &amp; Exercises </title>

	<introduction>
		<p>
			<assemblage color="green"><title>Summary of the Key Ideas</title>
				<p>
					<ul marker="">
						<li xml:id="summary-antiderivatives">
							<term> <em>Antiderivatives as Solutions to Differential Equations</em> </term>
							<ul marker="square">
								<li>
									Finding the general antiderivative of a function, <m>f(x)</m>, is equivalent to finding the general solution to the differential equation
									<me> \frac{dy}{dx} = f(x) </me>.
								</li>
							</ul>
						</li>
						<li xml:id="summary-direct-integration"> 
							<term> <em>Direct Integration</em> </term>
							<ul marker="square">
								<li>
									Process of integrating both sides of a differential equation to directly solve for the dependent variable, <m>y</m>.
								</li>
							</ul>
						</li>
					</ul>
				</p>
			</assemblage>
		</p>
		
	</introduction>

	<exercises>

		<exercisegroup cols="2"><title> General Solution </title>
	
			<introduction>
				<p>
					Find the general solution for each of the following differential equations. Combine constants where appropriate.
				</p>
			</introduction>
	
			<exercise>
				<statement>
					<m> \displaystyle \frac{dy}{dx} = 2x - 5 </m>
				</statement>
				<answer><title>Answer</title>
					<p>
						<m> \displaystyle y = x^2 - 5x + C </m>
					</p>
				</answer>
			</exercise>
	
			<exercise>
				<statement>
					<m> \displaystyle \frac{d}{dx}[y] = e^{2x} </m>
				</statement>
				<answer><title>Answer</title>
					<p>
						<m> \displaystyle y = \frac{1}{2}e^{2x} + C </m>
					</p>
				</answer>
			</exercise>
	
			<exercise>
				<statement>
					<m> \displaystyle \frac{d}{dx}[x \cdot y] = \cos(x) </m>
				</statement>
				<answer><title>Answer</title>
					<p>
						<m> \displaystyle y = \frac{\sin(x)}{x} + \frac{C}{x} </m>
					</p>
				</answer>
			</exercise>
	
			<exercise>
				<statement>
					<m> \displaystyle \frac{dy}{dt} = \frac{1}{t^2} + t </m>
				</statement>
				<answer><title>Answer</title>
					<p>
						<m> \displaystyle y = -\frac{1}{t} + \frac{1}{2}t^2 + C </m>
					</p>
				</answer>
			</exercise>
	
			<exercise>
				<statement>
					<m> \displaystyle \frac{dy}{dx} = x e^x </m>
				</statement>
				<answer><title>Answer</title>
					<p>
						<m> \displaystyle y = (x - 1)e^x + C </m>
					</p>
				</answer>
			</exercise>
	
			<exercise>
				<statement>
					<m> \displaystyle \left[\sin(x) \cdot y\right]^\prime = \cos^2(x) </m>
				</statement>
				<answer><title>Answer</title>
					<p>
						<m> \displaystyle y = \frac{\sin(x)}{2} + \frac{C}{\sin(x)} </m>
					</p>
				</answer>
			</exercise>
	
			<exercise>
				<statement>
					<m> \displaystyle y' = \ln(x) + x^2 </m>
				</statement>
				<answer><title>Answer</title>
					<p>
						<m> \displaystyle y = x \ln(x) - x + \frac{1}{3}x^3 + C </m>
					</p>
				</answer>
			</exercise>
	
			<exercise>
				<statement>
					<m> \displaystyle \frac{d}{dP}\left[e^P \cdot Q\right] = P </m>
				</statement>
				<answer><title>Answer</title>
					<p>
						<m> \displaystyle Q = e^{-P} \left(\frac{P}{e^P} + C \right) </m>
					</p>
				</answer>
			</exercise>
	
		</exercisegroup>

		<exercisegroup cols="2"><title> Particular Solution </title>
	
			<introduction>
				<p>
					Find the particular solution for each of the following differential equations with the given initial condition.
				</p>
			</introduction>
	
			<exercise>
				<statement>
					<m> \displaystyle \frac{dy}{dx} = 3x^2 + 2, \ \ y(1) = 4 </m>
				</statement>
				<answer><title>Answer</title>
					<p>
						<m> \displaystyle y = x^3 + 2x + 1 </m>
					</p>
				</answer>
			</exercise>
	
			<exercise>
				<statement>
					<m> \displaystyle \frac{d}{dt}[y] = \sin(t), \ \ y(0) = 2 </m>
				</statement>
				<answer><title>Answer</title>
					<p>
						<m> \displaystyle y = -\cos(t) + 3 </m>
					</p>
				</answer>
			</exercise>
	
			<exercise>
				<statement>
					<m> \displaystyle \frac{d}{dx}[x \cdot y] = e^x, \ \ y(1) = 0 </m>
				</statement>
				<answer><title>Answer</title>
					<p>
						<m> \displaystyle y = \frac{e^x}{x} - \frac{e}{x} </m>
					</p>
				</answer>
			</exercise>
	
			<exercise>
				<statement>
					<m> \displaystyle \frac{dy}{dx} = x^3 - 4, \ \ y(2) = 1 </m>
				</statement>
				<answer><title>Answer</title>
					<p>
						<m> \displaystyle y = \frac{x^4}{4} - 4x + 5 </m>
					</p>
				</answer>
			</exercise>
	
			<exercise>
				<statement>
					<m> \displaystyle \frac{dR}{dh} = \frac{1}{h} + h, \ \ R(1) = 3 </m>
				</statement>
				<answer><title>Answer</title>
					<p>
						<m> \displaystyle R = \ln|h| + \frac{h^2}{2} + \frac{5}{2} </m>
					</p>
				</answer>
			</exercise>
	
			<exercise>
				<statement>
					<m> \displaystyle \frac{d}{dx}\left[e^x \cdot y\right] = \sin(x), \ \ y(0) = 2 </m>
				</statement>
				<answer><title>Answer</title>
					<p>
						<m> \displaystyle y = e^{-x} \left(-\cos(x) + 3 \right) </m>
					</p>
				</answer>
			</exercise>

			<exercise>
				<statement>
					<m> \displaystyle y' = \cos(x) + x^2, \ \ y(0) = -2 </m>
				</statement>
				<answer><title>Answer</title>
					<p>
						<m> \displaystyle y = \sin(x) + \frac{x^3}{3} - 2 </m>
					</p>
				</answer>
			</exercise>
	
			<exercise>
				<statement>
					<m> \displaystyle \frac{d}{dx}\left[\tan(x) \cdot y\right] = \sec^2(x), \quad y\left(\frac{\pi}{4}\right) = 1 </m>
				</statement>
				<answer><title>Answer</title>
					<p>
						<m> \displaystyle y = \frac{x \sec^2(x)}{\tan(x)} + \frac{\pi/4 - 1}{\tan(x)} </m>
					</p>
				</answer>
			</exercise>
	
		</exercisegroup>

		<exercise>
			<statement>
				<p>
					Attempt to apply direct integration to the differential equation
					<me> \frac{dy}{dx} = x + y</me>.
					Get to the point where it becomes clear that you cannot solve for <m>y</m> directly. What is the obstacle?
				</p>
			</statement>
			<answer><title>Answer</title>
				<p>
					<p>
					Integrating both sides gives
					<md>
						<mrow> \int \frac{dy}{dx}\ dx	\amp = \int\left(x + y\right)\ dx 		</mrow>
						<mrow> 					y + C_1	\amp = \int x\ dx + \int y\ dx 			</mrow>
						<mrow> 					y + C_1	\amp = \frac12 x^2 + C_2 + \int y\ dx	</mrow>
						<mrow> 			y - \int y\ dx	\amp = \frac12 x^2 + C_2 - C_1  		</mrow>
					</md>
					Without knowing <m>y</m>, we cannot simplify <m>\int y\ dx</m>. So the obstacle is that we are unable to combine the these <m>y</m> variables into a single <m>y</m> on the left side. 
				</p>
				</p>
			</answer>
		</exercise>

		<exercisegroup>
		
			<introduction>
				<p>
					Convert this idea from the integrating factor into some exercises for the direct integration method.
				</p>
			</introduction>
		
			<exercise>
				<statement>
					<note>
						To Readers: This is not an exercise (yet).  Ignore it.
					</note>
					<p>
						In this chapter, we will study a solution technique that will help us solve differential equations that are first order and linear. Consider this (carefully selected) example.
						<men xml:id="original_de">
							x^7 \cdot \frac{dy}{dx} + 7x^{6}\cdot y = e^x
						</men>
						Notice that the dependent variable is <m>y</m> and the independent variable is <m>x</m>, so we seek to find a formula for <m>y</m> in terms of <m>x</m>. The DE is also first order and linear.
					</p>
				</statement>
				<solution><title> Solution </title>
					<p>
						What makes this DE special is that the left hand side can be rewritten as follows.
						<men xml:id="rewritten_de">
							\frac{d}{dx}\Big(x^7 \cdot y \Big) = e^x
						</men>
						We can verify this by actually using the product rule to take the derivative on the left hand side:
						<md>
							<mrow>\frac{d}{dx}\Big(x^7 \cdot y \Big)</mrow>
							<mrow>   =\amp\  \frac{d}{dx}\Big(\underbrace{x^7}_{f(x)} \cdot \underbrace{y}_{g(x)} \Big)</mrow>
							<mrow>   =\amp\ f(x) \cdot g'(x) + f'(x) \cdot g(x)</mrow>
							<mrow>   =\amp\ x^7 \cdot \frac{dy}{dx} + 7x^{6}\cdot y</mrow>
						</md>
					</p>
							
					<p>
						Now that we have confirmed that Equation <xref ref="rewritten_de"/> is equivalent to Equation <xref ref="original_de"/>, we can proceed in solving the DE. 
					</p>
							
					<p>
						The unknown function we want to solve for is <m>y</m>, and it is part of the product we are taking the derivative of in Equation <xref ref="rewritten_de"/>. So we begin by undoing that differentiation by integrating both sides of Equation <xref ref="rewritten_de"/> with respect to <m>x</m>:
						
						<md>
							<mrow>
								\int \frac{d}{dx}\Big(x^7 \cdot y \Big) dx =\amp\ \int e^x dx
							</mrow>
							<mrow>
								x^7 \cdot y	  =\amp\ e^x + C
							</mrow>
						</md>
					</p>
							
					<p>
						We can now just divide both sides of Equation by the coefficient on <m>y</m> to obtain the general solution.
						<me>y = \frac{e^x}{x^7} + \frac{C}{x^7}</me>
					</p>
							
					<p>
						Recall that we said this was a carefully selected DE. This very special DE had the property that we could undo the product rule on its left hand side. This is not, in general, the case when we encounter a first order linear DE. For example, consider this DE.
					</p>
				</solution>
			</exercise>
		
		</exercisegroup>
	
	</exercises>

</subsection>