<subsection xmlns:xi="http://www.w3.org/2001/XInclude"><title> General Solutions </title>
	
    <p>
		The general solution to any <xref ref="def-nhcc" text="title"/> can be expressed as the sum of a homogeneous part, <m>y_h</m>, and a particular part, <m>y_p</m>,
		<me>
			y = y_h + y_p
		</me>.
		To better understand each part, lets start with a concrete example and then generalize the concept. 
	</p>

	<p>
		To see that the solution is the sum of two parts, lets plug <m>y = y_h + y_p</m> into the equation to see where these parts come from.
		<md>
			<mrow> (y_h + y_p)'' + 2(y_h + y_p)' + 3(y_h + y_p) =\ &amp; 9x </mrow>
			<mrow> y_h'' + y_p'' + 2y_h' + 2y_p' + 3y_h + 3y_p =\ &amp; 9x \qquad {\it \text{apply derivatives}}</mrow>
			<mrow> y_h'' + 2y_h' + 3y_h + y_p'' + 2y_p' + 3y_p =\ &amp; 9x \qquad {\it \text{group}\ y_h\ \text{and}\ y_p}</mrow>
			<mrow> 
				\us{\Large 0}{\us{\downarrow}{\ub{(y_h'' + 2y_h' + 3y_h)}}} 
				+ 
				\us{\Large 9x}{\us{\downarrow}{\ub{(y_p'' + 2y_p' + 3y_p)}}} 
				=\ &amp; 9x 
			</mrow>
		</md> 

	</p>

	<p>
		To solve this equation, we first find the complementary solution, <m>y_h</m>, by solving the homogeneous equation:
		<me>
			\frac{d^2y_h}{dt^2} + 4\frac{dy_h}{dt} + 4y_h = 0
		</me>
	</p>

	<p>
		We can solve this equation by assuming a solution of the form <m>y_h = e^{rt}</m> and substituting it into the equation. This gives us the characteristic equation:
		<me>
			r^2 + 4r + 4 = 0
		</me>
	</p>

	<p>
		Solving this equation gives us the characteristic roots <m>r_1 = -2</m> and <m>r_2 = -2</m>. Therefore, the complementary solution is:
		<me>
			y_h = c_1e^{-2t} + c_2te^{-2t}
		</me>
	</p>

	<p>
		Next, we find the particular solution, <m>y_p</m>, by guessing a solution of the form <m>y_p = Ae^{-2t}</m> and substituting it into the original equation. This gives us the particular solution:
		<me>
			y_p = -\frac{1}{2}e^{-2t}
		</me>
	</p>

	<p>
		Therefore, the general solution to the original differential equation is:
		<me>
			y = c_1e^{-2t} + c_2te^{-2t} - \frac{1}{2}e^{-2t}
		</me>
	</p>

	<p>
		This general solution can be expressed as the sum of the complementary and particular solutions:
		<me>
			y = y_h + y_p
		</me>
	</p>

	<p>
		By understanding the general solution as the sum of these two parts, we can solve a wide range of nonhomogeneous differential equations.
	</p>

	<p>
		To further explore the concept of general solutions, let's consider a few more examples.
	</p>

	<xi:include href="./c3-s3-ss2-interactives.ptx" />

</subsection>