<section xmlns:xi="http://www.w3.org/2001/XInclude"><title> IF: Step-By-Step </title>

	<p>
		Now that we are familiar with the strategy behind the integrating factor method, let's streamline the process into a sequence of steps, summarized below.
	</p>

	<exploration xml:id="if-method"><title> Integrating Factor </title>
		<p>
			The general solution to the first-order linear DE in the standard form
			<men xml:id="if-method-de">
				\frac{dy}{dx} + P(x)\ y = Q(x),
			</men>
			can be determined through the following steps:
		
			<dl width="narrow">
				<li xml:id="if-step-1"><title> Step 1: Find the Integrating Factor </title>
					<me>\mu = e^{\int P(x) dx}</me>.
				</li>
				<li xml:id="if-step-2"><title> Step 2: Rewrite the DE </title>
					<p>
						Multiply the equation by <m>\mu</m>, and rewrite it in the form
						<men xml:id="if-method-de-rewrite"> 
							\frac{d}{dx}\left[\mu\ y\right] = \mu\ Q(x). 
						</men>
					</p>
				</li>
				<li xml:id="if-step-3"><title> Step 3: Apply Direct Integration </title>
					Integrate both sides of <xref ref="if-method-de-rewrite" /> and solve for <m>y</m>.
				</li>
			</dl>
		</p>
	</exploration> 

	<p>
		Now let's apply this to some examples.
	</p>

	<example xml:id="if-intro-exercise">

        <statement>
            <p> 
				Find the general solution to the differential equation 
			</p>
			<me>y' + 6y = 1</me>.
        </statement>

		<solution>

			<p>
				<xref ref="if-step-1" text="title" />.
				<m>\ds \quad \mu = e^{\int 6\ dx} = e^{6x}</m>
			</p>

			<p>
				<xref ref="if-step-2" text="title" />.
				<p>
					<sidebyside widths="20% 60%">
						<p>
							Multiply by <m>\mu</m>:
						</p>
						<p>
							<m>\ds e^{6x}y' + 6e^{6x}y = e^{6x} </m>
						</p>
					</sidebyside>
					<sidebyside widths="20% 60%">
						<p>
							Rewrite:
						</p>
						<p>
							<m>\ds \frac{d}{dx}\left[e^{6x}y\right] = e^{6x} </m>
						</p>
					</sidebyside>
				</p>
			</p>

			<p>
				<xref ref="if-step-3" text="title" />
				<md>
					<mrow> e^{6x}y \amp = \int e^{6x}\ dx </mrow>
					<mrow> y \amp = \frac{1}{6}e^{-6x} + C. </mrow>
				</md>
				
			</p>

		</solution>

    </example>

	<example xml:id="example-if-examples-01">
		<p>
			Solve
			<me>-\frac{4}{t^2} \cdot M =  t^5 - \frac{1}{t} \cdot\frac{dM}{dt} + 1.</me>
		</p>

		<solution>
			<p>
				We always begin by classifying the DE.  You should confirm that this DE is
				first order and linear, and therefore it is appropriate to use our integrating factor technique.
				Keep in mind that our goal is to find an unknown function <m>M(t)</m> that satisfies this
				equation.
			</p>

			<p>
				We work first to get the DE in an appropriate form so that we can un-do the product rule.
				We begin by getting the dependent variable, <m>M</m> and its derivative on the same side of
				the equation, and then we multiply both sides of the equation by <m>t</m> so that the coefficient
				on the derivative is 1.
				<mdn>
					<mrow xml:id="this_equn1">	\frac{1}{t}\cdot \frac{dM}{dt} - \frac{4}{t^2} \cdot M	\amp =  t^5 + 1	</mrow>
					<mrow>					\frac{dM}{dt} - \frac{4}{t} \cdot M	\amp = t^6 + t </mrow>
				</mdn>
			</p>

			<p>
				If follow the process we took in the previous example, we would first multiply by
				the unknown function <m>z</m> that will help us un-do the product rule, then we would determine
				<m>z</m>.  Instead, let's first determine <m>z</m>, and then we'll multiply by it.  As in (<xref ref="undo_prod3" />),
				we need to identify the function <m>P</m> that is attached to the independent variable by
				multiplication.  In equation (<xref ref="this_equn1" />), we have <m>P(t) = -\frac{4}{t}</m>, (note the inclusion
				of the negative sign) so we know that
				the function <m>z</m> that will help us un-do the product rule is given by
				<me>z = e^{\int P(t) dt} = e^{\int -\frac{4}{t} dt} = e^{-4\ln t}.</me>
				(Note, again, that we seek only one function <m>z</m>, so we omit the absolute value and the <m>+C</m>
				that we normally see when we integrate the function  <m>P(t) = -\frac{4}{t}.</m>)
			</p>

			<p>
				While our integrating factor <m>z</m> is technically correct, it can (and should) be simplified
				using rules of logarithms as follows.
				<me>z = e^{-4\ln t} = e^{\ln (t^{-4})} = t^{-4}.</me>
			</p>

			<p>
				We'll end up using lots of rules of logarithms throughout this chapter; review those
				rules (HERE) if you need a refresher.
			</p>

			<p>
				Now that we have identified the integrating factor <m>z</m>, we can multiply both
				sides of the DE (which we put in standard form in (<xref ref="this_equn1" />)) by it.
				<md>
					<mrow>	t^{-4} \cdot \frac{dM}{dt} - t^{-4}\cdot \frac{4}{t} \cdot M	\amp = t^{-4}(t^6 + t)	</mrow>
					<mrow>	t^{-4} \cdot \frac{dM}{dt} - \cdot \frac{4}{t^5} \cdot M	\amp = t^2 + t^{-3}	</mrow>
				</md>
			</p>

			<p>
				If we have correctly determined the integrating factor, then we should be able to
				un-do the product rule on the left hand side.  Notice that we can identify the functions
				<m>f</m> and <m>g</m> as follows.
				<me>\underbrace{t^{-4}}_{\scriptsize f}\cdot \underbrace{\frac{dM}{dt}}_{\scriptsize g'}
					+ \underbrace{- \frac{4}{t^5}}_{\scriptsize f'}\cdot \underbrace{M}_{\scriptsize g}
						= t^2 + t^{-3}.</me>
			</p>

			<p>
				It is critical that you verify that the function <m>z</m> does, in fact, create a situation
				where we see a function <m>f</m> and its derivative <m>f'</m> as shown above.  In this case,
				<md>
					<mrow>	f'(t)	\amp = \frac{d}{dt} \Big(f(t)\Big)	</mrow>
					<mrow>				\amp = \frac{d}{dt}\Big( t^{-4} \Big)	</mrow>
					<mrow>				\amp = -4t^{-5}	</mrow>
					<mrow>				\amp = -\frac{4}{t^5},	</mrow>
				</md>
				so we can confirm that we have correctly identified the functions <m>f</m> and <m>g</m> to un-do
				the product rule.  This, we can re-write the left hand side of the equation as follows.
				<me>\frac{d}{dt}\Big( t^{-4}\cdot M \Big) = t^2 + t^{-3}.</me>
			</p>

			<p>
				We've made a big step forward, here!  Remember that our goal is to find the
				unknown function <m>M</m>, so we are much closer since we <m>M</m> appears in only one place
				in this equation.  In order to un-do the differentiation, we can integrate both sides of the
				equation.
				<md>
					<mrow>	\int  \frac{d}{dt}\Big( t^{-4}\cdot M \Big)dt	\amp = \int t^2 + t^{-3} dt	</mrow>
					<mrow>					t^{-4}\cdot M	\amp = \frac{1}{3}t^{3} - \frac{1}{2}t^{-2} + C	</mrow>
					<mrow>					\frac{M}{t^4}	\amp = \frac{1}{3}t^{3} - \frac{1}{2}t^{-2} + C	</mrow>
				</md>
			</p>

			<p>
				Finally, we can solve for <m>M</m> by multiplying both sides of the equation by <m>t^4.</m>
				<me>M = \frac{1}{3}t^{7} - \frac{1}{2}t^2 + Ct^4</me>
			</p>

			<p>
				We have made a point of simplifying whenever possible, and you should look to
				do that as you work.  You may be tempted to replace the <m>Ct^3</m> with a single constant;
				remember, however, that a constant times a function is not a constant, so we cannot
				simplify that last term any further.
			</p>

			<p>
				Hence, we have found the solution to the DE.  We can always verify our solution
				by substituting back in to the original DE.  This is optional, but the details are included here.
				<md>
					<mrow>	LHS	\amp = -\frac{4}{t^2} \cdot M 	</mrow>
					<mrow>	\amp = -\frac{4}{t^2} \cdot \left( \frac{1}{3}t^{7} - \frac{1}{2}t^2 + Ct^4 \right)	</mrow>
					<mrow>	\amp = -\frac{4}{3}t^5 + 2 - 4Ct^2	</mrow>
				</md>

				<md>
					<mrow>	RHS	\amp =  t^5 - \frac{1}{t} \cdot\frac{dM}{dt} + 1	</mrow>
					<mrow>	\amp = t^5 - \frac{1}{t} \cdot\frac{d}{dt}\left( \frac{1}{3}t^{7} - \frac{1}{2}t^2 + Ct^4 \right) + 1	</mrow>
					<mrow>	\amp = t^5 - \frac{1}{t} \cdot \left( \frac{7}{3}t^{6} - t + 4Ct^3 \right) + 1	</mrow>
					<mrow>	\amp = t^5 -\frac{7}{3}t^{5} +1 - 4Ct^2 + 1	</mrow>
					<mrow>	\amp = -\frac{4}{3}t^5 + 2 - 4Ct^2	</mrow>
					<mrow>	\amp = LHS	</mrow>
				</md>
			</p>
		</solution>
	</example>

	<example xml:id="example-if-examples-02">
		<p>
			Solve the following initial value problem.
			<me>A = \sec\theta A' - \frac{\theta e^{\theta^2 + \sin\theta}}{\cos \theta}, \hspace{1cm} A(0) = -\frac{1}{2}</me>
		</p>

		<solution>
			<p>
				As always, we begin by identifying the independent and dependent variables
				and classifying the DE.
				<ul>
					<li>  independent variable:  <m>\theta</m>	</li>
					<li>  dependent variable:  <m>A</m>	</li>
					<li>  order:  first order	</li>
					<li>  linearity:  linear	</li>
					<li>  goal:  solve for the unknown function <m>A(\theta)</m>	</li>
				</ul>
			</p>

			<p>
				Since this DE is first order and linear, we can use the integrating factor technique.
				We begin to put the DE in <em> standard form</em> for this technique by getting
				the dependent variable and its derivative on the left hand side of the equals sign.
				<md>
					<mrow>	A	\amp = \sec\theta A' - \frac{\theta e^{\theta^2 + \sin\theta}}{\cos \theta}	</mrow>
					<mrow>	-\sec\theta A' + A	\amp =  - \frac{\theta e^{\theta^2 + \sin\theta}}{\cos \theta}	</mrow>
				</md>
			</p>

			<p>
				Next we want to make the coefficient on the <m>A'</m> term equal to 1.  We can divide by
				<m>-\sec \theta</m>, which is equivalent to multiplying by <m>-\cos \theta.</m>
				<men xml:id="this_st_form"> A' - \cos\theta A	=  \theta e^{\theta^2 + \sin\theta}</men>
			</p>

			<p>
				Now we can identify the function <m>P(\theta)</m>, which consists of whatever is attached to the dependent
				variable <m>A</m> by multiplication.  In this case, <m>P(\theta) = - \cos \theta</m>.  Then we find <m>z</m> as follows.
				<me>z = e^{\int P(\theta) d\theta} = e^{\int -\cos \theta d\theta} = e^{-\sin \theta}</me>
			</p>

			<p>
				(As before, we need only one integrating factor <m>z</m>, so we omit the <m>+C</m> we normally see when we	evaluate an indefinite integral).
			</p>

			<p>
				Once we have identified our integrating factor, we can multiply both sides of the DE in its standard form (as in equation (<xref ref="this_st_form" />)) by the function <m>z</m>.
				<md>
					<mrow>	e^{-\sin \theta}A' - \cos\theta e^{-\sin \theta}A	\amp =  \theta e^{\theta^2 + \sin\theta}e^{-\sin \theta}	</mrow>
					<mrow>									\amp =  \theta e^{\theta^2 + \sin\theta-\sin \theta}	</mrow>
					<mrow>									\amp = \theta e^{\theta^2}	</mrow>
				</md>
			</p>

			<p>
				If we have correctly determined the integrating factor <m>z</m>, we should be able to un-do the product
				rule on the left hand side.  We can identify the functions <m>f</m> and <m>g</m> below:
				<me>\underbrace{e^{-\sin \theta}}_{\scriptsize f}\cdot \underbrace{A'}_{\scriptsize g'}
					+ \underbrace{- \cos\theta e^{-\sin \theta}}_{\scriptsize f'}\cdot \underbrace{A}_{\scriptsize g}
						= \theta e^{\theta^2}.</me>
			</p>

			<p>
				It is critical that you verify that the function <m>z</m> does, in fact, create a situation
				where we see a function <m>f</m> and its derivative <m>f'</m> as shown above.  In this case,
				<md>
					<mrow>	f'(t)	\amp = \frac{d}{dt} \Big(f(t)\Big)	</mrow>
					<mrow>				\amp = \frac{d}{dt}\Big( e^{-\sin \theta} \Big)	</mrow>
					<mrow>				\amp = e^{-\sin \theta} \cdot \frac{d}{dt}\Big( -\sin\theta \Big)	</mrow>
					<mrow>				\amp = e^{-\sin \theta} \cdot \Big( -\cos\theta \Big)	</mrow>
					<mrow>				\amp = -\cos\theta e^{-\sin \theta},	</mrow>
				</md>
				so we can confirm that we have correctly identified the functions <m>f</m> and <m>g</m> to un-do
				the product rule.  This, we can re-write the left hand side of the equation as follows.
				<me>\frac{d}{dt}\Big( e^{-\sin \theta}\cdot A \Big) = \theta e^{\theta^2}.</me>
			</p>

			<p>
				Our goal is to solve for <m>A</m>.  Since it is currently inside the derivative, we will integrate
				both sides of the equation.
				<md>
					<mrow>	\int \frac{d}{dt}\Big( e^{-\sin \theta}\cdot A \Big) d\theta	\amp = \int \theta e^{\theta^2} d\theta	</mrow>
					<mrow>						e^{-\sin \theta}\cdot A	\amp =  \int \theta e^{\theta^2} d\theta	</mrow>
				</md>
			</p>

			<p>
				In order to evaluate the integral on the right hand side, we can make the substitution
				<m>u = \theta^2</m>, which means that <m>du = 2\theta d\theta</m>, or equivalently <m>\frac{1}{2}du = \theta d\theta</m>.
				<md>
					<mrow>	e^{-\sin \theta}\cdot A	\amp =  \int  \underbrace{e^{\theta^2}}_{\scriptsize e^u} \underbrace{\theta d\theta}_{\scriptsize \frac{1}{2}du}	</mrow>
					<mrow>					\amp = \int \frac{1}{2}e^u du	</mrow>
					<mrow>					\amp = \frac{1}{2}e^u + C	</mrow>
					<mrow>					\amp = \frac{1}{2}e^{\theta^2} + C	</mrow>
				</md>
			</p>

			<p>
				Now we can solve for <m>A</m>.
				<md>
					<mrow>	A	\amp = \frac{1}{2}\frac{e^{\theta^2}}{e^{-\sin \theta}} + \frac{C}{e^{- \sin \theta}}	</mrow>
					<mrow>				\amp = \frac{1}{2}e^{\theta^2 + \sin \theta} + Ce^{\sin \theta}	</mrow>
				</md>
			</p>

			<p>
				Finally, we need to apply the initial condition we are provided so that we can determine the constant <m>C</m>.
				<md>
					<mrow>	-\frac{1}{2}	\amp = A(0)	</mrow>
					<mrow>			\amp = \frac{1}{2}e^{0^2 + \sin(0)} + Ce^{\sin(0)}	</mrow>
					<mrow>			\amp = \frac{1}{2}e^0 + Ce^0	</mrow>
					<mrow>			\amp = \frac{1}{2} + C	</mrow>
					<mrow>		-1	\amp = C	</mrow>
				</md>
			</p>

			<p>
				We can then write the particular solution to the initial value problem.
				<me>A = \frac{1}{2}e^{\theta^2 + \sin \theta} - e^{\sin \theta}</me>
			</p>

			<p>
				As usual, we can check our answer by substituting back into the original DE.  While this step is
				not required, it is always a good idea to check and we include the details here.
				<md>
					<mrow>	LHS	\amp = A	</mrow>
					<mrow>	\amp = \frac{1}{2}e^{\theta^2 + \sin \theta} - e^{\sin \theta}	</mrow>
				</md>

				<md>
					<mrow>	RHS	\amp = \sec\theta A' - \frac{\theta e^{\theta^2 + \sin\theta}}{\cos \theta}	</mrow>
					<mrow>	\amp = \sec\theta\cdot \frac{d}{d\theta}\left( \frac{1}{2}e^{\theta^2 + \sin \theta} - e^{\sin \theta} \right) - \frac{\theta e^{\theta^2 + \sin\theta}}{\cos \theta}	</mrow>
					<mrow>	\amp = \sec\theta\cdot \left[ \frac{1}{2}e^{\theta^2 + \sin \theta}\cdot\frac{d}{d\theta}\left( \theta^2 + \sin \theta \right) 	</mrow>
					<mrow>				- e^{\sin\theta} \cdot \frac{d}{d\theta}\left( \sin \theta \right) \right]
									- \frac{\theta e^{\theta^2 + \sin\theta}}{\cos \theta}	</mrow>
					<mrow>	\amp = \sec\theta\cdot \left[ \theta e^{\theta^2 + \sin \theta} + \frac{1}{2}\cos \theta e^{\theta^2 + \sin \theta}
									- \cos \theta e^{\sin\theta} \right]
									- \frac{\theta e^{\theta^2 + \sin\theta}}{\cos \theta}	</mrow>
					<mrow>	\amp = \frac{1}{\cos\theta}\cdot \left[ \theta e^{\theta^2 + \sin \theta} + \frac{1}{2}\cos \theta e^{\theta^2 + \sin \theta}
									- \cos \theta e^{\sin\theta} \right]
									- \frac{\theta e^{\theta^2 + \sin\theta}}{\cos \theta}	</mrow>
					<mrow>	\amp = \frac{\theta e^{\theta^2 + \sin \theta}}{\cos\theta} + \frac{1}{2}e^{\theta^2 + \sin \theta}
									- e^{\sin\theta}
									- \frac{\theta e^{\theta^2 + \sin\theta}}{\cos \theta}	</mrow>
					<mrow>	\amp = \frac{1}{2}e^{\theta^2 + \sin \theta} - e^{\sin\theta}	</mrow>
					<mrow>	\amp = LHS	</mrow>
				</md>
			</p>
		</solution>
	</example>

	<example>
		
		<p>
			Consider the following DE.
			<me>x^2y' = 5x^3 + 2x^3y </me>
		</p>

		<solution>
		
			<p>
				First we note that this equation is first order and linear.
			</p>

			<p>
				Our first step would be to move closer to seeing the form shown in <xref ref="undo_prod3" />.
				As such, we will put the terms containing the derivative, <m>y'</m>, and the function, <m>y</m>, on the same of the equation.
				<me>x^2 y' - 2x^3 y = 5x^3</me>
			</p>

			<p>
				In an ideal world, we would immediately be able to un-do the product rule on the left hand
				side of the equation.  Unfortunately, this doesn't work right now, so we need to do a little work to
				force it to work. %Obviously this sentence is awful.
				We would still like to push this into the form shown in (<xref ref="undo_prod3" />), so we can first divide the entire equation by the coefficient on <m>y'</m>,
				<me>y' - 2x y = 5x,</me>
				and then multiply by the function <m>z</m> that will help us un-do the product rule.
				<men xml:id="int_factor_ex1"> z\cdot y' - 2x z\cdot y = z\cdot 5x </men>
			</p>

			<p>
				In Example 6, we showed that the function <m>z</m> we need is given by <m>z = e^{\int P(x) dx}</m>.  We need only identify the function <m>P(x)</m> as in (<xref ref="undo_prod3" />).
				For this DE, we have <m>P(x) = -2x</m>.  Take special note of the inclusion of the negative sign.
				Hence, we have
				<me>z = e^{\int P(x) dx} = e^{\int -2x dx} = e^{-x^2}.</me>
			</p>

			<p>
				Note that we have assumed that the constant of integration is zero because we
				know we need just one function <m>z</m>, and we choose the simplest one.  Now we can replace
				the replace the <m>z</m>'s in Equation (<xref ref="int_factor_ex1" />) with <m>z = e^{-x^2}</m> to yield
				<me>e^{-x^2}\cdot y' - 2x e^{-x^2}\cdot y = 5xe^{-x^2}.</me>
			</p>

			<p>
				If we've done everything correctly so far, we should be able to undo the product rule
				on the left hand side.  We can identify functions <m>f</m> and <m>g</m> as follows:
				<me>\underbrace{e^{-x^2}}_{\scriptsize f}\cdot \underbrace{y'}_{\scriptsize g'}
					- \underbrace{2x e^{-x^2}}_{\scriptsize f'}\cdot \underbrace{y}_{\scriptsize g}
						= 5xe^{-x^2}.</me>
			</p>

			<p>
				We need to verify at this step that if we take the derivative of <m>f(x) = e^{-x^2}</m>, we
				do actually get the expression we've labeled as <m>f'</m>.  In this case, we do get <m>f'(x) = -2xe^{-x^2}</m>,
				as expected, so we have correctly determined the function <m>z</m> that will help us un-do the
				product rule.  This function, that plays a central role in this solution technique, is called the
				<term> integrating factor </term>.
			</p>

			<p>
				We have identified how we can un-do the product rule so now we need to do just that.
				<me>\frac{d}{dx}\Big( \underbrace{e^{-x^2}}_{\scriptsize f}\cdot \underbrace{y}_{\scriptsize g} \Big)
					= 5xe^{-x^2}.</me>
			</p>

			<p>
				We have just made a huge step forward in solving this DE!  We have made it so that
				the unknown function <m>y</m> now appears in the equation only once, so we can now work to solve
				for <m>y</m>.  As it stands, the function <m>y</m> is inside a derivative, so we can integrate both sides
				(with respect to the independent variable).
				<me>\int \frac{d}{dx}\Big( e^{-x^2} \cdot y \Big)dx = \int 5xe^{-x^2}dx</me>
			</p>

			<p>
				The integration and differentiation will un-do each other on the left hand side.  On
				the right hand side, we need a substitution, <m>u = -x^2</m>, in order to achieve the integration.
				This means <m>du = -2x dx</m>, or equivalently <m>-\frac{1}{2}du =x dx.</m>
				<md>
					<mrow>	e^{-x^2} \cdot y	\amp = \int 5xe^{-x^2}dx	</mrow>
					<mrow>			\amp = 5\int e^{-x^2}\cdot x dx	</mrow>
					<mrow>			\amp = 5 \int e^{u}\cdot -\frac{1}{2} du	</mrow>
					<mrow>			\amp = -\frac{5}{2}\int e^u du	</mrow>
					<mrow>			\amp = -\frac{5}{2}\int e^u + C	</mrow>
					<mrow>			\amp = -\frac{5}{2}e^{-x^2} + C	</mrow>
				</md>
			</p>

			<p>
				We are almost done; we need only divide both sides of the equation by <m>e^{-x^2}</m>
				to solve for <m>y</m>.
				<me>y = -\frac{5}{2} + \frac{C}{e^{-x^2}}</me>
			</p>

			<p>
				While the equation above is a valid solution, we may prefer to rewrite the second
				term using rules of exponents to yield
				<me>y = -\frac{5}{2} + Ce^{x^2}.</me>
			</p>

			<p>
				We have now found the general solution to the DE.  As always, we can verify that
				we have found the correct solution by substituting back into the original DE. %Put this in a collapsible?
				<md>
					<mrow> \mbox{LHS}	\amp = x^2y'	</mrow>
					<mrow>			\amp = x^2 \cdot \frac{d}{dx}\left( -\frac{5}{2} + Ce^{x^2} \right)	</mrow>
					<mrow>			\amp = x^2 \cdot \left( 0 + 2Cxe^{x^2} \right)	</mrow>
					<mrow>			\amp = 2C x^3 e^{x^2}	</mrow>
				</md>

				<md>
					<mrow>	\mbox{RHS}	\amp = 5x^3 + 2x^3y	</mrow>
					<mrow>			\amp = 5x^3 + 2x^3\left( -\frac{5}{2} + Ce^{x^2} \right)	</mrow>
					<mrow>			\amp = 5x^3 - 5x^3+ 2C x^3 e^{x^2}	</mrow>
					<mrow>			\amp = 2C x^3 e^{x^2}	</mrow>
				</md>
			</p>

			<p>
				Since we get the same result when we substitute our solution in on the right and left
				hand sides of the DE, we confirm that we did find the solution.
			</p>
		
		</solution>

	</example>

	<xi:include href="./c2-s3-ss4-interactives.ptx" />

</section>