<subsection xmlns:xi="http://www.w3.org/2001/XInclude"><title> <m>\lap\{f^{(n)}(t)\}</m> </title>

	<example>
			
		<m>\quad</m> Show that <m>\ds \lap\{f'(t)\} = s\lap\{f(t)\} - f(0), \quad s \gt 0</m>.

		<solution>
			<tabular>
				<col width="20%" halign="right" valign="top"/>
				<col width="80%" halign="left" valign="top"/>
				<row>
					<cell valign="top"><p><m>\ds \lap\{ f'(t) \} =</m></p></cell>
					<cell>
						<m>\ds =\int_0^{\infty} e^{-st} f'(t) dt </m>
					</cell>
					<cell/>
				</row>
				<row>
					<cell><xref ref="lt-derivative-key-step-1" text="title"/></cell>
					<cell>
						<m>\ds \left[ e^{-st} f(t) \right]_0^{\infty} - \int_0^{\infty} (-s e^{-st}) f(t) dt </m>
					</cell>
					<cell/>
				</row>
				<row>
					<cell><xref ref="lt-derivative-key-step-2" text="title"/></cell>
					<cell>
						<m>\ds \left[ e^{-st} f(t) \right]_0^{\infty} + s \ub{\int_0^{\infty} e^{-st} f(t) dt}_{\large \lap\{ f(t) \}} </m>
					</cell>
					<cell/>
				</row>
				<row>
					<cell><m>=</m></cell>
					<cell>
						<m>\ds \lim_{t \to \infty} \left( e^{-st} f(t) \right) - e^{-s \cdot 0} f(0) + s \lap\{ f(t) \} </m>
					</cell>
					<cell/>
				</row>
				<row>
					<cell><xref ref="lt-derivative-key-step-3" text="title"/></cell>
					<cell>
						<m>\ds 0 - f(0) + s \lap\{ f(t) \} </m></cell>
					<cell/>
				</row>
				<row>
					<cell><m>=</m></cell>
					<cell>
						<m>\ds s \lap\{ f(t) \} - f(0) </m>
					</cell>
					<cell/>
				</row>
			</tabular>
		</solution>
	</example>

	<p>
		The importance of this result cannot be overstated. Even if you did not completely understand the solution, this property highlights why Laplace transforms are so useful in solving differential equations. It essentially removes derivatives from the equation!
	</p>

	<p>
		This property hides another secret as well. It recursively <q>removes</q> derivatives one at a time. That is,
		<md>
			<mrow> 
				\lap\{ f'(t) \}	
					=\amp\ \us{\swarrow}{\ul{\color{green} s \lap\{ f(t)	\} - f(0)}}
			</mrow>
			<mrow> 
				\lap\{ f''(t) \}	
					=\amp\ s {\color{green} \lap\{ f'(t) \}} - f'(0)
			</mrow>
			<mrow> 
					=\amp\ s \Big[{\color{green} \lap\{f(t)\} - f(0)} \Big] - f'(0)
			</mrow>
			<mrow> 
					=\amp\ \us{\swarrow \hspace{5em}}{\ul{\color{blue} s \lap\{f(t)\} - sf(0) - f'(0)}}
			</mrow>
			<mrow> 
				\lap\{ f'''(t) \}	
					=\amp\ s {\color{blue} \lap\{ f''(t) \}} - f''(0)
			</mrow>
			<mrow> 
					=\amp\ s \Big[{\color{blue} s \lap\{f(t)\} - sf(0) - f'(0)}\Big] - f''(0)
			</mrow>
			<mrow> 
					=\amp\ s^3 \lap\{f(t)\} - s^2 f(0) - s f'(0) - f''(0)
			</mrow>
			<mrow> \vdots </mrow>
		</md>
		and the pattern continues for higher derivatives.
	</p>

	<assemblage xml:id="lt-properties-P3-P5"><title>Laplace Transform Properties <m>P_3-P_5</m></title>
		<p>
			Let <m>F(s) = \lap\{f(t)\}</m> and <m>G(s) = \lap\{g(t)\}</m>.
		</p>

		<p>
			<dl width="narrow">
				<li xml:id="P3"><title><m>P_3.</m></title>
					<m>\ds \lap\{ f'(t) \} = sF(s) - f(0) </m>
				</li>
				<li xml:id="P4"><title><m>P_4.</m></title>
					<m>\ds \lap\{ f''(t) \} = s^2F(s) - sf(0) - f'(0) </m>
				</li>
				<li xml:id="P5"><title><m>P_5.</m></title>
					<m>\ds \lap\{ f'''(t) \} = s^3F(s) - s^2f(0) - sf'(0) - f''(0) </m>
				</li>
			</dl>
		</p>
	</assemblage>

	<xi:include href="./c4-s2-ss3-interactives.ptx" />

</subsection>