<subsection xmlns:xi="http://www.w3.org/2001/XInclude"><title> Common Forms </title>
    
    <p>
        The Laplace Transform Method begins with the <xref ref="lt-roadmap-step1" text="custom">forward transformation</xref> of a differential equation with an unknown function <m>y(t)</m> into an algebraic equation with an unknown function <m>Y(s)</m>. Once <m>Y(s)</m> is determined, the final step is to recover the original function, <m>y(t)</m>, by reversing the transformation using an inverse Laplace transform, denoted as <m>\laplacesym^{-1}</m>.
    </p>

    <figure xml:id="lt-roadmap-step4">
        <caption>
            The Backward Laplace Transform: Reversing the process to recover the solution, <m>y(t)</m>, from the transformed equation.
        </caption>
        <image source="figures/LT-Diagram-Focused-Step-4.png" width="100%">
            <shortdescription>The Backward Laplace Transform</shortdescription>
        </image>
    </figure>

    <p>
        The inverse Laplace transform, like any inverse operation, undoes the effect of the forward transform. For example, applying <m>\cos^{-1}</m> to both sides of 
        <md>
            <mrow> \cos(\pi/4) = \sqrt{2}/2 \quad \implies\amp \quad \cos^{-1}(\cos(\pi/4)) = \cos^{-1}(\sqrt{2}/2) </mrow>
            <mrow>                          \quad \implies\amp \quad \pi/4 = \cos^{-1}(\sqrt{2}/2)                  </mrow>
        </md>
        reverses the cosine operation, bringing us back to the angle. Similarly, applying <m>\laplacesym^{-1}</m> to both sides of 
        <md>
            <mrow> \lap{e^{-3t}} = \frac{1}{s+3}  \quad \implies\amp \quad \ilap{\lap{e^{-3t}}} = \ilap{\frac{1}{s+3}}  </mrow>
            <mrow>                                  \quad \implies\amp \quad e^{-3t} = \ilap{\frac{1}{s+3}}                 </mrow>
        </md>,
        tells us that the inverse Laplace transform of <m>1/(s+3)</m> is <m>e^{-3t}</m>.
    </p>

    <p>
        <table halign="center" xml:id="common-lt-table"><title> <em>Common Laplace Transforms. <m>a, b</m> are constant, <m>n = 1, 2, \ldots</m></em> </title>
            <tabular halign="center">
                <row>
                    <cell/>
                    <cell><m>t</m>-functions</cell>
                    <cell colspan="2"><m>s</m>-functions</cell>
                </row>
                <row>
                    <cell/>
                    <cell><m>\downarrow</m></cell>
                    <cell colspan="2"><m>\downarrow</m></cell>
                </row>
                <row bottom="minor">
                    <cell right="minor"/>
                    <cell right="minor"><m>f(t)</m></cell>
                    <cell colspan="2"><m>\lap{ f(t) }</m></cell>
                </row>
                <row bottom="minor">
                    <cell right="minor"><m>L_1</m></cell>
                    <cell right="minor"><m>1</m></cell>
                    <cell><m>\ds \frac{1}{s}</m></cell>
                    <cell><m>s \gt 0</m></cell>
                </row>
                <row bottom="minor">
                    <cell right="minor"><m>L_2</m></cell>
                    <cell right="minor"><m>e^{at}</m></cell>
                    <cell><m>\ds \frac{1}{s-a}</m></cell>
                    <cell><m>s \gt a</m></cell>
                </row>
                <row bottom="minor">
                    <cell right="minor"><m>L_3</m></cell>
                    <cell right="minor"><m>t^n</m></cell>
                    <cell><m>\ds \frac{n!}{s^{n+1}}</m></cell>
                    <cell><m>s \gt 0</m></cell>
                </row>
                <row bottom="minor">
                    <cell right="minor"><m>L_4</m></cell>
                    <cell right="minor"><m>\sin (bt)</m></cell>
                    <cell><m>\ds \frac{b}{s^2 + b^2}</m></cell>
                    <cell><m>s \gt 0</m></cell>
                </row>
                <row bottom="minor">
                    <cell right="minor"><m>L_5</m></cell>
                    <cell right="minor"><m>\cos(bt)</m></cell>
                    <cell><m>\ds \frac{s}{s^2 + b^2}</m></cell>
                    <cell><m>s \gt 0</m></cell>
                </row>
                <row bottom="minor">
                    <cell right="minor"><m>L_6</m></cell>
                    <cell right="minor"><m>t^n e^{at}</m></cell>
                    <cell><m>\ds \frac{n!}{(s-a)^{n+1}}</m></cell>
                    <cell><m>s \gt a</m></cell>
                </row>
                <row bottom="minor">
                    <cell right="minor"><m>L_7</m></cell>
                    <cell right="minor"><m>e^{at} \sin(bt)</m></cell>
                    <cell><m>\ds \frac{b}{(s-a)^2 + b^2}</m></cell>
                    <cell><m>s \gt a</m></cell>
                </row>
                <row>
                    <cell right="minor"><m>L_8</m></cell>
                    <cell right="minor"><m>e^{at} \cos(bt)</m></cell>
                    <cell><m>\ds \frac{s-a}{(s-a)^2 + b^2}</m></cell>
                    <cell><m>s \gt a</m></cell>
                </row>
                <!-- <row>
                    <cell/>
                    <cell><m>\uparrow</m></cell>
                    <cell><m>\uparrow</m></cell>
                    <cell></cell>
                </row>
                <row>
                    <cell/>
                    <cell><m>t</m>-function</cell>
                    <cell><m>s</m>-function</cell>
                    <cell></cell>
                </row> -->
            </tabular>
        </table>

    </p>

    <p>
        <table halign="center" xml:id="lt-properties-table"><title> <em>Laplace Transforms Properties, <m>{\small \lap{ y(t) } = Y(t), \ \lap{ z(t) } = Z(t)}</m></em> </title>
            <tabular halign="center">
                <row bottom="minor">
                    <cell right="minor"/>
                    <cell><term>Properties</term></cell>
                </row>
                <row bottom="minor">
                    <cell right="minor"><m>P_1</m></cell>
                    <cell><m>\ds \lap{ a y(t) \pm b z(t) } = a Y(s) \pm b Z(s) \vphantom{\frac{d}{d}}</m></cell>
                </row>
                <row bottom="minor">
                    <cell right="minor"><m>P_2</m></cell>
                    <cell><m>\ds \lap{ e^{at} y(t) } = Y(s-a) \vphantom{\frac{d}{d}}</m></cell>
                </row>
                <row bottom="minor">
                    <cell right="minor"><m>P_3</m></cell>
                    <cell><m>\ds \lap{ y'(t) } = s\,Y(s) - y(0) \vphantom{\frac{d}{d}}</m></cell>
                </row>
                <row bottom="minor">
                    <cell right="minor"><m>P_4</m></cell>
                    <cell><m>\ds \lap{ y''(t) } = s^2\,Y(s) - s\,y(0) - y'(0) \vphantom{\frac{d}{d}}</m></cell>
                </row>
                <row bottom="minor">
                    <cell right="minor"><m>P_5</m></cell>
                    <cell><m>\ds \lap{ y'''(t) } = s^3\,Y(s) - s^2\,y(0) - s\,y'(0) - y''(0) \vphantom{\frac{d}{d}}</m></cell>
                </row>
                <row>
                    <cell right="minor"><m>P_6</m></cell>
                    <cell><m>\ds \lap{ y^n y(t) } = (-1)^n \frac{d^{(n)}}{ds^{(n)}}Y(s) \vphantom{\frac{d}{d}}</m></cell>
                </row>
            </tabular>
        </table>

    </p>

    <p>
        The <xref ref="lt-table-L1-L8" text="custom">table of common forward transforms</xref> doubles as a table for backward transforms. When working with inverse Laplace transforms, we start with the function of <m>s</m> (right) and seek the corresponding function in <m>t</m> (left). Let's see how this works through a few examples.
    </p>

    <p>
        Before diving into specifics, we need to mention the linearity property of the inverse Laplace transform, which will be crucial in this discussion.
        <assemblage xml:id="ilt-properties-P1"><title>Inverse Laplace Transform Property</title>
            <p>
                For any constants <m>a</m> and <m>b</m> and functions of <m>s</m> <m>F(s)</m> and <m>G(s)</m>, 
                <dl width="narrow">
                    <li xml:id="iP1">
                        <m>\ds \ilap{ a f(t) \pm b g(t) } = a \ilap{f(t)} \pm b \ilap{g(t)}</m>
                    </li>
                </dl>
            </p>
        </assemblage>
    </p>

    <example>
        <m>\quad</m>Find the inverse Laplace transforms of each function. 
        
        <tabular>
            <col width="20%" halign="center"/>
            <col width="75%"/>
            <row>
                <cell><m>\ds \frac{3}{s^2 + 9}</m></cell>
                <cell>
                    <p>
                        <m>\hspace{27em}</m>
                        <solution>
                            <p>
                                This matches the <m>L_4</m> form with <m>b=3</m>. So,
                                <me>
                                    \text{By } <xref ref="L4" text="custom">L_4</xref>, \quad \lap^{-1}\left\{\frac{3}{s^2 + 9}\right\} = \sin(3t).
                                </me>
                            </p>
                        </solution>
                    </p>
                </cell>
            </row>
            <row>
                <cell><m>\ds \frac{s - 2}{(s - 2)^2 + 16}</m></cell>
                <cell>
                    <p>
                        <m>\hspace{27em}</m>
                        <solution>
                            <p>
                                This matches the <m>L_7</m> form with <m>a=2</m> and <m>b=4</m>. So,
                                <me>
                                    \text{By } <xref ref="L7" text="custom">L_7</xref>, \quad \lap^{-1}\left\{\frac{s - 2}{(s - 2)^2 + 16}\right\} = e^{2t}\cos(4t)
                                </me>.
                            </p>
                        </solution>
                    </p>
                </cell>
            </row>
            <row>
                <cell><m>\ds \frac{24}{s^5}</m></cell>
                <cell>
                    <p>
                        <m>\hspace{27em}</m>
                        <solution>
                            <p>
                                The <m>s^5</m> in the denominator points us toward <m>L_3</m> with <m>n=4</m>.
                                <me>
                                    \text{By } <xref ref="L3" text="custom">L_3</xref>, \quad \ilap{\frac{24}{s^5}} = \ilap{\frac{4!}{s^{4+1}}} = t^4.
                                </me>
                            </p>
                        </solution>
                    </p>
                </cell>
            </row>
        </tabular>
        
    </example>

    <p>
        These examples demonstrate how to find the backward Laplace Transform when the <m>s</m>-function matches a form in the table of common forward transforms. However, not all functions will align perfectly with the table, and sometimes additional steps or modifications are needed. In the next subsections, we will explore properties of backward Laplace transforms and techniques for modifying the <m>s</m>-function before applying the inverse transform in the table.
    </p>

    <xi:include href="./c4-s2-ss1-interactives.ptx" />

</subsection>
