<section><title> Linear Systems </title>

	<introduction>
		<p>
			WRITE THIS
		</p>
	</introduction>

	<subsection label="second-order-to-system0"><title> Turning a Second-Order Equation into a System </title>
		<p>
			So far, we've looked at systems that involve multiple variables like <m>x(t)</m> and <m>y(t)</m>. But what if you start with just a single second-order differential equation? It turns out you can rewrite it as a system of first-order equations.
		</p>

		<p>
			For example, consider the second-order equation:
		</p>

		<me>
			y'' + 3y' + 2y = 0
		</me>

		<p>
			This equation involves only one dependent variable, <m>y(t)</m>, but it's second-order. To convert it into a system, we introduce a new variable:
		</p>

		<me>
			u = y, \quad v = y'
		</me>

		<p>
			That means <m>u' = y' = v</m>. And since <m>y'' = v'</m>, we can rewrite the original equation as:
		</p>

		<me>
			v' = -3v - 2u
		</me>

		<p>
			Now we have a system of two first-order equations:
		</p>

		<exercise label="chkpt-building-up-to-systems-1-3-10"><title>Derivative Substitution</title>
			<statement correct="yes">
				<p>
					In order to rewrite a second-order equation as a system, we can replace <m>y'</m> with a new variable and then express <m>y''</m> as the derivative of that new variable.
				</p>
			</statement>
			<feedback>
				<p>
					Correct. Introducing <m>x_1 = y</m> and <m>x_2 = y'</m> allows us to write <m>y''</m> as <m>x_2'</m> and form a system.
				</p>
			</feedback>
		</exercise>

		<md>
			<mrow> u' \amp = v </mrow>
			<mrow> v' \amp = -3v - 2u </mrow>
		</md>

		<p>
			This is a <em>partially coupled system</em>: <m>u</m> depends on <m>v</m>, and <m>v</m> depends on <m>u</m>. Together, they describe the same behavior as the original second-order equation.
		</p>

		<p>
			Writing a higher-order equation as a system helps us apply all the tools we're developing for first-order systemsâ€”especially when we introduce matrix methods.
		</p>

		<example xml:id="ex-second-order-to-system0">
			<title> From a Second-Order Equation to a System </title>
			<statement>
			<p>
				Rewrite the second-order equation <m>y'' - y = 0</m> as a system of first-order equations.
			</p>
			</statement>
			<solution>
			<p>
				Let <m>u = y</m> and <m>v = y'</m>. Then:
			</p>

			<me>
				u' = v
			</me>
			<p>
				and
			</p>
			<me>
				v' = y'' = y = u
			</me>

			<p>
				So the system becomes:
			</p>

			<md>
				<mrow> u' \amp = v </mrow>
				<mrow> v' \amp = u </mrow>
			</md>
			</solution>
		</example>

		<exercise label="chkpt-building-up-to-systems-1-3-20"><title>From Second Order to System</title>
			<statement>
				<p>
					What is the correct system corresponding to <m>y'' + 4y = 0</m> if we define <m>x_1 = y</m>, <m>x_2 = y'</m>?
				</p>
			</statement>
			<choices>
				<choice>
					<statement><p><m>x_1' = x_2</m>, <m>x_2' = -4x_2</m></p></statement>
					<feedback><p>That would be true if the original equation were <m>y'' + 4y'</m>. Double-check which variable is being multiplied by 4.</p></feedback>
				</choice>
				<choice>
					<statement><p><m>x_1' = x_2</m>, <m>x_2' = -4x_1 + x_2</m></p></statement>
					<feedback><p>Too many termsâ€”there's no <m>y'</m> in the original equation.</p></feedback>
				</choice>
				<choice correct="yes">
					<statement><p><m>x_1' = x_2</m>, <m>x_2' = -4x_1</m></p></statement>
					<feedback><p>Yes! <m>x_2' = y'' = -4y = -4x_1</m> is exactly what we want.</p></feedback>
				</choice>
				<choice>
					<statement><p><m>x_1' = x_1</m>, <m>x_2' = -4x_2</m></p></statement>
					<feedback><p>This system doesn't reflect the original equation at all.</p></feedback>
				</choice>
			</choices>
		</exercise>

		<conclusion><title> ðŸ“¤ Wrap-Up </title>
			<paragraphs><title> Summary </title>
				<p>
					<ul>
					<li>You can rewrite a second-order differential equation as a system of first-order equations by introducing new variables.</li>
					<li>This system often looks like a partially coupled system: each new variable depends on the other.</li>
					<li>This conversion is a key step in applying system-solving methods to second-order problems.</li>
					</ul>
				</p>
			</paragraphs>

			<paragraphs><title> Reading Questions </title>
				<exercise><title> Answer the Following </title>
					<task label="rqs-building-up-to-systems-1-3-1"><title>Understanding Converted Systems</title>
					<statement>
						<p>
						When you convert a second-order equation into a first-order system, which of the following are always true?
						</p>
					</statement>
					<choices>
						<choice correct="yes">
						<statement><p>The system has two first-order equations.</p></statement>
						<feedback><p>Yes. One for <m>y</m> and one for <m>y'</m>.</p></feedback>
						</choice>
						<choice correct="yes">
						<statement><p>The system involves two new variables: one for <m>y</m>, one for <m>y'</m>.</p></statement>
						<feedback><p>Exactly. This substitution is the key step.</p></feedback>
						</choice>
						<choice>
						<statement><p>The resulting system is always uncoupled.</p></statement>
						<feedback><p>Not true. The new variables often depend on each other.</p></feedback>
						</choice>
						<choice correct="yes">
						<statement><p>The system represents the same solutions as the original equation.</p></statement>
						<feedback><p>Correct. It's just a different form of the same information.</p></feedback>
						</choice>
						<choice>
						<statement><p>You can only use this method for linear equations.</p></statement>
						<feedback><p>This method also works for nonlinear second-order equations.</p></feedback>
						</choice>
					</choices>
					</task>

					<task label="rqs-building-up-to-systems-1-3-2"><title>Match Equations to Their Systems</title>
					<statement>
						<p>
						Match each second-order differential equation to the correct system using <m>x_1 = y</m> and <m>x_2 = y'</m>.
						</p>
					</statement>
					<feedback>
						<p>
						Each system reflects <m>x_1' = x_2</m> and an expression for <m>x_2'</m> based on <m>y''</m>.
						</p>
					</feedback>
					<cardsort>
						<match>
						<premise><m>y'' + y = 0</m></premise>
						<response><m>x_1' = x_2,\quad x_2' = -x_1</m></response>
						</match>
						<match>
						<premise><m>y'' - 2y' = 0</m></premise>
						<response><m>x_1' = x_2,\quad x_2' = 2x_2</m></response>
						</match>
						<match>
						<premise><m>y'' = y</m></premise>
						<response><m>x_1' = x_2,\quad x_2' = x_1</m></response>
						</match>
						<match>
						<premise><m>y'' = -y'</m></premise>
						<response><m>x_1' = x_2,\quad x_2' = -x_2</m></response>
						</match>
					</cardsort>
					</task>
				</exercise>
			</paragraphs>
		</conclusion>
	</subsection>

	<subsection label="second-order-to-system"><title>Turning a Second-Order Equation into a System</title>

<p>
	You've already learned how to solve second-order differential equations like:
</p>

<me>
	y'' + 3y' + 2y = 0
</me>

<p>
	But there's another way to think about this equationâ€”one that will be useful throughout this chapter. We can rewrite any second-order equation as a system of first-order equations by introducing new variables.
</p>

<p>
	Let's define:
</p>

<me>
	x_1 = y, \quad x_2 = y'
</me>

<p>
	Then <m>x_1'</m> is just <m>x_2</m>, and <m>x_2'</m> is <m>y''</m>. But we already know what <m>y''</m> is from the original equation:
</p>

<me>
	y'' = -3y' - 2y = -3x_2 - 2x_1
</me>

<p>
	So we can rewrite the second-order equation as the system:
</p>

<md>
	<mrow> x_1' \amp = x_2 </mrow>
	<mrow> x_2' \amp = -3x_2 - 2x_1 </mrow>
</md>

<p>
	Now we have a system of two first-order equations involving <m>x_1</m> and <m>x_2</m>. This system describes exactly the same behavior as the original second-order equation, just in a different form.
</p>

<p>
	Why would we want to do this? Because this form allows us to apply everything we're about to learn about systems: solution techniques, phase plane analysis, and numerical methods. And it works for <em>any</em> second-order equationâ€”not just the linear ones.
</p>

<example xml:id="ex-second-order-to-system">
	<title>Rewrite as a System</title>
	<statement>
	<p>
		Rewrite the second-order equation <m>y'' - y = 0</m> as a system of first-order equations.
	</p>
	</statement>
	<solution>
	<p>
		Define <m>x_1 = y</m>, <m>x_2 = y'</m>. Then:
	</p>
	<me>
		x_1' = x_2
	</me>
	<p>And</p>
	<me>
		x_2' = y'' = y = x_1
	</me>
	<p>So the system is:</p>
	<md>
		<mrow> x_1' \amp = x_2 </mrow>
		<mrow> x_2' \amp = x_1 </mrow>
	</md>
	</solution>
</example>

<conclusion>
	<title>ðŸ“¤ Wrap-Up</title>
	<paragraphs>
	<title>Summary</title>
	<p>
		<ul>
		<li>Any second-order differential equation can be written as a system of first-order equations by introducing new variables.</li>
		<li>This system has the same solutions as the original equationâ€”just organized differently.</li>
		<li>Working with systems lets us apply powerful techniques that work across a wide range of problems, including systems and higher-order equations.</li>
		</ul>
	</p>
	</paragraphs>
</conclusion>
</subsection>

	<subsection label="fully-coupled-systems_v1">
		<title> Fully Coupled Systems </title>

		<p>
			Finally, we arrive at a system where the variables influence each other completely:
		</p>

		<me>
			\begin{aligned}
			\frac{dx}{dt} \amp = ax + by \\
			\frac{dy}{dt} \amp = cx + dy
			\end{aligned}
		</me>

		<p>
			Neither equation stands aloneâ€”we can't solve for <m>x(t)</m> or <m>y(t)</m> without considering both. The system is now <em>fully coupled</em>.
		</p>

		<p>
			This is where we truly need to treat the system as a single object. We'll write it in vector form:
		</p>

		<me>
			\vec{X}' = A \vec{X}, \quad A = \begin{bmatrix} a \amp b \\ c \amp d \end{bmatrix}
		</me>

		<p>
			We'll learn how to solve these systems using matrix methods. But even now, we can explore how solutions behave visually.
		</p>

		<figure xml:id="fig-fully-coupled-phase-plane">
			<caption>Phase portrait of a fully coupled system, showing spiral or saddle behavior depending on the matrix <m>A</m>.</caption>
			<image src="images/fully-coupled-phase-plane.svg"/>
		</figure>

		<reading-questions>
			<question>
			<title> Interdependence </title>
			<statement>What makes a system fully coupled? How does that affect how we approach the problem?</statement>
			<hint>Look at the right-hand sides: can either equation be solved on its own?</hint>
			</question>
		</reading-questions>
	</subsection>

	<subsection label="fully-coupled-systems_v0">
	<title>When Variables Depend on Each Other</title>

	<p>
		We've now seen two types of systems: uncoupled systems, where each variable evolves independently, and partially coupled systems, where one variable depends on the other. Now let's look at the final case: when <em>both</em> variables affect each other.
	</p>

	<p>
		Consider this system:
	</p>

	<md>
		<mrow> \frac{dx}{dt} \amp = x + y \quad \text{with} \quad x(0) = 2 </mrow>
		<mrow> \frac{dy}{dt} \amp = x - y \quad \text{with} \quad y(0) = 0 </mrow>
	</md>

	<p>
		Both equations involve both variables. This is a <em>fully coupled</em> systemâ€”neither equation can be solved in isolation.
	</p>

	<p>
		In the previous section, we solved the system step-by-step because one equation was independent. That doesn't work here. Any change in <m>x</m> affects <m>y</m>, and <m>y</m> also influences <m>x</m>. The two variables evolve together, and we have to treat the system as a whole.
	</p>

	<p>
		At this point, we don't yet have the tools to solve such a system exactly. But we can still learn a lot by thinking about what the equations say and by sketching their behavior.
	</p>

	<example xml:id="ex-fully-coupled-narrative">
		<title>A Fully Coupled System</title>
		<statement>
		<p>
			Consider the system:
		</p>
		<md>
			<mrow> \frac{dx}{dt} \amp = x + y \quad \text{with} \quad x(0) = 2 </mrow>
			<mrow> \frac{dy}{dt} \amp = x - y \quad \text{with} \quad y(0) = 0 </mrow>
		</md>
		</statement>
		<solution>
		<p>
			Since both equations involve both <m>x</m> and <m>y</m>, there's no way to solve one without the other. However, we can still describe how the system behaves.
		</p>

		<p>
			- When <m>y</m> is positive, it pushes <m>x'</m> higher and pulls <m>y'</m> lower.
			- When <m>y</m> is negative, the opposite happens.
			- When <m>x = y</m>, we get: <m>x' = 2x</m> and <m>y' = 0</m>â€”so the solution moves right along a horizontal path.
			- When <m>x = -y</m>, we get: <m>x' = 0</m> and <m>y' = -2y</m>â€”motion is vertical.
		</p>

		<p>
			If we graph this system as a vector field in the <m>(x, y)</m> plane, we'll see curved trajectoriesâ€”possibly spiraling, possibly diverging. We'll explore these possibilities in more detail later.
		</p>
		</solution>
	</example>

	<p>
		Even without a complete solution, it's helpful to study how a system behaves by looking at its direction field or using technology to plot solution curves.
	</p>

	<p>
		Later, we'll learn a method for solving systems like this exactly by using something called <em>eigenvalues</em>. But for now, it's important to recognize when a system is fully coupled and why it's fundamentally different from the types we've already seen.
	</p>

	<conclusion><title>ðŸ“¤ Wrap-Up</title>

		<paragraphs><title>Summary</title>
		<p>
			<ul>
			<li>Fully coupled systems are those where all variables interact with each other.</li>
			<li>You can't solve one equation independentlyâ€”the system must be treated as a whole.</li>
			<li>We can often understand the behavior of a fully coupled system using visual tools like direction fields or technology, even before learning formal solution methods.</li>
			</ul>
		</p>
		</paragraphs>

	</conclusion>
	</subsection>

	<subsection label="what-is-a-linear-system">
<title>What Counts as a Linear System?</title>

<p>
	In this chapter, we'll learn how to understand and solve systems of differential equations that are <em>linear</em>. But what exactly does that mean?
</p>

<p>
	A system of differential equations is called <em>linear</em> if all of the dependent variables and their derivatives appear in a linear way: no powers, no products of variables, and no nonlinear functions like <m>\sin(x)</m> or <m>e^y</m>.
</p>

<p>
	For example, this is a linear system:
</p>

<md>
	<mrow> \frac{dx}{dt} \amp = 2x + 3y </mrow>
	<mrow> \frac{dy}{dt} \amp = -x + y </mrow>
</md>

<p>
	Each equation is a linear combination of <m>x</m> and <m>y</m>. The coefficients (2, 3, -1, 1) are just numbers. This system is both linear and has <em>constant coefficients</em>, which is the case we'll focus on.
</p>

<p>
	In contrast, the following system is <em>not</em> linear:
</p>

<md>
	<mrow> \frac{dx}{dt} \amp = xy </mrow>
	<mrow> \frac{dy}{dt} \amp = y^2 - x </mrow>
</md>

<p>
	The first equation contains a product <m>xy</m>, and the second equation contains a square <m>y^2</m>. That makes this a <em>nonlinear</em> system, which we'll learn to analyze later using different techniques.
</p>

<p>
	Linear systems are a powerful class of systems to study because they're flexible enough to model real-world interactionsâ€”like population dynamics, circuits, or mechanical motionâ€”and simple enough that we can often solve or analyze them exactly.
</p>

<p>
	In this section, we'll focus entirely on linear systems with constant coefficients. These take the form:
</p>

<md>
	<mrow> \frac{dx}{dt} \amp = a_{11}x + a_{12}y </mrow>
	<mrow> \frac{dy}{dt} \amp = a_{21}x + a_{22}y </mrow>
</md>

<p>
	where the numbers <m>a_{ij}</m> are constants. Even though we're not yet using matrix notation, this structure sets the stage for powerful techniques that make systems easier to understand and solve.
</p>

<conclusion>
	<title>ðŸ“¤ Wrap-Up</title>

	<paragraphs><title>Summary</title>
	<p>
		<ul>
		<li>A system is <em>linear</em> if the dependent variables appear without powers, products, or nonlinear functions.</li>
		<li>We'll focus on 2Ã—2 systems of the form <m>x' = ax + by</m>, <m>y' = cx + dy</m>, where all coefficients are constants.</li>
		<li>Linear systems are easier to analyze and solve than nonlinear onesâ€”and they still capture many interesting behaviors.</li>
		</ul>
	</p>
	</paragraphs>

</conclusion>
</subsection>

<subsection label="solving-by-exponentials">
<title>Solving a Linear System Using Exponentials</title>

<p>
	When we first learned to solve constant-coefficient equations like <m>y' = ky</m>, we guessed that the solution would be an exponential function: <m>y(t) = Ce^{kt}</m>. That same idea works for linear systems.
</p>

<p>
	Suppose we're given the system:
</p>

<md>
	<mrow> \frac{dx}{dt} \amp = 3x + 4y </mrow>
	<mrow> \frac{dy}{dt} \amp = -4x + 3y </mrow>
</md>

<p>
	Since the equations are linear with constant coefficients, we'll try guessing:
</p>

<me>
	x(t) = Ae^{rt}, \quad y(t) = Be^{rt}
</me>

<p>
	This guess assumes that both <m>x</m> and <m>y</m> grow (or decay, or oscillate) at the same exponential rate <m>r</m>, but with possibly different coefficients <m>A</m> and <m>B</m>.
</p>

<p>
	Let's plug the guess into the system. First, compute:
</p>

<me>
	x' = Ar e^{rt}, \quad y' = Br e^{rt}
</me>

<p>
	Substituting into the system:
</p>

<md>
	<mrow> Ar e^{rt} \amp = 3Ae^{rt} + 4Be^{rt} </mrow>
	<mrow> Br e^{rt} \amp = -4Ae^{rt} + 3Be^{rt} </mrow>
</md>

<p>
	Now divide both equations by <m>e^{rt}</m> (which is never zero) to get:
</p>

<md>
	<mrow> Ar \amp = 3A + 4B </mrow>
	<mrow> Br \amp = -4A + 3B </mrow>
</md>

<p>
	This is a system of algebraic equations in <m>A</m> and <m>B</m>, with <m>r</m> as a parameter. We can solve this by elimination or substitution, but really we're trying to find values of <m>r</m> that allow nontrivial solutions <m>(A, B) \ne (0, 0)</m>.
</p>

<p>
	That turns out to be an eigenvalue problemâ€”which we'll fully explore soonâ€”but for now, we'll give you the answer: the values of <m>r</m> that work here are <m>r = 3 \pm 4i</m>.
</p>

<p>
	So the general solution to this system is a combination of complex exponentials:
</p>

<me>
	x(t), y(t) = \text{linear combinations of } e^{(3 + 4i)t},\ e^{(3 - 4i)t}
</me>

<p>
	These are spirals! The <m>3</m> in the exponent causes the solution to grow, and the <m>4i</m> causes it to rotate. If we plotted the solution curves in the <m>(x, y)</m> plane, we would see spirals moving outward from the origin.
</p>

<p>
	We'll return to the full method (and remove the mystery) when we introduce eigenvalues and eigenvectors. For now, it's enough to understand that we can solve linear systems by guessing exponentialsâ€”and that the result may involve both growth and oscillation.
</p>

<example xml:id="ex-spiral-system">
	<title>Behavior of a Spiral System</title>
	<statement>
	<p>
		Consider the system:
	</p>
	<md>
		<mrow> \frac{dx}{dt} \amp = 2x + y </mrow>
		<mrow> \frac{dy}{dt} \amp = -x + 2y </mrow>
	</md>
	<p>
		Without solving, describe what you expect the phase portrait to look like.
	</p>
	</statement>
	<solution>
	<p>
		The system has constant coefficients and is linear, so we expect exponential solutions. Based on the symmetry and signs in the equations, we can guess that the eigenvalues will be complex with a positive real part.
	</p>

	<p>
		That suggests spiral behavior moving outward from the origin. The system has a spiral source at the origin.
	</p>
	</solution>
</example>

<conclusion>
	<title>ðŸ“¤ Wrap-Up</title>
	<paragraphs>
	<title>Summary</title>
	<p>
		<ul>
		<li>For constant-coefficient linear systems, we can guess solutions of the form <m>x(t) = Ae^{rt}</m>, <m>y(t) = Be^{rt}</m>.</li>
		<li>This leads to an algebraic system for <m>A</m>, <m>B</m>, and <m>r</m>.</li>
		<li>In most cases, we'll need tools from linear algebra to finish the solutionâ€”but even now, we can recognize the behavior of exponential solutions: decay, growth, spirals, and oscillation.</li>
		</ul>
	</p>
	</paragraphs>
</conclusion>
</subsection>

<subsection label="numerical-solutions-linear-systems">
<title>Numerical Solutions and the Flow of Information</title>

<p>
	What if you can't solve a system exactly, or you just want to understand what the solution looks like? One powerful option is to approximate the solution step by step. Let's see how that works for a linear system.
</p>

<p>
	Suppose we have the system:
</p>

<md>
	<mrow> \frac{dx}{dt} \amp = x + y </mrow>
	<mrow> \frac{dy}{dt} \amp = -x + y </mrow>
</md>

<p>
	With initial conditions: <m>x(0) = 1</m>, <m>y(0) = 0</m>. We'll use Euler's Method to approximate <m>x(t)</m> and <m>y(t)</m> for small steps of time.
</p>

<p>
	At each step, we estimate the new values of <m>x</m> and <m>y</m> using their current values and their derivatives:
</p>

<me>
	x_{\text{new}} = x + h \cdot (x + y), \quad y_{\text{new}} = y + h \cdot (-x + y)
</me>

<p>
	Try it with <m>h = 0.1</m>. At <m>t = 0</m>, we have:
</p>

<me>
	x_0 = 1, \quad y_0 = 0
</me>

<p>
	Then:
</p>

<me>
	x_1 = 1 + 0.1(1 + 0) = 1.1, \quad y_1 = 0 + 0.1(-1 + 0) = -0.1
</me>

<p>
	You can already see the feedback: <m>x</m> increases, <m>y</m> decreases in response to <m>x</m>, which then affects <m>x</m> again at the next step.
</p>

<p>
	Let's do one more step:
</p>

<me>
	x_2 = 1.1 + 0.1(1.1 - 0.1) = 1.1 + 0.1(1.0) = 1.2, \quad y_2 = -0.1 + 0.1(-1.1 - 0.1) = -0.1 + 0.1(-1.2) = -0.22
</me>

<p>
	We can continue this process to build a full table or plot of <m>(x(t), y(t))</m>. Each step shows how the system evolves, one moment at a time.
</p>

<p>
	This method doesn't require solving equationsâ€”it only requires evaluating derivatives. And it works for any system, linear or nonlinear.
</p>

<example xml:id="ex-euler-steps-system">
	<title>Euler's Method Applied to a System</title>
	<statement>
	<p>
		Use Euler's method with step size <m>h = 0.2</m> to estimate the values of <m>x</m> and <m>y</m> at <m>t = 0.2</m> and <m>t = 0.4</m> for the system:
	</p>

	<md>
		<mrow> \frac{dx}{dt} \amp = y </mrow>
		<mrow> \frac{dy}{dt} \amp = -x </mrow>
	</md>

	<p>With initial conditions <m>x(0) = 1</m>, <m>y(0) = 0</m>.</p>
	</statement>

	<solution>
	<p>
		Step 1: At <m>t = 0</m>, we have <m>x = 1</m>, <m>y = 0</m>.
	</p>

	<p>
		<m>x_1 = 1 + 0.2(0) = 1</m>, <m>y_1 = 0 + 0.2(-1) = -0.2</m>
	</p>

	<p>
		Step 2: At <m>t = 0.2</m>, <m>x = 1</m>, <m>y = -0.2</m>:
	</p>

	<p>
		<m>x_2 = 1 + 0.2(-0.2) = 0.96</m>, <m>y_2 = -0.2 + 0.2(-1) = -0.4</m>
	</p>

	<p>
		So we estimate:
		<m>(x(0.2), y(0.2)) \approx (1, -0.2)</m>, <m>(x(0.4), y(0.4)) \approx (0.96, -0.4)</m>
	</p>
	</solution>
</example>

<!-- <corollary><title> Euler's Method Visualized </title>
	<statement>
		<p>
			<sidebyside width="80%" margins="15% 5%">
				<interactive xml:id="initial-condition"
					platform="jsxgraph"
					aspect="5:2"
					dark-mode-enabled="yes"
					source="code/jsxgraph/eulers-method-systems/initial-condition.js"
				>
					<slate xml:id="euler-spiral-system-plot1" surface="jsxboard" aspect="5:2" />
					<static>
						<image source="code/jsxgraph/img-labels/t.png" width="70%"> Need to Add </image>
					</static>
				</interactive>
			</sidebyside>
		</p>
	</statement>
</corollary> -->

<corollary><title> Euler's Method Visualized </title>
	<statement>
		<p>
			<sidebyside width="80%" margins="15% 5%">
				<interactive xml:id="euler-spiral-system"
					platform="jsxgraph"
					aspect="5:2"
					dark-mode-enabled="yes"
					source="code/jsxgraph/eulers-method-systems/euler-spiral-system.js"
				>
					<slate xml:id="euler-spiral-system-plot1" surface="jsxboard" aspect="5:2" />
					<static>
						<image source="code/jsxgraph/img-labels/t.png" width="70%"> Need to Add </image>
					</static>
				</interactive>
			</sidebyside>
		</p>
	</statement>
</corollary>

<conclusion>
	<title>ðŸ“¤ Wrap-Up</title>
	<paragraphs>
	<title>Summary</title>
	<p>
		<ul>
		<li>We can approximate solutions to systems by updating each variable using its derivative.</li>
		<li>Euler's Method makes the interaction between variables explicit: at each step, the value of one variable influences how the other changes.</li>
		<li>This helps build intuition about the flow of information in dynamical systemsâ€”even when exact solutions are out of reach.</li>
		</ul>
	</p>
	</paragraphs>
</conclusion>
</subsection>



</section>

