<subsection xmlns:xi="http://www.w3.org/2001/XInclude"><title> Nonhomogeneous Equations </title>
	
	<p>
		In the previous chapter, we solved linear homogeneous constant coefficient equations of the form
		<me>
			a_n\ y^{(n)} + \cdots + a_2\ y'' + a_1\ y' + a_0\ y = 0
		</me>.
		Such equations are called <em>homogeneous</em> because of the zero on the right-hand side. In this chapter, we explore how to solve the more general case of <em>nonhomogeneous</em> equations, which include a non-zero function on the right-hand side, like so
		<me>
			a_n\ y^{(n)} + \cdots + a_2\ y'' + a_1\ y' + a_0\ y = f(x)
		</me>.
		For ease of discussion, will use the shorthand LNCC equations to refer to Linear Nonhomogeneous Constant Coefficient equations.
	</p>

	<p>
		Recall, the solution of a homogeneous equation is made up of <m>e^{r x}</m> terms which have the unique property of being like terms with its derivatives. This is needed so the terms on the left-hand side can cancel out to zero.
	</p>

	<figure xml:id="lhcc-vs-lcc-solution-type">
		<caption>Comparison of a homogeneous equation (<em>left</em>) and a nonhomogeneous equation (<em>right</em>). In both, the solutions must simplify in a specific way when substituted into the equation.</caption>
		<sidebyside widths="42% 45%">
			<image width="100%">
				<latex-image>
				
					\begin{tikzpicture}[join=round,rounded corners,&gt;=stealth,shorten &gt;=1pt,shorten &lt;=1pt,thick]
	
						\node (text) 	at (1.8,1.1) 	{\(e^{r x}-\)like};
						
						\node (blank1) at (0.3,0.4) {};
						\filldraw[fill=blue!20,fill opacity=0.2]
							(0,0)--(0.6,0)--(0.6,0.5)--(0,0.5)--cycle;
						
						\node 			at (0.75,0.35)	{$^{\prime\prime}$};
						\node 			at (1.0,0.25)	{$-$};
						\node 			at (1.3,0.25)	{$4$};
						
						\node (blank2) at (1.8,0.4) {};
						\filldraw[fill=blue!20,fill opacity=0.2]
							(1.5,0)--(2.1,0)--(2.1,0.5)--(1.5,0.5)--cycle;
		
						\node 			at (2.2,0.35)	{$^{\prime}$};
						\node 			at (2.4,0.25)	{$+$};
						\node 			at (2.7,0.25)	{$3$};
		
						\node (blank3) at (3.2,0.4) {};
						\filldraw[fill=blue!20,fill opacity=0.2]
							(2.9,0)--(3.5,0)--(3.5,0.5)--(2.9,0.5)--cycle;
						\node 			at (3.8,0.25)	{$=$};
						\node 			at (4.2,0.25)	{$0$};
						
						\draw[-&gt;,thick] (text.west)		--	+(-0.2,0) -| (blank1); 
						\draw[-&gt;,thick] (text)		--	+(0,-0.4) -| (blank2); 
						\draw[-&gt;,thick] (text.east)		--	+(0.1,0) -| (blank3); 
						
					\end{tikzpicture}
				</latex-image>
			</image>
			<image width="100%">
				<latex-image>
				
					\begin{tikzpicture}[join=round,rounded corners,&gt;=stealth,shorten &gt;=1pt,shorten &lt;=1pt,thick]
	
						\node (text) 	at (1.8,1.1) 	{\(f(x)-\)like};
						
						\node (blank1) at (0.3,0.4) {};
						\filldraw[fill=blue!20,fill opacity=0.2]
							(0,0)--(0.6,0)--(0.6,0.5)--(0,0.5)--cycle;
						
						\node 			at (0.75,0.35)	{$^{\prime\prime}$};
						\node 			at (1.0,0.25)	{$-$};
						\node 			at (1.3,0.25)	{$4$};
						
						\node (blank2) at (1.8,0.4) {};
						\filldraw[fill=blue!20,fill opacity=0.2]
							(1.5,0)--(2.1,0)--(2.1,0.5)--(1.5,0.5)--cycle;
		
						\node 			at (2.2,0.35)	{$^{\prime}$};
						\node 			at (2.4,0.25)	{$+$};
						\node 			at (2.7,0.25)	{$3$};
		
						\node (blank3) at (3.2,0.4) {};
						\filldraw[fill=blue!20,fill opacity=0.2]
							(2.9,0)--(3.5,0)--(3.5,0.5)--(2.9,0.5)--cycle;
						\node 			at (3.8,0.25)	{$=$};
						\node 			at (4.4,0.25)	{$f(x)$};
						
						\draw[-&gt;,thick] (text.west)		--	+(-0.3,0) -| (blank1); 
						\draw[-&gt;,thick] (text)		--	+(0,-0.4) -| (blank2); 
						\draw[-&gt;,thick] (text.east)		--	+(0.3,0) -| (blank3); 
						
					\end{tikzpicture}
				</latex-image>
			</image>
		</sidebyside>
	</figure>

	<p>
		In contrast, nonhomogeneous equations must have solutions that make the left-hand side simplify to <m>f(x)</m>, rather than zero. For this to happen, the solution should be <q><m>f(x)-</m>like</q> in the sense that it shares terms with <m>f(x)</m>. For example, consider the equation
		<me>
			y'' - 4y' + 3y = 9x
		</me>.
		When the solution, <m>y</m>, is plugged into the equation, the left-side terms must simplify to <m>9x</m>. So, <m>y</m> must be <q><m>9x</m> like</q>, but what is does <q><m>9x</m> like</q> mean? As you will see in the sections that follow, it means <m>y</m> has the form <m>y = Ax+B</m>. For now, let's just verify that <m>y = 3x + 4</m> is the <q><m>9x</m> like</q> solution that corresponds to this equation.
	</p>

	<example>
		<p>
			Verify that <m>y = 3x + 4</m> is a particular solution to the equation
			<me>y'' - 4y' + 3y = 9x</me>.
		</p>
		
		<solution>
			<p>
				To verify, we substitute <m>y = 3x + 4</m> into the equation:
				<md>
					<mrow> y'' - 4y' + 3y =\amp\ 9x </mrow>
					<mrow> 0 - 4(3) + 3(3x + 4) =\amp\ 9x </mrow>
					<mrow> -12 + 9x + 12 =\amp\ 9x </mrow>
					<mrow> 9x =\amp\ 9x \quad \checkmark </mrow>
				</md>
			</p>
		</solution>
	</example>
	
	<xi:include href="./p3-c2-s1-interactives.ptx" />

</subsection>