<section xml:id="using-the-lt-table">
	<title> Using the Laplace Transform Table </title>
	
	<introduction>
		<p>
			Need an INTRO
		</p>
	</introduction>

	<table xml:id="lt-table-L1-L12">
		<tabular top="minor" bottom="minor" left="minor" right="minor" halign="center" width="100%">
			<row bottom="none">
				<cell/>
				<cell>Forcing Function</cell>
				<cell>Laplace Transform</cell>
				<cell>Existence</cell>
			</row>
			<row>
				<cell/>
				<cell><me>f(t)</me></cell>
				<cell><me>\lap{f(t)} = F(s)</me></cell>
				<cell>Condition</cell>
			</row>
			<row>
				<cell>L<m>_1</m></cell>
				<cell><me>1</me></cell>
				<cell><me>\frac{1}{s}</me></cell>
				<cell><me>s &gt; 0</me></cell>
			</row>
			<row>
				<cell>L<m>_2</m></cell>
				<cell><me>e^{at}</me></cell>
				<cell><me>\frac{1}{s - a}</me></cell>
				<cell><me>s &gt; 0</me></cell>
			</row>
			<row>
				<cell>L<m>_3</m></cell>
				<cell><me>t^n</me></cell>
				<cell><me>\frac{n!}{s^{n+1}}</me></cell>
				<cell><me>s &gt; 0</me></cell>
			</row>
			<row>
				<cell>L<m>_4</m></cell>
				<cell><me>\sin(bt)</me></cell>
				<cell><me>\frac{b}{s^2+b^2}</me></cell>
				<cell><me>s &gt; 0</me></cell>
			</row>
			<row>
				<cell>L<m>_5</m></cell>
				<cell><me>\cos(bt)</me></cell>
				<cell><me>\frac{s}{s^2+b^2}</me></cell>
				<cell><me>s &gt; 0</me></cell>
			</row>
			<row>
				<cell>L<m>_6</m></cell>
				<cell><me>e^{at}\ t^n</me></cell>
				<cell><me>\frac{n!}{(s-a)^{n+1}}</me></cell>
				<cell><me>s &gt; a</me></cell>
			</row>
			<row>
				<cell>L<m>_7</m></cell>
				<cell><me>e^{at}\sin(bt)</me></cell>
				<cell><me>\frac{b}{(s-a)^2+b^2}</me></cell>
				<cell><me>s &gt; a</me></cell>
			</row>
			<row>
				<cell>L<m>_8</m></cell>
				<cell><me>e^{at}\cos(bt)</me></cell>
				<cell><me>\frac{s-a}{(s-a)^2+b^2}</me></cell>
				<cell><me>s &gt; a</me></cell>
			</row>
			<row>
				<cell>L<m>_9</m></cell>
				<cell><me>y'(t)</me></cell>
				<cell><me>sY(s) - y(0)</me></cell>
				<cell><me>s &gt; 0</me></cell>
			</row>
			<row>
				<cell>L<m>_{10}</m></cell>
				<cell><me>y''(t)</me></cell>
				<cell><me>s^2Y(s) - sy(0) - y'(0)</me></cell>
				<cell><me>s &gt; 0</me></cell>
			</row>
			<row>
				<cell>L<m>_{11}</m></cell>
				<cell><me>y'''(t)</me></cell>
				<cell><me>s^3Y(s) - s^2y(0) - sy'(0) - y''(0)</me></cell>
				<cell><me>s &gt; 0</me></cell>
			</row>
			<row>
				<cell>L<m>_{12}</m></cell>
				<cell><me>t^n f(t)</me></cell>
				<cell><me>(-1)^n \frac{d^{(n)}}{ds^{(n)}}F(s)</me></cell>
				<cell><me>s &gt; 0</me></cell>
			</row>
		</tabular>
	</table>

	<subsection><title> Table of Laplace Transforms </title>
		<lemma><title> üëÄ <em>Reading Preparation</em> </title>

			<p>
		
				Needs to be completed.
				
			</p>
		
		</lemma>

		<p>
			We have done a lot of work computing common transforms and deriving the properties of the Laplace transform. Now, we can summarize all of this information in a table for quick reference.
		</p>

		<assemblage xml:id="lt-table-L1-L12-shit"><title> ‚ú≥Ô∏è Common Laplace Transforms and Properties </title>
			<p>
				Assume <m>F(s) = \lap{f(t)}</m>, <m>a</m>, <m>b</m> are constant, and <m>n=0,1,2,3,\ldots</m>
			</p>

			<p>
				<sidebyside widths="5% 17% 50% 8%" margins="10% 10%" valign="middle">
					<p/>
					<p> <me> f(t) </me> </p>
					<p> <me> \lap{f(t)} = F(s) </me> </p>
					<p/>
				</sidebyside>
				<sidebyside widths="5% 17% 50% 8%" margins="10% 10%" valign="middle">
					<p> <me>L_{1}</me> </p>
					<p> <me> 1 </me> </p>
					<p> <me>\frac{1}{s}</me> </p>
					<p> <me>\vphantom{\int}s &gt; 0</me> </p>
				</sidebyside>
				<sidebyside widths="5% 17% 50% 8%" margins="10% 10%" valign="middle">
					<p> <me>L_{2}</me> </p>
					<p> <me> e^{at} </me> </p>
					<p> <me>\frac{1}{s - a}</me> </p>
					<p> <me>\vphantom{\int}s &gt; 0</me> </p>
				</sidebyside>
				<sidebyside widths="5% 17% 50% 8%" margins="10% 10%" valign="middle">
					<p> <me>L_{3}</me> </p>
					<p> <me> t^n </me> </p>
					<p> <me>\frac{n!}{s^{n+1}}</me> </p>
					<p> <me>\vphantom{\int}s &gt; 0</me> </p>
				</sidebyside>
				<sidebyside widths="5% 17% 50% 8%" margins="10% 10%" valign="middle">
					<p> <me>L_{4}</me> </p>
					<p> <me>\sin(bt)</me> </p>
					<p> <me>\frac{b}{s^2+b^2}</me> </p>
					<p> <me>\vphantom{\int}s &gt; 0</me> </p>
				</sidebyside>
				<sidebyside widths="5% 17% 50% 8%" margins="10% 10%" valign="middle">
					<p> <me>L_{5}</me> </p>
					<p> <me>\cos(bt)</me> </p>
					<p> <me>\frac{s}{s^2+b^2}</me> </p>
					<p> <me>\vphantom{\int}s &gt; 0</me> </p>
				</sidebyside>
				<sidebyside widths="5% 17% 50% 8%" margins="10% 10%" valign="middle">
					<p> <me>L_{6}</me> </p>
					<p> <me> e^{at}\ t^n </me> </p>
					<p> <me>\frac{n!}{(s-a)^{n+1}}</me> </p>
					<p> <me>\vphantom{\int}s &gt; a</me> </p>
				</sidebyside>
				<sidebyside widths="5% 17% 50% 8%" margins="10% 10%" valign="middle">
					<p> <me>L_{7}</me> </p>
					<p> <me> e^{at}\sin(bt) </me> </p>
					<p> <me>\frac{b}{(s-a)^2+b^2}</me> </p>
					<p> <me>\vphantom{\int}s &gt; a</me> </p>
				</sidebyside>
				<sidebyside widths="5% 17% 50% 8%" margins="10% 10%" valign="middle">
					<p> <me>L_{8}</me> </p>
					<p> <me> e^{at}\cos(bt) </me> </p>
					<p> <me>\frac{s-a}{(s-a)^2+b^2}</me> </p>
					<p> <me>\vphantom{\int}s &gt; a</me> </p>
				</sidebyside>
				<sidebyside widths="5% 17% 50% 8%" margins="10% 10%" valign="middle">
					<p> <me>L_{9}</me> </p>
					<p> <me> y'(t) </me> </p>
					<p> <me>sY(s) - y(0) </me> </p>
					<p> <me>\vphantom{\int}s &gt; 0</me> </p>
				</sidebyside>
				<sidebyside widths="5% 17% 50% 8%" margins="10% 10%" valign="middle">
					<p> <me>L_{10}</me> </p>
					<p> <me> y''(t) </me> </p>
					<p> <me>s^2Y(s) - sy(0) - y'(0) </me> </p>
					<p> <me>\vphantom{\int}s &gt; 0</me> </p>
				</sidebyside>
				<sidebyside widths="5% 17% 50% 8%" margins="10% 10%" valign="middle">
					<p> <me>L_{11}</me> </p>
					<p> <me> y'''(t) </me> </p>
					<p> <me>s^3Y(s) - s^2y(0) - sy'(0) - y''(0) </me> </p>
					<p> <me>\vphantom{\int}s &gt; 0</me> </p>
				</sidebyside>
				<sidebyside widths="5% 17% 50% 8%" margins="10% 10%" valign="middle">
					<p> <me>L_{12}</me> </p>
					<p> <me> t^n f(t) </me> </p>
					<p> <me>(-1)^n \frac{d^{(n)}}{ds^{(n)}}F(s)</me> </p>
					<p> <me>\vphantom{\int}s &gt; 0</me> </p>
				</sidebyside>
			</p>
		</assemblage>

		<mdn>
			<mrow xml:id="LL1"> \begin{array}{p{5cm}p{5cm}p{5cm}} \text{L}_1 \amp 1 \amp \dfrac{1}{s} \end{array} </mrow>
			<mrow xml:id="LL2"> \begin{array}{ccc} \text{L}_2 \amp e^{at} \amp \dfrac{1}{s - a} \end{array} </mrow>
			<mrow xml:id="LL3"> \begin{array}{ccc} \text{L}_3 \amp t^n \amp \dfrac{n!}{s^{n+1}} \end{array} </mrow>
			<mrow xml:id="LL4"> \begin{array}{ccc} \text{L}_4 \amp \sin(bt) \amp \dfrac{b}{s^2+b^2} \end{array} </mrow>
			<mrow xml:id="LL5"> \begin{array}{ccc} \text{L}_5 \amp \cos(bt) \amp \dfrac{s}{s^2+b^2} \end{array} </mrow>
			<mrow xml:id="LL6"> \begin{array}{ccc} \text{L}_6 \amp e^{at} t^n \amp \dfrac{n!}{(s-a)^{n+1}} \end{array} </mrow>
			<mrow xml:id="LL7"> \begin{array}{ccc} \text{L}_7 \amp e^{at}\sin(bt) \amp \dfrac{b}{(s-a)^2+b^2} \end{array} </mrow>
			<mrow xml:id="LL8"> \begin{array}{ccc} \text{L}_8 \amp e^{at}\cos(bt) \amp \dfrac{s-a}{(s-a)^2+b^2} \end{array} </mrow>
			<mrow xml:id="LL9"> \begin{array}{ccc} \text{L}_9 \amp y'(t) \amp sY(s) - y(0) \end{array} </mrow>
			<mrow xml:id="LL10"> \begin{array}{ccc} \text{L}_{10} \amp y''(t) \amp s^2Y(s) - sy(0) - y'(0) \end{array} </mrow>
			<!-- <mrow xml:id="LL2"> \lap{e^{at}} \amp = \frac{1}{s - a} </mrow>
			<mrow xml:id="LL3"> \lap{t^n} \amp = \frac{n!}{s^{n+1}} </mrow>
			<mrow xml:id="LL4"> \lap{\sin(bt)} \amp = \frac{b}{s^2+b^2} </mrow>
			<mrow xml:id="LL5"> \lap{\cos(bt)} \amp = \frac{s}{s^2+b^2} </mrow>
			<mrow xml:id="LL6"> \lap{e^{at} t^n} \amp = \frac{n!}{(s-a)^{n+1}} </mrow>
			<mrow xml:id="LL7"> \lap{e^{at}\sin(bt)} \amp = \frac{b}{(s-a)^2+b^2} </mrow>
			<mrow xml:id="LL8"> \lap{e^{at}\cos(bt)} \amp = \frac{s-a}{(s-a)^2+b^2} </mrow>
			<mrow xml:id="LL9"> \lap{f'(t)} \amp = sF(s) - f(0) </mrow>
			<mrow xml:id="LL10"> \lap{f''(t)} \amp = s^2F(s) - sf(0) - f'(0) </mrow>
			<mrow xml:id="LL11"> \lap{f'''(t)} \amp = s^3F(s) - s^2f(0) - sf'(0) - f''(0) </mrow>
			<mrow xml:id="LL12"> \lap{t^n f(t)} \amp = (-1)^n \frac{d^n}{ds^n}F(s) </mrow> -->
		</mdn>

		<assemblage xml:id="L1-L12-transforms"><title> ‚ú≥Ô∏è Laplace Transform Table </title>
			<p>
				Assume <m>F(s) = \lap{f(t)}</m>, <m>a</m>, <m>b</m> are constant, and <m>n=0,1,2,3,\ldots</m>
				<paragraphs xml:id="L1-L12">
					<title> Common Laplace Transforms </title>
						<dl>
							<li>
								<title>L<m>_1</m></title>
								<p>
									<me>\lap{1} = \frac{1}{s}</me>
								</p>
							</li>
							<li>
								<title>L<m>_2</m></title>
								<p>
									<me>\lap{e^{at}} = \frac{1}{s - a}</me>
								</p>
							</li>
							<li>
								<title>L<m>_3</m></title>
								<p>
									<me>\lap{t^n} = \frac{n!}{s^{n+1}}</me>
								</p>
							</li>
							<li>
								<title>L<m>_4</m></title>
								<p>
									<me>\lap{\sin(bt)} = \frac{b}{s^2+b^2}</me>
								</p>
							</li>
							<li>
								<title>L<m>_5</m></title>
								<p>
									<me>\lap{\cos(bt)} = \frac{s}{s^2+b^2}</me>
								</p>
							</li>
							<li>
								<title>L<m>_6</m></title>
								<p>
									<me>\lap{e^{at} t^n} = \frac{n!}{(s-a)^{n+1}}</me>
								</p>
							</li>
							<li>
								<title>L<m>_7</m></title>
								<p>
									<me>\lap{e^{at}\sin(bt)} = \frac{b}{(s-a)^2+b^2}</me>
								</p>
							</li>
							<li>
								<title>L<m>_8</m></title>
								<p>
									<me>\lap{e^{at}\cos(bt)} = \frac{s-a}{(s-a)^2+b^2}</me>
								</p>
							</li>
							<li>
								<title>L<m>_9</m></title>
								<p>
									<me>\lap{f'(t)} = sF(s) - f(0)</me>
								</p>
							</li>
							<li>
								<title>L<m>_{10}</m></title>
								<p>
									<me>\lap{f''(t)} = s^2F(s) - sf(0) - f'(0)</me>
								</p>
							</li>
							<li>
								<title>L<m>_{11}</m></title>
								<p>
									<me>\lap{f'''(t)} = s^3F(s) - s^2f(0) - sf'(0) - f''(0)</me>
								</p>
							</li>
							<li>
								<title>L<m>_{12}</m></title>
								<p>
									<me>\lap{t^n f(t)} = (-1)^n \frac{d^n}{ds^n}F(s)</me>
								</p>
							</li>
						</dl>
				</paragraphs>
				<paragraphs xml:id="L1">
					<title>L<m>_1</m><m>\ds\quad\lap{ 1 } = \frac{1}{s}, \quad s &gt; 0</m></title>
				</paragraphs>
				<paragraphs xml:id="L2">
					<title>L<m>_2</m><m>\ds\quad\lap{ e^{at} } = \frac{1}{s - a}, \quad s &gt;a </m></title>
				</paragraphs>
				<paragraphs xml:id="L3">
					<title>L<m>_3</m><m>\ds\quad\lap{ t^n } = \frac{n!}{s^{n+1}}, \quad s &gt;0, \quad n = 1, 2, 3, \ldots </m></title>
				</paragraphs>
				<paragraphs xml:id="L4">
					<title>L<m>_4</m><m>\ds\quad\lap{ \sin(bt) } = \frac{b}{s^2+b^2}, \quad s &gt;0</m></title>
				</paragraphs>
				<paragraphs xml:id="L5">
					<title>L<m>_5</m><m>\ds\quad\lap{ \cos(bt) } = \frac{s}{s^2+b^2}, \quad s &gt;0</m></title>
				</paragraphs>
				<paragraphs xml:id="L6">
					<title>L<m>_6</m><m>\ds\quad\lap{ e^{at}\ t^n } = \frac{n!}{(s-a)^{n+1}}, \quad s &gt;a, \quad n = 0, 1, 2, 3, \ldots </m></title>
				</paragraphs>
				<paragraphs xml:id="L7">
					<title>L<m>_7</m><m>\ds\quad\lap{ e^{at}\sin(bt) } = \frac{b}{(s-a)^2+b^2}, \quad s &gt;a</m></title>
				</paragraphs>
				<paragraphs xml:id="L8">
					<title>L<m>_8</m><m>\ds\quad\lap{ e^{at}\cos(bt) } = \frac{s-a}{(s-a)^2+b^2}, \quad s &gt;a</m></title>
				</paragraphs>
				<paragraphs>
					<title> Laplace Transform of Derivatives </title>
				</paragraphs>
				<paragraphs xml:id="L9">
					<title>L<m>_9</m><m>\ds\quad\lap{ f'(t) } = sF(s) - f(0), \quad s &gt; 0</m></title>
				</paragraphs>
				<paragraphs xml:id="L10">
					<title>L<m>_{10}</m><m>\ds\quad\lap{ f''(t) } = s^2F(s) - sf(0) - f'(0), \quad s &gt; 0</m></title>
				</paragraphs>
				<paragraphs xml:id="L11">
					<title>L<m>_{11}</m><m>\ds\quad\lap{ f'''(t) } = s^3F(s) - s^2f(0) - sf'(0) - f''(0), \quad s &gt; 0</m></title>
				</paragraphs>
				<paragraphs xml:id="L12">
					<title>L<m>_{12}</m><m>\ds\quad\lap{ t^n f(t) } = (-1)^n \frac{d^n}{ds^n}F(s), \quad s &gt; 0, \quad n = 0, 1, 2, 3, \ldots </m></title>
				</paragraphs>
			</p>
		</assemblage>
	</subsection>

	<objectives label="using-the-lt-table-wrapup">
		<ul>
			<li> 
			
			</li>
		</ul>
	</objectives>

	<fact label="using-the-lt-table-cyu">
		<statement>
			<p>
				Answer the following questions related to LNCC equations. Assume

				<task label="p4-c2-s1-1-rq1"><title> <em>The table of common forward Laplace transforms can also be used to find inverse Laplace transforms</em> </title>
					<statement correct="yes">
						<p>
							The table of common forward Laplace transforms can also be used to find inverse Laplace transforms
						</p>
					</statement>
					<feedback>
						<p>
							True. The same table used for forward transforms is used for backward transforms, but in reverse order.
						</p>
					</feedback>
				</task>
				
				<task label="p4-c2-s1-1-rq2"><title> <em>The inverse Laplace transform undoes the effect of the forward Laplace transform, allowing us to recover the original function <m>y(t)</m> from <m>Y(s)</m></em> </title>
					<statement correct="yes">
						<p>
							The inverse Laplace transform undoes the effect of the forward Laplace transform, allowing us to recover the original function <m>y(t)</m> from <m>Y(s)</m>
						</p>
					</statement>
					<feedback>
						<p>
							True. The inverse Laplace transform reverses the forward transformation, converting <m>Y(s)</m> back into <m>y(t)</m>.
						</p>
					</feedback>
				</task>
				
				<task label="p4-c2-s1-1-rq3"><title> <em>In the Laplace Transform Method, the backward transform <m><fillin characters="5" /></m></em> </title>
					<statement>
						<p>
							<em>In the Laplace Transform Method, the backward transform <m><fillin characters="5" /></m></em>
						</p>
					</statement>
					<choices randomize="yes">
						<choice>
							<statement>converts a differential equation into an algebraic equation.</statement>
							<feedback>
								<p>No, this describes the forward Laplace transform.</p>
							</feedback>
						</choice>
						<choice>
							<statement>solves the algebraic equation for <m>Y(s)</m>.</statement>
							<feedback>
								<p>No, solving for <m>Y(s)</m> happens after applying the forward transform.</p>
							</feedback>
						</choice>
						<choice correct="yes">
							<statement>recovers the original function <m>y(t)</m> from <m>Y(s)</m>.</statement>
							<feedback>
								<p>Correct! The inverse Laplace transform brings us back to the original function <m>y(t)</m>.</p>
							</feedback>
						</choice>
						<choice>
							<statement>eliminates initial conditions from the equation.</statement>
							<feedback>
								<p>No, initial conditions are incorporated into the transformed equation, not eliminated.</p>
							</feedback>
						</choice>
					</choices>
				</task>
				
				<task label="p4-c2-s1-1-rq4"><title> <em><m>\ds\quad \ilap{\frac{3}{s^2 + 9}} = <fillin characters="6" /></m></em> </title>
					<statement>
						<p>
							<em><m>\ds\quad \ilap{\frac{3}{s^2 + 9}} = <fillin characters="6" /></m></em>
						</p>
					</statement>
					<choices randomize="yes">
						<choice correct="yes">
							<statement><m>\sin(3t)</m></statement>
							<feedback>
								<p>Correct! The inverse Laplace transform of <m>\ds\frac{3}{s^2 + 9}</m> is <m>\sin(3t)</m>.</p>
							</feedback>
						</choice>
						<choice>
							<statement><m>\cos(3t)</m></statement>
							<feedback>
								<p>No, the correct transform for <m>\ds\frac{3}{s^2 + 9}</m> is <m>\sin(3t)</m>, not <m>\cos(3t)</m>.</p>
							</feedback>
						</choice>
						<choice>
							<statement><m>e^{3t}</m></statement>
							<feedback>
								<p>No, this is not the correct inverse transform for the given expression.</p>
							</feedback>
						</choice>
						<choice>
							<statement><m>\ds\frac{3}{s-3}</m></statement>
							<feedback>
								<p>No, this is not an inverse transform expression.</p>
							</feedback>
						</choice>
					</choices>
				</task>
				
				<task label="p4-c2-s1-1-rq6"><title> <em><m>\ds\quad \ilap{\frac{1}{s+3}} = <fillin characters="6" /></m></em> </title>
					<statement>
						<p>
							<em><m>\ds\quad \ilap{\frac{1}{s+3}} = <fillin characters="6" /></m></em>
						</p>
					</statement>
					<choices randomize="yes">
						<choice correct="yes">
							<statement><m>e^{-3t}</m></statement>
							<feedback>
								<p>Correct! The inverse Laplace transform of <m>\ds\frac{1}{s+3}</m> is indeed <m>e^{-3t}</m>.</p>
							</feedback>
						</choice>
						<choice>
							<statement><m>e^{3t}</m></statement>
							<feedback>
								<p>No, the correct answer is <m>e^{-3t}</m>, not <m>e^{3t}</m>.</p>
							</feedback>
						</choice>
						<choice>
							<statement><m>e^{-t}</m></statement>
							<feedback>
								<p>No, the exponent should be <m>-3t</m>, not <m>-t</m>.</p>
							</feedback>
						</choice>
						<choice>
							<statement><m>\ds\frac{1}{s-3}</m></statement>
							<feedback>
								<p>No, this is not the correct inverse Laplace transform.</p>
							</feedback>
						</choice>
					</choices>
				</task>
				
				<task label="p4-c2-s1-1-rq7"><title> <em><m>\ds\quad \ilap{\frac{24}{s^5}} = <fillin characters="6" /></m></em> </title>
					<statement>
						<p>
							<em><m>\ds\quad \ilap{\frac{24}{s^5}} = <fillin characters="6" /></m></em>
						</p>
					</statement>
					<choices randomize="yes">
						<choice>
							<statement><m>t^3</m></statement>
							<feedback>
								<p>No, this is incorrect. The correct answer is <m>t^4</m>.</p>
							</feedback>
						</choice>
						<choice correct="yes">
							<statement><m>t^4</m></statement>
							<feedback>
								<p>Correct! The inverse Laplace transform of <m>\ds\frac{24}{s^5}</m> is <m>t^4</m>.</p>
							</feedback>
						</choice>
						<choice>
							<statement><m>t^2</m></statement>
							<feedback>
								<p>No, the correct answer is <m>t^4</m>, not <m>t^2</m>.</p>
							</feedback>
						</choice>
						<choice>
							<statement><m>\ds\frac{1}{s^5}</m></statement>
							<feedback>
								<p>No, this is the original function in the <m>s</m>-domain, not its inverse transform.</p>
							</feedback>
						</choice>
					</choices>
				</task>
				
				<task label="p4-c2-s1-1-rq8"><title> <em><m>\ds\quad \ilap{\frac{2}{s^2 + 4}} = <fillin characters="6" /></m></em> </title>
					<statement>
						<p>
							<em><m>\ds\quad \ilap{\frac{2}{s^2 + 4}} = <fillin characters="6" /></m></em>
						</p>
					</statement>
					<choices randomize="yes">
						<choice correct="yes">
							<statement><m>\sin(2t)</m></statement>
							<feedback>
								<p>Correct! The inverse Laplace transform of <m>\ds\frac{2}{s^2 + 4}</m> is <m>\sin(2t)</m>.</p>
							</feedback>
						</choice>
						<choice>
							<statement><m>\cos(2t)</m></statement>
							<feedback>
								<p>No, the correct inverse Laplace transform is <m>\sin(2t)</m>, not <m>\cos(2t)</m>.</p>
							</feedback>
						</choice>
						<choice>
							<statement><m>e^{2t}</m></statement>
							<feedback>
								<p>No, the correct inverse transform is <m>\sin(2t)</m>, not <m>e^{2t}</m>.</p>
							</feedback>
						</choice>
						<choice>
							<statement><m>t^2</m></statement>
							<feedback>
								<p>No, the correct answer is <m>\sin(2t)</m>, not <m>t^2</m>.</p>
							</feedback>
						</choice>
					</choices>
				</task>
				
				<task label="p4-c2-s1-1-rq9"><title> <em><m>\ds\quad \ilap{\frac{1}{s - 5}} = <fillin characters="6" /></m></em> </title>
					<statement>
						<p>
							<em><m>\ds\quad \ilap{\frac{1}{s - 5}} = <fillin characters="6" /></m></em>
						</p>
					</statement>
					<choices randomize="yes">
						<choice correct="yes">
							<statement><m>e^{5t}</m></statement>
							<feedback>
								<p>Correct! The inverse Laplace transform of <m>\ds\frac{1}{s - 5}</m> is <m>e^{5t}</m>.</p>
							</feedback>
						</choice>
						<choice>
							<statement><m>e^{-5t}</m></statement>
							<feedback>
								<p>No, the correct answer is <m>e^{5t}</m>, not <m>e^{-5t}</m>.</p>
							</feedback>
						</choice>
						<choice>
							<statement><m>\cos(5t)</m></statement>
							<feedback>
								<p>No, this is not the correct inverse transform for the given expression.</p>
							</feedback>
						</choice>
						<choice>
							<statement><m>\sin(5t)</m></statement>
							<feedback>
								<p>No, the correct inverse transform for <m>\ds\frac{1}{s - 5}</m> is <m>e^{5t}</m>.</p>
							</feedback>
						</choice>
					</choices>
				</task>
				
				<task label="p4-c2-s1-1-rq10"><title> <em><m>\ds\quad \ilap{\frac{1}{(s+4)^2}} = <fillin characters="6" /></m></em> </title>
					<statement>
						<em><m>\ds\quad \ilap{\frac{1}{s - 5}} = <fillin characters="6" /></m></em>
					</statement>
					<choices randomize="yes">
						<choice correct="yes">
							<statement><m>te^{-4t}</m></statement>
							<feedback>
								<p>Correct! The inverse Laplace transform of <m>\ds\frac{1}{(s+4)^2}</m> is <m>te^{-4t}</m>.</p>
							</feedback>
						</choice>
						<choice>
							<statement><m>e^{4t}</m></statement>
							<feedback>
								<p>No, the correct answer is <m>te^{-4t}</m>, not <m>e^{4t}</m>.</p>
							</feedback>
						</choice>
						<choice>
							<statement><m>t^2e^{-4t}</m></statement>
							<feedback>
								<p>No, the correct inverse transform is <m>te^{-4t}</m>, not <m>t^2e^{-4t}</m>.</p>
							</feedback>
						</choice>
						<choice>
							<statement><m>e^{-4t}</m></statement>
							<feedback>
								<p>No, the correct answer is <m>te^{-4t}</m>, not <m>e^{-4t}</m>.</p>
							</feedback>
						</choice>
					</choices>
				</task>
			</p>
		</statement>
	</fact>
</section>