<subsection xmlns:xi="http://www.w3.org/2001/XInclude"><title>Transforming Equations</title>
		
	<p>
		Throughout this section, we learned how to apply Laplace transforms to individual functions. However, our goal is to solve differential equations, which means we need to understand how to transform an entire differential equation, including its initial conditions. This brings us back to the first step in the Laplace Transform Method roadmap.
	</p>
	
	<p>
		<image source="figures/LT-Diagram-Focused-Step-1.png" width="100%">
			<shortdescription>Step 1: The Forward Laplace Transform</shortdescription>
		</image>
	</p>

	<p>
		Our goal here is to apply the Laplace transform to both sides of this equation using the common transforms and properties we've discussed. Recall that applying a Laplace transform to a function can be thought of as multiplying the function by <m>e^{-st}</m> and integrating with respect to <m>t</m>. However, instead of explicitly writing out this process for every term, we simply apply the Laplace operator, <m>\laplacesym</m>, to both sides of the equation. Let's break this down with an example.
	</p>

	<example>
	
		<m>\quad</m>Apply the Laplace Transform to the initial-value problem
		<me>
			y'' + 3y' + 2y = -40e^{3t}, \quad y(0) = 0, \quad y'(0) = 1,
		</me>
		
		<solution>
			<p>
				First, apply <m>\laplacesym</m> to both sides of the equation
				<me>
					\lap{y'' + 3y' + 2y} = \lap{-40e^{3t}}
				</me>,
				and use the <xref ref="P1" text="custom"> linearity property, <m>P_1</m> </xref> 
				<me>
					\ub{\lap{y''}}_{(1)} + 3\ub{\lap{y'}}_{(2)} + 2\ub{\lap{y}}_{(3)} = -40\ub{\lap{e^{3t}}}_{(4)}
				</me>,
				to split this into four separate transforms. For this example, we will look at each one individually.
				<md>
					<mrow> 
						(1)\ :\quad \amp \lap{y''} = s^2Y - s\os{\large 0}{\os{\Large \shortparallel}{y(0)}} - \os{\large 1}{\os{\Large \shortparallel}{y'(0)}} = s^2 Y - 1 \vphantom{\frac{1}{1}} \quad <xref ref="P4" text="title"/>
					</mrow>
					<mrow> 
						(2)\ :\quad \amp \lap{y'} = sY - y(0) = sY \vphantom{\frac{1}{1}} \quad <xref ref="P3" text="title"/>
					</mrow>
					<mrow> 
						(3)\ :\quad \amp \lap{y} = Y \vphantom{\frac{1}{1}}
					</mrow>
					<mrow> 
						(4)\ :\quad \amp \lap{e^{3t}} = \frac{1}{s - 3} \quad <xref ref="L2" text="title"/>
					</mrow>
				</md>
			</p>

			<p>
				Plugging <m>(1) - (4)</m> back into the equation, we get
				<md>
					<mrow>
						s^2Y - 1 + 3sY + 2Y =\amp\ \frac{-40}{s - 3}, \quad \text{or}
					</mrow>
					<mrow>
						s^2Y + 3sY + 2Y - 1 =\amp\ \frac{-40}{s - 3}
					</mrow>
				</md>
			</p>
		</solution>
	</example>

	<p>
		To further illustrate this process, consider one more example.
	</p>

	<example>
	
		<m>\quad</m>Apply the Laplace Transform to the initial-value problem
		<me>
			y'' - 4y' + 6y = t^2, \quad y(0) = 2, \quad y'(0) = 0
		</me>. 
		
		<solution>
			<p>
				Applying the Laplace transform to both sides gives:
				<md>
					<mrow> 
						\lap{y'' - 4y' + 6y} =\amp\ \lap{t^2}
					</mrow>
					<mrow> 
						\lap{y''} - 4\lap{y'} + 6\lap{y} =\amp\ \lap{t^2}
					</mrow>
					<mrow> 
						s^2Y - s\os{\large 2}{\os{\Large \shortparallel}{y(0)}} - \os{\large 0}{\os{\Large \shortparallel}{y'(0)}} - 4(sY - \os{\large 2}{\os{\Large \shortparallel}{y(0)}}) + 6Y =\amp\ \frac{2}{s^3}
					</mrow>
					<mrow>
						s^2Y - 2s - 4sY + 8 + 6Y =\amp\ \frac{2}{s^3}	 
					</mrow>
					<mrow> 
						s^2Y - 4sY + 6Y - 2s + 8 =\amp\ \frac{2}{s^3}
					</mrow>
				</md>
			</p>
		</solution>
	</example>
	
	<p>
		In both examples, the differential equations have been transformed into algebraic equations, where solving for <m>Y</m> will be the next step in the Laplace Transform Roadmap.
	</p>

	<xi:include href="./c4-s1-ss5-interactives.ptx" />
	  
</subsection>
