<subsection xmlns:xi="http://www.w3.org/2001/XInclude"><title><m>\lap\{t^n\}</m></title>

	<p>
		Next, we'll explore the Laplace transform of the power function <m>t^n</m>, where <m>n</m> is a non-negative integer. We've already encountered the case where <m>n = 0</m>, since <m>t^0 = 1</m> and its transform is given by <xref ref="L1" text="custom"><m>L_1</m></xref>. Now, let's start with <m>n = 1</m> and work our way up to find a general formula for the Laplace transform of <m>t^n</m>.
	</p>

	<example>
		<p>
			Compute <m>\lap\{t\}</m>.
		</p>
	
		<solution>
			<p>
				We'll begin by applying the definition of the Laplace transform:
				<md>
					<mrow> 
						\lap\{ t \}
							\amp= \int_0^{\infty} e^{-st} \cdot t\ dt 
					</mrow>
					<mrow> 				
							\amp= \lim_{b \to \infty} \int_0^b t e^{-st}\, dt \quad (s \ne 0) \quad <xref text="custom" ref="LT-s-ne-0-t">Why is <m>s \ne 0</m>?</xref>
					</mrow>
				</md>
				Using integration by parts, we have:
				<md>
					<mrow> 
						\phantom{\lap\{t\}}
							\amp= \lim_{b \to \infty} \left[-\frac{b}{s}e^{-sb} + \frac{1}{s^2}\right] \quad <xref text="custom" ref="reason-int-by-parts-texpt">Integration by parts</xref>
					</mrow>
				</md>
				As <m>b</m> approaches infinity:
				<md>
					<mrow> 
						\phantom{\lap\{t\}}
							\amp= \left[-\frac{1}{s}\lim_{b \to \infty}\frac{b}{e^{sb}} + \frac{1}{s^2}\right] \quad (s &gt; 0) \quad <xref text="custom" ref="LT-s-gt-0-t">\text{Why is } s &gt; 0?</xref>
					</mrow>
					<mrow> 
						\phantom{\lap\{t\}}
							\amp= \left[0 + \frac{1}{s^2}\right] \quad <xref text="custom" ref="reason-limit-to-zero-t">Why is the limit 0?</xref>
					</mrow>
					<mrow> 		
							\amp= \frac{1}{s^2}, \quad s \gt 0
					</mrow>
				</md>
				Therefore, <m>\ds \lap\{ t \} = \frac{1}{s^2}</m>, valid for <m>s &gt; 0</m>.
			</p>
		</solution>
	</example>
	
	<p>
		Using similar steps, we can derive the following results:
	</p>

	<example>
		<p>
			<ul marker="square">
				<li>	
					<m> \ds \lap\{t^2\} = \frac{2}{s^3}, \quad s \gt 0 \quad </m> <xref ref="std_LT_01" text="custom">Solution</xref>
				</li>
				<li>	
					<m> \ds \lap\{t^3\} = \frac{6}{s^4}, \quad s \gt 0 \quad </m> <xref ref="std_LT_02" text="custom">Solution</xref> 
				</li>
				<li>
					<m> \ds \lap\{t^4\} = \frac{24}{s^5}, \quad s \gt 0 \quad </m> <xref ref="std_LT_03" text="custom">Solution</xref> 
				</li>
			</ul>
		</p>
	</example>

	<p>
		Do you notice the emerging pattern? Let's rewrite the numerators:
		<ul marker="">
			<li>	
				<m> \ds \lap\{t^2\} = \frac{2}{s^3} = \frac{2 \cdot 1}{s^3} = \frac{2!}{s^3} </m>
			</li>
			<li>	
				<m> \ds \lap\{t^3\} = \frac{6}{s^4} = \frac{3 \cdot 2 \cdot 1}{s^4} = \frac{3!}{s^4} </m>
			</li>
			<li>
				<m> \ds \lap\{t^4\} = \frac{24}{s^5} = \frac{4 \cdot 3 \cdot 2 \cdot 1}{s^5} = \frac{4!}{s^5} </m>
			</li>
			<li>
				<m> \hspace{6em} \vdots </m>
			</li>
			<li>
				<m> \ds \lap\{t^n\} = \frac{n!}{s^{n+1}} </m>
			</li>
		</ul>
		Thus, the general formula for the Laplace transform of <m>t^n</m> is:
		<me>\ds \lap\{t^n\} = \frac{n!}{s^{n+1}}, \quad s &gt; 0.</me>
	</p>

	<assemblage xml:id="lt-table-L3"><title>Common Laplace Transform <m>L_3</m></title>
		<p>
			<dl width="narrow">
				<li xml:id="L3"><title><m>{\LARGE \vphantom{\int}}L_3</m></title>
					<m>\ds \lap\{ t^n \} = \frac{n!}{s^{n+1}}, \quad s &gt;0, \quad n = 1, 2, 3, \ldots </m>
				</li>
			</dl>
		</p>
	</assemblage>

	<xi:include href="./c4-s1-ss4-interactives.ptx" />

</subsection>