<subsection xmlns:xi="http://www.w3.org/2001/XInclude"><title> <m>\lap\{e^{at}f(t)\}</m> </title>

	<example>
		
		<m>\quad</m> Compute	<m> \lap\{e^{7t}\cos(3t)\} </m>.

		<solution>
			<p>
				By the definition of the Laplace transform, we have
				<md>
					<mrow> 
						\lap\{e^{7t}\cos(3t)\} 
							=\amp \int_0^{\infty} e^{-st} e^{7t}\cos(3t) dt
					</mrow>
					<mrow> 
							=\amp \int_0^{\infty} e^{-st+7t} \cos(3t) dt
					</mrow>
					<mrow> 
							=\amp \int_0^{\infty} e^{-(s-7)t} \cos(3t) dt
					</mrow>
					<mrow> 
							=\amp \ub{\int_0^{\infty} e^{-(s_0)t} \cos(3t) dt}_{\lap\{\cos(3t)\}}, \quad \text{where } s_0 = s-7
					</mrow>
					<mrow>
							=\amp\ \frac{s_0}{s_0^2 + 9}  \qquad (s_0 \gt 0)
					</mrow>
					<mrow>
							=\amp\ \frac{s-7}{(s-7)^2 + 9} \qquad (s-7 \gt 0 \text{ or } s \gt 7)
					</mrow>
				</md>
			</p>
		</solution>
	</example>

	<assemblage xml:id="lt-properties-P1-P2"><title>Laplace Transform Properties</title>
		<p>
			Let <m>F(s) = \lap\{f(t)\}</m> and <m>G(s) = \lap\{g(t)\}</m>.
		</p>

		<p>
			<dl width="narrow">
				<li><title><m>P_1.</m></title>
					<m>\hspace{-3em}\ds \lap\{ a f(t) \pm b g(t) \} = a F(s) \pm b G(s), \quad a, b </m> are constants
				</li>
				<li xml:id="P2"><title><m>P_2.</m></title>
					<m>\hspace{-3em}\ds \lap\{ e^{at} f(t) \} = F(s-a), \quad a </m> is a constant
				</li>
			</dl>
		</p>
	</assemblage>

	<p>
		If we multiply <m>e^{at}</m> by the functions <m>t^n</m>, <m>\cos(bt)</m> and <m>\sin(bt)</m>, this property adds three more common Laplace transforms to our collection, as shown below.
	</p>

	<assemblage xml:id="lt-table-L1-L8"><title>Common Laplace Transforms</title>
		<p>
			<dl width="narrow">
				<li><title><m>{\LARGE \vphantom{\int}}L_1.</m></title>
					<m>\hspace{-3em}\ds \lap\{ 1 \} = \frac{1}{s}, \quad s &gt;0 </m>
				</li>
				<li><title><m>{\LARGE \vphantom{\int}}L_2.</m></title>
					<m>\hspace{-3em}\ds \lap\{ e^{at} \} = \frac{1}{s - a}, \quad s &gt;a, \quad a \text{ is a constant} </m>
				</li>
				<li><title><m>{\LARGE \vphantom{\int}}L_3.</m></title>
					<m>\hspace{-3em}\ds \lap\{ t^n \} = \frac{n!}{s^{n+1}}, \quad s &gt;0,\ n = 1, 2, 3, \ldots </m>
				</li>
				<li><title><m>{\LARGE \vphantom{\int}}L_4.</m></title>
					<m>\hspace{-3em}\ds \lap\{ \sin(bt) \} = \frac{b}{s^2+b^2}, \quad s &gt;0, \quad b \text{ is constant} </m>
				</li>
				<li><title><m>{\LARGE \vphantom{\int}}L_5.</m></title>
					<m>\hspace{-3em}\ds \lap\{ \cos(bt) \} = \frac{s}{s^2+b^2}, \quad s &gt;0, \quad b \text{ is constant} </m>
				</li>
				<li xml:id="L6"><title><m>{\LARGE \vphantom{\int}}L_6.</m></title>
					<m>\hspace{-3em}\ds \lap\{ t^n e^{at} \} = \frac{n!}{(s-a)^{n+1}}, \quad s &gt;a, \quad a \text{ is constant},\ n = 1, 2, 3, \ldots </m>
				</li>
				<li xml:id="L7"><title><m>{\LARGE \vphantom{\int}}L_7.</m></title>
					<m>\hspace{-3em}\ds \lap\{ e^{at}\cos(bt) \} = \frac{s-a}{(s-a)^2+b^2}, \quad s &gt;a, \quad a, b \text{ are constants} </m>
				</li>
				<li xml:id="L8"><title><m>{\LARGE \vphantom{\int}}L_8.</m></title>
					<m>\hspace{-3em}\ds \lap\{ e^{at}\sin(bt) \} = \frac{b}{(s-a)^2+b^2}, \quad s &gt;a, \quad a, b \text{ are constants} </m>
				</li>
			</dl>
		</p>
	</assemblage>

	<xi:include href="./c4-s2-ss2-interactives.ptx" />

</subsection>