<subsection xmlns:xi="http://www.w3.org/2001/XInclude"><title><m>\lap\{e^{at}\}</m></title>

	<p>
		The exponential function is commonly encountered in differential equations, making its Laplace transform especially important. Let's explore the Laplace transform of the exponential function <m>e^{at}</m>, where <m>a</m> is a constant. We'll start with a specific example, setting <m>a = 7</m>, and then generalize the result.
	</p>

	<example>

		<m>\quad</m> Compute <m> \lap \{ e^{7t} \} </m>.

		<solution>
			<p>
				We begin by applying the definition of the Laplace transform:
				<md>
					<mrow> 
						\lap\{ e^{7t} \} 
						\amp= \int_0^{\infty} e^{-st} \cdot e^{7t}\ dt
					</mrow>
					<mrow> 
						\amp= \lim_{b \to \infty}\int_0^b e^{(-s+7)t}\ dt
					</mrow>
				</md>
				For this improper integral to converge, the exponent <m>-s+7</m> must be negative, meaning:
				<me> 
					-s+7 \lt 0 \hspace{0.5cm}\Rightarrow \hspace{0.5cm} -s \lt -7 \hspace{0.5cm}\Rightarrow \hspace{0.5cm} s \gt 7
				</me>.
				Thus, we proceed under the assumption that <m>s \gt 7</m>.
				<md>
					<mrow> 
						\lap\{ e^{7t} \} 
							\amp= \lim_{b \to \infty}\int_0^b e^{(-s+7)t}\, dt
					</mrow>
					<mrow> 
							\amp= \lim_{b \to \infty} \frac{1}{7-s} e^{(-s+7)t} \Bigg|_0^b
					</mrow>
					<mrow> 
							\amp= \frac{1}{-s+7} \left[ \lim_{b \to \infty} \left( e^{(-s+7)b} - e^{0} \right) \right]
					</mrow>
					<mrow> 
							\amp= \frac{1}{-s+7} \left[ \lim_{b \to \infty} e^{(-s+7)b} - 1 \right]
					</mrow>
					<mrow>
							\amp= \frac{1}{-s+7} \left[ 0 - 1 \right] \qquad \Big(e^{(\text{negative})b} \to 0\Big)
					</mrow>
					<mrow>
							\amp= -\frac{1}{-s+7} = \frac{1}{s-7}. \quad \text{for } s \gt 7
					</mrow>
				</md>
				Thus, the Laplace transform of <m>e^{7t}</m> is:
				<me>\ds \lap\{e^{7t}\} = \frac{1}{s - 7}, \quad s \gt 7.</me>
			</p>
		</solution>

	</example>

	<p>
		To generalize this result, let's replace <m>7</m> with a constant <m>a</m>.
	</p>

	<example>

		<m>\quad</m> Show that <m>\ds \lap \{ e^{at} \} = \frac{1}{s - a} </m>.

		<solution>
			<p>
				We follow a similar process, starting with the definition of the Laplace transform:
				<md>
					<mrow> 
						\lap\{ e^{at} \} 
						\amp= \int_0^{\infty} e^{-st} \cdot e^{at}\ dt
					</mrow>
					<mrow> 
						\amp= \lim_{b \to \infty}\int_0^b e^{(-s+a)t}\ dt
					</mrow>
				</md>
				For the integral to converge, the exponent <m>-s+a</m> must be negative, which requires <m>\ -s+a \lt 0\ </m> or <m>\ s \gt a</m> to proceed
				<md>
					<mrow> 
						\lap\{ e^{at} \} 
						\amp= \lim_{b \to \infty}\int_0^b e^{(-s+a)t}\ dt
					</mrow>
					<mrow> 
						\amp= \lim_{b \to \infty} \frac{1}{-s+a} e^{(-s+a)t} \Bigg|_0^b
					</mrow>
					<mrow> 
						\amp= \frac{1}{-s+a} \left[ \lim_{b \to \infty} \left( e^{(-s+a)b} - e^{0} \right) \right]
					</mrow>
					<mrow> 
						\amp= \frac{1}{-s+a} \left[ \lim_{b \to \infty} e^{(-s+a)b} - 1 \right]
					</mrow>
					<mrow>
						\amp= \frac{1}{-s+a} \left[ 0 - 1 \right]
					</mrow>
					<mrow>
						\amp= -\frac{1}{-s+a} = \frac{1}{s-a}. \quad \text{for } s \gt a
					</mrow>
				</md>
				Thus, the Laplace transform of <m>e^{at}</m> is:
				<me>\ds \lap\{e^{at}\} = \frac{1}{s - a}, \quad s \gt a.</me>
			</p>
		</solution>

	</example>

	<p>
		With this result, we can now add the Laplace transform of <m>e^{at}</m> to our list of common Laplace transforms.
	</p>

	<assemblage xml:id="lt-table-L2"><title>Common Laplace Transform <m>L_2</m></title>
		<p>
			<dl width="narrow">
				<li xml:id="L2"><title><m>{\LARGE \vphantom{\int}}L_2</m></title>
					<m>\ds \lap\{ e^{at} \} = \frac{1}{s - a}, \quad s \gt a, \quad a \text{ is a constant} </m>
				</li>
			</dl>
		</p>
	</assemblage>

	<xi:include href="./c4-s1-ss3-interactives.ptx" />

</subsection>