<subsection xmlns:xi="http://www.w3.org/2001/XInclude"><title> Solutions to Differential Equations </title>

	<p>
        A solution to any equation—whether algebraic or differential—is a value or function that <q>satisfies</q> the equation. To <em>satisfy</em> an equation means that when the value or function is substituted into the equation, it reduces to a true statement, such as <m>0=0</m> or <m>1=1</m>.
    </p>

    <p>
        For example, consider the equation <me>y^3 = 3y + 2</me>. To verify if <m>y=2</m> is a solution, we substitute <m>2</m> and <m>0</m> in for <m>y</m> and check:
    </p>

    <sidebyside widths="12% 38% 12% 38%">
        <p>
            <me>
                \ul{y = 2}:
            </me>
        </p>
        <p>
            <md>
                <mrow> (2)^3 =\amp\ 3(2) + 2             </mrow>
                <mrow> 8     =\amp\ 6 + 2                </mrow>
                <mrow> 8     =\amp\ 8    \quad✅ </mrow>
            </md>
        </p>
        <p>
            <me>
                \ul{y = 0}:
            </me>
        </p>
        <p>
            <md>
                <mrow> (0)^3    =   \amp\ 3(0) + 2      </mrow>
                <mrow> 0        =   \amp\ 0 + 2         </mrow>
                <mrow> 0       \ne   \amp\ 2    \quad❌ </mrow>
            </md>
        </p>
    </sidebyside>

	<p>
        Since <m>y=2</m> results in a true statement, it is a solution. On the other hand, <m>y=0</m> does not satisfy the equation and is not a solution.
    </p>

	<p>
        Now, consider differential equations. Here, solutions are <em>functions</em> instead of single values. Verifying solutions to differential equations involves substituting the function and its derivatives into the equation. Let's explore this with an example.
    </p>

    <p>
        Determine whether <m>y = 3x</m> and <m>y = e^{3x}</m> are solutions to the differential equation <m>\ds y' = 3y.</m>
    </p>

    <sidebyside widths="12% 38% 12% 38%">
        <p>
            <me>
                \ul{y = 3x}:
            </me>
        </p>
        <p>
            <md>
                <mrow>               y' = 3y                   </mrow>
                <mrow> \left[3x\right]' = 3(3x)                 </mrow>
                <mrow> 3              \ne 9x      \quad❌ </mrow>
            </md>
        </p>
        <p>
            <me>
                \ul{y = e^{3x}}:
            </me>
        </p>
        <p>
            <md>
                <mrow>                    y' = 3y                        </mrow>
                <mrow> \left[e^{3x}\right]' = 3e^{3x}                     </mrow>
                <mrow> e^{3x} \cdot 3       = 3e^{3x}        \quad✅ </mrow>
            </md>
        </p>
    </sidebyside>
	
	<p>
		This shows that <m>y=e^{3x}</m> is a solution to <m>\ds y^\prime = 3y</m>, but <m>y=3x</m> is not.
	</p>

	<p>
        Let's practice verifying solutions through additional examples.
    </p>

	<example>

		<p>
			<statement>
				<p>
					Determine if <m>\ y= 2x^2\ </m> is a solution to 
					<me>xy' - 2x^2 = y</me>.
				</p>
			</statement>
		</p>

		<p>
			<solution>
				<p>
					Although it is not required, let's move all terms to the left-side of the equation, like so
					<me>xy' - 2x^2 - y = 0</me>.
				</p>

				<p>
					Doing this allows us to focus on simplifying just one side of the equation after plugging in <m>\ y= 2x^2</m>. 
					<md>
						<mrow> 									xy' - 2x^2 - y		=\amp 0			</mrow>
						<mrow> x\left( 2x^2 \right)' - 2x^2 - \left( 2x^2 \right)	=\amp 0			</mrow>
						<mrow> 					x\left( 4x \right) - 2x^2 - 2x^2	=\amp 0			</mrow>
						<mrow> 									4x^2 - 2x^2 - 2x^2	=\amp 0			</mrow>
						<mrow> 													0	=\amp 0	\quad✅ </mrow>
					</md>
					Therefore, <m>y= 2x^2</m> is a solution to <m>xy' - 2x^2 = y.</m>
				</p>
			</solution>
		</p>

	</example>

	<example>

		<p>
			<statement>
				<p>
					Determine if <m>\ P = \sin t\ </m> is a solution to 
					<me>2P'' + P = \sin t</me>.
				</p>
			</statement>
		</p>

		<p>
			<solution>
				<p>
					Since <m>P''</m> appears in the equation, lets compute it first.
					<me>	
						P = \sin t, \quad P' = \cos t, \quad P'' = -\sin t
					</me>
				</p>

				<p>
					Moving all the terms to the left and plugging in <m>P</m> and <m>P''</m>, we get
					<md>
						<mrow> 							2P'' + P - \sin t	=	\amp\ 0			</mrow>
						<mrow> 2\left( -\sin t \right) + (\sin t) - \sin t	=	\amp\ 0			</mrow>
						<mrow> -2\sin t + \cancel{\sin t} - \cancel{\sin t}	=	\amp\ 0			</mrow>
						<mrow> 									-2\sin t	\ne	\amp\ 0	\quad❌</mrow>
					</md>
					Therefore, <m>P = \sin t</m> is <term> not a solution </term> to <m>2P'' + P = \sin t.</m>
				</p>
			</solution>
		</p>

	</example>
	
	<p>
		You can even verify that a function is a solution to a differential equation when the function contains constants as the next two examples show.
	</p>

	<example xml:id="one-de-many-solns">

		<p>
			<statement>
				<p>
					Show that the functions 
					<me>y = e^{2x},\ \ y = 2e^{2x},\ \ y = 3e^{2x},\ \ y = -7e^{2x},\ \ y = 0.3e^{2x},\ \ y = \pi e^{2x} </me> 
					are solutions to the differential equation
					<me>\quad y' - 2y = 0</me>.
				</p>
			</statement>
		</p>

		<p>
			<solution>
				<p>
					Verifying each function individually would be repetitive because they all follow the same pattern: 
					<me>y = (\text{some number})\ e^{2x} \quad \text{or} \quad y = c e^{2x} </me>, 
					where <m>c</m> can be any constant. Let's show that <m>y = c e^{2x}</m> is a solution.
				</p>
				
				<p>
					Substitute <m>\ y = c e^{2x}\ </m> into the differential equation:
					<md>
						<mrow> 									y' - 2y	=\amp\ 0	</mrow>
						<mrow> 	\left(c e^{2x}\right)' - 2(c e^{2x})	=\amp\ 0	</mrow>
						<mrow> 				c e^{2x} (2) - 2c e^{2x}	=\amp\ 0	</mrow>
						<mrow> 					2c e^{2x} - 2c e^{2x}	=\amp\ 0	</mrow>
						<mrow> 										0	=\amp\ 0	</mrow>
					</md>
					Therefore, <m>y = c e^{2x}</m> is a solution for any value of constant, <m>c</m>.
				</p>
			</solution>
		</p>

	</example>

	<example xml:id="two-constant-solution-verification">

		<p>
			<statement>
				<p>
					Verify that <m>\ y = c_1 e^{-x} + c_2e^{x} + x^2 + 2\ </m> is a solution to
					<me>y'' - y = -x^2</me>.
				</p>
			</statement>
		</p>

		<p>
			<solution>

				<p>
					Move terms to left: <m>\quad y'' - y + x^2 = 0</m>
				</p>
		
				<p>
					Plug in <m>\ y = c_1 e^{-x} + c_2e^{x} + x^2 + 2\ </m> and simplify:
					<md>
						<mrow> 	\left( c_1 e^{-x} + c_2e^{x} + x^2 + 2 \right)'' - (c_1 e^{-x} + c_2e^{x} + x^2 + 2) + x^2 =\amp\ 0	</mrow>
						<mrow> 	\left( -c_1 e^{-x} + c_2e^{x} + 2x \right)' - c_1 e^{-x} - c_2e^{x} - x^2 - 2 + x^2 =\amp\ 0	</mrow>
						<mrow> 	c_1 e^{-x} + c_2e^{x} + 2 - c_1 e^{-x} - c_2e^{x} - x^2 - 2 + x^2 =\amp\ 0	</mrow>
						<mrow> 		0	=\amp\ 0	</mrow>
					</md>
					Therefore, <m>y = c_1 e^{-x} + c_2e^{x} + x^2 + 2</m> is a solution to
					<me>y'' - y = -x^2</me>.
				</p>

			</solution>
		</p>

	</example>

	<xi:include href="./chkpts-1-4-1-solns-to-des.ptx" />

</subsection>