<subsection xmlns:xi="http://www.w3.org/2001/XInclude"><title> Initial Conditions </title>

	<p>
		Solving a differential equation usually starts with finding its general solution, which represents all possible solutions up to one or more constants. Each constant can take any value, leading to infinitely many solutions.
	</p>

	<p>
		In real-world problems, we often reduce the number of possible solutions by specifying criteria that our solution must satisfy. Such criteria is imposed through <term>initial conditions</term>, which are known values of the solution or its derivatives at a particular point. With enough conditions, we can typically find all the constants in a general solution.
	</p>

	<sidebyside widths="30% 60%">
		<p>
			<image>
				<latex-image>
					\begin{tikzpicture}
						\draw[thick, -&gt;] (1, 0) -- (1, 5.6) node[above] {$h$ (ft)};
						\draw[thick, fill=gray!20] (-1.6, 0) rectangle (0.0, 5) node[midway] {Building};
						\node[circle, draw=red, fill=red!40, dashed, inner sep=2.6pt, label={left:$h(0)$}] at (1, 5) {};
						\draw[thick, red, -&gt;] (1.5, 5.2) -- (1.5, 4.8) node[midway, right] {$32\ \large\mathrm{\sfrac{ft}{s^2}}$};
						\node[circle, fill=red, inner sep=2.6pt, label={left:$h(t)$}] (mass) at (1, 1.8) {};
						\draw[thick, red, -&gt;] (1.5, 2.0) -- (1.5, 1.6) node[midway, right] {$32\ \large\mathrm{\sfrac{ft}{s^2}}$};
						\draw[thick] (-0.5, 0) -- (2.5, 0);
					\end{tikzpicture}
				</latex-image>
			</image>
		</p>
		<p>
			For example, consider an object in free fall with constant acceleration <m>32 \text{ ft/s}^2</m>. If <m>h(t)</m> is its height above the ground, the motion is described by the differential equation:
			<me>
				h''(t) = -32 \ \mathrm{ft/s^2}.
			</me>
			The general solution for the object's position is:
			<me>
				h(t) = c_1 + c_2t - 16t^2.
			</me>
		</p>
	</sidebyside>

	<p>
		This solution is a template for any object falling with constant acceleration. To make this solution more practical, let's impose the following criteria:
	</p>

	<ul>
		<li>The object starts at the top of a <m>100\ \mathrm{ft}</m> building.</li>
		<li>The object is dropped from rest.</li>
	</ul>


	<p>
		In terms of <m>h(t)</m>, this criteria can be translated as the two initial conditions
		<me>
			h(0) = 100\ \mathrm{ft} \quad \text{and} \quad h'(0) = 0\ \mathrm{ft/s}.
		</me>
	</p>

	<p>
		This new information forces <m>c_1</m> and <m>c_2</m> to take on specific values in the general solution, since
	</p>

	<p>
		<sidebyside widths="55% 3% 42%" margins="0% 0%">
			
			<p>
				<md>
					<mrow>	h(t)	=\amp\ c_1 + c_2t - 16t^2		</mrow>
					<mrow>		100	=\amp\ c_1 + c_2(0) - 16(0)^2	</mrow>
					<mrow>					100	=\amp\ c_1						</mrow>
				</md>
			</p>
			<p/>
			<p>
				<md>
					<mrow>	h'(t)	=\amp\ c_2 - 32t				</mrow>
					<mrow>		0	=\amp\ c_2 - 32(0)				</mrow>
					<mrow>				0	=\amp\ c_2						</mrow>
				</md>.
			</p>
		</sidebyside>
	</p>

	<p>
		This results in the particular solution
		<me>
			h(t) = 100 - 16t^2
		</me>,
		which describes the position of an object that, <em>specifically</em>, starts at <m>100 \ \mathrm{ft}</m> and is dropped with an initial velocity of <m>0 \ \mathrm{ft/s}</m>.
	</p>

	<p>
		When a differential equation includes initial conditions, it is called an <term>initial value problem</term>, which produces a particular solution rather than a general solution. Let's explore this further with examples.
	</p>

	<example xml:id="p1-c2-s5-example-1"><title> Finding a constant in a General Solution </title>

		<p>
			<statement>
				<p>
					Find the particular solution to the initial-value problem
					<me xml:id="p1-c2-s5-example-1-de"> 
						\frac{dy}{dx} = 2xy - 6x, \quad y(0) = 2
					</me>,
					given that the general solution is <m>\quad\ds y = ce^{x^2} + 3</m>.
				</p>
			</statement>
		</p>

		<p>
			<solution>
				<p>
					The initial condition <m>y(0) = 2</m> tells us that <m>y</m> must equal 2 when <m>x = 0</m>. Substituting into the general solution:
					<md>
						<mrow> y =  ce^{x^2} + 3 \quad \overset{y\ =\ 2,\ x\ =\ 0}{\Rightarrow} \quad	2	=\amp\  ce^{0^2} + 3	</mrow>
						<mrow>							 												2	=\amp\  c + 3		</mrow>
						<mrow>																			-1	=\amp\  c			</mrow>
					</md>
				</p>
				<p>
					Thus, the particular solution is:
					<me>
						y = -e^{x^2} + 3.
					</me>
				</p>
			</solution>
		</p>

	</example>

	<p>
		Here is one more example a particular solution from the general solution and initial conditions.
	</p>

	<example><title> General Sol. + Initial Values <m>\to</m> Particular Sol </title>
	
		<p>
			<statement>
				<p>
					Solve the initial value problem
					<me>
						y'' - y' - 12y = 0, \quad y(0) = 4, \quad y'(0) = -5
					</me>,
					given that the general solution is <m>\quad\ds y = c_1e^{-3t} + c_2e^{4t}</m>.
				</p>
			</statement>
		</p>

		<p>
			<solution>
				<p>
					If you are interested in the verification steps, see the solution below.
				</p>
			
				<solution><title>Verification as a solution</title>
					<p>
						First find <m>y, y', \text{ and } y''</m>:
						<md>
							<mrow> y	=\amp\ c_1e^{-3t} + c_2e^{4t}		</mrow>
							<mrow> y'	=\amp\ -3c_1e^{-3t} + 4c_2e^{4t}	</mrow>
							<mrow> y''	=\amp\ 9c_1e^{-3t} + 16c_2e^{4t}	</mrow>
						</md>
					</p>
				
					<p>
						and substitute these into <m>y'' - y' - 12y</m> and simplify:
						<md>
							<mrow>
								y'' - y' - 12y =\amp\ \left(9c_1e^{-3t} + 16c_2e^{4t}\right) 
							</mrow>
							<mrow>		
								\amp\ \hspace{1em} - \left( -3c_1e^{-3t} + 4c_2e^{4t} \right) -12\left( c_1e^{-3t} + c_2e^{4t} \right)
							</mrow>
							<mrow>
								=\amp\ \ul{\ul{9c_1e^{-3t}}} + \ul{16c_2e^{4t}} 
							</mrow>
							<mrow>
								\amp\ \hspace{1em} + \ul{\ul{3c_1e^{-3t}}} - \ul{4c_2e^{4t}} - \ul{\ul{12c_1e^{-3t}}} - \ul{12c_2e^{4t}}
							</mrow>
							<mrow>
								=\amp\ 0
							</mrow>
						</md>
						Which shows <m>0 = 0</m> and so <m>y(t) = c_1e^{-3t} + c_2e^{4t}</m> is a solution.
					</p>
				</solution>

				<p>
					We would like determine the spcific values of <m>c_1</m> and <m>c_2</m> that correspond to the initial conditions <m>y(0) = 4</m> and <m>y'(0) = -5</m>. 
				</p>

				<p>
					Now let's apply the initial conditions:
				</p>

				<p>
					<sidebyside>
						<p>
							<md>
								<mrow>	y(t) 	=\amp\ c_1e^{-3t} + c_2e^{4t}				</mrow>
								<mrow>		4	=\amp\ c_1e^{-3\cdot 0} + c_2e^{4\cdot 0}	</mrow>
								<mrow>		4	=\amp\ c_1 + c_2							</mrow>
							</md>
						</p>
						<p>
							<md>
								<mrow>	y'(t) 	=\amp\ -3c_1e^{-3t} + 4c_2e^{4t}			</mrow>
								<mrow>		-5	=\amp\ -3c_1e^{-3\cdot 0} + 4c_2e^{4\cdot 0}	</mrow>
								<mrow>		-5	=\amp\ -3c_1 + 4c_2							</mrow>
							</md>
						</p>
					</sidebyside>
				</p>
			
				<p>
					We now have two equations and two unknowns,
					<md>
						<mrow>	 c_1 +  c_2	=\amp\ 	4 	</mrow>
						<mrow> -3c_1 + 4c_2	=\amp\ -5 	</mrow>
					</md>
					There are multiple ways to solve this system of equations, and the reader is encouraged to verify that	<m>c_1 = 3</m> and <m>c_2 = 1</m>.
				</p>
			
				<p>
					Thus, the particular solution to this initial-value problem is
					<me>
						y = 3e^{-3t} + e^{4t}
					</me>.
				</p>
		
			</solution>
		</p>
	
	</example>

	<xi:include href="./chkpts-1-4-3-initial-conditions.ptx" />

	<p>
		In sum, specifying criteria for a desired solution is done with initial conditions. This reduces the ambiguity of the general solution by forcing its constants to assume values that lead to solutions consistent with these conditions.
	</p>


</subsection>