<reading-questions><title> Check your Understanding </title>
    
    <exercise><title> True/False </title>
        <statement correct="no">
        <p>
            The differential equation, <m>\displaystyle \frac{dy}{dx} - x(y^2 + y) = 0</m>, is in <xref ref="separable-form" text="custom">separable form</xref>.
        </p>
        </statement>
        <feedback>
            <p>
                This equation is not currently in <xref ref="separable-form" text="custom">separable form</xref>. However, it can be placed in separable form by moving the <m>x(y^2 + y)</m> term to the right-side of the equation.
            </p>
        </feedback>
    </exercise>
            
    <exercise><title> Fill-In </title>
        <introduction>
                Use algebra to show the differential equation is separable. Give the <m>x</m> terms in the left blank and the <m>y</m> terms in the right blank.
                <me> \frac{dy}{dx} - y\cos(x) = y.</me>
        </introduction>
            
        <webwork xml:id="ww_3">
            <description>
                Show that the DE is separable by typing in the separable form.
            </description>
    
            <pg-code>
                Context()->variables->add(y => 'Real');
                $f_x = Formula("1 + cos(x)");
                $g_y = Formula("y");
            </pg-code>
    
            <statement>
                <p>
                    <tabular halign="center">
                        <col width="10%"/>

                        <row><cell/> 
                            <cell><m>f(x)</m></cell><cell/> 
                            <cell><m>g(y)</m></cell><cell/>
                        </row>

                        <row>
                            <cell>
                                <m>\displaystyle \frac{dy}{dx} = \Large{(}</m>
                            </cell>
                            <cell>
                                <var name="$f_x" width="10" />
                            </cell>
                            <cell><m>\Large{)}\cdot\Large{(}</m></cell>
                            <cell>
                                <var name="$g_y" width="10" />
                            </cell>
                            <cell><m>\Large{)}</m></cell>
                        </row>
                    </tabular>
                </p>
            </statement>
    
            <solution>
                Move the <m> y\cos x </m> term to the right and factor out <m>y</m>.
                <md>
                <mrow> \frac{dy}{dx} - y\cos(x) = y \amp \implies \frac{dy}{dx} = y + y\cos(x) </mrow>
                <mrow>                              \amp \implies \frac{dy}{dx} = (1 + \cos(x))y </mrow>
                </md>
            </solution>
        </webwork>
    </exercise>

</reading-questions>