<subsection><title> Fundamentals - Additional Examples &amp; Notes </title>

	<example xml:id="de-two-solutions">

		<statement>
			<p>
				Verify if both <m>y= 2e^{-3t}</m> and <m>y= e^{4t}</m> are solutions to 
				<me>y'' - y' - 12y = 0</me>.
			</p>
		</statement>

		<solution>
			<p>
				Find <m>y'</m> and <m>y''</m> since they appear in the equation.
				<md>
					<mrow>	y	=\amp\  2e^{-3t}								</mrow>
					<mrow>	y' 	=\amp\  2e^{-3t}\left(-3\right)	=	-6e^{-3t}	</mrow>
					<mrow>	y'' =\amp\ -6e^{-3t}\left(-3\right)	=	18e^{-3t}	</mrow>
				</md>
			</p>

			<p>
				Plug <m>y, y',</m> and <m>y''</m> into the DE and simplify.
				<md>
					<mrow> 													y'' - y' - 12y	=\amp\ 0									</mrow>
					<mrow> 18e^{-3t} - \left( -6e^{-3t} \right) - 12\left( 2e^{-3t} \right)	=\amp\ 0									</mrow>
					<mrow> 								18e^{-3t} + 6e^{-3t} - 24e^{-3t}	=\amp\ 0									</mrow>
					<mrow> 																0	=\amp\ 0	\quad✅	</mrow>
				</md>
				Therefore, <m>y= 2e^{-3t}</m> is a solution to <m>y'' - y' - 12y = 0.</m>
			</p>
		
			<p>
				Find <m>y'</m> and <m>y''</m> since they appear in the DE.
				<md>
					<mrow>	y	=\amp\  e^{4t}								</mrow>
					<mrow>	y' 	=\amp\  e^{4t}\left(4\right)	=	4e^{4t}	</mrow>
					<mrow>	y'' =\amp\ 4e^{4t}\left(4\right)	=	16e^{4t}</mrow>
				</md>
			</p>

			<p>
				Plug <m>y, y',</m> and <m>y''</m> into the DE and simplify.
				<md>
					<mrow> 								y'' - y' - 12y	=\amp\ 0									</mrow>
					<mrow> 16e^{4t} - 4e^{4t} - 12\left( e^{4t} \right)	=\amp\ 0									</mrow>
					<mrow> 				16e^{4t} - 4e^{4t} - 12e^{4t}	=\amp\ 0									</mrow>
					<mrow> 											0	=\amp\ 0	\quad✅	</mrow>
				</md>
				Therefore, <m>y= e^{4t}</m> is a solution to <m>y'' - y' - 12y = 0.</m>
			</p>
		</solution>

	</example>

	<example>

		<statement>
			<p>
				Verify if <m>\ds\ y = 3\sin(x^2) </m> is a solution to 
				<me>y' - xy'' = 12x^2\sin(x^2)</me>.
			</p>
		</statement>

		<solution>
			<p>
				Find <m>y'</m> and <m>y''</m> since they appear in the equation and move all terms to the left-side.
				<md>
					<mrow>	y	=\amp\  3\sin(x^2)									</mrow>
					<mrow>	y' 	=\amp\  3\cos(x^2) \cdot 2x	=	6x\cos(x^2)	</mrow>
					<mrow>	y'' =\amp\ 6\cos(x^2) - 12x\sin(x^2)	=	6\cos(x^2) - 12x\sin(x^2)	</mrow>
				</md>
			</p>

			<p>
				Plug in <m>y, y',</m> and <m>y''</m> and simplify.
				<md>
					<mrow> 												
						y' - xy'' - 12x^2\sin(x^2) 	
							=\amp\ 0	
					</mrow>
					<mrow> 
						6x\cos(x^2) - x\left( 6\cos(x^2) - 12x\sin(x^2) \right) - 12x^2\sin(x^2)
							=\amp\ 0																
					</mrow>
					<mrow> 
						\cancel{6x\cos(x^2)} - \cancel{6x\cos(x^2)} - \cancel{12x^2\sin(x^2)} - \cancel{12x^2\sin(x^2)}	
							=\amp\ 0
						</mrow>
					<mrow> 
						0	=\amp\ 0
					</mrow>
				</md>
				Therefore, <m>y= 3\sin(x^2)</m> is a solution to <m>y' - 12x^2\sin(x^2) = xy''.</m>
			</p>
		</solution>

	</example>

	<example>
		<statement>
			<p>
				Identify the linear and nonlinear terms in the following differential equation.
				<me>
					e^{t}y^{(7)} + (t+1)y'y''' - t \ln y'' - y' \sin t - \tan y + \frac{4}{y} = \frac{3}{t}
				</me>
			</p>
		</statement>
		<solution>
			<p>
				To determine the linearity of a term we only need to consider the dependent variables (column <m>3</m> below). We are looking for a single <m>y</m> or derivative of <m>y</m> raised to the power of <m>1</m>. If we find such a term, we label it as linear. Otherwise, it is nonlinear. Let's separate the different parts in the following table.
			</p>

			<tabular>
				<col width="25%" halign="center" right="minor"/>
				<col width="25%" halign="center" right="minor"/>
				<col width="25%" halign="center" right="minor"/>
				<col width="25%" halign="center"/>
				<row bottom="minor">
					<cell>Term</cell>
					<cell>Coefficient</cell>
					<cell>Dependent Variables</cell>
					<cell>Linearity</cell>
				</row>
				<row>
					<cell><m>\ds e^{t}\ y^{(7)}</m></cell>
					<cell><m>\ds e^{t}</m></cell>
					<cell><m>\ds y^{(7)}</m></cell>
					<cell>linear</cell>
				</row>
				<row>
					<cell><m>\ds (t+1)y'y'''</m></cell>
					<cell><m>\ds (t+1)</m></cell>
					<cell><m>\ds y'y'''</m></cell>
					<cell>nonlinear</cell>
				</row>
				<row>
					<cell><m>\ds t \ln y''</m></cell>
					<cell><m>\ds t</m></cell>
					<cell><m>\ds \ln y</m></cell>
					<cell>nonlinear</cell>
				</row>
				<row>
					<cell><m>\ds y' \sin t</m></cell>
					<cell><m>\ds \sin t</m></cell>
					<cell><m>\ds y'</m></cell>
					<cell>linear</cell>
				</row>
				<row>
					<cell><m>\ds \tan y</m></cell>
					<cell><m>\ds 1</m></cell>
					<cell><m>\ds \tan y</m></cell>
					<cell>nonlinear</cell>
				</row>
				<row>
					<cell><m>\ds \frac{4}{y}</m></cell>
					<cell><m>\ds 4</m></cell>
					<cell><m>\ds \frac{1}{y}</m></cell>
					<cell>nonlinear</cell>
				</row>
				<row>
					<cell right="none"></cell>
					<cell right="none"></cell>
					<cell right="none"><m>\ds \uparrow</m></cell>
					<cell></cell>
				</row>
				<row>
					<cell right="none"></cell>
					<cell right="none"></cell>
					<cell right="none">
						<line>Linearity depends</line>
						<line>on this column only</line>
					</cell>
					<cell></cell>
				</row>
			</tabular>
			
			<p>
				Note, since constant terms do not contain a dependent variable, they are necessarily linear. So, in the context of differential equations, <m>\ds\frac{3}{t}</m> is also a linear term.
			</p>
		</solution>

	</example>

	<example>
		<title>Example: Classify Terms</title>
		<statement>
			<p>
				Consider the following differential equation:
				<me>
					e^{t}y^{(7)} + (t+1)y'y''' - t \ln y'' - y' \sin t - \tan y + \frac{4}{y} = \frac{3}{t}.
				</me>
				Let's determine the linearity of each term.
			</p>
		</statement>
		<solution>
			<p>
				To classify terms, focus on the dependent variable <m>y</m> and its derivatives. The table below summarizes the linearity of each term:
			</p>
			<tabular>
				<col width="25%" halign="center" />
				<col width="25%" halign="center" />
				<col width="25%" halign="center" />
				<col width="25%" halign="center" />
				<row>
					<cell>Term</cell>
					<cell>Coefficient</cell>
					<cell>Dependent Variable</cell>
					<cell>Linearity</cell>
				</row>
				<row>
					<cell><m>e^t y^{(7)}</m></cell>
					<cell><m>e^t</m></cell>
					<cell><m>y^{(7)}</m></cell>
					<cell>Linear</cell>
				</row>
				<row>
					<cell><m>(t+1)y'y'''</m></cell>
					<cell><m>(t+1)</m></cell>
					<cell><m>y'y'''</m></cell>
					<cell>Nonlinear</cell>
				</row>
				<row>
					<cell><m>t \ln y''</m></cell>
					<cell><m>t</m></cell>
					<cell><m>\ln y''</m></cell>
					<cell>Nonlinear</cell>
				</row>
				<row>
					<cell><m>y' \sin t</m></cell>
					<cell><m>\sin t</m></cell>
					<cell><m>y'</m></cell>
					<cell>Linear</cell>
				</row>
				<row>
					<cell><m>\tan y</m></cell>
					<cell><m>1</m></cell>
					<cell><m>\tan y</m></cell>
					<cell>Nonlinear</cell>
				</row>
				<row>
					<cell><m>\frac{4}{y}</m></cell>
					<cell><m>4</m></cell>
					<cell><m>\frac{1}{y}</m></cell>
					<cell>Nonlinear</cell>
				</row>
			</tabular>
			<p>
				Note that terms involving constant coefficients or independent variables, such as <m>\frac{3}{t}</m>, are linear because they do not involve the dependent variable <m>y</m> or its derivatives.
			</p>
		</solution>
	</example>

	<note><title> <em>Don't assume a function that satisfies a DE is a general solution!</em> </title>
		<p>
			A function that contains constants and satisfies a differential equation <em>does not mean it is the general solution</em> since it could be missing a term. For example, you could easily show that <m>y = \frac{1}{2}x^2 + c_1 x</m> is a solution to 
			<me>\quad y'' = 1</me>, 
			but you already know from <xref ref="two-constant-solution-verification"/> that <m>y = \frac{1}{2}x^2 + c_1 x + c_2</m> is a solution, which is more general than <m>y = \frac{1}{2}x^2 + c_1 x</m>.
		</p>
	</note>

	<assemblage xml:id="identifying-nonlinear-terms"><title> Identifying Nonlinear Terms </title>
		<p>
			A term is nonlinear if it contains a dependent variable, <m>y</m> or <m>y^{(n)}</m>, that is
		</p>
		<p>
			<ul marker="square">
				<li>
					<p>
						Raised to a power other than 1, e.g., <m>y^2</m> or <m>(y')^{-4}</m>.
					</p>
				</li>
				<li>
					<p>
						Inside another function, e.g., <m>\ln(y)</m> or <m>\sin(y)</m>.
					</p>
				</li>
				<li>
					<p>
						Multiplied or divided by another <m>y</m> or <m>y^{(n)}</m>, e.g., <m>y y'''</m> or <m>\ds\frac{y'}{y}</m>.
					</p>
				</li>
			</ul>
		</p>
	</assemblage>

</subsection>