<subsection><title> Solutions to Differential Equations </title>

	<example xml:id="de-two-solutions">

		<statement>
			<p>
				Verify if both <m>y= 2e^{-3t}</m> and <m>y= e^{4t}</m> are solutions to 
				<me>y'' - y' - 12y = 0</me>.
			</p>
		</statement>

		<solution>
			<p>
				Find <m>y'</m> and <m>y''</m> since they appear in the equation.
				<md>
					<mrow>	y	=\amp\  2e^{-3t}								</mrow>
					<mrow>	y' 	=\amp\  2e^{-3t}\left(-3\right)	=	-6e^{-3t}	</mrow>
					<mrow>	y'' =\amp\ -6e^{-3t}\left(-3\right)	=	18e^{-3t}	</mrow>
				</md>
			</p>

			<p>
				Plug <m>y, y',</m> and <m>y''</m> into the DE and simplify.
				<md>
					<mrow> 													y'' - y' - 12y	=\amp\ 0									</mrow>
					<mrow> 18e^{-3t} - \left( -6e^{-3t} \right) - 12\left( 2e^{-3t} \right)	=\amp\ 0									</mrow>
					<mrow> 								18e^{-3t} + 6e^{-3t} - 24e^{-3t}	=\amp\ 0									</mrow>
					<mrow> 																0	=\amp\ 0	\quad✅	</mrow>
				</md>
				Therefore, <m>y= 2e^{-3t}</m> is a solution to <m>y'' - y' - 12y = 0.</m>
			</p>
		
			<p>
				Find <m>y'</m> and <m>y''</m> since they appear in the DE.
				<md>
					<mrow>	y	=\amp\  e^{4t}								</mrow>
					<mrow>	y' 	=\amp\  e^{4t}\left(4\right)	=	4e^{4t}	</mrow>
					<mrow>	y'' =\amp\ 4e^{4t}\left(4\right)	=	16e^{4t}</mrow>
				</md>
			</p>

			<p>
				Plug <m>y, y',</m> and <m>y''</m> into the DE and simplify.
				<md>
					<mrow> 								y'' - y' - 12y	=\amp\ 0									</mrow>
					<mrow> 16e^{4t} - 4e^{4t} - 12\left( e^{4t} \right)	=\amp\ 0									</mrow>
					<mrow> 				16e^{4t} - 4e^{4t} - 12e^{4t}	=\amp\ 0									</mrow>
					<mrow> 											0	=\amp\ 0	\quad✅	</mrow>
				</md>
				Therefore, <m>y= e^{4t}</m> is a solution to <m>y'' - y' - 12y = 0.</m>
			</p>
		</solution>

	</example>

	<example>

		<statement>
			<p>
				Verify if <m>\ds\ y = 3\sin(x^2) </m> is a solution to 
				<me>y' - xy'' = 12x^2\sin(x^2)</me>.
			</p>
		</statement>

		<solution>
			<p>
				Find <m>y'</m> and <m>y''</m> since they appear in the equation and move all terms to the left-side.
				<md>
					<mrow>	y	=\amp\  3\sin(x^2)									</mrow>
					<mrow>	y' 	=\amp\  3\cos(x^2) \cdot 2x	=	6x\cos(x^2)	</mrow>
					<mrow>	y'' =\amp\ 6\cos(x^2) - 12x\sin(x^2)	=	6\cos(x^2) - 12x\sin(x^2)	</mrow>
				</md>
			</p>

			<p>
				Plug in <m>y, y',</m> and <m>y''</m> and simplify.
				<md>
					<mrow> 												
						y' - xy'' - 12x^2\sin(x^2) 	
							=\amp\ 0	
					</mrow>
					<mrow> 
						6x\cos(x^2) - x\left( 6\cos(x^2) - 12x\sin(x^2) \right) - 12x^2\sin(x^2)
							=\amp\ 0																
					</mrow>
					<mrow> 
						\cancel{6x\cos(x^2)} - \cancel{6x\cos(x^2)} - \cancel{12x^2\sin(x^2)} - \cancel{12x^2\sin(x^2)}	
							=\amp\ 0
						</mrow>
					<mrow> 
						0	=\amp\ 0
					</mrow>
				</md>
				Therefore, <m>y= 3\sin(x^2)</m> is a solution to <m>y' - 12x^2\sin(x^2) = xy''.</m>
			</p>
		</solution>

	</example>

	<!-- <note><title> <em>Don't assume a function that satisfies a DE is a general solution!</em> </title>
		<p>
			A function that contains constants and satisfies a differential equation <em>does not mean it is the general solution</em> since it could be missing a term. For example, you could easily show that <m>y = \frac{1}{2}x^2 + c_1 x</m> is a solution to 
			<me>\quad y'' = 1</me>, 
			but you already know from <xref ref="two-constant-solution-verification"/> that <m>y = \frac{1}{2}x^2 + c_1 x + c_2</m> is a solution, which is more general than <m>y = \frac{1}{2}x^2 + c_1 x</m>.
		</p>
	</note> -->

</subsection>