<subsection><title> Fundamentals - Additional Examples &amp; Notes </title>

	<example xml:id="antiderivative-example">
	
		<statement>
			<p>
				Solve the initial-value problem 
				<me>2y' - 4\sin x = 2, \quad y(0) = 5 </me>.
			</p>
		</statement>
			
		<solution>

			<p>
				Start by isolating the derivative, <m>y'</m>, on one side of the equation
				<md>
					<mrow> y' \amp = 1 + 2 \sin x </mrow>.
				</md>
				Integrate both sides with respect to <m>x</m> to leave us with <m>y</m> on the left side
				<md>
					<mrow> \int y'\ dx 	\amp = \int \left(1 + 2 \sin x\right) \ dx 				</mrow>
					<mrow> 	y + c_1 	\amp = x - 2 \cos x + c_2 								</mrow>
					<mrow> 			y 	\amp = x - 2 \cos x + \boxed{c_2 - c_1}\leftarrow c		</mrow>
					<mrow> 		y(x)	\amp  = x - 2 \cos x + c 								</mrow>.
				</md>
			</p>

			<p>
				Finally, apply the initial condition <m>y(0) = 5</m> to find <m>c</m>
				<md>
					<mrow> 				y(0)	\amp = 5 </mrow>
					<mrow> (0) - 2 \cos(0) + c	\amp = 5 </mrow>
					<mrow> 			0 - 2 + c	\amp = 5 </mrow>
					<mrow> 					c	\amp = 7 </mrow>.
				</md>
				Thus, the solution to the differential equation is <m>\quad y = x - 2 \cos x + 7 </m>.
			</p>

		</solution>

	</example>

	<example xml:id="show-separable-example">
	
		<statement>
			<p>
				Show the differential equations are separable.
				<me> 
					y^2\frac{d^2y}{dx^2} = x, \qquad 
					t - ss' = - s, \qquad 
					y\frac{dy}{dx} + 8x^2e^{x + \cos y} = 6x^2e^x
				</me>.
			</p>
		</statement>
		
		<solution><title> <term>Attention to Detail</term> </title>
			<p>
				This is a bit of a trick question to remind you of the first-order requirement of a separable equation. Since this equation is second-order, <em>separability does not apply</em>.
			</p>
		</solution>

		<solution><title> <term>Isolate the Derivative First</term> </title>
			<p>
				To see that this equation is separable, we need to check that it can be rearranged in <xref ref="separable-form" text="custom">separable form</xref>. Isolating <m> s' </m> we get
				<me> s' = \frac{s + t}{s} </me>
				and it should be clear that there is no way to separate <m>t</m> and <m>s</m> by <em>multiplication</em> in the numerator, so this equation <em>is not separable</em>.
			</p>
		</solution>

		<solution><title> <term>Everything but the Kitchen Sink</term> </title>

			<p>
				This example uses a little of everything we discussed, so strap in. 
			</p>

			<p>
				Noticing that the equation is first-order, we start by isolating <m>dy/dx</m>
				<md>
					<mrow>
						y\frac{dy}{dx} + 8x^2e^{x + \cos y} = 6x^2e^x 
					</mrow>
					<mrow>
						\frac{dy}{dx} = \frac{6x^2e^x - 8x^2e^{x + \cos y}}{y}
					</mrow>
				</md>
			</p>

			<p>
				Next, we can rewrite the exponent in the numerator as a product
				<me>
					\frac{dy}{dx} = \frac{6x^2e^x - 8x^2e^{x}e^{\cos y}}{y}
				</me>
				and recognize that there is a common factor in the numerator
				<me>
					\frac{dy}{dx} = \frac{2x^2e^x(3 - 4e^{\cos y})}{y}
				</me>.
			</p>

			<p>
				From here, we write the result as a product of fractions,
				<me>
					\frac{dy}{dx} = \frac{2x^2e^x}{1} \cdot \frac{3 - 4e^{\cos y}}{y} 
				</me>,
				and see that the equation is now <em>separable</em>.
			</p>

		</solution>
	
	</example>

	<exercise label="chkpt-separable-form-showing-forms-5"><title> <em>Work-it-Out</em> </title>

		<introduction>
			<p>
				Write the differential equation,
				<me> 
					\frac{dy}{dx} - y\cos(x) = y
				</me>,
				in <xref ref="separable-form" text="custom">separable form</xref> by identifying <m>f(x)</m> and <m>g(y)</m>.
			</p>
		</introduction>
			
		<webwork xml:id="p2-c2-s1-i4-ww">
			<description>
				Show that the DE is separable by giving the separable form.
			</description>
	
			<pg-code>
				Context()->variables->add(y => 'Real');
				$fx = Formula("1 + cos(x)");
				$gy = Formula("y");
			</pg-code>
	
			<statement>

				<p>
					<tabular halign="center">
					
						<row>
							<cell><m>\displaystyle \frac{dy}{dx} = \Big( </m></cell>
							<cell><var name="$fx" width="10" /></cell>
							<cell><m>\Big) \cdot \Big( </m></cell>
							<cell><var name="$gy" width="10" /></cell>
							<cell><m>\Big)</m></cell>
						</row>
						<row>
							<cell/>
							<cell><m>f(x)</m></cell>
							<cell/>
							<cell><m>g(y)</m></cell>
							<cell/>
						</row>

					</tabular>
				
				</p>

			</statement>

			<solution><title> Solution </title>
				<p>
					Move the <m> y\cos x </m> term to the right and factor out <m>y</m>.
					<md>
						<mrow> \frac{dy}{dx} - y\cos(x) = y \amp \implies \frac{dy}{dx} = y + y\cos(x) </mrow>
						<mrow>							  \amp \implies \frac{dy}{dx} = (1 + \cos(x))y </mrow>
					</md>
				</p>
			</solution>
			
		</webwork>

	</exercise>

	<exercise label="chkpt-separable-form-showing-forms-6"><title> <em>Work-it-Out</em> </title>
		
		<introduction>
			<p>
				Write the differential equation,
				<me>
					tP\frac{dP}{dt} = e^tP^2 - e^t
				</me>,
				in <xref ref="separable-form" text="custom">separable form</xref> by identifying <m>f(t)</m> and <m>g(P)</m>.
			</p><p/>
		</introduction>
		
		<webwork xml:id="p2-c2-s1-i5-ww">
			<description>
				Show that the DE is separable by giving the separable form.
			</description>
	
			<pg-code>
				Context()->variables->add(t => 'Real');
				Context()->variables->add(P => 'Real');
				$ft = Formula("e^(t)/t");
				$gP = Formula("(P^2 - 1)/P");
			</pg-code>
	
			<statement>

				<p>
					<tabular halign="center">
					
						<row>
							<cell><m>\quad\ds \frac{dP}{dt} = \Big( </m></cell>
							<cell><var name="$ft" width="5" /></cell>
							<cell><m>\Big) \cdot \Big( </m></cell>
							<cell><var name="$gP" width="5" /></cell>
							<cell><m>\Big)</m></cell>
						</row>
						<row>
							<cell/>
							<cell><m>f(t)</m></cell>
							<cell/>
							<cell><m>g(P)</m></cell>
							<cell/>
						</row>

					</tabular>
				
				</p>

			</statement>

			<!-- <hint>
				Isolate the derivative, factor out <m>e^t</m>, and split the fraction.
			</hint> -->
	
			<solution><title> Solution </title>
				<p>
					We isolate the derivative and group the terms as shown below. Notice how we separated the product of two fractions <m>\left(\frac{AB}{CD} = \frac{A}{C}\cdot \frac{B}{D}\right)</m>.
					<me>
						tP\frac{dP}{dt}
							= e^tP^2 - e^t 
							= \frac{e^t \cdot (P^2 - 1)}{t \cdot P} 
							= \frac{e^t}{t} \cdot \frac{P^2 - 1}{P} 
							= \underset{f(t)}{\boxed{\frac{e^t}{t}}}\underset{g(P)}{\left(\boxed{\frac{P^2 - 1}{P}}\right)}
					</me>.
				</p>
			</solution>
			
		</webwork>
		
	</exercise>


</subsection>