<subsection xml:id="r-01-14" xmlns:xi="http://www.w3.org/2001/XInclude">
<title>Completing the Square</title>

<p>
Completing the square will be necessary when finding the inverse Laplace transform 
of some rational functions. Recall that we use completing the square when we have 
a quadratic expression that isn't a perfect square, but we'd like to add the right 
number to it to make it a perfect square. We will also need to subtract the same 
number to compensate for what we added (so that we are effectively adding zero and 
not changing the value of the expression). Here's an example.
</p>

<example xml:id="ex_complete_square_01">
<title>Complete the square for <m>x^2 - 18x - 10</m></title>

    <p>
    If you prefer to see a video of this example, 
    <xref ref="video-complete_square_01" text="custom"> click here </xref>
    </p>
    
	<p>
	<md>
		<mrow>x^2 - 18x - 10	\amp= (x^2 - 18x) - 10							</mrow>
		<mrow>					\amp= (x^2 - 18x + 81) - 81 - 10				</mrow>
		<mrow>					\amp= (x^2 - 18x + 81) - 81 - 10				</mrow>
		<mrow>					\amp=(x - 9)^2 - 91								</mrow>
	</md>
	</p>
</example>

<p>
There are a lot of details left out here. If you need a more complete refresher on 
how to complete the square, there is a primer (with examples, and some practice
problems--answers included) available in CANVAS.
</p>

<p>
<term> Complete the square for each of the following expressions. Verify by expanding 
your expression.</term>

<ol>
	<li> <m>x^2 + 8x + 28 \qquad</m>		
	<solution>		
	<md>
		<mrow>x^2 + 8x + 28	\amp= (x^2 + 8x + 16) - 16 + 28						</mrow>
		<mrow>				\amp= (x+4)^2 - 16+28								</mrow>
		<mrow>				\amp= (x+4)^2 + 12									</mrow>
	</md>
	</solution>
	<answer>
		<m> (x+4)^2 + 12 </m>
	</answer>
	</li>

	<li> <m>x^2 - 12x \qquad</m>		
	<solution>		
	<md>
		<mrow>x^2 - 12x	\amp= (x^2 - 12x + 36) - 36								</mrow>
		<mrow>			\amp= (x-6)^2 - 36										</mrow>
	</md>
	</solution>
	<answer>
		<m> (x-6)^2 - 36 </m>
	</answer>
	</li>

	<li> <m>2x^2 - 8x - 7 \qquad</m>		
	<solution>		
	<md>
		<mrow>2x^2 - 8x - 7	\amp= (2x^2 - 8x) - 7								</mrow>
		<mrow>				\amp= 2(x^2 - 4x) - 7								</mrow>
		<mrow>				\amp= 2(x^2 - 4x + 4 - 4) - 7						</mrow>
		<mrow>				\amp= 2(x^2 - 4x + 4) - 8 - 7						</mrow>
		<mrow>				\amp= 2(x-2)^2 - 8 - 7								</mrow>
		<mrow>				\amp= 2(x-2)^2 - 15									</mrow>
	</md>
	</solution>
	<answer>
		<m> 2(x-2)^2 - 15 </m>
	</answer>
	</li>
	
	<li> <m>4x^2  + 8x - 65 \qquad</m>
	<solution>	(Needs to be written)	
	<md>
		<mrow>		\amp= 														</mrow>
		<mrow>		\amp= 														</mrow>
		<mrow>		\amp= 														</mrow>
	</md>
	</solution>
	<answer>
		<m> 	 </m>
	</answer>
	</li>
	
	<li> <m>-2x^2 + 20x -47 \qquad</m>
	<solution>	(Needs to be written)	
	<md>
		<mrow>		\amp= 														</mrow>
		<mrow>		\amp= 														</mrow>
		<mrow>		\amp= 														</mrow>
	</md>
	</solution>
	<answer>
		<m> 	 </m>
	</answer>
	</li>
	
	<li> <m>-x^2 - 16x - 57 \qquad</m>		
	<solution>		
	<md>
		<mrow>-x^2 - 16x - 57	\amp= -(x^2 +16x) - 57							</mrow>
		<mrow>					\amp= -(x^2 +16x + 64 - 64) - 57				</mrow>
		<mrow>					\amp= -(x^2 + 16x + 64) + 64 -57				</mrow>
		<mrow>					\amp= -(x+8)^2 + 64 - 57						</mrow>
		<mrow>					\amp= -(x+8)^2 + 7								</mrow>
	</md>		
	</solution>
	<answer>
		<m> -(x+8)^2 + 7 </m>
	</answer>
	</li>
</ol>
</p>
</subsection>