<subsection xml:id="r-01-20" xmlns:xi="http://www.w3.org/2001/XInclude">

<title>Recursive functions</title>

{


<p>
We often use subscript notation when the function is a <em> recursive function,</em> where we rely on knowing
previous values in order to compute the next value, as in the example below.  

	<p>
    If you prefer to see a video of this example, 
    <xref ref="video-recursive_functions_01" text="custom"> click here </xref>
    </p>
    
	\begin{quote}
	<em> Example:</em>  Suppose <m>a_{n+1} = 3a_{n} + 2</m> and <m>a_0 = 3.</m>
	
	<ol>
	
		<li>
[(a)] Find the value of <m>a_1.</m>
	<answer>\it Answer:}
	
	One way to read this definition is:  ``To get the next value of <m>a</m>--the value at <m>n+1,</m> we take 3 times the
	previous value of <m>a</m>--the value at <m>n</m>--and then add two.
	
	In this example, we know the value of <m>a</m> at <m>n=0,</m> because we are given that <m>a_0 = 3.</m>  Then we can
	find the next value of <m>a</m>--the value at <m>n = 1</m>--as follows:
	<md>
		<mrow>a_1	\amp= 3a_0 + 2</mrow>
		<mrow>\amp= 3\cdot 3 + 2</mrow>
		<mrow>\amp= 11.</mrow>
	</md>
			</answer>
		</li>

		<li>
[(b)]  Find the value of <m>a_4.</m>

	<em> Answer:</em>
		
	If we use the formula above, with <m>n = 3,</m> then we have
		<me> a_{4} = 3a_{3} + 2. </me>
	It looks like we actually need to know the value of <m>a_3</m>...and it turns out that in order to know the value of 
	<m>a_3</m> we actually need to know the value of <m>a_2</m>...which requires that we know the value of <m>a_1</m>--which
	we already found.  So here goes:
	<md>
		<mrow>a_2	\amp= 3a_1 + 2</mrow>
		<mrow>\amp= 3\cdot 11 + 2</mrow>
		<mrow>\amp= 35</mrow>
		<mrow>\amp</mrow>
		<mrow>a_3	\amp= 3a_2 + 2</mrow>
		<mrow>\amp= 3\cdot 35 + 2</mrow>
		<mrow>\amp= 107</mrow>
		<mrow>\amp</mrow>
		<mrow>a_4	\amp= 3a_3 + 2</mrow>
		<mrow>\amp= 3\cdot 107 + 2</mrow>
		<mrow>\amp= 323.</mrow>
	</md>
		</li>
</ol>
		
	The bottom line with recursive functions is that if we know <m>a_0,</m> we can find <m>a_1,</m> and then we can 
	find <m>a_2,</m> and so on.
	But if we want to know <m>a_{17},</m> for example, we need to know ALL of the previous <m>a</m>-values 
	<m>a_0, a_1, a_2, \ldots , a_{16}</m>.
	<answer>\it Side note:  You may recall some of this from studying sequences and series in calculus.  In calculus we 
	sometimes looked for a pattern so we could avoid having to compute all previous values.  That's a great skill,
	and it might even work for the examples below, but we won't generally be able to do that in differential equations.}
	\end{quote}
			</answer>
</p>

<p>
Now you try: 

</p>

<p>
<em> Given the definition of a recursive function in subscript notation, find the value of the given 
		term.</em>
<ol>
	
		<li>
  If <m>a_{n+1} = a_n - 2</m> and <m>a_0 = 16,</m> evaluate <m>a_3.</m> 		
	<solution>		
	<md>
		<mrow>n = 0:  	a_1	\amp= a_0 - 2</mrow>
		<mrow>\amp= 16 - 2</mrow>
		<mrow>\amp= 14</mrow>
		<mrow>\amp</mrow>
		<mrow>n = 1:  	a_2	\amp= a_1 - 2</mrow>
		<mrow>\amp= 14 - 2</mrow>
		<mrow>\amp= 12</mrow>
		<mrow>\amp</mrow>
		<mrow>n = 2:  	a_3	\amp= a_2 - 2</mrow>
		<mrow>\amp= 12 - 2</mrow>
		<mrow>\amp= 10</mrow>
	</md>
		
		
	</solution>
	<answer>
		<me> a_3 = 10 </me>
		 
	</answer>
	
	
	
		</li>
	
		<li>
  If <m>y_{n+1} = \sin(y_n)</m> and <m>y_0 = 0,</m> evaluate <m>y_4.</m>  		
	<solution>		
	<md>
		<mrow>n = 0:  	y_1	\amp= \sin(y_0)</mrow>
		<mrow>\amp= \sin(0)</mrow>
		<mrow>\amp= 0</mrow>
		<mrow>\amp</mrow>
		<mrow>n = 1:  	y_2	\amp= \sin(y_1)</mrow>
		<mrow>\amp= \sin(0)</mrow>
		<mrow>\amp= 0</mrow>
		<mrow>\amp</mrow>
		<mrow>n = 2:  	y_3	\amp= \sin(y_2)</mrow>
		<mrow>\amp= \sin(0)</mrow>
		<mrow>\amp= 0</mrow>
		<mrow>\amp</mrow>
		<mrow>n = 3:  	y_4	\amp= \sin(y_3)</mrow>
		<mrow>\amp= \sin(0)</mrow>
		<mrow>\amp= 0</mrow>
	</md>
		
	</solution>
	<answer>
		<me> y_4 = 0 </me>
		 
	</answer>
	
	
	
		</li>
	
		<li>
  If <m>x_{n+1} = x_n^2 - x_n</m> and <m>x_0 = 5,</m> evaluate <m>x_2.</m> 		
	<solution>		
	<md>
		<mrow>n = 0:  	x_1	\amp= x_0^2 - x_0</mrow>
		<mrow>\amp= 5^2 - 5</mrow>
		<mrow>\amp= 20</mrow>
		<mrow>\amp</mrow>
		<mrow>n = 1:  	x_2	\amp= x_1^2 - x_1</mrow>
		<mrow>\amp= 20^2 - 20</mrow>
		<mrow>\amp= 380</mrow>
	</md>
		
	</solution>
	<answer>
		<me> x_2 = 380 </me>
		 
	</answer>
	
	</li>
</ol>
</p>
</subsection>