<section label="common-transforms">
	<title> Common Transforms </title>
	
	<introduction>
		<p>
			Now that we've defined the Laplace transform, the next step is to build a basic toolkit of common transforms. These are formulas for frequently encountered functions like constants, exponentials, powers of <m>t</m>, and trigonometric functions. Learning these transforms will allow you to compute Laplace transforms quickly, without evaluating integrals from scratch each time.
		</p>

		<p>
			We'll derive these formulas using straightforward examples and then generalize the results. You'll see how the Laplace transform simplifies when applied to each type of function and how certain patterns repeat across different cases.
		</p>

		<lemma><title> Exponential Functions </title>

			<p>
				<task label="prep-common-transforms-1"><title> Exponential Integration Rules </title>
					<statement>
						<p>
							Match each exponential integrand with its antiderivative. Assume <m>K</m> is a constant.
						</p>
					</statement>
					<cardsort>
						<match>
							<premise><m>\ds \int e^{5t} dt</m></premise>
							<response><m>\ds \frac{1}{5} e^{5t} + C</m></response>
						</match>
						<match>
							<premise><m>\ds \int e^{-3t} dt</m></premise>
							<response><m>\ds \frac{-1}{3} e^{-3t} + C</m></response>
						</match>
						<match>
							<premise><m>\ds \int e^{Kt} dt</m></premise>
							<response><m>\ds \frac{1}{K} e^{Kt} + C</m></response>
						</match>
						<match>
							<premise><m>\ds \int e^{(7-s)t} dt</m></premise>
							<response><m>\ds \frac{1}{7 - s} e^{(7-s)t} + C</m></response>
						</match>
					</cardsort>
				</task>
		
				<task label="prep-common-transforms-2"><title> How is <m>s</m> Treated During Integration? </title>
					<statement>
						<p>
							In the Laplace transform integral, the variable <m>s</m> is treated as a <fillin characters="10" /> during the integration process.
						</p>
					</statement>
					<choices randomize="yes">
						<choice correct="yes">
							<statement>constant</statement>
							<feedback>
								<p>
									Correct! When evaluating the integral, <m>s</m> is treated as a constant, since the integration is with respect to <m>t</m>.
								</p>
							</feedback>
						</choice>
						<choice>
							<statement>variable</statement>
							<feedback>
								<p>
									No, even though <m>s</m> is a variable overall, it is treated as a constant during the integration.
								</p>
							</feedback>
						</choice>
						<choice>
							<statement>coefficient</statement>
							<feedback>
								<p>
									No, while <m>s</m> acts like a coefficient in <m>e^{-st}</m>, it's conceptually treated as a constant in the integration.
								</p>
							</feedback>
						</choice>
						<choice>
							<statement>limit</statement>
							<feedback>
								<p>
									No, <m>s</m> is not a limit of integration, it appears inside the integrand.
								</p>
							</feedback>
						</choice>
					</choices>
				</task>
		
				<task label="prep-common-transforms-3"><title> Choosing <m>u</m> and <m>dv</m> in <m>\int t^2 e^{-st} dt</m> </title>
					<statement>
						<p>
							Which functions should you choose as <m>u</m> and <m>dv</m> when applying integration by parts to <m>\int t^2 e^{-st} dt</m>?
						</p>
					</statement>
					<choices randomize="yes">
						<choice correct="yes">
							<statement><m>u = t^2,\quad dv = e^{-st} dt</m></statement>
							<feedback>
								<p>Correct! This choice simplifies with each integration by parts.</p>
							</feedback>
						</choice>
						<choice>
							<statement><m>u = e^{-st},\quad dv = t^2 dt</m></statement>
							<feedback>
								<p>No, this makes integration more difficult. We want to differentiate <m>t^2</m> and integrate the exponential.</p>
							</feedback>
						</choice>
						<choice>
							<statement><m>u = st,\quad dv = t dt</m></statement>
							<feedback>
								<p>These choices are not aligned with the integrand <m>t^2 e^{-st}</m>.</p>
							</feedback>
						</choice>
					</choices>
				</task>
		
			</p>
		
		</lemma>
	</introduction>

	<subsection label="constant-function-transform">
		<title> Laplace Transform of a Constant </title>

		<p>
			We begin with the simplest case: the constant function <m>f(t) = 1</m>. By the definition of the Laplace transform,
			<me>
				\lap{1} = \int_0^\infty e^{-st}\, dt.
			</me>
		</p>
		<p>
			This integral converges when <m>s \lt 0</m> and evaluates to
			<me xml:id="lt-L1">
				\text{L}_1:\quad\lap{1} = \frac{1}{s}, \quad s \gt 0
			</me>.
		</p>
		<p>
			The details for this transform mirror the <xref ref="laplace-transform-of-5" text="custom">solution for <m>\lap{5}</m></xref> in the previous section. 
		</p>
	</subsection>

	<subsection label="exponential-function-transform">
		<title> Laplace Transform of Exponentials </title>

		<p>
			To get the transform formula for exponentials of the form <m>f(t) = e^{at}</m>, where <m>a</m> is a constant, we will first find it for <m>e^{7t}</m>:
		</p>

		<proof label="common-exp-7t-details">
			<title> <me>\lap{e^{7t}} = \frac{1}{s - 7}, \quad s \gt 7</me>Click here for details </title>
			<p>
				Using the definition of the Laplace transform we get
				<me>
					\lap{ e^{7t} }
					= \int_0^{\infty} e^{-st} \cdot e^{7t}\ dt
					= \lim_{b \to \infty}\int_0^b e^{(7-s)t}\ dt
				</me>.
			</p>

			<p>
				Focusing just on the integral and treating <m>7-s</m> as constant, we let <m>u=7-s</m> and apply <m>u</m>-substitution:
				<md>
					<mrow>
						\int_0^b e^{(7-s)t}\, dt
						<xref text="custom" ref="lt-example-2-details"><m>\os{\large ‚ùî}{=}</m></xref> 
						\frac{1}{7-s} e^{(7-s)t} \Bigg|_0^b
						\amp = \frac{1}{7-s} \left( e^{(7-s)b} - e^{0} \right)
					</mrow>
					<mrow>
						\amp = \frac{1}{7-s} \left( e^{(7-s)b} - 1 \right)
					</mrow>
				</md>
			</p>

			<p>
				Now, we compute the limit of this expression as <m>b \to \infty</m>:
				<md>
					<mrow>
						\lim_{b \to \infty} \frac{1}{7-s} \left( e^{(7-s)b} - 1 \right)
						\amp = \frac{1}{7-s} \Bigg[ \ub{\lim_{b \to \infty} e^{(7-s)b}}_{L} - \lim_{b \to \infty} 1 \Bigg]
					</mrow>
				</md>.
			</p>

			<p>
				As before, <m>L</m> goes to <m>0</m> if the <term><xref ref="graph-of-exp-t" text="custom">power of the exponential function</xref></term> goes to <m>-\infty</m>. This only happens if <m>7-s</m> is negative. That is, <m>\ 7-s \lt 0\ </m> or <m>\ 7 \lt s</m>. 
			</p>

			<p>
				So, as long as <m>s \gt 7</m>, then <m>L \to 0</m> and the transform becomes 
				<me>
					\lap{e^{7t}} = \frac{1}{s - 7}, \quad s \gt 7
				</me>.
			</p>
		</proof>

		<p>
			Replacing <m>7</m> with an <m>a</m> in this solution leads to the general formula:
			<me xml:id="lt-L2">
				\text{L}_2:\quad\lap{e^{at}} = \frac{1}{s - a}, \quad s \gt a
			</me>,
			where <m>a</m> is a constant.
		</p>

		<task label="chkpt-71">
			<title> üìñ‚ùì Give the Transform </title>
			<statement>
				<me>\lap{e^{-3t}} = <fillin characters="2"/> </me>
			</statement>
			<choices randomize="yes">
				<choice correct="yes">
					<statement><m>\ds\frac{1}{s+3}</m></statement>
					<feedback>
						<p>
							Correct! The Laplace transform of <m>e^{-3t}</m> is <m>\ds\frac{1}{s+3}</m>.
						</p>
					</feedback>
				</choice>
				<choice>
					<statement><m>\ds\frac{1}{s-3}</m></statement>
					<feedback>
						<p>
							No, this would be the transform of <m>e^{3t}</m>. Double-check the sign of the exponent.
						</p>
					</feedback>
				</choice>
				<choice>
					<statement><m>\ds\frac{1}{s-3t}</m></statement>
					<feedback>
						<p>
							No, <m>t</m> should not appear in the final expression, only <m>s</m>.
						</p>
					</feedback>
				</choice>
				<choice>
					<statement><m>\ds\frac{3}{s+3}</m></statement>
					<feedback>
						<p>
							No, the numerator should be 1, not 3. This is not a scaled exponential.
						</p>
					</feedback>
				</choice>
			</choices>
		</task>
	</subsection>

	<subsection label="power-function-transform">
		<title> Laplace Transform of Powers of <m>t</m> </title>

		<p>
			Now let's consider power functions, <m>f(t) = t^n</m> where <m>n</m> is a non-negative integer.
			<me>
				\lap{t^n} = \frac{n!}{s^{n+1}}, \quad s > 0.
			</me>
		</p>
		<p>
			We already found the transforms for <m>n = 0</m> and <m>n = 1</m> since
			<ul>
				<li><m>n=0:\qquad\lap{t^0} = \lap{1} = \dfrac{1}{s}</m></li>
				<li><m>n=1:\qquad\lap{t^1} = \lap{t} = \dfrac{1}{s^2}</m></li>
			</ul>
			We could find <m>\lap{t^2}</m> next, but it is more instructive to show following relationship:
		</p>

		<proof label="common-t-sqrd-details">
			<title> <me>\lap{t^2} = \frac{2}{s}\cdot \lap{t}, \quad s \gt 0</me>Click here for details </title>
			<p>
				Applying the definition and writing the integral as a limit, we have
				<me>
					\lap{ t^2 } = \lim_{b \to \infty} \ub{\int_0^b e^{-st} \cdot t^2\ dt}_{I}
				</me>.
			</p>

			<p>
				Applying integration by parts to <m>I</m> once in <m>\lap{ t^2 }</m> shows
				<md>
					<mrow>
						\lap{ t^2 }
						\amp = \lim_{b \to \infty} \left[-\frac{b^2}{s}e^{-sb} + \frac{2}{s}\int_0^b e^{-st}\cdot t\ dt\right]
						<xref ref="lt-example-tsqrd-IVP-details" text="custom">üîçHow?</xref>
					</mrow>
					<mrow>
						\amp = -\frac{1}{s} \lim_{b \to \infty} \left[-\frac{b^2}{e^{sb}}\right] + \frac{2}{s}\lim_{b \to \infty}\int_0^b e^{-st}\cdot t\ dt
					</mrow>
					<mrow>
						\amp = -\frac{1}{s}\ub{\lim_{b \to \infty}\frac{b^2}{e^{sb}}}_{L} + \frac{2}{s}\ub{\int_0^\infty e^{-st}\cdot t\ dt}_{\large\lap{t}}
					</mrow>.
				</md>
			</p>

			<p>
				Noticing that the improper integral is just <m>\lap{t}</m>, we have
				<me>
					\lap{ t^2 } = -\frac{1}{s}\cdot L + \frac{2}{s}\cdot \lap{t}
				</me>,
				but <m>L=0</m> if <m>s \gt 0</m> <xref ref="lt-example-tsqrd-LH-details" text="custom">(üîçHow?)</xref>, so we have the relationship
			</p>

			<me>
				\lap{t^2} = \frac{2}{s}\cdot \lap{t}, \quad s \gt 0
			</me>.
		</proof>
		
		<p>
			You can use this work as a template for a general recursive relationship:
		</p>

		<proof label="common-recursive-power-function-details">
			<title> <me>\lap{t^n} = \frac{n}{s}\cdot \lap{t^{n-1}}, \quad s \gt 0</me>Click here for details </title>

			<p>
				Replacing <m>2</m> with <m>n</m> in the previous solution, we have
				<me>
					\lap{ t^n } = \lim_{b \to \infty} \ub{\int_0^b e^{-st} \cdot t^n\ dt}_{I}
				</me>.
			</p>

			<p>
				Applying integration by parts to <m>I</m> once in <m>\lap{ t^{n} }</m> shows
				<md>
					<mrow>
						\lap{ t^{n} }
						\amp = \lim_{b \to \infty} \left[-\frac{b^n}{e^{sb}} + \frac{n}{s}\int_0^b e^{-st}\cdot t^{n-1}\ dt\right]
						<xref ref="lt-example-tnth-IVP-details" text="custom">üîçHow?</xref>
					</mrow>
					<mrow>
						\amp = -\frac{1}{s} \lim_{b \to \infty} \left[-\frac{b^n}{e^{sb}}\right] + \frac{n}{s}\lim_{b \to \infty}\int_0^b e^{-st}\cdot t^{n-1}\ dt
					</mrow>
					<mrow>
						\amp = -\frac{1}{s}\ub{\lim_{b \to \infty}\frac{b^n}{e^{sb}}}_{L} + \frac{n}{s}\ub{\int_0^\infty e^{-st}\cdot t^{n-1}\ dt}_{\large\lap{t^{n-1}}}
					</mrow>.
				</md>
			</p>

			<p>
				Noticing that the improper integral is just <m>\lap{t^{n-1}}</m>, we have
				<me>
					\lap{ t^{n} } = -\frac{1}{s}\cdot L + \frac{n}{s}\cdot \lap{t^{n-1}}
				</me>,
				but <m>L=0</m> if <m>s \gt 0</m> <xref ref="lt-example-tnth-LH-details" text="custom">(üîçHow?)</xref>, so we have the relationship
			</p>

			<me>
				\lap{t^{n}} = \frac{n}{s}\cdot \lap{t^{n-1}}, \quad s \gt 0
			</me>.
		</proof>

		<p>
			To get the general formula we apply this relationship repeatedly for increasing <m>n</m>:
			<me> 
				\begin{array}{crcl}
					n=1:	\amp \lap{t}	\amp =	\amp \dfrac{1}{s}\cdot\lap{1}		=	{\DLO\dfrac{1}{s^2}}\\
					n=2:	\amp \lap{t^2}	\amp =	\amp \dfrac{2}{s}\cdot\lap{t}		=	\dfrac{2}{s}\cdot{\DLO\dfrac{1}{s^2}} = {\DLBa\dfrac{2\cdot 1}{s^3}}\\
					n=3:	\amp \lap{t^3}	\amp =	\amp \dfrac{3}{s}\cdot\lap{t^2}		=	\dfrac{3}{s}\cdot{\DLBa\dfrac{2\cdot 1}{s^3}} = {\DLO\dfrac{3\cdot 2\cdot 1}{s^4}}\\
					n=4:	\amp \lap{t^4}	\amp =	\amp \dfrac{4}{s}\cdot\lap{t^3}		=	\dfrac{4}{s}\cdot{\DLO\dfrac{3\cdot 2\cdot 1}{s^4}} = {\DLBa\dfrac{4\cdot 3\cdot 2\cdot 1}{s^5}}\\
					\vdots	\amp \vdots\quad\amp	\amp \qquad\qquad\vdots\\
					n=n:	\amp \lap{t^n} 	\amp = 	\amp \dfrac{n}{s}\cdot\lap{t^{n-1}}	=	\dfrac{n}{s}\cdot\dfrac{(n-1)\dotsm 4\cdot 3\cdot 2\cdot 1}{s^{n}}
				\end{array}
			</me>.
		</p>

		<p>
			The pattern indicates that the Laplace transform of <m>t^n</m> is given by
		</p>

		<me xml:id="lt-L3">
			\text{L}_3:\quad\lap{t^n} = \frac{n!}{s^{n+1}}, \quad s \gt 0, \quad n = 0, 1, 2, \ldots
		</me>
	</subsection>
	
	<subsection label="sine-cosine-function-transform">
		<title> Laplace Transforms of Sine and Cosine </title>

		<p>
			Finally, we derive the Laplace transforms of <m>\sin(bt)</m> and <m>\cos(bt)</m>.
		</p>

		<p>
			To make the derivation easier, we will find the transform of <m>\cos(3t)</m> first.
		</p>

		<proof><title> <me>\lap{\cos(3t)} = \frac{s}{s^2 + 3^2}, \quad s \gt 0</me>Click here for details </title>
			<p>
				Applying the definition and writing the integral as a limit, we have
				<me>
					\lap{ \cos(3t)} = \int_0^{\infty} e^{-st} \cdot \cos(3t)\ dt = \lim_{b \to \infty} \ub{\int_0^{b} e^{-st} \cos(3t)\ dt}_{I}
				</me>.
			</p>

			<p>
				Treating <m>s</m> constant, we apply integration by parts to <m>I</m> as follows:
			</p>

			<me>
				I = -\frac{e^{-st}}{s} \cos(3t) \Bigg|_0^b - \frac{3}{s}\int_0^{b} e^{-st} \sin(3t)\ dt
			</me>,

			<aside><title> Integration by Parts </title>
				<p>
					1st Integration by Parts
					<md>
						<mrow>	u	\amp = \cos(3t)				</mrow>
						<mrow>	du	\amp = -3\sin(3t)\ dt		</mrow>
						<mrow>	v	\amp = -\sfrac{e^{-st}}{s}	</mrow>
						<mrow>	dv	\amp = e^{-st}\ dt			</mrow>
					</md>
					2nd Integration by Parts
					<md>
						<mrow>	u	\amp = \sin(3t)				</mrow>
						<mrow>	du	\amp = 3\cos(3t)\ dt		</mrow>
						<mrow>	v	\amp = -\sfrac{e^{-st}}{s}	</mrow>
						<mrow>	dv	\amp = e^{-st}\ dt			</mrow>
					</md>
				</p>
			</aside>

			<p>
				but this requires a second integration by parts:
				<md>
					<mrow>
						I
						\amp = -\frac{e^{-st}}{s} \cos(3t) \Bigg|_0^b - \frac{3}{s} \left[ -\frac{e^{-st}}{s} \sin(3t)\Bigg|_0^b + \frac{3}{s} \int_0^{b} e^{-st} \cos(3t)\ dt \right]
					</mrow>
					<mrow>
						\amp = \left(-\frac{e^{-st}}{s} \cos(3t) + \frac{3e^{-st}}{s^2} \sin(3t)\right)\Bigg|_0^b - \frac{9}{s^2} \ub{\int_0^{b} e^{-st} \cos(3t)\ dt}_{I}
					</mrow>
				</md>.
			</p>

			<p>
				Since the integral <m>I</m> reappeared, we actually have
				<me>
					I = \left(-\frac{e^{-st}}{s} \cos(3t) + \frac{3e^{-st}}{s^2} \sin(3t)\right)\Bigg|_0^b - \frac{9}{s^2} I
				</me>.
				Evaluating the limits of integration and solving for <m>I</m>, we find
				<md>
					<mrow>
						I + \frac{9}{s^2} I  \amp = \left(-\frac{e^{-st}}{s} \cos(3t) + \frac{3e^{-st}}{s^2} \sin(3t)\right)\Bigg|_0^b
					</mrow>
					<mrow>
						I\left(\frac{s^2+9}{s^2}\right) \amp = \left(-\frac{e^{-sb}}{s} \cos(3b) + \frac{3e^{-sb}}{s^2} \sin(3b) + \frac{1}{s} \right)
					</mrow>
					<mrow> 
						I	\amp = \frac{s^2}{s^2+9}\left(-\frac{e^{-sb}}{s} \cos(3b) + \frac{3e^{-sb}}{s^2} \sin(3b) + \frac{1}{s} \right)
					</mrow>
				</md>
			</p>

			<p>
				Finally, the limit of <m>I</m> as <m>b \to \infty</m> is the sum of the limits
				<md>
					<mrow>
						\lim_{b \to \infty} I = \amp
					</mrow>
					<mrow>
						\frac{s^2}{s^2+9} \amp \Bigg(
							- \frac{1}{s}\ub{\lim_{b \to \infty} e^{-sb} \cos(3b)}_{L_1}
							+ \frac{3}{s^2}\ub{\lim_{b \to \infty} e^{-sb} \sin(3b)}_{L_2} 
							+ \frac{1}{s}
						\Bigg)
					</mrow>
				</md>
				Since <xref ref="lt-example-4-details" text="custom"><m>L_1\to0</m> &amp; <m>L_2\to0</m> if <m>s \gt 0</m></xref>, we can conclude that
				<me>
					\lap{\cos(3t)} = \frac{s}{s^2 + 9}, \quad s \gt 0
				</me>.
			</p>
		</proof>

		<p>
			Replacing the constants <m>3</m> and <m>9</m> with <m>b</m> and <m>b^2</m>, respectively, shows that
			<me xml:id="lt-L4">
				\text{L}_4:\quad\lap{\cos(bt)} = \frac{s}{s^2 + b^2}, \quad s \gt 0
			</me>.
		</p>

		<p>
			The derivation of the formula for the Laplace transform of sine, given by
			<me xml:id="lt-L5">
				\text{L}_5:\quad\lap{\sin(bt)} = \frac{b}{s^2 + b^2}, \quad s \gt 0
			</me>,
			follows a similar approach and is left as exercise for you to try on your own.
		</p>
	</subsection>

	<objectives label="common-transforms-wrapup">
		<ul marker="square">
			<li>
				<p>
					We now have the following common Laplace transforms:
					<ul>
						<li><m> \ds\lap{1} = \frac{1}{s}, \quad s \gt 0 </m>,</li>
						<li><m> \ds\lap{e^{at}} = \frac{1}{s - a}, \quad s \gt a </m>,</li>
						<li><m> \ds\lap{t^n} = \frac{n!}{s^{n+1}}, \quad s \gt 0, \quad n = 0, 1, 2, \ldots </m>,</li>
						<li><m> \ds\lap{\cos(bt)} = \frac{s}{s^2 + b^2}, \quad s \gt 0 </m>,</li>
						<li><m> \ds\lap{\sin(bt)} = \frac{b}{s^2 + b^2}, \quad s \gt 0 </m>.</li>
					</ul>
				</p>
			</li>
		</ul>
	</objectives>
</section>