<section><title> Abandoned Content</title>

	<p>
		This chapter contains content that was abandoned during the development of the book. It is not part of the final version.
	</p>

	<p>
		The table below summarizes the common Laplace transforms that we derived in this section.
	</p>

	<assemblage xml:id="lt-table-L1-L8-v2"><title> ✳️ Common Laplace Transforms <m>L_1-L_8</m> </title>
		<p>
			Let <m>a</m> and <m>b</m> be constant.
			<dl width="narrow">
				<li><title> <m>{\LARGE \vphantom{\int}}L_1</m> </title>
					<m>\ds \lap{ 1 } = \frac{1}{s}, \quad s &gt;0 </m>
				</li>
				<li><title> <m>{\LARGE \vphantom{\int}}L_2</m> </title>
					<m>\ds \lap{ e^{at} } = \frac{1}{s - a}, \quad s &gt;a </m>
				</li>
				<li><title> <m>{\LARGE \vphantom{\int}}L_3</m> </title>
					<m>\ds \lap{ t^n } = \frac{n!}{s^{n+1}}, \quad s &gt;0, \quad n = 1, 2, 3, \ldots </m>
				</li>
				<li><title> <m>{\LARGE \vphantom{\int}}L_4</m> </title>
					<m>\ds \lap{ \sin(bt) } = \frac{b}{s^2+b^2}, \quad s &gt;0</m>
				</li>
				<li><title> <m>{\LARGE \vphantom{\int}}L_5</m> </title>
					<m>\ds \lap{ \cos(bt) } = \frac{s}{s^2+b^2}, \quad s &gt;0 </m>
				</li>
				<li><title> <m>{\LARGE \vphantom{\int}}L_6</m> </title>
					<m>\lap{ t^n e^{at} } = \ds\frac{n!}{(s-a)^{n+1}}, \quad s &gt;a </m>
				</li>
				<li><title> <m>{\LARGE \vphantom{\int}}L_7.</m> </title>
					<m>\ds \lap{ e^{at}\sin(bt) } = \frac{b}{(s-a)^2+b^2}, \quad s &gt;a </m>
				</li>
				<li><title> <m>{\LARGE \vphantom{\int}}L_8.</m> </title>
					<m>\ds \lap{ e^{at}\cos(bt) } = \frac{s-a}{(s-a)^2+b^2}, \quad s &gt;a</m>
				</li>
			</dl>
		</p>
	</assemblage>

	<assemblage xml:id="lt-table-L1-L12-v2"><title> ✳️ Common Laplace Transform and Properties </title>
		<p>
			Assume <m>F(s) = \lap{f(t)}</m>, <m>a</m>, <m>b</m> are constant, and <m>n=0,1,2,3,\ldots</m>
		</p>

		<p>
			<image><latex-image>\begin{tikzpicture}\draw(-5,0)--(5,0);\end{tikzpicture}</latex-image></image>
			<sidebyside widths="5% 12% 36% 11%" valign="middle" margin="18%">
				<p> <me>\small \text{ID} </me> </p>
				<p> <me>\small f(t) </me> </p>
				<p> <me>\small \lap{f(t)} = F(s) </me> </p>
				<p> <me>\small \text{Condition} </me> </p>
			</sidebyside>
			<image><latex-image>\begin{tikzpicture}\draw(-5,0)--(5,0);\end{tikzpicture}</latex-image></image>
			<sidebyside widths="5% 12% 36% 11%" valign="middle" margin="18%">
				<p> <me>\small L_{1}</me> </p>
				<p> <me>\small 1 </me> </p>
				<p> <me>\small \frac{1}{s}</me> </p>
				<p> <me>\small s &gt; 0</me> </p>
			</sidebyside>
			<image><latex-image>\begin{tikzpicture}\draw(-5,0)--(5,0);\end{tikzpicture}</latex-image></image>
			<sidebyside widths="5% 12% 36% 11%" valign="middle" margin="18%">
				<p> <me>\small L_{2}</me> </p>
				<p> <me>\small e^{at} </me> </p>
				<p> <me>\small \frac{1}{s - a}</me> </p>
				<p> <me>\small s &gt; 0</me> </p>
			</sidebyside>
			<image><latex-image>\begin{tikzpicture}\draw(-5,0)--(5,0);\end{tikzpicture}</latex-image></image>
			<sidebyside widths="5% 12% 36% 11%" valign="middle" margin="18%">
				<p> <me>\small L_{3}</me> </p>
				<p> <me>\small t^n </me> </p>
				<p> <me>\small \frac{n!}{s^{n+1}}</me> </p>
				<p> <me>\small s &gt; 0</me> </p>
			</sidebyside>
			<image><latex-image>\begin{tikzpicture}\draw(-5,0)--(5,0);\end{tikzpicture}</latex-image></image>
			<sidebyside widths="5% 12% 36% 11%" valign="middle" margin="18%">
				<p> <me>\small L_{4}</me> </p>
				<p> <me>\small \sin(bt)</me> </p>
				<p> <me>\small \frac{b}{s^2+b^2}</me> </p>
				<p> <me>\small s &gt; 0</me> </p>
			</sidebyside>
			<image><latex-image>\begin{tikzpicture}\draw(-5,0)--(5,0);\end{tikzpicture}</latex-image></image>
			<sidebyside widths="5% 12% 36% 11%" valign="middle" margin="18%">
				<p> <me>\small L_{5}</me> </p>
				<p> <me>\small \cos(bt)</me> </p>
				<p> <me>\small \frac{s}{s^2+b^2}</me> </p>
				<p> <me>\small s &gt; 0</me> </p>
			</sidebyside>
			<image><latex-image>\begin{tikzpicture}\draw(-5,0)--(5,0);\end{tikzpicture}</latex-image></image>
			<sidebyside widths="5% 12% 36% 11%" valign="middle" margin="18%">
				<p> <me>\small L_{6}</me> </p>
				<p> <me>\small e^{at}\ t^n </me> </p>
				<p> <me>\small \ds\frac{n!}{(s-a)^{n+1}}</me> </p>
				<p> <me>\small s &gt; a</me> </p>
			</sidebyside>
			<image><latex-image>\begin{tikzpicture}\draw(-5,0)--(5,0);\end{tikzpicture}</latex-image></image>
			<sidebyside widths="5% 12% 36% 11%" valign="middle" margin="18%">
				<p> <me>\small L_{7}</me> </p>
				<p> <me>\small e^{at}\sin(bt) </me> </p>
				<p> <me>\small \frac{b}{(s-a)^2+b^2}</me> </p>
				<p> <me>\small s &gt; a</me> </p>
			</sidebyside>
			<image><latex-image>\begin{tikzpicture}\draw(-5,0)--(5,0);\end{tikzpicture}</latex-image></image>
			<sidebyside widths="5% 12% 36% 11%" valign="middle" margin="18%">
				<p> <me>\small L_{8}</me> </p>
				<p> <me>\small e^{at}\cos(bt) </me> </p>
				<p> <me>\small \frac{s-a}{(s-a)^2+b^2}</me> </p>
				<p> <me>\small s &gt; a</me> </p>
			</sidebyside>
			<image><latex-image>\begin{tikzpicture}\draw(-5,0)--(5,0);\end{tikzpicture}</latex-image></image>
			<sidebyside widths="5% 12% 36% 11%" valign="middle" margin="18%">
				<p> <me>\small L_{9}</me> </p>
				<p> <me>\small f'(t) </me> </p>
				<p> <me>\small sF(s) - f(0) </me> </p>
				<p> <me>\small s &gt; 0</me> </p>
			</sidebyside>
			<image><latex-image>\begin{tikzpicture}\draw(-5,0)--(5,0);\end{tikzpicture}</latex-image></image>
			<sidebyside widths="5% 12% 36% 11%" valign="middle" margin="18%">
				<p> <me>\small L_{10}</me> </p>
				<p> <me>\small f''(t) </me> </p>
				<p> <me>\small s^2F(s) - sf(0) - f'(0) </me> </p>
				<p> <me>\small s &gt; 0</me> </p>
			</sidebyside>
			<image><latex-image>\begin{tikzpicture}\draw(-5,0)--(5,0);\end{tikzpicture}</latex-image></image>
			<sidebyside widths="5% 12% 36% 11%" valign="middle" margin="18%">
				<p> <me>\small L_{11}</me> </p>
				<p> <me>\small f'''(t) </me> </p>
				<p> <me>\small s^3F(s) - s^2f(0) - sf'(0) - f''(0) </me> </p>
				<p> <me>\small s &gt; 0</me> </p>
			</sidebyside>
			<image><latex-image>\begin{tikzpicture}\draw(-5,0)--(5,0);\end{tikzpicture}</latex-image></image>
			<sidebyside widths="5% 12% 36% 11%" valign="middle" margin="18%">
				<p> <me>\small L_{12}</me> </p>
				<p> <me>\small t^n f(t) </me> </p>
				<p> <me>\small (-1)^n \frac{d^{(n)}}{ds^{(n)}}F(s)</me> </p>
				<p> <me>\small s &gt; 0</me> </p>
			</sidebyside>
		</p>
	</assemblage>

	<assemblage xml:id="lt-table-L1"><title> ✳️ Common Laplace Transform and Properties </title>
		<p>
			Assume <m>F(s) = \lap{f(t)}</m>, <m>a</m>, <m>b</m> are constant, and <m>n=0,1,2,3,\ldots</m>.
		</p>

		<p>
			<sidebyside widths="5% 80% 15%" valign="middle">
				<p> <me> \text{ID} </me> </p>
				<p> <me> \lap{f(t)} = F(s) </me> </p>
				<p> <me> \text{Condition} </me> </p>
			</sidebyside>
			<image><latex-image>\begin{tikzpicture}\draw(-5,0)--(5,0);\end{tikzpicture}</latex-image></image>
			<sidebyside widths="5% 80% 15%" valign="middle">
				<p> <me>L_1</me> </p>
				<p> <me>\lap{ 1 } = \frac{1}{s}</me> </p>
				<p> <me>\vphantom{\int}s &gt; 0</me> </p>
			</sidebyside>
			<sidebyside widths="5% 80% 15%" valign="middle">
				<p> <me>L_2</me> </p>
				<p> <me>\lap{ e^{at} } = \frac{1}{s - a}</me> </p>
				<p> <me>\vphantom{\int}s &gt; 0</me> </p>
			</sidebyside>
			<sidebyside widths="5% 80% 15%" valign="middle">
				<p> <me>L_3</me> </p>
				<p> <me>\lap{ t^n } = \frac{n!}{s^{n+1}}</me> </p>
				<p> <me>\vphantom{\int}s &gt; 0</me> </p>
			</sidebyside>
			<sidebyside widths="5% 80% 15%" valign="middle">
				<p> <me>L_4</me> </p>
				<p> <me>\lap{\sin(bt)} = \frac{b}{s^2+b^2}</me> </p>
				<p> <me>\vphantom{\int}s &gt; 0</me> </p>
			</sidebyside>
			<sidebyside widths="5% 80% 15%" valign="middle">
				<p> <me>L_5</me> </p>
				<p> <me>\lap{\cos(bt)} = \frac{s}{s^2+b^2}</me> </p>
				<p> <me>\vphantom{\int}s &gt; 0</me> </p>
			</sidebyside>
			<sidebyside widths="5% 80% 15%" valign="middle">
				<p> <me>L_6</me> </p>
				<p> <me>\lap{ e^{at}\ t^n } = \ds\frac{n!}{(s-a)^{n+1}}</me> </p>
				<p> <me>\vphantom{\int}s &gt; a</me> </p>
			</sidebyside>
			<sidebyside widths="5% 80% 15%" valign="middle">
				<p> <me>L_7</me> </p>
				<p> <me>\lap{ e^{at}\sin(bt) } = \frac{b}{(s-a)^2+b^2}</me> </p>
				<p> <me>\vphantom{\int}s &gt; a</me> </p>
			</sidebyside>
			<sidebyside widths="5% 80% 15%" valign="middle">
				<p> <me>L_8</me> </p>
				<p> <me>\lap{ e^{at}\cos(bt) } = \frac{s-a}{(s-a)^2+b^2}</me> </p>
				<p> <me>\vphantom{\int}s &gt; a</me> </p>
			</sidebyside>
			<sidebyside widths="5% 80% 15%" valign="middle">
				<p> <me>L_9</me> </p>
				<p> <me>\lap{ f'(t) } = sF(s) - f(0) </me> </p>
				<p> <me>\vphantom{\int}s &gt; 0</me> </p>
			</sidebyside>
			<sidebyside widths="5% 80% 15%" valign="middle">
				<p> <me>L_{10}</me> </p>
				<p> <me>\lap{ f''(t) } = s^2F(s) - sf(0) - f'(0) </me> </p>
				<p> <me>\vphantom{\int}s &gt; 0</me> </p>
			</sidebyside>
			<sidebyside widths="5% 80% 15%" valign="middle">
				<p> <me>L_{11}</me> </p>
				<p> <me>\lap{ f'''(t) } = s^3F(s) - s^2f(0) - sf'(0) - f''(0) </me> </p>
				<p> <me>\vphantom{\int}s &gt; 0</me> </p>
			</sidebyside>
			<sidebyside widths="5% 80% 15%" valign="middle">
				<p> <me>L_{12}</me> </p>
				<p> <me>\lap{ t^n f(t) } = (-1)^n \frac{d^{(n)}}{ds^{(n)}}F(s)</me> </p>
				<p> <me>\vphantom{\int}s &gt; 0</me> </p>
			</sidebyside>
		</p>

	</assemblage>

	<assemblage xml:id="lt-linearity-property-P6"><title> ✳️ Laplace Transform Property <m>P_1</m> </title>
		<p>
			Let <m>F(s) = \lap{f(t)}</m> and <m>G(s) = \lap{g(t)}</m>.
			<dl width="narrow">
				<li><title> <m>P_1</m> </title>
					<m>\ds \lap{ a f(t) \pm b g(t) } = a F(s) \pm b G(s), \quad a, b </m> are constants
				</li>
				<li><title> <m>P_2.</m> </title>
					<m>\ds \lap{ e^{at} f(t) } = F(s-a), \quad a </m> is a constant
				</li>
				<li><title> <m>P_3.</m> </title>
					<m>\ds \lap{ f'(t) } = sF(s) - f(0) </m>
				</li>
				<li><title> <m>P_4.</m> </title>
					<m>\ds \lap{ f''(t) } = s^2F(s) - sf(0) - f'(0) </m>
				</li>
				<li><title> <m>P_5.</m> </title>
					<m>\ds \lap{ f'''(t) } = s^3F(s) - s^2f(0) - sf'(0) - f''(0) </m>
				</li>
				<li><title> <m>{\LARGE \vphantom{\int}}P_6.</m> </title>
					<m>\ds \lap{ t^n f(t) } = (-1)^n \frac{d^{(n)}}{ds^{(n)}}F(s), \quad n = 1, 2, 3, \ldots </m>
				</li>
			</dl>
		</p>
	</assemblage>
	
</section>