
<subsection xmlns:xi="http://www.w3.org/2001/XInclude"><title> Summary &amp; Exercises </title>

	<introduction>
		<p>
			The LHCC chapter (Linear Homogeneous Differential Equations with Constant Coefficients) in "Linear Constant Coefficient Methods" introduces a systematic method to solve higher-order linear differential equations. Here's a summary based on the content:
		</p>

		<assemblage color="green"><title>Summary of the Key Ideas</title>
			<p>
					<ul>
						<li xml:id="summary-lhcc-1">
							<term>Linear Homogeneous Differential Equations with Constant Coefficients (LHCC)</term>
							<ul marker="square">
								<li>These are differential equations where each term consists of a derivative of the unknown function multiplied by a constant.</li>
								<li>The general form of an LHCC equation is:
									<me>a_n\ y^{(n)} + a_{n-1}\ y^{(n-1)} + \dots + a_1\ y' + a_0\ y = 0</me>.
								</li>
							</ul>
						</li>
						<li xml:id="summary-lhcc-2">
							<term>The Characteristic Equation</term>
							<ul marker="square">
								<li>By assuming a solution of the form <m>y = e^{rx}</m>, an LHCC can be reduced to a characteristic polynomial in <m>r</m>.</li>
								<li>The solutions to the characteristic equation determine the form of the general solution.</li>
							</ul>
						</li>
						<li xml:id="summary-lhcc-3">
							<term>Solution Types</term>
							<ul marker="square">
								<li>Let <m>r</m> be a solution to the characteristic equation (CE).</li>
								<li>
									If <m>r</m> is different from all other solutions of the CE, then
									<me>c e^{r x}</me>
									is a term of the general solution.
								</li>
								<li>
									If <m>r</m> is equal to, say, three other solutions of the CE, then 
									<me>c_1 e^{r x} + c_2 x e^{r x} + c_3 x^2 e^{r x}</me>
									are terms of the general solution.
								</li>
								<li>
									If <m>r = \alpha + i\beta</m> or <m>r = \alpha - i\beta</m>, then the general solution contains
									<me>e^{\alpha x}(c_1\sin(\beta x)+c_2\cos(\beta x))</me>.
								</li>
							</ul>
						</li>
					</ul>
				</p>
		</assemblage>
		
		<exploration xml:id="lhcc-method"><title>LHCC Method</title>
			<p>
				The general solution to a linear homogeneous differential equation with constant coefficients (LHCC) of the form
				<men>
					a_n\ y^{(n)} + a_{n-1}\ y^{(n-1)} + \cdots + a_2\ y'' + a_1\ y' + a_0\ y = 0,
				</men>
				can be found through the following steps...
			</p>
			<dl width="narrow">
				<li xml:id="lhcc-step1"><title>Step 1: Solve the Characteristic Equation </title>
					<p>
						Solve the characteristic equation (CE) 
						<me>
							a_n\ r^{n} + a_{n-1}\ r^{n-1} + \cdots + a_2\ r^2 + a_1\ r + a_0 = 0,
						</me>
						
					</p>
				</li>
				<li xml:id="lhcc-step2"><title>Step 2: Write Down the General Solution </title>
					<p>
						<ul marker="square">
							<li>
								<em>Real &amp; Different:</em> <m> r_1, r_2, \dots, r_n </m>
								<me>y(x) = c_1 e^{r_1 x} + c_2 e^{r_2 x} + \dots + c_n e^{r_n x}</me>.
							</li>
		
							<li>
								<em>Real &amp; Repeated:</em> <m> r_1 </m> (multiplicity <m> m </m>)
								<me>y(x) = (c_1 + c_2 x + \dots + c_m x^{m-1}) e^{r_1 x}</me>.
							</li>
		
							<li>
								<em>Complex:</em> <m> \alpha \pm i\beta </m>
								<me>y(x) = e^{\alpha x} \left(c_1 \cos(\beta x) + c_2 \sin(\beta x)\right)</me>.
							</li>

							<li>
								<em>For mixed root types</em>, combine the corresponding terms to form the complete general solution.
							</li>
						</ul>
					</p>
				</li>
			</dl>
		</exploration>
		
	</introduction>

	<exercises>

		<exercise xml:id="tba">
			<statement>
				<p> Show why <m>x</m> is needed in the general solution for repeated roots of the CE </p>
			</statement>
			<solution><title> Solution </title>
				<p>
					
				</p>
			</solution>
			<answer><title>Answer</title>
				<p>
					
				</p>
			</answer>
		</exercise>

		<exercisegroup><title> Classify the following differential equations as either homogeneous or nonhomogeneous </title>
				
			<p>*NEED EXERCISES</p>
	
			<exercise>
				<statement>
					<m> \ds 4y'' - 36y' = 0 </m>
				</statement>
				<solution><title> Solution </title>
					<p>
						
					</p>
				</solution>
				<answer><title>Answer</title>
					<p>
						
					</p>
				</answer>
			</exercise>
	
		</exercisegroup>
		
		<exercisegroup><title> Find the general solution for each of the following </title>
			<exercise>
				<statement>
					<m> \ds 4y'' -36y' = 0 </m>
				</statement>
				<solution><title> Solution </title>
					<p>
						<m> </m>
					</p>
				</solution>
				<answer><title>Answer</title>
					<p>
						
					</p>
				</answer>
			</exercise>
		
			<exercise>
				<statement>
					<m> \ds 4y'' -36y = 0. </m>
				</statement>
				<solution><title> Solution </title>
					<p>
						<m> </m>
					</p>
				</solution>
				<answer><title>Answer</title>
					<p>
						
					</p>
				</answer>
			</exercise>
		
			<exercise>
				<statement>
					<m> \ds y''- y' - 11y = 0 </m>
				</statement>
				<solution><title> Solution </title>
					<p>
						<m> </m>
					</p>
				</solution>
				<answer><title>Answer</title>
					<p>
						
					</p>
				</answer>
			</exercise>
		
			<exercise>
				<statement>
					<m> \ds 2\frac{d^2 \theta}{dt^2} -6\frac{d\theta}{dt} - 8\theta = 0 </m>
				</statement>
				<solution><title> Solution </title>
					<p>
						
					</p>
				</solution>
				<answer><title>Answer</title>
					<p>
						
					</p>
				</answer>
			</exercise>
		
		</exercisegroup>
		
		<exercisegroup><title> Solve the following initial value problems </title>
			<exercise>
				<statement>
					<m> \ds 4y'' -36y = 0 \hspace{1cm} c_1 </m> an <m> \ds c_2 </m> that satisfy thegiven initial conditions.
				</statement>
				<solution><title> Solution </title>
					<p>
				We already have the general solution <m> \ds y = c_1e^{3t} + c_2e^{-3t} </m> .  In order to use the initial conditions, we will eventually need the first derivative, so let's find that now. <m> \ds y' = 3c_1e^{3t} -3 c_2e^{-3t} </m> Now we can see what comes of the first initial condition <m> \ds y(0) = 4. </m>
					<md>
						<mrow>  y(0)	 															\amp =  4 </mrow>
						<mrow>  c_1e^{3\cdot 0} + c_2e^{-3\cdot 0}	\amp =  4 </mrow>
						<mrow>  c_1 + c_2	 													\amp =  4 </mrow>
					</md>
					Now we can use the other initial condition <m> \ds y'(0) = -6. </m>
					<md>
						<mrow>  y'(0)	 																\amp =  -6 </mrow>
						<mrow>  3c_1e^{3\cdot 0} -3 c_2e^{-3\cdot 0}	\amp =  -6 </mrow>
						<mrow>  3c_1 - 3c_2	 													\amp =  -6 </mrow>
					</md>
					Notice that the resulting equations, (\ref{eq7}) and (\ref{eq8}) constitute a system of two linear equations in two unknowns, and we should be able to solve for the unknown <m> \ds c_1 </m> an <m> \ds c_2 </m> .  There are multiple ways to achieve this.  One possibility is to solve fo <m> \ds c_2 </m> in equation (\ref{eq7}) and then substitute into equation (\ref{eq8}) as follows.
					<md>
						<mrow>  c_2	 							\amp =  4 - c_1	</mrow>
						<mrow>  3c_1 - 3(4 - c_1)	\amp = -6 			</mrow>
						<mrow>  3c_1 - 12 + 3c_1	\amp = -6 			</mrow>
						<mrow>  6c_1 - 12					\amp = -6 			</mrow>
						<mrow>  6c_1							\amp =  6 			</mrow>
						<mrow>  c_1	 							\amp =  1 			</mrow>
						<mrow>  c_2	 							\amp =  4 - 1 	</mrow>
						<mrow>   									\amp =  3 			</mrow>
					</md>
					Hence, we have the solution <m> \ds y = e^{3t} + 3e^{-3t}. </m> <em> Note:  it's not clear whether the independent variable i <m> \ds x </m> o <m> \ds t </m> , so you could replace th <m> \ds t </m> 's wit <m> \ds x </m> 's.</em>
					</p>
				</solution>
				<answer><title>Answer</title>
					<p>
						<m> \ds y = e^{3t} + 3e^{-3t} </m> o <m> \ds y = e^{3x} + 3e^{-3x} </m>
					</p>
				</answer>
			</exercise>
		
			<exercise>
				<statement>
					<m> \ds \ds 2\frac{d^2 \theta}{dt^2} -6\frac{d\theta}{dt} - 8\theta = 0,\hspace{1cm} \theta(0) = 12, \hspace{1cm} \theta'(0) = -2 </m>
				</statement>
				<solution><title> Solution </title>
					<p>
						
					</p>
				</solution>
				<answer><title>Answer</title>
					<p>
						
					</p>
				</answer>
			</exercise>
		
		</exercisegroup>
		
		<exercisegroup><title> Boundary Value Problems </title>
			<exercise>
				<statement>
					Solve the following boundary value problem.<m> \ds y'' - y = 0, \hspace{1cm} y(0) = 1, \hspace{1cm} y(1) = 2e- \frac{1}{e}</m>
				</statement>
				<solution><title> Solution </title>
					<p>
				We begin by verifying the following: 
					<line>  the DE is linear, </line>
					<line>  the DE is homogeneous, and </line>
					<line>  the DE has constant coefficients. </line>
					Since all of the conditions are true, we can safely proceed to find the general solution.  We write down and then solve the characteristic equation, as follows.
					<md>
						<mrow>  r^2 - 1	 	\amp =  0 						</mrow>
						<mrow>  r^2	 			\amp =  1 						</mrow>
						<mrow>  r	 				\amp =  \pm \sqrt{1} 	</mrow>
						<mrow>  r	 				\amp =  \pm 1 				</mrow>
		
					</md>
					Since <m> \ds r = 1 </m> an <m> \ds r = -1 </m> are distinct, real roots, the general solution is given by <m> \ds y = c_1e^{t} + c_2e^{-t}. </m> Now we can see what comes of the first boundary condition <m> \ds y(0) = 1. </m>
					<md>
						<mrow>  y(0)	 \amp =  1 </mrow>
						<mrow>  c_1e^{0} + c_2e^{-0}	 \amp =  1 </mrow>
						<mrow>  c_1 + c_2	 \amp =  1  </mrow>
					</md>
					Now we can use the other boundary condition <m> \ds y(1) = 2e- \frac{1}{e}. </m>
					<md>
						<mrow>  y(1)	 \amp =  2e- \frac{1}{e} </mrow>
						<mrow>  c_1e^{1} + c_2e^{-1}	 \amp =  2e- \frac{1}{e} </mrow>
						<mrow>  c_1\cdot e + c_2\cdot \frac{1}{e}	 \amp =  2e- \frac{1}{e}  </mrow>
					</md>
					Notice that the resulting equations, (\ref{eq11}) and (\ref{eq12}) constitute a system of two linear equations in two unknowns, and we should be able to solve for the unknown <m> \ds c_1 </m> an <m> \ds c_2 </m> .  There are multiple ways to achieve this.  One possibility is to solve fo <m> \ds c_2 </m> in equation (\ref{eq11}) and then substitute into equation (\ref{eq12}) as follows.
					<md>
						<mrow>  c_2	 \amp =  1 - c_1 </mrow>
						<mrow>  c_1\cdot e + (1 - c_1)\cdot \frac{1}{e}	 \amp =  2e- \frac{1}{e} </mrow>
						<mrow>  c_1\cdot e + \frac{1}{e} - c_1\cdot \frac{1}{e}	 \amp =  2e- \frac{1}{e} </mrow>
						<mrow>  c_1\cdot e - c_1\cdot \frac{1}{e}	 \amp =  2e - \frac{2}{e} </mrow>
						<mrow>  c_1\left(e - \frac{1}{e}  \right)	 \amp =  2e - \frac{2}{e} </mrow>
						<mrow>  c_1	 \amp =  \frac{2e - \frac{2}{e}}{e - \frac{1}{e}} </mrow>
						<mrow>   \amp =  \frac{2e - \frac{2}{e}}{e - \frac{1}{e}} \cdot \frac{e}{e} </mrow>
						<mrow>   \amp =  \frac{2e^2 - 2}{e^2 - 1} </mrow>
						<mrow>   \amp =  \frac{2(e^2 - 1)}{e^2 - 1} </mrow>
						<mrow>   \amp =  2 </mrow>
						<mrow>  c_2	 \amp =  1 - 2 </mrow>
						<mrow>   \amp =  -1  </mrow>
					</md>
					Hence, we have the solution <m> \ds y = 2e^{t} - e^{-t}. </m>
					</p>
				</solution>
				<answer><title>Answer</title>
					<p>
						<m> \ds y = 2e^{t} - e^{-t} </m>
					</p>
				</answer>
			</exercise>
		
		</exercisegroup>
		
		<exercisegroup><title> Solve the following DEs </title>
			<exercise>
				<statement>
					<m> \ds w'' + 6w' + 9w = 0 </m>
				</statement>
				<solution><title> Solution </title>
					<p>
						<m> \ds w'' + 6w' + 9w = 0 </m>
					</p>
				</solution>
				<answer><title>Answer</title>
					<p>
						
					</p>
				</answer>
			</exercise>
		
			<exercise>
				<statement>
					<m> \ds m'' = 2m' - m </m>
				</statement>
				<solution><title> Solution </title>
					<p>
						<m> \ds m'' = 2m' - m </m>
					</p>
				</solution>
				<answer><title>Answer</title>
					<p>
						
					</p>
				</answer>
			</exercise>
		
		</exercisegroup>
		
		<exercisegroup><title> Initial Value Problems </title>
			<exercise>
				<statement>
					Solve the following initial value problem.<m> \ds \frac{d^2z}{dx^2} - 4\frac{dz}{dx} + 4z = 0, \hspace{0.5cm} z(1) = 1, \hspace{0.5cm} z'(1) = 1</m>
				</statement>
				<solution><title> Solution </title>
					<p>
				We begin by verifying the following: 
					<line>  the DE is linear, </line>
					<line>  the DE is homogeneous, and </line>
					<line>  the DE has constant coefficients. </line>
		Since all of the conditions are true, we can safely proceed by writing the characteristic equation and then solving it (either by factoring or using the quadratic equation).
					<md>
						<mrow>  r^2 - 4r + 4	\amp =  0 </mrow>
						<mrow>  (r-2)(r-2)		\amp =  0 </mrow>
						<mrow>  r	 						\amp =  2 \mbox{ (double root)}  </mrow>
					</md>
					Sinc <m> \ds r=2 </m> is a repeated real root, the general solution is
					<md>
						<mrow>  z	\amp =  c_1e^{2x} + c_2xe^{2x} </mrow>
						<mrow>  	\amp =  (c_1 + c_2x)e^{2x} </mrow>
		
					</md>
					In order to use the initial conditions, we will eventually need the first derivative, so let's find that now.  Note that we will use the product rule to take the derivative.
					<md>
						<mrow>  z'	\amp =  (c_1+ c_2x)\cdot 2e^{2x} + c_2 \cdot e^{2x} 	</mrow>
						<mrow>   		\amp =  (2c_1+ 2c_2x)e^{2x} + c_2e^{2x} 							</mrow>
						<mrow>   		\amp =  (2c_1 + 2c_2x + c_2)e^{2x} 										</mrow>
		
					</md>
					Now we can see what comes of the first initial condition <m> \ds z(1) = 1. </m>
					<md>
						<mrow>  z(1)	 \amp =  1 </mrow>
						<mrow>  (c_1 + c_2\cdot 1)e^{2\cdot 1}	 \amp =  1 </mrow>
						<mrow>  (c_1 + c_2)e^{2}	 \amp =  1 </mrow>
						<mrow>  c_1 + c_2	 \amp =  \frac{1}{e^2} </mrow>
						<mrow>  c_1 + c_2	 \amp =  e^{-2}  </mrow>
					</md>
					Now we can use the other initial condition <m> \ds \theta'(0) = -2. </m>
					<md>
						<mrow>  z'(1)	 \amp =  1 </mrow>
						<mrow>  (2c_1 + 2c_2\cdot 1 + c_2)e^{2\cdot 1}	 \amp =  1 </mrow>
						<mrow>  (2c_1 + 3c_2)e^{2}	 \amp =  1 </mrow>
						<mrow>  2c_1 + 3c_2	 \amp =  \frac{1}{e^2} </mrow>
						<mrow>  2c_1 + 3c_2	 \amp =  e^{-2}  </mrow>
					</md>
					Notice that the resulting equations, (\ref{eq13}) and (\ref{eq14}) constitute a system of two linear equations in two unknowns, and we should be able to solve for the unknown <m> \ds c_1 </m> and <m> \ds c_2 </m> .  There are multiple ways to achieve this.  One possibility is to solve for <m> \ds c_2 </m> in equation (\ref{eq13}) and then substitute into equation (\ref{eq14}) as follows.
					<md>
						<mrow>  c_2	 \amp =  e^{-2} - c_1 </mrow>
						<mrow>  2c_1 +3(e^{-2} - c_1)	 \amp =  e^{-2} </mrow>
						<mrow>  2c_1 +3e^{-2} - 3c_1	 \amp =  e^{-2} </mrow>
						<mrow>  -c_1 + 3e^{-2}	 \amp =  e^{-2} </mrow>
						<mrow>  -c_1	 \amp =  e^{-2} - 3e^{-2} </mrow>
						<mrow>  -c_1	 \amp =  - 2e^{-2} </mrow>
						<mrow>  c_1	 \amp =  2e^{-2} </mrow>
						<mrow>  c_2	 \amp =  e^{-2} - 2e^{-2} </mrow>
						<mrow>   \amp =  -e^{-2} </mrow>
		
					</md>
					Hence, we have the solution
					<md>
						<mrow>  z		\amp =  (2e^{-2} - e^{-2}x)e^{2x}, \mbox{ or}	</mrow>
						<mrow>   		\amp =  (2 - x)e^{-2}e^{2x}, \mbox{ or} 			</mrow>
						<mrow>   		\amp =  (2 - x)e^{-2 + 2x}, \mbox{ or} 				</mrow>
						<mrow>   		\amp =  (2 - x)e^{2x - 2}. 										</mrow>
		
					</md>
					
					</p>
				</solution>
				<answer><title>Answer</title>
					<p>
						<m> \ds z = (2e^{-2} - e^{-2}x)e^{2x} </m> or <m> \ds z = (2 - x)e^{2x - 2} </m>
					</p>
				</answer>
			</exercise>
		
		</exercisegroup>
		
		<exercisegroup><title> Solve the following DEs </title>
			<exercise>
				<statement>
					<m> \ds y'' + 4y' + 53y = 0 </m>
				</statement>
				<solution><title> Solution </title>
					<p>
						<m> \ds y'' + 4y' + 53y = 0 </m>
					</p>
				</solution>
				<answer><title>Answer</title>
					<p>
						
					</p>
				</answer>
			</exercise>
		
			<exercise>
				<statement>
					<m> \ds z''=-36z </m>
				</statement>
				<solution><title> Solution </title>
					<p>
						<m> \ds z''=-36z </m>
					</p>
				</solution>
				<answer><title>Answer</title>
					<p>
						
					</p>
				</answer>
			</exercise>
		
		</exercisegroup>
		
		<exercisegroup><title> Solve the following DEs </title>
			<exercise>
				<statement>
					<m> \ds y'' = -24y' - 144y </m> 
				</statement>
				<solution><title> Solution </title>
					<p>
						<m> \ds y'' = -24y' - 144y </m> 
					</p>
				</solution>
				<answer><title>Answer</title>
					<p>
						
					</p>
				</answer>
			</exercise>
		
			<exercise>
				<statement>
					<m> \ds \frac{d^2w}{dx^2} - 49w = 0 </m>
				</statement>
				<solution><title> Solution </title>
					<p>
						<m> \ds \frac{d^2w}{dx^2} - 49w = 0 </m>
					</p>
				</solution>
				<answer><title>Answer</title>
					<p>
						
					</p>
				</answer>
			</exercise>
		
			<exercise>
				<statement>
					<m> \ds \frac{d^2w}{dx^2} + 49w = 0 </m>	
				</statement>
				<solution><title> Solution </title>
					<p>
						<m> \ds \frac{d^2w}{dx^2} + 49w = 0 </m>	
					</p>
				</solution>
				<answer><title>Answer</title>
					<p>
						
					</p>
				</answer>
			</exercise>
		
			<exercise>
				<statement>
					<m> \ds z''- z' - 42z = 0 </m>
				</statement>
				<solution><title> Solution </title>
					<p>
						<m> \ds z''- z' - 42z = 0 </m>
					</p>
				</solution>
				<answer><title>Answer</title>
					<p>
						
					</p>
				</answer>
			</exercise>
		
		</exercisegroup>
		
		<exercisegroup><title> Find the general solution <m> \ds y(t) </m> for a linear, homogeneous DEwith constant coefficients which has the given characteristic equation </title>
			<exercise>
				<statement>
					<m> \ds (r-1)^2(r+3)(r^2 + 2r + 5)^2 = 0 </m>	
				</statement>
				<solution><title> Solution </title>
					<p>
						<m> \ds (r-1)^2(r+3)(r^2 + 2r + 5)^2 = 0 </m>	
					</p>
				</solution>
				<answer><title>Answer</title>
					<p>
						
					</p>
				</answer>
			</exercise>
		
			<exercise>
				<statement>
					<m> \ds (r+1)^2 (r-6)^3(r^2+1)(r^2 + 4) = 0 </m>
				</statement>
				<solution><title> Solution </title>
					<p>
						<m> \ds (r+1)^2 (r-6)^3(r^2+1)(r^2 + 4) = 0 </m>
					</p>
				</solution>
				<answer><title>Answer</title>
					<p>
						
					</p>
				</answer>
			</exercise>
		
		</exercisegroup>

		<exercisegroup><title> Compute the derivative of each of the following functions </title>
			
			<exercise>
				<statement>
					<m> \, \ds f(x) = \ln x\cos x </m>
				</statement>
				<answer><title>Answer</title>
					<p>
						<line><m> \ds 
					f'(x)	= \left(\frac{1}{x}\right)\cos x + \ln x \left(-\sin x\right) 
									= \frac{\cos x}{x} - \ln x \sin x
					</m></line>
					</p>
				</answer>
			</exercise>
			
		</exercisegroup>

		<exercise label="p3-c1-summary-rq1"><title> Classifying Practice </title>
			<statement>
				<p>
					Select each classification label that applies to the equation
					<me>y'' = y' + 6y</me>
				</p>
			</statement>
			<choices>
				<choice correct="yes">
					<statement>Linear</statement>
					<feedback>Correct, each of the terms are linear.</feedback>
				</choice>
				<choice correct="yes">
					<statement>Homogeneous</statement>
					<feedback>Correct, the constant term is zero.</feedback>
				</choice>
				<choice correct="yes">
					<statement>Constant Coefficients</statement>
					<feedback>Correct, each coefficient is constant.</feedback>
				</choice>
				<choice correct="yes">
					<statement>LHCC</statement>
					<feedback>Correct!</feedback>
				</choice>
			</choices>
		</exercise>

		<exercise label="p3-c1-summary-rq2"><title> Classifying Practice </title>
			<statement>
				<p>
					Select each classification label that applies to the equation
					<me>3y''' + y'- \sin(y) = 0</me>
				</p>
			</statement>
			<choices multiple-correct="yes">
				<choice>
					<statement>Linear</statement>
					<feedback>Incorrect, <m>\sin(y)</m> is a nonlinear term.</feedback>
				</choice>
				<choice>
					<statement>Homogeneous</statement>
					<feedback>Technically, only linear equations can be labeled as homogeneous or not. Since the equation is nonlinear, we do not select it. </feedback>
				</choice>
				<choice>
					<statement>Constant Coefficients</statement>
					<feedback>Technically, only linear equations can be labeled as having constant coefficients or not. Since the equation is nonlinear, we do not select it. </feedback>
				</choice>
				<choice>
					<statement>LHCC</statement>
					<feedback>Incorrect.</feedback>
				</choice>
			</choices>
		</exercise>

		<exercise label="p3-c1-summary-rq3"><title> Classifying Practice </title>
			<statement>
				<p>
					Select each classification label that applies to the equation
					<me>y''- 6 = 0</me>
				</p>
			</statement>
			<choices multiple-correct="yes">
				<choice correct="yes">
					<statement>Linear</statement>
					<feedback>Correct, both terms are linear.</feedback>
				</choice>
				<choice>
					<statement>Homogeneous</statement>
					<feedback>Incorrect, the constant term, <m>6</m>, is non-zero. </feedback>
				</choice>
				<choice correct="yes">
					<statement>Constant Coefficients</statement>
					<feedback>Correct, each coefficient is constant. </feedback>
				</choice>
				<choice>
					<statement>LHCC</statement>
					<feedback>Incorrect.</feedback>
				</choice>
			</choices>
		</exercise>

		<exercise label="p3-c1-summary-rq4"><title> Classifying Practice </title>
			<statement>
				<p>
					Select each classification label that applies to the equation
					<me>\frac{d^3y}{dt^3} + k\frac{dy}{dt} = ty, \qquad k \text{ is constant}</me>
				</p>
			</statement>
			<choices multiple-correct="yes">
				<choice correct="yes">
					<statement>Linear</statement>
					<feedback>Correct, all terms are linear.</feedback>
				</choice>
				<choice correct="yes">
					<statement>Homogeneous</statement>
					<feedback>Correct, the constant term is zero. </feedback>
				</choice>
				<choice>
					<statement>Constant Coefficients</statement>
					<feedback>Incorrect, the <m>y</m> term coefficient, <m>t</m>, is not constant. </feedback>
				</choice>
				<choice>
					<statement>LHCC</statement>
					<feedback>Incorrect.</feedback>
				</choice>
			</choices>
		</exercise>
	
	</exercises>

</subsection> 