<exercises>
<title>Exercises</title>
	
<exercisegroup>
	<title> Find the general solution for each of the following </title>
		<exercise>
			<statement>
				<m> \ds 4y'' -36y' = 0 </m>
			</statement>
			<solution><title> Solution </title>
				<p>
					<m> </m>
				</p>
			</solution>
			<answer>
				
			</answer>
		</exercise>
	
		<exercise>
			<statement>
				<m> \ds 4y'' -36y = 0. </m>
			</statement>
			<solution><title> Solution </title>
				<p>
					<m> </m>
				</p>
			</solution>
			<answer>
				
			</answer>
		</exercise>
	
		<exercise>
			<statement>
				<m> \ds y''- y' - 11y = 0 </m>
			</statement>
			<solution><title> Solution </title>
				<p>
					<m> </m>
				</p>
			</solution>
			<answer>
				
			</answer>
		</exercise>
	
		<exercise>
			<statement>
				<m> \ds 2\frac{d^2 \theta}{dt^2} -6\frac{d\theta}{dt} - 8\theta = 0 </m>
			</statement>
			<solution><title> Solution </title>
				<p>
					
				</p>
			</solution>
			<answer>
				
			</answer>
		</exercise>
	
	</exercisegroup>
	
	<exercisegroup>
	<title> Solve the following initial value problems </title>
		<exercise>
			<statement>
				<m> \ds 4y'' -36y = 0 \hspace{1cm} c_1 </m> an <m> \ds c_2 </m> that satisfy thegiven initial conditions.
			</statement>
			<solution><title> Solution </title>
				 We already have the general solution <m> \ds y = c_1e^{3t} + c_2e^{-3t} </m> .  In order to use the initial conditions, we will eventually need the first derivative, so let's find that now. <m> \ds y' = 3c_1e^{3t} -3 c_2e^{-3t} </m> Now we can see what comes of the first initial condition <m> \ds y(0) = 4. </m>
				<md>
					<mrow>  y(0)	 															\amp =  4 </mrow>
					<mrow>  c_1e^{3\cdot 0} + c_2e^{-3\cdot 0}	\amp =  4 </mrow>
					<mrow>  c_1 + c_2	 													\amp =  4 </mrow>
				</md>
				 Now we can use the other initial condition <m> \ds y'(0) = -6. </m>
				<md>
					<mrow>  y'(0)	 																\amp =  -6 </mrow>
					<mrow>  3c_1e^{3\cdot 0} -3 c_2e^{-3\cdot 0}	\amp =  -6 </mrow>
					<mrow>  3c_1 - 3c_2	 													\amp =  -6 </mrow>
				</md>
				 Notice that the resulting equations, (\ref{eq7}) and (\ref{eq8}) constitute a system of two linear equations in two unknowns, and we should be able to solve for the unknown <m> \ds c_1 </m> an <m> \ds c_2 </m> .  There are multiple ways to achieve this.  One possibility is to solve fo <m> \ds c_2 </m> in equation (\ref{eq7}) and then substitute into equation (\ref{eq8}) as follows.
				<md>
					<mrow>  c_2	 							\amp =  4 - c_1	</mrow>
					<mrow>  3c_1 - 3(4 - c_1)	\amp = -6 			</mrow>
					<mrow>  3c_1 - 12 + 3c_1	\amp = -6 			</mrow>
					<mrow>  6c_1 - 12					\amp = -6 			</mrow>
					<mrow>  6c_1							\amp =  6 			</mrow>
					<mrow>  c_1	 							\amp =  1 			</mrow>
					<mrow>  c_2	 							\amp =  4 - 1 	</mrow>
					<mrow>   									\amp =  3 			</mrow>
				</md>
				 Hence, we have the solution <m> \ds y = e^{3t} + 3e^{-3t}. </m> <em> Note:  it's not clear whether the independent variable i <m> \ds x </m> o <m> \ds t </m> , so you could replace th <m> \ds t </m> 's wit <m> \ds x </m> 's.</em>
			</solution>
			<answer>
				<m> \ds y = e^{3t} + 3e^{-3t} </m> o <m> \ds y = e^{3x} + 3e^{-3x} </m>
			</answer>
		</exercise>
	
		<exercise>
			<statement>
				<m> \ds \ds 2\frac{d^2 \theta}{dt^2} -6\frac{d\theta}{dt} - 8\theta = 0,\hspace{1cm} \theta(0) = 12, \hspace{1cm} \theta'(0) = -2 </m>
			</statement>
			<solution><title> Solution </title>
				<p>
					
				</p>
			</solution>
			<answer>
				
			</answer>
		</exercise>
	
	</exercisegroup>
	
	<exercisegroup>
		<exercise>
			<statement>
				 Solve the following boundary value problem.<m> \ds y'' - y = 0, \hspace{1cm} y(0) = 1, \hspace{1cm} y(1) = 2e- \frac{1}{e}</m>
			</statement>
			<solution><title> Solution </title>
				We begin by verifying the following: 
				 <line>  the DE is linear, </line>
				 <line>  the DE is homogeneous, and </line>
				 <line>  the DE has constant coefficients. </line>
				 Since all of the conditions are true, we can safely proceed to find the general solution.  We write down and then solve the characteristic equation, as follows.
				<md>
					<mrow>  r^2 - 1	 	\amp =  0 						</mrow>
					<mrow>  r^2	 			\amp =  1 						</mrow>
					<mrow>  r	 				\amp =  \pm \sqrt{1} 	</mrow>
					<mrow>  r	 				\amp =  \pm 1 				</mrow>
	 
				</md>
				Since <m> \ds r = 1 </m> an <m> \ds r = -1 </m> are distinct, real roots, the general solution is given by <m> \ds y = c_1e^{t} + c_2e^{-t}. </m> Now we can see what comes of the first boundary condition <m> \ds y(0) = 1. </m>
				<md>
					<mrow>  y(0)	 \amp =  1 </mrow>
					<mrow>  c_1e^{0} + c_2e^{-0}	 \amp =  1 </mrow>
					<mrow>  c_1 + c_2	 \amp =  1  </mrow>
				</md>
				Now we can use the other boundary condition <m> \ds y(1) = 2e- \frac{1}{e}. </m>
				<md>
					<mrow>  y(1)	 \amp =  2e- \frac{1}{e} </mrow>
					<mrow>  c_1e^{1} + c_2e^{-1}	 \amp =  2e- \frac{1}{e} </mrow>
					<mrow>  c_1\cdot e + c_2\cdot \frac{1}{e}	 \amp =  2e- \frac{1}{e}  </mrow>
				</md>
				Notice that the resulting equations, (\ref{eq11}) and (\ref{eq12}) constitute a system of two linear equations in two unknowns, and we should be able to solve for the unknown <m> \ds c_1 </m> an <m> \ds c_2 </m> .  There are multiple ways to achieve this.  One possibility is to solve fo <m> \ds c_2 </m> in equation (\ref{eq11}) and then substitute into equation (\ref{eq12}) as follows.
				<md>
					<mrow>  c_2	 \amp =  1 - c_1 </mrow>
					<mrow>  c_1\cdot e + (1 - c_1)\cdot \frac{1}{e}	 \amp =  2e- \frac{1}{e} </mrow>
					<mrow>  c_1\cdot e + \frac{1}{e} - c_1\cdot \frac{1}{e}	 \amp =  2e- \frac{1}{e} </mrow>
					<mrow>  c_1\cdot e - c_1\cdot \frac{1}{e}	 \amp =  2e - \frac{2}{e} </mrow>
					<mrow>  c_1\left(e - \frac{1}{e}  \right)	 \amp =  2e - \frac{2}{e} </mrow>
					<mrow>  c_1	 \amp =  \frac{2e - \frac{2}{e}}{e - \frac{1}{e}} </mrow>
					<mrow>   \amp =  \frac{2e - \frac{2}{e}}{e - \frac{1}{e}} \cdot \frac{e}{e} </mrow>
					<mrow>   \amp =  \frac{2e^2 - 2}{e^2 - 1} </mrow>
					<mrow>   \amp =  \frac{2(e^2 - 1)}{e^2 - 1} </mrow>
					<mrow>   \amp =  2 </mrow>
					<mrow>  c_2	 \amp =  1 - 2 </mrow>
					<mrow>   \amp =  -1  </mrow>
				</md>
				 Hence, we have the solution <m> \ds y = 2e^{t} - e^{-t}. </m>
			</solution>
			<answer>
				<m> \ds y = 2e^{t} - e^{-t} </m>
			</answer>
		</exercise>
	
	</exercisegroup>
	
	<exercisegroup>
	<title> Solve the following DEs </title>
		<exercise>
			<statement>
				<m> \ds w'' + 6w' + 9w = 0 </m>
			</statement>
			<solution><title> Solution </title>
				<p>
					<m> \ds w'' + 6w' + 9w = 0 </m>
				</p>
			</solution>
			<answer>
				
			</answer>
		</exercise>
	
		<exercise>
			<statement>
				<m> \ds m'' = 2m' - m </m>
			</statement>
			<solution><title> Solution </title>
				<p>
					<m> \ds m'' = 2m' - m </m>
				</p>
			</solution>
			<answer>
				
			</answer>
		</exercise>
	
	</exercisegroup>
	
	<exercisegroup>
		<exercise>
			<statement>
				 Solve the following initial value problem.<m> \ds \frac{d^2z}{dx^2} - 4\frac{dz}{dx} + 4z = 0, \hspace{0.5cm} z(1) = 1, \hspace{0.5cm} z'(1) = 1</m>
			</statement>
			<solution><title> Solution </title>
				 We begin by verifying the following: 
				 <line>  the DE is linear, </line>
				 <line>  the DE is homogeneous, and </line>
				 <line>  the DE has constant coefficients. </line>
	 Since all of the conditions are true, we can safely proceed by writing the characteristic equation and then solving it (either by factoring or using the quadratic equation).
				<md>
					<mrow>  r^2 - 4r + 4	\amp =  0 </mrow>
					<mrow>  (r-2)(r-2)		\amp =  0 </mrow>
					<mrow>  r	 						\amp =  2 \mbox{ (double root)}  </mrow>
				</md>
				 Sinc <m> \ds r=2 </m> is a repeated real root, the general solution is
				<md>
					<mrow>  z	\amp =  c_1e^{2x} + c_2xe^{2x} </mrow>
					<mrow>  	\amp =  (c_1 + c_2x)e^{2x} </mrow>
	 
				</md>
				 In order to use the initial conditions, we will eventually need the first derivative, so let's find that now.  Note that we will use the product rule to take the derivative.
				<md>
					<mrow>  z'	\amp =  (c_1+ c_2x)\cdot 2e^{2x} + c_2 \cdot e^{2x} 	</mrow>
					<mrow>   		\amp =  (2c_1+ 2c_2x)e^{2x} + c_2e^{2x} 							</mrow>
					<mrow>   		\amp =  (2c_1 + 2c_2x + c_2)e^{2x} 										</mrow>
	 
				</md>
				 Now we can see what comes of the first initial condition <m> \ds z(1) = 1. </m>
				<md>
					<mrow>  z(1)	 \amp =  1 </mrow>
					<mrow>  (c_1 + c_2\cdot 1)e^{2\cdot 1}	 \amp =  1 </mrow>
					<mrow>  (c_1 + c_2)e^{2}	 \amp =  1 </mrow>
					<mrow>  c_1 + c_2	 \amp =  \frac{1}{e^2} </mrow>
					<mrow>  c_1 + c_2	 \amp =  e^{-2}  </mrow>
				</md>
				 Now we can use the other initial condition <m> \ds \theta'(0) = -2. </m>
				<md>
					<mrow>  z'(1)	 \amp =  1 </mrow>
					<mrow>  (2c_1 + 2c_2\cdot 1 + c_2)e^{2\cdot 1}	 \amp =  1 </mrow>
					<mrow>  (2c_1 + 3c_2)e^{2}	 \amp =  1 </mrow>
					<mrow>  2c_1 + 3c_2	 \amp =  \frac{1}{e^2} </mrow>
					<mrow>  2c_1 + 3c_2	 \amp =  e^{-2}  </mrow>
				</md>
				 Notice that the resulting equations, (\ref{eq13}) and (\ref{eq14}) constitute a system of two linear equations in two unknowns, and we should be able to solve for the unknown <m> \ds c_1 </m> and <m> \ds c_2 </m> .  There are multiple ways to achieve this.  One possibility is to solve for <m> \ds c_2 </m> in equation (\ref{eq13}) and then substitute into equation (\ref{eq14}) as follows.
				<md>
					<mrow>  c_2	 \amp =  e^{-2} - c_1 </mrow>
					<mrow>  2c_1 +3(e^{-2} - c_1)	 \amp =  e^{-2} </mrow>
					<mrow>  2c_1 +3e^{-2} - 3c_1	 \amp =  e^{-2} </mrow>
					<mrow>  -c_1 + 3e^{-2}	 \amp =  e^{-2} </mrow>
					<mrow>  -c_1	 \amp =  e^{-2} - 3e^{-2} </mrow>
					<mrow>  -c_1	 \amp =  - 2e^{-2} </mrow>
					<mrow>  c_1	 \amp =  2e^{-2} </mrow>
					<mrow>  c_2	 \amp =  e^{-2} - 2e^{-2} </mrow>
					<mrow>   \amp =  -e^{-2} </mrow>
	 
				</md>
				 Hence, we have the solution
				<md>
					<mrow>  z		\amp =  (2e^{-2} - e^{-2}x)e^{2x}, \mbox{ or}	</mrow>
					<mrow>   		\amp =  (2 - x)e^{-2}e^{2x}, \mbox{ or} 			</mrow>
					<mrow>   		\amp =  (2 - x)e^{-2 + 2x}, \mbox{ or} 				</mrow>
					<mrow>   		\amp =  (2 - x)e^{2x - 2}. 										</mrow>
	 
				</md>
				
			</solution>
			<answer>
				<m> \ds z = (2e^{-2} - e^{-2}x)e^{2x} </m> or <m> \ds z = (2 - x)e^{2x - 2} </m>
			</answer>
		</exercise>
	
	</exercisegroup>
	
	<exercisegroup>
	<title> Solve the following DEs </title>
		<exercise>
			<statement>
				<m> \ds y'' + 4y' + 53y = 0 </m>
			</statement>
			<solution><title> Solution </title>
				<p>
					<m> \ds y'' + 4y' + 53y = 0 </m>
				</p>
			</solution>
			<answer>
				
			</answer>
		</exercise>
	
		<exercise>
			<statement>
				<m> \ds z''=-36z </m>
			</statement>
			<solution><title> Solution </title>
				<p>
					<m> \ds z''=-36z </m>
				</p>
			</solution>
			<answer>
				
			</answer>
		</exercise>
	
	</exercisegroup>
	
	<exercisegroup>
	<title> Solve the following DEs </title>
		<exercise>
			<statement>
				<m> \ds y'' = -24y' - 144y </m> 
			</statement>
			<solution><title> Solution </title>
				<p>
					<m> \ds y'' = -24y' - 144y </m> 
				</p>
			</solution>
			<answer>
				
			</answer>
		</exercise>
	
		<exercise>
			<statement>
				<m> \ds \frac{d^2w}{dx^2} - 49w = 0 </m>
			</statement>
			<solution><title> Solution </title>
				<p>
					<m> \ds \frac{d^2w}{dx^2} - 49w = 0 </m>
				</p>
			</solution>
			<answer>
				
			</answer>
		</exercise>
	
		<exercise>
			<statement>
				<m> \ds \frac{d^2w}{dx^2} + 49w = 0 </m>	
			</statement>
			<solution><title> Solution </title>
				<p>
					<m> \ds \frac{d^2w}{dx^2} + 49w = 0 </m>	
				</p>
			</solution>
			<answer>
				
			</answer>
		</exercise>
	
		<exercise>
			<statement>
				<m> \ds z''- z' - 42z = 0 </m>
			</statement>
			<solution><title> Solution </title>
				<p>
					<m> \ds z''- z' - 42z = 0 </m>
				</p>
			</solution>
			<answer>
				
			</answer>
		</exercise>
	
	</exercisegroup>
	
	<exercisegroup>
	<title> Find the general solution <m> \ds y(t) </m> for a linear, homogeneous DEwith constant coefficients which has the given characteristic equation </title>
		<exercise>
			<statement>
				<m> \ds (r-1)^2(r+3)(r^2 + 2r + 5)^2 = 0 </m>	
			</statement>
			<solution><title> Solution </title>
				<p>
					<m> \ds (r-1)^2(r+3)(r^2 + 2r + 5)^2 = 0 </m>	
				</p>
			</solution>
			<answer>
				
			</answer>
		</exercise>
	
		<exercise>
			<statement>
				<m> \ds (r+1)^2 (r-6)^3(r^2+1)(r^2 + 4) = 0 </m>
			</statement>
			<solution><title> Solution </title>
				<p>
					<m> \ds (r+1)^2 (r-6)^3(r^2+1)(r^2 + 4) = 0 </m>
				</p>
			</solution>
			<answer>
				
			</answer>
		</exercise>
	
		</exercisegroup>

</exercises>