<section xmlns:xi="http://www.w3.org/2001/XInclude"><title> General Solutions </title>

	<p>
		In any nonhomogeneous differential equation, the solution should, to some extent, resemble the right-hand side and we can logically guess what function the solution should look like. Yet, hidden within the overall solution could be terms that cancel out each other, affecting only the structure without contributing directly to the right-hand side.
	</p>

	<p>
		To explore this, consider the following linear nonhomogeneous constant coefficient (LNCC) equation alongside its homogeneous counterpart:
		<mdn>
			<mrow xml:id="lncc-eqn1"> y'' - 4y' + 3y =\amp\ 9x</mrow>
			<mrow xml:id="lncc-eqn2"> y'' - 4y' + 3y =\amp\ 0</mrow>
		</mdn>.
		We already know that <m>y = 3x + 4</m> is a solution to the nonhomogeneous equation <xref ref="lncc-eqn1" />, while the solution to the homogeneous equation <xref ref="lncc-eqn2" /> is <m>y = c_1e^{x} + c_2e^{3x}</m>. Let's plug these solutions into their respective equations:
		<md>
			<mrow> 
				3x+4 \quad \os{\text{into}}{\longrightarrow} \quad \amp y'' - 4y' + 3y  \quad \os{\text{simplifies to}}{\longrightarrow}  \quad 9x
			</mrow>
			<mrow> 
				c_1e^{x} + c_2e^{3x} \quad \os{\hphantom{\text{into}}}{\longrightarrow} \quad \amp y'' - 4y' + 3y  \quad \os{\hphantom{\text{simplifies to}}}{\longrightarrow}  \quad 0
			</mrow>
			<mrow>
				c_1e^{x} + c_2e^{3x} + 3x + 4 \quad \os{\hphantom{\text{into}}}{\longrightarrow} \quad \amp y'' - 4y' + 3y \quad \os{\hphantom{\text{simplifies to}}}{\longrightarrow} \quad \, ?
			</mrow>
		</md>
		Now, what happens if we combine these solutions into one?
	</p>

	<p>
		Given that derivatives distribute over addition, the homogeneous terms will simplify to zero, and the particular terms will simplify to <m>9x</m>, as they did individually. Therefore, the combined solution <m>y = c_1e^{x} + c_2e^{3x} + 3x + 4</m> must be a valid solution to the nonhomogeneous equation <xref ref="lncc-eqn1" />.
	</p>

	<p>
		This leads us to the fundamental principle of LNCC equations: the general solution is made up of two parts:
		<me>
			y = \ub{c_1e^{x} + c_2e^{3x}}_{\text{homogeneous part}} + \ub{3x + 4}_{\text{particular part}}
		</me>
		Here, the <em>homogeneous part</em> (<m>y_h</m>) cancels out when substituted into the original equation, while the <em>particular part</em> (<m>y_p</m>) accounts for the non-zero right-hand side.
	</p>
	
	<p>
		<assemblage xml:id="lncc-general-solution-parts"><title>LNCC General Solution Parts</title>
			<p>
				The linear nonhomogeneous constant coefficient (LNCC) equation 
				<men xml:id="lncc-general-equation">
					a_n y^{(n)} + \cdots + a_1 y' + a_0 y = f(x)
				</men>
				has a solution with a <term>homogeneous</term> and <term>particular</term> part given by
				<men xml:id="lncc-general-solution">
					y = y_h + y_p
				</men>.
				where <m>y_h</m>, found by solving the LHCC equation
				<me>
					a_n y^{(n)} + \cdots + a_2 y'' + a_1 y' + a_0 y = 0
				</me>,
				contains the terms of the solution that cancel out, whereas, <m>y_p</m> contains the terms that simplify to <m>f(x)</m> when <xref ref="lncc-general-solution"/> is plugged into <xref ref="lncc-general-equation"/>
			</p>
		</assemblage>
	</p>


	<example>
		<m>\ \ </m> Find the general solution to the differential equation

		<p>
			<me>
				y'' - 4y' - 12y = 3{e^{5t}}
			</me>
			given that the the particular solution is known to be <m>y_p(t) =  -\frac{3}{7}{{e}^{5t}}</m>.
		</p>
		<solution>
			<p>
				The general solution has the form:
				<me>y = y_h + y_p</me>
				Since <m>y_p</m> is given, we only need to solve the homogeneous equation:
				<me>y'' - 4y' - 12y = 0</me>
				Using the characteristic equation:
				<md>
					<mrow> r^2 - 4r - 12 	=\amp\ 0											</mrow>
					<mrow> (r - 6)(r + 2) 	=\amp\ 0 \quad \Rightarrow \quad r_1 = 6, r_2 = -2	</mrow>
				</md>
				The homogeneous solution is:
				<me> y_h(t) = c_1e^{-2t} + c_2e^{6t} </me>
				Therefore, the general solution is:
				<me> y = c_1e^{-2t} + c_2e^{6t} -\frac{3}{7}{e^{5t}} </me>
			</p>
		</solution>
	</example>

	<p>
		Before we can tackle solving these equations from scratch, we need a strategy for finding the particular solution <m>y_p</m>, which will be covered in the upcoming sections.
	</p>

	<xi:include href="./p3-c2-s2-interactives.ptx" />

</section>