<section xmlns:xi="http://www.w3.org/2001/XInclude"><title> Antiderivatives </title>

	<p>
		When you find an antiderivative, you're actually solving a basic differential equation. For example, consider finding the general antiderivative of <m>x^2</m>. The calculus approach would compute the integral
		<me>
			\int x^2\ dx = \frac13 x^3 + C
		</me>.
		The differential equations approach, on the other hand, seeks all functions whose derivative is <m>x^2</m>. This means solving for <m>y</m> in the equation:
		<men xml:id="antiderivative-eqn">\frac{d}{dx}[y] = x^2</men>
		Note, we could also express this equation in the following equivalent ways:
		<me>\frac{dy}{dx} = x^2 \quad \text{or} \quad y^\prime = x^2</me>.
	</p>
		
	<p>
		To solve for <m>y</m>, we integrate both sides with respect to <m>x</m>, like so:
		<md>
			<mrow> \int\frac{d}{dx}[y]\ dx	\amp = \int x^2\ dx				</mrow>
			<mrow> 					y + C_1	\amp = \frac13 x^3 + C_2		</mrow>
			<mrow> 						y	\amp = \frac13 x^3 + C_2-C_1 \quad \implies \quad y = \frac13 x^3 + C	</mrow>
		</md>
		where <m>C = C_2-C_1</m> is a constant.
		<fn>
			Combining constants like this is a common practice in differential equations and is something you'll see often in this text.
		</fn>
		Although this method might seem excessive for simple problems, it illustrates the core concept of isolating the dependent variable and expressing it in terms of the independent variable, <m>x</m>.
	</p>

	<example xml:id="antiderivative-example"><title> Solve by Antiderivatives </title>

		<statement>
			<p>
				Solve the differential equation
			</p>
			<me> 2y' - 4\sin x = 2, \quad y(0) = 5 </me>
			
		</statement>

		<solution>
			
			<p>
				Start by isolating the derivative, <m>y'</m>, on one side of the equation
				<md>
					<mrow> y' \amp = 1 + 2 \sin x </mrow>.
				</md>
				Integrate both sides with respect to <m>x</m> to leave us with <m>y</m> on the left side
				<md>
					<mrow> \int y'\ dx 	\amp = \int \left(1 + 2 \sin x\right) \ dx 				</mrow>
					<mrow> 	y + C_1 	\amp = x - 2 \cos x + C_2 								</mrow>
					<mrow> 			y 	\amp = x - 2 \cos x + \fbox{\(C_2 - C_1\)}\leftarrow C	</mrow>
					<mrow> 		y(x)	\amp  = x - 2 \cos x + C 								</mrow>.
				</md>
			</p>

			<p>
				Finally, apply the initial condition <m>y(0) = 5</m> to find <m>C</m>
				<md>
					<mrow> 				y(0)	\amp = 5 </mrow>
					<mrow> (0) - 2 \cos(0) + C	\amp = 5 </mrow>
					<mrow> 			0 - 2 + C	\amp = 5 </mrow>
					<mrow> 					C	\amp = 7 </mrow>.
				</md>
				Thus, the solution to the differential equation is <m>\quad y = x - 4 \cos x + 7 </m>.
			</p>
				

		</solution>

	</example>

	<xi:include href="./p2-c1-s1-interactives.ptx" />
  
</section>