<exercises><title> Step-By-Step Exercises </title>

	<example xml:id="de-two-solutions">

		<statement>
			<p>
				Verify if both <m>y= 2e^{-3t}</m> and <m>y= e^{4t}</m> are solutions to 
				<me>y'' - y' - 12y = 0</me>.
			</p>
		</statement>

		<solution>
			<p>
				Find <m>y'</m> and <m>y''</m> since they appear in the equation.
				<md>
					<mrow>	y	=\amp\  2e^{-3t}								</mrow>
					<mrow>	y' 	=\amp\  2e^{-3t}\left(-3\right)	=	-6e^{-3t}	</mrow>
					<mrow>	y'' =\amp\ -6e^{-3t}\left(-3\right)	=	18e^{-3t}	</mrow>
				</md>
			</p>

			<p>
				Plug <m>y, y',</m> and <m>y''</m> into the DE and simplify.
				<md>
					<mrow> 													y'' - y' - 12y	=\amp\ 0									</mrow>
					<mrow> 18e^{-3t} - \left( -6e^{-3t} \right) - 12\left( 2e^{-3t} \right)	=\amp\ 0									</mrow>
					<mrow> 								18e^{-3t} + 6e^{-3t} - 24e^{-3t}	=\amp\ 0									</mrow>
					<mrow> 																0	=\amp\ 0	\quad✅	</mrow>
				</md>
				Therefore, <m>y= 2e^{-3t}</m> is a solution to <m>y'' - y' - 12y = 0.</m>
			</p>
		
			<p>
				Find <m>y'</m> and <m>y''</m> since they appear in the DE.
				<md>
					<mrow>	y	=\amp\  e^{4t}								</mrow>
					<mrow>	y' 	=\amp\  e^{4t}\left(4\right)	=	4e^{4t}	</mrow>
					<mrow>	y'' =\amp\ 4e^{4t}\left(4\right)	=	16e^{4t}</mrow>
				</md>
			</p>

			<p>
				Plug <m>y, y',</m> and <m>y''</m> into the DE and simplify.
				<md>
					<mrow> 								y'' - y' - 12y	=\amp\ 0									</mrow>
					<mrow> 16e^{4t} - 4e^{4t} - 12\left( e^{4t} \right)	=\amp\ 0									</mrow>
					<mrow> 				16e^{4t} - 4e^{4t} - 12e^{4t}	=\amp\ 0									</mrow>
					<mrow> 											0	=\amp\ 0	\quad✅	</mrow>
				</md>
				Therefore, <m>y= e^{4t}</m> is a solution to <m>y'' - y' - 12y = 0.</m>
			</p>
		</solution>

	</example>

	<example>

		<statement>
			<p>
				Verify if <m>\ds\ y = 3\sin(x^2) </m> is a solution to 
				<me>y' - xy'' = 12x^2\sin(x^2)</me>.
			</p>
		</statement>

		<solution>
			<p>
				Find <m>y'</m> and <m>y''</m> since they appear in the equation and move all terms to the left-side.
				<md>
					<mrow>	y	=\amp\  3\sin(x^2)									</mrow>
					<mrow>	y' 	=\amp\  3\cos(x^2) \cdot 2x	=	6x\cos(x^2)	</mrow>
					<mrow>	y'' =\amp\ 6\cos(x^2) - 12x\sin(x^2)	=	6\cos(x^2) - 12x\sin(x^2)	</mrow>
				</md>
			</p>

			<p>
				Plug in <m>y, y',</m> and <m>y''</m> and simplify.
				<md>
					<mrow> 												
						y' - xy'' - 12x^2\sin(x^2) 	
							=\amp\ 0	
					</mrow>
					<mrow> 
						6x\cos(x^2) - x\left( 6\cos(x^2) - 12x\sin(x^2) \right) - 12x^2\sin(x^2)
							=\amp\ 0																
					</mrow>
					<mrow> 
						\cancel{6x\cos(x^2)} - \cancel{6x\cos(x^2)} - \cancel{12x^2\sin(x^2)} - \cancel{12x^2\sin(x^2)}	
							=\amp\ 0
						</mrow>
					<mrow> 
						0	=\amp\ 0
					</mrow>
				</md>
				Therefore, <m>y= 3\sin(x^2)</m> is a solution to <m>y' - 12x^2\sin(x^2) = xy''.</m>
			</p>
		</solution>

	</example>

	<example>
	
		<statement>
			<p>
				Verify that <m>y = Ce^{-5x^2} + \frac{3}{5}</m> is a solution to the DE
				<me>\frac{dy}{dx} = \big( 2x \big) \big( 3 - 5y \big)</me>
			</p>
		</statement>
	
		<solution>
			<p>
				Working out the left and right hand sides of this DE, we have:
	
				<sidebyside widths="45% 55%" margins="auto" valign="top" halign="center">
					<p>
						<md>
							<mrow> LHS: </mrow>
							<mrow> \frac{dy}{dx}
									=\amp\ \frac{d}{dx}\left( Ce^{-5x^2} + \frac{3}{5} \right)</mrow>
							<mrow> 	=\amp\ Ce^{-5x^2} \cdot \frac{d}{dx}(-5x^2) + 0</mrow>
							<mrow> 	=\amp\ Ce^{-5x^2} \cdot -10x</mrow>
							<mrow> 	=\amp\ -10Cxe^{-5x^2}</mrow>
						</md>
					</p>
					<p>
						<md>
							<mrow> RHS: </mrow>
							<mrow> 	\big(2x\big)\amp\big(3 - 5y\big)</mrow>
							<mrow> 	=\amp\ 2x \left[3 - 5\left(Ce^{-5x^2} + \frac{3}{5}\right) \right]</mrow>
							<mrow> 	=\amp\ 2x \left[ 3 - 5Ce^{-5x^2} - 3 \right]</mrow>
							<mrow> 	=\amp\ 2x \left[-5Ce^{-5x^2}\right]</mrow>
							<mrow> 	=\amp\ -10Cxe^{-5x^2}</mrow>
						</md>
					</p>
				</sidebyside>
			</p>
	
			<p>
				Since <m>LHS = RHS</m>, we have verified that
				<m>y = Ce^{-5x^2} + \frac{3}{5}</m> is a solution to
				<me>\frac{dy}{dx} = \big( 2x \big) \big( 3 - 5y \big)</me>
			</p>
		</solution>
	
	</example>

	<example xml:id="antiderivative-example">

		<statement>
			<p>
				Solve the initial-value problem 
				<me>2y' - 4\sin x = 2, \quad y(0) = 5 </me>.
			</p>
		</statement>

		<solution>

			<p>
				Start by isolating the derivative, <m>y'</m>, on one side of the equation
				<md>
					<mrow> y' \amp = 1 + 2 \sin x </mrow>.
				</md>
				Integrate both sides with respect to <m>x</m> to leave us with <m>y</m> on the left side
				<md>
					<mrow> \int y'\ dx 	\amp = \int \left(1 + 2 \sin x\right) \ dx 				</mrow>
					<mrow> 	y + c_1 	\amp = x - 2 \cos x + c_2 								</mrow>
					<mrow> 			y 	\amp = x - 2 \cos x + \boxed{c_2 - c_1}\leftarrow c		</mrow>
					<mrow> 		y(x)	\amp  = x - 2 \cos x + c 								</mrow>.
				</md>
			</p>

			<p>
				Finally, apply the initial condition <m>y(0) = 5</m> to find <m>c</m>
				<md>
					<mrow> 				y(0)	\amp = 5 </mrow>
					<mrow> (0) - 2 \cos(0) + c	\amp = 5 </mrow>
					<mrow> 			0 - 2 + c	\amp = 5 </mrow>
					<mrow> 					c	\amp = 7 </mrow>.
				</md>
				Thus, the solution to the differential equation is <m>\quad y = x - 2 \cos x + 7 </m>.
			</p>

		</solution>

	</example>

</exercises>