<section xmlns:xi="http://www.w3.org/2001/XInclude" xml:id="sec-method-euler"><title> Euler's Method </title>

	<objectives>
		<introduction>
			<p>
				After this chapter, you will be able to ...
			</p>
		</introduction>
		<ol>
			<li>  </li>
			<li>  </li>
			<li>  </li>
		</ol>
	</objectives>

	<introduction>
		<p>
			Euler's method operates on a very intuitive principle: starting from an initial point, the method uses the differential equation itself to take small steps along the direction of the slope given by the equation. At each step, the method calculates the slope of the unknown function at the current point, then moves a small distance in the direction of this slope to find the next point. By repeating this process, Euler's method generates a sequence of points that approximates the true solution curve of the differential equation.
		</p>
	
		<exploration xml:id="euler-method"><title> Euler's Method </title>
			<p>
				An approximate solution to the first order differential equation
				<men xml:id="euler-method-de">
					y' = f(x, y), \quad y(a) = y_0 
				</men>
				can be found on the interval <m>[a, b]</m> through the following steps...
			</p>
			<dl width="narrow">
				<li xml:id="euler-step1"><title>Step 1: Set-up </title>
					<p>
						<line>Choose <m>h</m>.</line>
						<line>Break <m>[a, b]</m> into
						<m>
							x_0,\ x_1,\ x_2,\ ...,\ x_{N-1},\ x_{N},
						</m>
						separated by <m>h</m>.
						</line>
					</p>
				</li>
				<li xml:id="euler-step2"><title>Step 2: Find Approximation Formula <m>y_{i+1}</m> </title>
					<p>
						<line>Substitute <m>x_i</m> into <xref ref="euler-method-de"/> &amp; rewrite <m>y(x_i)</m> as <m>y_i</m> and <m>y^\prime(x_i)</m> as <m>y^\prime_i</m>.</line>
						<line>Replace <m>y^\prime_i</m> with <m>\frac{1}{h}(y_{i+1} - y_{i})</m>.</line>
						<line>Isolate <m>y_{i+1}</m>.</line>
					</p>
				</li>
				<li xml:id="euler-step3"><title>Step 3: Compute Approximation Values </title>
					<p>
						<line>Find <m>y_1, y_2, ... , y_N</m> using the approximation formula.</line>
					</p>
				</li>
			</dl>
		</exploration>
		
		<p>
			Use Euler's Method to approximate the solution to the initial-value problem,

			<mdn>
				<mrow xml:id="euler-ex-01-de">	y'(x) - 2xy(x) = 0	\amp </mrow>
				<mrow xml:id="euler-ex-01-ic">	y(0) = 2, \amp </mrow>
			</mdn>
			at the <m>x</m>-values <m>0,\ 0.5,\ 1,\ 1.5,\ 2 \ </m>(spaced 0.5 apart).
		</p>

		<p>
			Euler's method works by replacing <m>y'(x)</m> in <xref ref="euler-ex-01-de"/> with it's forward-difference approximation, giving us 
			<me>
				\frac{1}{h}\Big(y(x+h) - y(x)\Big) - 2 xy(x) = 0
			</me>
			and if we let <m>h</m> be the space between the <m>x</m>-values (0.5), then we have
			<me>
				\frac{1}{0.5}\Big(y(x+0.5) - y(x)\Big) - 2 xy(x) = 0.
			</me>
		</p>

		<p>
			To see how this is helpful, we isolate <m>y'(x+h)</m> as follows
			<md>
				<mrow>	\frac{1}{0.5}\Big(y(x+0.5) - y(x)\Big) 	=\ \amp 2 xy(x)	</mrow>
				<mrow>							y(x+0.5) - y(x)	=\ \amp xy(x)	</mrow>
			</md>
			and the final step gives the approximation formula
			<men xml:id="euler-ex-01-approx">
				y(x+0.5) = y(x) + xy(x).
			</men>
		</p>

		<p>
			Note that we already know <m>y(0) = 2</m> from <xref ref="euler-ex-01-ic"/>, so to find the rest of the approximation points, we plug <m>x = 0, 0.5, 1, 1.5</m> into <xref ref="euler-ex-01-approx"/>, as shown below.
		</p>

		<p>
			<tabular top="major" valign="top">
				<col width="0%" />
				<col width="45%" />
				<col width="20%" />
				<row bottom="minor">
					<cell> <m>x</m> </cell>
					<cell halign="center"> Approximation Formula <xref ref="euler-ex-01-approx"/> </cell>
					<cell> Approximation </cell>
				</row>
				<row bottom="minor">
					<cell> <m>0</m> </cell>
					<cell halign="left"> 
						<line><m>y(0+0.5) = y(0) + (0)y(0)</m></line>
						<line><m>\phantom{y(0+0.5)} = 2 + (0)(2) </m></line>
						<line><m>\phantom{y(0+0.5)} = 2 </m></line>
					</cell>
					<cell> <m>y(0.5) = 2</m> </cell>
				</row>

				<row bottom="minor">
					<cell> <m>0.5</m> </cell>
					<cell halign="left"> 
						<line><m>y(0.5+0.5) = y(0.5) + (0.5)y(0.5)</m></line>
						<line><m>\phantom{y(0.5+0.5)} = 2 + (0.5)(2) </m></line>
						<line><m>\phantom{y(0.5+0.5)} = 3 </m></line>
					</cell>
					<cell> <m>y(1) = 3</m> </cell>
				</row>

				<row bottom="minor">
					<cell> <m>1</m> </cell>
					<cell halign="left"> 
						<line><m>y(1+0.5) = y(1) + (1)y(1)</m></line>
						<line><m>\phantom{y(1+0.5)} = 3 + (1)(3) </m></line>
						<line><m>\phantom{y(1+0.5)} = 6 </m></line>
					</cell>
					<cell> <m>y(1.5) = 6</m> </cell>
				</row>

				<row bottom="major">
					<cell> <m>1.5</m> </cell>
					<cell halign="left"> 
						<line><m>y(1.5+0.5) = y(1.5) + (1.5)y(1.5)</m></line>
						<line><m>\phantom{y(1.5+0.5)} = 6 + (1.5)(6) </m></line>
						<line><m>\phantom{y(1.5+0.5)} = 15 </m></line>
					</cell>
					<cell> <m>y(2) = 15</m> </cell>
				</row>
			</tabular>

		</p>


		

	</introduction>

	<xi:include href="method-euler-step-1-verify.ptx" />
	<xi:include href="method-euler-step-2-find-y-approx.ptx" />
	<xi:include href="method-euler-step-3-get-approximation.ptx" />

</section>