<exercises><title> Exercises </title>

	<exercisegroup><title> Step-by-Step </title>

		<introduction>
			<p>
				Maybe write 1 or 2 simple scaffolded problems here?
			</p>
		</introduction>

		<exercise>
			<p>
				<statement>
					Given the differential equation <m> \displaystyle \frac{dy}{dx} = xy^2 </m>, determine if it is separable. If so, rewrite it in the separated form.
				</statement>
				<solution>
					<p>
						The equation is separable because we can write it as:
						<me> \frac{1}{y^2} dy = x dx </me>
					</p>
				</solution>
				<answer>
					<m> \displaystyle \frac{1}{y^2} dy = x dx </m>
				</answer>
			</p>
			<p>
				<statement>
					Continuing from the previous problem, integrate the left side of the separated equation with respect to <m>y</m>.
				</statement>
				<solution>
					<p>
						Integrating <m> \displaystyle \frac{1}{y^2} dy </m> with respect to <m>y</m>, we get:
						<me> -\frac{1}{y} + C_1 </me>
					</p>
				</solution>
				<answer>
					<m> \displaystyle -\frac{1}{y} + C_1 </m>
				</answer>
			</p>
			<p>
				<statement>
					Now, integrate the right side of the separated equation with respect to <m>x</m>.
				</statement>
				<solution>
					<p>
						Integrating <m> x dx </m> with respect to <m>x</m>, we get:
						<me> \frac{1}{2}x^2 + C_2 </me>
					</p>
				</solution>
				<answer>
					<m> \displaystyle \frac{1}{2}x^2 + C_2 </m>
				</answer>
			</p>
			<p>
				<statement>
					Combine the results from the previous exercises to form the general solution to the differential equation.
				</statement>
				<solution>
					<p>
						Equating the two integrals, we get:
						<me> -\frac{1}{y} + C_1 = \frac{1}{2}x^2 + C_2 </me>
						By grouping constants, we can represent them with a single constant:
						<me> -\frac{1}{y} = \frac{1}{2}x^2 + C </me>
						Where <m>C = C_2 - C_1</m>.
					</p>
				</solution>
				<answer>
					<m> \displaystyle -\frac{1}{y} = \frac{1}{2}x^2 + C </m>
				</answer>
			</p>
		</exercise>
	
	</exercisegroup>

	<exercisegroup><title> Warm Up </title>

		<introduction>
			<p>
				Solve using separation of variables, if possible.
			</p>
		</introduction>

		<exercise>
			<statement>
				<p><m> \displaystyle \frac{dy}{dx} = y^2 </m></p>
			</statement>
		</exercise>

		<exercise>
			<statement>
				<p><m> \displaystyle \frac{dy}{dx} = x^2y </m></p>
			</statement>
		</exercise>

		<exercise>
			<statement>
				<p><m> \displaystyle \frac{dy}{dx} = e^{x+y} </m></p>
			</statement>
		</exercise>

		<exercise>
			<statement>
				<p><m> \displaystyle \frac{dy}{dx} = \frac{x}{y} </m></p>
			</statement>
		</exercise>

		<exercise>
			<statement>
				<p><m> \displaystyle \frac{dy}{dx} = \cos(x) \sec(y) </m></p>
			</statement>
		</exercise>

		<exercise>
			<statement>
				<p><m> \displaystyle \frac{dy}{dx} = \frac{2x}{1+y^2} </m></p>
			</statement>
		</exercise>

		<exercise>
			<statement>
				<p><m> \displaystyle \frac{dy}{dx} = 2-y </m></p>
			</statement>
		</exercise>

		<exercise>
			<statement>
				<p><m> \displaystyle \frac{dy}{dx} = \frac{y-x}{y+x} </m></p>
			</statement>
		</exercise>

		<exercise>
			<statement>
				<p><m> \displaystyle \frac{dy}{dx} = y^2 \sec^2(x) </m></p>
			</statement>
		</exercise>

		<exercise>
			<statement>
				<p><m> \displaystyle \frac{dy}{dx} = \frac{1}{xy} </m></p>
			</statement>
		</exercise>

	</exercisegroup>

	<exercisegroup><title> Further Practice </title>

		<introduction>
			<p>
				Solve using separation of variables, if possible.
			</p>
		</introduction>

		<exercise>
			<statement>
				<m> \displaystyle \frac{dy}{dx} = x y </m>
			</statement>
			<solution>
				<md>
					<mrow>  \frac{dy}{y} \amp = x dx </mrow>
					<mrow>  \int \frac{dy}{y} \amp = \int x dx </mrow>
					<mrow>  \ln|y| \amp = \frac{1}{2}x^2 + C_1 </mrow>
					<mrow>  y \amp = Ce^{\frac{1}{2}x^2} </mrow>
				</md>
			</solution>
			<answer>
				<m> \displaystyle y = Ce^{\frac{1}{2}x^2} </m>
			</answer>
		</exercise>

		<exercise>
			<statement>
				<m> \displaystyle \frac{dy}{dx} = \frac{x^2 + 1}{y} </m>
			</statement>
			<solution>
				<md>
					<mrow>  y dy \amp = (x^2 + 1) dx </mrow>
					<mrow>  \int y dy \amp = \int (x^2 + 1) dx </mrow>
					<mrow>  \frac{1}{2}y^2 \amp = \frac{1}{3}x^3 + x + C_1 </mrow>
					<mrow>  y^2 \amp = \frac{2}{3}x^3 + 2x + 2C_1 </mrow>
				</md>
			</solution>
			<answer>
				<m> \displaystyle y^2 = \frac{2}{3}x^3 + 2x + C_2 </m>
			</answer>
		</exercise>

		<exercise>
			<statement>
				<m> \displaystyle \frac{dy}{dx} = \frac{1 - x^2}{y^2} </m>
			</statement>
			<solution>

				<md>
					<mrow>  \frac{dy}{dx}	 \amp =  \frac{1 - x^2}{y^2} </mrow>
					<mrow>  y^2 dy	 \amp =  (1-x^2)dx </mrow>
					<mrow>  \int y^2 dy	 \amp =  \int (1-x^2)dx </mrow>
					<mrow>  \frac{1}{3}y^3	 \amp =  x - \frac{1}{3}x^3 + C_1 </mrow>
					<mrow>  y^3	 \amp =  3x - x^3 + 3C_1 </mrow>
					<mrow>  y	 \amp =  \sqrt[3]{3x - x^3 + 3C_1}, \mbox{ or} </mrow>
					<mrow>  y	 \amp =  \sqrt[3]{3x - x^3 + C_2} </mrow>

				</md>
				<em> Note:  since, in general <m> \displaystyle \sqrt[3]{a+b} \ne \sqrt[3]{a} + \sqrt[3]{b} </m> , we CANNOT simplify the solution to <m> \displaystyle y  = \sqrt[3]{3x - x^3} + C.</m> </em>
			</solution>
			<answer>
				<m> \displaystyle y = \sqrt[3]{3x - x^3 + C_2} </m>
			</answer>
		</exercise>

		<exercise>
			<statement>
				<m> \displaystyle y' - 2y = y\sin x </m>
			</statement>
			<solution>

				<md>
					<mrow>  y' - 2y	 \amp =  y\sin x </mrow>
					<mrow>  y'	 \amp =  2y + y\sin x </mrow>
					<mrow>  \frac{dy}{dx}	 \amp =  y(2 + \sin x) </mrow>
					<mrow>  \frac{1}{y} dy	 \amp =  (2 + \sin x)dx </mrow>
					<mrow>  \int \frac{1}{y} dy	 \amp =  \int (2 + \sin x)dx </mrow>
					<mrow>  \ln|y|	 \amp =  2x - \cos x + C_1 </mrow>
					<mrow>  e^{\ln|y|}	 \amp =  e^{2x - \cos x + C_1} </mrow>
					<mrow>  |y|	 \amp =  e^{2x - \cos x}\cdot e^{C_1} </mrow>
					<mrow>  y	 \amp =  \pm e^{2x - \cos x}\cdot e^{C_1} </mrow>
					<mrow>  y	 \amp =  \underbrace{\pm e^{C_1}}_{\scriptsize = C_2}\cdot e^{2x - \cos x} </mrow>
					<mrow>  y	 \amp =  C_2e^{2x - \cos x} </mrow>
				</md>

			</solution>
			<answer>
				<m> \displaystyle y = C_2e^{2x - \cos x}  </m>
			</answer>
		</exercise>

		<exercise>
			<statement>
				<m> \displaystyle x\frac{dv}{dx} = \frac{1-4v^2}{3v} </m>
			</statement>
			<solution>

				<md>
					<mrow>  x\frac{dv}{dx}	 \amp =  \frac{1-4v^2}{3v} </mrow>
					<mrow>  \frac{dv}{dx}	 \amp =  \frac{1-4v^2}{3v}\cdot \frac{1}{x} </mrow>
					<mrow>  \frac{3v}{1-4v^2} dv	 \amp =  \frac{1}{x} dx </mrow>
					<mrow>  \int \frac{3v}{1-4v^2} dv	 \amp =  \int \frac{1}{x} dx </mrow>

				</md>
				For the integral on the left hand side, we will need to do a substitution.  If we le <m> \displaystyle u = 1-4v^2, </m> the <m> \displaystyle du = -8vdv, </m> and therefor <m> \displaystyle -\frac{1}{8}du = vdv. </m>  Then we have the following:
				<md>
					<mrow>  3\int \frac{v}{1-4v^2} dv	 \amp =  \int \frac{1}{x} dx </mrow>
					<mrow>  3\int \underbrace{\frac{1}{1-4v^2}}_{\scriptsize 1/u} \underbrace{vdv}_{\scriptsize -\frac{1}{8}du}  \amp =  \int \frac{1}{x} dx </mrow>
					<mrow>  3\int \frac{1}{u}\cdot -\frac{1}{8}du	 \amp =  \int \frac{1}{x} dx </mrow>
					<mrow>  -\frac{3}{8} \int \frac{1}{u}du	 \amp =  \int \frac{1}{x} dx </mrow>
					<mrow>  -\frac{3}{8} \ln|u|	 \amp =  \ln|x| + C_1 </mrow>
					<mrow>  -\frac{3}{8} \ln|1 - 4v^2|	 \amp =  \ln|x| + C_1 </mrow>
					<mrow>  \ln|1 - 4v^2|	 \amp =  -\frac{8}{3} \left(\ln|x| + C_1\right) </mrow>
					<mrow>  \ln|1 - 4v^2|	 \amp =  -\frac{8}{3}\ln|x| + -\frac{8}{3}C_1 </mrow>
					<mrow>  \ln|1 - 4v^2|	 \amp =  \ln\left(|x|^{-8/3}\right) + -\frac{8}{3}C_1 </mrow>
					<mrow>  \ln|1 - 4v^2|	 \amp =  \ln\left(x^{-8/3}\right) + -\frac{8}{3}C_1  \mbox <m> \hspace{1cm} \displaystyle x^{-8/3} =|x|^{-8/3} </m> )} </mrow>
					<mrow>  e^{\ln|1 - 4v^2|}	 \amp =  e^{\ln\left(x^{-8/3}\right) + -\frac{8}{3}C_1} </mrow>
					<mrow>  |1 - 4v^2|	 \amp =  e^{\ln\left(x^{-8/3}\right)}\cdot e^{-\frac{8}{3}C_1} </mrow>
					<mrow>  |1 - 4v^2|	 \amp =  x^{-8/3}\cdot e^{-\frac{8}{3}C_1} </mrow>
					<mrow>  1 - 4v^2	 \amp =  \pm e^{-\frac{8}{3}C_1}\cdot x^{-8/3} </mrow>
					<mrow>  1 - 4v^2	 \amp =  \underbrace{\pm e^{-\frac{8}{3}C_1}}_{\scriptsize = C_2}\cdot x^{-8/3} </mrow>
					<mrow>  1 - 4v^2	 \amp =  C_2x^{-8/3} </mrow>

				</md>

				<md>
					<mrow>  - 4v^2	 \amp =  C_2x^{-8/3} - 1 </mrow>
					<mrow>  v^2	 \amp =  \frac{C_2}{-4}x^{-8/3} + \frac{1}{4} </mrow>
					<mrow>  v^2	 \amp =  \underbrace{\frac{C_2}{-4}}_{\scriptsize = C_3}x^{-8/3} + \frac{1}{4} </mrow>
					<mrow>  v^2	 \amp =  C_3x^{-8/3} + \frac{1}{4} </mrow>
					<mrow>  v	 \amp =  \pm \sqrt{C_3x^{-8/3} + \frac{1}{4}} </mrow>
				</md>

			</solution>
			<answer>
				<m> \displaystyle v = \pm \sqrt{C_3x^{-8/3} + \frac{1}{4}}  </m>
			</answer>
		</exercise>


		<exercise>
			<statement>
				<m>\displaystyle \frac{dy}{dx} = \frac{4-2x}{3y^2-5} </m>
			</statement>
			<solution>
				When we separate the variables and integrate both sides, we get
				<me> \int (3y^2-5)dy =  \int (4-2x)dx</me>
				<me> y^3-5y=4x-x^2+C </me>
				Since the equation cannot readily be solved for <m>y</m> as an explicit function of <m>x</m>, we are done.
			</solution>
			<answer>
				<m> y^3-5y=4x-x^2+C </m>
			</answer>
		</exercise>

		<exercise>
			<statement>
				<m>\displaystyle \frac{dy}{dx} = 6x(y-1)^{2/3}</m>
			</statement>
			<solution>
				Separation of variables gives:
				<md>
					<mrow>\displaystyle\int  \frac{1}{3(y-1)^2/3} dy = \int 2xdx</mrow>
					<mrow>				(y-1)^1/3\amp=\displaystyle x^2+C</mrow>
					<mrow>				y(x)\amp=\displaystyle 1+(x^2+C)^3</mrow>
				</md>
			</solution>
			<answer>
				<m>\displaystyle y(x)\amp=\displaystyle 1+(x^2+C)^3</m>
			</answer>
		</exercise>

	</exercisegroup>

	<exercisegroup><title> Initial Value Problems </title>

		<introduction>
			<p>
				Solve each of the following initial value problems using separation of variables, if possible.
			</p>
		</introduction>

		<exercise>
			<statement>
				<m>\displaystyle \frac{dy}{dx} = -6xy,  \hspace{0.5cm} y(0)=7.</m>
			</statement>
			<solution>
				Informally, we divide both side of the differential equation by <m>y</m> and multiply each side by <m>dx</m> to get
				<me> \frac{dy}y = -6xdx.	</me>
				<me> \int \frac{dy}y =  \int (-6x)dx</me>
				<me> \ln|y|=-3x^2+C </me>
				<me>\ln|y|=-3x^2+C</me>
				<me>|y|=e^{-3x^2+C}</me>
				<me>y=\pm e^C e^{-3x^2}</me>

				and hence

				<me>y(x) = Ae^{-3x^2} \qquad (A = \pm e^C)</me>

				The condition <m>y(0) = 7</m> yields <m>A =7</m>, so the desired solution is

				<me>y(x) = 7e^{-3x^2}</me>

			</solution>
			<answer>
				<me>y(x) = 7e^{-3x^2}</me>
			</answer>
		</exercise>

		<exercise>
			<statement>
				<m> \displaystyle \frac{dz}{dt} = 2tz^2, \hspace{0.5cm} z(1) = 2 </m>
			</statement>
			<solution>
				First we find the general solution:
				<md>
					<mrow>  \frac{dz}{dt}	 \amp =  2tz^2 </mrow>
					<mrow>  \frac{1}{z^2}dz	 \amp =  2tdt </mrow>
					<mrow>  \int \frac{1}{z^2}dz	 \amp =  \int 2tdt </mrow>
					<mrow>  -\frac{1}{z}	 \amp =  t^2 + C_1 </mrow>
					<mrow>  z	 \amp =  -\frac{1}{t^2 + C_1} </mrow>
				</md>

				Using the initial condition <m>z(1) = 2</m>:
				<md>
					<mrow>  2	 \amp =  -\frac{1}{1^2 + C_1} </mrow>
					<mrow>  2	 \amp =  -\frac{1}{1 + C_1} </mrow>
					<mrow>  C_1	 \amp =  -\frac{1}{2} - 1 </mrow>
					<mrow>  C_1	 \amp =  -\frac{3}{2} </mrow>
				</md>

				So the solution to the initial value problem is:
				<md>
					<mrow>  z(t)	 \amp =  -\frac{1}{t^2 - \frac{3}{2}} </mrow>
				</md>
			</solution>
			<answer>
				<m> z(t) = -\frac{1}{t^2 - \frac{3}{2}} </m>
			</answer>
		</exercise>

		<exercise>
			<statement>
				<m> \displaystyle \frac{dy}{d\theta} = y\sin\theta, \hspace{0.5cm} \displaystyle y(\pi) = -3 </m>
			</statement>
			<solution>
				First we find the general solution:
				<md>
					<mrow>  \frac{dy}{d\theta}	 \amp =  y\sin\theta </mrow>
					<mrow>  \frac{1}{y}dy	 \amp =  \sin\theta d\theta </mrow>
					<mrow>  \int \frac{1}{y}dy	 \amp =  \int \sin\theta d\theta </mrow>
					<mrow>  \ln|y|	 \amp =  -\cos\theta + C_1 </mrow>
					<mrow>  e^{\ln|y|}	 \amp =  e^{-\cos\theta + C_1} </mrow>
					<mrow>  |y|	 \amp =  e^{-\cos\theta}\cdot e^{C_1} </mrow>
					<mrow>  y	 \amp =  \pm e^{C_1}e^{-\cos\theta} </mrow>
					<mrow>   \amp =  \underbrace{\pm e^{C_1}}_{\scriptsize = C_2}e^{-\cos\theta} </mrow>
					<mrow>   \amp =  C_2e^{-\cos\theta}  </mrow>
				</md>
				Then we use the initial conditio <m> \displaystyle y(\pi) = -3 </m> .
				<md>
					<mrow>  -3	 \amp =  y(\pi) </mrow>
					<mrow>   \amp =  C_2e^{-\cos\pi} </mrow>
					<mrow>   \amp =  C_2e^{-(-1)} </mrow>
					<mrow>   \amp =  C_2e </mrow>
					<mrow>  -\frac{3}{e}	 \amp =  C_2, \mbox{ or} </mrow>
					<mrow>  C_2	 \amp =  -3e^{-1} </mrow>

				</md>
				Hence, the solution i <m> \displaystyle y = -3e^{-1}e^{-\cos\theta} </m> , or <m> \displaystyle y = -3e^{-\cos\theta-1} </m> .
			</solution>
			<answer>
				<m> \displaystyle y = -3e^{-1}e^{-\cos\theta} </m>, or  <m> \displaystyle y = -3e^{-\cos\theta-1} </m>
			</answer>
		</exercise>

		<exercise>
			<statement>
				<m> \displaystyle \frac{dy}{dx} - 8x^3e^{-2y} = 0, \hspace{0.5cm} \displaystyle y(1) = 0 </m>
			</statement>
			<solution>
				First we find the general solution:
				<md>
					<mrow>  \frac{dy}{dx} - 8x^3e^{-2y}	 \amp =  0 </mrow>
					<mrow>  \frac{dy}{dx}	 \amp =  8x^3e^{-2y} </mrow>
					<mrow>  \frac{1}{e^{-2y}}dy	 \amp =  8x^3dx </mrow>
					<mrow>  e^{2y}dy	 \amp =  8x^3dx </mrow>
					<mrow>  \int e^{2y}dy	 \amp =  \int 8x^3dx </mrow>
					<mrow>  \frac{1}{2}e^{2y}	 \amp =  2x^4 + C_1 </mrow>
					<mrow>  e^{2y}	 \amp =  4x^4 + 2C_1 </mrow>
					<mrow>  \ln(e^{2y})	 \amp =  \ln(4x^4 + 2C_1) </mrow>
					<mrow>  2y	 \amp =  \ln(4x^4 + 2C_1) </mrow>
					<mrow>  y	 \amp =  \frac{1}{2}\ln(4x^4 + 2C_1), \mbox{ or} </mrow>
					<mrow>   \amp =  \frac{1}{2}\ln(4x^4 + C_2), \mbox{ or} </mrow>
					<mrow>   \amp =  \ln\Big[(4x^4 + C_2)^{1/2}\Big], \mbox{ or} </mrow>
					<mrow>   \amp =  \ln\Big[\sqrt{4x^4 + C_2}\Big] </mrow>

				</md>
				Then we use the initial conditio <m> \displaystyle y(1) = 0 </m> .
				<md>
					<mrow>  0	 \amp =  y(1) </mrow>
					<mrow>  0	 \amp =  \ln\Big[\sqrt{4\cdot 1^4 + C_2}\Big] </mrow>
					<mrow>  0	 \amp =  \ln\Big[\sqrt{4 + C_2}\Big] </mrow>
					<mrow>  e^0	 \amp =  e^{\ln\Big[\sqrt{4 + C_2}\Big]} </mrow>
					<mrow>  1	 \amp =  \sqrt{4 + C_2} </mrow>
					<mrow>  1^2	 \amp =  \Big[\sqrt{4 + C_2}\Big]^2 </mrow>
					<mrow>  1	 \amp =  4+C_2 </mrow>
					<mrow>  -3	 \amp =  C_2 </mrow>

				</md>
				Hence, the solution i <m> \displaystyle y = \frac{1}{2}\ln(4x^4 - 3) </m> , or <m> \displaystyle y = \ln\Big[\sqrt{4x^4 - 3}\Big] </m> .
			</solution>
			<answer>
				<m> \displaystyle y = \frac{1}{2}\ln(4x^4 - 3) </m> , or <m> \displaystyle y = \ln\Big[\sqrt{4x^4 - 3}\Big] </m>
			</answer>
		</exercise>

	</exercisegroup>

	<exercisegroup><title> Applications </title>

		<exercise>
			<statement>
				A 4-lb roast, initially at <m>50^{\circ}F</m>, is placed in a <m>375^{\circ} F</m> oven at 5:00 PM After 75 minutes it is found that the temperature <m>T(t)</m> of the roast is <m>125^{\circ}</m> F. When will the roast be <m>150^{\circ}F</m> (medium rate)?
			</statement>

			<solution>
				We take time <m>t</m> in minutes, with <m>t = 0</m> corresponding to 5:00 PM We also assume (somewhat unrealistically) that at any instant the temperature <m>T(t)</m> of the roast is uniform throughout. We have <m>T(t) \lt A = 375</m>, <m>T(0)=50</m>, and <m>T(75) =125</m>.

				Hence
				<md>
					<mrow>\displaystyle  \frac{dT}{dt}  = k(375-T)</mrow>
					<mrow>				\int \frac{1}{375-T}dT\amp=\displaystyle \int kdt</mrow>
					<mrow>				y(x)\amp=\displaystyle 1+(x^2+C)^3</mrow>
					<mrow>			-\ln(375-T)=\amp kt+C</mrow>
				</md>

				Now <m>T(0)=50</m>, implies that <m>B = 325</m>, so <m>T(t) = 375-325e^{kt}</m>. We also know that <m>T = 125</m> when <m>t = 75</m>. Substitution of these values in the preceding equation yields

				<me> k=-\frac{1}{75}\ln\left(\frac{250}{325}\right)\approx 0.0035.</me>

				Hence we finally solve the equation

				<me>150=375-325e^{(-0.0035)t}</me>

				for <m>t = -[\ln(225/325)]/[0.0035] \approx 105</m> (min), the total cooking time required.Because the roast was placed in the oven at 5:00 PM, it it should be removed at about 6:45 PM
			</solution>
			<answer>
				<m>t = -[\ln(225/325)]/[0.0035] \approx 105(min)</m>
			</answer>
		</exercise>
	</exercisegroup>
		
	<exercisegroup><title> Conceptual Questions </title>

		<exercise>
			<statement>
				Explain why separating variables works as a method for solving ordinary differential equations. 
			</statement>
			<solution>
				<p>
					Separation of variables works by isolating all terms involving <m>y</m> to one side and all terms involving <m>x</m> to the other. When this can be done, both sides can be integrated independently, allowing for the solution of the differential equation. This method effectively transforms the problem of solving a differential equation into the simpler task of integrating functions.
				</p>
			</solution>
		</exercise>

		<exercise>
			<statement>
				Why is it important for the equation to be "separable" in order to use the method of separation of variables? What does it mean for a differential equation to be separable?
			</statement>
			<solution>
				<p>
					For the method of separation of variables to be used, we must be able to write the differential equation in the form <m>g(y) dy = h(x) dx</m>, effectively separating the variables <m>y</m> and <m>x</m> onto different sides of the equation. When a differential equation can be written in this way, it is called separable. Separability is crucial because it allows us to integrate each side with respect to its own variable, leading to a solution for <m>y</m> in terms of <m>x</m>.
				</p>
			</solution>
		</exercise>

		<exercise>
			<statement>
				Provide an example of a differential equation that is not separable and explain why the method of separation of variables cannot be applied to it.
			</statement>
			<solution>
				<p>
					
				</p>
			</solution>
		</exercise>

		<exercise>
			<statement>
				In solving a differential equation using separation of variables, why might the constant of integration appear on both sides of the resulting equation?
			</statement>
			<solution>
				<p>
					After separating variables, we integrate both sides of the equation. Each integration will typically introduce its own constant of integration. Therefore, when we combine the results of these integrations, we often see a constant on both sides. These constants can often be combined into a single constant by subtracting one from the other.
				</p>
			</solution>
		</exercise>

		<exercise>
			<statement>
				Some differential equations solved using separation of variables yield implicit solutions, while others yield explicit solutions. Explain the difference between implicit and explicit solutions, and provide examples of each.
			</statement>
			<solution>
				<p>
					
				</p>
			</solution>
		</exercise>

		<exercise>
			<statement>
				True/False: Every first-order ordinary differential equation can be solved using the method of separation of variables.
			</statement>
			<solution>
				<p>
					
				</p>
			</solution>
		</exercise>

		<!-- Multiple Choice -->
		<exercise>
			<statement>
				<p>Which of the following differential equations is <em>not</em> separable?</p>
				<ol type="a">
					<li><m> \frac{dy}{dx} = y \cos(x) </m></li>
					<li><m> \frac{dy}{dx} = y + e^x </m></li>
					<li><m> \frac{dy}{dx} = \sin(x) \sin(y) </m></li>
					<li><m> \frac{dy}{dx} = x^2y </m></li>
				</ol>
			</statement>
		</exercise>

		<!-- True/False -->
		<exercise>
			<statement>
				<p>True/False: If a differential equation is separable, its solution will always be an explicit function of <m> x </m>.</p>
			</statement>
		</exercise>

		<!-- Fill-in-the-blank -->
		<exercise>
			<statement>
				<p>The process of writing a differential equation in the form <m> M(y)dy = N(x)dx </m> is called _________ of variables.</p>
			</statement>
		</exercise>

		<!-- Multiple Choice -->
		<exercise>
			<statement>
				<p>Which of the following cannot be directly solved by separation of variables?</p>
				<ol type="a">
					<li><m> \frac{dy}{dx} = x + y </m></li>
					<li><m> \frac{dy}{dx} = xy </m></li>
					<li><m> \frac{dy}{dx} = \sin(x)y </m></li>
					<li><m> \frac{dy}{dx} = \frac{x}{y} </m></li>
				</ol>
			</statement>
		</exercise>

		<!-- True/False -->
		<exercise>
			<statement>
				<p>True/False: The method of separation of variables can be directly applied to higher-order differential equations.</p>
			</statement>
		</exercise>


		<!-- True/False -->
		<exercise>
			<statement>
				<p>True/False: If you can write a differential equation in the form <m> h(y) \frac{dy}{dx} = g(x) </m>, then it is separable.</p>
			</statement>
		</exercise>

		<!-- Multiple Choice -->
		<exercise>
			<statement>
				<p>A differential equation of the form <m> \frac{dy}{dx} = g(x) </m> without a <m> y </m> term:</p>
				<ol type="a">
					<li>Is always separable</li>
					<li>Is never separable</li>
					<li>Can be separable depending on <m> g(x) </m></li>
					<li>Is an implicit equation</li>
				</ol>
			</statement>
		</exercise>

	</exercisegroup>

		<exercise>
		  <title>A structured exercise</title>
		  <introduction>
			<p>
			  Here is where we give the student the background information
			  required to start accomplishing tasks.
			</p>
		  </introduction>
		
		  <task>
			<p>
				Solve a separable DE using separation of variables.
			</p>
			<p>
				<webwork xml:id="ww_piss">
			
					<pg-code>
					$a = random(4,9,1);
					$b = random(2,9,1);
					$ans = FormulaUpToConstant("1/$a e^{$a x}- $b/2 x^2");
					</pg-code>
			
					<statement>
					<p>
						<m>y(x) =</m> <var name="$ans" width="25" />
					</p>
					</statement>
			
					<solution>
					<m></m>.
					</solution>
				</webwork>
			</p>

	  
		  </task>
		
		  <task>
			<statement>
			  <p>
				The second step to do.
				We'll be lazy and just include an answer.
			  </p>
			</statement>
			<answer>
			  <p>
				Just the answer.
			  </p>
			</answer>
		  </task>
		
		  <conclusion>
			<p>
			  A little wrap up.
			</p>
		  </conclusion>
		
		</exercise>

</exercises>
