<section xml:id="review-exp-and-logs"><title> Exponential and Logarithmic Functions </title>

	<p>
		Recall the following rules for exponential and logarithmic functions.

		<assemblage><title> Exponential Rules </title>

		<tabular>
			<col halign="center" />
			<col />
			<col halign="center" />

			<row halign="center">
				<cell/>
				<cell bottom="minor">General</cell>
				<cell/>
				<cell bottom="minor">Natural (<m>a=e</m>)</cell>
			</row>

			<row bottom="none">
				<cell><m>E_1:</m></cell>
				<cell>
					<md><mrow xml:id="exp_rule_01">\displaystyle (ab)^x = a^x \cdot b^x</mrow></md>
				</cell>
				<cell/>
				<cell>
					<md><mrow xml:id="exp_rule_01e">\displaystyle (eb)^x = e^x \cdot b^x</mrow></md>
				</cell>
			</row>

			<row bottom="none">
				<cell><m>E_2:</m></cell>
				<cell>
					<md><mrow xml:id="exp_rule_02">\displaystyle a^x \cdot a^y = a^{x+y}</mrow></md>
				</cell>
				<cell/>
				<cell>
					<md><mrow xml:id="exp_rule_02e">\displaystyle e^x \cdot e^y = e^{x+y}</mrow></md>
				</cell>
			</row>

			<row bottom="none">
				<cell><m>E_3:</m></cell>
				<cell>
					<md><mrow xml:id="exp_rule_03">\displaystyle (a^x)^y = a^{xy}</mrow></md>
				</cell>
				<cell/>
				<cell>
					<md><mrow xml:id="exp_rule_03e">\displaystyle (e^x)^y = e^{xy}</mrow></md>
				</cell>
			</row>

			<row bottom="none">
				<cell><m>E_4:</m></cell>
				<cell>
					<md><mrow xml:id="exp_rule_04">\displaystyle a^{-x} = \frac{1}{a^x}</mrow></md>
				</cell>
				<cell/>
				<cell>
					<md><mrow xml:id="exp_rule_04e">\displaystyle e^{-x} = \frac{1}{e^x}</mrow></md>
				</cell>
			</row>

		</tabular>

		</assemblage>

	</p>

	<p>
		<assemblage><title> Logarithmic Rules </title>

		<tabular>
			<col halign="center" />
			<col />
			<col halign="center" />

			<row halign="center">
				<cell/>
				<cell bottom="minor">General</cell>
				<cell/>
				<cell bottom="minor">Natural (<m>a=e</m>)</cell>
			</row>

			<row bottom="none">
				<cell><m>L_1:</m></cell>
				<cell>
					<md><mrow xml:id="log_rule_01">\displaystyle \log_b (b^x) = x</mrow></md>
				</cell>
				<cell/>
				<cell>
					<md><mrow xml:id="ln_rule_01">\displaystyle \ln(e^x) = x</mrow></md>
				</cell>
			</row>

			<row bottom="none">
				<cell><m>L_2:</m></cell>
				<cell>
					<md><mrow xml:id="log_rule_02">\displaystyle b^{\log_b(x)} = x</mrow></md>
				</cell>
				<cell/>
				<cell>
					<md><mrow xml:id="ln_rule_02">\displaystyle e^{\ln(x)} = x</mrow></md>
				</cell>
			</row>

			<row bottom="none">
				<cell><m>L_3:</m></cell>
				<cell>
					<md><mrow xml:id="log_rule_03">\displaystyle \log_b(1) = 0</mrow></md>
				</cell>
				<cell/>
				<cell>
					<md><mrow xml:id="ln_rule_03">\displaystyle \ln(1) = 0</mrow></md>
				</cell>
			</row>

			<row bottom="none">
				<cell><m>L_4:</m></cell>
				<cell>
					<md><mrow xml:id="log_rule_04">\displaystyle \log_b(xy) = \log_b(x) + \log_b(y)</mrow></md>
				</cell>
				<cell/>
				<cell>
					<md><mrow xml:id="ln_rule_04">\displaystyle \ln(xy) = \ln(x) + \ln(y)</mrow></md>
				</cell>
			</row>

			<row bottom="none">
				<cell><m>L_5:</m></cell>
				<cell>
					<md><mrow xml:id="log_rule_05">\displaystyle \log_b\left(\frac{\displaystyle x}{\displaystyle y}\right) = \log_b(x) - \log_b(y)</mrow></md>
				</cell>
				<cell/>
				<cell>
					<md><mrow xml:id="ln_rule_05">\displaystyle \ln\left(\frac{\displaystyle x}{\displaystyle y}\right) = \ln(x) - \ln(y)</mrow></md>
				</cell>
			</row>

		</tabular>

		</assemblage>

	</p>

	<p>
		Let's look at a couple of examples, starting with an equation containing exponentials.
	</p>

	<example xml:id="r-01-04-exp_logs_ex_01">
		<p>
			Solve for <m>x</m>: <m>\displaystyle \quad e^{3x+z} - e^z = y</m>
		</p>
		<solution>
			<p>
				If you prefer to see a video of this example, <url href="https://www.youtube.com/watch?v=QdZekQ5_T2E"><c>click here</c></url>
			</p>
			
			<p>
				We might begin by isolating the exponential that contains <m>x</m> and then
				taking the natural log of both sides.

				<md>
					<mrow>
						e^{3x+z} - e^z			\amp= y
					</mrow>
					<mrow>
						e^{3x+z} 				\amp= y + e^z
					</mrow>
					<mrow>
						<xref text="custom" ref="ln_rule_01"><m>\overset{L_1}{\hookrightarrow}\qquad</m></xref>
						\ln\big(e^{3x+z}\big)	\amp= \ln\big(y + e^z\big)
					</mrow>
					<mrow>
						3x + z					\amp= \ln\big(y + e^z\big)
					</mrow>
					<mrow>
						3x						\amp= \ln\big(y + e^z\big) - z
					</mrow>
					<mrow>
						x						\amp= \frac{1}{3}\ln\big(y + e^z\big) - \frac{1}{3}z
					</mrow>
				</md>
			</p>

			<p>
				It's worth noting that we cannot break up that log on the right hand side.
				There's no "rule" that helps when we have addition inside a logarithm.
			</p>

			<p>
				There is another way to approach this if notice that <m>z</m> appears inside both
				exponential terms.

				<md>
					<mrow>
						<xref text="custom" ref="exp_rule_02e"><m>\overset{E_2}{\hookrightarrow}\qquad</m></xref>
						e^{3x+z} - e^z			\amp= y
					</mrow>
					<mrow>
						e^{3x}\cdot e^{z} - e^z	\amp= y
					</mrow>
					<mrow>
						e^z(e^{3x} - 1)			\amp= y
					</mrow>
					<mrow>
						e^{3x} - 1				\amp= \frac{y}{e^z}
						<xref text="custom" ref="exp_rule_04e"><m>\qquad\overset{E_4}{\hookleftarrow}</m></xref>
					</mrow>
					<mrow>
						e^{3x} - 1				\amp= ye^{-z}
					</mrow>
					<mrow>
						e^{3x}					\amp=  ye^{-z} + 1
					</mrow>
					<mrow>
						<xref text="custom" ref="ln_rule_01"><m>\overset{L_1}{\hookrightarrow}\qquad</m></xref>
						\ln\big( e^{3x} \big)	\amp= \ln \big( ye^{-z} + 1\big)
					</mrow>
					<mrow>
						3x						\amp= \ln \big( ye^{-z} + 1 \big) 
					</mrow>
					<mrow>
						x						\amp= \frac{1}{3}\ln\big(ye^{-z}+1\big)
					</mrow>
				</md>
				The answers may look different, but they are equivalent and both are correct.
			</p>
		</solution>
	</example>

	<p>
		Now let's look at an example involving logarithms.
	</p>

	<example xml:id="r-01-04-exp_logs_ex_02">
		<p>
			Solve for <m>x</m>: <m>\displaystyle \quad \ln(x+y) = 5 + \ln(z)</m>
		</p>

		<solution>
			<p>
				If you prefer to see a video of this example, <url href="https://www.youtube.com/watch?v=7xG6SisdjYE"><c>click here</c></url>
			</p>

			<p>
				We'll carefully apply the rules above. We want to get our hands on <m>x</m>,
				and right now its inside a logarithm. In order to undo that, we'll exponentiate
				both sides.

				<md>
					<mrow>	
						\ln(x+y)		\amp= 5 + \ln(z)
					</mrow>
					<mrow>
						<xref text="custom" ref="ln_rule_02"><m>\overset{L_2}{\hookrightarrow}\qquad</m></xref>
						e^{\ln(x+y)}	\amp= e^{\big(5 + \ln(z)\big)}				
						<xref text="custom" ref="exp_rule_02e"><m>\qquad\overset{E_2}{\hookleftarrow}</m></xref>
					</mrow>
					<mrow>
						x + y			\amp= e^{5} \cdot e^{\ln(z)}		
						<xref text="custom" ref="ln_rule_02"><m>\qquad\overset{L_2}{\hookleftarrow}</m></xref>
					</mrow>
					<mrow>
						x				\amp= e^{5}z - y
					</mrow>
				</md>

			</p>

		</solution>

	</example>

	<p>Now you should try. Be careful!</p>

	<p>
		<term> Use algebra and the rules above to solve for <m>x</m> in each of the following equations.</term>

		<ol>
		<li><m>e^{x+y} = 12</m>
			<solution>
				<md>
					<mrow>		e^{x+y}	\amp= 12											</mrow>
					<mrow> \ln(e^{x+y}) \amp= \ln(12)										</mrow>
					<mrow>			x+y	\amp= \ln(12)										</mrow>
					<mrow>			  x	\amp= \ln(12) - y									</mrow>
				</md>
			</solution>
			<answer>
			<me> x = \ln(12) - y </me>
			</answer>
		</li>
		<li> <m>e^{x+y}  + e^x= 12</m>
			<solution>
				<md>
					<mrow>		 e^{x+y}  + e^x	\amp= 12									</mrow>
					<mrow>   e^x\cdot e^y + e^x \amp= 12									</mrow>
					<mrow>		   e^x(e^y + 1)	\amp= 12									</mrow>
					<mrow>					e^x	\amp= \frac{12}{e^y + 1}					</mrow>
					<mrow>			   \ln(e^x)	\amp= \ln \left( \frac{12}{e^y + 1} \right)	</mrow>
					<mrow>					
											x	\amp= \ln \left( \frac{12}{e^y + 1} \right),\qquad \text{or}	
					</mrow>
					<mrow>						\amp= \ln(12) - \ln(e^y + 1)				</mrow>
				</md>
			</solution>
			<answer>
			<md>
				<mrow> x	\amp= \ln\left( \frac{12}{e^y + 1} \right), \qquad \text{or}</mrow>
				<mrow>		\amp= \ln(12) - \ln(e^y + 1)</mrow>
			</md>
			</answer>
		</li>
		<li> <m>e^x = 1 \qquad</m>
			<solution>
			<md>
				<mrow> 		e^x	\amp= 1													</mrow>
				<mrow> \ln(e^x)	\amp= \ln(1)											</mrow>
				<mrow>		  x	\amp= 0													</mrow>
			</md>
			</solution>
			<answer>
			<me> x = 0 </me>
			</answer>
		</li>
		<li> <m>\ln x = 3\ln z \qquad</m>
			<solution>
			<md>
				<mrow> 		\ln x	\amp= 3\ln z										</mrow>
				<mrow>   e^{\ln x}	\amp= e^{3\ln z}									</mrow>
				<mrow>   e^{\ln x}	\amp= e^{\ln (z^3)}									</mrow>
				<mrow>			x	\amp= z^3											</mrow>
			</md>
			</solution>
			<answer>
			<me> x = z^3 </me>
			</answer>
		</li>
		<li> <m>y + \ln x = 4 \qquad</m>
			<solution>
			<md>
				<mrow>y + \ln x	\amp= 4													</mrow>
				<mrow>    \ln x	\amp= 4 - y												</mrow>
				<mrow> e^{\ln x}\amp= e^{4 - y}											</mrow>
				<mrow>		  x	\amp= e^{4-y}											</mrow>
			</md>
			</solution>
			<answer>
			<me> x = e^{4-y} </me>
			</answer>
		</li>
		<li> <m>\ln y + \ln x = 4 \qquad</m>
			<solution>
			<md>
				<mrow>  \ln y + \ln x	\amp= 4											</mrow>
				<mrow>			\ln x	\amp= 4 - \ln y									</mrow>
				<mrow>		e^{\ln x}	\amp= e^{4 - \ln y}								</mrow>
				<mrow>				x	\amp= e^{4 - \ln y}								</mrow>
				<mrow>					\amp= e^4 \cdot e^{-\ln y}						</mrow>
				<mrow>					\amp= e^4 \cdot e^{\ln (y^{-1})}				</mrow>
				<mrow>					\amp= e^4 \cdot y^{-1}							</mrow>
				<mrow>					\amp= e^4 \cdot \frac{1}{y}						</mrow>
				<mrow>					\amp= \frac{e^4}{y}								</mrow>
			</md>
			</solution>
			<answer>
			<me> x = \frac{e^4}{y} </me>
			</answer>
		</li>
		<li> <m>\ln x = 8\ln y + 5 \qquad</m>
			<solution>
			<md>
				<mrow> 		\ln x	\amp= 8\ln y + 5									</mrow>
				<mrow>   e^{\ln x}	\amp= e^{8\ln y + 5}								</mrow>
				<mrow>		  	x	\amp= e^{8\ln y}\cdot e^5							</mrow>
				<mrow>				\amp= e^{\ln (y^8)}\cdot e^5						</mrow>
				<mrow>				\amp= y^8\cdot e^5									</mrow>
				<mrow>				\amp= e^5 y^8										</mrow>
			</md>
			</solution>
			<answer>
			<me> x = e^5 y^8 </me>
			</answer>
		</li>
		</ol>
	</p>

</section>
