<subsection xml:id="r-01-10" xmlns:xi="http://www.w3.org/2001/XInclude">

<title>Partial Fraction Decomposition</title>

<p>
You probably encountered partial fraction decomposition in Calculus 2 because it is 
sometimes needed when integrating rational functions. We will encounter partial
fraction decomposition when we solve differential equations with Laplace transforms.
</p>

<p>
Recall that we use this method when we have a rational function and we'd like to 
break it into smaller pieces. Part of that process is factoring the denominator 
and determining the type of factors (distinct linear, repeated linear, distinct 
irreducible quadratic, or repeated irreducible quadratic) and knowing the 
corresponding form of the partial fraction decomposition. Then we do algebra to 
determine the coefficients.
</p>

<p>
Find the partial fraction decomposition for each of the following rational functions.

<ol>
	<li> <m>g(x) = \ds \frac{1}{x^2 - 5x+6} \qquad</m>
	<solution>	
	<me>g(x) = \frac{1}{x^2 - 5x+6} = \frac{1}{(x-3)(x-2)} 
									= \frac{A}{x-3} + \frac{B}{x-2}	</me>
	<md>
		<mrow>\frac{1}{(x-3)(x-2)}\cdot (x-3)(x-2)	
											=\amp\ \left[\frac{A}{x-3} + \frac{B}{x-2} 
														\right] \cdot (x-3)(x-2)</mrow>
		<mrow>							1	=\amp\ A(x-2) + B(x-3)				</mrow>
		<mrow>							0x+1=\amp\ Ax - 2A + Bx - 3B				</mrow>
		<mrow>							0x+1=\amp\ (A+B)x + (-2A - 3B)			</mrow>
	</md>
	<sidebyside widths="40% 10% 40%" margins="auto" valign="top">
	<p><md>
		<mrow>	A+B	=\amp\ 0 </mrow>
		<mrow>	B	=\amp\ -A</mrow>
		<mrow>	</mrow>
	</md></p>
	<p> and </p>
	<p><md>
		<mrow>-2A - 3B 	=\amp\ 1	</mrow>
		<mrow>2A - 3(-A) 			=\amp\ 1	</mrow>
		<mrow>A				=\amp\ 1	</mrow>
	</md></p>
	</sidebyside>
	<me> B = -A = -1 </me>
	<me>  \Rightarrow g(x) = \frac{1}{x-3} + \frac{-1}{x-2}</me>
	</solution>
	<answer>
		<me> g(x) = \frac{1}{x-3} + \frac{-1}{x-2} </me>
	</answer>
	</li>
	
	<li> <m>h(x) = \ds \frac{4x+7}{x^2 - 7x} \qquad</m>
	<solution>	
	<md>
		<mrow>h(x) = \frac{4x+7}{x^2 - 7x}	=\amp\ \frac{4x+7}{x(x-7)}</mrow>
		<mrow>\frac{4x+7}{x(x-7)}	=\amp\ \frac{A}{x} + \frac{B}{x-7}</mrow>
		<mrow>\frac{4x+7}{x(x-7)}\cdot x(x-7)	=\amp\ \left[\frac{A}{x} + \frac{B}{x-7}\right] \cdot x(x-7)</mrow>
		<mrow>4x+7	=\amp\ A(x-7) + Bx</mrow>
		<mrow>4x+7	=\amp\ Ax - 7A + Bx</mrow>
		<mrow>4x+7	=\amp\ (A+B)x + (-7A)</mrow>
	</md>
	<md>
		<mrow>\Rightarrow A+B	=\amp\ 4		\amp\text{and }</mrow> 
		<mrow>-7A	=\amp\ 7</mrow>
		<mrow>\amp		\amp 		A	=\amp\ -1</mrow>
		<mrow>(-1)+B	=\amp\ 4		\amp 			\amp</mrow>
		<mrow>B	=\amp\ 5 	\amp 			\amp</mrow>
	</md>
		<me> \Rightarrow h(x) = \frac{-1}{x} + \frac{5}{x-7}</me>
		</solution>
		<answer>
			<me> h(x) = \frac{-1}{x} + \frac{5}{x-7} </me>
		</answer>
	</li>
	
	<li> <m>r(x) = \ds \frac{20x^2+65x+115}{(x^2+9)(x+11)} \qquad</m> 		
	<solution>	
	<md>
		<mrow>r(x) = \frac{20x^2+65x+115}{(x^2+9)(x+11)}	=\amp\ \frac{Ax+B}{x^2 + 9} + \frac{C}{x+11}</mrow>
													\frac{20x^2+65x+115}{(x^2+9)(x+11)}\cdot (x^2+9)(x+11)	
					=\amp\ \left[\frac{Ax+B}{x^2 + 9} + \frac{C}{x+11}\right] \cdot (x^2+9)(x+11)
		<mrow>20x^2+65x+115	=\amp\ (Ax+B)(x+11) + C(x^2 + 9)</mrow>
		<mrow>20x^2+65x+115	=\amp\ Ax^2+11Ax + Bx+11B + Cx^2 + 9C</mrow>
		<mrow>20x^2+65x+115	=\amp\ (A + C)x^2 + (11A + B)x + (11B + 9C)</mrow>
	</md>
		Equating coefficients yields a system of three equations in three unknowns, which we solve.
	<md>
		<mrow>A+C	=\amp\ 20	\amp	11A + B	=\amp\ 65		\amp		11B + 9C	=\amp\ 115</mrow>
		<mrow>C	=\amp\ 20-A	\amp			\amp			\amp				\amp</mrow>
		<mrow>\amp		\amp			\amp			\amp 11B + 9(20-A)	=\amp\ 115</mrow>
		<mrow>\amp		\amp			\amp			\amp 11B + 180 - 9A	=\amp\ 115</mrow>
		<mrow>\amp		\amp			\amp			\amp		11B - 9A	=\amp\ -65</mrow>
		<mrow>\amp		\amp		B	=\amp\ 65 - 11A	\amp				\amp</mrow>
		<mrow>\amp		\amp			\amp			\amp 11(65-11A) - 9A	=\amp\ -65</mrow>
		<mrow>\amp		\amp			\amp			\amp 715 - 121A - 9A	=\amp\ -65</mrow>
		<mrow>\amp		\amp			\amp			\amp 		-130A	=\amp\ -780</mrow>
		<mrow>\amp		\amp			\amp			\amp			A	=\amp\ 6</mrow>
		<mrow>\amp		\amp		B	=\amp\ 65 - 11(6)	\amp				\amp</mrow>
		<mrow>\amp		\amp			=\amp\ - 1		\amp				\amp</mrow>
		<mrow>C	=\amp\ 20-6	\amp			\amp			\amp				\amp</mrow>
		<mrow>=\amp\ 14	\amp			\amp			\amp				\amp</mrow>
	</md>
	Hence,
		<me> r(x) = \frac{6x-1}{x^2 + 9} + \frac{14}{x+11}. </me>
	</solution>
	<answer>
		<me> r(x) = \frac{6x-1}{x^2 + 9} + \frac{14}{x+11} </me>
	</answer>
	</li>
</ol>

Find the <em>FORM</em> of the partial fraction decomposition for each of the following. 
Make sure you completely factor each denominator before determining the decomposition.
You need not find the values of the coefficients <m>A,</m> <m>B,</m> etc.

<ol>
	<li> <m>\ds v(x) = \frac{x^5 - 2x^4 - 6x^3 + 13x^2 - 3x - 27}{x^3 - 2x^2 - 3x}</m>  </li>
	
	<li> <m>\ds u(x) = \frac{8x^2 - 51x + 41}{x^2 - 6x + 5}</m> </li>
	
	<li> <m>\ds g(x) = \frac{17x - 11}{x^2(x-3)} \qquad</m>		
	<solution>
		
	Since the denominator is already factored, we see that the denominator has the following factors:
	<ul>
		<li> <m>x</m> (linear, double) </li>
		<li> <m>x-3</m> (linear, distinct) </li>
	</ul>
	Hence, the FORM of the partial fraction decomposition is:
		
		<me> g(x) = \frac{A}{x} + \frac{B}{x^2} + \frac{C}{x-3}. </me>
	</solution>
	<answer>
		<me> g(x) = \frac{A}{x} + \frac{B}{x^2} + \frac{C}{x-3} </me>
	</answer>
	</li>
	
	<li> <m>\ds h(x) = \frac{x+12}{(x^2 - 4)^2} \qquad</m>		
	<solution>
	Here we need to finish factoring the denominator:
		
		<me> h(x) = \frac{x+12}{(x^2 - 4)^2} = \frac{x+12}{[(x-2)(x+2)]^2} = \frac{x+12}{(x-2)^2(x+2)^2} </me>
		
	Now we see that the denominator has the following factors:
	<ul>
		<li> <m>(x-2)</m> (linear, double) </li>
		<li> <m>(x+2)</m> (linear, double) </li>
	</ul>
	Hence, the FORM of the partial fraction decomposition is:
	
		<me> h(x) = \frac{A}{x-2} + \frac{B}{(x-2)^2} + \frac{C}{x+2} + \frac{D}{(x+2)^2}. </me>
		
	</solution>
	<answer>
		<me> h(x) = \frac{A}{x-2} + \frac{B}{(x-2)^2} + \frac{C}{x+2} + \frac{D}{(x+2)^2} </me>
	</answer>
	</li>
	
	<li> <m>\ds r(x) = \frac{3x-14}{(x+1)(x^2 + 2x + 1)} \qquad</m>  		
	<solution>
	Here we need to finish factoring the denominator:
	
		<me> r(x) = \frac{3x-14}{(x+1)(x^2 + 2x + 1)} = \frac{3x-14}{(x+1)(x+1)(x+1)} = \frac{3x-14}{(x+1)^3} </me>
	
	Now we see that <m>(x+1)</m> (which is linear), is a factor (three times) of the denominator.
		
	Hence, the FORM of the partial fraction decomposition is:

		<me> r(x) = \frac{A}{x+1} + \frac{B}{(x+1)^2} + \frac{C}{(x+1)^3}. </me>

	</solution>
	<answer>
		<me> r(x) = \frac{A}{x+1} + \frac{B}{(x+1)^2} + \frac{C}{(x+1)^3} </me>
	</answer>
	</li>
	
	<li> <m>\ds s(x) = \frac{111}{(x^2 - 9)(x^2+9)} \qquad</m>		
	<solution>
	Here we need to finish factoring the denominator:

		<me> s(x) = \frac{111}{(x^2 - 9)(x^2+9)} = \frac{111}{(x-3)(x+3)(x^2 + 9)} </me>
	Now we see that the denominator has the following factors:
	<ul>
		<li> <m>(x-3)</m> (linear, single) </li>
		<li> <m>(x+3)</m> (linear, single) </li>
		<li> <m>(x^2 + 9)</m> (irreducible quadratic, single) </li>
	</ul>
	Hence, the FORM of the partial fraction decomposition is:

		<me> s(x) = \frac{A}{x-3} + \frac{B}{x+3} + \frac{Cx+D}{x^2 + 9}. </me>
		
	</solution>
	<answer>
		<me>  s(x) = \frac{A}{x-3} + \frac{B}{x+3} + \frac{Cx+D}{x^2 + 9} </me>
	</answer>
	</li>
</ol>

</p>
</subsection>
