<section xml:id="r-01-17" xmlns:xi="http://www.w3.org/2001/XInclude">

<title>Writing the equation of a line in point-slope form</title> 

{


<p>
When asked for the general form for the equation of a line, most people give
	<me> \mbox{slope-intercept form of a line: } y = mx+b.</me>
This form is great, but there is another form that is useful, and easy to remember if we
remember the formula for slope of a line.  Recall that if we are given two points
<m>(x_1, y_1)</m> and <m>(x, y),</m> the slope of the line between them is given by
	<me> m = \frac{y - y_1}{x - x_1}. </me>
We can rearrange this to yield
	<me> m(x - x_1) = y - y_1, </me>
or as we more commonly see it
	<me> \mbox{\bf slope-intercept form of a line: } y - y_1 = m(x - x_1).</me>
Sometimes it's useful to take it a step further and solve for <m>y</m> by adding <m>y_1</m> to both sides,
which leads to 
	<me> y = m(x - x_1) + y_1. </me>
	
	\begin{quote}
	<em> Example:</em>  Given the points <m>(3,7)</m> and <m>(-1,2)</m>, (i) write the equation of the line 
	through the points in point-slope form, and then (ii) solve for the dependent variable <m>y.</m>
	<answer>\it Answer:}
	<md>
		<mrow>\ampm = \frac{2 - 7}{-1 - 3} = \frac{5}{4}	</mrow>
		<mrow>\amp</mrow>
		<mrow>\ampy - y_1 = m(x - x_1)</mrow>
		<mrow>\amp</mrow>
		<mrow>\amp\mbox{(i) }y - 7 = \frac{5}{4}(x-3)	  \mbox{ OR }  y - 2	= \frac{5}{4}(x+1)</mrow>
		<mrow>\amp</mrow>
		<mrow>\amp\mbox{(ii) }y = \frac{5}{4}(x-3) + 7  \mbox{ OR }  y	= \frac{5}{4}(x+1) + 2</mrow>
	</md>
%%	
%%		<m>\ds m = \frac{2 - 7}{-1 - 3} = \frac{5}{4} </m>(note that either 
%%						order of the points will work here)
%%
%%		<m> y - y_1 = m(x - x_1)</m>
%%		
%%		(i)<m>\ds y - 7 = \frac{5}{4}(x-3)</m>
%%							 OR 
%%		
%%		(ii)<m>\ds y = \frac{5}{4}(x-3) + 7</m>
%		
%		(i)<m>\ds y - 7 = \frac{5}{4}(x-3)</m>(note that you 
%						can choose either of the given points here)
%		
%		(ii)<m>\ds y = \frac{5}{4}(x-3) + 7</m>
	\end{quote}
	</answer>
</p>

<p>
Now you try: }

<em> Use the given points to: (i) write the equation, in point-slope form, of the line through the points, 
	and then (ii) solve for the dependent variable $y.$</em>
<ol>
	
		<li>
  <m>(6, -1)</m> and <m>(2, -9)</m>		
	<solution>		
	
		<m>\ds m = \frac{-1 + 9}{6 - 2} = \frac{8}{4} = 2</m> 

		(i)<m>y +1 = 2(x-6)</m>
		
		(ii)<m>y = 2(x-6) - 1</m>
		
	</solution>
	<answer>
		
		(i)<m>y +1 = 2(x-6)</m>
		
		(ii)<m>y = 2(x-6) - 1</m>
		 }
	</answer>
	
	
		</li>
	
		<li>
  <m>(5, 0)</m> and <m>(1, 2)</m> 		
	<solution>		
	
		<m>\ds m = \frac{0 - 2}{5 - 1} = \frac{-2}{4} = -\frac{1}{2}</m> 

		(i)<m>\ds y - 0 = -\frac{1}{2}(x-5)</m>
		
		(ii)<m>\ds y = -\frac{1}{2}(x-5)</m>
		
	</solution>
	<answer>
		
		(i)<m>\ds y - 0 = -\frac{1}{2}(x-5)</m>
		
		(ii)<m>\ds y = -\frac{1}{2}(x-5)</m>
		 }
		</answer>
	
	
		</li>
	
		<li>
  <m>(-3, -7)</m> and <m>(0, 4)</m> 		
	<solution>		
	
		<m>\ds m = \frac{-7 - 4}{-3 - 0} = \frac{-11}{-3} = \frac{11}{3}</m> 

		(i)<m>\ds y + 7 = \frac{11}{3}(x+3)</m>
		
		(ii)<m>\ds y = \frac{11}{3}(x+3) - 7</m>
		
	</solution>
	<answer>
		
		(i)<m>\ds y + 7 = \frac{11}{3}(x+3)</m>
		
		(ii)<m>\ds y = \frac{11}{3}(x+3) - 7</m>
		 }
		</answer>
	</li>
</ol>
</p>
</section>