<subsection xmlns:xi="http://www.w3.org/2001/XInclude"><title> Initial Conditions &amp; Particular Solutions </title>
	
	<p>
		Solving a differential equation typically starts with finding the general solution that defines all the possible solutions (family of solutions). For example, later on in this text, we will show that the differential equation
		<men xml:id="initial-condition-de">y'' - y' - 12y = 0</men>
		has the general solution
		<men xml:id="initial-condition-gen-sol">y(t) = c_1e^{-3t} + c_2e^{4t}.</men>
		While the general solution gives us a family of possible solutions, in practical scenarios, we are usually interested in the specific solution where the constants are known. This is where initial conditions come into playâ€”they allow us to determine the particular solution that applies to the problem at hand.
	</p>

	<p>
		An <term>initial condition</term> is a starting value of the solution or its derivatives. For example, consider the free fall of an object due to gravity where <m>s(t)</m> is the position (distance from the ground) of this object at time <m>t</m>. Assuming the ball is dropped from the top of a 100 ft building, what initial information do you know? Let <m>t=0</m> be the time when the ball is dropped, then the initial conditions are given in the following table.
	</p>

	<p>
		The following table summarizes the initial conditions for our example, highlighting the key information required to determine the particular solution:
	</p>

	<tabular>
		<col right="minor" halign="center"/>
		<col halign="center"/>
		<row bottom="minor">
			<cell>Information at <m>t=0</m></cell>
			<cell>Initial Condition</cell>
		</row>
		<row>
			<cell>The ball is at the top of a 100 ft building.</cell>
			<cell><m>s(0) = 100 \text{ ft}</m></cell>
		</row>
		<row>
			<cell>The ball is dropped from rest (initial velocity is zero).</cell>
			<cell><m>s'(0) = 0 \text{ ft/s}</m></cell>
		</row>
	</tabular>
	
	<p>
		Without these initial conditions, the solution is incomplete and not applicable to any specific scenario. Assuming the solution must be consistent with these conditions forces the constants in the general solution to take specific values, giving us a particular solution.
	</p>
	
	<example>
	
		<m>\ \ </m>Solve the initial value problem
		<me> y'' - y' - 12y = 0, \quad y(0) = 4, \quad y'(0) = -2</me>. 
		
		<solution><title> Solution </title>
			<p>
				Since we already know the general solution to <xref ref="initial-condition-de"/> is given by 
				<me>y = c_1e^{-3t} + c_2e^{4t}</me>. 
				If you are interested in the verification steps, see the solution below.
			</p>
		
			<solution><title>Verification as a solution</title>

				<p>
					First find <m>y, y', \text{ and } y''</m>:
					<md>
						<mrow> y	=\amp\ c_1e^{-3t} + c_2e^{4t}		</mrow>
						<mrow> y'	=\amp\ -3c_1e^{-3t} + 4c_2e^{4t}	</mrow>
						<mrow> y''	=\amp\ 9c_1e^{-3t} + 16c_2e^{4t}	</mrow>
					</md>
				</p>
			
				<p>
					and substitute these into <m>y'' - y' - 12y</m> and simplify:
					<md>
						<mrow>
							y'' - y' - 12y =\amp\ \left(9c_1e^{-3t} + 16c_2e^{4t}\right) 
						</mrow>
						<mrow>		
							\amp\ \hspace{1em} - \left( -3c_1e^{-3t} + 4c_2e^{4t} \right) -12\left( c_1e^{-3t} + c_2e^{4t} \right)
						</mrow>
						<mrow>
							=\amp\ \ul{\ul{9c_1e^{-3t}}} + \ul{16c_2e^{4t}} 
						</mrow>
						<mrow>
							\amp\ \hspace{1em} + \ul{\ul{3c_1e^{-3t}}} - \ul{4c_2e^{4t}} - \ul{\ul{12c_1e^{-3t}}} - \ul{12c_2e^{4t}}
						</mrow>
						<mrow>
							=\amp\ 0
						</mrow>
					</md>
					Which shows <m>0 = 0</m> and so <m>y = c_1e^{-3t} + c_2e^{4t}</m> is a solution.
				</p>
		</solution>

			<p>
				We would like determine the spcific values of <m>c_1</m> and <m>c_2</m> that correspond to the initial conditions <m>y(0) = 4</m> and <m>y'(0) = -2</m>. 
			</p>

			<p>
				Since one initial condition involves the derivative, we will need to compute this before applying this condition.
				<me>y' = -3c_1e^{-3t} + 4c_2e^{4t}.</me>
			</p>
		
			<p>
				Now let's apply the initial conditions:
				<md>
				<mrow>y(0)	=\amp\ 4		\amp\Rightarrow \hspace{0.2cm} 	4
					=\amp\ c_1e^{-3\cdot 0} + c_2e^{4\cdot 0}</mrow>
				<mrow>			\amp	\amp	4
					=\amp\ c_1 + c_2		</mrow>
				<mrow>			\amp	\amp	\amp	</mrow>
				<mrow>y'(0)	=\amp\ -5	\amp\Rightarrow \hspace{0.2cm} 	-5
					=\amp\ -3c_1e^{-3\cdot} + 4c_2e^{4\cdot}	</mrow>
				<mrow>			\amp	\amp	-5	=\amp\ -3c_1 + 4c_2	</mrow>
				</md>
			</p>
		
			<p>
				We now have two equations and two unknowns,
				<md>
					<mrow>	 c_1 +  c_2	=\amp\ 	4 	</mrow>
					<mrow> -3c_1 + 4c_2	=\amp\ -5 	</mrow>
				</md>
				There are multiple ways to solve this system of equations, and the reader is encouraged to verify that	<m>c_1 = 3</m> and <m>c_2 = 1</m>. Here is one
		
				<solution><title>Solving for <m>c_1</m> and <m>c_2</m></title>
					<p>
				We will solve for <m>c_2</m> in the first equation and then
					substitute into the second.
					<md>
						<mrow>4					=\amp\ c_1 + c_2										</mrow>
						<mrow>\Rightarrow c_2	=\amp\ 4 - c_1								</mrow>
						<mrow>					\amp															</mrow>
						<mrow>-5				=\amp\ -3c_1 + 4c_2								</mrow>
						<mrow>\Rightarrow -5	=\amp\ -3c_1 + 4(4 - c_1)		</mrow>
						<mrow>-5				=\amp\ -3c_1 + 16 - 4c_1						</mrow>
						<mrow>-21				=\amp\ -7c_1												</mrow>
						<mrow>3					=\amp\ c_1													</mrow>
						<mrow>					\amp															</mrow>
						<mrow>c_2				=\amp\ 4 - c_1											</mrow>
						<mrow>					=\amp\ 4 - 3												</mrow>
						<mrow>					=\amp\ 1														</mrow>
					</md>
					</p>
				</solution>
		
			</p>
		
			<p>
				Thus, the solution we that satisfies the DE and both of the provided initial conditions is	<me> y = 3e^{-3t} + e^{4t}. </me>
			</p>
	
		</solution>
	
	</example>

	<example xml:id="p1-c2-s5-example-1">

		<m>\ \ </m>Solve the initial value problem
		<men xml:id="p1-c2-s5-example-1-de"> \frac{dy}{dx} = 2xy - 6x, \quad y(0) = 2</men>
		Given that the general solution is <m>\ds\ y = ce^{x^2} + 3</m>. 

		<solution><title> Solution </title>
			<p>
				The initial condition, <m>y(0) = 2</m>, tells us that <q><m>y</m> must equal 2 when <m>x</m> is 0</q>. When we substitute <m>y=2</m> and <m>x=0</m> into the general solution, we see that we can solve for <m>c</m>.
				<md>
					<mrow> y =  ce^{x^2} + 3 \quad \overset{y\ =\ 2,\ x\ =\ 0}{\Rightarrow} \quad	2	=\amp\  ce^{0^2} + 3	</mrow>
					<mrow>							 												2	=\amp\  c + 3		</mrow>
					<mrow>																			-1	=\amp\  c			</mrow>
				</md>
			</p>
		
			<p>
				Therefore, <m>y(0) = 2</m> forces <m>c = -1</m> and we get the particular solution
				<me>y = -e^{x^2} + 3</me>.
			</p>
		</solution>
	</example>

	<p>
		Initial conditions can also be visualized. <xref ref="initial-conditions-figure-1" /> the initial condition, <m>y(0) = 2</m>, is shown as the point <m>(0,2)</m> on the <m>y</m>-axis. The blue curve is the particular solution we found above and is the only solution in the family that passes through this point.
	</p>

	<sidebyside widths="46% 2% 50%" margins="0%">

		<stack>
			<p>
				<em>In the graph, the point on the <m>y</m>-axis is the initial condition. You can change the initial condition by dragging the point up and down along the <m>y</m>-axis.</em>
			</p>

			<p>
				As you drag the point, make the following observations:
			</p>

			<ul marker="square">
				<li> 
					Each new value of <m>y(0)</m> gives a new value of <m>c</m>, which corresponds to a new particular solution (blue curve). 
				</li>
				<li> 
					Only one particular solution from the family of solutions (green curves) passes through the initial condition.  
				</li>
			</ul>
		</stack>

		<p/>

		<figure xml:id="initial-conditions-figure-1">
			<interactive xml:id="interactive-drag-ic" platform="jsxgraph" source="code/initial-condition.js">

				<slate xml:id="interactive-drag-ic-slate" surface="jsxboard" />

			</interactive>
			<caption>The family of solutions (green curves) and a particular solution (blue curve) passing through <m>y(0)</m>.</caption>
		</figure>

	</sidebyside>

	<p>
		In summary, the process of solving a differential equation typically begins with finding a general solution. However, to apply this solution to real-world problems, we rely on initial conditions to determine a particular solution that accurately represents the system's specific circumstances.
	</p>

	<!-- <xi:include href="./chkpts-5-initial-conditions.ptx" /> -->

</subsection>