<subsection><title> Orphaned Content </title>

    <introduction>
        <p>
            This is just a place to put content that was written and may or not be used.
        </p>
    </introduction>

    <paragraphs><title>Additional Narrative</title>
        <p>
            So far, we have seen three examples of how to find a Laplace transform of a given function, but we have not discussed why this idea is relevant to differential equations. In the next section, we will tie these two concepts together and illustrate how Laplace transform can be used to solve a differential equation.
        </p>
    </paragraphs>

	<paragraphs><title> Additional Examples </title>


        <example xml:id="ex_lt_defn_01">
            <p>
                Find the Laplace transform of the function <m>g(t) = 15</m>.
            </p>
        
            <solution>
                <p>
                    By the above definition, we have
                    <md>
                        <mrow> \lap\{ g(t) \}	\amp= \lap\{ 15 \}	</mrow>
                        <mrow>					\amp= \int_0^{\infty} \left(15\right)e^{-st}dt \qquad \text{(improper integral)}	</mrow>
                        <mrow>					\amp= \lim_{b \to \infty}\int_0^b 15 e^{-st}dt	</mrow>
                        <mrow>					\amp= 15 \lim_{b \to \infty}\int_0^b e^{-st}dt \qquad (s\text{ is constant here})	</mrow>
                    </md>
                    At this point, we need to assume that <m>s\ne0</m> in order to continue. If you are curious as to why, see this <xref text="custom" ref="LT-s-ne-0-15">note</xref> for an explanation. Next, we integrate using the substitution <m>u=-st</m>.
                  </p>
        
                <p>
                    <md>
                        <mrow>	\amp= 15\lim_{b \to \infty} -\frac{1}{s}e^{-st}\Big|_{t=0}^{t=b}	</mrow>
                        <mrow>	\amp= 15\lim_{b \to \infty} -\frac{1}{s}\left[ e^{-sb} - e^{-s\cdot 0} \right]	</mrow>
                        <mrow>	
                                \amp= 15 \cdot -\frac{1}{s} \lim_{b \to \infty} \Big[ e^{-sb} - 1 \Big] \qquad \leftarrow <xref text="custom" ref="reason-factor-out-s">why?</xref>
                        </mrow>
                        <mrow>	
                                \amp= -\frac{15}{s}	\Big[ \lim_{b \to \infty} e^{-sb} - \us{=\ 1}{\ub{\lim_{b \to \infty} 1}} \Big]
                        </mrow>
                    </md>
                </p>
        
                <p>
                    Now let's focus on the remaining limit. It turns out that we have to put one more restriction on <m>s</m> since the limit will change based on whether <m>s</m> is positive or negative. Let's consider both cases.
                </p>
    
                <p>
                    Case 1: <m>\quad s\lt 0</m>, If <m>b \to \infty</m>, then <m>-sb \to +\infty</m> and so <m>\ds\lim_{b \to \infty} e^{-sb} = \infty</m>.
                    <me> = -\frac{15}{s} \left[\left( \lim_{b \to \infty} e^{-sb} \right) - 1 \right] = \infty</me>
                </p>
        
                <p>
                    Case 2: <m>\quad s\gt 0</m>. If <m>b \to \infty</m>, then <m>-sb \to -\infty</m> and so <m>\ds\lim_{b \to \infty} e^{-sb} = 0</m>.
                    <me> = -\frac{15}{s} \left[\left( \lim_{b \to \infty} e^{-sb} \right) - 1 \right] = -\frac{15}{s} \left[0 - 1\right] = \frac{15}{s}</me>
                </p>
        
                <p>
                    In case 1 (<m>s\lt0</m>), the improper integral is not finite, whereas in case 2 (<m>s\gt0</m>), the integral is finite and is equal to <m>15/s</m>.
                </p>
        
                <p>
                    In conclusion, we have found that
                    <me>\lap\{15\} = \frac{15}{s}</me>,
                    assuming <m>s \gt 0</m>.
                </p>
            </solution>
        
        </example>
        
        <example xml:id="ex_lt_defn_02">
            <p>
                Find the Laplace transform of <m>x(t) = e^{7t}</m>.
            </p>
        
            <solution>
                <p>
                    We use the definition of Laplace transform to get us started.
                    <md>
                        <mrow> \lap\{ x(t) \} \amp= \lap\{ e^{7t} \} 				</mrow>
                        <mrow> 		\amp= \int_0^{\infty} \left(e^{7t}\right)e^{-st}\ dt 				</mrow>
                        <mrow> 		\amp= \lim_{b \to \infty}\int_0^b e^{-st + 7t}\ dt	</mrow>
                        <mrow> 		\amp= \lim_{b \to \infty}\int_0^b e^{(7-s)t}\ dt 		</mrow>
                    </md>
                    As before, we need restrict some values of <m>s</m> in order for this
                    improper integral to exist . In this case, we will need <m>7 - s</m>, in the exponent, to be non-zero and negative. That is, we need
                    <me> 7 - s \lt 0 \hspace{0.5cm}\Rightarrow \hspace{0.5cm}7 \lt s. </me>
                    Hence, we move forward with the assumption that <m>s \gt 7</m>.
                    <md>
                        <mrow> 	\amp= \lim_{b \to \infty}\int_0^b e^{(7-s)t}dt </mrow>
                        <mrow>	\amp= \lim_{b \to \infty} \frac{1}{7-s}e^{(7-s)t}\Bigg|_0^b</mrow>
                        <mrow>	\amp= \frac{1}{7-s}\lim_{b \to \infty}
                                                \left[ e^{(7-s)b} - e^{(7-s)\cdot 0}\right]</mrow>
                        <mrow>	\amp= \frac{1}{7-s}\lim_{b \to \infty}
                                                \left[ e^{(7-s)b} - 1\right]</mrow>
                        <mrow>	\amp= \frac{1}{7-s}
                                                \left[\lim_{b \to \infty}e^{(7-s)b}
                                                - \lim_{b \to \infty}1\right]</mrow>
                        <mrow>	\amp= \frac{1}{7-s} \left[ 0 - 1\right] \quad
                                                <xref text="custom" ref="reason-limit-to-zero-e7t">why is the limit 0?</xref></mrow>
                        <mrow>	\amp= \frac{-1}{7-s} \hspace{4.4cm}	</mrow>
                        <mrow>	\amp= \frac{1}{s - 7}, 					\quad s \gt 7 	</mrow>
                    </md>
                    Thus, the Laplace transform of <m>x(t) = e^{7t}</m> is
                    <me>\ds \lap\{e^{7t}\} = \frac{1}{s - 7}</me>.
                </p>
            </solution>
        
        </example>
        
        <example xml:id="ex_lt_defn_03">
            <p>
                Find the Laplace transform of <m>q(t) = 11t</m>.
            </p>
        
            <solution>
                <p>
                    Let's use the definition of Laplace transform to get us going.
                    <md>
                        <mrow> 
                            \lap\{ 11t \}
                                \amp= \int_0^{\infty} \left(11t\right) e^{-st}\ dt 
                        </mrow>
                        <mrow> 				
                                \amp= 11\lim_{b \to \infty} \int_0^b te^{-st} dt \quad s \ne 0 \quad <xref text="custom" ref="LT-s-ne-0-11t">why is <m>s \ne 0</m>?</xref>\hspace{4.8cm}
                        </mrow>
                    </md>
                    <md>
                        <mrow> 
                            \phantom{\lap\{11t\}}
                                \amp= 11\lim_{b \to \infty} \left[-\frac{b}{s}e^{-sb} - \frac{1}{s^2}e^{-sb} + \frac{1}{s^2}\right]\quad <xref text="custom" ref="reason-int-by-parts-texpt">Integration by parts</xref>\hspace{2.5cm}
                        </mrow>
                    </md>
                    <md>
                        <mrow> \phantom{\lap\{11t\}}\amp= 11 \left[-\lim_{b \to \infty}\frac{b}{s}e^{-sb}
                                            - \lim_{b \to \infty}\frac{1}{s^2}e^{-sb}
                                            + \lim_{b \to \infty}\frac{1}{s^2}\right]</mrow>
                        <mrow> \amp= 11 \left[-\frac{1}{s}\lim_{b \to \infty}be^{-sb}
                                            - \frac{1}{s^2}\lim_{b \to \infty}e^{-sb}
                                            + \frac{1}{s^2}\right]\quad s > 0 \quad
                                                <xref text="custom" ref="LT-s-gt-0-11t">why is s > 0?</xref>\hspace{1.0cm}</mrow>
                    </md>
                    <md>
                        <mrow> \phantom{\lap\{11t\}}\amp= 11 \left[-\frac{1}{s}\cdot 0
                                            - \frac{1}{s^2}\cdot 0 + \frac{1}{s^2}\right]\quad
                                                <xref text="custom" ref="reason-limit-to-zero-11t">why are the limits 0?</xref>
                                                \hspace{3.6cm}</mrow>
                        <mrow> 		\amp= \frac{11}{s^2}, \quad s \gt 0 						</mrow>
                    </md>
                    Hence, we have <m>\ds \lap\{ 11t \} = \frac{11}{s^2}</m>, under the condition that <m>s>0</m>.
                </p>
            </solution>
        </example>
        
		
	</paragraphs>
	
	<reading-questions><title> Additional Practice </title>
    
    </reading-questions>

</subsection>