<introduction>

	<p>
		Our study of the Laplace Transform method begins with step 1 of the <xref ref="lt-roadmap" text="custom">Laplace Transform Roadmap</xref>, which we will refer to as the forward Laplace transform. 
	</p>

	<p>
		<image source="figures/LT-Diagram-Focused-Step-1.png" width="100%">
			<shortdescription>(for accessibility)</shortdescription>
		</image>
	</p>

	<p>
		To apply the Laplace transform to a differential equation is to rewrite both the left and right sides of the equation into the form shown in step 1 above.
	</p>

	<p>
		<tabular halign="center" valign="top">
			<row>
				<cell><m>\hspace{3em}</m>LHS</cell>
				<cell></cell>
				<cell>RHS</cell>
			</row>
			<row>
				<cell halign="right"><m>\us{y(0)=0,\ y'(0)=1}{y''+3y'+2y}</m></cell>
				<cell><m>=</m></cell>
				<cell><m>-40e^{3t}</m></cell>
			</row>
			<!-- <row>
				<cell><m>y(0)=0, y'(0)=1</m></cell>
				<cell></cell>
				<cell></cell>
			</row> -->
			<row>
				<cell><m>\hspace{3em}\downarrow</m></cell>
				<cell></cell>
				<cell><m>\downarrow</m></cell>
			</row>
			<row>
				<cell><m>s^2Y + 3sY + 2Y + 9</m></cell>
				<cell><m>=</m></cell>
				<cell><m>\ds -\frac{40}{s-3}</m></cell>
			</row>
		</tabular>
	</p>

	<p>
		Our objective for this section is to see how a Laplace transform converts the RHS function, <m>-40e^{3t}</m>, into <m>-\frac{40}{s-3}</m>. The next section explores how the derivatives and the initial conditions on the LHS become <m>s^2Y + 3sY + 2Y + 9</m>.
	</p>
	
</introduction>
