<section><title> Forward Transforms </title>

	<introduction>

		<p>
			To begin our exploration of the Laplace Transform, we start with the first step in the <xref ref="lt-roadmap" text="custom">Laplace Transform Roadmap</xref>, known as the forward Laplace transform. This step is foundational, as it sets the stage for the subsequent transformations outlined in the roadmap.
		</p>

		<p>
			<image source="figures/LT-Diagram-Focused-Step-1.png" width="100%">
				<shortdescription>Step 1: The Forward Laplace Transform</shortdescription>
			</image>
		</p>

		<p>
			Applying the forward Laplace transform to a differential equation involves converting both the left-hand side (LHS) and right-hand side (RHS) of the equation into their Laplace-transformed counterparts.
		</p>

		<p>
			This section investigates how individual functions, like <m>-40e^{3t}</m> in step 1, are transformed into expressions such as <m>-\frac{40}{s-3}</m>. In the next section, we will show where the <m>s^2Y + 3sY + 2Y + 9</m> comes from in the forward transform.
		</p>
		
	</introduction>

	<subsection xmlns:xi="http://www.w3.org/2001/XInclude"><title> Motivation </title>

		<p>
			The power of the Laplace transform lies in its ability to simplify the process of solving differential equations by leveraging the properties of integration by parts and the behavior of exponential functions. To illustrate this, let's revisit the integration by parts formula:
			<me> 
				\int u\ dv = uv - \int v\ du 
			</me>.
			Here, if <m>u</m> and <m>v</m> are functions of <m>t</m>, then <m>dv=v'\, dt</m> and <m>du=u'\, dt</m>. The formula can be rewritten as:
			<me> 
				\ub{\int u v'\, dt}_{\text{derivative on }v} = u v - \ub{\int v u'\, dt}_{\text{derivative on }u}
			</me>.
			Notice how the derivative initially applied to <m>v</m> on the left-hand side is transferred to <m>u</m> on the right-hand side. This property allows us to move derivatives from one function to another within an integral, a concept that is central to the Laplace transform.
		</p>

		<p>
			To see this in action, consider the integral
			<me> 
				\int e^{-st} y' \, dt
			</me>.
			Choosing <m>u = e^{-st}</m> and <m>dv = y' \, dt</m> in the integration by parts formula gives us
			<me> 
				\os{\quad (1)}{\int \us{u}{\us{\uparrow}{\ul{e^{-st}\vphantom{y'}}}} \ \us{dv}{\us{\uparrow}{\ul{y' dt}}}} = 
				\os{(2)}{\us{u}{\vphantom{\int}\us{\uparrow}{\ul{e^{-st}\vphantom{y}}}} \ \us{v}{\us{\uparrow}{\ul{y}}}} - 
				\os{\quad (3)}{\int \us{v}{\us{\uparrow}{\ul{y}}} \ \us{du}{\us{\uparrow}{\ul{(-s e^{-st} \ dt \vphantom{y})}}}}
			</me>.
			Here, we see that the derivative associated with <m>y'</m>, in integral <m>(1)</m>, was transferred onto <m>e^{-st}</m> and neither <m>(2)</m> nor <m>(3)</m> contain <m>y'</m>. 
		</p>

		<p>
			As you will see in the next section, this process of systematically transferring derivatives to exponential functions is at the heart of the Laplace transform. So, it should be no surprise when you encounter both an integral and the exponential function <m>e^{-st}</m> in its definition.
		</p>

		<xi:include href="./c4-s1-ss1-interactives.ptx" />

	</subsection>

	<subsection xmlns:xi="http://www.w3.org/2001/XInclude"><title>Definition</title>

		<p>
			In the previous section, we mentioned the importance of integration by parts and <m>e^{-st}</m> to the Laplace transform process. In fact, applying a Laplace transform to an equation is equivalent to multiplying both sides by <m>e^{-st}</m> and integrating with respect to <m>t</m>. For example, applying this to our model equation gives:
			<md>
				<mrow> 
					e^{-st} \left( y'' + 3y' + 2y \right) 
						=\amp\ e^{-st} \left( -40e^{3t} \right)
				</mrow>
				<mrow> 
					\int e^{-st} \left( y'' + 3y' + 2y \right) \, dt 
						=\amp\ \int e^{-st} \left( -40e^{3t} \right) \, dt
				</mrow>
				<mrow> 
					\ub{\int e^{-st} {\color{blue} y''} \, dt}_{\text{transform of } {\color{blue} y''}} + 
					3\ub{\int e^{-st} {\color{blue} y'} \, dt}_{\text{transform of } {\color{blue} y'}} + 
					2\ub{\int e^{-st} {\color{blue} y} \, dt}_{\text{transform of } {\color{blue} y}} 
						=\amp\ \ub{\int e^{-st} \left( {\color{blue} -40e^{3t}} \right) \, dt}_{\text{transform of } {\color{blue} -40e^{3t}}}
				</mrow>
			</md>.
			We formalize this with the following definition.
		</p>

		<definition><title>Laplace Transform</title>
			<statement>
				The <term>Laplace Transform</term> of a given function <m>f(t)</m> is defined as

				<me> \lap\left\{ {\color{blue} f(t)} \right\} = \int_0^{\infty} e^{-st} {\color{blue} f(t)}\ dt,</me>

				provided that the integral exists (i.e., the improper integral converges).
			</statement>
		</definition>

		<p>
			This definition might seem intimidating at first, but let's break it down. The <m>\infty</m> in the upper limit indicates that the Laplace transform is an improper integral. In calculus, we learn that such an integral can be rewritten as a limit. Specifically,
			<me>
				\int_0^{\infty} e^{-st} f(t)\, dt = \ub{\lim_{b \to \infty} \ob{\int_0^b e^{-st} f(t)\, dt}^{\text{step 1: compute the integral}}}_{\text{step 2: compute the limit}}.
			</me>
			Also, note that the integral involves two variables, <m>s</m> and <m>t</m>, but we integrate with respect to <m>t</m>. If you haven't encountered this before, simply treat <m>s</m> as a constant during the integration. Let's dive into an example to clarify this further.
		</p>
		
		<example>

			<m>\quad</m>Compute <m>\ds \lap\{1\}</m>.

			<solution>
				<p>
					By the definition above, we have the improper integral
					<men xml:id="lt-1-example-eqn-1"> 
						\lap\{1\} = \int_0^{\infty} \left(1\right)e^{-st}dt = \lim_{b \to \infty} \ub{\int_0^b e^{-st}dt}_{I}
					</men>.
					To compute <m>I</m>, treat <m>s</m> as a constant and integrate with respect to <m>t</m>.
					<md>

						<mrow>				
							\int_0^b e^{-st}dt
								\amp= \int_0^b e^{-st}dt  \qquad (u = -st)	
						</mrow>
						<mrow>				
								\amp=  -\frac{1}{s} \int_0^b e^{u} dt
						</mrow>
						<mrow>				
								\amp=  -\frac{1}{s} e^{u}\Big|_{t=0}^{t=b}
						</mrow>
						<mrow>			
								\amp= -\frac{1}{s}e^{-st}\Big|_{t=0}^{t=b}	
						</mrow>
						<mrow>			
								\amp= -\frac{1}{s}\left[ e^{-sb} - e^{-s\cdot 0} \right] = -\frac{1}{s}\left[ e^{-sb} - 1 \right] = I
						</mrow>
					</md>
					Now that we have <m>I</m>, we can plug it into the limit above.
					<md>
						<mrow> 
							\lim_{b \to \infty} \int_0^b e^{-st}dt 
								\amp= \lim_{b \to \infty} -\frac{1}{s}\left[ e^{-sb} - 1 \right]	
						</mrow>
						<mrow> 
								\amp= -\frac{1}{s} \lim_{b \to \infty} \Big[ e^{-sb} - 1 \Big] 
									\qquad \leftarrow <xref text="custom" ref="reason-factor-out-s">why?</xref>
						</mrow>
						<mrow> 
								\amp= -\frac{1}{s} \Big[ \ub{\lim_{b \to \infty} e^{-sb}}_{L} - \us{=\ 1}{\ub{\lim_{b \to \infty} 1}} \Big] 
						</mrow>
					</md>
				</p>
		
				<p>
					Let's analyze the remaining limit, <m>L</m>, which depends on the value of <m>s</m>. 
					<line>Note: the <m>\frac{1}{s}</m> term in front of the limit implies <m>s \ne 0</m>.</line>
					<ul>
						<li>
							<p>
								<line><m>s &lt; 0:\ </m> Since <m>\ds e^{-(\text{negative})b} = e^{(\text{positive})b} \to \infty</m> as <m>b \to \infty</m></line>
								<line><m>\hspace{4.0em} \implies\ </m> limit diverges (does not exist) when <m>s &lt; 0</m>.</line>
							</p>
						</li>
						<li>
							<p>
								<line><m>s &gt; 0:\ </m> Since <m>\ds e^{-(\text{positive})b} = e^{(\text{negative})b} \to 0</m> as <m>b \to \infty</m></line>
								<line><m>\hspace{4.0em} \implies\ </m> limit converges (exists) when <m>s &gt; 0</m>.</line>
							</p>
						</li>
					</ul>
					To visualize this, here is a <xref ref="compare-exp-graphs" text="custom">graph</xref> comparing <m>s=-1.2\ </m> versus <m>\, +1.2</m>.
				</p>
		
				<p>
					Therefore, when <m>s &gt; 0</m> the Laplace transform exists and evaluates to
					<me>\lap\{1\} = -\frac{1}{s} [0 - 1] = \frac{1}{s} \quad \text{for } s \gt 0.</me>
				</p>
			</solution>
		
		</example>

		<p>
			Now that you've seen an example, let's discuss a few important points:

			<ul marker="square">
				<li>
					<p>
						The integral, <m>I</m>, in <xref ref="lt-1-example-eqn-1"/> was initially a function of both <m>s</m> and <m>b</m>, but after evaluating the limit, it became a function of <m>s</m> alone. In general, every Laplace transform results in a function of <m>s</m>, and it's customary to denote the Laplace transform of a function <m>f(t)</m> as <m>F(s)</m>. For example,
						<me> \lap\{f(t)\} = F(s) \quad \text{or} \quad \lap\{q(t)\} = Q(s).</me>
					</p>
				</li>
				<li>
					<p>
						We also identified the values of <m>s</m> for which the integral converges. While these values are important, they generally do not affect the solution of the differential equations in practice. Nonetheless, we will continue to note them as we build our Laplace transform toolbox.
					</p>
				</li>
				<li>
					<p>
						The notation for the Laplace transform involves the symbol <m>\lap.</m> The curly braces that accompany it are not optional; they indicate precisely which function we are transforming.
					</p>
				</li>
			</ul>
		</p>

		<p>
			At this point, we've introduced our first “common” Laplace transform—a transform that will recur frequently. As we proceed through this chapter, we'll add more transforms to this list.
		</p>

		<assemblage xml:id="lt-table-L1"><title>Common Laplace Transform <m>L_1</m></title>
			<p>
				<dl width="narrow">
					<li xml:id="L1"><title><m>{\LARGE \vphantom{\int}}L_1</m></title>
						<m>\ds \lap\{ 1 \} = \frac{1}{s}, \quad s &gt; 0 </m>
					</li>
				</dl>
			</p>
		</assemblage>

		<xi:include href="./c4-s1-ss2-interactives.ptx" />

	</subsection>

	<subsection xmlns:xi="http://www.w3.org/2001/XInclude"><title><m>\lap\{e^{at}\}</m></title>

		<p>
			The exponential function is commonly encountered in differential equations, making its Laplace transform especially important. Let's explore the Laplace transform of the exponential function <m>e^{at}</m>, where <m>a</m> is a constant. We'll start with a specific example, setting <m>a = 7</m>, and then generalize the result.
		</p>

		<example>

			<m>\quad</m> Compute <m> \lap \{ e^{7t} \} </m>.

			<solution>
				<p>
					We begin by applying the definition of the Laplace transform:
					<md>
						<mrow> \lap\{ e^{7t} \} \amp= \int_0^{\infty} e^{7t} \cdot e^{-st}\, dt </mrow>
						<mrow> \amp= \lim_{b \to \infty}\int_0^b e^{(7-s)t}\, dt </mrow>
					</md>
					For this improper integral to converge, the exponent <m>7-s</m> must be negative, meaning:
					<me> 7 - s \lt 0 \hspace{0.5cm}\Rightarrow \hspace{0.5cm} s \gt 7. </me>
					Thus, we proceed under the assumption that <m>s \gt 7</m>.
					<md>
						<mrow> 
							\lap\{ e^{7t} \} 
								\amp= \lim_{b \to \infty}\int_0^b e^{(7-s)t}\, dt
						</mrow>
						<mrow> 
								\amp= \lim_{b \to \infty} \frac{1}{7-s} e^{(7-s)t} \Bigg|_0^b
						</mrow>
						<mrow> 
								\amp= \frac{1}{7-s} \left[ \lim_{b \to \infty} \left( e^{(7-s)b} - e^{0} \right) \right]
						</mrow>
						<mrow> 
								\amp= \frac{1}{7-s} \left[ \lim_{b \to \infty} e^{(7-s)b} - 1 \right]
						</mrow>
						<mrow>
								\amp= \frac{1}{7-s} \left[ 0 - 1 \right] \qquad \Big(e^{(\text{negative})b} \to 0\Big)
						</mrow>
						<mrow>
								\amp= \frac{-1}{7-s} = \frac{1}{s-7}. \quad \text{for } s \gt 7
						</mrow>
					</md>
					Thus, the Laplace transform of <m>e^{7t}</m> is:
					<me>\ds \lap\{e^{7t}\} = \frac{1}{s - 7}, \quad s \gt 7.</me>
				</p>
			</solution>

		</example>

		<p>
			To generalize this result, let's replace <m>7</m> with a constant <m>a</m>.
		</p>

		<example>

			<m>\quad</m> Show that <m>\ds \lap \{ e^{at} \} = \frac{1}{s - a} </m>.

			<solution>
				<p>
					We follow a similar process, starting with the definition of the Laplace transform:
					<md>
						<mrow> \lap\{ e^{at} \} \amp= \int_0^{\infty} e^{at} \cdot e^{-st}\, dt </mrow>
						<mrow> \amp= \lim_{b \to \infty}\int_0^b e^{(a-s)t}\, dt </mrow>
					</md>
					For the integral to converge, the exponent <m>a-s</m> must be negative, which requires <m>\ a - s \lt 0\ </m> or <m>\ s \gt a</m> to proceed
					<md>
						<mrow> \lap\{ e^{at} \} \amp= \lim_{b \to \infty}\int_0^b e^{(a-s)t}\, dt </mrow>
						<mrow> \amp= \lim_{b \to \infty} \frac{1}{a-s} e^{(a-s)t} \Bigg|_0^b </mrow>
						<mrow> \amp= \frac{1}{a-s} \left[ \lim_{b \to \infty} \left( e^{(a-s)b} - e^{0} \right) \right] </mrow>
						<mrow> \amp= \frac{1}{a-s} \left[ \lim_{b \to \infty} e^{(a-s)b} - 1 \right] </mrow>
						<mrow> \amp= \frac{1}{a-s} \left[ 0 - 1 \right] </mrow>
						<mrow> \amp= \frac{-1}{a-s} = \frac{1}{s-a}. \quad \text{for } s \gt a </mrow>
					</md>
					Thus, the Laplace transform of <m>e^{at}</m> is:
					<me>\ds \lap\{e^{at}\} = \frac{1}{s - a}, \quad s \gt a.</me>
				</p>
			</solution>

		</example>

		<p>
			With this result, we can now add the Laplace transform of <m>e^{at}</m> to our list of common Laplace transforms.
		</p>

		<assemblage xml:id="lt-table-L2"><title>Common Laplace Transform <m>L_2</m></title>
			<p>
				<dl width="narrow">
					<li xml:id="L2"><title><m>{\LARGE \vphantom{\int}}L_2</m></title>
						<m>\ds \lap\{ e^{at} \} = \frac{1}{s - a}, \quad s \gt a, \quad a \text{ is a constant} </m>
					</li>
				</dl>
			</p>
		</assemblage>

		<xi:include href="./c4-s1-ss3-interactives.ptx" />

	</subsection>

	<subsection xmlns:xi="http://www.w3.org/2001/XInclude"><title><m>\lap\{t^n\}</m></title>

		<p>
			Next, we'll explore the Laplace transform of the power function <m>t^n</m>, where <m>n</m> is a non-negative integer. We've already encountered the case where <m>n = 0</m>, since <m>t^0 = 1</m> and its transform is given by <xref ref="L1" text="custom"><m>L_1</m></xref>. Now, let's start with <m>n = 1</m> and work our way up to find a general formula for the Laplace transform of <m>t^n</m>.
		</p>

		<example>
			<p>
				Compute <m>\lap\{t\}</m>.
			</p>

			<solution>
				<p>
					We'll begin by applying the definition of the Laplace transform:
					<md>
						<mrow> 
							\lap\{ t \}
								\amp= \int_0^{\infty} t \cdot e^{-st}\, dt 
						</mrow>
						<mrow> 				
								\amp= \lim_{b \to \infty} \int_0^b t e^{-st}\, dt \quad (s \ne 0) \quad <xref text="custom" ref="LT-s-ne-0-t">Why is <m>s \ne 0</m>?</xref>
						</mrow>
					</md>
					Using integration by parts, we have:
					<md>
						<mrow> 
							\phantom{\lap\{t\}}
								\amp= \lim_{b \to \infty} \left[-\frac{b}{s}e^{-sb} + \frac{1}{s^2}\right] \quad <xref text="custom" ref="reason-int-by-parts-texpt">Integration by parts</xref>
						</mrow>
					</md>
					As <m>b</m> approaches infinity:
					<md>
						<mrow> 
							\phantom{\lap\{t\}}
								\amp= \left[-\frac{1}{s}\lim_{b \to \infty}\frac{b}{e^{sb}} + \frac{1}{s^2}\right] \quad (s &gt; 0) \quad <xref text="custom" ref="LT-s-gt-0-t">\text{Why is } s &gt; 0?</xref>
						</mrow>
						<mrow> 
							\phantom{\lap\{t\}}
								\amp= \left[0 + \frac{1}{s^2}\right] \quad <xref text="custom" ref="reason-limit-to-zero-t">Why is the limit 0?</xref>
						</mrow>
						<mrow> 		
								\amp= \frac{1}{s^2}, \quad s \gt 0
						</mrow>
					</md>
					Therefore, <m>\ds \lap\{ t \} = \frac{1}{s^2}</m>, valid for <m>s &gt; 0</m>.
				</p>
			</solution>
		</example>

		<p>
			Using similar steps, we can derive the following results:
		</p>

		<example>
			<p>
				<ul marker="square">
					<li>	
						<m> \ds \lap\{t^2\} = \frac{2}{s^3}, \quad s \gt 0 \quad </m> <xref ref="std_LT_01" text="custom">Solution</xref>
					</li>
					<li>	
						<m> \ds \lap\{t^3\} = \frac{6}{s^4}, \quad s \gt 0 \quad </m> <xref ref="std_LT_02" text="custom">Solution</xref> 
					</li>
					<li>
						<m> \ds \lap\{t^4\} = \frac{24}{s^5}, \quad s \gt 0 \quad </m> <xref ref="std_LT_03" text="custom">Solution</xref> 
					</li>
				</ul>
			</p>
		</example>

		<p>
			Do you notice the emerging pattern? Let's rewrite the numerators:
			<ul marker="">
				<li>	
					<m> \ds \lap\{t^2\} = \frac{2}{s^3} = \frac{2 \cdot 1}{s^3} = \frac{2!}{s^3} </m>
				</li>
				<li>	
					<m> \ds \lap\{t^3\} = \frac{6}{s^4} = \frac{3 \cdot 2 \cdot 1}{s^4} = \frac{3!}{s^4} </m>
				</li>
				<li>
					<m> \ds \lap\{t^4\} = \frac{24}{s^5} = \frac{4 \cdot 3 \cdot 2 \cdot 1}{s^5} = \frac{4!}{s^5} </m>
				</li>
				<li>
					<m> \hspace{6em} \vdots </m>
				</li>
				<li>
					<m> \ds \lap\{t^n\} = \frac{n!}{s^{n+1}} </m>
				</li>
			</ul>
			Thus, the general formula for the Laplace transform of <m>t^n</m> is:
			<me>\ds \lap\{t^n\} = \frac{n!}{s^{n+1}}, \quad s &gt; 0.</me>
		</p>

		<assemblage xml:id="lt-table-L3"><title>Common Laplace Transform <m>L_3</m></title>
			<p>
				<dl width="narrow">
					<li xml:id="L3"><title><m>{\LARGE \vphantom{\int}}L_3</m></title>
						<m>\ds \lap\{ t^n \} = \frac{n!}{s^{n+1}}, \quad s &gt;0, \quad n = 1, 2, 3, \ldots </m>
					</li>
				</dl>
			</p>
		</assemblage>

		<xi:include href="./c4-s1-ss4-interactives.ptx" />

	</subsection>

	<subsection xmlns:xi="http://www.w3.org/2001/XInclude"><title> <m>\lap\{\sin(bt)\},\ \lap\{\cos(bt)\}</m> </title>

		<p>
			In this section, we will explore the Laplace transforms of the sine and cosine functions. These transforms are particularly important because sine and cosine frequently appear in the solutions of differential equations.
		</p>

		<example>

			<m>\quad</m>Compute <m>\lap\{\cos(3t)\}</m>.
			
			<solution>
				<p>
					We start by applying the definition of the Laplace transform:
					<me>
						\lap \{ \cos(3t) \} = \int_0^{\infty} e^{-st} \cos(3t)\, dt 
					</me>.
					While we could proceed with integration by parts, a more efficient approach is to use the Euler's formula representation of cosine:
					<me>
						\cos(3t) = \frac{e^{3it} + e^{-3it}}{2}.
					</me>
					Substituting this into the integral gives:
					<md>
						<mrow> 
							\lap \{ \cos(3t) \} 
								=\amp \frac{1}{2} \int_0^{\infty} e^{-st} \left(e^{3it} + e^{-3it}\right)\, dt 
						</mrow>
						<mrow>
							=\amp \frac{1}{2} \left[\int_0^{\infty} e^{-(s - 3i)t}\, dt + \int_0^{\infty} e^{-(s + 3i)t}\, dt\right]
						</mrow>
						<mrow>
							=\amp \frac{1}{2} \left[\lap\{e^{3it}\} + \lap\{e^{-3it}\}\right].
						</mrow>
					</md>
					Using the known Laplace transforms for exponential functions, we have:
					<md>
						<mrow>
							\lap \{ \cos(3t) \} 
								=\amp \frac{1}{2} \left[\frac{1}{s - 3i} + \frac{1}{s + 3i}\right]
						</mrow>
						<mrow>
							=\amp \frac{1}{2} \left[\frac{s + 3i + s - 3i}{(s - 3i)(s + 3i)}\right]
						</mrow>
						<mrow>
							=\amp \frac{s}{s^2 + 9}.
						</mrow>
					</md>
					Therefore, the Laplace transform of <m>\cos(3t)</m> is:
					<me>
						\lap \{\cos(3t)\} = \frac{s}{s^2 + 9}.
					</me>
				</p>
			</solution>
		</example>

		<example>

			<m>\quad</m>Compute <m>\lap\{\sin(-4t)\}</m>.

			<solution>
				<p>
					Again, we begin with the definition of the Laplace transform:
					<me>
						\lap \{ \sin(-4t) \} = \int_0^{\infty} e^{-st} \sin(-4t)\, dt.
					</me>
					As with the cosine, we can use the Euler's formula for sine:
					<me>
						\sin(-4t) = \frac{e^{-4it} - e^{4it}}{2i}.
					</me>
					Substituting this into the integral, we get:
					<md>
						<mrow> 
							\lap \{ \sin(-4t) \} 
								=\amp \frac{1}{2i} \int_0^{\infty} e^{-st} \left(e^{-4it} - e^{4it}\right)\, dt 
						</mrow>
						<mrow>
							=\amp \frac{1}{2i} \left[\int_0^{\infty} e^{-(s + 4i)t}\, dt - \int_0^{\infty} e^{-(s - 4i)t}\, dt\right]
						</mrow>
						<mrow>
							=\amp \frac{1}{2i} \left[\lap\{e^{-4it}\} - \lap\{e^{4it}\}\right].
						</mrow>
					</md>
					Substituting the known Laplace transforms, we have:
					<md>
						<mrow>
							\lap \{ \sin(-4t) \} 
								=\amp \frac{1}{2i} \left[\frac{1}{s + 4i} - \frac{1}{s - 4i}\right]
						</mrow>
						<mrow>
							=\amp \frac{1}{2i} \left[\frac{s - 4i - (s + 4i)}{(s + 4i)(s - 4i)}\right]
						</mrow>
						<mrow>
							=\amp \frac{4}{s^2 + 16}.
						</mrow>
					</md>
					Thus, the Laplace transform of <m>\sin(-4t)</m> is:
					<me>
						\lap \{\sin(-4t)\} = \frac{4}{s^2 + 16}.
					</me>
				</p>
			</solution>
		</example>

		<p>
			We can generalize these results by replacing <m>3</m> and <m>4</m> with <m>b</m> in the above examples. The updated common transforms are as follows:
		</p>

		<assemblage xml:id="lt-table-L4-L5"><title>Common Laplace Transforms <m>L_3</m>, <m>L_4</m></title>
			<p>
				<dl width="narrow">
					<li xml:id="L4"><title><m>{\LARGE \vphantom{\int}}L_4</m></title>
						<m>\ds \lap\{ \sin(bt) \} = \frac{b}{s^2+b^2}, \quad s &gt;0, \quad b \text{ is a constant} </m>
					</li>
					<li xml:id="L5"><title><m>{\LARGE \vphantom{\int}}L_5</m></title>
						<m>\ds \lap\{ \cos(bt) \} = \frac{s}{s^2+b^2}, \quad s &gt;0, \quad b \text{ is a constant} </m>
					</li>
				</dl>
			</p>
		</assemblage>

		<xi	href="./c4-s1-ss5-interactives.ptx" />

	</subsection>

</section>