<section xmlns:xi="http://www.w3.org/2001/XInclude"><title> Finding the Integrating Factor </title>	

	<introduction>

		<p>
			In the previous section, we saw that rewriting a first-order linear differential equation so that one side is a <q>completed</q> derivative allows us to solve it using direct integration. However, many equations do not initially have this form.
		</p>

		<p>
			The key to overcoming this issue is finding a function‚Äîcalled the <term>integrating factor</term>‚Äîthat, when multiplied onto the equation, transforms it into a single derivative. That is, given the standard form:
		</p>

		<men xml:id="if-standard-form00">
			\frac{dy}{dx} + P(x) y = Q(x),
		</men>

		<p>
			we seek a function <m>\mu(x)</m> such that:
		</p>

		<men xml:id="if-completed-derivative">
			\frac{d}{dx} [\mu(x) y] = \mu(x) Q(x).
		</men>

		<p>
			This section focuses on systematically determining <m>\mu(x)</m> for any first-order linear differential equation. We begin with an example that illustrates the core idea, then generalize the approach to derive a general formula.
		</p>

		<p>
			By the end of this section, you will be able to:
		</p>

		<p>
			<sidebyside widths="2% 5% 93%" valign="top">
				<p/><p> 1Ô∏è‚É£</p>
				<p>Recognize when a first-order linear equation requires an integrating factor.</p>
			</sidebyside>
			<sidebyside widths="2% 5% 93%" valign="top">
				<p/><p> 2Ô∏è‚É£</p>
				<p>Use a step-by-step approach to determine <m>\mu(x)</m>.</p>
			</sidebyside>
			<sidebyside widths="2% 5% 93%" valign="top">
				<p/><p> 3Ô∏è‚É£</p>
				<p>Understand why the integrating factor method always works.</p>
			</sidebyside>
		</p>

		<p>
			Before moving on, remember these key points:
		</p>

		<p>
			<sidebyside widths="2% 5% 93%" valign="top">
				<p/><p>‚úÖ</p>
				<p>A derivative can be <q>completed</q> in <em>any</em> first-order linear equation.</p>
			</sidebyside>
			<sidebyside widths="2% 5% 93%" valign="top">
				<p/><p>‚úÖ</p>
				<p>The equation must be multiplied by a function to complete the derivative.</p>
			</sidebyside>
			<sidebyside widths="2% 5% 93%" valign="top">
				<p/><p>‚úÖ</p>
				<p>The completed derivative is formed by reversing the product rule.</p>
			</sidebyside>
		</p>

		<p>
			Now, let's explore how to find the integrating factor step by step.
		</p>

	</introduction>

	<subsection><title> A Motivating Example </title>
		
		<introduction>
			<p>
				In the previous section, we saw that certain first-order linear differential equations can be rewritten so that the left-hand side is a single derivative. However, most equations do not initially have this structure. Instead, they are missing a crucial function that allows us to apply the <em>product rule in reverse</em>.
			</p>

			<p>
				The goal now is to illustrate how to determine this missing function‚Äîknown as the <term>integrating factor</term>‚Äîso that we can rewrite one of the sides as a single derivative.
			</p>

			<p>
				Consider the equation:
			</p>

			<men xml:id="if-example-incomplete-eqn">
				\frac{dy}{dx} + 2y = 5.
			</men>

			<p>
				The claim is that the left side of this equation is currently an incomplete product rule that can be completed and reversed by multiplying a function <m>\mu</m> onto both sides of the equation. In short, this allows us to rewrite <xref ref="if-example-incomplete-eqn"/> as
			</p>

			<me>
				\frac{d}{dx} \left[\mu y \right] = 5\mu.
			</me>

			<p>
				However, the question still remains: <em>Which function, <m>\mu</m>, does this?</em> Let's find out.
			</p>

		</introduction>

		<subsubsection><title> Finding <m>\mu(x)</m>: A Step-by-Step Breakdown </title>

			<p>
				The strategy for determining <m>\mu(x)</m> can be visualized in <xref ref="if-strategy-1"/> or with the optional slide show, below.
			</p>

			<theorem><title> Finding <m>\mu</m> Slide Show for Equation <xref ref="if-example-incomplete-eqn"/> </title>
				<statement>
					<p>
						<interactive xml:id="if-derivation-interactive" platform="javascript" width="88%" aspect="1.75:1" source="code/if-example-slide-show-1.js" preview="figures/if-strategy-3.png">
							<slate width="88%" aspect="1.75:1" xml:id="if-derivation-canvas" surface="canvas" />
						</interactive>
					</p>
				</statement>
			</theorem>

			<figure xml:id="if-strategy-1">
				<caption>A visual illustration of how to find <m>\mu(x)</m> given that we want to rewrite the <em>Starting Equation</em> <xref ref="starting-equation"/> as the <em>Goal Equation</em> <xref ref="goal-equation"/>.</caption>
				
				<sidebyside valign="middle" halign="right left" widths="10% 26% 45% 19%">
					<p/>
					<p>
						1Ô∏è‚É£  Multiply by <m>\ds\mu\ \left\lbrace\begin{array}{c}\\\\\\\end{array}\right.</m>
					</p>
					<p>
						<mdn>
							<mrow xml:id="starting-equation">
								\frac{dy}{dx} + 2 y \amp = 5
							</mrow>
							<mrow xml:id="middle-equation-1">
								\mu\frac{dy}{dx} + {\color{blue} \us{\downarrow}{\boxed{ 2\mu }}} y\amp = 5\mu
							</mrow>
						</mdn>
					</p>
					<p/>
				</sidebyside>

				<sidebyside valign="middle" halign="right left" widths="10% 26% 45% 19%">
					<p/>
					<p>
						3Ô∏è‚É£ Condition on <m>\mu</m>
					</p>
					<p>
						<me>
							{\color{blue} \boxed{\frac{d\mu}{dx} = 2\mu}}
						</me>
					</p>
					<p/>
				</sidebyside>

				<sidebyside valign="bottom" halign="right left" widths="10% 26% 45% 19%">
					<p/>
					<p>
						2Ô∏è‚É£ Product Rule <m>\ds\ \left\lbrace\vphantom{\begin{array}{c}\\\\\\\end{array}}\right.</m>
					</p>
					<p>
						<mdn>
							<mrow xml:id="middle-equation-2">	\mu\frac{dy}{dx} + {\color{blue} \os{\uparrow}{\boxed{\frac{d\mu}{dx}}}} y	\amp = 5 \mu </mrow>
							<mrow xml:id="goal-equation">	\frac{d}{dx} \left[\mu y \right]	\amp = 5\mu </mrow>
						</mdn>
					</p>
					<p/>
				</sidebyside>
			</figure>

			<p>
				The details of each step is broken down, in order, as follows:
			</p>

			<p>
				<sidebyside widths="2% 6% 92%">
					<p/>
					<p>
						1Ô∏è‚É£
					</p>
					<p>
						Multiply <xref ref="starting-equation"/> by <m>\mu</m> to get <xref ref="middle-equation-1"/>.
					</p>
				</sidebyside>

				<sidebyside widths="2% 6% 92%">
					<p/>
					<p>
						2Ô∏è‚É£
					</p>
					<p>
						Use the product rule on the left side of <xref ref="goal-equation"/> to get <xref ref="middle-equation-2"/>.
					</p>
				</sidebyside>

				<sidebyside widths="2% 6% 92%">
					<p/>
					<p>
						3Ô∏è‚É£
					</p>
					<p>
						In order for <xref ref="starting-equation"/> and <xref ref="goal-equation"/> to be equal, <xref ref="middle-equation-1"/> and <xref ref="middle-equation-2"/> must also be equal. Therefore, we arrive at the following condition on <m>\mu</m>:
						<men xml:id="if-condition-equation">
							\frac{d\mu}{dx} = 2\mu
						</men>.
					</p>
				</sidebyside>
			</p>

			<p>
				This is a <term>separable differential equation</term>, which has the general solution
				<me>
					\mu(x) = ce^{2x}
				</me>.
			</p>

			<p>
				Although, any non-zero choice for <m>c</m> will yield a function that converts <xref ref="starting-equation"/> into <xref ref="goal-equation"/>, the convention is to chose <m>c=1</m>. Therefore, the integrating factor for equation <xref ref="if-example-incomplete-eqn"/> is <m>\mu(x) = e^{2x}</m>.
			</p>

			<theorem><title>Solving Equation <xref ref="if-condition-equation"/></title>
				<statement>
					<p>
						<md>
							<mrow>	\frac{d\mu}{dx} = 2\mu \quad \implies \quad
									\frac{1}{\mu}\ d\mu			\amp = 2 dx			</mrow>
							<mrow>	\int \frac{1}{\mu}\ d\mu	\amp = \int 2 dx	</mrow>
							<mrow>	\ln|\mu|					\amp = 2x + c		</mrow>
							<mrow>	\mu(x)						\amp = ce^{2x}		</mrow>
						</md>
					</p>
				</statement>
			</theorem>

		<xi:include href="./c4-exercises/c4-chkpts-2-1-motivating-example.ptx" />

		</subsubsection>

		<conclusion>
			<p>
				By multiplying <xref ref="if-example-incomplete-eqn"/> by <m>e^{2x}</m>, we are able to transform it into:
			</p>

			<me>
				\frac{d}{dx} \left[ e^{2x} y \right] = 5e^{2x}.
			</me>

			<p>
				Once in this form, we can solve for <m>y</m> using direct integration. This example demonstrates how to find the integrating factor for a specific equation. Next, we will generalize this idea by finding a formula that gives <m>\mu</m> for any first-order linear differential equation.
			</p>
		</conclusion>

	</subsection>

	<subsection><title> The General Integrating Factor Formula </title>

		<introduction>

			<p>
				We are now ready to determine the general formula for <m>\mu</m> given <em>any</em> first-order linear differential equation. Before we can find <m>\mu</m>, we must first put our equation in <term>standard form</term>, given by
			</p>

			<men xml:id="if-standard-form">
				\frac{dy}{dx} + P(x)\ y = Q(x)
			</men>.

			<p>
				Now, we want the function, <m>\mu</m>, we multiply onto <xref ref="if-standard-form"/> to write it in the form
			</p>

			<men xml:id="if-combined-form">
				\frac{d}{dx} \left[ \mu y \right] = \mu Q(x).
			</men>

			<theorem xml:id="std-form-explained0"><title> <em>Why All 1st-Order Linear Equations have a Standard Form</em> </title>
		
				<statement>
					<p>
						All first-order linear differential equations contain at most, <m>y'</m> terms, <m>y</m> terms, and constant terms, allowing you to organize such an equation as
						<me>
							A(x)y' + B(x)y = C(x)
						</me>.
						Dividing both sides by the leading coefficient, <m>A(x)</m>, and renaming the <m>y</m> and constant coefficients as <m>P</m> and <m>Q</m>, gives the standard form
						<me>
							y' + \us{P(x)}{\ub{\frac{B(x)}{A(x)}}}y	= \us{Q(x)}{\ub{\frac{C(x)}{A(x)}}}	
							\quad \implies \quad
							y' + P(x)y	= Q(x)
						</me>.
					</p>
				</statement>

			</theorem>

		</introduction>

		<subsubsection><title> Deriving the Formula </title>

			<p>
				As with the motivating example, we start by multiplying both sides of the differential equation by an unknown function <m>\mu</m>:
			</p>

			<men xml:id="if-mu-standard-form">
				\mu \frac{dy}{dx} + \mu P(x) y = \mu Q(x).
			</men>

			<p>
				The left side can only turn into <m>\frac{d}{dx} \left[ \mu y \right]</m>, if it is also equal to this derivative's expanded product rule form. In particular, we need the following to be true:
			</p>

			<me>
				\ob{
					\mu \frac{dy}{dx} + \us{\Large üö©}{\ul{\mu P(x)}}\ y
				}^{\large\text{left-side of }<xref ref="if-mu-standard-form"/>} = 
				\ob{
					\mu \frac{dy}{dx} + \us{\Large üö©}{\ul{\frac{d\mu}{dx}}}\ y
				}^{\large\text{expanded }\frac{d}{dx} \left[ \mu y \right]} 
			</me>.

			<p>
				As you can see, the two sides are identical, except for the flagged üö© expressions. This means, <xref ref="if-mu-standard-form"/> can only be written as <xref ref="if-combined-form"/> if <m>\mu</m> also satisfies 
			</p>

			<men xml:id="if-sov-eqn">
				\frac{d\mu}{dx} = \mu P(x).
			</men>

			<p>
				To find such a function, <m>\mu</m>, we solve equation <xref ref="if-sov-eqn"/> using separation of variables.
			</p>

			<sidebyside widths="15% 25% 45% 15%" valign="middle">
				<p/>
				<p>
					Separate:
				</p>
				<p>
					<me>
						\frac{1}{\mu}\ d\mu = P(x)\ dx
					</me>
				</p>
				<p/>
			</sidebyside>

			<sidebyside widths="15% 25% 45% 15%" valigns="top middle middle middle">
				<p/>
				<p>
					Integrate:
				</p>
				<p>
					<md>
						<mrow>	\int \frac{1}{\mu}\ d\mu	\amp = \int P(x)\ dx	</mrow>  
						<mrow>	\ln|\mu|					\amp = \int P(x) dx		</mrow>
					</md>
				</p>
				<p/>
			</sidebyside>

			<aside>
				<p>
					<term>üìå Note.</term> The absolute value is dropped since the sign of the integrating factor is taken to be positive by convention.
				</p>
			</aside>

			<sidebyside widths="15% 28% 42% 15%" valign="middle">
				<p/>
				<p>
					Solve for <m>\mu(x)</m>:
				</p>
				<p>
					<me>
						\mu(x) = e\vphantom{\sum}^{{\Large\int} P(x)\ dx}
					</me>.
				</p>
				<p/>
			</sidebyside>

			<assemblage xml:id="integrating-factor-general-formula"><title> Integrating Factor: General Formula </title>
				<p>
					The <term>integrating factor</term> for a first-order linear differential equation in standard form
					<me>
						y' + P(x)y = Q(x)
					</me>
					is given by	
					<m>
						\ \ds\mu(x) = e\vphantom{\sum}^{{\Large\int} P(x)\ dx}
					</m>.
				</p>
			</assemblage>

			<p>
				Now that we have derived the general formula, let's apply it to a few examples.
			</p>

		</subsubsection>

		<subsubsection><title> Examples of Integrating Factors </title>
			
			<example xml:id="integrating-factor-basic-example"><title> Basic Integrating Factor </title>

				<p>
					<statement>
						<p>
							Find the integrating factor <m>\mu(x)</m> for the differential equation:
						</p>

						<me>
							\frac{dy}{dx} + 4y = x.
						</me>
					</statement>
				</p>
			
				<solution>
					<p>
						The equation is in standard form with <m>P(x) = 4</m>. Using the formula:
					</p>

					<me>
						\mu(x) = e^{\int P(x) dx} = e^{\int 4 dx} = e^{4x}
					</me>.

					<p>
						Thus, the integrating factor is <m>e^{4x}</m>.
					</p>
				</solution>
			</example>

			<example xml:id="integrating-factor-log-example"><title> Integrating Factor with a Log Function </title>

				<p>
					<statement>
						<p>
							Determine the integrating factor <m>\mu(x)</m> for the differential equation:
						</p>

						<me>
							\frac{dy}{dx} + \frac{2}{x} y = x^3, \quad x > 0.
						</me>
					</statement>
				</p>

				<solution>
					<p>
						The equation is in standard form with <m>P(x) = \frac{2}{x}</m>. Using the formula:
					</p>

					<me>
						\mu(x) = e^{\int P(x) dx} = e^{\int \frac{2}{x} dx}.
					</me>

					<p>
						Evaluating the integral:
					</p>

					<me>
						\mu(x) = e^{2 \ln x} = x^2.
					</me>

					<p>
						Thus, the integrating factor is <m>x^2</m>.
					</p>
				</solution>
			</example>

			<example xml:id="integrating-factor-trig-example"><title> Integrating Factor with a Trigonometric Function </title>

				<p>
					<statement>
						<p>
							Compute the integrating factor <m>\mu(x)</m> for the differential equation:
						</p>

						<me>
							\frac{dy}{dx} + \tan x \cdot y = \cos x.
						</me>
					</statement>
				</p>

				<solution>
					<p>
						The equation is in standard form with <m>P(x) = \tan x</m>. Using the formula:
					</p>

					<me>
						\mu(x) = e^{\int P(x) dx} = e^{\int \tan x dx}.
					</me>

					<p>
						Evaluating the integral:
					</p>

					<me>
						\mu(x) = e^{\ln | \sec x |} = \sec x.
					</me>

					<p>
						Thus, the integrating factor is <m>\sec x</m>.
					</p>
				</solution>
			</example>

		</subsubsection>

		<conclusion>
		
			<p>
				In this section, we derived the general formula for the integrating factor and demonstrated how to compute it with a few examples. The key takeaway is that the integrating factor always takes the form
			</p>

			<me>
				\mu(x) = e^{\int P(x) dx}
			</me>,

			<p>
				and once we have it, we can multiply it onto our equation to rewrite the left-hand side as a single derivative. In the next section, we will apply this approach step-by-step to solve first-order linear differential equations.
			</p>

		</conclusion>

		<xi:include href="./c4-exercises/c4-chkpts-2-2-general-integrating-factor.ptx" />

	</subsection>
	
</section>