<section xmlns:xi="http://www.w3.org/2001/XInclude"><title> Integrating Factor Method </title>	
	
	<introduction>

		<p>
			The <term>Integrating Factor (IF) Method</term> is a systematic approach for solving <em>any</em> first-order linear differential equation. The key idea is to transform the equation into a form where the left-hand side becomes a single derivative, allowing us to solve it using direct integration.
		</p>

		<p>
			Before diving in, let's recap the integrating factor story so far ...
		</p>

		<p>
			<sidebyside widths="5% 5% 90%" valign="top">
				<p/><p>ðŸ“Œ</p>
				<p>First-order linear equations can always be written in <xref ref="if-standard-form" text="custom"><term>standard form</term></xref>.</p>
			</sidebyside>
			<sidebyside widths="5% 5% 90%" valign="top">
				<p/><p>ðŸ“Œ</p>
				<p>From standard form, the equation is multiplied by an <xref ref="if-standard-form" text="custom"><term>integrating factor</term></xref>, which provides the part needed to reverse a product rule.</p>
			</sidebyside>
			<sidebyside widths="5% 5% 90%" valign="top">
				<p/><p>ðŸ“Œ</p>
				<p>Reversing the product rule completes a derivative on the left so that direct integration can be use to find the general solution.</p>
			</sidebyside>
		</p>

		<p>
			Here is what this process looks like on an equation we have seen before:
		</p>

		<p>
			<sidebyside valign="top" widths="5% 30% 60% 5%">
				<p/>
				<p>
					Standard Form:
				</p>
				<p>
					<md>
						<mrow>
							\frac{dy}{dx} + 2 y = 5
						</mrow>
						<mrow>
							\phantom{\text{ Multiply by } e^{2x}} \downarrow \text{ Multiply by } e^{2x}
						</mrow>
					</md>
				</p>
				<p/>
			</sidebyside>
			<sidebyside valign="top" widths="5% 30% 60% 5%">
				<p/>
				<p>
					Standard Form with integrating factor:
				</p>
				<p>
					<md>
						<mrow>
							e^{2x}\frac{dy}{dx}	+ 2e^{2x} y = 5e^{2x}
						</mrow>
						<mrow>
							\phantom{\text{ Reverse Product Rule}} \downarrow \text{ Reverse Product Rule}
						</mrow>
					</md>
				</p>
				<p/>
			</sidebyside>
			<sidebyside valign="middle" widths="5% 30% 60% 5%">
				<p/>
				<p>
					Completed Derivative:
				</p>
				<p>
					<md>
						<mrow>
							\frac{d}{dx} \left[e^{2x} y \right] = 5e^{2x}
						</mrow>
						<!-- <mrow>
							\phantom{\text{Direct Integration}} \downarrow \text{Direct Integration}
						</mrow> -->
					</md>
				</p>
				<p/>
			</sidebyside>
		</p>

		<p>
			In this section, we will break down this method, guiding you step by step, until we reach the final solution.
		</p>

	</introduction>

	<subsection><title> Method Steps </title>

		<introduction>
			<p>
				The integrating factor method is a step-by-step process that works for all first-order linear differential equations and is summarized as follows.
			</p>
		</introduction>

		<aside>
			<p>
				<term>ðŸ“Œ Note.</term> By convention, the integration constant is ignored in the integrating factor since any nonzero multiple of <m>\mu</m> will still work to reverse the product rule.
			</p>
		</aside>

		<exploration xml:id="if-method"><title> Integrating Factor (IF) </title>

			<p>
				Given a first-order linear equation in standard form:
			</p>

			<men xml:id="if-steps-standard-form">
				y' + P(x) y = Q(x),
			</men>

			<p>
				the general solution can be found through the following <em>three-step process</em>:
			</p>

			<dl width="narrow">

				<li xml:id="if-step-1"><title> Step 1: Find the Integrating Factor </title>

					<p>
						Identify <m>P(x)</m> and compute the <em>integrating factor</em>:
					</p>

					<p>
						<me>
							\mu = e\vphantom{\large|}^{\textstyle\int P(x)\ dx}
						</me>.
					</p>
					
				</li>

				<li xml:id="if-step-2"><title> Step 2: Multiply by <m>\mu</m> to Complete the Derivative </title>

					<p>
						Multiply both sides of equation <xref ref="if-steps-standard-form"/> by <m>\mu</m> and reverse the product rule on the left side.
					</p>

					<p>
						<mdn>
							<mrow>	
								\mu\frac{dy}{dx} + P(x) \mu y			\amp = Q(x)	\mu
							</mrow>
							<mrow xml:id="if-method-reversed-product-rule">
								\frac{d}{dx}\left[\mu \cdot y\right]	\amp = Q(x) \mu
							</mrow>
						</mdn>.
					</p>

				</li>

				<li xml:id="if-step-3"><title> Step 3: Solve Using Direct Integration </title>

					<p>
						Integrate both sides of equation <xref ref="if-method-reversed-product-rule"/> and solve for <m>y</m> to find the general solution.
					</p>
			
				</li>

			</dl>

		</exploration>

		<conclusion>
			<p>
				The integrating factor method provides a structured approach to solving first-order linear equations. The <em>three key steps</em>â€”finding <m>\mu(x)</m>, transforming the equation, and integratingâ€”apply universally to all such equations.
			</p>

			<p>
				In the next section, we will apply this process through several worked examples to reinforce understanding.
			</p>
		</conclusion>

		<xi:include href="./c4-exercises/c4-chkpts-3-1-if-method-steps.ptx" />

	</subsection>

	<subsection><title> Examples </title>

		<introduction>
			<p>
				In this section, we apply the <em>Integrating Factor Method</em> to various first-order linear differential equations. These examples will illustrate the full process, from identifying the integrating factor to solving for <m>y(x)</m>.
			</p>

			<p>
				Let's start with a straightforward example to demonstrate how the integrating factor method works in practice. This example requires minimal manipulation since the equation is already in standard form.
			</p>

		</introduction>

		<example xml:id="if-intro-exercise"><title> A Simple Example </title>
		
			<p>
				<statement>
					<p>
						Find the general solution to the equation
					</p>
					<p>
						<me>
							y' + 6y = 1
						</me>.
					</p>
				</statement>
			</p>

			<p>
				<solution>

					<p>
						This is a first-order linear equation and it is already in standard form, so we proceed with the integrating factor method.
					</p>

					<p>
						<term> <xref ref="if-step-1" text="title"/> </term>
					</p>

					<p>
						Identify <m>P(x)</m> and compute <m>\mu</m>
						<me>
							y' + \os{P}{\boxed{6}}\ y = 1\quad \rightarrow \quad \mu = e^{\int 6\ dx} = e^{6x}
						</me>
						<em>Recall, we can ignore the integration constant for the integrating factor.</em>
					</p>

					<p>
						<term> <xref ref="if-step-2" text="title"/> </term>
					</p>

					<p>
						Multiply both sides by <m>e^{6x}</m> and reverse the product rule on the left side.
						<md>
							<mrow> e^{6x}y' + 6e^{6x}y						\amp = e^{6x}	</mrow>
							<mrow> \frac{d}{dx}\left[e^{6x}\cdot y\right]	\amp = e^{6x}	</mrow>
						</md>
					</p>

					<p>
						<term> <xref ref="if-step-3" text="title"/> </term>
					</p>

					<p>
						<md>
							<mrow> \int \frac{d}{dx}\left[e^{6x}\cdot y\right]\ dx	\amp = \int e^{6x}\ dx			</mrow>
							<mrow> e^{6x}\cdot y									\amp = \frac{1}{6} e^{6x} + c	</mrow>
							<mrow> y												\amp = \frac{1}{6} + ce^{-6x}.	</mrow>
						</md>
					</p>
				</solution>
			</p>

		</example>

		<example xml:id="if-standard-form-conversion"><title> Converting to Standard Form </title>

			<p>
				<statement>
					<p>
						Solve the equation
					</p>
					<p>
						<me>x^2y' = 5x^3 + 2x^3y </me>.
					</p>
				</statement>
			</p>

			<p>
				<solution>

					<p>
						This equation is first-order and linear, but is not in standard form, so we rewrite it as
						<me>
							y' - 2x y = 5x
						</me>
						and now we can apply the integrating factor method.
					</p>

					<p>
						<term> <xref ref="if-step-1" text="title"/> </term>
					</p>

					<p>
						Identify <m>P(x)</m> and compute <m>\mu</m>
						<me>
							y' + \os{P}{\boxed{-2x}} y = 5x \quad \rightarrow \quad \mu = e^{\int -2x\ dx} = e^{-x^2}
						</me>
					</p>

					<p>
						<term> <xref ref="if-step-2" text="title"/> </term>
					</p>

					<p>
						Multiply by <m>e^{-x^2}</m> and reverse the product rule on the left.
						<md>
							<mrow> e^{-x^2}y' - 2x e^{-x^2}y				\amp = 5xe^{-x^2}	</mrow>
							<mrow> \frac{d}{dx}\left[e^{-x^2}\cdot y\right]	\amp = 5xe^{-x^2}	</mrow>
						</md>
					</p>

					<p>
						<term> <xref ref="if-step-3" text="title"/> </term>
					</p>

					<p>
						Here, the integral on the right is computed with <m>u</m>-substitution:
					</p>

					<sidebyside widths="80% 20%" valign="top">
						<p>
							<md>
								<mrow> \int \frac{d}{dx}\left[e^{-x^2}\cdot y\right]dx	\amp = \int 5xe^{-x^2}dx		</mrow>
								<mrow> e^{-x^2}\cdot y									\amp = -\frac52 \int e^{u}du	</mrow>
								<mrow> e^{-x^2}\cdot y									\amp = -\frac52 e^{u} + c		</mrow>
								<mrow> e^{-x^2}\cdot y									\amp = -\frac52 e^{-x^2} + c	</mrow>
								<mrow> y												\amp = -\frac52 + ce^{x^2}		</mrow>
							</md>
						</p>
						<p>
							<md>
								<mrow> u = -x^2</mrow>
							</md>
						</p>
					</sidebyside>
					

					<solution><title> Verify the Solution </title>
						
						<p>
							We have found the general solution, but it is worth remembering that we can verify our solution by substituting back into the original equation.
						</p>

						<sidebyside>
							<p>
								<md>
									<mrow>	\ul{LHS}														</mrow>
									<mrow>	x^2y'															</mrow>
									<mrow>	x^2 \cdot \frac{d}{dx}\left( -\frac{5}{2} + ce^{x^2} \right)	</mrow>
									<mrow>	x^2 \cdot \left( 0 + 2cxe^{x^2} \right)							</mrow>
									<mrow>	2c x^3 e^{x^2}	\quadâœ…											</mrow>
								</md>
							</p>

							<p>
								<md>
									<mrow>	\ul{RHS}											</mrow>
									<mrow>	5x^3 + 2x^3y										</mrow>
									<mrow>	5x^3 + 2x^3\left( -\frac{5}{2} + ce^{x^2} \right)	</mrow>
									<mrow>	5x^3 - 5x^3+ 2c x^3 e^{x^2}							</mrow>
									<mrow>	2c x^3 e^{x^2}	\quadâœ…								</mrow>
								</md>
							</p>
						</sidebyside>
						
						<p>
							The same result on the left &amp; right confirms our solution.
						</p>
					</solution>

				</solution>
			</p>

		</example>

		<example xml:id="if-ln-example"><title> Integrating Factor with Logarithm </title>

			<p>
				<statement>
					<p>
						Find the general solution to the differential equation
					</p>
					<p>
						<me>-\frac{4M}{t^2} =  t^5 - \frac{1}{t}\frac{dM}{dt} + 1.</me>
					</p>
				</statement>
			</p>

			<p>
				<solution>

					<p>
						This equation is first-order and linear, but is not in standard form, so we rewrite it as
						<md>
							<mrow> \frac{1}{t} \frac{dM}{dt} - \frac{4}{t^2} \cdot M		\amp =  t^5 + 1	</mrow>
							<mrow> \frac{dM}{dt} + \us{P}{\boxed{-\frac{4}{t}}} \cdot M		\amp = t^6 + t	</mrow>
						</md>
						and now we can apply the integrating factor method.
					</p>

					<p>
						<sidebyside widths="22% 78%" valign="middle">
							
							<p>
								Find Integrating Factor
							</p>

							<p>
								<me>
									\mu = e\vphantom{\large|}^{\int \sfrac{-4}{t}\ dt} = e^{-4\ln t} = e^{\ln t^{-4}} = t^{-4}
								</me>
							</p>

						</sidebyside>
					</p>

					<p>
						<sidebyside widths="22% 78%" valign="middle">
							
							<p>
								Multiply by <m>t^{-4}</m>
							</p>

							<p>
								<md>
									<mrow>
										t^{-4} \frac{dM}{dt} - t^{-4} \frac{4}{t} M
											\amp = t^{-4}(t^6 + t)
									</mrow>
								</md>
							</p>

						</sidebyside>
					</p>

					<p>
						<sidebyside widths="22% 78%" valign="middle">
							
							<p>
								Complete the Derivative
							</p>

							<p>
								<md>
									<mrow>
										\frac{d}{dt}\left[ \frac{1}{t^4} M \right]
											\amp = t^2 + t^{-3}
									</mrow>
								</md>
							</p>

						</sidebyside>
					</p>

					<p>
						<sidebyside widths="22% 78%" valign="middle">
							
							<p>
								Integrate Both Sides
							</p>

							<p>
								<md>
									<mrow>
										\int \frac{d}{dt}\left[ \frac{1}{t^4} M \right]\ dt
											= \int \left(t^2 + t^{-3}\right) dt
									</mrow>
								</md>
							</p>

						</sidebyside>
					</p>

					<p>
						<sidebyside widths="22% 78%" valign="middle">
							
							<p>
								Isolate <m>M</m>
							</p>

							<p>
								<md>
									<mrow>
										\frac{1}{t^4} M = \frac{1}{3}t^{3} - \frac{1}{2}t^{-2} + c
									</mrow>
								</md>
							</p>

						</sidebyside>
					</p>

					<p>
						<sidebyside widths="22% 78%" valign="middle">
							
							<p>
								General Solution
							</p>

							<p>
								<me>
									M = \frac{1}{3}t^{7} - \frac{1}{2}t^2 + ct^4
								</me>.
							</p>

						</sidebyside>
					</p>

				</solution>
			</p>

		</example>

		<example><title> An Equation Involving Integration by Parts </title>

			<p>
				<statement>
					<p>
						Solve the equation:
						<me> t^2 y' + 2ty = t^3 \ln t </me>.
					</p>
				</statement>
			</p>

			<p>
				<solution>

					<p>
						We put the equation in standard form to identify <m>P(x)</m> and compute the integrating factor.
					</p>
				
					<p>
						<me>
							y' + \us{P}{\boxed{\frac{2}{t}}}\ y = t \ln t \quad \implies \quad
							\mu(t) = e^{\large \int (\sfrac{2}{t})\, dt} = e^{2 \ln t} = t^2
						</me>
					</p>
				
					<p>
						Multiply by <m>e^{1/x}</m> and reverse the product rule on the left side.
						<md>
							<mrow> t^2 y' + 2t y					\amp = t^3 \ln t	</mrow>
							<mrow> \frac{d}{dt} \left[t^2 y\right]	\amp = t^3 \ln t	</mrow>
						</md>
					</p>
				
					<p>
						Now, integrate both sides and use <xref ref="ibp-formula" text="custom">integration by parts</xref> on the right.
					</p>

					<p>
						<sidebyside widths="3% 60% 35% 2%" valigns="top top top top">

							<p/>
							<p>
								<md>
									<mrow>
										\int \frac{d}{dt} \big[t^2 y\big] dt \amp = \int t^3 \ln t\ dt
									</mrow>
									<mrow>	
										t^2 y	=
										\us{\textcolor{BurntOrange}{ u}}{\us{\textcolor{BurntOrange} \uparrow}{\ul{\vphantom{\frac11}\ln t}}}
										\cdot
										\us{\textcolor{BurntOrange}{ v}}{\us{\textcolor{BurntOrange} \uparrow}{\ul{\frac14 t^4}}}
										\amp\ - \int
										\us{\textcolor{BurntOrange}{ v}}{\us{\textcolor{BurntOrange} \uparrow}{\ul{\frac14 t^4}}}
										\cdot
										\us{\textcolor{BurntOrange}{du}}{\us{\textcolor{BurntOrange} \uparrow}{\ul{\frac{1}{t}\ dt}}}
									</mrow>
									<mrow>	t^2 y	= \frac14 t^4 \ln t \amp\ - \frac14 \int  t^3\ dt					</mrow>
									<mrow>	t^2 y	= \frac{t^4}{4} \ln t \amp\ - \frac{t^4}{16} + c						</mrow>
									<mrow>		y	= \frac{t^2}{4} \ln t \amp\ - \frac{t^2}{16} + c\,t^2				</mrow>
								</md>
							</p>
							<p>
								<md>
									<mrow>	\small\textcolor{BurntOrange}{				u = \ln t,}	\amp \ \ \small\textcolor{BurntOrange}{v = \frac14t^4}	</mrow>
									<mrow>	\small\textcolor{BurntOrange}{	du = \frac{1}{t}\ dt,}	\amp \ \ \small\textcolor{BurntOrange}{dv = t^3\ dt}	</mrow>
								</md>
							</p>
							<p/>

						</sidebyside>
					</p>

					<p>
						Finally, solve for <m>y</m>:
						<md>
							<mrow>	y = \frac{t^2}{4} \ln t - \frac{t^2}{16} + c\,t^2	</mrow>
						</md>
					</p>

				</solution>
			</p>

		</example>

		<example><title> An Initial-Valued Problem </title>

			<p>
				<statement>
					<p>
						Solve the initial value problem.
						<me>
							A = \sec\theta A' - \frac{\theta e^{\large\theta^2 + \sin\theta}}{\cos \theta}, \hspace{1cm} A(0) = -\frac{1}{2}
						</me>.
					</p>
				</statement>
			</p>

			<p>
				<solution>

					<p>
						Let's put the equation in standard form. After replacing <m>\sec\theta</m> with <m>\frac{1}{\cos\theta}</m>and moving the <m>A'</m> term to the left, we have
					</p>
				
					<p>
						<me>
							\frac{1}{\cos\theta} A' - A = \frac{\theta e^{\large\theta^2 + \sin\theta}}{\cos \theta}
						</me>.
					</p>

					<p>
						Multiplying this by <m>\cos\theta</m> allows us to identify <m>P</m> and compute <m>\mu</m> as
						<me>
							A' + \us{P}{\boxed{- \cos\theta}}\ A = \theta e^{\large \theta^2 + \sin\theta}
							\quad \implies \quad
							\mu = e\vphantom{\large|}^{\large\int -\cos\theta d\theta} = e^{\large -\sin\theta}
						</me>
					</p>

					<p>
						Multiply by <m>e^{1/x}</m> and reverse the product rule on the left side.
						<md>
							<mrow> e^{\large -\sin\theta}A' - \cos\theta e^{\large -\sin\theta}A = \theta e^{\large\theta^2 + \sin\theta}	</mrow>
							<mrow> \frac{d}{d\theta}\left[ e^{\large -\sin\theta}A \right] = \theta e^{\large\theta^2}	</mrow>
						</md>.
					</p>
				
					<p>
						Integrate both sides and use <m>u</m>-substitution on the right side.
					</p>

					<p>
						<sidebyside widths="10% 60% 25% 5%" valigns="top top top top">

							<p/>
							<p>
								<md>
									<mrow>
										\int \frac{d}{d\theta}\left[ e^{\large -\sin\theta}A \right] d\theta = \int \theta e^{\large\theta^2} d\theta
									</mrow>
									<mrow>
										e^{\large -\sin\theta}A = \frac{1}{2}e^{\large\theta^2} + c
									</mrow>
									<mrow>
										A = \frac{1}{2}e^{\large\theta^2 + \sin\theta} + ce^{\large\sin\theta}
									</mrow>
								</md>
							</p>
							<p>
								<md>
									<mrow>	u	\amp = \theta^2			</mrow>
									<mrow>	du	\amp = 2\theta\ d\theta	</mrow>
								</md>
							</p>
							<p/>

						</sidebyside>

					</p>

					<p>
						Finally, we apply the initial condition to determine the constant <m>c</m>.
						<md>
							<mrow> -\frac{1}{2} = A(0) \amp = \frac{1}{2}e^{\large 0^2 + \sin(0)} + ce^{\large\sin(0)}	</mrow>
							<mrow>  \amp = \frac{1}{2}e^0 + ce^0 	</mrow>
							<mrow> \amp = \frac{1}{2} + c\quad \implies \quad c = -1	</mrow>
						</md>
					</p>

					<p>
						We can then write the particular solution to the initial value problem.
						<me>A(\theta) = \frac{1}{2}e^{\large\theta^2 + \sin\theta} - e^{\large\sin\theta}</me>
					</p>
				</solution>
			</p>

		</example>

		<conclusion>

			<p>
				These examples demonstrate the versatility of the <em>Integrating Factor Method</em>. Regardless of the complexity of the given equation, the same <em>three-step approach</em>â€”computing <m>\mu(x)</m>, transforming the equation, and solving via integrationâ€”provides a reliable solution strategy.
			</p>

			<p>
				In the next section, we will explore applications of the integrating factor method in real-world problems.
			</p>

		</conclusion>

		<xi:include href="./c4-exercises/c4-chkpts-3-2-if-examples.ptx" />

	</subsection>

</section> 