<theorem xml:id="std-form-explained"><title> <em>1st-Order Linear Standard Form Explained</em> </title>
		
	<statement>
		<p>
			Since a general linear differential equation looks like
			<me> 
				a_n(x)y^{(n)} + \cdots + a_2(x)y'' + a_1(x)y' + a_0(x)y = f(x)
			</me>,
			the first-order case (<m>n=1</m>), simplifies to
			<me> 
				a_1(x)y' + a_0(x)y = f(x)
			</me>.
			Dividing by the coefficient of <m>y'</m>, and renaming the new coefficients as <m>P</m> and <m>Q</m>, gives the standard form
			<me>
				y' + \us{P(x)}{\ub{\frac{a_0(x)}{a_1(x)}}}y	= \us{Q(x)}{\ub{\frac{f(x)}{a_1(x)}}}	
				\quad \implies \quad 
				y' + P(x)y	= Q(x)
			</me>.
		</p>
	</statement>

</theorem>