<section xmlns:xi="http://www.w3.org/2001/XInclude"><title> 2nd-Order Equations </title>

	<p>
		Now that we've mastered first-order LHCC equations, it's time to explore second-order LHCC equations. These are slightly more complex but follow a similar approach. We'll see how the characteristic equation helps us find solutions and look at the different cases that arise depending on the nature of the roots.
	</p>

	<p>
		Consider the following second-order equation:
		<men xml:id="second-order-lhcc-intro-de"> y'' - 5y' + 6y = 0 </men>
		Substituting <m>y = e^{rx}</m> into this equation, we get:
		<md>
			<mrow> \left[e^{rx}\right]'' - 5 \left[e^{rx}\right]' + 6 \left[e^{rx}\right] =	\amp\ 0							</mrow>
			<mrow> r^2 e^{rx} - 5r e^{rx} + 6 e^{rx} =										\amp\ 0							</mrow>
			<mrow> (r^2 - 5r + 6) e^{rx} =													\amp\ 0 \qquad (e^{rx} \ne 0)	</mrow>
			<mrow> \text{characteristic equation} \rightarrow \qquad r^2 - 5r + 6 =			\amp\ 0							</mrow>
			<mrow> r_1 = 2, \quad  r_2 =													\amp\ 3							</mrow>
		</md>.
		Therefore, <m>y = e^{2x}</m> and <m>y = e^{3x}</m> are solutions, and the general solution is the combination of these two:
		<me> y = C_1 e^{2x} + C_2 e^{3x} </me>.
	</p>

	<p>
		In general, for any second-order LHCC equation of the form:
		<men xml:id="second-order-lhcc-de"> a y'' + b y' + c y = 0 </men>
		The characteristic equation is:
		<men xml:id="second-order-lhcc-characteristic-equation"> a r^2 + b r + c = 0 </men>
		This quadratic equation will have two solutions, which could be either real or complex. The general solution depends on the nature of these solutions, and we will now explore the different  cases. Before moving on, we highly recommend taking a minute to review some <xref ref="solving-the-quadratic-equation" text="custom">concepts related to solving quadratic equations</xref>.
	</p>

	<p>
		Let <m>r_1</m> and <m>r_2</m> be the solutions to the characteristic equation. When <m>r_1 \ne r_2</m>, the general solution is:
		<men xml:id="second-order-lhcc-solution-r1-notequalto-r2"> y = C_1\, e^{r_1 x} + C_2\, e^{r_2 x} </men>
		However, if <m>r_1 = r_2</m>, the terms combine into like terms, 
		<me> 
			y = C_1\, e^{r_1 x} + C_2\, e^{r_2 x} = \color{blue}\us{ \large \text{like terms}}{\us{\nwarrow}{\ul{C_1\, e^{r_1 x}}} + \us{\nearrow}{\ul{C_2\, e^{r_1 x}}}} = (\us{C}{\ub{C_1 + C_2}})\, e^{r_1 x}
		</me>,
		which is an incomplete solution. To fix this, we multiply the second term by <m>x</m>, resulting in the correct general solution:
		<fn>
			<p>
				See <xref ref="tba"/> for an outline of why the extra <m>x</m> is required in the general solution of a second order LHCC equation when <m>r_1=r_2</m>.
			</p>
		</fn>
		<me> y = C_1\, e^{r_1 x} + C_2\, x e^{r_1 x} </me>
	</p>

	<p>
		Although, the above explanation covers the situation when <m>r_1</m> and <m>r_2</m> are equal or not, we will split the <m>r_1 \ne r_2</m> case into <xref ref="second-order-lhcc-complex-case" text="custom">two cases that treat real or complex values separately</xref>. The three cases are summarized below.
	</p>

	<assemblage><title> Summary of Cases </title>
		<p>
			Let <m>r_1</m> and <m>r_2</m> be the solutions of the characteristic equation associated with the second-order LHCC equation. The general solution is:
			<dl width="wide">
				<li xml:id="lhcc-case-1"><title>Case 1 (real &amp; <m>\ne</m>)</title>
					<m>
						\ds y = C_1 e^{r_1 x} + C_2 e^{r_2 x} \quad (r_1 \ne r_2)
					</m>
				</li>
				<li xml:id="lhcc-case-2"><title>Case 2 (real &amp; <m>=</m>)</title>
					<m>
						\ds y = (C_1 + C_2 x) e^{r_1 x} \quad (r_1 = r_2)
					</m>
				</li>
				<li xml:id="lhcc-case-3"><title>Case 3 (complex)</title>
					<line>
						<m>
							\ds y = e^{\alpha x} (C_1 \cos(\beta x) + C_2 \sin(\beta x))
						</m>
					</line>
					<line>
						<m>
							\ds (r = \alpha \pm i\beta \implies r_1 = \alpha + i\beta, \ r_2 = \alpha - i\beta)
						</m>
					</line>
				</li>
			</dl>
		</p>
	</assemblage>

	<p>
		Let's now practice solving some second-order LHCC equations.
	</p>

	<example>


		<p>
			Find the general solutions for each LHCC equation.
			<sidebyside widths="30% 70%">
				<p>
					<m> y'' - 5y' + 6y = 0 </m>
				</p>
				<p>
					<solution><title> Solution </title>
						<p>
							First, write down and solve the characteristic equation:
							<md>
								<mrow> r^2 - 5r + 6 =\amp\ 0 </mrow>
								<mrow> (r-2)(r-3) =\amp\ 0 </mrow>
								<mrow> r_1 = 2 \quad \text{and} \quad r_2 =\amp\ 3 </mrow>
							</md>.
							Since <m>r_1</m> and <m>r_2</m> are real and <m>r_1 \ne r_2</m>, we are in <xref ref="lhcc-case-1" text="custom">Case 1</xref>. Therefore, the general solution is:
							<me> y = C_1 e^{2x} + C_2 e^{3x} </me>.
						</p>
					</solution>
				</p>
			</sidebyside>
		</p>
		
		<p>
			<sidebyside widths="30% 70%">
				<p>
					<m> y'' + 4y' + 4y = 0 </m>
				</p>

				<p>
					<solution><title> Solution </title>
						<p>
							The characteristic equation is:
							<md>
								<mrow> r^2 + 4r + 4 =\amp\ 0 </mrow>
								<mrow> (r+2)(r+2) =\amp\ 0 </mrow>
								<mrow> r_1 = -2 \quad \text{and} \quad r_2 =\amp\ -2 \quad \leftarrow <xref ref="lhcc-case-2" text="custom">Case 2</xref> </mrow>
							</md>.
							Therefore, the general solution is:
							<me> y = (C_1 + C_2 x) e^{-2x} </me>.
						</p>
					</solution>
				</p>
			</sidebyside>
		</p>

		<p>
			<sidebyside widths="30% 70%">
				<p>
					<m> y'' + 2y' + 5y = 0 </m>
				</p>
		
				<p>
					<solution><title> Solution </title>
						<p>
							The characteristic equation in this problem is:
							<md>
								<mrow> r^2 + 2r + 5 = 0\amp </mrow>
								<mrow> r = \us{\alpha}{\boxed{-1}} \pm \us{\beta}{\boxed{2}}i \amp\ \quad \leftarrow <xref ref="lhcc-case-3" text="custom">Case 3</xref> </mrow>
							</md>.
							Here, <m>\alpha = -1</m> and <m>\beta = 2</m>. So the general solution is:
							<me> y = e^{-x} (C_1 \cos(2x) + C_2 \sin(2x)) </me>.
						</p>
					</solution>
				</p>
			</sidebyside>
		</p>
	</example>

	<xi:include href="./p3-c1-s4-interactives.ptx" />

</section>