<subsection xmlns:xi="http://www.w3.org/2001/XInclude"><title> Selecting Forms </title> 

	<introduction>

		<p>
			Recall that the first step of the Laplace Transform Method involves a <xref ref="lt-roadmap-step1" text="custom">forward transformation</xref>, which converts the <m>y(t)</m>-equation into an equation containing <m>Y(S)</m> and <m>s</m>. Now, we skip ahead to the final step of the method, where we reverse this process to return to the <m>y(t)</m>-equation, revealing the solution to the original differential equation.
		</p>

		<figure xml:id="lt-roadmap-step3">
			<caption>
				The Backward Laplace Transform. Converting the <m>Y(s)</m>-algebra equation back into the <m>y(t)</m>-solution.
			</caption>
			<image source="figures/Laplace-Roadmap-Step-3.png" width="100%">
				<shortdescription>(for accessibility)</shortdescription>
			</image>
		</figure>
		
		<p>
			This section will guide you through Step 3 of the Laplace Transform Method: identifying common forms, matching them to <m>Y(s)</m>, and ultimately recovering <m>y(t)</m>. Mastering this step will enable you to complete the solution of differential equations using the Laplace Transform Method.
		</p>

	</introduction>

	<subsubsection><title> Matched Forms </title> 

		<p>
			The Laplace Transform Method begins with the <xref ref="lt-roadmap-step1" text="custom">forward</xref> Laplace transform of a differential equation with an unknown function <m>y(t)</m> into an algebraic equation involving the transformed function <m>Y(s)</m>. Once we have solved for <m>Y(s)</m>, the final step is to recover the original function, <m>y(t)</m>, by applying the <xref ref="lt-roadmap-step3" text="custom">backward</xref> (inverse) Laplace transform, denoted as <m>\laplacesym^{-1}</m>.
		</p>

		<p>
			Much like how <m>\cos^{-1}</m> reverses the cosine function, applying <m>\laplacesym^{-1}</m> to both sides of a Laplace-transformed expression brings us back to the original function. For example, if
			<me>
				\lap{e^{-3t}} = \frac{1}{s+3},
			</me>
			then, applying the inverse Laplace transform gives:
			<me>
				\ilap{\frac{1}{s+3}} = e^{-3t}.
			</me>
			To identify the appropriate inverse Laplace transform, we rely on the common transforms in the table below, where we match the function of <m>s</m> on the right and the inverse is the function of <m>t</m> on the left.
		</p>

		<table halign="center" xml:id="common-lt-table"><title> <em>Common Laplace Transforms. <m>a, b</m> are constant, <m>n = 1, 2, \ldots</m></em> </title>
			<tabular halign="center">
				<row>
					<cell/>
					<cell><m>t</m>-functions</cell>
					<cell colspan="2"><m>s</m>-functions</cell>
				</row>
				<row>
					<cell/>
					<cell><m>\downarrow</m></cell>
					<cell colspan="2"><m>\downarrow</m></cell>
				</row>
				<row bottom="minor">
					<cell right="minor"/>
					<cell right="minor"><m>f(t)</m></cell>
					<cell colspan="2"><m>\lap{ f(t) }</m></cell>
				</row>
				<row bottom="minor">
					<cell right="minor"><m>L_1</m></cell>
					<cell right="minor"><m>1</m></cell>
					<cell><m>\ds \frac{1}{s}</m></cell>
					<cell><m>s \gt 0</m></cell>
				</row>
				<row bottom="minor">
					<cell right="minor"><m>L_2</m></cell>
					<cell right="minor"><m>e^{at}</m></cell>
					<cell><m>\ds \frac{1}{s-a}</m></cell>
					<cell><m>s \gt a</m></cell>
				</row>
				<row bottom="minor">
					<cell right="minor"><m>L_3</m></cell>
					<cell right="minor"><m>t^n</m></cell>
					<cell><m>\ds \frac{n!}{s^{n+1}}</m></cell>
					<cell><m>s \gt 0</m></cell>
				</row>
				<row bottom="minor">
					<cell right="minor"><m>L_4</m></cell>
					<cell right="minor"><m>\sin (bt)</m></cell>
					<cell><m>\ds \frac{b}{s^2 + b^2}</m></cell>
					<cell><m>s \gt 0</m></cell>
				</row>
				<row bottom="minor">
					<cell right="minor"><m>L_5</m></cell>
					<cell right="minor"><m>\cos(bt)</m></cell>
					<cell><m>\ds \frac{s}{s^2 + b^2}</m></cell>
					<cell><m>s \gt 0</m></cell>
				</row>
				<row bottom="minor">
					<cell right="minor"><m>L_6</m></cell>
					<cell right="minor"><m>t^n e^{at}</m></cell>
					<cell><m>\ds \frac{n!}{(s-a)^{n+1}}</m></cell>
					<cell><m>s \gt a</m></cell>
				</row>
				<row bottom="minor">
					<cell right="minor"><m>L_7</m></cell>
					<cell right="minor"><m>e^{at} \sin(bt)</m></cell>
					<cell><m>\ds \frac{b}{(s-a)^2 + b^2}</m></cell>
					<cell><m>s \gt a</m></cell>
				</row>
				<row>
					<cell right="minor"><m>L_8</m></cell>
					<cell right="minor"><m>e^{at} \cos(bt)</m></cell>
					<cell><m>\ds \frac{s-a}{(s-a)^2 + b^2}</m></cell>
					<cell><m>s \gt a</m></cell>
				</row>
				<!-- <row>
					<cell/>
					<cell><m>\uparrow</m></cell>
					<cell><m>\uparrow</m></cell>
					<cell></cell>
				</row>
				<row>
					<cell/>
					<cell><m>t</m>-function</cell>
					<cell><m>s</m>-function</cell>
					<cell></cell>
				</row> -->
			</tabular>
		</table>

		<p>
			Many functions can be matched by simply observing the denominator. The following table summarizes common patterns for matching denominators with their associated inverse transforms:
		</p>

		<table halign="center" xml:id="backward-lt-rules-of-thumb"><title> Matching Guide: <m>s</m>-function <m>\rightarrow</m> Inverse Transform </title>
			<tabular halign="center">
				<row bottom="minor">
					<cell right="minor"> Denominator </cell>
					<cell right="minor"> <m>s</m> in Numerator? </cell>
					<cell> Transform </cell>
				</row>
				<row bottom="minor">
					<cell right="minor"><m>s</m></cell>
					<cell right="minor"> - </cell>
					<cell><m>L_1</m></cell>
				</row>
				<row bottom="minor">
					<cell right="minor"><m>s^{\text{power}}</m></cell>
					<cell right="minor"> - </cell>
					<cell><m>L_3</m></cell>
				</row>
				<row bottom="minor">
					<cell right="minor"><m>s \pm \text{shift}</m></cell>
					<cell right="minor"> - </cell>
					<cell><m>L_2</m></cell>
				</row>
				<row bottom="minor">
					<cell right="minor"><m>(s \pm \text{shift})^{\text{power}}</m></cell>
					<cell right="minor"> - </cell>
					<cell><m>L_6</m></cell>
				</row>
				<row bottom="minor">
					<cell right="minor"><m>s^2 + \text{number}</m></cell>
					<cell right="minor">
						<line>no</line>
						<line>yes</line>
					</cell>
					<cell>
						<line><m>L_4</m></line>
						<line><m>L_5</m></line>
					</cell>
				</row>
				<row bottom="minor">
					<cell right="minor"><m>(s \pm \text{shift})^2 + \text{number}</m></cell>
					<cell right="minor">
						<line>no</line>
						<line>yes</line>
					</cell>
					<cell>
						<line><m>L_7</m></line>
						<line><m>L_8 + L_7</m></line>
					</cell>
				</row>
			</tabular>
		</table>

		<p>
			Now, let's look at some examples.
		</p>

		<example>
			<p>
				Find the inverse Laplace transforms of each function.
				<sidebyside widths="24% 76%">
					<p>
						<m>\ds\hspace{1.5em}\frac{3}{s^2 + 9}</m>
					</p>
					<p>
						<solution><title> Solution </title>
							<p>
								This matches the <xref ref="L4" text="custom"><m>L_4</m></xref> form with <m>b=3</m>. So,
								<me>
									\ilap{\frac{3}{s^2 + 9}} = \sin(3t).
								</me>
							</p>
						</solution>
					</p>
				</sidebyside>
				<sidebyside widths="24% 76%">
					<p>
						<m>\ds\frac{s - 2}{(s - 2)^2 + 16}</m>
					</p>
					<p>
						<solution><title> Solution </title>
							<p>
								This matches the <xref ref="L7" text="custom"><m>L_7</m></xref> form with <m>a=2</m> and <m>b=4</m>. So,
								<me>
									\ilap{\frac{s - 2}{(s - 2)^2 + 16}} = e^{2t}\cos(4t)
								</me>.
							</p>
						</solution>
					</p>
				</sidebyside>
				<sidebyside widths="24% 76%">
					<p>
						<m>\ds\hspace{2.4em}\frac{24}{s^5}</m>
					</p>
					<p>
						<solution><title> Solution </title>
							<p>
								This matches the <xref ref="L3" text="custom"><m>L_3</m></xref> with <m>n=4</m>.
								<me>
									\ilap{\frac{24}{s^5}} = \ilap{\frac{4!}{s^{4+1}}} = t^4.
								</me>
							</p>
						</solution>
					</p>
				</sidebyside>
			</p>
			
		</example>

		<p>
			These examples demonstrate how to find the inverse Laplace Transform when the <m>s</m>-function matches a form on the right side of the common transforms table. However, not all functions will align perfectly with the table, and additional adjustments are needed to match the forms. In the next discussion, we will explore how to modify the <m>s</m>-function to match the common forms in the table.
		</p>
	
		<xi:include href="./p4-c2-s1-1-interactives.ptx" />

	</subsubsection>

	<subsubsection><title> Mismatched Forms </title>

		<p>
			When working with Laplace transforms, it's common to encounter algebraic expressions that don't perfectly match the standard forms we use for the inverse Laplace transform. In these cases, we need to manipulate the expression to make it fit one of the known forms.
		</p>

		<p>
			For example, consider the expression:
			<me> \frac{1}{s^2 + 25} \qquad \leftarrow \ \text{looks like} \quad \frac{b}{s^2 + b^2}. </me>
			While it's not an exact match, we can observe from the denominator that <m>b = 5.</m>
		</p>

		<p>
			However, the numerator doesn't match yet. To correct this, we need a 5 in the numerator. We can't just multiply the numerator by 5 without changing the value, so instead, we multiply the entire expression by <m>\ds\frac{5}{5}</m>, which is equivalent to multiplying by 1:
			<md>
				<mrow>\frac{1}{s^2 + 25} 	=\amp\ \frac{1}{s^2 + 5^2} </mrow>
				<mrow>						=\amp\ \frac{5}{5} \cdot \frac{1}{s^2 + 5^2} </mrow>
				<mrow>						=\amp\ \frac{1}{5} \cdot \frac{5}{s^2 + 5^2} \quad \us{\text{match}}{\os{\text{perfect}}{\leftarrow}}\ \frac{b}{s^2 + b^2}</mrow>
			</md>
			Multiplying by <m>\ds\frac{5}{5}</m> doesnâ€™t change the value of the expression, but it allows us to match the standard form.
		</p>

		<p>
			One of the most common adjustments is introducing a missing constant in the numerator, as we did earlier. By multiplying both the numerator and denominator by this constant, we maintain the expression's value while transforming it into a recognizable form. Letâ€™s look at some examples:
		</p>

		<example>
			<p>
				Compute the inverse Laplace transforms for each.
			</p>

			<tabular>
				<col width="20%" halign="center"/>
				<col width="75%"/>
				<row>
					<cell><m>\ds \frac{12}{s}</m></cell>
					<cell>
						<p>
							<m>\hspace{27em}</m>
							<solution><title> Solution </title>
								<p>
									The <m>s</m> in the denominator tells us that we need <m>L_1</m>. Before we do, let's factor out <m>12</m>:
									<me>\ds \ilap{\frac{12}{s}} = 12 \cdot \ilap{\frac{1}{s}} = 12 \cdot 1 = 12</me>.
								</p>
							</solution>
						</p>
					</cell>
				</row>
				<row>
					<cell><m>\ds \frac{5}{s^2 + 4}</m></cell>
					<cell>
						<p>
							<m>\hspace{27em}</m>
							<solution><title> Solution </title>
								<p>
									Since the denominator has the form, <m>s^2 + \text{number}</m>, and there is no <m>s</m> in the numerator, we should apply <m>L_4</m>. As before, it is helpful to first factor out the constant <m>5</m>, 
									<me>\ds \ilap{\frac{5}{s^2 + 4}} = 5\ \ilap{\frac{1}{s^2 + 4}} \quad \leftarrow <xref ref="L4" text="custom">L_4</xref> (b=2)</me>.
									According to <m>L_4</m>, we are missing <m>2</m> in the numerator. Let's put it there by multiplying by <m>2/2</m>, like so
									<md>
										<mrow> = 5\ \ilap{\frac{2}{2}\frac{1}{s^2 + 4}} =\amp\ 5\ \ilap{\frac{1}{2}\frac{2}{s^2 + 4}}</mrow>
										<mrow>										  =\amp\ \frac{5}{2} \ilap{\frac{2}{s^2 + 4}}</mrow>
										<mrow>										  =\amp\ \frac{5}{2} \sin(2t)</mrow>
									</md>
								</p>
							</solution>
						</p>
					</cell>
				</row>
				<row>
					<cell><m>\ds \frac{17}{s^4}</m></cell>
					<cell>
						<p>
							<m>\hspace{27em}</m>
							<solution><title> Solution </title>
								<p>
									This denominator has the form <m>s^{\text{power}}</m>, which matches <m>L_3</m> with <m>n = 3</m>. 
									<me>\ds \ilap{\frac{17}{s^4}} = 17\ \ilap{\frac{1}{s^4}} \quad \leftarrow <xref ref="L3" text="custom">L_3</xref> (n=3)</me>.
									In this case, the numerator is missing a <m>3!</m>. We can introduce it by multiplying by <m>3!/3!</m>, like so
									<md>
										<mrow> = 17\ \ilap{\frac{3!}{3!}\frac{1}{s^4}} = \frac{17}{3!} \ilap{\frac{3!}{s^4}} = \frac{17}{6} t^3</mrow>
									</md>
								</p>
							</solution>
						</p>
					</cell>
				</row>
				<row>
					<cell><m>\ds \frac{7s}{s^2 + 25}</m></cell>
					<cell>
						<p>
							<m>\hspace{27em}</m>
							<solution><title> Solution </title>
								<p>
									<me><xref ref="L5" text="custom">L_5</xref>, b=5</me>
									<me> \ilap{\frac{7s}{s^2 + 25}} = 7\ \ilap{\frac{s}{s^2 + 25}} = 7\ \cos(5t)</me>
								</p>
							</solution>
						</p>
					</cell>
				</row>
				<row>
					<cell><m>\ds \frac{10}{(s - 3)^2 + 11}</m></cell>
					<cell>
						<p>
							<m>\hspace{27em}</m>
							<solution><title> Solution </title>
								<p>
									The form of this denominator is <m>\ul{(s \pm \text{shift})^{2} + \text{number}}</m> and has no <m>s</m> in the numerator. Therefore,
									<md>
										<mrow> \ilap{\frac{10}{(s - 3)^2 + 11}} \amp\ \quad <xref ref="L7" text="custom"><m>L_7</m></xref> (a=3,\ b=\sqrt{11})</mrow>
										<mrow>	=\amp\ 10\ \ilap{\frac{\sqrt{11}}{\sqrt{11}}\frac{1}{(s - 3)^2 + 11}}</mrow>
										<mrow>	=\amp\ \frac{10}{\sqrt{11}} \ilap{\frac{\sqrt{11}}{(s - 3)^2 + 11}}</mrow>
										<mrow>	=\amp\ \frac{10}{\sqrt{11}} e^{3t} \sin(\sqrt{11}t)</mrow>
									</md>

								</p>
							</solution>
						</p>
					</cell>
				</row>
				<row>
					<cell><m>\ds \frac{2}{(s+7)^5}</m></cell>
					<cell>
						<p>
							<m>\hspace{27em}</m>
							<solution><title> Solution </title>
								<p>
									The denominator, <m>\ul{(s \pm \text{shift})^{\text{power}}}</m>, indicates an <m>e^{at}</m> and a <m>t^n</m> term. Therefore,
									<md>
										<mrow> \ilap{\frac{2}{(s+7)^5}} \amp\ \quad <xref ref="L6" text="custom"><m>L_6</m></xref> (a=-7, n=4)</mrow>
										<mrow>  
												=\amp\ 2\ \ilap{\frac{4!}{4!}\frac{1}{(s+7)^5}}
										</mrow>
										<mrow> 
												=\amp\ \frac{2}{4!} \ilap{\frac{4!}{(s+7)^5}}
										</mrow>
										<mrow>
											=\amp\ \frac{1}{12} t^4 e^{-7t}
									</mrow>
									</md>
								</p>
							</solution>
						</p>
					</cell>
				</row>
			</tabular>
		</example>

		<xi:include href="./p4-c2-s1-2-interactives.ptx" />
		
	</subsubsection>

</subsection>