<subsection xmlns:xi="http://www.w3.org/2001/XInclude"><title> <m>\lap\{e^{at}\}</m> </title>

	<p>
		While we are gleaning information from previous examples, let's recall <xref ref="ex_lt_defn_02"/>, from the previous section. There, we showed that

		<me> \lap\{ e^{7t} \} = \frac{1}{s-7}, \quad s \gt 7.</me>

		What do you suppose is the Laplace transform of the function <m>e^{23 t}</m>?  We can surmise another property that shows us how to take Laplace transforms of exponential functions.

		<sidebyside widths="90%" margins="auto" valign="middle">
			<p>
				<term>Property:</term>  The Laplace transform of <m>e^{at}</m> is given by
				<me> \lap\{ e^{at} \} = \frac{1}{s - a}. </me>
			</p>
		</sidebyside>
	</p>

	<example>

		<m>\quad</m> Compute <m> \lap \{ e^{7t} \} </m>.

		<solution>
			<p>
				We use the definition of Laplace transform to get us started.
				<md>
					<mrow> \lap\{ x(t) \} \amp= \lap\{ e^{7t} \} 				</mrow>
					<mrow> 		\amp= \int_0^{\infty} \left(e^{7t}\right)e^{-st}\ dt 				</mrow>
					<mrow> 		\amp= \lim_{b \to \infty}\int_0^b e^{-st + 7t}\ dt	</mrow>
					<mrow> 		\amp= \lim_{b \to \infty}\int_0^b e^{(7-s)t}\ dt 		</mrow>
				</md>
				As before, we need restrict some values of <m>s</m> in order for this
				improper integral to exist . In this case, we will need <m>7 - s</m>, in the exponent, to be non-zero and negative. That is, we need
				<me> 7 - s \lt 0 \hspace{0.5cm}\Rightarrow \hspace{0.5cm}7 \lt s. </me>
				Hence, we move forward with the assumption that <m>s \gt 7</m>.
				<md>
					<mrow> 	\amp= \lim_{b \to \infty}\int_0^b e^{(7-s)t}dt </mrow>
					<mrow>	\amp= \lim_{b \to \infty} \frac{1}{7-s}e^{(7-s)t}\Bigg|_0^b</mrow>
					<mrow>	\amp= \frac{1}{7-s}\lim_{b \to \infty}
											\left[ e^{(7-s)b} - e^{(7-s)\cdot 0}\right]</mrow>
					<mrow>	\amp= \frac{1}{7-s}\lim_{b \to \infty}
											\left[ e^{(7-s)b} - 1\right]</mrow>
					<mrow>	\amp= \frac{1}{7-s}
											\left[\lim_{b \to \infty}e^{(7-s)b}
											- \lim_{b \to \infty}1\right]</mrow>
					<mrow>	\amp= \frac{1}{7-s} \left[ 0 - 1\right] \quad
											<xref text="custom" ref="reason-limit-to-zero-e7t">why is the limit 0?</xref></mrow>
					<mrow>	\amp= \frac{-1}{7-s} \hspace{4.4cm}	</mrow>
					<mrow>	\amp= \frac{1}{s - 7}, 					\quad s \gt 7 	</mrow>
				</md>
				Thus, the Laplace transform of <m>x(t) = e^{7t}</m> is
				<me>\ds \lap\{e^{7t}\} = \frac{1}{s - 7}</me>.
			</p>
		</solution>

	</example>

	<example>

		<m>\quad</m> Show <m>\ds \lap \{ e^{at} \} = \frac{1}{s - a} </m>.

		<solution>
			<p>
				We use the definition of Laplace transform to get us started.
				<md>
					<mrow> \lap\{ x(t) \} \amp= \lap\{ e^{at} \} 				</mrow>
					<mrow> 		\amp= \int_0^{\infty} \left(e^{at}\right)e^{-st}\ dt 				</mrow>
					<mrow> 		\amp= \lim_{b \to \infty}\int_0^b e^{-st + at}\ dt	</mrow>
					<mrow> 		\amp= \lim_{b \to \infty}\int_0^b e^{(a-s)t}\ dt 		</mrow>
				</md>
				As before, we need restrict some values of <m>s</m> in order for this
				improper integral to exist . In this case, we will need <m>a - s</m>, in the exponent, to be non-zero and negative. That is, we need
				<me> a - s \lt 0 \hspace{0.5cm}\Rightarrow \hspace{0.5cm}a \lt s. </me>
				Hence, we move forward with the assumption that <m>s \gt a</m>.
				<md>
					<mrow> 	\amp= \lim_{b \to \infty}\int_0^b e^{(a-s)t}dt </mrow>
					<mrow>	\amp= \lim_{b \to \infty} \frac{1}{a-s}e^{(a-s)t}\Bigg|_0^b</mrow>
					<mrow>	\amp= \frac{1}{a-s}\lim_{b \to \infty}
											\left[ e^{(a-s)b} - e^{(a-s)\cdot 0}\right]</mrow>
					<mrow>	\amp= \frac{1}{a-s}\lim_{b \to \infty}
											\left[ e^{(a-s)b} - 1\right]</mrow>
					<mrow>	\amp= \frac{1}{a-s}
											\left[\lim_{b \to \infty}e^{(a-s)b}
											- \lim_{b \to \infty}1\right]</mrow>
					<mrow>	\amp= \frac{1}{a-s} \left[ 0 - 1\right] \quad
											<xref text="custom" ref="reason-limit-to-zero-e7t">why is the limit 0?</xref></mrow>
					<mrow>	\amp= \frac{-1}{a-s} \hspace{4.4cm}	</mrow>
					<mrow>	\amp= \frac{1}{s - a}, 					\quad s \gt a 	</mrow>
				</md>
				Thus, the Laplace transform of <m>x(t) = e^{at}</m> is
				<me>\ds \lap\{e^{at}\} = \frac{1}{s - a}</me>.			
			</p>
		</solution>

	</example>

	<p>
		We can continue to use the definition to determine the Laplace transform
	</p>

	<assemblage xml:id="lt-table-L1-L2"><title>Common Laplace Transforms</title>
		<p>
			<dl width="narrow">
				<li><title><m>{\LARGE \vphantom{\int}}L_1.</m></title>
					<m>\ds \lap\{ 1 \} = \frac{1}{s}, \quad s &gt;0 </m>
				</li>
				<li xml:id="L2"><title><m>{\LARGE \vphantom{\int}}L_2.</m></title>
					<m>\ds \lap\{ e^{at} \} = \frac{1}{s - a}, \quad s &gt;a, \quad a \text{ is a constant} </m>
				</li>
			</dl>
		</p>
	</assemblage>

	<xi:include href="./c4-s1-ss2-interactives.ptx" />

</subsection>