<subsection xmlns:xi="http://www.w3.org/2001/XInclude"><title> Properties -O </title>

	<paragraphs><title> Linearity Property </title>
		
		
		<p>
			Now that we've explored individual Laplace transforms, let's see how we can combine them using a fundamental property: linearity.
		</p>

		<example>

			<m>\quad</m> Use the definition of the Laplace transform to compute
			
			<me> \lap\{15 + 6e^{7t} - 11t\}. </me>
			
			<solution>
				<p>
					Starting from the definition:
					<md>
						<mrow> 
							\lap\{15\ +\amp\ 6e^{7t} - 11t\}	
						</mrow>
						<mrow>		
								=\amp\ \int_0^{\infty} e^{-st} \cdot \left(15 + 6e^{7t} - 11t\right)\ dt
						</mrow>
						<mrow>
								=\amp\ \int_0^{\infty} \left( 15e^{-st} + 6e^{-st} \cdot e^{7t} - 11e^{-st} \cdot t \right)\ dt
						</mrow>
						<mrow>	
								=\amp\ \int_0^{\infty} 15e^{-st} \cdot 1\ dt + \int_0^{\infty} 6e^{-st} \cdot e^{7t}\ dt + \int_0^{\infty} 11e^{-st} \cdot t\ dt
						</mrow>
						<mrow>	
								=\amp\ 15\int_0^{\infty} e^{-st}\cdot 1\ dt + 6\int_0^{\infty} e^{-st} \cdot e^{7t}\ dt - 11\int_0^{\infty} e^{-st} \cdot t\ dt
						</mrow>
					</md>
					Each of the integrals above correspond to a Laplace transform we've already seen.
					<md>
						<mrow>
							\amp= 15\lap\{1\} + 6\lap\{ e^{7t} \} - 11\lap\{ t \},
						</mrow>
						<mrow>
							\amp= \ub{\frac{15}{s}}_{s \gt 0} + 6\ub{\frac{1}{s - 7}}_{s \gt 7} - 11\ub{\frac{1}{s^2}}_{s \gt 0}.
						</mrow>
					</md>
				</p>
			
				<p>
					To satisfy all the conditions on <m>s</m>, we must have <m>s \gt 7</m> since that ensures all terms are defined. Therefore, 
					<me> \lap\{15 + 6e^{7t} - 11t\} = \frac{15}{s} + 6\cdot \frac{1}{s-7} - \frac{11}{s^2}, \quad s \gt 7. </me>
				</p>
			</solution>
		</example>

		<p>
			This example illustrates how Laplace transforms inherit some of their properties directly from integrals. In particular, if <m>a</m> and <m>b</m> are constants, then:
			<me> \lap\{ a f(t) \pm b g(t) \} = a \lap\{ f(t) \} \pm b \lap\{ g(t) \}, </me>
		</p>

		<assemblage xml:id="lt-properties-P1"><title>Laplace Transform Property <m>P_1</m></title>
			<p>
				Let <m>F(s) = \lap{f(t)}</m> and <m>G(s) = \lap{g(t)}</m>.
			</p>

			<p>
				<dl width="narrow">
					<li xml:id="P1"><title><m>P_1</m></title>
						<m>\ds \lap\{ a f(t) \pm b g(t) \} = a F(s) \pm b G(s), \quad a, b </m> are constants
					</li>
				</dl>
			</p>
		</assemblage>

	</paragraphs>

	<xi:include	href="./c4-s1-ss4-1-interactives.ptx" />

	<paragraphs><title> Translational Property </title>

		<example>
			
			<m>\quad</m> Compute	<m> \lap\{e^{7t}\cos(3t)\} </m>.
	
			<solution>
				<p>
					By the definition of the Laplace transform, we have
					<md>
						<mrow> 
							\lap\{e^{7t}\cos(3t)\} 
								=\amp \int_0^{\infty} e^{-st} e^{7t}\cos(3t) dt
						</mrow>
						<mrow> 
								=\amp \int_0^{\infty} e^{-st+7t} \cos(3t) dt
						</mrow>
						<mrow> 
								=\amp \int_0^{\infty} e^{-(s-7)t} \cos(3t) dt
						</mrow>
						<mrow> 
								=\amp \ub{\int_0^{\infty} e^{-(s_0)t} \cos(3t) dt}_{\lap\{\cos(3t)\}}, \quad \text{where } s_0 = s-7
						</mrow>
						<mrow>
								=\amp\ \frac{s_0}{s_0^2 + 9}  \qquad (s_0 \gt 0)
						</mrow>
						<mrow>
								=\amp\ \frac{s-7}{(s-7)^2 + 9} \qquad (s-7 \gt 0 \text{ or } s \gt 7)
						</mrow>
					</md>
				</p>
			</solution> 
		</example>
	
		<assemblage xml:id="lt-properties-P2"><title>Laplace Transform Property <m>P_2</m></title>
			<p>
				Let <m>F(s) = \lap\{f(t)\}</m> and <m>G(s) = \lap\{g(t)\}</m>.
			</p>
	
			<p>
				<dl width="narrow">
					<li xml:id="P2"><title><m>P_2.</m></title>
						<m>\ds \lap\{ e^{at} f(t) \} = F(s-a), \quad a </m> is a constant
					</li>
				</dl>
			</p>
		</assemblage>
	
		<p>
			If we multiply <m>e^{at}</m> by the functions <m>t^n</m>, <m>\cos(bt)</m> and <m>\sin(bt)</m>, this property adds three more common Laplace transforms to our collection, as shown below.
		</p>
	
		<assemblage xml:id="lt-table-L6-L8"><title>Common Laplace Transforms <m>L_6-L_8</m></title>
			<p>
				<dl width="narrow">
					<li xml:id="L6"><title><m>{\LARGE \vphantom{\int}}L_6</m></title>
						<m>\lap\{ t^n e^{at} \} = \ds\frac{n!}{(s-a)^{n+1}}, \quad s &gt;a </m>
					</li>
					<li xml:id="L7"><title><m>{\LARGE \vphantom{\int}}L_7.</m></title>
						<m>\ds \lap\{ e^{at}\cos(bt) \} = \frac{s-a}{(s-a)^2+b^2}, \quad s &gt;a</m>
					</li>
					<li xml:id="L8"><title><m>{\LARGE \vphantom{\int}}L_8.</m></title>
						<m>\ds \lap\{ e^{at}\sin(bt) \} = \frac{b}{(s-a)^2+b^2}, \quad s &gt;a </m>
					</li>
				</dl>
			</p>
		</assemblage>
	
	</paragraphs>

	<xi:include	href="./c4-s1-ss4-2-interactives.ptx" />

	<paragraphs><title> Derivative Property </title>

		<example>
				
			<m>\quad</m> Show that <m>\ds \lap\{f'(t)\} = s\lap\{f(t)\} - f(0), \quad s \gt 0</m>.
	
			<solution>
				<tabular>
					<col width="20%" halign="right" valign="top"/>
					<col width="80%" halign="left" valign="top"/>
					<row>
						<cell valign="top"><p><m>\ds \lap\{ f'(t) \} =</m></p></cell>
						<cell>
							<m>\ds =\int_0^{\infty} e^{-st} f'(t) dt </m>
						</cell>
						<cell/>
					</row>
					<row>
						<cell><xref ref="lt-derivative-key-step-1" text="title"/></cell>
						<cell>
							<m>\ds \left[ e^{-st} f(t) \right]_0^{\infty} - \int_0^{\infty} (-s e^{-st}) f(t) dt </m>
						</cell>
						<cell/>
					</row>
					<row>
						<cell><xref ref="lt-derivative-key-step-2" text="title"/></cell>
						<cell>
							<m>\ds \left[ e^{-st} f(t) \right]_0^{\infty} + s \ub{\int_0^{\infty} e^{-st} f(t) dt}_{\large \lap\{ f(t) \}} </m>
						</cell>
						<cell/>
					</row>
					<row>
						<cell><m>=</m></cell>
						<cell>
							<m>\ds \lim_{t \to \infty} \left( e^{-st} f(t) \right) - e^{-s \cdot 0} f(0) + s \lap\{ f(t) \} </m>
						</cell>
						<cell/>
					</row>
					<row>
						<cell><xref ref="lt-derivative-key-step-3" text="title"/></cell>
						<cell>
							<m>\ds 0 - f(0) + s \lap\{ f(t) \} </m></cell>
						<cell/>
					</row>
					<row>
						<cell><m>=</m></cell>
						<cell>
							<m>\ds s \lap\{ f(t) \} - f(0) </m>
						</cell>
						<cell/>
					</row>
				</tabular>
			</solution>
		</example>
	
		<p>
			The importance of this result cannot be overstated. Even if you did not completely understand the solution, this property highlights why Laplace transforms are so useful in solving differential equations. It essentially removes derivatives from the equation!
		</p>
	
		<p>
			This property hides another secret as well. It recursively <q>removes</q> derivatives one at a time. That is,
			<md>
				<mrow> 
					\lap\{ f'(t) \}	
						=\amp\ \us{\swarrow}{\ul{\color{green} s \lap\{ f(t)	\} - f(0)}}
				</mrow>
				<mrow> 
					\lap\{ f''(t) \}	
						=\amp\ s {\color{green} \lap\{ f'(t) \}} - f'(0)
				</mrow>
				<mrow> 
						=\amp\ s \Big[{\color{green} \lap\{f(t)\} - f(0)} \Big] - f'(0)
				</mrow>
				<mrow> 
						=\amp\ \us{\swarrow \hspace{5em}}{\ul{\color{blue} s \lap\{f(t)\} - sf(0) - f'(0)}}
				</mrow>
				<mrow> 
					\lap\{ f'''(t) \}	
						=\amp\ s {\color{blue} \lap\{ f''(t) \}} - f''(0)
				</mrow>
				<mrow> 
						=\amp\ s \Big[{\color{blue} s \lap\{f(t)\} - sf(0) - f'(0)}\Big] - f''(0)
				</mrow>
				<mrow> 
						=\amp\ s^3 \lap\{f(t)\} - s^2 f(0) - s f'(0) - f''(0)
				</mrow>
				<mrow> \vdots </mrow>
			</md>
			and the pattern continues for higher derivatives.
		</p>
	
		<assemblage xml:id="lt-properties-P3-P5"><title>Laplace Transform Properties <m>P_3-P_5</m></title>
			<p>
				Let <m>F(s) = \lap\{f(t)\}</m> and <m>G(s) = \lap\{g(t)\}</m>.
			</p>
	
			<p>
				<dl width="narrow">
					<li xml:id="P3"><title><m>P_3.</m></title>
						<m>\ds \lap\{ f'(t) \} = sF(s) - f(0) </m>
					</li>
					<li xml:id="P4"><title><m>P_4.</m></title>
						<m>\ds \lap\{ f''(t) \} = s^2F(s) - sf(0) - f'(0) </m>
					</li>
					<li xml:id="P5"><title><m>P_5.</m></title>
						<m>\ds \lap\{ f'''(t) \} = s^3F(s) - s^2f(0) - sf'(0) - f''(0) </m>
					</li>
				</dl>
			</p>
		</assemblage>
	
	</paragraphs>

	<xi:include	href="./c4-s1-ss4-3-interactives.ptx" />

	<paragraphs><title> <m>\lap\{t^n f(t)\}</m> </title>

		<p>
			Let's build on what we did in the previous section.
		</p>
	
		<example>
				
			<m>\quad</m> Show that <m>\ds \lap\{tf(t)\} = -\frac{d}{ds}\left[\lap\{f(t)\}\right]</m>.
	
			<solution>
				<p>
					For this problem it is actually easier to start on the right side and show it is equal to the left.
				</p>
				<tabular>
					<col width="30%" halign="right" valign="top"/>
					<col width="60%" halign="left" valign="top"/>
					<row>
						<cell valign="top"><p><m>\ds -\frac{d}{ds}\left[\lap\{f(t)\}\right] =</m></p></cell>
						<cell>
							<m>\ds -\frac{d}{ds}\left[\int_0^{\infty} e^{-st} f(t) dt\right] </m>
						</cell>
					</row>
					<row>
						<cell><m>=</m></cell>
						<cell>
							<m>\ds -\int_0^{\infty} \frac{\partial}{\partial s}\left[e^{-st} f(t)\right] dt </m>
						</cell>
					</row>
					<row>
						<cell><m>=</m></cell>
						<cell>
							<m>\ds -\int_0^{\infty} f(t)\frac{\partial}{\partial s}\left[e^{-st}\right] dt </m>
						</cell>
					</row>
					<row>
						<cell><m>=</m></cell>
						<cell>
							<m>\ds -\int_0^{\infty} f(t) \left(-te^{-st}\right)  dt </m>
						</cell>
					</row>
					<row>
						<cell><m>=</m></cell>
						<cell>
							<m>\ds \int_0^{\infty} e^{-st} tf(t) dt </m>
						</cell>
					</row>
					<row>
						<cell><m>=</m></cell>
						<cell>
							<m>\ds \lap\{tf(t)\} </m>
						</cell>
					</row>
				</tabular>
			</solution>
		</example>
	
		<p>
			This shows that multiplying a function by <m>t</m> inside a Laplace transform is equivalent to taking the derivative of the Laplace transform of the same function, multiplied by <m>-1</m>. It turns our that each power of <m>t</m> adds another neagtive one and derivative.
		</p>
	
		<example>
				
			<m>\quad</m> Show that <m>\ds \lap\{t^2f(t)\} = \frac{d^2}{ds^2}\left[\lap\{f(t)\}\right]</m>.
	
			<solution>
				<p>
					For this problem it is actually easier to start on the right side and show it is equal to the left.
				</p>
				<tabular>
					<col width="30%" halign="right" valign="top"/>
					<col width="60%" halign="left" valign="top"/>
					<row>
						<cell valign="top"><p><m>\ds \frac{d^2}{ds^2}\left[\lap\{f(t)\}\right] =</m></p></cell>
						<cell>
							<m>\ds \frac{d^2}{ds^2}\left[\int_0^{\infty} e^{-st} f(t) dt\right] </m>
						</cell>
					</row>
					<row>
						<cell><m>=</m></cell>
						<cell>
							<m>\ds \int_0^{\infty} \frac{\partial^2}{\partial s^2}\left[e^{-st} f(t)\right] dt </m>
						</cell>
					</row>
					<row>
						<cell><m>=</m></cell>
						<cell>
							<m>\ds \int_0^{\infty} f(t)\frac{\partial^2}{\partial s^2}\left[e^{-st}\right] dt </m>
						</cell>
					</row>
					<row>
						<cell><m>=</m></cell>
						<cell>
							<m>\ds \int_0^{\infty} f(t) \left((-t)^2e^{-st}\right)  dt </m>
						</cell>
					</row>
					<row>
						<cell><m>=</m></cell>
						<cell>
							<m>\ds \int_0^{\infty} e^{-st} t^2f(t) dt </m>
						</cell>
					</row>
					<row>
						<cell><m>=</m></cell>
						<cell>
							<m>\ds \lap\{t^2f(t)\} </m>
						</cell>
					</row>
				</tabular>
			</solution>
		</example>
	
		<p>
			A similar process shows that for any power of <m>t</m>, the Laplace transform is the <m>n</m>-th derivative of the Laplace transform of the function, with the sign alternating. The general property is given by
			<me> \lap\{t^n f(t)\} = (-1)^n \frac{d^{(n)}}{ds^{(n)}}F(s), \quad n = 1, 2, 3, \ldots </me>.
			The only difference is that you are taking the <m>n</m>-th derivative of <m>e^{-st}f(t)</m> inside the integral.
		</p>
	
		<assemblage xml:id="lt-properties-P6"><title>Laplace Transform Property<m>P_6</m></title>
			<p>
				Let <m>F(s) = \lap\{f(t)\}</m> and <m>G(s) = \lap\{g(t)\}</m>.
			</p>
	
			<p>
				<dl width="narrow">
					<li xml:id="P6"><title><m>{\LARGE \vphantom{\int}}P_6.</m></title>
						<m>\ds \lap\{ t^n f(t) \} = (-1)^n \frac{d^{(n)}}{ds^{(n)}}F(s), \quad n = 1, 2, 3, \ldots </m>
					</li>
				</dl>
			</p>
		</assemblage>
	
	</paragraphs>
	
	<xi:include	href="./c4-s1-ss4-4-interactives.ptx" />

</subsection>