<subsection xmlns:xi="http://www.w3.org/2001/XInclude"><title> Properties of Laplace Transforms </title>

	<p>
		Now that we've explored individual Laplace transforms, its time to delve into some of the key properties that make the Laplace transform such a powerful tool for solving differential equations. These properties allow us to manipulate and combine transforms in ways that simplify complex problems.
	</p>

	<paragraphs><title>Linearity</title>
	
		<p>
			The first property we'll explore is linearity. This property is foundational because it allows us to break down and combine transforms easily. The linearity of the Laplace transform is similar to the linearity of integrals, where we can distribute the transform across addition and subtraction, and pull out constants.
		</p>

	</paragraphs>

	<example>
		<m>\quad</m> Use the definition of the Laplace transform to compute:
		
		<me> \lap{15 + 6e^{7t} - 11t}. </me>
		
		<solution>
			<p>
				Let's start by applying the definition of the Laplace transform:
				<md>
					<mrow> 
						\lap{15\ +\amp\ 6e^{7t} - 11t}	
					</mrow>
					<mrow>		
							=\amp\ \int_0^{\infty} e^{-st} \cdot \left(15 + 6e^{7t} - 11t\right)\ dt
					</mrow>
					<mrow>
							=\amp\ \int_0^{\infty} \left( 15e^{-st} + 6e^{-st} \cdot e^{7t} - 11e^{-st} \cdot t \right)\ dt
					</mrow>
				</md>
				Here, we've expanded the expression inside the integral. Notice that each term is something we've already encountered in previous sections. We can now use the linearity property to separate the integral:
				<md>
					<mrow>	
						=\amp\ 15\int_0^{\infty} e^{-st}\cdot 1\ dt + 6\int_0^{\infty} e^{-st} \cdot e^{7t}\ dt - 11\int_0^{\infty} e^{-st} \cdot t\ dt
					</mrow>
					<mrow>
						=\amp\ 15\lap{1} + 6\lap{ e^{7t} } - 11\lap{ t }.
					</mrow>
				</md>
				We already know the Laplace transforms of these individual functions:
				<md>
					<mrow>
						=\amp\ \ub{\frac{15}{s}}_{s \gt 0} + 6\ub{\frac{1}{s - 7}}_{s \gt 7} - 11\ub{\frac{1}{s^2}}_{s \gt 0}.
					</mrow>
				</md>
				To satisfy all the conditions on <m>s</m>, we must have <m>s \gt 7</m> since that ensures all terms are defined. Therefore:
				<me>
					\lap{15 + 6e^{7t} - 11t} = \frac{15}{s} + 6\cdot \frac{1}{s-7} - \frac{11}{s^2}, \quad s \gt 7.
				</me>
			</p>
		</solution>
	</example>

	<p>
		This example demonstrates the linearity property in action. The general statement of the linearity property is as follows: if <m>a</m> and <m>b</m> are constants, then:
		<me> \lap{ a f(t) \pm b g(t) } = a \lap{ f(t) } \pm b \lap{ g(t) }, </me>
		or, equivalently:
		<me> \lap{ a f(t) \pm b g(t) } = a F(s) \pm b G(s). </me>
	</p>
	
	<assemblage xml:id="lt-properties-P1"><title>Laplace Transform Property <m>P_1</m></title>
		<p>
			<dl width="narrow">
				<li xml:id="P1"><title><m>{\LARGE \vphantom{\int}}P_1</m></title>
					<m>\ds \lap{ a f(t) \pm b g(t) } = a \lap{f(t)} \pm b \lap{g(t)}</m>
				</li>
			</dl>
		</p>
	</assemblage>
	
	<xi:include	href="./c4-s1-ss4-1-interactives.ptx" />

	<paragraphs><title>Multiplication by <m>e^{at}</m></title>
	
		<p>
			The translation property, also known as the first shifting theorem, allows us to handle functions multiplied by an exponential term, <m>e^{at}</m>. This property is particularly useful for simplifying the Laplace transforms of products of exponential functions and other functions, such as sine, cosine, or polynomials.
		</p>

	</paragraphs>

	<example>
		
		<m>\quad</m> Compute <m> \lap{e^{7t}\cos(3t)} </m>.
		
		<solution>
			<p>
				By the definition of the Laplace transform, we have:
				<md>
					<mrow> 
						\lap{e^{7t}\cos(3t)} 
							=\amp \int_0^{\infty} e^{-st} e^{7t}\cos(3t)\ dt
					</mrow>
					<mrow> 
							=\amp \int_0^{\infty} e^{-st+7t} \cos(3t)\ dt
					</mrow>
					<mrow> 
							=\amp \int_0^{\infty} e^{-(s-7)t} \cos(3t)\ dt
					</mrow>
					<mrow> 
							=\amp \ub{\int_0^{\infty} e^{-(s_0)t} \cos(3t)\ dt}_{\lap{\cos(3t)}}, \quad \text{where } s_0 = s-7
					</mrow>
					<mrow>
							=\amp\ \frac{s_0}{s_0^2 + 9}  \qquad (s_0 \gt 0)
					</mrow>
					<mrow>
							=\amp\ \frac{s-7}{(s-7)^2 + 9} \qquad (s-7 \gt 0 \text{ or } s \gt 7)
					</mrow>
				</md>
				Thus, the Laplace transform of <m>e^{7t}\cos(3t)</m> is:
				<me>\ds \lap{e^{7t}\cos(3t)} = \frac{s-7}{(s-7)^2 + 9}, \quad s \gt 7.</me>
			</p>
		</solution>
	</example>

	<p>
		The translation property can be generalized for any function <m>f(t)</m> multiplied by <m>e^{at}</m>. The property is formally stated as:
		<me> \lap{ e^{at} f(t) } = F(s-a), </me>
		where <m>F(s)</m> is the Laplace transform of <m>f(t)</m>.
	</p>

	<assemblage xml:id="lt-properties-P2"><title>Laplace Transform Property <m>P_2</m></title>
		<p>
			Let <m>F(s) = \lap{f(t)}</m>.
		</p>

		<p>
			<dl width="narrow">
				<li xml:id="P2"><title><m>P_2</m></title>
					<m>\ds \lap{ e^{at} f(t) } = F(s-a), \quad a </m> is a constant.
				</li>
			</dl>
		</p>
	</assemblage>
	
	<p>
		By applying this property to the functions <m>t^n</m>, <m>\cos(bt)</m>, and <m>\sin(bt)</m>, we can derive additional common Laplace transforms:
	</p>
	
	<assemblage xml:id="lt-table-L6-L8"><title>Common Laplace Transforms <m>L_6-L_8</m></title>
		<p>
			<dl width="narrow">
				<li xml:id="L6"><title><m>{\LARGE \vphantom{\int}}L_6</m></title>
					<m>\lap{ t^n e^{at} } = \ds\frac{n!}{(s-a)^{n+1}}, \quad s >a </m>
				</li>
				<li xml:id="L7"><title><m>{\LARGE \vphantom{\int}}L_7</m></title>
					<m>\ds \lap{ e^{at}\sin(bt) } = \frac{b}{(s-a)^2+b^2}, \quad s >a </m>
				</li>
				<li xml:id="L8"><title><m>{\LARGE \vphantom{\int}}L_8</m></title>
					<m>\ds \lap{ e^{at}\cos(bt) } = \frac{s-a}{(s-a)^2+b^2}, \quad s >a</m>
				</li>
			</dl>
		</p>
	</assemblage>

	<xi:include	href="./c4-s1-ss4-2-interactives.ptx" />

	<paragraphs><title>Derivative Transform</title>
	
		<p>
			The derivative property of the Laplace transform is one of its most powerful aspects, especially when solving differential equations. This property allows us to transform differential equations into algebraic equations, making them easier to solve.
		</p>

	</paragraphs>

	<example>
		<m>\quad</m> Show that <m>\ds \lap{f'(t)} = s\lap{f(t)} - f(0), \quad s \gt 0</m>.
	
		<solution>
			<tabular>
				<col width="20%" halign="right" valign="top"/>
				<col width="80%" halign="left" valign="top"/>
				<row>
					<cell valign="top"><p><m>\ds \lap{ f'(t) } =</m></p></cell>
					<cell>
						<m>\ds \int_0^{\infty} e^{-st} f'(t)\ dt </m>
					</cell>
				</row>
				<row>
					<cell><xref ref="lt-derivative-key-step-1" text="title"/></cell>
					<cell>
						<m>\ds \left[ e^{-st} f(t) \right]_0^{\infty} - \int_0^{\infty} (-s e^{-st}) f(t)\ dt </m>
					</cell>
				</row>
				<row>
					<cell><xref ref="lt-derivative-key-step-2" text="title"/></cell>
					<cell>
						<m>\ds \left[ e^{-st} f(t) \right]_0^{\infty} + s \ub{\int_0^{\infty} e^{-st} f(t)\ dt}{\large \lap{ f(t) }} </m>
					</cell>
				</row>
				<row>
					<cell><m>=</m></cell>
					<cell>
						<m>\ds \lim_{t \to \infty} \left( e^{-st} f(t) \right) - e^{-s \cdot 0} f(0) + s \lap{ f(t) } </m>
					</cell>
				</row>
				<row>
					<cell><xref ref="lt-derivative-key-step-3" text="title"/></cell>
					<cell>
						<m>\ds 0 - f(0) + s \lap{ f(t) } </m>
					</cell>
				</row>
				<row>
					<cell><m>=</m></cell>
					<cell>
						<m>\ds s \lap{ f(t) } - f(0) </m>
					</cell>
				</row>
			</tabular>
		</solution>
	</example>

	<p>
		This result is crucial for solving differential equations. Essentially, it allows us to eliminate derivatives from an equation, transforming the problem into an algebraic form that's easier to solve. But there's moreâ€”this property also works recursively, allowing us to handle higher-order derivatives as well.
	</p>
	
	<p>
		For example, let's see how this property extends to second and third derivatives:
		<md>
			<mrow> 
				\lap{ f'(t) }	
					=\amp\ \us{\swarrow}{\ul{\color{green} s \lap{ f(t)	} - f(0)}}
			</mrow>
			<mrow> 
				\lap{ f''(t) }	
					=\amp\ s {\color{green} \lap{ f'(t) }} - f'(0)
			</mrow>
			<mrow> 
					=\amp\ s \Big[{\color{green} \lap{f(t)} - f(0)} \Big] - f'(0)
			</mrow>
			<mrow> 
					=\amp\ \us{\swarrow \hspace{5em}}{\ul{\color{blue} s \lap{f(t)} - sf(0) - f'(0)}}
			</mrow>
			<mrow> 
				\lap{ f'''(t) }	
					=\amp\ s {\color{blue} \lap{ f''(t) }} - f''(0)
			</mrow>
			<mrow> 
					=\amp\ s \Big[{\color{blue} s \lap{f(t)} - sf(0) - f'(0)}\Big] - f''(0)
			</mrow>
			<mrow> 
					=\amp\ s^3 \lap{f(t)} - s^2 f(0) - s f'(0) - f''(0)
			</mrow>
			<mrow> \vdots </mrow>
		</md>
		And the pattern continues for higher derivatives.
	</p>

	<assemblage xml:id="lt-properties-P3-P5"><title>Laplace Transform Properties <m>P_3-P_5</m></title>
		<p>
			Let <m>F(s) = \lap{f(t)}</m>.
		</p>

		<p>
			<dl width="narrow">
				<li xml:id="P3"><title><m>P_3</m></title>
					<m>\ds \lap{ f'(t) } = sF(s) - f(0) </m>
				</li>
				<li xml:id="P4"><title><m>P_4</m></title>
					<m>\ds \lap{ f''(t) } = s^2F(s) - sf(0) - f'(0) </m>
				</li>
				<li xml:id="P5"><title><m>P_5</m></title>
					<m>\ds \lap{ f'''(t) } = s^3F(s) - s^2f(0) - sf'(0) - f''(0) </m>
				</li>
			</dl>
		</p>

	</assemblage>

	<xi:include	href="./c4-s1-ss4-3-interactives.ptx" />

	<paragraphs><title>Multiplication by <m>t^n</m></title>
	
		<p>
			The final property we'll explore is how the Laplace transform handles functions multiplied by a power of <m>t</m>. This property is especially useful when dealing with polynomial terms in differential equations.
		</p>

	</paragraphs>

	<example>

		<m>\quad</m> Show that <m>\ds \lap{tf(t)} = -\frac{d}{ds}\left[\lap{f(t)}\right]</m>.
		
		<solution>
			<p>
				For this problem, it's easier to start on the right side and show that it equals the left:
			</p>
			<tabular>
				<col width="30%" halign="right" valign="top"/>
				<col width="60%" halign="left" valign="top"/>
				<row>
					<cell valign="top"><p><m>\ds -\frac{d}{ds}\left[\lap{f(t)}\right] =</m></p></cell>
					<cell>
						<m>\ds -\frac{d}{ds}\left[\int_0^{\infty} e^{-st} f(t)\ dt\right] </m>
					</cell>
				</row>
				<row>
					<cell><m>=</m></cell>
					<cell>
						<m>\ds -\int_0^{\infty} \frac{\partial}{\partial s}\left[e^{-st} f(t)\right]\ dt </m>
					</cell>
				</row>
				<row>
					<cell><m>=</m></cell>
					<cell>
						<m>\ds -\int_0^{\infty} f(t)\frac{\partial}{\partial s}\left[e^{-st}\right]\ dt </m>
					</cell>
				</row>
				<row>
					<cell><m>=</m></cell>
					<cell>
						<m>\ds -\int_0^{\infty} f(t) \left(-te^{-st}\right)\ dt </m>
					</cell>
				</row>
				<row>
					<cell><m>=</m></cell>
					<cell>
						<m>\ds \int_0^{\infty} e^{-st} tf(t)\ dt </m>
					</cell>
				</row>
				<row>
					<cell><m>=</m></cell>
					<cell>
						<m>\ds \lap{tf(t)} </m>
					</cell>
				</row>
			</tabular>
		</solution>
	</example>

	<p>
		This shows that multiplying a function by <m>t</m> inside a Laplace transform is equivalent to taking the derivative of the Laplace transform of the same function, multiplied by <m>-1</m>. It turns out that each additional power of <m>t</m> adds another negative sign and derivative.
	</p>

	<example>

		<m>\quad</m> Show that <m>\ds \lap{t^2f(t)} = \frac{d^2}{ds^2}\left[\lap{f(t)}\right]</m>.
		
		<solution>

			<p>
				Again, it's easier to start on the right side and work our way to the left:
			</p>

			<tabular>
				<col width="30%" halign="right" valign="top"/>
				<col width="60%" halign="left" valign="top"/>
				<row>
					<cell valign="top"><p><m>\ds \frac{d^2}{ds^2}\left[\lap{f(t)}\right] =</m></p></cell>
					<cell>
						<m>\ds \frac{d^2}{ds^2}\left[\int_0^{\infty} e^{-st} f(t)\ dt\right] </m>
					</cell>
				</row>
				<row>
					<cell><m>=</m></cell>
					<cell>
						<m>\ds \int_0^{\infty} \frac{\partial^2}{\partial s^2}\left[e^{-st} f(t)\right]\ dt </m>
					</cell>
				</row>
				<row>
					<cell><m>=</m></cell>
					<cell>
						<m>\ds \int_0^{\infty} f(t)\frac{\partial^2}{\partial s^2}\left[e^{-st}\right]\ dt </m>
					</cell>
				</row>
				<row>
					<cell><m>=</m></cell>
					<cell>
						<m>\ds \int_0^{\infty} f(t) \left((-t)^2e^{-st}\right)\ dt </m>
					</cell>
				</row>
				<row>
					<cell><m>=</m></cell>
					<cell>
						<m>\ds \int_0^{\infty} e^{-st} t^2f(t)\ dt </m>
					</cell>
				</row>
				<row>
					<cell><m>=</m></cell>
					<cell>
						<m>\ds \lap{t^2f(t)} </m>
					</cell>
				</row>
			</tabular>
		</solution>
	</example>

	<p>
		A similar process shows that for any power of <m>t</m>, the Laplace transform is the <m>n</m>-th derivative of the Laplace transform of the function, with the sign alternating. The general property is given by:
		<me> \lap{t^n f(t)} = (-1)^n \frac{d^{(n)}}{ds^{(n)}}F(s), \quad n = 1, 2, 3, \ldots </me>.
		The only difference is that you are taking the <m>n</m>-th derivative of <m>e^{-st}f(t)</m> inside the integral.
	</p>
	
	<assemblage xml:id="lt-properties-P6"><title>Laplace Transform Property <m>P_6</m></title>
		<p>
			Let <m>F(s) = \lap{f(t)}</m>.
		</p>

		<p>
			<dl width="narrow">
				<li xml:id="P6"><title><m>P_6</m></title>
					<m>\ds \lap{ t^n f(t) } = (-1)^n \frac{d^{(n)}}{ds^{(n)}}F(s), \quad n = 1, 2, 3, \ldots </m>
				</li>
			</dl>
		</p>
	</assemblage>

	<xi:include	href="./c4-s1-ss4-4-interactives.ptx" />

</subsection> 