
<subsection xmlns:xi="http://www.w3.org/2001/XInclude"><title> Summary &amp; Exercises </title>

	<introduction>
		
		<p>
			<assemblage color="green"><title>Summary of the Key Ideas</title>
				<p>
					<term> <em> Method</em> </term>
					<p>
						
					</p>
				</p>
			</assemblage>
		</p>
		
	</introduction>

	<exercises>

		<exercisegroup>
			<title></title>
				<exercise>
					<statement>
						<alert>Use the definition of Laplace Transform</alert> (above) to find the Laplace Transform of <m> \ds h(t) = 7t. </m>
					</statement>
					<solution>
						 \\ In order to evaluate this integral, we will need to compute an integration by parts. When that time comes, we will choose <m> \ds u = t </m> an <m> \ds dv = e^{-st}. </m>  Then we take the derivative o <m> \ds u </m> to fin <m> \ds du </m> and the antiderivative o <m> \ds dv </m> to fin <m> \ds v </m> , as follows.
						<md>
							<mrow>  u	 \amp =  t 						\amp dv	\amp= e^{-st}dt </mrow>
							<mrow>  \Rightarrow du	 \amp =  dt\hspace{1cm}\mbox{}	\amp \Rightarrow v	\amp= -\frac{1}{s}e^{-st}  </mrow>
						</md>
						 Note also that we will use L'Hospital's Rule when we have a limit of for <m> \ds \frac{\infty}{\infty}. </m>
						<md>
							<mrow>  H(s)	 \amp =  \lap\{ h(t) \} </mrow>
							<mrow>   \amp =  \int_0^{\infty}e^{-st}h(t) dt </mrow>
							<mrow>   \amp =  \int_0^{\infty}e^{-st}\cdot 7t dt </mrow>
							<mrow>   \amp =  \lim_{b \to \infty} \int_0^b e^{-st}\cdot 7t dt </mrow>
							<mrow>   \amp =   7\cdot \lim_{b \to \infty} \int_0^b te^{-st} dt </mrow>
							<mrow>   \amp =   7\cdot \lim_{b \to \infty} \left[t\cdot\left(-\frac{1}{s}e^{-st}\right)\Bigg|_0^b - \int_0^b -\frac{1}{s}e^{-st} dt\right] </mrow>
							<mrow>   \amp =   7\cdot \lim_{b \to \infty} \left[-\frac{t}{se^{st}}\Bigg|_0^b + \frac{1}{s}\int_0^b e^{-st} dt\right] </mrow>
							<mrow>   \amp =   7\cdot \lim_{b \to \infty} \left[-\frac{t}{se^{st}} + \frac{1}{s} \cdot -\frac{1}{s}e^{-st} \right]_0^b </mrow>
							<mrow>   \amp =   7\cdot \lim_{b \to \infty} \left[-\frac{t}{se^{st}} - \frac{1}{s^2 e^{st}} \right]_0^b </mrow>
						</md>
			
						<md>
							<mrow>   \amp =   7\cdot \lim_{b \to \infty} \left[\left( -\frac{b}{se^{sb}} - \frac{1}{s^2 e^{sb}} \right) - \left( -\frac{0}{se^{s\cdot 0}} - \frac{1}{s^2 e^{s\cdot 0}} \right) \right] </mrow>
							<mrow>   \amp =   7\cdot \lim_{b \to \infty} \left[\left( -\frac{b}{se^{sb}} - \frac{1}{s^2 e^{sb}} \right) - \left( 0 - \frac{1}{s^2} \right) \right] </mrow>
							<mrow>   \amp =   7\cdot \lim_{b \to \infty} \left[-\frac{b}{se^{sb}} - \frac{1}{s^2 e^{sb}}+ \frac{1}{s^2} \right] </mrow>
							<mrow>   \amp =   7\cdot \lim_{b \to \infty} \left[-\frac{b}{se^{sb}} \right] - 7\cdot \lim_{b \to \infty} \left[\frac{1}{s^2 e^{sb}} \right] + 7\cdot \lim_{b \to \infty} \left[\frac{1}{s^2} \right] </mrow>
							<mrow>   \amp =   -7\cdot \frac{1}{s} \cdot \lim_{b \to \infty} \left[\frac{b}{e^{sb}} \right] - 7\cdot \frac{1}{s^2}\cdot \lim_{b \to \infty} \left[\frac{1}{e^{sb}} \right] + 7\cdot \frac{1}{s^2} </mrow>
							<mrow>   \amp =   -\frac{7}{s} \cdot  \lim_{b \to \infty} \left[\frac{1}{se^{sb}} \right] - \frac{7}{s^2}\cdot \lim_{b \to \infty} \left[\frac{1}{e^{sb}} \right] + \frac{7}{s^2} \mbox{ (using L'H Rule)} </mrow>
							<mrow>   \amp =   -\frac{7}{s^2} \cdot  \lim_{b \to \infty} \left[\frac{1}{e^{sb}} \right] - \frac{7}{s^2}\cdot \lim_{b \to \infty} \left[\frac{1}{e^{sb}} \right] + \frac{7}{s^2} </mrow>
							<mrow>   \amp =   -\frac{7}{s^2} \cdot  0 - \frac{7}{s^2}\cdot 0 + \frac{7}{s^2} </mrow>
							<mrow>   \amp =   \frac{7}{s^2} </mrow>
						</md>
			
					</solution>
					<answer>
						<m> \ds H(s) = \frac{7}{s^2} </m>
					</answer>
				</exercise>
			
		</exercisegroup>
				
		<exercisegroup>
		<title></title>
			<exercise>
		
				<statement>
					<alert>Use the definition of Laplace Transform</alert> (above) to find the Laplace Transform of <m>\ds h(t) = e^{at}</m> where <m>a</m> is some constant.
				</statement>
		
				<solution>
						\\
					<md>
						<mrow>  W(s)	 \amp =  \lap\{ w(t) \} </mrow>
						<mrow>   \amp =  \int_0^{\infty}e^{-st}w(t) dt </mrow>
						<mrow>   \amp =  \int_0^{\infty}e^{-st}\cdot e^{at} dt </mrow>
						<mrow>   \amp =  \lim_{b \to \infty} \int_0^b e^{-st}\cdot e^{at} dt </mrow>
						<mrow>   \amp =  \lim_{b \to \infty} \int_0^b e^{-st + at}dt </mrow>
						<mrow>   \amp =  \lim_{b \to \infty} \int_0^b e^{(-s + a)t}dt </mrow>
						<mrow>   \amp =  \lim_{b \to \infty} \left[ \frac{1}{-s+a} \cdot e^{(-s + a)t} \right]_0^b </mrow>
						<mrow>   \amp =  \lim_{b \to \infty} \left[ \left(\frac{1}{-s+a} \cdot e^{(-s + a)\cdot b}\right) - \left(\frac{1}{-s+a} \cdot e^{(-s + a)\cdot 0}\right) \right] </mrow>
						<mrow>   \amp =  \lim_{b \to \infty} \left[ \left(\frac{1}{-s+a} \cdot e^{(-s + a)\cdot b}\right) - \left(\frac{1}{-s+a} \cdot 1\right) \right] </mrow>
						<mrow>   \amp =  \lim_{b \to \infty} \left[ \frac{1}{-s+a} \cdot e^{(-s + a)\cdot b} - \frac{1}{-s+a} \right] </mrow>
						<mrow>   \amp =  \lim_{b \to \infty} \left[ \frac{1}{-s+a} \cdot e^{(-s + a)\cdot b} \right] - \lim_{b \to \infty} \left[ \frac{1}{-s+a} \right] </mrow>
						<mrow>   \amp =  \frac{1}{-s+a} \cdot \lim_{b \to \infty} \left[ e^{(-s + a)\cdot b} \right] - \frac{1}{-s+a} </mrow>
						<mrow>   \amp =  \frac{1}{-s+a} \cdot 0 - \frac{1}{-s+a} \mbox{ (assumin <m> \ds -s+a </m> is negative)} </mrow>
						<mrow>   \amp =  - \frac{1}{-s+a} </mrow>
						<mrow>   \amp =  \frac{1}{s-a}  </mrow>
					</md>
		
				</solution>
		
				<answer>
					<m> \ds W(s) = \frac{1}{s-a} </m>
				</answer>
		
			</exercise>
		
		</exercisegroup>
		
		<exercisegroup>
		<title></title>
			<exercise>
				<statement>
					<alert>Use the definition of Laplace Transform</alert> (above) to find the Laplace Transform of <m>\ds y(t) = 7t + e^{5t}</m>.
				</statement>
				<solution>
						\\ We will use the results from the previous two questions.
					<md>
						<mrow>  Y(s)	 \amp =  \lap\{ y(t) \} </mrow>
						<mrow>   \amp =  \int_0^{\infty}e^{-st}y(t) dt </mrow>
						<mrow>   \amp =  \int_0^{\infty}e^{-st}\cdot (7t + e^{5t}) dt </mrow>
						<mrow>   \amp =  \int_0^{\infty}(e^{-st}\cdot 7t + e^{-st}\cdot e^{5t}) dt </mrow>
						<mrow>   \amp =  \int_0^{\infty}e^{-st}\cdot 7t dt + \int_0^{\infty}(e^{-st}\cdot e^{5t} dt </mrow>
						<mrow>   \amp =  \lap\{ 7t \} + \lap\{ e^{5t} \} </mrow>
						<mrow>   \amp= \frac{7}{s^2} + \frac{1}{s-5} </mrow>
					</md>
						Notice that what we showed in the middle of all this is that <m> \ds \lap\{ 7t + e^{5t} \} = \lap\{ 7t \} + \lap\{ e^{5t} \}. </m> This is an example of the linearity property of Laplace Transforms.
				</solution>
				<answer>
					<m> \ds Y(s) = \frac{7}{s^2} + \frac{1}{s-5} </m>
				</answer>
			</exercise>
		
		</exercisegroup>
		
		<exercisegroup>
		<title></title>
			<exercise>
				<statement>
					<alert>Use the definition of Laplace Transform</alert> (above) to find the Laplace Transform of the function
						<m>\ds
							d(t) = \left\{
							\begin{array}{ll}
							0,	\amp t \lt 0\\
							7,	\amp 0 \le t \lt 3\\
							0,	\amp t \ge 3\\
							\end{array} \right.
						</m>
				</statement>
				<solution>
		
					<md>
						<mrow>  D(s)	 \amp =  \lap\{ d(t) \} </mrow>
						<mrow>   \amp =  \int_0^{\infty}e^{-st}d(t) dt </mrow>
						<mrow>   \amp =  \int_0^3 e^{-st}\cdot 7 dt + \int_3^{\infty} e^{-st}\cdot 0 dt </mrow>
						<mrow>   \amp =  7\int_0^3 e^{-st}dt + 0 </mrow>
						<mrow>   \amp =  7 \cdot \left[\frac{1}{-s}e^{-st}\right]_0^3 </mrow>
						<mrow>   \amp =  7 \cdot \left[\left(\frac{1}{-s}e^{-s\cdot 3}\right) - \left(\frac{1}{-s}e^{-s\cdot 0}\right)\right] </mrow>
						<mrow>   \amp =  7 \cdot \left[\left(\frac{1}{-s}e^{-s\cdot 3}\right) - \left(\frac{1}{-s}\cdot 1\right)\right] </mrow>
						<mrow>   \amp =  7 \cdot \left[-\frac{1}{s}e^{-3s} +\frac{1}{s}\cdot 1\right] </mrow>
						<mrow>   \amp =  7 \cdot \left[-\frac{1}{s}e^{-3s} +\frac{1}{s}\right] </mrow>
						<mrow>   \amp =  \frac{7}{s} - \frac{7}{s}e^{-3s} </mrow>
		
					</md>
		
				</solution>
				<answer>
					<m> \ds D(s) = \frac{7}{s} - \frac{7}{s}e^{-3s} </m>
				</answer>
			</exercise>
		
		</exercisegroup>

		<!--========== Exercise Group 1 ==========--> 
<exercisegroup>
	<title>
	<p>
	
	</p>
	<p/> <!-- added for vertical space -->
	</title>
		<exercise> <!--== Problem 1 ==-->
			<statement>
				
			</statement>
			<solution>
				<m> \ds g(t) = t^3 e^{-9t} </m>
			</solution>
			<answer>
				
			</answer>
		</exercise>
	
	</exercisegroup>
	
	<!--========== Exercise Group 2 ==========--> 
	<exercisegroup>
	<title>
	<p>
	
	</p>
	<p/> <!-- added for vertical space -->
	</title>
		<exercise> <!--== Problem 2 ==-->
			<statement>
				<m> \ds g(t) = t^3 e^{-9t} </m>
			</statement>
			<solution>
				
				<md>
					<mrow>  G(s)	 \amp =  \lap\{ g(t) \} </mrow>
					<mrow>   \amp =  \lap\{ t^3 e^{-9t} \} </mrow>
					<mrow>   \amp =  \frac{3!}{\big(s-(-9)\big)^{3+1}} \mbox{ (by L6)} </mrow>
					<mrow>   \amp =  \frac{6}{(s+9)^4} </mrow>
	 
				</md>
				
			</solution>
			<answer>
				<m> \ds G(s) = \frac{6}{(s+9)^4} </m>
			</answer>
		</exercise>
	
	</exercisegroup>
	
	<!--========== Exercise Group 3 ==========--> 
	<exercisegroup>
	<title>
	<p>
	
	</p>
	<p/> <!-- added for vertical space -->
	</title>
		<exercise> <!--== Problem 3 ==-->
			<statement>
				<m> \ds h(t) = e^{2t} - t^3 + t^2 - \sin (5t) </m>
			</statement>
			<solution>
				
				<md>
					<mrow>  H(s)	 \amp =  \lap\{ h(t) \} </mrow>
					<mrow>   \amp =  \lap\{ e^{2t} - t^3 + t^2 - \sin (5t) \} </mrow>
					<mrow>   \amp =  \lap\{ e^{2t} \} - \lap\{ t^3 \} + \lap\{ t^2 \} - \lap\{ \sin(5t) \} \mbox{ (by L9)} </mrow>
					<mrow>   \amp =  \frac{1}{s-2} - \frac{3!}{s^{3+1}} + \frac{2!}{s^{2+1}} - \frac{5}{s^2 + 5^2} \mbox{ (by L2, L3 and L4)} </mrow>
					<mrow>   \amp =  \frac{1}{s-2} - \frac{6}{s^4} + \frac{2}{s^3} - \frac{5}{s^2 + 25} </mrow>
	 
				</md>
				
			</solution>
			<answer>
				<m> \ds H(s) = \frac{1}{s-2} - \frac{5}{s^4} + \frac{2}{s^3} - \frac{5}{s^2 + 25} </m>
			</answer>
		</exercise>
	
	</exercisegroup>
	
	<!--========== Exercise Group 4 ==========--> 
	<exercisegroup>
	<title>
	<p>
	
	</p>
	<p/> <!-- added for vertical space -->
	</title>
		<exercise> <!--== Problem 4 ==-->
			<statement>
				<m> \ds f(t) = e^{-2t}\sin(2t) + t^2 e^{3t} </m>
			</statement>
			<solution>
				
				<md>
					<mrow>  F(s)	 \amp =  \lap\{ f(t) \} </mrow>
					<mrow>   \amp =  \lap\{ e^{-2t}\sin(2t) + t^2 e^{3t} \} </mrow>
					<mrow>   \amp =  \lap\{ e^{-2t}\sin(2t)\} + \lap\{t^2 e^{3t} \} \mbox{ (by L9)} </mrow>
					<mrow>   \amp =  \frac{2}{\big(s- (-2) \big)^2 + 2^2} + \frac{2!}{(s-3)^{2+1}} \mbox{ (by L7 and L6)} </mrow>
					<mrow>   \amp =  \frac{2}{(s+2)^2 + 4} + \frac{2}{(s-3)^3} </mrow>
	 
				</md>
				
			</solution>
			<answer>
				<m> \ds F(s) = \frac{2}{(s+2)^2 + 4} + \frac{2}{(s-3)^3} </m>
			</answer>
		</exercise>
	
	</exercisegroup>
	
	<!--========== Exercise Group 5 ==========--> 
	<exercisegroup>
	<title>
	<p>
	
	</p>
	<p/> <!-- added for vertical space -->
	</title>
		<exercise> <!--== Problem 5 ==-->
			<statement>
				<m> \ds q(t) = 8t\cos(6t) + e^{3t}\sin(4t) </m>
			</statement>
			<solution>
				 For this solution, we will need to use property L14 wit <m> \ds f(t) = \cos(6t). </m>  We will need to know the Laplace transform for this function, so let's do that now.
				<md>
					<mrow>  F(s)	 \amp =  \lap\{ f(t) \} </mrow>
					<mrow>   \amp =  \lap\{ \cos(6t) \} </mrow>
					<mrow>   \amp =  \frac{s}{s^2 + 6^2} \mbox{ (by L5)} </mrow>
					<mrow>   \amp =  \frac{s}{s^2 + 36} </mrow>
	 
				</md>
				 Then we have the following.  Note that when we use the quotient rule to take the derivative o <m> \ds F(s) </m> .
				<md>
					<mrow>  Q(s)	 \amp =  \lap\{ q(t) \} </mrow>
					<mrow>   \amp =  \lap\{ 8t\cos(6t) + e^{3t}\sin(4t) \} </mrow>
					<mrow>   \amp =  8\lap\{ t\cos(6t) \} + \lap\{ e^{3t}\sin(4t) \} \mbox{ (by L9)} </mrow>
					<mrow>   \amp =  8\lap\{ t\cos(6t) \} + \frac{4}{(s-3)^2 + 4^2} \mbox{ (by L7)} </mrow>
					<mrow>   \amp =  8\lap\{ t\cos(6t) \} + \frac{4}{(s-3)^2 + 16} </mrow>
					<mrow>   \amp =  8\lap\{ t\cdot f(t) \} + \frac{4}{(s-3)^2 + 16} </mrow>
					<mrow>   \amp =  8\cdot (-1)^1 \cdot \frac{d}{ds}F(s) + \frac{4}{(s-3)^2 + 16} \mbox{ (by L14)} </mrow>
					<mrow>   \amp =  -8 \cdot \frac{d}{ds}\left( \frac{s}{s^2 + 36} \right) + \frac{4}{(s-3)^2 + 16} </mrow>
					<mrow>   \amp =  -8 \cdot  \frac{(s^2 + 36)\cdot 1 - s\cdot (2s + 0)}{(s^2 + 36)^2} + \frac{4}{(s-3)^2 + 16} </mrow>
					<mrow>   \amp =  -8 \cdot  \frac{s^2 + 36 - 2s^2}{(s^2 + 36)^2} + \frac{4}{(s-3)^2 + 16} </mrow>
					<mrow>   \amp =  -\frac{8(36 - s^2)}{(s^2 + 36)^2} + \frac{4}{(s-3)^2 + 16} </mrow>
	 
				</md>
				
			</solution>
			<answer>
				<m> \ds Q(s) = -\frac{8(36 - s^2)}{(s^2 + 36)^2} + \frac{4}{(s-3)^2 + 16} </m>
			</answer>
		</exercise>
	
	</exercisegroup>
	
	<!--========== Exercise Group 6 ==========--> 
	<exercisegroup>
	<title>
	<p>
	
	</p>
	<p/> <!-- added for vertical space -->
	</title>
		<exercise> <!--== Problem 6 ==-->
			<statement>
				<m> \ds p(t) = t^2 \sin(3t) </m>
			</statement>
			<solution>
				 For this solution, we will need to use property L14 wit <m> \ds f(t) = \sin(3t). </m>  We will need to know the Laplace transform for this function, so let's do that now.
				<md>
					<mrow>  F(s)	 \amp =  \lap\{ f(t) \} </mrow>
					<mrow>   \amp =  \lap\{ \sin(3t) \} </mrow>
					<mrow>   \amp =  \frac{3}{s^2 + 3^2} \mbox{ (by L5)} </mrow>
					<mrow>   \amp =  \frac{3}{s^2 + 9}  </mrow>
				</md>
				 In using L14, we will also need the second derivative o <m> \ds F(s), </m> so we work to compute that now.  Note that we will use the chain rule when we take the derivative o <m> \ds (s^2 + 9)^2 </m> .
				<md>
					<mrow>  F'(s)	 \amp =  \frac{d}{ds}\left( \frac{3}{s^2 + 9} \right) </mrow>
					<mrow>   \amp =  \frac{(s^2 + 9) \cdot 0 - 3 \cdot (2s+0)}{(s^2 + 9)^2} </mrow>
					<mrow>   \amp =  \frac{-6s}{(s^2 + 9)^2} </mrow>
					<mrow>  F''(s)	 \amp =  \frac{(s^2 + 9)^2 \cdot (-6) - (-6s) \cdot 2(s^2 + 9)(2s)}{(s^2 + 9)^4} </mrow>
					<mrow>   \amp =  \frac{-6(s^2 + 9)^2 + 24s^2(s^2 +9)}{(s^2 + 9)^4} </mrow>
					<mrow>   \amp =  \frac{6(s^2 + 9)\left[-(s^2 + 9) + 4s^2\right]}{(s^2 + 9)^4} </mrow>
					<mrow>   \amp =  \frac{6\left[-s^2 - 9 + 4s^2\right]}{(s^2 + 9)^3} </mrow>
					<mrow>   \amp =  \frac{6\left[3s^2 - 9\right]}{(s^2 + 9)^3} </mrow>
					<mrow>   \amp =  \frac{18\left[s^2 - 3\right]}{(s^2 + 9)^3}  </mrow>
				</md>
				 Then we have the following.
				<md>
					<mrow>  P(s)	 \amp =  \lap\{ t^2 \sin(3t) \} </mrow>
					<mrow>   \amp =  \lap\{ t^2 f(t) \} </mrow>
					<mrow>   \amp =  (-1)^2 \cdot F''(s) \mbox{ (by L14)} </mrow>
					<mrow>   \amp =  1 \cdot \frac{18\left[s^2 - 3\right]}{(s^2 + 9)^3} </mrow>
					<mrow>   \amp =  \frac{18\left[s^2 - 3\right]}{(s^2 + 9)^3} </mrow>
	 
				</md>
				
			</solution>
			<answer>
				<m> \ds P(s) = \frac{18\left[s^2 - 3\right]}{(s^2 + 9)^3} </m>
			</answer>
		</exercise>
	
	</exercisegroup>
	
	</exercises>

</subsection>