<!-- LICENSING
  This file is part of the textbook "Exploring Differential Equations, An Interactive, Student-Centered Approach" by Geoffrey Cox.
  License: Creative Commons Attribution-ShareAlike 4.0 International (CC BY-SA 4.0)
  You are free to:
    ‚Ä¢ Share ‚Äî copy and redistribute the material in any medium or format.
    ‚Ä¢ Adapt ‚Äî remix, transform, and build upon the material for any purpose, even commercially.
  Under the following terms:
    ‚Ä¢ Attribution ‚Äî You must give appropriate credit, provide a link to the license, and indicate if changes were made.
    ‚Ä¢ ShareAlike ‚Äî If you remix, transform, or build upon the material, you must distribute your contributions under the same license.
  Full license text: https://creativecommons.org/licenses/by-sa/4.0/legalcode
  Recommended attribution: "Exploring Differential Equations" by Geoffrey Cox, licensed CC BY-SA 4.0.
-->
<section label="lt-method-step1">
	<title>Step 1 ‚Äî Into the Laplace Domain</title>

	<introduction>
		<p>
			The first step of the Laplace transform method is to convert a differential equation‚Äîwhere the unknown appears through derivatives‚Äîinto an algebraic equation in the Laplace domain. This transformation makes it easier to isolate the unknown and move toward a solution.
		</p>
	</introduction>

	<subsection label="lt-method-step1-overview">
		<title>Crossing Into the Laplace Domain</title>

		<p>
			In terms of the roadmap, we can visualize this first step as follows:
		</p>

		<assemblage xml:id="lt-roadmap-step-1"><title>Step <e component="emoji">1Ô∏è‚É£</e>: Into the Laplace Domain (Forward Transform)</title>
			<p>
				<sidebyside widths="32% 18% 42%" valign="middle">
					<p>
						<me>\ul{\qquad\textbf{Original Domain}\qquad}</me>
					</p>
					<p/>
					<p>
						<me>\DLBa\textbf{Laplace Domain}</me>
					</p>
				</sidebyside>
				<sidebyside widths="32% 18% 42%" valign="top">
					<p>
						<md>
							<mrow>\os{\vphantom{m}}{y'' - 9y = 10e^{2t}}</mrow>
							<mrow>y(0) = 1,\quad y'(0) = -7</mrow>
							<mrow>\os{\large <e component="emoji">üî∫</e> <e component="emoji">üî∫</e> <e component="emoji">üî∫</e> <e component="emoji">üî∫</e> <e component="emoji">üî∫</e>}{\text{Differential Equation}}</mrow>
						</md>
					</p>
					<p>
						<md>
							<mrow>\underrightarrow{\text{<e component="emoji">1Ô∏è‚É£</e> Forward}}</mrow>
							<mrow>\text{Apply}\ \laplacesym</mrow>
							<mrow/>
						</md>
					</p>
					<p>
						<assemblage>
							<p>
								<md>
									<mrow>\DLBa s^2Y - 9Y - s + 7 = \frac{10}{s - 2}</mrow>
									<mrow>\DLBa\dotsm</mrow>
								</md>
							</p>
						</assemblage>
					</p>
				</sidebyside>
			</p>
		</assemblage>

	<p>
		Simply put, forward transforming a differential equation into the Laplace domain means applying the Laplace transform to both sides of the equation. The result is an algebraic equation where the derivatives have been converted into powers of <m>s</m> and the new unknown is <m>Y</m>.
	</p>
	</subsection>

	<subsection xml:id="lt-forward-mechanics">
		<title>Basic Mechanics of the Forward Transform</title>

		<p>
				Symbolically, applying the forward Laplace transform to the differential equation
	<me>
		y'' - 9y = 10e^{2t}, \quad y(0) = 1,\quad y'(0) = -7
	</me>
	amounts to applying it to both sides of the equation as follows:
	<me>
		\lap{y'' - 9y} = \lap{10e^{2t}}
	</me>.
		</p>

		<p>
			Using the <xref ref="lt-P1" text="custom">linearity property</xref>, we can see that the transform applies to each term:
			<me>\lap{y''} - 9\lap{y} = 10\lap{e^{2t}}.</me>
		</p>

		<p>
			Letting <m>Y(s) = \lap{y(t)}</m> and applying rule <xref ref="lt-R2" text="custom">R<m>_2</m></xref> for <m>\lap{y''}</m> and common transform <xref ref="lt-L2" text="custom">L<m>_2</m></xref>, we get:
			<me>s^2 Y(s) - s y(0) - y'(0) - 9 Y(s) = 10 \left(\frac{1}{s-2}\right).</me>
		</p>
		
		<p>
			This is where the initial conditions come into play. Substituting the initial conditions and simplifying gives the desired Laplace domain equation:
			<me>s^2Y - 9Y - s + 7 = \frac{10}{s - 2}.</me>
		</p>

		<p>
			Our new unknown is <m>Y</m>, and since the derivatives have been eliminated, we can use algebra to solve for it. In fact, the solution to our differential equation is actually hiding inside <m>Y</m>. So, by solving for <m>Y</m> you are also solving for <m>y(t)</m> at the same time!
		</p>

		<p>
			Let's practice this with one more example.
		</p>
		
		<example xml:id="lt-forward-lt-example">
			<title>Forward Transforming Equations</title>
			<statement>
				<p>
					Forward transform the following equations into the Laplace domain:
					<me>
						\begin{array}{l}
							y'' - 4y' + 6y = t^2,\\
							y(0) = 2, \quad y'(0) = 0
						\end{array}
					</me>
				</p>
			</statement>

			<solution>
				<p>
					First applying the Laplace transform to both sides:
					<me>
						\lap{y'' - 4y' + 6y} = \lap{t^2}
					</me>.
				</p>

				<p>
					Now, use the <xref ref="lt-P1" text="custom">linearity property</xref>:
					<me>
						\lap{y''} - 4\lap{y'} + 6\lap{y} = \lap{t^2}
					</me>.
				</p>
				
				<p>
					Let <m>Y = \lap{y}</m>, and apply rules <xref ref="lt-R2" text="custom">R<m>_2</m> &amp; R<m>_1</m></xref> and common transform <xref ref="lt-L3" text="custom">L<m>_3</m></xref>
					<me>
						\left[s^2 Y(s) - s y(0) - y'(0)\right] -4\left[sY(s) - y(0)\right] + 6 Y(s) = \frac{1}{s^3}
					</me>.
				</p>

				<p>
					Finally, plug in the initial conditions, <m>y(0) = 2,\ y'(0) = 0</m> and clean up:
					<me>
						s^2 Y(s) - 4sY(s) + 6Y(s) - 2s + 8 = \frac{2}{s^3}
					</me>.
				</p>
			</solution>
		</example>

		<exercise label="lt-method-step1-chkpt-1">
			<title><e component="emoji">üìñ‚ùì</e> Select the Forward Transform</title>
			<statement>
				<p>
					Which of the following represents the correct Laplace transform of the equation <me>y'' - 4y' + 6y = t^2, \quad y(0) = 2, \quad y'(0) = -1</me>?
				</p>
			</statement>
			<choices randomize="yes">
				<choice correct="yes">
					<statement><m>\ds s^2Y - 4sY + 6Y - 2s + 9 = \frac{2}{s^3}</m></statement>
					<feedback>Correct: apply the transform rules for derivatives, substitute <m>y(0)=2</m>, <m>y'(0)=-1</m>, and use <m>\lap{t^2}=\dfrac{2}{s^3}</m>.</feedback>
				</choice>
				<choice>
					<statement><m>\ds s^2Y - 4sY + 6Y - 2s = \frac{2}{s^3}</m></statement>
					<feedback>This answer is missing the constant term that comes from applying the initial conditions.</feedback>
				</choice>
				<choice>
					<statement><m>\ds s^2Y - 4sY + 6Y - 2s + 7 = \frac{2}{s^3}</m></statement>
					<feedback>Check the sign of the <m>y'(0)</m> term in <m>\lap{y''}</m>; with <m>y'(0)=-1</m> it contributes <m>+1</m>, not <m>-1</m>.</feedback>
				</choice>
				<choice>
					<statement><m>\ds s^2Y - 4sY + 6Y + 9 = \frac{2}{s^3}</m></statement>
					<feedback>This answer is missing the <m>-2s</m> term that comes from the <m>-s y(0)</m> part of <m>\lap{y''}</m>.</feedback>
				</choice>
			</choices>
		</exercise>

		<p>
				Now that you've seen the mechanical steps involved with applying the Laplace transform to a differential equation, it is important to take a moment to see what's happening behind the scenes during this process. 
		</p>
	</subsection>

	<subsection label="lt-forward-intro">
		<title>What is Going on Behind the Scenes?</title>

		<exercise label="lt-method-step1-chkpt-2">
			<title><e component="emoji">üìñ‚ùì</e> Applying the Laplace Transform to an Equation</title>
			<statement>
				<p>
					<em> Fill-in-the-blanks: </em>
				</p>
				<p>
					The process of applying a Laplace transform to a differential equation involves multiplying the equation by <fillin characters="13" /> and <fillin characters="13" /> with respect to <m>t</m>.
				</p>
				<p/>
			</statement>
			<choices randomize="yes">
			<choice>
				<statement><m>e^{-t},</m> integrating</statement>
				<feedback>
				<p>
					No, this misses the <m>s</m> parameter in the exponential. It should be <m>e^{-st}</m>.
				</p>
				</feedback>
			</choice>
			<choice correct="yes">
				<statement><m>e^{-st},</m> integrating</statement>
				<feedback>
				<p>
					Correct! The Laplace transform involves multiplying the original function by <m>e^{-st}</m> and then integrating with respect to <m>t</m>.
				</p>
				</feedback>
			</choice>
			<choice>
				<statement><m>e^{st},</m> integrating</statement>
				<feedback>
				<p>
					No, the exponent should have a negative sign: <m>e^{-st}</m>.
				</p>
				</feedback>
			</choice>
			<choice>
				<statement><m>e^{-st},</m> differentiating</statement>
				<feedback>
				<p>
					No, the Laplace transform requires integration, not differentiation.
				</p>
				</feedback>
			</choice>
			<choice>
				<statement><m>s,</m> differentiating</statement>
				<feedback>
				<p>
					No, the transform uses <m>e^{-st}</m> and integration, not the variable <m>s</m> directly or differentiation.
				</p>
				</feedback>
			</choice>
			</choices>
		</exercise>

		<p>
      Since the Laplace transform only applies to functions, applying a <q>forward transform to a differential equation</q> really means we are taking the Laplace transform of both sides of that equation. So applying a forward transformation to the initial-value problem
			<me>y' - 9y = 10 e^{7t}, \quad y(0) = 1</me>
			implies that we multiply both sides of the equation by <m>e^{-st}</m> and integrate from <m>0</m> to <m>\infty</m>:
		</p>

		<sbsgroup widths="35% 65%" valign="middle">
			<sidebyside>
				<p><me>\ul{\qquad\text{Symbolically}\qquad}</me></p>
				<p><me>\ul{\qquad\text{Behind the Scenes Math}\qquad}</me></p>
			</sidebyside>
			<sidebyside>
				<p><me>\small\lap{y' - 9y} = \lap{10 e^{7t}}</me></p>
				<p>
					<md>
						<mrow>\small\left(y' - 9y\right) e^{-st} \amp = (10 e^{7t}) e^{-st}</mrow>
						<mrow>\small\int_0^{\infty} \left(y' - 9y\right) e^{-st} dt \amp = \int_0^{\infty} (10 e^{7t}) e^{-st} dt</mrow>
					</md>
				</p>
			</sidebyside>
		</sbsgroup>

		<p>
			Next, we use the linearity of the integral:
		</p>

		<sidebyside widths="35% 65%" valign="middle">
			<p><me>\small\lap{y'} - 9\lap{y} = 10\lap{e^{7t}}</me></p>
			<p><me>\small\us{\large I_1}{\ul{\int_0^{\infty} (y') e^{-st} dt}} - 9 \int_0^{\infty} (y) e^{-st} dt = 10 \us{\large I_2}{\ul{\int_0^{\infty} (e^{7t}) e^{-st} dt}}</me></p>
		</sidebyside>

		<p>
			After applying integration by parts to <m>I_1</m>, the derivative is transferred from <m>y(t)</m> to <m>e^{-st}</m>, resulting in a factor of <m>s</m> and an evaluation of <m>y(t)</m> at <m>t=0</m> and <m>t=b</m>:
		</p>

		<sidebyside widths="42% 58%" valign="middle">
			<p>
				<me>\small
					-y(0) + sY(s) - 9 Y(s) = 10 \left(\frac{1}{s-7}\right)
				</me>
			</p>
			<p><me>\leftarrow\ \text{Symbolically}</me></p>
		</sidebyside>

		<sidebyside widths="36% 64%" valign="middle">
			<p><me>\text{Mathematically}\ \rightarrow </me></p>
			<p>
				<md>
					<mrow>\small
						\us{\large\text{as}\ b\ \to\ \infty}{\ul{\cancelto{\large 0}{e^{-sb}y(b)}}}<fn>assuming <m>y(t)</m> grows no faster than the exponential decays.</fn> - y(0) 
						+ s\int_0^{\infty} e^{-st}y\, dt - 9\int_0^{\infty} e^{-st}y\, dt = \frac{10}{s-7}
					</mrow>
				</md>
				
			</p>
		</sidebyside>
		
		<p>
				The details for computing <m>I_2 = \lap{e^{7t}}</m> are given <xref ref="common-exp-7t-details" text="custom">here</xref>.
		</p>

		<p>
			Since the two integrals are <m>\lap{y} = Y(s)</m>, the symbolic and mathematical paths come back together as  
			<me>
				sY(s) - 9 Y(s) - y(0) = \frac{10}{s-7}
			</me>.
		</p>

		<p>
			By transforming our equation into this new form, we have momentarily stored <m>y(t)</m> inside the function <m>Y</m>. Therefore, solving for <m>Y</m> indirectly also solves for <m>y(t)</m>.
		</p>

		<assemblage>
			<title>Step 1 ‚Äî Into the Laplace Domain Summary</title>
			<p>
				Apply <m>\laplacesym</m> to each term of the differential equation; derivatives become powers of <m>s</m> and initial conditions drop in as constants, leaving an algebraic equation in <m>Y(s)</m>.
			</p>
		</assemblage>
	</subsection>

</section>
