
<subsection xmlns:xi="http://www.w3.org/2001/XInclude"><title> Summary &amp; Exercises </title>

	<introduction>
		
		<p>
			<assemblage color="green"><title>Summary of the Key Ideas</title>
				<p>
					<term> <em> Method</em> </term>
					<p>
						
					</p>
				</p>
			</assemblage>
		</p>
		
		<assemblage xml:id="lt-table-L1-L8"><title>Common Laplace Transforms</title>
			<p>
				<dl width="narrow">
					<li><title><m>{\LARGE \vphantom{\int}}L_1.</m></title>
						<m>\hspace{-3em}\ds \lap\{ 1 \} = \frac{1}{s}, \quad s &gt;0 </m>
					</li>
					<li><title><m>{\LARGE \vphantom{\int}}L_2.</m></title>
						<m>\hspace{-3em}\ds \lap\{ e^{at} \} = \frac{1}{s - a}, \quad s &gt;a, \quad a \text{ is a constant} </m>
					</li>
					<li><title><m>{\LARGE \vphantom{\int}}L_3.</m></title>
						<m>\hspace{-3em}\ds \lap\{ t^n \} = \frac{n!}{s^{n+1}}, \quad s &gt;0,\ n = 1, 2, 3, \ldots </m>
					</li>
					<li><title><m>{\LARGE \vphantom{\int}}L_4.</m></title>
						<m>\hspace{-3em}\ds \lap\{ \sin(bt) \} = \frac{b}{s^2+b^2}, \quad s &gt;0, \quad b \text{ is constant} </m>
					</li>
					<li><title><m>{\LARGE \vphantom{\int}}L_5.</m></title>
						<m>\hspace{-3em}\ds \lap\{ \cos(bt) \} = \frac{s}{s^2+b^2}, \quad s &gt;0, \quad b \text{ is constant} </m>
					</li>
					<li><title><m>L_6</m></title>
						<m>\lap\{ t^n e^{at} \} = \ds\frac{n!}{(s-a)^{n+1}}, \quad s &gt;a </m>
					</li>
					<li><title><m>{\LARGE \vphantom{\int}}L_7.</m></title>
						<m>\hspace{-3em}\ds \lap\{ e^{at}\cos(bt) \} = \frac{s-a}{(s-a)^2+b^2}, \quad s &gt;a, \quad a, b \text{ are constants} </m>
					</li>
					<li><title><m>{\LARGE \vphantom{\int}}L_8.</m></title>
						<m>\hspace{-3em}\ds \lap\{ e^{at}\sin(bt) \} = \frac{b}{(s-a)^2+b^2}, \quad s &gt;a, \quad a, b \text{ are constants} </m>
					</li>
				</dl>
			</p>
		</assemblage>

		<assemblage xml:id="lt-properties-P1-P6"><title>Laplace Transform Properties</title>
			<p>
				Let <m>F(s) = \lap\{f(t)\}</m> and <m>G(s) = \lap\{g(t)\}</m>.
			</p>
	
			<p>
				<dl width="narrow">
					<li><title><m>P_1.</m></title>
						<m>\hspace{-3em}\ds \lap\{ a f(t) \pm b g(t) \} = a F(s) \pm b G(s), \quad a, b </m> are constants
					</li>
					<li><title><m>P_2.</m></title>
						<m>\hspace{-3em}\ds \lap\{ e^{at} f(t) \} = F(s-a), \quad a </m> is a constant
					</li>
					<li><title><m>P_3.</m></title>
						<m>\hspace{-3em}\ds \lap\{ f'(t) \} = sF(s) - f(0) </m>
					</li>
					<li><title><m>P_4.</m></title>
						<m>\hspace{-3em}\ds \lap\{ f''(t) \} = s^2F(s) - sf(0) - f'(0) </m>
					</li>
					<li><title><m>P_5.</m></title>
						<m>\hspace{-3em}\ds \lap\{ f'''(t) \} = s^3F(s) - s^2f(0) - sf'(0) - f''(0) </m>
					</li>
					<li><title><m>{\LARGE \vphantom{\int}}P_6.</m></title>
						<m>\hspace{-3em}\ds \lap\{ t^n f(t) \} = (-1)^n \frac{d^{(n)}}{ds^{(n)}}F(s), \quad n = 1, 2, 3, \ldots </m>
					</li>
				</dl>
			</p>
		</assemblage>

	</introduction>

	<exercises>

		<exercisegroup cols="1"><title>Forward Transform</title>

			<introduction>
				<p>
					Compute the forward Laplace Transforms using the <xref ref="lt-table-L1-L8" text="custom">common transform table</xref> and <xref ref="lt-properties-P1-P6" text="custom">properties</xref>.
				</p>
			</introduction>
			
			<exercise>
				
				<statement>
					<m> \ds \lap\{t^3 e^{-9t}\} </m>
				</statement>

				<answer>
					<md>
						<mrow>  
							\lap\{ t^3 e^{-9t} \}	
								=\amp \frac{3!}{\big(s-(-9)\big)^{3+1}}	\quad <xref ref="L6" text="title"/>\ (a=2, n=4)
						</mrow>
						<mrow>	=\amp \frac{6}{(s+9)^4}		</mrow>
					</md>
				</answer>

			</exercise>

			<exercise>

				<statement>
					<m>\ds \lap\{e^{2t} - t^3 - \sin (5t)\}</m>
				</statement>
				<solution>
					
					<md>
						<mrow>
							\lap\{e^{2t} - t^3 - \sin (5t)\}
								=\amp\ \lap\{ e^{2t} \} - \lap\{ t^3 \} - \lap\{ \sin(5t) \} \quad <xref ref="P1" text="title"/>
						</mrow>
						<mrow>
								=\amp\  \frac{1}{s-2} - \frac{3!}{s^{3+1}} - \frac{5}{s^2 + 5^2} \quad 
									<xref ref="L2" text="title"/>, <xref ref="L3" text="title"/>, <xref ref="L4" text="title"/>
						</mrow>
						<mrow>   
								=\amp\  \frac{1}{s-2} - \frac{6}{s^4} - \frac{5}{s^2 + 25} 
						</mrow>
					</md>
					
				</solution>

			</exercise>

			<exercise>

				<statement>
					<m> \ds \lap\{e^{-2t}\sin(2t) + t^2 e^{3t}\} </m>
				</statement>
				<solution>
					
					<md>
						<mrow>  F(s)	 \amp =  \lap\{ f(t) \} </mrow>
						<mrow>   \amp =  \lap\{ e^{-2t}\sin(2t) + t^2 e^{3t} \} </mrow>
						<mrow>   \amp =  \lap\{ e^{-2t}\sin(2t)\} + \lap\{t^2 e^{3t} \} \mbox{ (by L9)} </mrow>
						<mrow>   \amp =  \frac{2}{\big(s- (-2) \big)^2 + 2^2} + \frac{2!}{(s-3)^{2+1}} \mbox{ (by L7 and L6)} </mrow>
						<mrow>   \amp =  \frac{2}{(s+2)^2 + 4} + \frac{2}{(s-3)^3} </mrow>
		
					</md>
					
				</solution>
				<answer>
					<m>\ds L_7\ (a=2), L_9\ (n=2, a=3)</m>
					<md>
						<mrow> \lap\{e^{-2t}\sin(2t) + t^2 e^{3t}\}	=\amp \frac{2}{(s+2)^2 + 4} + \frac{2}{(s-3)^3}	</mrow>
						<mrow> 											=\amp \frac{2}{(s+2)^2 + 4} + \frac{2}{(s-3)^3}	</mrow>
					</md>
				</answer>

			</exercise>

			<exercise>

				<statement>
					<m>\ds \lap\{8t\cos(6t) + e^{3t}\sin(4t)\}</m>
				</statement>
				<solution>
					For this solution, we will need to use property L14 wit <m> \ds f(t) = \cos(6t). </m>  We will need to know the Laplace transform for this function, so let's do that now.
					<md>
						<mrow>  F(s)	 \amp =  \lap\{ f(t) \} </mrow>
						<mrow>   \amp =  \lap\{ \cos(6t) \} </mrow>
						<mrow>   \amp =  \frac{s}{s^2 + 6^2} \mbox{ (by L5)} </mrow>
						<mrow>   \amp =  \frac{s}{s^2 + 36} </mrow>
		
					</md>
					Then we have the following.  Note that when we use the quotient rule to take the derivative o <m> \ds F(s) </m> .
					<md>
						<mrow>  Q(s)	 \amp =  \lap\{ q(t) \} </mrow>
						<mrow>   \amp =  \lap\{ 8t\cos(6t) + e^{3t}\sin(4t) \} </mrow>
						<mrow>   \amp =  8\lap\{ t\cos(6t) \} + \lap\{ e^{3t}\sin(4t) \} \mbox{ (by L9)} </mrow>
						<mrow>   \amp =  8\lap\{ t\cos(6t) \} + \frac{4}{(s-3)^2 + 4^2} \mbox{ (by L7)} </mrow>
						<mrow>   \amp =  8\lap\{ t\cos(6t) \} + \frac{4}{(s-3)^2 + 16} </mrow>
						<mrow>   \amp =  8\lap\{ t\cdot f(t) \} + \frac{4}{(s-3)^2 + 16} </mrow>
						<mrow>   \amp =  8\cdot (-1)^1 \cdot \frac{d}{ds}F(s) + \frac{4}{(s-3)^2 + 16} \mbox{ (by L14)} </mrow>
						<mrow>   \amp =  -8 \cdot \frac{d}{ds}\left( \frac{s}{s^2 + 36} \right) + \frac{4}{(s-3)^2 + 16} </mrow>
						<mrow>   \amp =  -8 \cdot  \frac{(s^2 + 36)\cdot 1 - s\cdot (2s + 0)}{(s^2 + 36)^2} + \frac{4}{(s-3)^2 + 16} </mrow>
						<mrow>   \amp =  -8 \cdot  \frac{s^2 + 36 - 2s^2}{(s^2 + 36)^2} + \frac{4}{(s-3)^2 + 16} </mrow>
						<mrow>   \amp =  -\frac{8(36 - s^2)}{(s^2 + 36)^2} + \frac{4}{(s-3)^2 + 16} </mrow>
		
					</md>
					
				</solution>
				<answer>
					<m>\ds L_3\ (n=9)</m>
					<me>\lap\{t^9\} = \frac{9!}{s^{9+1}} = \frac{9!}{s^{10}} </me>
				</answer>

			</exercise>

			<exercise>
				
				<statement>
					<m> \ds \lap\{t^2 \sin(3t)\} </m>
				</statement>
				<solution>
					For this solution, we will need to use property L14 wit <m> \ds f(t) = \sin(3t). </m>  We will need to know the Laplace transform for this function, so let's do that now.
					<md>
						<mrow>  F(s)	 \amp =  \lap\{ f(t) \} </mrow>
						<mrow>   \amp =  \lap\{ \sin(3t) \} </mrow>
						<mrow>   \amp =  \frac{3}{s^2 + 3^2} \mbox{ (by L5)} </mrow>
						<mrow>   \amp =  \frac{3}{s^2 + 9}  </mrow>
					</md>
					In using L14, we will also need the second derivative o <m> \ds F(s), </m> so we work to compute that now.  Note that we will use the chain rule when we take the derivative o <m> \ds (s^2 + 9)^2 </m> .
					<md>
						<mrow>  F'(s)	 \amp =  \frac{d}{ds}\left( \frac{3}{s^2 + 9} \right) </mrow>
						<mrow>   \amp =  \frac{(s^2 + 9) \cdot 0 - 3 \cdot (2s+0)}{(s^2 + 9)^2} </mrow>
						<mrow>   \amp =  \frac{-6s}{(s^2 + 9)^2} </mrow>
						<mrow>  F''(s)	 \amp =  \frac{(s^2 + 9)^2 \cdot (-6) - (-6s) \cdot 2(s^2 + 9)(2s)}{(s^2 + 9)^4} </mrow>
						<mrow>   \amp =  \frac{-6(s^2 + 9)^2 + 24s^2(s^2 +9)}{(s^2 + 9)^4} </mrow>
						<mrow>   \amp =  \frac{6(s^2 + 9)\left[-(s^2 + 9) + 4s^2\right]}{(s^2 + 9)^4} </mrow>
						<mrow>   \amp =  \frac{6\left[-s^2 - 9 + 4s^2\right]}{(s^2 + 9)^3} </mrow>
						<mrow>   \amp =  \frac{6\left[3s^2 - 9\right]}{(s^2 + 9)^3} </mrow>
						<mrow>   \amp =  \frac{18\left[s^2 - 3\right]}{(s^2 + 9)^3}  </mrow>
					</md>
					Then we have the following.
					<md>
						<mrow>  P(s)	 \amp =  \lap\{ t^2 \sin(3t) \} </mrow>
						<mrow>   \amp =  \lap\{ t^2 f(t) \} </mrow>
						<mrow>   \amp =  (-1)^2 \cdot F''(s) \mbox{ (by L14)} </mrow>
						<mrow>   \amp =  1 \cdot \frac{18\left[s^2 - 3\right]}{(s^2 + 9)^3} </mrow>
						<mrow>   \amp =  \frac{18\left[s^2 - 3\right]}{(s^2 + 9)^3} </mrow>
		
					</md>
				</solution>
				<answer>
					<m> \ds P(s) = \frac{18\left[s^2 - 3\right]}{(s^2 + 9)^3} </m>
				</answer>

			</exercise>
		
		</exercisegroup>

		<exercisegroup><title>Applying the Forward Laplace Transform</title>

			<introduction>
				<p>
					Use the forward Laplace transform to solve the following differential equations.
				</p>
			</introduction>
	
			<exercise>
				<statement>
					Solve the differential equation <m>y'' + 3y' + 2y = 0</m> given the initial conditions <m>y(0) = 2</m> and <m>y'(0) = -1</m>.
				</statement>
				<solution>
					Apply the Laplace transform to both sides of the equation:
					<me>\lap\{y'' + 3y' + 2y\} = \lap\{0\}</me>.
					Using the properties of the Laplace transform for derivatives, we have:
					<me>s^2Y(s) - sy(0) - y'(0) + 3[sY(s) - y(0)] + 2Y(s) = 0</me>.
					Substitute the initial conditions <m>y(0) = 2</m> and <m>y'(0) = -1</m>:
					<me>s^2Y(s) - 2s + 1 + 3sY(s) - 6 + 2Y(s) = 0</me>.
					Combine like terms:
					<me>(s^2 + 3s + 2)Y(s) - 2s - 5 = 0</me>.
					Solve for <m>Y(s)</m>:
					<me>Y(s) = \frac{2s + 5}{s^2 + 3s + 2}</me>.
					Factor the denominator:
					<me>Y(s) = \frac{2s + 5}{(s + 1)(s + 2)}</me>.
					Use partial fraction decomposition to find the inverse Laplace transform:
					<me>Y(s) = \frac{A}{s + 1} + \frac{B}{s + 2}</me>.
					Solve for <m>A</m> and <m>B</m>:
					<me>Y(s) = \frac{1}{s + 1} - \frac{3}{s + 2}</me>.
					Finally, take the inverse Laplace transform to find <m>y(t)</m>:
					<me>y(t) = e^{-t} - 3e^{-2t}</me>.
				</solution>
				<answer>
					<m>y(t) = e^{-t} - 3e^{-2t}</m>
				</answer>
			</exercise>
	
			<exercise>
				<statement>
					Solve the differential equation <m>y' + 4y = 10e^{-2t}</m> with the initial condition <m>y(0) = 3</m>.
				</statement>
				<solution>
					Apply the Laplace transform to both sides:
					<me>\lap\{y' + 4y\} = \lap\{10e^{-2t}\}</me>.
					Use the properties of the Laplace transform:
					<me>sY(s) - y(0) + 4Y(s) = \frac{10}{s + 2}</me>.
					Substitute the initial condition <m>y(0) = 3</m>:
					<me>(s + 4)Y(s) - 3 = \frac{10}{s + 2}</me>.
					Solve for <m>Y(s)</m>:
					<me>Y(s) = \frac{10}{(s + 4)(s + 2)} + \frac{3}{s + 4}</me>.
					Use partial fraction decomposition:
					<me>Y(s) = \frac{A}{s + 4} + \frac{B}{s + 2}</me>.
					Find <m>A</m> and <m>B</m>:
					<me>A = \frac{7}{2}, B = -\frac{5}{2}</me>.
					Inverse Laplace transform gives:
					<me>y(t) = \frac{7}{2}e^{-4t} - \frac{5}{2}e^{-2t}</me>.
				</solution>
				<answer>
					<m>y(t) = \frac{7}{2}e^{-4t} - \frac{5}{2}e^{-2t}</m>
				</answer>
			</exercise>
	
		</exercisegroup>

		<exercisegroup><title>Transformation of Functions</title>
	
			<introduction>
				<p>
					Find the Laplace transforms for the following functions using the Laplace transform properties.
				</p>
			</introduction>
	
			<exercise>
				<statement>
					<m>\ds \lap\{t^3 e^{-2t}\}</m>
				</statement>
				<solution>
					Use the first shifting theorem:
					<me>\lap\{t^3 e^{-2t}\} = \frac{3!}{(s + 2)^{4}}</me>.
				</solution>
				<answer>
					<m>\ds \frac{6}{(s + 2)^4}</m>
				</answer>
			</exercise>
	
			<exercise>
				<statement>
					<m>\ds \lap\{t\sin(3t)\}</m>
				</statement>
				<solution>
					Use the integration by parts method:
					<me>\lap\{t\sin(3t)\} = -\frac{2s}{(s^2 + 9)^2}</me>.
				</solution>
				<answer>
					<m>\ds -\frac{2s}{(s^2 + 9)^2}</m>
				</answer>
			</exercise>
	
			<exercise>
				<statement>
					<m>\ds \lap\{e^{5t}\cos(4t)\}</m>
				</statement>
				<solution>
					Apply the second shifting theorem:
					<me>\lap\{e^{5t}\cos(4t)\} = \frac{s - 5}{(s - 5)^2 + 16}</me>.
				</solution>
				<answer>
					<m>\ds \frac{s - 5}{(s - 5)^2 + 16}</m>
				</answer>
			</exercise>
	
		</exercisegroup>
		
	</exercises>

</subsection>