<introduction>
		
	<p>
		Just a place to put unused content.
	</p>

	<paragraphs><title>Examples</title>
		<example>
	
			<statement>
				<p>
					Verify that <m>y = Ce^{-5x^2} + \frac{3}{5}</m> is a solution to the DE
					<me>\frac{dy}{dx} = \big( 2x \big) \big( 3 - 5y \big)</me>
				</p>
			</statement>
		
			<solution>
				<p>
					Working out the left and right hand sides of this DE, we have:
		
					<sidebyside widths="45% 55%" margins="auto" valign="top" halign="center">
						<p>
							<md>
								<mrow> LHS: </mrow>
								<mrow> \frac{dy}{dx}
										=\amp\ \frac{d}{dx}\left( Ce^{-5x^2} + \frac{3}{5} \right)</mrow>
								<mrow> 	=\amp\ Ce^{-5x^2} \cdot \frac{d}{dx}(-5x^2) + 0</mrow>
								<mrow> 	=\amp\ Ce^{-5x^2} \cdot -10x</mrow>
								<mrow> 	=\amp\ -10Cxe^{-5x^2}</mrow>
							</md>
						</p>
						<p>
							<md>
								<mrow> RHS: </mrow>
								<mrow> 	\big(2x\big)\amp\big(3 - 5y\big)</mrow>
								<mrow> 	=\amp\ 2x \left[3 - 5\left(Ce^{-5x^2} + \frac{3}{5}\right) \right]</mrow>
								<mrow> 	=\amp\ 2x \left[ 3 - 5Ce^{-5x^2} - 3 \right]</mrow>
								<mrow> 	=\amp\ 2x \left[-5Ce^{-5x^2}\right]</mrow>
								<mrow> 	=\amp\ -10Cxe^{-5x^2}</mrow>
							</md>
						</p>
					</sidebyside>
				</p>
		
				<p>
					Since <m>LHS = RHS</m>, we have verified that
					<m>y = Ce^{-5x^2} + \frac{3}{5}</m> is a solution to
					<me>\frac{dy}{dx} = \big( 2x \big) \big( 3 - 5y \big)</me>
				</p>
				
			</solution>
		
		</example>
	</paragraphs>
	
	<paragraphs><title>Exercises</title>
		
	</paragraphs>

	<paragraphs><title>Narrative</title>
		
	</paragraphs>


 </introduction>