<reading-questions><title> Check your Understanding </title>
    
    <exercise><title> True/False </title>
        <statement correct="yes">
            <p>
                The differential equation, <m>\displaystyle \frac{dy}{dx} = x + xy^2</m>, is <xref ref="separable" text="custom">separable</xref>.
            </p>
        </statement>
        <feedback>
            <p>
                Factoring out an <m>x</m> allows us to group the terms like so: 
                <me>
                    \frac{dy}{dx} = x + xy^2 = x(1 + y^2) =\underset{f(x)}{\fbox{\(x\)}}\underset{g(y)}{\left(\fbox{\(1 + y^2\)}\right)}.
                </me>
            </p>
        </feedback>
    </exercise>

    <exercise><title> True/False </title>
        <statement correct="yes">
            <p>
                The differential equation, <m>\displaystyle \frac{dP}{dt} = \frac{e^tP^2 - e^t}{tP}</m>, is <xref ref="separable" text="custom">separable</xref>.
            </p>
        </statement>
        <feedback>
            <p>
                We group the terms as shown below. Notice how we separated the product of two fractions <m>\left(\frac{AB}{CD} = \frac{A}{C}\cdot \frac{B}{D}\right)</m>.
                <me>
                    \frac{dP}{dt} = \frac{e^tP^2 - e^t}{tP} = \frac{e^t \cdot (P^2 - 1)}{t \cdot P} = \frac{e^t}{t} \cdot \frac{P^2 - 1}{P} = \underset{f(t)}{\fbox{\(\frac{e^t}{t}\)}}\underset{g(P)}{\left(\fbox{\(\frac{P^2 - 1}{P}\)}\right)}.
                </me>
            </p>
        </feedback>
    </exercise>

    <exercise><title> True/False </title>
        <statement correct="no">
            <p>
                The differential equation, <m>\displaystyle \frac{dP}{dt} = \frac{P^2 - tP}{P}</m>, is <xref ref="separable" text="custom">separable</xref>.
            </p>
        </statement>
        <feedback>
            <p>
                No matter how we rearrange the terms, we cannot separate the <m>t</m>'s and <m>P</m>'s by multiplication. We could factor out a <m>P</m>, but that doesn't help, as you can see here
                <me>
                    \frac{dP}{dt} = \frac{P^2 - tP}{P} = \frac{P(P - t)}{P} = P - t.
                </me>
            </p>
        </feedback>
    </exercise>

    <exercise><title> Show Separable </title>
        <introduction>
            <p>
                Write the differential equation in <xref ref="separable-form" text="custom">separable form</xref> by identifying <m>f(x)</m> and <m>g(y)</m>.
                <me> \frac{dy}{dx} = x + xy^2 </me>
            </p>
        </introduction>
            
        <webwork> 

            <pg-code>
                Context()->variables->add(y => 'Real');
                $fx = Formula("x");
                $gy = Formula("1 + y^2");
            </pg-code>

            <statement>

                <p>
                    <tabular halign="center">
                    
                        <row>
                            <cell><m>\displaystyle \frac{dy}{dx} = \Big( </m></cell>
                            <cell><var name="$fx" width="10" /></cell>
                            <cell><m>\Big) \cdot \Big( </m></cell>
                            <cell><var name="$gy" width="10" /></cell>
                            <cell><m>\Big)</m></cell>
                        </row>
                        <row>
                            <cell/>
                            <cell><m>f(x)</m></cell>
                            <cell/>
                            <cell><m>g(y)</m></cell>
                            <cell/>
                        </row>

                      </tabular>
                
                </p>

            </statement>

        </webwork>
    </exercise>

    <exercise><title> True/False </title>
        <statement correct="no">
        <p>
            The differential equation, <m>\displaystyle \frac{dy}{dx} - x(y^2 + y) = 0</m>, is in <xref ref="separable-form" text="custom">separable form</xref>.
        </p>
        </statement>
        <feedback>
            <p>
                This equation is not currently in <xref ref="separable-form" text="custom">separable form</xref>. However, it can be placed in separable form by moving the <m>x(y^2 + y)</m> term to the right-side of the equation.
            </p>
        </feedback>
    </exercise>
            
    <exercise><title> Fill-In </title>
        <introduction>
                Use algebra to show the differential equation is separable. Give the <m>x</m> terms in the left blank and the <m>y</m> terms in the right blank.
                <me> \frac{dy}{dx} - y\cos(x) = y.</me>
        </introduction>
            
        <webwork xml:id="ww_3">
            <description>
                Show that the DE is separable by typing in the separable form.
            </description>
    
            <pg-code>
                Context()->variables->add(y => 'Real');
                $f_x = Formula("1 + cos(x)");
                $g_y = Formula("y");
            </pg-code>
    
            <statement>
                <p>
                    <tabular halign="center">
                        <col width="10%"/>

                        <row><cell/> 
                            <cell><m>f(x)</m></cell><cell/> 
                            <cell><m>g(y)</m></cell><cell/>
                        </row>

                        <row>
                            <cell>
                                <m>\displaystyle \frac{dy}{dx} = \Large{(}</m>
                            </cell>
                            <cell>
                                <var name="$f_x" width="10" />
                            </cell>
                            <cell><m>\Large{)}\cdot\Large{(}</m></cell>
                            <cell>
                                <var name="$g_y" width="10" />
                            </cell>
                            <cell><m>\Large{)}</m></cell>
                        </row>
                    </tabular>
                </p>
            </statement>
    
            <solution>
                Move the <m> y\cos x </m> term to the right and factor out <m>y</m>.
                <md>
                <mrow> \frac{dy}{dx} - y\cos(x) = y \amp \implies \frac{dy}{dx} = y + y\cos(x) </mrow>
                <mrow>                              \amp \implies \frac{dy}{dx} = (1 + \cos(x))y </mrow>
                </md>
            </solution>
        </webwork>
    </exercise>

</reading-questions>