<subsection xmlns:xi="http://www.w3.org/2001/XInclude"><title> Verifying Solutions </title>

	<p>
        In the previous section, we discussed what it means for a function to be a solution to a differential equation. Now, we turn our attention to how we can verify that a proposed function is indeed a solution.
    </p>

    <p>
        The process of verifying a solution is straightforward: you substitute the proposed function into the differential equation and check whether the equation holds true. This simple test helps ensure that the function satisfies the relationship defined by the differential equation.

		<note xml:id="move-terms-when-verifying"><title>Beginner Tip: Move all terms to One Side</title>
			Remember, the following differential equations are identical:
			<me>
				y^\prime = 3y \quad \text{and} \quad y^\prime - 3y = 0
			</me>.
			Meaning that you are free to use either form when verifying solutions. For beginners, it is often easier to verify solutions using the second form, as you just have to show the left-side of equation simplifies to zero, giving you <m>0=0</m>.
		</note>
		Let's look at a few examples.
	</p>

	<example>
		<m>\quad</m>Verify that <m>\ y= 2x^2\ </m> is a solution to <m>\ xy' - 2x^2 = y</m>.

		<solution>

			<p>
				Let's begin by moving all terms to the left-side of the equation.
				<me>xy' - 2x^2 - y = 0</me>
			</p>

			<p>
				To reduce errors and break the problem into more manageable steps, we will compute and simplify the derivatives appearing in the equation.
				<me>
					y	= 2x^2,	\quad	y' = 4x
				</me>
			</p>

			<p>
				Finally, we substitute in <m>y</m> and <m>y'</m> and simplify.
				<md>
					<mrow> 									xy' - 2x^2 - y	=\amp\ 0									</mrow>
					<mrow> x\left(4x\right) - 2x^2 - \left( 2x^2 \right)	=\amp\ 0 									</mrow>
					<mrow> 								4x^2 - 2x^2 - 2x^2	=\amp\ 0									</mrow>
					<mrow> 												0	=\amp\ 0	\quad \leftarrow \text{true}	</mrow>
				</md>
				Therefore, <m>y= 2x^2</m> is a solution to <m>xy' - 2x^2 = y.</m>
			</p>

		</solution>

	</example>
	
	<example>
		<m>\quad</m>Verify that <m>\ P = \sin t\ </m> is a solution to <m>\ 2P'' + P = \sin t</m>.

		<solution>

			<p>
				As before, we compute <m>P''</m> since it appears in the equation and move all terms to the left-side.
				<me>	
					P = \sin t, \quad P' = \cos t, \quad P'' = -\sin t
				</me>
			</p>

			<p>
				Plug <m>P</m> and <m>P''</m> in and simplify.
				<md>
					<mrow> 							2P'' + P - \sin t	=\amp\ 0									</mrow>
					<mrow> 2\left( -\sin t \right) + \sin t - \sin t	=\amp\ 0									</mrow>
					<mrow> -2\sin t + \cancel{\sin t} - \cancel{\sin t}	=\amp\ 0									</mrow>
					<mrow> 									-2\sin t	=\amp\ 0\quad \leftarrow \text{false}	</mrow>
				</md>
				Therefore, <m>P = \sin t</m> is <term> not a solution </term> to <m>2P'' + P = \sin t.</m>
			</p>

		</solution>

	</example>

	<example xml:id="de-two-solutions">
		<m>\quad</m>Verify that both <m>y= 2e^{-3t}</m> and <m>y= e^{4t}</m> are solutions to 
		<me>\quad y'' - y' - 12y = 0</me>.

		<solution><title><m>\quad y= 2e^{-3t}</m></title>
			<p>
				Find <m>y'</m> and <m>y''</m> since they appear in the equation.
				<md>
					<mrow>	y	=\amp\  2e^{-3t}								</mrow>
					<mrow>	y' 	=\amp\  2e^{-3t}\left(-3\right)	=	-6e^{-3t}	</mrow>
					<mrow>	y'' =\amp\ -6e^{-3t}\left(-3\right)	=	18e^{-3t}	</mrow>
				</md>
			</p>

			<p>
				Plug <m>y, y',</m> and <m>y''</m> into the DE and simplify.
				<md>
					<mrow> 													y'' - y' - 12y	=\amp\ 0									</mrow>
					<mrow> 18e^{-3t} - \left( -6e^{-3t} \right) - 12\left( 2e^{-3t} \right)	=\amp\ 0									</mrow>
					<mrow> 								18e^{-3t} + 6e^{-3t} - 24e^{-3t}	=\amp\ 0									</mrow>
					<mrow> 																0	=\amp\ 0	\quad \leftarrow \text{true}	</mrow>
				</md>
				Therefore, <m>y= 2e^{-3t}</m> is a solution to <m>y'' - y' - 12y = 0.</m>
			</p>

		</solution>

		<solution><title><m>\quad y= e^{4t}</m></title>
			<p>
				Find <m>y'</m> and <m>y''</m> since they appear in the DE.
				<md>
					<mrow>	y	=\amp\  e^{4t}								</mrow>
					<mrow>	y' 	=\amp\  e^{4t}\left(4\right)	=	4e^{4t}	</mrow>
					<mrow>	y'' =\amp\ 4e^{4t}\left(4\right)	=	16e^{4t}</mrow>
				</md>
			</p>

			<p>
				Plug <m>y, y',</m> and <m>y''</m> into the DE and simplify.
				<md>
					<mrow> 								y'' - y' - 12y	=\amp\ 0									</mrow>
					<mrow> 16e^{4t} - 4e^{4t} - 12\left( e^{4t} \right)	=\amp\ 0									</mrow>
					<mrow> 				16e^{4t} - 4e^{4t} - 12e^{4t}	=\amp\ 0									</mrow>
					<mrow> 											0	=\amp\ 0	\quad \leftarrow \text{true}	</mrow>
				</md>
				Therefore, <m>y= e^{4t}</m> is a solution to <m>y'' - y' - 12y = 0.</m>
			</p>

		</solution>

	</example>

	<example>
		<m>\quad</m>Verify that <m>\ y = 3\sin(x^2)\ </m> is a solution to 
		<me>y' - xy'' = 12x^2\sin(x^2)</me>.

		<solution>

			<p>
				: <m>\quad y' - xy'' - 12x^2\sin(x^2) = 0</m>
			</p>

			<p>
				. Find <m>y'</m> and <m>y''</m> since they appear in the DE.
				<md>
					<mrow>	y	=\amp\  3\sin(x^2)									</mrow>
					<mrow>	y' 	=\amp\  3\cos(x^2) \cdot 2x	=	6x\cos(x^2)	</mrow>
					<mrow>	y'' =\amp\ 6\cos(x^2) - 12x\sin(x^2)	=	6\cos(x^2) - 12x\sin(x^2)	</mrow>
				</md>
			</p>

			<p>
				Plug <m>y, y',</m> and <m>y''</m> into the DE and simplify.
				<md>
					<mrow> 												
						y' - xy'' - 12x^2\sin(x^2) 	
							=\amp\ 0	
					</mrow>
					<mrow> 
						6x\cos(x^2) - x\left( 6\cos(x^2) - 12x\sin(x^2) \right) - 12x^2\sin(x^2)
							=\amp\ 0																
					</mrow>
					<mrow> 
						\cancel{6x\cos(x^2)} - \cancel{6x\cos(x^2)} - \cancel{12x^2\sin(x^2)} - \cancel{12x^2\sin(x^2)}	
							=\amp\ 0
						</mrow>
					<mrow> 
						0	=\amp\ 0
					</mrow>
				</md>
				Therefore, <m>y= 3\sin(x^2)</m> is a solution to <m>y' - 12x^2\sin(x^2) = xy''.</m>
			</p>

		</solution>

	</example>

	<p>
        As you work through more complex differential equations, this verification process becomes a valuable tool. It allows you to confirm whether a function is a valid solution before proceeding with further analysis or applications.
    </p>

    <p>
        In the next section, we'll explore different techniques for finding solutions to differential equations, but always rememberâ€”verification is key!
    </p>

	<example xml:id="two-constant-solution-verification"><title> <em>Solution Verification with Two Constants</em> </title>
		<p>
			Verify that <m>y = \frac{1}{2}x^2 + c_1 x + c_2</m> is a solution to <m>\quad y'' = 1</m>.
		</p>
	
		<solution>

			<p>
				Move terms to left: <m>\quad y'' - 1 = 0</m>
			</p>
	
			<p>
				Find <m>y''</m> since it appears in the DE.
				<md>
					<mrow>	y	=\amp\  \frac{1}{2}x^2 + c_1 x + c_2									</mrow>
					<mrow>	y' 	=\amp\  x + c_1													</mrow>
					<mrow>	y'' =\amp\  1														</mrow>
				</md>
			</p>
			<p>
				Plug <m>y''</m> into the DE and simplify.
				<md>
					<mrow> 	y'' - 1	=\amp\ 0	</mrow>
					<mrow> 	1 - 1	=\amp\ 0	</mrow>
					<mrow> 		0	=\amp\ 0	</mrow>
				</md>
				Therefore, <m>y = \frac{1}{2}x^2 + c_1 x + c_2</m> is a solution to <m>y'' = 1</m>. 
				<fn>
					In fact, it is the general solution, but we don't show that here. 
				</fn>
			</p>
	
		</solution>
	
	</example>

	<example>
	
		<p>
		Solve <me> y'' - y' - 12y = 0, \quad y(0) = 4, \quad y'(0) = -2. </me>
		</p>
	
		<solution>
	
		<p>
			The general solution to this DE was already found  to be
			<me>y = c_1e^{-3t} + c_2e^{4t}</me>.
			Notice that two initial conditions are provided in this example. This extra piece of information is needed since our general solution contains two constants.
		</p>
	
		<p>
			Since one initial condition involves the derivative, we will need to compute this before applying this condition.
			<me>y' = -3c_1e^{-3t} + 4c_2e^{4t}.</me>
		</p>
	
		<p>
			Now let's apply the initial conditions:
			<md>
			<mrow>y(0)	=\amp\ 4		\amp\Rightarrow \hspace{0.2cm} 	4
				=\amp\ c_1e^{-3\cdot 0} + c_2e^{4\cdot 0}</mrow>
			<mrow>			\amp	\amp	4
				=\amp\ c_1 + c_2		</mrow>
			<mrow>			\amp	\amp	\amp	</mrow>
			<mrow>y'(0)	=\amp\ -5	\amp\Rightarrow \hspace{0.2cm} 	-5
				=\amp\ -3c_1e^{-3\cdot} + 4c_2e^{4\cdot}	</mrow>
			<mrow>			\amp	\amp	-5	=\amp\ -3c_1 + 4c_2	</mrow>
			</md>
		</p>
	
		<p>
			We now have two equations and two unknowns,
			<md>
			<mrow>	 c_1 +  c_2	=\amp\ 	4 	</mrow>
			<mrow> -3c_1 + 4c_2	=\amp\ -5 	</mrow>
			</md>
			There are multiple ways to solve this system of equations, and the reader is encouraged to verify that	<m>c_1 = 3</m> and <m>c_2 = 1</m>. Here is one
	
			<solution>
	
			We will solve for <m>c_2</m> in the first equation and then
			substitute into the second.
			<md>
				<mrow>4					=\amp\ c_1 + c_2										</mrow>
				<mrow>\Rightarrow c_2	=\amp\ 4 - c_1								</mrow>
				<mrow>					\amp															</mrow>
				<mrow>-5				=\amp\ -3c_1 + 4c_2								</mrow>
				<mrow>\Rightarrow -5	=\amp\ -3c_1 + 4(4 - c_1)		</mrow>
				<mrow>-5				=\amp\ -3c_1 + 16 - 4c_1						</mrow>
				<mrow>-21				=\amp\ -7c_1												</mrow>
				<mrow>3					=\amp\ c_1													</mrow>
				<mrow>					\amp															</mrow>
				<mrow>c_2				=\amp\ 4 - c_1											</mrow>
				<mrow>					=\amp\ 4 - 3												</mrow>
				<mrow>					=\amp\ 1														</mrow>
			</md>
	
			</solution>
	
		</p>
	
		<p>
			Thus, the solution we that satisfies the DE and both of the provided initial conditions is	<me> y = 3e^{-3t} + e^{4t}. </me>
		</p>
	
		</solution>
	
	</example>

	<note><title> <em>Don't assume a function that satisfies a DE is a general solution!</em> </title>
		<p>
			A function that contains constants and satisfies a differential equation <em>does not mean it is the general solution</em> since it could be missing a term. For example, you could easily show that <m>y = \frac{1}{2}x^2 + c_1 x</m> is also a solution to 
			<me>\quad y'' = 1</me>, 
			but you already know from <xref ref="two-constant-solution-verification"/> that <m>y = \frac{1}{2}x^2 + c_1 x + c_2</m> is a solution, which is more general than <m>y = \frac{1}{2}x^2 + c_1 x</m>.
		</p>
	</note>
	
	<example>
	
		<p>
			Verify that <m>\ds y = Ce^{x^2} + 3</m>, where <m>C</m> is any constant, is a solution to the DE
			<me>\ds \frac{dy}{dx} = 2xy - 6x.</me>
		</p>
	
		<solution>
	
			<p>
				We'll approach this the same way we approached the algebraic equation in the example above: we will to substitute the function <m>\ds y = Ce^{x^2} + 3</m> in on the left and right hand sides of the equation
		
				<sidebyside widths="45% 55%" margins="auto" valign="top" halign="center">
					<p>
						<md>
						<mrow> \overset{LHS\vphantom{\Big|}}{\frac{dy}{dx}}
							=\amp\ \frac{d}{dx}\left( Ce^{x^2} + 3 \right)</mrow>
						<mrow> 	=\amp\ C\frac{d}{dx}\left( e^{x^2} \right) + \frac{d}{dx}\left( 3 \right)</mrow>
						<mrow> 	=\amp\ C \cdot e^{x^2} \cdot \frac{d}{dx}\left( x^2 \right) + 0</mrow>
						<mrow> 	=\amp\  C \cdot e^{x^2} \cdot 2x</mrow>
						<mrow> 	=\amp\  2Cxe^{x^2}</mrow>
						</md>
					</p>
					<p>
						<md>
						<mrow> 	\overset{RHS\vphantom{\Big|}}{2xy - 6x}
							=\amp\ 2x \left( Ce^{x^2} + 3 \right) - 6x</mrow>
						<mrow> 	=\amp\ 2Cxe^{x^2} + 6x - 6x</mrow>
						<mrow> 	=\amp\ 2Cxe^{x^2}</mrow>
						</md>
					</p>
				</sidebyside>
		
				Since both the <m>LHS</m> and <m>RHS</m> turn out to be	<m>2Cxe^{x^2}</m>, we have shown that <m>\ds y = Ce^{x^2} + 3</m> satisfies and is, thus, a	solution to	<m>\ds \frac{dy}{dx} = 2xy - 6x.</m>
			</p>
	
		</solution>
	
	</example>

	<note><title>Example Notes</title>
	
		<p>
			Since we used a generic constant <m>C</m>, we have shown that <m>\ds y = Ce^{x^2} + 3</m> is a solution for any value we like for the constant <m>C</m>. In particular,
			<ul>
			<li>for <m>C=-41, \quad y = -41e^{x^2} + 3 \quad</m> is a solution.</li>
			<li>for <m>C=199, \quad y = 199e^{x^2} + 3 \quad</m> is a solution.</li>
			<li>for <m>C=0, \quad y = 3 \quad</m> is a solution.</li>
			</ul>
			Since there is no limit to what <m>C</m> we can choose, this DE must have an infinite number of solutions. In the next section, we will describe this idea further.
		</p>
		
	</note>

	<example>
	
		<p>
			Determine if <m>y = c_1e^{-3t} + c_2e^{4t}</m> is a solution to the DE <m>y'' - y' - 12y = 0</m> where <m>c_1</m> and <m>c_2</m> are constants.
		</p>
	
		<solution>

			<p>
				Find <m>y, y', \text{ and } y''</m>.
				<md>
					<mrow>y		=\amp\ c_1e^{-3t} + c_2e^{4t} \hspace{-0.4cm}
						\amp\Rightarrow\hspace{0.1cm}
						y'	=\amp\ -3c_1e^{-3t} + 4c_2e^{4t} \hspace{-0.4cm}
						\amp\Rightarrow\hspace{0.1cm}
						y''	=\amp\ 9c_1e^{-3t} + 16c_2e^{4t}
					</mrow>
				</md>
			</p>
		
			<p>
				and substitute
				<md>
					<mrow>LHS	=\amp\ y'' - y' - 12y										</mrow>
					<mrow>		=\amp\ \left(9c_1e^{-3t} + 16c_2e^{4t}\right)
						- \left( -3c_1e^{-3t} + 4c_2e^{4t} \right)
						- 12\left( c_1e^{-3t} + c_2e^{4t} \right)				</mrow>
					<mrow>		=\amp\ 9c_1e^{-3t} + 16c_2e^{4t} + 3c_1e^{-3t}
						- 4c_2e^{4t} - 12c_1e^{-3t} - 12c_2e^{4t}			</mrow>
					<mrow>		=\amp\ \left( 9c_1e^{-3t} + 3c_1e^{-3t} - 12c_1e^{-3t} \right)
						+ \left( 16c_2e^{4t} - 4c_2e^{4t} - 12c_2e^{4t} \right)	</mrow>
					<mrow>		\amp = 0													</mrow>
					<mrow>		=\amp\ RHS													</mrow>
				</md>
				Which shows that <m>y = c_1e^{-3t} + c_2e^{4t}</m> is a solution to <m>y'' - y' - 12y = 0.</m>
			</p>
	
		</solution>
	
	</example>
	
	<note><title>Example Notes</title>
	
		<p>
			In this example, we showed that the function <m>y = c_1e^{-3t} + c_2e^{4t}</m> was a solution <m>y'' - y' - 12y = 0</m>.
		</p>
	
		<p>
			Notice that we were able to verify the solution, even though the constants, <m>c_1</m> and <m>c_2</m>, were not known. This suggests that you can substitute any values of <m>c_1</m> and <m>c_2</m> into the solution and it will still be a solution to the DE. <em> Try it! </em>
		</p>
	
		<p>
			Now, since there are infinitely many choices for <m>c_1</m> and <m>c_2</m>,	then, logically, there must be infinitely many solutions to the DE,	<m>y'' - y' - 12y = 0</m>.
		</p>
		
	</note>

	<example>
	
		<statement>
			<p>
				Verify that <m>y = Ce^{-5x^2} + \frac{3}{5}</m> is a solution to the DE
				<me>\frac{dy}{dx} = \big( 2x \big) \big( 3 - 5y \big)</me>
			</p>
		</statement>
	
		<solution>
			<p>
				Working out the left and right hand sides of this DE, we have:
	
				<sidebyside widths="45% 55%" margins="auto" valign="top" halign="center">
					<p>
						<md>
							<mrow> LHS: </mrow>
							<mrow> \frac{dy}{dx}
									=\amp\ \frac{d}{dx}\left( Ce^{-5x^2} + \frac{3}{5} \right)</mrow>
							<mrow> 	=\amp\ Ce^{-5x^2} \cdot \frac{d}{dx}(-5x^2) + 0</mrow>
							<mrow> 	=\amp\ Ce^{-5x^2} \cdot -10x</mrow>
							<mrow> 	=\amp\ -10Cxe^{-5x^2}</mrow>
						</md>
					</p>
					<p>
						<md>
							<mrow> RHS: </mrow>
							<mrow> 	\big(2x\big)\amp\big(3 - 5y\big)</mrow>
							<mrow> 	=\amp\ 2x \left[3 - 5\left(Ce^{-5x^2} + \frac{3}{5}\right) \right]</mrow>
							<mrow> 	=\amp\ 2x \left[ 3 - 5Ce^{-5x^2} - 3 \right]</mrow>
							<mrow> 	=\amp\ 2x \left[-5Ce^{-5x^2}\right]</mrow>
							<mrow> 	=\amp\ -10Cxe^{-5x^2}</mrow>
						</md>
					</p>
				</sidebyside>
			</p>
	
			<p>
				Since <m>LHS = RHS</m>, we have verified that
				<m>y = Ce^{-5x^2} + \frac{3}{5}</m> is a solution to
				<me>\frac{dy}{dx} = \big( 2x \big) \big( 3 - 5y \big)</me>
			</p>
			
		</solution>
	
	</example>

	<xi:include href="./c1-s2-ss2-interactives.ptx" />

	

</subsection>