<section xmlns:xi="http://www.w3.org/2001/XInclude"><title> Matching Forms </title>

	<p>
		When we study Laplace Transforms, we will frequently want to manipulate an algebraic expression to make it match a given form.
	</p>

	<p>
		Suppose we have the expression
		<me> \frac{1}{s^2 + 25}, </me>
		and we think it looks much like the form
		<me> \frac{b}{s^2 + b^2}. </me>
		It's not a perfect match, though. Based on the denominator, we might guess <m>b = 5.</m>  
	</p>

	<p>
		Notice that this would make the denominator a perfect match, 
		<me> \frac{1}{s^2 + 25} = \frac{1}{s^2 + 5^2}. </me>  
		However, the numerator still isn't quite right. It would be correct if we would 
		multiply the numerator by 5. But if we multiply the numerator by 5, we would change 
		the expression. In order to NOT change the expression, we will instead multiply by 
		<m>\frac{5}{5},</m> as follows:
		<md>
			<mrow>	\frac{1}{s^2 + 25}	=\amp\ \frac{1}{s^2 + 5^2}						</mrow>
			<mrow>						=\amp\ \frac{5}{5}\cdot \frac{1}{s^2 + 5^2}		</mrow>
			<mrow>						=\amp\ \frac{1}{5}\cdot \frac{5}{s^2 + 5^2}		</mrow>
			<mrow>						=\amp\ \frac{1}{5}\cdot \frac{b}{s^2 + b^2}, 
															\text{ where } b=5			</mrow>
		</md>
		Notice that when we multiply by <m>\frac{5}{5}</m>, we are just multiplying by one, so we
		don't change the value of the expression.
	</p>
	
	<p>
		In the previous section, we explored how to directly compute backward Laplace transforms when the function of <m>s</m> matches a form in the <xref ref="common-lt-table" text="custom">common forward transform table</xref>. However, in practice, not all <m>s</m>-functions will align perfectly with these forms. In fact, the most challenging part of the Laplace Transform Method lies in preparing the <m>s</m>-function for the backward step. This process involves modifications of the function before matching the known forms in our table. In this discussion, we will cover some of the minor modifications that will need for the Laplace Transform Method.
	</p>

	<p>
		Many of the forms in <xref ref="common-lt-table"/> can be matched just by observing the denominator of the <m>s</m>-function. The following table outlines the connection between the denominator and it associated transform.
		<table halign="center" xml:id="backward-lt-rules-of-thumb"><title> <em>Matching Guide: <m>s</m>-function <m>\rightarrow</m> Inverse Transform</em> </title>
			<tabular halign="center">
				<row bottom="minor">
					<cell right="minor" >denominator			</cell>
					<cell right="minor" ><m>s</m> in numerator? </cell>
					<cell			   >transform			  </cell>
				</row>
				<row bottom="minor">
					<cell right="minor" ><m>s</m>   </cell>
					<cell right="minor" >-		  </cell>
					<cell			   ><m>L_1</m> </cell>
				</row>
				<row bottom="minor">
					<cell right="minor" ><m>s^{\text{power}}</m>	</cell>
					<cell right="minor" >-						  </cell>
					<cell			   ><m>L_3</m>				 </cell>
				</row>
				<row bottom="minor">
					<cell right="minor" ><m>s \pm \text{shift}</m>  </cell>
					<cell right="minor" >-						  </cell>
					<cell			   ><m>L_2</m>				 </cell>
				</row>
				<row bottom="minor">
					<cell right="minor" ><m>(s \pm \text{shift})^{\text{power}}</m> </cell>
					<cell right="minor" >-										  </cell>
					<cell			   ><m>L_6</m>								 </cell>
				</row>
				<row bottom="minor">
					<cell right="minor"><m>s^{2} + \text{number}</m>	</cell>
					<cell right="minor">
						<line>no</line>
						<line>yes</line>
					</cell>
					<cell>
						<line><m>L_4</m></line>
						<line><m>L_5</m></line>
					</cell>
				</row>
				<row bottom="minor">
					<cell right="minor"><m>(s \pm \text{shift})^{2} + \text{number}</m> </cell>
					<cell right="minor">
						<line>no</line>
						<line>yes</line>
					</cell>
					<cell>
						<line><m>L_7</m></line>
						<line><m>L_8 + L_7</m></line>
					</cell>
				</row>
			</tabular>
		</table>

	</p>

	<paragraphs><title>Missing Constants</title>

		<p>
			The most common adjustment needed to match one of the <m>s</m>-functions in <xref ref="common-lt-table"/> is to introduce a missing constant in the numerator. This is done by multiplying the numerator and denominator by this constant as shown in the following examples. 
		</p>

		<example>

			<m>\ \ </m>Compute the inverse Laplace transforms for each.

			<tabular>
				<col width="20%" halign="center"/>
				<col width="75%"/>
				<row>
					<cell><m>\ds \frac{12}{s}</m></cell>
					<cell>
						<p>
							<m>\hspace{27em}</m>
							<solution>
								<p>
									The <m>s</m> in the denominator tells us that we need <m>L_1</m>. Before we do, let's factor out <m>12</m>:
									<me>\ds \ilap{\frac{12}{s}} = 12 \cdot \ilap{\frac{1}{s}} = 12 \cdot 1 = 12</me>.
								</p>
							</solution>
						</p>
					</cell>
				</row>
				<row>
					<cell><m>\ds \frac{5}{s^2 + 4}</m></cell>
					<cell>
						<p>
							<m>\hspace{27em}</m>
							<solution>
								<p>
									Since the denominator has the form, <m>s^2 + \text{number}</m>, and there is no <m>s</m> in the numerator, we should apply <m>L_4</m>. As before, it is helpful to first factor out the constant <m>5</m>, 
									<me>\ds \ilap{\frac{5}{s^2 + 4}} = 5\ \ilap{\frac{1}{s^2 + 4}} \quad \leftarrow <xref ref="L4" text="custom">L_4</xref> (b=2)</me>.
									According to <m>L_4</m>, we are missing <m>2</m> in the numerator. Let's put it there by multiplying by <m>2/2</m>, like so
									<md>
										<mrow> = 5\ \ilap{\frac{2}{2}\frac{1}{s^2 + 4}} =\amp\ 5\ \ilap{\frac{1}{2}\frac{2}{s^2 + 4}}</mrow>
										<mrow>										  =\amp\ \frac{5}{2} \ilap{\frac{2}{s^2 + 4}}</mrow>
										<mrow>										  =\amp\ \frac{5}{2} \sin(2t)</mrow>
									</md>
								</p>
							</solution>
						</p>
					</cell>
				</row>
				<row>
					<cell><m>\ds \frac{17}{s^4}</m></cell>
					<cell>
						<p>
							<m>\hspace{27em}</m>
							<solution>
								<p>
									This denominator has the form <m>s^{\text{power}}</m>, which matches <m>L_3</m> with <m>n = 3</m>. 
									<me>\ds \ilap{\frac{17}{s^4}} = 17\ \ilap{\frac{1}{s^4}} \quad \leftarrow <xref ref="L3" text="custom">L_3</xref> (n=3)</me>.
									In this case, the numerator is missing a <m>3!</m>. We can introduce it by multiplying by <m>3!/3!</m>, like so
									<md>
										<mrow> = 17\ \ilap{\frac{3!}{3!}\frac{1}{s^4}} = \frac{17}{3!} \ilap{\frac{3!}{s^4}} = \frac{17}{6} t^3</mrow>
									</md>
								</p>
							</solution>
						</p>
					</cell>
				</row>
				<row>
					<cell><m>\ds \frac{7s}{s^2 + 25}</m></cell>
					<cell>
						<p>
							<m>\hspace{27em}</m>
							<solution>
								<p>
									The denominator here is <m>s^2 + \text{number}</m>, which matches <m>L_5</m> with <m>b = 5</m>. Therefore,
									<md>
										<mrow> \ilap{\frac{7s}{s^2 + 25}}   =\amp\ 7\ \ilap{\frac{s}{s^2 + 25}} \quad \leftarrow <xref ref="L5" text="custom"><m>L_5</m></xref> (b=5)</mrow>
										<mrow>							  =\amp\ 7\ \cos(5t)</mrow>
									</md>.
								</p>
							</solution>
						</p>
					</cell>
				</row>
				<row>
					<cell><m>\ds \frac{10}{(s - 3)^2 + 11}</m></cell>
					<cell>
						<p>
							<m>\hspace{27em}</m>
							<solution>
								<p>
									The form of this denominator is <m>\ul{(s \pm \text{shift})^{2} + \text{number}}</m> and has no <m>s</m> in the numerator. This matches <m>L_7</m> with <m>a = 3</m> and <m>b = 5</m>. Therefore,
									<md>
										<mrow> \ilap{\frac{10}{(s - 3)^2 + 11}}</mrow>
										<mrow>	  =\amp\ 10\ \ub{\ilap{\frac{\sqrt{11}}{\sqrt{11}}\frac{1}{(s - 3)^2 + 11}}}_{\large <xref ref="L7" text="custom"><m>L_7</m></xref> (a=3,\ b=5)}</mrow>
										<mrow>	  =\amp\ \frac{10}{\sqrt{11}} \ilap{\frac{\sqrt{11}}{(s - 3)^2 + 11}}</mrow>
										<mrow>	  =\amp\ \frac{10}{\sqrt{11}} e^{3t} \sin(\sqrt{11}t)</mrow>
									</md>

								</p>
							</solution>
						</p>
					</cell>
				</row>
				<row>
					<cell><m>\ds \frac{2}{(s+7)^5}</m></cell>
					<cell>
						<p>
							<m>\hspace{27em}</m>
							<solution>
								<p>
									The denominator, <m>\ul{(s \pm \text{shift})^{\text{power}}}</m>, matches <m>L_6</m> with <m>a = -7</m> and <m>n = 4</m>. Therefore,
									<md>
										<mrow> 
											\ilap{\frac{2}{(s+7)^5}} 
												=\amp\ 2\ \ub{\ilap{\frac{4!}{4!}\frac{1}{(s+7)^5}}}_{\large <xref ref="L6" text="custom"><m>L_6</m></xref> (a=-7,\ n=4)}
										</mrow>
										<mrow> 
												=\amp\ \frac{2}{4!} \ilap{\frac{4!}{(s+7)^5}}
										</mrow>
										<mrow>
											=\amp\ \frac{1}{12} t^4 e^{-7t}
									</mrow>
									</md>
								</p>
							</solution>
						</p>
					</cell>
				</row>
			</tabular>
		</example>

	</paragraphs>

	<xi:include href="./p4-c2-s2-1-interactives.ptx" />

	<paragraphs><title>Splitting a Fraction</title>

		<p>
			Another common modification is when the <m>s</m>-function contains a sum of different common forms. In these cases, you can usually split the fraction as the sum of these forms.
		</p>

		<example>

			<m>\ \ </m>Compute the inverse Laplace transforms for each.

			<tabular>
				<col width="20%" halign="center"/>
				<col width="75%"/>
				<row>
					<cell><m>\ds \frac{2s - 3}{s^2 + 16}</m></cell>
					<cell>
						<p>
							<m>\hspace{27em}</m>
							<solution>
								<p>
									The key to this problem is to split the fraction into two separate terms:
									<me>\ds \frac{2s - 3}{s^2 + 16} = \frac{2s}{s^2 + 16} - \frac{3}{s^2 + 16}.</me>
									Notice the first term matches with <m>L_5</m> and the second term matches with <m>L_4</m>, so
									<md>
										<mrow>  \amp\ \ilap{\frac{2s-3}{s^2 + 16}}											 </mrow>
										<mrow>  \amp \hspace{3em}= 2\ \ilap{\frac{s}{s^2 + 16}} - 3\ \ilap{\frac{1}{4}\frac{4}{s^2 + 16}}   </mrow>
										<mrow>  \amp \hspace{3em}= 2\ \cos(4t) - \frac{3}{4} \sin(2t)									   </mrow>
									</md>
								</p>
							</solution>
						</p>
					</cell>
				</row>
				<row>
					<cell><m>\ds \frac{s^3 + 2s - 7}{s^7}</m></cell>
					<cell>
						<p>
							<m>\hspace{27em}</m>
							<solution>
								<p>
									We can split the fraction into the terms,
									<me>\ds \frac{s^3 + 2s - 7}{s^7} = \frac{s^3}{s^7} + \frac{2s}{s^7} - \frac{7}{s^7} = \frac{1}{s^4} + \frac{2}{s^6} - \frac{7}{s^7}.</me>
									and apply the inverse Laplace transform to each
									<md>
										<mrow> \ilap{\frac{1}{s^4}} = \frac{1}{3!}\ilap{\frac{3!}{s^4}} = \frac{1}{3!}t^3</mrow>
										<mrow> \ilap{\frac{2}{s^6}} = \frac{2}{5!}\ilap{\frac{5!}{s^6}} = \frac{2}{5!}t^5</mrow>
										<mrow> \ilap{\frac{7}{s^7}} = \frac{7}{6!}\ilap{\frac{6!}{s^7}} = \frac{7}{6!}t^6</mrow>
									</md>
									Therefore, the inverse transform is
									<me>\ds \ilap{\frac{s^3 + 2s - 7}{s^7}} = \frac{1}{3!}t^3 + \frac{2}{5!}t^5 - \frac{7}{6!}t^6.</me>
								</p>
							</solution>
						</p>
					</cell>
				</row>
			</tabular>
		</example>

	</paragraphs>

	<p>
		This section explored two relatively minor modifications needed to match and find the backward Laplace transform. However, some <m>s</m>-functions require more complex techniques to reach the desired form. In the next section, we will discuss how completing the square can help us match the form where the <m>s</m>-variable is shifted.
	</p>

	<xi:include href="./p4-c2-s2-2-interactives.ptx" />
   
</section>