<section xmlns:xi="http://www.w3.org/2001/XInclude" xml:id="sec-lhcc-step-3"><title> Step 3: Give Solution </title>

	<introduction>

		<outcomes>
			<ul>
				<li> 
					Find the general solution from the characteristic equation solutions.
				</li>
				<li> 
					Master <xref text="custom" ref="lhcc-step3"> Step 3 </xref> of <xref ref="lhcc-method" text="title"/>
				</li>
			</ul>
		</outcomes>

		<p>
			We are nearly prepared to apply the full <xref ref="lhcc-method" text="title"/> to an <xref ref="lhcc-eqn" text="custom"> LHCC equation </xref>. The only thing left to do is discuss how to use the solutions of the characteristic equation to find the general solution. 
		</p>

		<p>
			As a review, suppose we want to find the general solution to the LHCC differential equation
			<men xml:id="full-lhcc-eqn1">
				y'' - 9 y = 0.
			</men>
			According to <xref ref="concept-lhcc-terms"/>, all the parts of the solution should look like <m>e^{rx}</m>. With this in mind, we plugged <m>y = e^{rx}</m> into <xref ref="full-lhcc-eqn1"/>, leading to the characteristic equation
			<me>
				r^2 - 9 = 0,
			</me>
			which has solutions <m>r_1 = 3, r_2 = -3</m>. Therefore, the general solution is a combination of <m>e^{3x}</m> and <m>e^{-3x}</m>, given by
			<men  xml:id="full-lhcc-sol1">
				y(x) = c_1\ e^{3x} + c_2\ e^{-3x}
			</men>
			where <m>c_1, c_2</m> are unknown constants.
		</p>

		<p>
			This example shows how the solutions to the characteristic equation lead to the general solution, but not every case works out this nicely. The next few sections, break down differences for each cases that you may encounter.
		</p>

	</introduction>

	<xi:include href="lhcc-step-3-p1-2nd-order.ptx" />
	<xi:include href="lhcc-step-3-p2-higher-order.ptx" />
	<xi:include href="interactives/lhcc-step-3-p2-interactives.ptx" />

</section>