<section xmlns:xi="http://www.w3.org/2001/XInclude" xml:id="sec-lhcc-char-eqn"><title> Characteristic Equation </title>

	<introduction>

		<p>
			Every <xref ref="lhcc-eqn" text="custom">LHCC differential equation</xref> has a corresponding characteristic equation and the connection between them is based on the following idea.
		</p>

		<lemma xml:id="concept-lhcc-terms">
			<statement>
				<p>
					Solutions to <xref ref="lhcc-eqn" text="custom">LHCC</xref> equations are composed of <m>e^{rx}</m> terms where <m>r</m> is a constant that depends on the differential equation.
				</p>
			</statement>
		</lemma>

		<p>
			To clarify this statement,
			<me>
				y = C_1 e^{4x} + C_2 e^{-x}
			</me>
			is a sample solution of some LHCC equation. The <m>e^{4x}</m> and <m>e^{-x}</m> terms correspond to <m>r=4</m> and <m>r=-1</m> in <xref ref="concept-lhcc-terms"/>, respectively. Let's investigate this concept further with an example.
		</p>

		<example xml:id="lhcc-example-01">
			<statement>
				<p>
					Find any <m>r</m> values that make <m>y = e^{rx}</m> a solution to the LHCC equation
					<men xml:id="lhcc-example-01-eqn-01">
						y'' - 9y = 0.
					</men>
				</p>
			</statement>
			<solution>
				<p>
					Approach this as if you were verifying that <m>y = e^{rx}</m> is a solution to <xref ref="lhcc-example-01-eqn-01"/>. So, plug it into the equation and check if left and right-hand sides are equal.
				</p>

				<p>
					Since we need <m>y^{\prime\prime}</m>, let's compute this first.
				</p>
				<tabular>
					<row>
						<cell><m>\displaystyle y' = e^{rx} \cdot (r) = re^{rx}</m></cell>
						<cell><em>(chain rule)</em></cell>
					</row>
					<row>
						<cell><m>\displaystyle y'' = [re^{rx}]^{\prime} = r[e^{rx}]^{\prime}  = r(e^{rx} \cdot (r)) = r^2e^{rx}</m></cell>
						<cell><em>(chain rule)</em></cell>
					</row>
				</tabular>
				<p>
					Plugging <m>y^{\prime\prime}</m> and <m>y</m> into the left side of <xref ref="lhcc-example-01-eqn-01"/> gives
				</p>
				<tabular>
					<row>
						<cell><m>\displaystyle r^2e^{rx} - 9e^{rx} = 0 </m></cell>
						<cell/>
					</row>
					<row>
						<cell><m>\displaystyle (r^2 - 9)\ e^{rx} = 0</m></cell>
						<cell><em>(factor out <m>e^{rx}</m>)</em></cell>
					</row>
				</tabular>
				<p>
					Now, <m>y = e^{rx}</m> is only a solution if we can show LHS = RHS (<em><m>0 = 0</m> in this case</em>). It should be clear that this depends on the values of <m>r</m>. This is just an algebra problem where we must solve for <m>r</m>.
				</p>
				<tabular>
					<row>
						<cell><m>\displaystyle r^2 - 9 = 0,</m></cell>
						<cell><m>\displaystyle e^{rx} = 0</m></cell>
						<cell><em>(set each factor to 0)</em></cell>
					</row>
					<row>
						<cell><m>r = \pm 3,</m></cell>
						<cell>
							<em>no solution</em>
							<fn>
								Attempting to solve <m>\displaystyle e^{rx} = 0</m> for <m>r</m> by applying <m>\ln</m> would give
								<me>
									\displaystyle \ln(e^{rx}) = \ln(0) \, \leftarrow \text{not defined}
								</me>
							</fn>
						</cell>
						<cell/>
					</row>
				</tabular>
				<p>
					So, the only <m>r</m> values that make the LHS = RHS is <m>r = -3, 3</m>.
				</p>
			</solution>
		</example>

		<p>
			The previous example showed us that finding the values of <m>r</m> that make <m>y = e^{rx}</m> a solution to <m> y'' - 9y = 0</m> amounts to solving 
			<men xml:id="lhcc-example-01-ce">
				r^2 - 9 = 0
			</men>
			for <m>r</m>. It turns out that <xref ref="lhcc-example-01-ce"/> is exactly the characteristic equation in <xref text="custom" ref="lhcc-step2"> Step 2 </xref> of the <xref ref="lhcc-method" text="title"/>.
		</p>

		<p>
			Every LHCC equation has a characteristic equation that can be found in the same way as in <xref ref="lhcc-example-01"/>. In particular, you plug <m>y = e^{rx}</m> into the DE and factor out an <m>e^{rx}</m> term. Let's work out the details, but first, notice the pattern of derivatives when using the chain rule on <m>y = e^{rx}</m> at each step.
			<me>
				y = e^{rx} \quad \rightarrow \quad y' = re^{rx} \quad \rightarrow \quad y'' = r^2e^{rx} \quad \rightarrow \, \dots \, \rightarrow \quad y^{(n)} = r^ne^{rx}
			</me>
			<!-- <tabular>
				<row>
					<cell><m>\displaystyle y = e^{rx}</m></cell>
				</row>
				<row>
					<cell><m>\displaystyle y' = re^{rx}</m></cell>
				</row>
				<row>
					<cell><m>\displaystyle y'' = r^2e^{rx}</m></cell>
				</row>
				<row>
					<cell><m>\vdots</m></cell>
				</row>
				<row>
					<cell><m>\displaystyle y^{(n)} = r^ne^{rx}</m></cell>
				</row>
			</tabular> -->
		</p>

		<p>
			Plugging each of these into <xref ref="lhcc-eqn"/> leads to
		</p>

		<tabular>
			<row>
				<cell colspan="2"><m>\displaystyle a_n\ r^ne^{rx} + \cdots + a_2\ r^2e^{rx} + a_1\ re^{rx} + a_0\ e^{rx} = 0 </m></cell>
				<cell/>
			</row>
			<row>
				<cell colspan="2"><m>\displaystyle (a_n\ r^n + \cdots + a_2\ r^2 + a_1\ r + a_0)\ e^{rx} = 0</m></cell>
				<cell><em>(factor out <m>e^{rx}</m>)</em></cell>
			</row>
			<row halign="center">
				<cell><m>\displaystyle a_n\ r^n + \cdots + a_2\ r^2 + a_1\ r + a_0 = 0,</m></cell>
				<cell><m>\displaystyle e^{rx} = 0</m></cell>
				<cell><em>(set each factor to 0)</em></cell>
			</row>
			<row halign="center">
				<cell><m>\uparrow</m></cell>
				<cell><m>\uparrow</m></cell>
				<cell/>
			</row>
			<row halign="center">
				<cell><em>characteristic equation!</em></cell>
				<cell><em>no solution</em></cell>
				<cell/>
			</row>
		</tabular>

		<p>
			Going through this process a few times should convince you that there is a simple relationship between the differential equation and its corresponding characteristic equation. Looking at the equations side-by-side shows that the derivatives of <m>y</m> map directly to the powers of <m>r</m>.
			<!-- <tabular>
				<row>
					<cell><m> a_n\ y^{(n)} + a_{n-1}\ y^{(n-1)} + \cdots + a_2\ y'' + a_1\ y' + a_0\ y = 0 </m></cell>
				</row>
				<row>
					<cell><m> a_n\ y^{(n)} + a_{n-1}\ y^{(n-1)} + \cdots + a_2\ y'' + a_1\ y' + a_0\ y = 0 </m></cell>
				</row>
				<row>
					<cell><m> a_n\ r^n + a_{n-1}\ r^{n-1} + \cdots + a_2\ r^2 + a_1\ r+ a_0\ = 0 </m></cell>
				</row>
			</tabular> -->

			<!-- a_n\ \underset{\downarrow}{	\underline{y^{(n)}}}	\amp + \cdots +	\amp a_2\ \underset{\downarrow}{\underline{y''}}	\amp + \amp	a_1\ \underset{\downarrow}{	\underline{y'}}	\amp + \amp	a_0\ \underset{\downarrow}{\underline{y}}	\amp =	\amp 0\\ -->
			
			<me>
				\begin{matrix}
					a_n\ \underline{y^{(n)}}	\amp + \cdots +	\amp a_2\ \underline{y''}	\amp +	\amp	a_1\ \underline{y'}		\amp +	\amp	a_0\ \underline{y}		\amp =\ 0	\\
						\ \ \ \downarrow		\amp			\amp    \ \ \ \downarrow	\amp 	\amp	   \ \ \ \downarrow		\amp 	\amp	   \ \ \ \downarrow		\amp	 	\\
					a_n\ \underline{r^n}		\amp + \cdots +	\amp a_2\ \underline{r^2}	\amp +	\amp	a_1\ \underline{r^1}	\amp +	\amp	a_0\ \underset{=\ 1}{\underline{r^0}}	\amp =\ 0
				\end{matrix}
			</me>

		</p>
		
		<definition xml:id="def-lhcc-ce">
			<statement>
				<p>
					The <term>characteristic equation</term> of an <xref ref="lhcc-eqn" text="custom"> LHCC equation </xref> is given by
					<men xml:id="def-lhcc-ce-eqn">
						a_n\ r^{n} + \cdots + a_2\ r^2 + a_1\ r + a_0 = 0.
					</men>
				</p>
			</statement>
		</definition>

		<example>
			<p>
				Give the characteristic equation of the differential equation
				<me>
					y'' + 5y' - y = 0.
				</me>
			</p>

			<solution>
				<p>
					<me>
						r^2 + 5r - 1 = 0
					</me>
				</p>
			</solution>
	
		</example>

	</introduction>

	<!-- <xi:include href="./interactive-sections/03-lhcc-char-eqn-interactives.ptx" /> -->

	<!-- <xi:include href="./02-homogeneous-solution-exercises.ptx" /> -->

</section>
