<section xmlns:xi="http://www.w3.org/2001/XInclude" xml:id="sec-lt-defn"><title> DEFNITION </title>
	
	<introduction>

	<p>
		Give some statement leading to the definition....
	</p>

	<p>
		Edit Notes:
		<ul>
			<li> We should probably address the <m>s</m> in the integral somewhere.</li>
		</ul>
	</p>

	<definition>
	<title> Laplace Transform </title>
		<statement>
		The <term>Laplace Transform</term> of a function <m>y(t)</m> is given by

		<me> \LAP\left\{ y(t) \right\} = \int_0^{\infty} \left(y(t)\right) e^{-st}dt, </me>

		given that the integral exists (i.e. the improper integral is finite).
		</statement>
	</definition>

	<p>
		There's a lot to unpack with this definition, but let's begin with a few examples illustrating the definition before diving into the details.
	<!--
		As we work through the following examples, we will practice using the definition, as well as gathering facts about how the Laplace transform works. You will no doubt find the solutions to these examples a bit cumbersome We hope to draw some conclusions as we move forward that help us find the Laplace transform quickly without having to use the (admittedly somewhat cumbersome) definition every time.
	-->
	</p>


	</introduction>

	<example xml:id="ex_lt_defn_01">
		<p>
			Find the Laplace transform of the function <m>g(t) = 15</m>.
		</p>
		<p/>
	
		<solution>
			<p>
				By the above definition, we have
			<md>
				<mrow> \LAP\{ g(t) \}	\amp= \LAP\{ 15 \} 								</mrow>
				<mrow>		\amp= \int_0^{\infty} \left(15\right)e^{-st}dt
											\qquad \text{(improper integral)}</mrow>
					<mrow>		\amp= \lim_{b \to \infty}\int_0^b 15 e^{-st}dt	</mrow>
					<mrow>		\amp= 15 \lim_{b \to \infty}\int_0^b e^{-st}dt
											\qquad (s\text{ is constant here})</mrow>
			</md>
				At this point, we need to assume that <m>s\ne0</m> in order to continue. If you are curious as to why, see this <xref text="custom" ref="LT-s-ne-0-15">note</xref> for an explanation. Next, we integrate using the substitution <m>u=-st</m>.
		  </p>
	
			<p>
				<md>
					<mrow>		\amp= 15\lim_{b \to \infty} -\frac{1}{s}e^{-st}\Big|_0^b</mrow>
					<mrow>		\amp= 15\lim_{b \to \infty} -\frac{1}{s}\left[ e^{-sb} - e^{-s\cdot 0} \right]</mrow>
					<mrow>		\amp= -\frac{15}{s} \lim_{b \to \infty} \Big[ e^{-sb} - 1 \Big] \qquad \leftarrow
						<xref text="custom" ref="reason-factor-out-s">why can -1/s be pulled out?</xref></mrow>
				<mrow>		\amp= -\frac{15}{s}	\left[ \left(\lim_{b \to \infty} e^{-sb} \right) - \left( \lim_{b \to \infty} 1 \right)\right]</mrow>
				<mrow>		\amp= -\frac{15}{s}	\left[ \left(\lim_{b \to \infty} e^{-sb} \right) - 1 \right]</mrow>
			</md>
			</p>
	
			<p>
				Now let's focus on the remaining limit. It turns out that we have to put one more restriction on <m>s</m> since the limit will change based on whether <m>s</m> is positive or negative. Let's consider both cases.
			</p>
	
	
			<p>
				Case 1: <m>\quad s\lt 0</m>, If <m>b \to \infty</m>, then <m>-sb \to +\infty</m> and so <m>\DS\lim_{b \to \infty} e^{-sb} = \infty</m>.
				<me> = -\frac{15}{s} \left[\left( \lim_{b \to \infty} e^{-sb} \right) - 1 \right] = \infty</me>
			</p>
	
			<p>
				Case 2: <m>\quad s\gt 0</m>. If <m>b \to \infty</m>, then <m>-sb \to -\infty</m> and so <m>\DS\lim_{b \to \infty} e^{-sb} = 0</m>.
				<me> = -\frac{15}{s} \left[\left( \lim_{b \to \infty} e^{-sb} \right) - 1 \right] = -\frac{15}{s} \left[0 - 1\right] = \frac{15}{s}</me>
			</p>
	
			<p>
				In case 1 (<m>s\lt0</m>), the improper integral is not finite, whereas in case 2 (<m>s\gt0</m>), the integral is finite and is equal to <m>15/s</m>.
			</p>
	
			<p>
				In conclusion, we have found that
				<me>\LAP\{15\} = \frac{15}{s}</me>,
				assuming <m>s \gt 0</m>.
			</p>
		</solution>
	
	</example>
	
	<example xml:id="ex_lt_defn_02">
		<p>
			Find the Laplace transform of <m>x(t) = e^{7t}</m>.
		</p>
		<p/>
	
		<solution>
			<p>
				We use the definition of Laplace transform to get us started.
			<md>
				<mrow> \LAP\{ x(t) \} \amp= \LAP\{ e^{7t} \} 				</mrow>
				<mrow> 		\amp= \int_0^{\infty} \left(e^{7t}\right)e^{-st}\ dt 				</mrow>
				<mrow> 		\amp= \lim_{b \to \infty}\int_0^b e^{-st + 7t}\ dt	</mrow>
				<mrow> 		\amp= \lim_{b \to \infty}\int_0^b e^{(7-s)t}\ dt 		</mrow>
			</md>
	
				As before, we need restrict some values of <m>s</m> in order for this
				improper integral to exist . In this case, we will need <m>7 - s</m>, in the exponent, to be non-zero and negative. That is, we need
	
				<me> 7 - s \lt 0 \hspace{0.5cm}\Rightarrow \hspace{0.5cm}7 \lt s. </me>
	
				Hence, we move forward with the assumption that <m>s \gt 7</m>.
	
			<md>
				<mrow> 	\amp= \lim_{b \to \infty}\int_0^b e^{(7-s)t}dt </mrow>
				<mrow>	\amp= \lim_{b \to \infty} \frac{1}{7-s}e^{(7-s)t}\Bigg|_0^b</mrow>
				<mrow>	\amp= \frac{1}{7-s}\lim_{b \to \infty}
										\left[ e^{(7-s)b} - e^{(7-s)\cdot 0}\right]</mrow>
				<mrow>	\amp= \frac{1}{7-s}\lim_{b \to \infty}
										\left[ e^{(7-s)b} - 1\right]</mrow>
				<mrow>	\amp= \frac{1}{7-s}
										\left[\lim_{b \to \infty}e^{(7-s)b}
										- \lim_{b \to \infty}1\right]</mrow>
				<mrow>	\amp= \frac{1}{7-s} \left[ 0 - 1\right] \quad
										<xref text="custom" ref="reason-limit-to-zero-e7t">why is the limit 0?</xref></mrow>
				<mrow>	\amp= \frac{-1}{7-s} \hspace{4.4cm}	</mrow>
				<mrow>	\amp= \frac{1}{s - 7}, 					\quad s \gt 7 	</mrow>
			</md>
	
				Thus, the Laplace transform of <m>x(t) = e^{7t}</m> is
				<me>\DS \LAP\{e^{7t}\} = \frac{1}{s - 7}</me>.
			</p>
		</solution>
	
	</example>
	
	<example xml:id="ex_lt_defn_03">
		<p>
			Find the Laplace transform of <m>q(t) = 11t</m>.
		</p>
		<p/>
	
		<solution>
			<p>
			Let's use the definition of Laplace transform to get us going.
	
				<md>
					<mrow> \LAP\{ 11t \} \amp= \int_0^{\infty} \left(11t\right) e^{-st}\ dt </mrow>
					<mrow> 						 \amp= 11\lim_{b \to \infty} \int_0^b te^{-st} dt \quad s \ne 0
																	\quad <xref text="custom" ref="LT-s-ne-0-11t">why is <m>s \ne 0</m>?</xref>
																	\hspace{4.8cm}</mrow>
				</md>
					<md>
					<mrow> \phantom{\LAP\{11t\}}\amp= 11\lim_{b \to \infty}
									\left[-\frac{b}{s}e^{-sb} - \frac{1}{s^2}e^{-sb} + \frac{1}{s^2}\right]\quad
											<xref text="custom" ref="reason-int-by-parts-texpt">Integration by parts</xref>
											\hspace{2.5cm}</mrow>
					</md>
					<md>
						<mrow> \phantom{\LAP\{11t\}}\amp= 11 \left[-\lim_{b \to \infty}\frac{b}{s}e^{-sb}
										- \lim_{b \to \infty}\frac{1}{s^2}e^{-sb}
										+ \lim_{b \to \infty}\frac{1}{s^2}\right]</mrow>
					<mrow> \amp= 11 \left[-\frac{1}{s}\lim_{b \to \infty}be^{-sb}
										- \frac{1}{s^2}\lim_{b \to \infty}e^{-sb}
										+ \frac{1}{s^2}\right]\quad s > 0 \quad
											<xref text="custom" ref="LT-s-gt-0-11t">why is s > 0?</xref>\hspace{1.0cm}</mrow>
				</md>
					<md>
					<mrow> \phantom{\LAP\{11t\}}\amp= 11 \left[-\frac{1}{s}\cdot 0
										- \frac{1}{s^2}\cdot 0 + \frac{1}{s^2}\right]\quad
											<xref text="custom" ref="reason-limit-to-zero-11t">why are the limits 0?</xref>
											\hspace{3.6cm}</mrow>
						<mrow> 		\amp= \frac{11}{s^2}, \quad s \gt 0 						</mrow>
				</md>
	
	
	
			Hence, we have <m>\DS \LAP\{ 11t \} = \frac{11}{s^2}</m>, under the condition that <m>s>0</m>.
			</p>
		</solution>
	</example>
	
	<p>
		So far, we have seen three examples of how to find a Laplace transform of a given function, but we have not discussed why this idea is relevant to differential equations. In the next section, we will tie these two concepts together and illustrate how Laplace transform can be used to solve a differential equation.
	</p>
	
	<p>
		 Before moving forward, let's conclude this section by listing out a few important take-aways from the examples of this section.
		<ul>
			<li>
				In every example, we started with a function of <m>t</m> and after computing the Laplace transform, we ended up with a function of a new variable <m>s</m>. A common convention is to use upper case function names for the Laplace transform of a given lower case function. For example,
				<me> \LAP\{f(t)\} = F(s) \quad \text{ or } \quad \LAP\{q(t)\} = Q(s).</me>
				In this book, we will often say "<m>F(s)</m> is the Laplace transform of <m>f(t)</m>".
				This naming	convention might seem unimportant, but it will be very helpful when using these Laplace transforms to solve differential equations.
			</li>
			<li>
				The notation often used for Laplace transform involved the symbol <m>\LAP.</m> The curly braces that accompany are not optional; they are not just grouping symbols. We use them to indicate we are taking the Laplace transform of the function within the curly braces.
			</li>
			<li>
				The integral has two variables, <m>s</m> and <m>t</m>, and we integrate with respect to <m>t</m>. You may not have done anything like this before; all we need to do is treat
				<m>	s</m> like a constant.
			</li>
			<li>
				The last couple of words in the definition say, "given that the integral exists."	We will end up putting restrictions on the variable <m>s</m> that make sure that the
				integral exists.
			</li>
		</ul>
	</p>

</section>
