<?xml version="1.0" encoding="UTF-8" ?>

<!-- 15-DEsReview_matching_forms_part1 -->

<section xml:id="r-01-15" xmlns:xi="http://www.w3.org/2001/XInclude">

<title>Matching Forms, Part 1</title>

<p>
When we study Laplace Transforms, we will frequently want
to manipulate an algebraic expression to make it match a given form.
</p>

<p>
If you prefer to see a video of this example, 
<xref ref="video-matching_terms_01" text="custom"> click here </xref>
</p>

<p>
Suppose we have the expression

<me> \frac{1}{s^2 + 25}, </me>

and we think it looks much like the form

<me> \frac{b}{s^2 + b^2}. </me>

It's not a perfect match, though. Based on the denominator, we might guess <m>b = 5.</m>  
</p>

<p>
Notice that this would make the denominator a perfect match, 

<me> \frac{1}{s^2 + 25} = \frac{1}{s^2 + 5^2}. </me>  

However, the numerator still isn't quite right. It would be correct if we would 
multiply the numerator by 5. But if we multiply the numerator by 5, we would change 
the expression. In order to NOT change the expression, we will instead multiply by 
<m>\frac{5}{5},</m> as follows:

<md>
	<mrow>	\frac{1}{s^2 + 25}	\amp= \frac{1}{s^2 + 5^2}						</mrow>
	<mrow>						\amp= \frac{5}{5}\cdot \frac{1}{s^2 + 5^2}		</mrow>
	<mrow>						\amp= \frac{1}{5}\cdot \frac{5}{s^2 + 5^2}		</mrow>
	<mrow>						\amp= \frac{1}{5}\cdot \frac{b}{s^2 + b^2}, 
													\text{ where } b=5			</mrow>
</md>

Notice that when we multiply by <m>\frac{5}{5}</m>, we are just multiplying by one, so we
don't change the value of the expression.
</p>

<p>
Maybe write now you're wondering what the point is. Being able to use appropriate algebra 
to "match" forms is <em>really</em> important when we work with Laplace Transforms. Since 
it's really just algebra, now is a great time to practice that skill--so when we are in 
the middle of studying Laplace Transforms, you can just focus on the "new" stuff.

<ol>
	<li> 
	<p>
	Manipulate each of the following expressions into the form 
	<m>\quad \DS \frac{b}{s^2 + b^2}.</m>
	
	<ol>
		<li> <m>\DS \frac{1}{s^2 + 49} \quad </m>		
		<solution>		
    	<md>	
    		<mrow>\frac{1}{s^2 + 49}\amp= \frac{1}{s^2 + 7^2}					</mrow>
    		<mrow>					\amp= \frac{7}{7}\cdot \frac{1}{s^2 + 7^2}	</mrow>
    		<mrow>					\amp= \frac{1}{7}\cdot \frac{7}{s^2 + 7^2}	</mrow>
    		<mrow>					\amp= \frac{1}{7}\cdot \frac{b}{s^2 + b^2}, 
													\text{ where <m>b=7</m>}	</mrow>
    	</md>
    	</solution>
    	<answer>
    		<m>\DS \frac{1}{7}\cdot \frac{7}{s^2 + 7^2} </m>
    	</answer>
		</li>
	
		<li> <m>\DS \frac{12}{s^2 + 16} \quad </m>		
    	<solution>		
    	<md>	
    		<mrow>\frac{12}{s^2 + 16}	\amp= 12 \cdot \frac{1}{s^2 + 4^2}</mrow>
    		<mrow>\amp= \frac{4}{4}\cdot 12 \cdot \frac{1}{s^2 + 4^2}</mrow>
    		<mrow>\amp= \frac{1}{4}\cdot 12 \cdot \frac{4}{s^2 + 4^2}</mrow>
    		<mrow>\amp= \frac{12}{4}\cdot \frac{4}{s^2 + 4^2}</mrow>
    		<mrow>\amp= 3\cdot \frac{b}{s^2 + b^2}, \text{ where <m>b=4</m>}</mrow>
    	</md>
    		
    	</solution>
    	<answer>
    		<m>\DS 3\cdot \frac{4}{s^2 + 4^2} </m>
    		 
    	</answer>
		</li>
	
		<li> <m>\DS \frac{3}{s^2 + 5} \quad </m>		
    	<solution>		
    	<md>	
    		<mrow>\frac{3}{s^2 + 5}	\amp= 3 \cdot \frac{1}{s^2 + (\sqrt{5})^2}</mrow>
    		<mrow>\amp= \frac{\sqrt{5}}{\sqrt{5}}\cdot 3\cdot \frac{1}{s^2 + (\sqrt{5})^2}</mrow>
    		<mrow>\amp= \frac{1}{\sqrt{5}}\cdot 3\cdot \frac{\sqrt{5}}{s^2 + (\sqrt{5})^2}</mrow>
    		<mrow>\amp= \frac{3}{\sqrt{5}}\cdot \frac{b}{s^2 + b^2}, \text{ where <m>b=\sqrt{5}</m>}</mrow>
    	</md>
    		
    	</solution>
    	<answer>
    		<m>\DS \frac{3}{\sqrt{5}}\cdot \frac{\sqrt{5}}{s^2 + (\sqrt{5})^2} </m>
    	</answer>
		</li>
	</ol>
	</p>
	</li>

	<li> 
	<p>
	Manipulate each of the following expressions into the form 
	<m>\quad \DS \frac{s}{s^2 + b^2}.</m>
	
	<ol>	
		<li> <m>\DS \frac{4s}{s^2 + 9} \quad </m> 		
    	<solution>		
    	<md>	
    		<mrow>\frac{4s}{s^2 + 9}	\amp= 4 \cdot \frac{s}{s^2 + 3^2}</mrow>
    		<mrow>\amp= 4\cdot \frac{s}{s^2 + b^2}, \text{ where <m>b=3</m>}</mrow>
    	</md>
    		
    		
    	</solution>
    	<answer>
    		<m>\DS 4 \cdot \frac{s}{s^2 + 3^2} </m>
    	</answer>
		</li>
	
		<li> <m>\DS \frac{s}{2s^2 + 8} \quad </m> 		
    	<solution>		
    	<md>	
    		<mrow>\frac{s}{2s^2 + 8}	\amp= \frac{1}{2} \cdot \frac{s}{s^2 + 4}</mrow>
    		<mrow>\amp= \frac{1}{2} \cdot \frac{s}{s^2 + 2^2}</mrow>
    		<mrow>\amp= \frac{1}{2}\cdot \frac{s}{s^2 + b^2}, \text{ where <m>b=2</m>}</mrow>
    	</md>
    	</solution>
    	<answer>
    		<m>\DS \frac{1}{2} \cdot \frac{s}{s^2 + 2^2} </m>
    	</answer>
		</li>
	</ol>
	</p>
	</li>
	
	<li>
	<p>
	Manipulate each of the following expressions into the form 
	<m>\quad \DS \frac{n!}{s^{n+1}}.</m>

	<ol>
		<li> <m>\DS \frac{1}{s^5} \quad </m> 		
    	<solution>		
    	<md>	
    		<mrow>\frac{1}{s^5}	\amp= \frac{1}{s^{4+1}}</mrow>
    		<mrow>\amp= \frac{4!}{4!} \cdot \frac{1}{s^{4+1}}</mrow>
    		<mrow>\amp= \frac{1}{4!}\cdot \frac{4!}{s^{4+1}}</mrow>
    		<mrow>\amp= \frac{1}{24}\cdot \frac{n!}{s^{n+1}}, \text{ where <m>n=4</m>}</mrow>
    	</md>
    	</solution>
    	<answer>
    		<m>\DS \frac{1}{24}\cdot \frac{4!}{s^{4+1}} </m>
    	</answer>
		</li>
	
		<li> <m>\DS \frac{7}{s^3} \quad </m>		
    	<solution>		
    	<md>	
    		<mrow>\frac{7}{s^3}	\amp= 7\cdot \frac{1}{s^{2+1}}</mrow>
    		<mrow>\amp= \frac{2!}{2!} \cdot 7 \cdot \frac{1}{s^{2+1}}</mrow>
    		<mrow>\amp= \frac{1}{2!}\cdot 7 \cdot \frac{2!}{s^{2+1}}</mrow>
    		<mrow>\amp= \frac{7}{2} \cdot \frac{2!}{s^{2+1}}</mrow>
    		<mrow>\amp= \frac{7}{2}\cdot \frac{n!}{s^{n+1}}, \text{ where <m>n=2</m>}</mrow>
    	</md>
    	</solution>
    	<answer>
    		<m>\DS \frac{7}{2}\cdot \frac{2!}{s^{2+1}} </m>
    	</answer>
		</li>
	
		<li> <m>\DS \frac{2}{5s^4} \quad </m>		
    	<solution>		
    	<md>	
    		<mrow>\frac{2}{5s^4}	\amp= \frac{2}{5}\cdot \frac{1}{s^{4}}</mrow>
    		<mrow>\amp= \frac{2}{5}\cdot \frac{1}{s^{3+1}}</mrow>
    		<mrow>\amp= \frac{3!}{3!} \cdot \frac{2}{5} \cdot \frac{1}{s^{3+1}}</mrow>
    		<mrow>\amp= \frac{1}{3!}\cdot \frac{2}{5} \cdot \frac{3!}{s^{3+1}}</mrow>
    		<mrow>\amp= \frac{1}{6}\cdot \frac{2}{5} \cdot \frac{3!}{s^{3+1}}</mrow>
    		<mrow>\amp= \frac{2}{30}\cdot \frac{3!}{s^{3+1}}</mrow>
    		<mrow>\amp= \frac{1}{15} \cdot \frac{3!}{s^{3+1}}</mrow>
    		<mrow>\amp= \frac{1}{15}\cdot \frac{n!}{s^{n+1}}, \text{ where <m>n=3</m>}</mrow>
    	</md>
    	</solution>
    	<answer>
    		<m>\DS \frac{1}{15} \cdot \frac{3!}{s^{3+1}} </m>
    	</answer>
		</li>
	</ol>
	</p>
	</li>
</ol>
</p>
</section>