<?xml version="1.0" encoding="UTF-8" ?>

<!-- 16-DEsReview_matching_forms_part2 -->

<section xml:id="r-01-16" xmlns:xi="http://www.w3.org/2001/XInclude">

<title>Matching Forms, Part 2</title>

<p>
Two other forms we may wish to match when we study Laplace transforms are
<me> \frac{b}{(s-a)^2 + b^2} \mbox{ and } \frac{s-a}{(s-a)^2 + b^2}. </me>
As before, we work toward <em> making the denominator match first</em>, and then we sort
out the numerator second.

</p>

<example xml:id="ex_matching_forms_part_2">
    <title>
    	Write <m>\DS\frac{s-6}{s^2 - 4s + 29}</m> in the form 
    	<m>\DS\frac{s-a}{(s-a)^2 + b^2}</m>
    </title>
    
    <p>
    If you prefer to see a video of this example, 
    <xref ref="video-matching_terms_02" text="custom"> click here </xref>
    </p>
        
    <p>
    <aside>
    Since <m>\DS\frac{s-6}{s^2 - 4s + 29}</m> has a quadratic function in the 
    denominator, it makes sense that we would try to match it with one of the 
    forms above, however, the form of the numerator suggests matching it with the 
    second expression.
    </aside>
    
    As we mentioned earlier, we'll try to make the denominator match first. Since both 
    of the forms we're trying to match are of the form <m>(s-a)^2 + b^2,</m> we will 
    complete the square first:
    
    	<me> s^2 - 4s + 29 = (s-2)^2 + 25. </me>
    
    (If you still don't remember how to complete the square, look up that primer and 
    do the previous exercises in that section above.)
    </p>
    
    <p>
    Let's rewrite the given expression as follows.
    	
    <md> 
    	<mrow>\frac{s-6}{s^2 - 4s + 29}	\amp= \frac{s-6}{(s-2)^2 + 25}			</mrow>
    	<mrow>							\amp= \frac{s-6}{(s-2)^2 + 5^2}			</mrow>
    </md>
    </p>
    
    <p>
    We've got the denominator in exactly the right form--it looks just like
    <m>(s-a)^2 + b^2,</m> with <m>a = 2</m> and <m>b = 5</m>. As in the previous 
    section, once we've gotten the denominator in shape, we turn our attention to 
    the numerator. If we look back at the two forms we are trying to match, we see 
    that our expression has an <m>s</m> in the numerator, so it's more like 
    <m>\DS \frac{s-a}{(s-a)^2 + b^2}</m>. It would be exactly right if we had
    <m>s-a</m> in the numerator, which in this case would be <m>s-2</m>.
    </p>
    
    <p>
    What we do have in the numerator is <m>s-6</m>; and we would like it to be 
    <m>s-2,</m> which means if we added 4, we'd have exactly the right thing. If we 
    want to add 4, we'll need to compensate by also subtracting 4, like this:
    	
    <md>
    	<mrow> \frac{s-6}{(s-2)^2 + 5^2}\amp= \frac{s-6+4-4}{(s-2)^2 + 5^2},	</mrow>
    	<mrow>							\amp= \frac{(s-6+4)-4}{(s-2)^2 + 5^2},	</mrow>
    	<mrow>							\amp= \frac{(s-2) - 4}{(s-2)^2 + 5^2}.	</mrow>
    </md>
    
    </p>
    
    <p>
    Great!  Now we can split this single fraction into two separate fractions:
    	
	<me> \frac{(s-2) - 4}{(s-2)^2 + 5^2} = 
		\underbrace{\frac{s-2}{(s-2)^2 + 5^2}}_{match!} - \frac{4}{(s-2)^2 + 5^2} </me>
    
    We're almost there!  The first fraction is a perfect match for the form 
    <m>\frac{s-a}{(s-a)^2 + b^2}</m> (with <m>a = 2</m> and <m>b = 5</m>); but we 
    still have another expression that is not yet a match. The remaining fraction 
    looks like it could eventually match the form <m>\frac{b}{(s-a)^2 + b^2}</m>.
    We would need to have a 5 in the numerator, and we currently have a 4. But we 
    can fix that as we did in the previous section:
    	
    <md>
    	<mrow>\frac{4}{(s-2)^2 + 5^2}	\amp= 4\cdot\frac{1}{(s-2)^2 + 5^2}		</mrow>
    	<mrow>							\amp= 4\cdot\frac{5}{5}\cdot 
														\frac{1}{(s-2)^2 + 5^2}	</mrow>
    	<mrow>							\amp= 4\cdot\frac{1}{5}\cdot 
														\frac{5}{(s-2)^2 + 5^2}	</mrow>
    	<mrow>							\amp= \frac{4}{5}\cdot 
														\frac{5}{(s-2)^2 + 5^2}	</mrow>
    </md>
    	
    Now let's put it all together. Here's everything we did:

    <md>	
    	<mrow>\frac{s-6}{s^2 - 4s + 9}	\amp= \frac{s-6}{(s-2)^2 + 25} \mbox{</mrow>
    							(we completed the square)}
    	<mrow>\amp= \frac{s-6}{(s-2)^2 + 5^2} \mbox{</mrow>
    							(we rewrote the denominator)}
    	<mrow>\amp=  \frac{s-6+4-4}{(s-2)^2 + 5^2} \mbox{</mrow>
    							(we added and subtracted 4 in the numerator...)}
    	<mrow>\amp= \frac{(s-2) - 4}{(s-2)^2 + 5^2} \mbox{</mrow>
    							(...so that we could make the numerator match part of the denom)}
    	<mrow>\amp= \frac{s-2}{(s-2)^2 + 5^2} - \frac{4}{(s-2)^2 + 5^2} \mbox{</mrow>
    							(split into fractions)}
    	<mrow>\amp= \frac{s-2}{(s-2)^2 + 5^2} - 4\cdot\frac{5}{5}\cdot \frac{1}{(s-2)^2 + 5^2}</mrow>
    							\mbox{(work on the second fraction...)}
    	<mrow>\amp= \frac{s-2}{(s-2)^2 + 5^2} - \frac{4}{5}\cdot \frac{5}{(s-2)^2 + 5^2}
    							\mbox{(...so now it is also in form)}
    							</mrow>
    </md>
    
    </p>
    
    <p>
    As mentioned before, being able to use appropriate algebra to 
    "match" forms is <em> really</em> important when we work with Laplace Transforms. Since it's really
    just algebra, now is a great time to practice that skill--so when we are in the middle of studying 
    Laplace Transforms, you can just focus on the "new" stuff.
    </p>
</example>

<p>
Now you try some!

<ol>
	<li> 
	<p>
	Manipulate each of the following expressions to make it match 
	the form <m>\DS \frac{b}{(s-a)^2 + b^2}</m> and/or <m>\DS \frac{s-a}{(s-a)^2 + b^2}.</m>
	<ol>	
		<li> <m>\DS \frac{s+3}{s^2 - 6s + 10}</m>		
		<solution>		
		<md>	
    		<mrow>\frac{s+3}{s^2 - 6s + 10}	\amp= \frac{s+3}{(s^2 - 6s) + 10}</mrow>
    		<mrow>\amp= \frac{s+3}{(s^2 - 6s + 9 - 9) + 10}</mrow>
    		<mrow>\amp= \frac{s+3}{(s^2 - 6s + 9) - 9 + 10}</mrow>
    		<mrow>\amp= \frac{s+3}{(s - 3)^2 - 9 + 10}</mrow>
    		<mrow>\amp= \frac{s+3}{(s - 3)^2 + 1}</mrow>
    		<mrow>\amp= \frac{s+3}{(s - 3)^2 + 1^2}</mrow>
    		<mrow>\amp= \frac{(s-3+3)+3}{(s - 3)^2 + 1^2}</mrow>
    		<mrow>\amp= \frac{(s-3)+3+3}{(s - 3)^2 + 1^2}</mrow>
    		<mrow>\amp= \frac{(s-3)+6}{(s - 3)^2 + 1^2}</mrow>
    		<mrow>\amp= \frac{s-3}{(s - 3)^2 + 1^2} +  \frac{6}{(s - 3)^2 + 1^2}</mrow>
    		<mrow>\amp= \frac{s-3}{(s - 3)^2 + 1^2} +  6\cdot \frac{1}{(s - 3)^2 + 1^2}						</mrow>
    		<mrow>\amp= \frac{s - a}{(s - a)^2 +b^2} + 6\cdot \frac{b}{(s - a)^2 +b^2}, 
    								\mbox{ where <m>a = 3</m> and <m>b = 1</m>}</mrow>
    	</md>
		</solution>
		<answer>
			<me>  \frac{s-3}{(s - 3)^2 + 1^2} +  6\cdot \frac{1}{(s - 3)^2 + 1^2} </me>
		</answer>
		</li>
	
		<li> <m>\DS \frac{s}{s^2 - 8s + 25}</m> 		
		<solution>		
		<md>	
    		<mrow>\frac{s}{s^2 - 8s + 25}	\amp= \frac{s}{(s^2 - 8s) + 25}</mrow>
    		<mrow>\amp= \frac{s}{(s^2 - 8s + 16 - 16) + 25}</mrow>
    		<mrow>\amp= \frac{s}{(s^2 - 8s + 16) - 16 + 25}</mrow>
    		<mrow>\amp= \frac{s}{(s - 4)^2 - 16 + 25}</mrow>
    		<mrow>\amp= \frac{s}{(s - 4)^2 +9}</mrow>
    		<mrow>\amp= \frac{s}{(s - 4)^2 +3^2}</mrow>
    		<mrow>\amp= \frac{(s - 4) + 4}{(s - 4)^2 +3^2}</mrow>
    		<mrow>\amp= \frac{s - 4}{(s - 4)^2 +3^2} + \frac{4}{(s - 4)^2 +3^2}</mrow>
    		<mrow>\amp= \frac{s - 4}{(s - 4)^2 +3^2} + 4\cdot \frac{1}{(s - 4)^2 +3^2}</mrow>
    		<mrow>\amp= \frac{s - 4}{(s - 4)^2 +3^2} + \frac{3}{3}\cdot 4\cdot \frac{1}{(s - 4)^2 +3^2}</mrow>
    		<mrow>\amp= \frac{s - 4}{(s - 4)^2 +3^2} + \frac{1}{3}\cdot 4\cdot \frac{3}{(s - 4)^2 +3^2}</mrow>
    		<mrow>\amp= \frac{s - 4}{(s - 4)^2 +3^2} + \frac{4}{3}\cdot \frac{3}{(s - 4)^2 +3^2}</mrow>
    		<mrow>\amp= \frac{s - a}{(s - a)^2 +b^2} + \frac{4}{3}\cdot \frac{b}{(s - a)^2 +b^2}, </mrow>
    								\mbox{ where <m>a = 4</m> and <m>b = 3</m>}
    	</md>
    	</solution>
    	<answer>
    		<me> \frac{s - 4}{(s - 4)^2 +3^2} + \frac{4}{3}\cdot \frac{3}{(s - 4)^2 +3^2} </me>
    		 
    	</answer>
		</li>
	
		<li> <m>\DS \frac{s}{s^2 + 8s + 25}</m>		
    	<solution>		
    	<md>	
    		<mrow>\frac{s}{s^2 + 8s + 25}	\amp= \frac{s}{(s^2 + 8s) + 25}</mrow>
    		<mrow>\amp= \frac{s}{(s^2 + 8s + 16 - 16) + 25}</mrow>
    		<mrow>\amp= \frac{s}{(s^2 + 8s + 16) - 16 + 25}</mrow>
    		<mrow>\amp= \frac{s}{(s + 4)^2 - 16 + 25}</mrow>
    		<mrow>\amp= \frac{s}{(s + 4)^2 +9}</mrow>
    		<mrow>\amp= \frac{s}{(s + 4)^2 +3^2}</mrow>
    		<mrow>\amp= \frac{(s + 4) - 4}{(s + 4)^2 +3^2}</mrow>
    		<mrow>\amp= \frac{s + 4}{(s + 4)^2 +3^2} - \frac{4}{(s + 4)^2 +3^2}</mrow>
    		<mrow>\amp= \frac{s + 4}{(s + 4)^2 +3^2} - 4\cdot \frac{1}{(s + 4)^2 +3^2}</mrow>
    		<mrow>\amp= \frac{s + 4}{(s + 4)^2 +3^2} - \frac{3}{3}\cdot 4\cdot \frac{1}{(s + 4)^2 +3^2}</mrow>
    		<mrow>\amp= \frac{s + 4}{(s + 4)^2 +3^2} - \frac{1}{3}\cdot 4\cdot \frac{3}{(s + 4)^2 +3^2}</mrow>
    		<mrow>\amp= \frac{s + 4}{(s + 4)^2 +3^2} - \frac{4}{3}\cdot \frac{3}{(s + 4)^2 +3^2}</mrow>
    		<mrow>\amp= \frac{s - a}{(s - a)^2 +b^2} - \frac{4}{3}\cdot \frac{b}{(s - a)^2 +b^2}, </mrow>
    								\mbox{ where <m>a = -4</m> and <m>b = 3</m>}
    	</md>
    		
    		
    	</solution>
    	<answer>
    		<me> \frac{s + 4}{(s + 4)^2 +3^2} - \frac{4}{3}\cdot \frac{3}{(s + 4)^2 +3^2} </me>
    		 
    	</answer>
		</li>
	
		<li> <m>\DS \frac{s-5}{s^2 +12s + 72}</m> 		
    	<solution>		
    	<md>	
    		<mrow>\frac{s-5}{s^2 +12s + 72}	\amp= \frac{s-5}{(s^2 +12s) + 72}</mrow>
    		<mrow>\amp=  \frac{s-5}{(s^2 +12s + 36 - 36) + 72}</mrow>
    		<mrow>\amp=  \frac{s-5}{(s^2 +12s + 36) - 36 + 72}</mrow>
    		<mrow>\amp=  \frac{s-5}{(s + 6)^2 - 36 + 72}</mrow>
    		<mrow>\amp=  \frac{s-5}{(s + 6)^2 + 36}</mrow>
    		<mrow>\amp=  \frac{s-5}{(s + 6)^2 + 6^2}</mrow>
    		<mrow>\amp=  \frac{(s+6-6)-5}{(s + 6)^2 + 6^2}</mrow>
    		<mrow>\amp=  \frac{(s+6)-6-5}{(s + 6)^2 + 6^2}</mrow>
    		<mrow>\amp=  \frac{(s+6)-11}{(s + 6)^2 + 6^2}</mrow>
    		<mrow>\amp=  \frac{s+6}{(s + 6)^2 + 6^2} + \frac{-11}{(s + 6)^2 + 6^2}</mrow>
    		<mrow>\amp=  \frac{s+6}{(s + 6)^2 + 6^2} -11\cdot \frac{1}{(s + 6)^2 + 6^2}</mrow>
    		<mrow>\amp=  \frac{s+6}{(s + 6)^2 + 6^2} - \frac{6}{6} \cdot 11\cdot \frac{1}{(s + 6)^2 + 6^2}</mrow>
    		<mrow>\amp=  \frac{s+6}{(s + 6)^2 + 6^2} - \frac{1}{6} \cdot 11\cdot \frac{6}{(s + 6)^2 + 6^2}</mrow>
    		<mrow>\amp=  \frac{s+6}{(s + 6)^2 + 6^2} - \frac{11}{6}\cdot \frac{6}{(s + 6)^2 + 6^2}</mrow>
    		<mrow>\amp= \frac{s - a}{(s - a)^2 +b^2} - \frac{11}{6}\cdot \frac{b}{(s - a)^2 +b^2}, </mrow>
    								\mbox{ where <m>a = -6</m> and <m>b = 6</m>}
    	</md>
    	</solution>
    	<answer>
    		<me> \frac{s+6}{(s + 6)^2 + 6^2} - \frac{11}{6}\cdot \frac{6}{(s + 6)^2 + 6^2} </me>
    	</answer>
		</li>
	</ol>
	</p>
	</li>

	<li> 
	<p>
	Now that's you've been practicing manipulating expressions to get them to match a particular,
	specific form, it's time to practice picking out which form an expression is most like.
	
	Find the form(s) on the right that best match the expression on the left. It may not be a perfect
	match, but could be manipulated (as we did above) to get into the correct form(s).
	<ol>
		<li> (EXAMPLE)  <m>\DS \frac{1}{(s-3)^5}</m>
		<answer> This best matches form F. </answer>
		</li>
	
		<li> <m>\DS \frac{12}{s^2 + 15}</m>%D
		</li>
	
		<li> <m>\DS \frac{7}{1-s}</m> %B
		</li>
	
		<li> <m>\DS \frac{-1}{s}</m> %A
		</li>
	
		<li> <m>\DS \frac{s-1}{s^2  + 4s + 1}</m> %forms G and H
		</li>
	
		<li> <m>\DS \frac{7}{2s^2}</m> %C
		</li>
	
		<li> <m>\DS \frac{s+2}{s^2 + 9}</m> %forms D and E
		</li>
	</ol>
	<ol>
		<li> <m>\DS \frac{1}{s}</m>
		</li>
	
		<li> <m>\DS \frac{1}{s-a}</m>
		</li>
	
		<li> <m>\DS \frac{n!}{s^{n+1}}</m>
		</li>
	
		<li> <m>\DS \frac{b}{s^2 + b^2}</m>
		</li>
	
		<li> <m>\DS \frac{s}{s^2 + b^2}</m>
		</li>
	
		<li> <m>\DS \frac{n!}{(s-a)^{n+1}}</m>
		</li>
	
		<li> <m>\DS \frac{b}{(s-a)^2 + b^2}</m>
		</li>
	
		<li> <m>\DS \frac{s-a}{(s-a)^2 + b^2}</m>
		</li>
	</ol>
	<solution>		
	<ol>
		<li> This best matches form F.
		
		</li>
	
		<li> This best matches form D.
	
		</li>
	
		<li> This best matches form B.
	
		</li>
	
		<li> This best matches form A.
	
		</li>
	
		<li> This best matches form forms G and H.
	
		</li>
	
		<li> This best matches form C.
	
		</li>
	
		<li> This best matches form forms D and E.
		</li>
	</ol>
	</solution>
	</p>
	</li>
</ol>
</p>
</section>