<section xmlns:xi="http://www.w3.org/2001/XInclude" xml:id="sec-lt-piecewise-funcs-pt2"><title>Solving DEs with Piecewise Functions</title>

	<p>
		Recall that we already had a solution technique (Undetermined Coefficients) that allowed us to solve linear DEs with constant coefficients, so long as the non-homogeneous part of the DE is continuous (and has a specific form).  We now finally have all of the tools we need to be able to solve DEs where the non-homogenous part is discontinuous.
	</p>

	<example xml:id="ex_solve_ivp_w_pw_func">
		<p>
			Solve the following initial value problem.
			<me> i''(t) + 4i(t) = g(t),  i(0) = 0,  i'(0) = 0, </me>
			where
			<me>
				g(t) = \left\{ 
				\begin{array}{ll}
					1,	\amp t \lt 1,\\
					-1,	\amp 1 \le t \lt 2,\\
					0,	\amp t \ge 2
				\end{array} \right.
			</me>
		</p>

		<p/>
		<solution>
			<p>
				We observe that this DE is linear and has constant coefficients. It is non-homogeneous, but the non-homogenous part of the DE, the function <m>g(t),</m> is a piecewise defined function.  As such, the only solution technique we have available in using Laplace transforms.

			</p>

			<p>
				In order to take the Laplace transform of the DE, we first need to rewrite <m>g(t)</m> in terms of unit step functions. (If you need to review this process, refer back to section NAME/NUMBER.)
				<me> g(t) = 1 - 2\ U(t-1) + U(t-2). </me>
				
			</p>

			<p>
				Thus, the DE can be written
				<me> i''(t) + 4i(t) = 1 - 2\ U(t-1) + U(t-2). </me>
			</p>

			<p>
				We take the Laplace transform of both sides of the DE, apply properties from our table, and use the provided initial conditions as follows.
				<md>
					<mrow>\LAP\{ i''(t) + 4i(t) \}	\amp= \LAP\{1 - 2\ U(t-1) + U(t-2)\}</mrow>
					<mrow>\LAP\{ i''(t)\} + \LAP\{4i(t) \}	\amp= \LAP\{1\} - 2\LAP\{U(t-1)\} + \LAP\{U(t-2)\}</mrow>
					<mrow>\Big[s^2 I(s) - s\cdot i(0) - i'(0)\Big] + 4I(s)	\amp= \frac{1}{s} - \frac{2e^{-s}}{s} + \frac{e^{-2s}}{s}</mrow>
					<mrow>\Big[s^2 I(s) - s\cdot 0 - \cdot 0\Big] + 4I(s)	\amp= \frac{1}{s}\Big[1 - 2e^{-s} + e^{-2s}\Big]</mrow>
					<mrow>s^2 I(s)+ 4I(s)	\amp= \frac{1}{s}\Big[1 - 2e^{-s} + e^{-2s}\Big]</mrow>
				</md>

			</p>

			<p>
				Next we solve for <m>I(s).</m>
				<md>
					<mrow>[s^2+ 4]I(s)	\amp= \frac{1}{s}\Big[1 - 2e^{-s} + e^{-2s}\Big]</mrow>
					<mrow>I(s)	\amp= \frac{1}{s(s^2 + 4)}\Big[1 - 2e^{-s} + e^{-2s}\Big]</mrow>
					<mrow>\amp= F(s)\cdot \Big[1 - 2e^{-s} + e^{-2s}\Big]</mrow>
					<mrow>\amp= F(s) - 2e^{-s}F(s) + e^{-2s}F(s),</mrow>
				</md>
			</p>

			<p>
				where <m>F(s) = \DS \frac{1}{s(s^2 + 4)}.</m>

			</p>

			<p>
				We see those exponentials which means we will need to use  <xref ref="LT-Table-L16" text="custom"><m>L16</m></xref> to find the inverse Laplace transform.  In order to do that, we also know that we will need the inverse Laplace transform of <m>F(s),</m> so we work on that, first.  We note that a partial fraction decomposition is needed.
				<md>
					<mrow>\frac{1}{s(s^2 + 4)}	\amp= \frac{A}{s} + \frac{Bs+C}{s^2 + 4}</mrow>
					<mrow>s(s^2 + 4) \cdot \frac{1}{s(s^2 + 4)}	\amp= \left[\frac{A}{s} + \frac{Bs+C}{s^2 + 4}\right]\cdot s(s^2 + 4)</mrow>
					<mrow>1	\amp= A(s^2 + 4) + (Bs+C)s</mrow>
					<mrow>1	\amp= As^2 + 4A + Bs^2 + Cs</mrow>
					<mrow>0s^2 + 0s + 1	\amp= (A+B)s^2 + Cs + 4A</mrow>
				</md>
				
				<md>
					<mrow>A+B	\amp= 0			\amp	C	\amp= 0	\amp	4A	\amp= 1</mrow>
					<mrow>\amp			\amp		\amp	\amp	A	\amp= \frac{1}{4}</mrow>
					<mrow>\frac{1}{4} + B	\amp= 0			\amp		\amp	\amp		\amp</mrow>
					<mrow>B	\amp= -\frac{1}{4}	\amp		\amp	\amp		\amp</mrow>
				</md>
			</p>

			<p>
				Therefore we have
				<me> F(s) = \frac{\frac{1}{4}}{s} - \frac{\frac{1}{4}s}{s^2 + 4}. </me>
				
			</p>

			<p>
				We now take the inverse Laplace transform.
				<md>
					<mrow>f(t)	\amp= \LAP^{-1}\left\{ F(s) \right\}</mrow>
					<mrow>\amp= \LAP^{-1}\left\{ \frac{\frac{1}{4}}{s} - \frac{\frac{1}{4}s}{s^2 + 4} \right\}</mrow>
					<mrow>\amp= \frac{1}{4}\LAP^{-1}\left\{ \frac{1}{s}\right\} - \frac{1}{4}\LAP^{-1}\left\{\frac{s}{s^2 + 2^2} \right\}</mrow>
					<mrow>\amp= \frac{1}{4}\cdot 1 - \frac{1}{4}\cos(2t)</mrow>
					<mrow>\amp= \frac{1}{4} - \frac{1}{4}\cos(2t)</mrow>
				</md>
				
			</p>

			<p>
				Now we are prepared to return to the actual question at hand.  We return to our equation for <m>I(s):</m>
				<me>I(s)	= F(s) - 2e^{-s}F(s) + e^{-2s}F(s).</me>
			</p>

			<p>
				We take the inverse Laplace transform, using  <xref ref="LT-Table-L16" text="custom"><m>L16</m></xref>.
				<md>
					<mrow>i(t)	\amp= \LAP^{-1}\left\{ F(s) - 2e^{-s}F(s) + e^{-2s}F(s) \right\}</mrow>
					<mrow>\amp= \LAP^{-1}\left\{ F(s) \right\} - 2\LAP^{-1}\left\{ e^{-s}F(s) \right\} + \LAP^{-1}\left\{ e^{-2s}F(s) \right\}</mrow>
					<mrow>\amp= f(t) - 2f(t-1)U(t-1) + f(t-2)U(t-2)</mrow>
					<mrow>\amp= \left[ \frac{1}{4} - \frac{1}{4}\cos(2t) \right]</mrow>
						- 2\left[ \frac{1}{4} - \frac{1}{4}\cos\Big(2(t-1)\Big) \right]U(t-1)
						+ \left[ \frac{1}{4} - \frac{1}{4}\cos\Big(2(t-2)\Big) \right]U(t-2)
				</md>

			</p>

			<p>
			(Maybe include here a graph of the solution...explain how the initial conditions are seen in the solution...and how the solution changes at <m>t = 1</m> and at <m>t = 2</m> because the external forcing function changes at those times...)
			</p>
		</solution>
	</example>

</section>