<section xmlns:xi="http://www.w3.org/2001/XInclude" xml:id="sec-lt-forward"><title> FORWARD </title>

	<introduction>

		<p>
			We can continue to use the definition to determine the Laplace transform, we notice more
			and more patterns.  We summarize some common properties in the table below.
		</p>

		<p>
			<table halign="center" xml:id="lt_table_L1-L13">
			<title><em> (Initial) Table of Laplace Transforms</em></title>
				<tabular top = "minor" left="minor" right="minor" halign="center" bottom="minor">
					<row>
						<cell/>
						<cell><m>f(t)</m></cell>
						<cell><m>F(s) = \LAP\{ f(t) \}</m></cell>
						<cell><m>Condition/Notes</m></cell>
					</row>
					<row>
						<cell><m>L1</m></cell><cell><m>1</m></cell><cell><m>\DS \frac{1}{s}</m></cell><cell><m>s>0</m></cell>
					</row>
					<row>
						<cell><m>L2</m></cell><cell><m>e^{at}</m></cell><cell><m>\DS \frac{1}{s-a}</m></cell><cell><m>s>a</m></cell>
					</row>
					<row>
						<cell><m>L3</m></cell><cell><m>t^n, \hspace{0.25cm}n = 1, 2, \ldots</m></cell><cell><m>\DS \frac{n!}{s^{n+1}}</m></cell><cell><m>s>0</m></cell>
					</row>
					<row>
						<cell><m>L4</m></cell><cell><m>\sin (bt)</m></cell><cell><m>\DS \frac{b}{s^2 + b^2}</m></cell><cell><m>s>0</m></cell>
					</row>
					<row>
						<cell><m>L5</m></cell><cell><m>\cos(bt)</m></cell><cell><m>\DS \frac{s}{s^2 + b^2}</m></cell><cell><m>s>0</m></cell>
					</row>
					<row>
						<cell><m>L6</m></cell><cell><m>t^n e^{at},  \hspace{0.25cm}n = 1, 2, \ldots</m></cell><cell><m>\DS \frac{n!}{(s-a)^{n+1}}</m></cell><cell><m>s>a</m></cell>
					</row>
					<row>
						<cell><m>L7</m></cell><cell><m>e^{at} \sin(bt)</m></cell><cell><m>\DS \frac{b}{(s-a)^2 + b^2}</m></cell><cell><m>s>a</m></cell>
					</row>
					<row>
						<cell><m>L8</m></cell><cell><m>e^{at} \cos(bt)</m></cell><cell><m>\DS \frac{s-a}{(s-a)^2 + b^2}</m></cell><cell><m>s>a</m></cell>
					</row>
					<row>
						<cell><m>L9</m></cell><cell><m>a f(t) + b g(t)</m></cell><cell><m>\DS a \LAP\{ f(t) \} + b \LAP\{ g(t) \}</m></cell><cell><m>a, b \text{ constant}</m></cell>
					</row>
					<row>
						<cell><m>L10</m></cell><cell><m>f'(t)</m></cell><cell><m>sF(s) - f(0)</m></cell><cell/>
					</row>
					<row>
						<cell><m>L11</m></cell><cell><m>f''(t)</m></cell><cell><m>s^2 F(s) - sf(0) - f'(0)</m></cell><cell/>
					</row>
					<row>
						<cell><m>L12</m></cell><cell><m>f^{(n)}(t)</m></cell><cell><m>s^n F(s) - s^{n-1}f(0) - s^{n-2}f'(0) - \cdots - f^{(n-1)}(0)</m></cell><cell/>
					</row>
					<row>
						<cell><m>L13</m></cell><cell><m>t^n f(t)</m></cell><cell><m>\DS (-1)^n\frac{d^n}{ds^n}\big( F(s) \big) = (-1)^nF^{(n)}(s)</m></cell><cell/>
					</row>
				</tabular>
			</table>

			<aside><p>Remove L12, narrow L13, make L9 a property box, move n=1,2,3,... to right column.</p></aside>

		<!-- INCORPORATE THIS INTO EXAMPLES/EXERCISES
			<tabular top = "minor" left="minor" right="minor" halign="center" bottom="minor">
				<row>
					<cell><m>L10</m></cell><cell><m>f'(t)</m></cell><cell><m>s\LAP\{ f(t) \} - f(0)</m></cell><cell/>
				</row>
				<row>
					<cell><m>L11</m></cell><cell><m>f''(t)</m></cell><cell><m>s\LAP\{ f'(t) \} - f'(0)</m></cell><cell/>
				</row>
				<row>
					<cell><m>L12</m></cell><cell><m>f^{(n)}(t)</m></cell><cell><m>s\LAP\{ f^{(n-1)}(t) \} - f^{(n-1)}(0)</m></cell><cell/>
				</row>
				<row>
					<cell><m>L13</m></cell><cell><m>t^n f(t)</m></cell><cell><m>\DS (-1)^n\frac{d^n}{ds^n}\big( \LAP\{ f(t) \} \big)</m></cell><cell/>
				</row>
			</tabular>
		-->

		</p>

		<p>
			This table can be enormously helpful to us as we take Laplace transforms; we save lots of time and effort by using this established table of properties instead of using the (admittedly laborious) definition of Laplace transform.  Let's practice this now.
		</p>
		
	</introduction>

	<example xml:id="ex_lt_using_table_01">
        <p>
            Find the Laplace transform of the function <m>y(t) = 15 - 4e^{9t} + 11t^3.</m>
        </p>

        <solution>
            <p>
                We will use properties in the table as follows.
                <md>
                    <mrow>Y(s)	\amp= \LAP\{ y(t) \}</mrow>
                    <mrow>\amp= \LAP\{ 15 - 4e^{9t} + 11t^3 \}</mrow>
                    <mrow>\amp= 15\LAP\{ 1 \} - 4\LAP\{ e^{9t} \} + 11\LAP\{ t^3 \} \qquad (<xref ref="LT-Table-L9" text="custom"><m>L9</m></xref>)</mrow>
                    <mrow>\amp= 15\cdot \UB{\frac{1}{s}}_{s \gt 0} 
                        - 4\cdot \UB{\frac{1}{s - 9}}_{s \gt 9} 
                        + 11 \cdot \UB{\frac{3!}{s^{3 + 1}}}_{s \gt 0} \qquad
                                (<xref ref="LT-Table-L1" text="custom"><m>L1</m></xref>, <xref ref="LT-Table-L2" text="custom"><m>L2</m></xref>, \, and \,<xref ref="LT-Table-L3" text="custom"><m>L3</m></xref>) </mrow>
                    <mrow>\amp= \frac{15}{s} - \frac{4}{s-9} + \frac{66}{s^4}, \hspace{0.5cm} s \gt 9 </mrow>
                </md>
            </p>
        </solution>
    </example>

    <example xml:id="ex_lt_using_table_02">
        <p>
            Find <m>\LAP \{ e^{3t}\sin(6t)  - t^3e^{-5t} \}.</m>
        </p>

        <solution>
            <p>
                We will use properties in the table as follows.
                <md>
                    <mrow>\amp=\LAP\{ e^{3t}\sin(6t)  - t^3e^{-5t} \}</mrow>
                    <mrow>\amp= \LAP\{ e^{3t}\sin(6t) \} - \LAP\{ t^2e^{-5t} \} \qquad (<xref ref="LT-Table-L9" text="custom"><m>L9</m></xref>) </mrow>
                    <mrow>\amp= \UB{\frac{6}{(s-3)^2 + 6^2}}_{s \gt 3} - \UB{\frac{2!}{\Big(s - (-5)\Big)^{2+1}}}_{s>-5} \qquad (<xref ref="LT-Table-L7" text="custom"><m>L7</m></xref>\, and \,<xref ref="LT-Table-L6" text="custom"><m>L6</m></xref>) </mrow>
                    <mrow>\amp= \frac{6}{(s-3)^2 + 36} - \frac{2}{(s+5)^3}, \hspace{0.5cm} s \gt 3</mrow>
                </md>
            </p>
        </solution>
    </example>

    <example xml:id="ex_lt_using_table_03">
        <p>
            Find the Laplace transform of the function <m>g(t) = t^2 \cos(8t).</m>
        </p>

        <solution>
            <p>
                Before we begin, we note that it's very tempting to think that because we know the Laplace transforms of both <m>t^2</m> and <m>\cos(8t),</m> we can simply multiply those together to get the desired Laplace transform. However,  this is not the case, just as similar statements were not true for finding the derivatives and integrals of the products of functions. Rather, we will need to use property <xref ref="LT-Table-L13" text="custom"><m>L13</m></xref>, with <m>n = 2</m> and <m>f(t) = \cos(8t).</m>
                <md>
                    <mrow>G(s)	\amp= \LAP\{ g(t) \}</mrow>
                    <mrow>\amp= \LAP\{ t^2 \cos(8t) \}</mrow>
                    <mrow>\amp= \LAP\{ t^2 f(t) \}</mrow>
                    <mrow>\amp= (-1)^2\cdot \frac{d^2}{ds^2}\big( F(s) \big)</mrow>
                </md>
            </p>

            <p>
                We need to know what <m>F(s)</m> is before we can proceed.  Let's go back to the naming system we have instituted.  If we have a capital <m>F(s),</m> that is the Laplace transform of a function lower case <m>f(t).</m>  We identified that function previously:  <m>f(t) = \cos(8t).</m> We use <xref ref="LT-Table-L5" text="custom"><m>L5</m></xref> to find its Laplace transform. 
                <me> F(s) = \frac{s}{s^2 + 64},  s>0 </me>
                Then we continue finding <m>G(s)</m> by taking two derivatives (using the quotient rule for derivatives; details are omitted here).
                <md>
                    <mrow>G(s)	\amp= (-1)^2\cdot \frac{d^2}{ds^2}\big( F(s) \big)</mrow>
                    <mrow>\amp= 1 \cdot \frac{d^2}{ds^2}\left( \frac{s}{s^2 + 64} \right)</mrow>
                    <mrow>\amp= \frac{d}{ds}\left( \frac{-s^2 + 64}{(s^2 + 64)^2} \right)</mrow>
                    <mrow>\amp= \frac{2s^3 + 128s}{(s^2 + 64)^3}</mrow>
                </md>
            </p>
        </solution>
    </example>
	
</section>