<section xmlns:xi="http://www.w3.org/2001/XInclude" xml:id="sec-lt-method-pt1"><title>Solving DEs via Laplace Transforms</title>

		<p>
			So far we've learned the definition of Laplace transform, developed a table so that we could more easily find Laplace transforms, and then figured out how to use the table to take inverse Laplace transforms. We are finally ready to use all of this to actually solve some DEs. First, let's refer once more to the roadmap <xref ref="LT-Diagram"/> we'll use when we solve DEs using this technique. 
		</p>

		<p>
			Before we begin, we should take note of when it's appropriate to use this technique. We can use Laplace transforms to solve DEs that are linear, have constant coefficients, and for which we have initial conditions. (We can relax this last condition if we want to, but for the most part we will focus on solving initial value problems.)
		</p>

		<example>
			<p>
				Solve the following initial value problem. <me> x'' - 4x' + 13x = 54e^{-t},  x(0) = 0,  x'(0) = 0 </me>
			</p>
			<solution>
				<p>
					We intend to use Laplace transforms to solve this IVP, but we need to verify that  this is an appropriate technique. We can verify that this is
					<ul>
						<li>
							the DE is linear, 
						</li>
						<li>
							the DE has constant coefficients, and
						</li>
						<li>
							initial conditions are <m>\DS x(0) = 0,  x'(0) = 0 </m>.
						</li>
				</ul>
				</p>

				<p>
					Hence, it is appropriate to proceed with the Laplace transform solution technique. We also note that <m>x</m> is the dependent variable and <m>t</m> is the independent variable, so our goal is to find a function <m>x(t)</m> that satisfies the DE and the initial conditions.
				</p>

				<aside>
					<p>
						Margin note:  We could actually use the method of undetermined coefficients. You are encouraged to do this and verify that the solution is the same.
					</p>
				</aside>

				<p>
					Following the <xref ref="LT-Diagram" text="custom">diagram</xref>, we begin by taking the Laplace transform of the DE. Let's look at some of the individual pieces.
					<ul>
						<li>
							We will need to take the Laplace transform of <m>x''</m>. Keep in mind that while it	is not explicitly written, we do know that <m>x</m> is a function of <m>t</m>, so this could be written <m>x''(t).</m>  For the first time, we will use  <xref ref="LT-Table-L11" text="custom"><m>L11</m></xref>, being careful with our naming convention.
							<me> \LAP\{ x'' \} = s^2X(s) - sx(0) - x'(0) </me>
						</li>
						<li>
							Similarly,
							<me> \LAP\{ x' \} = sX(s) - x(0). </me>
						</li>
						<li>
							We also need to be careful about taking the Laplace transform of <m>x</m> itself.	Since <m>x(t)</m> is our unknown function, we don't know what we get when we take its Laplace transform,  The only thing we can do is use the naming convention we have established:  the Laplace transform of a function <m>x(t)</m> is the function <m>X(s).</m> That is,
							<me> \LAP\{ x \} = X(s). </me>
						</li>
				</ul>
				</p>

				<p>
					With these facts in mind, we proceed to take the Laplace transform of both sides of the DE, using linearity as needed.
					<md>
						<mrow>\LAP\{x'' - 4x' + 13x\}	\amp= \LAP\{54e^{-t}\}</mrow>
						<mrow>\LAP\{x''\} - 4\LAP\{x'\} + 13\LAP\{x\}	\amp= 54\cdot\LAP\{e^{-t}\}</mrow>
						<mrow>\Big[s^2X(s) - sx(0) - x'(0) \Big] - 4\Big[ sX(s) - x(0) \Big] + 13X(s)	\amp= \frac{54}{s+1}</mrow>
					</md>
				</p>

				<p>
					We can use the provided initial conditions and then simplify the equation. 
					<md>
						<mrow>\Big[ s^2X(s) - s\cdot 0 - 0 \Big] - 4\Big[ sX(s) - 0 \Big] + 13X(s)	\amp= \frac{54}{s+1}</mrow>
						<mrow>s^2X(s)  - 4sX(s) + 13X(s)	\amp= \frac{54}{s+1}</mrow>
					</md>
				</p>

				<p>
					Now we are prepared to move on to the second step suggested in the roadmap in  (<xref ref="LT-Diagram" text="custom">the figure</xref>):  use algebra to solve for <m>X(s).</m>
					<md>
						<mrow>X(s)\Big[ s^2  - 4s + 13\Big]	\amp= \frac{54}{s+1}</mrow>
						<mrow>X(s)	\amp= \frac{54}{(s+1)(s^2  - 4s + 13)}</mrow>
					</md>
				</p>

				<p>
					The next step we need to take is to find the inverse Laplace transform of both sides of the equation.
					<md>
						<mrow>\LAP^{-1}\{X(s)\}	\amp= \LAP^{-1}\left\{\frac{54}{(s+1)(s^2  - 4s + 13)} \right\}</mrow>
						<mrow>x(t)	\amp=\LAP^{-1}\left\{\frac{54}{(s+1)(s^2  - 4s + 13)} \right\}</mrow>
					</md>
				</p>

				<p>
					We are almost done!  Our goal is to find the unknown function <m>x(t)</m>, and we have isolated <m>x(t)</m> on the left hand side of the equation. The only thing we have left to do is find the inverse Laplace transform of the right hand side. Here we refer back to the techniques we learned in the previous section. In particular, we are going to need to find the partial fraction decomposition of the rational function. First we note that the quadratic expression is irreducible, confirmed by the addition outside the parentheses when we complete the  square (which we will use later).
					<md>
						<mrow>s^2  - 4s + 13	\amp= (s^2  - 4s) + 13</mrow>
						<mrow>\amp= (s^2  - 4s + 4) + 13 - 4</mrow>
						<mrow>\amp= (s-2)^2 + 9</mrow>
						<mrow>\amp= (s-2)^2 + 3^2</mrow>
					</md>

				</p>

				<p>
					After applying partial fraction decomposition, we obtain 
					<!-- OMIT DETAILS
					has the form,
					<me> \frac{54}{(s+1)(s^2  - 4s + 13)} = \frac{A}{s+1} + \frac{Bs + C}{s^2 - 4s + 13}, </me>
					and we find <m>A</m>, <m>B</m>, and <m>C</m> by
					<md>
						<mrow>54	\amp= A(s^2 - 4s + 13) + (Bs+C)(s+1)</mrow>
						<mrow>54	\amp= As^2 - 4As + 13A + Bs^2 + Bs + Cs + C</mrow>
						<mrow>0s^2 + 0s + 54	\amp= (A + B)s^2 + (-4A + B + C)s + (13A + C)</mrow>
					</md>

					<md>
						<mrow>A+B	\amp= 0		\amp -4A +B+C	\amp= 0	\amp 	13A + C	\amp= 54</mrow>
						<mrow>A	\amp= -B	\amp			\amp	\amp			\amp</mrow>
						<mrow>\amp		\amp -4(-B)+B+C	\amp= 0	\amp 13(-B)+C	\amp= 54</mrow>
						<mrow>\amp		\amp 	5B + C	\amp= 0	\amp -13B + C	\amp= 54</mrow>
						<mrow>\amp		\amp		C	\amp= -5B	\amp		\amp</mrow>
						<mrow>\amp		\amp			\amp	\amp -13B + (-5B)	\amp= 54</mrow>
						<mrow>\amp		\amp			\amp	\amp 		-18B	\amp= 54</mrow>
						<mrow>\amp		\amp			\amp	\amp		B	\amp= -3</mrow>
						<mrow>A	\amp= -(-3)	\amp		C	\amp= -5(-3)\amp			\amp</mrow>
						<mrow>\amp= 3		\amp			\amp= 15\amp			\amp</mrow>
					</md>
					Hence,
					-->
					<me> \frac{54}{(s+1)(s^2  - 4s + 13)} = \frac{3}{s+1} + \frac{-3s + 15}{s^2 - 4s + 13}.</me>
				</p>

				<p>
					Now we proceed to do more algebraic manipulation to find the inverse Laplace transform. 
					<md>
						<mrow>
							x(t)	\amp= \LAP^{-1}\left\{\frac{54}{(s+1)(s^2  - 4s + 13)} \right\}
						</mrow>
						<mrow>
							\amp= \LAP^{-1}\left\{\frac{3}{s+1} + \frac{-3s + 15}{s^2 - 4s + 13} \right\}
						</mrow>
						<mrow>
							\amp= 3\cdot \LAP^{-1}\left\{\frac{1}{s+1}\right\} -3\cdot \LAP^{-1}\left\{\frac{s - 5}{s^2 - 4s + 13} \right\}
						</mrow>
						<mrow>
							\amp= 3e^{-t} - 3 \cdot \LAP^{-1}\left\{\frac{s - 5}{(s - 2)^2 + 3^2} \right\}
						</mrow>
						<mrow>
							\amp= 3e^{-t} - 3 \cdot \LAP^{-1}\left\{\frac{(s - 2) - 3}{(s - 2)^2 + 3^2} \right\}
						</mrow>
						<mrow>
							\amp= 3e^{-t} - 3 \cdot \LAP^{-1}\left\{\frac{s - 2}{(s - 2)^2 + 3^2} - \frac{3}{(s - 2)^2 + 3^2}\right\}
						</mrow>
						<mrow>
							\amp= 3e^{-t} - 3 \cdot \left[\LAP^{-1}\left\{\frac{s - 2}{(s - 2)^2 + 3^2} \right\} - \LAP^{-1}\left\{\frac{3}{(s - 2)^2 + 3^2}\right\} \right]
						</mrow>
						<mrow>
							\amp= 3e^{-t} - 3 \cdot \left[e^{2t}\cos(3t) - e^{2t}\sin(3t) \right]
						</mrow>
						<mrow>
							\amp= 3e^{-t} - 3e^{2t}\cos(3t) + 3e^{2t}\sin(3t)
						</mrow>
					</md>
				</p>

				<p>
					Thus, we have found the desired unknown function 
					<me> x(t) = 3e^{-t} - 3e^{2t}\cos(3t) + 3e^{2t}\sin(3t). </me>
					this isn't correct...?
				</p>

				<p>
					<xref ref="LT-Solving_w_LTs_verify_soln" text="custom">Optional: verify the solution.</xref>
				</p>

				<p>
					In this example, we used LTs to solve the differential equation with algebra, not integration. We then confirmed our solution was correct by verifying it satisfied both the original DE and the initial conditions.
				</p>
			</solution>
		</example>

		<p>
			In summary, if we have a DE that is linear, has constant coefficients,  and has initial conditions, we can solve using the Laplace transform solution technique. For the purposes of this discussion, we will assume that <m>t</m> is the independent variable and  that <m>y</m> is the dependent variable. We solve via the Laplace transform as follows.
			<ul>
				<li>
					Take the Laplace transform of the DE. This should yield an algebraic equation that contains <m>s</m>, <m>Y(s)</m> and the initial conditions <m>y(0),</m> <m>y'(0),</m> etc.
				</li>
				<li>
					Substitute in the given values for the initial conditions. 
				</li>
				<li>
					Use algebra to solve for <m>Y(s).</m>
				</li>
				<li>
					Take the inverse Laplace transform of both sides of the equation to yield the solution <m>y(t).</m>
				</li>
				<li>
					If desired, check that you have the correct solution by verifying that it satisfies the DE and the initial conditions.
				</li>
			</ul>
		</p>

	<example>
		<p>
		Solve 
		<me> y'' + 3y' + 2y = 4t,  y(0) = 1,  y'(0) = 0 </me>
		</p>
		<solution>
			<p>
				We intend to use Laplace transforms to solve this IVP, but we need to verify that  this is an appropriate technique. We can verify that this is
				<ul>
					<li>
						the DE is linear, 
					</li>
					<li>
						the DE has constant coefficients, and
					</li>
					<li>
						initial conditions are provided.
					</li>
				</ul>
			</p>

			<p>
				Hence, it is appropriate to proceed with the Laplace transform solution technique. We also note that <m>y</m> is the dependent variable and <m>t</m> is the independent variable, so our goal is to find a function <m>y(t)</m> that satisfies the DE and the initial conditions.
			</p>

			<aside>
				<p>
					Margin note:  We could actually use the method of undetermined coefficients. You are encouraged to do this and verify that the solution is the same.
				</p>
			</aside>

			<p>
				We begin by taking the Laplace transform of both sides of the DE, using linearity as needed.
				<md>
					<mrow>\LAP\{y'' + 3y' + 2y\}	\amp= \LAP\{ 4t \}</mrow>
					<mrow>\LAP\{y''\} + 3\LAP\{y'\} + 2\LAP\{y\}	\amp= 4\cdot\LAP\{ t \}</mrow>
					<mrow>\Big[s^2Y(s) - sy(0) - y'(0) \Big] + 3\Big[ sY(s) - y(0) \Big] + 2Y(s)	\amp= \frac{4}{s^2}</mrow>
				</md>
			</p>

			<p>
				Now we use the provided initial conditions. 
				<md>
					<mrow>\Big[s^2Y(s) - s\cdot 1 - 0 \Big] + 3\Big[ sY(s) - 1 \Big] + 2Y(s)	\amp= \frac{4}{s^2}</mrow>
					<mrow>s^2Y(s) - s  + 3sY(s) - 3 + 2Y(s)	\amp= \frac{4}{s^2}</mrow>
				</md>
			</p>

			<p>
				Next we will use algebra to solve for <m>Y(s).</m> 
				<md>
					<mrow>s^2Y(s)+ 3sY(s) + 2Y(s)	\amp= \frac{4}{s^2} + s + 3</mrow>
					<mrow>Y(s)\Big[ s^2 + 3s + 2 \Big]	\amp= \frac{4}{s^2} + \frac{s^3}{s^2} + \frac{3s^2}{s^2}</mrow>
					<mrow>\amp= \frac{4 + s^3 + 3s^2}{s^2}</mrow>
					<mrow>Y(s)	\amp= \frac{s^3 + 3s^2 + 4}{s^2(s^2 + 3s + 2)}</mrow>
					<mrow>\amp= \frac{s^3 + 3s^2 + 4}{s^2(s + 2)(s + 1)}</mrow>
				</md>
			</p>

			<p>
				We need to find the inverse Laplace transform of both sides of the equation. In order to do that, we apply partial fraction decomposition to the rational function on the right hand side, giving
				<me>\frac{s^3 + 3s^2 + 4}{s^2(s + 2)(s + 1)} = \frac{-3}{s} + \frac{2}{s^2} + \frac{-2}{s+2} + \frac{6}{s+1}.</me>
			</p>
				
				
			<!-- OMITTED PDF DETAILS
			<p>
				We have a repeated linear factor, <m>s^2</m>, and two other linear factors, so the form of the partial fraction decomposition can be written as
				<me> \frac{s^3 + 3s^2 + 4}{s^2(s + 2)(s + 1)} = \frac{A}{s} + \frac{B}{s^2} + \frac{C}{s+2} + \frac{D}{s+1} </me>
			</p>

			<p>
				(PFD details...can be omitted?) 
				<md>
					<mrow>s^3 + 3s^2 + 4	\amp= A(s)(s+2)(s+1) + B(s+2)(s+1) + C(s^2)(s+1) + D(s^2)(s+2)</mrow>
					<mrow>\amp= As(s^2 + 3s + 2) + B(s^2 + 3s + 2) + Cs^3 + Cs^2 + Ds^3 + 2Ds^2</mrow>
					<mrow>\amp= As^3 + 3As^2 + 2As + Bs^2 + 3Bs + 2B + Cs^3 + Cs^2 + Ds^3 + 2Ds^2</mrow>
					<mrow>s^3 + 3s^2 + 0s + 4	\amp= (A + C + D)s^3 + (3A + B + C+ 2D)s^2 + (2A + 3B)s + (2B)</mrow>
				</md>

				<md>
					<mrow>A+C+D	\amp= 1		\amp 3A+B+C+2D	\amp= 3	\amp 	2A+3B	\amp= 0		\amp 2B	\amp= 4</mrow>
					<mrow>\amp		\amp			\amp	\amp			\amp		\amp B	\amp= 2</mrow>
					<mrow>\amp		\amp 3A+2+C+2D	\amp= 3	\amp	2A+ 3(2)	\amp= 0		\amp	\amp</mrow>
					<mrow>\amp		\amp 3A+C+2D	\amp= 1	\amp		2A	\amp= -6	\amp	\amp</mrow>
					<mrow>\amp		\amp			\amp	\amp		A	\amp= -3	\amp	\amp</mrow>
					<mrow>-3+C+D	\amp= 1		\amp 3(-3)+C+ 2D	\amp= 1	\amp			\amp		\amp	\amp</mrow>
					<mrow>C+D	\amp= 4		\amp	C+2D	\amp= 10 \amp			\amp		\amp	\amp</mrow>
					<mrow>C	\amp= 4 - D	\amp			\amp	\amp			\amp		\amp	\amp</mrow>
					<mrow>\amp		\amp (4-D) + 2D	\amp= 10 \amp			\amp		\amp	\amp</mrow>
					<mrow>\amp		\amp 	4 + D	\amp= 10 \amp			\amp		\amp	\amp</mrow>
					<mrow>\amp		\amp		D	\amp= 6	\amp			\amp		\amp	\amp</mrow>
					<mrow>C	\amp= 4-6	\amp			\amp	\amp			\amp		\amp	\amp</mrow>
					<mrow>\amp= -2	\amp			\amp	\amp			\amp		\amp	\amp</mrow>
				</md>
			</p>

			<p>
				Hence, we have 
				<me>\frac{s^3 + 3s^2 + 4}{s^2(s + 2)(s + 1)} = \frac{-3}{s} + \frac{2}{s^2} + \frac{-2}{s+2} + \frac{6}{s+1} </me>
			</p>
			-->

			<p>
				Now we are prepared to take the inverse Laplace transform. 
				<md>
					<mrow>Y(s)	\amp= \frac{-3}{s} + \frac{2}{s^2} + \frac{-2}{s+2} + \frac{6}{s+1}</mrow>
				\LAP^{-1}\left\{ Y(s) \right\}	
					<mrow>\amp= \LAP^{-1}\left\{ \frac{-3}{s} + \frac{2}{s^2} + \frac{-2}{s+2} + \frac{6}{s+1} \right\}</mrow>
					<mrow>y(t)	\amp= -3\cdot\LAP^{-1}\left\{ \frac{1}{s} \right\}</mrow> 
						+ 2\LAP^{-1}\left\{ \frac{1}{s^2} \right\}
						- 2\cdot \LAP^{-1}\left\{ \frac{1}{s+2} \right\}
						+ 6 \cdot \LAP^{-1}\left\{ \frac{1}{s+1} \right\}
					<mrow>\amp= -3 + 2t - 2e^{-2t} + 6e^{-t}</mrow>
				</md>
			</p>

			<p>
				Thus, we have found the desired unknown function 
				<me> y(t) = -3 + 2t - 2e^{-2t} + 6e^{-t}. </me>
			</p>

			<p>
				Optional:  verify the solution 
				<md>
					<mrow>y'(t)	\amp= 0 + 2 + 4e^{-2t} - 6e^{-t}</mrow>
					<mrow>y''(t)	\amp= 0 - 8e^{-2t}+ 6e^{-t}</mrow>
				</md>
				
				<md>
					<mrow>LHS	\amp= y'' + 3y' + 2y</mrow>
					<mrow>\amp= \left( - 8e^{-2t}+ 6e^{-t} \right) </mrow>
						+ 3\left( 2 + 4e^{-2t} - 6e^{-t} \right) 
						+ 2\left( -3 + 2t - 2e^{-2t} + 6e^{-t} \right)		
					<mrow>\amp= -8e^{-2t}+ 6e^{-t}</mrow>
						+ 6 + 12e^{-2t} - 18e^{-t}
						- 6 + 4t - 4e^{-2t} + 12e^{-t}
					<mrow>\amp= 4t</mrow>
					<mrow>\amp= RHS</mrow>
				</md>
			</p>

			<p>
				We also verify the initial conditions: 
				<md>
					<mrow>y(0)	\amp= -3 + 2(0) - 2e^{-2(0)} + 6e^{-0}</mrow>
					<mrow>\amp= -3 + 0 - 2+ 6</mrow>
					<mrow>\amp= 1</mrow>
					<mrow>\amp</mrow>
					<mrow>y'(0)	\amp= 2 + 4e^{-2(0)} - 6e^{-0}</mrow>
					<mrow>\amp= 2 + 4 - 6</mrow>
					<mrow>\amp= 0</mrow>
				</md>
			</p>

		</solution>
	</example>

</section>