<subsection xml:id="s-zz-extra_stuff" xmlns:xi="http://www.w3.org/2001/XInclude">

    <paragraphs xml:id="std_LT_01">
    <title/>
        <aside>
            <p>
                Key Steps
                <me>
                    \begin{array}{ll}
                        (1) \amp \text{IBP with }\\
                            \amp u = t^2, dv = e^{-st} dt\\
                        (2) \amp \text{factor out } -\frac{1}{s}\\
                        (3) \amp \text{definition of the}\\
                            \amp \text{Laplace transform of } t\\
                        (4) \amp \text{convert evaluation at } \infty\\
                            \amp \text{to the limit at } \infty \\
                        (5) \amp \text{L'Hopital's Rule }\\
                    \end{array}
                </me>
            </p>
        </aside>
        <md>
            <mrow> \LAP\{ t^2 \}	
                    \amp= \int_0^{\infty} e^{-st}\cdot t^2 dt 				</mrow>
            <mrow>  \amp\OS{(1)}{=} t^2 \cdot -\frac{1}{s}e^{-st}\Bigg|_0^{\infty}
                        - \int_0^{\infty} -\frac{1}{s}e^{-st}\cdot 2tdt </mrow>
            <mrow>  \amp\OS{(2)}{=} -\frac{1}{s}\left[ t^2e^{-st}\Bigg|_0^{\infty}
                        - 2\int_0^{\infty}e^{-st}\cdot tdt \right]		</mrow>
            <mrow>  \amp\OS{(3)}{=} -\frac{1}{s}\left[t^2e^{-st}\Bigg|_0^{\infty}
                        - 2\LAP\{ t \} \right]							</mrow>
            <mrow>  \amp\OS{(4)}{=} -\frac{1}{s}\left[ \lim_{b \to \infty}
                        t^2e^{-st}\Bigg|_0^{b} - 2\LAP\{ t \} \right]		</mrow>
            <mrow>  \amp= -\frac{1}{s}\left[ \lim_{b \to \infty}
                        \left( b^2e^{-sb} - 0^2\cdot e^{-s\cdot 0} \right)
                        - 2\cdot \frac{1}{s^2} \right]					</mrow>
            <mrow>  \amp= -\frac{1}{s}\left[ \lim_{b \to \infty}
                        b^2e^{-sb} - 0 - \frac{2}{s^2} \right]			</mrow>
            <mrow>  \amp= -\frac{1}{s}\left[ \lim_{b \to \infty}
                        \frac{b^2}{e^{sb}} - \frac{2}{s^2} \right]		</mrow>
            <mrow>  \amp\OS{(5)}{=} -\frac{1}{s}\left[ \lim_{b \to \infty}
                        \frac{2b}{se^{sb}} - \frac{2}{s^2} \right]		</mrow>
            <mrow>  \amp= -\frac{1}{s}\left[ \frac{2}{s}\lim_{b \to \infty}
                        \frac{b}{e^{sb}} - \frac{2}{s^2} \right]		</mrow>
            <mrow>  \amp= -\frac{1}{s}\left[ \frac{2}{s}\lim_{b \to \infty}
                        \frac{1}{se^{sb}} - \frac{2}{s^2} \right]		</mrow>
            <mrow>  \amp= -\frac{1}{s}\left[ \frac{2}{s}\cdot 0
                        - \frac{2}{s^2} \right]							</mrow>
            <mrow>  \amp= \frac{2}{s^3} 									</mrow>
        </md>
    </paragraphs>

    <paragraphs xml:id="std_LT_02">
    <title/>
        <aside>
            <p>
                Key Steps
                <me>
                    \begin{array}{ll}
                        (1) \amp \text{IBP with }\\
                            \amp u = t^3, dv = e^{-st} dt\\
                        (2) \amp \text{factor out } -\frac{1}{s}\\
                        (3) \amp \text{definition of the}\\
                            \amp \text{Laplace transform of } t\\
                        (4) \amp \text{convert evaluation at } \infty\\
                            \amp \text{to the limit at } \infty \\
                        (5) \amp \text{L'Hopital's Rule }\\
                    \end{array}
                </me>
            </p>
        </aside>
        <md>
            <mrow> \LAP\{ t^3 \}	
                    \amp= \int_0^{\infty} e^{-st}\cdot t^3 dt </mrow>
            <mrow>  \amp\OS{(1)}{=} t^3 \cdot -\frac{1}{s}e^{-st}\Bigg|_0^{\infty} - \int_0^{\infty} -\frac{1}{s}e^{-st}\cdot 3t^2dt </mrow>
            <mrow>  \amp\OS{(2)}{=} -\frac{1}{s}\left[ t^3e^{-st}\Bigg|_0^{\infty} - 3\int_0^{\infty}e^{-st}\cdot t^2 dt \right]</mrow>
            <mrow>  \amp\OS{(3)}{=} -\frac{1}{s}\left[ \lim_{b \to \infty}t^3 e^{-st}\Bigg|_0^{b} - 3\LAP\{ t^2 \} \right]</mrow>
            <mrow>  \amp\OS{(4)}{=} -\frac{1}{s}\left[ \lim_{b \to \infty}\left( b^3 e^{-sb} - 0^3\cdot e^{-s\cdot 0} \right) - 3\cdot \frac{2}{s^3} \right]</mrow>
            <mrow>  \amp= -\frac{1}{s}\left[ \lim_{b \to \infty}b^3 e^{-sb} - 0 - \frac{6}{s^3} \right]</mrow>
            <mrow>  \amp= -\frac{1}{s}\left[ \lim_{b \to \infty}\frac{b^3}{e^{sb}} - \frac{6}{s^3} \right]</mrow>
            <mrow>  \amp\OS{(5)}{=} -\frac{1}{s}\left[ \lim_{b \to \infty}\frac{3b^2}{se^{sb}} - \frac{6}{s^3} \right]</mrow>
            <mrow>  \amp= -\frac{1}{s}\left[ \frac{3}{s}\lim_{b \to \infty}\frac{b^2}{e^{sb}} - \frac{6}{s^3} \right]</mrow>
            <mrow>  \amp= -\frac{1}{s}\left[ \frac{3}{s}\lim_{b \to \infty}\frac{2b}{se^{sb}} - \frac{6}{s^3} \right]</mrow>
            <mrow>  \amp= -\frac{1}{s}\left[ \frac{6}{s^2}\lim_{b \to \infty}\frac{b}{e^{sb}} - \frac{6}{s^3} \right]</mrow>
            <mrow>  \amp= -\frac{1}{s}\left[ \frac{6}{s^2}\lim_{b \to \infty}\frac{1}{se^{sb}} - \frac{6}{s^3} \right]</mrow>
            <mrow>  \amp= -\frac{1}{s}\left[ \frac{6}{s^2}\cdot 0 - \frac{6}{s^3} \right]</mrow>
            <mrow>  \amp= \frac{6}{s^4} </mrow>
        </md>
    </paragraphs>

    <paragraphs xml:id="std_LT_03">
    <title/>
        <aside>
            <p>
                Key Steps
                <me>
                    \begin{array}{ll}
                        (1) \amp \text{IBP with }\\
                            \amp u = t^4, dv = e^{-st} dt\\
                        (2) \amp \text{factor out } -\frac{1}{s}\\
                        (3) \amp \text{definition of the}\\
                            \amp \text{Laplace transform of } t\\
                        (4) \amp \text{convert evaluation at } \infty\\
                            \amp \text{to the limit at } \infty \\
                        (5) \amp \text{L'Hopital's Rule }\\
                    \end{array}
                </me>
            </p>
        </aside>
        <md>
            <mrow> \LAP\{ t^4 \}	
                    \amp= \int_0^{\infty} e^{-st}\cdot t^4 dt </mrow>
            <mrow>  \amp\OS{(1)}{=} t^4 \cdot -\frac{1}{s}e^{-st}\Bigg|_0^{\infty} - \int_0^{\infty} -\frac{1}{s}e^{-st}\cdot 4t^3dt</mrow>
            <mrow>  \amp\OS{(2)}{=} -\frac{1}{s}\left[ t^4e^{-st}\Bigg|_0^{\infty} - 4\int_0^{\infty}e^{-st}\cdot t^3 dt \right]</mrow>
            <mrow>  \amp\OS{(3)}{=} -\frac{1}{s}\left[ \lim_{b \to \infty}t^4 e^{-st}\Bigg|_0^{b} - 4\LAP\{ t^3 \} \right]</mrow>
            <mrow>  \amp\OS{(4)}{=} -\frac{1}{s}\left[ \lim_{b \to \infty}\left( b^4 e^{-sb} - 0^4\cdot e^{-s\cdot 0} \right) - 4\cdot \frac{6}{s^4} \right]</mrow>
            <mrow>  \amp= -\frac{1}{s}\left[ \lim_{b \to \infty}b^4 e^{-sb} - 0 - \frac{24}{s^4} \right]</mrow>
            <mrow>  \amp= -\frac{1}{s}\left[ \lim_{b \to \infty}\frac{4b^3}{se^{sb}} - \frac{24}{s^4} \right]</mrow>
            <mrow>  \amp= -\frac{1}{s}\left[ \frac{4}{s}\lim_{b \to \infty}\frac{b^3}{e^{sb}} - \frac{24}{s^4} \right]</mrow>
            <mrow>  \amp\OS{(5)}{=} -\frac{1}{s}\left[ \frac{4}{s}\lim_{b \to \infty}\frac{3b^2}{se^{sb}} - \frac{24}{s^4} \right]</mrow>
            <mrow>  \amp= -\frac{1}{s}\left[ \frac{12}{s^2}\lim_{b \to \infty}\frac{b^2}{e^{sb}} - \frac{24}{s^4} \right]</mrow>
            <mrow>  \amp= -\frac{1}{s}\left[ \frac{12}{s^2}\lim_{b \to \infty}\frac{2b}{se^{sb}} - \frac{24}{s^4} \right]</mrow>
            <mrow>  \amp= -\frac{1}{s}\left[ \frac{24}{s^3}\lim_{b \to \infty}\frac{b}{e^{sb}} - \frac{24}{s^4} \right]</mrow>
            <mrow>  \amp= -\frac{1}{s}\left[ \frac{24}{s^3}\lim_{b \to \infty}\frac{1}{se^{sb}} - \frac{24}{s^4} \right]</mrow>
            <mrow>  \amp= -\frac{1}{s}\left[ \frac{24}{s^3}\cdot 0 - \frac{24}{s^4} \right]</mrow>
            <mrow>  \amp= \frac{24}{s^5}</mrow>
        </md>
    </paragraphs>

    <paragraphs xml:id="tyu_intro_01_C"> <title/>
        Yes, good job!
    </paragraphs>

    <paragraphs xml:id="tyu_intro_01_I"> <title/>
        No, that's incorrect. The dependent variable is always the variable with the derivative.
    </paragraphs>

    <md>
        <mrow xml:id="LT-Table-L1">
            \amp L1: \quad \DS \LAP\{ 1 \} = \frac{1}{s}, \quad s>0
        </mrow>
    </md>
    <md>
        <mrow xml:id="LT-Table-L2">
            \amp L2: \quad \DS \LAP\{ e^{at} \} = \frac{1}{s-a}, \quad s>a
        </mrow>
    </md>
    <md>
        <mrow xml:id="LT-Table-L3">
            \amp L3: \quad \DS \LAP\{ t^n \} = \frac{n!}{s^{n+1}}, \quad s>0
        </mrow>
    </md>
    <md>
        <mrow xml:id="LT-Table-L4">
            \amp L4: \quad \DS \LAP\{ \sin (bt) \} = \frac{b}{s^2 + b^2}, \quad s>0
        </mrow>
    </md>
    <md>
        <mrow xml:id="LT-Table-L5">
            \amp L5: \quad \DS \LAP\{ \cos(bt) \} = \frac{s}{s^2 + b^2}, \quad s>0
        </mrow>
    </md>
    <md>
        <mrow xml:id="LT-Table-L6">
            \amp L6: \quad \DS \LAP\{ t^n e^{at} \} = \frac{n!}{(s-a)^{n+1}}, \quad s>a 
        </mrow>
    </md>
    <md>
        <mrow xml:id="LT-Table-L7">
            \amp L7: \quad \DS \LAP\{ e^{at} \sin(bt) \} = \frac{b}{(s-a)^2 + b^2}, \quad s>a
        </mrow>
    </md>
    <md>
        <mrow xml:id="LT-Table-L8">
            \amp L8: \quad \DS \LAP\{ e^{at} \cos(bt) \} = \frac{s-a}{(s-a)^2 + b^2}, \quad s>a
        </mrow>
    </md>
    <md>
        <mrow xml:id="LT-Table-L9">
            \amp L9: \quad \DS \LAP\{ a f(t) + b g(t) \} = a \LAP\{ f(t) \} + b \LAP\{ g(t) \}, \quad a, b \text{ constant}
        </mrow>
    </md>
    <md>
        <mrow xml:id="LT-Table-L10">
            \amp L10: \quad \DS \LAP\{ f'(t) \} = sF(s) - f(0)
        </mrow>
    </md>
    <md>
        <mrow xml:id="LT-Table-L11">
            \amp L11: \quad \DS \LAP\{ f''(t) \} = s^2 F(s) - sf(0) - f'(0)			
        </mrow>
    </md>
    <md>
        <mrow xml:id="LT-Table-L12">
            \amp L12: \quad \DS \LAP\{ f^{(n)}(t) \} = s^n F(s) - s^{n-1}f(0) - s^{n-2}f'(0) - \cdots - f^{(n-1)}(0)
        </mrow>
    </md>
    <md>
        <mrow xml:id="LT-Table-L13">
            \amp L13: \quad \DS \LAP\{ t^n f(t) \} = (-1)^n\frac{d^n}{ds^n}\big( \LAP\{ t^n f(t) \} \big)
        </mrow>
    </md>
    <md>
        <mrow xml:id="LT-Table-L14">
            \amp L14: \quad \DS \LAP\{ U(t-a) \} = \frac{e^{-as}}{s}
        </mrow>
    </md>
    <md>
        <mrow xml:id="LT-Table-L15">
            \amp L15: \quad \DS \LAP\{ f(t) U(t-a) \} = e^{-as} \LAP\{ f(t+a) \}
        </mrow>
    </md>
    <md>
        <mrow xml:id="LT-Table-L16">
            \amp L16: \quad \DS \LAP\{ f(t-a)U(t-a) \} = e^{-as}F(s)
        </mrow>
    </md>

    <paragraphs xml:id="LT-Table-L14-L16">
    <title/>
        <md>
            <mrow>\amp L14: \quad \DS \LAP\{ U(t-a) \} = \frac{e^{-as}}{s}</mrow>
            <mrow>\amp L15: \quad \DS \LAP\{ f(t) U(t-a) \} = e^{-as} \LAP\{ f(t+a) \}</mrow>
            <mrow>\amp L16: \quad \DS \LAP\{ f(t-a)U(t-a) \} = e^{-as}F(s)</mrow>
        </md>
    </paragraphs>

    <paragraphs xml:id="LT-PDF-Details-01">
    <title/>
        <p>
            <md>
                <mrow>4s^3 \amp - 13s^2 + 74s + 27</mrow>
                <mrow>\amp= (As + B)(s+1)^2 + C(s+1)(s^2 - 6s + 25) + D(s^2 - 6s + 25)</mrow>
                <mrow>
                    \amp= (As + B)(s^2 + 2s + 1) + (Cs+C)(s^2 - 6s + 25) + Ds^2 - 6Ds + 25D
                </mrow> 
                <mrow>
                    \amp= As^3 + 2As^2 + As  + Bs^2 + 2Bs + B + Cs^3 - 6Cs^2 + 25Cs + Cs^2 - 6Cs + 25C + Ds^2 - 6Ds + 25D
                </mrow> 
                <mrow>
                    \amp= (A + C)s^3 + (2A+ B - 6C + C + D)s^2 + (A+ 2B + 25C- 6C- 6D)s + (B + 25C + 25D)
                </mrow> 
                <mrow>
                    \amp= (A + C)s^3 + (2A+ B - 5C + D)s^2 + (A+ 2B + 19C- 6D)s + (B + 25C + 25D)
                </mrow> 
           </md>
        </p>

        <p>
            Equating coefficients gives us four equations in four unknowns.
            <md>
                <mrow>
                A+C	\amp= 4	\amp	2A+B-5C+D	\amp= -13	\amp A + 2B + 19C - 6D	\amp= 74 \amp B+ 25C + 25D \amp= 27
                </mrow>
                <mrow>	A	\amp= 4-C\amp				\amp		\amp				\amp		\amp\amp</mrow>
                <mrow>		 \amp	\amp 2(4 - C)+B-5C+D	\amp= -13	\amp (4-C)+2B+19C-6D	\amp= 74	\amp\amp</mrow>
                <mrow>		 \amp	\amp 	B - 7C + D	\amp= -21	\amp 	2B+18C-6D	\amp= 70	\amp\amp</mrow>
                <mrow>		 \amp	\amp	B	\amp= 7C - D - 21		\amp				\amp		\amp\amp</mrow>
                <mrow>		 \amp	\amp				\amp	\amp 2(7C - D - 21)+18C-6D	\amp= 70	\amp</mrow> 
                <mrow>		 (7C - D - 21) + 25C + 25D	\amp= 27</mrow>
                <mrow>		 \amp	\amp				\amp		\amp		32C-8D	\amp= 112	\amp</mrow>
                <mrow>		 32C + 24D	\amp= 48</mrow>
                <mrow>		 \amp	\amp				\amp		\amp 			32C	\amp= 8D + 112 \amp\amp</mrow>
                <mrow>		 \amp	\amp				\amp		\amp				\amp		\amp</mrow>
                <mrow>		 (8D + 112) + 24D	\amp= 48</mrow>
                <mrow>		 \amp	\amp				\amp		\amp				\amp		\amp</mrow>
                <mrow>		 32D	\amp= -64</mrow>
                <mrow>		 \amp	\amp				\amp		\amp				\amp		\amp</mrow>
                <mrow>		 D	\amp= -2</mrow>
                <mrow>		 \amp	\amp				\amp		\amp 			32C	\amp= 8(-2) + 112 \amp\amp</mrow>
                <mrow>		 \amp	\amp				\amp		\amp				\amp= 96	\amp\amp</mrow>
                <mrow>		 \amp	\amp				\amp		\amp			C	\amp= 3		\amp\amp</mrow>
                <mrow>		 \amp	\amp	B	\amp= 7(3) - (-2) - 21\amp	\amp				\amp		\amp\amp</mrow>
                <mrow>		 \amp	\amp		\amp= 2		\amp		\amp				\amp		\amp\amp</mrow>
                <mrow>	A	\amp= 4 - (3)\amp	\amp		\amp		\amp				\amp		\amp\amp</mrow>
                <mrow>		\amp= 1	\amp		\amp		\amp		\amp				\amp		\amp\amp</mrow>
            </md>
        </p>
    </paragraphs>

    <paragraphs xml:id="LT-PDF-Details-02">
    <title/>
    	<p>
            Partial fraction decomposition has the form,
            <me> \frac{54}{(s+1)(s^2  - 4s + 13)} = \frac{A}{s+1} + \frac{Bs + C}{s^2 - 4s + 13}, </me>
            and we find <m>A</m>, <m>B</m>, and <m>C</m> by
			<md>
				<mrow>54	\amp= A(s^2 - 4s + 13) + (Bs+C)(s+1)</mrow>
				<mrow>54	\amp= As^2 - 4As + 13A + Bs^2 + Bs + Cs + C</mrow>
				<mrow>0s^2 + 0s + 54	\amp= (A + B)s^2 + (-4A + B + C)s + (13A + C)</mrow>
			</md>

			<md>
				<mrow>A+B	\amp= 0		\amp -4A +B+C	\amp= 0	\amp 	13A + C	\amp= 54</mrow>
				<mrow>A	\amp= -B	\amp			\amp	\amp			\amp</mrow>
				<mrow>\amp		\amp -4(-B)+B+C	\amp= 0	\amp 13(-B)+C	\amp= 54</mrow>
				<mrow>\amp		\amp 	5B + C	\amp= 0	\amp -13B + C	\amp= 54</mrow>
				<mrow>\amp		\amp		C	\amp= -5B	\amp		\amp</mrow>
				<mrow>\amp		\amp			\amp	\amp -13B + (-5B)	\amp= 54</mrow>
				<mrow>\amp		\amp			\amp	\amp 		-18B	\amp= 54</mrow>
				<mrow>\amp		\amp			\amp	\amp		B	\amp= -3</mrow>
				<mrow>A	\amp= -(-3)	\amp		C	\amp= -5(-3)\amp			\amp</mrow>
				<mrow>\amp= 3		\amp			\amp= 15\amp			\amp</mrow>
			</md>
		</p>
    </paragraphs>  

    <paragraphs xml:id="LT-Solving_w_LTs_verify_soln">
    <title/>
    	<p>
            <md>
				<mrow>x(t)	\amp= 3e^{-t} - 3e^{2t}\cos(3t) + 3e^{2t}\sin(3t)</mrow>
				<mrow>\amp= 3e^{-t} + e^{2t} \Big[ 3\sin(3t) - 3\cos(3t) \Big]</mrow>
				<mrow>\amp</mrow>
				<mrow>x'(t)	\amp= -3e^{-t} + e^{2t}\Big[ 9\cos(3t) + 9\sin(3t) \Big]</mrow>
							+ 2e{2t}\Big[ 3\sin(3t) - 3\cos(3t) \Big]
				<mrow>\amp= -3e^{-t} + e^{2t}\Big[ 9\cos(3t) + 9\sin(3t) + 6\sin(3t) - 6\cos(3t) \Big]</mrow>
				<mrow>\amp= -3e^{-t} + e^{2t}\Big[ 3\cos(3t) + 15\sin(3t) \Big]</mrow>
				<mrow>\amp</mrow>
				<mrow>x''(t)	\amp= 3e^{-t} + e^{2t}\Big[ -9\sin(3t) + 45\cos(3t) \Big]</mrow>
							+ 2e^{2t}\Big[ 3\cos(3t) + 15\sin(3t) \Big]
				<mrow>\amp= 3e^{-t} + e^{2t}\Big[ -9\sin(3t) + 45\cos(3t) + 6\cos(3t) + 30\sin(3t)  \Big]</mrow>
				<mrow>\amp= 3e^{-t} + e^{2t}\Big[ 21\sin(3t) + 51\cos(3t) \Big]</mrow>
			</md>
			
			<md>
				<mrow>LHS	\amp= x'' - 4x' + 13x</mrow>
				<mrow>\amp= \left( 3e^{-t} + e^{2t}\Big[ 21\sin(3t) + 51\cos(3t) \Big] \right) </mrow>
					- 4\left( -3e^{-t} + e^{2t}\Big[ 3\cos(3t) + 15\sin(3t) \Big] \right) 
					+ 13\left( 3e^{-t} + e^{2t} \Big[ 3\sin(3t) - 3\cos(3t) \Big] \right)
				<mrow>\amp= 3e^{-t} + e^{2t}\Big[ 21\sin(3t) + 51\cos(3t) \Big] </mrow>
					+ 12e^{-t} + e^{2t}\Big[ -12\cos(3t) - 60\sin(3t) \Big]  
					+ 39e^{-t} + e^{2t} \Big[ 39\sin(3t) - 39\cos(3t) \Big]
				<mrow>\amp= 3e^{-t} + e^{2t}\Big[ 21\sin(3t) + 51\cos(3t) \Big] </mrow>
					+ 12e^{-t} + e^{2t}\Big[ -12\cos(3t) - 60\sin(3t) \Big]  
					+ 39e^{-t} + e^{2t} \Big[ 39\sin(3t) - 39\cos(3t) \Big]
				<mrow>\amp= 54e^{-t}</mrow>
				<mrow>\amp= RHS</mrow>
			</md>
		</p>

		<p>
			We also verify the initial conditions: 
			<md>
				<mrow>x(0)	\amp= 3e^{-0} + e^{2\cdot 0} \Big[ 3\sin(3\cdot 0) - 3\cos(3\cdot 0) \Big]</mrow>
				<mrow>\amp= 3 + \Big[ 3\cdot 0 - 3\cdot 1 \Big]</mrow>
				<mrow>\amp= 3 - 3</mrow>
				<mrow>\amp= 0</mrow>
				<mrow>\amp</mrow>
				<mrow>x'(0)	\amp= -3e^{-0} + e^{2\cdot 0}\Big[ 3\cos(3\cdot 0) + 15\sin(3\cdot 0) \Big]</mrow>
				<mrow>\amp= -3 + \Big[ 3\cdot 1 + 15\cdot 0 \Big]</mrow>
				<mrow>\amp= - 3 + 3</mrow>
				<mrow>\amp= 0</mrow>
			</md>
		</p>
    </paragraphs>  

</subsection>
