<subsection xml:id="lt-details" xmlns:xi="http://www.w3.org/2001/XInclude">

  <paragraphs xml:id="LT-s-ne-0-15">
    <title/>
    Notice that when <m>s=0</m>, the term in the integral becomes <m>\DS e^{0t} = 1</m> and we, instead, would get
    <md>
      <mrow>		\amp= 15 \lim_{b \to \infty}\int_0^b 1\ dt
                  = 15 \lim_{b \to \infty} t\Big|_0^b
                  = 15 \lim_{b \to \infty} b = \infty. 	</mrow>
    </md>
    This shows that when <m>s=0</m>, the integral does not converge (<em>does not exist</em>) as required by the definition of the Laplace Transform. Therefore, when working with Laplace transforms, it is common restrict some values of <m>s</m>.
  </paragraphs>

  <paragraphs xml:id="LT-s-ne-0-11t">
    <title/>
    When <m>s=0</m>, the the integral becomes
    <md>
      <mrow>		\amp= \lim_{b \to \infty} \int_0^b 11t\ dt
                    = \lim_{b \to \infty} \frac{11t^2}{2}\Big|_0^b
                    = \frac{11}{2} \lim_{b \to \infty} b^2 = \infty. 	</mrow>
    </md>
    Therefore, we must have <m>s\ne0</m> for this integral to be finite.
  </paragraphs>

  <paragraphs xml:id="LT-s-gt-0-11t">
    <title/>
    If <m>s \lt 0</m>, then as <m>b \to \infty</m>, we would have <m>\DS e^{-sb} \to \infty</m> and so
    <me>\lim_{b \to \infty} \OS{\infty}{\OS{\uparrow}{\boxed{b}}}\ \US{\infty}{\US{\downarrow}{\boxed{e^{-sb}}}} = \infty.</me>
    This shows the Laplace transform would not exist if <m>s \lt 0</m>. Therefore, we must require <m>s \gt 0</m>.
  </paragraphs>

  <paragraphs xml:id="reason-factor-out-s">
    <title/>
    Since the limit only controls <m>b</m>, we treat <m>s</m> as a constant, hence <m>\DS-\frac{1}{s}</m> is also a constant that can be pulled out of the limit.
  </paragraphs>

  <paragraphs xml:id="reason-limit-to-zero-e7t">
    <title/>
    Since <m>b \to \infty</m>, then <m>\OS{negative}{\OB{(7-s)}}b \to -\infty</m> and therefore,
    <m>\DS e^{\!\!\OS{\Large negative}{\OB{(7-s)}}\!\!b} \to 0</m>
  </paragraphs>

  <paragraphs xml:id="reason-limit-to-zero-11t">
    <title/>
    We've seen the second limit, but let's review it again. If  <m>s \gt 0</m>, then <m>sb \to \infty</m> and
    <me>
      \lim_{b \to \infty} e^{-sb} = \lim_{b \to \infty}
      \frac{1}{\US{\infty}{\US{\downarrow}{\boxed{e^{sb}}}}} = 0
    </me>

    The first limit requires L'Hopital's rule. Remember, when using L'Hopital's rule here, we must take derivatives with respect to <m>b</m> (where <m>s</m> is constant). Here are the details:
    <md>
      <mrow> \lim_{b \to \infty}be^{-sb}
        \amp= \lim_{b \to \infty}\frac{\OS{\infty}{\OS{\uparrow}{\boxed{b}}}}{\US{\infty}{\US{\downarrow}{\boxed{e^{sb}}}}}
          \,\US{LH}{=}\, \lim_{b \to \infty}\frac{1}{se^{sb}}
          = \frac{1}{s}\lim_{b \to \infty}\frac{1}{\US{\infty}{\US{\downarrow}{\boxed{e^{sb}}}}}
          = 0, \quad s \gt 0</mrow>
    </md>
  </paragraphs>

  <paragraphs xml:id="reason-int-by-parts-texpt">
    <title/>
    <md>
      <mrow>  u = t,\quad\amp dv = e^{-st}dt, </mrow>
      <mrow> du = dt,\quad\amp v = -\frac{1}{s}e^{-st}  </mrow>
    </md>
    <md>
      <mrow>  \int_0^b te^{-st} dt
                \amp= \left[t \cdot \left( -\frac{1}{s}e^{-st} \right)
              - \int \left( -\frac{1}{s}e^{-st} \right) dt\right]\Bigg|_0^b	</mrow>
      <mrow> 		\amp= \left[-\frac{t}{s}e^{-st}
              + \frac{1}{s}\int e^{-st} dt\right]\Bigg|_0^b </mrow>
      <mrow> 		\amp= \left[-\frac{t}{s}e^{-st}
              - \frac{1}{s^2}e^{-st}\right]\Bigg|_0^b</mrow>
      <mrow> 		\amp= \left[\left(-\frac{b}{s}e^{-sb} - \frac{1}{s^2}e^{-sb}\right)
                  - \left(-\frac{0}{s^2}e^{-s\cdot 0} - \frac{1}{s^2}e^{-s\cdot 0}\right)\right]</mrow>
      <mrow> 		\amp= \left[-\frac{b}{s}e^{-sb} - \frac{1}{s^2}e^{-sb}
                + \frac{1}{s^2}\right]	</mrow>
    </md>
  </paragraphs>

</subsection>
