<section xmlns:xi="http://www.w3.org/2001/XInclude"><title> Preparing the Backward Transform </title>

	<introduction>
		<p>
			So far, we have explored the forward (initial step) and backward (final step) Laplace transforms, as illustrated in the figures below.
			<image source="figures/Laplace-Roadmap-Step-1.png" width="100%">
				<shortdescription>(for accessibility)</shortdescription>
			</image>
			<image source="figures/Laplace-Roadmap-Step-3.png" width="100%">
				<shortdescription>(for accessibility)</shortdescription>
			</image>
			However, the transition between these two steps often requires some algebraic manipulation before the backward transform can be applied, as shown in the following figure.
			<image source="figures/Laplace-Roadmap-Step-2.png" width="45%">
				<shortdescription>(for accessibility)</shortdescription>
			</image>
		</p>
	
		<p>
			After solving for <m>Y</m> in Step 2a, the goal is to express <m>Y</m> as a sum of simpler components whose inverse Laplace transforms can be easily identified using the right-hand column of the <xref ref="common-lt-table" text="custom">Laplace Transform Table</xref>. This may involve algebraic techniques such as splitting rational functions, completing the square, or partial fraction decomposition. These methods will be covered in this section.
		</p>
    </introduction>

	<subsection><title> Splitting Fractions </title>

		<p>
			One useful algebraic manipulation in preparing for the inverse Laplace transform is splitting a rational function that has a sum or difference in the numerator. This technique simplifies the expression into recognizable forms, making it easier to apply known Laplace transform pairs. Let's explore two examples where splitting fractions proves useful.
		</p>
		
		<example>
			<m>\ \ </m>Compute the inverse Laplace transforms for each.
			<p>
				<sidebyside widths="22% 78%">
					<p>
						<m>\ds \frac{2s - 3}{s^2 + 16}</m>
					</p>
					<p>
						<solution><title> Solution </title>
							<p>
								The key to solving this problem is to split the fraction into two simpler terms:
								<me>\ds \frac{2s - 3}{s^2 + 16} = \frac{2s}{s^2 + 16} - \frac{3}{s^2 + 16}.</me>
								Now, we can apply the inverse Laplace transform to each term separately. The first term matches the Laplace transform of <m>\cos(4t)</m> (<xref ref="L5" text="custom"><m>L_5</m></xref>), and the second term corresponds to the Laplace transform of <m>\sin(4t)</m> (<xref ref="L4" text="custom"><m>L_4</m></xref>):
								<md>
									<mrow>\amp\ \ilap{\frac{2s - 3}{s^2 + 16}} </mrow>
									<mrow>\amp\ = 2\ \ilap{\frac{s}{s^2 + 16}} - 3\ \ilap{\frac{1}{s^2 + 16}} </mrow>
									<mrow>\amp\ = 2 \cos(4t) - \frac{3}{4} \sin(4t). </mrow>
								</md>
							</p>
						</solution>
					</p>
				</sidebyside>
	
				<sidebyside widths="22% 78%">
					<p>
						<m>\ds\frac{s^3 - 7}{s^7}</m>
					</p>
					<p>
						<solution><title> Solution </title>
							<p>
								We can split the fraction into the terms,
								<me>\ds \frac{s^3 - 7}{s^7} = \frac{s^3}{s^7} - \frac{7}{s^7} = \frac{1}{s^4} - \frac{7}{s^7}.</me>
								and apply the inverse Laplace transform (<xref ref="L3" text="custom"><m>L3</m></xref>) to each
								<md>
									<mrow> \ilap{\frac{s^3 - 7}{s^7}}	=\amp\ \ilap{\frac{1}{s^4} - \frac{7}{s^7}}</mrow>
									<mrow>									=\amp\ \ilap{\frac{1}{s^4}} - 7\ilap{\frac{1}{s^7}}</mrow>
									<mrow>									=\amp\ \frac{1}{3!}\ilap{\frac{3!}{s^4}} - \frac{7}{6!}\ilap{\frac{6!}{s^7}}</mrow>
									<mrow>									=\amp\ \frac{1}{6}t^3 - \frac{7}{720}t^6</mrow>
								</md>
							</p>
						</solution>
					</p>
				</sidebyside>
			</p>
		</example>

		<p>
			This section demonstrates how relatively simple modifications, such as splitting fractions, can make it easier to find the inverse Laplace transform. However, some functions of <m>s</m> may require more advanced techniques. In the next section, we will explore how completing the square can help match the forms needed for a backward transform when the <m>s</m>-variable is shifted.
		</p>
	
		<xi:include href="./p4-c2-s2-1-interactives.ptx" />
	</subsection>

	<subsection><title>Completing the Square</title>

		<p>
			As you progress through the Laplace Transform Method, you will often encounter <xref ref="rational-function" text="custom">rational functions</xref> that do not immediately match any known form in the <xref ref="common-lt-table" text="custom">table of Laplace transforms</xref>. For example, the function 
			<me>\frac{s - 6}{s^2 + 5s + 1}</me> 
			does not align with standard forms. A common approach is to rewrite the denominator in the form <m>(s - a)^2 + b^2</m>, allowing it to match known transforms like <m>L_7</m> or <m>L_8</m>. This technique, called completing the square, is essential for converting quadratic expressions into forms that are easier to work with in inverse Laplace computations.
		</p>

		<p>
			Completing the square is particularly useful when the quadratic expression in the denominator has complex roots. As a quick check, recall from <xref ref="solving-the-quadratic-equation" text="custom">solving quadratic equations</xref> that if the discriminant 
			<me>b^2 - 4ac</me> 
			is negative, the quadratic function has complex roots. This indicates that completing the square is the correct approach, as the following examples will demonstrate.
		</p>
	
		<example>
			<m>\ \ </m>Compute the inverse Laplace transforms of the following functions:
			<me>H(s) = \frac{s-1}{s^2 - 2s + 5}, \quad K(s) = \frac{11}{s^2 - 6s + 14}, \quad P(s) = \frac{s+3}{s^2 + 2s + 10}.</me>
			
			<solution><title><m>\ilap{H(s)}</m></title>
				<p>
					The discriminant of the denominator <m>s^2 - 2s + 5</m> is 
					<me>b^2 - 4ac = (-2)^2 - 4(1)(5) = 4 - 20 = -16</me>, 
					which is negative. Therefore, completing the square is necessary:
					<md>
						<mrow> s^2 - 2s + 5 = (s^2 - 2s) + 5	=\amp\ (\ob{s^2 - 2s + 1}^{(s - 1)^2} - 1) + 5   </mrow>
						<mrow>								  =\amp\ (s - 1)^2 + 4							 </mrow>
					</md>.
					Rewriting <m>H(s)</m> gives:
					<me>\frac{s-1}{s^2 - 2s + 5} = \frac{s-1}{(s - 1)^2 + 4},</me>
					which matches <xref ref="L8" text="title"/> (<m>a=1, b=2</m>). Therefore,
					<me>h(t) = \ilap{H(s)} = e^{t}\cos(2t).</me>
				</p>
			</solution>
	
			<solution><title><m>\ilap{K(s)}</m></title>
				<p>
					The discriminant of the denominator <m>s^2 - 6s + 14</m> is:
					<me>b^2 - 4ac = (-6)^2 - 4(1)(14) = 36 - 56 = -20</me>, 
					indicating that completing the square is necessary:
					<md>
						<mrow> s^2 - 6s + 14 = (s^2 - 6s) + 14  =\amp (\ob{s^2 - 6s + 9}^{(s - 3)^2} - 9) + 14  </mrow>
						<mrow>								  =\amp (s - 3)^2 + 5							 </mrow>
					</md>.
					Rewriting <m>K(s)</m> as:
					<me>
						\frac{11}{s^2 - 6s + 14} 
							= \ub{\frac{11}{(s - 3)^2 + 5}}_{\large \text{Match with } L_7} 
							= \frac{11}{\sqrt{5}}\ub{\frac{\sqrt{5}}{(s - 3)^2 + 5}}_{\large <xref ref="L7" text="custom"><m>L_7</m></xref> (a = 3, b = \sqrt{5})}
					</me>. 
					Therefore,
					<md>
						<mrow>
							k(t) = \ilap{K(s)} =\amp\ \frac{11}{\sqrt{5}}e^{3t}\sin(\sqrt{5}t)
						</mrow>
					</md>.
				</p>
			</solution>
	
			<solution><title><m>\ilap{P(s)}</m></title>
				<p>
					Completing the square for the denominator of <m>P(s)</m> gives:
					<me>
						\frac{s+3}{s^2 + 2s + 10} = \frac{s+3}{(s + 1)^2 + 9}
					</me>.
					However, the numerator <m>s + 3</m> does not match <m>s + 1</m>. To resolve this, we rewrite <m>3</m> as <m>1 + 2</m> and group terms:
					<md>
						<mrow>  
							\frac{s+3}{s^2 + 2s + 10}
								=\amp\ \frac{s + 1 + 2}{(s + 1)^2 + 9}
						</mrow>
						<mrow>
								=\amp\ \frac{s+1}{(s + 1)^2 + 9} + \frac{2}{(s + 1)^2 + 9}
						</mrow>
						<mrow>
								=\amp\ \ub{\frac{s+1}{(s + 1)^2 + 9}}_{\large <xref ref="L8" text="title"/>\ (a=-1, b=3)} 
									+ \frac{2}{3}\ub{\frac{3}{(s + 1)^2 + 9}}_{\large <xref ref="L7" text="title"/>\ (a=-1, b=3)}
						</mrow>	
					</md>,
					Now, apply the inverse Laplace transform:
					<md>
						<mrow>  
							p(t) =\amp\ \ilap{P(s)}
						</mrow>
						<mrow>
								=\amp\ \ilap{ \frac{s+1}{(s + 1)^2 + 9} } + \frac{2}{3}\ilap{ \frac{3}{(s + 1)^2 + 9} }
						</mrow>
						<mrow>
								=\amp\ e^{-t}\cos(3t) + \frac{2}{3}e^{-t}\sin(3t)
						</mrow>	
					</md>
				</p>
			</solution>
		</example>

		<p>
			Completing the square is a crucial technique when working with quadratic expressions in the denominator of Laplace transforms. It allows for the backward transformations by rewriting the <m>s</m>-function in a form that aligns with known inverse Laplace transforms. In the next subsection, we will explore another technique: partial fraction decomposition, which helps break down more complex rational functions into simpler parts that can be easily matched to common inverse transforms.
		</p>

		<xi:include href="./p4-c2-s2-2-interactives.ptx" />

	</subsection>
	
	<subsection><title>Partial Fraction Decomposition</title>

		<p>
			In the Laplace Transform Method, we often encounter rational functions with polynomial denominators that can be factored into simpler linear or quadratic terms. In such cases, partial fraction decomposition becomes a powerful technique. By breaking the original rational function into simpler fractions, each corresponding to a known form in the Laplace Transform Table, we can efficiently compute the inverse Laplace transform.
		</p>

		<p>
			The key idea is to express a complex rational function as a sum of simpler fractions, each with a simpler denominator. For example, if the denominator can be factored as <m>(s - a)(s - b)</m>, we can rewrite the function as:
			<me>\frac{f(s)}{(s - a)(s - b)} = \frac{A}{s - a} + \frac{B}{s - b}.</me>
			Once expressed in this way, we can directly apply the inverse Laplace transform to each term. Let’s explore a series of examples to demonstrate this approach.
		</p>

		<example>
			<m>\ \ </m>Find the inverse Laplace transforms of each function.
			<me>Y(s) = \frac{2s + 5}{(s + 1)(s + 4)}, \quad P(s) = \frac{s}{s^2 - s + 6}, \quad Q(s) = \frac{3s + 4}{s^2 - 2s + 1}.</me>
	
			<solution><title><m>\ilap{Y(s)}</m></title>
				<p>
					First, decompose <m>Y(s)</m> into partial fractions:
					<me>\frac{2s + 5}{(s + 1)(s + 4)} = \frac{A}{s + 1} + \frac{B}{s + 4}.</me>
					Multiply both sides by <m>(s + 1)(s + 4)</m>, 
					<me>2s + 5 = A(s + 4) + B(s + 1).</me>
					and solve for <m>A</m> and <m>B</m> by selecting convenient values for <m>s</m>:
					<sidebyside widths="8% 80%">
						<p>
							<md>
								<mrow>s = -1: \amp</mrow>
								<mrow></mrow>
								<mrow>s = -4: \amp</mrow>
								<mrow></mrow>
							</md>
						</p>
						<p>
							<md>
								<mrow>2(-1) + 5 =	\amp\ A(-1 + 4) + B(-1 + 1)</mrow>
								<mrow>3 =			\amp\ A(3) + B(0) \quad\implies\quad A=1</mrow>
								<mrow>2(-4) + 5 =	\amp\ A(-4 + 4) + B(-4 + 1)</mrow>
								<mrow>-3 =			\amp\ A(0) + B(-3) \quad\implies\quad B=1</mrow>
							</md>
						</p>>
					</sidebyside>
					Therefore, the partial fraction decomposition is:
					<me>\frac{2s + 5}{(s + 1)(s + 4)} = \frac{1}{s + 1} + \frac{1}{s + 4}.</me>
					Applying the inverse Laplace transform to each term:
					<me>\ilap{Y(s)} = \ilap{\frac{1}{s + 1}} + \ilap{\frac{1}{s + 4}} = e^{-t} + e^{-4t}.</me>
				</p>
			</solution>
	
			<solution><title><m>\ilap{P(s)}</m></title>
				<p>
					First, factor the quadratic denominator:
					<me>s^2 - s - 6 = (s + 2)(s - 3).</me>
					Now decompose <m>P(s)</m> into partial fractions:
					<me>\frac{s}{(s + 2)(s - 3)} = \frac{A}{s + 2} + \frac{B}{s - 3}.</me>
					Multiply both sides by <m>(s + 2)(s - 3)</m>,
					<me>s = A(s - 3) + B(s + 2).</me>
					and solve for <m>A</m> and <m>B</m> by selecting convenient values for <m>s</m>:
					<sidebyside widths="8% 80%">
						<p>
							<md>
								<mrow>s = -2: \amp</mrow>
								<mrow></mrow>
								<mrow>s = 3: \amp</mrow>
								<mrow></mrow>
							</md>
						</p>
						<p>
							<md>
								<mrow>-2 =	\amp\ A(-2 - 3) + B(-2 + 2)</mrow>
								<mrow>-2 =	\amp\ A(-5) + B(0) \quad\implies\quad A=2/5</mrow>
								<mrow>3 =	\amp\ A(3 - 3) + B(3 + 2)</mrow>
								<mrow>3 =	\amp\ A(0) + B(5) \quad\implies\quad B=3/5</mrow>
							</md>
						</p>
					</sidebyside>
					The partial fraction decomposition is:
					<me>\frac{s}{(s + 2)(s - 3)} = \frac{2/5}{s + 2} + \frac{3/5}{s - 3}.</me>
					Therefore:
					<me>\ilap{P(s)} = \frac25 e^{-2t} + \frac35 e^{3t}.</me>
				</p>
			</solution>
	
			<solution><title><m>\ilap{Q(s)}</m></title>
				<p>
					Factor the quadratic denominator:
					<me>s^2 - 2s + 1 = (s - 1)^2.</me>
					Decompose <m>Q(s)</m> into partial fractions:
					<me>\frac{3s + 4}{(s - 1)^2} = \frac{A}{s - 1} + \frac{B}{(s - 1)^2}.</me>
					Multiply both sides by <m>(s - 1)^2</m>,
					<me>s = A(s - 1) + B.</me>
					and solve for <m>A</m> and <m>B</m> by selecting convenient values for <m>s</m>:
					<sidebyside widths="8% 80%">
						<p>
							<md>
								<mrow>s = 1: \amp</mrow>
								<mrow></mrow>
								<mrow>s = 0: \amp</mrow>
								<mrow></mrow>
							</md>
						</p>
						<p>
							<md>
								<mrow>3(1) + 4 =	\amp\ A(1 - 1) + B</mrow>
								<mrow>7 =			\amp\ A(0) + B \quad\implies\quad B=7</mrow>
								<mrow>3(0) + 4 =	\amp\ A(0 - 1) + B</mrow>
								<mrow>4 =			\amp\ -A + 7 \quad\implies\quad A=3</mrow>
							</md>
						</p>
					</sidebyside>
					The partial fraction decomposition is:
					<me>\frac{3}{s - 1} + \frac{7}{(s - 1)^2}.</me>
					Therefore:
					<me>\ilap{Q(s)} = 3e^{t} + 7te^{t}.</me>
				</p>
			</solution>
		</example>

		<p>
			Partial fraction decomposition also works for more complex rational functions with higher-degree polynomials in the denominator. The key is to factor the denominator as much as possible, then apply the decomposition to each term. Let's examine a more complex case involving cubic and quartic denominators.
		</p>

		<example>
			<m>\ \ </m>Find the inverse Laplace transforms of each function.
			<me>R(s) = \frac{2s^2 + 5s + 1}{s^3 - s}, \quad S(s) = \frac{4s^3 + 3s^2 - 2s + 1}{s^4 - 1}.</me>
	
			<solution><title><m>\ilap{R(s)}</m></title>
				<p>
					First, factor the cubic denominator:
					<me>s^3 - s = s(s - 1)(s + 1).</me>
					Now decompose <m>R(s)</m> into partial fractions:
					<me>R(s) = \frac{2s^2 + 5s + 1}{s(s - 1)(s + 1)} = \frac{A}{s} + \frac{B}{s - 1} + \frac{C}{s + 1}</me>
					and multiply both sides by <m>s(s - 1)(s + 1)</m> to get
					<me>2s^2 + 5s + 1 = A(s - 1)(s + 1) + B(s)(s + 1) + C(s)(s - 1).</me>
					and solve for <m>A, B,</m> and <m>C</m> by selecting convenient values for <m>s</m>:
					<sidebyside widths="10% 70% 18%">
						<p>
							<md>
								<mrow>s = 0: \amp</mrow>
								<mrow></mrow>
								<mrow>s = 1: \amp</mrow>
								<mrow></mrow>
								<mrow>s = -1: \amp</mrow>
								<mrow></mrow>
							</md>
						</p>
						<p>
							<md>
								<mrow>1 =	\amp\ A(-1)(1) + B(0)(1) + C(0)(-1)</mrow>
								<mrow>1 =	\amp\ -A</mrow>
								<mrow>8 =	\amp\ A(0)(2) + B(1)(2) + C(1)(0)</mrow>
								<mrow>8 =	\amp\ 2B</mrow>
								<mrow>-2 =	\amp\ A(1)(0) + B(-1)(0) + C(-1)(-2)</mrow>
								<mrow>-2 =	\amp\ 2C</mrow>
							</md>
						</p>
						<p>
							<md>
								<mrow></mrow>
								<mrow>A=\amp\ -1</mrow>
								<mrow></mrow>
								<mrow>B=\amp\ 4</mrow>
								<mrow></mrow>
								<mrow>C=\amp\ -1</mrow>
							</md>
						</p>
					</sidebyside>
					Therefore,
					<md>
						<mrow>\ilap{R(s)}	=\amp\ \ilap{\frac{-1}{s} + \frac{4}{s - 1} + \frac{-1}{s + 1}}.</mrow>
						<mrow>r(t)			=\amp\ -1 + 4e^{t} - e^{-t}.</mrow>
					</md>
				</p>
			</solution>
	
			<solution><title><m>\ilap{S(s)}</m></title>
				<p>
					Factor the quartic denominator:
					<me>s^4 - 1 = (s^2 - 1)(s^2 + 1) = (s - 1)(s + 1)(s^2 + 1).</me>
					Decompose <m>S(s)</m> into partial fractions:
					<me>\frac{4s^3 + 3s^2 - 2s + 1}{(s - 1)(s + 1)(s^2 + 1)} = \frac{A}{s - 1} + \frac{B}{s + 1} + \frac{Cs + D}{s^2 + 1}.</me>
					and multiply both sides by <m>(s - 1)(s + 1)(s^2 + 1)</m> to get
					<md>
						<mrow>4s^3 + 3s^2 - 2s + 1 = A(s + 1)(s^2 +\amp\ 1)	+ B(s - 1)(s^2 + 1)</mrow>
						<mrow> 											+\amp\ (Cs+D)(s - 1)(s + 1).</mrow>
					</md>
					and solve for <m>A, B, C,</m> and <m>D</m> by selecting convenient values for <m>s</m>:
					<sidebyside widths="12% 80%">
						<p>
							<md>
								<mrow>s = 1: \amp</mrow>
								<mrow>\vphantom{\frac32}</mrow>
								<mrow>s = -1: \amp</mrow>
								<mrow>\vphantom{\frac32}</mrow>
								<mrow>s = 0: \amp</mrow>
								<mrow>\vphantom{\frac32}</mrow>
								<mrow>s = -2: \amp</mrow>
								<mrow>\vphantom{\frac32}</mrow>
							</md>
						</p>
						<p>
							<md>
								<mrow>6 =	\amp\ A(2)(2) + B(0)(2) + (C(1) + D)(0)(2)</mrow>
								<mrow>6 =	\amp\ 4A \qquad\implies\qquad A = \frac32</mrow>
								<mrow>2 =	\amp\ A(0)(2) + B(-2)(2) + (C(-1) + D)(-2)(0)</mrow>
								<mrow>2 =	\amp\ -4B \qquad\implies\qquad B = -\frac12</mrow>
								<mrow>1 =	\amp\ A(1)(1) + B(-1)(1) + (C(0) + D)(-1)(1)</mrow>
								<mrow>1 =	\amp\ \frac32 + \frac12 - D \qquad\implies\qquad D = 1</mrow>
								<mrow>-15 =	\amp\ A(-1)(3) + B(-3)(3) + (C(-2) + D)(-3)(-1)</mrow>
								<mrow>-15 =	\amp\ -3A - 9B + -6C + 3D</mrow>
								<mrow>-15 =	\amp\ -\frac92 + \frac92 + -6C + 3(1) \quad\implies\quad C = 3</mrow>
							</md>
						</p>
					</sidebyside>
					Therefore,
					<md>
						<mrow>\ilap{S(s)}	=\amp\ \ilap{\frac{\frac32}{s - 1} - \frac{\frac12}{s + 1} + \frac{3s + 1}{s^2 + 1}}.</mrow>
						<mrow>s(t)			=\amp\ \frac32 e^{t} - \frac12 e^{-t} + 3\cos(t) + \sin(t).</mrow>
					</md>
				</p>
			</solution>
		</example>

		<p>
			Partial fraction decomposition simplifies complex rational functions, breaking them into manageable terms that correspond to known inverse Laplace transforms. In the next section, we will explore advanced techniques, including handling repeated roots and higher-order polynomials.
		</p>
	
		<xi:include href="./p4-c2-s2-3-interactives.ptx" />

	</subsection>

</section>
