<subsubsection xml:id="quick-ref-uc"><title> Undermined Coefficients </title>

	<worksheet><title> Key Terms &amp; Concepts </title>

		<p>
			<assemblage><title> ✳️ Summary of the Key Ideas </title>
				<p>
					<ul marker="square">
						<li> The method of undetermined coefficients is used to solve non-homogeneous linear differential equations.</li>
						<li> The general solution to a non-homogeneous equation is the sum of the general solution to the corresponding homogeneous equation and a particular solution.</li>
						<li> The method involves guessing the form of the particular solution based on the form of the non-homogeneous term and solving for the coefficients.</li>
						<li> The method is applicable when the non-homogeneous term can be expressed as a linear combination of known functions.</li>
					</ul>
				</p>
			</assemblage>
		</p>

		<p>
			<dl>
				<li xml:id="summary-lhcc"><title> LHCC Equation </title>
					<p>
						An LHCC equation is a Linear Homogeneous Differential Equations with Constant Coefficients and have the form
						<me>
							a_n y^{(n)} + \cdots + a_1 y' + a_0 y = 0
						</me>.
					</p>
				</li>
				<li xml:id="summary-characteristic-eqn"><title> Characteristic Equation </title>
					<p>
						
					</p>
				</li>
				<li xml:id="summary-lhcc-general-solns"><title> LHCC General Solutions </title>
					<p>
						
					</p>
				</li>
			</dl>
		</p>

		<p>
			<dl>
				<li xml:id="summary-lncc"><title> LNCC Equation </title>
					<p>
						An LNCC equation is a Linear Nonhomogeneous Differential Equations with Constant Coefficients and have the form
						<men xml:id="summary-lncc-equation">
							a_n y^{(n)} + \cdots + a_1 y' + a_0 y = f(x)
						</men>.
					</p>
				</li>
				<li xml:id="summary-forcing-function"><title> Forcing Function </title>
					<p>
						A forcing function is the constant term in <xref ref="summary-lncc-equation"/>, denoted by <m>f(x)</m>.
					</p>
				</li>
				<li xml:id="summary-particular-soln"><title> Particular Solution </title>
					<p>
						A particular solution, <m>y_h</m>, is a function that can be plugged into <xref ref="summary-lncc-equation"/> and all the terms combine to give the forcing function, <m>f(x)</m>.
					</p>
				</li>
				<li xml:id="summary-homogeneous-soln"><title> Homogeneous Solution </title>
					<p>
						A homogeneous solution, <m>y_h</m>, is a function such that, when it is plugged into <xref ref="summary-lncc-equation"/> all the terms cancel to zero. That is, <m>y_h</m> is the solution to the homogeneous version of <xref ref="summary-lncc-equation"/> (<m> f(x) = 0 </m>). 
					</p>
				</li>
				<li xml:id="summary-lncc-general-soln"><title> General Solutions </title>
					<p>
						The general solution to  <xref ref="summary-lncc-equation"/> is the sum of the homogeneous and particular solutions, that is
						<me>
							y = y_h + y_p
						</me>.
					</p>
				</li>
			</dl>
		</p>
		
		<tabular top="minor" bottom="minor" right="minor" left="minor" halign="center">
			<col top="none" halign="center"/>
			<col halign="center"/>
			<col halign="right" right="none"/>
			<col halign="left"/>
			<col halign="center"/>
			<row left="none">
				<cell></cell>
				<cell><m>y</m></cell>
				<cell><m>y'' - 4y' + 3{\color{blue} y} =\!\!\!</m></cell>
				<cell>LHS</cell>
				<cell>LHS <m> \os{?}{=} 9x</m></cell>
			</row>

			<row>
				<cell>1</cell>
				<cell><m>3</m></cell>
				<cell><m>(3)'' - 4(3)' + 3({\color{blue} 3}) =\!\!\!</m></cell>
				<cell><m>{\color{blue} 9}</m></cell>
				<cell>No</cell>
			</row>

			<row>
				<cell>2</cell>
				<cell><m>3x</m></cell>
				<cell><m>(3x)'' - 4(3x)' + 3({\color{blue} 3x}) =\!\!\!</m></cell>
				<cell><m>-12 + {\color{blue} 9x}</m></cell>
				<cell>No</cell>
			</row>

			<row>
				<cell>3</cell>
				<cell><m>x^4</m></cell>
				<cell><m>(x^4)'' - 4(x^4)' + 3({\color{blue} x^4}) =\!\!\!</m></cell>
				<cell><m>12x^2 - 16x^3 + {\color{blue} 3x^4}</m></cell>
				<cell>No</cell>
			</row>

			<row>
				<cell>4</cell>
				<cell><m>x^2+3x</m></cell>
				<cell><m>(x^2+3x)'' - 4(x^2+3x)' + 3({\color{blue} x^2}+3x) =\!\!\!</m></cell>
				<cell><m>-10 + x + {\color{blue} 3x^2}</m></cell>
				<cell>No</cell>
			</row>

			<row>
				<cell>5</cell>
				<cell><m>3x-6</m></cell>
				<cell><m>(3x-6)'' - 4(3x-6)' + 3({\color{blue} 3x}-6) =\!\!\!</m></cell>
				<cell><m>-30+{\color{blue} 9x}</m></cell>
				<cell>No</cell>
			</row>

			<row>
				<cell>6</cell>
				<cell><m>3x+4</m></cell>
				<cell><m>(3x+4)'' - 4(3x+4)' + 3({\color{blue} 3x}+4) =\!\!\!</m></cell>
				<cell><m>{\color{blue} 9x}</m></cell>
				<cell>Yes</cell>
			</row>
		</tabular>

		<p>
			Based on this table, we note that the correct solution is <m>y = 3x + 4</m> and
			<ul marker="square">
				<li>
					<p>
						Row 1 shows that a constant term alone could never produce an <m>x</m> term.
					</p>
				</li>
				<li>
					<p>
						Derivatives reduce the power of a polynomial, so the highest power term (highlighted in blue) comes from the <m>y</m> term.
						<fn>
							<m>y'' - 4y' + \os{\large y\text{ term}}{\boxed{3y}}</m>
						</fn>
					</p>
				</li>
				<li>
					<p>
						Rows 3 &amp; 4 illustrate the solution can't have a <m>x^2</m> or higher-degree term.
					</p>
				</li>
				<li>
					<p>
						Row 6 shows the solution (<m>3x+4</m>) needed an <m>x</m> term and constant term even though the right-hand side, <m>9x</m>, has only an <m>x</m> term.
					</p>
				</li>
			</ul>
		</p>

		<subsection><title> LNCC Equations </title>

			<figure xml:id="lhcc-vs-lcc-solution-type">
				<caption>Comparison of a homogeneous equation (<em>left</em>) and a nonhomogeneous equation (<em>right</em>). In both, the solutions must simplify in a specific way when substituted into the equation.</caption>
				<sidebyside widths="33% 33% 34%">
					<image width="100%">
						<latex-image>
						
							\begin{tikzpicture}[join=round,rounded corners,&gt;=stealth,shorten &gt;=1pt,shorten &lt;=1pt,thick]
			
								\node (text) 	at (1.8,1.1) 	{\(e^{r x}-\)like};
								
								\node (blank1) at (0.3,0.4) {};
								\filldraw[fill=blue!20,fill opacity=0.2]
									(0,0)--(0.6,0)--(0.6,0.5)--(0,0.5)--cycle;
								
								\node 			at (0.75,0.35)	{$^{\prime\prime}$};
								\node 			at (1.0,0.25)	{$-$};
								\node 			at (1.3,0.25)	{$4$};
								
								\node (blank2) at (1.8,0.4) {};
								\filldraw[fill=blue!20,fill opacity=0.2]
									(1.5,0)--(2.1,0)--(2.1,0.5)--(1.5,0.5)--cycle;
				
								\node 			at (2.2,0.35)	{$^{\prime}$};
								\node 			at (2.4,0.25)	{$+$};
								\node 			at (2.7,0.25)	{$3$};
				
								\node (blank3) at (3.2,0.4) {};
								\filldraw[fill=blue!20,fill opacity=0.2]
									(2.9,0)--(3.5,0)--(3.5,0.5)--(2.9,0.5)--cycle;
								\node 			at (3.8,0.25)	{$=$};
								\node 			at (4.2,0.25)	{$0$};
								
								\draw[-&gt;,thick] (text.west)		--	+(-0.2,0) -| (blank1);
								\draw[-&gt;,thick] (text)		--	+(0,-0.4) -| (blank2);
								\draw[-&gt;,thick] (text.east)		--	+(0.1,0) -| (blank3);
								
							\end{tikzpicture}
						</latex-image>
					</image>
					<image width="100%">
						<latex-image>
						
							\begin{tikzpicture}[join=round,rounded corners,&gt;=stealth,shorten &gt;=1pt,shorten &lt;=1pt,thick]
			
								\node (text) 	at (1.8,1.1) 	{\(f(x)-\)like};
								
								\node (blank1) at (0.3,0.4) {};
								\filldraw[fill=blue!20,fill opacity=0.2]
									(0,0)--(0.6,0)--(0.6,0.5)--(0,0.5)--cycle;
								
								\node 			at (0.75,0.35)	{$^{\prime\prime}$};
								\node 			at (1.0,0.25)	{$-$};
								\node 			at (1.3,0.25)	{$4$};
								
								\node (blank2) at (1.8,0.4) {};
								\filldraw[fill=blue!20,fill opacity=0.2]
									(1.5,0)--(2.1,0)--(2.1,0.5)--(1.5,0.5)--cycle;
				
								\node 			at (2.2,0.35)	{$^{\prime}$};
								\node 			at (2.4,0.25)	{$+$};
								\node 			at (2.7,0.25)	{$3$};
				
								\node (blank3) at (3.2,0.4) {};
								\filldraw[fill=blue!20,fill opacity=0.2]
									(2.9,0)--(3.5,0)--(3.5,0.5)--(2.9,0.5)--cycle;
								\node 			at (3.8,0.25)	{$=$};
								\node 			at (4.4,0.25)	{$f(x)$};
								
								\draw[-&gt;,thick] (text.west)		--	+(-0.3,0) -| (blank1);
								\draw[-&gt;,thick] (text)		--	+(0,-0.4) -| (blank2);
								\draw[-&gt;,thick] (text.east)		--	+(0.3,0) -| (blank3);
								
							\end{tikzpicture}
						</latex-image>
					</image>
					<image width="100%">
					<latex-image>
					
						\begin{tikzpicture}[join=round,rounded corners,&gt;=stealth,shorten &gt;=1pt,shorten &lt;=1pt,thick]
							\node (text1) 	at (1.4,0.5) 	{\scriptsize equal};
							\node (text2) 	at (3.4,0.7) 	{\scriptsize equal};
							
							\def\LA{0.1}
							\def\WA{0.64}
							\def\LB{1.27}
							\def\WB{1.65}
							\def\LC{3.33}
							\def\WC{0.3}
							\def\LD{4.2}
							\def\WD{0.28}

							\node[anchor=west] (eqn)	at (0,0)	{$\,3A\ x + \,- 4A + 3B\, = \ 9\ x + 0\ .$};
							\node (xterm1) at (\LA+\WA/2,0.1) {};
							\node (xterm2) at (\LC+\WC/2,0.1) {};
							\node (cterm1) at (\LB+\WB/2,0.1) {};
							\node (cterm2) at (\LD+\WD/2,0.1) {};
							
							\filldraw[fill=red!20,fill opacity=0.2,thin,draw=red]
								(\LA,-0.2)--(\WA,-0.2)--(\WA,0.2)--(\LA,0.2)--cycle;
							\filldraw[fill=blue!20,fill opacity=0.2,thin,draw=blue]
								(\LB,-0.2)--(\LB+\WB,-0.2)--(\LB+\WB,0.2)--(\LB,0.2)--cycle;
							\filldraw[fill=red!20,fill opacity=0.2,thin,draw=red]
								(\LC,-0.2)--(\LC+\WC,-0.2)--(\LC+\WC,0.2)--(\LC,0.2)--cycle;
							\filldraw[fill=blue!20,fill opacity=0.2,thin,draw=blue]
								(\LD,-0.2)--(\LD+\WD,-0.2)--(\LD+\WD,0.2)--(\LD,0.2)--cycle;
							
							\draw[-&gt;,thin] (text1.west)		--	+(-0.06,0.0) -| (xterm1);
							\draw[-&gt;,thin] (text1.east)		--	+(0.06,0.0) -| (xterm2);
							\draw[-&gt;,thin] (text2.west)		--	+(-0.06,0.0) -| (cterm1);
							\draw[-&gt;,thin] (text2.east)		--	+(0.06,0.0) -| (cterm2);
							
						\end{tikzpicture}
					</latex-image>
			</image>
				</sidebyside>
			</figure>
			
		</subsection>

		<table xml:id="yp-forms-table-row-1"><title> row 1 </title>
			<tabular top="medium" left="medium" right="medium" bottom="minor">
				<col halign="center" top="none" right="minor"/>
				<col halign="center" right="minor"/>
				<col halign="center"/>
				<row left="none" bottom="medium">
					<cell right="medium"/>
					<cell><term></term><m>f(x)\ </m> type</cell>
					<cell><term><m>y_p</m> Form</term></cell>
				</row>
				<row>
					<cell>1</cell>
					<cell><m>a</m> (constant)</cell>
					<cell><m>A</m></cell>
				</row>
			</tabular>
		</table>

		<table xml:id="yp-forms-table-row-2"><title> row 2 </title>		
			<tabular top="medium" left="medium" right="medium" bottom="minor">
				<col halign="center" top="none" right="minor"/>
				<col halign="center" right="minor"/>
				<col halign="center"/>
				<row left="none" bottom="medium">
					<cell right="medium"/>
					<cell><term></term><m>f(x)\ </m> type</cell>
					<cell><term><m>y_p</m> Form</term></cell>
				</row>
				<row>
					<cell>2</cell>
					<cell><m>ax + b</m></cell>
					<cell><m>Ax + B</m></cell>
				</row>
			</tabular>
		</table>

		<table xml:id="yp-forms-table-row-3"><title> row 3 </title>
			<tabular top="medium" left="medium" right="medium" bottom="minor">
				<col halign="center" top="none" right="minor"/>
				<col halign="center" right="minor"/>
				<col halign="center"/>
				<row left="none" bottom="medium">
					<cell right="medium"/>
					<cell><term></term><m>f(x)\ </m> type</cell>
					<cell><term><m>y_p</m> Form</term></cell>
				</row>
				<row>
					<cell>3</cell>
					<cell><m>ax^2 + bx + c</m></cell>
					<cell><m>Ax^2 + Bx + C</m></cell>
				</row>
			</tabular>
		</table>

		<table xml:id="yp-forms-table-row-4"><title> row 4 </title>
			<tabular top="medium" left="medium" right="medium" bottom="minor">
				<col halign="center" top="none" right="minor"/>
				<col halign="center" right="minor"/>
				<col halign="center"/>
				<row left="none" bottom="medium">
					<cell right="medium"/>
					<cell><term></term><m>f(x)\ </m> type</cell>
					<cell><term><m>y_p</m> Form</term></cell>
				</row>
				<row>
					<cell>4</cell>
					<cell><m>ax^3 + bx^2 + cx + d</m></cell>
					<cell><m>Ax^3 + Bx^2 + Cx + D</m></cell>
				</row>
			</tabular>
		</table>

		<table xml:id="yp-forms-table-row-5"><title> row 5 </title>
			<tabular top="medium" left="medium" right="medium" bottom="minor">
				<col halign="center" top="none" right="minor"/>
				<col halign="center" right="minor"/>
				<col halign="center"/>
				<row left="none" bottom="medium">
					<cell right="medium"/>
					<cell><term></term><m>f(x)\ </m> type</cell>
					<cell><term><m>y_p</m> Form</term></cell>
				</row>
				<row>
					<cell>5</cell>
					<cell><m>a e^{\ds\alpha x}</m></cell>
					<cell><m>A e^{\ds\alpha x}</m></cell>
				</row>
			</tabular>
		</table>

		<table xml:id="yp-forms-table-row-6"><title> row 6 </title>
			<tabular top="medium" left="medium" right="medium" bottom="minor">
				<col halign="center" top="none" right="minor"/>
				<col halign="center" right="minor"/>
				<col halign="center"/>
				<row left="none" bottom="medium">
					<cell right="medium"/>
					<cell><term></term><m>f(x)\ </m> type</cell>
					<cell><term><m>y_p</m> Form</term></cell>
				</row>
				<row bottom="medium">
					<cell>6</cell>
					<cell><m>a \sin(\beta x) + b \cos(\beta x)</m></cell>
					<cell><m>A \sin(\beta x) + B \cos(\beta x)</m></cell>
				</row>
			</tabular>
		</table>
	</worksheet>

</subsubsection>