<section xmlns:xi="http://www.w3.org/2001/XInclude"><title> The Integrating Factor </title>

	<p>
		In the previous section, we introduced the idea of solving first-order linear differential equations by manipulating the equation into a form that allows direct integration. This process involved applying a <q>backward</q> product rule to make the left-hand side a perfect derivative. However, most equations are not in the form to do this directly. Instead, there is a missing piece, called the <em>integrating factor</em> that is required for transformation to take place and is the focus of this section.
	</p>

	<p>
		To see this <q>missing</q> piece, lets consider the differential equation:
		<men xml:id="if-example-eqn"> 
			\frac{dy}{dx} + 2y = 5 
		</men>.
		We would like to apply the backward product rule to the left side, but it seems to be missing something. Let's try to figure out what this missing piece is by multipying both sides by something:
		<men xml:id="if-example-eqn-w-missing-piece">
			\us{?}{\boxed{\phantom{\large |P}}}\frac{dy}{dx} + 2\ \us{?}{\boxed{\phantom{\large |P}}}\ y = 5\ \us{?}{\boxed{\phantom{\large |P}}}
		</men>.
		With this missing piece and the fact that <m>y</m> and <m>dy/dx</m> appear in the equation, we should be able to rewrite the equation as:
		<men xml:id="if-example-eqn-goal-w-missing-piece">
			\frac{d}{dx} \Big[\ \us{?}{\boxed{\phantom{\large |P}}} \cdot y\ \Big] = 5\ \us{?}{\boxed{\phantom{\large |P}}}
		</men>.
		To determine what this missing piece is, we need to see where <xref ref="if-example-eqn"/> (start) and <xref ref="if-example-eqn-goal-w-missing-piece"/> (goal) meet in the middle. This is shown below.
		<sidebyside widths="45% 55%" valign="middle">
			<p>
				Notice, the two middle equations agree everywhere except for the expressions in blue. In order for the start and goal equations to be the same, these expressions must match. In other words, the piece that we need to get <xref ref="if-example-eqn-goal-w-missing-piece"/> must satisfy
				<me> 
					{\color{blue} \frac{d\ \boxed{\phantom{|P}}}{dx} = 2\ \boxed{\phantom{|P}}} 
				</me>.
				But, this is the differential equation
				<me>
					\frac{d\mu}{dx} = 2 \mu
				</me>
				where <m>\mu</m> is the unknown!
			</p>
			<p>
				<image source="figures/IF-Idea-GIF-1-repeat.gif" width="100%">
					<shortdescription>(for accessibility)</shortdescription>
				</image>
			</p>
		</sidebyside>
	</p>

	<p>
		Solving this requires you to notice that it is separable and a <xref ref="if-intro-example-details" text="custom">quick calculation</xref> shows that <m>\mu = e^{2x}</m> is the solution. Therefore, if you multiply both sides of <xref ref="if-example-eqn"/> by <m>\mu = e^{2x}</m>, you can use the backward product rule to write the equation as
		<me> \frac{d}{dx}\left[ e^{2x} \cdot y \right] = 5e^{2x} </me>,
		which can then be solved by <xref ref="direct-integration" text="custom">direct integration</xref>. 
	</p>

	<p>
		The function, <m>\mu = e^{2x}</m>, that allowed us to rewrite the equation is called the <em>integrating factor</em>. The general form for this factor is outlined as follows. 
	</p>

	<theorem xml:id="integrating-factor"><title>The Integrating Factor</title>
		<statement>
			<p>
				The <term>integrating factor</term> for the first-order linear differential equation
				<me xml:id="standard-first-order-linear-de">y' + P(x)y = Q(x)</me>
				is <m>\mu = e^{\int P(x) dx}</m>. Multiplying both sides by <m>\mu</m> transforms the equation into:
				<me>\frac{d}{dx}\left[\mu(x) \cdot y\right] = \mu(x)Q(x)</me>.
			</p>
		</statement>
		
		<proof><title>Derivation of the Integrating Factor</title>
			<p>
				Note, all first-order linear differential equations can be written in the form
				<men xml:id="if-general-eqn"> 
					\frac{dy}{dx} + P(x) y = Q(x)
				</men>,
				where <m>P(x)</m> and <m>Q(x)</m> are functions of <m>x</m>. The goal is to write the left-side as a single derivative. However, backward product rule is missing a piece, <m>\mu(x)</m>, that we still need to find. We find <m>\mu(x)</m> by multiplying it onto <xref ref="if-general-eqn"/>, like so
				<sidebyside widths="50% 50%">
					<p>
						<md>
							<mrow> \frac{dy}{dx} + P(x)\amp\ y = Q(x) </mrow>
							<mrow> \mu \frac{dy}{dx} + {\color{blue} \mu P(} \amp\ {\color{blue}\! x)} y = \mu Q(x) </mrow>
							<mrow> {\color{blue} \updownarrow}\ \ \amp \ {\color{blue} \text{match &amp; solve}}</mrow>
							<mrow> \mu \frac{dy}{dx} + {\color{blue} \frac{d\mu}{dx}}\amp\ y = \mu Q(x) </mrow>
							<mrow> \frac{d}{dx}\big[\mu \cdot \amp\ y\big] = \mu Q(x) </mrow>
						</md>
					</p>
					
					<p>
						<md>
							<mrow> {\color{blue} \frac{d\mu}{dx} =}\amp\ {\color{blue} \mu P(x)} </mrow>
							<mrow> {\color{blue} \frac{1}{\mu}d\mu =}\amp\ {\color{blue} P(x) dx} </mrow>
							<mrow> {\color{blue} \int \frac{1}{\mu}d\mu =}\amp\ {\color{blue} \int P(x) dx} </mrow>
							<mrow> {\color{blue} \ln|\mu| =}\amp\ {\color{blue} \int P(x) dx} </mrow>
							<mrow> {\color{blue} \mu =}\amp\ {\color{blue} e^{\int P(x) dx}} </mrow>
						</md>
					</p>
				</sidebyside>
					
			</p>
		</proof>
	</theorem>

	<xi:include href="./p2-c3-s2-interactives.ptx" />

</section>