<section xmlns:xi="http://www.w3.org/2001/XInclude"><title>Definition</title>

	<p>
		In the previous section, we mentioned the importance of integration by parts and <m>e^{-st}</m> to the Laplace transform process. To perform a Laplace transform is to multiply both sides of an equation by <m>e^{-st}</m> and integrate with respect to <m>t</m>. For instance, applying this process to the equation 
		<me>
			e^{-st} \left( y'' + 3y' + 2y \right) = -40e^{3t}
		</me>
		would look like this:
		<md>
			<mrow> 
				e^{-st} \left( y'' + 3y' + 2y \right) 
					=\amp\ e^{-st} \left( -40e^{3t} \right)
			</mrow>
			<mrow> 
				\int e^{-st} \left( y'' + 3y' + 2y \right) \, dt 
					=\amp\ \int e^{-st} \left( -40e^{3t} \right) \, dt
			</mrow>
			<mrow> 
				\ub{\int e^{-st} {\color{blue} y''} \, dt}_{\text{transform of } {\color{blue} y''}} + 
				3\ub{\int e^{-st} {\color{blue} y'} \, dt}_{\text{transform of } {\color{blue} y'}} + 
				2\ub{\int e^{-st} {\color{blue} y} \, dt}_{\text{transform of } {\color{blue} y}} 
					=\amp\ \ub{\int e^{-st} \left( {\color{blue} -40e^{3t}} \right) \, dt}_{\text{transform of } {\color{blue} -40e^{3t}}}
			</mrow>
		</md>.
		As this shows, applying the transform to the equation amounts to applying it to each term of our original equation (in blue). The following definition of the Laplace transform makes this more precise.
	</p>

	<definition><title>Laplace Transform</title>
		<statement>
			The <term>Laplace Transform</term> of a given function <m>f(t)</m> is defined as

			<me> \lap{ {\color{blue} f(t)} } = \int_0^{\infty} e^{-st} {\color{blue} f(t)}\ dt,</me>

			provided that the integral exists (i.e., the improper integral converges).
		</statement>
	</definition>

	<p>
		This definition may appear daunting at first glance, but let's break it down. The <m>\infty</m> in the upper limit signals that we are dealing with an improper integral. In calculus, we learned that improper integrals can be understood as limits. Specifically:
	</p>
	
	<me>
		\int_0^{\infty} e^{-st} f(t)\, dt = \ub{\lim_{b \to \infty} \ob{\int_0^b e^{-st} f(t)\, dt}^{\text{step 1: compute the integral}}}_{\text{step 2: compute the limit}}
	</me>
	
	<p>
		Notice that while the integral involves both <m>s</m> and <m>t</m>, the integration is performed with respect to <m>t</m>. If you're unfamiliar with handling multiple variables like this, simply treat <m>s</m> as a constant during the integration process. Now, let's walk through an example to see this concept in action.
	</p>
	
	<example>

		<m>\ \ </m>Compute <m>\ds \lap{1}</m>.

		<solution>
			<p>
				By the definition above, we have the improper integral
				<men xml:id="lt-1-example-eqn-1"> 
					\lap{1} = \int_0^{\infty} e^{-st} \cdot 1\ dt = \lim_{b \to \infty} \ub{\int_0^b e^{-st}dt}_{I}
				</men>.
				To evaluate this, we treat <m>s</m> as a constant and integrate with respect to <m>t</m>.
				<md>
					<mrow>				
						I = \int_0^b e^{-st}dt
						=\amp\ -\frac{1}{s}e^{-st}\Big|_{t=0}^{t=b}
					</mrow>
					<mrow>			
						=\amp\ -\frac{1}{s}\left[ e^{-sb} - e^{-s\cdot 0} \right]
					</mrow>
					<mrow>			
						=\amp\ -\frac{1}{s}\left[ e^{-sb} - 1 \right]
					</mrow>
				</md>
				Now that we have <m>I</m>, we can plug it into the limit above.
				<md>
					<mrow> 
						\lim_{b \to \infty} -\frac{1}{s}\left[ e^{-sb} - 1 \right]
						=\amp\ -\frac{1}{s} \lim_{b \to \infty} \Big[ e^{-sb} - 1 \Big] 
						\qquad \leftarrow <xref text="custom" ref="reason-factor-out-s">why?</xref>
					</mrow>
					<mrow> 
							=\amp\ -\frac{1}{s} \Big[ \ub{\lim_{b \to \infty} e^{-sb}}_{L} - \us{=\ 1}{\ub{\lim_{b \to \infty} 1}} \Big] 
					</mrow>
				</md>
			</p>
	
			<p>
				The value of the remaining limit, <m>L</m>, depends on whether <m>s</m> is positive or negative. So we consider both cases:
				<ul>
					<li>
						<p>
							<line><m>s &lt; 0:\ </m> Since <m>\ds e^{-(\text{negative})b} = e^{(\text{positive})b} \to \infty</m> as <m>b \to \infty</m></line>
							<line><m>\hspace{4.0em} \implies\ </m> limit diverges (does not exist) when <m>s &lt; 0</m>.</line>
						</p>
					</li>
					<li>
						<p>
							<line><m>s &gt; 0:\ </m> Since <m>\ds e^{-(\text{positive})b} = e^{(\text{negative})b} \to 0</m> as <m>b \to \infty</m></line>
							<line><m>\hspace{4.0em} \implies\ </m> limit converges (exists) when <m>s &gt; 0</m>.</line>
						</p>
					</li>
				</ul>
				To visualize this, here is a <xref ref="compare-exp-graphs" text="custom">graph</xref> comparing <m>s=-1.2\ </m> versus <m>\, +1.2</m>.
			</p>
	
			<p>
				Therefore, when <m>s &gt; 0</m> the Laplace transform exists and evaluates to
				<me>\lap{1} = -\frac{1}{s} [0 - 1] = \frac{1}{s} \quad \text{for } s \gt 0.</me>
			</p>
		</solution>
	
	</example>

	<p>
		Now that we've worked through an example, here are a few key takeaways:
	</p>
	
	<ul marker="square">
		<li>
		<p>
			The Laplace transform always results in a function of <m>s</m>. We typically denote the Laplace transform of <m>f(t)</m> as <m>F(s)</m>. For instance,
			<me> \lap{f(t)} = F(s) \quad \text{or} \quad \lap{q(t)} = Q(s).</me>
		</p>
		</li>
	
		<li>
		<p>
			The values of <m>s</m> for which the integral converges are crucial. While these values usually don't affect the solution to the differential equation, we will make a habit of noting them as we build our Laplace transform toolbox.
		</p>
		</li>
	
		<li>
		<p>
			The notation <m>\lap{}</m> includes curly braces to indicate the function being transformed. These braces are essential, not optional.
		</p>
		</li>
	</ul>
	
	<p>
		With this, we've introduced our first Laplace transform. In the next section, we will explore a collection of common transforms that are used to solve differential equations.
	</p>

	<assemblage xml:id="lt-table-L1"><title>Common Laplace Transform <m>L_1</m></title>
		<p>
			<dl width="narrow">
				<li xml:id="L1"><title><m>{\LARGE \vphantom{\int}}L_1</m></title>
					<m>\ds \lap{ 1 } = \frac{1}{s}, \quad s &gt; 0 </m>
				</li>
			</dl>
		</p>
	</assemblage>


	<xi:include href="./p4-c1-s2-interactives.ptx" />

	
	
	
	
	
	
	
	
	
	
	

</section>
