<subsection xmlns:xi="http://www.w3.org/2001/XInclude"><title>Unit-Step Functions</title>

	<aside>
		<p><xref ref="audio-test1" text="custom"><em>Read Aloud</em></xref>.</p>
		<figure xml:id="audio-test1">
			<caption>Listen to the Audio</caption>
			<audio xml:id="audio-test" source="audio/test-recording-1.mp3" width="100%" />
		</figure>
	</aside>

	<p>
		The two solution techniques we have been studying most recently (undetermined coefficients and laplace transform methods) can be used to solve differential equations that are linear and have constant coefficients. Recall, however, that we would not be able to use the method of undetermined coefficients when the nonhomogeneous function is discontinuous. We will be able to use Laplace transforms to solve such equations, but we first need	to understand the <em>unit step function</em>, which will be used to rewrite discontinuous functions in a particular way.
	</p>
	
	<p>
		We begin by introducing the definition of the standard unit step function.
	</p>

	<definition xml:id="unit-step-function">
		<statement>
			<p>
				The <em> unit step function</em>, <m>U(t)</m>, is defined and graphed as below.
			</p>
			<sidebyside widths="40% 50%">
				<p>
					<me> 
						U(t) = \left\{ 
						\begin{array}{ll}
							0,	&amp; t \lt 0\\
							1,	&amp; t \ge 0
						\end{array} \right.
					</me>
				</p>
				<p>
					<image width="100%">
						<latex-image>
							\begin{tikzpicture}[domain=-3:3]
								\def\a{-2.5}
								\def\b{2.5}
								\def\c{0}

								% Draw the axes
								\draw[thick, -&gt;] (\a, 0) -- (\b, 0) node[right] {$t$};
								\draw[thick, -&gt;] (0, -0.5) -- (0, 1.8);
				
								% Draw the grid
								\draw[very thin,color=gray] (\a,-0.5) grid (\b,1.5);
				
								% Unit step function
								\draw[very thick,blue] (\a,0) -- (\c,0);
								\draw[dashed, blue] (\c,0) -- (\c,1);
								\draw[very thick,blue] (\c,1) -- (\b,1) node[above] {$U(t)$};
								
								% Open circle at the step
								\draw[fill=white] (\c,0) circle (0.08);
								
								% Solid dot at the point of the step
								\filldraw[blue] (\c,1) circle (0.08) node[left] {$1$};
				
							\end{tikzpicture}
						</latex-image>
					</image>
				</p>
			</sidebyside>
		</statement>
	</definition>

	<sidebyside width="60%">
		<stack>

			<image width="100%">
				<latex-image>
					\begin{tikzpicture}[domain=-4:4]
						\def\a{-3}
						\def\b{-2}
						\def\c{1}
						\def\d{3}

						% Draw the axes
						\draw[thick, -&gt;] (\a, 0) -- (\d, 0) node[right] {$t$};
						\draw[thick, -&gt;] (0, -0.5) -- (0, 1.8);
		
						% Draw the grid
						\draw[very thin,color=gray] (\a,-0.5) grid (\d,1.5);
		
						% Unit step function
						\draw[very thick,blue] (\a,0) -- (\b,0);
						\draw[dashed, blue] (\b,0) -- (\b,1);
						\draw[very thick,blue] (\b,1) -- (\d,1);
						\draw[blue] (2,1) node[above] {$U(t+2)$};
						
						% Open circle at the step
						\draw[fill=white] (\b,0) circle (0.08) node[below] {$\b$};
						
						% Solid dot at the point of the step
						\filldraw[blue] (\b,1) circle (0.08) node[left] {$1$};
		
					\end{tikzpicture}
				</latex-image>
			</image>
	
			<image width="100%">
				<latex-image>
					\begin{tikzpicture}[domain=-4:4]
						\def\a{-3}
						\def\b{-2}
						\def\c{1}
						\def\d{3}

						% Draw the axes
						\draw[thick, -&gt;] (\a, 0) -- (\d, 0) node[right] {$t$};
						\draw[thick, -&gt;] (0, -0.5) -- (0, 1.8);
		
						% Draw the grid
						\draw[very thin,color=gray] (\a,-0.5) grid (\d,1.5);
		
						% Unit step function
						\draw[very thick,blue] (\a,0) -- (\c,0);
						\draw[dashed, blue] (\c,0) -- (\c,1);
						\draw[very thick,blue] (\c,1) -- (\d,1);
						\draw[blue] (2,1) node[above] {$U(t-1)$};
						
						% Open circle at the step
						\draw[fill=white] (\c,0) circle (0.08) node[below] {$\c$};
						
						% Solid dot at the point of the step
						\filldraw[blue] (\c,1) circle (0.08) node[left] {$1$};
		
					\end{tikzpicture}
				</latex-image>
			</image>

			<image width="100%">
				<latex-image>
					\begin{tikzpicture}[domain=-4:4]
						\def\a{-3}
						\def\b{-2}
						\def\c{1}
						\def\d{3}

						% Draw the axes
						\draw[thick, -&gt;] (\a, 0) -- (\d, 0) node[right] {$t$};
						\draw[thick, -&gt;] (0, -0.5) -- (0, 1.8);
		
						% Draw the grid
						\draw[very thin,color=gray] (\a,-0.5) grid (\d,1.5);
		
						% Unit step function
						\draw[very thick,blue] (\a,0) -- (\b,0);
						\draw[dashed, blue] (\b,0) -- (\b,1);
						\draw[very thick,blue] (\b,1) -- (\c,1);
						\draw[dashed, blue] (\c,1) -- (\c,0);
						\draw[very thick,blue] (\c,0) -- (\d,0);
						\draw[blue] (-0.5,1) node[above] {$U(t+2)-U(t-1)$};
						
						% Open circle at the step
						\draw[fill=white] (\b,0) circle (0.08) node[below] {$\b$};
						\draw[fill=white] (\c,1) circle (0.08);
						
						% Solid dot at the point of the step
						\filldraw[blue] (\b,1) circle (0.08) node[left] {$1$};
						\filldraw[blue] (\c,0) circle (0.08) node[below] {$\c$};
					\end{tikzpicture}
				</latex-image>
			</image>

		</stack>
		
	</sidebyside>

	<example><title>Let <m>U(t)</m> be the unit step function and <m> f(t) = t^2-2 </m>. Then compute the following values</title>

		<solution><title> <m>U(2.7)</m> </title>
			<p>
				Since <m>t = 2.7 \ge 0</m> (positive),
				<me>U(2.7) = 1.</me>
			</p>
		</solution>

		<solution><title> <m>U(-5.32)</m> </title>

			<p>
				Since <m>-5.32 &lt; 0</m> (negative), 
				<me>U(-5.32) = 0.</me>
			</p>
		
		</solution>

		<solution><title> <m>U(2)\cdot f(2)</m> </title>

			<p>
				<me> U(2)\cdot f(2) = 1\cdot f(2) = (2)^2 - 2 = (4 - 2) = 2.</me>
			</p>

		</solution>

		<solution><title> <m>U(-3)\cdot f(-3)</m> </title>

			<p>
				<me> U(-3)\cdot f(-3) = 0\cdot ((-3)^2 - 2) = 0\cdot (9 - 2) = 0.</me>
			</p>

		</solution>

		<solution><title> <m>U(k)\cdot f(k)</m>, where <m>k \ge 0</m> </title>

			<p>
				Since <m>k \ge 0,</m> we know that <m>U(k) = 1,</m> so
				<me> U(k)\cdot f(k) = 1\cdot f(k) = k^2 - 2.</me>
			</p>

		</solution>

		<solution><title> <m>U(k)\cdot f(k)</m>, where <m>k &lt; 0</m> </title>

			<p>
				Since <m>k \lt 0,</m> we know that <m>U(k) = 0,</m> so
				<me> U(k)\cdot f(k) = 0\cdot f(k) = 0.</me>
			</p>

		</solution>

	</example>

	<p>
		It's important to remember that from this point forward, that the unit step function is well-defined. There is only one unit step function, <m>U(t)</m>, in the same way that there is only one sine function, <m>\sin(t).</m>  We will now build on the definition to learn more about how this function behaves.
	</p>

	<example>
		<p>
			Consider the function <m>f(t) = U(t-3)</m> and complete the following:
			<ol>
				<li>evaluate <m>f(2)</m>.</li>
				<li>evaluate  <m>f(7.43)</m>.</li>
				<li>evaluate  <m>f(-1)</m>.</li>
				<li>evaluate <m>f(k),</m> where <m>k \gt 3</m>.</li>
				<li>evaluate  <m>f(k),</m> where <m>k \lt 3</m>.</li>
				<li>Sketch <m>f(t).</m></li>
				<li>Write <m>f(t)</m> as a piecewise defined function.</li>
			</ol>
		</p>
		
		<p/>
		<solution><title> Solution </title>
			<p>
				<ol>
					<li>
						Notice that <m>f(2) = U(2-3) = U(-1)</m>.  Since the input to the unit step function is	negative, we have <m>f(2) = 0.</m>
					</li>
					<li>
						Similar to the previous question, <m>f(7.43) = U(7.43-3) = U(4.43)</m>.  In this case, the input to the unit step function is positive, so we have <m>f(7.43) = 1.</m>
					</li>
					<li>
						As in the previous two questions, we evaluate <m>f(-1)</m> as follows.
						<me> f(-1) = U(-1 - 3) = U(-4) = 0 </me>
					</li>
					<li>
						Suppose <m>k \gt 3.</m> If we substitute <m>k</m> into the function <m>f</m>, we have <m>f(k) = U(k-3).</m>	In order to evaluate this, we need to know if the input to the unit step function, <m>k - 3</m>, is positive or negative.  Since <m>k \gt 3,</m> we know that <m>k - 3</m> is positive, and therefore
						<me> f(k) = U(k-3) = 1. </me>
					</li>
					<li>
						Suppose now that <m>k \lt 3.</m> If we substitute <m>k</m> into the function <m>f</m>, we have <m>f(k) = U(k-3).</m>	Since <m>k \lt 3,</m> we know that the input to the unit step function, <m>k - 3</m>, is negative, and therefore
						<me> f(k) = U(k-3) = 0. </me>
					</li>
					<li>
						<sidebyside widths="90%" margins="auto" valign="middle">
							<image source="figures/soln_fig2.png" />
						</sidebyside>
						<image xml:id="unit-step-t-minus-3-plot" width="60%">
							<sageplot>
								U = plot(0, (x, -2, 2.9), color='blue', thickness=4, ymin=-1, ymax=1.5, fontsize=20, ticks=[1,1])
								U += plot(1, (x, 3, 5), color='blue', thickness=4, ymin=-1, ymax=1.5, fontsize=20, ticks=[1,1])
								U += point([3,0], color = "blue", faceted=True, size = 80)
								U += point([3,0], color = "white", faceted=True, size = 15)
								U += point([3,1], color = "blue", faceted=True, size = 80)
								U
							</sageplot>
						</image>
					</li>
					<li>
						<me> f(t) =  \left\{ 
							\begin{array}{ll}
								0,	\amp t \lt 3\\
								1,	\amp t \ge 3
							\end{array} \right.
						</me>
					</li>
				</ol>
			</p>
		</solution>
	</example>

	<p>
		This result is consistent with our understanding of shifting functions.  That is, if we want to sketch the graph of the function <m>U(t-3),</m> then we can shift the graph of <m>U(t)</m> three units to the right. Another way to think about this is that the function <m>U(t-3)</m> changes its behavior at <m>t = 3</m> (in that its output is 0 when the input variable <m>t</m> is less than 3 and its output is 1 when the input variable <m>t</m> is greater than 3).
	</p>

	<p>
		Using this same line of thinking, if <m>g(t) = U(t-7),</m> we can surmise that <m>g</m> changes behavior at <m>t = 7</m>.
	</p>

	<example><title>Sketch the function <m>p(t) = -2\ U(t-2)</m></title>
		<solution><title> Sketch <m>p(t)</m> </title>
			<p>
				Since <m>U(t-2)</m> is <m>U(t)</m> shifted to the right by <m>2</m>, the jump in the graph occurs at <m>t=2</m> (see below). Additionally, multiplying by <m>-2</m> reflects the graph about the <m>x</m>-axis and scales it by <m>2</m>, as shown below.
			</p>

			<sidebyside width="75%">
					<image width="100%">
						<latex-image>
							\begin{tikzpicture}

								\def\a{-1}
								\def\t1{2}
								\def\b{5}

								% Axis, Ticks and labels
								\draw[-&gt;] (\a, 0) -- (\b, 0) node[anchor=north] {$t$};
								\draw[-&gt;] (0, -2.6) -- (0, 1.6) node[anchor=east] {$g(t)$};
								\node at (-0.2, 1) {$1$};
								\draw[shift={(0,1)},color=black] (2pt,0pt) -- (-2pt,0pt);
								\node at (-0.3, -2) {$-2$};
								\draw[shift={(0,-2)},color=black] (2pt,0pt) -- (-2pt,0pt);
								\node[anchor=north] at (\t1, 0) {$2$};
								\draw[shift={(\t1,0)},color=black] (0pt,2pt) -- (0pt,-2pt);
								
								% Function plot
								\draw[thick, blue] (\a, 0) -- (\t1, 0);
								\draw[thick, blue] (\t1, -2) -- (\b, -2);
								\draw[thick, black!60!green, opacity=0.3] (\t1, 1) -- (\b, 1);

								% Dots and labels
								\filldraw[black!60!green, opacity=0.8] (\t1, 1) circle (2pt) node[anchor=south west] {$U(t-2)$};
								\filldraw[blue] (\t1, -2) circle (2pt) node[anchor=south west] {$-2U(t-2)$};
								\draw[dashed, opacity=0.2] (\t1, 1) -- (\t1, -2);
								

							\end{tikzpicture}
						</latex-image>
					</image>
			</sidebyside>
		</solution>
	</example>

	<xi:include href="./p4-c5-s1-interactives.ptx" />

</subsection>