<section xmlns:xi="http://www.w3.org/2001/XInclude"><title> Laplace Transforms </title>

	<paragraphs xml:id="LT-s-ne-0-15">
		<title/>
		Notice that when <m>s=0</m>, the term in the integral becomes <m>\ds e^{0t} = 1</m> and we, instead, would get
		<md>
		<mrow>		\amp= 15 \lim_{b \to \infty}\int_0^b 1\ dt
					= 15 \lim_{b \to \infty} t\Big|_0^b
					= 15 \lim_{b \to \infty} b = \infty. 	</mrow>
		</md>
		This shows that when <m>s=0</m>, the integral does not converge (<em>does not exist</em>) as required by the definition of the Laplace Transform. Therefore, when working with Laplace transforms, it is common restrict some values of <m>s</m>.
	</paragraphs>
	
	<paragraphs xml:id="LT-s-ne-0-11t">
		<title/>
		When <m>s=0</m>, the the integral becomes
		<md>
		<mrow>		\amp= \lim_{b \to \infty} \int_0^b 11t\ dt
						= \lim_{b \to \infty} \frac{11t^2}{2}\Big|_0^b
						= \frac{11}{2} \lim_{b \to \infty} b^2 = \infty. 	</mrow>
		</md>
		Therefore, we must have <m>s\ne0</m> for this integral to be finite.
	</paragraphs>
	
	<paragraphs xml:id="LT-s-gt-0-11t">
		<title/>
		If <m>s \lt 0</m>, then as <m>b \to \infty</m>, we would have <m>\ds e^{-sb} \to \infty</m> and so
		<me>\lim_{b \to \infty} \os{\infty}{\os{\uparrow}{\boxed{b}}}\ \us{\infty}{\us{\downarrow}{\boxed{e^{-sb}}}} = \infty.</me>
		This shows the Laplace transform would not exist if <m>s \lt 0</m>. Therefore, we must require <m>s \gt 0</m>.
	</paragraphs>
	
	<paragraphs xml:id="reason-factor-out-s">
		<title/>
		Since the limit only controls <m>b</m>, we treat <m>s</m> as a constant, hence <m>\ds-\frac{1}{s}</m> is also a constant that can be pulled out of the limit.
	</paragraphs>
	
	<paragraphs xml:id="reason-limit-to-zero-e7t">
		<title/>
		Since <m>b \to \infty</m>, then <m>\os{negative}{\ob{(7-s)}}b \to -\infty</m> and therefore,
		<m>\ds e^{\!\!\os{\Large negative}{\ob{(7-s)}}\!\!b} \to 0</m>
	</paragraphs>
	
	<paragraphs xml:id="reason-limit-to-zero-11t">
		<title/>
		We've seen the second limit, but let's review it again. If  <m>s \gt 0</m>, then <m>sb \to \infty</m> and
		<me>
		\lim_{b \to \infty} e^{-sb} = \lim_{b \to \infty}
		\frac{1}{\us{\infty}{\us{\downarrow}{\boxed{e^{sb}}}}} = 0
		</me>
	
		The first limit requires L'Hopital's rule. Remember, when using L'Hopital's rule here, we must take derivatives with respect to <m>b</m> (where <m>s</m> is constant). Here are the details:
		<md>
		<mrow> \lim_{b \to \infty}be^{-sb}
			\amp= \lim_{b \to \infty}\frac{\os{\infty}{\os{\uparrow}{\boxed{b}}}}{\us{\infty}{\us{\downarrow}{\boxed{e^{sb}}}}}
			\,\us{LH}{=}\, \lim_{b \to \infty}\frac{1}{se^{sb}}
			= \frac{1}{s}\lim_{b \to \infty}\frac{1}{\us{\infty}{\us{\downarrow}{\boxed{e^{sb}}}}}
			= 0, \quad s \gt 0</mrow>
		</md>
	</paragraphs>
	
	<paragraphs xml:id="reason-int-by-parts-texpt">
		<title/>
		<md>
		<mrow>  u = t,\quad\amp dv = e^{-st}dt, </mrow>
		<mrow> du = dt,\quad\amp v = -\frac{1}{s}e^{-st}  </mrow>
		</md>
		<md>
		<mrow>  \int_0^b te^{-st} dt
					\amp= \left[t \cdot \left( -\frac{1}{s}e^{-st} \right)
				- \int \left( -\frac{1}{s}e^{-st} \right) dt\right]\Bigg|_0^b	</mrow>
		<mrow> 		\amp= \left[-\frac{t}{s}e^{-st}
				+ \frac{1}{s}\int e^{-st} dt\right]\Bigg|_0^b </mrow>
		<mrow> 		\amp= \left[-\frac{t}{s}e^{-st}
				- \frac{1}{s^2}e^{-st}\right]\Bigg|_0^b</mrow>
		<mrow> 		\amp= \left[\left(-\frac{b}{s}e^{-sb} - \frac{1}{s^2}e^{-sb}\right)
					- \left(-\frac{0}{s^2}e^{-s\cdot 0} - \frac{1}{s^2}e^{-s\cdot 0}\right)\right]</mrow>
		<mrow> 		\amp= \left[-\frac{b}{s}e^{-sb} - \frac{1}{s^2}e^{-sb}
					+ \frac{1}{s^2}\right]	</mrow>
		</md>
	</paragraphs>

	<paragraphs xml:id="std_LT_01">
		<title/>
			<aside>
				<p>
					Key Steps
					<me>
						\begin{array}{ll}
							(1) \amp \text{IBP with }\\
								\amp u = t^2, dv = e^{-st} dt\\
							(2) \amp \text{factor out } -\frac{1}{s}\\
							(3) \amp \text{definition of the}\\
								\amp \text{Laplace transform of } t\\
							(4) \amp \text{convert evaluation at } \infty\\
								\amp \text{to the limit at } \infty \\
							(5) \amp \text{L'Hopital's Rule }\\
						\end{array}
					</me>
				</p>
			</aside>
			<md>
				<mrow> \lap\{ t^2 \}	
						\amp= \int_0^{\infty} e^{-st}\cdot t^2 dt 				</mrow>
				<mrow>  \amp\os{(1)}{=} t^2 \cdot -\frac{1}{s}e^{-st}\Bigg|_0^{\infty}
							- \int_0^{\infty} -\frac{1}{s}e^{-st}\cdot 2tdt </mrow>
				<mrow>  \amp\os{(2)}{=} -\frac{1}{s}\left[ t^2e^{-st}\Bigg|_0^{\infty}
							- 2\int_0^{\infty}e^{-st}\cdot tdt \right]		</mrow>
				<mrow>  \amp\os{(3)}{=} -\frac{1}{s}\left[t^2e^{-st}\Bigg|_0^{\infty}
							- 2\lap\{ t \} \right]							</mrow>
				<mrow>  \amp\os{(4)}{=} -\frac{1}{s}\left[ \lim_{b \to \infty}
							t^2e^{-st}\Bigg|_0^{b} - 2\lap\{ t \} \right]		</mrow>
				<mrow>  \amp= -\frac{1}{s}\left[ \lim_{b \to \infty}
							\left( b^2e^{-sb} - 0^2\cdot e^{-s\cdot 0} \right)
							- 2\cdot \frac{1}{s^2} \right]					</mrow>
				<mrow>  \amp= -\frac{1}{s}\left[ \lim_{b \to \infty}
							b^2e^{-sb} - 0 - \frac{2}{s^2} \right]			</mrow>
				<mrow>  \amp= -\frac{1}{s}\left[ \lim_{b \to \infty}
							\frac{b^2}{e^{sb}} - \frac{2}{s^2} \right]		</mrow>
				<mrow>  \amp\os{(5)}{=} -\frac{1}{s}\left[ \lim_{b \to \infty}
							\frac{2b}{se^{sb}} - \frac{2}{s^2} \right]		</mrow>
				<mrow>  \amp= -\frac{1}{s}\left[ \frac{2}{s}\lim_{b \to \infty}
							\frac{b}{e^{sb}} - \frac{2}{s^2} \right]		</mrow>
				<mrow>  \amp= -\frac{1}{s}\left[ \frac{2}{s}\lim_{b \to \infty}
							\frac{1}{se^{sb}} - \frac{2}{s^2} \right]		</mrow>
				<mrow>  \amp= -\frac{1}{s}\left[ \frac{2}{s}\cdot 0
							- \frac{2}{s^2} \right]							</mrow>
				<mrow>  \amp= \frac{2}{s^3} 									</mrow>
			</md>
	</paragraphs>

	<paragraphs xml:id="std_LT_02">
	<title/>
		<aside>
			<p>
				Key Steps
				<me>
					\begin{array}{ll}
						(1) \amp \text{IBP with }\\
							\amp u = t^3, dv = e^{-st} dt\\
						(2) \amp \text{factor out } -\frac{1}{s}\\
						(3) \amp \text{definition of the}\\
							\amp \text{Laplace transform of } t\\
						(4) \amp \text{convert evaluation at } \infty\\
							\amp \text{to the limit at } \infty \\
						(5) \amp \text{L'Hopital's Rule }\\
					\end{array}
				</me>
			</p>
		</aside>
		<md>
			<mrow> \lap\{ t^3 \}	
					\amp= \int_0^{\infty} e^{-st}\cdot t^3 dt </mrow>
			<mrow>  \amp\os{(1)}{=} t^3 \cdot -\frac{1}{s}e^{-st}\Bigg|_0^{\infty} - \int_0^{\infty} -\frac{1}{s}e^{-st}\cdot 3t^2dt </mrow>
			<mrow>  \amp\os{(2)}{=} -\frac{1}{s}\left[ t^3e^{-st}\Bigg|_0^{\infty} - 3\int_0^{\infty}e^{-st}\cdot t^2 dt \right]</mrow>
			<mrow>  \amp\os{(3)}{=} -\frac{1}{s}\left[ \lim_{b \to \infty}t^3 e^{-st}\Bigg|_0^{b} - 3\lap\{ t^2 \} \right]</mrow>
			<mrow>  \amp\os{(4)}{=} -\frac{1}{s}\left[ \lim_{b \to \infty}\left( b^3 e^{-sb} - 0^3\cdot e^{-s\cdot 0} \right) - 3\cdot \frac{2}{s^3} \right]</mrow>
			<mrow>  \amp= -\frac{1}{s}\left[ \lim_{b \to \infty}b^3 e^{-sb} - 0 - \frac{6}{s^3} \right]</mrow>
			<mrow>  \amp= -\frac{1}{s}\left[ \lim_{b \to \infty}\frac{b^3}{e^{sb}} - \frac{6}{s^3} \right]</mrow>
			<mrow>  \amp\os{(5)}{=} -\frac{1}{s}\left[ \lim_{b \to \infty}\frac{3b^2}{se^{sb}} - \frac{6}{s^3} \right]</mrow>
			<mrow>  \amp= -\frac{1}{s}\left[ \frac{3}{s}\lim_{b \to \infty}\frac{b^2}{e^{sb}} - \frac{6}{s^3} \right]</mrow>
			<mrow>  \amp= -\frac{1}{s}\left[ \frac{3}{s}\lim_{b \to \infty}\frac{2b}{se^{sb}} - \frac{6}{s^3} \right]</mrow>
			<mrow>  \amp= -\frac{1}{s}\left[ \frac{6}{s^2}\lim_{b \to \infty}\frac{b}{e^{sb}} - \frac{6}{s^3} \right]</mrow>
			<mrow>  \amp= -\frac{1}{s}\left[ \frac{6}{s^2}\lim_{b \to \infty}\frac{1}{se^{sb}} - \frac{6}{s^3} \right]</mrow>
			<mrow>  \amp= -\frac{1}{s}\left[ \frac{6}{s^2}\cdot 0 - \frac{6}{s^3} \right]</mrow>
			<mrow>  \amp= \frac{6}{s^4} </mrow>
		</md>
	</paragraphs>

	<paragraphs xml:id="std_LT_03">
	<title/>
		<aside>
			<p>
				Key Steps
				<me>
					\begin{array}{ll}
						(1) \amp \text{IBP with }\\
							\amp u = t^4, dv = e^{-st} dt\\
						(2) \amp \text{factor out } -\frac{1}{s}\\
						(3) \amp \text{definition of the}\\
							\amp \text{Laplace transform of } t\\
						(4) \amp \text{convert evaluation at } \infty\\
							\amp \text{to the limit at } \infty \\
						(5) \amp \text{L'Hopital's Rule }\\
					\end{array}
				</me>
			</p>
		</aside>
		<md>
			<mrow> \lap\{ t^4 \}	
				\amp= \int_0^{\infty} e^{-st}\cdot t^4 dt
			</mrow>
			<mrow>  
				\amp\os{(1)}{=} t^4 \cdot -\frac{1}{s}e^{-st}\Bigg|_0^{\infty} - \int_0^{\infty} -\frac{1}{s}e^{-st}\cdot 4t^3dt
			</mrow>
			<mrow>  
				\amp\os{(2)}{=} -\frac{1}{s}\left[ t^4e^{-st}\Bigg|_0^{\infty} - 4\int_0^{\infty}e^{-st}\cdot t^3 dt \right]
			</mrow>
			<mrow>  
				\amp\os{(3)}{=} -\frac{1}{s}\left[ \lim_{b \to \infty}t^4 e^{-st}\Bigg|_0^{b} - 4\lap\{ t^3 \} \right]
			</mrow>
			<mrow>  
				\amp\os{(4)}{=} -\frac{1}{s}\left[ \lim_{b \to \infty}\left( b^4 e^{-sb} - 0^4\cdot e^{-s\cdot 0} \right) - 4\cdot \frac{6}{s^4} \right]
			</mrow>
			<mrow>  
				\amp= -\frac{1}{s}\left[ \lim_{b \to \infty}b^4 e^{-sb} - 0 - \frac{24}{s^4} \right]
			</mrow>
			<mrow>  
				\amp= -\frac{1}{s}\left[ \lim_{b \to \infty}\frac{4b^3}{se^{sb}} - \frac{24}{s^4} \right]
			</mrow>
			<mrow>  
				\amp= -\frac{1}{s}\left[ \frac{4}{s}\lim_{b \to \infty}\frac{b^3}{e^{sb}} - \frac{24}{s^4} \right]
			</mrow>
			<mrow>  
				\amp\os{(5)}{=} -\frac{1}{s}\left[ \frac{4}{s}\lim_{b \to \infty}\frac{3b^2}{se^{sb}} - \frac{24}{s^4} \right]
			</mrow>
			<mrow>  
				\amp= -\frac{1}{s}\left[ \frac{12}{s^2}\lim_{b \to \infty}\frac{b^2}{e^{sb}} - \frac{24}{s^4} \right]
			</mrow>
			<mrow>  
				\amp= -\frac{1}{s}\left[ \frac{12}{s^2}\lim_{b \to \infty}\frac{2b}{se^{sb}} - \frac{24}{s^4} \right]
			</mrow>
			<mrow>  
				\amp= -\frac{1}{s}\left[ \frac{24}{s^3}\lim_{b \to \infty}\frac{b}{e^{sb}} - \frac{24}{s^4} \right]
			</mrow>
			<mrow>  
				\amp= -\frac{1}{s}\left[ \frac{24}{s^3}\lim_{b \to \infty}\frac{1}{se^{sb}} - \frac{24}{s^4} \right]
			</mrow>
			<mrow>  
				\amp= -\frac{1}{s}\left[ \frac{24}{s^3}\cdot 0 - \frac{24}{s^4} \right]
			</mrow>
			<mrow>  
				\amp= \frac{24}{s^5}
			</mrow>
		</md>
	</paragraphs>

	<p>
		Key Steps
		<ul>
			<li xml:id="lt-derivative-key-step-1">
				Integration by parts with <m>u = f(t)</m> and <m>dv = e^{-st} dt</m>
			</li>
			<li xml:id="lt-derivative-key-step-2">
				<m>s</m> is a constant in this integral, so we can bring it out.
			</li>
			<li xml:id="lt-derivative-key-step-3">
				<m>e^{-st} f(t) = \frac{f(t)}{e^{st}}</m> must go to zero. 
			</li>
		</ul>
	</p>

	<paragraphs xml:id="lt-derivative"><title/>
		<p>
			<!-- <sbsgroup widths="90%"> -->
				<sidebyside widths="20% 70% 10%" valign="top">
					<p>
						<m>\ds \lap\{ f'(t) \}</m>
					</p>
					<p>
						<line><m>\ds =\int_0^{\infty} e^{-st} f'(t) dt </m></line>
						<line><m>\ds =\left[ e^{-st} f(t) \right]_0^{\infty} - \int_0^{\infty} (-s e^{-st}) f(t) dt </m></line>
					</p>
					<p>
						<xref ref="lt-derivative-key-step-1" text="custom">(?)</xref>
					</p>
				</sidebyside>
				<!-- <sidebyside>
					
				</sidebyside>
				<sidebyside>
					
				</sidebyside>
				<sidebyside>
					
				</sidebyside> -->
			<!-- </sbsgroup> -->
		</p>
		<tabular>
			<col width="20%" halign="right" valign="top"/>
			<col width="80%" halign="left" valign="top"/>
			<row>
				<cell valign="top"><p><m>\ds \lap\{ f'(t) \}</m></p></cell>
				<cell><p><m>\ds =\int_0^{\infty} e^{-st} f'(t) dt </m></p></cell>
				<cell></cell>
			</row>
			<row>
				<cell></cell>
				<cell><p><m>\ds =\left[ e^{-st} f(t) \right]_0^{\infty} - \int_0^{\infty} (-s e^{-st}) f(t) dt </m></p></cell>
				<cell><p><xref ref="lt-derivative-key-step-1" text="custom">(?)</xref></p></cell>
			</row>
			<row>
				<cell></cell>
				<cell><m>\ds =\left[ e^{-st} f(t) \right]_0^{\infty} + s \ub{\int_0^{\infty} e^{-st} f(t) dt}_{\large \lap\{ f(t) \}} </m></cell>
				<cell><xref ref="lt-derivative-key-step-2" text="custom">(?)</xref></cell>
			</row>

			<row>
				<cell></cell>
				<cell><m>\ds =\lim_{t \to \infty} \left( e^{-st} f(t) \right) - e^{-s \cdot 0} f(0) + s \lap\{ f(t) \} </m></cell>
				<cell></cell>
			</row>
			<row>
				<cell></cell>
				<cell><m>\ds = 0 - f(0) + s \lap\{ f(t) \} </m></cell>
				<cell><xref ref="lt-derivative-key-step-3" text="custom">(?)</xref></cell>
			</row>

			<row>
				<cell></cell>
				<cell><m>\ds = s \lap\{ f(t) \} - f(0) </m></cell>
				<cell></cell>
			</row>
		</tabular>
		
	</paragraphs>
	

	<paragraphs xml:id="tyu_intro_01_C"> <title/>
		Yes, good job!
	</paragraphs>

	<paragraphs xml:id="tyu_intro_01_I"> <title/>
		No, that's incorrect. The dependent variable is always the variable with the derivative.
	</paragraphs>

	<assemblage>
		<p>
			<dl width="narrow">
				<li xml:id="LT-Table-L1"><title><m>\LARGE \vphantom{\int}</m>L1.</title>
					<m>\ds \lap\{ 1 \} = \frac{1}{s}, \quad s &gt;0 </m>
				</li>
				<li xml:id="LT-Table-L2"><title><m>\LARGE \vphantom{\int}</m>L2.</title>
					<m>\ds \lap\{ e^{at} \} = \frac{1}{s-a}, \quad s &gt;a</m>
				</li>
				<li xml:id="LT-Table-L3"><title><m>\LARGE \vphantom{\int}</m>L3.</title>
					<m>\ds \lap\{ t^n \} = \frac{n!}{s^{n+1}}, \quad s &gt;0 </m>
				</li>
				<li xml:id="LT-Table-L4"><title><m>\LARGE \vphantom{\int}</m>L4.</title>
					<m>\ds \lap\{ \sin (bt) \} = \frac{b}{s^2 + b^2}, \quad s &gt;0</m>
				</li>
				<li xml:id="LT-Table-L5"><title><m>\LARGE \vphantom{\int}</m>L5.</title>
					<m>\ds \lap\{ \cos(bt) \} = \frac{s}{s^2 + b^2}, \quad s &gt;0</m>
				</li>
				<li xml:id="LT-Table-L6"><title><m>\LARGE \vphantom{\int}</m>L6.</title>
					<m>\ds \lap\{ t^n e^{at} \} = \frac{n!}{(s-a)^{n+1}}, \quad s &gt;a </m>
				</li>
				<li xml:id="LT-Table-L7"><title><m>\LARGE \vphantom{\int}</m>L7.</title>
					<m>\ds \lap\{ e^{at} \sin(bt) \} = \frac{b}{(s-a)^2 + b^2}, \quad s &gt;a</m>
				</li>
				<li xml:id="LT-Table-L8"><title><m>\LARGE \vphantom{\int}</m>L8.</title>
					<m>\ds \lap\{ e^{at} \cos(bt) \} = \frac{s-a}{(s-a)^2 + b^2}, \quad s &gt;a</m>
				</li>
				<li xml:id="LT-Table-L9"><title><m>\LARGE \vphantom{\int}</m>L9.</title>
					<m>\ds \lap\{ a f(t) + b g(t) \} = a \lap\{ f(t) \} + b \lap\{ g(t) \}, \quad a, b \text{ constant}</m>
				</li>
				<li xml:id="LT-Table-L10"><title><m>\LARGE \vphantom{\int}</m>L10.</title>
					<m>\ds \lap\{ f'(t) \} = sF(s) - f(0)</m>
				</li>
				<li xml:id="LT-Table-L11"><title><m>\LARGE \vphantom{\int}</m>L11.</title>
					<m>\ds \lap\{ f''(t) \} = s^2 F(s) - sf(0) - f'(0)</m>
				</li>
				<li xml:id="LT-Table-L12"><title><m>\LARGE \vphantom{\int}</m>L12.</title>
					<m>\ds \lap\{ f^{(n)}(t) \} = s^n F(s) - s^{n-1}f(0) - s^{n-2}f'(0) - \cdots - f^{(n-1)}(0)</m>
				</li>
				<li xml:id="LT-Table-L13"><title><m>\LARGE \vphantom{\int}</m>L13.</title>
					<m>\ds \lap\{ t^n f(t) \} = (-1)^n\frac{d^n}{ds^n}\big( \lap\{ t^n f(t) \} \big)</m>
				</li>
				<li xml:id="LT-Table-L14"><title><m>\LARGE \vphantom{\int}</m>L14.</title>
					<m>\ds \lap\{ U(t-a) \} = \frac{e^{-as}}{s}</m>
				</li>
				<li xml:id="LT-Table-L15"><title><m>\LARGE \vphantom{\int}</m>L15.</title>
					<m>\ds \lap\{ f(t) U(t-a) \} = e^{-as} \lap\{ f(t+a) \}</m>
				</li>
				<li xml:id="LT-Table-L16"><title><m>\LARGE \vphantom{\int}</m>L16.</title>
					<m>\ds \lap\{ f(t-a)U(t-a) \} = e^{-as}F(s)</m>
				</li>
			</dl>
		</p>
	</assemblage>

	<!-- <md>
		<mrow xml:id="LT-Table-L1">
			\amp L1: \quad \ds \lap\{ 1 \} = \frac{1}{s}, \quad s>0
		</mrow>
	</md>
	<md>
		<mrow xml:id="LT-Table-L2">
			\amp L2: \quad \ds \lap\{ e^{at} \} = \frac{1}{s-a}, \quad s>a
		</mrow>
	</md>
	<md>
		<mrow xml:id="LT-Table-L3">
			\amp L3: \quad \ds \lap\{ t^n \} = \frac{n!}{s^{n+1}}, \quad s>0
		</mrow>
	</md>
	<md>
		<mrow xml:id="LT-Table-L4">
			\amp L4: \quad \ds \lap\{ \sin (bt) \} = \frac{b}{s^2 + b^2}, \quad s>0
		</mrow>
	</md>
	<md>
		<mrow xml:id="LT-Table-L5">
			\amp L5: \quad \ds \lap\{ \cos(bt) \} = \frac{s}{s^2 + b^2}, \quad s>0
		</mrow>
	</md>
	<md>
		<mrow xml:id="LT-Table-L6">
			\amp L6: \quad \ds \lap\{ t^n e^{at} \} = \frac{n!}{(s-a)^{n+1}}, \quad s>a 
		</mrow>
	</md>
	<md>
		<mrow xml:id="LT-Table-L7">
			\amp L7: \quad \ds \lap\{ e^{at} \sin(bt) \} = \frac{b}{(s-a)^2 + b^2}, \quad s>a
		</mrow>
	</md>
	<md>
		<mrow xml:id="LT-Table-L8">
			\amp L8: \quad \ds \lap\{ e^{at} \cos(bt) \} = \frac{s-a}{(s-a)^2 + b^2}, \quad s>a
		</mrow>
	</md>
	<md>
		<mrow xml:id="LT-Table-L9">
			\amp L9: \quad \ds \lap\{ a f(t) + b g(t) \} = a \lap\{ f(t) \} + b \lap\{ g(t) \}, \quad a, b \text{ constant}
		</mrow>
	</md>
	<md>
		<mrow xml:id="LT-Table-L10">
			\amp L10: \quad \ds \lap\{ f'(t) \} = sF(s) - f(0)
		</mrow>
	</md>
	<md>
		<mrow xml:id="LT-Table-L11">
			\amp L11: \quad \ds \lap\{ f''(t) \} = s^2 F(s) - sf(0) - f'(0)			
		</mrow>
	</md>
	<md>
		<mrow xml:id="LT-Table-L12">
			\amp L12: \quad \ds \lap\{ f^{(n)}(t) \} = s^n F(s) - s^{n-1}f(0) - s^{n-2}f'(0) - \cdots - f^{(n-1)}(0)
		</mrow>
	</md>
	<md>
		<mrow xml:id="LT-Table-L13">
			\amp L13: \quad \ds \lap\{ t^n f(t) \} = (-1)^n\frac{d^n}{ds^n}\big( \lap\{ t^n f(t) \} \big)
		</mrow>
	</md>
	<md>
		<mrow xml:id="LT-Table-L14">
			\amp L14: \quad \ds \lap\{ U(t-a) \} = \frac{e^{-as}}{s}
		</mrow>
	</md>
	<md>
		<mrow xml:id="LT-Table-L15">
			\amp L15: \quad \ds \lap\{ f(t) U(t-a) \} = e^{-as} \lap\{ f(t+a) \}
		</mrow>
	</md>
	<md>
		<mrow xml:id="LT-Table-L16">
			\amp L16: \quad \ds \lap\{ f(t-a)U(t-a) \} = e^{-as}F(s)
		</mrow>
	</md> -->

	<paragraphs xml:id="LT-Table-L14-L16">
	<title/>
		<md>
			<mrow>\amp L14: \quad \ds \lap\{ U(t-a) \} = \frac{e^{-as}}{s}</mrow>
			<mrow>\amp L15: \quad \ds \lap\{ f(t) U(t-a) \} = e^{-as} \lap\{ f(t+a) \}</mrow>
			<mrow>\amp L16: \quad \ds \lap\{ f(t-a)U(t-a) \} = e^{-as}F(s)</mrow>
		</md>
	</paragraphs>

	<paragraphs xml:id="LT-PDF-Details-01">
	<title/>
		<p>
			<md>
				<mrow>4s^3 \amp - 13s^2 + 74s + 27</mrow>
				<mrow>\amp= (As + B)(s+1)^2 + C(s+1)(s^2 - 6s + 25) + D(s^2 - 6s + 25)</mrow>
				<mrow>
					\amp= (As + B)(s^2 + 2s + 1) + (Cs+C)(s^2 - 6s + 25) + Ds^2 - 6Ds + 25D
				</mrow> 
				<mrow>
					\amp= As^3 + 2As^2 + As  + Bs^2 + 2Bs + B + Cs^3 - 6Cs^2 + 25Cs + Cs^2 - 6Cs + 25C + Ds^2 - 6Ds + 25D
				</mrow> 
				<mrow>
					\amp= (A + C)s^3 + (2A+ B - 6C + C + D)s^2 + (A+ 2B + 25C- 6C- 6D)s + (B + 25C + 25D)
				</mrow> 
				<mrow>
					\amp= (A + C)s^3 + (2A+ B - 5C + D)s^2 + (A+ 2B + 19C- 6D)s + (B + 25C + 25D)
				</mrow> 
			</md>
		</p>

		<p>
			Equating coefficients gives us four equations in four unknowns.
			<md>
				<mrow>
				A+C	\amp= 4	\amp	2A+B-5C+D	\amp= -13	\amp A + 2B + 19C - 6D	\amp= 74 \amp B+ 25C + 25D \amp= 27
				</mrow>
				<mrow>	A	\amp= 4-C\amp				\amp		\amp				\amp		\amp\amp</mrow>
				<mrow>		 \amp	\amp 2(4 - C)+B-5C+D	\amp= -13	\amp (4-C)+2B+19C-6D	\amp= 74	\amp\amp</mrow>
				<mrow>		 \amp	\amp 	B - 7C + D	\amp= -21	\amp 	2B+18C-6D	\amp= 70	\amp\amp</mrow>
				<mrow>		 \amp	\amp	B	\amp= 7C - D - 21		\amp				\amp		\amp\amp</mrow>
				<mrow>		 \amp	\amp				\amp	\amp 2(7C - D - 21)+18C-6D	\amp= 70	\amp</mrow> 
				<mrow>		 (7C - D - 21) + 25C + 25D	\amp= 27</mrow>
				<mrow>		 \amp	\amp				\amp		\amp		32C-8D	\amp= 112	\amp</mrow>
				<mrow>		 32C + 24D	\amp= 48</mrow>
				<mrow>		 \amp	\amp				\amp		\amp 			32C	\amp= 8D + 112 \amp\amp</mrow>
				<mrow>		 \amp	\amp				\amp		\amp				\amp		\amp</mrow>
				<mrow>		 (8D + 112) + 24D	\amp= 48</mrow>
				<mrow>		 \amp	\amp				\amp		\amp				\amp		\amp</mrow>
				<mrow>		 32D	\amp= -64</mrow>
				<mrow>		 \amp	\amp				\amp		\amp				\amp		\amp</mrow>
				<mrow>		 D	\amp= -2</mrow>
				<mrow>		 \amp	\amp				\amp		\amp 			32C	\amp= 8(-2) + 112 \amp\amp</mrow>
				<mrow>		 \amp	\amp				\amp		\amp				\amp= 96	\amp\amp</mrow>
				<mrow>		 \amp	\amp				\amp		\amp			C	\amp= 3		\amp\amp</mrow>
				<mrow>		 \amp	\amp	B	\amp= 7(3) - (-2) - 21\amp	\amp				\amp		\amp\amp</mrow>
				<mrow>		 \amp	\amp		\amp= 2		\amp		\amp				\amp		\amp\amp</mrow>
				<mrow>	A	\amp= 4 - (3)\amp	\amp		\amp		\amp				\amp		\amp\amp</mrow>
				<mrow>		\amp= 1	\amp		\amp		\amp		\amp				\amp		\amp\amp</mrow>
			</md>
		</p>
	</paragraphs>

	<paragraphs xml:id="LT-PDF-Details-02">
	<title/>
		<p>
			Partial fraction decomposition has the form,
			<me> \frac{54}{(s+1)(s^2  - 4s + 13)} = \frac{A}{s+1} + \frac{Bs + C}{s^2 - 4s + 13}, </me>
			and we find <m>A</m>, <m>B</m>, and <m>C</m> by
			<md>
				<mrow>54	\amp= A(s^2 - 4s + 13) + (Bs+C)(s+1)</mrow>
				<mrow>54	\amp= As^2 - 4As + 13A + Bs^2 + Bs + Cs + C</mrow>
				<mrow>0s^2 + 0s + 54	\amp= (A + B)s^2 + (-4A + B + C)s + (13A + C)</mrow>
			</md>

			<md>
				<mrow>A+B	\amp= 0		\amp -4A +B+C	\amp= 0	\amp 	13A + C	\amp= 54</mrow>
				<mrow>A	\amp= -B	\amp			\amp	\amp			\amp</mrow>
				<mrow>\amp		\amp -4(-B)+B+C	\amp= 0	\amp 13(-B)+C	\amp= 54</mrow>
				<mrow>\amp		\amp 	5B + C	\amp= 0	\amp -13B + C	\amp= 54</mrow>
				<mrow>\amp		\amp		C	\amp= -5B	\amp		\amp</mrow>
				<mrow>\amp		\amp			\amp	\amp -13B + (-5B)	\amp= 54</mrow>
				<mrow>\amp		\amp			\amp	\amp 		-18B	\amp= 54</mrow>
				<mrow>\amp		\amp			\amp	\amp		B	\amp= -3</mrow>
				<mrow>A	\amp= -(-3)	\amp		C	\amp= -5(-3)\amp			\amp</mrow>
				<mrow>\amp= 3		\amp			\amp= 15\amp			\amp</mrow>
			</md>
		</p>
	</paragraphs>  

	<paragraphs xml:id="LT-Solving_w_LTs_verify_soln">
	<title/>
		<p>
			<md>
				<mrow>x(t)	\amp= 3e^{-t} - 3e^{2t}\cos(3t) + 3e^{2t}\sin(3t)</mrow>
				<mrow>\amp= 3e^{-t} + e^{2t} \Big[ 3\sin(3t) - 3\cos(3t) \Big]</mrow>
				<mrow>\amp</mrow>
				<mrow>x'(t)	\amp= -3e^{-t} + e^{2t}\Big[ 9\cos(3t) + 9\sin(3t) \Big]</mrow>
							+ 2e{2t}\Big[ 3\sin(3t) - 3\cos(3t) \Big]
				<mrow>\amp= -3e^{-t} + e^{2t}\Big[ 9\cos(3t) + 9\sin(3t) + 6\sin(3t) - 6\cos(3t) \Big]</mrow>
				<mrow>\amp= -3e^{-t} + e^{2t}\Big[ 3\cos(3t) + 15\sin(3t) \Big]</mrow>
				<mrow>\amp</mrow>
				<mrow>x''(t)	\amp= 3e^{-t} + e^{2t}\Big[ -9\sin(3t) + 45\cos(3t) \Big]</mrow>
							+ 2e^{2t}\Big[ 3\cos(3t) + 15\sin(3t) \Big]
				<mrow>\amp= 3e^{-t} + e^{2t}\Big[ -9\sin(3t) + 45\cos(3t) + 6\cos(3t) + 30\sin(3t)  \Big]</mrow>
				<mrow>\amp= 3e^{-t} + e^{2t}\Big[ 21\sin(3t) + 51\cos(3t) \Big]</mrow>
			</md>
			
			<md>
				<mrow>LHS	\amp= x'' - 4x' + 13x</mrow>
				<mrow>\amp= \left( 3e^{-t} + e^{2t}\Big[ 21\sin(3t) + 51\cos(3t) \Big] \right) </mrow>
					- 4\left( -3e^{-t} + e^{2t}\Big[ 3\cos(3t) + 15\sin(3t) \Big] \right) 
					+ 13\left( 3e^{-t} + e^{2t} \Big[ 3\sin(3t) - 3\cos(3t) \Big] \right)
				<mrow>\amp= 3e^{-t} + e^{2t}\Big[ 21\sin(3t) + 51\cos(3t) \Big] </mrow>
					+ 12e^{-t} + e^{2t}\Big[ -12\cos(3t) - 60\sin(3t) \Big]  
					+ 39e^{-t} + e^{2t} \Big[ 39\sin(3t) - 39\cos(3t) \Big]
				<mrow>\amp= 3e^{-t} + e^{2t}\Big[ 21\sin(3t) + 51\cos(3t) \Big] </mrow>
					+ 12e^{-t} + e^{2t}\Big[ -12\cos(3t) - 60\sin(3t) \Big]  
					+ 39e^{-t} + e^{2t} \Big[ 39\sin(3t) - 39\cos(3t) \Big]
				<mrow>\amp= 54e^{-t}</mrow>
				<mrow>\amp= RHS</mrow>
			</md>
		</p>

		<p>
			We also verify the initial conditions: 
			<md>
				<mrow>x(0)	\amp= 3e^{-0} + e^{2\cdot 0} \Big[ 3\sin(3\cdot 0) - 3\cos(3\cdot 0) \Big]</mrow>
				<mrow>\amp= 3 + \Big[ 3\cdot 0 - 3\cdot 1 \Big]</mrow>
				<mrow>\amp= 3 - 3</mrow>
				<mrow>\amp= 0</mrow>
				<mrow>\amp</mrow>
				<mrow>x'(0)	\amp= -3e^{-0} + e^{2\cdot 0}\Big[ 3\cos(3\cdot 0) + 15\sin(3\cdot 0) \Big]</mrow>
				<mrow>\amp= -3 + \Big[ 3\cdot 1 + 15\cdot 0 \Big]</mrow>
				<mrow>\amp= - 3 + 3</mrow>
				<mrow>\amp= 0</mrow>
			</md>
		</p>
	</paragraphs>
	
		

</section>