<section xmlns:xi="http://www.w3.org/2001/XInclude"><title> Integrating Factor Method </title>

	<p>
		The integrating factor method provides a systematic approach to solving first-order linear differential equations. These equations can be written in the <em>standard form</em> as:
		<fn>
			<p>
				A general linear differential equation looks like:
				<me> 
					a_n(x)y^{(n)} + \cdots + a_2(x)y'' + a_1(x)y' + a_0(x)y = f(x)
				</me>.
				The first-order case simplifies to:
				<me> 
					a_1(x)y' + a_0(x)y = f(x)
				</me>,
				By dividing through by <m>a_1(x)</m>, this reduces to:
				<me>
					y' + \us{P(x)}{\ub{\frac{a_0(x)}{a_1(x)}}}y = \us{Q(x)}{\ub{\frac{f(x)}{a_1(x)}}}
				</me>.
				This form is called the **standard form** of a first-order linear differential equation:
				<me> 
					y' + P(x)y = Q(x)
				</me>.
			</p>
		</fn>
		<men xml:id="if-standard-form"> 
			y' + P(x)y = Q(x)
		</men>.
		The key to solving such equations lies in finding an <xref ref="integrating-factor" text="custom">integrating factor</xref> that simplifies the left-hand side of the equation into a form that can be solve via <xref ref="direct-integration" text="custom">direct integration</xref>.
	</p>

	<p>
		Now that we've introduced the integrating factor method, let's break down the step-by-step process:
	</p>

	<exploration xml:id="if-method"><title> Integrating Factor Method </title>
		<p>
			Here's the procedure for solving a first-order linear differential equation:
		
			<dl width="narrow">
				<li xml:id="if-step-1"><title> Get the Standard Form &amp; Identify <m>P</m> </title>
					<m>
						\ds\hspace{8.5em}\frac{dy}{dx} + P(x) y = Q(x)
					</m>
				</li>
				<li xml:id="if-step-2"><title> Find the Integrating Factor <m>\mu</m> </title>
					<m>
						\ds\hspace{8.5em}\mu(x) = e^{\int P(x) dx}
					</m>
				</li>
				<li xml:id="if-step-3"><title> Multiply the Equation by <m>\mu</m> &amp; Reverse the Product Rule </title>
					<md>
						<mrow> \mu(x)\frac{dy}{dx} + \mu(x) P(x) y 			=\amp\ \mu(x) Q(x)	</mrow>
						<mrow> \frac{d}{dx}\left[\mu(x)\cdot y\right] 		=\amp\ \mu(x) Q(x) 	</mrow>
					</md>
				</li>
				<li xml:id="if-step-4"><title> Apply Direct Integration </title>
					<m> 
						\ds\hspace{8.5em}\int \frac{d}{dx}\left[\mu(x)\cdot y\right]\ dx = \int\mu(x) Q(x)\ dx
					</m>
				</li>
			</dl>
		</p>
	</exploration> 

	<p>
		Now that we've laid out the method, let's apply it to some concrete examples. In each case, we will follow the four steps outlined above: (1) put the equation into standard form, (2) compute the integrating factor, (3) multiply the equation and simplify using the product rule, and (4) integrate to find the solution.
	</p>

	<example xml:id="if-intro-exercise">
		<m>\ \ </m> Find the general solution to the equation:
		<p> 
			<me>y' + 6y = 1</me>.
		</p>

		<solution><title> Solution </title>
			<p>
				This is a first-order linear equation, so the integrating factor method applies. Since it's already in standard form, we proceed by identifying <m>P(x)</m>.
			</p>

			<p>
				<xref ref="if-step-1" text="title"/>.
				<md>
					<mrow> y' + \os{P}{\boxed{6}}\ y = 1	</mrow>
				</md>
			</p>

			<p>
				<xref ref="if-step-2" text="title"/>.
				<md>
					<mrow> \mu(x) = e^{\int 6\ dx} = e^{6x}	</mrow>
				</md>
				<em>Note: We ignore the constant from integration since we only need one integrating factor to reverse the product rule.</em>
			</p>

			<p>
				<xref ref="if-step-3" text="title"/>.
				<md>
					<mrow> e^{6x}y' + 6e^{6x}y						=\amp\ e^{6x}	</mrow>
					<mrow> \frac{d}{dx}\left[e^{6x}\cdot y\right]	=\amp\ e^{6x}	</mrow>
				</md>
			</p>

			<p>
				<xref ref="if-step-4" text="title"/>.
				<md>
					<mrow> \int \frac{d}{dx}\left[e^{6x}\cdot y\right]\ dx	=\amp\ \int e^{6x}\ dx			</mrow>
					<mrow> e^{6x}\cdot y									=\amp\ \frac{1}{6} e^{6x} + c	</mrow>
					<mrow> y												=\amp\ \frac{1}{6} + ce^{-6x}.	</mrow>
				</md>
			</p>
		</solution>

	</example>

	<example>
		<p>
			Solve the equation: 
			<me>x^2y' = 5x^3 + 2x^3y </me>.
		</p>

		<solution><title> Solution </title>
			<p>
				Rewriting this equation in standard form, we apply the integrating factor method.
			</p>

			<p>
				<xref ref="if-step-1" text="title"/>.
				<md>
					<mrow> y' + \os{P}{\boxed{-2x}} y = 5x	</mrow>
				</md>
			</p>

			<p>
				<xref ref="if-step-2" text="title"/>.
				<md>
					<mrow> \mu(x) = e^{\int -2x\ dx} = e^{-x^2}	</mrow>
				</md>
			</p>

			<p>
				<xref ref="if-step-3" text="title"/>.
				<md>
					<mrow> e^{-x^2}y' - 2x e^{-x^2}y				=\amp\ 5xe^{-x^2}	</mrow>
					<mrow> \frac{d}{dx}\left[e^{-x^2}\cdot y\right]	=\amp\ 5xe^{-x^2}	</mrow>
				</md>
			</p>

			<p>
				<xref ref="if-step-4" text="title"/>.
				<md>
					<mrow> \int \frac{d}{dx}\left[e^{-x^2}\cdot y\right]dx	=\amp\ \int 5xe^{-x^2}dx		</mrow>
					<mrow> e^{-x^2}\cdot y									=\amp\ -\frac{5}{2}e^{-x^2} + c	</mrow>
					<mrow> y												=\amp\ -\frac{5}{2} + ce^{x^2}	</mrow>
				</md>
			</p>

			<solution><title> Solution </title>
		
				<p>
					First we note that this equation is first order and linear, so the integrating factor method applies.
				</p>
	
				<p>
					<xref ref="if-step-1" text="title"/>.
					<md>
						<mrow> y' + \os{P}{\boxed{-2x}} y = 5x	</mrow>
					</md>
				</p>
	
				<p>
					<xref ref="if-step-2" text="title"/>.
					<md>
						<mrow> \mu = e^{\int -2x dx} = e^{-x^2}	</mrow>
					</md>
				</p>
	
				<p>
					<xref ref="if-step-3" text="title"/>.
					<md>
						<mrow> e^{-x^2}y' - 2x e^{-x^2}y				=\amp\ 5xe^{-x^2}	</mrow>
						<mrow> \frac{d}{dx}\left[e^{-x^2}\cdot y\right]	=\amp\ 5xe^{-x^2}	</mrow>
					</md>
				</p>
	
				<p>
					<xref ref="if-step-4" text="title"/>.
					<md>
						<mrow> \int \frac{d}{dx}\left[e^{-x^2}\cdot y\right]dx	=\amp\ \int 5xe^{-x^2}dx		</mrow>
						<mrow> e^{-x^2}\cdot y									=\amp\ -\frac{5}{2}e^{-x^2} + c	</mrow>
						<mrow> y												=\amp\ -\frac{5}{2} + ce^{x^2}	</mrow>
					</md>
				</p>
	
				<solution><title>Verify the Solution</title>
					<p>
						We have found the general solution, but it is worth remembering that we can always verify that we have the correct solution by substituting back into the original equation.
						<md>
							<mrow> \mbox{LHS}	\amp = x^2y'														</mrow>
							<mrow>				\amp = x^2 \cdot \frac{d}{dx}\left( -\frac{5}{2} + ce^{x^2} \right)	</mrow>
							<mrow>				\amp = x^2 \cdot \left( 0 + 2cxe^{x^2} \right)						</mrow>
							<mrow>				\amp = 2c x^3 e^{x^2}												</mrow>
						</md>
		
						<md>
							<mrow>	\mbox{RHS}	\amp = 5x^3 + 2x^3y											</mrow>
							<mrow>				\amp = 5x^3 + 2x^3\left( -\frac{5}{2} + ce^{x^2} \right)	</mrow>
							<mrow>				\amp = 5x^3 - 5x^3+ 2c x^3 e^{x^2}							</mrow>
							<mrow>				\amp = 2c x^3 e^{x^2} = \mbox{LHS}							</mrow>
						</md>
						Since we get the same result when we substitute our solution in on the right and left hand sides of the DE, we confirm that we did find the solution.
					</p>
		</solution>
			
			</solution>

		</solution>

	</example>

	<example>

		<p>
			Find the general solution to the differential equation  
			<me>-\frac{4}{t^2} \cdot M =  t^5 - \frac{1}{t} \cdot\frac{dM}{dt} + 1.</me>
		</p>

		<solution><title> Solution </title>
			<p>
				Since the equation is first order and linear, we can apply the integrating factor method. Here are the steps to solve for <m>M(t)</m>.
			</p>

			<p>
				<xref ref="if-step-1" text="title"/>.
				<md>
					<mrow> \frac{1}{t}\cdot \frac{dM}{dt} - \frac{4}{t^2} \cdot M	\amp =  t^5 + 1	</mrow>
					<mrow> \frac{dM}{dt} + \us{P}{\boxed{-\frac{4}{t}}} \cdot M		\amp = t^6 + t	</mrow>
				</md>
			</p>

			<p>
				<xref ref="if-step-2" text="title"/>.
				<md>
					<mrow> \mu = e^{\large \int \sfrac{-4}{t}\ dt} = e^{-4\ln t} = e^{\ln t^{-4}} = t^{-4} = \frac{1}{t^4}	</mrow>
				</md>
				<em>Note: Since we only need one integrating factor, we ignore absolute value you would normally get from integrating <m>\sfrac{1}{t}</m>.</em>
			</p>

			<p>
				<xref ref="if-step-3" text="title"/>.
				<md>
					<mrow>
						\frac{1}{t^4} \cdot \frac{dM}{dt} - \frac{1}{t^4}\cdot \frac{4}{t} \cdot M	\amp = \frac{1}{t^4}(t^6 + t)
					</mrow>
					<mrow>
						\frac{1}{t^4}\cdot \frac{dM}{dt} - \frac{4}{t^5} \cdot M					\amp = t^2 + t^{-3}
					</mrow>
					<mrow>
						\frac{d}{dt}\left[ \frac{1}{t^4}\cdot M \right]								\amp = t^2 + t^{-3}
					</mrow>
					
				</md>
			</p>

			<p>
				<xref ref="if-step-4" text="title"/>.
				<md>
					<mrow>
						\int  \frac{d}{dt}\left[ \frac{1}{t^4}\cdot M \right]\ dt	\amp = \int t^2 + t^{-3} dt
					</mrow>
					<mrow> 
						\frac{1}{t^4}\cdot M	\amp = \frac{1}{3}t^{3} - \frac{1}{2}t^{-2} + c
					</mrow>
					<mrow> 
						M	\amp = \frac{1}{3}t^{7} - \frac{1}{2}t^2 + ct^4 
					</mrow>

				</md>
			</p>
		</solution>

	</example>

	<p>
		In summary, the integrating factor method can be used to solve any first-order linear equation by transforming it into a form that can be easily solved through direct integration.
	</p>

	<xi:include href="./p2-c3-s3-interactives.ptx" />

</section>