<subsection xmlns:xi="http://www.w3.org/2001/XInclude"><title> Higher-Order Equations </title>

	<p>
		Solving higher-order linear homogeneous constant coefficient (LHCC) equations is an extension of the methods used for second-order equations. The basic strategy remains the same: solve the characteristic equation, then construct the general solution. However, for higher-order equations, the characteristic equation is a higher-degree polynomial, which can make finding the solutions more challenging.
	</p>

	<definition xml:id="def-characteristic-equation">
		<title><em>LHCC Characteristic Equation</em></title>
		<statement>
			<p>
				The <term>characteristic equation</term> of an <m>n</m>-th order LHCC equation
				<me>a_n\ y^{(n)} + a_{n-1}\ y^{(n-1)} + \cdots + a_1\ y' + a_0\ y = 0</me>
				is the <m>n</m>-th degree polynomial
				<fn>
					<xref ref="characteristic-eqn-details" text="custom">Click here for an explanation.</xref>
				</fn>
				<me>a_n\ r^n + a_{n-1}\ r^{n-1} + \cdots + a_1 r + a_0 = 0</me>.
				The solutions to this polynomial, <m>r_1, r_2, \dots r_n</m>, correspond to the roots that determine the form of the general solution.
			</p>
		</statement>
	</definition>
	
	<p>
		In general, the characteristic equation will have <m>n</m> roots, which may be real or complex and may also include repeated roots. Each root of the characteristic equation leads to a term in the general solution of the LHCC. Examples in the table below illustrate the process of constructing these general solutions based on the different types of roots.
	</p>

	<table xml:id="higher-order-lhcc-general-solution-examples"><title>Examples of LHCC General Solutions</title>
		<tabular left="minor" right="minor" top="minor" bottom="minor" halign="center">
			<row>
				<cell>
					<line>Characteristic Equation</line>
					<line>Solutions</line>
				</cell>
				<cell>General Solution</cell>
			</row>
			<row>
				<cell>
					<line><m>r = 3, -3, 5.3</m></line>
					<line><em>(3rd order)</em></line>
				</cell>
				<cell><me>c_1e^{3t} + c_2e^{-3t} + c_3e^{5.3t}</me></cell>
			</row>
			<row>
				<cell>
					<line><m>r = 6 \pm i\sqrt{7.7}, 0</m></line>
					<line><em>(3rd order)</em></line>
				</cell>
				<cell><me>e^{6t}\left(c_1\sin(\sqrt{7.7}t) + c_2\cos(\sqrt{7.7}t)\right) + c_3</me></cell>
			</row>
			<row>
				<cell>
					<line><m>r = -4 \text{ (triple)}, 5.3</m></line>
					<line><em>(4th order)</em></line>
				</cell>
				<cell><me>(c_1t^2 + c_2t + c_3)e^{-4t} + c_4e^{5.3t}</me></cell>
			</row>
			<row>
				<cell>
					<line><m>r = \pm \frac{i}{2}, 2 \pm i</m></line>
					<line><em>(4th order)</em></line>
				</cell>
				<cell><me>c_1\sin\left(\frac{t}{2}\right) + c_2\cos\left(\frac{t}{2}\right) + e^{2t}(c_3\sin t + c_4\cos t)</me></cell>
			</row>
			<row>
				<cell>
					<line><m>r = 0 \text{ (double)}, 3 \text{ (5-repeats)}</m></line>
					<line><em>(7th order)</em></line>
				</cell>
				<cell><me>c_1t + c_2 + (c_3t^4 + c_4t^3 + c_5t^2 + c_6t + c_7)e^{3t}</me></cell>
			</row>
			<row>
				<cell>
					<line><m>r = \pm i, \pi \text{ (double)}, 5</m></line>
					<line><em>(5th order)</em></line>
				</cell>
				<cell><me>c_1\sin t + c_2\cos t + (c_3t + c_4)e^{\pi t} + c_5e^{5t}</me></cell>
			</row>
		</tabular>
	</table>

	<p>
		As the table demonstrates, constructing the general solution of an LHCC equation is systematic once you have the roots of the characteristic equation. However, solving higher-order polynomial equations by hand can be difficult. The next example shows a few algebra techniques you can use to handle higher degree equations.
	</p>

	<example>

		<p>
			Solve the following characteristic equations.
			<ol>
				<li> <m> 4 r^2 - 9 = 0 </m> </li>
				<li> <m> r^3 + 3 r^2 - 4 r = 0 </m> </li>
				<li> <m> r^5 + 10 r^4 = 0 </m> </li>
				<li> <m> r^5 - 4 r^3 = 0 </m> </li>
				<li> <m> r^4 - 25 = 0 </m> </li>
				<li> <m> r^4 - 5r^2 + 4 = 0 </m> </li>
			</ol>
		</p>

		<solution><title> Solution </title>
			<p>
				Note: DoS = Difference of Squares.
				<ol>
					<li>
						<p>
							<tabular>
								<row>
									<cell><m> 4 r^2 - 9 = 0 </m></cell>
									<cell> <m>\leftarrow</m> DoS </cell>
								</row>
								<row>
									<cell><m> (2 r + 3)(2 r - 3) = 0 </m></cell>
									<cell/>
								</row>
								<row>
									<cell><m> 2 r + 3 = 0, \quad 2 r - 3 = 0 </m></cell>
									<cell></cell>
								</row>
								<row>
									<cell><m> \displaystyle r_1 = -\frac32, \quad r_2 = \frac32 </m></cell>
									<cell></cell>
								</row>
							</tabular>
						</p>
					</li>

					<li>
						<p>
							<tabular>
								<row>
									<cell><m> r^3 + 3 r^2 - 4 r = 0 </m></cell>
									<cell> <m>\leftarrow r </m> common </cell>
								</row>
								<row>
									<cell><m> r\ (r^2 + 3 r - 4) = 0 </m></cell>
									<cell/>
								</row>
								<row>
									<cell><m> r\ (r + 4)(r - 1) = 0 </m></cell>
									<cell></cell>
								</row>
								<row>
									<cell><m> \displaystyle r_1 = 0, \quad r_2 = -4, \quad r_3 = 1 </m></cell>
									<cell></cell>
								</row>
							</tabular>
						</p>
					</li>
					
					<li>
						<p>
							<tabular>
								<row>
									<cell><m> r^5 + 10 r^4 = 0 </m></cell>
									<cell> <m>\leftarrow r^4 </m> common </cell>
								</row>
								<row>
									<cell><m> r^4\ (r + 10) = 0 </m></cell>
									<cell/>
								</row>
								<row>
									<cell><m> \displaystyle r_1 = 0\ (\text{4 repeats}), \quad r_2 = -10 </m></cell>
									<cell></cell>
								</row>
							</tabular>
						</p>
						<p>
							<em> Technically, <m>r^4 = (r-0)^4</m> and represents 4 repeated factors. </em>
						</p>
					</li>

					<li>
						<p>
							<tabular>
								<row>
									<cell><m> r^5 - 4 r^3 = 0 </m></cell>
									<cell> <m>\leftarrow</m> common </cell>
								</row>
								<row>
									<cell><m> r^3\ (r^2  - 4) = 0 </m></cell>
									<cell> <m>\leftarrow</m> DoS </cell>
								</row>
								<row>
									<cell><m> r^3\ (r + 2)(r - 2) = 0 </m></cell>
									<cell/>
								</row>
								<row>
									<cell><m> \displaystyle r_1 = 0\ (\text{3 repeats}), \quad r_2 = -2, \quad r_3 = 2 </m></cell>
									<cell></cell>
								</row>
							</tabular>
						</p>
					</li>

					<li>
						<p>
							<tabular>
								<row>
									<cell><m> r^4 - 25 = 0 </m></cell>
									<cell> <m>\leftarrow</m> DoS </cell>
								</row>
								<row>
									<cell><m> (r^2 + 5)(r^2  - 5) = 0 </m></cell>
									<cell> <m>\leftarrow</m> DoS </cell>
								</row>
								<row>
									<cell><m> (r^2 + 5)(r - \sqrt{5})(r + \sqrt{5}) = 0 </m></cell>
									<cell/>
								</row>
								<row>
									<cell><m> r^2 + 5 = 0, \quad r - \sqrt{5} = 0, \quad r + \sqrt{5} = 0 </m></cell>
									<cell></cell>
								</row>
								<row>
									<cell><m> \displaystyle r_1 = -i\sqrt{5}, \quad r_2 = i\sqrt{5}, \quad r_3 = -\sqrt{5}, \quad r_4 = \sqrt{5} </m></cell>
									<cell></cell>
								</row>
							</tabular>
						</p>
					</li>

					<li>
						<p>
							<md>
								<mrow> r^4 - 5r^2 + 4 = 0 </mrow>
							</md>.
							Let <m>u = r^2</m>, then we can rewrite the equation as:
							<md>
								<mrow> u^2 - 5u + 4 = 0 </mrow>
							</md>.
							Solving for <m>u</m>, we get:
							<md>
								<mrow> u = 1, \quad u = 4 </mrow>
							</md>.
							Thus, <m>r^2 = 1</m> gives <m>r = \pm 1</m>, and <m>r^2 = 4</m> gives <m>r = \pm 2</m>. The general solution is:
							<me> y = c_1 e^{x} + c_2 e^{-x} + c_3 e^{2x} + c_4 e^{-2x} </me>.
						</p>
					</li>
				</ol>
			</p>
		</solution>
	</example>

	<p>
		These factoring techniques useful, but they only apply to specific forms of polynomials and it is unlikely that you will be lucky enough to encounter such forms in practice. Therefore, it is reasonable to use technology to aid you with these tyes of problems. Many software tools are available and you are encouraged to use any that you are familiar with.
	</p>

	<example>

		<p>
			Find the general solution to the LHCC equations
			<ol>
				<li> <m> y''' - 6y'' + 11y' - 6y = 0 </m> </li>
				<li> <m> 2 y^{(4)} + 9 y''' + y'' - 21 y' + 9 y  = 0 </m> </li>
			</ol>
			using the <xref ref="poly-factor-p" text="title"/>.
		</p>

		<solution><title> Solution </title>
			<p>
		<ol>
				<li> 
					<p>
						First, write down the characteristic equation:
						<md>
							<mrow> r^3 - 6r^2 + 11r - 6 = 0 </mrow>
						</md>.
						Plugging this into to the factoring tool shows that it factors as <m> (r-3)(r-2)(r-1) </m>.	Solving for <m>r</m>, we get
						<md>
							<mrow> r = 1, \quad r = 2, \quad r = 3 </mrow>
						</md>.
						Therefore, the general solution is:
						<me> y = c_1 e^{x} + c_2 e^{2x} + c_3 e^{3x} </me>.
					</p>
				</li>
				<li> 
					<p>
						The characteristic equation is:
						<me>
							9 r^5 - 4 r^4 + r + 10 = 0
						</me>
						which is challenging to solve by hand. However, typing it into factoring tool above shows that it can be factored as
						<me>
							2\left(r+3\right)^2 \left(r-1\right) \left(r-\frac12\right) = 0
						</me>,
						which gives the solutions
						<me>
							r = -3, \quad r = -3, \quad r = 1, \quad r = \frac12
						</me>.
						Therefore, the general solution is:
						<me>
							y = (c_1x + c_2) e^{-3x} + c_3 e^{x} + c_4 e^{\frac12 x}
						</me>.
					</p>
				</li>
			</ol>
			
			</p>
		</solution>
	</example>
	
	<p>
		Besides factoring software, another options is to use numerical solvers. The next example illustrates this.
	</p>
	
	<example>
		<p>
			Consider the fifth-order LHCC equation:
			<me> y^{(5)} - 4y''' + 3y'' - y = 0 </me>.
		</p>
		<solution><title> Solution </title>
			<p>
				The characteristic equation is:
				<me> r^5 - 4r^3 + 3r^2 - 1 = 0 </me>.
				Solving this polynomial equation analytically is challenging, so we use a numerical solver (<url href="https://www.wolframalpha.com/input?i=r%5E5-4*r%5E3%2B3*r%5E2-1">Wolfram Alpha</url>). This equation has five roots. Three are real:
				<me> r_1 \approx -2.29, \quad r_2 \approx -0.46, \quad r_3 \approx 1.52, </me>
				and two are complex:
				<me> r_4 \approx 0.61 + 0.5i, \quad r_5 \approx 0.61 - 0.5i </me>.
				The general solution, incorporating these roots, is:
				<md> 
					<mrow> y = c_1 e^{-2.29x} + c_2 e^{-0.46x}	+\amp\ c_3 e^{1.52x}								</mrow>
					<mrow> 										+\amp\ e^{0.61x} (c_4 \cos(0.5x) + c_5 \sin(0.5x))	</mrow>
				</md>.
				<me>y = c_1e^{-2.29t} + c_2e^{-0.46t} + c_3e^{1.52t} + e^{0.61t}(c_4\cos(0.5t) + c_5\sin(0.5t))</me>.
			</p>
		</solution>
	</example>
	
	<p>
		By recognizing the nature of the roots and utilizing appropriate technology for solving polynomial equations, we can tackle higher-order LHCC equations with confidence.
	</p>

	<xi:include href="./p3-c1-s5-interactives.ptx" />

</subsection> 