<subsection xmlns:xi="http://www.w3.org/2001/XInclude"><title> Integrating Factor (IF) Method </title>	
	
	<introduction>
		<p>
			The integrating factor method provides a systematic approach to solving any first-order linear differential equations. These equations can always be written in the following <term>standard form</term>
			
			<men xml:id="if-standard-form"> 
				y' + P(x)\ y = Q(x)
			</men>.
		</p>


		<theorem><title>Standard Form Explained</title>
				
			<statement>
				<p>
					A general linear differential equation looks like:
					<me> 
						a_n(x)y^{(n)} + \cdots + a_2(x)y'' + a_1(x)y' + a_0(x)y = f(x)
					</me>.
					The first-order case simplifies to:
					<me> 
						a_1(x)y' + a_0(x)y = f(x)
					</me>,
					Dividing by the coefficient of <m>y'</m>, gives the standard form, since
					<me>
						y' + \us{P(x)}{\ub{\frac{a_0(x)}{a_1(x)}}}y	= \us{Q(x)}{\ub{\frac{f(x)}{a_1(x)}}}	
						\quad \implies \quad 
						y' + P(x)y	= Q(x)
					</me>.
				</p>
			</statement>

		</theorem>

		<p>	
			The key to solving such equations lies in providing an <xref ref="def-integrating-factor" text="custom">integrating factor</xref> that permits an <q>un-doing</q> of a product rule on the left-hand side of the equation, leading to an equation that can be solved by <xref ref="direct-integration" text="custom">direct integration</xref>.
		</p>

	</introduction>

	<subsubsection xmlns:xi="http://www.w3.org/2001/XInclude"><title> Integrating Factor Method Steps </title>

		<p>
			Now that we've introduced the integrating factor method, let's break down the step-by-step process:
		</p>

		<exploration xml:id="if-method"><title> Integrating Factor (IF) </title>
			<p>
				A differential equation that is first-order and linear can be written as
				<men xml:id="if-standard-eqn">
					\frac{dy}{dx} + P(x) y = Q(x)
				</men>
				and its general solution can be found through the steps below.
				<dl width="narrow">
					<li xml:id="if-step-1"><title> Get the Integrating Factor </title>
						<p>
							Identify <m>P(x)</m> and compute the integrating factor
							<me>
								\mu = e\vphantom{\large|}^{\textstyle\int P(x)\ dx}
							</me>
							
						</p>
					</li>
					<li xml:id="if-step-2"><title> Reverse the Product Rule </title>
						<p>
							Multiply <xref ref="if-standard-eqn"/> by <m>\mu</m> and reverse the product rule on the left-side of the new equation.
						</p>

						<p>
							<sidebyside valigns="middle middle middle top" widths="15% 5% 55% 10%">
								<p>
									<q>reverse</q> product rule
								</p>
								<p>
									<me>
										\left\lbrace\vphantom{\begin{array}{c}\\\\\\\end{array}}\right.
									</me>
								</p>
								<p>
									<md>
										<mrow>	\mu\frac{dy}{dx} + P(x) \mu y	=\amp\ Q(x)	\mu	</mrow>
										<mrow>\frac{d}{dx}\left[\mu \cdot y\right]	=\amp\ Q(x) \mu	</mrow>
									</md>
								</p>
								<p/>
							</sidebyside>
						</p>
					</li>
					<li xml:id="if-step-3"><title> Apply Direct Integration </title>
						<p>
							Finally, apply <xref ref="direct-integration" text="custom">direct integration</xref> to remove the derivative and isolate <m>y</m>.
						</p>

						<p>
							<me> 
								\int \frac{d}{dx}\left[\mu \cdot y\right]\ dx = \int Q(x) \mu\ dx
							</me>
						</p>
					</li>
				</dl>
			</p>
		</exploration>

		<xi:include href="./chkpts-3-1-if-method-steps.ptx" />

	</subsubsection>

	<subsubsection xmlns:xi="http://www.w3.org/2001/XInclude"><title> Integrating Factor Method Examples </title>

		<p>
			Now that we've laid out the method, let's apply it to some concrete examples. In each case, we will put the equation into standard form, compute the integrating factor, use it to rewrite the equation, and integrate to find the solution.
		</p>

		<example xml:id="if-intro-exercise">

			<p>
				<statement>
					<p>
						Find the general solution to the equation
					</p>
					<p>
						<me> 
							y' + 6y = 1
						</me>.
					</p>
				</statement>
			</p>

			<p>
				<solution>

					<p>
						This is a first-order linear equation and it is already in standard form, so we proceed with the integrating factor method.
					</p>

					<p>
						<term> <xref ref="if-step-1" text="custom">Step 1: Integrating Factor</xref> </term>
					</p>

					<p>
						Identify <m>P(x)</m> and compute <m>\mu</m>
						<me>
							y' + \os{P}{\boxed{6}}\ y = 1\quad \rightarrow \quad \mu = e^{\int 6\ dx} = e^{6x}
						</me>
						<em>Recall, we can ignore the integration constant for the integrating factor.</em>
					</p>

					<p>
						<term> <xref ref="if-step-2" text="custom">Step 2: Reverse Product Rule</xref> </term>
					</p>

					<p>
						Multiply both sides by <m>e^{6x}</m> and reverse the product rule on the left side.
						<md>
							<mrow> e^{6x}y' + 6e^{6x}y						=\amp\ e^{6x}	</mrow>
							<mrow> \frac{d}{dx}\left[e^{6x}\cdot y\right]	=\amp\ e^{6x}	</mrow>
						</md>
					</p>

					<p>
						<term> <xref ref="if-step-3" text="custom">Step 3: Direct Integration</xref> </term>
					</p>

					<p>
						<md>
							<mrow> \int \frac{d}{dx}\left[e^{6x}\cdot y\right]\ dx	=\amp\ \int e^{6x}\ dx			</mrow>
							<mrow> e^{6x}\cdot y									=\amp\ \frac{1}{6} e^{6x} + c	</mrow>
							<mrow> y												=\amp\ \frac{1}{6} + ce^{-6x}.	</mrow>
						</md>
					</p>
				</solution>
			</p>

		</example>

		<example>

			<p>
				<statement>
					<p>
						Solve the equation
					</p>
					<p>
						<me>x^2y' = 5x^3 + 2x^3y </me>.
					</p>
				</statement>
			</p>

			<p>
				<solution>

					<p>
						This equation is first-order and linear, but is not in standard form, so we rewrite it as
						<me>
							y' - 2x y = 5x
						</me>
						and now we can apply the integrating factor method.
					</p>

					<p>
						<term> <xref ref="if-step-1" text="custom">Step 1: Integrating Factor</xref> </term>
					</p>

					<p>
						Identify <m>P(x)</m> and compute <m>\mu</m>
						<me>
							y' + \os{P}{\boxed{-2x}} y = 5x \quad \rightarrow \quad \mu = e^{\int -2x\ dx} = e^{-x^2}
						</me>
					</p>

					<p>
						<term> <xref ref="if-step-2" text="custom">Step 2: Reverse Product Rule</xref> </term>
					</p>

					<p>
						Multiply by <m>e^{-x^2}</m> and reverse the product rule on the left.
						<md>
							<mrow> e^{-x^2}y' - 2x e^{-x^2}y				=\amp\ 5xe^{-x^2}	</mrow>
							<mrow> \frac{d}{dx}\left[e^{-x^2}\cdot y\right]	=\amp\ 5xe^{-x^2}	</mrow>
						</md>
					</p>

					<p>
						<term> <xref ref="if-step-3" text="custom">Step 3: Direct Integration</xref> </term>
					</p>

					<p>
						<md>
							<mrow> \int \frac{d}{dx}\left[e^{-x^2}\cdot y\right]dx	=\amp\ \int 5xe^{-x^2}dx		</mrow>
							<mrow> e^{-x^2}\cdot y									=\amp\ -\frac{5}{2}e^{-x^2} + c	</mrow>
							<mrow> y												=\amp\ -\frac{5}{2} + ce^{x^2}	</mrow>
						</md>
					</p>

					<solution><title>Verify the Solution</title>

						
						<p>
							We have found the general solution, but it is worth remembering that we can verify our solution by substituting back into the original equation.
						</p>

						<sidebyside>
							<p>
								<md>
									<mrow>	\ul{LHS}														</mrow>
									<mrow>	x^2y'															</mrow>
									<mrow>	x^2 \cdot \frac{d}{dx}\left( -\frac{5}{2} + ce^{x^2} \right)	</mrow>
									<mrow>	x^2 \cdot \left( 0 + 2cxe^{x^2} \right)							</mrow>
									<mrow>	2c x^3 e^{x^2}	\quad✅											</mrow>
								</md>
							</p>

							<p>
								<md>
									<mrow>	\ul{RHS}											</mrow>
									<mrow>	5x^3 + 2x^3y										</mrow>
									<mrow>	5x^3 + 2x^3\left( -\frac{5}{2} + ce^{x^2} \right)	</mrow>
									<mrow>	5x^3 - 5x^3+ 2c x^3 e^{x^2}							</mrow>
									<mrow>	2c x^3 e^{x^2}	\quad✅								</mrow>
								</md>
							</p>
						</sidebyside>
						
						<p>
							The same result on the left &amp; right confirms our solution.
						</p>
					</solution>

				</solution>
			</p>

		</example>

		<example>

			<p>
				<statement>
					<p>
						Find the general solution to the differential equation
					</p>
					<p>
						<me>-\frac{4}{t^2} \cdot M =  t^5 - \frac{1}{t} \cdot\frac{dM}{dt} + 1.</me>
					</p>
				</statement>
			</p>

			<p>
				<solution>

					<p>
						This equation is first-order and linear, but is not in standard form, so we rewrite it as
						<md>
							<mrow> \frac{1}{t}\cdot \frac{dM}{dt} - \frac{4}{t^2} \cdot M	\amp =  t^5 + 1	</mrow>
							<mrow> \frac{dM}{dt} + \us{P}{\boxed{-\frac{4}{t}}} \cdot M		\amp = t^6 + t	</mrow>
						</md>
						and now we can apply the integrating factor method.
					</p>
					

					<p>
						<sidebyside widths="20% 80%" valigns="top middle">
							
							<p>
								Integrating <m>\rightarrow</m> Factor 
							</p>

							<p>
								<me> 
									\mu = e\vphantom{\large|}^{\int \sfrac{-4}{t}\ dt} = e^{-4\ln t} = e^{\ln t^{-4}} = t^{-4} = \frac{1}{t^4}
								</me>
							</p>

						</sidebyside>
					</p>

					<p>
						<sidebyside widths="20% 80%" valigns="top middle">
							
							<p>
								Reverse <m>\rightarrow</m> Product Rule
							</p>

							<p>
								<md>
									<mrow>
										\frac{1}{t^4} \frac{dM}{dt} - \frac{1}{t^4} \frac{4}{t} M
											\amp = \frac{1}{t^4}(t^6 + t)
									</mrow>
									<mrow>
										\frac{1}{t^4} \frac{dM}{dt} - \frac{4}{t^5} M
											\amp = t^2 + t^{-3}
									</mrow>
									<mrow>
										\frac{d}{dt}\left[ \frac{1}{t^4} M \right]
											\amp = t^2 + t^{-3}
									</mrow>
								</md>
							</p>

						</sidebyside>
					</p>

					<p>
						<sidebyside widths="20% 80%" valigns="top middle">
							
							<p>
								Direct <m>\rightarrow</m> Integration 
							</p>

							<p>
								<md>
									<mrow>
										\int \frac{d}{dt}\left[ \frac{1}{t^4} M \right]\ dt
											\amp = \int \left(t^2 + t^{-3}\right) dt
									</mrow>
									<mrow> 
										\frac{1}{t^4} M
											\amp = \frac{1}{3}t^{3} - \frac{1}{2}t^{-2} + c
									</mrow>
								</md>
							</p>

						</sidebyside>
					</p>

					<p>
						<sidebyside widths="20% 80%" valigns="top middle">
							
							<p>
								General <m>\rightarrow</m> Solution
							</p>

							<p>
								<me>
									M = \frac{1}{3}t^{7} - \frac{1}{2}t^2 + ct^4
								</me>.
							</p>

						</sidebyside>
					</p>

				</solution>
			</p>

		</example>

		<p>
			The next set of examples will require more advanced algebra and/or calculus techniques, but they will still follow the same three-step process illustrated in the previous examples.
		</p>

		<example>

			<p>
				<statement>
					<p>
						Solve the differential equation: 
						<me>x^2 y' - y = 1, \quad x > 0</me>.
					</p>
				</statement>
			</p>
			
			<p>
				<solution>
					<p>
						This is a first-order linear differential equation, so we can apply the integrating factor method.
					</p>
				
					<p>
						<xref ref="if-step-1" text="title"/>.
						<md>
							<mrow> y' + \us{P}{\boxed{-\frac{1}{x^2}}}\ y = \frac{1}{x^2}	</mrow>
						</md>
					</p>
				
					<p>
						<xref ref="if-step-1" text="title"/>.
						<md>
							<mrow> \mu(x) = e^{\large \int -\sfrac{1}{x^2} dx} = e^{1/x}	</mrow>
						</md>
					</p>
				
					<p>
						<xref ref="if-step-2" text="title"/>.
						<md>
							<mrow> e^{1/x}y' - \frac{e^{1/x}}{x^2} y	=\amp\ \frac{e^{1/x}}{x^2}	</mrow>
							<mrow> \frac{d}{dx}\left[e^{1/x} y\right]	=\amp\ \frac{e^{1/x}}{x^2}	</mrow>
						</md>
					</p>
				
					<p>
						<xref ref="if-step-3" text="title"/>.
						<md>
							<mrow> \int \frac{d}{dx}\left[e^{1/x} y\right] dx =\amp\ \int \frac{e^{1/x}}{x^2} dx \quad \left(u = \sfrac{1}{x}\right)	</mrow>
							<mrow> e^{1/x} y =\amp\ \int -e^u du	</mrow>
							<mrow> e^{1/x} y =\amp\ -e^u + c	</mrow>
							<mrow> e^{1/x} y =\amp\ -e^{1/x} + c	</mrow>
						</md>
						Now, we can solve for <m>y</m>:
						<md>
							<mrow> y = -1 + ce^{-1/x}	</mrow>
						</md>
					</p>
				</solution>
			</p>

		</example>

		<example>

			<p>
				<statement>
					<p>
						Solve the equation: 
						<me> t^2 y' + 2ty = t^3 \ln t </me>.
					</p>
				</statement>
			</p>

			<p>
				<solution>
					<p>
						This is a linear equation, and we will solve it using the integrating factor method.
					</p>

					<p>
						<xref ref="if-step-1" text="title"/>.
						<md>
							<mrow> y' + \frac{2}{t} y = t \ln t </mrow>
						</md>
					</p>

					<p>
						<xref ref="if-step-1" text="title"/>.
						<md>
							<mrow> \mu(t) = e^{\large \int (\sfrac{2}{t})\, dt} = e^{2 \ln t} = t^2	</mrow>
						</md>
					</p>

					<p>
						<xref ref="if-step-2" text="title"/>.
						<md>
							<mrow> t^2 y' + 2t y					=\amp\ t^3 \ln t	</mrow>
							<mrow> \frac{d}{dt} \left[t^2 y\right]	=\amp\ t^3 \ln t	</mrow>
						</md>
					</p>

					<p>
						<xref ref="if-step-3" text="title"/>.
						<md>
							<mrow> \int \frac{d}{dt} \left[t^2 y\right] dt	=\amp\ \int t^3 \ln t\ dt	</mrow>
							<mrow> t^2 y									=\amp\ \int t^3 \ln t\ dt	</mrow>
						</md>
						Using <xref ref="ibp-formula" text="custom">integration by parts</xref> on the integral with
						<md>
							<mrow>u = \ln t,			\amp \quad v = \frac14t^4	</mrow>
							<mrow>du = \frac{1}{t}\ dt,	\amp \quad dv = t^3\ dt		</mrow>
						</md>
						gives us
						<md>
							<mrow> t^2 y	=\amp\ \frac14 t^4 \ln t - \int \frac14 t^4 \cdot \frac{1}{t}\ dt	</mrow>
							<mrow> t^2 y	=\amp\ \frac14 t^4 \ln t - \frac14 \int  t^3\ dt	</mrow>
							<mrow> t^2 y	=\amp\ \frac{t^4}{4} \ln t - \frac{t^4}{16} + c	</mrow>
							<mrow> y		=\amp\ \frac{t^2}{4} \ln t - \frac{t^2}{16} + c\,t^2	</mrow>
						</md>
					</p>
				</solution>
			</p>

		</example>

		<example>

			<p>
				<statement>
					<p>
						Solve the initial value problem. 
						<me>A = \sec\theta A' - \frac{\theta e^{\theta^2 + \sin\theta}}{\cos \theta}, \hspace{1cm} A(0) = -\frac{1}{2}</me>.
					</p>
				</statement>
			</p>

			<p>
				<solution>
					<p>
						Before applying the integration factor method, we note that the equation is first order and linear.
					</p>

					<p>
						<xref ref="if-step-1" text="title"/>.
						<md>
							<mrow>
								\sec\theta A' - A
									=\amp\ \frac{\theta e^{\theta^2 + \sin\theta}}{\cos \theta}	\qquad \text{Note: } \sec\theta = \frac{1}{\cos\theta}
							</mrow>
							<mrow>
								A' + \us{P}{\boxed{- \cos\theta}}\ A	
									=\amp\ \theta e^{\theta^2 + \sin\theta}
							</mrow>
						</md>
					</p>

					<p>
						<xref ref="if-step-1" text="title"/>.
						<md>
							<mrow> \mu = e^{\int -\cos\theta d\theta} = e^{-\sin\theta}	</mrow>
						</md>
					</p>

					<p>
						<xref ref="if-step-2" text="title"/>.
						<md>
							<mrow> e^{-\sin\theta}A' - \cos\theta e^{-\sin\theta}A = \theta e^{\theta^2 + \sin\theta}	</mrow>
							<mrow> \frac{d}{d\theta}\left[ e^{-\sin\theta}A \right] = \theta e^{\theta^2}	</mrow>
						</md>
					</p>

					<p>
						<xref ref="if-step-3" text="title"/>.
						<md>
							<mrow>
								\int \frac{d}{d\theta}\left[ e^{-\sin\theta}A \right] d\theta = \int \theta e^{\theta^2} d\theta
							</mrow>
							<mrow>
								e^{-\sin\theta}A = \frac{1}{2}e^{\theta^2} + c
							</mrow>
							<mrow>
								A = \frac{1}{2}e^{\theta^2 + \sin\theta} + ce^{\sin\theta}
							</mrow>
						</md>
					</p>

					<p>
						Finally, we apply the initial condition to determine the constant <m>c</m>.
						<md>
							<mrow> -\frac{1}{2} = A(0) = \frac{1}{2}e^{0^2 + \sin(0)} + ce^{\sin(0)} = \frac{1}{2}e^0 + ce^0= \frac{1}{2} + c	</mrow>
							<mrow> -1 = c	</mrow>
						</md>
					</p>

					<p>
						We can then write the particular solution to the initial value problem.
						<me>A(\theta) = \frac{1}{2}e^{\theta^2 + \sin\theta} - e^{\sin\theta}</me>
					</p>
				</solution>
			</p>

		</example>

		<p>
			The integrating factor method is a versatile tool for solving first-order linear differential equations. By reducing the equation to a form that allows for direct integration, we can tackle a wide variety of problems with confidence. The examples in this chapter illustrate the broad applicability of this technique, and practice with a range of equations will solidify your understanding of how to use it effectively.
		</p>

		<xi:include href="./chkpts-3-2-if-method-examples.ptx" />

	</subsubsection>

</subsection>