<exercise label="chkpts-sov-method-examples"><title> <em>Check your Understanding</em> </title>

	<introduction>
		<p>
			Complete the questions on each tab to check your understanding.
		</p>
	</introduction>

	<task label="chkpt-sov-method-examples-1" randomize="true" adaptive="yes"><title> <em>Drag-N-Drop</em> </title>

		<statement>
			<p>
				Suppose you want to use separation of variables method to determine the general solution of the differential equation
				<men xml:id="chkpt-sov-method-examples-1-eqn">
					\ds \frac{dq}{dt} - 3qt^2 = 2q
				</men>.
			</p>
			<p>
				Match the scrambled tasks (on the left) to the task order (on the right) that it should be performed to use this method.
			</p>
		</statement>

		<feedback>
			<p>
				Review the <xref ref="sov-method" text="custom">SOV Method</xref>.
			</p>
		</feedback>

		<matches>
			<match>
				<premise>
					<p>
						<line><m>\text{Equation is 1st-order âœ…}</m></line>
					</p>
				</premise>
				
				<response>
					<p>
						<m>\text{Task 1}</m>
					</p>
				</response>
			</match>

			<match>
				<premise>
					<p>
						<m>\ds \frac{dq}{dt} = q(2 + 3t^2)</m>
					</p>
				</premise>
				<response>
					<p>
						<m>\text{Task 2}</m>
					</p>
				</response>
			</match>
			<match>
				<premise>
					<p>
						<m>\ds \frac{1}{q}\ dq = (2 + 3t^2)\ dt</m>
					</p>
				</premise>
				<response>
					<p>
						<m>\text{Task 3}</m>
					</p>
				</response>
			</match>
			<match>
				<premise>
					<p>
						<m>\ds \int \frac{1}{q} dq = \int (2 + 3t^2) dt</m>
					</p>
				</premise>
				
				<response>
					<p>
						<m>\text{Task 4}</m>
					</p>
				</response>
			</match>
			<match>
				<premise>
					<p>
						<line><m>\ds \ln|q| = 2t^2 + t^3 + c</m></line>
					</p>
				</premise>
				<response>
					<p>
						<m>\text{Task 5}</m>
					</p>	
				</response>
			</match>
			<match>
				<premise>
					<p>
						<line><m>\ds q = c e\vphantom{|}^{\large 2t^2 + t^3}</m></line>
					</p>
				</premise>
				<response>
					<p>
						<m>\text{Task 6}</m>
					</p>
				</response>
			</match>
		</matches>

	</task>

	<task label="chkpt-sov-method-examples-2"><title> <em>Select-the-Best-Answer</em> </title>

		<statement>
			<p>
				In the equation <m>y^2 y' - 1 = 6x^2</m>, what is the first step to solve it using the separation of variables method?
			</p>
		</statement>

		<choices>
			<choice>
				<statement>
					<p>
						Integrate both sides.
					</p>
				</statement>
				<feedback>
					<p>
						Incorrect. You need to separate the variables before integrating.
					</p>
				</feedback>
			</choice>
			<choice>
				<statement>
					<p>
						Isolate <m>y</m>, if possible.
					</p>
				</statement>
				<feedback>
					<p>
						Incorrect. You should first separate the variables.
					</p>
				</feedback>
			</choice>
			<choice>
				<statement>
					<p>
						Divide both sides by <m>y^2</m>
					</p>
				</statement>
				<feedback>
					<p>
						Incorrect. You should first separate the variables.
					</p>
				</feedback>
			</choice>
			<choice correct="yes">
				<statement>
					<p>
						Show it is separable.
					</p>
				</statement>
				<feedback>
					<p>
						Correct! This rearrangement allows us to apply separation of variables.
					</p>
				</feedback>
			</choice>
		</choices>

	</task>

	<task label="chkpt-sov-method-examples-3"><title> <em>Select-the-Best-Answer</em> </title>

		<statement>
			<p>
				Which of the following are valid ways to combine constants when finalizing your solution? Select ALL that apply.
			</p>
		</statement>

		<choices>
			<choice correct="yes">
				<statement>
					<blockquote>
						<md>
							<mrow>	|y|	=\amp\,	e^{2x + c_1}	</mrow>
							<mrow>	y	=\amp\,	c_2 e^{2x}		</mrow>
						</md>
					</blockquote>
				</statement>
				<feedback>
					<p>
						Correct, since
						<md>
							<mrow>	|y|	=\amp\,	e^{2x + c_1}										</mrow>
							<mrow>	y	=\amp\,	\pm e^{2x + c_1}									</mrow>
							<mrow>	y	=\amp\,	\pm e^{2x} \cdot e^{c_1}							</mrow>
							<mrow>	y	=\amp\,	c_2 e^{2x}	\quad \text{where } c_2 = \pm e^{c_1}	</mrow>
						</md>
					</p>
				</feedback>
			</choice>
			<choice correct="yes">
				<statement>
					<blockquote>
						<md>
							<mrow>	\frac{y^2}{2}	=\amp\,	\sin(x) + c_1	</mrow>
							<mrow>	y^2				=\amp\,	2\sin(x) + c_2	</mrow>
						</md>
					</blockquote>
				</statement>
				<feedback>
					<p>
						Correct, since
						<md>
							<mrow>	\frac{y^2}{2}	=\amp\,	\sin(x) + c_1									</mrow>
							<mrow>	y^2				=\amp\,	\sin(x) + 2c_1									</mrow>
							<mrow>	y^2				=\amp\,	2\sin(x) + c_2	\quad \text{where } c_2 = 2c_1	</mrow>
						</md>
					</p>
				</feedback>
			</choice>
			<choice>
				<statement>
					<blockquote>
						<md>
							<mrow>	y^2	=\amp\,	2\sin(x) + c_2				</mrow>
							<mrow>	y	=\amp\,	\pm\sqrt{2\sin(x)} + c_3	</mrow>
						</md>
					</blockquote>
				</statement>
				<feedback>
					<p>
						Incorrect, you should not combine constants here since <m>\quad\sqrt{A + B} \neq \sqrt{A} + \sqrt{B}</m>.
					</p>

					<p>
						Your solution should be written as
						<md>
							<mrow>	y^2	=\amp\,	2\sin(x) + c_2											</mrow>
							<mrow>	y	=\amp\,	\pm\sqrt{2\sin(x) + c_2}\quad \leftarrow\text{ done}	</mrow>
						</md>
					</p>
				</feedback>
			</choice>
			<choice>
				<statement>
					<blockquote>
						<md>
							<mrow>	e^y	=\amp\,	3y + c_1		</mrow>
							<mrow>	y	=\amp\,	\ln(3y) + c_2	</mrow>
						</md>
					</blockquote>
				</statement>
				<feedback>
					
					<p>
						Incorrect, you should not combine constants here since <m>\ln(A + B) \neq \ln(A) + \ln(B)</m>.
					</p>

					<p>
						Your solution should be
						<md>
							<mrow>	e^y	=\amp\,	3y + c_1									</mrow>
							<mrow>	y	=\amp\,	\ln(3y + c_1)\quad \leftarrow\text{ done}	</mrow>
						</md>
					</p>
				</feedback>
			</choice>
			<choice>
				<statement>
					<blockquote>
						<md>
							<mrow>	xy	=\amp\,	e^x + c_1	</mrow>
							<mrow>	y	=\amp\,	\frac{e^x}{x} + c_2	</mrow>
						</md>
					</blockquote>
				</statement>
				<feedback>
					<p>
						Incorrect, you should not combine constants here since <m>\frac{c_1}{x}</m> is not constant. Instead your solution should be left as
						<md>
							<mrow>	xy	=\amp\,	e^x + c_1													</mrow>
							<mrow>	y	=\amp\,	\frac{e^x + c_1}{x}											</mrow>
							<mrow>	y	=\amp\,	\frac{e^x}{x} + \frac{c_1}{x}\quad \leftarrow\text{ done}	</mrow>
						</md> 
					</p>
				</feedback>
			</choice>
			<choice correct="yes">
				<statement>
					<blockquote>
						<md>
							<mrow>	\sqrt{y}	=\amp\,	c_1e^{3x}		</mrow>
							<mrow>	y			=\amp\,	c_2\, e^{6x}	</mrow>
						</md>
					</blockquote>
				</statement>
				<feedback>
					<p>
						Correct, since
						<md>
							<mrow>	\sqrt{y}	=\amp\,	c_1e^{3x}									</mrow>
							<mrow>	y			=\amp\,	(c_1e^{3x})^2								</mrow>
							<mrow>	y			=\amp\,	c_1^2(e^{3x})^2								</mrow>
							<mrow>	y			=\amp\,	c_2\, e^{6x}\quad \text{where } c_2 = c_1^2	</mrow>
						</md>
					</p>
				</feedback>
			</choice>
		</choices>

	</task>

</exercise>