
<section xmlns:xi="http://www.w3.org/2001/XInclude"><title> Summary &amp; Exercises </title>

	<introduction>
		
		<p>
			<assemblage color="green"><title>Summary of the Key Ideas</title>
				<p>
					<term> <em> Method</em> </term>
					<p>
						
					</p>
				</p>
			</assemblage>
		</p>

	</introduction>

	<exercises>

		<exercisegroup>
			<title></title>
				<exercise>
					<statement>
						<alert>Use the definition of Laplace Transform</alert> (above) to find the Laplace Transform of the function
							<m>\ds
								d(t) = \left\{
								\begin{array}{ll}
								0,	\amp t \lt 0\\
								7,	\amp 0 \le t \lt 3\\
								0,	\amp t \ge 3\\
								\end{array} \right.
							</m>
					</statement>
					<solution><title> Solution </title>
			
						<md>
							<mrow>  D(s)	 \amp =  \lap{ d(t) } </mrow>
							<mrow>   \amp =  \int_0^{\infty}e^{-st}d(t) dt </mrow>
							<mrow>   \amp =  \int_0^3 e^{-st}\cdot 7 dt + \int_3^{\infty} e^{-st}\cdot 0 dt </mrow>
							<mrow>   \amp =  7\int_0^3 e^{-st}dt + 0 </mrow>
							<mrow>   \amp =  7 \cdot \left[\frac{1}{-s}e^{-st}\right]_0^3 </mrow>
							<mrow>   \amp =  7 \cdot \left[\left(\frac{1}{-s}e^{-s\cdot 3}\right) - \left(\frac{1}{-s}e^{-s\cdot 0}\right)\right] </mrow>
							<mrow>   \amp =  7 \cdot \left[\left(\frac{1}{-s}e^{-s\cdot 3}\right) - \left(\frac{1}{-s}\cdot 1\right)\right] </mrow>
							<mrow>   \amp =  7 \cdot \left[-\frac{1}{s}e^{-3s} +\frac{1}{s}\cdot 1\right] </mrow>
							<mrow>   \amp =  7 \cdot \left[-\frac{1}{s}e^{-3s} +\frac{1}{s}\right] </mrow>
							<mrow>   \amp =  \frac{7}{s} - \frac{7}{s}e^{-3s} </mrow>
			
						</md>
			
					</solution>
					<answer>
						<m> \ds D(s) = \frac{7}{s} - \frac{7}{s}e^{-3s} </m>
					</answer>
				</exercise>
			
		</exercisegroup>

		
		
		<!--========== Exercise Group 1 ==========--> 
<exercisegroup>
	<title>
	<p>
	 Express each function below in terms of unit step functions andthen compute its Laplace transform.
	</p>
	<p/> <!-- added for vertical space -->
	</title>
		<exercise> <!--== Problem 1 ==-->
			<statement>
				<m> \ds g(t) = \left\{ \begin{array}{ll} 0,	\amp t \le 1\\ 2,	\amp 1 \le t \le 2\\ 1,	\amp 2 \le t \le 3\\ 3,	\amp t \ge 3\\\end{array} \right. </m> 	\showto{student}{\vspace{1cm}}
			</statement>
			<solution><title> Solution </title>
				<p>
					
				</p>
			</solution>
			<answer>
				
			</answer>
		</exercise>
	
		<exercise> <!--== Problem 2 ==-->
			<statement>
				  \includegraphics[scale = 0.35,trim = 0 3in 0 0]{figs/12_LTs_unit_step/fig1.png}\\\vspace{0.8in}
			</statement>
			<solution><title> Solution </title>
				<p>
					
				</p>
			</solution>
			<answer>
				
			</answer>
		</exercise>
	
	</exercisegroup>
	
	<!--========== Exercise Group 2 ==========--> 
	<exercisegroup>
	<title>
	<p>
	 Sketch the graph of the given function and determine its Laplacetransform.
	</p>
	<p/> <!-- added for vertical space -->
	</title>
		<exercise> <!--== Problem 3 ==-->
			<statement>
				<m> \ds w(t) = U(t-1) - U(t-4) </m>
			</statement>
			<solution><title> Solution </title>
				<p>
					<m> \ds w(t) = U(t-1) - U(t-4) </m>
				</p>
			</solution>
			<answer>
				
			</answer>
		</exercise>
	
		<exercise> <!--== Problem 4 ==-->
			<statement>
				<m> \ds y(t) = (t-1)^2U(t-3) </m>
			</statement>
			<solution><title> Solution </title>
				<p>
					<m> \ds y(t) = (t-1)^2U(t-3) </m>
				</p>
			</solution>
			<answer>
				
			</answer>
		</exercise>
	
		<exercise> <!--== Problem 5 ==-->
			<statement>
				<m> \ds x(t) = te^{3t}U(t+\pi/4) </m> 
			</statement>
			<solution><title> Solution </title>
				<p>
					<m> \ds x(t) = te^{3t}U(t+\pi/4) </m> 
				</p>
			</solution>
			<answer>
				
			</answer>
		</exercise>
	
	</exercisegroup>
	
	<!--========== Exercise Group 3 ==========--> 
	<exercisegroup>
	<title>
	<p>
	Find the inverse Laplace transform of each function.
	</p>
	<p/> <!-- added for vertical space -->
	</title>
		<exercise> <!--== Problem 6 ==-->
			<statement>
				<m> \ds Y(s) = \frac{e^{-2s}}{s-1} </m>
			</statement>
			<solution><title> Solution </title>
				<p>
					<m> \ds Y(s) = \frac{e^{-2s}}{s-1} </m>
				</p>
			</solution>
			<answer>
				
			</answer>
		</exercise>
	
		<exercise> <!--== Problem 7 ==-->
			<statement>
				<m> \ds H(s) = \frac{e^{-2s} - 3e^{-4s}}{s+2} </m>
			</statement>
			<solution><title> Solution </title>
				<p>
					<m> \ds H(s) = \frac{e^{-2s} - 3e^{-4s}}{s+2} </m>
				</p>
			</solution>
			<answer>
				
			</answer>
		</exercise>
	
		<exercise> <!--== Problem 8 ==-->
			<statement>
				<m> \ds M(s) = \frac{e^{-3s}}{s^2+9} </m>
			</statement>
			<solution><title> Solution </title>
				<p>
					<m> \ds M(s) = \frac{e^{-3s}}{s^2+9} </m>
				</p>
			</solution>
			<answer>
				
			</answer>
		</exercise>
	
		<exercise> <!--== Problem 9 ==-->
			<statement>
				<m> \ds X(s) = \frac{e^{-s}(s-5)}{(s+1)(s+2)} </m> vspace{1cm}
			</statement>
			<solution><title> Solution </title>
				<p>
					<m> \ds X(s) = \frac{e^{-s}(s-5)}{(s+1)(s+2)} </m> vspace{1cm}
				</p>
			</solution>
			<answer>
				
			</answer>
		</exercise>
	
	</exercisegroup>
	
	<!--========== Exercise Group 4 ==========--> 
	<exercisegroup>
	<title>
	<p>
	Solve each initial value problem.
	</p>
	<p/> <!-- added for vertical space -->
	</title>
		<exercise> <!--== Problem 10 ==-->
			<statement>
				<m> \ds z'' + 3z' + 2z = e^{-3t}U(t-2), \hspace{0.5cm}z(0) = 2,\hspace{0.5cm}z'(0) = -3 </m>
			</statement>
			<solution><title> Solution </title>
				<p>
					
				</p>
			</solution>
			<answer>
				
			</answer>
		</exercise>
	
		<exercise> <!--== Problem 11 ==-->
			<statement>
				<m> \ds w'' + w = U(t-2) - U(t-4), \hspace{0.5cm}w(0) = 1,\hspace{0.5cm}w'(0) = 0 </m>
			</statement>
			<solution><title> Solution </title>
				<p>
					
				</p>
			</solution>
			<answer>
				
			</answer>
		</exercise>
	
	</exercisegroup>

	<exercisegroup><title>Special Cases and Applications</title>
	
		<introduction>
			<p>
				Explore the behavior of Laplace transforms in the following special cases.
			</p>
		</introduction>

		<exercise>
			<statement>
				What is the Laplace transform of a unit step function <m>u(t - 3)</m>?
			</statement>
			<solution><title> Solution </title>
				Use the shifting property of the unit step function:
				<me>\lap{u(t - 3)} = \frac{e^{-3s}}{s}</me>.
			</solution>
			<answer>
				<m>\ds \frac{e^{-3s}}{s}</m>
			</answer>
		</exercise>

		<exercise>
			<statement>
				Find the Laplace transform of the impulse function <m>\delta(t - 2)</m>.
			</statement>
			<solution><title> Solution </title>
				Apply the definition of the Laplace transform for the impulse function:
				<me>\lap{\delta(t - 2)} = e^{-2s}</me>.
			</solution>
			<answer>
				<m>\ds e^{-2s}</m>
			</answer>
		</exercise>

	</exercisegroup>
	
	</exercises>

</section>