<?xml version="1.0" encoding="UTF-8" ?>

<!--********************************************************************-->

<section xml:id="sect-02-02-details" xmlns:xi="http://www.w3.org/2001/XInclude">

  <p xml:id="abuse_of_notation_01">
    In the examples that follow, we will be treating derivative of <m>y</m>
    with respect to <m>x</m> (i.e. <m>dy/dx</m>) as a fraction of the
    differentials, <m>dy</m> and <m>dx</m>. You will see us moving <m>dx</m>
    to the other side of the equation using properties of algebra. We
    mention this because, technically, the derivative cannot be broken up
    this way. Fortunately, "abusing the notation" in this way leads to a
    convenient sequence of steps for solving these differential equations.
  </p>

  <remark xml:id="abuse_of_notation_02">
  <p>
    Suppose we have a DE of the form
    <me>\frac{dy}{dx} = f(x)\cdot g(y).</me>
    We can divide by <m>g(y)</m>, to yield
    <me>\frac{1}{g(y)}\frac{dy}{dx} = f(x).</me>
    Just to make this a little more straightforward, let's agree to define a new function <m>G</m> by
    <me>G(y) = \frac{1}{g(y)}.</me>
    Then we can rewrite the DE as
    <me>G(y) \cdot \frac{dy}{dx} = f(x).</me>
    Here it's important to remember that <m>y</m> is actually a function of <m>x</m>. Let's write it as
    <me>y = h(x).</me>
    <aside>
      * or is it better to use <m>\phi</m> here?? That would be the common way a text would do it.
      (Actually, that's the unknown function we're trying to solve for!)
    </aside>
    Then <m>G(y)</m> is actually equal to <m>G\big(h(x)\big)</m>, and <m>\frac{dy}{dx}</m> is the same thing as <m>h'(x)</m>. So our DE can be written
    <me>G\big(h(x)\big)h'(x) = f(x).</me>
    Now we can integrate both sides with respect to <m>x</m>.
    <men xml:id="pre_usub">
        \int G\big(h(x)\big)h'(x) dx = \int f(x) dx.
    </men>
    If that left hand side isn't obvious to you, you might do a <m>u</m>-substitution to simplify it. In that case, you would let <m>u = h(x)</m>, in which case <m>du = h'(x) dx.</m> Then equation (<xref ref="pre_usub" />) would become
    <me> \int G(u)du = \int f(x) dx.</me>
    If this makes sense, then it shouldn't be <em>too</em> much of a leap to do a <m>y</m>-substitution instead of	a <m>u</m>-substitution. That is, instead of letting <m>u = h(x)</m>, we will let <m>y = h(x)</m>,
    <aside>
      * actually, this is the definition of <m>h</m>
    </aside>
    in which case <m>dy = h'(x) dx.</m>  With this (sensible!) choice of substitution, equation (<xref ref="pre_usub" />) would become
    <me> \int G(y)dy = \int f(x) dx.</me>
    This justifies why we integrate on the left hand side with respect to <m>y</m>, while we integrate with respect to <m>x</m> on the right hand side; it's simply because <m>y</m> is a function of <m>x</m>.
  </p>
  </remark>

  <p xml:id="details_01">
    Let <m>u = 3 - 5y</m>. Then <m>du = -5dy.</m>
  </p>

</section>
