<!-- LICENSING
  This file is part of the textbook "Exploring Differential Equations, An Interactive, Student-Centered Approach" by Geoffrey Cox.
  License: Creative Commons Attribution-ShareAlike 4.0 International (CC BY-SA 4.0)
  You are free to:
    ‚Ä¢ Share ‚Äî copy and redistribute the material in any medium or format.
    ‚Ä¢ Adapt ‚Äî remix, transform, and build upon the material for any purpose, even commercially.
  Under the following terms:
    ‚Ä¢ Attribution ‚Äî You must give appropriate credit, provide a link to the license, and indicate if changes were made.
    ‚Ä¢ ShareAlike ‚Äî If you remix, transform, or build upon the material, you must distribute your contributions under the same license.
  Full license text: https://creativecommons.org/licenses/by-sa/4.0/legalcode
  Recommended attribution: "Exploring Differential Equations" by Geoffrey Cox, licensed CC BY-SA 4.0"
-->
<section xml:id="intro-systems">
	<title>Introducing Systems of Differential Equations</title>

	<introduction>
        <p>
            When we first started studying differential equations, we focused on <em>one equation and one dependent variable</em>. 
            But the real world is rarely that simple. Populations of predators and prey change together, chemical reactions involve several substances interacting, and mechanical systems often involve multiple moving parts. 
        </p>
        <p>
            In this chapter, we'll explore what happens when more than one quantity is changing at once ‚Äî 
            and how we can describe that with <em>systems of differential equations</em>.
        </p>
	</introduction>

    <subsection xml:id="what-are-systems">
        <title>What Are Systems?</title>

        <p>
            A <em>system of differential equations</em> is exactly what it sounds like: 
            a collection of differential equations that must be solved <em>together</em>. 
            Instead of tracking a single unknown function, we track several unknowns ‚Äî 
            and they may influence each other.
        </p>

        <p>
            For example, consider two unknown functions, <m>x(t)</m> and <m>y(t)</m>, governed by:
        </p>

        <md>
            <mrow>\frac{dx}{dt} \amp = f(x, y)</mrow>
            <mrow>\frac{dy}{dt} \amp = g(x, y)</mrow>
        </md>

        <p>
            Here <m>f</m> and <m>g</m> describe how each quantity changes over time ‚Äî possibly depending on the other quantity. 
            This setup is common in science and engineering because many real-world situations involve several connected variables evolving at the same time.
        </p>

        <paragraphs>
            <title>How Are They Different?</title>
            <p>
                Unlike single equations, systems can include <em>interaction</em>. One variable might depend on another ‚Äî or they might depend on each other. This can produce richer behaviors like oscillations, balance points, or feedback loops. Solving systems sometimes calls for new tools, like matrix methods, but the ideas will still build on what you already know.
            </p>

			<p>
				For example, here are some linear systems that have varying levels of dependency between the equations.
			</p>

			<sbsgroup widths="33.3% 33.3% 33.3%">
				<sidebyside>
					<p><me>\ul{\quad\text{Uncoupled}\quad}</me></p>
					<p><me>\ul{\quad\text{Partially-Coupled}\quad}</me></p>
					<p><me>\ul{\quad\text{Fully-Coupled}\quad}</me></p>
				</sidebyside>
				<sidebyside>
					<p>
						<md>
							<mrow>\frac{dx}{dt} \amp = 6x</mrow>
							<mrow>\frac{dy}{dt} \amp = 3y</mrow>
						</md>
					</p>
					<p>
						<md>
							<mrow>\frac{dx}{dt} \amp = 6x</mrow>
							<mrow>\frac{dy}{dt} \amp = 3y - x</mrow>
						</md>
					</p>
					<p>
						<md>
							<mrow>\frac{dx}{dt} \amp = 6x + 2y</mrow>
							<mrow>\frac{dy}{dt} \amp = 3y - x</mrow>
						</md>
					</p>
				</sidebyside>
				<sidebyside>
					<p><me>\text{No variable cross-over}</me></p>
					<p><me>\text{Some variable cross-over}</me></p>
					<p><md><mrow>\text{All variables appear in}</mrow><mrow>\text{all equations}</mrow></md></p>
				</sidebyside>
			</sbsgroup>

			<p>
				The uncoupled system is no more than two independent differential equations that you have solved before. Far more interesting are the coupled systems, where changes in one variable directly influence changes in the other. 
			</p>
        </paragraphs>
	</subsection>

    <subsection xml:id="uncoupled-systems">
        <title>Uncoupled Systems</title>

        <p>
            Let's start simple. Suppose we have two unknowns, <m>x(t)</m> and <m>y(t)</m>, but they don't influence each other:
        </p>

        <md>
            <mrow>\frac{dx}{dt} \amp = -x \quad \text{with} \ x(0) = 0.6</mrow>
            <mrow>\frac{dy}{dt} \amp = -2y \quad \text{with} \ y(0) = 1.2</mrow>
        </md>

        <p>
            These are called <em>uncoupled</em> because the <m>x</m>-equation has no <m>y</m> and the <m>y</m>-equation has no <m>x</m>. 
            There's no interaction ‚Äî they're basically two separate problems packaged together.
        </p>

        <example xml:id="ex-uncoupled">
            <title><e component="emoji">üìñ‚ùì</e>  Example of an Uncoupled System</title>
            <statement>
                <p>
                    Solve the uncoupled system:
                </p>
                <md>
                    <mrow>\frac{dx}{dt} \amp = -x \quad \text{with} \ x(0) = 0.6</mrow>
                    <mrow>\frac{dy}{dt} \amp = -2y \quad \text{with} \ y(0) = 1.2</mrow>
                </md>
            </statement>
            <solution>
                <p>
                    Each equation can be solved on its own:
                </p>

                <me>
                    x(t) = 0.6 e^{-t}, \qquad y(t) = 1.2 e^{-2t}
                </me>

                <p>
                    Even though they evolve separately, we think of the combined solution as a <em>pair</em>:
                </p>

                <me>
                    (x(t), y(t)) = \left(0.6 e^{-t}, 1.2 e^{-2t}\right).
                </me>

                <p>
                    You might imagine <m>x(t)</m> describing a cup of coffee cooling while <m>y(t)</m> describes a soda warming up ‚Äî two unrelated processes happening side by side.
                </p>

				<figure xml:id="fig-uncoupled-phase-plane">
					<caption>Solution trajectories in the phase plane for the uncoupled system <m>x' = -x</m>, <m>y' = -2y</m>. Arrows indicate the direction of motion as time increases.</caption>
					<image width="50%">
						<latex-image>
							\begin{tikzpicture}

								\def\tmin{-0.2}		\def\tmax{2.4}		\def\tstep{0.2}	
								\def\xymin{-0.2}	\def\xymax{2.5}		\def\xystep{0.2}
								
								\def\xo{0.6}	\def\yo{1.3}		% Initial conditions

								\begin{axis}[
									scale=0.6,
									height=6cm, width=12cm,
									xlabel={$t$}, ylabel={$y$},
									grid=none,
									tick style={thick},
									line width=1pt,
									axis lines=middle,
									xtick distance=1, ytick distance=4,
									minor x tick num=1, minor y tick num=1,
									xmin=\tmin, xmax=\tmax, ymin=\xymin, ymax=\xymax,
									legend style={at={(0.4,1)}, anchor=north west, line width=1pt},
									%legend pos=outer north east, % Places the legend outside the axis, top-right,
								]
									\addplot [
										domain=\tmin:\tmax, 
										samples=100, 
										color=red,
										variable=t,
									]{\xo*e^(-t)};
									\addlegendentry{$x(t) = \xo e^{-t}$}

									\addplot [
										domain=\tmin:\tmax, 
										samples=100, 
										color=blue,
										variable=t,
									]{\yo*e^(-2*t)};
									\addlegendentry{$y(t) = \yo e^{-2t}$}

								\end{axis}
							\end{tikzpicture}
						</latex-image>
					</image>
				</figure>
            </solution>
        </example>

		<exercise xml:id="intro-systems-chkpt-1">
			<title><e component="emoji">üìñ‚ùì</e>  Uncoupled or Not?</title>
			<statement correct="no">
				<p>
					The following system is uncoupled:
				</p>
				<md>
					<mrow>\frac{dx}{dt} \amp = 2x</mrow>
					<mrow>\frac{dy}{dt} \amp = -3y + x</mrow>
				</md>
			</statement>
		</exercise>
	</subsection>

	<assemblage label="intro-systems-wrap-up">
		<title>üì§ Wrap-Up</title>
		<p>
			<paragraphs label="intro-systems-takeaways">
				<title>üóùÔ∏è Key Takeaways..</title>
				<ul marker="square">
					<li><em>Uncoupled systems</em> have no interaction between equations: each variable evolves independently.</li>
					<li>You solve each equation on its own, then pair the solutions as <m>(x(t), y(t))</m>.</li>
					<li>These are the simplest systems ‚Äî but they're still systems!</li>
				</ul>
			</paragraphs>
		</p>
	</assemblage>

	<!-- ================================================================ -->
	<!-- WRAP-UP + READING QUESTIONS                                      -->
	<!-- ================================================================ -->
	<subsection label="intro-systems-wrap-up">
		<title>üì§ Wrap-Up</title>

		<assemblage label="intro-systems-wrap-up-takeaways">
			<p>
				üóùÔ∏è <m>\textbf{Key Takeaways...}</m>
				<ul marker="square">
					<li></li>
				</ul>
			</p>
		</assemblage>
		<paragraphs label="intro-systems-cyu">
			<title>Check Your Understanding</title>

			<exercise label="intro-systems-cyu-bundle">
				<title><e component="emoji">ü§îüí≠</e> Separation of Variables Reading Questions</title>

				<task label="intro-systems-cyu-1">
					<title><e component="emoji">ü§îüí≠</e> SOV and Nonlinear Equations</title>
					<statement correct="no">
						<p>
							The separation of variables method cannot be applied to non-linear differential equations.
						</p>
					</statement>
					<feedback>
						<p>
							Being able to solve non-linear differential equations is one of the strengths of the separation of variables method.
						</p>
					</feedback>
				</task>
				<task label="intro-systems-cyu-2">
					<title><e component="emoji">ü§îüí≠</e> Sort the Steps in Order</title>

					<statement>
						<p>
							CONVERT TO PARSONS.. Suppose you want to use separation of variables method to determine the general solution of the differential equation
							<men xml:id="chkpt-intro-systems-examples-1-eqn">
								\ds \frac{dq}{dt} - 3qt^2 = 2q
							</men>.
						</p>
						<p>
							Match the scrambled tasks (on the left) to the task order (on the right) that it should be performed to use this method.
						</p>
					</statement>
					<feedback>
						<p>
							Review the <xref ref="intro-systems" text="custom">SOV Method</xref>.
						</p>
					</feedback>
					<cardsort>
						<match>
							<premise>
								<p>
									Equation is 1st-order ‚úÖ
								</p>
							</premise>
							
							<response>
								<p>
									<m>\text{Task 1}</m>
								</p>
							</response>
						</match>
						<match>
							<premise>
								<p>
									<m>\ds \frac{dq}{dt} = q(2 + 3t^2)</m>
								</p>
							</premise>
							<response>
								<p>
									<m>\text{Task 2}</m>
								</p>
							</response>
						</match>
						<match>
							<premise>
								<p>
									<m>\ds \frac{1}{q}\ dq = (2 + 3t^2)\ dt</m>
								</p>
							</premise>
							<response>
								<p>
									<m>\text{Task 3}</m>
								</p>
							</response>
						</match>
						<match>
							<premise>
								<p>
									<m>\ds \int \frac{1}{q} dq = \int (2 + 3t^2) dt</m>
								</p>
							</premise>
							
							<response>
								<p>
									<m>\text{Task 4}</m>
								</p>
							</response>
						</match>
						<match>
							<premise>
								<p>
									<line><m>\ds \ln|q| = 2t^2 + t^3 + c</m></line>
								</p>
							</premise>
							<response>
								<p>
									<m>\text{Task 5}</m>
								</p>	
							</response>
						</match>
						<match>
							<premise>
								<p>
									<line><m>\ds q = c e\vphantom{|}^{\large 2t^2 + t^3}</m></line>
								</p>
							</premise>
							<response>
								<p>
									<m>\text{Task 6}</m>
								</p>
							</response>
						</match>
					</cardsort>
				</task>
				<task label="intro-systems-cyu-3">
					<title><e component="emoji">ü§îüí≠</e> Combining Constants</title>

					<statement>
						<p>
							Which of the following are valid ways to combine constants when finalizing your solution? Select ALL that apply.
						</p>
					</statement>
					<choices randomize="yes">
						<choice correct="yes">
							<statement>
								<m>
									\quad \left\{
									\begin{align}
										|y|	\amp = e^{2x + c_1}\\ 
										y	\amp = c_2 e^{2x} 
									\end{align}
									\right.\qquad
								</m> 
								where <m>c_2=\pm e^{c_1}</m>.
							</statement>
							<feedback>
								<p>
									Correct, since
									<md>
										<mrow>	|y|	\amp =,	e^{2x + c_1}										</mrow>
										<mrow>	y	\amp =,	\pm e^{2x + c_1}									</mrow>
										<mrow>	y	\amp =,	\pm e^{2x} \cdot e^{c_1}							</mrow>
										<mrow>	y	\amp =,	c_2 e^{2x}	\quad \text{where } c_2 = \pm e^{c_1}	</mrow>
									</md>
								</p>
							</feedback>
						</choice>
						<choice correct="yes">
							<statement>
								<m>
									\quad \left\{
									\begin{align}
										\frac{y^2}{2} \amp = \sin(x) + c_1\\ 
										y^2 \amp = 2\sin(x) + c_2 
									\end{align}
									\right.\qquad
								</m> 
								where <m>c_2 = 2c_1</m>.
							</statement>
							<feedback>
								<p>
									Correct, since
									<md>
										<mrow>	\frac{y^2}{2}	\amp =,	\sin(x) + c_1									</mrow>
										<mrow>	y^2				\amp =,	\sin(x) + 2c_1									</mrow>
										<mrow>	y^2				\amp =,	2\sin(x) + c_2	\quad \text{where } c_2 = 2c_1	</mrow>
									</md>
								</p>
							</feedback>
						</choice>
						<choice>
							<statement>
								<m>
									\quad \left\{
									\begin{align}
										y^2	\amp = 2\sin(x) + c_2\\ 
										y	\amp = \pm\sqrt{2\sin(x)} + c_3 
									\end{align}
									\right.\qquad
								</m> 
								where <m>c_3=\pm \sqrt{c_2}</m>.
							</statement>
							<feedback>
								<p>
									Incorrect, you should not combine constants here since <m>\quad\sqrt{A + B} \neq \sqrt{A} + \sqrt{B}</m>.
								</p>

								<p>
									Your solution should be written as
									<md>
										<mrow>	y^2	\amp =,	2\sin(x) + c_2											</mrow>
										<mrow>	y	\amp =,	\pm\sqrt{2\sin(x) + c_2}\quad \leftarrow\text{ done}	</mrow>
									</md>
								</p>
							</feedback>
						</choice>
						<choice>
							<statement>
								<m>
									\quad \left\{
									\begin{align}
										e^y	\amp =	3y + c_1\\ 
										y	\amp =	\ln(3y) + c_2 
									\end{align}
									\right.\qquad
								</m> 
								where <m>c_2= \ln(c_1)</m>.
							</statement>
							<feedback>
								
								<p>
									Incorrect, you should not combine constants here since <m>\ln(A + B) \neq \ln(A) + \ln(B)</m>.
								</p>

								<p>
									Your solution should be
									<md>
										<mrow>	e^y	\amp =,	3y + c_1									</mrow>
										<mrow>	y	\amp =,	\ln(3y + c_1)\quad \leftarrow\text{ done}	</mrow>
									</md>
								</p>
							</feedback>
						</choice>
						<choice>
							<statement>
								<m>
									\quad \left\{
									\begin{align}
										xy	\amp =	e^x + c_1\\ 
										y	\amp =	\frac{e^x}{x} + c_2 
									\end{align}
									\right.\qquad
								</m> 
								where <m>\ds c_2=\frac{c_1}{x}</m>.
							</statement>
							<feedback>
								<p>
									Incorrect, you should not combine constants here since <m>\frac{c_1}{x}</m> is not constant. Instead your solution should be left as
									<md>
										<mrow>	xy	\amp =,	e^x + c_1													</mrow>
										<mrow>	y	\amp =,	\frac{e^x + c_1}{x}											</mrow>
										<mrow>	y	\amp =,	\frac{e^x}{x} + \frac{c_1}{x}\quad \leftarrow\text{ done}	</mrow>
									</md>
								</p>
							</feedback>
						</choice>
						<choice correct="yes">
							<statement>
								<m>
									\quad \left\{
									\begin{align}
										\sqrt{y}	\amp =	c_1e^{3x}\\ 
										y			\amp =	c_2\, e^{6x} 
									\end{align}
									\right.\qquad
								</m> 
								where <m>c_2= c_1^2</m>.
							</statement>
							<feedback>
								<p>
									Correct, since
									<md>
										<mrow>	\sqrt{y}	\amp =,	c_1e^{3x}									</mrow>
										<mrow>	y			\amp =,	(c_1e^{3x})^2								</mrow>
										<mrow>	y			\amp =,	c_1^2(e^{3x})^2								</mrow>
										<mrow>	y			\amp =,	c_2\, e^{6x}\quad \text{where } c_2 = c_1^2	</mrow>
									</md>
								</p>
							</feedback>
						</choice>
					</choices>
				</task>
			</exercise>
		</paragraphs>
	</subsection>
</section>