<!-- LICENSING
  This file is part of the textbook "Exploring Differential Equations, An Interactive, Student-Centered Approach" by Geoffrey Cox.
  License: Creative Commons Attribution-ShareAlike 4.0 International (CC BY-SA 4.0)
  You are free to:
    ‚Ä¢ Share ‚Äî copy and redistribute the material in any medium or format.
    ‚Ä¢ Adapt ‚Äî remix, transform, and build upon the material for any purpose, even commercially.
  Under the following terms:
    ‚Ä¢ Attribution ‚Äî You must give appropriate credit, provide a link to the license, and indicate if changes were made.
    ‚Ä¢ ShareAlike ‚Äî If you remix, transform, or build upon the material, you must distribute your contributions under the same license.
  Full license text: https://creativecommons.org/licenses/by-sa/4.0/legalcode
  Recommended attribution: "Exploring Differential Equations" by Geoffrey Cox, licensed CC BY-SA 4.0"
-->
<section label="second-order-to-system">
	<title>Second-Order Equations to First-Order Systems</title>		

	<introduction>
		<p>
            So far, we've looked at systems that involve multiple variables like <m>x(t)</m> and <m>y(t)</m>. But what if you start with just a single second-order differential equation? It turns out you can rewrite it as a system of first-order equations.
        </p>
	</introduction>

	<subsection label="second-order-to-system-1">
		<title>Turning a Second-Order Equation into a System</title>

		<p>
			For example, consider the second-order equation:
		</p>

		<me>
			y'' + 3y' + 2y = 0
		</me>

		<p>
			This equation involves only one dependent variable, <m>y(t)</m>, but it's second-order. To convert it into a system, we introduce a new variable:
		</p>

		<me>
			u = y, \quad v = y'
		</me>

		<p>
			That means <m>u' = y' = v</m>. And since <m>y'' = v'</m>, we can rewrite the original equation as:
		</p>

		<me>
			v' = -3v - 2u
		</me>

		<p>
			Now we have a system of two first-order equations:
		</p>

		<md>
			<mrow> u' \amp = v </mrow>
			<mrow> v' \amp = -3v - 2u </mrow>
		</md>

		<exercise label="second-order-to-system-chkpt-1">
			<title><e component="emoji">üìñ‚ùì</e> Derivative Substitution</title>
			<statement correct="yes">
				<p>
					In order to rewrite a second-order equation as a system, we can replace <m>y'</m> with a new variable and then express <m>y''</m> as the derivative of that new variable.
				</p>
			</statement>
			<feedback>
				<p>
					Correct. Introducing <m>x_1 = y</m> and <m>x_2 = y'</m> allows us to write <m>y''</m> as <m>x_2'</m> and form a system.
				</p>
			</feedback>
		</exercise>
	</subsection>

	<!-- ================================================================ -->
	<!-- WRAP-UP + READING QUESTIONS                                      -->
	<!-- ================================================================ -->
	<assemblage label="second-order-to-system-wrap-up">
		<title>üì§ Wrap-Up</title>
		<p>
			<paragraphs label="second-order-to-system-takeaways">
				<title>üóùÔ∏è Key Takeaways..</title>
				<ul marker="square">
					<li>You can convert a second-order linear differential equation into a system of first-order linear system of equations.</li>
				</ul>
			</paragraphs>

			<paragraphs label="second-order-to-system-cyu">
				<title>Check Your Understanding</title>

				<exercise xml:id="second-order-to-system-cyu-bundle">
					<title><e component="emoji">üìñ‚ùì</e> Second-Order Equations to First-Order Systems</title>
					<task label="second-order-to-system-cyu-1">
						<title><e component="emoji">üìñ‚ùì</e> Understanding Converted Systems</title>
						<statement>
							<p>
							When you convert a second-order equation into a first-order system, which of the following are always true?
							</p>
						</statement>
						<choices randomize="yes">
							<choice correct="yes">
							<statement><p>The system has two first-order equations.</p></statement>
							<feedback><p>Yes. One for <m>y</m> and one for <m>y'</m>.</p></feedback>
							</choice>
							<choice correct="yes">
							<statement><p>The system involves two new variables: one for <m>y</m>, one for <m>y'</m>.</p></statement>
							<feedback><p>Exactly. This substitution is the key step.</p></feedback>
							</choice>
							<choice>
							<statement><p>The resulting system is always uncoupled.</p></statement>
							<feedback><p>Not true. The new variables often depend on each other.</p></feedback>
							</choice>
							<choice correct="yes">
							<statement><p>The system represents the same solutions as the original equation.</p></statement>
							<feedback><p>Correct. It's just a different form of the same information.</p></feedback>
							</choice>
							<choice>
							<statement><p>You can only use this method for linear equations.</p></statement>
							<feedback><p>This method also works for nonlinear second-order equations.</p></feedback>
							</choice>
						</choices>
					</task>

					<task label="second-order-to-system-cyu-2">
						<title><e component="emoji">üìñ‚ùì</e> Match Equations to Their Systems</title>
						<statement>
							<p>
							Match each second-order differential equation to the correct system using <m>x_1 = y</m> and <m>x_2 = y'</m>.
							</p>
						</statement>
						<feedback>
							<p>
							Each system reflects <m>x_1' = x_2</m> and an expression for <m>x_2'</m> based on <m>y''</m>.
							</p>
						</feedback>
						<cardsort>
							<match>
							<premise><m>y'' + y = 0</m></premise>
							<response><m>x_1' = x_2,\quad x_2' = -x_1</m></response>
							</match>
							<match>
							<premise><m>y'' - 2y' = 0</m></premise>
							<response><m>x_1' = x_2,\quad x_2' = 2x_2</m></response>
							</match>
							<match>
							<premise><m>y'' = y</m></premise>
							<response><m>x_1' = x_2,\quad x_2' = x_1</m></response>
							</match>
							<match>
							<premise><m>y'' = -y'</m></premise>
							<response><m>x_1' = x_2,\quad x_2' = -x_2</m></response>
							</match>
						</cardsort>
					</task>

					<task label="second-order-to-system-cyu-3">
						<title><e component="emoji">üìñ‚ùì</e> From Second Order to System</title>
						<statement>
							<p>
								What is the correct system corresponding to <m>y'' + 4y = 0</m> if we define <m>x_1 = y</m>, <m>x_2 = y'</m>?
							</p>
						</statement>
						<choices randomize="yes">
							<choice>
								<statement><p><m>x_1' = x_2</m>, <m>x_2' = -4x_2</m></p></statement>
								<feedback><p>That would be true if the original equation were <m>y'' + 4y'</m>. Double-check which variable is being multiplied by 4.</p></feedback>
							</choice>
							<choice>
								<statement><p><m>x_1' = x_2</m>, <m>x_2' = -4x_1 + x_2</m></p></statement>
								<feedback><p>Too many terms, there's no <m>y'</m> in the original equation.</p></feedback>
							</choice>
							<choice correct="yes">
								<statement><p><m>x_1' = x_2</m>, <m>x_2' = -4x_1</m></p></statement>
								<feedback><p>Yes! <m>x_2' = y'' = -4y = -4x_1</m> is exactly what we want.</p></feedback>
							</choice>
							<choice>
								<statement><p><m>x_1' = x_1</m>, <m>x_2' = -4x_2</m></p></statement>
								<feedback><p>This system doesn't reflect the original equation at all.</p></feedback>
							</choice>
						</choices>
					</task>
				</exercise>
			</paragraphs>
		</p>
	</assemblage>
	<!-- ================================================================ -->
	<!-- WRAP-UP + READING QUESTIONS                                      -->
	<!-- ================================================================ -->
	<subsection label="second-order-to-system-wrap-up">
		<title>üì§ Wrap-Up</title>

		<assemblage label="second-order-to-system-wrap-up-takeaways">
			<p>
				üóùÔ∏è <m>\textbf{Key Takeaways...}</m>
				<ul marker="square">
					<li></li>
				</ul>
			</p>
		</assemblage>
		<paragraphs label="second-order-to-system-cyu">
			<title>Check Your Understanding</title>

			<exercise label="second-order-to-system-cyu-bundle">
				<title><e component="emoji">ü§îüí≠</e> Separation of Variables Reading Questions</title>

				<task label="second-order-to-system-cyu-1">
					<title><e component="emoji">ü§îüí≠</e> SOV and Nonlinear Equations</title>
					<statement correct="no">
						<p>
							The separation of variables method cannot be applied to non-linear differential equations.
						</p>
					</statement>
					<feedback>
						<p>
							Being able to solve non-linear differential equations is one of the strengths of the separation of variables method.
						</p>
					</feedback>
				</task>
				<task label="second-order-to-system-cyu-2">
					<title><e component="emoji">ü§îüí≠</e> Sort the Steps in Order</title>

					<statement>
						<p>
							CONVERT TO PARSONS.. Suppose you want to use separation of variables method to determine the general solution of the differential equation
							<men xml:id="chkpt-second-order-to-system-examples-1-eqn">
								\ds \frac{dq}{dt} - 3qt^2 = 2q
							</men>.
						</p>
						<p>
							Match the scrambled tasks (on the left) to the task order (on the right) that it should be performed to use this method.
						</p>
					</statement>
					<feedback>
						<p>
							Review the <xref ref="second-order-to-system" text="custom">SOV Method</xref>.
						</p>
					</feedback>
					<cardsort>
						<match>
							<premise>
								<p>
									Equation is 1st-order ‚úÖ
								</p>
							</premise>
							
							<response>
								<p>
									<m>\text{Task 1}</m>
								</p>
							</response>
						</match>
						<match>
							<premise>
								<p>
									<m>\ds \frac{dq}{dt} = q(2 + 3t^2)</m>
								</p>
							</premise>
							<response>
								<p>
									<m>\text{Task 2}</m>
								</p>
							</response>
						</match>
						<match>
							<premise>
								<p>
									<m>\ds \frac{1}{q}\ dq = (2 + 3t^2)\ dt</m>
								</p>
							</premise>
							<response>
								<p>
									<m>\text{Task 3}</m>
								</p>
							</response>
						</match>
						<match>
							<premise>
								<p>
									<m>\ds \int \frac{1}{q} dq = \int (2 + 3t^2) dt</m>
								</p>
							</premise>
							
							<response>
								<p>
									<m>\text{Task 4}</m>
								</p>
							</response>
						</match>
						<match>
							<premise>
								<p>
									<line><m>\ds \ln|q| = 2t^2 + t^3 + c</m></line>
								</p>
							</premise>
							<response>
								<p>
									<m>\text{Task 5}</m>
								</p>	
							</response>
						</match>
						<match>
							<premise>
								<p>
									<line><m>\ds q = c e\vphantom{|}^{\large 2t^2 + t^3}</m></line>
								</p>
							</premise>
							<response>
								<p>
									<m>\text{Task 6}</m>
								</p>
							</response>
						</match>
					</cardsort>
				</task>
				<task label="second-order-to-system-cyu-3">
					<title><e component="emoji">ü§îüí≠</e> Combining Constants</title>

					<statement>
						<p>
							Which of the following are valid ways to combine constants when finalizing your solution? Select ALL that apply.
						</p>
					</statement>
					<choices randomize="yes">
						<choice correct="yes">
							<statement>
								<m>
									\quad \left\{
									\begin{align}
										|y|	\amp = e^{2x + c_1}\\ 
										y	\amp = c_2 e^{2x} 
									\end{align}
									\right.\qquad
								</m> 
								where <m>c_2=\pm e^{c_1}</m>.
							</statement>
							<feedback>
								<p>
									Correct, since
									<md>
										<mrow>	|y|	\amp =,	e^{2x + c_1}										</mrow>
										<mrow>	y	\amp =,	\pm e^{2x + c_1}									</mrow>
										<mrow>	y	\amp =,	\pm e^{2x} \cdot e^{c_1}							</mrow>
										<mrow>	y	\amp =,	c_2 e^{2x}	\quad \text{where } c_2 = \pm e^{c_1}	</mrow>
									</md>
								</p>
							</feedback>
						</choice>
						<choice correct="yes">
							<statement>
								<m>
									\quad \left\{
									\begin{align}
										\frac{y^2}{2} \amp = \sin(x) + c_1\\ 
										y^2 \amp = 2\sin(x) + c_2 
									\end{align}
									\right.\qquad
								</m> 
								where <m>c_2 = 2c_1</m>.
							</statement>
							<feedback>
								<p>
									Correct, since
									<md>
										<mrow>	\frac{y^2}{2}	\amp =,	\sin(x) + c_1									</mrow>
										<mrow>	y^2				\amp =,	\sin(x) + 2c_1									</mrow>
										<mrow>	y^2				\amp =,	2\sin(x) + c_2	\quad \text{where } c_2 = 2c_1	</mrow>
									</md>
								</p>
							</feedback>
						</choice>
						<choice>
							<statement>
								<m>
									\quad \left\{
									\begin{align}
										y^2	\amp = 2\sin(x) + c_2\\ 
										y	\amp = \pm\sqrt{2\sin(x)} + c_3 
									\end{align}
									\right.\qquad
								</m> 
								where <m>c_3=\pm \sqrt{c_2}</m>.
							</statement>
							<feedback>
								<p>
									Incorrect, you should not combine constants here since <m>\quad\sqrt{A + B} \neq \sqrt{A} + \sqrt{B}</m>.
								</p>

								<p>
									Your solution should be written as
									<md>
										<mrow>	y^2	\amp =,	2\sin(x) + c_2											</mrow>
										<mrow>	y	\amp =,	\pm\sqrt{2\sin(x) + c_2}\quad \leftarrow\text{ done}	</mrow>
									</md>
								</p>
							</feedback>
						</choice>
						<choice>
							<statement>
								<m>
									\quad \left\{
									\begin{align}
										e^y	\amp =	3y + c_1\\ 
										y	\amp =	\ln(3y) + c_2 
									\end{align}
									\right.\qquad
								</m> 
								where <m>c_2= \ln(c_1)</m>.
							</statement>
							<feedback>
								
								<p>
									Incorrect, you should not combine constants here since <m>\ln(A + B) \neq \ln(A) + \ln(B)</m>.
								</p>

								<p>
									Your solution should be
									<md>
										<mrow>	e^y	\amp =,	3y + c_1									</mrow>
										<mrow>	y	\amp =,	\ln(3y + c_1)\quad \leftarrow\text{ done}	</mrow>
									</md>
								</p>
							</feedback>
						</choice>
						<choice>
							<statement>
								<m>
									\quad \left\{
									\begin{align}
										xy	\amp =	e^x + c_1\\ 
										y	\amp =	\frac{e^x}{x} + c_2 
									\end{align}
									\right.\qquad
								</m> 
								where <m>\ds c_2=\frac{c_1}{x}</m>.
							</statement>
							<feedback>
								<p>
									Incorrect, you should not combine constants here since <m>\frac{c_1}{x}</m> is not constant. Instead your solution should be left as
									<md>
										<mrow>	xy	\amp =,	e^x + c_1													</mrow>
										<mrow>	y	\amp =,	\frac{e^x + c_1}{x}											</mrow>
										<mrow>	y	\amp =,	\frac{e^x}{x} + \frac{c_1}{x}\quad \leftarrow\text{ done}	</mrow>
									</md>
								</p>
							</feedback>
						</choice>
						<choice correct="yes">
							<statement>
								<m>
									\quad \left\{
									\begin{align}
										\sqrt{y}	\amp =	c_1e^{3x}\\ 
										y			\amp =	c_2\, e^{6x} 
									\end{align}
									\right.\qquad
								</m> 
								where <m>c_2= c_1^2</m>.
							</statement>
							<feedback>
								<p>
									Correct, since
									<md>
										<mrow>	\sqrt{y}	\amp =,	c_1e^{3x}									</mrow>
										<mrow>	y			\amp =,	(c_1e^{3x})^2								</mrow>
										<mrow>	y			\amp =,	c_1^2(e^{3x})^2								</mrow>
										<mrow>	y			\amp =,	c_2\, e^{6x}\quad \text{where } c_2 = c_1^2	</mrow>
									</md>
								</p>
							</feedback>
						</choice>
					</choices>
				</task>
			</exercise>
		</paragraphs>
	</subsection>
</section>