<?xml version="1.0" encoding="UTF-8" ?>

	<!--********************************************************************-->

	<section xml:id="r-01-01" xmlns:xi="http://www.w3.org/2001/XInclude">
	<title>Differentiation</title>

	<p>
	Throughout the DEs course, we will be differentiating AND integrating. Let's review 
	a few common rules used for differentiation.
		
	<ul marker="">
		<li xml:id="product_rule">	Product Rule:
			<m>
				\ds\qquad \frac{d}{dx}[f(x) \cdot g(x)] = f(x)\cdot \frac{d}{dx}g(x) + g(x)\cdot \frac{d}{dx}f(x) 
			</m>
		</li>
		<li><m/></li>
		<li xml:id="quotient_rule">Quotient Rule:
			<m>
				\ds\qquad \frac{d}{dx}\left[\displaystyle \frac{f(x)}{g(x)}\right] = \ds \frac{g(x) \cdot \displaystyle \frac{d}{dx}f(x) - f(x) \cdot \displaystyle \frac{d}{dx}g(x)}{[g(x)]^2} 
			</m>
		</li>
		<li><m/></li>
		<li xml:id="chain_rule">Chain Rule:
			<m>
				\ds\qquad \frac{d}{dx}f\big(g(x)\big) = f'\big(g(x)\big) \cdot g'(x) 
			</m>
		</li>
	</ul>
		
	</p>

	<p>
	Consider the following example.
	</p>

	<example xml:id="rr_derivative_review">
	<title>Find the derivative of <m>h(x) = (x^5 + 4)\sin(e^x)</m></title>

	<p>
	If you prefer to see a video of this example, 
	<xref ref="video-product_rule" text="custom"> click here </xref>
	</p>

	<p>
	We have a product of functions, so we will need to use the product rule. We also have 
	a composition of functions because <m>e^x</m> is inside of an sine function, so we will need to use the chain rule. Here's how it works.

	<md>	
		<mrow>h'(x)	=\amp\ \ub{\frac{d}{dx} \Big[\ub{(x^5 + 4)}_{f} \cdot 
						\ub{\sin(e^x)}_{g} \Big]}_{
						<xref ref="product_rule" text="custom">product rule</xref>} 		</mrow>
		<mrow>		=\amp\ (x^5+4)\cdot	
			<xref ref="chain_rule" text="custom">
				<m>\ds\ub{\frac{d}{dx}\Big( \sin(e^x) \Big)}_{\text{chain rule}}</m>
			</xref>
					+ \sin(e^x) \cdot \frac{d}{dx}\Big( x^5 + 4 \Big)			</mrow>
		<mrow>	=\amp\ (x^5+4)\cdot\cos(e^x) \cdot \frac{d}{dx}\Big( e^x \Big) 
					+ \sin(e^x) \cdot 5x^4										</mrow>
		<mrow>	=\amp\ (x^5+4)\cdot\cos(e^x) \cdot e^x + 5x^4\sin(e^x)			</mrow>
		<mrow>	=\amp\ (x^5+4)e^x\cos(e^x) + 5x^4\sin(e^x)						</mrow>
	</md>
	</p>
	</example>

	<p>
	Now you try.
	</p>

	<p>
	<term> Find the indicated derivatives.</term>
	<ol>	
		<li><m>\ds \frac{d}{dz}\Big( e^{3z+6} \Big) \qquad</m> 
		<solution>
		<md>
			<mrow>\frac{d}{dz}\Big( e^{3z+6} \Big)	
					=\amp\ e^{3z+6} \cdot \frac{d}{dz}\Big( 3z+6 \Big) \qquad 
							<xref ref="chain_rule" text="custom">chain rule</xref>				</mrow>
			<mrow>	=\amp\ e^{3z+6} \cdot (3) 										</mrow>
			<mrow>	=\amp\ 3e^{3z+6}													</mrow>
		</md>
		</solution>
		<answer>
			<me>3e^{3z+6}</me>
		</answer>
		</li>
		<li><m>\ds \frac{d}{dx}\Big( x^2e^{(\sin x)} \Big) \qquad</m>
		<solution>
		<md>
			<mrow>
				<xref ref="product_rule" text="custom">
					<m>\frac{d}{dx}\Big( x^2e^{(\sin x)} \Big)</m>
				</xref>
						=\amp\ 	x^2 \cdot
				<xref ref="chain_rule" text="custom">
					<m>\frac{d}{dx}\Big(e^{(\sin x)} \Big)</m>
				</xref>
						+ 	e^{(\sin x)}\cdot \frac{d}{dx}\Big(x^2\Big)				</mrow>
			<mrow>	=\amp\ x^2 \cdot e^{(\sin x)}\cdot\frac{d}{dx}\Big(\sin x \Big)
						+ 	e^{(\sin x)}\cdot 2x 									</mrow>
			<mrow>	=\amp\ x^2\cdot e^{(\sin x)}\cdot\cos x + 2xe^{(\sin x)}			</mrow>
			<mrow>	=\amp\ x^2 e^{(\sin x)}\cos x + 2xe^{(\sin x)}					</mrow>
		</md>
		</solution>
		<answer>
			<me>x^2 e^{(\sin x)}\cos x + 2xe^{(\sin x)}</me>
		</answer>
		</li>
		<li><m>\ds \frac{d}{dt}\Big( (t+t^2)^{-1} \Big) \qquad</m>
		<solution>
		<md>
			<mrow>\frac{d}{dt}\Big( (t+t^2)^{-1} \Big)	
					=\amp\ (-1)(t+t^2)^{-2} \cdot \frac{d}{dt}\Big( t+t^2 \Big) \qquad 
							<xref ref="chain_rule" text="custom">chain rule</xref>				</mrow>
			<mrow>	=\amp\ (-1)(t+t^2)^{-2} \cdot (1 + 2t)							</mrow>
			<mrow>	=\amp\ \frac{-(1+2t)}{(t+t^2)^2}									</mrow>
		</md>
		</solution>
		<answer>
			<me>\frac{-(1+2t)}{(t+t^2)^2}</me>
		</answer>
		</li>
		<li><m>\ds \frac{d}{ds}\Big( \ln(4s+7) \Big) \qquad</m>
		<solution>
		<md>
			<mrow>\frac{d}{ds}\Big( \ln(4s+7) \Big)	
					=\amp\ \frac{1}{4s+7} \cdot \frac{d}{ds}\Big( 4s+7 \Big) \qquad 
							<xref ref="chain_rule" text="custom">chain rule</xref>				</mrow>
			<mrow>	=\amp\ \frac{1}{4s+7} \cdot (4)									</mrow>
			<mrow>	=\amp\ \frac{4}{4s+7}											</mrow>
		</md>
		</solution>
		<answer>
			<me>\frac{4}{4s+7}</me>
		</answer>
		</li>
	</ol>
		
	</p>

</section>