<section xml:id="r-01-03" xmlns:xi="http://www.w3.org/2001/XInclude"><title> Integration by parts </title>

	<p>
		Integration by parts may be a good choice when the integrand contains a product. Recall the formula for integration by parts.
		<men xml:id="ibp-formula"> 
			\int u \cdot dv = u\cdot v - \int v \cdot du 
		</men>
	</p>

	<p>
		Let's consider the following example.
	</p>

	<example xml:id="r-01-03-IBP_ex_01"><title>Evaluate <m>\ds \int t^3 \ln t \ dt </m></title>
		
		<p>
			We choose <m>u</m> and <m>dv</m> as follows:
			<me>  u = \ln t \hspace{2cm} dv = t^3 \ dt. </me>  
			Then we find <m>du</m> by taking the derivative of <m>u</m> and <m>v</m> by taking the antiderivative of <m>dv</m>:
			<me> du = \frac{1}{t}dt  \hspace{2cm} v = \frac{1}{4}t^4. </me>
			Thus we have:
			<md>
				<mrow>\int t^3 \ln t dt	=\amp\ \int  \ln t \cdot t^3dt					</mrow>
				<mrow>=\amp\ \int \ub{\ln t}_{u} \cdot \ub{t^3 dt}_{dv}					</mrow>
				<mrow>=\amp\ \int u\cdot dv												</mrow>
				<mrow>=\amp\ u\cdot v - \int v \cdot du									</mrow>
				<mrow>=\amp\ \ln t \cdot \frac{1}{4}t^4 - \int \frac{1}{4}t^4 
								\cdot \frac{1}{t}dt									</mrow>
				<mrow>=\amp\ \frac{1}{4}t^4\ln t - \frac{1}{4}\int t^3 dt				</mrow>
				<mrow>=\amp\ \frac{1}{4}t^4\ln t - \frac{1}{4}\cdot \frac{1}{4}t^4 + C	</mrow>
				<mrow>=\amp\ \frac{1}{4}t^4\ln t - \frac{1}{16}t^4 + C					</mrow>	
			</md>
		</p>
	</example>
				
	<p> Now you try some. </p>

	<p>
		<term> Evaluate each of the following integrals.  Use proper notation.</term>
		<ol>
			<li>
				<m>\ds \int (x - 1)e^x \ dx \qquad</m>
				<solution>	
					We choose <m>u</m> and <m>dv</m> as follows:
					<me>  u = x-1 \hspace{2cm} dv = e^x dx. </me>  
					Then we find <m>du</m> by taking the derivative of <m>u</m> and <m>v</m> by 
					taking the antiderivative of <m>dv</m>:
					<me> du = dx  \hspace{2cm} v = e^x. </me>
					Thus we have:
					<md>
						<mrow>\int (x - 1)e^x dx	=\amp\ \int \ub{(x - 1)}_{u} 
															\ub{e^x dx}_{dv}					</mrow>
						<mrow>						=\amp\ \int u\cdot dv						</mrow>
						<mrow>						=\amp\ u\cdot v - \int v \cdot du			</mrow>
						<mrow>						=\amp\ (x-1)e^x - \int e^x dx				</mrow>
						<mrow>						=\amp\ (x-1)e^x - e^x + C					</mrow>
						<mrow>						=\amp\ xe^x - e^x - e^x + C					</mrow>
						<mrow>						=\amp\ (x-2)e^x + C							</mrow>	
					</md>
				</solution>
				<answer> <me> (x-2)e^x + C </me> </answer>
			</li>
			<li>
				<m>\ds \int x^2 \sin x \ dx \qquad</m>
				<solution>	
					We choose <m>u</m> and <m>dv</m> as follows:
					<me>  u = x^2 \hspace{2cm} dv = \sin x \ dx. </me>  
					Then we find <m>du</m> by taking the derivative of <m>u</m> and <m>v</m> by 
					taking the antiderivative of <m>dv</m>:
					<me> du = 2xdx  \hspace{2cm} v = -\cos x. </me>
					Thus we have:
					<md>
						<mrow>\int x^2 \sin x dx=\amp\ \int \ub{x^2}_{u} 
																\ub{\sin x dx}_{dv}				</mrow>
						<mrow>					=\amp\ \int u\cdot dv							</mrow>
						<mrow>					=\amp\ u\cdot v - \int v \cdot du				</mrow>
						<mrow>					=\amp\ x^2(-\cos x) - \int -\cos x \cdot 2x dx	</mrow>
						<mrow>					=\amp\ -x^2\cos x + \int 2x\cos x dx				</mrow>	
					</md>
					The remaining integral, <m>\int 2x\cos x dx,</m> is simpler than the one we 
					started with, but we will need to do another integration by parts in order to
					evaluate it.  Here we choose
					<me>  u = 2x \hspace{2cm} dv = \cos x dx. </me>  
					Then we find <m>du</m> by taking the derivative of <m>u</m> and <m>v</m> by 
					taking the antiderivative of <m>dv</m>:
					<me> du = 2dx  \hspace{2cm} v = \sin x. </me>
					Now we pick up where we left off:
					<md>
						<mrow>\int x^2 \sin x dx=\amp\ -x^2\cos x + \int 2x\cos x dx</mrow>
						<mrow>					=\amp\ -x^2\cos x + \int \ub{2x}_{u}
																		\ub{\cos x dx}_{dv}		</mrow>
						<mrow>					=\amp\ -x^2\cos x + \int u\cdot dv</mrow>
						<mrow>					=\amp\  -x^2\cos x + u\cdot v - \int v \cdot du	</mrow>
						<mrow>					=\amp\ -x^2\cos x + 2x(\sin x) 
																	- \int \sin x \cdot 2 dx	</mrow>
						<mrow>					=\amp\ -x^2\cos x + 2x\sin x - 2\int \sin x dx	</mrow>
						<mrow>					=\amp\ -x^2\cos x + 2x\sin x - 2(-\cos x) +C		</mrow>
						<mrow>					=\amp\ -x^2\cos x + 2x\sin x + 2\cos x +C		</mrow>
						<mrow>					=\amp\ (2-x^2)\cos x + 2x\sin x +C				</mrow>	
					</md>
				</solution>
				<answer> <me> (2-x^2)\cos x + 2x\sin x +C </me> </answer>
			</li>
		</ol>
	</p>

</section>
