<!-- LICENSING
  This file is part of the textbook "Exploring Differential Equations, An Interactive, Student-Centered Approach" by Geoffrey Cox.
  License: Creative Commons Attribution-ShareAlike 4.0 International (CC BY-SA 4.0)
  You are free to:
    ‚Ä¢ Share ‚Äî copy and redistribute the material in any medium or format.
    ‚Ä¢ Adapt ‚Äî remix, transform, and build upon the material for any purpose, even commercially.
  Under the following terms:
    ‚Ä¢ Attribution ‚Äî You must give appropriate credit, provide a link to the license, and indicate if changes were made.
    ‚Ä¢ ShareAlike ‚Äî If you remix, transform, or build upon the material, you must distribute your contributions under the same license.
  Full license text: https://creativecommons.org/licenses/by-sa/4.0/legalcode
  Recommended attribution: "Exploring Differential Equations" by Geoffrey Cox, licensed CC BY-SA 4.0"
-->
<section label="lt-definition">
	<title>Defining the Laplace Transform</title>

	<introduction>
		<p>
			We've seen how integration by parts transfers derivatives from one function to another inside an integral. Now we take the next step: defining a transform that systematically applies this principle.
		</p>
		<p>
			In this section, we'll see how this transform is constructed and how it converts functions of <m>t</m> into functions of <m>s</m>. You'll also see how to compute Laplace transforms from the definition.
		</p>
	</introduction>

	<subsection xml:id="lt-motivation">
		<title>Why Use the Laplace Transform?</title>
		<p>
			To see where we're headed, imagine you need to solve the differential equation
			<me>
				y'(t) - 9y(t) = 10 e^{2t}.
			</me>
		</p>

		<p>
			Suppose you multiply both sides by <m>e^{-st}</m> and integrate with respect to <m>t</m>:
			<me>
				\int \left[y'(t) - 9y(t)\right] e^{-st} \, dt = \int 10 e^{2t} e^{-st} \, dt.
			</me>
		</p>

		<p>
			The left-hand side contains a derivative inside the integral. From the previous section, you know we can transfer this derivative to the exponential function. Doing so removes the derivative from <m>y(t)</m>, essentially allowing you to use algebra to isolate it.
		</p>

		<p>
			This is the idea behind the Laplace transform and the motivation for its definition.
		</p>	
	</subsection>

	<subsection xml:id="lt-def-basic-definition">
		<title>Definition of the Laplace Transform</title>

		<definition xml:id="laplace-transform-definition"><title>Laplace Transform</title>
			<statement>
				<p>
					Given a function <m>f(t)</m> defined for <m>t \geq 0</m>, its Laplace transform, denoted <m>\lap{f(t)}</m>, is defined by
					<me>
						\lap{f(t)} = \int_0^{\infty} e^{-st} f(t) \, dt,
					</me>
					provided the integral converges. The result is a new function, typically written as a capitalized version of the variable you are transforming. In this case:
					<me>
						F(s) = \lap{f(t)}.
					</me>
				</p>
			</statement>
		</definition>
		
		<exercise label="lt-definition-chkpt-1">
			<title><e component="emoji">üìñ‚ùì</e>  Spot the Error in the Definition</title>
			<statement>
				<p>
					Click on the incorrect part of the Laplace transform definition.
				</p>
			</statement>
			<areas>
				<p/>
				<sidebyside widths="28% 44% 28%">
					<p/>
					<p>
					<area correct="no"><m>\ds \laplacesym</m></area>
					<m>\big\{</m>
					<area correct="no"><m>f(t)</m></area>
					<m>\big\}</m>
					<m>=</m>
					<area correct="no"><m>\ds \int_{0}^{\infty}</m></area>
					<area correct="yes"><m>\ds e^{st}</m></area>
					<area correct="no"><m>\ds f(t)</m></area>
					<area correct="no"><m>\ds dt</m></area>
					</p>
					<p/>
				</sidebyside>
			</areas>
		</exercise>

		<paragraphs xml:id="lt-improper-integrals">
			<title>Working with Improper Integrals</title>
			<p>
				Notice that the Laplace transform involves an improper integral: the upper limit is <m>\infty</m>. In calculus, we handle this by replacing <m>\infty</m> with a variable <m>b</m>, computing the definite integral, and then taking the limit as <m>b \to \infty</m>:
				<me>
					\lap{f(t)} = \int_0^{\infty} e^{-st} f(t)\, dt = \ub{\lim_{b \to \infty} \ob{\int_0^b e^{-st} f(t)\, dt}^{\large\text{(step 1)}}}_{\large\text{(step 2)}}
				</me>.
			</p>

			<p>
				When calculating Laplace transforms, you first compute the integral with respect to <m>t</m>, treating <m>s</m> as a constant. Then you compute the limit of the result as <m>b</m> approaches <m>\infty</m>.
			</p>

			<p>
				The Laplace transform exists if this limit produces a finite value. Often, exponential decay from <m>e^{-st}</m> guarantees convergence when <m>s</m> is large enough.
			</p>

			<exercise label="lt-definition-chkpt-2">
				<title><e component="emoji">üìñ‚ùì</e>  Convergence Requirement for Laplace Transforms</title>
				<statement>
					<p>
						To compute an improper integral, you write it as a limit of a definite integral. For example,
						<me>
							\int_0^{\infty} e^{-st} t^3 \, dt = \lim_{b \to \infty} \ub{\int_0^{b} e^{-st} t^3 \, dt}_{\ds I}
						</me>.
					</p>
					<p>
						Select variables/constants would you expect to see after computing the integral, <m>I</m>, but before taking the limit.
					</p>
					<p/>
				</statement>
				<choices randomize="yes">
					<choice correct="yes">
						<statement><m>\ s</m></statement>
						<feedback>The variable <m>s</m> is a constant in <m>e^{-st} t^3</m> so it will also appear in the antiderivative.</feedback>
					</choice>
					<choice correct="yes">
						<statement><m>\ b</m></statement>
						<feedback>The variable <m>b</m> gets plugged into <m>t</m> after you find the antiderivative.</feedback>
					</choice>
					<choice correct="no">
						<statement><m>\ t</m></statement>
						<feedback>Since the variable of integration is <m>t</m>, you plug the limits of integration, <m>0</m> and <m>b</m>, into <m>t</m> once you have the antiderivative.</feedback>	
					</choice>
					<choice correct="no">
						<statement><m>\ c</m> (integration constant)</statement>
						<feedback>We are computing a definite integral, not an indefinite one.</feedback>
					</choice>
				</choices>
			</exercise>
		</paragraphs>
	</subsection>
						
	<reading-questions>
		<title>üëÄ Quick Review: Exponential Properties</title>
		<p>
			To get through the transform rule derivations, you'll need to be familiar with some key exponential properties that will appear throughtout this chapter.
		</p>

		<paragraphs xml:id="exponential-antiderivative">
			<title>Exponential Antiderivative</title>
			<p>
				For any constant <m>K</m>, we have:
				<me>
					\int e^{Kt}\ dt = \frac1{K} e^{Kt} + C
				</me>.
				While this can be found by substituting <m>u=Kt</m>, it is such a common antiderivative that you should just know it without this extra step. 
			</p>	
		</paragraphs>
						
		<paragraphs xml:id="exponential-end-behavior">
			<title>Exponential End Behavior</title>
			<p>
				The end behavior can be seen from the most basic exponential function:
			</p>

			<sidebyside widths="35% 5% 30%" margins="15% 15%" valign="middle">
				<p>
					<image width="50%">
						<latex-image>
							\begin{tikzpicture}[samples=50]
								% === colors ===
								\def\fColor{blue}

								% === figure/domain/tick bounds ===
								\def\tmin{-2.2}	\def\tmax{2.45}
								\def\ymin{-1.8}		\def\ymax{7.5}
								\def\tticks{1, 2}
								\def\yticks{2, 4}

								% === Function definitions ===
								\newcommand{\f}[1]{e^(#1)}	\def\ftex{e^t}

								\begin{axis}[
									width=15cm, height=7cm, scale=0.4,
									xlabel={$t$}, ylabel={$y$},
									grid=none,
									tick style={thick},
									line width=1pt,
									axis lines=middle,
									xtick distance=1, ytick distance=4,
									minor x tick num=1, minor y tick num=1,
									xmin=\tmin, xmax=\tmax, ymin=\ymin, ymax=\ymax,
								]
								
									% Read and plot data from file
									\addplot [domain=\tmin:\tmax, \fColor] {e^x};

									% === Labels ===
									\node[\fColor, font=\large, above] at (1.5, 5) {$\ftex$};
								\end{axis}
							\end{tikzpicture}
						</latex-image>
					</image>
				</p>
				<p/>
				<p>
					<md alignment="alignat">
						<mrow> t \to -\infty	\amp\ \ \Rightarrow\ \ \amp e^{t} \to 0</mrow>
						<mrow> t \to \infty		\amp\ \ \Rightarrow\ \ \amp e^{t} \to \infty</mrow>
					</md>
				</p>
			</sidebyside>

			<p>
				In general, the end behavior depends on whether the power goes to <m>+\infty</m> or <m>-\infty</m>:
				<ul>
					<li><m>\quad \text{power} \to +\infty\quad\Rightarrow\quad e^{\text{power}} \to +\infty</m></li>
					<li><m>\quad \text{power} \to -\infty\quad\Rightarrow\quad e^{\text{power}} \to 0</m></li>
				</ul>
			</p>

			<p>
				In this section, we will take limits as <m>b \to \infty</m>. Your goal will be to figure out if <m>b \to \infty</m> causes the power to go to <m>+\infty</m> or <m>-\infty</m>. Only then will you know where <m>\ds e^{\text{power}}</m> goes.
			</p>
		</paragraphs>

		<exercise><title><e component="emoji">üìñ‚ùì</e>  Checkpoint: Exponential Properties</title>
			<task label="lt-def-prep-1">
				<title>Exponential Antiderivative</title>
				<statement>
					<p>
						Evaluate: <m>\ds\int_0^b e^{-3t}\ dt</m>
					</p>
				</statement>
				<choices randomize="yes">
					<choice correct="yes"><statement><m>\quad\ds \frac{1 - e^{-3b}}{3}</m></statement></choice>
					<choice><statement><m>\quad\ds \frac{1}{3}e^{-3b}</m></statement></choice>
					<choice><statement><m>\quad\ds -\frac{1}{3}e^{-3b}</m></statement></choice>
					<choice><statement><m>\quad\ds -\frac{1}{3}e^{3b}</m></statement></choice>
				</choices>
			</task>
	
			<task label="lt-def-prep-2">
				<title>Exponential End Behavior</title>
				<statement>
					<p>
						Determine if each limit is -·Äë, <m>0</m>, or ·Äë.
					</p>
					<p>
						Click on one of the three options next to each limit to select your answer.
					</p>
					<p>
						Assume <m>s</m> is a positive constant.
					</p>
				</statement>

				<areas>
					<p/>
					<sbsgroup widths="15% 13% 50%" margins="11% 11%" valign="middle">
						<sidebyside>
							<p><me>\lim_{b \to \infty} e^{\ds b}</me></p>
							<p><me> = <fillin characters="2" /></me></p>
							<p>
								<tabular>
									<col halign="right"/>
									<col halign="center" />
									<col halign="center" />
									<row>
										<cell><area correct="no"><m>\large\ -\infty\ </m></area></cell>
										<cell><area correct="no"><m>\large\ 0\ </m></area></cell>
										<cell><area correct="yes"><m>\large\ +\infty\ </m></area></cell>
									</row>
								</tabular>
							</p>
						</sidebyside>
						<sidebyside>
							<p><me>\lim_{b \to \infty} e^{\ds -3b}</me></p>
							<p><me> = <fillin characters="2" /></me></p>
							<p>
								<tabular>
									<col halign="right"/>
									<col halign="center" />
									<col halign="center" />
									<row>
										<cell><area correct="no"><m>\large\ -\infty\ </m></area></cell>
										<cell><area correct="yes"><m>\large\ 0\ </m></area></cell>
										<cell><area correct="no"><m>\large\ +\infty\ </m></area></cell>
									</row>
								</tabular>
							</p>
						</sidebyside>
						<sidebyside>
							<p><me>\lim_{b \to \infty} e^{\ds sb}</me></p>
							<p><me> = <fillin characters="2" /></me></p>
							<p>
								<tabular>
									<col halign="right"/>
									<col halign="center" />
									<col halign="center" />
									<row>
										<cell><area correct="no"><m>\large\ -\infty\ </m></area></cell>
										<cell><area correct="no"><m>\large\ 0\ </m></area></cell>
										<cell><area correct="yes"><m>\large\ +\infty\ </m></area></cell>
									</row>
								</tabular>
							</p>
						</sidebyside>
						<sidebyside>
							<p><me>\lim_{b \to \infty}e^{\ds -sb}</me></p>
							<p><me> = <fillin characters="2" /></me></p>
							<p>
								<tabular>
									<col halign="right"/>
									<col halign="center" />
									<col halign="center" />
									<row>
										<cell><area correct="no"><m>\large\ -\infty\ </m></area></cell>
										<cell><area correct="yes"><m>\large\ 0\ </m></area></cell>
										<cell><area correct="no"><m>\large\ +\infty\ </m></area></cell>
									</row>
								</tabular>
							</p>
						</sidebyside>
					</sbsgroup>
				</areas>
			</task>

			<task label="lt-definition-chkpt-3-0">
				<title>Figure out the Limits</title>
				<statement>
					<p>
						Give each limit by filling in one of the following: <c>0</c>, 
						<c>inf</c> (<m>\infty</m>), 
						<c>-inf</c> (<m>-\infty</m>).
					</p>
					<p>
						<ul marker="square">
							<li>
								If <m>b \to \infty</m> then 
								<m>-4b\to</m> <fillin width="2" mode="string" answer="-inf" />
								and
								<m>\ds\lim_{b \to \infty} e^{-4b} = </m> <fillin width="2" mode="string" answer="0" />
							</li>
						</ul>
						Assume that <m>s</m> is a <em>positive</em> constant.
						<ul marker="square">
							<li>
								If <m>b \to \infty</m> then
								<m>-sb\to</m> <fillin width="2" mode="string" answer="-inf" /> and
								<m>\ds\lim_{b \to \infty} e^{-sb} = </m> <fillin width="2" mode="string" answer="0" />
							</li>
						</ul>
						Assume that <m>s</m> is a <em>negative</em> constant.
						<ul marker="square">
							<li>
								If <m>b \to \infty</m> then
								<m>-sb\to</m> <fillin width="2" mode="string" answer="inf" />
								and
								<m>\ds\lim_{b \to \infty} e^{-sb} = </m> <fillin width="2" mode="string" answer="inf" />
							</li>
						</ul>
					</p>
				</statement>
				
				<evaluation>
					<evaluate>
						<test correct="yes"><strcmp use-answer="no">-\s*inf</strcmp></test>
						<test><strcmp>.*</strcmp>
							<feedback>Incorrect. Where would <m>-4</m> times something that goes to <m>\infty</m> must go?</feedback>
						</test>
					</evaluate>
					<evaluate>
						<test><strcmp use-answer="yes" /></test>
						<test><strcmp>.*</strcmp>
							<feedback>Incorrect. Think about where <m>-4b</m> goes as <m>b</m> goes to <m>\infty</m>, then decide where <m>e^{-4b}</m> should go.</feedback>
						</test>
					</evaluate>
					<evaluate>
						<test correct="yes"><strcmp use-answer="no" >-\s*inf</strcmp></test>
						<test><strcmp>.*</strcmp>
							<feedback>Incorrect. If <m>s</m> is positive, then <m>-sb</m> is a negative number times something that goes to <m>\infty</m>.</feedback>
						</test>
					</evaluate>
					<evaluate>
						<test><strcmp use-answer="yes" /></test>
						<test><strcmp>.*</strcmp>
							<feedback>Incorrect. Think about where <m>-sb</m> goes as <m>b</m> goes to <m>\infty</m>, then decide where <m>e^{-sb}</m> should go.</feedback>
						</test>
					</evaluate>
					<evaluate>
						<test correct="yes"><strcmp use-answer="no">inf</strcmp></test>
						<test><strcmp>.*</strcmp>
							<feedback>Incorrect. If <m>s</m> is negative, then <m>-sb</m> is a positive number times something that goes to <m>\infty</m>.</feedback>
						</test>
					</evaluate>
					<evaluate>
						<test correct="yes"><strcmp use-answer="no">inf</strcmp></test>
						<test><strcmp>.*</strcmp>
							<feedback>Incorrect. Think about where <m>-sb</m> goes as <m>b</m> goes to <m>\infty</m>, then decide where <m>e^{-sb}</m> should go.</feedback>
						</test>
					</evaluate>
				</evaluation>
			</task>
		</exercise>
	</reading-questions>

	<subsection xml:id="lt-def-first-examples">
		<title>First Examples of Laplace Transforms</title>
		<p>
			Let's see how the definition works by computing Laplace transforms for simple functions. We'll start with a constant function and a linear function.
		</p>

		<example xml:id="laplace-first-examples">
			<title>First Look at Laplace Transforms</title>
			<p>
				Find the Laplace transform of 
				<ol marker="(a)">
					<li>
						<statement>
							<p><m>f(t) = 5</m> (constant function)</p>
						</statement>
						<solution xml:id="laplace-transform-of-5">
							<title><m>\rightarrow \lap{5}</m></title>
							<p>
								By the definition above, we have the improper integral
								<men xml:id="lt-def-example-eqn-1">
									\lap{5} = \int_0^{\infty} e^{-st} \cdot 5\ dt = \lim_{b \to \infty} \ub{\int_0^b 5e^{-st}dt}_{I}
								</men>.
							</p>

							<p>
								Assuming <m>s</m> and <m>b</m> are constant, we integrate <m>I</m> with respect to <m>t</m>:
								<me>
									I = \int_0^b 5e^{-st}dt = -\frac{5}{s}e^{-st}\Big|_{t=0}^{t=b} = -\frac{5}{s}\left[ e^{-sb} - 1 \right]
								</me>.
							</p>

							<proof xml:id="lt-example-1-details"><title>üîç Next, we compute the limit of <m>I</m> as <m>b \to \infty</m> (with <m>s</m> constant):</title>
								<p>
									üîç Since the limit only controls <m>b</m>, we can think of <m>s</m> as a number (like <m>2</m>). This means that <m>\ds-\frac{5}{s}</m> is also a number that can be pulled out of the limit using the limit property from calculus:
									<me>\ds\lim_{x \to \infty} c \cdot f(x) = c \cdot \lim_{x \to \infty} f(x), \quad c\ \text{is constant}</me>
								</p>
							</proof>

							<md>
								<mrow>
									\lim_{b \to \infty} I = \lim_{b \to \infty} -\frac{5}{s}\left[ e^{-sb} - 1 \right] 
										\amp = -\frac{5}{s} \lim_{b \to \infty} \Big[ e^{-sb} - 1 \Big]
								</mrow>
								<mrow>
										\amp = -\frac{5}{s} \Big[ \ub{\lim_{b \to \infty} e^{-sb}}_{L} - 1 \Big]
								</mrow>
							</md>

							<p> 
								We find the limit using the <xref ref="exponential-end-behavior" text="custom">end behavior of the exponential</xref>. There are two possiblities:<fn> <m>s = 0</m> is excluded since it would lead to <me>\int_0^{\infty}5e^{-0t}\ dt = \int_0^{\infty}5\ dt = \infty</me></fn>
								<ol marker="(1)">
									<li> <m>s</m> is positive: <m>\ds\quad-sb \to -\infty \ \ \Rightarrow\ \ \lim_{b \to \infty}\ e^{-sb} = 0</m> </li>
									<li> <m>s</m> is negative: <m>\ds\quad-sb \to +\infty \ \ \Rightarrow\ \ \lim_{b \to \infty}\ e^{-sb} = \infty</m> </li>
								</ol>
							</p>

							<p>
								Since we only get convergence when <m>s</m> is positive, we must require <m>s \gt 0</m> in the Laplace transform of <m>5</m>:
								<me>
									\lap{5} = -\frac{1}{s} [0 - 1] = \frac{1}{s} \quad \text{for } s \gt 0
								</me>.
							</p>
						</solution>
					</li>
					<li>
						<statement>
							<p><m>f(t)=t</m></p>
						</statement>
						<solution xml:id="laplace-transform-of-t-power-1"><title><m>\rightarrow \lap{t}</m></title>

							<p>
								Applying the definition and writing the integral as a limit, we have
								<me>
									\lap{ t }	= \lim_{b \to \infty} {\ub{\int_0^b e^{-st} \cdot t\ dt}_{I}}
								</me>.
							</p>

							<p>
								<proof xml:id="lt-example-t-IVP-details"><title>üîç Computing <m>I</m> with integration by parts, gives us</title>
									<p>
										üîç Choosing
										<md>
											<mrow> u = t,	\quad\amp	dv = e^{-st}dt, 		</mrow>
											<mrow> du = dt,	\quad\amp	v = -\frac{1}{s}e^{-st}	</mrow>
										</md>
										integration by parts gives
										<md>
											<mrow>
												\int_0^b e^{-st} \cdot t\ dt
													\amp = -\frac{t}{s}e^{-st} - \int_0^b \left( -\frac{1}{s}e^{-st} \right) dt
											</mrow>
											<mrow> 	
													\amp = -\frac{t}{s}e^{-st}+ \frac{1}{s}\int_0^b e^{-st} dt
											</mrow>
											<mrow> 	
													\amp = \left(-\frac{t}{s}e^{-st}- \frac{1}{s^2}e^{-st}\right) \Bigg|_0^b
											</mrow>
											<mrow> 	
													\amp = \left(-\frac{b}{s}e^{-sb} - \frac{1}{s^2}e^{-sb}\right) - \left(0 - \frac{1}{s^2}\right)
											</mrow>
											<mrow> 	
													\amp = -\frac{b}{s}e^{-sb} - \frac{1}{s^2}e^{-sb} + \frac{1}{s^2}
											</mrow>
										</md>
									</p>
								</proof>
								<md>
									<mrow>
										{I}	\amp\ { = -\frac{b}{s}e^{-sb} - \frac{1}{s^2}e^{-sb} + \frac{1}{s^2}}
									</mrow>
								</md>
							</p>

							<p>
								Next, we compute the limit of <m>I</m> as <m>b \to \infty</m>:
								<md>
									<mrow>
										\lim_{b \to \infty} {I} \amp = \lim_{b \to \infty} \left({ -\frac{b}{s}e^{-sb} - \frac{1}{s^2}e^{-sb} + \frac{1}{s^2}}\right)
									</mrow>
									<mrow>
										\amp = -\frac{1}{s}\lim_{b \to \infty} be^{-sb} - \frac{1}{s^2}\lim_{b \to \infty} e^{-sb} + \lim_{b \to \infty} \frac{1}{s^2}
									</mrow>
									<mrow>
										\amp = -\frac{1}{s}\ub{\lim_{b \to \infty} \frac{b}{e^{sb}}}_{L_1} - \frac{1}{s^2}\ub{\lim_{b \to \infty} e^{-sb}}_{L_2} + \frac{1}{s^2}
									</mrow>
								</md> 
							</p>

							<proof xml:id="lt-example-t-LH-details"><title>üîç As long as <m>s \gt 0</m>, both <m>L_1</m> and <m>L_2</m> go to zero</title>
								<p>
									üîç Assuming <m>s \gt 0</m>, the limits are computed by:
									<ul marker="square">
										<li>
											<p>
												<m>
													\ds L_1 
													= \lim_{b \to \infty}\frac{\os{\infty}{\os{\uparrow}{\boxed{b}}}}{\us{\infty}{\us{\downarrow}{\boxed{e^{sb}}}}}
													\,\us{LH}{=}\, \lim_{b \to \infty}\frac{1}{se^{sb}}
													= \frac{1}{s}\lim_{b \to \infty}\frac{1}{\us{\infty}{\us{\downarrow}{\boxed{e^{sb}}}}} = 0
												</m>
											</p>
										</li>
										<li>
											<p>
												<m>
													\ds L_2
													= \lim_{b \to \infty}\frac{1}{\us{\infty}{\us{\downarrow}{\boxed{e^{sb}}}}} = 0
												</m>
											</p>
										</li>
									</ul>
									where <m>LH</m> denotes L'H√¥pital's Rule was applied to the limit.
								</p>
							</proof>

							<p>
								Therefore, the Laplace transform of <m>t</m> is
								<me>
									\lap{ t } = \frac{1}{s^2}, \quad s &gt; 0
								</me>.
							</p>
						</solution>
					</li>
				</ol>
			</p>
		</example>

		<p>
			These examples show the typical process: set up the improper integral, compute it as a definite integral, then take the limit as <m>b \to \infty</m>. You'll see how <m>s</m> emerges naturally from this process.
		</p>
		<p>
			In upcoming sections, we'll build a library of Laplace transforms for the most common functions and learn properties that make these computations even faster.
		</p>
	</subsection>

	<!-- ================================================================ -->
	<!-- WRAP-UP + READING QUESTIONS                                      -->
	<!-- ================================================================ -->
	<subsection label="lt-definition-wrap-up">
		<title>üì§ Wrap-Up</title>

		<assemblage label="lt-definition-wrap-up-takeaways">
			<p>
				üóùÔ∏è <m>\textbf{Key Takeaways...}</m>
				<ul marker="square">
					<li>The Laplace transform converts a function of <m>t</m> into a function of <m>s</m> using <me>\lap{f(t)} = \int_0^\infty e^{-st} f(t)\, dt.</me></li>
					<li>The Laplace transform is an improper integral evaluated by rewriting it as <me>\int_0^{\infty} e^{-st} f(t)\, dt = \lim_{b \to \infty} \int_0^b e^{-st} f(t)\, dt</me>.</li>
					<li>The result is a function of <m>s</m> and exists only when the integral converges.</li>
				</ul>
			</p>
		</assemblage>
	</subsection>
</section>