<!-- LICENSING
  This file is part of the textbook "Exploring Differential Equations, An Interactive, Student-Centered Approach" by Geoffrey Cox.
  License: Creative Commons Attribution-ShareAlike 4.0 International (CC BY-SA 4.0)
  You are free to:
    ‚Ä¢ Share ‚Äî copy and redistribute the material in any medium or format.
    ‚Ä¢ Adapt ‚Äî remix, transform, and build upon the material for any purpose, even commercially.
  Under the following terms:
    ‚Ä¢ Attribution ‚Äî You must give appropriate credit, provide a link to the license, and indicate if changes were made.
    ‚Ä¢ ShareAlike ‚Äî If you remix, transform, or build upon the material, you must distribute your contributions under the same license.
  Full license text: https://creativecommons.org/licenses/by-sa/4.0/legalcode
  Recommended attribution: "Exploring Differential Equations" by Geoffrey Cox, licensed CC BY-SA 4.0"
-->
<section xml:id="lt-reference-guide">
	<title>The Laplace Transform Reference Guide</title>

	<introduction>
		<p>
			In this final section, we summarize everything we've done. Below, you will find tables for the most common Laplace transforms and the properties used to combine and manipulate them. These will provide a useful resource in the next chapter where we begin solving differential equations using the Laplace transform method.
		</p>
	</introduction>

	<subsection label="lt-reference-tables">
		<title>Laplace Transform Tables</title>

		<p>
			We have done a lot of work computing common transforms and deriving the properties of the Laplace transform. Now, we can summarize all of this information in tables for quick reference.
		</p>

		<p>
			We begin with the specific transforms of exponentials, polynomial terms, sine/cosine, and the products of these functions. In later chapters, we will encounter new types of functions that we need to transform, so this table will continue to grow as we go.   
		</p>

		<sidebyside label="lt-common-table" width="80%">
			<p>
				<table xml:id="lt-table-common">
					<title>Table of Common Laplace Transforms</title>
					<tabular top="major" bottom="minor" left="major" right="minor" halign="center" width="100%">
						<col/>
						<col/>
						<col/>
						<col right="major"/>
						<row bottom="major">
							<cell/>
							<cell>
								<line>Function</line>
								<line>(<m>t</m>-Domain)</line>
								<line><me>f(t)</me></line>
							</cell>
							<cell>
								<line>Laplace Transform</line>
								<line>(<m>s</m>-Domain)</line>
								<line><me>\lap{f(t)} = F(s)</me></line>
							</cell>
							<cell>
								<line/>
								<line>Existence</line>
								<line>Condition</line>
							</cell>
						</row>
						<row>
							<cell>L<m>_1</m></cell>
							<cell><me>1</me></cell>
							<cell><me>\frac{1}{s}</me></cell>
							<cell><me>s &gt; 0</me></cell>
						</row>
						<row>
							<cell>L<m>_2</m></cell>
							<cell><me>e^{at}</me></cell>
							<cell><me>\frac{1}{s - a}</me></cell>
							<cell><me>s &gt; a</me></cell>
						</row>
						<row>
							<cell>L<m>_3</m></cell>
							<cell><me>t^n</me></cell>
							<cell><me>\frac{n!}{s^{n+1}}</me></cell>
							<cell><me>s &gt; 0</me></cell>
						</row>
						<row>
							<cell>L<m>_4</m></cell>
							<cell><me>\sin(bt)</me></cell>
							<cell><me>\frac{b}{s^2+b^2}</me></cell>
							<cell><me>s &gt; 0</me></cell>
						</row>
						<row>
							<cell>L<m>_5</m></cell>
							<cell><me>\cos(bt)</me></cell>
							<cell><me>\frac{s}{s^2+b^2}</me></cell>
							<cell><me>s &gt; 0</me></cell>
						</row>
						<row>
							<cell>L<m>_6</m></cell>
							<cell><me>e^{at}\ t^n</me></cell>
							<cell><me>\frac{n!}{(s-a)^{n+1}}</me></cell>
							<cell><me>s &gt; a</me></cell>
						</row>
						<row>
							<cell>L<m>_7</m></cell>
							<cell><me>e^{at}\sin(bt)</me></cell>
							<cell><me>\frac{b}{(s-a)^2+b^2}</me></cell>
							<cell><me>s &gt; a</me></cell>
						</row>
						<row bottom="major">
							<cell>L<m>_8</m></cell>
							<cell><me>e^{at}\cos(bt)</me></cell>
							<cell><me>\frac{s-a}{(s-a)^2+b^2}</me></cell>
							<cell><me>s &gt; a</me></cell>
						</row>
					</tabular>
				</table>
			</p>
		</sidebyside>

		<task label="lt-reference-guide-chkpt-1">
			<title><e component="emoji">üìñ‚ùì</e>  What's Missing in each Transform?</title>
			<statement>
				<p>
					Select the missing piece from each Laplace transform.
				</p>
			</statement>
			<areas>
				<p/>
				<sbsgroup widths="44% 14% 14% 14% 14%" valign="middle" margins="0% 0%">
					<sidebyside widths="44% 56%">
						<p><me>\ul{\quad\qquad\text{Transforms}\qquad\quad}</me></p>
						<p><me>\ul{\quad\qquad\qquad\text{Possible Answers}\qquad\qquad\quad}</me></p>
					</sidebyside>
					<sidebyside>
						<p><me>\ds\lap{t^4} = \frac{<fillin characters="1" />}{s^5}</me></p>
						<p><area correct="no" ><m>3!</m></area></p>
						<p><area correct="no" ><m>4!</m></area></p>
						<p><area correct="yes"><m>5!</m></area></p>
						<p><area correct="no" ><m>6!</m></area></p>
					</sidebyside>
					<sidebyside>
						<p><me>\ds\lap{t^3} = \frac{6}{<fillin characters="1" />}</me></p>
						<p><area correct="no" ><m>s^2</m></area></p>
						<p><area correct="no" ><m>t^2</m></area></p>
						<p><area correct="yes"><m>s^4</m></area></p>
						<p><area correct="no" ><m>t^4</m></area></p>
					</sidebyside>
					<sidebyside>
						<p><me>\ds\lap{<fillin characters="1" />} = \frac{479001600}{s^{13}}</me></p>
						<p><area correct="no" ><m>s^{12}</m></area></p>
						<p><area correct="yes"><m>t^{12}</m></area></p>
						<p><area correct="no" ><m>s^{14}</m></area></p>
						<p><area correct="no" ><m>t^{14}</m></area></p>
					</sidebyside>
					<sidebyside>
						<p><me>\ds\lap{\sin(-3t)} = \frac{<fillin characters="1" />}{s^2 + 9}</me></p>
						<p><area correct="yes"><m>1</m></area></p>
						<p><area correct="no" ><m>s</m></area></p>
						<p><area correct="no" ><m>b</m></area></p>
						<p><area correct="no" ><m>s^2</m></area></p>
					</sidebyside>
					<sidebyside>
						<p><me>\ds\lap{<fillin characters="1" />} = \frac{s}{s^2 + 4}</me></p>
						<p><area correct="no" ><m>\cos(4t)</m></area></p>
						<p><area correct="no" ><m>\sin(2t)</m></area></p>
						<p><area correct="no" ><m>\cos(t)</m></area></p>
						<p><area correct="yes"><m>\cos(2t)</m></area></p>
					</sidebyside>
				</sbsgroup>
			</areas>
		</task>

		<p>
			The next set of transforms are more general rules you can apply in different situations.
		</p>

		<sidebyside label="lt-rules-table"  width="80%">
			<p>
				<table xml:id="lt-table-rules">
					<title>Table of Laplace Transform Rules</title>
					<tabular top="major" bottom="minor" left="major" right="minor" halign="center" width="100%">
						<col/>
						<col/>
						<col/>
						<col right="major"/>
						<row bottom="none">
							<cell/>
							<cell>Function (<m>t</m>-Domain)</cell>
							<cell>Laplace Transform (<m>s</m>-Domain)</cell>
							<cell>Existence</cell>
						</row>
						<row bottom="major">
							<cell/>
							<cell><me>f(t)</me></cell>
							<cell><me>\lap{f(t)} = F(s)</me></cell>
							<cell>Condition</cell>
						</row>
						<row>
							<cell>R<m>_{1}</m></cell>
							<cell><me>f'(t)</me></cell>
							<cell><me>sF(s) - f(0)</me></cell>
							<cell><me>s &gt; 0</me></cell>
						</row>
						<row>
							<cell>R<m>_{2}</m></cell>
							<cell><me>f''(t)</me></cell>
							<cell><me>s^2F(s) - sf(0) - f'(0)</me></cell>
							<cell><me>s &gt; 0</me></cell>
						</row>
						<row>
							<cell>R<m>_{3}</m></cell>
							<cell><me>f'''(t)</me></cell>
							<cell><me>s^3F(s) - s^2f(0) - sf'(0) - f''(0)</me></cell>
							<cell><me>s &gt; 0</me></cell>
						</row>
						<row>
							<cell>R<m>_{4}</m></cell>
							<cell><me>e^{at} f(t)</me></cell>
							<cell><me>F(s-a)</me></cell>
							<cell><me>s &gt; 0</me></cell>
						</row>
						<row bottom="major">
							<cell>R<m>_{5}</m></cell>
							<cell><me>t^n f(t)</me></cell>
							<cell><me>(-1)^n \frac{d^n}{ds^n}\Big[F(s)\Big]</me></cell>
							<cell><me>s &gt; 0</me></cell>
						</row>
					</tabular>
				</table>
			</p>
		</sidebyside>

		<p>
			Finally, we list the Laplace transform properties. It is short for now, but we will add more to this table later.
		</p>

		<sidebyside label="lt-properties-table"  width="80%">
			<p>
				<table xml:id="lt-table-properties">
					<title>Table of Laplace Transform Properties</title>
					<tabular top="major" bottom="minor" left="major" right="minor" halign="center" width="100%">
						<col/>
						<col/>
						<col/>
						<col right="major"/>
						<row bottom="major">
							<cell/>
							<cell>Property Type</cell>
							<cell>Property</cell>
						</row>
						<row bottom="major">
							<cell>P<m>_{1}</m></cell>
							<cell>Linearity</cell>
							<cell><me>\lap{ a f(t) \pm b g(t) } = a \lap{f(t)} \pm b \lap{g(t)}</me></cell>
						</row>
					</tabular>
				</table>
			</p>
		</sidebyside>
	</subsection>

	<subsection label="lt-next-steps">
		<title>Next Step: Solving Differential Equations</title>
		<p>
			Everything you've learned in this chapter prepares you to solve differential equations using the Laplace transform. In the next chapter, you will see how these tools turn the process of solving differential equations into solving simple algebraic equations, especially when initial conditions are involved.
		</p>
	</subsection>

	<fact label="using-the-lt-table-cyu">
		<statement>
			<p>
				Answer the following questions.
				<task label="lt-reference-guide-chkpt-2"><title><e component="emoji">üìñ‚ùì</e>  Transform of <m>\sin(5t)</m></title>
					<statement>
						<p>
							<m>\ds\lap{\sin(5t)} = </m> ?
						</p>
					</statement>
					<choices randomize="yes">
						<choice correct="yes">
							<statement><m>\ds\frac{5}{s^2 + 25}</m></statement>
							<feedback>
								<p>
									Correct! This follows the formula <m>\lap{\sin(bt)} = \frac{b}{s^2 + b^2}</m> with <m>b = 5</m>.
								</p>
							</feedback>
						</choice>
						<choice>
							<statement><m>\ds\frac{s}{s^2 + 25}</m></statement>
							<feedback>
								<p>
									Incorrect. That's the transform of <m>\cos(5t)</m>, not <m>\sin(5t)</m>.
								</p>
							</feedback>
						</choice>
						<choice>
							<statement><m>\ds\frac{1}{s^2 + 25}</m></statement>
							<feedback>
								<p>
									Incorrect. The frequency coefficient <m>5</m> must appear in the numerator.
								</p>
							</feedback>
						</choice>
						<choice>
							<statement><m>\ds\frac{5}{s^2 + 5^2}</m></statement>
							<feedback>
								<p>
									This is mathematically correct but not simplified. Choose the version with <m>25</m> in the denominator.
								</p>
							</feedback>
						</choice>
					</choices>
				</task>
				<task label="lt-reference-guide-chkpt-3"><title><e component="emoji">üìñ‚ùì</e>  Transform of <m>\cos(-3t)</m></title>
					<statement>
						<p>
							<m>\ds\lap{\cos(-3t)} = </m> ?
						</p>
					</statement>
					<choices randomize="yes">
						<choice>
							<statement><m>\ds\frac{3}{s^2 + 9}</m></statement>
							<feedback>
								<p>
									Incorrect. The numerator for cosine should be <m>s</m>, not the frequency.
								</p>
							</feedback>
						</choice>
						<choice>
							<statement><m>\ds\frac{s}{s^2 - 9}</m></statement>
							<feedback>
								<p>
									Incorrect. The denominator should be <m>s^2 + 9</m>, not <m>s^2 - 9</m>.
								</p>
							</feedback>
						</choice>
						<choice correct="yes">
							<statement><m>\ds\frac{s}{s^2 + 9}</m></statement>
							<feedback>
								<p>
									Correct! Cosine is even, so <m>\cos(-3t)</m> = <m>\cos(3t)</m>, and its transform is <m>\ds\frac{s}{s^2 + 9}</m>.
								</p>
							</feedback>
						</choice>
						<choice>
							<statement><m>\ds\frac{3}{s^2 - 9}</m></statement>
							<feedback>
								<p>
									Incorrect. Both the numerator and denominator are wrong for cosine transforms.
								</p>
							</feedback>
						</choice>
					</choices>
				</task>
			</p>
		</statement>
	</fact>

	<!-- ================================================================ -->
	<!-- WRAP-UP + READING QUESTIONS                                      -->
	<!-- ================================================================ -->
	<subsection label="lt-reference-guide-wrap-up">
		<title>üì§ Wrap-Up</title>

		<assemblage label="lt-reference-guide-wrap-up-takeaways">
			<p>
				üóùÔ∏è <m>\textbf{Key Takeaways...}</m>
				<ul marker="square">
					<li></li>
				</ul>
			</p>
		</assemblage>
		<paragraphs label="lt-reference-guide-cyu">
			<title>Check Your Understanding</title>

			<exercise label="lt-reference-guide-cyu-bundle">
				<title><e component="emoji">ü§îüí≠</e> Separation of Variables Reading Questions</title>

				<task label="lt-reference-guide-cyu-1">
					<title><e component="emoji">ü§îüí≠</e> SOV and Nonlinear Equations</title>
					<statement correct="no">
						<p>
							The separation of variables method cannot be applied to non-linear differential equations.
						</p>
					</statement>
					<feedback>
						<p>
							Being able to solve non-linear differential equations is one of the strengths of the separation of variables method.
						</p>
					</feedback>
				</task>
				<task label="lt-reference-guide-cyu-2">
					<title><e component="emoji">ü§îüí≠</e> Sort the Steps in Order</title>

					<statement>
						<p>
							CONVERT TO PARSONS.. Suppose you want to use separation of variables method to determine the general solution of the differential equation
							<men xml:id="chkpt-lt-reference-guide-examples-1-eqn">
								\ds \frac{dq}{dt} - 3qt^2 = 2q
							</men>.
						</p>
						<p>
							Match the scrambled tasks (on the left) to the task order (on the right) that it should be performed to use this method.
						</p>
					</statement>
					<feedback>
						<p>
							Review the <xref ref="lt-reference-guide" text="custom">SOV Method</xref>.
						</p>
					</feedback>
					<cardsort>
						<match>
							<premise>
								<p>
									Equation is 1st-order ‚úÖ
								</p>
							</premise>
							
							<response>
								<p>
									<m>\text{Task 1}</m>
								</p>
							</response>
						</match>
						<match>
							<premise>
								<p>
									<m>\ds \frac{dq}{dt} = q(2 + 3t^2)</m>
								</p>
							</premise>
							<response>
								<p>
									<m>\text{Task 2}</m>
								</p>
							</response>
						</match>
						<match>
							<premise>
								<p>
									<m>\ds \frac{1}{q}\ dq = (2 + 3t^2)\ dt</m>
								</p>
							</premise>
							<response>
								<p>
									<m>\text{Task 3}</m>
								</p>
							</response>
						</match>
						<match>
							<premise>
								<p>
									<m>\ds \int \frac{1}{q} dq = \int (2 + 3t^2) dt</m>
								</p>
							</premise>
							
							<response>
								<p>
									<m>\text{Task 4}</m>
								</p>
							</response>
						</match>
						<match>
							<premise>
								<p>
									<line><m>\ds \ln|q| = 2t^2 + t^3 + c</m></line>
								</p>
							</premise>
							<response>
								<p>
									<m>\text{Task 5}</m>
								</p>	
							</response>
						</match>
						<match>
							<premise>
								<p>
									<line><m>\ds q = c e\vphantom{|}^{\large 2t^2 + t^3}</m></line>
								</p>
							</premise>
							<response>
								<p>
									<m>\text{Task 6}</m>
								</p>
							</response>
						</match>
					</cardsort>
				</task>
				<task label="lt-reference-guide-cyu-3">
					<title><e component="emoji">ü§îüí≠</e> Combining Constants</title>

					<statement>
						<p>
							Which of the following are valid ways to combine constants when finalizing your solution? Select ALL that apply.
						</p>
					</statement>
					<choices randomize="yes">
						<choice correct="yes">
							<statement>
								<m>
									\quad \left\{
									\begin{align}
										|y|	\amp = e^{2x + c_1}\\ 
										y	\amp = c_2 e^{2x} 
									\end{align}
									\right.\qquad
								</m> 
								where <m>c_2=\pm e^{c_1}</m>.
							</statement>
							<feedback>
								<p>
									Correct, since
									<md>
										<mrow>	|y|	\amp =,	e^{2x + c_1}										</mrow>
										<mrow>	y	\amp =,	\pm e^{2x + c_1}									</mrow>
										<mrow>	y	\amp =,	\pm e^{2x} \cdot e^{c_1}							</mrow>
										<mrow>	y	\amp =,	c_2 e^{2x}	\quad \text{where } c_2 = \pm e^{c_1}	</mrow>
									</md>
								</p>
							</feedback>
						</choice>
						<choice correct="yes">
							<statement>
								<m>
									\quad \left\{
									\begin{align}
										\frac{y^2}{2} \amp = \sin(x) + c_1\\ 
										y^2 \amp = 2\sin(x) + c_2 
									\end{align}
									\right.\qquad
								</m> 
								where <m>c_2 = 2c_1</m>.
							</statement>
							<feedback>
								<p>
									Correct, since
									<md>
										<mrow>	\frac{y^2}{2}	\amp =,	\sin(x) + c_1									</mrow>
										<mrow>	y^2				\amp =,	\sin(x) + 2c_1									</mrow>
										<mrow>	y^2				\amp =,	2\sin(x) + c_2	\quad \text{where } c_2 = 2c_1	</mrow>
									</md>
								</p>
							</feedback>
						</choice>
						<choice>
							<statement>
								<m>
									\quad \left\{
									\begin{align}
										y^2	\amp = 2\sin(x) + c_2\\ 
										y	\amp = \pm\sqrt{2\sin(x)} + c_3 
									\end{align}
									\right.\qquad
								</m> 
								where <m>c_3=\pm \sqrt{c_2}</m>.
							</statement>
							<feedback>
								<p>
									Incorrect, you should not combine constants here since <m>\quad\sqrt{A + B} \neq \sqrt{A} + \sqrt{B}</m>.
								</p>

								<p>
									Your solution should be written as
									<md>
										<mrow>	y^2	\amp =,	2\sin(x) + c_2											</mrow>
										<mrow>	y	\amp =,	\pm\sqrt{2\sin(x) + c_2}\quad \leftarrow\text{ done}	</mrow>
									</md>
								</p>
							</feedback>
						</choice>
						<choice>
							<statement>
								<m>
									\quad \left\{
									\begin{align}
										e^y	\amp =	3y + c_1\\ 
										y	\amp =	\ln(3y) + c_2 
									\end{align}
									\right.\qquad
								</m> 
								where <m>c_2= \ln(c_1)</m>.
							</statement>
							<feedback>
								
								<p>
									Incorrect, you should not combine constants here since <m>\ln(A + B) \neq \ln(A) + \ln(B)</m>.
								</p>

								<p>
									Your solution should be
									<md>
										<mrow>	e^y	\amp =,	3y + c_1									</mrow>
										<mrow>	y	\amp =,	\ln(3y + c_1)\quad \leftarrow\text{ done}	</mrow>
									</md>
								</p>
							</feedback>
						</choice>
						<choice>
							<statement>
								<m>
									\quad \left\{
									\begin{align}
										xy	\amp =	e^x + c_1\\ 
										y	\amp =	\frac{e^x}{x} + c_2 
									\end{align}
									\right.\qquad
								</m> 
								where <m>\ds c_2=\frac{c_1}{x}</m>.
							</statement>
							<feedback>
								<p>
									Incorrect, you should not combine constants here since <m>\frac{c_1}{x}</m> is not constant. Instead your solution should be left as
									<md>
										<mrow>	xy	\amp =,	e^x + c_1													</mrow>
										<mrow>	y	\amp =,	\frac{e^x + c_1}{x}											</mrow>
										<mrow>	y	\amp =,	\frac{e^x}{x} + \frac{c_1}{x}\quad \leftarrow\text{ done}	</mrow>
									</md>
								</p>
							</feedback>
						</choice>
						<choice correct="yes">
							<statement>
								<m>
									\quad \left\{
									\begin{align}
										\sqrt{y}	\amp =	c_1e^{3x}\\ 
										y			\amp =	c_2\, e^{6x} 
									\end{align}
									\right.\qquad
								</m> 
								where <m>c_2= c_1^2</m>.
							</statement>
							<feedback>
								<p>
									Correct, since
									<md>
										<mrow>	\sqrt{y}	\amp =,	c_1e^{3x}									</mrow>
										<mrow>	y			\amp =,	(c_1e^{3x})^2								</mrow>
										<mrow>	y			\amp =,	c_1^2(e^{3x})^2								</mrow>
										<mrow>	y			\amp =,	c_2\, e^{6x}\quad \text{where } c_2 = c_1^2	</mrow>
									</md>
								</p>
							</feedback>
						</choice>
					</choices>
				</task>
			</exercise>
		</paragraphs>
	</subsection>
</section>