<section>
	<title>Laplace Transform - Extra Details &amp; Resources</title>

	<!-- <paragraphs xml:id="lt-example-1-details000"><title>Explain why <m>\ds\lim_{b \to \infty} -\frac{5}{s}\left[ e^{-sb} - 1 \right] = -\frac{5}{s} \lim_{b \to \infty} \left[ e^{-sb} - 1 \right]</m></title>
		<p>
			 Since the limit only controls <m>b</m>, we can think of <m>s</m> as a number (like <m>2</m>). This means that <m>\ds-\frac{5}{s}</m> is also a number that can be pulled out of the limit using the limit property from calculus:
			<me>\ds\lim_{x \to \infty} c \cdot f(x) = c \cdot \lim_{x \to \infty} f(x), \quad c\ \text{is constant}</me>
		</p>
	</paragraphs> -->

	<!-- <paragraphs xml:id="graph-of-e-to-x000"><title>Exponential Behavior as its Power go to <m>\pm\infty</m></title>
		<figure xml:id="figure-e-to-x">
			<caption>
				The general limiting behavior of an exponential function as it's power goes to <m>+\infty</m> or <m>-\infty</m>.
			</caption>
			<image width="100%">
				<latex-image>
					\begin{tikzpicture}
						\begin{axis}[
							axis lines=middle,
							domain=-4.5:4.5,
							samples=100,
							ymin=-5,	ymax=16,
							xmin=-4.5,	xmax=4.5,
							ticklabel style = {font=\large}
						]
							\addplot[red, very thick] {exp(x)};
							\node at (-1.3,1.5)	[anchor=east, scale=1.2] {$0 \leftarrow e^{\text{ power}}$};
							\node at (2.4,10.5)	[anchor=west, scale=1.2] {$e^\text{ power}$};
							\node at (2.9,13)	[anchor=west, scale=1.2, rotate=-20] {$\uparrow$};
							\node at (3,14.5)	[anchor=west, scale=1.2] {$\infty$};
							\node at (1.3,-4)	[anchor=west, scale=1.1] {$\text{power } \rightarrow \infty$};
							\node at (-1,-4)	[anchor=east, scale=1.1] {$-\infty \leftarrow \text{ power}$};
						\end{axis}
					\end{tikzpicture}
				</latex-image>
			</image>
		</figure>
	</paragraphs> -->

	<!-- <paragraphs xml:id="lt-example-t-IVP-details000"><title>How?</title>
		<p>
			 Choosing
			<md>
				<mrow> u = t,	\quad\amp	dv = e^{-st}dt, 		</mrow>
				<mrow> du = dt,	\quad\amp	v = -\frac{1}{s}e^{-st}	</mrow>
			</md>
			integration by parts gives
			<md>
				<mrow>
					\int_0^b e^{-st} \cdot t\ dt
						\amp = -\frac{t}{s}e^{-st} - \int_0^b \left( -\frac{1}{s}e^{-st} \right) dt
				</mrow>
				<mrow> 	
						\amp = -\frac{t}{s}e^{-st}+ \frac{1}{s}\int_0^b e^{-st} dt
				</mrow>
				<mrow> 	
						\amp = \left(-\frac{t}{s}e^{-st}- \frac{1}{s^2}e^{-st}\right) \Bigg|_0^b
				</mrow>
				<mrow> 	
						\amp = \left(-\frac{b}{s}e^{-sb} - \frac{1}{s^2}e^{-sb}\right) - \left(0 - \frac{1}{s^2}\right)
				</mrow>
				<mrow> 	
						\amp = -\frac{b}{s}e^{-sb} - \frac{1}{s^2}e^{-sb} + \frac{1}{s^2}
				</mrow>
			</md>
		</p>
	</paragraphs> -->

	<!-- <paragraphs xml:id="lt-example-t-LH-details000"><title>How?</title>
		<p>
			 If <m>s \lt 0</m> then the power of <m>e^{-sb}</m> goes to <m>+\infty</m> as <m>b\to\infty</m>, so <m>L_1=be^{-sb} \to \infty</m> and <m>L_2=e^{-sb} \to \infty</m>. Therefore, we assume <m>s \gt 0</m> and compute the limits as
			<ul marker="square">
				<li>
					<p>
						<m>
							\ds L_1 
							= \lim_{b \to \infty}\frac{\os{\infty}{\os{\uparrow}{\boxed{b}}}}{\us{\infty}{\us{\downarrow}{\boxed{e^{sb}}}}}
							\,\us{LH}{=}\, \lim_{b \to \infty}\frac{1}{se^{sb}}
							= \frac{1}{s}\lim_{b \to \infty}\frac{1}{\us{\infty}{\us{\downarrow}{\boxed{e^{sb}}}}} = 0
						</m>
					</p>
				</li>
				<li>
					<p>
						<m>
							\ds L_2
							= \lim_{b \to \infty}\frac{1}{\us{\infty}{\us{\downarrow}{\boxed{e^{sb}}}}} = 0
						</m>
					</p>
				</li>
			</ul>
			where <m>LH</m> denotes L'H么pital's Rule was applied to the limit.
		</p>
	</paragraphs> -->

	<!-- <paragraphs xml:id="lt-example-2-details000"><title>How?</title>
		<p>
			 Using <m>u</m>-substitution with
			<md>
				<mrow>
					u	\amp = \ob{(7-s)}^{\text{constant}}t
				</mrow>
				<mrow>
					du	\amp = (7-s)dt \quad \Rightarrow \quad dt = \frac{du}{7-s}
				</mrow>
			</md>
			the integral is compute as
			<md>
				<mrow>
					\int_0^b e^{(7-s)t}\ dt	= \int_{t=0}^{t=b} e^{u}\frac{du}{7-s}
					\amp = \frac{1}{7-s}\int_{t=0}^{t=b} e^{u}\ du
				</mrow>
				<mrow>
					\amp = \frac{1}{7-s} \left[ e^{u} - 1 \right]\Bigg|_{t=0}^{t=b}
				</mrow>
				<mrow>
					\amp = \frac{1}{7-s} \left[ e^{7-s} - 1 \right]\Bigg|_{0}^{b}
				</mrow>
			</md>.
		</p>
	</paragraphs> -->





	<!-- <paragraphs xml:id="lt-example-tnth-IVP-details000"><title>How?</title>
		<p>
			<md>
				<mrow> u = t^n,				\quad\amp	dv = e^{-st}dt, 		</mrow>
				<mrow> du = nt^{n-1}\ dt,	\quad\amp	v = -\frac{1}{s}e^{-st}	</mrow>
			</md>
			integration by parts gives
			<md>
				<mrow>
					\lap{ t^{n} }
					\amp = \lim_{b \to \infty} \left[-\frac{t^{n}}{s}e^{-sb}\Bigg|_0^b - \int_0^b \left(-\frac{1}{s}e^{-st}\right)\cdot nt^{n-1}\ dt\right]
				</mrow>
				<mrow>
					\amp = \lim_{b \to \infty} \left[\left(-\frac{b^n}{s}e^{-sb} - 0\right) + \frac{n}{s}\int_0^b e^{-st}\cdot t^{n-1}\ dt\right]
				</mrow>
				<mrow>
					\amp = \lim_{b \to \infty} \left[-\frac{b^n}{e^{sb}} + \frac{n}{s}\int_0^b e^{-st}\cdot t^{n-1}\ dt\right]
				</mrow>
			</md>
		</p>
	</paragraphs> -->

	<!-- <paragraphs xml:id="lt-example-tnth-LH-details000"><title>How?</title>
		<p>
			The reasoning is the same as in <xref ref="lt-example-tnth-IVP-details" text="custom">previous solution</xref> except we apply L'H么pital's rule <em>n</em> times. So we have
			<md>
				<mrow>
					\lim_{b \to \infty}\frac{b^n}{e^{sb}}\
					\amp\os{\large\left(\frac{\infty}{\infty}\right)}{\us{LH}{=}}
					\lim_{b \to \infty}\frac{nb^{n-1}}{se^{sb}}
					= \frac{n}{s}\lim_{b \to \infty}\frac{b^{n-1}}{e^{sb}}
				</mrow>
				<mrow>
					\amp\os{\large\left(\frac{\infty}{\infty}\right)}{\us{LH}{=}}
					\frac{n}{s}\lim_{b \to \infty}\frac{(n-1)b^{n-2}}{se^{sb}}
					= \frac{n(n-1)}{s^2}\lim_{b \to \infty}\frac{b^{n-2}}{e^{sb}}
				</mrow>
				<mrow>
					\amp \qquad\qquad \vdots \quad LH\ \ n-2 \text{ more times}
				</mrow>
				<mrow>
					\amp\os{\large\left(\frac{\infty}{\infty}\right)}{\us{LH}{=}}
					\frac{n!}{s^n}\lim_{b \to \infty}\frac{1}{se^{sb}}
					= \frac{n!}{s^{n+1}}\lim_{b \to \infty}\frac{1}{\us{\infty}{\us{\downarrow}{\boxed{e^{sb}}}}}
					= 0
				</mrow>
			</md>
		</p>
	</paragraphs> -->

	<!-- <paragraphs xml:id="lt-example-4-details000"><title>How?</title>
		<p>
			 If <m>s &gt; 0</m>, then we know that <m>e^{-sb} \to 0</m> as <m>b \to \infty</m> and both <m>\cos(3b)</m> and <m>\sin(3b)</m> oscillate between <m>-1</m> and <m>1</m>, Thus, their product must approach zero. That is,
			<me>
				\lim_{b \to \infty} e^{-sb} \cos(3b) = 0 \quad \text{and} \quad \lim_{b \to \infty} e^{-sb} \sin(3b) = 0
			</me>
		</p>
	</paragraphs> -->







	<!-- <paragraphs xml:id="example-key-steps"><title>Key Steps</title>
		<p>
			Key Steps
			<dl>
				<li xml:id="lt-derivative-key-step-1"><title><m>\os{[1]}{=}</m></title>
					Integration by parts with <m>u = f(t)</m> and <m>dv = e^{-st} dt</m>
				</li>
				<li xml:id="lt-derivative-key-step-2"><title><m>\os{[2]}{=}</m></title>
					<m>s</m> is a constant in this integral, so we can bring it out.
				</li>
				<li xml:id="lt-derivative-key-step-3"><title><m>\os{[3]}{=}</m></title>
					<m>\ds e^{-st} f(t) = \frac{f(t)}{e^{st}}</m> must go to zero.
				</li>
			</dl>
		</p>
	</paragraphs> -->




	

	

	


	<!-- <theorem xml:id="std_LT_01"><title> </title>
		<p>
				<aside>
					<p>
						Key Steps
						<me>
							\begin{array}{ll}
								(1) \amp \text{IBP with }\\
									\amp u = t^2, dv = e^{-st} dt\\
								(2) \amp \text{factor out } -\frac{1}{s}\\
								(3) \amp \text{definition of the}\\
									\amp \text{Laplace transform of } t\\
								(4) \amp \text{convert evaluation at } \infty\\
									\amp \text{to the limit at } \infty \\
								(5) \amp \text{L'H么pital's Rule }\\
							\end{array}
						</me>
					</p>
				</aside>
				<md>
					<mrow> \lap{ t^2 }	
							\amp = \int_0^{\infty} e^{-st}\cdot t^2 dt 				</mrow>
					<mrow>  \amp\os{(1)}{=} t^2 \cdot -\frac{1}{s}e^{-st}\Bigg|_0^{\infty}
								- \int_0^{\infty} -\frac{1}{s}e^{-st}\cdot 2tdt </mrow>
					<mrow>  \amp\os{(2)}{=} -\frac{1}{s}\left[ t^2e^{-st}\Bigg|_0^{\infty}
								- 2\int_0^{\infty}e^{-st}\cdot tdt \right]		</mrow>
					<mrow>  \amp\os{(3)}{=} -\frac{1}{s}\left[t^2e^{-st}\Bigg|_0^{\infty}
								- 2\lap{ t } \right]							</mrow>
					<mrow>  \amp\os{(4)}{=} -\frac{1}{s}\left[ \lim_{b \to \infty}
								t^2e^{-st}\Bigg|_0^{b} - 2\lap{ t } \right]		</mrow>
					<mrow>  \amp = -\frac{1}{s}\left[ \lim_{b \to \infty}
								\left( b^2e^{-sb} - 0^2\cdot e^{-s\cdot 0} \right)
								- 2\cdot \frac{1}{s^2} \right]					</mrow>
					<mrow>  \amp = -\frac{1}{s}\left[ \lim_{b \to \infty}
								b^2e^{-sb} - 0 - \frac{2}{s^2} \right]			</mrow>
					<mrow>  \amp = -\frac{1}{s}\left[ \lim_{b \to \infty}
								\frac{b^2}{e^{sb}} - \frac{2}{s^2} \right]		</mrow>
					<mrow>  \amp\os{(5)}{=} -\frac{1}{s}\left[ \lim_{b \to \infty}
								\frac{2b}{se^{sb}} - \frac{2}{s^2} \right]		</mrow>
					<mrow>  \amp = -\frac{1}{s}\left[ \frac{2}{s}\lim_{b \to \infty}
								\frac{b}{e^{sb}} - \frac{2}{s^2} \right]		</mrow>
					<mrow>  \amp = -\frac{1}{s}\left[ \frac{2}{s}\lim_{b \to \infty}
								\frac{1}{se^{sb}} - \frac{2}{s^2} \right]		</mrow>
					<mrow>  \amp = -\frac{1}{s}\left[ \frac{2}{s}\cdot 0
								- \frac{2}{s^2} \right]							</mrow>
					<mrow>  \amp = \frac{2}{s^3} 									</mrow>
				</md>
		</p>
	</theorem> -->

	<!-- <theorem xml:id="std_LT_02"><title> </title>
		<p>
			<aside>
				<p>
					Key Steps
					<me>
						\begin{array}{ll}
							(1) \amp \text{IBP with }\\
								\amp u = t^3, dv = e^{-st} dt\\
							(2) \amp \text{factor out } -\frac{1}{s}\\
							(3) \amp \text{definition of the}\\
								\amp \text{Laplace transform of } t\\
							(4) \amp \text{convert evaluation at } \infty\\
								\amp \text{to the limit at } \infty \\
							(5) \amp \text{L'H么pital's Rule }\\
						\end{array}
					</me>
				</p>
			</aside>
			<md>
				<mrow> \lap{ t^3 }	
						\amp = \int_0^{\infty} e^{-st}\cdot t^3 dt </mrow>
				<mrow>  \amp\os{(1)}{=} t^3 \cdot -\frac{1}{s}e^{-st}\Bigg|_0^{\infty} - \int_0^{\infty} -\frac{1}{s}e^{-st}\cdot 3t^2dt </mrow>
				<mrow>  \amp\os{(2)}{=} -\frac{1}{s}\left[ t^3e^{-st}\Bigg|_0^{\infty} - 3\int_0^{\infty}e^{-st}\cdot t^2 dt \right]</mrow>
				<mrow>  \amp\os{(3)}{=} -\frac{1}{s}\left[ \lim_{b \to \infty}t^3 e^{-st}\Bigg|_0^{b} - 3\lap{ t^2 } \right]</mrow>
				<mrow>  \amp\os{(4)}{=} -\frac{1}{s}\left[ \lim_{b \to \infty}\left( b^3 e^{-sb} - 0^3\cdot e^{-s\cdot 0} \right) - 3\cdot \frac{2}{s^3} \right]</mrow>
				<mrow>  \amp = -\frac{1}{s}\left[ \lim_{b \to \infty}b^3 e^{-sb} - 0 - \frac{6}{s^3} \right]</mrow>
				<mrow>  \amp = -\frac{1}{s}\left[ \lim_{b \to \infty}\frac{b^3}{e^{sb}} - \frac{6}{s^3} \right]</mrow>
				<mrow>  \amp\os{(5)}{=} -\frac{1}{s}\left[ \lim_{b \to \infty}\frac{3b^2}{se^{sb}} - \frac{6}{s^3} \right]</mrow>
				<mrow>  \amp = -\frac{1}{s}\left[ \frac{3}{s}\lim_{b \to \infty}\frac{b^2}{e^{sb}} - \frac{6}{s^3} \right]</mrow>
				<mrow>  \amp = -\frac{1}{s}\left[ \frac{3}{s}\lim_{b \to \infty}\frac{2b}{se^{sb}} - \frac{6}{s^3} \right]</mrow>
				<mrow>  \amp = -\frac{1}{s}\left[ \frac{6}{s^2}\lim_{b \to \infty}\frac{b}{e^{sb}} - \frac{6}{s^3} \right]</mrow>
				<mrow>  \amp = -\frac{1}{s}\left[ \frac{6}{s^2}\lim_{b \to \infty}\frac{1}{se^{sb}} - \frac{6}{s^3} \right]</mrow>
				<mrow>  \amp = -\frac{1}{s}\left[ \frac{6}{s^2}\cdot 0 - \frac{6}{s^3} \right]</mrow>
				<mrow>  \amp = \frac{6}{s^4} </mrow>
			</md>
		</p>
	</theorem> -->

	<!-- <theorem xml:id="std_LT_03"><title> </title>
		<p>
			<aside>
				<p>
					Key Steps
					<me>
						\begin{array}{ll}
							(1) \amp \text{IBP with }\\
								\amp u = t^4, dv = e^{-st} dt\\
							(2) \amp \text{factor out } -\frac{1}{s}\\
							(3) \amp \text{definition of the}\\
								\amp \text{Laplace transform of } t\\
							(4) \amp \text{convert evaluation at } \infty\\
								\amp \text{to the limit at } \infty \\
							(5) \amp \text{L'H么pital's Rule }\\
						\end{array}
					</me>
				</p>
			</aside>
			<md>
				<mrow> \lap{ t^4 }	
					\amp = \int_0^{\infty} e^{-st}\cdot t^4 dt
				</mrow>
				<mrow>
					\amp\os{(1)}{=} t^4 \cdot -\frac{1}{s}e^{-st}\Bigg|_0^{\infty} - \int_0^{\infty} -\frac{1}{s}e^{-st}\cdot 4t^3dt
				</mrow>
				<mrow>
					\amp\os{(2)}{=} -\frac{1}{s}\left[ t^4e^{-st}\Bigg|_0^{\infty} - 4\int_0^{\infty}e^{-st}\cdot t^3 dt \right]
				</mrow>
				<mrow>
					\amp\os{(3)}{=} -\frac{1}{s}\left[ \lim_{b \to \infty}t^4 e^{-st}\Bigg|_0^{b} - 4\lap{ t^3 } \right]
				</mrow>
				<mrow>
					\amp\os{(4)}{=} -\frac{1}{s}\left[ \lim_{b \to \infty}\left( b^4 e^{-sb} - 0^4\cdot e^{-s\cdot 0} \right) - 4\cdot \frac{6}{s^4} \right]
				</mrow>
				<mrow>
					\amp = -\frac{1}{s}\left[ \lim_{b \to \infty}b^4 e^{-sb} - 0 - \frac{24}{s^4} \right]
				</mrow>
				<mrow>
					\amp = -\frac{1}{s}\left[ \lim_{b \to \infty}\frac{4b^3}{se^{sb}} - \frac{24}{s^4} \right]
				</mrow>
				<mrow>
					\amp = -\frac{1}{s}\left[ \frac{4}{s}\lim_{b \to \infty}\frac{b^3}{e^{sb}} - \frac{24}{s^4} \right]
				</mrow>
				<mrow>
					\amp\os{(5)}{=} -\frac{1}{s}\left[ \frac{4}{s}\lim_{b \to \infty}\frac{3b^2}{se^{sb}} - \frac{24}{s^4} \right]
				</mrow>
				<mrow>
					\amp = -\frac{1}{s}\left[ \frac{12}{s^2}\lim_{b \to \infty}\frac{b^2}{e^{sb}} - \frac{24}{s^4} \right]
				</mrow>
				<mrow>
					\amp = -\frac{1}{s}\left[ \frac{12}{s^2}\lim_{b \to \infty}\frac{2b}{se^{sb}} - \frac{24}{s^4} \right]
				</mrow>
				<mrow>
					\amp = -\frac{1}{s}\left[ \frac{24}{s^3}\lim_{b \to \infty}\frac{b}{e^{sb}} - \frac{24}{s^4} \right]
				</mrow>
				<mrow>
					\amp = -\frac{1}{s}\left[ \frac{24}{s^3}\lim_{b \to \infty}\frac{1}{se^{sb}} - \frac{24}{s^4} \right]
				</mrow>
				<mrow>
					\amp = -\frac{1}{s}\left[ \frac{24}{s^3}\cdot 0 - \frac{24}{s^4} \right]
				</mrow>
				<mrow>
					\amp = \frac{24}{s^5}
				</mrow>
			</md>
		</p>
	</theorem> -->

	<!-- <theorem xml:id="LT-PDF-Details-02"><title> </title>
		<p>
			Partial fraction decomposition has the form,
			<me> \frac{54}{(s+1)(s^2  - 4s + 13)} = \frac{A}{s+1} + \frac{Bs + C}{s^2 - 4s + 13}, </me>
			and we find <m>A</m>, <m>B</m>, and <m>C</m> by
			<md>
				<mrow>54	\amp = A(s^2 - 4s + 13) + (Bs+C)(s+1)</mrow>
				<mrow>54	\amp = As^2 - 4As + 13A + Bs^2 + Bs + Cs + C</mrow>
				<mrow>0s^2 + 0s + 54	\amp = (A + B)s^2 + (-4A + B + C)s + (13A + C)</mrow>
			</md>

			<md>
				<mrow>A+B	\amp = 0		\amp -4A +B+C	\amp = 0	\amp 	13A + C	\amp = 54</mrow>
				<mrow>A	\amp = -B	\amp			\amp	\amp			\amp</mrow>
				<mrow>\amp		\amp -4(-B)+B+C	\amp = 0	\amp 13(-B)+C	\amp = 54</mrow>
				<mrow>\amp		\amp 	5B + C	\amp = 0	\amp -13B + C	\amp = 54</mrow>
				<mrow>\amp		\amp		C	\amp = -5B	\amp		\amp</mrow>
				<mrow>\amp		\amp			\amp	\amp -13B + (-5B)	\amp = 54</mrow>
				<mrow>\amp		\amp			\amp	\amp 		-18B	\amp = 54</mrow>
				<mrow>\amp		\amp			\amp	\amp		B	\amp = -3</mrow>
				<mrow>A	\amp = -(-3)	\amp		C	\amp = -5(-3)\amp			\amp</mrow>
				<mrow>\amp = 3		\amp			\amp = 15\amp			\amp</mrow>
			</md>
		</p>
	</theorem> -->

	<!-- <theorem xml:id="LT-Solving_w_LTs_verify_soln"><title> </title>
		<p>
			<md>
				<mrow>x(t)	\amp = 3e^{-t} - 3e^{2t}\cos(3t) + 3e^{2t}\sin(3t)</mrow>
				<mrow>\amp = 3e^{-t} + e^{2t} \Big[ 3\sin(3t) - 3\cos(3t) \Big]</mrow>
				<mrow>\amp</mrow>
				<mrow>x'(t)	\amp = -3e^{-t} + e^{2t}\Big[ 9\cos(3t) + 9\sin(3t) \Big]</mrow>
							+ 2e{2t}\Big[ 3\sin(3t) - 3\cos(3t) \Big]
				<mrow>\amp = -3e^{-t} + e^{2t}\Big[ 9\cos(3t) + 9\sin(3t) + 6\sin(3t) - 6\cos(3t) \Big]</mrow>
				<mrow>\amp = -3e^{-t} + e^{2t}\Big[ 3\cos(3t) + 15\sin(3t) \Big]</mrow>
				<mrow>\amp</mrow>
				<mrow>x''(t)	\amp = 3e^{-t} + e^{2t}\Big[ -9\sin(3t) + 45\cos(3t) \Big]</mrow>
							+ 2e^{2t}\Big[ 3\cos(3t) + 15\sin(3t) \Big]
				<mrow>\amp = 3e^{-t} + e^{2t}\Big[ -9\sin(3t) + 45\cos(3t) + 6\cos(3t) + 30\sin(3t)  \Big]</mrow>
				<mrow>\amp = 3e^{-t} + e^{2t}\Big[ 21\sin(3t) + 51\cos(3t) \Big]</mrow>
			</md>
			
			<md>
				<mrow>LHS	\amp = x'' - 4x' + 13x</mrow>
				<mrow>\amp = \left( 3e^{-t} + e^{2t}\Big[ 21\sin(3t) + 51\cos(3t) \Big] \right) </mrow>
					- 4\left( -3e^{-t} + e^{2t}\Big[ 3\cos(3t) + 15\sin(3t) \Big] \right)
					+ 13\left( 3e^{-t} + e^{2t} \Big[ 3\sin(3t) - 3\cos(3t) \Big] \right)
				<mrow>\amp = 3e^{-t} + e^{2t}\Big[ 21\sin(3t) + 51\cos(3t) \Big] </mrow>
					+ 12e^{-t} + e^{2t}\Big[ -12\cos(3t) - 60\sin(3t) \Big]
					+ 39e^{-t} + e^{2t} \Big[ 39\sin(3t) - 39\cos(3t) \Big]
				<mrow>\amp = 3e^{-t} + e^{2t}\Big[ 21\sin(3t) + 51\cos(3t) \Big] </mrow>
					+ 12e^{-t} + e^{2t}\Big[ -12\cos(3t) - 60\sin(3t) \Big]
					+ 39e^{-t} + e^{2t} \Big[ 39\sin(3t) - 39\cos(3t) \Big]
				<mrow>\amp = 54e^{-t}</mrow>
				<mrow>\amp = RHS</mrow>
			</md>
		</p>

		<p>
			We also verify the initial conditions:
			<md>
				<mrow>x(0)	\amp = 3e^{-0} + e^{2\cdot 0} \Big[ 3\sin(3\cdot 0) - 3\cos(3\cdot 0) \Big]</mrow>
				<mrow>\amp = 3 + \Big[ 3\cdot 0 - 3\cdot 1 \Big]</mrow>
				<mrow>\amp = 3 - 3</mrow>
				<mrow>\amp = 0</mrow>
				<mrow>\amp</mrow>
				<mrow>x'(0)	\amp = -3e^{-0} + e^{2\cdot 0}\Big[ 3\cos(3\cdot 0) + 15\sin(3\cdot 0) \Big]</mrow>
				<mrow>\amp = -3 + \Big[ 3\cdot 1 + 15\cdot 0 \Big]</mrow>
				<mrow>\amp = - 3 + 3</mrow>
				<mrow>\amp = 0</mrow>
			</md>
		</p>
	</theorem> -->
	
</section>