<subsection xmlns:xi="http://www.w3.org/2001/XInclude"><title> <m>\lap\{\sin(bt)\},\ \lap\{\cos(bt)\}</m> </title>

	<p>
		We can use the definition of the Laplace transform to find the Laplace transforms of sine and cosine functions.
	</p>

	<example>

		<m>\quad</m> Compute <m> \lap \{ \cos(3t) \} </m>.

		<solution>
			<p>
				By the definition of the Laplace transform, we have
				<me>
					\lap \{ \cos(3t) \} = \int_0^{\infty} e^{-st} \cos(3t) dt 
				</me>.
				We could write this improper integral as a limit and use integration by parts on the integral. However, we could also rewrite cosine as 
				<me>
					\cos(3t) = \frac{e^{3it} + e^{-3it}}{2}
				</me>.
				Then, we can write
				<md>
					<mrow> 
						\lap \{ \cos(3t) \} 
							=\amp \frac{1}{2} \ub{\int_0^{\infty} e^{-st} e^{3it} dt}_{\lap\{e^{3it}\}} + 
								\frac{1}{2} \ub{\int_0^{\infty} e^{-st} e^{-3it} dt}_{\lap\{e^{-3it}\}}
					</mrow>
					<mrow> 
							=\amp \frac{1}{2} \lap\{e^{3it}\} + \frac{1}{2} \lap\{e^{-3it}\}
					</mrow>
					<mrow> 
							=\amp \frac{1}{2} \left[\frac{1}{s - 3i} + \frac{1}{s + 3i}\right]
					</mrow>
					<mrow> 
							=\amp \frac{1}{2} \left[\frac{s+3i + s-3i}{(s - 3i)(s + 3i)}\right]
					</mrow>
					<mrow> 
							=\amp \frac{s}{s^2 + 9}
					</mrow>
				</md>
			</p>
		</solution>
	</example>

	<example>

		<m>\quad</m> Compute <m> \lap \{ \sin(-4t) \} </m>.

		<solution>
			<p>
				By the definition of the Laplace transform, we have
				<me>
					\lap \{ \sin(-4t) \} = \int_0^{\infty} e^{-st} \sin(-4t) dt
				</me>.
				Similar to cosine, we can rewrite sine as
				<me>
					\sin(-4t) = \frac{e^{-4it} - e^{4it}}{2i}
				</me>.
				So,
				<md>
					<mrow> 
						\lap \{ \sin(-4t) \} 
							=\amp \frac{1}{2i} \ub{\int_0^{\infty} e^{-st} e^{-4it} dt}_{\lap\{e^{-4it}\}} - 
								\frac{1}{2i} \ub{\int_0^{\infty} e^{-st} e^{4it} dt}_{\lap\{e^{4it}\}}
					</mrow>
					<mrow> 
							=\amp \frac{1}{2i} \lap\{e^{-4it}\} - \frac{1}{2i} \lap\{e^{4it}\}
					</mrow>
					<mrow> 
							=\amp \frac{1}{2i} \left[\frac{1}{s + 4i} - \frac{1}{s - 4i}\right]
					</mrow>
					<mrow> 
							=\amp \frac{1}{2i} \left[\frac{s - 4i - s - 4i}{(s + 4i)(s - 4i)}\right]
					</mrow>
					<mrow> 
							=\amp \frac{4}{s^2 + 16}
					</mrow>
				</md>
			</p>
		</solution>
	</example>

	<assemblage xml:id="lt-table-L1-L5"><title>Common Laplace Transforms</title>
		<p>
			<dl width="narrow">
				<li><title><m>{\LARGE \vphantom{\int}}L_1.</m></title>
					<m>\ds \lap\{ 1 \} = \frac{1}{s}, \quad s &gt;0 </m>
				</li>
				<li><title><m>{\LARGE \vphantom{\int}}L_2.</m></title>
					<m>\ds \lap\{ e^{at} \} = \frac{1}{s - a}, \quad s &gt;a, \quad a \text{ is a constant} </m>
				</li>
				<li><title><m>{\LARGE \vphantom{\int}}L_3.</m></title>
					<m>\ds \lap\{ t^n \} = \frac{n!}{s^{n+1}}, \quad s &gt;0, \quad n = 1, 2, 3, \ldots </m>
				</li>
				<li xml:id="L4"><title><m>{\LARGE \vphantom{\int}}L_4.</m></title>
					<m>\ds \lap\{ \sin(bt) \} = \frac{b}{s^2+b^2}, \quad s &gt;0, \quad b \text{ is a constant} </m>
				</li>
				<li xml:id="L5"><title><m>{\LARGE \vphantom{\int}}L_5.</m></title>
					<m>\ds \lap\{ \cos(bt) \} = \frac{s}{s^2+b^2}, \quad s &gt;0, \quad b \text{ is a constant} </m>
				</li>
			</dl>
		</p>
	</assemblage>

	<xi:include href="./c4-s1-ss4-interactives.ptx" />

</subsection>