<subsection xmlns:xi="http://www.w3.org/2001/XInclude"><title> Step 3: Give Solution </title>

	<introduction>

		<outcomes>
			<ul>
				<li> 
					Find the general solution from the characteristic equation solutions.
				</li>
				<li> 
					Master ? Step 3 ? of ?
				</li>
			</ul>
		</outcomes>

		<p>
			We are nearly prepared to apply the full ? to an ? LHCC equation ?. The only thing left to do is discuss how to use the solutions of the characteristic equation to find the general solution. 
		</p>

		<p>
			As a review, suppose we want to find the general solution to the LHCC differential equation
			<men xml:id="full-lhcc-eqn1">
				y'' - 9 y = 0.
			</men>
			According to <xref ref="concept-lhcc-terms"/>, all the parts of the solution should look like <m>e^{rx}</m>. With this in mind, we plugged <m>y = e^{rx}</m> into <xref ref="full-lhcc-eqn1"/>, leading to the characteristic equation
			<me>
				r^2 - 9 = 0,
			</me>
			which has solutions <m>r_1 = 3, r_2 = -3</m>. Therefore, the general solution is a combination of <m>e^{3x}</m> and <m>e^{-3x}</m>, given by
			<men  xml:id="full-lhcc-sol1">
				y(x) = c_1\ e^{3x} + c_2\ e^{-3x}
			</men>
			where <m>c_1, c_2</m> are unknown constants.
		</p>

		<p>
			This example shows how the solutions to the characteristic equation lead to the general solution, but not every case works out this nicely. The next few sections, break down differences for each cases that you may encounter.
		</p>

	</introduction>

	<introduction>
		<p>
			We start with ? LHCC equations ? of order 2 for two important reasons: (1) they represent the most common form you will encounter, and (2) the ideas discussed in this section naturally extend to higher order cases.
		</p>

		<p>
			<lemma xml:id="concept-lhcc-strategy-cases"><title>Order 2 LHCC General Solution Cases</title><p/>
				<statement>
					<p>
						The 2nd order LHCC DE
						<men xml:id="lhcc-cases-de">
							a\ y'' + b\ y' + c\ y = 0,
						</men>
						with characteristic equation 
						<men xml:id="lhcc-cases-ce">
							a\ r^2 + b\ r + c = 0,
						</men>
						has one the following three general solutions:
						<dl width="narrow">
							<li xml:id="lhcc-case-1"><title> Case 1: if <m>r = r_1, r_2 \,\,</m> are real and different, then </title>
								<p>
									<me> y(x) = c_1\ e^{r_1 x} + c_2\ e^{r_2 x} </me>
								</p>
							</li>
							<li xml:id="lhcc-case-2"><title> Case 2: if <m>r = r_1, r_2 \,\,</m> are real and equal, then </title>
								<p>
									<me> y(x) = c_1\ e^{r_1 x} + c_2\ x\ e^{r_2 x} </me>
								</p>
							</li>
							<li xml:id="lhcc-case-3"><title> Case 3: if <m>r = \alpha \pm i \beta \,\,</m> is complex, then </title>
								<p>
									<me> y(x) = e^{\alpha\ x} (c_1\ \sin(\beta x) + c_2\ \cos(\beta x)) </me>
								</p>
							</li>
						</dl>
					</p>
				</statement>
			</lemma> 
		</p>
	</introduction>

	<xi:include href="./c3-s1-ss3-interactives.ptx" />

</subsection>