<exercises><title> Warm-ups &amp; Drills </title>
		
	<exercise><title> Inverse Transforms using Linearity </title>
		<p>
			<statement>
				<p>
					Apply a backward transform (step 4) to revert each Laplace solution back into a function of <m>t</m>.
				</p>
				<tabular>
					<col width="20%" halign="center"/>
					<col width="75%"/>
					<row>
						<cell><m>\ds \frac{12}{s}</m></cell>
						<cell>
							<p>
								<m>\hspace{27em}</m>
								<solution>
									<p>
										The <m>s</m> in the denominator tells us that we need <m>L_1</m>. Before we do, let's factor out <m>12</m>:
										<me>\ds \ilap{\frac{12}{s}} = 12 \cdot \ilap{\frac{1}{s}} = 12 \cdot 1 = 12</me>.
									</p>
								</solution>
							</p>
						</cell>
					</row>
					<row>
						<cell><m>\ds \frac{5}{s^2 + 4}</m></cell>
						<cell>
							<p>
								<m>\hspace{27em}</m>
								<solution>
									<p>
										Since the denominator has the form, <m>s^2 + \text{number}</m>, and there is no <m>s</m> in the numerator, we should apply <m>L_4</m>. As before, it is helpful to first factor out the constant <m>5</m>,
										<me>\ds \ilap{\frac{5}{s^2 + 4}} = 5\ \ilap{\frac{1}{s^2 + 4}} \quad \leftarrow <xref ref="L4" text="custom">L_4</xref> (b=2)</me>.
										According to <m>L_4</m>, we are missing <m>2</m> in the numerator. Let's put it there by multiplying by <m>2/2</m>, like so
										<md>
											<mrow> = 5\ \ilap{\frac{2}{2}\frac{1}{s^2 + 4}} \amp = 5\ \ilap{\frac{1}{2}\frac{2}{s^2 + 4}}</mrow>
											<mrow>										  \amp = \frac{5}{2} \ilap{\frac{2}{s^2 + 4}}</mrow>
											<mrow>										  \amp = \frac{5}{2} \sin(2t)</mrow>
										</md>
									</p>
								</solution>
							</p>
						</cell>
					</row>
					<row>
						<cell><m>\ds \frac{17}{s^4}</m></cell>
						<cell>
							<p>
								<m>\hspace{27em}</m>
								<solution>
									<p>
										This denominator has the form <m>s^{\text{power}}</m>, which matches <m>L_3</m> with <m>n = 3</m>.
										<me>\ds \ilap{\frac{17}{s^4}} = 17\ \ilap{\frac{1}{s^4}} \quad \leftarrow <xref ref="L3" text="custom">L_3</xref> (n=3)</me>.
										In this case, the numerator is missing a <m>3!</m>. We can introduce it by multiplying by <m>3!/3!</m>, like so
										<md>
											<mrow> = 17\ \ilap{\frac{3!}{3!}\frac{1}{s^4}} = \frac{17}{3!} \ilap{\frac{3!}{s^4}} = \frac{17}{6} t^3</mrow>
										</md>
									</p>
								</solution>
							</p>
						</cell>
					</row>
					<row>
						<cell><m>\ds \frac{7s}{s^2 + 25}</m></cell>
						<cell>
							<p>
								<m>\hspace{27em}</m>
								<solution>
									<p>
										<me><xref ref="L5" text="custom">L_5</xref>, b=5</me>
										<me> \ilap{\frac{7s}{s^2 + 25}} = 7\ \ilap{\frac{s}{s^2 + 25}} = 7\ \cos(5t)</me>
									</p>
								</solution>
							</p>
						</cell>
					</row>
					<row>
						<cell><m>\ds \frac{10}{(s - 3)^2 + 11}</m></cell>
						<cell>
							<p>
								<m>\hspace{27em}</m>
								<solution>
									<p>
										The form of this denominator is <m>\ul{(s \pm \text{shift})^{2} + \text{number}}</m> and has no <m>s</m> in the numerator. Therefore,
										<md>
											<mrow> \ilap{\frac{10}{(s - 3)^2 + 11}} \amp\ \quad <xref ref="L7" text="custom"><m>L_7</m></xref> (a=3,\ b=\sqrt{11})</mrow>
											<mrow>	\amp = 10\ \ilap{\frac{\sqrt{11}}{\sqrt{11}}\frac{1}{(s - 3)^2 + 11}}</mrow>
											<mrow>	\amp = \frac{10}{\sqrt{11}} \ilap{\frac{\sqrt{11}}{(s - 3)^2 + 11}}</mrow>
											<mrow>	\amp = \frac{10}{\sqrt{11}} e^{3t} \sin(\sqrt{11}t)</mrow>
										</md>

									</p>
								</solution>
							</p>
						</cell>
					</row>
					<row>
						<cell><m>\ds \frac{2}{(s+7)^5}</m></cell>
						<cell>
							<p>
								<m>\hspace{27em}</m>
								<solution>
									<p>
										The denominator, <m>\ul{(s \pm \text{shift})^{\text{power}}}</m>, indicates an <m>e^{at}</m> and a <m>t^n</m> term. Therefore,
										<md>
											<mrow> \ilap{\frac{2}{(s+7)^5}} \amp\ \quad <xref ref="L6" text="custom"><m>L_6</m></xref> (a=-7, n=4)</mrow>
											<mrow>
													\amp = 2\ \ilap{\frac{4!}{4!}\frac{1}{(s+7)^5}}
											</mrow>
											<mrow>
													\amp = \frac{2}{4!} \ilap{\frac{4!}{(s+7)^5}}
											</mrow>
											<mrow>
												\amp = \frac{1}{12} t^4 e^{-7t}
										</mrow>
										</md>
									</p>
								</solution>
							</p>
						</cell>
					</row>
				</tabular>
			</statement>
		</p>
	</exercise>

	<exercise><title> Step 3 Practice </title>

		<p>
			<statement>
				<p>
					Prepare each Laplace solution (step 3) for a backward transformation, then transform it back into a function of <m>t</m> (step 4).
				</p>
				<ol>
					<li>
						<p>
							<m>\ds Y(s) = \frac{11}{s^2 - 6s + 14}</m>
						</p>
					</li>

					<li>
						<p>
							<m>\ds Y(s) = \frac{s+3}{s^2 + 2s + 10}</m>
						</p>
					</li>

					<li>
						<p>
							<m>\ds P(s) = \frac{s}{s^2 - s + 6}</m>
						</p>
					</li>
				</ol>
			</statement>
		</p>

		<p>
			<solution>
				<p>
					The discriminant of the denominator <m>s^2 - 6s + 14</m> is:
					<me>b^2 - 4ac = (-6)^2 - 4(1)(14) = 36 - 56 = -20</me>,
					indicating that completing the square is necessary:
					<md>
						<mrow> s^2 - 6s + 14 = (s^2 - 6s) + 14  =\amp (\ob{s^2 - 6s + 9}^{(s - 3)^2} - 9) + 14  </mrow>
						<mrow>								  =\amp (s - 3)^2 + 5							 </mrow>
					</md>.
					Rewriting <m>K(s)</m> as:
					<me>
						\frac{11}{s^2 - 6s + 14}
							= \ub{\frac{11}{(s - 3)^2 + 5}}_{\large \text{Match with } L_7}
							= \frac{11}{\sqrt{5}}\ub{\frac{\sqrt{5}}{(s - 3)^2 + 5}}_{\large <xref ref="L7" text="custom"><m>L_7</m></xref> (a = 3, b = \sqrt{5})}
					</me>.
					Therefore,
					<md>
						<mrow>
							k(t) = \ilap{K(s)} \amp = \frac{11}{\sqrt{5}}e^{3t}\sin(\sqrt{5}t)
						</mrow>
					</md>.
				</p>
			</solution>
	
			<solution>
				<p>
					Completing the square for the denominator of <m>P(s)</m> gives:
					<me>
						\frac{s+3}{s^2 + 2s + 10} = \frac{s+3}{(s + 1)^2 + 9}
					</me>.
					However, the numerator <m>s + 3</m> does not match <m>s + 1</m>. To resolve this, we rewrite <m>3</m> as <m>1 + 2</m> and group terms:
					<md>
						<mrow>
							\frac{s+3}{s^2 + 2s + 10}
								\amp = \frac{s + 1 + 2}{(s + 1)^2 + 9}
						</mrow>
						<mrow>
								\amp = \frac{s+1}{(s + 1)^2 + 9} + \frac{2}{(s + 1)^2 + 9}
						</mrow>
						<mrow>
								\amp = \ub{\frac{s+1}{(s + 1)^2 + 9}}_{\large <xref ref="L8" text="title"/>\ (a=-1, b=3)}
									+ \frac{2}{3}\ub{\frac{3}{(s + 1)^2 + 9}}_{\large <xref ref="L7" text="title"/>\ (a=-1, b=3)}
						</mrow>	
					</md>,
					Now, apply the inverse Laplace transform:
					<md>
						<mrow>
							p(t) \amp = \ilap{P(s)}
						</mrow>
						<mrow>
								\amp = \ilap{ \frac{s+1}{(s + 1)^2 + 9} } + \frac{2}{3}\ilap{ \frac{3}{(s + 1)^2 + 9} }
						</mrow>
						<mrow>
								\amp = e^{-t}\cos(3t) + \frac{2}{3}e^{-t}\sin(3t)
						</mrow>	
					</md>
				</p>
			</solution>
	
			<solution>
				<p>
					First, factor the quadratic denominator:
					<me>s^2 - s - 6 = (s + 2)(s - 3).</me>
					Now decompose <m>P(s)</m> into partial fractions:
					<me>\frac{s}{(s + 2)(s - 3)} = \frac{A}{s + 2} + \frac{B}{s - 3}.</me>
					Multiply both sides by <m>(s + 2)(s - 3)</m>,
					<me>s = A(s - 3) + B(s + 2).</me>
					and solve for <m>A</m> and <m>B</m> by selecting convenient values for <m>s</m>:
					<sidebyside widths="8% 80%">
						<p>
							<md>
								<mrow>s = -2: \amp</mrow>
								<mrow></mrow>
								<mrow>s = 3: \amp</mrow>
								<mrow></mrow>
							</md>
						</p>
						<p>
							<md>
								<mrow>-2 	\amp = A(-2 - 3) + B(-2 + 2)</mrow>
								<mrow>-2 	\amp = A(-5) + B(0) \quad\implies\quad A=2/5</mrow>
								<mrow>3 	\amp = A(3 - 3) + B(3 + 2)</mrow>
								<mrow>3 	\amp = A(0) + B(5) \quad\implies\quad B=3/5</mrow>
							</md>
						</p>
					</sidebyside>
					The partial fraction decomposition is:
					<me>\frac{s}{(s + 2)(s - 3)} = \frac{2/5}{s + 2} + \frac{3/5}{s - 3}.</me>
					Therefore:
					<me>\ilap{P(s)} = \frac25 e^{-2t} + \frac35 e^{3t}.</me>
				</p>
			</solution>
		</p>

	</exercise>

	<exercise><title> <m>\lap{(t - 2)\, u_2(t)}</m> </title>
		<p>
			<statement>
				<p>
					Compute the Laplace transform of the piecewise function
					<me>
						h(t) = \left\{
						\begin{array}{ll}
							0, &amp; t \lt 2\\
							t - 2, &amp; t \ge 2
						\end{array}
						\right.
					</me>
				</p>
			</statement>
		</p>
		<solution><title> <m>\rightarrow \lap{h(t)}</m> </title>
			<p>
				Since this piecewise function is of the form
				<me>
					h(t) = \left(t - 2\right)\cdot
					\left\{
						\begin{array}{ll}
							0, &amp; t \lt 2\\
							1, &amp; t \ge 2
						\end{array}
					\right.
					\quad = \left(t - 2\right)\cdot u_2(t)
				</me>.
			</p>
			<p>
				To compute <m>\lap{h(t)}</m> using the <xref ref="laplace-f-uc" text="custom">transform rule</xref> with <m>c=2</m>, we first label <m>f(t)</m>: 
			</p>
			<me>
				\lap{h(t)} = 
				\laplacesym \big\{{\BO \us{f(t)}{\us{\uparrow}{(t - 2)}}}\, u_2(t)\big\} 
				= e^{-2s} \lap{{\BO f(t+2)}}
			</me>
			<p>
				Since <m>g(t) = t - 2</m>, then <m>f(t + 2) = (t+2) - 2 = t</m> and we have
				<me>
					\lap{h(t)} = e^{-2s} \lap{t} = e^{-2s} \cdot \frac{1}{s^2} = \frac{e^{-2s}}{s^2}
				</me>.
			</p>
		</solution>
	</exercise>

	<exercise><title> Laplace of a Delayed Polynomial Pulse </title>
		<statement>
		<p>
			Compute the Laplace transform of the function
			<me>
			m(t) =
			\left\{
				\begin{array}{ll}
				0,		\amp t \lt 1 \\
				t^2,	\amp 1 \le t \lt 3 \\
				0,		\amp t \ge 3
				\end{array}
			\right.
			</me>
		</p>
		</statement>
		<solution><title> <m>\rightarrow \lap{m(t)}</m> </title>
			
			<p>
				We can rewrite this function as
				<me>
					m(t) = t^2 \cdot
					\left\{
						\begin{array}{ll}
							0,	\amp t \lt 1\\
							1,	\amp 1 \le t \lt 3\\
							0,	\amp t \ge 3
						\end{array}
					\right.
					\quad = t^2 \cdot [u_1(t) - u_3(t)]
				</me>.
			</p>

			<p>
				Now we compute
			</p>

			<sidebyside widths="68% 32%" valign="top">
				<p>
					<md>
						<mrow>
							\laplacesym\amp \big\{m(t)\big\}
							= \laplacesym \big\{{\BO \us{f(t)}{\us{\uparrow}{\ul{t^2}}}}\, u_1(t)\big\} 
							- \laplacesym \big\{{\BO \us{f(t)}{\us{\uparrow}{\ul{t^2}}}}\, u_3(t)\big\}
						</mrow>
						<mrow>
							\amp
							= e^{-s} \lap{{\BO f(t+1)}} - e^{-3s} \lap{{\BO f(t+3)}}
						</mrow>
						<mrow>
							\amp
							= e^{-s} \lap{{\BO t^2 + 2t + 1}} - e^{-3s} \lap{{\BO t^2 + 6t + 9}}
						</mrow>
					</md>
				</p>
				<p>
					<md>
						<mrow>
							\BO f(t+1)\
							\amp\BO = (t+1)^2
						</mrow>
						<mrow>
							\amp\BO = t^2 + 2t + 1
						</mrow>
						<mrow>
							\BO f(t+3)\
							\amp\BO = (t+3)^2
						</mrow>
						<mrow>
							\amp\BO = t^2 + 6t + 9
						</mrow>
					</md>
				</p>
			</sidebyside>
			Computing each of the common Laplace transforms, we get
			<me>
				\lap{m(t)}
				= e^{-s}\left(\frac{6}{s^4} + \frac{4}{s^3} + \frac{1}{s^2}\right) 
				- e^{-3s}\left(\frac{6}{s^4} + \frac{12}{s^3} + \frac{9}{s^2}\right)
			</me>
			
		</solution>
	</exercise>

	<exercise><title> Turning a Function <em>off</em> at <m>t = 1</m> </title>
		<p>
			<statement>
				<p>
					Rewrite the piecewise function
					<me>
						f(t) = \left\{
						\begin{array}{ll}
							2e^{-\sfrac{t^2}{2}},	&amp; t \lt 1\\
							0,			&amp; t \ge 1
						\end{array} \right.
					</me>
					as the product of <m>2e^{-\sfrac{t^2}{2}}</m> and a unit step function.
				</p>
			</statement>
		</p>

		<solution>
			<p>
				The function is initially <m>2e^{-\sfrac{t^2}{2}}</m> and then becomes <m>0</m> at <m>t=1</m>. So the piecewise function, <m>f(t)</m>, is equivalent to
				<md>
					<mrow>
						f(t) \amp = \left\{
							\begin{array}{ll}
								2e^{-\sfrac{t^2}{2}},	&amp; t \lt 1\\
								0,						&amp; t \ge 1
							\end{array} 
						\right.
					</mrow>
					<mrow/>
					<mrow>
						\amp = 2e^{-\sfrac{t^2}{2}} \cdot {\color{BurntOrange}\ub{
						\left\{
							\begin{array}{ll}
								1,	&amp; t \lt 1\\
								0,	&amp; t \ge 1
							\end{array} 
						\right.}_{\large 1 - u_{1}(t)}}
					</mrow>
				</md>
				and therefore, the piecewise function, <m>f(t)</m>, can be written as
				<me>
					f(t) = 2e^{-\sfrac{t^2}{2}} \cdot (1 - u_{1}(t))
				</me>,
				and has the following graph
			</p>

			<p>
				<sidebyside width="80%" margins="10%">
					<figure xml:id="tsqrd-on-then-off-at-neg10"><caption> Graph of <m>2e^{-\sfrac{t^2}{2}} \cdot u_{1}(t)</m> </caption>
						<image>
							<latex-image>
								\begin{tikzpicture}[domain=-3:3, samples=200, scale=0.7]
		
									% === Piecewise Function with 2 Parts ===

									% === colors ===
									\def\ofColor{blue}				\def\ofFill{\ofColor!15}
									\def\onColor{green!60!black}	\def\onFill{\onColor!15}

									% === figure/domain/tick bounds ===
									\def\tmin{-3.8}	\def\tmax{3.8}
									\def\ymin{-1.3}	\def\ymax{2.8}

									\def\a{\tmin}	\def\b{\tmax}
									
									\def\tticks{
										-2 / $-2$,
										-1 / $-1$,
										1  / $1$,
										2  / $2$,
									}
									\def\yticks{
										-1 / $-1$,
										1  / $1$,
									}
								
									% === Transistions ===
									\def\c{1}
									\fill[\ofFill]				(\tmin	, \ymin) rectangle (\c		, \ymax);
									\fill[\onFill]				(\c		, \ymin) rectangle (\tmax	, \ymax);
									\draw[very thin, dashed]	(\c		, \ymin) 		-- (\c		, \ymax);
									\node[font=\small, below] at ({\c}, -0.1) {$c$};
								
									% === Function definitions ===
									\newcommand{\f}[1]{2*exp(-(0.5*#1*#1))}	\def\ftex{2e^{-\sfrac{t^2}{2}}}
									\newcommand{\uL}[1]{0}	\def\uLtex{0}
									\newcommand{\uR}[1]{1}	\def\uRtex{1}
								
									% === Axes ===
									\draw[-&gt;] (\tmin, 0) -- (\tmax, 0);
									\draw[-&gt;] (0, \ymin) -- (0, \ymax);
									\node[font=\scriptsize, below] at (\tmax - 0.1 , 0) {$t$};
									
									% === Tick marks and labels ===
									\foreach \t /\n in \tticks {
										\draw[gray, shift={(\t,0)}] (0pt,2pt) -- (0pt,-2pt) node[black, below, font=\scriptsize] {\n};
									}

									\foreach \t /\n in \yticks {
										\draw[gray, shift={(0,\t)}] (2pt,0pt) -- (-2pt,0pt) node[black, left, font=\scriptsize] {\n};
									}

									% === Function plots on [a, c] ===
									\draw[\onColor, thin, dashed]	plot[domain=\a:\c, variable=\t]	(\t, {1-\uL{\t}});
									\draw[\onColor, very thick]		plot[domain=\a:\c, variable=\t]	(\t, {\f{\t}});
									
									% === Function plots on [c, b] ===
									\draw[\ofColor!50, thin, dashed]	plot[domain=\c:\b, variable=\t]			(\t, {\f{\t}});
									\draw[\ofColor, very thick]			plot[domain=\c+0.06:\b, variable=\t]	(\t, {1-\uR{\t}});

									% === Points at t=c ===
									\draw[\ofColor, very thick]	(\c,{1-\uR{\c}})	circle[radius=3pt];
									\fill[\onColor]					(\c,{\f{\c}})	circle[radius=3pt];

									% === Function Labels ===
									\node[\onColor, font=\scriptsize, above] at ({(\tmin + \c)/2-1}, 1)	{$1-u(t) = 1$};
									\node[\ofColor, font=\scriptsize, above] at ({(\c + \tmax)/2}, 0)		{$1-u(t) = 0$};
									\node[\onColor, font=\scriptsize, above] at ({(\tmin + \c)/2}, \ymin)	{$\text{``off''}$};
									\node[\ofColor, font=\scriptsize, above] at ({(\c + \tmax)/2}, \ymin)	{$\text{``on''}$};
									\node[font=\small, above] at ({(\c + \tmax)/2}, 1)		{$\ftex\cdot\color{\ofColor}{0}$};
									\node[font=\small, below] at ({(\tmin + \c)/2}, \ymax)	{$\ftex\cdot\color{\onColor}{1}$};
								\end{tikzpicture}
							</latex-image>
						</image>
					</figure>
				</sidebyside>
			</p>
		</solution>
	</exercise>

	<example><title> Let <m>U(t)</m> be the unit step function and <m> f(t) = t^2-2 </m>. Then compute the following values </title>

		<solution><title> <m>U(2.7)</m> </title>
			<p>
				Since <m>t = 2.7 \ge 0</m> (positive),
				<me>
					U(2.7) = 1
				</me>.
			</p>
		</solution>

		<solution><title> <m>U(-5.32)</m> </title>

			<p>
				Since <m>-5.32 &lt; 0</m> (negative),
				<me>
					U(-5.32) = 0
				</me>.
			</p>
		
		</solution>

		<solution><title> <m>U(2)\cdot f(2)</m> </title>

			<p>
				<me>
					U(2)\cdot f(2) = 1\cdot f(2) = (2)^2 - 2 = (4 - 2) = 2
				</me>.
			</p>

		</solution>

		<solution><title> <m>U(-3)\cdot f(-3)</m> </title>

			<p>
				<me>
					U(-3)\cdot f(-3) = 0\cdot ((-3)^2 - 2) = 0\cdot (9 - 2) = 0
				</me>.
			</p>

		</solution>

		<solution><title> <m>U(k)\cdot f(k)</m>, where <m>k \ge 0</m> </title>

			<p>
				Since <m>k \ge 0,</m> we know that <m>U(k) = 1,</m> so
				<me>
					U(k)\cdot f(k) = 1\cdot f(k) = k^2 - 2
				</me>.
			</p>

		</solution>

		<solution><title> <m>U(k)\cdot f(k)</m>, where <m>k &lt; 0</m> </title>

			<p>
				Since <m>k \lt 0,</m> we know that <m>U(k) = 0,</m> so
				<me>
					U(k)\cdot f(k) = 0\cdot f(k) = 0
				</me>.
			</p>

		</solution>

	</example>

	<example>
		<p>
			Consider the function <m>f(t) = U(t-3)</m> and complete the following:
			<ol>
				<li>evaluate <m>f(2)</m>.</li>
				<li>evaluate	<m>f(7.43)</m>.</li>
				<li>evaluate	<m>f(-1)</m>.</li>
				<li>evaluate <m>f(k),</m> where <m>k \gt 3</m>.</li>
				<li>evaluate	<m>f(k),</m> where <m>k \lt 3</m>.</li>
				<li>Sketch <m>f(t).</m></li>
				<li>Write <m>f(t)</m> as a piecewise defined function.</li>
			</ol>
		</p>
		
		<p/>
		<solution>
			<p>
				<ol>
					<li>
						Notice that <m>f(2) = U(2-3) = U(-1)</m>.	Since the input to the unit step function is	negative, we have <m>f(2) = 0.</m>
					</li>
					<li>
						Similar to the previous question, <m>f(7.43) = U(7.43-3) = U(4.43)</m>.	In this case, the input to the unit step function is positive, so we have <m>f(7.43) = 1.</m>
					</li>
					<li>
						As in the previous two questions, we evaluate <m>f(-1)</m> as follows.
						<me>
							f(-1) = U(-1 - 3) = U(-4) = 0
						</me>
					</li>
					<li>
						Suppose <m>k \gt 3.</m> If we substitute <m>k</m> into the function <m>f</m>, we have <m>f(k) = U(k-3).</m>	In order to evaluate this, we need to know if the input to the unit step function, <m>k - 3</m>, is positive or negative.	Since <m>k \gt 3,</m> we know that <m>k - 3</m> is positive, and therefore
						<me>
							f(k) = U(k-3) = 1
						</me>.
					</li>
					<li>
						Suppose now that <m>k \lt 3.</m> If we substitute <m>k</m> into the function <m>f</m>, we have <m>f(k) = U(k-3).</m>	Since <m>k \lt 3,</m> we know that the input to the unit step function, <m>k - 3</m>, is negative, and therefore
						<me>
							f(k) = U(k-3) = 0
						</me>.
					</li>
					<li>
						<sidebyside widths="90%" margins="auto" valign="middle">
							<image source="figures/soln_fig2.png" />
						</sidebyside>
						<image xml:id="unit-step-t-minus-3-plot" width="60%">
							<sageplot>
								U = plot(0, (x, -2, 2.9), color='blue', thickness=4, ymin=-1, ymax=1.5, fontsize=20, ticks=[1,1])
								U += plot(1, (x, 3, 5), color='blue', thickness=4, ymin=-1, ymax=1.5, fontsize=20, ticks=[1,1])
								U += point([3,0], color = "blue", faceted=True, size = 80)
								U += point([3,0], color = "white", faceted=True, size = 15)
								U += point([3,1], color = "blue", faceted=True, size = 80)
								U
							</sageplot>
						</image>
					</li>
					<li>
						<me>
							f(t) =	\left\{
							\begin{array}{ll}
								0,	\amp t \lt 3\\
								1,	\amp t \ge 3.
							\end{array} \right.
						</me>
					</li>
				</ol>
			</p>
		</solution>
	</example>

	<example><title>Forcing with a Step Function</title>
		<p>
			<statement>
				<p>
					Solve the initial value problem using the Laplace transform:
				</p>
				<me>
					y'' + 4y = u_3(t), \quad y(0) = 0,\quad y'(0) = 0
				</me>
			</statement>
		</p>

		<solution>
			<p>
				<theorem xml:id="lt-roadmap-example-4"><title> Roadmap-Summary </title>
					<p>
						<sidebyside widths="30% 12% 58%" valign="middle">
							<p>
								<md>
									<mrow>	y'' + 4y = u_3(t)	</mrow>
									<mrow>	\small y(0) = 0,\ y'(0) = 0	</mrow>
								</md>
							</p>
							<p><me>\os{\Large\text{1️⃣}}{\us{\large\text{forward}}{\os{\large\laplacesym}{\longrightarrow}}}</me></p>
							<p>
								<me>
									s^2Y + 4Y = \frac{e^{-3s}}{s}
								</me>
							</p>
						</sidebyside>
						<sidebyside widths="60% 10% 30%" valign="middle">
							<p/>
							<p><me>\downarrow</me></p>
							<p>
								2️⃣ Solve for <m>Y</m>
							</p>
						</sidebyside>
					</p>
					<p>
						<sidebyside widths="40% 10% 50%" valign="middle">
							<p/>
							<p/>
							<p>
								<me>
									Y(s) = \frac{e^{-3s}}{s(s^2 + 4)}
								</me>
							</p>
						</sidebyside>
					</p>
					<p>
						<sidebyside widths="60% 10% 30%" valign="middle">
							<p/>
							<p><me>\downarrow</me></p>
							<p>
								3️⃣ Prepare for <m>\laplacesym^{-1}</m>
							</p>
						</sidebyside>
						<sidebyside widths="38% 12% 50%" valign="middle">
							<p>
								<me>
									y(t) = u_3(t)\left(1 - \cos(2(t - 3))\right)
								</me>
							</p>
							<p><me>\os{\Large\text{4️⃣}}{\us{\large\text{backward}}{\os{\large\laplacesym^{-1}}{\longleftarrow}}}</me></p>
							<p>
								<me>
									Y(s) = \frac{e^{-3s}}{s(s^2 + 4)}
								</me>
							</p>
						</sidebyside>
					</p>
				</theorem>
			</p>

			<p><term>Step 1: Apply the Laplace Transform</term>.</p>
			<p>
				<sidebyside widths="83% 17%" valign="bottom">
					<p>
						<md>
							<mrow>
								\lap{y'' + 4y} = \lap{u_3(t)}
							</mrow>
							<mrow>
								s^2Y + 4Y \amp = \frac{e^{-3s}}{s}
							</mrow>
						</md>
					</p>
					<p>
						<md>
							<mrow>				\amp\text{ Laplace}	</mrow>
							<mrow>	\leftarrow	\amp\text{ Equation}	</mrow>
						</md>
					</p>
				</sidebyside>
			</p>

			<p><term>Step 2: Solve for <m>Y(s)</m></term>.</p>
			<p>
				<sidebyside widths="15% 50% 35%" valign="bottom">
					<p/>
					<p>
						<md>
							<mrow>	(s^2 + 4)Y	\amp = \frac{e^{-3s}}{s}	</mrow>
							<mrow>	Y(s)		\amp = \frac{e^{-3s}}{s(s^2 + 4)}	</mrow>
						</md>
					</p>
					<p>
						<md>
							<mrow>	\leftarrow\text{ Laplace Solution}\vphantom{\frac12}	</mrow>
						</md>
					</p>
				</sidebyside>
			</p>

			<p><term>Step 3: Prepare for the Inverse Transform</term>.</p>
			<p>
				The exponential factor <m>e^{-3s}</m> indicates a delay. Focus on the base transform:
				<me>
					\frac{1}{s(s^2 + 4)}
				</me>
				<p>
					From the table, this matches the transform of <m>1 - \cos(2t)</m>. Therefore:
				</p>
				<me>
					\ilap{ \frac{1}{s(s^2 + 4)} } = 1 - \cos(2t)
				</me>
				<p>
					The delay is applied using the shift theorem.
				</p>
			</p>

			<p><term>Step 4: Take the Inverse Transform</term>.</p>
			<p>
				<md>
					<mrow>
						y(t) = \ilap{ \frac{e^{-3s}}{s(s^2 + 4)} } = u_3(t)\left[1 - \cos(2(t - 3))\right]
					</mrow>
				</md>
			</p>

			<p>
				Therefore, the solution is:
				<me>
					y(t) = u_3(t)\left(1 - \cos(2(t - 3))\right)
				</me>
			</p>
		</solution>
	</example>

	<example><title> Sketch the function <m>p(t) = -2\ U(t-2)</m> </title>
		<solution><title> Sketch <m>p(t)</m> </title>
			<p>
				Since <m>U(t-2)</m> is <m>U(t)</m> shifted to the right by <m>2</m>, the jump in the graph occurs at <m>t=2</m> (see below). Additionally, multiplying by <m>-2</m> reflects the graph about the <m>x</m>-axis and scales it by <m>2</m>, as shown below.
			</p>

			<sidebyside width="75%">
					<image width="100%">
						<latex-image>
							\begin{tikzpicture}

								\def\tmin{-1}
								\def\t1{2}
								\def\tmax{5}

								% Axis, Ticks and labels
								\draw[-&gt;] (\tmin, 0) -- (\tmax, 0) node[anchor=north] {$t$};
								\draw[-&gt;] (0, -2.6) -- (0, 1.6) node[anchor=east] {$g(t)$};
								\node at (-0.2, 1) {$1$};
								\draw[shift={(0,1)},color=black] (2pt,0pt) -- (-2pt,0pt);
								\node at (-0.3, -2) {$-2$};
								\draw[shift={(0,-2)},color=black] (2pt,0pt) -- (-2pt,0pt);
								\node[anchor=north] at (\t1, 0) {$2$};
								\draw[shift={(\t1,0)},color=black] (0pt,2pt) -- (0pt,-2pt);
								
								% Function plot
								\draw[thick, blue] (\tmin, 0) -- (\t1, 0);
								\draw[thick, blue] (\t1, -2) -- (\tmax, -2);
								\draw[thick, black!60!green, opacity=0.3] (\t1, 1) -- (\tmax, 1);

								% Dots and labels
								\filldraw[black!60!green, opacity=0.8] (\t1, 1) circle (2pt) node[anchor=south west] {$U(t-2)$};
								\filldraw[blue] (\t1, -2) circle (2pt) node[anchor=south west] {$-2U(t-2)$};
								\draw[dashed, opacity=0.2] (\t1, 1) -- (\t1, -2);
								

							\end{tikzpicture}
						</latex-image>
					</image>
			</sidebyside>
		</solution>
	</example>
</exercises>