<subsection xmlns:xi="http://www.w3.org/2001/XInclude"><title> Integrating Factor Method </title>

	<p>
		The integrating factor method uses a three-step strategy to solve first-order linear differential equations in the <em>standard form</em>:
		<fn>
			<p>
				Every linear differential equation looks like
				<me> 
					a_n(x)y^{(n)} + \cdots + a_2(x)y'' + a_1(x)y' + a_0(x)y = f(x)
				</me>.
				The first-order version of this is
				<me> 
					a_1(x)y' + a_0(x)y = f(x)
				</me>,
				but we can divide both sides of this equation by <m>a_1(x)</m>:
				<me>
					y' + \us{P(x)}{\ub{\frac{a_0(x)}{a_1(x)}}}y = \us{Q(x)}{\ub{\frac{f(x)}{a_1(x)}}}
				</me>.
				Since every first-order linear differential equation can always be written as
				<me> 
					y' + P(x)y = Q(x) 
				</me>,
				we call this the first-order linear <em>standard form</em>.
			</p>
		</fn>
		<men xml:id="if-standard-form"> 
			y' + P(x)y = Q(x)
		</men>.
		The heart of this method is the first step: finding the correct integrating factor. The second step uses this factor to write the left side as a single derivative. Finally, the last step finds the solution by <xref ref="direct-integration" text="custom">direct integration</xref>.
	</p>

	<paragraphs><title> Step 1: Finding the Integrating Factor </title>
	
		<p>
			Understanding how to find the integrating factor is crucial. Let's carefully walk through this important process.
		</p>
		<p>
			Consider the differential equations (specific on the left, general on the right):
			<sidebyside>
				<p>
					<me> 
						\us{\text{product rule?}}{\ub{y' + x^2 y}} = 5x^2 
					</me>,
				</p>
				<p>
					<me> 
						\us{\text{product rule?}}{\ub{y' + P(x)y}} = Q(x) 
					</me>.
				</p>
			</sidebyside>
			We would like to rewrite the left side as a single derivative using the <xref ref="if-product-rule" text="custom">backward product rule</xref>. However, the <m>y'</m> alone suggests there is a missing second function that the product rule needs. Maybe there is a function that we can multiply both sides of the equation by to get the desired product rule. Let's call it <m>\mu</m> for now and see if we can find it. We start by multiplying both sides by <m>\mu</m>:
			<sidebyside>
				<p>
					<me> 
						\mu y' + 3x^2 \mu y = 5x^2\mu 
					</me>.
				</p>
				<p>
					<me> 
						\mu y' + P(x)\mu y = Q(x)\mu 
					</me>.
				</p>
			</sidebyside>

			Notice that the left side almost looks like the product rule <m>\left[ \mu y \right]' = \mu y' + \mu' y</m>, except for the boxed value where <m>\mu'</m> should be (see below).

			<sidebyside>
				<p>
					<me> 
						\overset{\ds \mu}	{\overset{\downarrow}{\vphantom{\Big[}\ds \mu}} 	\cdot 
						\overset{\ds y'}	{\overset{\downarrow}{\vphantom{\Big[}\ds y'}} 		+ 
						\overset{\ds \color{blue}{\mu'}}	{\overset{\downarrow}{\vphantom{\Big[}\ds \color{blue}{\fbox{\(3x^2 \mu\)}}}}	\cdot 
						\overset{\ds y}		{\overset{\downarrow}{\vphantom{\Big[}\ds y}} 		= 
						5x^2\mu 
					</me>,
				</p>
				<p>
					<me> 
						\overset{\ds \mu}	{\overset{\downarrow}{\vphantom{\Big[}\ds \mu}} 	\cdot 
						\overset{\ds y'}	{\overset{\downarrow}{\vphantom{\Big[}\ds y'}} 		+ 
						\overset{\ds \color{blue}{\mu'}}	{\overset{\downarrow}{\vphantom{\Big[}\ds \color{blue}{\fbox{\(P(x) \mu\)}}}}	\cdot 
						\overset{\ds y}		{\overset{\downarrow}{\vphantom{\Big[}\ds y}} 		= 
						Q(x)\mu 
					</me>.
				</p>
			</sidebyside>

			This shows that the <m>\mu</m> that works is the one that satisfies
			<sidebyside>
				<p>
					<me> 
						\mu' = 3x^2 \mu
					</me>
				</p>
				<p>
					<me> 
						\mu' = P(x) \mu
					</me>.
				</p>
			</sidebyside>

			Careful inspection shows that these are separable differential equations where the unknown <m>\mu</m> can be found using separation of variables!

			<sidebyside>
				<p>
					<md>
						<mrow>	\int \frac{1}{\mu}d\mu	\amp = \int 3x^2\ dx										</mrow>
						<mrow>				\ln|\mu|	\amp = x^3 + C												</mrow>
						<mrow>						\mu	\amp = \pm e^{x^3 + C}										</mrow>
						<mrow>						\mu	\amp = {\color{green} \us{C}{\fbox{\(\pm e^C\)}}} e^{x^3}	</mrow>
						<mrow>						\mu	\amp = Ce^{x^3}												</mrow>
					</md>
				</p>
				<p>
					<md>
						<mrow>	\int \frac{1}{\mu}d\mu	\amp = \int P(x)\ dx	</mrow>
						<mrow>				\ln|\mu|	\amp = \int P(x)\ dx		</mrow>
						<mrow>						\mu	\amp = e^{\int P(x)\ dx}	</mrow>
					</md>
				</p>
			</sidebyside>

			Although the solution conatains a constant, we only need one function that works, so we set <m>C = 1</m>. The function <m>\mu</m> is called the <em>integrating factor</em> and finding it is the first step toward solving a first order differential equation.
		</p>

		<assemblage xml:id="integrating-factor"><title> The Integrating Factor </title>
			<p>
				The <term>integrating factor</term> for the first-order linear differential equation
			</p>
			<p>
				<me> y' + P(x)y = Q(x) </me>
				is given by	<m>\ds \mu = e^{\int P(x)\ dx} </m> and represents the function, when multiplied onto both sides of the equation, needed to write the left side as a derivative.
			</p>
		</assemblage>
	</paragraphs>

	<paragraphs><title> Step 2: Rewriting the Equation </title>
	
		With the integrating factor in hand, we are ready to write the left side as a derivative using the <xref ref="if-product-rule" text="custom">backward product rule</xref>.
		<sidebyside>
			<p>
				Integrating Factor: <m>\mu = e^{x^3}</m>
				<md>
					<mrow>					y' + x^2 y	=\ \amp 5x^2		</mrow>
					<mrow>	e^{x^3}y' + x^2 e^{x^3}y	=\ \amp 5x^2e^{x^3}	</mrow>
					<mrow>	\left[ e^{x^3}y \right]'	=\ \amp 5x^2e^{x^3}	</mrow>
				</md>
			</p>
			<p>
				Integrating Factor: <m>\mu = e^{\int P(x)\ dx}</m>
				<md>
					<mrow>				y' + P(x)y	=\ \amp Q(x)		</mrow>
					<mrow>		\mu y' + P(x) \mu y	=\ \amp Q(x) \mu	</mrow>
					<mrow>	\left[ \mu y \right]'	=\ \amp Q(x) \mu	</mrow>
				</md>.
			</p>
		</sidebyside>
	</paragraphs>

	<paragraphs><title> Step 3: Solving the Equation </title>
	
		<p>
			The final step is to apply <xref ref="direct-integration" text="custom">direct integration</xref>. This was covered in a previous section, so we will skip some of the details here.
		</p>

		<sidebyside widths="50% 38%">
			<p>
				<md>
					<mrow>	\int \left[ e^{x^3}y \right]' \ dx	=\ \amp \int 5x^2e^{x^3} \ dx	</mrow>
					<mrow>							e^{x^3}y	=\ \amp \frac{5}{3} e^{x^3} + C	</mrow>
					<mrow>									y	=\ \amp \frac{5}{3} + Ce^{-x^3}	</mrow>
				</md>
			</p>
			<p>
				<md>
					<mrow>	\int \left[ \mu y \right]' \ dx	=\ \amp \int Q(x) \mu \ dx					</mrow>
					<mrow>							\mu y	=\ \amp \int Q(x) \mu \ dx					</mrow>
					<mrow>								y	=\ \amp \frac{1}{\mu} \int Q(x) \mu \ dx	</mrow>
				</md>
				where <m>\mu = e^{\int P(x)\ dx}</m>.
			</p>
		</sidebyside>

		<p>
			<assemblage xml:id="integrating-factor-general-solution"><title> General Solution </title>
				<p>
					The general solution for the first-order linear differential equation
				</p>
				<p>
					<me> 
						y' + P(x)y = Q(x) 
					</me>
					is given by	
					<me>
						y = \frac{1}{\mu} \int Q(x) \mu \ dx 
					</me> where <m>\mu = e^{\int P(x)\ dx}</m> is the integrating factor.
				</p>
			</assemblage>
		</p>
	</paragraphs>

	<p>
		In summary, the integrating factor method is a three-step process that utilizes the integrating factor to rewrite the left side of the equation, enabling direct integration and leading to the general solution.
	</p>

	<xi:include href="./c2-s3-ss3-interactives.ptx" />
	
</subsection>