<section xmlns:xi="http://www.w3.org/2001/XInclude"><title> Characteristic Equation </title>

	<p>
		The previous section showed us that solutions to LHCC equations involve <m>e^{rx}</m> terms. We will now build on this idea by showing that every LHCC equation is associated with another equation that allows us to find the specific <m>r</m>-values that give us our solutions. Let's explore this by looking at a few concrete examples, starting the equation
		<me>y' - 5y = 0</me>,
		Now, imagine we wanted verify that <m>y = e^{rx}</m> is a solution to this equation. To do this, we plug it into the equation and see if it leads to <m>0=0</m>. In this case, we get
		<md>
			<mrow>	\left[e^{rx}\right]' - 5 \left[e^{rx}\right] =\amp\ 0 </mrow>
			<mrow>	r e^{rx} - 5 e^{rx} =\amp\ 0 </mrow>
			<mrow>	\us{\text{must be 0}}{\ub{(r - 5) e^{rx}}} =\amp\ 0 </mrow>
		</md>,
		which shows that the left-side must also be <m>0</m>, but this only happens for specific <m>r</m>-values. To find them, we note that <m>e^{rx}</m> is never zero, and solve
		<md>
			<mrow>	(r - 5) e^{rx}	=\amp \ 0 \qquad (\text{divide by } e^{rx})</mrow>
			<mrow>			r - 5	=\amp \ 0 \quad \rightarrow \quad r = 5</mrow>
		</md>,
		showing that <m>e^{5x}</m> is a solution. 
	</p>

	<p>
		Now, let's consider a second order equation, say 
		<me>y'' - 5y' + 6y = 0</me>.
		Plugging <m>y = e^{rx}</m> into this equation, we have
		<md>
			<mrow>	\left[e^{rx}\right]'' - 5 \left[e^{rx}\right]' + 6 \left[e^{rx}\right] =\amp\ 0 </mrow>
			<mrow>	r^2 e^{rx} - 5 r e^{rx} + 6 e^{rx} =\amp\ 0 </mrow>
			<mrow>	(r^2 - 5r + 6) e^{rx} =\amp\ 0 </mrow>
		</md>
		Again, <m>e^{rx}</m> is never zero, so we must have <m>r^2 - 5r + 6 = 0</m>. Solving this quadratic equation gives <m>r = 2</m> and <m>r = 3</m>, yielding the solutions <m>e^{2x}</m> and <m>e^{3x}</m>.
	</p>
	
	<p>
		Regardless of the order, every LHCC equation can be approached in a similar way. To help us with the general equation, observe how each derivative of <m>e^{rx}</m> adds a multiple of <m>r</m> (by the chain rule). In particular,
		<me>
			y = e^{rx} \ \ \os{\text{chain rule}}{\rightarrow} \ \ 
			y' = re^{rx} \ \ \os{\text{chain rule}}{\rightarrow} \ \ 
			y'' = r^2e^{rx} \quad \os{\text{chain rule}}{\rightarrow \, \dots \, \rightarrow} \quad 
			y^{(n)} = r^ne^{rx}
		</me>.
		We are now ready to plug <m>y = e^{rx}</m> into the general <xref ref="lhcc-equation" text="custom">LHCC equation</xref>:
		<md>
			<mrow>	
				a_n\ \left[e^{rx}\right]^{(n)} + \cdots + a_2\ \left[e^{rx}\right]'' + a_1\ \left[e^{rx}\right]' + a_0\ e^{rx} =\amp\ 0 
			</mrow>
			<mrow>	a_n\ r^n e^{rx} + \cdots + a_2\ r^2 e^{rx} + a_1\ r e^{rx} + a_0\ e^{rx} =\amp\ 0 </mrow>
			<mrow>	\left(a_n\ r^n + \cdots + a_2\ r^2 + a_1\ r + a_0\right)e^{rx}  =\amp\ 0 </mrow>
		</md>.
		Following the same pattern as before, we get the <m>r</m>-values we need by solving
		<me>
			a_n\ r^n + \cdots + a_2\ r^2 + a_1\ r + a_0 = 0
		</me>.
		This polynomial equation that gives us the <m>r</m>-values we need to write down our solutions is referred to as the <em>characteristic equation</em>.
	</p>
	
	<definition xml:id="def-characteristic-equation"><title> <em>LHCC Characteristic Equation</em> </title>
	
		<statement>
			<p>
				The <term>characteristic equation</term> of a <xref ref="lhcc-equation" text="custom">linear homogeneous differential equations with constant coefficients</xref> is given by the <m>n</m>-th degree polynomial equation
			</p>
			<men xml:id="characteristic-equation"> 
				a_n\ r^n + \cdots + a_2\ r^2 + a_1\ r + a_0 = 0	
			</men>.
		</statement>
	</definition>

	<example>
		<p>
			Give the characteristic equation of the differential equation
			<me>
				y'' + 5y' - y = 0.
			</me>
		</p>

		<solution>
			<p>
				<me>
					r^2 + 5r - 1 = 0
				</me>
			</p>
		</solution>

	</example>

	
	<xi:include href="./p3-c1-s3-interactives.ptx" />	

</section>
