<!-- LICENSING
  This file is part of the textbook "Exploring Differential Equations, An Interactive, Student-Centered Approach" by Geoffrey Cox.
  License: Creative Commons Attribution-ShareAlike 4.0 International (CC BY-SA 4.0)
  You are free to:
    ‚Ä¢ Share ‚Äî copy and redistribute the material in any medium or format.
    ‚Ä¢ Adapt ‚Äî remix, transform, and build upon the material for any purpose, even commercially.
  Under the following terms:
    ‚Ä¢ Attribution ‚Äî You must give appropriate credit, provide a link to the license, and indicate if changes were made.
    ‚Ä¢ ShareAlike ‚Äî If you remix, transform, or build upon the material, you must distribute your contributions under the same license.
  Full license text: https://creativecommons.org/licenses/by-sa/4.0/legalcode
  Recommended attribution: "Exploring Differential Equations" by Geoffrey Cox, licensed CC BY-SA 4.0"
-->
<section xml:id="solving-linear-systems">
    <title>Solving Linear Systems</title>

    <introduction>
        <p>
            We've explored what linear systems are, how to visualize their behavior, and even how to write them neatly in vector form.  
            Now it's time to start <em>solving</em> them.  
        </p>
        <p>
            We'll begin with the classic trick that worked for single equations ‚Äî guessing exponential solutions ‚Äî then finish by showing how to approximate solutions step by step with a numerical method.
        </p>
    </introduction>

    <!-- ============================= -->
    <!-- SUBSECTION: Numerical Methods -->
    <!-- ============================= -->
    <subsection xml:id="numerical-methods">
        <title>Numerical Solutions for Linear Systems</title>

        <p>
            Not every system is easy to solve exactly.  
            Sometimes, you just want to <em>see</em> what the solution looks like ‚Äî or approximate it for a while.  
            That's where numerical methods shine.
        </p>

        <p>
            One of the simplest is <em>Euler's Method</em>, which you've seen for single equations.  
            We'll now apply it to systems.
        </p>

        <p>
            Suppose we have:
        </p>

        <md>
            <mrow>\frac{dx}{dt} \amp = x + y</mrow>
            <mrow>\frac{dy}{dt} \amp = -x + y</mrow>
        </md>

        <p>
            With initial conditions <m>x(0) = 1</m>, <m>y(0) = 0</m>, and a step size of <m>h = 0.1</m>.
        </p>

        <example xml:id="ex-euler-system">
            <title>Euler's Method for a System</title>
            <statement>
                <p>
                    Use Euler's method to take two steps for the system above.
                </p>
            </statement>
            <solution>
                <p>
                    <term>Step 1:</term> At <m>t = 0</m>, we have <m>x_0 = 1</m>, <m>y_0 = 0</m>.  
                    The derivatives are <m>x' = 1 + 0 = 1</m>, <m>y' = -1 + 0 = -1</m>.
                </p>

                <p>
                    Update:
                </p>

                <me>
                    x_1 = 1 + 0.1(1) = 1.1, \qquad y_1 = 0 + 0.1(-1) = -0.1.
                </me>

                <p>
                    <term>Step 2:</term> At <m>t = 0.1</m>, we have <m>x_1 = 1.1</m>, <m>y_1 = -0.1</m>.  
                    Now <m>x' = 1.1 + (-0.1) = 1.0</m>, <m>y' = -1.1 + (-0.1) = -1.2</m>.
                </p>

                <p>
                    Update again:
                </p>

                <me>
                    x_2 = 1.1 + 0.1(1.0) = 1.2, \qquad y_2 = -0.1 + 0.1(-1.2) = -0.22.
                </me>

                <p>
                    We now have approximate values after two steps:
                </p>

                <me>
                    (x(0.2), y(0.2)) \approx (1.2, -0.22).
                </me>

                <p>
                    Each step shows how <m>x</m> and <m>y</m> <q>talk</q> to each other as time progresses.
                </p>
            </solution>
        </example>

        <p>
            Euler's Method may be simple, but it makes the <em>flow of information</em> between variables visible:  
            each update for <m>x</m> affects <m>y</m> on the next step, and vice versa.
        </p>

    </subsection>

	<assemblage label="solving-linear-systems-wrap-up">
		<title>üì§ Wrap-Up</title>
		<p>
			<paragraphs label="solving-linear-systems-takeaways">
				<title>üóùÔ∏è Key Takeaways..</title>
				<ul marker="square">
                    <li>Euler's Method updates each variable using its derivative at the current step.</li>
                    <li>For systems, each update can feed into the next ‚Äî showing the back-and-forth between variables.</li>
                    <li>Numerical methods are essential for understanding systems that can't be solved exactly.</li>
				</ul>
			</paragraphs>

			<paragraphs label="solving-linear-systems-cyu">
				<title>Check Your Understanding</title>
                    <exercise xml:id="rq-numerical-methods">
                        <title>Numerical Methods for Systems</title>

                        <task label="rq-num-1">
                            <title>Euler's Method Thinking</title>
                            <statement>
                                <p>
                                    What does Euler's Method do when applied to a system of DEs?
                                </p>
                            </statement>
                            <choices randomize="yes">
                                <choice correct="yes">
                                    <statement><p>It updates each variable step by step using its derivative at the current point.</p></statement>
                                </choice>
                                <choice correct="yes">
                                    <statement><p>It shows how the variables influence each other from one step to the next.</p></statement>
                                </choice>
                                <choice correct="no">
                                    <statement><p>It provides the exact solution in one step.</p></statement>
                                    <feedback><p>Euler's Method is an approximation technique, not an exact one-step solution.</p></feedback>
                                </choice>
                                <choice correct="no">
                                    <statement><p>It can only be used for uncoupled systems.</p></statement>
                                    <feedback><p>Euler's Method works for any system, coupled or not.</p></feedback>
                                </choice>
                            </choices>
                        </task>

                        <task label="rq-num-2">
                            <title>Interpreting Numerical Results</title>
                            <statement>
                                <p>
                                    When we use Euler's Method on a system, what do the computed points <m>(x_n, y_n)</m> represent?
                                </p>
                            </statement>
                            <choices randomize="yes">
                                <choice correct="yes">
                                    <statement><p>They are approximate values of the solution at specific time steps.</p></statement>
                                </choice>
                                <choice correct="no">
                                    <statement><p>They are exact values that replace the need for solving the system algebraically.</p></statement>
                                    <feedback><p>They're approximate ‚Äî we still use exact methods when possible.</p></feedback>
                                </choice>
                                <choice correct="no">
                                    <statement><p>They are estimates of the system's coefficients.</p></statement>
                                    <feedback><p>Euler's Method updates <m>x</m> and <m>y</m>, not the coefficients.</p></feedback>
                                </choice>
                            </choices>
                        </task>
                    </exercise>
			</paragraphs>
		</p>
	</assemblage>
	<!-- ================================================================ -->
	<!-- WRAP-UP + READING QUESTIONS                                      -->
	<!-- ================================================================ -->
	<subsection label="sov-method-wrap-up">
		<title>üì§ Wrap-Up</title>

		<assemblage label="sov-method-wrap-up-takeaways">
			<p>
				üóùÔ∏è <m>\textbf{Key Takeaways...}</m>
				<ul marker="square">
					<li></li>
				</ul>
			</p>
		</assemblage>
		<paragraphs label="sov-method-cyu">
			<title>Check Your Understanding</title>

			<exercise label="sov-method-cyu-bundle">
				<title><e component="emoji">ü§îüí≠</e> Separation of Variables Reading Questions</title>

				<task label="sov-method-cyu-1">
					<title><e component="emoji">ü§îüí≠</e> SOV and Nonlinear Equations</title>
					<statement correct="no">
						<p>
							The separation of variables method cannot be applied to non-linear differential equations.
						</p>
					</statement>
					<feedback>
						<p>
							Being able to solve non-linear differential equations is one of the strengths of the separation of variables method.
						</p>
					</feedback>
				</task>
				<task label="sov-method-cyu-2">
					<title><e component="emoji">ü§îüí≠</e> Sort the Steps in Order</title>

					<statement>
						<p>
							CONVERT TO PARSONS.. Suppose you want to use separation of variables method to determine the general solution of the differential equation
							<men xml:id="chkpt-sov-method-examples-1-eqn">
								\ds \frac{dq}{dt} - 3qt^2 = 2q
							</men>.
						</p>
						<p>
							Match the scrambled tasks (on the left) to the task order (on the right) that it should be performed to use this method.
						</p>
					</statement>
					<feedback>
						<p>
							Review the <xref ref="sov-method" text="custom">SOV Method</xref>.
						</p>
					</feedback>
					<cardsort>
						<match>
							<premise>
								<p>
									Equation is 1st-order ‚úÖ
								</p>
							</premise>
							
							<response>
								<p>
									<m>\text{Task 1}</m>
								</p>
							</response>
						</match>
						<match>
							<premise>
								<p>
									<m>\ds \frac{dq}{dt} = q(2 + 3t^2)</m>
								</p>
							</premise>
							<response>
								<p>
									<m>\text{Task 2}</m>
								</p>
							</response>
						</match>
						<match>
							<premise>
								<p>
									<m>\ds \frac{1}{q}\ dq = (2 + 3t^2)\ dt</m>
								</p>
							</premise>
							<response>
								<p>
									<m>\text{Task 3}</m>
								</p>
							</response>
						</match>
						<match>
							<premise>
								<p>
									<m>\ds \int \frac{1}{q} dq = \int (2 + 3t^2) dt</m>
								</p>
							</premise>
							
							<response>
								<p>
									<m>\text{Task 4}</m>
								</p>
							</response>
						</match>
						<match>
							<premise>
								<p>
									<line><m>\ds \ln|q| = 2t^2 + t^3 + c</m></line>
								</p>
							</premise>
							<response>
								<p>
									<m>\text{Task 5}</m>
								</p>	
							</response>
						</match>
						<match>
							<premise>
								<p>
									<line><m>\ds q = c e\vphantom{|}^{\large 2t^2 + t^3}</m></line>
								</p>
							</premise>
							<response>
								<p>
									<m>\text{Task 6}</m>
								</p>
							</response>
						</match>
					</cardsort>
				</task>
				<task label="sov-method-cyu-3">
					<title><e component="emoji">ü§îüí≠</e> Combining Constants</title>

					<statement>
						<p>
							Which of the following are valid ways to combine constants when finalizing your solution? Select ALL that apply.
						</p>
					</statement>
					<choices randomize="yes">
						<choice correct="yes">
							<statement>
								<m>
									\quad \left\{
									\begin{align}
										|y|	\amp = e^{2x + c_1}\\ 
										y	\amp = c_2 e^{2x} 
									\end{align}
									\right.\qquad
								</m> 
								where <m>c_2=\pm e^{c_1}</m>.
							</statement>
							<feedback>
								<p>
									Correct, since
									<md>
										<mrow>	|y|	\amp =,	e^{2x + c_1}										</mrow>
										<mrow>	y	\amp =,	\pm e^{2x + c_1}									</mrow>
										<mrow>	y	\amp =,	\pm e^{2x} \cdot e^{c_1}							</mrow>
										<mrow>	y	\amp =,	c_2 e^{2x}	\quad \text{where } c_2 = \pm e^{c_1}	</mrow>
									</md>
								</p>
							</feedback>
						</choice>
						<choice correct="yes">
							<statement>
								<m>
									\quad \left\{
									\begin{align}
										\frac{y^2}{2} \amp = \sin(x) + c_1\\ 
										y^2 \amp = 2\sin(x) + c_2 
									\end{align}
									\right.\qquad
								</m> 
								where <m>c_2 = 2c_1</m>.
							</statement>
							<feedback>
								<p>
									Correct, since
									<md>
										<mrow>	\frac{y^2}{2}	\amp =,	\sin(x) + c_1									</mrow>
										<mrow>	y^2				\amp =,	\sin(x) + 2c_1									</mrow>
										<mrow>	y^2				\amp =,	2\sin(x) + c_2	\quad \text{where } c_2 = 2c_1	</mrow>
									</md>
								</p>
							</feedback>
						</choice>
						<choice>
							<statement>
								<m>
									\quad \left\{
									\begin{align}
										y^2	\amp = 2\sin(x) + c_2\\ 
										y	\amp = \pm\sqrt{2\sin(x)} + c_3 
									\end{align}
									\right.\qquad
								</m> 
								where <m>c_3=\pm \sqrt{c_2}</m>.
							</statement>
							<feedback>
								<p>
									Incorrect, you should not combine constants here since <m>\quad\sqrt{A + B} \neq \sqrt{A} + \sqrt{B}</m>.
								</p>

								<p>
									Your solution should be written as
									<md>
										<mrow>	y^2	\amp =,	2\sin(x) + c_2											</mrow>
										<mrow>	y	\amp =,	\pm\sqrt{2\sin(x) + c_2}\quad \leftarrow\text{ done}	</mrow>
									</md>
								</p>
							</feedback>
						</choice>
						<choice>
							<statement>
								<m>
									\quad \left\{
									\begin{align}
										e^y	\amp =	3y + c_1\\ 
										y	\amp =	\ln(3y) + c_2 
									\end{align}
									\right.\qquad
								</m> 
								where <m>c_2= \ln(c_1)</m>.
							</statement>
							<feedback>
								
								<p>
									Incorrect, you should not combine constants here since <m>\ln(A + B) \neq \ln(A) + \ln(B)</m>.
								</p>

								<p>
									Your solution should be
									<md>
										<mrow>	e^y	\amp =,	3y + c_1									</mrow>
										<mrow>	y	\amp =,	\ln(3y + c_1)\quad \leftarrow\text{ done}	</mrow>
									</md>
								</p>
							</feedback>
						</choice>
						<choice>
							<statement>
								<m>
									\quad \left\{
									\begin{align}
										xy	\amp =	e^x + c_1\\ 
										y	\amp =	\frac{e^x}{x} + c_2 
									\end{align}
									\right.\qquad
								</m> 
								where <m>\ds c_2=\frac{c_1}{x}</m>.
							</statement>
							<feedback>
								<p>
									Incorrect, you should not combine constants here since <m>\frac{c_1}{x}</m> is not constant. Instead your solution should be left as
									<md>
										<mrow>	xy	\amp =,	e^x + c_1													</mrow>
										<mrow>	y	\amp =,	\frac{e^x + c_1}{x}											</mrow>
										<mrow>	y	\amp =,	\frac{e^x}{x} + \frac{c_1}{x}\quad \leftarrow\text{ done}	</mrow>
									</md>
								</p>
							</feedback>
						</choice>
						<choice correct="yes">
							<statement>
								<m>
									\quad \left\{
									\begin{align}
										\sqrt{y}	\amp =	c_1e^{3x}\\ 
										y			\amp =	c_2\, e^{6x} 
									\end{align}
									\right.\qquad
								</m> 
								where <m>c_2= c_1^2</m>.
							</statement>
							<feedback>
								<p>
									Correct, since
									<md>
										<mrow>	\sqrt{y}	\amp =,	c_1e^{3x}									</mrow>
										<mrow>	y			\amp =,	(c_1e^{3x})^2								</mrow>
										<mrow>	y			\amp =,	c_1^2(e^{3x})^2								</mrow>
										<mrow>	y			\amp =,	c_2\, e^{6x}\quad \text{where } c_2 = c_1^2	</mrow>
									</md>
								</p>
							</feedback>
						</choice>
					</choices>
				</task>
			</exercise>
		</paragraphs>
	</subsection>
</section>