<section>
	<title>Chapter 13 Exercises</title>

	<reading-questions label="c13-quick-answer">
		<title>ᯓ★❓Quick-Answer Questions</title>
		<p>
			<exercise><title>Multiple-Choice</title>

			</exercise>

			<exercise><title>Short-Answer</title>

			</exercise>
		</p>
	</reading-questions>

	<exercises>
		<title>Exercises</title>

        <exercisegroup>
            <title>Euler's Method for Systems</title>

            <introduction>
                <p>
                    Consider the initial-valued system
                    <md>
                        <mrow> y'	 \amp =  3z,\quad 	\amp y(2)	\amp = 3, </mrow>
                        <mrow> z'	 \amp =  y+z^2,		\amp z(2)	\amp = -4. </mrow>
                    </md>
                    and answer the following:
                </p>
            </introduction>

            <exercise>
                <statement>
                    Compute two iterations of Euler's method using step size <m> \ds h = 0.1. </m>
                </statement>
                <solution>
                    <p>
                        Compute two iterations of Euler's method using step size <m> \ds h = 0.1. </m>
                    </p>
                </solution>
                <answer>
                    <p>
                        
                    </p>
                </answer>
            </exercise>

            <exercise>
                <statement>
                    What is the meaning of your answer?
                </statement>
                <solution>
                    <p>
                        What is the meaning of your answer?
                    </p>
                </solution>
                <answer>
                    <p>
                        
                    </p>
                </answer>
            </exercise>
        </exercisegroup>

        <exercise>
            <title>Euler's Method for Systems</title>

            <statement>
                <p>
                    Consider the initial-valued system
                    <md>
                        <mrow> x'	 \amp =  2x - y + t,	\amp x(0) = 6, </mrow>
                        <mrow> y' 	 \amp =  x,				\amp y(0) = 2. </mrow>
                    </md>
                    Approximate <m> \ds x(0.2) </m> and <m> \ds y(0.2) </m> using <m>\Delta t = 0.1</m>.
                </p>
            </statement>
            <solution>
                <p>
            <md>
                    <mrow>  \mbox{Preliminaries:	}	\amp \amp	f_1(t,x,y)	 \amp =  2x - y + t </mrow>
                    <mrow>  \amp \amp	f_2(t,x,y)	 \amp =  x </mrow>
                    <mrow>  \amp \amp	\Delta t	 \amp =  0.1 </mrow>
                    <mrow>  \amp \amp	t_0	 \amp =  0 </mrow>
                    <mrow>  \amp \amp	x_0	 \amp =  6 </mrow>
                    <mrow>  \amp \amp	y_0	 \amp =  2 </mrow>
                    <mrow>  \amp \amp		 \amp \mbox{Iteration 1:}		\amp \amp	t_1	 \amp =  t_0 + \Delta t </mrow>
                    <mrow>  \amp \amp		 \amp =  0 + 0.1 </mrow>
                    <mrow>  \amp \amp		 \amp =  0.1 </mrow>
                    <mrow>  \amp \amp	x_1	 \amp =  x_0 + \Delta t \cdot f_1(t_0,x_0,y_0) </mrow>
                    <mrow>  \amp \amp		 \amp =  6 + 0.1 \cdot f_1(0,6,2) </mrow>
                    <mrow>  \amp \amp		 \amp =  6 + 0.1 \cdot [2(6) - 2 + 0] </mrow>
                    <mrow>  \amp \amp		 \amp =  7 </mrow>
                    <mrow>  \amp \amp	y_1	 \amp =  y_0 + \Delta t\cdot f_2(t_0,x_0,y_0) </mrow>
                    <mrow>  \amp \amp		 \amp =  2 + 0.1 \cdot f_2(0,6,2) </mrow>
                    <mrow>  \amp \amp		 \amp =  2 + 0.1 \cdot [6] </mrow>
                    <mrow>  \amp \amp		 \amp =  2.6 </mrow>
                    <mrow>  \amp \amp		 \amp \mbox{Iteration 2:}		\amp \amp	t_2	 \amp =  t_1 + \Delta t </mrow>
                    <mrow>  \amp \amp		 \amp =  0.1 + 0.1 </mrow>
                    <mrow>  \amp \amp		 \amp =  0.2 </mrow>
                    <mrow>  \amp \amp	x_2	 \amp =  x_1 + \Delta t \cdot f_1(t_1,x_1,y_1) </mrow>
                    <mrow>  \amp \amp		 \amp =  7 + 0.1 \cdot f_1(0.1,7,2.6) </mrow>
                    <mrow>  \amp \amp		 \amp =  7 + 0.1 \cdot [2(7) - 2.6 + 0.1] </mrow>
                    <mrow>  \amp \amp		 \amp =  8.15 </mrow>
                    <mrow>  \amp \amp	y_2	 \amp =  y_1 + \Delta t\cdot f_2(t_1,x_1,y_1) </mrow>
                    <mrow>  \amp \amp		 \amp =  2.6 + 0.1 \cdot f_2(0.1,7,2.6) </mrow>
                    <mrow>  \amp \amp		 \amp =  2.6 + 0.1 \cdot [7] </mrow>
                    <mrow>  \amp \amp		 \amp =  3.3  </mrow>
                </md>
                Therefore <m> \ds x(0.2) \approx 8.15 </m> an <m> \ds y(0.2) \approx 3.3. </m>
                </p>
            </solution>
            <answer>
                <p>
                    <m> \ds x(0.2) \approx 8.15 </m> <m> \hspace{0.5cm} \ds y(0.2) \approx 3.3. </m>
                </p>
            </answer>
        </exercise>

		<exercisegroup cols="2">
			<title>Reduction of Order</title>

			<introduction>
				<p>
					Reduce each of the following to a system of first-order differential equations.
				</p>
			</introduction>

			<exercise>
				<statement>
					<m> \ds y'' - 4y' + 4y = 0 </m>
				</statement>
				<solution>
					<p>
						<m> \ds y'' - 4y' + 4y = 0 </m>
					</p>
				</solution>
				<answer>
					<p>
						
					</p>
				</answer>
			</exercise>

			<exercise>
				<statement>
					<m> \ds x^2 y''' = 2y' </m>
				</statement>
				<solution>
					<p>
						<m> \ds x^2 y''' = 2y' </m>
					</p>
				</solution>
				<answer>
					<p>
						
					</p>
				</answer>
			</exercise>

			<exercise>
				<statement>
					<m> \ds y'' + x = 12 \ds x' + 2yt = \cos t </m>
				</statement>
				<solution>
					<p>
				We have one second-order and one first-order DE, which means we will need three variables to generate a systemof three first-order DEs.\\ Let <m> \ds u = y </m> <m> \ds v = y', </m> an <m> \ds w = x </m> .  Then we have the following.
					<md>
						<mrow> u'	 \amp =  y' = v \label{eq14-9}  </mrow>
					</md>
					Substituting into the first DE yields the following.
					<md>
						<mrow>  y'' + x	 \amp =  12 \nonumber </mrow>
						<mrow>  v' + w	 \amp =  12 \nonumber </mrow>
						<mrow>  v'	 \amp =  12 - w \label{eq14-10}  </mrow>
					</md>
					Substituting into the second DE yields the following.
					<md>
						<mrow>  w' + 2ut	 \amp =  \cos t \nonumber </mrow>
						<mrow>  w'	 \amp =  \cos t - 2ut \label{eq14-11}  </mrow>
					</md>
					Then equations (\ref{eq14-9}), (\ref{eq14-10}) and (\ref{eq14-11}) constitute a system of first-order DEs in the variable <m> \ds u </m> <m> \ds v </m> , and <m> \ds w </m> , as below:
					<md>
						<mrow>  u'	 \amp =  v </mrow>
						<mrow>  v'	 \amp =  12 - w </mrow>
						<mrow>  w'	 \amp =  \cos t - 2ut  </mrow>
					</md>
					
					</p>
				</solution>
				<answer>
					<p>
						<m> \ds u' = v, \ds v' = 12 - w, \ds w' = \cos t - 2ut </m> where <m> \ds u = y, \ds v = y', </m> an <m> \ds w = x </m>
					</p>
				</answer>
			</exercise>
		</exercisegroup>

		<exercisegroup>
			<title>Basic Euler's Method</title>

			<introduction>
				<p>
					Consider the IVP below.<m> \dsy'	= 2x - 3y + 1,\quad y(1)	= 5</m>
				</p>
			</introduction>

		<title> 
		<p>

		</p>
		<p/>
		</title>
			<exercise>
				<statement>
					<em> Euler's Method for Higher Order DEs \amp Systems</em> Consider the IVP below. <m> \ds y'' + 2y' + y^2 = 0\quad  \ds y(0.2) </m> using step size <m> \ds h = 0.1 </m> .
				</statement>
				<solution>
					<p>
				First we convert the second-order DE to a system of two first-order DEs. Let <m> \ds u = y </m> and <m> \ds v = y' </m> .  Then \begin{equation} u' = y' = v\label{eq14-12} \end{equation} and \begin{equation} v' = (y')' = y''.\label{eq14-13} \end{equation} Substituting equations (\ref{eq14-12}) and (\ref{eq14-13}) into the DE yields the following.
					<md>
						<mrow>  y'' + 2y' + y^2	 \amp =  0 \nonumber  </mrow>
						<mrow>  v' + 2v + u^2	 \amp =  0 \nonumber  </mrow>
						<mrow>  v'	 \amp =  -2v - u^2 \label{eq14-14}  </mrow>
					</md>
					Then equations (\ref{eq14-12}) and (\ref{eq14-14}) constitute a system of first-order DEs in the variable <m> \ds u </m> and <m> \ds v </m> .
					<md>
						<mrow>  u'	 \amp =  v </mrow>
						<mrow>  v'	 \amp =  -2v - u^2 </mrow>

					</md>
					Note that we can also convert the initial conditions to the new variables:
					<md>
						<mrow> u(0)	 \amp =  1 </mrow>
						<mrow>  v(0)	 \amp =  2  </mrow>
					</md>
					Now we can use Euler's method as follows.
					<md>
						<mrow>  \mbox{Preliminaries:	}	\amp \amp	f_1(t,u,v)	 \amp =  v </mrow>
						<mrow>  \amp \amp	f_2(t,u,v)	 \amp =  -2v-u^2 </mrow>
						<mrow>  \amp \amp	h	 \amp =  0.1 </mrow>
						<mrow>  \amp \amp	t_0	 \amp =  0 </mrow>
						<mrow>  \amp \amp	u_0	 \amp =  1 </mrow>
						<mrow>  \amp \amp	v_0	 \amp =  2 </mrow>
						<mrow>  \amp \amp		 \amp \mbox{Iteration 1:}		\amp \amp	t_1	 \amp =  t_0 + h </mrow>
						<mrow>  \amp \amp		 \amp =  0 + 0.1 </mrow>
						<mrow>  \amp \amp		 \amp =  0.1 </mrow>
						<mrow>  \amp \amp	u_1	 \amp =  u_0 + h \cdot f_1(t_0,u_0,v_0) </mrow>
						<mrow>  \amp \amp		 \amp =  1 + 0.1 \cdot f_1(0,1,2) </mrow>
						<mrow>  \amp \amp		 \amp =  1 + 0.1 \cdot [2] </mrow>
						<mrow>  \amp \amp		 \amp =  1.2 </mrow>
						<mrow>  \amp \amp	v_1	 \amp =  v_0 + h\cdot f_2(t_0,u_0,v_0) </mrow>
						<mrow>  \amp \amp		 \amp =  2 + 0.1 \cdot f_2(0,1,2) </mrow>
						<mrow>  \amp \amp		 \amp =  2 + 0.1 \cdot [-2(2) - (1)^2] </mrow>
						<mrow>  \amp \amp		 \amp =  1.5 </mrow>
						<mrow>  \amp \amp		 \amp \mbox{Iteration 2:}		\amp \amp	t_2	 \amp =  t_1 + h </mrow>
						<mrow>  \amp \amp		 \amp =  0.1 + 0.1 </mrow>
						<mrow>  \amp \amp		 \amp =  0.2 </mrow>
						<mrow>  \amp \amp	u_2	 \amp =  u_1 + h \cdot f_1(t_1,u_1,v_1) </mrow>
						<mrow>  \amp \amp		 \amp =  1.2 + 0.1 \cdot f_1(0.1, 1.2, 1.5) </mrow>
						<mrow>  \amp \amp		 \amp =  1.2 + 0.1 \cdot [1.5] </mrow>
						<mrow>  \amp \amp		 \amp =  1.35 </mrow>
						<mrow>  \amp \amp	v_2	 \amp =  v_1 + h\cdot f_2(t_1,u_1,v_1) </mrow>
						<mrow>  \amp \amp		 \amp =  1.5 + 0.1 \cdot f_2(0.1, 1.2, 1.5) </mrow>
						<mrow>  \amp \amp		 \amp =  1.5 + 0.1 \cdot [-2(1.5) - (1.2)^2] </mrow>
						<mrow>  \amp \amp		 \amp =  1.0560  </mrow>
					</md>
					Therefore <m> \ds u(0.2) \approx 1.35 </m> an <m> \ds v(0.2) \approx 1.0560. </m>	This mean <m> \ds y(0.2) \approx 1.35 </m> (and, even though we were not asked for it specifically <m> \ds y'(0.2) \approx 1.0560 </m> ).
					</p>
				</solution>
				<answer>
					<p>
						<m> \ds y(0.2) \approx 1.35 </m>
					</p>
				</answer>
			</exercise>

		</exercisegroup>

		<exercisegroup>
			<title>Basic Euler's Method</title>

			<introduction>
				<p>
					Consider the IVP below.<m> \dsy'	= 2x - 3y + 1,\quad y(1)	= 5</m>
				</p>
			</introduction>

		<title> 
		<p>
		Use Euler's Method to approximate <m> \ds y(3.2) </m> wher <m> \ds y </m> is the solution to <m> \ds y'' - 2y = e^{t-3} \cos t,\quad  y(3) = -1,\quad y'(3) = 0, </m>
		</p>
		<p/>
		</title>
			<exercise>
				<statement>
					usin <m> \ds \Delta t = 0.2. </m> \label{partA_euler}
				</statement>
				<solution>
					<p>
				First we convert the second-order DE to a system of two first-order DEs. Let <m> \ds u = y </m> and <m> \ds v = y' </m> .  Then \begin{equation} u' = y' = v\label{eq14-15} \end{equation} and \begin{equation} v' = (y')' = y''.\label{eq14-16} \end{equation} Substituting equations (\ref{eq14-14}) and (\ref{eq14-15}) into the DE yields the following.
					<md>
						<mrow>  y'' - 2y	 \amp =  e^{t-3} \cos t \nonumber  </mrow>
						<mrow>  v' - 2u	 \amp =  e^{t-3}\cos t \nonumber  </mrow>
						<mrow>  v'	 \amp =  e^{t-3}\cos t +2u \label{eq14-17}  </mrow>
					</md>
					Then equations (\ref{eq14-15}) and (\ref{eq14-17}) constitute a system of first-order DEs in the variable <m> \ds u </m> and <m> \ds v </m> .
					<md>
						<mrow>  u'	 \amp =  v </mrow>
						<mrow>  v'	 \amp =  e^{t-3}\cos t +2u  </mrow>
					</md>
					Note that we can also convert the initial conditions to the new variables:
					<md>
						<mrow> u(3)	 \amp =  -1 </mrow>
						<mrow>  v(3)	 \amp =  0  </mrow>
					</md>
					Now we can use Euler's method as follows.
					<md>
						<mrow>  \mbox{Preliminaries:	}	\amp \amp	f_1(t,u,v)	 \amp =  v </mrow>
						<mrow>  \amp \amp	f_2(t,u,v)	 \amp =  e^{t-3}\cos t +2u </mrow>
						<mrow>  \amp \amp	\Delta t 	 \amp =  0.2 </mrow>
						<mrow>  \amp \amp		t_0	 \amp =  3 </mrow>
						<mrow>  \amp \amp		u_0	 \amp =  -1 </mrow>
						<mrow>  \amp \amp		v_0	 \amp =  0 </mrow>
						<mrow>  \amp \amp		 \amp \mbox{Iteration 1:}		\amp \amp	t_1	 \amp =  t_0 + \Delta t </mrow>
						<mrow>  \amp \amp		 \amp =  3 + 0.2 </mrow>
						<mrow>  \amp \amp		 \amp =  3.2 </mrow>
						<mrow>  \amp \amp	u_1	 \amp =  u_0 + \Delta t \cdot f_1(t_0,u_0,v_0) </mrow>
						<mrow>  \amp \amp		 \amp =  -1 + 0.2 \cdot f_1(3, -1, 0) </mrow>
						<mrow>  \amp \amp		 \amp =  -1 + 0.2 \cdot [0] </mrow>
						<mrow>  \amp \amp		 \amp =  -1 </mrow>
						<mrow>  \amp \amp	v_1	 \amp =  v_0 + \Delta t \cdot f_2(t_0,u_0,v_0) </mrow>
						<mrow>  \amp \amp		 \amp =  0 + 0.2 \cdot f_2(3, -1, 0) </mrow>
						<mrow>  \amp \amp		 \amp =  0 + 0.2 \cdot [e^{3-3}\cos(3) + 2(-1)] </mrow>
						<mrow>  \amp \amp		 \amp =  -0.5980  </mrow>
					</md>
					Therefore <m> \ds u(3.2) \approx -1 </m> , which mean <m> \ds y(3.2) \approx -1 </m> (and, even though we were not asked for it specifically, we also know <m> \ds y'(3.2) \approx -0.5980 </m> ).
					</p>
				</solution>
				<answer>
					<p>
						<m> \ds y(3.2) \approx -1 </m>
					</p>
				</answer>
			</exercise>

			<exercise>
				<statement>
					using <m> \ds \Delta t = 0.1 </m>
				</statement>
				<solution>
					<p>
				We will use the system of DEs developed in part \ref{partA_euler} Now we can use Euler's method as follows.
					<md>
						<mrow>  \mbox{Preliminaries:	}	\amp \amp	f_1(t,u,v)	 \amp =  v </mrow>
						<mrow>  \amp \amp	f_2(t,u,v)	 \amp =  e^{t-3}\cos t +2u </mrow>
						<mrow>  \amp \amp	h	 \amp =  0.1 </mrow>
						<mrow>  \amp \amp	t_0	 \amp =  3 </mrow>
						<mrow>  \amp \amp	u_0	 \amp =  -1 </mrow>
						<mrow>  \amp \amp	v_0	 \amp =  0 </mrow>
						<mrow>  \amp \amp		 \amp \mbox{Iteration 1:}		\amp \amp	t_1	 \amp =  t_0 + h </mrow>
						<mrow>  \amp \amp		 \amp =  3 + 0.1 </mrow>
						<mrow>  \amp \amp		 \amp =  3.1 </mrow>
						<mrow>  \amp \amp	u_1	 \amp =  u_0 + h \cdot f_1(t_0,u_0,v_0) </mrow>
						<mrow>  \amp \amp		 \amp =  -1 + 0.1 \cdot f_1(3, -1, 0) </mrow>
						<mrow>  \amp \amp		 \amp =  -1 + 0.1 \cdot [0] </mrow>
						<mrow>  \amp \amp		 \amp =  -1 </mrow>
						<mrow>  \amp \amp	v_1	 \amp =  v_0 + h\cdot f_2(t_0,u_0,v_0) </mrow>
						<mrow>  \amp \amp		 \amp =  0 + 0.1 \cdot f_2(3, -1, 0) </mrow>
						<mrow>  \amp \amp		 \amp =  0 + 0.1 \cdot [e^{3-3}\cos(3) + 2(-1)] </mrow>
						<mrow>  \amp \amp		 \amp =  -0.2990 </mrow>
						<mrow>  \amp \amp		 \amp \mbox{Iteration 2:}		\amp \amp	t_2	 \amp =  t_1 + h </mrow>
						<mrow>  \amp \amp		 \amp =  3.1 + 0.1 </mrow>
						<mrow>  \amp \amp		 \amp =  3.2 </mrow>
						<mrow>  \amp \amp	u_2	 \amp =  u_1 + h \cdot f_1(t_1,u_1,v_1) </mrow>
						<mrow>  \amp \amp		 \amp =  -1 + 0.1 \cdot f_1(3.1, -1, -0.2990) </mrow>
						<mrow>  \amp \amp		 \amp =  -1 + 0.1 \cdot [-0.2990] </mrow>
						<mrow>  \amp \amp		 \amp =  -1.0299 </mrow>
						<mrow>  \amp \amp	v_2	 \amp =  v_1 + h\cdot f_2(t_1,u_1,v_1) </mrow>
						<mrow>  \amp \amp		 \amp =  -0.2990 + 0.1 \cdot f_2(3.1, -1, -0.2990) </mrow>
						<mrow>  \amp \amp		 \amp =  -0.2990 + 0.1 \cdot [e^{3.1 - 3}\cos(3.1) + 2(-1)] </mrow>
						<mrow>  \amp \amp		 \amp =  -0.6094  </mrow>
					</md>
					Therefore <m> \ds u(3.2) \approx -1.0299 </m> , which mean <m> \ds y(3.2) \approx -1.0299 </m> (and, even though we were not asked for it specifically, we also know <m> \ds y'(3.2) \approx -0.6094 </m> ).\\ %
					</p>
				</solution>
				<answer>
					<p>
						<m> \ds y(3.2) \approx -1.0299 </m>
					</p>
				</answer>
			</exercise>

		</exercisegroup>
	</exercises>

</section>