<section label="lt-roadmap">
	<title> Laplace Method 4 Step Roadmap </title>

	<introduction>
		<p>
			NEED AN INTRO
		</p>
	</introduction>

	<subsection label="roadmap-overview">
		<title> Roadmap Overview </title>

		<p>
		The overall strategy is summarized in the <xref ref="lt-roadmap" text="Laplace transform roadmap"/>. This four-step process begins by transforming the differential equation into the Laplace domain (step 1). In this new setting, we solve the algebraic Laplace equation (step 2), manipulate the solution into a simpler form if needed (step 3), and finally apply the inverse Laplace transform to return to the time domain (step 4).
		</p>

		<figure xml:id="lt-roadmap"><title> ✳️ Laplace Transform Roadmap </title>
			<caption>
				A visual guide outlining the four-step process of using Laplace transforms to solve initial value problems.
			</caption>
			<image source="figures/lt-roadmap-step-1-4.png" width="80%"/>
		</figure>

		<assemblage xml:id="lt-roadmap-full">
			<title> Laplace Method Roadmap </title>
			<p>
				<sidebyside widths="37% 12% 45%" valign="middle">
					<p>
						<me>\textbf{Original Differential Equation}</me>
					</p>
					<p/>
					<p>
						<me>\DLBa\textbf{Laplace Domain}</me>
					</p>
				</sidebyside>
				<sidebyside widths="29% 10% 41%" valign="bottom">
					<p>
						<md>
							<mrow>y'' - 9y = 10e^{2t}</mrow>
							<mrow>y(0) = 1,\quad y'(0) = -7</mrow>
							<mrow/>
							<mrow/>
							<mrow/>
							<mrow/>
							<mrow/>
							<mrow/>
							<mrow>\textbf{Solution}</mrow>
							<mrow>\vphantom{\sum_{m}} y = e^{3t} + 2e^{-3t} - 2e^{2t}</mrow>
						</md>
					</p>
					<p>
						<md>
							<mrow>\os{\Large\text{1️⃣}}{\us{\large\text{forward}}{\os{\large\laplacesym}{\longrightarrow}}}</mrow>
							<mrow/>
							<mrow/>
							<mrow/>
							<mrow/>
							<mrow/>
							<mrow> \os{\Large\text{4️⃣}}{\us{\large\text{backward}}{\os{\large\laplacesym^{-1}}{\longleftarrow}}} </mrow>
						</md>
						<me>
							
						</me>
					</p>
					<p>
						<assemblage>
							<p>
								<md>
									<mrow>\DLBa s^2Y - 9Y - s + 7 = \frac{10}{s - 2}</mrow>
									<mrow>\vphantom{\sum^{m}_{m}}\downarrow\quad \text{ 2️⃣ Solve for}\ Y</mrow>
									<mrow>\DLBa Y = \frac{1}{s^2 - 9}\left( \frac{10}{s - 2} + s - 7 \right) </mrow>
									<mrow>\vphantom{\sum^{m}_{m}}\downarrow\ \ \text{ 3️⃣ Prepare for Inverse}</mrow>
									<mrow>\DLBa Y = \frac{1}{s - 3} + \frac{2}{s + 3} - \frac{2}{s - 2} </mrow>
								</md>
							</p>
						</assemblage>
					</p>
				</sidebyside>
			</p>
		</assemblage>

		<p>
			This chapter breaks the method into manageable pieces. First, we will define the Laplace transform, motivate why it works, and build a set of useful properties. Next, we will explore the details of each step in the method. Finally, we will work through a variety of examples to show how this approach is used to efficiently solve initial value problems.
		</p>

		<p>
			The heart of the Laplace transform method lies in its ability to convert a differential equation into an algebraic equation. This transformation takes place in what we call the <em>Laplace domain</em>, a mathematical space where derivatives become algebraic expressions and initial conditions are naturally incorporated into the equation.
		</p>

		<p>
			In this section, we will break down how to solve the model equation
			<men xml:id="lt-model-eqn-w-ics"> 
				y'' - 9y = 10e^{2t}, \quad y(0) = 1, \quad y'(0) = -7
			</men>
			using the steps outlined in the <xref ref="lt-roadmap" text="custom">Laplace Transform Roadmap</xref>:
		</p>
			
		<ol marker="(i)">
			<li>
				<p>
					We begin with <xref ref="lt-roadmap-step-1" text="custom">step 1</xref>, where the forward transform moves the differential equation into the Laplace domain.
				</p>
			</li>
			<li>
				<p>
					Then, we jump to <xref ref="lt-roadmap-step-4" text="custom">step 4</xref> to explore how the transformed equation is converted back into the original domain using a backward transform.
				</p>
			</li>
			<li>
				<p>
					Finally, we examine <xref ref="lt-roadmap-step-2-3" text="custom">steps 2 and 3</xref>, which take place entirely within the Laplace domain and lead to the solution of the original equation.
				</p>
			</li>
		</ol>
	</subsection>

	<subsection label="roadmap-into-lap-domain">
		<title> Step 1: Into the Laplace Domain (Forward Transform) </title>
		<assemblage><title>Step 1: Into the Laplace Domain (Forward Transform)</title>
			<p>
			
			<image source="figures/lt-4-step-map-step-1.png" width="100%"/>
	</p>
		</assemblage>

		<sidebyside>
			<p>
				<assemblage>
					<title>piss</title>
					<p>
						<paragraphs><title>FUCK</title></paragraphs>
					</p>
				</assemblage>
			</p>
			<p>
				<assemblage>
					<p>
						<paragraphs><title>ME</title></paragraphs>
					</p>
				</assemblage>
			</p>
		</sidebyside>

		<assemblage xml:id="lt-roadmap-step-1"><title> Step 1 - Into the Laplace Domain (Forward Transform) </title>
					<p>
				<sidebyside widths="39% 14% 47%" valign="middle">
					<p>
						<me>\text{Original Differential Equation}</me>
					</p>
					<p/>
					<p>
						<me>\text{Laplace Domain}</me>
					</p>
				</sidebyside>
				<sidebyside widths="39% 14% 47%" valign="middle">
					<p>
						<md>
							<mrow>y'' - 9y = 10e^{2t}</mrow>
							<mrow>y(0) = 1,\quad y'(0) = -7</mrow>
						</md>
					</p>
					<p>
						<me>
							\os{\Large\text{1️⃣}}{\us{\large\text{forward}}{\os{\large\laplacesym}{\longrightarrow}}}
						</me>
					</p>
					<p>
						<assemblage>
							<p>
						<md>
							<mrow>\us{\ds\text{Laplace Equation}}{s^2Y - 9Y - s + 7 = \frac{10}{s - 2}}</mrow>
						</md>
					</p>
						</assemblage>
					</p>
				</sidebyside>
				<!-- <sidebyside widths="39% 14% 47%" valign="middle">
					<p>
						<me>\text{Differential Equation}</me>
					</p>
					<p/>
					<p>
						<me>\text{Laplace Equation}</me>
					</p>
				</sidebyside> -->
			</p>
		</assemblage>
		
	</subsection>

	<subsection label="roadmap-out-of-lap-domain">
		<title> Step 4 - Out of the Laplace Domain </title>
		<assemblage xml:id="lt-roadmap-step-4"><title> Step 4 - Out of the Laplace Domain (Backward Transform) </title>
			<p>
				<sidebyside widths="39% 15% 46%" valign="top">
					<p>
						<md>
							<mrow>	\vphantom{M}													</mrow>
							<mrow>	\ub{y\vphantom{\frac{1}{s - 3}} = e^{3t} + 2e^{-3t} - 2e^{2t}}	</mrow>
						</md>
					</p>
					<p>
						<me>
							\os{\Large\text{4️⃣}}{\us{\large\text{backward}}{\os{\large\laplacesym^{-1}}{\longleftarrow}}}
						</me>
					</p>
					<p>
						<md>
							<mrow>	\vphantom{M}													</mrow>
							<mrow>	\small\ub{Y = \frac{1}{s - 3} + \frac{2}{s + 3} - \frac{2}{s - 2}}	</mrow>
						</md>
						<me>
							
						</me>
					</p>
				</sidebyside>
				<sidebyside widths="39% 15% 46%" valign="middle">
					<p>
						<me>
							\text{Solution}
						</me>
					</p>
					<p/>
					<p>
						<me>
							\text{Laplace Solution (prepared)}
						</me>
					</p>
				</sidebyside>
			</p>
		</assemblage>
		<image source="figures/lt-4-step-map-step-4.png" width="100%"/>
	</subsection>

	<subsection label="roadmap-within-laplace-domain">
		<title> Steps 2 &amp; 3 - Within the Laplace Domain </title>
		<assemblage xml:id="lt-roadmap-step-2-3"><title> Steps 2 &amp; 3 - Solve for <m>Y</m> &amp; Prepare for <m>\laplacesym^{-1}</m> </title>
			<p>
				<sidebyside widths="4% 28% 12% 56%" valign="middle">
					<p/>
					<p>
						Laplace Equation
					</p>
					<p>
						<me>
							\longrightarrow
						</me>
					</p>
					<p>
						<me>
							s^2Y - 9Y - s + 7 = \frac{10}{s - 2}
						</me>
					</p>
				</sidebyside>
			</p>
			<p>
				<sidebyside widths="55% 10% 35%" valign="middle">
					<p/>
					<p><me>\downarrow</me></p>
					<p>
						2️⃣ Solve for <m>Y</m>
					</p>
				</sidebyside>
			</p>
			<p>
				<sidebyside widths="4% 28% 12% 56%" valign="middle">
					<p/>
					<p>
						Laplace Solution
					</p>
					<p>
						<me>
							\longrightarrow
						</me>
					</p>
					<p>
						<me>
							Y = \frac{1}{s^2 - 9}\left( \frac{10}{s - 2} + s - 7 \right)
						</me>
					</p>
				</sidebyside>
			</p>
			<p>
				<sidebyside widths="55% 10% 35%" valign="middle">
					<p/>
					<p><me>\downarrow</me></p>
					<p>
						3️⃣ Prepare for <m>\laplacesym^{-1}</m>
					</p>
				</sidebyside>
			</p>
			<p>
				<sidebyside widths="4% 28% 12% 56%" valign="middle">
					<p/>
					<p>
						Laplace Solution (prepared)
					</p>
					<p>
						<me>
							\longrightarrow
						</me>
					</p>
					<p>
						<me>
							Y = \frac{1}{s - 3} + \frac{2}{s + 3} - \frac{2}{s - 2}
						</me>
					</p>
				</sidebyside>
			</p>
		</assemblage>
		<image source="figures/lt-4-step-map-step-2.png" width="50%"/>
		<image source="figures/lt-4-step-map-step-3.png" width="50%"/>
	</subsection>

	<objectives label="lt-roadmap-wrapup">
		<ul>
			<li> 

			</li>
		</ul>
	</objectives>

	<fact label="lt-roadmap-cyu">
		<statement>
			<p>
				Answer the following questions related to 

			</p>
		</statement>
	</fact>
</section>