<section label="into-laplace-domain">
	<title> Forward Into the Laplace Domain </title>

	<introduction>
		<p>
			In <xref ref="lt-roadmap-full" text="custom">step 1 of the roadmap</xref>, we cross from the familiar realm of differential equations into a new landscape called the Laplace domain. This transition, known as the <q>forward Laplace transform</q>, converts differential equations into algebraic equations where it is much easier to isolate the unknown. It just so happens that when you isolate the unknown in the Laplace domain you are indirectly isolating the unknown in the original differential equation!
		</p>

		<assemblage xml:id="lt-roadmap-step-1"><title> Step 1Ô∏è‚É£: Into the Laplace Domain (Forward Transform) </title>
			<p>
				<sidebyside widths="32% 18% 42%" valign="middle">
					<p>
						<me>\ul{\qquad\textbf{Original Domain}\qquad}</me>
					</p>
					<p/>
					<p>
						<me>\DLBa\textbf{Laplace Domain}</me>
					</p>
				</sidebyside>
				<sidebyside widths="32% 18% 42%" valign="top">
					<p>
						<md>
							<mrow>\os{\vphantom{m}}{y'' - 9y = 10e^{2t}}</mrow>
							<mrow>y(0) = 1,\quad y'(0) = -7</mrow>
							<mrow>\os{\large üî∫ üî∫ üî∫ üî∫ üî∫}{\text{Differential Equation}}</mrow>
						</md>
					</p>
					<p>
						<md>
							<mrow>\underrightarrow{\text{1Ô∏è‚É£ Forward}}</mrow>
							<mrow>\text{Apply}\ \laplacesym</mrow>
							<mrow/>
						</md>
					</p>
					<p>
						<assemblage>
							<p>
								<md>
									<mrow>\DLBa s^2Y - 9Y - s + 7 = \frac{10}{s - 2}</mrow>
									<mrow>\DLBa\dotsm</mrow>
								</md>
							</p>
						</assemblage>
					</p>
				</sidebyside>
			</p>
		</assemblage>
	</introduction>

	<subsection><title> From a Differential Equation to a Laplace Equation </title>

		<task label="laplace-domain-chkpt-1">
			<title> üìñ‚ùì Applying the Laplace Transform to an Equation </title>
			<statement>
				<p>
					<em> Fill-in-the-blanks: </em>
				</p>
				<p>
					The process of applying a Laplace transform to a differential equation involves multiplying the equation by <fillin characters="13" /> and <fillin characters="13" /> with respect to <m>t</m>.
				</p>
				<p/>
			</statement>
			<choices randomize="yes">
			<choice>
				<statement><m>e^{-t},</m> integrating</statement>
				<feedback>
				<p>
					No, this misses the <m>s</m> parameter in the exponential. It should be <m>e^{-st}</m>.
				</p>
				</feedback>
			</choice>
			<choice correct="yes">
				<statement><m>e^{-st},</m> integrating</statement>
				<feedback>
				<p>
					Correct! The Laplace transform involves multiplying the original function by <m>e^{-st}</m> and then integrating with respect to <m>t</m>.
				</p>
				</feedback>
			</choice>
			<choice>
				<statement><m>e^{st},</m> integrating</statement>
				<feedback>
				<p>
					No, the exponent should have a negative sign: <m>e^{-st}</m>.
				</p>
				</feedback>
			</choice>
			<choice>
				<statement><m>e^{-st},</m> differentiating</statement>
				<feedback>
				<p>
					No, the Laplace transform requires integration, not differentiation.
				</p>
				</feedback>
			</choice>
			<choice>
				<statement><m>s,</m> differentiating</statement>
				<feedback>
				<p>
					No, the transform uses <m>e^{-st}</m> and integration, not the variable <m>s</m> directly or differentiation.
				</p>
				</feedback>
			</choice>
			</choices>
		</task>

		<p>
			While applying the Laplace transform directly from a table makes this step appear simple, it is important to understand the underlying mechanics of this process.
		</p>

		<p>
			Recall from earlier discussions that the essence of the Laplace transform involves multiplying the entire differential equation by the exponential function <m>e^{-st}</m> and then integrating from <m>0</m> to <m>\infty</m> with respect to <m>t</m>. Symbolically, we represent this operation as:
			<me>
				\ub{\int_0^{\infty} e^{-st} y''\, dt}_{\large\lap{y''}}
				- \ub{\int_0^{\infty} e^{-st} (9y)\, dt}_{\large\lap{9y}}
				= \ub{\int_0^{\infty} e^{-st}(10e^{2t})\, dt}_{\large\lap{10e^{2t}}}
			</me>
		</p>

		<p>
			Applying integration by parts to the integrals involving derivatives of the unknown function <m>y(t)</m> enables us to transfer these derivatives onto the <m>e^{-st}</m> terms, resulting in a power of <m>s</m> for each. After performing integration by parts twice on the first integral and computing the integral on the right-hand side, we arrive at:
			<me>
				-sy(0) - y'(0) + s^2\ub{\int_0^{\infty} e^{-st}y\, dt}_{\large\lap{y}=Y}
				- 9\ub{\int_0^{\infty} e^{-st}y\, dt}_{\large\lap{y}=Y}
				= \frac{10}{s-2}
			</me>
		</p>

		<p>
			Notice that the two integrals are <m>\lap{y}</m>, which can bundle up as just <m>Y</m>. Incorporating the provided initial conditions, <m>y(0) = 1</m> and <m>y'(0) = -7</m>, the equation simplifies neatly to the algebraic form:
			<me>
				s^2Y - 9Y - s + 7 = \frac{10}{s-2}
			</me>.
		</p>

		<p>
			By transforming our equation into this new form, we have temporarily hidden <m>y(t)</m> elegantly inside <m>Y</m>. Therefore, by solving for <m>Y</m>, we are effectively also solving for <m>y(t)</m> at the same time! While we will not be showing this every time we solve a different equation, it is nice to be able to appreciate the magic behind the curtain.
		</p>

		<p>
			In practice, we get the forward transforms from the <xref ref="lt-table-L1-12" text="custom">table of transforms</xref>, which is a much faster process. Let's demostrate this procedure with some examples.
		</p>

		<example><title> Forward Transforming Equations </title>
			<p>
				<statement>
					<p>
						Transform the initial-value problems into a Laplace equation within the Laplace domain:
						<ol>
							<li>
								<p>
									<m>\ds y'' - 9y = 10e^{2t}, \quad y(0) = 1, \quad y(0) = -7.</m>
								</p>
							</li>
							<li>
								<p>
									<m>\ds y'' - 4y' + 6y = t^2, \quad y(0) = 2, \quad y'(0) = 0.</m>
								</p>
							</li>
						</ol>
					</p>
				</statement>
			</p>

			<p>
				<solution>
					<p>
						First, we apply <m>\laplacesym</m> to both sides:
						<me>
							\lap{y'' - 9y} = \lap{10e^{2t}}
						</me>.
					</p>

					<p>
						Using the <xref ref="lt-linearity-property" text="custom">linearity property</xref>, we break this into four transforms
						<me>
							\ub{\lap{y''}}_{\large L_{10}} 
							+ 3\ub{\lap{y'}}_{\large L_9} 
							+ 2\ub{\lap{y}}_{\large Y} = -40\ub{\lap{e^{3t}}}_{\large L_2}
						</me>,
						and using <xref ref="lt-L10" text="custom">L<m>_10</m></xref>, <xref ref="lt-L9" text="custom">L<m>_9</m></xref>, and <xref ref="lt-L2" text="custom">L<m>_2</m></xref> from the <xref ref="lt-table-L1-12" text="custom">Laplace transform table</xref>, we transform the equation as follows:
					</p>

					<p>
						<me>
							s^2Y - s\os{\large 0}{\os{\Large \shortparallel}{y(0)}} - \os{\large 1}{\os{\Large \shortparallel}{y'(0)}} 
							+ 3s\left(sY - y(0)\right) + 2Y = -40\frac{1}{s - 3}
						</me>,
						or
						<me>
							s^2Y - 9Y - s + 7 = \frac{10}{s - 2}.
						</me>
					</p>
				</solution>

				<solution>
					<p>
						Applying the Laplace transform to both sides and using the Laplace transform table, we have:
						<md>
							<mrow>
								\lap{y'' - 4y' + 6y} 
								\amp = \lap{t^2}
							</mrow>
							<mrow>
								\lap{y''} - 4\lap{y'} + 6\lap{y} 
								\amp = \lap{t^2}
							</mrow>
							<mrow>
								s^2Y - s\os{\large 2}{\os{\Large \shortparallel}{y(0)}} 
								- \os{\large 0}{\os{\Large \shortparallel}{y'(0)}} 
								- 4(sY - \os{\large 2}{\os{\Large \shortparallel}{y(0)}}) + 6Y 
								\amp = \frac{2}{s^3}
							</mrow>
							<mrow>
								s^2Y - 2s - 4sY + 8 + 6Y 
								\amp = \frac{2}{s^3}
							</mrow>
							<mrow>
								s^2Y - 4sY + 6Y - 2s + 8 
								\amp = \frac{2}{s^3}
							</mrow>.
						</md>
					</p>
				</solution>
			</p>
		</example>

		<p> 
			These examples illustrate how we can transform differential equations into Laplace equations. Next, we'll explore how to reverse this process and uncover the original solution <m>y(t)</m> hidden within our transformed equations.
		</p>

	<exercise label="chkpts-forward-transforming-eqns"><title> <em>Answer-the-Following</em> </title>

		<introduction>
			<p>
				Complete the questions on each tab to check your understanding.
			</p>
		</introduction>
		
		<task label="p4-c1-s4-1-rq1"><title> <em>Applying the Laplace transform to a differential equation transforms the equation into an algebraic equation involving functions of <m>s</m></em> </title>
			<statement correct="yes">
				<p>
					Applying the Laplace transform to a differential equation transforms the equation into an algebraic equation involving functions of <m>s</m>
				</p>
			</statement>
			<feedback>
				<p>True. The Laplace transform converts a differential equation into an algebraic equation in <m>s</m>.</p>
			</feedback>
		</task>
		
		<task label="p4-c1-s4-1-rq2"><title> <em>Which of the following represents the correct Laplace transform of the equation <me>y'' + 3y' + 2y = -40e^{3t}, \quad y(0) = 1, \quad y'(0) = 0</me>?</em> </title>
			<statement/>
			<choices randomize="yes">
				<choice>
					<statement><m>\ds s^2Y + 3sY + 2Y = \frac{-40}{s-3}</m></statement>
					<feedback>
						<p>No, this is incorrect. Where are the initial conditions?</p>
					</feedback>
				</choice>
				<choice correct="yes">
					<statement><m>\ds s^2Y + 3sY + 2Y - s = \frac{-40}{s-3}</m></statement>
					<feedback>
						<p>Correct! This is the correct transformation of the given differential equation.</p>
					</feedback>
				</choice>
				<choice>
					<statement><m>\ds s^2Y + 3sY + 2Y + s = \frac{-40}{s - 3}</m></statement>
					<feedback>
						<p>No, this is close to the answer, but it is off by a sign.</p>
					</feedback>
				</choice>
				<choice>
					<statement><m>\ds s^2Y + 3sY + 2Y - 1 = \frac{-40}{s - 3}</m></statement>
					<feedback>
						<p>Incorrect, look closely at the initial conditions.</p>
					</feedback>
				</choice>
			</choices>
		</task>
		
		<task label="p4-c1-s4-1-rq3"><title> <em>Which of the following represents the correct Laplace transform of the equation <me>y'' - 4y' + 6y = t^2, \quad y(0) = 2, \quad y'(0) = -1</me>?</em> </title>
			<statement>
				<p>
					<em>Which of the following represents the correct Laplace transform of the equation <me>y'' - 4y' + 6y = t^2, \quad y(0) = 2, \quad y'(0) = -1</me>?</em>
				</p>
			</statement>
			<choices randomize="yes">
				<choice>
					<statement><m>\ds s^2Y - 4sY + 6Y - 2s = \frac{1}{s^3}</m></statement>
					<feedback>
						<p>No, this is incorrect. You are missing a term.</p>
					</feedback>
				</choice>
				<choice>
					<statement><m>\ds s^2Y - 4sY + 6Y + 2s - 1 = \frac{2}{s^3}</m></statement>
					<feedback>
						<p>No, this is close to the answer. Double check the signs of the initial conditions.</p>
					</feedback>
				</choice>
				<choice>
					<statement><m>\ds s^2Y - 4sY + 6Y + 1 = \frac{1}{s^3}</m></statement>
					<feedback>
						<p>No, this is incorrect. You are missing a term.</p>
					</feedback>
				</choice>
				<choice correct="yes">
					<statement><m>\ds s^2Y - 4sY + 6Y - 2s + 1 = \frac{2}{s^3}</m></statement>
					<feedback>
						<p>Correct! This is the correct transformation using the Laplace transform and applying initial conditions.</p>
					</feedback>
				</choice>
			</choices>
		</task>
		
		<task label="p4-c1-s4-1-rq4"><title> <em>What is the Laplace transform of the initial-value problem <me>y'' - 4y' + 6y = \sin t, \quad y(0) = 2, \quad y'(0) = 0</me>?</em> </title>
			<statement>
				<p>
					<em>What is the Laplace transform of the initial-value problem <me>y'' - 4y' + 6y = \sin t, \quad y(0) = 2, \quad y'(0) = 0</me>?</em>
				</p>
			</statement>
			<choices randomize="yes">
				<choice>
					<statement><m>s^2Y + 4sY + 6Y = \frac{1}{s^2 + 1}</m></statement>
					<feedback>
						<p>No, this is incorrect. Double-check the signs and the initial condition terms.</p>
					</feedback>
				</choice>
				<choice correct="yes">
					<statement><m>s^2Y - 4sY + 6Y - 2s + 8 = \frac{1}{s^2 + 1}</m></statement>
					<feedback>
						<p>Correct! This is the correct transformation of the initial-value problem.</p>
					</feedback>
				</choice>
				<choice>
					<statement><m>s^2Y - 4sY + 6Y = \frac{1}{s^2 + 1}</m></statement>
					<feedback>
						<p>No, this is incorrect. You are missing the initial condition terms on the left-hand side.</p>
					</feedback>
				</choice>
				<choice>
					<statement><m>Y = \frac{1}{s^2 + 1}</m></statement>
					<feedback>
						<p>No, this is incorrect. This only represents the transform of <m>t^2</m> and does not account for the left-hand side of the equation.</p>
					</feedback>
				</choice>
			</choices>
		</task>

	</exercise>
		
	</subsection>

	<objectives label="into-laplace-domain-wrapup">
		<ul>
			<li> 

			</li>
		</ul>
	</objectives>

	<fact label="into-laplace-domain-cyu">
		<statement>
			<p>
				Answer the following questions related to 

			</p>
		</statement>
	</fact>
</section>