<section label="out-of-laplace-domain">
	<title> Step 4: Out of the Laplace Domain </title>

	<introduction>

		<p>
			The heart of the Laplace transform method lies in its ability to convert a differential equation into an algebraic equation. This transformation takes place in what we call the <em>Laplace domain</em>, a mathematical space where derivatives become algebraic expressions and initial conditions are naturally incorporated into the equation.
		</p>

		<p>
			In this section, we will break down how to solve the model equation <xref ref="lt-model-eqn-w-ics"/>
			using the steps outlined in the <xref ref="lt-roadmap" text="custom">Laplace Transform Roadmap</xref>:
		</p>
			
		<ol marker="(i)">
			<li>
				<p>
					We begin with <xref ref="lt-roadmap-step-1" text="custom">step 1</xref>, where the forward transform moves the differential equation into the Laplace domain.
				</p>
			</li>
			<li>
				<p>
					Then, we jump to <xref ref="lt-roadmap-step-4" text="custom">step 4</xref> to explore how the transformed equation is converted back into the original domain using a backward transform.
				</p>
			</li>
			<li>
				<p>
					Finally, we examine <xref ref="lt-roadmap-step-2-3" text="custom">steps 2 and 3</xref>, which take place entirely within the Laplace domain and lead to the solution of the original equation.
				</p>
			</li>
		</ol>
		
	</introduction>

	<subsection><title> Out of the Laplace Domain (Backward Transform) </title>

		<reading-questions><title> üëÄ <em>Reading Preparation</em> </title>
			<p>
				Needs to be completed.
			</p>
		</reading-questions>

		<p>
			The forward Laplace transform guided us from differential equations into the simpler world of algebra. Now, it's time to complete our journey by returning home. The <q>backward Laplace transform</q>, or inverse transform, recovers our original solution <m>y(t)</m> from its algebraic counterpart in the Laplace domain. This critical step, represented by <m>\laplacesym^{-1}</m>, is the <xref ref="lt-roadmap" text="custom">final step of our roadmap</xref> and ties the entire process together neatly.
		</p>

		<!-- <assemblage xml:id="lt-roadmap-step-4"><title> Step 4 - Out of the Laplace Domain (Backward Transform) </title>
			<p>
				<sidebyside widths="39% 15% 46%" valign="top">
					<p>
						<md>
							<mrow>	\vphantom{M}													</mrow>
							<mrow>	\ub{y\vphantom{\frac{1}{s - 3}} = e^{3t} + 2e^{-3t} - 2e^{2t}}	</mrow>
						</md>
					</p>
					<p>
						<me>
							\os{\Large\text{4Ô∏è‚É£}}{\us{\large\text{backward}}{\os{\large\laplacesym^{-1}}{\longleftarrow}}}
						</me>
					</p>
					<p>
						<md>
							<mrow>	\vphantom{M}													</mrow>
							<mrow>	\small\ub{Y = \frac{1}{s - 3} + \frac{2}{s + 3} - \frac{2}{s - 2}}	</mrow>
						</md>
						<me>
							
						</me>
					</p>
				</sidebyside>
				<sidebyside widths="39% 15% 46%" valign="middle">
					<p>
						<me>
							\text{Solution}
						</me>
					</p>
					<p/>
					<p>
						<me>
							\text{Laplace Solution (prepared)}
						</me>
					</p>
				</sidebyside>
			</p>
		</assemblage> -->

		<p>
			<xref ref="lt-roadmap-step-4" text="title"/>
		</p>

		<subsubsection><title> Using the Table Laplace Transforms for Inverses </title>

			<p>
				The beauty of the Laplace transform table is that it not only simplifies forward transformations but also neatly provides the corresponding inverse transformations. To reverse the process, you simply match your Laplace solution <m>F(s)</m>, found on the right side of the table, to its inverse <m>f(t)</m>, appearing on the left. For example, <xref ref="lt-L2" text="custom">L<m>_2</m></xref> conveniently offers both:
			</p>

			<p>
				<sidebyside widths="10% 40% 10% 40%" valign="top">
					<p>
						Foward transform:
					</p>
					<p>
						<me>
							\lap{ e^{at} } = \frac{1}{s - a}
						</me>
					</p>
					<p>
						Backward transform:
					</p>
					<p>
						<me>
							\ilap{ \frac{1}{s - a} } = e^{at}
						</me>
					</p>
				</sidebyside>
			</p>

			<p>
				This matching approach is exactly how you'll exit the Laplace domain in step 4. Once you've simplified your algebraic solution <m>Y(s)</m> (step 3), finding its inverse becomes simply a matter of identifying the correct form from the table. Let's practice this with a few examples to sharpen our skills.
			</p>

			<example><title> Inverses using the Laplace Transform Table </title>
				<p>
					<statement>
						<p>
							Apply a backward transform (step 4) to convert each Laplace solution back into a function of <m>t</m>.
						</p>
						<p>
						<sidebyside widths="35% 65%">
							<p>
								<me>
									Y(s) = \frac{3}{s^2 + 9}
								</me>
							</p>
							<p>
								<solution>
									<p>
										This matches <xref ref="lt-L4" text="custom">L<m>_4</m></xref> with <m>b=3</m>. So,
										<md>
											<mrow>	\ilap{Y(s)}	\amp = \ilap{\frac{3}{s^2 + 9}}	</mrow>
											<mrow>	y(t)		\amp = \sin(3t)					</mrow>
										</md>.
									</p>
								</solution>
							</p>
						</sidebyside>
						</p>
						<p>
						<sidebyside widths="35% 65%">
							<p>
								<me>
									Q(s) = \frac{s - 2}{(s - 2)^2 + 16}
								</me>
							</p>
							<p>
								<solution>
									<p>
										This matches <xref ref="lt-L7" text="custom">L<m>_7</m></xref> with <m>a=2</m> and <m>b=4</m>. So,
										<md>
											<mrow>	\ilap{Q(s)}	\amp = \ilap{\frac{s - 2}{(s - 2)^2 + 16}}	</mrow>
											<mrow>	q(t)		\amp = e^{2t}\cos(4t)						</mrow>
										</md>.
									</p>
								</solution>
							</p>
						</sidebyside>
						</p>
						<p>
						<sidebyside widths="35% 65%">
							<p>
								<me>
									D(s) = \frac{24}{s^5}
								</me>
							</p>
							<p>
								<solution>
									<p>
										Noting that <m>24=4!</m> and using <xref ref="lt-L3" text="custom">L<m>_3</m></xref> with <m>n=4</m>, we get
										<md>
											<mrow>	\ilap{D(s)}	\amp = \ilap{\frac{4!}{s^5}}	</mrow>
											<mrow>	d(t)		\amp = t^4						</mrow>.
										</md>.
									</p>
								</solution>
							</p>
						</sidebyside>
						</p>
					</statement>
				</p>
			</example>

			<p>
				As you've seen, the inverse transform is straightforward when your solution directly matches a form in the Laplace transform table. In reality, though, you often need to make some clever adjustments before finding a perfect match. We'll explore those strategies in the next section.
			</p>
		
		</subsubsection>

		<subsubsection><title> Linearity of <m>\laplacesym^{-1}</m> </title>

			<p>
				Usually, the Laplace solution you're trying to invert isn't just one simple term; it's composed of multiple pieces. Fortunately, like the forward transform, the inverse Laplace transform is also linear. This means that inverse transforms of sums and constant multiples of functions can be broken down into smaller, more manageable steps.
			</p>

			<assemblage xml:id="lt-inverse-linearity"><title> Linearity of the Inverse Laplace Transform </title>
				<p>
					Suppose <m>f(s)</m> and <m>g(s)</m> are functions in the Laplace domain, and <m>a</m> and <m>b</m> are constants. Then we have:
					<me>
						\ilap{ af(s) \pm bg(s) } = a\ilap{ f(s) } \pm b\ilap{ g(s) }
					</me>
				</p>
			</assemblage>

			<p>
				Let's walk through an example to illustrate how this linearity property streamlines the backward transformation.
			</p>

			<example><title> Inverse Transforms using Linearity </title>
				<p>
					<statement>
						<p>
							Apply a backward transform (step 4) to revert each Laplace solution back into a function of <m>t</m>.
							<ol>
								<li>
									<p>
										<m>\ds Y(s) = \frac{12}{s} + \frac{7s}{s^2 + 25} </m>
									</p>
								</li>
								<li>
									<p>
										<m>\ds Y(s) = \frac{4}{(s - 2)^2 + 16} + \frac{2}{(s+7)^5}</m>
									</p>
								</li>
							</ol>
						</p>
					</statement>
				</p>
				<p>
					<solution>
						<p>
							The <m>s</m> in the denominator tells us that we need <m>L_1</m>. Before we do, let's factor out <m>12</m>:
							<me>\ds \ilap{\frac{12}{s}} = 12 \cdot \ilap{\frac{1}{s}} = 12 \cdot 1 = 12</me>.
						</p>
						<p>
							<me><xref ref="lt-L5" text="custom">L_5</xref>, b=5</me>
							<me> \ilap{\frac{7s}{s^2 + 25}} = 7\ \ilap{\frac{s}{s^2 + 25}} = 7\ \cos(5t)</me>
						</p>
					</solution>

					<solution>
						<p>
							The form of this denominator is <m>\ul{(s \pm \text{shift})^{2} + \text{number}}</m> and has no <m>s</m> in the numerator. Therefore,
							<md>
								<mrow> \ilap{\frac{10}{(s - 3)^2 + 11}} \amp\ \quad <xref ref="lt-L7" text="custom"><m>L_7</m></xref> (a=3,\ b=\sqrt{11})</mrow>
								<mrow>	\amp = 10\ \ilap{\frac{\sqrt{11}}{\sqrt{11}}\frac{1}{(s - 3)^2 + 11}}</mrow>
								<mrow>	\amp = \frac{10}{\sqrt{11}} \ilap{\frac{\sqrt{11}}{(s - 3)^2 + 11}}</mrow>
								<mrow>	\amp = \frac{10}{\sqrt{11}} e^{3t} \sin(\sqrt{11}t)</mrow>
							</md>

						</p>
						<p>
							The denominator, <m>\ul{(s \pm \text{shift})^{\text{power}}}</m>, indicates an <m>e^{at}</m> and a <m>t^n</m> term. Therefore,
							<md>
								<mrow> \ilap{\frac{2}{(s+7)^5}} \amp\ \quad <xref ref="lt-L6" text="custom"><m>L_6</m></xref> (a=-7, n=4)</mrow>
								<mrow>
										\amp = 2\ \ilap{\frac{4!}{4!}\frac{1}{(s+7)^5}}
								</mrow>
								<mrow>
										\amp = \frac{2}{4!} \ilap{\frac{4!}{(s+7)^5}}
								</mrow>
								<mrow>
									\amp = \frac{1}{12} t^4 e^{-7t}
							</mrow>
							</md>
						</p>
					</solution>
				</p>
			</example>

			<p>
				By leveraging linearity, we've simplified what initially appeared as complicated inverses into straightforward, table-based solutions. As you become more comfortable with this approach, you'll find inverse transformations much quicker and easier. However, sometimes we'll still need a bit more strategy, which we'll explore in the next section.
			</p>

		</subsubsection>

		<subsubsection><title> Minor Adjustments for a Perfect Match </title>

			<p> 
				Often, the Laplace solution you need to invert won't exactly match a form from the transform table right away. However, if the denominator matches, you're usually only a few minor adjustments away from a perfect match. These small tweaks usually involve adding a missing constant or splitting the fraction to align the numerator with the forms in the Laplace transform table.
			</p>

			<p> 
				Let's illustrate this with an example. Consider the Laplace solution: 
			</p>

			<me>
				Y(s) = \frac{2s + 3}{s^2 + 4}
			</me>.
			
			<p>
				Notice that the denominator, <m>s^2 + 4</m>, matches the denominator in both <xref ref="lt-L4" text="custom">L<m>_4</m></xref> or <xref ref="lt-L5" text="custom">L<m>_5</m></xref>. However, the numerator has two distinct terms. To clearly align this with the table, we split the fraction into two simpler fractions:
			</p>

			<me>
				Y(s) = \frac{2s}{s^2 + 4} + \frac{3}{s^2 + 4}
			</me>.

			<p>
				Then factor constants and reassess how they match with the table.
			</p>

			<me>
				Y(s) 
				= 2\ub{\frac{s}{s^2 + 4}}_{\large<xref ref="lt-L5" text="custom">L_5</xref>\text{ perfect}} 
				+ 3\ub{\frac{1}{s^2 + 4}}_{\large<xref ref="lt-L4" text="custom">L_4</xref>\text{ close}}
			</me>.

			<p> 
				The first term now perfectly matches <xref ref="lt-L5" text="custom">L<m>_5</m></xref> (with <m>b=2</m>). The second term, however, needs a <m>2</m> in its numerator to match <xref ref="lt-L4" text="custom">L<m>_4</m></xref>. To make this small adjustment, we multiply by <m>\sfrac{2}{2}</m>, a form of multiplying by 1:
			</p>

			<aside><title> Multiplying by <m>\sfrac{2}{2}</m> </title>
				<p>
					Multiplying by <m>\sfrac{2}{2}</m> is just multiplying by 1, preserving the original value. It's a useful technique for adjusting numerators without altering the equation.
				</p>
			</aside>

			<md>
				<mrow>	
					Y(s) \amp = 2\frac{s}{s^2 + 4} + 3\frac{1}{s^2 + 4} \cdot \frac{2}{2}
				</mrow>
				<mrow>	
					Y(s)	
					\amp = 2\ub{\frac{s}{s^2 + 4}}_{\large<xref ref="lt-L5" text="custom">L<m>_5</m></xref>\text{ perfect}} 
					+ \frac{3}{2}\ub{\frac{2}{s^2 + 4}}_{\large<xref ref="lt-L4" text="custom">L<m>_4</m></xref>\text{ perfect}}
				</mrow>
			</md>.

			<p>
				With these minor adjustments, the inverse transform becomes straightforward:
				<md>
					<mrow>	
						\ilap{Y(s)} = 2\ilap{\frac{s}{s^2 + 4}} + \frac{3}{2}\ilap{\frac{2}{s^2 + 4}}
					</mrow>
					<mrow>	
						y(t) = 2\cos(2t) + \frac{3}{2}\sin(2t)
					</mrow>
				</md>.
			</p>

			<p>
				Mastering these small algebraic manipulations simplifies your workflow considerably. Let's examine another example to reinforce this process:
			</p>
			
			<example><title> MAdjusting Laplace Solutions (Fraction Splitting) </title>
				<p>
					<statement>
						<p>
							Apply a backward transform (step 4) to revert the Laplace solution back into a function of <m>t</m>.
						</p>
						<p>
							<me>
								Y(s) = \frac{s^6 - 7s^3}{s^7}
							</me>
						</p>
					</statement>
				</p>

				<solution>
					<p>
						Since the denominator of <m>Y</m> already matches the form of the denominator in <xref ref="lt-L3" text="custom">L<m>_3</m></xref>, we split the fraction and simplify:
						
						<me>
							Y(s) = \frac{s^6}{s^7} - \frac{7s^3}{s^7} = \frac{1}{s} - 7\frac{1}{s^4}
						</me>.
					</p>

					<p>
						The first term matches <xref ref="lt-L1" text="custom">L<m>_1</m></xref> and the second term needs <m>3!</m> in the numerator to match <xref ref="lt-L3" text="custom">L<m>_3</m></xref>. So, updating the second term gives us
						<me>
							Y(s) = \frac{1}{s} - \frac{7}{3!}\frac{3!}{s^4}
						</me>.
					</p>
					<p>
						Now it is ready for the backward transform:
						<md>
							<mrow>	\ilap{Y(s)}	\amp = \ilap{\frac{1}{s}} - \frac{7}{3!}\ilap{\frac{3!}{s^4}}	</mrow>
							<mrow>	y(t)		\amp = 1 - \frac{7}{3!}t^3										</mrow>
						</md>
					</p>
				</solution>
			</example>

			<p>
				Another frequent adjustment is needed when dealing with forms like <xref ref="lt-L8" text="custom">L<m>_8</m></xref>. Consider the Laplace solution:
			</p>

			<me>
				Y(s) = \frac{s + c}{(s-a)^2 + b^2}
			</me>.

			<p>
				To match this form precisely, we need the numerator to have an explicit <m>(s - a)</m>. To achieve this, add and subtract <m>a</m> in the numerator:
			</p>

			<me>
				Y(s) = \frac{s - a + a + c}{(s-a)^2 + b^2}
			</me>.

			<aside><title> Adding and Subtracting <m>a</m></title>
				<p> 
					Adding and subtracting the same number does not change the value of the expression, but it is a useful trick for adjusting numerators into recognizable forms.
				</p>
			</aside>

			<p>
				Now split the fraction and note that <m>a+c</m> is just a number:
			</p>

			<me>
				Y(s) = \frac{s-a}{(s-a)^2 + b^2} + \frac{a + c}{(s-a)^2 + b^2}
			</me>.

			<p>
				The second term still needs a <m>b</m> in the numerator to match perfectly, so we multiply by <m>\sfrac{b}{b}</m>:
			</p>

			<me>
				Y(s) 
				= \ub{\frac{s-a}{(s-a)^2 + b^2}}_{\large\text{matches } <xref ref="lt-L8" text="custom">L_8</xref>} 
				+ \frac{a+c}{b}\ub{\frac{b}{(s-a)^2 + b^2}}_{\large\text{matches } <xref ref="lt-L7" text="custom">L_7</xref>}
			</me>.

			<p> 
				With this form, the inverse transform gives us
			</p>

			<me>
				y(t) = \cos(bt) + \frac{a+c}{b}\sin(bt)
			</me>.

			<example><title> Further Adjustments of Laplace Solutions </title>
				<p>
					<statement>
						<p>
							Apply a backward transform (step 4) to revert each Laplace solution back into a function of <m>t</m>.
							<ol>
								<li>
									<p>
										<m>\ds Y(s) = \frac{s - 5}{(s+4)^2 + 6}</m>
									</p>
								</li>
								<li>
									<p>
										<m>\ds Y(s) = \frac{3s + 9}{(s-2)^2 + 16}</m>
									</p>
								</li>
							</ol>
						</p>
					</statement>
				</p>
				
				<p>
					<solution>
						<p>
							Noticing that the first term needs <m>s+4</m> in the numerator, we add and subtract <m>4</m> to the numerator, then split the fraction:
						</p>
						<md>
							<mrow>	Y(s)	\amp = \frac{s + 4 - 4 - 5}{(s+4)^2 + 6}	</mrow>
							<mrow>	\amp = \frac{s + 4}{(s+4)^2 + 6} - 9\frac{1}{(s+4)^2 + 6}	</mrow>
						</md>
						<p>
							The first term matches with <xref ref="lt-L8" text="custom">L<m>_8</m></xref>, but the second term needs a <m>\sqrt{6}</m> in the numerator:
						</p>

						<me>
							Y(s)	
							= \ub{\frac{s + 4}{(s+4)^2 + 6}}_{\large\text{matches } <xref ref="lt-L8" text="custom">L_8</xref>} 
							- \ub{\frac{9}{\sqrt{6}}\frac{\sqrt{6}}{(s+4)^2 + 6}}_{\large\text{matches } <xref ref="lt-L7" text="custom">L_7</xref>}
						</me>
						<p>
							Now we have a form ready for the inverse Laplace transform:
						</p>
						<md>
							<mrow>	y(t)	\amp = e^{-4t}\cos(\sqrt{6}t) - \frac{9}{\sqrt{6}}e^{-4t}\sin(\sqrt{6}t)	</mrow>
						</md>.
					</solution>

					<solution>
						<p>
							The first term needs <m>s-2</m> in the numerator, but before adding and subtracting <m>2</m>, lets get <m>3</m> out of the way by factoring it out: 
						</p>

						<md>
							<mrow>	Y(s) = 3\frac{s + 3}{(s-2)^2 + 16}	\amp = 3\left(\frac{s - 2 + 2 + 3}{(s-2)^2 + 16}\right)	</mrow>
						</md>.

						<p>
							Now, splitting the fraction inside the parentheses and distributing the <m>3</m> gives us
						</p>

						<md>
							<mrow>	
								Y(s)
								\amp = 3\left(\frac{s - 2}{(s-2)^2 + 16} + \frac{5}{(s-2)^2 + 16}\right)
							</mrow>
							<mrow>
								\amp = 3\frac{s - 2}{(s-2)^2 + 16} + 15\frac{1}{(s-2)^2 + 16}
							</mrow>
							<mrow>
								\amp = 3\ub{\frac{s - 2}{(s-2)^2 + 16}}_{\large\text{matches } <xref ref="lt-L8" text="custom">L<m>_8</m></xref>}
								+ \frac{15}{4}\ub{\frac{4}{(s-2)^2 + 16}}_{\large\text{matches } <xref ref="lt-L7" text="custom">L<m>_7</m></xref>}
							</mrow>
						</md>.

						<p>
							Finally, the backward transform is given by
						</p>

						<md>
							<mrow>	y(t)	\amp = 3e^{2t}\cos(4t) + \frac{15}{4}e^{2t}\sin(4t)	</mrow>
						</md>.
					</solution>
				</p>
					
			</example>

			<p>
				With practice, these small adjustments become intuitive, greatly simplifying the process of moving back from the Laplace domain to your original solutions.
			</p>

		</subsubsection>

	<exercise label="chkpts-mis-matched-forms"><title> <em>Answer-the-Following</em> </title>

		<introduction>
			<p>
				Complete the questions on each tab to check your understanding.
			</p>
		</introduction>

		<task label="p4-c2-s1-2-rq1"><title> <em>The most challenging part of the Laplace transform method is preparing the <m>s</m>-function for the backward Laplace transform</em> </title>
			<statement correct="yes">
				<p>
					The most challenging part of the Laplace transform method is preparing the <m>s</m>-function for the backward Laplace transform
				</p>
			</statement>
			<feedback>
				<p>
					True. Preparing the s-function to match a known form in the backward Laplace transform table can be the most challenging step in the Laplace transform method.
				</p>
			</feedback>
		</task>
		
		<task label="p4-c2-s1-2-rq2"><title> <em><m>\ds\quad \ilap{\frac{7}{s^2}} = </m> <fillin characters="15"/></em> </title>
			<statement>
				<p>
					<em><m>\ds\quad \ilap{\frac{7}{s^2}} = </m> <fillin characters="15"/></em>
				</p>
			</statement>
			<choices randomize="yes">
				<choice>
					<statement><m>\ds\frac{t}{7}</m></statement>
					<feedback>
						<p>
							Incorrect.
						</p>
					</feedback>
				</choice>
				<choice>
					<statement><m>7t^2</m></statement>
					<feedback>
						<p>
							Incorrect.
						</p>
					</feedback>
				</choice>
				<choice correct="yes">
					<statement><m>7t</m></statement>
					<feedback>
						<p>
							Correct!
						</p>
					</feedback>
				</choice>
				<choice>
					<statement><m>\ds\frac{7}{t}</m></statement>
					<feedback>
						<p>
							Incorrect.
						</p>
					</feedback>
				</choice>
			</choices>
		</task>
		
		<task label="p4-c2-s1-2-rq3"><title> <em>Fill-in-the-blank. <m>\ds\quad \ilap{\frac{5}{s^4}} = \frac{5}{6}\ilap{\frac{<fillin characters="1"/>}{s^4}} </m></em> </title>
			<statement>
				<p>
					<em>Fill-in-the-blank. <m>\ds\quad \ilap{\frac{5}{s^4}} = \frac{5}{6}\ilap{\frac{<fillin characters="1"/>}{s^4}} </m></em>
				</p>
			</statement>
			<choices randomize="yes">
				<choice>
					<statement><m>9</m></statement>
					<feedback>
						<p>
							Incorrect.
						</p>
					</feedback>
				</choice>
				<choice>
					<statement><m>3</m></statement>
					<feedback>
						<p>
							Incorrect.
						</p>
					</feedback>
				</choice>
				<choice>
					<statement><m>4!</m></statement>
					<feedback>
						<p>
							Incorrect.
						</p>
					</feedback>
				</choice>
				<choice correct="yes">
					<statement><m>3!</m></statement>
					<feedback>
						<p>
							Correct!
						</p>
					</feedback>
				</choice>
			</choices>
		</task>
		
		<task label="p4-c2-s1-2-rq4"><title> <em>Which of the following <m>s</m>-functions require adjustment to match one of the common inverse Laplace transforms?</em> </title>
			<statement>
				<p>
					<em>Which of the following <m>s</m>-functions require adjustment to match one of the common inverse Laplace transforms?</em>
				</p>
			</statement>
			<choices randomize="yes">
				<choice>
					<statement><m>\ds\frac{s}{s^2 + 16}</m></statement>
					<feedback>
						<p>
							Incorrect. This function already matches a known cosine form and does not require any missing constants.
						</p>
					</feedback>
				</choice>
				<choice correct="yes">
					<statement><m>\ds\frac{8}{s^2 + 16}</m></statement>
					<feedback>
						<p>
							Correct! This function would require a missing constant adjustment to match the sine form, with the numerator needing to be <m>4</m>.
						</p>
					</feedback>
				</choice>
				<choice>
					<statement><m>\ds\frac{s - 3}{(s - 3)^2 + 25}</m></statement>
					<feedback>
						<p>
							Incorrect. This function already matches a known form and does not require any missing constants.
						</p>
					</feedback>
				</choice>
			</choices>
		</task>
		
		<task label="p4-c2-s1-2-rq5"><title> <em><m>\ds\quad \ilap{\frac{10}{(s - 2)^2 + 25}} = </m> <fillin characters="15"/></em> </title>
			<statement>
				<p>
					<em><m>\ds\quad \ilap{\frac{10}{(s - 2)^2 + 25}} = </m> <fillin characters="15"/></em>
				</p>
			</statement>
			<choices randomize="yes">
				<choice correct="yes">
					<statement><m>2e^{2t}\sin(5t)</m></statement>
					<feedback>
						<p>
							Correct! Factoring out <m>10</m> and placing the missing constant gives the correct form: <m>2e^{2t}\sin(5t)</m>.
						</p>
					</feedback>
				</choice>
				<choice>
					<statement><m>5e^{2t}\sin(5t)</m></statement>
					<feedback>
						<p>
							Incorrect. The correct answer requires factoring and rebalancing, giving <m>2e^{2t}\sin(5t)</m>.
						</p>
					</feedback>
				</choice>
				<choice>
					<statement><m>e^{2t}\cos(5t)</m></statement>
					<feedback>
						<p>
							Incorrect. The sine form, not cosine, matches this function.
						</p>
					</feedback>
				</choice>
			</choices>
		</task>

		<task label="p4-c2-s1-2-rq6"><title> <em>Fill-in-the-blank. <m>\ds\quad \ilap{\frac{10}{s^2 + 25}} = \frac{<fillin characters="1"/>}{5}\ilap{\frac{5}{s^2 + 25}} </m></em> </title>
			<statement>
				<p>
					<em>Fill-in-the-blank. <m>\ds\quad \ilap{\frac{10}{s^2 + 25}} = \frac{<fillin characters="1"/>}{5}\ilap{\frac{5}{s^2 + 25}} </m></em>
				</p>
			</statement>
			<choices randomize="yes">
				<choice correct="yes">
					<statement><m>10</m></statement>
					<feedback>
						<p>
							Correct!
						</p>
					</feedback>
				</choice>
				<choice>
					<statement><m>5</m></statement>
					<feedback>
						<p>
							Incorrect.
						</p>
					</feedback>
				</choice>
				<choice>
					<statement><m>2</m></statement>
					<feedback>
						<p>
							Incorrect.
						</p>
					</feedback>
				</choice>
				<choice>
					<statement><m>1</m></statement>
					<feedback>
						<p>
							Incorrect.
						</p>
					</feedback>
				</choice>
			</choices>
		</task>

	</exercise>

	</subsection>

	<objectives label="out-of-laplace-domain-wrapup">
		<ul>
			<li> 

			</li>
		</ul>
	</objectives>

	<fact label="out-of-laplace-domain-cyu">
		<statement>
			<p>
				Answer the following questions related to 

			</p>
		</statement>
	</fact>
</section>