<section><title> Abandoned Content</title>

	<p>
		This chapter contains content that was abandoned during the development of the book. It is not part of the final version.
	</p>

	<figure xml:id="lt-roadmap-step-1-fig">
		<caption>
			To enter the Laplace domain (step 1), we apply a forward transform (<m>\laplacesym</m>) to the original differential equation.
		</caption>
		<image source="figures/lt-roadmap-step-1.png" width="100%"/>
	</figure>

	<figure xml:id="lt-roadmap-step-3-fig">
		<caption>
			To leave the Laplace domain (step 4), we apply a backward transform (<m>\laplacesym^{-1}</m>) to the Laplace solution for <m>Y</m>.
		</caption>
		<image source="figures/lt-roadmap-step-3.png" width="100%"/>
	</figure>

	<assemblage xml:id="lt-roadmap-full"><title> Laplace Method Roadmap </title>
		<p>
			<sidebyside widths="38% 12% 50%" valign="middle">
				<p>
					<md>
						<mrow>	y'' - 9y = 10e^{2t}	</mrow>
						<mrow>	y(0) = 1, \quad y(0) = -7	</mrow>
					</md>
				</p>
				<p><me>\os{\Large\text{1️⃣}}{\us{\large\text{forward}}{\os{\large\laplacesym}{\longrightarrow}}}</me></p>
				<p>
					<me>
						s^2Y - 9Y - s + 7 = \frac{10}{s - 2}
					</me>
				</p>
			</sidebyside>
			<sidebyside widths="60% 10% 30%" valign="middle">
				<p/>
				<p><me>\downarrow</me></p>
				<p>
					2️⃣ Solve for <m>Y</m>
				</p>
			</sidebyside>
		</p>
		<p>
			<sidebyside widths="40% 10% 50%" valign="middle">
				<p/>
				<p/>
				<p>
					<me>
						Y = \frac{1}{s^2 - 9}\left( \frac{10}{s - 2} + s - 7 \right)
					</me>
				</p>
			</sidebyside>
		</p>
		<p>
			<sidebyside widths="60% 10% 30%" valign="middle">
				<p/>
				<p><me>\downarrow</me></p>
				<p>
					3️⃣ Prepare for <m>\laplacesym^{-1}</m>
				</p>
			</sidebyside>
			<sidebyside widths="38% 12% 50%" valign="middle">
				<p>
					<me>
						y = e^{3t} + 2e^{-3t} - 2e^{2t}
					</me>
				</p>
				<p><me>\os{\Large\text{4️⃣}}{\us{\large\text{backward}}{\os{\large\laplacesym^{-1}}{\longleftarrow}}}</me></p>
				<p>
					<me>
						Y = \frac{1}{s - 3} + \frac{2}{s + 3} - \frac{2}{s - 2}
					</me>
				</p>
			</sidebyside>
		</p>
	</assemblage>

	<assemblage xml:id="llt-roadmap-step-1"><title> Step 1 - Into the Laplace Domain (Forward Transform) </title>
		<p>
			<sidebyside widths="39% 14% 47%" valign="middle">
				<p>
					<md>
						<mrow>	y'' - 9y = 10e^{2t}				</mrow>
						<mrow>	\ub{y(0) = 1, \quad y(0) = -7}	</mrow>
					</md>
				</p>
				<p>
					<md>
						<mrow>	\os{\Large\text{1️⃣}}{\us{\large\text{forward}}{\os{\large\laplacesym}{\longrightarrow}}}	</mrow>
						<mrow>	\vphantom{\sum}																				</mrow>
					</md>
				</p>
				<p>
					<me>
						\ub{s^2Y - 9Y - s + 7 = \frac{10}{s - 2}}
					</me>
				</p>
			</sidebyside>
			<sidebyside widths="41% 12% 47%" valign="middle">
				<p>
					<me>
						\text{Differential Equation}
					</me>
				</p>
				<p/>
				<p>
					<me>
						\text{Laplace Equation}
					</me>
				</p>
			</sidebyside>
		</p>
	</assemblage>

	<assemblage xml:id="llt-roadmap-step-2"><title> Step 2 - Solve for <m>Y</m> </title>
		<p>
			<sidebyside widths="47% 3% 50%" valign="middle">
				<p>
					Isolate <m>Y</m> in the Laplace Equation to get the Laplace Solution.
				</p>
				<p/>
				<p>
					<me>
						s^2Y - 9Y - s + 7 = \frac{10}{s - 2}
					</me>
				</p>
			</sidebyside>
		</p>
		<p>
			<sidebyside widths="60% 10% 30%" valign="middle">
				<p/>
				<p><me>\downarrow</me></p>
				<p>
					2️⃣ Solve for <m>Y</m>
				</p>
			</sidebyside>
		</p>
		<p>
			<sidebyside widths="43% 7% 50%" valign="middle">
				<p>
					<me>
						\qquad\quad\text{Laplace Solution}
					</me>
				</p>
				<p>
					<me>
						\longrightarrow
					</me>
				</p>
				<p>
					<me>
						Y = \frac{1}{s^2 - 9}\left( \frac{10}{s - 2} + s - 7 \right)
					</me>
				</p>
			</sidebyside>
		</p>
	</assemblage>

	<assemblage xml:id="llt-roadmap-step-2"><title> Step 3 - Prepare for <m>\laplacesym^{-1}</m> </title>
		<p>
			<sidebyside widths="46% 6% 48%" valign="middle">
				<p>
					Prepare the Laplace solution for the backward transform so that the terms of Laplace solution resemble the right column of the transform table. This often requires partial fraction decomposition and/or completing the square.
				</p>
				<p/>
				<p>
					<md>
						<mrow>	Y = \frac{1}{s^2 - 9}\left( \frac{10}{s - 2} + s - 7 \right) </mrow>
						<mrow> \quad </mrow>
						<mrow>	\downarrow\quad\text{3️⃣ Prepare for } \laplacesym^{-1} </mrow>
						<mrow> \quad </mrow>
						<mrow>	Y = \frac{1}{s - 3} + \frac{2}{s + 3} - \frac{2}{s - 2} </mrow>
					</md>
				</p>
			</sidebyside>
		</p>
	</assemblage>

	<assemblage xml:id="llt-roadmap-step-2"><title> Steps 2 &amp; 3 - Solve for <m>Y</m> &amp; Prepare for <m>\laplacesym^{-1}</m> </title>
		<p>
			<sidebyside widths="4% 28% 12% 56%" valign="middle">
				<p/>
				<p>
					Laplace Equation
				</p>
				<p>
					<me>
						\longrightarrow
					</me>
				</p>
				<p>
					<me>
						s^2Y - 9Y - s + 7 = \frac{10}{s - 2}
					</me>
				</p>
			</sidebyside>
		</p>
		<p>
			<sidebyside widths="55% 10% 35%" valign="middle">
				<p/>
				<p><me>\downarrow</me></p>
				<p>
					2️⃣ Solve for <m>Y</m>
				</p>
			</sidebyside>
		</p>
		<p>
			<sidebyside widths="4% 28% 12% 56%" valign="middle">
				<p/>
				<p>
					Laplace Solution
				</p>
				<p>
					<me>
						\longrightarrow
					</me>
				</p>
				<p>
					<me>
						Y = \frac{1}{s^2 - 9}\left( \frac{10}{s - 2} + s - 7 \right)
					</me>
				</p>
			</sidebyside>
		</p>
		<p>
			<sidebyside widths="55% 10% 35%" valign="middle">
				<p/>
				<p><me>\downarrow</me></p>
				<p>
					3️⃣ Prepare for <m>\laplacesym^{-1}</m>
				</p>
			</sidebyside>
		</p>
		<p>
			<sidebyside widths="4% 28% 12% 56%" valign="middle">
				<p/>
				<p>
					Laplace Solution (prepared)
				</p>
				<p>
					<me>
						\longrightarrow
					</me>
				</p>
				<p>
					<me>
						Y = \frac{1}{s - 3} + \frac{2}{s + 3} - \frac{2}{s - 2}
					</me>
				</p>
			</sidebyside>
		</p>
	</assemblage>

	<assemblage xml:id="llt-roadmap-step-3"><title> Step 4 - Out of the Laplace Domain (Backward Transform) </title>
		<p>
			<sidebyside widths="39% 15% 46%" valign="top">
				<p>
					<md>
						<mrow>	\vphantom{M}													</mrow>
						<mrow>	\ub{y\vphantom{\frac{1}{s - 3}} = e^{3t} + 2e^{-3t} - 2e^{2t}}	</mrow>
					</md>
				</p>
				<p>
					<me>
						\os{\Large\text{4️⃣}}{\us{\large\text{backward}}{\os{\large\laplacesym^{-1}}{\longleftarrow}}}
					</me>
				</p>
				<p>
					<md>
						<mrow>	\vphantom{M}													</mrow>
						<mrow>	\small\ub{Y = \frac{1}{s - 3} + \frac{2}{s + 3} - \frac{2}{s - 2}}	</mrow>
					</md>
					<me>
						
					</me>
				</p>
			</sidebyside>
			<sidebyside widths="39% 15% 46%" valign="middle">
				<p>
					<me>
						\text{Solution}
					</me>
				</p>
				<p/>
				<p>
					<me>
						\text{Laplace Solution (prepared)}
					</me>
				</p>
			</sidebyside>
		</p>
	</assemblage>

	<subsection xml:id="lt-motivation">
		<title> Why Use the Laplace Transform? </title>
		<p>
			<em>Note: The following discussion attempts to motivate the Laplace transform. For clarity, we have omitted some details that we will address later.</em>
		</p>

		<p>
			To see where we're headed, imagine you need to solve the differential equation
			<me>
				y'(t) - 9y(t) = 10 e^{2t}.
			</me>
		</p>

		<p>
			Suppose you multiply both sides by <m>e^{-st}</m> and integrate with respect to <m>t</m>:
			<me>
				\int \left[y'(t) - 9y(t)\right] e^{-st} \, dt = \int 10 e^{2t} e^{-st} \, dt.
			</me>
		</p>

		<p>
			Distributing <m>e^{-st}</m> and separating the integrals, we can rewrite this as:
			<me>
				\int e^{-st} y'(t)\ dt - 9\int e^{-st} y(t)\ dt = \int e^{-st} \left( 10e^{2t} \right)\ dt.
			</me>
		</p>

		<p>
			From the previous section, you know we can transfer the derivative from <m>y'</m> to <m>e^{-st}</m>. Doing so gives something like:
			<me>
				\text{constant} + s\us{\large\text{set as}\ Y}{\ul{\int e^{-st} y(t)\ dt}} - 9\us{\large\text{set as}\ Y}{\ul{\int e^{-st} y(t)\ dt}} = \us{\large\text{function of}\ s}{\ul{\int e^{-st} \left( 10e^{2t} \right)\ dt}}
			</me>
			where the constant comes from the limits of integration. Letting <m>Y</m> be the common integral on the left and integrating with respect to <m>t</m> (treating <m>s</m> constant) on the right:
		</p>

		<me>
			\text{constant} + Y - 9Y = \text{function of } s
		</me>.

		<p>
			From here you can isolate <m>Y</m> on one side of the equation using algebra, but <m>y(t)</m> (i.e., the solution) is hiding inside <m>Y</m>. Luckily, applying an inverse will <q>release</q> <m>y(t)</m> from <m>Y</m> and giving us our solution at the same time.
		</p>	
	</subsection>
</section>