<subsection xmlns:xi="http://www.w3.org/2001/XInclude"><title> Initial Conditions &amp; Particular Solutions </title>
	
	<p>
		Solving a differential equation typically starts with finding the general solution that defines all the possible solutions (family of solutions). However, for a real-world problem, we make assumptions about the solution that help us isolate a <em>particular solution</em> from this family of solutions. This is where initial conditions come in.
	</p>

	<p>
		An <term>initial condition</term> is a starting value of the solution (i.e., dependent variable) or its derivatives. For example, consider the free fall of an object due to gravity. If <m>s(t)</m> is the position (distance from the ground) of this object at time <m>t</m>. Assuming the ball is dropped from the top of a 100 ft building, what initial information do you know? That is, what are the initial conditions? 
	</p>

	<p>
		Since we know the starting with a position of a 100 ft and starting velocity of zero, we can write the initial conditions as
		<me>
			s(0) = 100 \text{ ft} \quad \text{and} \quad s'(0) = 0 \text{ ft/s}.
		</me>
	</p>

	<p>
		Such conditions allow us to pinpoint one specific solution from the infinite set of possible solutions to a differential equation. When a differential equation includes an initial condition, it forms what is called an <term>initial value problem (IVP)</term>. The following example illustrates what an IVP looks like.
	</p>

	<!-- <example>

		<m>\quad</m> Consider the free fall of an object due to gravity. If <m>s(t)</m> is the position (distance from the ground) of this object at time <m>t</m> and since acceleration is the second derivative of position, we get the differential equation
		<me>
			\text{acceleration of object} \rightarrow \quad s''(t) = -32 \text{ ft/s}^2.
		</me>
		Assuming the ball is dropped from the top of a 100 ft building, what initial information do you know? That is, what are the initial conditions?

		<solution>
			<p>
				
			</p>
		</solution>
	</example> -->

	<example>

		<m>\quad</m> Solve the differential equation <me>\frac{dy}{dx} = 2xy - 6x</me> given the initial condition <m>y(0) = 0</m>.

		<solution>
			<p>
				The first step is to find the general solution to the differential equation. The general solution is 
				<me>y = Ce^{x^2} + 3.</me>
			</p>
			<p>
				To find the particular solution that satisfies the initial condition, substitute <m>x = 0</m> and <m>y = 0</m> into the general solution:
			</p>
			<md>
				<mrow>y = Ce^{x^2} + 3 \quad \Rightarrow \quad 0 = C \cdot e^{0^2} + 3</mrow>
				<mrow>0 = C + 3</mrow>
				<mrow>C = -3</mrow>
			</md>
			<p>
				Therefore, the particular solution that satisfies the initial condition is 
				<me>y = -3e^{x^2} + 3.</me>
			</p>
		</solution>
	</example>

	<example>

		<m>\quad</m> Suppose we want the solution to the differential equation 
		<me> \displaystyle \frac{dy}{dt} = 2ty - 6t, \quad y(0) = 2 </me>.

		<solution>
			<p>
				Etcept for the initial condition, this is the same equation we solved in the previous section, which has the general solution 
				<men xml:id="example-general-solution">y = ce^{t^2} + 3</men>. 
				The initial condition, <m>y(0) = 2</m>, tells us that "<m>y</m> must equal 2 when <m>t</m> is 0". When we substitute <m>y=2</m> and <m>t=0</m> into <xref ref="example-general-solution" />, we see that we can solve for <m>c</m>.
				<md>
					<mrow> y =  ce^{t^2} + 3 \quad \overset{y\ =\ 2,\ t\ =\ 0}{\Rightarrow} \quad	2	=\amp\  ce^{0^2} + 3	</mrow>
					<mrow>							 												2	=\amp\  c + 3		</mrow>
					<mrow>																			-1	=\amp\  c			</mrow>
				</md>
			</p>
		
			<p>
				Therefore, <m>y(0) = 2</m> forces <m>c = -1</m> and we get the particular solution
				<me>y = -e^{t^2} + 3</me>.
			</p>
		</solution>
	</example>

	<p>
		In <xref ref="initial-conditions-figure-1" /> can see the initial condition, <m>y(0) = 2</m>, as the point <m>(0,2)</m> on the <m>y</m>-axis. The blue curve is the particular solution we found above and is the only solution in the family that passes through this point.
	</p>

	<sidebyside widths="46% 2% 50%" margins="0%">
		<stack>
		<p>
			In the graph, the point on the <m>y</m>-axis is the initial condition. You can change the initial condition by dragging the point up and down along the <m>y</m>-axis.
		</p>

		<p>
			As you drag the point, make the following observations:
		</p>

		<ul marker="square">
			<li> 
			Each new value of <m>y(0)</m> gives a new value of <m>c</m>, which corresponds to a new particular solution (blue curve). 
			</li>
			<li> 
			Only one particular solution from the family of solutions (green curves) passes through the initial condition.  
			</li>
		</ul>
		</stack>
		<p />
		<figure xml:id="initial-conditions-figure-1">
		<interactive xml:id="interactive-drag-ic" platform="jsxgraph" source="code/initial-condition.js">
			<slate xml:id="interactive-drag-ic-slate" surface="jsxboard" />
			
		</interactive>
		<caption>The family of solutions (green curves) and a particular solution (blue curve) passing through <m>y(0)</m>.</caption>
		</figure>
	</sidebyside>

	<example>

		<m>\quad</m> Solve the differential equation <m>\ \frac{dy}{dx} = 2xy - 6x. </m>

		<solution>

		<p>
			The general solution to this differential equation is
			<me> y = Ce^{x^2} + 3. </me>
		</p>

		<p>
			To find the specific value of <m>C</m>, we need to use an initial condition. Let's say we know that <m>y(0) = 0</m>. This means that when <m>x = 0</m>, then <m>y = 0</m>.
		</p>

		<p>
			We can substitute these values of <m>x</m> and <m>y</m> into our general solution and solve for <m>C</m>.
			<md>
			<mrow> y =\amp\  Ce ^{x^2} + 3	\amp\Rightarrow \hspace{0.2cm} 0	=\amp\  Ce^{0^2} + 3</mrow>
			<mrow>\amp				\amp						 0	=\amp\  C + 3</mrow>
			<mrow>\amp				\amp						-3	=\amp\  C</mrow>
			</md>
		</p>

		<p>
			Therefore, the particular solution that satisfies the differential equation and the initial condition is
			<me> y = -3e^{x^2} + 3. </me>
		</p>
		
		</solution>

	</example>

	<p>
		In this example, we used the initial condition <m>y(0) = 0</m> to find the specific value of the constant <m>C</m> in the general solution. This allowed us to find a particular solution that satisfies both the differential equation and the initial condition.
	</p>

	<p>
		In the exercises that follow, you will have the opportunity to practice finding particular solutions using initial conditions.
	</p>    

	<p>
		Initial conditions do more than just narrow down the family of solutions. They also reflect real-world constraints and ensure the solution makes physical sense. For instance, in the free-fall example, the initial conditions reflect the real starting position and velocity of the object.
	</p>

	<p>
		By applying the initial conditions to the general solution, you can solve for the constants and obtain the particular solution that satisfies both the differential equation and the initial conditions.
	</p>
	

	<xi:include href="./c1-s2-ss5-interactives.ptx" />

</subsection>