<subsection xmlns:xi="http://www.w3.org/2001/XInclude"><title> <m>\lap</m> - Definition </title>

	<p>
		Give some statement leading to the definition....
	</p>

	<definition><title> Laplace Transform </title>
		<statement>
			The <term>Laplace Transform</term> of a function <m>y(t)</m> is given by

			<me> \lap\left\{ {\color{blue} y(t)} \right\} = \int_0^{\infty} {\color{blue} y(t)}\ e^{-st}dt, </me>

			given that the integral exists (i.e. the improper integral converges).
		</statement>
	</definition>

	<p>
		Some obvious features of the Laplace Transform include the following:
		<ul>
			<li>
				<p>
					The <m>\infty</m> in the upper limit of the integral makes the Laplace Transform an improper integral.
				</p>
			</li>
			<li>
				<p>
					After integrating and taking a limit, the Laplace Transform becomes a function of a new variable, <m>s</m>. That is,
					<me>
						\lap\left\{ \text{function of } t \right\} = \text{function of } s
					</me>
					
				</p>
			</li>
			<li>
				<p>
					The last couple of words in the definition say, "given that the integral exists." We will have to put restrictions on <m>s</m> to ensure this.
				</p>
			</li>
		</ul>

	</p>

	<p>
		There's a lot to unpack with this definition, but let's begin with a few examples illustrating the definition before diving into the details.As we work through the following examples, we will practice using the definition, as well as gathering facts about how the Laplace transform works. You will no doubt find the solutions to these examples a bit cumbersome We hope to draw some conclusions as we move forward that help us find the Laplace transform quickly without having to use the (admittedly somewhat cumbersome) definition every time.
	</p>

	<example>

		<m>\quad</m>Compute <m>\ds \lap\{1\}</m>.

	
		<solution>
			<p>
				By the above definition, we have the improper integral
				<me> 
					\lap\{1\} = \int_0^{\infty} \left(1\right)e^{-st}dt = \lim_{b \to \infty} \ub{\int_0^b e^{-st}dt}_{I}
				</me>.
				To compute <m>I</m>, we treat <m>s</m> as constant and integrate in <m>t</m>. 
				<md>

					<mrow>				
						\int_0^b e^{-st}dt
							\amp= \int_0^b e^{-st}dt  \qquad (u = -st)	
					</mrow>
					<mrow>				
							\amp=  -\frac{1}{s} \int_0^b e^{u} dt
					</mrow>
					<mrow>				
							\amp=  -\frac{1}{s} e^{u}\Big|_{t=0}^{t=b}
					</mrow>
					<mrow>			
							\amp= -\frac{1}{s}e^{-st}\Big|_{t=0}^{t=b}	
					</mrow>
					<mrow>			
							\amp= -\frac{1}{s}\left[ e^{-sb} - e^{-s\cdot 0} \right] = -\frac{1}{s}\left[ e^{-sb} - 1 \right] = I
					</mrow>
				</md>
				Now that we have <m>I</m>, we can plug it into the limit above.
				<md>
					<mrow> 
						\lim_{b \to \infty} \int_0^b e^{-st}dt 
							\amp= \lim_{b \to \infty} -\frac{1}{s}\left[ e^{-sb} - 1 \right]	
						</mrow>
					<mrow> 
							\amp= -\frac{1}{s} \lim_{b \to \infty} \Big[ e^{-sb} - 1 \Big] 
								\qquad \leftarrow <xref text="custom" ref="reason-factor-out-s">why?</xref>
						</mrow>
					<mrow> 
							\amp= -\frac{1}{s} \Big[ \ub{\lim_{b \to \infty} \frac{1}{e^{sb}}}_{L} - \us{=\ 1}{\ub{\lim_{b \to \infty} 1}} \Big] 
					</mrow>
				</md>
			</p>
	
			<p>
				Now let's focus on the remaining limit, <m>L</m>, which either converges or diverges, depending on <m>s</m>.
				<ul>
					<li>
						<p>
							<m>s = 0:\ </m> The <m>\ds \frac{1}{s}</m> to the left of <m>L</m> shows <m>s</m> cannot be <m>0</m>.
						</p>
					</li>
					<li>
						<p>
							<m>s &lt; 0:\ </m> Since <m>\ds \frac{1}{e^{(\text{negative})b}} \to \frac{1}{0^+} = \infty</m> as <m>b \to \infty</m>, <m>L</m> diverges.
						</p>
					</li>
					<li>
						<p>
							<m>s &gt; 0:\ </m> Since <m>\ds \frac{1}{e^{(\text{positive})b}} \to \frac{1}{\infty} = 0</m> as <m>b \to \infty</m>, <m>L=0</m>.
						</p>
					</li>
				</ul>
			</p>
	
			<p>
				Therefore, setting <m>L = 0</m>, we get 
				<me>\lap\{1\} = -\frac{1}{s} [0 - 1] = \frac{1}{s} \qquad \text{as long as } s \gt 0</me>.
			</p>
		</solution>
	
	</example>

	<assemblage xml:id="lt-table-L1"><title>Common Laplace Transforms</title>
		<p>
			<dl width="narrow">
				<li xml:id="L1"><title><m>{\LARGE \vphantom{\int}}L_1.</m></title>
					<m>\ds \lap\{ 1 \} = \frac{1}{s}, \quad s &gt;0 </m>
				</li>
			</dl>
		</p>
	</assemblage>
	
	<p>
		Before moving forward, let's conclude this section by listing out a few important take-aways from the examples of this section.
		<ul>
			<li>
				In every example, we started with a function of <m>t</m> and after computing the Laplace transform, we ended up with a function of a new variable <m>s</m>. A common convention is to use upper case function names for the Laplace transform of a given lower case function. For example,
				<me> \lap\{f(t)\} = F(s) \quad \text{ or } \quad \lap\{q(t)\} = Q(s).</me>
				In this book, we will often say "<m>F(s)</m> is the Laplace transform of <m>f(t)</m>".
				This naming	convention might seem unimportant, but it will be very helpful when using these Laplace transforms to solve differential equations.
			</li>
			<li>
				The notation often used for Laplace transform involved the symbol <m>\lap.</m> The curly braces that accompany are not optional; they are not just grouping symbols. We use them to indicate we are taking the Laplace transform of the function within the curly braces.
			</li>
			<li>
				The integral has two variables, <m>s</m> and <m>t</m>, and we integrate with respect to <m>t</m>. You may not have done anything like this before; all we need to do is treat
				<m>	s</m> like a constant.
			</li>
			<li>
				The last couple of words in the definition say, "given that the integral exists."	We will end up putting restrictions on the variable <m>s</m> that make sure that the
				integral exists.
			</li>
		</ul>
	</p>

	<xi:include href="./c4-s1-ss1-interactives.ptx" />

</subsection>
