<section><title> Orphaned Content </title>

	<introduction>
		<p>
			This is just a place to put content that was written and may or not be used.
		</p>
	</introduction>

	<paragraphs><title>Additional Narrative</title>
		
	</paragraphs>

	<paragraphs><title> Additional Examples </title>
		<example>
			<title>Example 1: Solving a First-Order Linear Differential Equation</title>
			<p>
				Consider the differential equation:
			</p>
			<me>
				y' + 3y = 6e^{2t}, \quad y(0) = 1
			</me>
	
			<p>
				Applying the Laplace transform to both sides, we get:
			</p>
			<me>
				sY(s) - y(0) + 3Y(s) = \frac{6}{s-2}
			</me>
			<p>
				Substituting the initial condition <m>y(0) = 1</m>, the equation becomes:
			</p>
			<me>
				sY(s) - 1 + 3Y(s) = \frac{6}{s-2}
			</me>
	
			<p>
				Rearranging and solving for <m>Y(s)</m>:
			</p>
			<me>
				Y(s)(s + 3) = 1 + \frac{6}{s-2}
			</me>
			<me>
				Y(s) = \frac{1}{s+3} + \frac{6}{(s-2)(s+3)}
			</me>
	
			<p>
				We can now decompose the second term using partial fractions:
			</p>
			<me>
				\frac{6}{(s-2)(s+3)} = \frac{A}{s-2} + \frac{B}{s+3}
			</me>
	
			<p>
				Solving for <m>A</m> and <m>B</m>, we get <m>A = 2</m> and <m>B = 4</m>. Therefore:
			</p>
			<me>
				Y(s) = \frac{1}{s+3} + \frac{2}{s-2} + \frac{4}{s+3}
			</me>
			<me>
				Y(s) = \frac{5}{s+3} + \frac{2}{s-2}
			</me>
	
			<p>
				Taking the inverse Laplace transform, we obtain the solution:
			</p>
			<me>
				y(t) = 5e^{-3t} + 2e^{2t}
			</me>
		</example>
	
		<example>
			<title>Example 2: Second-Order Differential Equation</title>
			<p>
				Consider the second-order differential equation:
			</p>
			<me>
				y'' + 4y = \cos(2t), \quad y(0) = 0, \quad y'(0) = 1
			</me>
	
			<p>
				Applying the Laplace transform:
			</p>
			<me>
				s^2Y(s) - sy(0) - y'(0) + 4Y(s) = \frac{s}{s^2 + 4}
			</me>
			<p>
				Substituting the initial conditions:
			</p>
			<me>
				s^2Y(s) - 1 + 4Y(s) = \frac{s}{s^2 + 4}
			</me>
	
			<p>
				Solving for <m>Y(s)</m>:
			</p>
			<me>
				Y(s)(s^2 + 4) = 1 + \frac{s}{s^2 + 4}
			</me>
	
			<p>
				After rearranging and solving, the inverse Laplace transform gives:
			</p>
			<me>
				y(t) = \sin(2t) + t
			</me>
		</example>
	</paragraphs>
	
	<reading-questions><title> Additional Practice </title>
	
	</reading-questions>

</section>