
<section xmlns:xi="http://www.w3.org/2001/XInclude"><title> Summary &amp; Exercises </title>

	<introduction>
		<p>
			<assemblage color="green"><title>Summary of the Key Ideas</title>
				<p>
					<term> <em> Method</em> </term>
					<p>
						
					</p>
				</p>
			</assemblage>
		</p>
		
	</introduction>

	<exercises>

		<exercisegroup><title> Compute the derivative of each of the following functions </title>
	
			<exercise>
				<statement>
					<m> \, \ds f(x) = \ln x\cos x </m>
				</statement>
				<answer>
					<line><m> \ds 
					f'(x)	= \left(\frac{1}{x}\right)\cos x + \ln x \left(-\sin x\right) 
									= \frac{\cos x}{x} - \ln x \sin x
					</m></line>
				</answer>
			</exercise>
	
		</exercisegroup>

		<exercisegroup><title> Find the integrating factor of each of the following differential equations </title>
		
			<exercise>
				<statement>
					<m> \ds y' - 4y = x </m>
				</statement>
				<answer>
					<line>
						<m> \ds </m>
					</line>
				</answer>
			</exercise>
	
		</exercisegroup>

		<exercisegroup>
			<exercise>
				<statement>
					Write the differential equation below in the form <m>y'+p(x)y=q(x)</m> and identify <m>p(x)</m> and <m>q(x)</m>.  Also, state the order and whether it is linear or not.
						<me> - 4xy' + 5y = \cos (x)\,y - 1 </me>
					<p/>
				</statement>
				<answer>
					<ul>
						<li> <m>\ds y' + \left(\frac{\cos x-5}{4x}\right) y = \frac{1}{4x}</m> </li>
						<li> <m>\ds p(x) = \frac{\cos x-5}{4x}</m> </li>
						<li> <m>\ds q(x) = \frac{1}{4x}</m> </li>
						<li> order is 1 </li>
						<li> it is linear </li>
					</ul>
				</answer>
			</exercise>
	
			<exercise>
				<statement>
					What classification of DEs be solved by applying an integrating factor?
					<p/>
				</statement>
				<answer>
					We can use an integrating factor to solve DEs that are <alert>linear and first order.</alert>
				</answer>
			</exercise>
	
		</exercisegroup>
	
		<exercisegroup>
			<title>
				Use an integrating factor to find the general solution to each equation
			</title>
				<exercise>
					<statement>
						<m> \ds \frac{dy}{dx} - y = e^{3x} </m>
						<p/>
					</statement>
					<solution>
						First we note that this DE is already in standard form for a first-order linear DE, <m> \ds \frac{dy}{dx} + P(x)y = f(x), </m> with <m> \ds P(x) = -1. </m>  Then we find the integrating factor <m> \ds z. </m>
						<md>
							<mrow>  z	 \amp =  e^{\Big(\mbox{an antiderivative of <m> \ds P(x) </m> }\Big)} </mrow>
							<mrow>   \amp =  e^{\Big(\mbox{an antiderivative of <m> \ds -1 </m> }\Big)} </mrow>
							<mrow>   \amp =  e^{-x} </mrow>
	
						</md>
						Now we multiply both sides of the DE by the integrating factor.
						<md>
							<mrow>  e^{-x}\cdot\frac{dy}{dx} - e^{-x}y	 \amp =  e^{-x}e^{3x} \nonumber </mrow>
							<mrow>  e^{-x}\cdot\frac{dy}{dx} - e^{-x}y	 \amp =  e^{2x}\nonumber  </mrow>
							<mrow>  \underbrace{e^{-x}}_{f}\cdot\underbrace{\frac{dy}{dx}}_{g'} + \underbrace{- e^{-x}}_{f'}\cdot\underbrace{y}_{g}  \amp =  e^{2x} \label{eq1}  </mrow>
						</md>
						Now we recall the product rule for derivatives: <m> \ds \frac{d}{dx}\Big( f\cdot g \Big) = f\cdot g' + f' \cdot g. </m> We note that the two terms on the left hand side of equation (\ref{eq1}) are the result of taking the derivative of the product.  Hence we can undo the product rule as follows: <m> \ds\frac{d}{dx}\Big(e^{-x}\cdot y \Big) = e^{2x}.</m> Now we can integrate both sides of the equation and then solve for the dependent variable.
						<md>
							<mrow>  \int \frac{d}{dx}\Big(e^{-x}\cdot y \Big)dx	 \amp =  \int e^{2x} dx </mrow>
							<mrow>  e^{-x}\cdot y	 \amp =  \frac{1}{2}e^{2x} + C </mrow>
							<mrow>  y	 \amp =  \frac{1}{2}\frac{e^{2x}}{e^{-x}} + \frac{C}{e^{-x}} </mrow>
							<mrow>   \amp =  \frac{1}{2}e^{2x}e^x + Ce^x </mrow>
							<mrow>   \amp =  \frac{1}{2}e^{3x} + Ce^x </mrow>
	
						</md>
	
					</solution>
					<answer>
						<m> \ds y = \frac{1}{2}e^{3x} + Ce^x </m>
					</answer>
				</exercise>
	
				<exercise>
					<statement>
						<m> \ds \frac{dy}{dx} = \frac{y}{x} + 2x + 1 </m> , where <m> \ds x>0 </m>
						<p/>
					</statement>
					<solution>
						First we put DE in standard form for a first-order linear DE <m> \ds \frac{dy}{dx} + P(x)y = f(x), </m> so we can identify <m> \ds P(x). </m>
						<md>
							<mrow>  \frac{dy}{dx}	 \amp =  \frac{y}{x} + 2x + 1 </mrow>
							<mrow>  \frac{dy}{dx} - \frac{y}{x}	 \amp =   2x + 1 </mrow>
							<mrow>  \frac{dy}{dx} + \left(- \frac{1}{x}\right)y	 \amp =   2x + 1 </mrow>
	
						</md>
						Thus, <m> \ds P(x) = - \frac{1}{x}. </m>  Then we find the integrating factor <m> \ds z. </m>
						<md>
							<mrow>  z	 \amp =  e^{\Big(\mbox{an antiderivative of <m> \ds P(x) </m> }\Big)} </mrow>
							<mrow>   \amp =  e^{\mbox{\Big(an antiderivative of <m> \ds -\frac{1}{x} </m> }\Big)} </mrow>
							<mrow>   \amp =  e^{-\ln|x|} </mrow>
							<mrow>   \amp =  e^{\ln (|x|^{-1})} </mrow>
							<mrow>   \amp =  |x|^{-1} </mrow>
							<mrow>   \amp =  \frac{1}{|x|} </mrow>
							<mrow>   \amp =  \frac{1}{x} \mbox{ (since <m> \ds x>0 </m> )}  </mrow>
						</md>
						Now we multiply both sides of the DE by the integrating factor.
						<md>
							<mrow>  \frac{1}{x}\cdot\frac{dy}{dx} + \frac{1}{x}\cdot \left(- \frac{1}{x}\right)y  \amp =  \frac{1}{x}(2x + 1) \nonumber </mrow>
							<mrow>  \frac{1}{x}\cdot\frac{dy}{dx} + \left(-\frac{1}{x^2}\right)\cdot y  \amp =  2 + \frac{1}{x} \nonumber </mrow>
							<mrow>  \underbrace{\frac{1}{x}}_{f}\cdot\underbrace{\frac{dy}{dx}}_{g'} + \underbrace{\left(-\frac{1}{x^2}\right)}_{f'}\cdot \underbrace{y}_{g}  \amp =  2 + \frac{1}{x} \label{eq2}  </mrow>
						</md>
						Now we recall the product rule for derivatives: <m> \ds \frac{d}{dx}\Big( f\cdot g \Big) = f\cdot g' + f' \cdot g. </m> We note that the two terms on the left hand side of equation (\ref{eq2}) are the result of taking the derivative of the product.  Hence we can undo the product rule as follows: <m> \ds\frac{d}{dx}\Big(\frac{1}{x}\cdot y \Big) = 2 + \frac{1}{x}.</m> Now we can integrate both sides of the equation and then solve for the dependent variable.
						<md>
							<mrow>  \int \frac{d}{dx}\Big(\frac{1}{x}\cdot y \Big)dx	 \amp =  \int \left(2 + \frac{1}{x} \right)dx </mrow>
							<mrow>  \frac{1}{x}\cdot y	 \amp =  2x + \ln|x| + C </mrow>
							<mrow>  \frac{1}{x}\cdot y	 \amp =  2x + \ln(x) + C \mbox{ (since <m> \ds x>0) </m> } </mrow>
							<mrow>  y	 \amp =  x \cdot (2x + \ln(x) + C) </mrow>
							<mrow>   \amp =  2x^2 + x\ln x + Cx </mrow>
	
						</md>
	
					</solution>
					<answer>
						<m> \ds y = 2x^2 + x\ln x + Cx </m>
					</answer>
				</exercise>
	
				<exercise>
					<statement>
						<m> \ds \frac{dr}{d\theta} + r\tan \theta = \sec \theta, </m> where <m> \ds -\frac{\pi}{2} \le \theta \le \frac{\pi}{2} </m>
						<p/>
					</statement>
					<solution>
						First we put DE in standard form for a first-order linear DE <m> \ds \frac{dy}{dx} + P(x)y = f(x), </m> so we can identify <m> \ds P(x). </m>  Notice that for this DE <m> \ds \theta </m> is the independent variable (i.e., it is like the <m> \ds x </m> ) and <m> \ds r </m> is the dependent variable (i.e., it is like the <m> \ds y </m> ).  Hence the standard form we will aim for is <m> \ds \frac{dr}{d\theta} + P(\theta)r = f(\theta), </m> and we want to identify <m> \ds P(\theta). </m>
						<md>
							<mrow>  \frac{dr}{d\theta} + r\tan \theta	 \amp =  \sec \theta </mrow>
							<mrow>  \frac{dr}{d\theta} + \tan \theta\cdot r	 \amp =  \sec \theta </mrow>
	
						</md>
						Thus, <m> \ds P(\theta) = \tan \theta. </m>  Then we find the integrating factor <m> \ds z. </m>
						<md>
							<mrow>  z	 \amp =  e^{\Big(\mbox{an antiderivative of <m> \ds P(\theta) </m> }\Big)} </mrow>
							<mrow>   \amp =  e^{\Big(\mbox{an antiderivative of <m> \ds \tan \theta </m> }\Big)} </mrow>
							<mrow>   \amp =  e^{-\ln|\cos \theta|} </mrow>
							<mrow>   \amp =  e^{\ln (|\cos \theta|^{-1})} </mrow>
							<mrow>   \amp =  |\cos \theta|^{-1} </mrow>
							<mrow>   \amp =  \frac{1}{|cos \theta|} </mrow>
							<mrow>   \amp =  \frac{1}{\cos \theta} \mbox{ (since <m> \ds -\frac{\pi}{2} \le \theta \le \frac{\pi}{2} </m> )} </mrow>
							<mrow>   \amp = \sec \theta </mrow>
	
						</md>
						Now we multiply both sides of the DE by the integrating factor.
						<md>
							<mrow>  \sec\theta \cdot\frac{dr}{d\theta} + \sec \theta\cdot \tan \theta\cdot r  \amp =  \sec\theta\cdot \sec \theta \nonumber </mrow>
							<mrow>  \sec\theta \cdot\frac{dr}{d\theta} + \sec \theta \tan \theta\cdot r  \amp =  \sec^2\theta \nonumber </mrow>
							<mrow>  \underbrace{\sec\theta}_{f} \cdot\underbrace{\frac{dr}{d\theta}}_{g'} + \underbrace{\sec \theta \tan \theta}_{f'}\cdot \underbrace{r}_{g}  \amp =  \sec^2\theta \label{eq3}  </mrow>
						</md>
						Now we recall the product rule for derivatives: <m> \ds \frac{d}{dx}\Big( f\cdot g \Big) = f\cdot g' + f' \cdot g. </m> We note that the two terms on the left hand side of equation (\ref{eq3}) are the result of taking the derivative of the product.  Hence we can undo the product rule as follows: <m> \ds\frac{d}{dx}\Big(\sec\theta\cdot r \Big) = \sec^2\theta.</m> Now we can integrate both sides of the equation and then solve for the dependent variable.
						<md>
							<mrow>  \int \frac{d}{dx}\Big(\sec\theta\cdot r \Big)d\theta	 \amp =  \int(\sec^2\theta) d\theta </mrow>
							<mrow>  \sec\theta\cdot r	 \amp =  \tan \theta + C </mrow>
							<mrow>  r	 \amp =  \frac{\tan \theta}{\sec\theta} + \frac{C}{\sec \theta} </mrow>
							<mrow>   \amp =  \tan\theta \cdot \cos \theta + C\cos\theta </mrow>
							<mrow>   \amp =  \frac{\sin\theta}{\cos\theta}\cdot \cos\theta + C\cos\theta </mrow>
							<mrow>   \amp =  \sin \theta + C\cos \theta </mrow>
	
						</md>
	
					</solution>
					<answer>
						<m> \ds r = \sin \theta + C\cos \theta </m>
					</answer>
				</exercise>
	
				<exercise>
					<statement>
						<m> \ds y\frac{dx}{dy} + 2x = 5y^3 </m>
						<p/>
					</statement>
					<solution>
						First we put DE in standard form for a first-order linear DE <m> \ds \frac{dy}{dx} + P(x)y = f(x), </m> so we can identify <m> \ds P(x). </m> ...EXCEPT for this DE, the roles of <m> \ds x </m> and <m> \ds y </m> are switched. Notice that here <m> \ds y </m> is the independent variable and <m> \ds x </m> is the dependent variable.  So we will aim for the standard for <m> \ds \frac{dx}{dy} + P(y)x = f(y), </m> and we want to identify <m> \ds P(y). </m>
						<md>
							<mrow>  y\frac{dx}{dy} + 2x	 \amp =  5y^3 </mrow>
							<mrow>  \frac{dx}{dy} + \frac{2}{y}x	 \amp =  5y^2 </mrow>
	
						</md>
						Thus, <m> \ds P(y) =  \frac{2}{y}. </m>  Then we find the integrating factor <m> \ds z. </m>
						<md>
							<mrow>  z	 \amp =  e^{\Big(\mbox{an antiderivative of <m> \ds P(y) </m> }\Big)} </mrow>
							<mrow>   \amp =  e^{\Big(\mbox{an antiderivative of <m> \ds \frac{2}{y} </m> }\Big)} </mrow>
							<mrow>   \amp =  e^{2\ln|y|} </mrow>
							<mrow>   \amp =  e^{\ln(|y|^2)} </mrow>
							<mrow>   \amp =  |y|^2 </mrow>
							<mrow>   \amp = y^2 </mrow>
	
						</md>
						Now we multiply both sides of the DE by the integrating factor.
						<md>
							<mrow>  y^2\cdot \frac{dx}{dy} + y^2\cdot \frac{2}{y}x	 \amp =  y^2\cdot 5y^2 \nonumber </mrow>
							<mrow>  y^2\cdot \frac{dx}{dy} + 2y\cdot x	 \amp =  5y^4 \nonumber </mrow>
							<mrow>  \underbrace{y^2}_{f} \cdot\underbrace{\frac{dx}{dy}}_{g'} + \underbrace{2y}_{f'}\cdot \underbrace{x}_{g}  \amp =  5y^4 \label{eq4}  </mrow>
						</md>
						Now we recall the product rule for derivatives: <m> \ds \frac{d}{dy}\Big( f\cdot g \Big) = f\cdot g' + f' \cdot g. </m> We note that the two terms on the left hand side of equation (\ref{eq4}) are the result of taking the derivative of the product.  Hence we can undo the product rule as follows: <m> \ds\frac{d}{dy}\Big(y^2\cdot x \Big) = 5y^4.</m> Now we can integrate both sides of the equation and then solve for the dependent variable.
						<md>
							<mrow>  \int \frac{d}{dy}\Big(y^2\cdot x \Big)dy	 \amp =  \int(5y^4) dy </mrow>
							<mrow>  y^2\cdot x	 \amp =  y^5 + C </mrow>
							<mrow>  x	 \amp =  \frac{y^5}{y^2} + \frac{C}{y^2} </mrow>
							<mrow>   \amp =  y^3 + \frac{C}{y^2} </mrow>
	
						</md>
	
					</solution>
					<answer>
						<m> \ds x = y^3 + \frac{C}{y^2} </m>
					</answer>
				</exercise>
	
		</exercisegroup>
	
		<exercisegroup>
			<title>
			Solve each initial value problem
			</title>
				<exercise>
					<statement>
						<m> \ds \frac{dy}{dx} - \frac{y}{x} = xe^x, </m> where <m> \ds x>1 </m> and <m> \ds y(1) = e-1 </m>
						<p/>
					</statement>
					<solution>
						<m> \ds \frac{dy}{dx} - \frac{y}{x} = xe^x, </m> where <m> \ds x>1 </m> and <m> \ds y(1) = e-1 </m>
					</solution>
					<answer>
	
					</answer>
				</exercise>
	
				<exercise>
					<statement>
						<m> \ds e^t z' = 1 - 4e^t z, \hspace{0.5cm} \ds z(0) = \frac{4}{3} </m>
						<p/>
					</statement>
					<solution>
						<m> \ds e^t z' = 1 - 4e^t z, \hspace{0.5cm} \ds z(0) = \frac{4}{3} </m>
					</solution>
					<answer>
	
					</answer>
				</exercise>
	
		</exercisegroup>
	
		<exercisegroup>
			<title>
			For each differential equation below, identify the appropriate statement and EXPLAIN how you know (You do not need to solve any of the equations.)
			<ol>
				<li>  Can be solved by separating variables, but not using an integrating factor. </li>
				<li>  Can be solved using an integrating factor, but not by separating variables. </li>
				<li>  Can be solved both by using integrating factor and by separating variables. </li>
				<li>  Cannot be solved using either technique.</li>
			</ol>
			</title>
				<exercise>
					<statement>
						<m> \ds x^2 \frac{dy}{dx} + \cos x = y </m>
						<p/>
					</statement>
					<solution>
						<p>
						This DE is first order and linear, so it can be solved using an integrating factor.
						</p>
						<p>
						It is not separable because when we solve for the derivative,
							<me> \frac{dy}{dx} = \frac{y - \cos x}{x^2}, </me>
						we see that there is no way to separate the variables on the right hand side via
						multiplication.
						</p>
						<p>
						Therefore, this DE can be solved using an integrating factor, but not by
						separating variables.
						</p>
					</solution>
					<answer>
						b. Can be solved using an integrating factor, but not by separating variables.
					</answer>
				</exercise>
	
				<exercise>
					<statement>
						<m> \ds \frac{dx}{dt} + xt = e^x </m>
						<p/>
					</statement>
					<solution>
						<p>
						This DE is first order but it is not linear (because the dependent variable, <m>x</m>, appears inside a function--in the <m>e^x</m> term), so it cannot be solved using an integrating factor.
						</p>
						<p>
						It is not separable because when we solve for the derivative,
									<me> \frac{dx}{dt} = e^x - xt, </me>
						we see that there is no way to separate the variables on the right hand side via multiplication.
						</p>
						<p>
						Therefore, this DE cannot be solved using either technique.
						</p>
					</solution>
					<answer>
						d. Cannot be solved using either technique.
					</answer>
				</exercise>
	
				<exercise>
					<statement>
						<m> \ds (t^2 + 1) \frac{dy}{dt} = yt - y </m>
						<p/>
					</statement>
					<solution>
						<p>
						This DE is first order and linear, so it can be solved using an integrating factor.
						</p>
						<p>
						It is separable, as shown: because when we solve for the derivative,
							<md>
								<mrow> (t^2 + 1) \frac{dy}{dt}	\amp = yt - y </mrow>
								<mrow> \frac{dy}{dt}						\amp = \frac{yt - y}{t^2+1} </mrow>
								<mrow> \frac{dy}{dt}						\amp = \frac{y(t - 1)}{t^2+1} </mrow>
								<mrow> \frac{dy}{dt}						\amp = y\cdot \frac{t - 1}{t^2+1}, </mrow>
							</md>
						we see that we can separate the variables on the right hand side via multiplication.
						</p>
						<p>
						Therefore, this DE can be solved both by using integrating factor and by separating variables.
						</p>
					</solution>
					<answer>
						c. Can be solved both by using integrating factor and by separating variables.
					</answer>
				</exercise>
	
				<exercise>
					<statement>
						<m> \ds \frac{dy}{dt} - y^2 t = t </m>
						<p/>
					</statement>
					<solution>
						<p>
						This DE is first order but it is not linear (because the dependent variable, <m>y</m>, is raised
						to a power--in the <m>y^2</m> term), so it cannot be solved using an integrating factor.
						</p>
						<p>
						It is separable, as shown: because when we solve for the derivative,
							<md>
								<mrow> \frac{dy}{dt} - y^2 t 	\amp = t </mrow>
								<mrow> \frac{dy}{dt}					\amp = t + y^2 t </mrow>
								<mrow> \frac{dy}{dt}					\amp = t\cdot (1 + y^2) </mrow>
							</md>
						we see that we can separate the variables on the right hand side via multiplication.
						</p>
						<p>
						Therefore, this DE can be solved by separating variables, but not using an integrating factor.
						</p>
					</solution>
					<answer>
						a. Can be solved by separating variables, but not using an integrating factor.
					</answer>
				</exercise>
	
				<exercise>
					<statement>
						<m> \ds 3r = \frac{dr}{d\theta} - \theta^3 </m>
						<p/>
					</statement>
					<solution>
						<p>
						This DE is first order and linear, so it can be solved using an integrating factor.
						</p>
						<p>
						It is not separable because when we solve for the derivative,
							<me> \frac{dr}{d\theta} = 3r + \theta^3, </me>
						we see that there is no way to separate the variables on the right hand side via multiplication.
						</p>
						<p>
						Therefore, this DE can be solved using an integrating factor, but not by separating variables.
						</p>
					</solution>
					<answer>
	
					</answer>
				</exercise>
	
		</exercisegroup>
	
		<exercisegroup>
			<title>
			Recall the first modeling scenario we did with M&amp;Ms. In the last section of the scenario, we switched from a discrete model to a continuous model, which led to the following DE. <m> \ds b'(t) = -0.5b(t) + 10 </m> Suppose there were initially 50 M&amp;Ms.  Then we also have the initial condition <m> \ds b(0) = 50 </m>
			</title>
				<exercise>
					<statement>
						Solve the initial value problem using an integrating factor.
						<p/>
					</statement>
					<solution>
						We begin by finding the general solution. First we put DE in standard form for a first-order linear DE <m> \ds \frac{dy}{dx} + P(x)y = f(x), </m> so we can identify <m> \ds P(x). </m>  Notice that for this DE <m> \ds t </m> is the independent variable (i.e., it is like the <m> \ds x </m> ) and <m> \ds b </m> is the dependent variable (i.e., it is like the <m> \ds y </m> ).  Hence the standard form we will aim for is <m> \ds \frac{db}{dt} + P(t)b = f(t), </m> and we want to identify <m> \ds P(t). </m>
						<md>
							<mrow>  b'(t)	 \amp =  -0.5b(t) + 10 </mrow>
							<mrow>  b'(t) + 0.5b(t)	 \amp =  10 </mrow>
							<mrow>  b' + 0.5b	 \amp =  10 </mrow>
	
						</md>
						Thus,  <m> \ds P(t) =  0.5. </m>  Then we find the integrating factor <m> \ds z. </m>
						<md>
							<mrow>  z	 \amp =  e^{\Big(\mbox{an antiderivative of <m> \ds P(t) </m> }\Big)} </mrow>
							<mrow>   \amp =  e^{\Big(\mbox{an antiderivative of <m> \ds 0.5 </m> }\Big)} </mrow>
							<mrow>   \amp =  e^{0.5t} </mrow>
	
						</md>
						Now we multiply both sides of the DE by the integrating factor.
						<md>
							<mrow>  e^{0.5t}\cdot b' + e^{0.5t}\cdot 0.5b	 \amp =  e^{0.5t}\cdot 10 \nonumber </mrow>
							<mrow>  e^{0.5t}\cdot b' + 0.5e^{0.5t}\cdot b	 \amp =  10e^{0.5t} \nonumber </mrow>
							<mrow>  \underbrace{e^{0.5t}}_{f}\cdot \underbrace{b'}_{g'} + \underbrace{0.5e^{0.5t}}_{f'}\cdot \underbrace{b}_{g}	 \amp =  10e^{0.5t} \label{eq60}  </mrow>
						</md>
						Now we recall the product rule for derivatives: <m> \ds \frac{d}{dt}\Big( f\cdot g \Big) = f\cdot g' + f' \cdot g. </m> We note that the two terms on the left hand side of equation (\ref{eq60}) are the result of taking the derivative of the product.  Hence we can undo the product rule as follows: <m> \ds\frac{d}{dt}\Big(e^{0.5t}\cdot b \Big) = 10e^{0.5t}.</m> Now we can integrate both sides of the equation and then solve for the dependent variable.
						<md>
							<mrow>  \int \frac{d}{dt}\Big(e^{0.5t}\cdot b \Big)dt	 \amp =  \int(10e^{0.5t}) dt </mrow>
							<mrow>  e^{0.5t}\cdot b	 \amp =  \frac{10}{0.5}e^{0.5t} + C </mrow>
							<mrow>  e^{0.5t}\cdot b	 \amp =  20e^{0.5t} + C </mrow>
							<mrow>  b	 \amp =  20 + Ce^{-0.5t} </mrow>
	
						</md>
						We now take the general solution and apply the initial condition <m> \ds b(0) = 50 </m> so that we can solve for the particular solution.
						<md>
							<mrow>  50	 \amp =  b(0) </mrow>
							<mrow>   \amp =  20 + Ce^{-0.5\cdot 0} </mrow>
							<mrow>   \amp =  20 + C </mrow>
							<mrow>  30	 \amp =  C </mrow>
	
						</md>
						Hence, the solution to this IVP is <m> \ds b = 20 + 30e^{-0.5t}. </m>
					</solution>
					<answer>
						<m> \ds b = 20 + 30e^{-0.5t}. </m>
					</answer>
				</exercise>
	
				<exercise>
					<statement>
						Solve the initial value problem by separating variables.
						<p/>
					</statement>
					<solution>
	
						<md>
							<mrow>  b'(t)	 \amp =  -0.5b(t) + 10 </mrow>
							<mrow>  \frac{db}{dt}	 \amp =  -0.5b + 10 </mrow>
							<mrow>  \frac{1}{-0.5b + 10}db	 \amp =  dt </mrow>
							<mrow>  \int \frac{1}{-0.5b + 10}db	 \amp =  \int dt </mrow>
							<mrow>  \frac{1}{-0.5}\ln|-0.5b + 10|	 \amp =  t+C </mrow>
							<mrow>  \ln|-0.5b + 10|	 \amp =  -0.5t-0.5C_1 </mrow>
							<mrow>  |-0.5b+10|	 \amp =  e^{-0.5t-0.5C_1} </mrow>
							<mrow>  -0.5b+10	 \amp =  \pm e^{-0.5t}e^{-0.5C_1} </mrow>
							<mrow>  -0.5b	 \amp =  \underbrace{\pm e^{-0.5C_1}}e^{-0.5t} - 10 </mrow>
							<mrow>  -0.5b	 \amp =  C_2e^{-0.5t} - 10 </mrow>
							<mrow>  b	 \amp =  \underbrace{\frac{C_2}{-0.5}}e^{-0.5t} - \frac{10}{-0.5} </mrow>
							<mrow>   \amp =  C_3e^{-0.5t}  + 20 </mrow>
	
						</md>
						We now take the general solution and apply the initial condition <m> \ds b(0) = 50 </m> so that we can solve for the particular solution.
						<md>
							<mrow>  50	 \amp =  b(0) </mrow>
							<mrow>   \amp =  C_3 e^{-0.5\cdot 0} + 20 </mrow>
							<mrow>   \amp =  C_3 + 20 </mrow>
							<mrow>  30	 \amp =  C_3 </mrow>
	
						</md>
						Hence, the solution to this IVP is <m> \ds b = 30e^{-0.5t} + 20. </m>
					</solution>
					<answer>
						<m> \ds b = 30e^{-0.5t} + 20 </m>
					</answer>
				</exercise>
	
				<exercise>
					<statement>
						Are your answers the same?
						<p/>
					</statement>
					<answer>
						Yes!  Same answer with either method.
					</answer>
				</exercise>
	
				<exercise>
					<statement>
						Plot the solution curve and compare with the data you collected in the modeling scenario.  How do they compare?
						<p/>
					</statement>
					<answer>
						<image source="sections/figures/MnM_soln_plot.png" />
					</answer>
				</exercise>
	
		</exercisegroup>
	
	</exercises>

</section>