<subsection xmlns:xi="http://www.w3.org/2001/XInclude"><title> Definition </title>

	<p>
		In the previous section we discussed how multiplying both sides of a differential equation by <m>e^{-st}</m> and integrating with respect to <m>t</m> is the initial step in the Laplace transform process to solve a differential equation. We make this more precise with the following definition.
	</p>

	<definition><title> Laplace Transform </title>
		<statement>
			The <term>Laplace Transform</term> of a given function <m>f(t)</m> is

			<me> \lap\left\{ {\color{blue} f(t)} \right\} = \int_0^{\infty} e^{-st} {\color{blue} f(t)}\ dt,</me>

			as long as the integral exists (i.e. the improper integral converges).
		</statement>
	</definition>

	<p>
		This definition is understanibly intimidating, but recall that the <m>\infty</m> on the upper limit indicates that the Laplace transform an improper integral. Calculus tells you that such an integral can be rewritten as a limit. That is,
		<me>
			\int_0^{\infty} e^{-st} f(t)\ dt = \ub{\lim_{b \to \infty} \ob{\int_0^b e^{-st} f(t)\ dt}^{\text{first compute integral}}}_{\text{then compute limit}}.
		</me>
		Also, the integral has two variables, <m>s</m> and <m>t</m>, and we integrate with respect to <m>t</m>. You may not have done anything like this before; all we need to do is treat <m>s</m> like a constant. Let's jump into an example to begin to break it down.
	</p>

	<p>
		
	</p>

	<example>

		<m>\quad</m>Compute <m>\ds \lap\{1\}</m>.

	
		<solution>
			<p>
				By the above definition, we have the improper integral
				<men xml:id="lt-1-example-eqn-1"> 
					\lap\{1\} = \int_0^{\infty} \left(1\right)e^{-st}dt = \lim_{b \to \infty} \ub{\int_0^b e^{-st}dt}_{I}
				</men>.
				To compute <m>I</m>, we treat <m>s</m> as constant and integrate in <m>t</m>. 
				<md>

					<mrow>				
						\int_0^b e^{-st}dt
							\amp= \int_0^b e^{-st}dt  \qquad (u = -st)	
					</mrow>
					<mrow>				
							\amp=  -\frac{1}{s} \int_0^b e^{u} dt
					</mrow>
					<mrow>				
							\amp=  -\frac{1}{s} e^{u}\Big|_{t=0}^{t=b}
					</mrow>
					<mrow>			
							\amp= -\frac{1}{s}e^{-st}\Big|_{t=0}^{t=b}	
					</mrow>
					<mrow>			
							\amp= -\frac{1}{s}\left[ e^{-sb} - e^{-s\cdot 0} \right] = -\frac{1}{s}\left[ e^{-sb} - 1 \right] = I
					</mrow>
				</md>
				Now that we have <m>I</m>, we can plug it into the limit above.
				<md>
					<mrow> 
						\lim_{b \to \infty} \int_0^b e^{-st}dt 
							\amp= \lim_{b \to \infty} -\frac{1}{s}\left[ e^{-sb} - 1 \right]	
						</mrow>
					<mrow> 
							\amp= -\frac{1}{s} \lim_{b \to \infty} \Big[ e^{-sb} - 1 \Big] 
								\qquad \leftarrow <xref text="custom" ref="reason-factor-out-s">why?</xref>
						</mrow>
					<mrow> 
							\amp= -\frac{1}{s} \Big[ \ub{\lim_{b \to \infty} \frac{1}{e^{sb}}}_{L} - \us{=\ 1}{\ub{\lim_{b \to \infty} 1}} \Big] 
					</mrow>
				</md>
			</p>
	
			<p>
				Let's turn our focus to the remaining limit, <m>L</m>, which either converges or diverges, depending on <m>s</m>.
				<ul>
					<li>
						<p>
							<m>s = 0:\ </m> The <m>\ds \frac{1}{s}</m> to the left of <m>L</m> shows <m>s</m> cannot be <m>0</m>.
						</p>
					</li>
					<li>
						<p>
							<m>s &lt; 0:\ </m> Since <m>\ds \frac{1}{e^{(\text{negative})b}} \to \frac{1}{0^+} = \infty</m> as <m>b \to \infty</m>, <m>L</m> diverges.
						</p>
					</li>
					<li>
						<p>
							<m>s &gt; 0:\ </m> Since <m>\ds \frac{1}{e^{(\text{positive})b}} \to \frac{1}{\infty} = 0</m> as <m>b \to \infty</m>, <m>L=0</m>.
						</p>
					</li>
				</ul>
			</p>
	
			<p>
				Therefore, setting <m>L = 0</m>, we get 
				<me>\lap\{1\} = -\frac{1}{s} [0 - 1] = \frac{1}{s} \qquad \text{as long as } s \gt 0</me>.
			</p>
		</solution>
	
	</example>

	<p>
		Now that you have seen an example, some comments are in order.

		<ul marker="square">
			<li>
				<p>
					The integral, <m>I</m>, in <xref ref="lt-1-example-eqn-1"/> was found to be a function of <m>s</m> and <m>b</m>, but after evaluating the limit, we ended up with a function of <m>s</m>. In general, every Laplace transform will be a function of <m>s</m> and a common convention is to use upper case function names for the Laplace transform of a given lower case function. For example,
					<me> \lap\{f(t)\} = F(s) \quad \text{ or } \quad \lap\{q(t)\} = Q(s).</me>
				</p>
			</li>
			<li>
				<p>
					We also determined the values of <m>s</m> for which the integral converges. As we build our Laplace transform toolbox, we will continue to note these values of <m>s</m>, but in practice, they do not impact the solution of the differential equations.     
				</p>
			</li>
			<li>
				The notation often used for Laplace transform involved the symbol <m>\lap.</m> The curly braces that accompany are not optional; they are not just grouping symbols. We use them to indicate we are taking the Laplace transform of the function within the curly braces.
			</li>
		</ul>

	</p>

	<p>
		At this point, we have our first <q>common</q> Laplace transform, that is, a Laplace transform that will be used frequently in the future. As we progress through this chapter, we will continue to add more transforms to this list.
	</p>

	<assemblage xml:id="lt-table-L1"><title>Common Laplace Transforms</title>
		<p>
			<dl width="narrow">
				<li xml:id="L1"><title><m>{\LARGE \vphantom{\int}}L_1.</m></title>
					<m>\hspace{-3em}\ds \lap\{ 1 \} = \frac{1}{s}, \quad s &gt;0 </m>
				</li>
			</dl>
		</p>
	</assemblage>

	<xi:include href="./c4-s1-ss2-interactives.ptx" />

</subsection>
