<?xml version="1.0" encoding="UTF-8" ?>

<!--********************************************************************-->

<exercises>
<title>Exercises</title>

<!--========== Exercise Group 1 ==========--> 
<exercisegroup>
<title>
<p>
<alert>Solve the following systems of differential equations.</alert>
</p>
<p/> <!-- added for vertical space -->
</title>
	<exercise> <!--== Problem 1 ==-->
		<statement>
			<m> \ds \frac{dx}{dt} = -x+y, \ds \frac{dy}{dt} = 2x, \ds x(0) = 0, \hspace{0.25cm} y(0) = 1 </m>
		</statement>
		<solution>
			 We can take the LT of each DE.  The result is two algebraic equations in two unknowns <m> \ds X(s) </m> an <m> \ds Y(s). </m>  We will solve the equations simultaneously as shown below.
			<md>
				<mrow>  \frac{dx}{dt}	 \amp =  -x+y				\amp			\frac{dy}{dt}	\amp = 2x </mrow>
				<mrow>  \lap\left\{\frac{dx}{dt}\right\}	 \amp =  \lap\left\{-x+y\right\}		\amp	\lap\left\{\frac{dy}{dt}\right\}	\amp = \lap\left\{2x\right\} </mrow>
				<mrow>  sX(s) - x(0)	 \amp =  -\lap\left\{x\right\} + \lap\left\{y\right\}	\amp			sY(s) - y(0)	\amp = 2	\lap\left\{x\right\} </mrow>
				<mrow>  sX(s) - 0	 \amp =  -X(s) + Y(s)					\amp				sY(s) - 1	\amp = 2X(s) </mrow>
				<mrow>  Y(s)	 \amp =  sX(s) + X(s)					\amp						\amp </mrow>
				<mrow>  \amp							\amp s\Big[ sX(s) + X(s) \Big] - 1	 \amp =  2X(s) </mrow>
				<mrow>  \amp							\amp		s^2 X(s) + sX(s) - 1	 \amp =  2X(s) </mrow>
				<mrow>  \amp							\amp	s^2X(s) + sX(s) - 2X(s)	 \amp =  1 </mrow>
				<mrow>  \amp							\amp 		X(s) [s^2 + s - 2]	 \amp =  1 </mrow>
				<mrow>  \amp							\amp					X(s)	 \amp =  \frac{1}{s^2 + s - 2} </mrow>
				<mrow>  \amp							\amp						 \amp =  \frac{1}{(s+2)(s-1)} </mrow>
				<mrow>  Y(s)	 \amp =  sX(s) + X(s)					\amp						\amp </mrow>
				<mrow>   \amp =  X(s)[s+1]					\amp						\amp </mrow>
				<mrow>   \amp =  \frac{1}{(s+2)(s-1)}\cdot (s+1)	\amp						\amp </mrow>
				<mrow>   \amp =  \frac{s+1}{(s+2)(s-1)}			\amp						\amp  </mrow>
			</md>
			 We need only take the inverse LT of each function in order to solve for the desired function <m> \ds x(t) </m> an <m> \ds y(t). </m> This means we will need to find a partial fraction decomposition for each.
			<md>
				<mrow>  \frac{1}{(s+2)(s-1)}	 \amp =  \frac{A}{s+2} + \frac{B}{s-1} </mrow>
				<mrow>  1	 \amp =  A(s-1) + B(s+2) </mrow>
				<mrow>  0s + 1	 \amp =  As - A + Bs + 2B </mrow>
				<mrow>   \amp =  (A+B)s + (-A + 2B)  </mrow>
			</md>
			
			<md>
				<mrow>  A+B	 \amp =  0		\amp 	-A + 2B	\amp = 1 </mrow>
				<mrow>  B	 \amp =  -A	\amp			\amp </mrow>
				<mrow>  \amp		\amp -A + 2(-A)	 \amp =  1 </mrow>
				<mrow>  \amp		\amp		-3A	 \amp =  1 </mrow>
				<mrow>  \amp		\amp		A	 \amp =  -\frac{1}{3} </mrow>
				<mrow>  B	 \amp =  -\left( -\frac{1}{3} \right)\amp \amp </mrow>
				<mrow>   \amp =  \frac{1}{3}\amp			\amp  </mrow>
			</md>
			 Hence,
			<md>
				<mrow>   X(s)	 \amp =  \frac{-\frac{1}{3}}{s+2} + \frac{\frac{1}{3}}{s-1} \nonumber </mrow>
				<mrow>   \amp =  \frac{1}{3}\left[ \frac{1}{s-1} - \frac{1}{s+2} \right] \label{eq13-1}  </mrow>
			</md>
			 Similarly, we will find a partial fraction decomposition fo <m> \ds Y(s). </m>
			<md>
				<mrow>  \frac{s+1}{(s+2)(s-1)}	 \amp =  \frac{A}{s+2} + \frac{B}{s-1} </mrow>
				<mrow>  s + 1	 \amp =  A(s-1) + B(s+2) </mrow>
				<mrow>   \amp =  As - A + Bs + 2B </mrow>
				<mrow>   \amp =  (A+B)s + (-A + 2B)  </mrow>
			</md>
			
			<md>
				<mrow>  A+B	 \amp =  1		\amp 	-A + 2B	\amp = 1 </mrow>
				<mrow>  B	 \amp =  1-A	\amp			\amp </mrow>
				<mrow>  \amp		\amp -A + 2(1-A)	 \amp =  1 </mrow>
				<mrow>  \amp		\amp	-3A + 2	 \amp =  1 </mrow>
				<mrow>  \amp		\amp		-3A	 \amp =  -1 </mrow>
				<mrow>  \amp		\amp		A	 \amp =  \frac{1}{3} </mrow>
				<mrow>  B	 \amp =  1-\left( \frac{1}{3} \right)\amp \amp </mrow>
				<mrow>   \amp =  \frac{2}{3}\amp			\amp  </mrow>
			</md>
			 Hence,
			<md>
				<mrow>   Y(s)	 \amp =  \frac{\frac{1}{3}}{s+2} + \frac{\frac{2}{3}}{s-1} \nonumber </mrow>
				<mrow>   \amp =  \frac{1}{3}\left[ \frac{1}{s+2} + 2\cdot \frac{1}{s-1} \right] \label{eq13-2}  </mrow>
			</md>
			 Now we need only find the inverse LT of equations (\ref{eq13-1}) and (\ref{eq13-2}).
			<md>
				<mrow>  x(t)	 \amp =   \lap^{-1}\left\{ X(s) \right\} </mrow>
				<mrow>   \amp =  \lap^{-1}\left\{ \frac{1}{3}\left[ \frac{1}{s-1} - \frac{1}{s+2} \right] \right\} </mrow>
				<mrow>   \amp =  \frac{1}{3}\left[ \lap^{-1}\left\{\frac{1}{s-1}\right\} - \lap^{-1}\left\{\frac{1}{s+2}\right\} \right] </mrow>
				<mrow>   \amp =  \frac{1}{3}\left[ e^t - e^{-2t} \right] </mrow>
				<mrow>  y(t)	 \amp =  \lap^{-1}\left\{ Y(s) \right\} </mrow>
				<mrow>   \amp =  \lap^{-1}\left\{ \frac{1}{3}\left[ \frac{1}{s+2} +2\cdot\frac{1}{s-1} \right] \right\} </mrow>
				<mrow>   \amp =  \frac{1}{3}\left[ \lap^{-1}\left\{\frac{1}{s+2}\right\} +2 \lap^{-1}\left\{\frac{1}{s-1}\right\} \right] </mrow>
				<mrow>   \amp =  \frac{1}{3}\left[ e^{-2t} + 2e^{t} \right] </mrow>
 
			</md>
			 This, the solution to this system is
			<md>
				<mrow>  x(t)	 \amp =  \frac{1}{3}e^t - \frac{1}{3}e^{-2t} </mrow>
				<mrow>  y(t)	 \amp =  \frac{1}{3}e^{-2t} + \frac{2}{3}e^t </mrow>
 
			</md>
			 (The following is not required, but is useful!)\\ \begin{quote} We can verify our solution.
			<md>
				<mrow>  \mbox{LHS of first DE}	 \amp =  \frac{dx}{dt} </mrow>
				<mrow>   \amp =  \frac{d}{dt}\left( \frac{1}{3}e^t - \frac{1}{3}e^{-2t} \right) </mrow>
				<mrow>   \amp =  \frac{1}{3}e^{t} + \frac{2}{3}e^{-2t} </mrow>
				<mrow>  \mbox{RHS of first DE}	 \amp =  -x+y </mrow>
				<mrow>   \amp =  -\left( \frac{1}{3}e^t - \frac{1}{3}e^{-2t} \right) + \left( \frac{1}{3}e^{-2t} + \frac{2}{3}e^t \right) </mrow>
				<mrow>   \amp =  \frac{1}{3}e^t + \frac{2}{3}e^{-2t} </mrow>
				<mrow>   \amp =  \mbox{LHS of first DE} </mrow>
				<mrow>  \mbox{LHS of second DE}	 \amp =  \frac{dy}{dt} </mrow>
				<mrow>   \amp =  \frac{d}{dt}\left( \frac{1}{3}e^{-2t} + \frac{2}{3}e^t \right) </mrow>
				<mrow>   \amp =  -\frac{2}{3}e^{-2t} + \frac{2}{3}e^t </mrow>
				<mrow>  \mbox{RHS of second DE}	 \amp =  2x </mrow>
				<mrow>   \amp =  2\left( \frac{1}{3}e^t - \frac{1}{3}e^{-2t} \right) </mrow>
				<mrow>   \amp =  \frac{2}{3}e^t - \frac{2}{3}e^{-2t} </mrow>
				<mrow>   \amp =  \mbox{LHS of second DE} </mrow>
				<mrow>  x(0)	 \amp =  \frac{1}{3}e^0 - \frac{1}{3}e^{-2\cdot 0} </mrow>
				<mrow>   \amp =  \frac{1}{3}\cdot 1 - \frac{1}{3}\cdot 1 </mrow>
				<mrow>   \amp =  0 </mrow>
				<mrow>  y(0)	 \amp =  \frac{1}{3}e^{-2\cdot 0} + \frac{2}{3}e^0 </mrow>
				<mrow>   \amp =  \frac{1}{3}\cdot 1 + \frac{2}{3}\cdot 1 </mrow>
				<mrow>   \amp =  1 </mrow>
 
			</md>
			 Hence, the solution satisfies both DEs and both initial conditions. \end{quote}
		</solution>
		<answer>
			<m> \ds x(t) = \frac{1}{3}e^t - \frac{1}{3}e^{-2t} \ds y(t) = \frac{1}{3}e^{-2t} + \frac{2}{3}e^t </m>
		</answer>
	</exercise>

	<exercise> <!--== Problem 2 ==-->
		<statement>
			<m> \ds \frac{dx}{dt} = x - 2y, \ds \frac{dy}{dt} = 5x - y, \ds x(0) = -1, \hspace{0.25cm} y(0) = 2 </m> showto{student}{\vspace{0.5cm}}
		</statement>
		<solution>
			 We can take the LT of each DE, starting with the first DE.  We will then solve fo <m> \ds X(s). </m>
			<md>
				<mrow>  \frac{dx}{dt}	 \amp =  x-2y \nonumber </mrow>
				<mrow>  \lap\left\{\frac{dx}{dt}\right\}	 \amp =  \lap\left\{x-2y\right\} \nonumber </mrow>
				<mrow>  sX(s) - x(0)	 \amp =  \lap\left\{x\right\} - 2 \lap\left\{y\right\} \nonumber </mrow>
				<mrow>  sX(s) + 1	 \amp =  X(s) - 2Y(s) \nonumber </mrow>
				<mrow>  sX(s) - X(s)	 \amp =  -2Y(s) - 1 \nonumber </mrow>
				<mrow>  X(s)[s-1]	 \amp =  -2Y(s) - 1\nonumber </mrow>
				<mrow>  X(s)	 \amp =  \frac{-2}{s-1}Y(s) - \frac{1}{s-1} \label{eq13-3}  </mrow>
			</md>
			 Now we take the LT of the second DE.  We will substitute in fo <m> \ds X(s) </m> using the result we found above.
			<md>
				<mrow>  \frac{dy}{dt}	 \amp =  5x - y </mrow>
				<mrow>  \lap\left\{\frac{dy}{dt}\right\}	 \amp =  \lap\left\{5x - y\right\} </mrow>
				<mrow>  sY(s) - y(0)	 \amp =  5\lap\left\{x\right\} - \lap\left\{y\right\} </mrow>
				<mrow>  sY(s) - 2	 \amp =  5X(s) - Y(s) </mrow>
				<mrow>  sY(s) - 2	 \amp =  5\left[ \frac{-2}{s-1}Y(s) - \frac{1}{s-1} \right] - Y(s) </mrow>
				<mrow>  sY(s) - 2	 \amp =  \frac{-10}{s-1}Y(s) - \frac{5}{s-1}- Y(s) </mrow>
				<mrow>  (s-1) \cdot \left( sY(s) - 2 \right)	 \amp =  \left( \frac{-10}{s-1}Y(s) - \frac{5}{s-1}- Y(s) \right) \cdot (s-1) </mrow>
				<mrow>  (s^2 - s)Y(s) - 2s + 2	 \amp =  -10Y(s) - 5 - (s-1)Y(s) </mrow>
				<mrow>  (s^2 - s)Y(s) + 10Y(s) + (s-1)Y(s)	 \amp =  2s - 2 - 5 </mrow>
				<mrow>  Y(s)[s^2 - s + 10 + s - 1]	 \amp =  2s - 7 </mrow>
				<mrow>  Y(s)[s^2 + 9]	 \amp =  2s - 7 </mrow>
				<mrow>  Y(s)	 \amp =  \frac{2s - 7}{s^2 + 9} </mrow>
 
			</md>
			 We now substitute this back into equation (\ref{eq13-3}).
			<md>
				<mrow>  X(s)	 \amp =  \frac{-2}{s-1}Y(s) - \frac{1}{s-1} </mrow>
				<mrow>   \amp =  \frac{-2}{s-1}\cdot\frac{2s - 7}{s^2 + 9} - \frac{1}{s-1} </mrow>
				<mrow>   \amp =  \frac{-4s+14}{(s-1)(s^2 + 9)} - \frac{1}{s-1}\cdot \frac{s^2 + 9}{s^2 + 9} </mrow>
				<mrow>   \amp =  \frac{(-4s + 14) - (s^2 + 9) }{(s-1)(s^2 + 9)} </mrow>
				<mrow>   \amp =  \frac{-4s + 14 - s^2 - 9) }{(s-1)(s^2 + 9)} </mrow>
				<mrow>   \amp =  \frac{-s^2 - 4s + 5}{(s-1)(s^2 + 9)} </mrow>
				<mrow>   \amp =  \frac{-(s^2 + 4s - 5)}{(s-1)(s^2 + 9)} </mrow>
				<mrow>   \amp =  \frac{-(s+5)(s-1)}{(s-1)(s^2 + 9)} </mrow>
				<mrow>   \amp =  \frac{-(s+5)}{s^2 + 9} </mrow>
				<mrow>   \amp =  \frac{-s-5}{s^2 + 9} </mrow>
 
			</md>
			 We need only take the inverse LT of each function in order to solve for the desired functions <m> \ds x(t) </m> an <m> \ds y(t). </m>
			<md>
				<mrow>  x(t)	 \amp =   \lap^{-1}\left\{ X(s) \right\} </mrow>
				<mrow>   \amp =  \lap^{-1}\left\{ \frac{-s-5}{s^2 + 9} \right\}  </mrow>
				<mrow>   \amp =  - \lap^{-1}\left\{ \frac{s}{s^2 + 9} \right\} - 5 \lap^{-1}\left\{ \frac{1}{s^2 + 9} \right\}  </mrow>
				<mrow>   \amp =  - \cos(3t) - 5 \lap^{-1}\left\{ \frac{1}{s^2 + 9} \right\}\cdot \frac{3}{3}  </mrow>
				<mrow>   \amp =  - \cos(3t) - 5 \lap^{-1}\left\{ \frac{3}{s^2 + 3^2} \right\}\cdot \frac{1}{3}  </mrow>
				<mrow>   \amp =  - \cos(3t) - \frac{5}{3} \sin(3t)  </mrow>
			</md>
			
			<md>
				<mrow>  y(t)	 \amp =  \lap^{-1}\left\{ Y(s) \right\} </mrow>
				<mrow>   \amp =  \lap^{-1}\left\{ \frac{2s - 7}{s^2 + 9} \right\} </mrow>
				<mrow>   \amp =  2\lap^{-1}\left\{ \frac{s}{s^2 + 9} \right\} - 7\lap^{-1}\left\{ \frac{1}{s^2 + 9} \right\} </mrow>
				<mrow>   \amp =  2\cos(3t) - 7\lap^{-1}\left\{ \frac{1}{s^2 + 9} \right\}\cdot \frac{3}{3} </mrow>
				<mrow>   \amp =  2\cos(3t) - 7\lap^{-1}\left\{ \frac{3}{s^2 + 3^2} \right\}\cdot \frac{1}{3} </mrow>
				<mrow>   \amp =  2\cos(3t) - \frac{7}{3}\sin(3t) </mrow>
 
			</md>
			 Thus, the solution to this system is
			<md>
				<mrow>  x(t)	 \amp =  -\cos(3t) - \frac{5}{3} \sin(3t) </mrow>
				<mrow>  y(t)	 \amp =  2\cos(3t) - \frac{7}{3}\sin(3t) </mrow>
 
			</md>
			 \vfill (The following is not required, but is useful!)\\ \begin{quote} We can verify our solution.
			<md>
				<mrow>  \mbox{LHS of first DE}	 \amp =  \frac{dx}{dt} </mrow>
				<mrow>   \amp =  \frac{d}{dt}\left( -\cos(3t) - \frac{5}{3} \sin(3t) \right) </mrow>
				<mrow>   \amp =  3\sin(3t) - 5\cos(3t) </mrow>
				<mrow>  \mbox{RHS of first DE}	 \amp =  x-2y </mrow>
				<mrow>   \amp =  \left( -\cos(3t) - \frac{5}{3} \sin(3t) \right) -2 \left( 2\cos(3t) - \frac{7}{3}\sin(3t) \right) </mrow>
				<mrow>   \amp =  -\cos(3t) - \frac{5}{3} \sin(3t) - 4\cos(3t) + \frac{14}{3}\sin(3t) </mrow>
				<mrow>   \amp =  -5\cos(3t) + \frac{9}{3}\sin(3t) </mrow>
				<mrow>   \amp =  -5\cos(3t) + 3\sin(3t)  </mrow>
				<mrow>   \amp =  \mbox{LHS of first DE} </mrow>
				<mrow>  \mbox{LHS of second DE}	 \amp =  \frac{dy}{dt} </mrow>
				<mrow>   \amp =  \frac{d}{dt}\left( 2\cos(3t) - \frac{7}{3}\sin(3t) \right) </mrow>
				<mrow>   \amp =  -6\sin(3t) - 7\cos(3t) </mrow>
				<mrow>  \mbox{RHS of second DE}	 \amp =  5x - y </mrow>
				<mrow>   \amp =  5\left( -\cos(3t) - \frac{5}{3} \sin(3t) \right) - \left( 2\cos(3t) - \frac{7}{3}\sin(3t) \right) </mrow>
				<mrow>   \amp =  -5\cos(3t) - \frac{25}{3} \sin(3t) - 2\cos(3t) + \frac{7}{3}\sin(3t) </mrow>
				<mrow>   \amp =  -7\cos(3t)- \frac{18}{3} \sin(3t) </mrow>
				<mrow>   \amp =  -7\cos(3t) - 6\sin(3t) </mrow>
				<mrow>   \amp =  \mbox{LHS of second DE} </mrow>
				<mrow>  x(0)	 \amp =  -\cos(3\cdot 0) - \frac{5}{3} \sin(3\cdot 0) </mrow>
				<mrow>   \amp =  -1 - 0 </mrow>
				<mrow>   \amp =  -1 </mrow>
				<mrow>  y(0)	 \amp =  2\cos(3\cdot 0) - \frac{7}{3}\sin(3\cdot 0) </mrow>
				<mrow>   \amp =  2\cdot 1 - 0 </mrow>
				<mrow>   \amp =  2  </mrow>
			</md>
			 Hence, the solution satisfies both DEs and both initial conditions. \end{quote}
		</solution>
		<answer>
			<m> \ds x(t) = -\cos(3t) - \frac{5}{3} \sin(3t) \ds y(t) = 2\cos(3t) - \frac{7}{3}\sin(3t) </m>
		</answer>
	</exercise>

	<exercise> <!--== Problem 3 ==-->
		<statement>
			<m> \ds y' - 2x = 1, \ds x' + y' - 3x - 3y = 2, \ds x(0) = 0, \hspace{0.25cm} y(0) = 0 </m>
		</statement>
		<solution>
			 We can take the LT of each DE, starting with the first DE.  We will then solve fo <m> \ds X(s). </m>
			<md>
				<mrow>  y' - 2x	 \amp =  1 \nonumber </mrow>
				<mrow>  \lap\left\{ y' - 2x \right\}	 \amp =  \lap\left\{ 1 \right\} \nonumber </mrow>
				<mrow>  sY(s) -y(0) - 2X(s)	 \amp =  \frac{1}{s} \nonumber </mrow>
				<mrow>  sY(s) - 0 - 2X(s)	 \amp =  \frac{1}{s} \nonumber </mrow>
				<mrow>  sY(s)	 \amp =  \frac{1}{s}+ 2X(s) \nonumber </mrow>
				<mrow>  Y(s)	 \amp =  \frac{1}{s^2} + \frac{2}{s}X(s) \label{eq13-5}  </mrow>
			</md>
			 Now we take the LT of the second DE.  We will substitute in fo <m> \ds Y(s) </m> using the result we found above.
			<md>
				<mrow>  x' + y' - 3x - 3y	 \amp =  2 </mrow>
				<mrow>  \lap\left\{ x' + y' - 3x - 3y \right\}	 \amp =  \lap\left\{2\right\} </mrow>
				<mrow>  sX(s) - x(0) + sY(s) - y(0) - 3X(s) - 3Y(s)	 \amp =  \frac{2}{s} </mrow>
				<mrow>  sX(s) - 0 + sY(s) - 0 - 3X(s) - 3Y(s)	 \amp =  \frac{2}{s} </mrow>
				<mrow>  sX(s) - 3X(s) + (s-3) Y(s)	 \amp =  \frac{2}{s} </mrow>
				<mrow>  sX(s) - 3X(s) + (s-3)\left[ \frac{1}{s^2} + \frac{2}{s}X(s) \right]	 \amp =  \frac{2}{s} </mrow>
				<mrow>  sX(s) - 3X(s) + \frac{s-3}{s^2} + \frac{2(s-3)}{s}X(s)	 \amp =  \frac{2}{s} </mrow>
				<mrow>  sX(s) - 3X(s) + \frac{2(s-3)}{s}X(s)	 \amp =  \frac{2}{s} - \frac{s-3}{s^2}  </mrow>
				<mrow>  s^2 \cdot \left[sX(s) - 3X(s) + \frac{2(s-3)}{s}X(s)\right]	 \amp =  s^2\cdot \left[\frac{2}{s} - \frac{s-3}{s^2}\right]  </mrow>
				<mrow>  s^3X(s) - 3s^2X(s) + 2s(s-3)X(s)	 \amp =  2s - (s-3) </mrow>
				<mrow>  X(s) [s^3 - 3s^2 + (2s^2 - 6s)]	 \amp =  2s - s + 3 </mrow>
				<mrow>  X(s)	[s^3 - s^2  - 6s]	 \amp =  s+3 </mrow>
				<mrow>  X(s)	 \amp =  \frac{s+3}{s^3 - s^2  - 6s} </mrow>
				<mrow>   \amp =  \frac{s+3}{s(s^2 - s - 6)} </mrow>
				<mrow>   \amp =  \frac{s+3}{s(s-3)(s+2)}  </mrow>
			</md>
			 We now substitute this back into equation (\ref{eq13-5}).
			<md>
				<mrow>  Y(s)	 \amp =  \frac{1}{s^2} + \frac{2}{s}X(s) </mrow>
				<mrow>   \amp =  \frac{1}{s^2} + \frac{2}{s}\cdot \frac{s+3}{s(s-3)(s+2)} </mrow>
				<mrow>   \amp =  \frac{1}{s^2} + \frac{2(s+3)}{s^2(s-3)(s+2)} </mrow>
				<mrow>   \amp =  \frac{1}{s^2}\cdot \frac{(s-3)(s+2)}{(s-3)(s+2)} + \frac{2(s+3)}{s^2(s-3)(s+2)} </mrow>
				<mrow>   \amp =  \frac{(s-3)(s+2) + 2(s+3)}{s^2(s-3)(s+2)} </mrow>
				<mrow>   \amp =  \frac{s^2 - s - 6 + 2s + 6}{s^2(s-3)(s+2)} </mrow>
				<mrow>   \amp =  \frac{s^2 + s}{s^2(s-3)(s+2)} </mrow>
				<mrow>   \amp =  \frac{s(s+1)}{s^2(s-3)(s+2)} </mrow>
				<mrow>   \amp =  \frac{s+1}{s(s-3)(s+2)}  </mrow>
			</md>
			 We need only take the inverse LT of each function in order to solve for the desired function <m> \ds x(t) </m> an <m> \ds y(t). </m> This means we will need to find a partial fraction decomposition for each.
			<md>
				<mrow>  \frac{s+3}{s(s-3)(s+2)}	 \amp =  \frac{A}{s} + \frac{B}{s-3} + \frac{C}{s+2} </mrow>
				<mrow>  s+3	 \amp =  A(s-3)(s+2) + B(s)(s+2) + C(s)(s-3) </mrow>
				<mrow>  0s^2 + s + 3	 \amp =  A(s^2 - s - 6) + B(s^2 + 2s) + C(s^2 - 3s) </mrow>
				<mrow>   \amp =  As^2  - As - 6A + Bs^2 + 2Bs + Cs^2 - 3Cs </mrow>
				<mrow>   \amp =  (A+B+C)s^2 + (-A + 2B- 3C)s + (-6A) </mrow>
 
			</md>
			
			<md>
				<mrow>  A+B+C	 \amp =  0					\amp 				-A + 2B - 3C	\amp = 1		\amp	-6A	\amp = 3 </mrow>
				<mrow>  \amp					\amp							\amp		\amp	A	 \amp =  -\frac{1}{2} </mrow>
				<mrow>  B + C	 \amp =  -A				\amp					2B - 3C	\amp = 1 + A	\amp		\amp </mrow>
				<mrow>  B + C	 \amp =  -\left( -\frac{1}{2} \right)	\amp	2B - 3C	\amp = 1 + \left( -\frac{1}{2} \right)	\amp		\amp </mrow>
				<mrow>  B + C	 \amp =  \frac{1}{2}			\amp 	2B - 3C	\amp = \frac{1}{2}				\amp		\amp </mrow>
				<mrow>  C	 \amp =  \frac{1}{2} - B		\amp			\amp						\amp		\amp </mrow>
				<mrow>  \amp	\amp 2B - 3\left( \frac{1}{2} - B \right)	 \amp =  \frac{1}{2}				\amp		\amp </mrow>
				<mrow>  \amp			\amp 2B - \frac{3}{2} + 3B	 \amp =  \frac{1}{2}				\amp		\amp </mrow>
				<mrow>  \amp					\amp 		5B	 \amp =  \frac{1}{2} + \frac{3}{2}		\amp		\amp </mrow>
				<mrow>  \amp					\amp		5B	 \amp =  2						\amp		\amp </mrow>
				<mrow>  \amp					\amp		B	 \amp =  \frac{2}{5}				\amp		\amp </mrow>
				<mrow>  C	 \amp =  \frac{1}{2} - B		\amp			\amp						\amp		\amp </mrow>
				<mrow>   \amp =  \frac{1}{2} - \frac{2}{5}	\amp			\amp						\amp		\amp </mrow>
				<mrow>   \amp =  \frac{1}{10}			\amp			\amp						\amp		\amp  </mrow>
			</md>
			 Hence,
			<md>
				<mrow>   X(s)	 \amp =  \frac{-\frac{1}{2}}{s} + \frac{\frac{2}{5}}{s-3} + \frac{\frac{1}{10}}{s+2} \nonumber </mrow>
				<mrow>   \amp =  -\frac{1}{2}\cdot \frac{1}{s} + \frac{2}{5}\cdot \frac{1}{s-3} + \frac{1}{10}\cdot \frac{1}{s+2}\label{eq13-5}  </mrow>
			</md>
			 Similarly, we will find a partial fraction decomposition fo <m> \ds Y(s). </m>
			<md>
				<mrow>  \frac{s+1}{s(s-3)(s+2)}	 \amp =  \frac{A}{s} + \frac{B}{s-3} + \frac{C}{s+2} </mrow>
				<mrow>  s+1	 \amp =  A(s-3)(s+2) + B(s)(s+2) + C(s)(s-3) </mrow>
				<mrow>  0s^2 + s + 1	 \amp =  A(s^2 - s - 6) + B(s^2 + 2s) + C(s^2 - 3s) </mrow>
				<mrow>   \amp =  As^2  - As - 6A + Bs^2 + 2Bs + Cs^2 - 3Cs </mrow>
				<mrow>   \amp =  (A+B+C)s^2 + (-A + 2B- 3C)s + (-6A) </mrow>
 
			</md>
			
			<md>
				<mrow>  A+B+C	 \amp =  0					\amp 				-A + 2B - 3C	\amp = 1		\amp	-6A	\amp = 1 </mrow>
				<mrow>  \amp					\amp							\amp		\amp	A	 \amp =  -\frac{1}{6} </mrow>
				<mrow>  B + C	 \amp =  -A				\amp					2B - 3C	\amp = 1 + A	\amp		\amp </mrow>
				<mrow>  B + C	 \amp =  -\left( -\frac{1}{6} \right)	\amp	2B - 3C	\amp = 1 + \left( -\frac{1}{6} \right)	\amp		\amp </mrow>
				<mrow>  B + C	 \amp =  \frac{1}{6}			\amp 	2B - 3C	\amp = \frac{5}{6}				\amp		\amp </mrow>
				<mrow>  C	 \amp =  \frac{1}{6} - B		\amp			\amp						\amp		\amp </mrow>
				<mrow>  \amp	\amp 2B - 3\left( \frac{1}{6} - B \right)	 \amp =  \frac{5}{6}				\amp		\amp </mrow>
				<mrow>  \amp			\amp 2B - \frac{1}{2} + 3B	 \amp =  \frac{5}{6}				\amp		\amp </mrow>
				<mrow>  \amp					\amp 		5B	 \amp =  \frac{5}{6} + \frac{1}{2}		\amp		\amp </mrow>
				<mrow>  \amp					\amp		5B	 \amp =  \frac{4}{3}				\amp		\amp </mrow>
				<mrow>  \amp					\amp		B	 \amp =  \frac{4}{15}				\amp		\amp </mrow>
				<mrow>  C	 \amp =  \frac{1}{6} - B		\amp			\amp						\amp		\amp </mrow>
				<mrow>   \amp =  \frac{1}{6} - \frac{4}{15}\amp			\amp						\amp		\amp </mrow>
				<mrow>   \amp =  \frac{5}{30} - \frac{8}{30}\amp			\amp						\amp		\amp </mrow>
				<mrow>   \amp =  -\frac{1}{10}			\amp			\amp						\amp		\amp  </mrow>
			</md>
			 Hence,
			<md>
				<mrow>   Y(s)	 \amp =  \frac{-\frac{1}{6}}{s} + \frac{\frac{4}{15}}{s-3} + \frac{-\frac{1}{10}}{s+2} \nonumber </mrow>
				<mrow>   \amp =  -\frac{1}{6}\cdot \frac{1}{s} + \frac{4}{15}\cdot \frac{1}{s-3} - \frac{1}{10}\cdot \frac{1}{s+2}\label{eq13-6}  </mrow>
			</md>
			 Now we need only find the inverse LT of equations (\ref{eq13-5}) and (\ref{eq13-6}).
			<md>
				<mrow>  x(t)	 \amp =   \lap^{-1}\left\{ X(s) \right\} </mrow>
				<mrow>   \amp =  \lap^{-1}\left\{ -\frac{1}{2}\cdot \frac{1}{s} + \frac{2}{5}\cdot \frac{1}{s-3} + \frac{1}{10}\cdot \frac{1}{s+2} \right\} </mrow>
				<mrow>   \amp =  -\frac{1}{2}\lap^{-1}\left\{ \frac{1}{s} \right\} + \frac{2}{5} \lap^{-1}\left\{ \frac{1}{s-3} \right\} + \frac{1}{10}\lap^{-1}\left\{ \frac{1}{s+2} \right\} </mrow>
				<mrow>   \amp =  -\frac{1}{2} + \frac{2}{5}e^{3t} + \frac{1}{10}e^{-2t} </mrow>
				<mrow>  y(t)	 \amp =  \lap^{-1}\left\{ Y(s) \right\} </mrow>
				<mrow>   \amp =  \lap^{-1}\left\{ -\frac{1}{6}\cdot \frac{1}{s} + \frac{4}{15}\cdot \frac{1}{s-3} - \frac{1}{10}\cdot \frac{1}{s+2} \right\} </mrow>
				<mrow>   \amp =  -\frac{1}{6}\lap^{-1}\left\{ \frac{1}{s} \right\} + \frac{4}{15}\lap^{-1}\left\{ \frac{1}{s-3} \right\} - \frac{1}{10} \lap^{-1}\left\{ \frac{1}{s+2} \right\} </mrow>
				<mrow>   \amp =  -\frac{1}{6}+ \frac{4}{15}e^{3t} - \frac{1}{10} e^{-2t} </mrow>
 
			</md>
			 Thus, the solution to this system is
			<md>
				<mrow>  x(t)	 \amp =  -\frac{1}{2} + \frac{2}{5}e^{3t} + \frac{1}{10}e^{-2t} </mrow>
				<mrow>  y(t)	 \amp =  -\frac{1}{6}+ \frac{4}{15}e^{3t} - \frac{1}{10} e^{-2t} </mrow>
 
			</md>
			 (The following is not required, but is useful!)\\ \begin{quote} We can verify that this is the solution.
			<md>
				<mrow>  \mbox{LHS of first DE}	 \amp =  y' - 2x </mrow>
				<mrow>   \amp =  \frac{d}{dt}\left( -\frac{1}{6}+ \frac{4}{15}e^{3t} - \frac{1}{10} e^{-2t} \right) - 2\Big( -\frac{1}{2} + \frac{2}{5}e^{3t} + \frac{1}{10}e^{-2t} \Big) </mrow>
				<mrow>   \amp =  \left( 0 + \frac{4}{5}e^{3t} + \frac{1}{5} e^{-2t} \right) + 1 - \frac{4}{5}e^{3t} - \frac{1}{5}e^{-2t} </mrow>
				<mrow>   \amp =  1 </mrow>
				<mrow>   \amp =  \mbox{RHS of first DE} </mrow>
				<mrow>  \mbox{RHS of second DE}	 \amp =  x' + y' - 3x - 3y </mrow>
				<mrow>   \amp =  \frac{d}{dt}\left( -\frac{1}{2} + \frac{2}{5}e^{3t} + \frac{1}{10}e^{-2t} \right) + \frac{d}{dt}\left( -\frac{1}{6}+ \frac{4}{15}e^{3t} - \frac{1}{10} e^{-2t} \right) </mrow>
				<mrow>  \amp \mbox{}\hspace{1cm} - 3 \left( -\frac{1}{2} + \frac{2}{5}e^{3t} + \frac{1}{10}e^{-2t} \right) - 3 \left( -\frac{1}{6}+ \frac{4}{15}e^{3t} - \frac{1}{10} e^{-2t} \right)\\  \amp =  \left(0 + \frac{6}{5}e^{3t} - \frac{1}{5}e^{-2t} \right) + \left( 0 + \frac{4}{5}e^{3t} + \frac{1}{5} e^{-2t} \right) </mrow>
				<mrow>  \amp \mbox{}\hspace{1cm} + \frac{3}{2} - \frac{6}{5}e^{3t} - \frac{3}{10}e^{-2t} + \frac{1}{2} - \frac{4}{5}e^{3t} + \frac{3}{10} e^{-2t}\\  \amp =  \left( \frac{6}{5} + \frac{4}{5} - \frac{6}{5} - \frac{4}{5} \right)e^{3t} + \left( - \frac{1}{5} + \frac{1}{5} - \frac{3}{10} + \frac{3}{10} \right)e^{2t} + \left( \frac{3}{2} + \frac{1}{2} \right) </mrow>
				<mrow>   \amp =  0 + 0 + 2 </mrow>
				<mrow>   \amp =  2 </mrow>
				<mrow>   \amp =  \mbox{RHS of second DE} </mrow>
				<mrow>  x(0)	 \amp =  -\frac{1}{2} + \frac{2}{5}e^{3\cdot 0} + \frac{1}{10}e^{-2\cdot 0} </mrow>
				<mrow>   \amp =  -\frac{1}{2} + \frac{2}{5} + \frac{1}{10} </mrow>
				<mrow>   \amp =  -\frac{5}{10} + \frac{4}{10} + \frac{1}{10} </mrow>
				<mrow>   \amp =  0 </mrow>
				<mrow>  y(0)	 \amp =  -\frac{1}{6} + \frac{4}{15}e^{3\cdot 0} - \frac{1}{10} e^{-2\cdot 0} </mrow>
				<mrow>   \amp =  -\frac{1}{6} + \frac{4}{15} - \frac{1}{10} </mrow>
				<mrow>   \amp =  -\frac{5}{30} + \frac{8}{30} - \frac{3}{30} </mrow>
				<mrow>   \amp =  0  </mrow>
			</md>
			 Hence, the solution satisfies both DEs and both initial conditions. \end{quote}
		</solution>
		<answer>
			<m> \ds x(t) = -\frac{1}{2} + \frac{2}{5}e^{3t} + \frac{1}{10}e^{-2t} \ds y(t) = -\frac{1}{6}+ \frac{4}{15}e^{3t} - \frac{1}{10} e^{-2t} </m>
		</answer>
	</exercise>

</exercisegroup>

</exercises>
