<!-- LICENSING
  This file is part of the textbook "Exploring Differential Equations, An Interactive, Student-Centered Approach" by Geoffrey Cox.
  License: Creative Commons Attribution-ShareAlike 4.0 International (CC BY-SA 4.0)
  You are free to:
    ‚Ä¢ Share ‚Äî copy and redistribute the material in any medium or format.
    ‚Ä¢ Adapt ‚Äî remix, transform, and build upon the material for any purpose, even commercially.
  Under the following terms:
    ‚Ä¢ Attribution ‚Äî You must give appropriate credit, provide a link to the license, and indicate if changes were made.
    ‚Ä¢ ShareAlike ‚Äî If you remix, transform, or build upon the material, you must distribute your contributions under the same license.
  Full license text: https://creativecommons.org/licenses/by-sa/4.0/legalcode
  Recommended attribution: "Exploring Differential Equations" by Geoffrey Cox, licensed CC BY-SA 4.0"
-->
<section label="whats-a-soln">
	<title>What is a Solution?</title>

	<introduction>
		<sidebyside width="90%" margins="0% 10%">
		<p>
			<aside component="web"><title>üéß Listen</title><p><video component="readings" source="audio/readings/c2/solution-basics-intro.mp3" width="100%" /></p></aside>
			A central goal in differential equations is learning how to find their solutions. In fact, most problems you'll encounter begin with a familiar prompt:
		</p>
		</sidebyside>

		<p>
			<blockquote>
				<em><q>Find the solution to the following differential equation.</q></em>
			</blockquote>
			This "solve and move on" mindset can sometimes obscure a deeper, more important question:
			<blockquote>
				<em><q>What does it actually mean to be a solution to a differential equation?</q></em>
			</blockquote>
		</p>

		<sidebyside width="90%" margins="0% 10%">
		<p>
			<aside component="web"><title>üéß Listen</title><p><video component="readings" source="audio/readings/c2/what-is-a-solution-intro.mp3" width="100%" /></p></aside>
			In algebra, a solution is any <em>value</em> that <q>satisfies</q> the algebraic equation. In contrast, a solution to a differential equation is any <em>function</em> that <q>satisfies</q> the differential equation. So, understanding what it means to satisfy a differential equation is the first step toward understanding its solutions.
		</p>
		</sidebyside>
	</introduction>

	<subsection label="satisfying-an-ae">
		<title>Satisfying an Algebraic Equation</title>

		<exercise label="chkpt-whats-a-soln-1">
			<title><e component="emoji">üìñ‚ùì</e>  What Kind of Mathematical Object is a Solution? </title>
			<statement>
				<p>
					In general, a solution to a differential equation is any <fillin characters="5" /> that satisfies it.
				</p>
			</statement>
			<choices randomize="yes">
				<choice correct="yes">
					<statement>function</statement>
					<feedback>
						<p>
							Yes, when you solve a differential equation, you are finding a function.
						</p>
					</feedback>
				</choice>
				<choice>
					<statement>derivative</statement>
					<feedback>
						<p>
							While derivatives are involved in differential equations, they do not describe solutions in general.
						</p>
					</feedback>
				</choice>
				<choice>
					<statement>number</statement>
					<feedback>
						<p>
							It is possible for a solution to be a number, but not in general.
						</p>
					</feedback>
				</choice>
				<choice>
					<statement>exponential</statement>
					<feedback>
						<p>
							Exponential functions are common solutions, but they do not represent all solutions in general.
						</p>
					</feedback>
				</choice>
			</choices>
		</exercise>

		<sidebyside width="90%" margins="0% 10%">
		<p>
			<aside component="web"><title>üéß Listen</title><p><video component="readings" source="audio/readings/c2/satisfying-an-ae.mp3" width="100%" /></p></aside>
			In algebra, we say that a value <em>satisfies</em> an equation if, when we substitute that value in place of the variable, it makes both sides of the equation equal. This gives a true statement, like <m>0=0</m> or <m>1=1</m>.
		</p>
		</sidebyside>

		<p>
			For example, consider the equation:
			<me>
				y^3 = 3y + 2.
			</me>
		</p>

		<p>
			Let's check whether <m>y = 2</m> and <m>y = 0</m> are solutions by substituting them into the equation.
		</p>

		<p>
			First, try <m>y = 2</m>.
			<md>
				<mrow> (2)^3	\amp = 3(2) + 2 </mrow>
				<mrow> 8		\amp = 6 + 2 </mrow>
				<mrow> 8		\amp = 8 </mrow>
			</md>
			That's a true statement, so <m>y = 2</m> satisfies the equation.
		</p>

		<p>
			Now check <m>y = 0</m>.
			<md>
				<mrow> (0)^3	\amp = 3(0) + 2 </mrow>
				<mrow> 0		\amp = 0 + 2 </mrow>
				<mrow> 0		\amp \ne 2 </mrow>
			</md>
			This is false, so <m>y = 0</m> does not satisfy the equation.
		</p>

		<p>
			To summarize: <m>y = 2</m> is a solution to the equation, while <m>y = 0</m> is not.
		</p>
	</subsection>

	<subsection xml:id="satisfying-a-de">
		<title>Satisfying a Differential Equation</title>

		<sidebyside width="90%" margins="0% 10%">
		<p>
			<aside component="web"><title>üéß Listen</title><p><video component="readings" source="audio/readings/c2/satisfying-a-de.mp3" width="100%" /></p></aside>
			In differential equations, solutions are <em>functions</em> rather than single values. To verify a solution, we substitute the function into the dependent variable in the equation. If both sides simplify to the same expression, then the function is a solution.
		</p>
		</sidebyside>

		<p>
			For instance, consider the differential equation:
		</p>

		<me>
			y' = 3y.
		</me>

		<p>
			To check whether <m>y = x^3</m> or <m>y = e^{3x}</m> is a solution, we substitute each into the equation and compare both sides.
		</p>

		<p>
			First, try <m>y = x^3</m>.
		</p>

		<md>
			<mrow> \left[x^3\right]'	\amp = 3(x^3) </mrow>
			<mrow> 3x^2					\amp \ne 3x^3 </mrow>
		</md>

		<p>
			Since these are not the same, <m>y = x^3</m> does not satisfy the equation.
		</p>

		<p>
			Now try <m>y = e^{3x}</m>.
		</p>

		<md>
			<mrow> \left[e^{3x}\right]'	\amp = 3(e^{3x}) </mrow>
			<mrow> 3e^{3x}				\amp = 3e^{3x} </mrow>
		</md>

		<p>
			Since both sides match, this is a true statement and <m>y = e^{3x}</m> is a solution.
		</p>

		<p>
			Here, a <q>true statement</q> means both sides simplify to the same function. When we substitute <m>y = x^3</m>, we get different expressions. But when we substitute <m>y = e^{3x}</m>, both sides match. Technically, we could rewrite <m>3e^{3x} = 3e^{3x}</m> as <m>0 = 0</m> by subtracting one side from the other, but it's enough to see that the functions match directly.
		</p>

		<exercise label="chkpt-whats-a-soln-2">
			<title><e component="emoji">üìñ‚ùì</e>  Quick Verification</title>
			<statement>
				<p>
					<m>y = x^2 + 3</m> is a solution to the differential equation
					<me>\frac{dy}{dx} - 3 = 2x</me>.
				</p>
			</statement>
			<choices randomize="yes">
				<choice>
					<statement>
						<p>
							True
						</p>
					</statement>
					<feedback>
						<p>
							Incorrect. <m>y = x^2 + 3</m> is not a solution since
							<md>
								<mrow>						\frac{dy}{dx} - 3   \amp =   2x							   </mrow>
								<mrow>	\frac{d}{dx}\left[x^2 + 3\right] - 3	\amp =   2x							   </mrow>
								<mrow>									2x - 3  \amp =   2x \quad \leftarrow \text{false} </mrow>
							</md>
						</p>
					</feedback>
				</choice>
				<choice correct="yes">
					<statement>
						<p>
							False
						</p>
					</statement>
					<feedback>
						<p>
							Correct! <m>y = x^2 + 3</m> is not a solution since
							<md>
								<mrow>						\frac{dy}{dx} - 3   \amp =   2x							   </mrow>
								<mrow>	\frac{d}{dx}\left[x^2 + 3\right] - 3	\amp =   2x							   </mrow>
								<mrow>									2x - 3  \amp =   2x \quad \leftarrow \text{false} </mrow>
							</md>
						</p>
					</feedback>
				</choice>
			</choices>
		</exercise>
	</subsection>

	<subsection label="verifying-solutions">
		<title>Verifying Solutions</title>

		<p>
			Verifying that a given function is a solution to a differential equation amounts to showing that it satisfies the equation. This typically involves taking any necessary derivatives of the function, substituting it into the equation, and simplifying both sides to see if they match. Here are some examples to illustrate this process.
		</p>

		<example>
			<statement>
				<p>
					Verify that <m>y = 2x^2\ </m> is a solution to <m>\ \ xy' - 2x^2 = y</m>.
				</p>
			</statement>
			
			<solution>
				<p>
					First, compute <m>y' = 4x</m> and plug both <m>y = 2x^2</m> and <m>y' = 4x</m> into the equation:
					<md>
						<mrow> x\left( 4x \right) - 2x^2	\amp= \left( 2x^2 \right) </mrow>
						<mrow> 								4x^2 - 2x^2	\amp= 2x^2 </mrow>
						<mrow>											2x^2	\amp= 2x^2	\quad‚úÖ </mrow>
					</md>
					This shows that <m>y = 2x^2</m> satisfies the equation and proves it is a solution.
				</p>
			</solution>
		</example>

		<example>
			<statement>
				<p>
					Verify that <m>P = \sin t\ </m> is a solution to <m>\ \ 2P'' + P = \sin t</m>.
				</p>
			</statement>

			<solution>
				<p>
					Since <m>P''</m> appears, compute the derivatives first:
					<me>	
						P = \sin t, \quad P' = \cos t, \quad P'' = -\sin t
					</me>
				</p>

				<p>
					Now substitute in the dependent variable along with its derivatives:
					<md>
						<mrow> 
							2\left( -\sin t \right) + \left( \sin t \right)	\amp = \sin t
						</mrow>
						<mrow>													-2\sin t + \sin t	\amp = \sin t </mrow>
						<mrow>																		-\sin t	\amp \ne \sin t \quad‚ùå </mrow>
					</md>
					Since the function on the left is different than the function on the right, <m>P = \sin t</m> does <term>not</term> satisfy the equation and is <term>not</term> a solution.
				</p>
			</solution>
		</example>

		<p>
			As you will soon learn, differential equations have many solutions and each of them share a common form, as the next example shows.
		</p>

		<example xml:id="example-whats-a-soln-1">
			<statement>
				<p>
					Show that the functions
					<me>y = e^{2x},\quad y = -5e^{2x},\quad y = \pi e^{2x},\quad y = 0</me>
					are all solutions to the differential equation
					<me>y' - 2y = 0</me>.
				</p>
			</statement>
			<solution>
				<p>
					Rather than verify each function separately, notice that they all are of the form <m>y = c e^{2x}</m>, where <m>c</m> is a constant. Let's verify the general case.
				</p>
				
				<p>
					Substitute <m>y = c e^{2x}</m> into the equation:
					<me>
						y' - 2y = (c e^{2x})' - 2(c e^{2x})	= 2c e^{2x} - 2c e^{2x}	= 0 \quad‚úÖ
					</me>
					So <m>y = c e^{2x}</m> is a solution for any constant <m>c</m>. In particular, this includes the functions
					<me>
						y = e^{2x},\quad y = -5e^{2x},\quad y = \pi e^{2x},\quad y = 0
					</me>
					for the constants <m>c = 1, -5, \pi, 0</m> respectively.
				</p>
			</solution>
		</example>

		<p>
			As you saw in the previous example, solutions can differ by a constant. Some solutions even involve multiple constants, as the next example shows.
		</p>

		<example xml:id="example-whats-a-soln-2">
			<statement>
				<p>
					Verify that <m>\ y = c_1\ x^2 + c_2 + \ln x\ </m> is a solution to
					<me>x^2y'' - xy' = 2</me>.
				</p>
			</statement>
			<solution>
				<p>
					Compute needed derivatives
					<me>
						y = c_1\ x^2 + c_2 - \ln x \ \ \Rightarrow \ \ 
						y' = 2 c_1\ x - \frac{1}{x} \ \ \Rightarrow \ \ 
						y'' = 2 c_1 + \frac{1}{x^2}
					</me>
					and substitute into the equation:
					<md>
						<mrow> 
							x^2\left( 2 c_1 + \frac{1}{x^2} \right) - x\left( 2 c_1\ x - \frac{1}{x} \right)
								\amp = 2
						</mrow>
						<mrow>
							2 c_1\ x^2 + 1 - 2 c_1\ x^2 + 1
								\amp = 2
						</mrow>
						<mrow>
							2	\amp = 2 \quad‚úÖ
						</mrow>
					</md>
					Thus, <m>\ y = c_1\ x^2 + c_2 + \ln x\ </m> is a solution to <m>y'' - y = -x^2</m>.
				</p>
			</solution>
		</example>
	</subsection>

	<outcomes label="whats-a-soln-takeaways">
		<ul marker="square">
			<li>
				In differential equations, a solution is a function that satisfies the equation. This means that when you plug it into the dependent variable, both sides simplify to the same expression.
			</li>
			<li>
				To verify a solution, take any necessary derivatives, substitute into the equation, and simplify. If both sides match, or reduce to something like <m>0 = 0</m>, then the function is a solution.
			</li>
		</ul>
	</outcomes>

</section>