<section xmlns:xi="http://www.w3.org/2001/XInclude"><title> Solution Basics </title>

	<introduction>

		<aside>
			<p>
				<audio source="readings/reading-whats-a-de-intro.mp3" width="100%" />
			</p>
		</aside>

		<p>
			One of the fundamental goals in differential equations is learning to find their solutions. In fact, most problems that you will encounter will start with: 
			<blockquote>
				<em><q>Find the solution to following differential equation.</q></em>
			</blockquote>
			While this might seem straightforward—just solve and move on—it leads to an important question that many students overlook:
			<blockquote>
				<em><q>What does it mean to be a solution to a differential equation?</q></em>
			</blockquote>
		</p>

		<p>
			At its core, a solution to a differential equation is not just a number or function you stumble upon; it's a function that satisfies the equation in every respect. This section will guide you through the key concepts of solutionsand by the end of this section, you will be able to verify whether a given function is a solution to a differential equation and identify it as either a general or particular solution.
		</p>
		
	</introduction>

	<subsection><title> What is a Solution? </title>

		<p>
			A solution to any equation—whether algebraic or differential—is a value or function that <q>satisfies</q> the equation. To <em>satisfy</em> an equation means that when the value or function is substituted into the equation, it reduces to a true statement, such as <m>0=0</m> or <m>1=1</m>.
		</p>

		<p>
			For example, consider the equation <me>y^3 = 3y + 2</me>. To verify if <m>y=2</m> is a solution, we substitute <m>2</m> and <m>0</m> in for <m>y</m> and check:
		</p>

		<sidebyside widths="12% 38% 12% 38%">
			<p>
				<me>
					\ul{y = 2}:
				</me>
			</p>
			<p>
				<md>
					<mrow> (2)^3 =\amp\ 3(2) + 2             </mrow>
					<mrow> 8     =\amp\ 6 + 2                </mrow>
					<mrow> 8     =\amp\ 8    \quad✅ </mrow>
				</md>
			</p>
			<p>
				<me>
					\ul{y = 0}:
				</me>
			</p>
			<p>
				<md>
					<mrow> (0)^3    =   \amp\ 3(0) + 2      </mrow>
					<mrow> 0        =   \amp\ 0 + 2         </mrow>
					<mrow> 0       \ne   \amp\ 2    \quad❌ </mrow>
				</md>
			</p>
		</sidebyside>

		<p>
			Since <m>y=2</m> results in a true statement, it is a solution. On the other hand, <m>y=0</m> does not satisfy the equation and is not a solution.
		</p>

		<p>
			Now, consider differential equations. Here, solutions are <em>functions</em> instead of single values. Verifying solutions to differential equations involves substituting the function and its derivatives into the equation. Let's explore this with an example.
		</p>

		<p>
			Determine whether <m>y = 3x</m> and <m>y = e^{3x}</m> are solutions to the differential equation <m>\ds y' = 3y.</m>
		</p>

		<sidebyside widths="12% 38% 12% 38%">
			<p>
				<me>
					\ul{y = 3x}:
				</me>
			</p>
			<p>
				<md>
					<mrow>               y' = 3y                   </mrow>
					<mrow> \left[3x\right]' = 3(3x)                 </mrow>
					<mrow> 3              \ne 9x      \quad❌ </mrow>
				</md>
			</p>
			<p>
				<me>
					\ul{y = e^{3x}}:
				</me>
			</p>
			<p>
				<md>
					<mrow>                    y' = 3y                        </mrow>
					<mrow> \left[e^{3x}\right]' = 3e^{3x}                     </mrow>
					<mrow> e^{3x} \cdot 3       = 3e^{3x}        \quad✅ </mrow>
				</md>
			</p>
		</sidebyside>
		
		<p>
			This shows that <m>y=e^{3x}</m> is a solution to <m>\ds y^\prime = 3y</m>, but <m>y=3x</m> is not.
		</p>

		<p>
			Let's practice verifying solutions through additional examples.
		</p>

		<example><title> A Couple of Warm-ups </title>

			<statement>
				<ol>
					<li>
						<p>
							Determine if <m>\ y= 2x^2\ </m> is a solution to <m>\quad\ds xy' - 2x^2 = y</m>.
						</p>
					</li>
					<li>
						<p>
							Determine if <m>\ P = \sin t\ </m> is a solution to <m>\quad\ds 2P'' + P = \sin t</m>.
						</p>
					</li>
				</ol>
			</statement>
			
			<solution>
				<p>
					Although it is not required, let's move all terms to the left-side of the equation, like so
					<me>xy' - 2x^2 - y = 0</me>.
				</p>

				<p>
					Doing this allows us to focus on simplifying just one side of the equation after plugging in <m>\ y= 2x^2</m>. 
					<md>
						<mrow> 									xy' - 2x^2 - y		=\amp 0			</mrow>
						<mrow> x\left( 2x^2 \right)' - 2x^2 - \left( 2x^2 \right)	=\amp 0			</mrow>
						<mrow> 					x\left( 4x \right) - 2x^2 - 2x^2	=\amp 0			</mrow>
						<mrow> 									4x^2 - 2x^2 - 2x^2	=\amp 0			</mrow>
						<mrow> 													0	=\amp 0	\quad✅ </mrow>
					</md>
					Therefore, <m>y= 2x^2</m> is a solution to <m>xy' - 2x^2 = y.</m>
				</p>
			</solution>

			<solution>
				<p>
					Since <m>P''</m> appears in the equation, lets compute it first.
					<me>	
						P = \sin t, \quad P' = \cos t, \quad P'' = -\sin t
					</me>
				</p>

				<p>
					Moving all the terms to the left and plugging in <m>P</m> and <m>P''</m>, we get
					<md>
						<mrow> 							2P'' + P - \sin t	=	\amp\ 0			</mrow>
						<mrow> 2\left( -\sin t \right) + (\sin t) - \sin t	=	\amp\ 0			</mrow>
						<mrow> -2\sin t + \cancel{\sin t} - \cancel{\sin t}	=	\amp\ 0			</mrow>
						<mrow> 									-2\sin t	\ne	\amp\ 0	\quad❌</mrow>
					</md>
					Therefore, <m>P = \sin t</m> is <term> not a solution </term> to <m>2P'' + P = \sin t.</m>
				</p>
			</solution>

		</example>
		
		<p>
			You can even verify that a function is a solution to a differential equation when the function contains constants as the next two examples show.
		</p>

		<example xml:id="one-de-many-solns"><title> Verifying Solutions with a Similar Form </title>

			<p>
				<statement>
					<p>
						Show that the functions 
						<me>y = e^{2x},\ \ y = 2e^{2x},\ \ y = 3e^{2x},\ \ y = -7e^{2x},\ \ y = 0.3e^{2x},\ \ y = \pi e^{2x} </me> 
						are solutions to the differential equation
						<me>\quad y' - 2y = 0</me>.
					</p>
				</statement>
			</p>

			<solution>
				<p>
					Verifying each function individually would be repetitive because they all follow the same pattern: 
					<me>y = (\text{some number})\ e^{2x} \quad \text{or} \quad y = c e^{2x} </me>, 
					where <m>c</m> can be any constant. Let's show that <m>y = c e^{2x}</m> is a solution.
				</p>
				
				<p>
					Substitute <m>\ y = c e^{2x}\ </m> into the differential equation:
					<md>
						<mrow> 									y' - 2y	=\amp\ 0	</mrow>
						<mrow> 	\left(c e^{2x}\right)' - 2(c e^{2x})	=\amp\ 0	</mrow>
						<mrow> 				c e^{2x} (2) - 2c e^{2x}	=\amp\ 0	</mrow>
						<mrow> 					2c e^{2x} - 2c e^{2x}	=\amp\ 0	</mrow>
						<mrow> 										0	=\amp\ 0	</mrow>
					</md>
					Therefore, <m>y = c e^{2x}</m> is a solution for any value of constant, <m>c</m>.
				</p>
			</solution>

		</example>

		<example xml:id="two-constant-solution-verification"><title> Verifying a Solution with Two Constants </title>

			<p>
				<statement>
					<p>
						Verify that <m>\ y = c_1 e^{-x} + c_2e^{x} + x^2 + 2\ </m> is a solution to
						<me>y'' - y = -x^2</me>.
					</p>
				</statement>
			</p>

			<p>
				<solution>

					<p>
						Move terms to left: <m>\quad y'' - y + x^2 = 0</m>
					</p>
			
					<p>
						Plug in <m>\ y = c_1 e^{-x} + c_2e^{x} + x^2 + 2\ </m> and simplify:
						<md>
							<mrow> 	\left( c_1 e^{-x} + c_2e^{x} + x^2 + 2 \right)'' - (c_1 e^{-x} + c_2e^{x} + x^2 + 2) + x^2 =\amp\ 0	</mrow>
							<mrow> 	\left( -c_1 e^{-x} + c_2e^{x} + 2x \right)' - c_1 e^{-x} - c_2e^{x} - x^2 - 2 + x^2 =\amp\ 0	</mrow>
							<mrow> 	c_1 e^{-x} + c_2e^{x} + 2 - c_1 e^{-x} - c_2e^{x} - x^2 - 2 + x^2 =\amp\ 0	</mrow>
							<mrow> 		0	=\amp\ 0	</mrow>
						</md>
						Therefore, <m>y = c_1 e^{-x} + c_2e^{x} + x^2 + 2</m> is a solution to
						<me>y'' - y = -x^2</me>.
					</p>

				</solution>
			</p>

		</example>

		<xi:include href="./c2-exercises/c2-chkpts-1-1-solns-to-des.ptx" />

	</subsection>

	<subsection><title> Solution Types </title>

		<p>
			By now, you understand that a solution to a differential equation is a function that satisfies the equation. However, a single differential equation can have multiple solutions, as demonstrated in <xref ref="one-de-many-solns"/>. In fact, the same example shows that a differential equation can have infinitely many solutions since <m>y = c e^{2x}</m> is a solution for infinitely many choices of the constant <m>c</m>.
		</p>

		<p>
			To make sense of this, we will classify solutions into three key categories:
		</p>

		<dl>
			<li>
				<title>General Solution:</title>
				<p>
					A general solution contains one or more arbitrary constants, such as <m>c</m> in <m>y = c e^{2x}</m> and provides a <q>template</q> for generating specific solutions by choosing values for these constants.
				</p>
			</li>
			<li>
				<title>Particular Solution:</title>
				<p>
					A particular solution is derived by assigning specific values to the constants in the general solution. For example, setting <m>c = 5</m> in <m>y = c e^{2x}</m> yields the particular solution <m>y = 5 e^{2x}</m>.
				</p>
			</li>
			<li>
				<title>Family of Solutions:</title>
				<p>
					This refers to the collection of all particular solutions. 
				</p>
			</li>
		</dl>

		<p>
			To illustrate, consider the differential equation <m>y' - 2y = 0</m> again:
		</p>
		<dl>
			<li><title>General Solution:</title>
				<p>
					<m>\ds y = c e^{2x}</m>
				</p>
			</li>
			<li><title>Particular Solutions:</title>
				<p>
					<m>\ds y = 5e^{2x}, \quad y = 3.1e^{2x}, \quad y = -2e^{2x}, \quad \text{etc.}</m>
				</p>
			</li>
			<li><title>Family of Solutions:</title>
				<p>
					<m>\ds \left\{ \text{ all possible particular solutions for each } c \ \right\}</m>
				</p>
			</li>
		</dl>

		<p>
			Here is an analogy to help clarify this idea. Imagine a family of solutions as a collection of all possible dates in October 2025. The general solution would be a template like <c>10/dd/2025</c>, while particular solutions would be specific dates, such as <c>10/01/2025</c>, <c>10/02/2025</c>, and so on.
		</p>

		<xi:include href="./c2-exercises/c2-chkpts-1-2-general-particular-solns.ptx" />

		<p>
			The distinction between these solution types is crucial because it lays the groundwork for understanding how initial conditions and other constraints narrow the infinite possibilities of the general solution into a unique particular solution. Keep this in mind as we explore more advanced differential equation techniques.
		</p>

		<theorem><title> <em>Constants do not always imply a general solution</em> </title>
			<p>
				Don't always assume that any solution that contains constants must be the general solution. For example,
				<me>
					y = \frac{1}{2}x^2 + c_1 x \quad \text{and} \quad y = \frac{1}{2}x^2 + c_1 x + c_2
				</me>, 
				are both solutions to <m>y'' = 1</m>, but only second one is the general solution. In fact, the first function is a special case of the second when <m>c_2 = 0</m>.
			</p>
		</theorem>

	</subsection>

	<subsection><title> Initial Conditions </title>

		<p>
			Solving a differential equation usually starts with finding its general solution, which represents all possible solutions up to one or more constants. Each constant can take any value, leading to infinitely many solutions.
		</p>

		<p>
			In real-world problems, we often reduce the number of possible solutions by specifying criteria that our solution must satisfy. Such criteria is imposed through <term>initial conditions</term>, which are known values of the solution or its derivatives at a particular point. With enough conditions, we can typically find all the constants in a general solution.
		</p>

		<sidebyside widths="30% 60%">
			<p>
				<image>
					<latex-image>
						\begin{tikzpicture}
							\draw[thick, -&gt;] (1, 0) -- (1, 5.6) node[above] {$h$ (ft)};
							\draw[thick, fill=gray!20] (-1.6, 0) rectangle (0.0, 5) node[midway] {Building};
							\node[circle, draw=red, fill=red!40, dashed, inner sep=2.6pt, label={left:$h(0)$}] at (1, 5) {};
							\draw[thick, red, -&gt;] (1.5, 5.2) -- (1.5, 4.8) node[midway, right] {$32\ \large\mathrm{\sfrac{ft}{s^2}}$};
							\node[circle, fill=red, inner sep=2.6pt, label={left:$h(t)$}] (mass) at (1, 1.8) {};
							\draw[thick, red, -&gt;] (1.5, 2.0) -- (1.5, 1.6) node[midway, right] {$32\ \large\mathrm{\sfrac{ft}{s^2}}$};
							\draw[thick] (-0.5, 0) -- (2.5, 0);
						\end{tikzpicture}
					</latex-image>
				</image>
			</p>
			<p>
				For example, consider an object in free fall with constant acceleration <m>32 \text{ ft/s}^2</m>. If <m>h(t)</m> is its height above the ground, the motion is described by the differential equation:
				<me>
					h''(t) = -32 \ \mathrm{ft/s^2}.
				</me>
				The general solution for the object's position is:
				<me>
					h(t) = c_1 + c_2t - 16t^2.
				</me>
			</p>
		</sidebyside>

		<p>
			This solution is a template for any object falling with constant acceleration. To make this solution more practical, let's impose the following criteria:
		</p>

		<ul>
			<li>The object starts at the top of a <m>100\ \mathrm{ft}</m> building.</li>
			<li>The object is dropped from rest.</li>
		</ul>


		<p>
			In terms of <m>h(t)</m>, this criteria can be translated as the two initial conditions
			<me>
				h(0) = 100\ \mathrm{ft} \quad \text{and} \quad h'(0) = 0\ \mathrm{ft/s}.
			</me>
		</p>

		<p>
			This new information forces <m>c_1</m> and <m>c_2</m> to take on specific values in the general solution, since
		</p>

		<p>
			<sidebyside widths="55% 3% 42%" margins="0% 0%">
				
				<p>
					<md>
						<mrow>	h(t)	=\amp\ c_1 + c_2t - 16t^2		</mrow>
						<mrow>		100	=\amp\ c_1 + c_2(0) - 16(0)^2	</mrow>
						<mrow>					100	=\amp\ c_1						</mrow>
					</md>
				</p>
				<p/>
				<p>
					<md>
						<mrow>	h'(t)	=\amp\ c_2 - 32t				</mrow>
						<mrow>		0	=\amp\ c_2 - 32(0)				</mrow>
						<mrow>				0	=\amp\ c_2						</mrow>
					</md>.
				</p>
			</sidebyside>
		</p>

		<p>
			This results in the particular solution
			<me>
				h(t) = 100 - 16t^2
			</me>,
			which describes the position of an object that, <em>specifically</em>, starts at <m>100 \ \mathrm{ft}</m> and is dropped with an initial velocity of <m>0 \ \mathrm{ft/s}</m>.
		</p>

		<p>
			When a differential equation includes initial conditions, it is called an <term>initial value problem</term>, which produces a particular solution rather than a general solution. Let's explore this further with examples.
		</p>

		<example xml:id="p1-c2-s5-example-1"><title> Finding a constant in a General Solution </title>

			<p>
				<statement>
					<p>
						Find the particular solution to the initial-value problem
						<me xml:id="p1-c2-s5-example-1-de"> 
							\frac{dy}{dx} = 2xy - 6x, \quad y(0) = 2
						</me>,
						given that the general solution is <m>\quad\ds y = ce^{x^2} + 3</m>.
					</p>
				</statement>
			</p>

			<p>
				<solution>
					<p>
						The initial condition <m>y(0) = 2</m> tells us that <m>y</m> must equal 2 when <m>x = 0</m>. Substituting into the general solution:
						<md>
							<mrow> y =  ce^{x^2} + 3 \quad \overset{y\ =\ 2,\ x\ =\ 0}{\Rightarrow} \quad	2	=\amp\  ce^{0^2} + 3	</mrow>
							<mrow>							 												2	=\amp\  c + 3		</mrow>
							<mrow>																			-1	=\amp\  c			</mrow>
						</md>
					</p>
					<p>
						Thus, the particular solution is:
						<me>
							y = -e^{x^2} + 3.
						</me>
					</p>
				</solution>
			</p>

		</example>

		<p>
			Here is one more example a particular solution from the general solution and initial conditions.
		</p>

		<example><title> General Sol. + Initial Values <m>\to</m> Particular Sol </title>
		
			<p>
				<statement>
					<p>
						Solve the initial value problem
						<me>
							y'' - y' - 12y = 0, \quad y(0) = 4, \quad y'(0) = -5
						</me>,
						given that the general solution is <m>\quad\ds y = c_1e^{-3t} + c_2e^{4t}</m>.
					</p>
				</statement>
			</p>

			<p>
				<solution>
					<p>
						If you are interested in the verification steps, see the solution below.
					</p>
				
					<solution><title>Verification as a solution</title>
						<p>
							First find <m>y, y', \text{ and } y''</m>:
							<md>
								<mrow> y	=\amp\ c_1e^{-3t} + c_2e^{4t}		</mrow>
								<mrow> y'	=\amp\ -3c_1e^{-3t} + 4c_2e^{4t}	</mrow>
								<mrow> y''	=\amp\ 9c_1e^{-3t} + 16c_2e^{4t}	</mrow>
							</md>
						</p>
					
						<p>
							and substitute these into <m>y'' - y' - 12y</m> and simplify:
							<md>
								<mrow>
									y'' - y' - 12y =\amp\ \left(9c_1e^{-3t} + 16c_2e^{4t}\right) 
								</mrow>
								<mrow>		
									\amp\ \hspace{1em} - \left( -3c_1e^{-3t} + 4c_2e^{4t} \right) -12\left( c_1e^{-3t} + c_2e^{4t} \right)
								</mrow>
								<mrow>
									=\amp\ \ul{\ul{9c_1e^{-3t}}} + \ul{16c_2e^{4t}} 
								</mrow>
								<mrow>
									\amp\ \hspace{1em} + \ul{\ul{3c_1e^{-3t}}} - \ul{4c_2e^{4t}} - \ul{\ul{12c_1e^{-3t}}} - \ul{12c_2e^{4t}}
								</mrow>
								<mrow>
									=\amp\ 0
								</mrow>
							</md>
							Which shows <m>0 = 0</m> and so <m>y(t) = c_1e^{-3t} + c_2e^{4t}</m> is a solution.
						</p>
					</solution>

					<p>
						We would like determine the spcific values of <m>c_1</m> and <m>c_2</m> that correspond to the initial conditions <m>y(0) = 4</m> and <m>y'(0) = -5</m>. 
					</p>

					<p>
						Now let's apply the initial conditions:
					</p>

					<p>
						<sidebyside>
							<p>
								<md>
									<mrow>	y(t) 	=\amp\ c_1e^{-3t} + c_2e^{4t}				</mrow>
									<mrow>		4	=\amp\ c_1e^{-3\cdot 0} + c_2e^{4\cdot 0}	</mrow>
									<mrow>		4	=\amp\ c_1 + c_2							</mrow>
								</md>
							</p>
							<p>
								<md>
									<mrow>	y'(t) 	=\amp\ -3c_1e^{-3t} + 4c_2e^{4t}			</mrow>
									<mrow>		-5	=\amp\ -3c_1e^{-3\cdot 0} + 4c_2e^{4\cdot 0}	</mrow>
									<mrow>		-5	=\amp\ -3c_1 + 4c_2							</mrow>
								</md>
							</p>
						</sidebyside>
					</p>
				
					<p>
						We now have two equations and two unknowns,
						<md>
							<mrow>	 c_1 +  c_2	=\amp\ 	4 	</mrow>
							<mrow> -3c_1 + 4c_2	=\amp\ -5 	</mrow>
						</md>
						There are multiple ways to solve this system of equations, and the reader is encouraged to verify that	<m>c_1 = 3</m> and <m>c_2 = 1</m>.
					</p>
				
					<p>
						Thus, the particular solution to this initial-value problem is
						<me>
							y = 3e^{-3t} + e^{4t}
						</me>.
					</p>
			
				</solution>
			</p>
		
		</example>

		<xi:include href="./c2-exercises/c2-chkpts-1-3-initial-conditions.ptx" />

		<p>
			In sum, specifying criteria for a desired solution is done with initial conditions. This reduces the ambiguity of the general solution by forcing its constants to assume values that lead to solutions consistent with these conditions.
		</p>


	</subsection>

	<subsection><title> Visualizing Solutions </title>

		<p>
			A powerful way to enhance your understanding of different solution types is through visualization. In this section, we will explore a graphical representation of a family of solutions and how an initial condition can help us pinpoint particular solutions from this family.
		</p>

		<p>
			Consider the differential equation
			<men xml:id="visualizing-solns-eqn">
				\frac{dy}{dx} = 2xy - 6x,
			</men>
			which has the general solution
			<me>
				y = c e^{x^2} + 3
			</me>.
			<aside><title> ℹ️ Details </title>
				<p>
					See <xref ref="visualization-verifying-gen-soln"/> for the steps to verify that <m>y = ce^{x^2} + 3</m>	is a general solution to equation <xref ref="visualizing-solns-eqn"/>.
				</p>
			</aside>
		</p>

		<p>
			As you know, the general solution contains a constant <m>c</m> that can take any real value. This constant generates a family of solutions, each corresponding to a different value of <m>c</m>. To visualize this family of solutions, we plot the general solution for various values of <m>c</m> as shown in <xref ref="family-of-solutions-figure"/>. 
		</p>

		<p>
			In the figure, each green curve represents a particular solution. The blue curve is a particular solution that passes through the initial condition <m>y(0)</m>. While the figure shows only a few members of the family of solutions, there exists a solution curve for every possible value of <m>c</m>.
		</p>
		
		<assemblage><title> Interactive Graph. Visualizing a Family of Solutions </title>
			<p>
				<sidebyside widths="42% 50%" margins="0% 4%">
					<stack>
						<p>
							<em>This figure is interactive. You can drag the initial condition up and down the <m>y</m>-axis to change the value of <m>y(0)</m>. 
							<!-- When you do, the particular solution (blue curve) will also change along with the new value for the constant <m>c</m>. -->
							</em>
						</p>
						<p>
							The figure shows the family of solutions for <xref ref="visualizing-solns-eqn"/>. Each green curve is of the form
							<me>
								y = ce^{x^2} + 3
							</me>
							for different values of <m>c</m>. The blue curve represents the particular solution that passes through the selected initial condition <m>y(0)</m>.
						</p>
						
					</stack>

					<figure xml:id="family-of-solutions-figure">
						<interactive xml:id="interactive-drag-ic" platform="jsxgraph" source="code/initial-condition.js">
							<slate xml:id="interactive-drag-ic-slate" surface="jsxboard" />
						</interactive>
						<caption>Family of solutions for <xref ref="visualizing-solns-eqn"/>.</caption>
					</figure>
				</sidebyside>
			</p>
		</assemblage>
		
		<xi:include href="./c2-exercises/c2-chkpts-1-4-visualizing-solns.ptx" />

		<theorem xml:id="visualization-verifying-gen-soln"><title> Verifying the Solution to <xref ref="visualizing-solns-eqn"/> </title>
			<statement>
				<p>
					To verify that <m>\ds y = ce^{x^2} + 3</m> is a solution, we move all terms to one side of the equation and substitute <m>\ds y = ce^{x^2} + 3</m> into the equation.
					<md>
						<mrow> 													\frac{dy}{dx} - 2xy + 6x	=\amp\ 0</mrow>
						<mrow> \frac{d}{dx}\left( ce^{x^2} + 3 \right) - 2x\left( ce^{x^2} + 3 \right) + 6x	=\amp\ 0</mrow>
						<mrow> 											2cxe^{x^2} - 2cxe^{x^2} - 6x + 6x	=\amp\ 0</mrow>
						<mrow> 																			0	=\amp\ 0</mrow>
					</md>
					This shows that <m>\ds y = ce^{x^2} + 3</m> is a solution to <m>\ds \frac{dy}{dx} = 2xy - 6x.</m>
				</p>
			</statement>
		</theorem>

	</subsection>

</section>