<!-- LICENSING
  This file is part of the textbook "Exploring Differential Equations, An Interactive, Student-Centered Approach" by Geoffrey Cox.
  License: Creative Commons Attribution-ShareAlike 4.0 International (CC BY-SA 4.0)
  You are free to:
    • Share — copy and redistribute the material in any medium or format.
    • Adapt — remix, transform, and build upon the material for any purpose, even commercially.
  Under the following terms:
    • Attribution — You must give appropriate credit, provide a link to the license, and indicate if changes were made.
    • ShareAlike — If you remix, transform, or build upon the material, you must distribute your contributions under the same license.
  Full license text: https://creativecommons.org/licenses/by-sa/4.0/legalcode
  Recommended attribution: "Exploring Differential Equations" by Geoffrey Cox, licensed CC BY-SA 4.0"
-->
<section label="whats-a-soln">
	<title>What is a Solution?</title>

	<introduction>

		<p>
			A central goal in differential equations is learning how to find their solutions. In fact, most problems you'll encounter begin with a familiar prompt:
		</p>

		<p>
			<blockquote>
				<em><q>Find the solution to the following differential equation.</q></em>
			</blockquote>
			This "solve and move on" mindset can sometimes obscure a deeper, more important question:
			<blockquote>
				<em><q>What does it actually mean to be a solution to a differential equation?</q></em>
			</blockquote>
		</p>

		<p>
			In algebra, a solution is any <em>value</em> that <q>satisfies</q> the algebraic equation. In contrast, a solution to a differential equation is any <em>function</em> that <q>satisfies</q> the differential equation. So, understanding what it means to satisfy a differential equation is the first step toward understanding its solutions.
		</p>

	</introduction>

	<subsection label="solns-to-eqns">
		<title>Solutions to Equations</title>

		<subsubsection label="solns-to-alg-eqns">
			<title>Solutions to Algebraic Equations</title>

			<p>
				In algebra, we say that a value <em>satisfies</em> an equation if, when we substitute that value in place of the variable, it makes both sides of the equation equal. This gives a true statement, like <m>0=0</m> or <m>1=1</m>.
			</p>

			<p>
				For example, consider the equation:
				<me>
					y^3 = 3y + 2.
				</me>
			</p>

			<p>
				Let's check whether <m>y = 2</m> and <m>y = 0</m> are solutions by substituting them into the equation. plugging them in we get:
			</p>

			<sidebyside>
				<p>
					<md>
						<mrow> (2)^3	\amp = 3(2) + 2 </mrow>
						<mrow> 8		\amp = 6 + 2 </mrow>
						<mrow> 8		\amp = 8 \quad ✅</mrow>
					</md>
				</p>
				<p>
					<md>
						<mrow> (0)^3	\amp = 3(0) + 2 </mrow>
						<mrow> 0		\amp = 0 + 2 </mrow>
						<mrow> 0		\amp \ne 2 \quad ❌</mrow>
					</md>
				</p>
			</sidebyside>

			<p>
				Since <m>8 = 8</m> is a true statement, <m>y = 2</m> satisfies the equation and is a solution. On the other hand, <m>y = 0</m> leads to a false statement (<m>0 = 2</m>), showing that it is not a solution.
			</p>

		</subsubsection>

		<subsubsection xml:id="solns-to-alg-eqns">
			<title>Solutions to Differential Equations</title>

			<p>
				In differential equations, solutions are <em>functions</em> rather than single values. To verify a solution, we substitute the function into the dependent variable in the equation. If both sides simplify to the same expression, then the function is a solution.
			</p>

			<p>
				For instance, consider the differential equation:
			</p>

			<me>
				y' = 3y.
			</me>

			<p>
				To check whether <m>y = x^3</m> or <m>y = e^{3x}</m> is a solution, we substitute each into the equation and compare both sides. In this case, we get:
			</p>

			<sidebyside>
				<p>
					<md>
						<mrow> \left[x^3\right]'	\amp = 3(x^3) </mrow>
						<mrow> 3x^2					\amp \ne 3x^3 \quad ❌</mrow>
					</md>
				</p>
				<p>
					<md>
						<mrow> \left[e^{3x}\right]'	\amp = 3(e^{3x}) </mrow>
						<mrow> 3e^{3x}				\amp = 3e^{3x} \quad ✅ </mrow>
					</md>
				</p>
			</sidebyside>

			<p>
				For differential equations, a solution satisfies the equation if both sides simplfy to the <em>exact</em> same function. 
				Since this only happened for the second function, we can conclude that <m>y = e^{3x}</m> is a solution, while <m>y = x^3</m> is not.
			</p>

			<exercise label="whats-a-soln-cyu-1">

				<task label="whats-a-soln-cyu-1-task-1">

					<statement correct="no">
						<p>
							To verify that a function satisfies a differential equation, you 
							<ol marker="(1)">
								<li>plug the function into the equation,</li>
								<li>simplify both sides of the equation, and</li>
								<li>solve the simplified equation for <m>x</m>.</li>
							</ol>
						</p>
					</statement>

					<feedback>
						<p>
							Statements (1) and (2) are true, but (3) is not. Statement (3) should instead read:
						</p>

						<p>
							(3) compare the functions on the left and right-hand sides of the simplified equation.
						</p>
					</feedback>

				</task>

				<task label="whats-a-soln-cyu-1-task-2">

					<statement correct="no">
						<p>
							The function, <m>y = x^2 + 3</m>, is a solution to the equation
							<me>\frac{dy}{dx} - 3 = 2x</me>.
						</p>
					</statement>

					<feedback>
						<p>
							The function <m>y = x^2 + 3</m> is not a solution since
							<md>
								<mrow>						\frac{dy}{dx} - 3   \amp =   2x							   </mrow>
								<mrow>	\frac{d}{dx}\left[x^2 + 3\right] - 3	\amp =   2x							   </mrow>
								<mrow>									2x - 3  \amp =   2x \quad \leftarrow \text{false} </mrow>
							</md>
						</p>
					</feedback>

				</task>

			</exercise>

		</subsubsection>

	</subsection>

	<subsection label="verifying-solutions">
		<title>Verifying Solutions</title>

		<p>
			Verifying that a given function is a solution to a differential equation amounts to showing that it satisfies the equation. This typically involves taking any necessary derivatives of the function, substituting it into the equation, and simplifying both sides to see if they match. Here are some examples to illustrate this process.
		</p>

		<example>
			<statement>
				<p>
					Verify that <m>y = 2x^2\ </m> is a solution to <m>\ \ xy' - 2x^2 = y</m>.
				</p>
			</statement>
			
			<solution>
				<p>
					First, compute <m>y' = 4x</m> and plug both <m>y = 2x^2</m> and <m>y' = 4x</m> into the equation:
					<md>
						<mrow> x\left( 4x \right) - 2x^2	\amp= \left( 2x^2 \right) </mrow>
						<mrow> 								4x^2 - 2x^2	\amp= 2x^2 </mrow>
						<mrow>											2x^2	\amp= 2x^2	\quad✅ </mrow>
					</md>
					This shows that <m>y = 2x^2</m> satisfies the equation and proves it is a solution.
				</p>
			</solution>
		</example>

		<example>
			<statement>
				<p>
					Verify that <m>P = \sin t\ </m> is a solution to <m>\ \ 2P'' + P = \sin t</m>.
				</p>
			</statement>

			<solution>
				<p>
					Since <m>P''</m> appears, compute the derivatives first:
					<me>	
						P = \sin t, \quad P' = \cos t, \quad P'' = -\sin t
					</me>
				</p>

				<p>
					Now substitute in the dependent variable along with its derivatives:
					<md>
						<mrow> 
							2\left( -\sin t \right) + \left( \sin t \right)	\amp = \sin t
						</mrow>
						<mrow>													-2\sin t + \sin t	\amp = \sin t </mrow>
						<mrow>																		-\sin t	\amp \ne \sin t \quad❌ </mrow>
					</md>
					Since the function on the left is different than the function on the right, <m>P = \sin t</m> does <term>not</term> satisfy the equation and is <term>not</term> a solution.
				</p>
			</solution>
		</example>

		<p>
			As you will soon learn, differential equations have many solutions and each of them share a common form, as the next example shows.
		</p>

		<example xml:id="example-whats-a-soln-1">
			<statement>
				<p>
					Show that the functions
					<me>y = e^{2x},\quad y = -5e^{2x},\quad y = \pi e^{2x},\quad y = 0</me>
					are all solutions to the differential equation
					<me>y' - 2y = 0</me>.
				</p>
			</statement>
			<solution>
				<p>
					Rather than verify each function separately, notice that they all are of the form <m>y = c e^{2x}</m>, where <m>c</m> is a constant. Let's verify the general case.
				</p>
				
				<p>
					Substitute <m>y = c e^{2x}</m> into the equation:
					<me>
						y' - 2y = (c e^{2x})' - 2(c e^{2x})	= 2c e^{2x} - 2c e^{2x}	= 0 \quad✅
					</me>
					So <m>y = c e^{2x}</m> is a solution for any constant <m>c</m>. In particular, this includes the functions
					<me>
						y = e^{2x},\quad y = -5e^{2x},\quad y = \pi e^{2x},\quad y = 0
					</me>
					for the constants <m>c = 1, -5, \pi, 0</m> respectively.
				</p>
			</solution>
		</example>

		<p>
			As you saw in the previous example, solutions can differ by a constant. Some solutions even involve multiple constants, as the next example shows.
		</p>

		<example xml:id="example-whats-a-soln-2">
			<statement>
				<p>
					Verify that <m>\ y = c_1\ x^2 + c_2 + \ln x\ </m> is a solution to
					<me>x^2y'' - xy' = 2</me>.
				</p>
			</statement>
			<solution>
				<p>
					Compute needed derivatives
					<me>
						y = c_1\ x^2 + c_2 - \ln x \ \ \Rightarrow \ \ 
						y' = 2 c_1\ x - \frac{1}{x} \ \ \Rightarrow \ \ 
						y'' = 2 c_1 + \frac{1}{x^2}
					</me>
					and substitute into the equation:
					<md>
						<mrow> 
							x^2\left( 2 c_1 + \frac{1}{x^2} \right) - x\left( 2 c_1\ x - \frac{1}{x} \right)
								\amp = 2
						</mrow>
						<mrow>
							2 c_1\ x^2 + 1 - 2 c_1\ x^2 + 1
								\amp = 2
						</mrow>
						<mrow>
							2	\amp = 2 \quad✅
						</mrow>
					</md>
					Thus, <m>\ y = c_1\ x^2 + c_2 + \ln x\ </m> is a solution to <m>y'' - y = -x^2</m>.
				</p>
			</solution>
		</example>

	</subsection>

	<outcomes label="whats-a-soln-takeaways">
		<ul marker="square">
			<li>
				In differential equations, a solution is a function that satisfies the equation. This means that when you plug it into the dependent variable, both sides simplify to the same expression.
			</li>
			<li>
				To verify a solution, take any necessary derivatives, substitute into the equation, and simplify. If both sides match, or reduce to something like <m>0 = 0</m>, then the function is a solution.
			</li>
		</ul>
	</outcomes>

</section>