<!-- LICENSING
  This file is part of the textbook "Exploring Differential Equations, An Interactive, Student-Centered Approach" by Geoffrey Cox.
  License: Creative Commons Attribution-ShareAlike 4.0 International (CC BY-SA 4.0)
  You are free to:
    • Share — copy and redistribute the material in any medium or format.
    • Adapt — remix, transform, and build upon the material for any purpose, even commercially.
  Under the following terms:
    • Attribution — You must give appropriate credit, provide a link to the license, and indicate if changes were made.
    • ShareAlike — If you remix, transform, or build upon the material, you must distribute your contributions under the same license.
  Full license text: https://creativecommons.org/licenses/by-sa/4.0/legalcode
  Recommended attribution: "Exploring Differential Equations" by Geoffrey Cox, licensed CC BY-SA 4.0.
-->
<section label="verifying-solutions">
	<title>Verifying Solutions</title>

	<p>
		Verifying that a given function is a solution to a differential equation amounts to showing that it satisfies the equation. This typically involves taking any necessary derivatives of the function, substituting them into the equation, and simplifying both sides to determine whether they match. Here are some examples to illustrate this process.
	</p>

	<example>
		<statement>
			<p>
				Verify that <m>y = 2x^2\ </m> is a solution to <m>\ \ xy' - 2x^2 = y</m>.
			</p>
		</statement>
		
		<solution>
			<p>
				First, compute <m>y' = 4x</m> and plug both <m>y = 2x^2</m> and <m>y' = 4x</m> into the equation:
				<md>
					<mrow> x\left( 4x \right) - 2x^2	\amp= \left( 2x^2 \right) </mrow>
					<mrow> 								4x^2 - 2x^2	\amp= 2x^2 </mrow>
					<mrow>											2x^2	\amp= 2x^2	\quad✅</mrow>
				</md>
				This shows that <m>y = 2x^2</m> satisfies the equation and proves it is a solution.
			</p>
		</solution>
	</example>

	<example>
		<statement>
			<p>
				Verify that <m>P = \sin t\ </m> is a solution to <m>\ \ 2P'' + P = \sin t</m>.
			</p>
		</statement>

		<solution>
			<p>
				Since <m>P''</m> appears, compute the derivatives first:
				<me>	
					P = \sin t, \quad P' = \cos t, \quad P'' = -\sin t
				</me>
			</p>

			<p>
				Now substitute in the dependent variable along with its derivatives:
				<md>
					<mrow> 
						2\left( -\sin t \right) + \left( \sin t \right)	\amp = \sin t
					</mrow>
					<mrow>													-2\sin t + \sin t	\amp = \sin t </mrow>
					<mrow>																		-\sin t	\amp \ne \sin t \quad❌</mrow>
				</md>
				Since the function on the left is different from the function on the right, <m>P = \sin t</m> does <term>not</term> satisfy the equation and is <term>not</term> a solution.
			</p>
		</solution>
	</example>

	<p>
		As you will soon learn, differential equations have many solutions and all of them share a common form, as the next example shows.
	</p>

	<example xml:id="example-whats-a-soln-1">
		<statement>
			<p>
				Show that the functions
				<me>y = e^{2x},\quad y = -5e^{2x},\quad y = \pi e^{2x},\quad y = 0</me>
				are all solutions to the differential equation
				<me>y' - 2y = 0</me>.
			</p>
		</statement>
		<solution>
			<p>
				Rather than verify each function separately, notice that they all are of the form <m>y = c e^{2x}</m>, where <m>c</m> is a constant. Let's verify the general case.
			</p>
			
			<p>
				Substitute <m>y = c e^{2x}</m> into the equation:
				<me>
					y' - 2y = (c e^{2x})' - 2(c e^{2x})	= 2c e^{2x} - 2c e^{2x}	= 0 \quad✅
				</me>
				So <m>y = c e^{2x}</m> is a solution for any constant <m>c</m>. In particular, this includes the functions
				<me>
					y = e^{2x},\quad y = -5e^{2x},\quad y = \pi e^{2x},\quad y = 0
				</me>
				for the constants <m>c = 1, -5, \pi, 0</m> respectively.
			</p>
		</solution>
	</example>

	<p>
		As you saw in the previous example, solutions can differ by a constant. Some solutions even involve multiple constants, as the next example shows.
	</p>

	<example xml:id="example-whats-a-soln-2">
		<statement>
			<p>
				Verify that <m>\ y = c_1\ x^2 + c_2 - \ln x\ </m> is a solution to
				<me>x^2y'' - xy' = 2</me>.
			</p>
		</statement>
		<solution>
			<p>
				Compute needed derivatives
				<me>
					y = c_1\ x^2 + c_2 - \ln x \ \ \Rightarrow \ \ 
					y' = 2 c_1\ x - \frac{1}{x} \ \ \Rightarrow \ \ 
					y'' = 2 c_1 + \frac{1}{x^2}
				</me>
				and substitute into the equation:
				<md>
					<mrow> 
						x^2\left( 2 c_1 + \frac{1}{x^2} \right) - x\left( 2 c_1\ x - \frac{1}{x} \right)
							\amp = 2
					</mrow>
					<mrow>
						2 c_1\ x^2 + 1 - 2 c_1\ x^2 + 1
							\amp = 2
					</mrow>
					<mrow>
						2	\amp = 2 \quad✅
					</mrow>
				</md>
				Thus, <m>\ y = c_1\ x^2 + c_2 - \ln x\ </m> is a solution to <m>x^2y'' - xy' = 2</m>.
			</p>
		</solution>
	</example>

</section>
