<subsection xmlns:xi="http://www.w3.org/2001/XInclude"><title> Overview </title>
	
	<p>
		The Laplace transform solution technique is less direct than other solution techniques. We typically start with a DE in terms of an independent variable <m>t</m>. Let's assume the dependent variable is <m>y</m> for now, so our goal is to solve for an unknown function <m>y</m> in terms of the independent variable <m>t</m>. We take the Laplace transform of the DE, and the result is an algebraic equation in terms of the variable <m>s</m> and a function <m>Y(s)</m>. We then solve for <m>Y(s)</m> using algebra. Finally, we get our desired solution by taking the inverse Laplace transform, as shown in figure (Figure number).
	</p>

	<!-- <p>
		<sidebyside widths="75%" margins="auto" valign="middle">
			<figure xml:id="LT-Diagram">
			<title/>
				<image source="figures/fig1.png" />
			</figure>
		</sidebyside>
	</p> -->

	<!-- <p>
		<assemblage xml:id="LT-Diagram">
			<tabular>
				<col halign="center" valign="middle" />
				<col halign="center" valign="middle" />
				<col halign="center" valign="middle" />
				<row>
					<cell>
						<line><m>y'' + 3y' + 2y = -40e^{3t}</m></line>
						<line><m>{\scriptsize y(0) = 0, \quad y'(0) = -9}</m></line>
					</cell>
					<cell><m>\large \overset{\Large \lap}{\underset{\text{forward}}{\longrightarrow}}</m></cell>
					<cell><m>\ds s^2Y + 3sY + 2Y + 9 = \frac{-40}{s-3}</m></cell>
				</row>
				<row>
					<cell/>
					<cell/>
					<cell><m>|</m></cell>
				</row>
				<row>
					<cell/>
					<cell/>
					<cell><m>\text{Solve for } Y</m></cell>
				</row>
				<row>
					<cell/>
					<cell/>
					<cell><m>\downarrow</m></cell>
				</row>
				<row>
					<cell/>
					<cell/>
					<cell><m>\ds Y = \frac{-1}{s^2+3s+2}\left(9 + \frac{40}{s-3}\right)</m></cell>
				</row>
				<row>
					<cell/>
					<cell/>
					<cell><m>|</m></cell>
				</row>
				<row>
					<cell/>
					<cell/>
					<cell>Prepare Backward Transform</cell>
				</row>
				<row>
					<cell/>
					<cell/>
					<cell><m>\downarrow</m></cell>
				</row>
				<row>
					<cell><m>y = e^{-t} + e^{-2t} - 2e^{3t}</m></cell>
					<cell><m>\large \overset{\Large \lap^{-1}}{\underset{\text{backward}}{\longleftarrow}}</m></cell>
					<cell><m>\ds Y = \frac{1}{s+1} - \frac{1}{s+2} + \frac{2}{s-3}</m></cell>
				</row>
			</tabular>
		</assemblage>
	</p> -->

	<p>
		<image source="figures/LT-Diagram-Focused-Step-1.png" width="100%">
			<shortdescription>(for accessibility)</shortdescription>
		</image>
	</p>

	<p>
		Before we solve any DEs with this new solution technique, we need to practice the pieces of the solution technique. Thus, we dedicate the next couple of sections on learning what the Laplace transform is, how to find the Laplace transform of a function, and how to take the inverse Laplace transform of a function. Then we will finally be solve DEs using this new solution technique.
	</p>

	<xi:include href="./c4-s4-ss1-interactives.ptx" />

</subsection>
