<!-- LICENSING
  This file is part of the textbook "Exploring Differential Equations, An Interactive, Student-Centered Approach" by Geoffrey Cox.
  License: Creative Commons Attribution-ShareAlike 4.0 International (CC BY-SA 4.0)
  You are free to:
    • Share — copy and redistribute the material in any medium or format.
    • Adapt — remix, transform, and build upon the material for any purpose, even commercially.
  Under the following terms:
    • Attribution — You must give appropriate credit, provide a link to the license, and indicate if changes were made.
    • ShareAlike — If you remix, transform, or build upon the material, you must distribute your contributions under the same license.
  Full license text: https://creativecommons.org/licenses/by-sa/4.0/legalcode
  Recommended attribution: "Exploring Differential Equations" by Geoffrey Cox, licensed CC BY-SA 4.0"
-->
<section xml:id="review-exponents-logarithms">
	<title>Exponential and Logarithmic Functions</title>

	<p>
		Exponential and logarithmic expressions appear constantly in differential equations. They arise in the solutions of linear equations, in the Laplace transform and its inverse, and in modeling exponential growth, decay, and oscillation. This review gathers the essential algebraic rules you’ll use throughout the course.
	</p>

	<assemblage>
		<title>✳️ Exponential Rules</title>

		<tabular>
			<col halign="center" />
			<col />
			<col halign="center" />
			<row halign="center">
				<cell/>
				<cell bottom="minor">General</cell>
				<cell/>
				<cell bottom="minor">Natural (<m>a=e</m>)</cell>
			</row>
			<row bottom="none">
				<cell><m>E_1:</m></cell>
				<cell>
					<md><mrow xml:id="exp_rule_01">\ds (ab)^x = a^x \cdot b^x</mrow></md>
				</cell>
				<cell/>
				<cell>
					<md><mrow xml:id="exp_rule_01e">\ds (eb)^x = e^x \cdot b^x</mrow></md>
				</cell>
			</row>
			<row bottom="none">
				<cell><m>E_2:</m></cell>
				<cell>
					<md><mrow xml:id="exp_rule_02">\ds a^x \cdot a^y = a^{x+y}</mrow></md>
				</cell>
				<cell/>
				<cell>
					<md><mrow xml:id="exp_rule_02e">\ds e^x \cdot e^y = e^{x+y}</mrow></md>
				</cell>
			</row>
			<row bottom="none">
				<cell><m>E_3:</m></cell>
				<cell>
					<md><mrow xml:id="exp_rule_03">\ds (a^x)^y = a^{xy}</mrow></md>
				</cell>
				<cell/>
				<cell>
					<md><mrow xml:id="exp_rule_03e">\ds (e^x)^y = e^{xy}</mrow></md>
				</cell>
			</row>
			<row bottom="none">
				<cell><m>E_4:</m></cell>
				<cell>
					<md><mrow xml:id="exp_rule_04">\ds a^{-x} = \frac{1}{a^x}</mrow></md>
				</cell>
				<cell/>
				<cell>
					<md><mrow xml:id="exp_rule_04e">\ds e^{-x} = \frac{1}{e^x}</mrow></md>
				</cell>
			</row>
		</tabular>
	</assemblage>

	<assemblage>
		<title>✳️ Logarithmic Rules</title>

		<tabular>
			<col halign="center" />
			<col />
			<col halign="center" />
			<row halign="center">
				<cell/>
				<cell bottom="minor">General</cell>
				<cell/>
				<cell bottom="minor">Natural (<m>a=e</m>)</cell>
			</row>
			<row bottom="none">
				<cell><m>L_1:</m></cell>
				<cell>
					<md><mrow xml:id="log_rule_01">\ds \log_b (b^x) = x</mrow></md>
				</cell>
				<cell/>
				<cell>
					<md><mrow xml:id="ln_rule_01">\ds \ln(e^x) = x</mrow></md>
				</cell>
			</row>
			<row bottom="none">
				<cell><m>L_2:</m></cell>
				<cell>
					<md><mrow xml:id="log_rule_02">\ds b^{\log_b(x)} = x</mrow></md>
				</cell>
				<cell/>
				<cell>
					<md><mrow xml:id="ln_rule_02">\ds e^{\ln(x)} = x</mrow></md>
				</cell>
			</row>
			<row bottom="none">
				<cell><m>L_3:</m></cell>
				<cell>
					<md><mrow xml:id="log_rule_03">\ds \log_b(1) = 0</mrow></md>
				</cell>
				<cell/>
				<cell>
					<md><mrow xml:id="ln_rule_03">\ds \ln(1) = 0</mrow></md>
				</cell>
			</row>
			<row bottom="none">
				<cell><m>L_4:</m></cell>
				<cell>
					<md><mrow xml:id="log_rule_04">\ds \log_b(xy) = \log_b(x) + \log_b(y)</mrow></md>
				</cell>
				<cell/>
				<cell>
					<md><mrow xml:id="ln_rule_04">\ds \ln(xy) = \ln(x) + \ln(y)</mrow></md>
				</cell>
			</row>
			<row bottom="none">
				<cell><m>L_5:</m></cell>
				<cell>
					<md><mrow xml:id="log_rule_05">\ds \log_b\left(\frac{\ds x}{\ds y}\right) = \log_b(x) - \log_b(y)</mrow></md>
				</cell>
				<cell/>
				<cell>
					<md><mrow xml:id="ln_rule_05">\ds \ln\left(\frac{\ds x}{\ds y}\right) = \ln(x) - \ln(y)</mrow></md>
				</cell>
			</row>
		</tabular>
	</assemblage>

	<p>
		These identities will help you solve equations involving exponentials or logarithms—common in modeling growth and decay, solving linear ODEs, and interpreting Laplace transforms.
	</p>

	<example xml:id="r-01-04-exp_logs_ex_01">
		<p>
			Solve for <m>x</m>: <m>\ds \quad e^{3x+z} - e^z = y</m>
		</p>
		<solution>
			
			<p>
				We might begin by isolating the exponential that contains <m>x</m> and then
				taking the natural log of both sides.

				<md>
					<mrow>
						e^{3x+z} - e^z			\amp = y
					</mrow>
					<mrow>
						e^{3x+z} 				\amp = y + e^z
					</mrow>
					<mrow>
						<xref text="custom" ref="ln_rule_01"><m>\overset{L_1}{\hookrightarrow}\qquad</m></xref>
						\ln\big(e^{3x+z}\big)	\amp = \ln\big(y + e^z\big)
					</mrow>
					<mrow>
						3x + z					\amp = \ln\big(y + e^z\big)
					</mrow>
					<mrow>
						3x						\amp = \ln\big(y + e^z\big) - z
					</mrow>
					<mrow>
						x						\amp = \frac{1}{3}\ln\big(y + e^z\big) - \frac{1}{3}z
					</mrow>
				</md>
			</p>

			<p>
				It's worth noting that we cannot break up that log on the right hand side.
				There's no "rule" that helps when we have addition inside a logarithm.
			</p>

			<p>
				There is another way to approach this if notice that <m>z</m> appears inside both
				exponential terms.

				<md>
					<mrow>
						<xref text="custom" ref="exp_rule_02e"><m>\overset{E_2}{\hookrightarrow}\qquad</m></xref>
						e^{3x+z} - e^z			\amp = y
					</mrow>
					<mrow>
						e^{3x}\cdot e^{z} - e^z	\amp = y
					</mrow>
					<mrow>
						e^z(e^{3x} - 1)			\amp = y
					</mrow>
					<mrow>
						e^{3x} - 1				\amp = \frac{y}{e^z}
						<xref text="custom" ref="exp_rule_04e"><m>\qquad\overset{E_4}{\hookleftarrow}</m></xref>
					</mrow>
					<mrow>
						e^{3x} - 1				\amp = ye^{-z}
					</mrow>
					<mrow>
						e^{3x}					\amp =  ye^{-z} + 1
					</mrow>
					<mrow>
						<xref text="custom" ref="ln_rule_01"><m>\overset{L_1}{\hookrightarrow}\qquad</m></xref>
						\ln\big( e^{3x} \big)	\amp = \ln \big( ye^{-z} + 1\big)
					</mrow>
					<mrow>
						3x						\amp = \ln \big( ye^{-z} + 1 \big)
					</mrow>
					<mrow>
						x						\amp = \frac{1}{3}\ln\big(ye^{-z}+1\big)
					</mrow>
				</md>
				The answers may look different, but they are equivalent and both are correct.
			</p>
		</solution>
	</example>

	<example xml:id="r-01-04-exp_logs_ex_02">
		<p>
			Solve for <m>x</m>: <m>\ds \quad \ln(x+y) = 5 + \ln(z)</m>
		</p>

		<solution>


			<p>
				We'll carefully apply the rules above. We want to get our hands on <m>x</m>,
				and right now its inside a logarithm. In order to undo that, we'll exponentiate
				both sides.

				<md>
					<mrow>	
						\ln(x+y)		\amp = 5 + \ln(z)
					</mrow>
					<mrow>
						<xref text="custom" ref="ln_rule_02"><m>\overset{L_2}{\hookrightarrow}\qquad</m></xref>
						e^{\ln(x+y)}	\amp = e^{\big(5 + \ln(z)\big)}				
						<xref text="custom" ref="exp_rule_02e"><m>\qquad\overset{E_2}{\hookleftarrow}</m></xref>
					</mrow>
					<mrow>
						x + y			\amp = e^{5} \cdot e^{\ln(z)}		
						<xref text="custom" ref="ln_rule_02"><m>\qquad\overset{L_2}{\hookleftarrow}</m></xref>
					</mrow>
					<mrow>
						x				\amp = e^{5}z - y
					</mrow>
				</md>

			</p>
		</solution>

	</example>

	<p>Now you try. Solve for <m>x</m> in each of the following equations using the rules above.</p>

	<ol>
		<li>
		<m>e^{x + y} = 12</m>
		<solution><md>
			<mrow>x = \ln(12) - y</mrow>
		</md></solution>
		<answer><me>x = \ln(12) - y</me></answer>
		</li>

		<li>
		<m>e^{x + y} + e^x = 12</m>
		<solution><md>
			<mrow>e^x(e^y + 1) = 12</mrow>
			<mrow>e^x = \frac{12}{e^y + 1}</mrow>
			<mrow>x = \ln(12) - \ln(e^y + 1)</mrow>
		</md></solution>
		<answer><me>x = \ln\left( \frac{12}{e^y + 1} \right)</me></answer>
		</li>

		<li>
		<m>e^x = 1</m>
		<solution><md>
			<mrow>x = \ln(1) = 0</mrow>
		</md></solution>
		<answer><me>x = 0</me></answer>
		</li>

		<li>
		<m>\ln x = 3 \ln z</m>
		<solution><md>
			<mrow>x = e^{\ln(z^3)} = z^3</mrow>
		</md></solution>
		<answer><me>x = z^3</me></answer>
		</li>

		<li>
		<m>y + \ln x = 4</m>
		<solution><md>
			<mrow>x = e^{4 - y}</mrow>
		</md></solution>
		<answer><me>x = e^{4 - y}</me></answer>
		</li>

		<li>
		<m>\ln y + \ln x = 4</m>
		<solution><md>
			<mrow>\ln(xy) = 4</mrow>
			<mrow>xy = e^4</mrow>
			<mrow>x = \frac{e^4}{y}</mrow>
		</md></solution>
		<answer><me>x = \frac{e^4}{y}</me></answer>
		</li>

		<li>
		<m>\ln x = 8 \ln y + 5</m>
		<solution><md>
			<mrow>x = e^{5} \cdot e^{\ln(y^8)} = e^5 y^8</mrow>
		</md></solution>
		<answer><me>x = e^5 y^8</me></answer>
		</li>
	</ol>

	<definition xml:id="eulers-formula">
		<title>Euler's Formula</title>
		<statement>
		<p>Euler’s formula relates complex exponentials to trigonometric functions. For any real number <m>\theta</m>:</p>
		<me>e^{i\theta} = \cos(\theta) + i\sin(\theta)</me>
		<p>As a result, we also have:</p>
		<me>e^{a + ib} = e^a \cdot e^{ib} = e^a(\cos(b) + i\sin(b))</me>
		<p>This identity is fundamental in solving linear differential equations with complex roots.</p>
		</statement>
	</definition>
</section>
