<subsection xmlns:xi="http://www.w3.org/2001/XInclude"><title>Writing Piecewise Functions in terms of Unit-Step Functions</title>
	
	<p>
		In the previous section, we were learning the definition of unit step function and finding a piecewise defined formula for the function. This was an important step for us as we got used to unit step functions, but we what we really need is to be able to do the opposite of what we have been doing in the previous section: when given a piecewise defined function, we need to be able to write the function in terms of unit step functions. Once we have this skill, we will focus on taking Laplace transforms involving unit step functions, which we will need when we solve DEs.
	</p>

	<p>
		Another useful way to think about unit step functions is to think about them as being on or off.  For example, <m>U(t-2)</m> has a value of zero, or is 'turned off', when <m>t \lt 2</m>, and when <m>t \gt 2,</m> <m>U(t-2)</m> has a value of 1, or is 'turned on'.  Framing unit step functions this way may be helpful as we move forward and consider more complicated functions.
	</p>

	<example><title> Complete the following for the function <m>w(t)</m> </title>

		<p>
			<me>w(t) = 6 + 5\ U(t-1) - 4\ U(t-3)</me>.
		</p>

		<solution><title> Sketch <m>w(t)</m> </title>
			<p>
				We can begin by identifying <m>t</m>-values where the function changes behavior.  We know that <m>U(t-1)</m> changes behavior at <m>t = 1</m> and <m>U(t-3)</m> changes behavior at <m>t = 3,</m>	so <m>w(t)</m> will change behavior at both <m>t = 1</m> and <m>t = 3.</m>  These <m>t</m>-values break the	<m>t</m>-number line into three regions:  (1)  <m>t \lt 1</m>, (2) <m>1 \lt t \lt 3,</m> and (3) <m>t \gt 3.</m>

				<image xml:id="unit-step-number-line-01" width="60%">
					<latex-image>
						\begin{tikzpicture}
							% Axis, ticks, and labels
							\draw[latex-latex] (-2.5,0) -- (5.5,0);
							\foreach \x in {-2,-1,0,1,2,3,4,5} \draw[shift={(\x,0)},color=black] (0pt,3pt) -- (0pt,-3pt);
							\foreach \x in {-2,-1,0,1,2,3,4,5} \draw[shift={(\x,0)},color=black] (0pt,0pt) -- (0pt,-3pt) node[below] {$\x$};

							\draw [line width=1.5mm, red  , opacity=0.3] (-2.5,0) -- node[align=center,above, opacity=1] {t \lt\ 1} (1,0) ;
							\draw [line width=1.5mm, black!60!green, opacity=0.3] (1,0)	-- node[align=center,above, opacity=1] {1 \lt\ t \lt\ 3} (3,0) ;
							\draw [line width=1.5mm, blue , opacity=0.3] (3,0)	-- node[align=center,above, opacity=1] {t \gt\ 3} (5.5,0) ;
						\end{tikzpicture}
					</latex-image>
				</image>

				<ul>
					<li>
						<p>
							<em> If we choose <m>t</m>-values such that <m>t \lt 1</m> (red):</em>
							<ul>
								<li><m>t-1</m> is negative, so <m>U(t-1) = 0,</m></li>
								<li><m>t-3</m> is negative, so <m>U(t-3) = 0.</m></li>
							</ul>
							<aside>
								<p>How about this for formatting the analysis?</p>
							</aside>
							Therefore, when <m>t \lt 1</m> (red), we have
							<me>w(t) = 6 + 5\ U(t-1) - 4\ U(t-3) = -3 + 5\cdot 0 - 4\cdot 0 = 6.</me>
						</p>
					</li>
				
					<li>
						<em> If we choose <m>t</m>-values such that <m>1 \lt t \lt 2</m>:</em> then <m>t - 1</m> is positive, so <m>U(t-1) = 1,</m>	and <m>t - 2</m> is negative, so <m>U(t-2) = 0.</m> Therefore  when <m>1 \lt t \lt 2,</m>	<m>w(t) = 6 + 5\ U(t-1) - 4\ U(t - 2) = 6 + 5\cdot 1 - 4 \cdot 0 = 11.</m>
					</li>
				
					<li>
						<em> If we choose <m>t</m>-values such that <m>t \gt 2</m>:</em> then <m>t - 1</m> is positive, so <m>U(t-1) = 1,</m>	and <m>t - 2</m> is positive, so <m>U(t-2) = 1.</m> Therefore  when <m>t \gt 2,</m>	<m>w(t) = 6 + 5\ U(t-1) - 4\ U(t - 2) = 6 + 5\cdot 1 - 4 \cdot 1 = 7.</m>
					</li>
				</ul>
			</p>

			<p>
				Thus, we can sketch the function as shown below.
				<image xml:id="unit-step-w-plot1" width="60%">
					<sageplot>
						U = plot(6, (x, -2, 0.9), color='red', thickness=4, ymin=-1, ymax=11.5, fontsize=20, ticks=[list(range(-2,6)),list(range(1,12,2))])
						U += plot(11, (x, 1, 1.9), color='green', thickness=4)
						U += plot(7, (x, 2, 5), color='blue', thickness=4)
						U += point([1,6], color = "red", faceted=True, size = 80)
						U += point([1,6], color = "white", faceted=True, size = 15)
						U += point([1,11], color = "green", faceted=True, size = 80)
						U += point([2,11], color = "green", faceted=True, size = 80)
						U += point([2,11], color = "white", faceted=True, size = 15)
						U += point([2,7], color = "blue", faceted=True, size = 80)
						U
					</sageplot>
				</image>
			</p>
		</solution>

		<solution><title> Write <m>w(t)</m> as a piecewise function. </title>
			<p>
				The piecewise defined function representation of <m>w(t)</m> is
				<me>w(t) = \left\{
					\begin{array}{ll}
						6,	&amp; t \lt 1,\\
						11,	&amp; 1\le t \lt 2,\\
						7,	&amp; t \ge 2.
					\end{array} \right.
				</me>
			</p>
		</solution>
	</example>

	<p>
		What lessons can we take away from this example?  When <m>t \lt 1,</m> both of the unit step functions are 'turned off', so the only thing contributing to the function is the constant term, <m>6.</m>  At <m>t = 1,</m> the first unit step function, <m>5\ U(t-1),</m> 'turns on', and the result is a jump discontinuity in the graph of the function at <m>t = 1,</m> and the function jumps from a value of <m>6</m> to a value of <m>6+5 = 11.</m>
	</p>

	<p>
		The function changes behavior next at <m>t = 2</m>, when the <m>-4\ U(t-2)</m> function 'turns on' and therefore the function jumps from the previous value of <m>11</m> to its final value of <m>11 + (-4) = 7.</m>
	</p>

	<example><title> Complete the following for the function <m>z(t)</m> </title>
	
		<p>
			<me>z(t) = 7 - 7\ U(t-2) + t^2\ U(t-4)</me>.
		</p>

		<solution><title> Evaluate <m>z(1)</m> </title>
			<p>
				<md>
					<mrow> z(1)	=\amp\ 7 - 7\ U(1-2) + (1)^2\ U(1-4)</mrow>
					<mrow>		=\amp\ 7 - 7\ \ub{U(-1)}_{=\ 0} + \ub{U(-3)}_{=\ 0} = 7</mrow>
				</md>
			</p>
		</solution>
		
		<solution><title> Evaluate <m>z(3)</m> </title>
			<p>
				<md>
					<mrow> z(3)	=\amp\ 7 - 7\ U(3-2) + (3)^2\ U(3-4)</mrow>
					<mrow>		=\amp\ 7 - 7\ \ub{U(1)}_{=\ 1} + 9\ \ub{U(-1)}_{=\ 0} = 0</mrow>
				</md>
			</p>
		</solution>

		<solution><title> Evaluate <m>z(10)</m> </title>
			<p>
				<md>
					<mrow> z(10)	=\amp\ 7 - 7\ U(10-2) + (10)^2\ U(10-4)</mrow>
					<mrow>			=\amp\ 7 - 7\ \ub{U(8)}_{=\ 1} + 100\ \ub{U(7)}_{=\ 1} = 100</mrow>
				</md>
			</p>
		</solution>

		<solution><title> Sketch <m>z(t)</m> </title>
			<p>
				We can begin by identifying <m>t</m>-values where the function changes behavior.  We
				know that <m>U(t-2)</m> changes behavior at <m>t = 2</m> and <m>U(t-4)</m> changes behavior at <m>t = 4,</m>
				so <m>z(t)</m> will change behavior at both <m>t = 2</m> and <m>t = 4.</m>  These <m>t</m>-values break the
				<m>t</m>-number line into three regions:  (1)  <m>t \lt 2</m>, (2) <m>2 \lt t \lt 4,</m> and (3) <m>t \gt 4.</m> (INSERT A SMALL
				PICTURE OF A NUMBER LINE IN THE MARGIN HERE?)
			</p>

			<ul>
			
				<li>
					<em> If we choose <m>t</m>-values such that <m>t \lt 2</m>:</em> Then <m>t - 2</m> is negative, so <m>U(t-2) = 0,</m>
					and <m>t - 4</m> is negative, so <m>U(t-4) = 0.</m> Therefore  when <m>t \lt 2,</m>
					<m>z(t) = 7 - 7\ U(t-2) +t^2\ U(t - 4) = 7 - 7\cdot 0 + t^2\cdot 0 = 7.</m>
				</li>
			
				<li>
					<em> If we choose <m>t</m>-values such that <m>2 \lt t \lt 4</m>:</em> then <m>t - 2</m> is positive, so <m>U(t-2) = 1,</m>
					and <m>t - 4</m> is negative, so <m>U(t-4) = 0.</m> Therefore  when <m>2 \lt t \lt 4,</m>
					<m>z(t) = 7 - 7\ U(t-2) - t^2\ U(t - 4) = 7 + 7\cdot 1 + t^2 \cdot 0 = 0.</m>
				</li>
			
				<li>
					<em> If we choose <m>t</m>-values such that <m>t \gt 4</m>:</em> then <m>t - 2</m> is positive, so <m>U(t-2) = 1,</m>
					and <m>t - 4</m> is positive, so <m>U(t-4) = 1.</m> Therefore  when <m>t \gt 4,</m>
					<m>z(t) = 7 - 7\ U(t-2) - t^2\ U(t - 4) = 7 - 7\cdot 1 + t^2\cdot 1 = t^2.</m>
				</li>
			</ul>
			<p>
				We see that when <m>t \gt 4</m>, the function should look like the parabola <m>t^2.</m>
				Thus, we can sketch the function as shown below.
				<image xml:id="unit-step-3term-w-t-squared-plot" width="60%">
					<sageplot>
						U = plot(0, (x, -2, 1.9), color='blue', thickness=4, ymin=-2.5, ymax=1.5, fontsize=20, ticks=[1,1])
						U += plot(-2, (x, 2, 5), color='blue', thickness=4, ymin=-2.5, ymax=1.5, fontsize=20, ticks=[1,1])
						U += point([2,0], color = "blue", faceted=True, size = 80)
						U += point([2,0], color = "white", faceted=True, size = 15)
						U += point([2,-2], color = "blue", faceted=True, size = 80)
						U
					</sageplot>
				</image>
			</p>
		</solution>

		<solution><title> Write <m>z(t)</m> as a piecewise function. </title>
			<p>
				We can write <m>z(t)</m> as a piecewise defined function as follows.
				<me>
					z(t) = \left\{
					\begin{array}{ll}
						7,	\amp t \lt 2,\\
						0,	\amp 2\le t \lt 4,\\
						t^2,\amp t \ge 4.
					\end{array} \right.
				</me>
			</p>
		</solution>
		
	</example>

	<p>
		Let's step back again and see what we can generalize from this example.  Notice that this function had a value of <m>7</m> for <m>t \lt 2.</m>  Then the unit step function <m>U(t-2)</m> became relevant, but because its coefficient was <m>-7</m>, it had the effect of 'turning off' the <m>7</m> that was already present.  It can be helpful for us moving forward to be able to think about negative coefficients as 'turning off' a function.
	</p>

	<p>
		This is also the first example that demonstrates a non-constant coefficient.  Notice that it behaves no differently than a constant coefficient; the unit step function served to turn the function on after <m>t = 4.</m>
	</p>

	<p>
		Let's reflect on what happened.  For the function <m>h(t) = 3\ U(t-2),</m> the 2 indicates that the function changes behavior at <m>t = 2,</m> and the 3 changes the amplitude of the nonzero portion of the function.
	</p>

	<example>
		<p>
			Sketch the function <m>s(t) = \sin t + (-\sin t + 4 - t)U(t-\pi).</m>
		</p>
				
		<p/>
		<solution>
			<p>
				We first identify where the function will change behavior.  In this case, it will change behavior
				only at <m>t = \pi.</m>  We can then think about the functions behavior for <m>t \lt \pi</m> and for <m>t \ge \pi.</m>  Notice
				that when <m>t \lt \pi,</m>  <m>U(t-\pi) = 0,</m> and therefore <m>s(t) = \sin t.</m>  When <m>t \ge \pi,</m> <m>U(t-\pi) = 1,</m> and then
				we have <m>s(t)= \sin t + (-\sin t +4 - t) \cdot 1 = 4 - t.</m>  This means we could write <m>s(t)</m> as the following piecewise
				defined function, and sketch it .
				<md>s(t) = \left\{
					\begin{array}{ll}
						\sin t,	\amp t \lt \pi,\\
						4 - t,	\amp t \ge \pi.
					\end{array} \right.
				</md>
			</p>

			<p>
				(INSERT FIGURE HERE)
			</p>
		</solution>
	</example>


	<example>
		<p>
			Sketch the function <m>v(t) = t+5 - (t+5)U(t-2) + (t-4)U(t-3).</m>
		</p>
		
		<p/>
		<solution>
			<p>
				We first identify where the function will change behavior: <m>t = 2</m> and <m>t = 3.</m> Since there are two <m>t</m>-values where the function changes behavior, we need to consider three regions of the number line:  (1) <m>t \lt 2</m>, (2) <m>2 \lt t \lt 3</m>, and (3) <m>t \gt 3.</m>

				<ul>
				
					<li>
						When <m>t \lt 2</m>, both unit step functions are 'turned off', so <m>v(t) = t+5.</m>
					</li>
					
					<li>
						When <m>2\le t \lt 3,</m> <m>v(t) = </m>
					</li>

				</ul>

				<md>s(t) = \left\{
					\begin{array}{ll}
						\sin t,	\amp t \lt \pi,\\
						4 - t,	\amp t \ge \pi.
					\end{array} \right.
				</md>
			</p>

			<p>
				(INSERT FIGURE HERE)
			</p>
		</solution>
	</example>

	<p>
		Now that we've determined what the function looks like, we can look back at the formula for	the function and see that we start with a sine function, but then at <m>t = \pi,</m> the sine function gets 'turned off' (because of the negative sign) and the linear function <m>4 - t</m> gets 'turned on'.
	</p>

	<example xml:id="ex_sketch_write_f_as_pw_func">
		<p>
			Sketch the function
			<me>
				f(t) = \left\{
				\begin{array}{ll}
					e^t,	\amp t \lt 1,\\
					t^3	\amp t \ge 1,
				\end{array} \right.
			</me>
			and then write the function in terms of unit step functions.
		</p>

		<p>
			(include a sketch of the function here)
		</p>

		<p/>
		<solution>
			<p>
				The first thing we want to take note of is for what <m>t</m>-values the function changes behavior. This function changes behavior at <m>t = 1,</m> and we will use a unit step function to help us capture that change in behavior, so we need a unit step function that has a discontinuity at <m>t = 1.</m> That is, we know we need at <m>U(t-1).</m> Thus, the form of our function is
				<me> f(t) = <fillin>{50}</fillin> + <fillin>{50}</fillin>\cdot U(t-1). </me>
			</p>

			<p>
				Now we need only determine what goes in the blanks. When <m>t \lt 1,</m> the unit step function <m>U(t-1)</m> will have a value of zero. We also know that when <m>t \lt 1,</m> <m>f(t) = e^t.</m> Therefore the first blank must be <m>e^t.</m> That is,
				<me> f(t) = e^t + <fillin>{50}</fillin>\cdot U(t-1). </me>
			</p>

			<p>
				When <m>t>1,</m> <m>U(t-1) = 1,</m> and <m>f(t) = t^3.</m> Thus we have
				<md>
					<mrow>t \gt 1:	f(t)	=\amp\ e^t + <fillin>{50}</fillin>\cdot 1</mrow>
					<mrow>t^3	=\amp\ e^t + <fillin>{50}</fillin>\cdot 1</mrow>
				</md>
			</p>

			<p>
				In order to make the equation true, it must be that the function that goes in the line is <m>-e^t + t^3,</m> so that we have
				<me> f(t) = e^t + (-e^t + t^3)\cdot U(t-1). </me>
			</p>

			<p>
				This makes sense because when <m>t = 1,</m> we "turn off" the <m>e^t</m> function and "turn on" the <m>t^3</m> function.
			</p>
		</solution>
	</example>
	

	<example xml:id="ex_write_h_as_">
		<p>
			Write the function
			<me>
				h(t) = \left\{
				\begin{array}{ll}
					4,	\amp t \lt 3,\\
					t - 2,	\amp 3 \le t \lt 5,\\
					7,	\amp t \ge 5
				\end{array} \right.
			</me>
			terms of unit step functions.
		</p>

		<p/>
		<solution>
			<p>
				We notice that the function changes behavior at <m>t = 3</m> and <m>t = 5.</m> That means that the form of the function is
				<me> h(t) = <fillin>{50}</fillin> + <fillin>{50}</fillin>\cdot U(t-3) + <fillin>{50}</fillin>\cdot U(t - 5). </me>
			</p>

			<p>
				Based on the previous example, we see that the left-most piece of the piecewise defined function fills in the first blank, as below.
				<me> h(t) = 4 + <fillin>{50}</fillin>\cdot U(t-3) + <fillin>{50}</fillin>\cdot U(t - 5) </me>
			</p>

			<p>
				In the next blank, we need to "turn off" the previous function and turn on new function, as we see here.
				<md>
					<mrow>h(t)	=\amp\ 4 + \Big(-4 + (t - 2)\Big)\cdot U(t-3) + <fillin>{50}</fillin>\cdot U(t - 5)</mrow>
					<mrow>=\amp\ 4 + (t - 6)\cdot U(t-3) + <fillin>{50}</fillin>\cdot U(t - 5)</mrow>
				</md>
			</p>

			<p>
				Similarly, we use the remaining blank to "turn off" the <m>t - 2</m> function and "turn on" the <m>7</m> function.	
				<md>
					<mrow>h(t)	=\amp\ 4 + (t - 6)\cdot U(t-3) + \Big( -(t - 2) + 7 \Big)\cdot U(t - 5)</mrow>
					<mrow>=\amp\ 4 + (t - 6)\cdot U(t-3) + (-t + 9)\cdot U(t - 5)</mrow>
				</md>
			</p>
		</solution>
	</example>

	<xi:include href="./p4-c5-s3-interactives.ptx" />

</subsection>