
<subsection xmlns:xi="http://www.w3.org/2001/XInclude"><title> Exercises </title>

	<xi:include href="./c10-exercises-conceptual.ptx" />

	<exercises>
		<exercisegroup><title> Turning a Second-Order Equation into a System </title>
			<introduction>
			<p>
				So far, we've looked at systems that involve multiple variables like <m>x(t)</m> and <m>y(t)</m>. But what if you start with just a single second-order differential equation? It turns out you can rewrite it as a system of first-order equations.
			</p>

			<p>
				For example, consider the second-order equation:
			</p>

			<me>
				y'' + 3y' + 2y = 0
			</me>

			<p>
				This equation involves only one dependent variable, <m>y(t)</m>, but it's second-order. To convert it into a system, we introduce a new variable:
			</p>

			<me>
				u = y, \quad v = y'
			</me>

			<p>
				That means <m>u' = y' = v</m>. And since <m>y'' = v'</m>, we can rewrite the original equation as:
			</p>

			<me>
				v' = -3v - 2u
			</me>

			<p>
				Now we have a system of two first-order equations:
			</p>

					<md>
				<mrow> u' \amp = v </mrow>
				<mrow> v' \amp = -3v - 2u </mrow>
			</md>
			</introduction>

			<exercise label="chkpt-building-up-to-systems-1-3-10"><title>Derivative Substitution</title>
				<statement correct="yes">
					<p>
						In order to rewrite a second-order equation as a system, we can replace <m>y'</m> with a new variable and then express <m>y''</m> as the derivative of that new variable.
					</p>
				</statement>
				<feedback>
					<p>
						Correct. Introducing <m>x_1 = y</m> and <m>x_2 = y'</m> allows us to write <m>y''</m> as <m>x_2'</m> and form a system.
					</p>
				</feedback>
			</exercise>

			<exercise><title> Answer the Following </title>
				<task label="rqs-building-up-to-systems-1-3-1"><title>Understanding Converted Systems</title>
				<statement>
					<p>
					When you convert a second-order equation into a first-order system, which of the following are always true?
					</p>
				</statement>
				<choices>
					<choice correct="yes">
					<statement><p>The system has two first-order equations.</p></statement>
					<feedback><p>Yes. One for <m>y</m> and one for <m>y'</m>.</p></feedback>
					</choice>
					<choice correct="yes">
					<statement><p>The system involves two new variables: one for <m>y</m>, one for <m>y'</m>.</p></statement>
					<feedback><p>Exactly. This substitution is the key step.</p></feedback>
					</choice>
					<choice>
					<statement><p>The resulting system is always uncoupled.</p></statement>
					<feedback><p>Not true. The new variables often depend on each other.</p></feedback>
					</choice>
					<choice correct="yes">
					<statement><p>The system represents the same solutions as the original equation.</p></statement>
					<feedback><p>Correct. It's just a different form of the same information.</p></feedback>
					</choice>
					<choice>
					<statement><p>You can only use this method for linear equations.</p></statement>
					<feedback><p>This method also works for nonlinear second-order equations.</p></feedback>
					</choice>
				</choices>
				</task>

				<task label="rqs-building-up-to-systems-1-3-2"><title>Match Equations to Their Systems</title>
				<statement>
					<p>
					Match each second-order differential equation to the correct system using <m>x_1 = y</m> and <m>x_2 = y'</m>.
					</p>
				</statement>
				<feedback>
					<p>
					Each system reflects <m>x_1' = x_2</m> and an expression for <m>x_2'</m> based on <m>y''</m>.
					</p>
				</feedback>
				<cardsort>
					<match>
					<premise><m>y'' + y = 0</m></premise>
					<response><m>x_1' = x_2,\quad x_2' = -x_1</m></response>
					</match>
					<match>
					<premise><m>y'' - 2y' = 0</m></premise>
					<response><m>x_1' = x_2,\quad x_2' = 2x_2</m></response>
					</match>
					<match>
					<premise><m>y'' = y</m></premise>
					<response><m>x_1' = x_2,\quad x_2' = x_1</m></response>
					</match>
					<match>
					<premise><m>y'' = -y'</m></premise>
					<response><m>x_1' = x_2,\quad x_2' = -x_2</m></response>
					</match>
				</cardsort>
				</task>
			</exercise>

			<exercise label="chkpt-building-up-to-systems-1-3-20"><title>From Second Order to System</title>
				<statement>
					<p>
						What is the correct system corresponding to <m>y'' + 4y = 0</m> if we define <m>x_1 = y</m>, <m>x_2 = y'</m>?
					</p>
				</statement>
				<choices>
					<choice>
						<statement><p><m>x_1' = x_2</m>, <m>x_2' = -4x_2</m></p></statement>
						<feedback><p>That would be true if the original equation were <m>y'' + 4y'</m>. Double-check which variable is being multiplied by 4.</p></feedback>
					</choice>
					<choice>
						<statement><p><m>x_1' = x_2</m>, <m>x_2' = -4x_1 + x_2</m></p></statement>
						<feedback><p>Too many termsâ€”there's no <m>y'</m> in the original equation.</p></feedback>
					</choice>
					<choice correct="yes">
						<statement><p><m>x_1' = x_2</m>, <m>x_2' = -4x_1</m></p></statement>
						<feedback><p>Yes! <m>x_2' = y'' = -4y = -4x_1</m> is exactly what we want.</p></feedback>
					</choice>
					<choice>
						<statement><p><m>x_1' = x_1</m>, <m>x_2' = -4x_2</m></p></statement>
						<feedback><p>This system doesn't reflect the original equation at all.</p></feedback>
					</choice>
				</choices>
			</exercise>

			<exercise xml:id="ex-second-order-to-system0">
				<title> From a Second-Order Equation to a System </title>
				<statement>
				<p>
					Rewrite the second-order equation <m>y'' - y = 0</m> as a system of first-order equations.
				</p>
				</statement>
				<solution>
				<p>
					Let <m>u = y</m> and <m>v = y'</m>. Then:
				</p>

				<me>
					u' = v
				</me>
				<p>
					and
				</p>
				<me>
					v' = y'' = y = u
				</me>

				<p>
					So the system becomes:
				</p>

				<md>
					<mrow> u' \amp = v </mrow>
					<mrow> v' \amp = u </mrow>
				</md>
				</solution>
			</exercise>
		</exercisegroup>
	</exercises>

</subsection>