<exercises><title> Step-By-Step Exercises </title>

	<exercise label="c2-ep-drag-n-drop-01" adaptive="yes"><title> <em>Drag-N-Drop</em> </title>

		<statement>
			<p>
				Reorder the steps required to solve the differential equation,
				<me>
					\frac{dy}{dx} - y\cos(x) = y
				</me>,
				using the separation of variables method.
			</p>
		</statement>

		<blocks>
			<block><p>	Check for 1st-order.									</p></block>
			<block><p>	<m>\ds \frac{dy}{dx} = y + y\cos(x) </m>				</p></block>
			<block><p>	<m>\ds \frac{dy}{dx} = (1 + \cos(x))y </m>				</p></block>
			<block><p>	<m>\ds \frac{1}{y} dy = (1 + \cos(x))dx </m>				</p></block>
			<block><p>	<m>\ds \int \frac{1}{y} dy = \int (1 + \cos(x))dx </m>	</p></block>
			<block><p>	<m>\ds \ln|y| = x + \sin(x) + C </m>					</p></block>
			<block><p>	<m>\ds y = Ce^{x + \sin(x)} </m>						</p></block>
		</blocks>

	</exercise>

	<exercise label="c2-cr-ww-02"><title> <em>Solve the Differential Equation</em> </title>

		<introduction>
			<p>
				Complete each step below to solve the differential equation
				<me> \frac{dy}{dx} - y\cos(x) = y.</me>
				These are the same steps used in this chapter's examples. 
			</p>
		</introduction>
			
		<webwork xml:id="c2-cr-ww-02-id"> 
			<description>
				Solve a separable DE using separation of variables.
			</description>

			<pg-code>
				Context()->variables->add(y => 'Real');
				Context()->variables->add(c => 'Real');
				$ans1a = 1;
				$ans1b = Formula("1+cos(x)");
				$ans1c = Formula("y");
				$ans2a = Formula("1+cos(x)");
				$ans2b = Formula("1/y");
				$ans3a = Formula("x+sin(x)");
				$ans3b = Formula("ln|y|");
				$ans = Formula("c*e^(x+sin(x))");
			</pg-code>

			<statement>
				<p>
					<xref ref="sov-step-1" text="title" />. Give the order and separable form:
				</p>

				<p>
					<tabular>
						<col halign="right" />
						<row>
							<cell><m>\text{order:}</m></cell>
							<cell><var name="$ans1a"  width="5" /></cell>
							<cell></cell>
							<cell><m>\displaystyle \frac{dy}{dx} = </m></cell>
							<cell><var name="$ans1b" width="10" /></cell>
							<cell><var name="$ans1c" width="10" /></cell>
							<cell><m>\quad\qquad\leftarrow\text{ separable form}</m></cell>
						</row>
						<row>
							<cell><m>\phantom{\text{order:}}</m></cell>
							<cell></cell>
							<cell></cell>
							<cell><m>\phantom{\displaystyle \frac{dy}{dx} = }</m></cell>
							<cell><m>\overline{\overset{\uparrow}{f(x)}}</m></cell>
							<cell><m>\overline{\overset{\uparrow}{g(y)}}</m></cell>
							<cell></cell>
						</row>
					</tabular>
				</p>

				<p>
					<xref ref="sov-step-2" text="title" />. Divide both sides of the separable form by <m>g(y)</m> and apply the integral to both sides:
				</p>

				<p>
					<tabular halign="center">
						<row>
							<cell><m>\displaystyle\int</m></cell>
							<cell><var name="$ans2b" width="10" /></cell>
							<cell><m>\displaystyle dy = \int </m></cell>
							<cell><var name="$ans2a" width="10" /></cell>
							<cell><m>dx</m></cell>
						</row>
					</tabular>
				</p>

				<p>
					Now, compute the integrals (we have provided the constants):
				</p>

				<p>
					<tabular halign="center">
						<row>
							<cell><var name="$ans3b" width="10" /></cell>
							<cell><m> + c_1 = </m></cell>
							<cell><var name="$ans3a" width="10" /></cell>
							<cell><m> + c_2</m></cell>
						</row>
					</tabular>
				</p>

				<p>
					<em>Don't forget the absolute value on the left antiderivative.</em>
				</p>

				<p>
					<xref ref="sov-step-3" text="title" />. Combine constants as far as possible and use <m>c</m> for the final combined constant.
				</p>

				<p>
					<tabular>
						<col halign="right"/>
						<row>
							<cell>
								<m>y(x) = </m> <var name="$ans" width="10" />
							</cell>
						</row>
					</tabular>
				</p>

			</statement>

		</webwork>

		<hint>
			<p>
				Use the property <m>e^{A + B} = e^{A} \cdot e^{B}</m> to obtain the final combined constant. 
			</p>
		</hint>

	</exercise>

	<exercise><title> Solve the IVP </title>

		<statement>
			<p>
				Solve the following initial value problem by completing each task.
			</p>
			<me>
				\frac{dz}{dy} - yz = y, \hspace{1cm} z(0) = 5
			</me>
		</statement>

				<areas>
		<ol>
			<li>
					<p>
						Select the variable that you are solving for: <m>\quad</m>
						<area correct="no">		<m>\, y \,</m> </area> <m>\quad</m>
						<area correct="yes">	<m>\, z \,</m> </area>
					</p>
			</li>
			<!-- <li>
				<areas>
					<p>
						Verify that the DE is first order. 
					</p>
				</areas>
			</li>
			<li>
				<areas>
					<p>
						Solve for the derivative of <m>z</m>:
						<me>
							\frac{dz}{dy} = \hspace{2.0cm}
						</me>
					</p>
				</areas>
			</li>
			<li>
				<areas>
					<p>
						Is it possible to write the right hand side of the equation as a product of functions where one of the functions does not contain the dependent variable, <m>z</m> and the other function does not contain the independent variable, <m>y</m>? 
						That is, can you write the DE in the form suggested below?
						<me>
							\frac{dz}{dy} = \Big( \hspace{2.0cm} \Big) \cdot \Big( \hspace{2.0cm} \Big)
						</me>
					</p>
				</areas>
			</li>
			<li>
				<areas>
					<p>
						Completely separate variables:
						<me>
							\frac{1}{1+z}dz = \hspace{2.0cm} dy
						</me>
					</p>
				</areas>
			</li>
			<li>
				<areas>
					<p>
						Integrate both sides of the equation:
						<md>
							<mrow> \int \frac{1}{1+z}dz	=\amp\ \int ydy</mrow>
							<mrow> \ln|1+z|	=\amp\ \frac{1}{2}y^2 + c</mrow>
						</md>
					</p>
				</areas>
			</li>
			<li>
				<areas>
					<p>
						Exponentiate both sides of the equation:
						<md>
							<mrow> \ln|1+z|	=\amp\ \frac{1}{2}y^2 + c</mrow>
							<mrow> e^{\ln|1+z|}	=\amp\ e^{\frac{1}{2}y^2 + c}</mrow>
							<mrow> |1+z|	=\amp\ e^{\frac{1}{2}y^2}\cdot e^c</mrow>
						</md>
					</p>
				</areas>
			</li>
			<li>
				<areas>
					<p>
						Solve for <m>z</m>:
						<md>
							<mrow> 1+z	=\amp\ \underbrace{\pm e^c}_{\text{rename } A} \cdot e^{\frac{1}{2}y^2}</mrow>
							<mrow> 1+z	=\amp\ Ae^{\frac{1}{2}y^2}		</mrow>
							<mrow> z	=\amp\ Ae^{\frac{1}{2}y^2} - 1	</mrow>
						</md>
					</p>
				</areas>
			</li>
			<li>
				<areas>
					<p>
						Use the initial condition, <m>z(0) = 5</m>, to solve for <m>A</m>.
					</p>
				</areas>
			</li>
			<li>
				<areas>
					<p>
						Finally, write the solution to the IVP.
						<me>
							z = \hspace{2.0cm}
						</me>
					</p>
				</areas>
			</li> -->
		</ol>
			</areas>
			
		<!-- <solution>
			<p>
				It's always worth it when you first start solving DEs to step back and make sure you identify independent and dependent variables. Here <m>z</m> is dependent and <m>y</m> is independent. That means when we're done we hope to have a function
				<me>
				z = \underbrace{\hspace{4.0cm}}_{\text{some function of } y}
				</me>
			</p>

			<p>
				Also, even though the terminology we use is <em>initial</em> condition, we typically won't use that piece of information until the very end.

				<aside>
					<p>
						* Until we get to Laplace Transforms...
					</p>
				</aside>
			</p>

			<p>
				First let's verify that the DE is first order (it is!), and then we go about solving for the derivative.
				<md>
					<mrow> \frac{dz}{dy} - yz	=\amp\ y</mrow>
					<mrow> \frac{dz}{dy} 	=\amp\ y + yz</mrow>
				</md>
			</p>

			<p>
				Now that we have solved for the derivative, is it possible write the right hand side of the equation as a product of functions where one of the functions does not contain the dependent variable, <m>z</m> and the other function does not contain the independent variable, <m>y</m>?  That is, we'd like to write the DE in the form suggested below.
				<me>
					\frac{dz}{dy} = \Big( \underbrace{\hspace{2.0cm}}_{\mbox{no z's}} \Big) \cdot
					\Big( \underbrace{\hspace{2.0cm}}_{\mbox{no x's}} \Big)
				</me>
				Hopefully you can see that there is a way, by factoring <m>y</m> out of each term on the right hand side, as below.
				<me>\frac{dz}{dy} = y(1 + z)</me>
			</p>

			<p>
				Now we need to completely separate variables.
				<me>\frac{1}{1+z}dz = ydy</me>
			</p>

			<p>
				The next step will be to integrate both sides of the equation. (If the integral on the right hand side is at all questionable to you, you should do take an extra step and actually do the substitution <m>u = 1+z.</m>)
				<md>
					<mrow> \int \frac{1}{1+z}dz	=\amp\ \int ydy</mrow>
					<mrow> \ln|1+z|	=\amp\ \frac{1}{2}y^2 + c</mrow>
				</md>
			</p>

			<p>
				As before, we write only one constant of integration (recall that we're skipping a couple of steps here; details provided in Example 6).
			</p>

			<p>
				Remember that our goal is to solve for the unknown function <m>z</m>. Since it's currently inside of a logarithm, we exponentiate both sides of the equation.
				<md>
					<mrow> \ln|1+z|	=\amp\ \frac{1}{2}y^2 + c</mrow>
					<mrow> e^{\ln|1+z|}	=\amp\ e^{\frac{1}{2}y^2 + c}</mrow>
					<mrow> |1+z|	=\amp\ e^{\frac{1}{2}y^2}\cdot e^c</mrow>
				</md>
			</p>

			<p>
				We continue solving for <m>z</m>.
				<md>
					<mrow> 1+z	=\amp\ \underbrace{\pm e^c}_{\text{rename } A} \cdot e^{\frac{1}{2}y^2}</mrow>
					<mrow> 1+z	=\amp\ Ae^{\frac{1}{2}y^2}		</mrow>
					<mrow> z	=\amp\ Ae^{\frac{1}{2}y^2} - 1	</mrow>
				</md>
			</p>

			<p>
				Now we can use that initial condition, <m>z(0) = 5</m>, to solve for <m>A</m>. The initial condition can be read,
				"when <m>y</m> is zero, <m>z</m> is 5."  We substitute into our solution accordingly.
				<md>
					<mrow> z	=\amp\ Ae^{\frac{1}{2}y^2} - 1</mrow>
					<mrow> 5	=\amp\ Ae^{\frac{1}{2}\cdot 0^2} - 1</mrow>
					<mrow> 5	=\amp\ Ae^0 - 1</mrow>
					<mrow> 6	=\amp\ A\cdot 1</mrow>
					<mrow> 6	=\amp\ A</mrow>
				</md>
				<aside>
					<p>
						* mention that we can't call <m>A = 6</m> our solution!
					</p>
				</aside>
			</p>

			<p>
				Therefore, the solution to the IVP is
				<me>z = 6e^{\frac{1}{2}y^2} - 1.</me>
			</p>
		</solution> -->

	</exercise>

	<exercisegroup><title> Step-by-Step </title>

		<introduction>
			<p>
				Maybe write 1 or 2 simple scaffolded problems here?
			</p>
		</introduction>

		<exercise>
			<p>
				<statement>
					Given the differential equation <m> \ds \frac{dy}{dx} = xy^2 </m>, determine if it is separable. If so, rewrite it in the separated form.
				</statement>
				<solution>
					<p>
						The equation is separable because we can write it as:
						<me> \frac{1}{y^2} dy = x dx </me>
					</p>
				</solution>
				<answer>
					<p>
						<m> \ds \frac{1}{y^2} dy = x dx </m>
					</p>
				</answer>
			</p>
			<p>
				<statement>
					Continuing from the previous problem, integrate the left side of the separated equation with respect to <m>y</m>.
				</statement>
				<solution>
					<p>
						Integrating <m> \ds \frac{1}{y^2} dy </m> with respect to <m>y</m>, we get:
						<me> -\frac{1}{y} + C_1 </me>
					</p>
				</solution>
				<answer>
					<p>
						<m> \ds -\frac{1}{y} + C_1 </m>
					</p>
				</answer>
			</p>
			<p>
				<statement>
					Now, integrate the right side of the separated equation with respect to <m>x</m>.
				</statement>
				<solution>
					<p>
						Integrating <m> x dx </m> with respect to <m>x</m>, we get:
						<me> \frac{1}{2}x^2 + C_2 </me>
					</p>
				</solution>
				<answer>
					<p>
						<m> \ds \frac{1}{2}x^2 + C_2 </m>
					</p>
				</answer>
			</p>
			<p>
				<statement>
					Combine the results from the previous exercises to form the general solution to the differential equation.
				</statement>
				<solution>
					<p>
						Equating the two integrals, we get:
						<me> -\frac{1}{y} + C_1 = \frac{1}{2}x^2 + C_2 </me>
						By grouping constants, we can represent them with a single constant:
						<me> -\frac{1}{y} = \frac{1}{2}x^2 + C </me>
						Where <m>C = C_2 - C_1</m>.
					</p>
				</solution>
				<answer>
					<p>
						<m> \ds -\frac{1}{y} = \frac{1}{2}x^2 + C </m>
					</p>
				</answer>
			</p>
		</exercise>
	
	</exercisegroup>

	<exercise><title> <em>Solve the Differential Equation</em> </title>

		<introduction>
			<p>
				Complete each step below to solve the differential equation
				<me> y'= e^{2x} - 5x. </me>
			</p>
		</introduction>
			
		<webwork xml:id="ww_5"> 

			<pg-code>
				Context()->variables->add(y => 'Real');
				$ans2a =Formula("e^{2 x} - 4 x");
				$ans2b = 1;
				$ans3a = 1;
				$ans3b = Formula("e^{2 x} - 4 x");
				$ans4a = Formula("y");
				$ans4b = FormulaUpToConstant("1/2 e^(2x) - 2 x^2");
				$ans = FormulaUpToConstant("1/2 e^{2x} - 2 x^2");
			</pg-code>

			<statement>
				<ol marker="1.">
					<li>
						Verify that the DE has first order. 
					</li>

					<li>
						<p>
							Write the DE into the separable form, <m> y'= f(x) \cdot g(y).</m>
						</p>
						<p>
							<m>f(x) =</m> <var name="$ans2a" width="15" /> , 
							<m>g(y) =</m> <var name="$ans2b" width="15" />
						</p>
					</li>

					<li>
						<p>
							Use algebra to move the <m>y</m> terms to the left
							<me> \frac{1}{g(y)} \cdot y'= f(x).</me>
							<var name="$ans3a" width="15" /> <m> \cdot y' = </m> <var name="$ans3b" width="15" />
						</p>
					</li>

					<li>
						<p>
							Integrate both sides with respect to <m>x</m>. Don't forget the integration constant, <m>+C</m>. 
							<me> y'= e^{2 x} - 4 x.</me>
							<var name="$ans4a" width="25" /> <m> = </m> <var name="$ans4b" width="25" />
						</p>
					</li>

					<li>
						<p>
							After working out the integrals on each side of the equation, you will be left with <m>y</m>'s on the left and <m>x</m>'s on the right. Finish the problem by using algebra to solve for <m>y</m>.
						</p>
						<p>
							<m>y(x) = </m> <var name="$ans" width="25" />
						</p>
					</li>
					
				</ol>

			</statement>

		</webwork>

	</exercise>

	<exercise><title> <em>Solve the Differential Equation</em> </title>
		<introduction>
			<p>
				Use algebra to show the differential equation is separable. Give the <m>x</m> terms in the left blank and the <m>y</m> terms in the right blank.
				<me> \frac{dy}{dx} - y\cos(x) = y.</me>
			</p>
		</introduction>
			
		<webwork xml:id="ww_6_2"> 
			<description>
				Solve a separable DE using separation of variables.
			</description>

			<pg-code>
				Context()->variables->add(y => 'Real');
				Context()->variables->add(t => 'Real');
				Context()->variables->add(C => 'Real');
				$a = random(2,8,1);
				$ans1 = 1;
				$ans2a = Formula("t^{$a}");
				$ans2b = Formula("1-y");
				$ans3a = Formula("1/(1-y)");
				$ans3b = Formula("t^{$a}");
				$ans4a = Formula("-ln(1-y)");
				$ans4b = FormulaUpToConstant("1/($a + 1)* t^{$a + 1}");
				$ans = Formula("1 - C*exp(-t^{$a+1}/($a + 1)) "); 
			</pg-code>

			<statement>
				<ol marker="1.">
					<li>
						Verify that the DE has first order. 
						<me> \frac{dy}{dt}= t^{<var name="$a" /> }-yt^{<var name="$a" /> } .</me>
						Order <m>=</m> <var name="$ans1"  width="15" />
					</li>

					<li>
						<p>
							Attempt to re-write the DE into the separable form
							<me> y'= f(t) \cdot g(y).</me>
							<m>f(t) =</m> <var name="$ans2a" width="15" /> , 
							<m>g(y) =</m> <var name="$ans2b" width="15" />
						</p>
					</li>

					<li>
						<p>
							Use algebra to move the <m>y</m> terms to the left
							<me> \frac{1}{g(y)} \cdot y'= f(t).</me>
							<var name="$ans3a" width="15" /> <m> \cdot y' = </m> <var name="$ans3b" width="15" />
						</p>
					</li>

					<li>
						<p>
							Integrate both sides with respect to <m>t</m>. Hint: Don't forget the +C after doing the indefinite integral. 
							<var name="$ans4a" width="25" /> <m> = </m> <var name="$ans4b" width="25" />
						</p>
					</li>

					<li>
						<p>
							After working out the integrals on each side of the equation, you will be left with <m>y</m>'s on the left and <m>t</m>'s on the right. Finish the problem by using algebra to solve for <m>y</m>.
						</p>
						<p>
							<m>y(t) = </m> <var name="$ans" width="25" />
						</p>
					</li>
					
				</ol>

			</statement>

		</webwork>
	</exercise>

</exercises>