
<exercises><title> Drill Exercises </title>

	<exercise label="c3-drill-exercises">

		<introduction>
			<p>
				Complete the following questions to test your conceptual understanding of the separation of variables method.
			</p>
		</introduction>

		<task label="c3-cr-click-on-01">

			<statement>
				<p>
					Click on each of the separable differential equations below.
				</p>
			</statement>

			<areas>
				<tabular>
					<row><cell><m/></cell></row>
					<row>
						<cell><area correct="yes">
							<m>\quad\ds x^2\frac{dy}{dx} - y = x^2y</m>
						</area></cell><cell/>
						<cell><area correct="no">
							<m>\quad\ds \frac{dy}{dx} + xy = y^2</m>
						</area></cell>
					</row>
					<row><cell><m/></cell></row>
					<row>
						<cell><area correct="yes">
							<m>\quad\ds \sqrt{x^2+1}\frac{dy}{dx} = y</m>
						</area></cell>
						<cell/>
						<cell><area correct="no">
							<m>\quad\ds xy\frac{dy}{dx} = x + y</m>
						</area></cell>
					</row>
					<row><cell><m/></cell></row>
					<row>
						<cell><area correct="yes">
							<m>\quad\ds x\frac{dy}{dx} - e^x = 3</m>
						</area></cell>
						<cell/>
						<cell><area correct="no">
							<m>\quad\ds \frac{dy}{dx} - x = \frac{y^2}{x}</m>
						</area></cell>
					</row>
					<row><cell><m/></cell></row>
				</tabular>
			</areas>

			<feedback>
				<p>
					A differential equation is separable if you can rearrange it to express it as a product of functions involving only <m>x</m> and <m>y</m> separately. Look for equations that can be manipulated into this form, even if they do not initially appear separable.
				</p>
			</feedback>

		</task>

	</exercise>

	<exercise label="c2-cr-ww-01"><title> <em>Separable Form</em> </title>

		<introduction>
			<p>
				Write each differential equation in the separable form
				<me>
					\frac{dy}{dx} = f(x)\cdot g(y)
				</me>.
			</p>
			<p>
				<em>Type your answer for <m>f(x)</m> into the left box and <m>g(y)</m> into the right box.</em>
			</p>
		</introduction>
			
		<webwork xml:id="c2-cr-ww-01-id">

			<description>
				Show a differential equation is separable.
			</description>
	
			<pg-code>
				Context()->variables->add(y => 'Real');
				$f1 = Formula("1 + cos(x)");
				$g1 = Formula("y");
				$f2 = Formula("1/x^2");
				$g2 = Formula("1 - y");
				$f3 = Formula("e^(x)/x");
				$g3 = Formula("(y^2 - 1)/y");
			</pg-code>
	
			<statement>
				
				<ol>
					<li>
						<p>
							<m>
								\quad\displaystyle	\frac{dy}{dx} - y\cos(x) = y 
								\quad\implies\quad	\frac{dy}{dx} = 
							</m>
							<var name="$f1" width="10" />
							<var name="$g1" width="10" />
						</p>
					</li>
					<li>
						<p>
							<m>
								\quad\displaystyle	x^2y + x^4\frac{dy}{dx} = x^2
								\quad\implies\quad	\frac{dy}{dx} = 
							</m>
							<var name="$f2" width="10" />
							<var name="$g2" width="10" />
						</p>
					</li>
					<li>
						<p>
							<m>
								\quad\displaystyle	xy\frac{dy}{dx} = e^xy^2 - e^x
								\quad\implies\quad	\frac{dy}{dx} =
							</m>
							<var name="$f3" width="10" />
							<var name="$g3" width="10" />
						</p>
					</li>
				</ol>

			</statement>
			
		</webwork>

		<solution>
			<ol>
				<li>
					<p>
						Move the <m> y\cos x </m> term to the right and factor out <m>y</m>.
						<md>
							<mrow>	\frac{dy}{dx}	\amp =	y + y\cos(x)	</mrow>
							<mrow>	\frac{dy}{dx}	\amp =	\ub{(1 + \cos(x))}_{f(x)}\us{g(y)}{\us{\uparrow}{\ul{y}}}	</mrow>
						</md>
					</p>
				</li>
				<li>
					<p>
						Isolate the derivative and group the terms as shown below.
						<md>
							<mrow>	\frac{dy}{dx}	\amp =	\frac{1}{x^2} - \frac{y}{x^2} \quad\leftarrow \text{common factor: } \frac{1}{x^2}	</mrow>
							<mrow>	\frac{dy}{dx}	\amp =	\us{f(x)}{\us{\uparrow}{\ul{\frac{1}{x^2}}}} \cdot\ub{(1 - y)}_{g(y)}				</mrow>
						</md>
					</p>
				</li>
				<li>
					<p>
						We isolate the derivative and group the terms as shown below.
						<md>
							<mrow>	xy\frac{dy}{dx}	\amp =	e^xy^2 - e^x																									</mrow>
							<mrow>	\frac{dy}{dx}	\amp =	\frac{e^xy^2 - e^x}{xy}	\quad\leftarrow \text{common factor: } e^x												</mrow>
							<mrow>	\frac{dy}{dx}	\amp =	\frac{e^x \cdot (y^2 - 1)}{x \cdot y} \quad\leftarrow \left(\frac{AB}{CD} = \frac{A}{C}\cdot \frac{B}{D}\right)	</mrow>
							<mrow>	\frac{dy}{dx}	\amp =	\us{f(x)}{\us{\uparrow}{\ul{\frac{e^x}{x}}}} \cdot	\ub{\frac{y^2 - 1}{y}}_{g(y)}								</mrow>
						</md>.
					</p>
				</li>
			</ol>
			
		</solution>

	</exercise>

</exercises>