
<subsection xmlns:xi="http://www.w3.org/2001/XInclude"><title> Exercises </title>

	<xi:include href="./c3-exercises-conceptual.ptx" />

	<exercises><title> Separable Form &amp; Separable Equations </title>

		<exercisegroup cols="2"><title> Show Separability </title>
			<introduction>
				<p>
					Determine whether the given differential equation is separable or not. As demonstrated in the examples, if the equation is separable, use parentheses to explicitly show the separable form.
				</p>
			</introduction>
	
			<exercise><title> <m>\ds \frac{dz}{dt} = \sin(z+t)</m> </title>
				<statement/>
				<solution>
					<p>
						<alert>not</alert> separable; there's no way to separate th <m> \ds z </m> an <m> \ds t </m> inside the sine term.
					</p>
				</solution>
				<answer>
					<p>
						<alert>not</alert> separable
					</p>
				</answer>
			</exercise>
	
			<exercise><title> <m>\ds s' = t\ln(s^{2t}) + 8t^2</m> </title>
				<statement/>
				<solution>
					<p>
				This doesn't look separable; but if we use a property of logarithms we can re-write as follows.
					<md>
						<mrow>  s'	 \amp =  t\ln(s^{2t}) + 8t^2 </mrow>
						<mrow>  \frac{ds}{dt}	 \amp =  t \cdot 2t\ln(s) + 8t^2 </mrow>
						<mrow>   \amp =  2t^2 \ln(s) + 8t^2 </mrow>
						<mrow>   \amp =  \big(t^2\big)\big(2\ln(s) + 8\big) </mrow>
					</md>
					Hence, this DE is <alert>separable</alert>.
					</p>
				</solution>
				<answer>
					<p>
						<alert>separable</alert>
					</p>
				</answer>
			</exercise>
	
			<exercise><title> <m>\ds \frac{dy}{dx} = 2y^3 + y + 4</m> </title>
				<statement/>
				<solution>
					<p>
				We can rearrange as follows.
					<md>
						<mrow>  \frac{dy}{dx}	 \amp =  \big(1\big)\big(2y^3 + y + 4\big) </mrow>
					</md>
					Hence, this DE is <alert>separable</alert>.
					</p>
				</solution>
				<answer>
					<p>
						<alert>separable</alert>
					</p>
				</answer>
			</exercise>
	
			<exercise><title> <m>\ds y' - xy = 0</m> </title>
				<statement/>
				<solution>
					<p>
				We can rearrange as follows.
					<md>
						<mrow>  y' - xy	 \amp =  0 </mrow>
						<mrow>  y'	 \amp =  \big(x\big)\big(y\big) </mrow>
					</md>
					Hence, this DE is <alert>separable</alert>.
					</p>
				</solution>
				<answer>
					<p>
						<alert>separable</alert>
					</p>
				</answer>
			</exercise>
	
			<exercise><title> <m>\ds y' = x+y</m> </title>
				<statement/>
				<solution>
					<p>
						<alert>not</alert> separable; there's no way to separate <m> \ds x </m> and <m> \ds y </m> via multiplication/division
					</p>
				</solution>
				<answer>
					<p>
						<alert>not</alert> separable
					</p>
				</answer>
			</exercise>
	
			<exercise><title> <m>\ds y'' + y' + y = 0</m> </title>
				<statement/>
				<solution>
					<p>
						<alert>not</alert> separable; this DE is second order, and DEs must be first order to be separable
					</p>
				</solution>
				<answer>
					<p>
						<alert>not</alert> separable
					</p>
				</answer>
			</exercise>
		</exercisegroup>

	</exercises>

	<exercises><title> Solve the Differential Equations </title>

		<exercisegroup cols="2"><title> Level 1 </title>
	
			<introduction>
				<p>
					Solve using separation of variables, if possible.
				</p>
			</introduction>

			<exercise><title> <m>\ds \frac{dy}{dx} = y^2 </m></title>
				<statement/>
				<answer>
					<p>
						<m> \ds y = \frac{1}{C-x} </m>
					</p>
				</answer>
			</exercise>
	
			<exercise><title> <m>\ds \frac{dy}{dx} = x^2y </m></title>
				<statement/>
			</exercise>
	
			<exercise><title> <m>\ds \frac{dy}{dx} = e^{x+y} </m></title>
				<statement/>
			</exercise>
	
			<exercise><title> <m>\ds \frac{dy}{dx} = \frac{x}{y} </m></title>
				<statement/>
			</exercise>
	
			<exercise><title> <m>\ds \frac{dy}{dx} = \cos(x) \sec(y) </m></title>
				<statement/>
			</exercise>
	
			<exercise><title> <m>\ds \frac{dy}{dx} = \frac{2x}{1+y^2} </m></title>
				<statement/>
			</exercise>
	
			<exercise><title> <m>\ds \frac{dy}{dx} = 2-y </m></title>
				<statement/>
			</exercise>
	
			<exercise><title> <m>\ds \frac{dy}{dx} = \frac{y-x}{y+x} </m></title>
				<statement/>
			</exercise>
	
			<exercise><title> <m>\ds \frac{dy}{dx} = y^2 \sec^2(x) </m></title>
				<statement/>
			</exercise>
	
			<exercise><title> <m>\ds \frac{dy}{dx} = \frac{1}{xy} </m></title>
				<statement/>
			</exercise>
			
		</exercisegroup>

		<exercisegroup cols="2"><title> Level 2 </title>
	
			<introduction>
				<p>
					Solve using separation of variables, if possible.
				</p>
			</introduction>
	
			<exercise><title> <m>\ds \frac{dy}{dx} = x y </m> </title>
				<statement/>
				<solution>
					<p>
						<md>
							<mrow>  \frac{dy}{y} \amp = x dx </mrow>
							<mrow>  \int \frac{dy}{y} \amp = \int x dx </mrow>
							<mrow>  \ln|y| \amp = \frac{1}{2}x^2 + C_1 </mrow>
							<mrow>  y \amp = Ce^{\frac{1}{2}x^2} </mrow>
						</md>
					</p>
				</solution>
				<answer>
					<p>
						<m> \ds y = Ce^{\frac{1}{2}x^2} </m>
					</p>
				</answer>
			</exercise>
	
			<exercise><title> <m>\ds \frac{dy}{dx} = \frac{x^2 + 1}{y} </m> </title>
				<statement/>
				<solution>
					<p>
						<md>
							<mrow>  y dy \amp = (x^2 + 1) dx </mrow>
							<mrow>  \int y dy \amp = \int (x^2 + 1) dx </mrow>
							<mrow>  \frac{1}{2}y^2 \amp = \frac{1}{3}x^3 + x + C_1 </mrow>
							<mrow>  y^2 \amp = \frac{2}{3}x^3 + 2x + 2C_1 </mrow>
						</md>
					</p>
				</solution>
				<answer>
					<p>
						<m> \ds y^2 = \frac{2}{3}x^3 + 2x + C_2 </m>
					</p>
				</answer>
			</exercise>
	
			<exercise><title> <m>\ds \frac{dy}{dx} = \frac{1 - x^2}{y^2} </m> </title>
				<statement/>
				<solution>
					<p>
						<md>
							<mrow>  \frac{dy}{dx}	 \amp =  \frac{1 - x^2}{y^2} </mrow>
							<mrow>  y^2 dy	 \amp =  (1-x^2)dx </mrow>
							<mrow>  \int y^2 dy	 \amp =  \int (1-x^2)dx </mrow>
							<mrow>  \frac{1}{3}y^3	 \amp =  x - \frac{1}{3}x^3 + C_1 </mrow>
							<mrow>  y^3	 \amp =  3x - x^3 + 3C_1 </mrow>
							<mrow>  y	 \amp =  \sqrt[3]{3x - x^3 + 3C_1}, \mbox{ or} </mrow>
							<mrow>  y	 \amp =  \sqrt[3]{3x - x^3 + C_2} </mrow>
						</md>
						<em> Note:  since, in general <m> \ds \sqrt[3]{a+b} \ne \sqrt[3]{a} + \sqrt[3]{b} </m> , we CANNOT simplify the solution to <m> \ds y  = \sqrt[3]{3x - x^3} + C.</m> </em>
					</p>
				</solution>
				<answer>
					<p>
						<m> \ds y = \sqrt[3]{3x - x^3 + C_2} </m>
					</p>
				</answer>
			</exercise>
	
			<exercise><title> <m>\ds y' - 2y = y\sin x </m> </title>
				<statement/>
				<solution>
					<p>
						<md>
							<mrow>  y' - 2y	 \amp =  y\sin x </mrow>
							<mrow>  y'	 \amp =  2y + y\sin x </mrow>
							<mrow>  \frac{dy}{dx}	 \amp =  y(2 + \sin x) </mrow>
							<mrow>  \frac{1}{y} dy	 \amp =  (2 + \sin x)dx </mrow>
							<mrow>  \int \frac{1}{y} dy	 \amp =  \int (2 + \sin x)dx </mrow>
							<mrow>  \ln|y|	 \amp =  2x - \cos x + C_1 </mrow>
							<mrow>  e^{\ln|y|}	 \amp =  e^{2x - \cos x + C_1} </mrow>
							<mrow>  |y|	 \amp =  e^{2x - \cos x}\cdot e^{C_1} </mrow>
							<mrow>  y	 \amp =  \pm e^{2x - \cos x}\cdot e^{C_1} </mrow>
							<mrow>  y	 \amp =  \underbrace{\pm e^{C_1}}_{\scriptsize = C_2}\cdot e^{2x - \cos x} </mrow>
							<mrow>  y	 \amp =  C_2e^{2x - \cos x} </mrow>
						</md>
					</p>
				</solution>
				<answer>
					<p>
						<m> \ds y = C_2e^{2x - \cos x}  </m>
					</p>
				</answer>
			</exercise>
	
			<exercise><title> <m>\ds x\frac{dv}{dx} = \frac{1-4v^2}{3v} </m> </title>
				<statement/>
				<solution>
					<p>
						<md>
							<mrow>  x\frac{dv}{dx}	 \amp =  \frac{1-4v^2}{3v} </mrow>
							<mrow>  \frac{dv}{dx}	 \amp =  \frac{1-4v^2}{3v}\cdot \frac{1}{x} </mrow>
							<mrow>  \frac{3v}{1-4v^2} dv	 \amp =  \frac{1}{x} dx </mrow>
							<mrow>  \int \frac{3v}{1-4v^2} dv	 \amp =  \int \frac{1}{x} dx </mrow>
		
						</md>
						For the integral on the left hand side, we will need to do a substitution.  If we le <m> \ds u = 1-4v^2, </m> the <m> \ds du = -8vdv, </m> and therefor <m> \ds -\frac{1}{8}du = vdv. </m>  Then we have the following:
						<md>
							<mrow>  3\int \frac{v}{1-4v^2} dv	 \amp =  \int \frac{1}{x} dx </mrow>
							<mrow>  3\int \underbrace{\frac{1}{1-4v^2}}_{\scriptsize 1/u} \underbrace{vdv}_{\scriptsize -\frac{1}{8}du}  \amp =  \int \frac{1}{x} dx </mrow>
							<mrow>  3\int \frac{1}{u}\cdot -\frac{1}{8}du	 \amp =  \int \frac{1}{x} dx </mrow>
							<mrow>  -\frac{3}{8} \int \frac{1}{u}du	 \amp =  \int \frac{1}{x} dx </mrow>
							<mrow>  -\frac{3}{8} \ln|u|	 \amp =  \ln|x| + C_1 </mrow>
							<mrow>  -\frac{3}{8} \ln|1 - 4v^2|	 \amp =  \ln|x| + C_1 </mrow>
							<mrow>  \ln|1 - 4v^2|	 \amp =  -\frac{8}{3} \left(\ln|x| + C_1\right) </mrow>
							<mrow>  \ln|1 - 4v^2|	 \amp =  -\frac{8}{3}\ln|x| + -\frac{8}{3}C_1 </mrow>
							<mrow>  \ln|1 - 4v^2|	 \amp =  \ln\left(|x|^{-8/3}\right) + -\frac{8}{3}C_1 </mrow>
							<mrow>  \ln|1 - 4v^2|	 \amp =  \ln\left(x^{-8/3}\right) + -\frac{8}{3}C_1  \mbox <m> \hspace{1cm} \ds x^{-8/3} =|x|^{-8/3} </m> )} </mrow>
							<mrow>  e^{\ln|1 - 4v^2|}	 \amp =  e^{\ln\left(x^{-8/3}\right) + -\frac{8}{3}C_1} </mrow>
							<mrow>  |1 - 4v^2|	 \amp =  e^{\ln\left(x^{-8/3}\right)}\cdot e^{-\frac{8}{3}C_1} </mrow>
							<mrow>  |1 - 4v^2|	 \amp =  x^{-8/3}\cdot e^{-\frac{8}{3}C_1} </mrow>
							<mrow>  1 - 4v^2	 \amp =  \pm e^{-\frac{8}{3}C_1}\cdot x^{-8/3} </mrow>
							<mrow>  1 - 4v^2	 \amp =  \underbrace{\pm e^{-\frac{8}{3}C_1}}_{\scriptsize = C_2}\cdot x^{-8/3} </mrow>
							<mrow>  1 - 4v^2	 \amp =  C_2x^{-8/3} </mrow>
		
						</md>
		
						<md>
							<mrow>  - 4v^2	 \amp =  C_2x^{-8/3} - 1 </mrow>
							<mrow>  v^2	 \amp =  \frac{C_2}{-4}x^{-8/3} + \frac{1}{4} </mrow>
							<mrow>  v^2	 \amp =  \underbrace{\frac{C_2}{-4}}_{\scriptsize = C_3}x^{-8/3} + \frac{1}{4} </mrow>
							<mrow>  v^2	 \amp =  C_3x^{-8/3} + \frac{1}{4} </mrow>
							<mrow>  v	 \amp =  \pm \sqrt{C_3x^{-8/3} + \frac{1}{4}} </mrow>
						</md>
	
					</p>
				</solution>
				<answer>
					<p>
						<m> \ds v = \pm \sqrt{C_3x^{-8/3} + \frac{1}{4}}  </m>
					</p>
				</answer>
			</exercise>
	
			<exercise><title> <m>\ds \frac{dy}{dx} = \frac{4-2x}{3y^2-5} </m> </title>
				<statement/>
				<solution>
					<p>
						When we separate the variables and integrate both sides, we get
						<me> \int (3y^2-5)dy =  \int (4-2x)dx</me>
						<me> y^3-5y=4x-x^2+C </me>
						Since the equation cannot readily be solved for <m>y</m> as an explicit function of <m>x</m>, we are done.
					</p>
				</solution>
				<answer>
					<p>
						<m> y^3-5y=4x-x^2+C </m>
					</p>
				</answer>
			</exercise>
	
			<exercise><title> <m>\ds \frac{dy}{dx} = 6x(y-1)^{2/3}</m> </title>
				<statement/>
				<solution>
					<p>
						Separation of variables gives:
						<md>
							<mrow>\ds\int  \frac{1}{3(y-1)^2/3} dy = \int 2xdx</mrow>
							<mrow>				(y-1)^1/3=\amp\ \ds x^2+C</mrow>
							<mrow>				y(x)=\amp\ \ds 1+(x^2+C)^3</mrow>
						</md>
					</p>
				</solution>
				<answer>
					<p>
						<m>\ds y(x)=\amp\ \ds 1+(x^2+C)^3</m>
					</p>
				</answer>
			</exercise>
	
		</exercisegroup>
	
		<exercisegroup cols="2"><title> Initial Value Problems </title>
	
			<introduction>
				<p>
					Solve each of the following initial value problems using separation of variables, if possible.
				</p>
			</introduction>
	
			<exercise>
				<title>
					<m>
						\left\{
							\begin{array}{l}
								\ds\frac{dy}{dx} = -6xy,\\
								y(0)=7
							\end{array}
						\right.\quad
					</m>
				</title>
				<statement/>
				<solution>
					<p>
						Informally, we divide both side of the differential equation by <m>y</m> and multiply each side by <m>dx</m> to get
						<me> \frac{dy}y = -6xdx.	</me>
						<me> \int \frac{dy}y =  \int (-6x)dx</me>
						<me> \ln|y|=-3x^2+C </me>
						<me>\ln|y|=-3x^2+C</me>
						<me>|y|=e^{-3x^2+C}</me>
						<me>y=\pm e^C e^{-3x^2}</me>
		
						and hence
		
						<me>y(x) = Ae^{-3x^2} \qquad (A = \pm e^C)</me>
		
						The condition <m>y(0) = 7</m> yields <m>A =7</m>, so the desired solution is
		
						<me>y(x) = 7e^{-3x^2}</me>
	
					</p>
				</solution>
				<answer>
					<p>
						<me>y(x) = 7e^{-3x^2}</me>
					</p>
				</answer>
			</exercise>
	
			<exercise>
				<title>
					<m>
						\left\{
							\begin{array}{l}
								\ds\frac{dz}{dt} = 2tz^2,\\
								z(1) = 2
							\end{array}
						\right.
					</m>
				</title>
				<statement/>
				<solution>
					<p>
						First we find the general solution:
						<md>
							<mrow>  \frac{dz}{dt}	 \amp =  2tz^2 </mrow>
							<mrow>  \frac{1}{z^2}dz	 \amp =  2tdt </mrow>
							<mrow>  \int \frac{1}{z^2}dz	 \amp =  \int 2tdt </mrow>
							<mrow>  -\frac{1}{z}	 \amp =  t^2 + C_1 </mrow>
							<mrow>  z	 \amp =  -\frac{1}{t^2 + C_1} </mrow>
						</md>
		
						Using the initial condition <m>z(1) = 2</m>:
						<md>
							<mrow>  2	 \amp =  -\frac{1}{1^2 + C_1} </mrow>
							<mrow>  2	 \amp =  -\frac{1}{1 + C_1} </mrow>
							<mrow>  C_1	 \amp =  -\frac{1}{2} - 1 </mrow>
							<mrow>  C_1	 \amp =  -\frac{3}{2} </mrow>
						</md>
		
						So the solution to the initial value problem is:
						<md>
							<mrow>  z(t)	 \amp =  -\frac{1}{t^2 - \frac{3}{2}} </mrow>
						</md>
					</p>
				</solution>
				<answer>
					<p>
						<m> z(t) = -\frac{1}{t^2 - \frac{3}{2}} </m>
					</p>
				</answer>
			</exercise>
	
			<exercise>
				<title>
					<m>
						\left\{
							\begin{array}{l}
								\ds\frac{dy}{d\theta} = y\sin\theta,\\
								y(\pi) = -3
							\end{array}
						\right.
					</m>
				</title>				<statement/>
				<solution>
					<p>
						First we find the general solution:
						<md>
							<mrow>  \frac{dy}{d\theta}	 \amp =  y\sin\theta </mrow>
							<mrow>  \frac{1}{y}dy	 \amp =  \sin\theta d\theta </mrow>
							<mrow>  \int \frac{1}{y}dy	 \amp =  \int \sin\theta d\theta </mrow>
							<mrow>  \ln|y|	 \amp =  -\cos\theta + C_1 </mrow>
							<mrow>  e^{\ln|y|}	 \amp =  e^{-\cos\theta + C_1} </mrow>
							<mrow>  |y|	 \amp =  e^{-\cos\theta}\cdot e^{C_1} </mrow>
							<mrow>  y	 \amp =  \pm e^{C_1}e^{-\cos\theta} </mrow>
							<mrow>   \amp =  \underbrace{\pm e^{C_1}}_{\scriptsize = C_2}e^{-\cos\theta} </mrow>
							<mrow>   \amp =  C_2e^{-\cos\theta}  </mrow>
						</md>
						Then we use the initial conditio <m> \ds y(\pi) = -3 </m> .
						<md>
							<mrow>  -3	 \amp =  y(\pi) </mrow>
							<mrow>   \amp =  C_2e^{-\cos\pi} </mrow>
							<mrow>   \amp =  C_2e^{-(-1)} </mrow>
							<mrow>   \amp =  C_2e </mrow>
							<mrow>  -\frac{3}{e}	 \amp =  C_2, \mbox{ or} </mrow>
							<mrow>  C_2	 \amp =  -3e^{-1} </mrow>
		
						</md>
						Hence, the solution i <m> \ds y = -3e^{-1}e^{-\cos\theta} </m> , or <m> \ds y = -3e^{-\cos\theta-1} </m> .
					</p>
				</solution>
				<answer>
					<p>
						<m> \ds y = -3e^{-1}e^{-\cos\theta} </m>, or  <m> \ds y = -3e^{-\cos\theta-1} </m>
					</p>
				</answer>
			</exercise>
	
			<exercise>
				<title>
					<m>
						\left\{
							\begin{array}{l}
								\ds\frac{dy}{dx} - 8x^3e^{-2y} = 0,\\
								y(1) = 0
							\end{array}
						\right.
					</m>
				</title>				<statement/>
				<solution>
					<p>
						First we find the general solution:
						<md>
							<mrow>  \frac{dy}{dx} - 8x^3e^{-2y}	 \amp =  0 </mrow>
							<mrow>  \frac{dy}{dx}	 \amp =  8x^3e^{-2y} </mrow>
							<mrow>  \frac{1}{e^{-2y}}dy	 \amp =  8x^3dx </mrow>
							<mrow>  e^{2y}dy	 \amp =  8x^3dx </mrow>
							<mrow>  \int e^{2y}dy	 \amp =  \int 8x^3dx </mrow>
							<mrow>  \frac{1}{2}e^{2y}	 \amp =  2x^4 + C_1 </mrow>
							<mrow>  e^{2y}	 \amp =  4x^4 + 2C_1 </mrow>
							<mrow>  \ln(e^{2y})	 \amp =  \ln(4x^4 + 2C_1) </mrow>
							<mrow>  2y	 \amp =  \ln(4x^4 + 2C_1) </mrow>
							<mrow>  y	 \amp =  \frac{1}{2}\ln(4x^4 + 2C_1), \mbox{ or} </mrow>
							<mrow>   \amp =  \frac{1}{2}\ln(4x^4 + C_2), \mbox{ or} </mrow>
							<mrow>   \amp =  \ln\Big[(4x^4 + C_2)^{1/2}\Big], \mbox{ or} </mrow>
							<mrow>   \amp =  \ln\Big[\sqrt{4x^4 + C_2}\Big] </mrow>
		
						</md>
						Then we use the initial conditio <m> \ds y(1) = 0 </m> .
						<md>
							<mrow>  0	 \amp =  y(1) </mrow>
							<mrow>  0	 \amp =  \ln\Big[\sqrt{4\cdot 1^4 + C_2}\Big] </mrow>
							<mrow>  0	 \amp =  \ln\Big[\sqrt{4 + C_2}\Big] </mrow>
							<mrow>  e^0	 \amp =  e^{\ln\Big[\sqrt{4 + C_2}\Big]} </mrow>
							<mrow>  1	 \amp =  \sqrt{4 + C_2} </mrow>
							<mrow>  1^2	 \amp =  \Big[\sqrt{4 + C_2}\Big]^2 </mrow>
							<mrow>  1	 \amp =  4+C_2 </mrow>
							<mrow>  -3	 \amp =  C_2 </mrow>
		
						</md>
						Hence, the solution i <m> \ds y = \frac{1}{2}\ln(4x^4 - 3) </m> , or <m> \ds y = \ln\Big[\sqrt{4x^4 - 3}\Big] </m>.
					</p>
				</solution>
				<answer>
					<p>
						<m> \ds y = \frac{1}{2}\ln(4x^4 - 3) </m> , or <m> \ds y = \ln\Big[\sqrt{4x^4 - 3}\Big] </m>
					</p>
				</answer>
			</exercise>
	
		</exercisegroup>

		<exercisegroup><title> Nested Differential Equations </title>
		
			<introduction>
				<p>
					Find a non-zero function <m>\mu(x)</m> that satisfies each of the following differential equations.
				</p>
				<hint>
					<p>
						For each equation, expand the derivative on the left side using the product rule. Then use algebra to find another differential equation nested within the original one.
					</p>
				</hint>
			</introduction>

			<exercise><title> <m>\ds\frac{d}{dx}\left[\mu\sin x\right] = \mu \cos x + 6 \mu \sin x</m> </title>

				<solution>
					<p>
						We want to find a non-zero function <m>\mu(x)</m> such that
						<me>
							\frac{d}{dx}\left[\mu\sin x\right] = \mu \cos x + 6 \mu \sin x.
						</me>
						Applying the product rule to the left side of this equation gives
						<me>
							\mu \cos x + \frac{d\mu}{dx} \sin x = \mu \cos x + 6 \mu \sin x.
						</me>
						Subtracting <m>\mu \cos x</m> from both sides gives
						<me>
							\frac{d\mu}{dx} \sin x = 6 \mu \sin x
						</me>,
						which implies that 
						<me>
							\frac{d\mu}{dx} = 6 \mu.
						</me>
						This is a separable differential equation that we can solve with separation of variables:
						<md>
							<mrow>	\frac{d\mu}{\mu}		\amp = 6 dx								</mrow>
							<mrow>	\int \frac{1}{\mu} d\mu	\amp = \int 6 dx						</mrow>
							<mrow>	\ln|\mu|				\amp = 6x + c_1							</mrow>
							<mrow>	|\mu|					\amp = e^{6x + c_1} = e^{c_1} e^{6x}	</mrow>
							<mrow>	\mu						\amp = \pm e^{c_1} e^{6x}				</mrow>
						</md>
						But, <m>\pm e^c_1</m> is just a constant, so we can write this as
						<me>
							\mu = ce^{6x}.
						</me>
						Since the question asks for a non-zero function, we can take <m>c = 1</m>. Thus, <m>\mu = e^{6x}</m> satisfies the given differential equation.
					</p>
				</solution>

			</exercise>

			<exercise><title> <m>\ds\frac{d}{dx}\left[\mu\ln x\right] = \frac{\mu}{x} + 2x \mu \ln x</m> </title>

				<solution>
					<p>
						We want to find a non-zero function <m>\mu(x)</m> such that
						<me>
							\frac{d}{dx}\left[\mu\ln x\right] = \mu \frac{\mu}{x} + 2x \mu \ln x.
						</me>
						Applying the product rule to the left side of this equation gives
						<me>
							\mu \frac{1}{x} + \frac{d\mu}{dx} \ln x = \mu \frac{\mu}{x} + 2x \mu \ln x.
						</me>
						Subtracting <m>\mu \frac{\mu}{x}</m> from both sides gives
						<me>
							\frac{d\mu}{dx} \ln x = 2x \mu \ln x
						</me>,
						which implies that
						<me>
							\frac{d\mu}{dx} = 2x \mu.
						</me>
						This is a separable differential equation that we can solve with separation of variables:
						<md>
							<mrow>	\frac{d\mu}{\mu}		\amp = 2x\ dx								</mrow>
							<mrow>	\int \frac{1}{\mu} d\mu	\amp = \int 2x\ dx						</mrow>
							<mrow>	\ln|\mu|				\amp = x^2 + c_1							</mrow>
							<mrow>	|\mu|					\amp = e^{x^2 + c_1} = e^{c_1} e^{x^2}	</mrow>
							<mrow>	\mu						\amp = \pm e^{c_1} e^{x^2}				</mrow>
						</md>
						But, <m>\pm e^c_1</m> is just a constant, so we can write this as
						<me>
							\mu = ce^{x^2}.
						</me>
						Since the question asks for a non-zero function, we can take <m>c = 1</m>. Thus, <m>\mu = e^{x^2}</m> satisfies the given differential equation.
					</p>
				</solution>

			</exercise>

			<exercise><title> <m>\ds\frac{d}{dx}\left[\mu y \right] = \mu \frac{dy}{dx} + 5 \mu y\quad </m> (<m>y</m> is some function of <m>x</m>) </title>

				<solution>
					<p>
						We want to find a non-zero function <m>\mu(x)</m> such that
						<me>
							\frac{d}{dx}\left[\mu y\right] = \mu \frac{dy}{dx} + 5 \mu y.
						</me>
						Applying the product rule to the left side of this equation gives
						<me>
							\mu \frac{dy}{dx} + \frac{d\mu}{dx} y = \mu \frac{dy}{dx} + 5 \mu y.
						</me>
						Subtracting <m>\mu \frac{dy}{dx}</m> from both sides gives
						<me>
							\frac{d\mu}{dx} y = 5 \mu y
						</me>,
						which implies that
						<me>
							\frac{d\mu}{dx} = 5 \mu.
						</me>
						This is a separable differential equation that we can solve with separation of variables:
						<md>
							<mrow>	\frac{d\mu}{\mu}		\amp = 5 dx								</mrow>
							<mrow>	\int \frac{1}{\mu} d\mu	\amp = \int 5 dx						</mrow>
							<mrow>	\ln|\mu|				\amp = 5x + c_1							</mrow>
							<mrow>	|\mu|					\amp = e^{5x + c_1} = e^{c_1} e^{5x}	</mrow>
							<mrow>	\mu						\amp = \pm e^{c_1} e^{5x}				</mrow>
						</md>
						But, <m>\pm e^c_1</m> is just a constant, so we can write this as
						<me>
							\mu = ce^{5x}.
						</me>
						Since the question asks for a non-zero function, we can take <m>c = 1</m>. Thus, <m>\mu = e^{5x}</m> satisfies the given differential equation.
					</p>
				</solution>

			</exercise>
		
		</exercisegroup>
	
		<exercisegroup><title> Applications </title>
	
			<exercise><title> Cooking Temperature </title>
			
				<statement>
					A 4-lb roast, initially at <m>50^{\circ}F</m>, is placed in a <m>375^{\circ} F</m> oven at 5:00 PM After 75 minutes it is found that the temperature <m>T(t)</m> of the roast is <m>125^{\circ}</m> F. When will the roast be <m>150^{\circ}F</m> (medium rate)?
				</statement>
	
				<solution>
					<p>
						We take time <m>t</m> in minutes, with <m>t = 0</m> corresponding to 5:00 PM We also assume (somewhat unrealistically) that at any instant the temperature <m>T(t)</m> of the roast is uniform throughout. We have <m>T(t) \lt A = 375</m>, <m>T(0)=50</m>, and <m>T(75) =125</m>. Hence
						<md>
							<mrow>\ds  \frac{dT}{dt}  = k(375-T)</mrow>
							<mrow>				\int \frac{1}{375-T}dT=\amp\ \ds \int kdt</mrow>
							<mrow>				y(x)=\amp\ \ds 1+(x^2+C)^3</mrow>
							<mrow>			-\ln(375-T)=\amp kt+C</mrow>
						</md>
		
						Now <m>T(0)=50</m>, implies that <m>B = 325</m>, so <m>T(t) = 375-325e^{kt}</m>. We also know that <m>T = 125</m> when <m>t = 75</m>. Substitution of these values in the preceding equation yields
		
						<me> k=-\frac{1}{75}\ln\left(\frac{250}{325}\right)\approx 0.0035.</me>
		
						Hence we finally solve the equation
		
						<me>150=375-325e^{(-0.0035)t}</me>
		
						for <m>t = -[\ln(225/325)]/[0.0035] \approx 105</m> (min), the total cooking time required.Because the roast was placed in the oven at 5:00 PM, it it should be removed at about 6:45 PM
					</p>
				</solution>
				<answer>
					<p>
						<m>t = -[\ln(225/325)]/[0.0035] \approx 105(min)</m>
					</p>
				</answer>
			</exercise>
		</exercisegroup>

	</exercises>

</subsection>