<exercises><title> Warm-ups &amp; Drills </title>

	<exercise label="c3-warm-ups-mc-tf"><title> Select the Best Answer </title>

		<task label="c3-warm-ups-mc-tf-01">
			<statement correct="yes">
				<p>
					The differential equation, below, is <xref ref="separable" text="custom">separable</xref>.
					<me>
						\frac{dy}{dx} = \frac{\cos x}{y}
					</me>
				</p>
			</statement>

			<feedback>
				<p>
					The equation is separable because it is first-order and can be written in the separable form
					<me>
						\frac{dy}{dx} = \cos x \left(\frac{1}{y}\right)
					</me>.
				</p>
			</feedback>
		</task>
		
		<task label="c3-warm-ups-mc-tf-02">
			<statement correct="yes">
				<p>
					The differential equation, below, is <xref ref="separable" text="custom">separable</xref>.
					<me>
						\frac{dy}{dx} = y^2
					</me>
				</p>
			</statement>
			<feedback>
				<p>
					The equation is separable because it is first-order and can be written in the separable form
					<me>
						\frac{dy}{dx} = y^2 = (1)(y^2) = \underset{f(x)}{\left(\boxed{1}\right)}\underset{g(y)}{\left(\boxed{y^2}\right)}
					</me>.
				</p>
			</feedback>
		</task>
			
		<task label="c3-warm-ups-mc-tf-03">
			<statement correct="yes">
				<p>
					The differential equation, below, is <xref ref="separable" text="custom">separable</xref>.
					<me>
						\frac{dy}{dx} = x - 1
					</me>
				</p>
			</statement>
			<feedback>
				<p>
					The equation is separable because it is first-order and can be written in the separable form
					<me>
						\frac{dy}{dx} = x - 1 = (x - 1)(1) = \underset{f(x)}{\left(\boxed{x - 1}\right)}\underset{g(y)}{\left(\boxed{1}\right)}.
					</me>
				</p>
			</feedback>
		</task>

		<task label="c3-warm-ups-mc-tf-04">
			<statement correct="yes">
				<p>
					The differential equation, below, is <xref ref="separable" text="custom">separable</xref>.
					<me>
						\frac{dy}{dx} = 15
					</me>
				</p>
			</statement>
			<feedback>
				<p>
					The equation is separable because it is first-order and can be written in the separable form
					<me>
						\frac{dy}{dx} = 15 = (15)(1) = \underset{f(x)}{\left(\boxed{15}\right)}\underset{g(y)}{\left(\boxed{1}\right)}.
					</me>
				</p>
			</feedback>
		</task>

		<task label="c3-warm-ups-mc-tf-05">
			<statement correct="no">
				<p>
					The differential equation,
					<me>
						x + \frac{dy}{dx} = y
					</me>,
					can be solved using the separation of variables method.
				</p>
			</statement>
			<feedback>
				<p>
					The differential equation is first order, but it is equivalent to
					<me>
						\frac{dy}{dx}=y-x
					</me>,
					which can not be written in the form <m>\ds\frac{dy}{dx}=f(x)g(y)</m>.
				</p>
			</feedback>
			<hint>
				<p>
					Check to see that the differential equation is first order and separable.
				</p>
			</hint>
		</task>

		<task label="c3-warm-ups-mc-tf-06">
			<statement correct="no">
				<p>
					The differential equation,
					<me>
						\frac{dz^2}{d^2t} = \cos^2(z)
					</me>,
					can be solved using the separation of variables method.
				</p>
			</statement>
			<feedback>
				<p>
					The differential equation is not first order, so it is not separable and cannot be solved using the separation of variables method.
				</p>
			</feedback>
			<hint>
				<p>
					Check to see that the differential equation is first order and separable.
				</p>
			</hint>
		</task>

		<task label="c3-warm-ups-mc-tf-07">

			<statement>
				<p>
					What is the first step to verify the differential equation below is separable?
					<me>
						\frac{dy}{dx} + \frac{x}{y^2} = 0
					</me>
				</p>
			</statement>

			<choices>
				<choice>
					<statement>
						<p>
							Integrating both sides with respect to <m>x</m>.
						</p>
					</statement>
					<feedback>
						<p>
							Incorrect. Integration should come after the equation is verified to be separable.
						</p>
					</feedback>
				</choice>
				<choice correct="yes">
					<statement>
						<p>
							Check to make sure the equation is first order.
						</p>
					</statement>
					<feedback>
						<p>
							Correct! The first step to verify the equation is separable is to make sure it is first order.
						</p>
					</feedback>
				</choice>
				<choice>
					<statement>
						<p>
							Combine the fractions on the left-side of the equation.
						</p>
					</statement>
					<feedback>
						<p>
							Incorrect. First of all, <m>\frac{dy}{dx}</m> is not a fraction. Even if it was this would not be the first step to verify separability.
						</p>
					</feedback>
				</choice>
				<choice>
					<statement>
						<p>
							Isolate <m>\ds\frac{dy}{dx}</m> on one side of the equation.
						</p>
					</statement>
					<feedback>
						<p>
							Incorrect. Isolating <m>\ds\frac{dy}{dx}</m> is required to verify the equation is separable, but there is one other detail to check first.
						</p>
					</feedback>
				</choice>
			</choices>

		</task>

	</exercise>

	<exercise label="c3-drill-practice-01"><title> Select the Separable Equations </title>

		<statement>
			<p>
				Click on each of the separable differential equations below.
			</p>
		</statement>

		<areas>
			<tabular>
				<row><cell><m/></cell></row>
				<row>
					<cell><area correct="yes">
						<m>\quad\ds x^2\frac{dy}{dx} - y = x^2y</m>
					</area></cell><cell/>
					<cell><area correct="no">
						<m>\quad\ds \frac{dy}{dx} + xy = y^2</m>
					</area></cell>
				</row>
				<row><cell><m/></cell></row>
				<row>
					<cell><area correct="yes">
						<m>\quad\ds \sqrt{x^2+1}\frac{dy}{dx} = y</m>
					</area></cell>
					<cell/>
					<cell><area correct="no">
						<m>\quad\ds xy\frac{dy}{dx} = x + y</m>
					</area></cell>
				</row>
				<row><cell><m/></cell></row>
				<row>
					<cell><area correct="yes">
						<m>\quad\ds x\frac{dy}{dx} - e^x = 3</m>
					</area></cell>
					<cell/>
					<cell><area correct="no">
						<m>\quad\ds \frac{dy}{dx} - x = \frac{y^2}{x}</m>
					</area></cell>
				</row>
				<row><cell><m/></cell></row>
			</tabular>
		</areas>

		<feedback>
			<p>
				A differential equation is separable if you can rearrange it to express it as a product of functions involving only <m>x</m> and <m>y</m> separately. Look for equations that can be manipulated into this form, even if they do not initially appear separable.
			</p>
		</feedback>

	</exercise>

	<exercise label="c3-drill-practice-02"><title> Determine the Separable Form </title>

		<introduction>
			<p>
				Write each differential equation in the separable form
				<me>
					\frac{dy}{dx} = f(x)\cdot g(y)
				</me>.
			</p>
			<p>
				<em>Type your answer for <m>f(x)</m> into the left box and <m>g(y)</m> into the right box.</em>
			</p>
		</introduction>
			
		<webwork xml:id="c2-cr-ww-01-id">

			<description>
				Show a differential equation is separable.
			</description>
	
			<pg-code>
				Context()->variables->add(y => 'Real');
				$f1 = Formula("1 + cos(x)");
				$g1 = Formula("y");
				$f2 = Formula("1/x^2");
				$g2 = Formula("1 - y");
				$f3 = Formula("e^(x)/x");
				$g3 = Formula("(y^2 - 1)/y");
			</pg-code>
	
			<statement>
				
				<ol>
					<li>
						<p>
							<m>
								\quad\displaystyle	\frac{dy}{dx} - y\cos(x) = y 
								\quad\implies\quad	\frac{dy}{dx} = 
							</m>
							<var name="$f1" width="10" />
							<var name="$g1" width="10" />
						</p>
					</li>
					<li>
						<p>
							<m>
								\quad\displaystyle	x^2y + x^4\frac{dy}{dx} = x^2
								\quad\implies\quad	\frac{dy}{dx} = 
							</m>
							<var name="$f2" width="10" />
							<var name="$g2" width="10" />
						</p>
					</li>
					<li>
						<p>
							<m>
								\quad\displaystyle	xy\frac{dy}{dx} = e^xy^2 - e^x
								\quad\implies\quad	\frac{dy}{dx} =
							</m>
							<var name="$f3" width="10" />
							<var name="$g3" width="10" />
						</p>
					</li>
				</ol>

			</statement>
			
		</webwork>

		<solution>
			<ol>
				<li>
					<p>
						Move the <m> y\cos x </m> term to the right and factor out <m>y</m>.
						<md>
							<mrow>	\frac{dy}{dx}	\amp =	y + y\cos(x)	</mrow>
							<mrow>	\frac{dy}{dx}	\amp =	\ub{(1 + \cos(x))}_{f(x)}\us{g(y)}{\us{\uparrow}{\ul{y}}}	</mrow>
						</md>
					</p>
				</li>
				<li>
					<p>
						Isolate the derivative and group the terms as shown below.
						<md>
							<mrow>	\frac{dy}{dx}	\amp =	\frac{1}{x^2} - \frac{y}{x^2} \quad\leftarrow \text{common factor: } \frac{1}{x^2}	</mrow>
							<mrow>	\frac{dy}{dx}	\amp =	\us{f(x)}{\us{\uparrow}{\ul{\frac{1}{x^2}}}} \cdot\ub{(1 - y)}_{g(y)}				</mrow>
						</md>
					</p>
				</li>
				<li>
					<p>
						We isolate the derivative and group the terms as shown below.
						<md>
							<mrow>	xy\frac{dy}{dx}	\amp =	e^xy^2 - e^x																									</mrow>
							<mrow>	\frac{dy}{dx}	\amp =	\frac{e^xy^2 - e^x}{xy}	\quad\leftarrow \text{common factor: } e^x												</mrow>
							<mrow>	\frac{dy}{dx}	\amp =	\frac{e^x \cdot (y^2 - 1)}{x \cdot y} \quad\leftarrow \left(\frac{AB}{CD} = \frac{A}{C}\cdot \frac{B}{D}\right)	</mrow>
							<mrow>	\frac{dy}{dx}	\amp =	\us{f(x)}{\us{\uparrow}{\ul{\frac{e^x}{x}}}} \cdot	\ub{\frac{y^2 - 1}{y}}_{g(y)}								</mrow>
						</md>.
					</p>
				</li>
			</ol>
			
		</solution>

	</exercise>
	
	<exercise label="c3-step-by-step-01" adaptive="yes"><title> Reorder the Steps </title>

		<statement>
			<p>
				Reorder the steps required to solve the differential equation,
				<me>
					\frac{dy}{dx} - y\cos(x) = y
				</me>,
				using the separation of variables method.
			</p>
		</statement>

		<blocks>
			<block><p>	Check for 1st-order.									</p></block>
			<block><p>	<m>\ds \frac{dy}{dx} = y + y\cos(x) </m>				</p></block>
			<block><p>	<m>\ds \frac{dy}{dx} = (1 + \cos(x))y </m>				</p></block>
			<block><p>	<m>\ds \frac{1}{y} dy = (1 + \cos(x))dx </m>				</p></block>
			<block><p>	<m>\ds \int \frac{1}{y} dy = \int (1 + \cos(x))dx </m>	</p></block>
			<block><p>	<m>\ds \ln|y| = x + \sin(x) + C </m>					</p></block>
			<block><p>	<m>\ds y = Ce^{x + \sin(x)} </m>						</p></block>
		</blocks>

	</exercise>

	<exercise label="c3-step-by-step-02"><title> Step-By-Step Initial-Valued Problem </title>

		<statement>
			<p>
				Use separation of variables to solve the initial value problem
			</p>
			<me>
				\frac{du}{dy} - u^2y = u^2, \hspace{1cm} u(0) = 5
			</me>.
		</statement>

		<areas>
			<ol>
				<li>
					<p>
						Select the variable that you are solving for: <m>\quad</m>
						<area correct="no">		<m>\, y \,</m>	</area> <m>\quad</m>
						<area correct="yes">	<m>\, u \,</m>	</area>
					</p>
				</li>
				<li>
					<p>
						Select the order of the equation: <m>\quad</m>
						<area correct="yes">	<m>\, 1 \,</m>	</area> <m>\quad</m>
						<area correct="no">		<m>\, 2 \,</m>	</area> <m>\quad</m>
						<area correct="no">		<m>\, 3 \,</m>	</area> <m>\quad</m>
						<area correct="no">		<m>\, 4 \,</m>	</area>
					</p>
				</li>
				<li>
					<p>
						Select the correct separable form:
					</p>
					<p>
						<tabular>
							<row>
								<cell> <area correct="no"> <m>\ds \frac{du}{dy} = u^2(y-1)	</m></area><m>\quad</m>	</cell>
								<cell> <area correct="no"> <m>\ds \frac{du}{dy} = u^2y		</m></area><m>\quad</m>	</cell>
								<cell> <area correct="yes"><m>\ds \frac{du}{dy} = u^2(1+y)	</m></area><m>\quad</m>	</cell>
								<cell> <area correct="no"> <m>\ds \frac{du}{dy} = -y		</m></area>				</cell>
							</row>
						</tabular>
					</p>
				</li>
				<li>
					<p>
						Select the next step following the correct answer to (c).
					</p>
					<p>
						<tabular>
							<row>
								<cell> <area correct="no"> <m>\ds\frac{1}{y+1}dy = u^2du	</m></area><m>\quad</m>	</cell>
								<cell> <area correct="yes"><m>\ds\frac{1}{u^2}du = (y+1)dy	</m></area><m>\quad</m>	</cell>
								<cell> <area correct="no"> <m>\ds\frac{1}{y}dy = u^2 du		</m></area>				</cell>
							</row>
						</tabular>
					</p>
				</li>
				<li>
					<p>
						Select the result after integrating correct answer to (d).
					</p>
					<p>
						<tabular>
							<row>
								<cell> <area correct="no"> <m>\ds\ln|u^2| = \frac{y^2}{2} + y + c		</m></area><m>\quad</m>	</cell>
								<cell> <area correct="no"> <m>\ds\frac{1}{u} = \frac{y^2}{2} + y + c	</m></area><m>\quad</m>	</cell>
								<cell> <area correct="yes"><m>\ds-\frac{1}{u} = \frac{y^2}{2} + y + c	</m></area>				</cell>
							</row>
						</tabular>
					</p>
				</li>
				<li>
					<p>
						Select the correct general solution.
					</p>
					<p>
						<tabular>
							<row>
								<cell> <area correct="yes"><m>\ds u = \left(-\frac{y^2}{2} + y + c\right)^{-1}	</m></area><m>\quad</m>	</cell>
								<cell> <area correct="no"> <m>\ds u = c + \left(-\frac{y^2}{2} + y\right)^{-1}	</m></area><m>\quad</m>	</cell>
								<cell> <area correct="no"> <m>\ds u = ce^{\large y^2 + y}						</m></area><m>\quad</m>	</cell>
							</row>
						</tabular>
					</p>
				</li>
				<li>
					<p>
						Select the correct particular solution.
					</p>
					<p>
						<tabular>
							<row>
								<cell> <area correct="no"> <m>\ds u = \left(-\frac{y^2}{2} + y + 5\right)^{-1}			</m></area><m>\quad</m>	</cell>
								<cell> <area correct="yes"><m>\ds u = \left(-\frac{y^2}{2} + y + \frac15\right)^{-1}	</m></area><m>\quad</m>	</cell>
								<cell> <area correct="no"> <m>\ds u = 5e^{\large y^2 + y }								</m></area>				</cell>
							</row>
						</tabular>
					</p>
				</li>
			</ol>
		</areas>

	</exercise>

	<exercisegroup><title> <em>Solve the Differential Equations</em> </title>
	
		<introduction>
			<p>
				Solve each of the following differential equations using the separation of variables method.
			</p>
		</introduction>
	
		<exercise label="c3-step-by-step-03"><title><m>\ds y'= e^{2x} - 5x</m></title>

			<introduction/>

			<webwork xml:id="c3-step-by-step-03-ww"> 
				<description>
					Solve a separable DE using separation of variables.
				</description>

				<pg-code>
					Context()->variables->add(y => 'Real');
					
					$f =Formula("e^{2 x} - 4 x");
					$order = 1;
					$f = Formula("e^{2 x} - 4 x");
					$g = Formula("1");
					$g_inv = Formula("1");
					$G = Formula("y");
					$F = Formula("1/2 e^(2x) - 2 x^2");
					$y_gen = FormulaUpToConstant("1/2 e^{2x} - 2 x^2");
				</pg-code>

				<statement>
					<p>
						<xref ref="sov-step-1" text="title" />. Give the order and separable form:
					</p>

					<p>
						<tabular>
							<col halign="right" />
							<row>
								<cell><m>\text{order:}</m></cell>
								<cell><var name="$order"  width="5" /></cell>
								<cell></cell>
								<cell><m>\displaystyle \frac{dy}{dx} = </m></cell>
								<cell><var name="$f" width="10" /></cell>
								<cell><var name="$g" width="10" /></cell>
								<cell><m>\quad\qquad\leftarrow\text{ separable form}</m></cell>
							</row>
							<row>
								<cell><m>\phantom{\text{order:}}</m></cell>
								<cell></cell>
								<cell></cell>
								<cell><m>\phantom{\displaystyle \frac{dy}{dx} = }</m></cell>
								<cell><m>\overline{\overset{\uparrow}{f(x)}}</m></cell>
								<cell><m>\overline{\overset{\uparrow}{g(y)}}</m></cell>
								<cell></cell>
							</row>
						</tabular>
					</p>

					<p>
						<xref ref="sov-step-2" text="title" />. Divide both sides of the separable form by <m>g(y)</m> and apply the integral to both sides:
					</p>

					<p>
						<tabular halign="center">
							<row>
								<cell><m>\displaystyle\int</m></cell>
								<cell><var name="$g_inv" width="10" /></cell>
								<cell><m>\displaystyle dy = \int </m></cell>
								<cell><var name="$f" width="10" /></cell>
								<cell><m>dx</m></cell>
							</row>
						</tabular>
					</p>

					<p>
						Now, compute the integrals (we have provided the constants):
					</p>

					<p>
						<tabular halign="center">
							<row>
								<cell><var name="$G" width="10" /></cell>
								<cell><m> + c_1 = </m></cell>
								<cell><var name="$F" width="10" /></cell>
								<cell><m> + c_2</m></cell>
							</row>
						</tabular>
					</p>

					<p>
						<em>Don't forget the absolute value on the left antiderivative.</em>
					</p>

					<p>
						<xref ref="sov-step-3" text="title" />. Combine constants as far as possible and use <m>c</m> for the final combined constant.
					</p>

					<p>
						<tabular>
							<col halign="right"/>
							<row>
								<cell>
									<m>y(x) = </m> <var name="$y_gen" width="10" />
								</cell>
							</row>
						</tabular>
					</p>

				</statement>

			</webwork>

			<hint>
				<p>
					Use the property <m>e^{A + B} = e^{A} \cdot e^{B}</m> to obtain the final combined constant. 
				</p>
			</hint>

		</exercise>

		<exercise label="c3-step-by-step-04"><title><m>\ds \frac{dy}{dx} = xy^2</m></title>

			<introduction/>

			<webwork xml:id="c3-step-by-step-04-ww"> 
				<description>
					Solve a separable DE using separation of variables.
				</description>

				<pg-code>
					Context()->variables->add(y => 'Real');
					Context()->variables->add(c => 'Real');
					
					$order = 1;
					$f = Formula("x");
					$g = Formula("y^2");
					$g_inv = Formula("1/y^2");
					$F = Formula("1/2*x^2");
					$G = Formula("-1/y");
					$y_gen = Formula("1/(-1/2*x^2+c)");
				</pg-code>

				<statement>
					<p>
						<xref ref="sov-step-1" text="title" />. Give the order and separable form:
					</p>

					<p>
						<tabular>
							<col halign="right" />
							<row>
								<cell><m>\text{order:}</m></cell>
								<cell><var name="$order"  width="5" /></cell>
								<cell></cell>
								<cell><m>\displaystyle \frac{dy}{dx} = </m></cell>
								<cell><var name="$f" width="10" /></cell>
								<cell><var name="$g" width="10" /></cell>
								<cell><m>\quad\qquad\leftarrow\text{ separable form}</m></cell>
							</row>
							<row>
								<cell><m>\phantom{\text{order:}}</m></cell>
								<cell></cell>
								<cell></cell>
								<cell><m>\phantom{\displaystyle \frac{dy}{dx} = }</m></cell>
								<cell><m>\overline{\overset{\uparrow}{f(x)}}</m></cell>
								<cell><m>\overline{\overset{\uparrow}{g(y)}}</m></cell>
								<cell></cell>
							</row>
						</tabular>
					</p>

					<p>
						<xref ref="sov-step-2" text="title" />. Divide both sides of the separable form by <m>g(y)</m> and apply the integral to both sides:
					</p>

					<p>
						<tabular halign="center">
							<row>
								<cell><m>\displaystyle\int</m></cell>
								<cell><var name="$g_inv" width="10" /></cell>
								<cell><m>\displaystyle dy = \int </m></cell>
								<cell><var name="$f" width="10" /></cell>
								<cell><m>dx</m></cell>
							</row>
						</tabular>
					</p>

					<p>
						Now, compute the integrals (we have provided the constants):
					</p>

					<p>
						<tabular halign="center">
							<row>
								<cell><var name="$G" width="10" /></cell>
								<cell><m> + c_1 = </m></cell>
								<cell><var name="$F" width="10" /></cell>
								<cell><m> + c_2</m></cell>
							</row>
						</tabular>
					</p>

					<p>
						<em>Don't forget the absolute value on the left antiderivative.</em>
					</p>

					<p>
						<xref ref="sov-step-3" text="title" />. Combine constants as far as possible and use <m>c</m> for the final combined constant.
					</p>

					<p>
						<tabular>
							<col halign="right"/>
							<row>
								<cell>
									<m>y(x) = </m> <var name="$y_gen" width="10" />
								</cell>
							</row>
						</tabular>
					</p>

				</statement>

			</webwork>

			<hint>
				<p>
					Use the property <m>e^{A + B} = e^{A} \cdot e^{B}</m> to obtain the final combined constant. 
				</p>
			</hint>

		</exercise>

		<exercise label="c3-step-by-step-05"><title><m>\ds\frac{dy}{dx} - y\cos(x) = y</m></title>

			<introduction/>
				
			<webwork xml:id="c3-step-by-step-02-ww"> 
				<description>
					Solve a separable DE using separation of variables.
				</description>

				<pg-code>
					Context()->variables->add(y => 'Real');
					Context()->variables->add(c => 'Real');
					$order = 1;
					$f = Formula("1+cos(x)");
					$g = Formula("y");
					$g_inv = Formula("1/y");
					$F = Formula("x+sin(x)");
					$G = Formula("ln|y|");
					$y_gen = Formula("c*e^(x+sin(x))");
				</pg-code>

				<statement>
					<p>
						<xref ref="sov-step-1" text="title" />. Give the order and separable form:
					</p>

					<p>
						<tabular>
							<col halign="right" />
							<row>
								<cell><m>\text{order:}</m></cell>
								<cell><var name="$order"  width="5" /></cell>
								<cell></cell>
								<cell><m>\displaystyle \frac{dy}{dx} = </m></cell>
								<cell><var name="$f" width="10" /></cell>
								<cell><var name="$g" width="10" /></cell>
								<cell><m>\quad\qquad\leftarrow\text{ separable form}</m></cell>
							</row>
							<row>
								<cell><m>\phantom{\text{order:}}</m></cell>
								<cell></cell>
								<cell></cell>
								<cell><m>\phantom{\displaystyle \frac{dy}{dx} = }</m></cell>
								<cell><m>\overline{\overset{\uparrow}{f(x)}}</m></cell>
								<cell><m>\overline{\overset{\uparrow}{g(y)}}</m></cell>
								<cell></cell>
							</row>
						</tabular>
					</p>

					<p>
						<xref ref="sov-step-2" text="title" />. Divide both sides of the separable form by <m>g(y)</m> and apply the integral to both sides:
					</p>

					<p>
						<tabular halign="center">
							<row>
								<cell><m>\displaystyle\int</m></cell>
								<cell><var name="$g_inv" width="10" /></cell>
								<cell><m>\displaystyle dy = \int </m></cell>
								<cell><var name="$f" width="10" /></cell>
								<cell><m>dx</m></cell>
							</row>
						</tabular>
					</p>

					<p>
						Now, compute the integrals (we have provided the constants):
					</p>

					<p>
						<tabular halign="center">
							<row>
								<cell><var name="$G" width="10" /></cell>
								<cell><m> + c_1 = </m></cell>
								<cell><var name="$F" width="10" /></cell>
								<cell><m> + c_2</m></cell>
							</row>
						</tabular>
					</p>

					<p>
						<em>Don't forget the absolute value on the left antiderivative.</em>
					</p>

					<p>
						<xref ref="sov-step-3" text="title" />. Combine constants as far as possible and use <m>c</m> for the final combined constant.
					</p>

					<p>
						<tabular>
							<col halign="right"/>
							<row>
								<cell>
									<m>y(x) = </m> <var name="$y_gen" width="10" />
								</cell>
							</row>
						</tabular>
					</p>

				</statement>

			</webwork>

			<hint>
				<p>
					Use the property <m>e^{A + B} = e^{A} \cdot e^{B}</m> to obtain the final combined constant. 
				</p>
			</hint>

		</exercise>
	
	</exercisegroup>
	
</exercises>