<subsection xmlns:xi="http://www.w3.org/2001/XInclude"><title> Second-Order LHCC </title>

	<introduction>

		<p>
			We start with ? LHCC equations ? of order 2 for two important reasons: (1) they represent the most common form you will encounter, and (2) the ideas discussed in this section naturally extend to higher order cases.
		</p>

		<p>
			<lemma xml:id="concept-lhcc-strategy-cases"><title>Order 2 LHCC General Solution Cases</title><p/>
				<statement>
					<p>
						The 2nd order LHCC DE
						<men xml:id="lhcc-cases-de">
							a\ y'' + b\ y' + c\ y = 0,
						</men>
						with characteristic equation 
						<men xml:id="lhcc-cases-ce">
							a\ r^2 + b\ r + c = 0,
						</men>
						has one the following three general solutions:
						<dl width="narrow">
							<li xml:id="lhcc-case-1"><title> Case 1: if <m>r = r_1, r_2 \,\,</m> are real and different, then </title>
								<p>
									<me> y(x) = c_1\ e^{r_1 x} + c_2\ e^{r_2 x} </me>
								</p>
							</li>
							<li xml:id="lhcc-case-2"><title> Case 2: if <m>r = r_1, r_2 \,\,</m> are real and equal, then </title>
								<p>
									<me> y(x) = c_1\ e^{r_1 x} + c_2\ x\ e^{r_2 x} </me>
								</p>
							</li>
							<li xml:id="lhcc-case-3"><title> Case 3: if <m>r = \alpha \pm i \beta \,\,</m> is complex, then </title>
								<p>
									<me> y(x) = e^{\alpha\ x} (c_1\ \sin(\beta x) + c_2\ \cos(\beta x)) </me>
								</p>
							</li>
						</dl>
					</p>
				</statement>
			</lemma> 
		</p>

		<p>
			Now that you know how to identify which types of differential equations can be solved using the ? (? Step 1 ?), you are ready for the next step, which involves solving an equation linked to the differential equation we would like to solve. This equation is referred to as the characteristic equation and is the focus of this section.
		</p>

	</introduction>

	<introduction>

		<p>
			Every ?LHCC differential equation? has a corresponding characteristic equation and the connection between them is based on the following idea.
		</p>

		<lemma xml:id="concept-lhcc-terms">
			<statement>
				<p>
					Solutions to ?LHCC? equations are composed of <m>e^{rx}</m> terms where <m>r</m> is a constant that depends on the differential equation.
				</p>
			</statement>
		</lemma>

		<p>
			To clarify this statement,
			<me>
				y = C_1 e^{4x} + C_2 e^{-x}
			</me>
			is a sample solution of some LHCC equation. The <m>e^{4x}</m> and <m>e^{-x}</m> terms correspond to <m>r=4</m> and <m>r=-1</m> in <xref ref="concept-lhcc-terms"/>, respectively. Let's investigate this concept further with an example.
		</p>

		<example xml:id="lhcc-example-01">
			<statement>
				<p>
					Find any <m>r</m> values that make <m>y = e^{rx}</m> a solution to the LHCC equation
					<men xml:id="lhcc-example-01-eqn-01">
						y'' - 9y = 0.
					</men>
				</p>
			</statement>
			<solution>
				<p>
					Approach this as if you were verifying that <m>y = e^{rx}</m> is a solution to <xref ref="lhcc-example-01-eqn-01"/>. So, plug it into the equation and check if left and right-hand sides are equal.
				</p>

				<p>
					Since we need <m>y^{\prime\prime}</m>, let's compute this first.
				</p>
				<tabular>
					<row>
						<cell><m>\displaystyle y' = e^{rx} \cdot (r) = re^{rx}</m></cell>
						<cell><em>(chain rule)</em></cell>
					</row>
					<row>
						<cell><m>\displaystyle y'' = [re^{rx}]^{\prime} = r[e^{rx}]^{\prime}  = r(e^{rx} \cdot (r)) = r^2e^{rx}</m></cell>
						<cell><em>(chain rule)</em></cell>
					</row>
				</tabular>
				<p>
					Plugging <m>y^{\prime\prime}</m> and <m>y</m> into the left side of <xref ref="lhcc-example-01-eqn-01"/> gives
				</p>
				<tabular>
					<row>
						<cell><m>\displaystyle r^2e^{rx} - 9e^{rx} = 0 </m></cell>
						<cell/>
					</row>
					<row>
						<cell><m>\displaystyle (r^2 - 9)\ e^{rx} = 0</m></cell>
						<cell><em>(factor out <m>e^{rx}</m>)</em></cell>
					</row>
				</tabular>
				<p>
					Now, <m>y = e^{rx}</m> is only a solution if we can show LHS = RHS (<em><m>0 = 0</m> in this case</em>). It should be clear that this depends on the values of <m>r</m>. This is just an algebra problem where we must solve for <m>r</m>.
				</p>
				<tabular>
					<row>
						<cell><m>\displaystyle r^2 - 9 = 0,</m></cell>
						<cell><m>\displaystyle e^{rx} = 0</m></cell>
						<cell><em>(set each factor to 0)</em></cell>
					</row>
					<row>
						<cell><m>r = \pm 3,</m></cell>
						<cell>
							<em>no solution</em>
							<fn>
								Attempting to solve <m>\displaystyle e^{rx} = 0</m> for <m>r</m> by applying <m>\ln</m> would give
								<me>
									\displaystyle \ln(e^{rx}) = \ln(0) \, \leftarrow \text{not defined}
								</me>
							</fn>
						</cell>
						<cell/>
					</row>
				</tabular>
				<p>
					So, the only <m>r</m> values that make the LHS = RHS is <m>r = -3, 3</m>.
				</p>
			</solution>
		</example>

		<p>
			The previous example showed us that finding the values of <m>r</m> that make <m>y = e^{rx}</m> a solution to <m> y'' - 9y = 0</m> amounts to solving 
			<men xml:id="lhcc-example-01-ce">
				r^2 - 9 = 0
			</men>
			for <m>r</m>. It turns out that <xref ref="lhcc-example-01-ce"/> is exactly the characteristic equation in ? Step 2 ? of the ?.
		</p>

		<p>
			Every LHCC equation has a characteristic equation that can be found in the same way as in <xref ref="lhcc-example-01"/>. In particular, you plug <m>y = e^{rx}</m> into the DE and factor out an <m>e^{rx}</m> term. Let's work out the details, but first, notice the pattern of derivatives when using the chain rule on <m>y = e^{rx}</m> at each step.
			<me>
				y = e^{rx} \quad \rightarrow \quad y' = re^{rx} \quad \rightarrow \quad y'' = r^2e^{rx} \quad \rightarrow \, \dots \, \rightarrow \quad y^{(n)} = r^ne^{rx}
			</me>
			<!-- <tabular>
				<row>
					<cell><m>\displaystyle y = e^{rx}</m></cell>
				</row>
				<row>
					<cell><m>\displaystyle y' = re^{rx}</m></cell>
				</row>
				<row>
					<cell><m>\displaystyle y'' = r^2e^{rx}</m></cell>
				</row>
				<row>
					<cell><m>\vdots</m></cell>
				</row>
				<row>
					<cell><m>\displaystyle y^{(n)} = r^ne^{rx}</m></cell>
				</row>
			</tabular> -->
		</p>

		<p>
			Plugging each of these into ? leads to
		</p>

		<tabular>
			<row>
				<cell colspan="2"><m>\displaystyle a_n\ r^ne^{rx} + \cdots + a_2\ r^2e^{rx} + a_1\ re^{rx} + a_0\ e^{rx} = 0 </m></cell>
				<cell/>
			</row>
			<row>
				<cell colspan="2"><m>\displaystyle (a_n\ r^n + \cdots + a_2\ r^2 + a_1\ r + a_0)\ e^{rx} = 0</m></cell>
				<cell><em>(factor out <m>e^{rx}</m>)</em></cell>
			</row>
			<row halign="center">
				<cell><m>\displaystyle a_n\ r^n + \cdots + a_2\ r^2 + a_1\ r + a_0 = 0,</m></cell>
				<cell><m>\displaystyle e^{rx} = 0</m></cell>
				<cell><em>(set each factor to 0)</em></cell>
			</row>
			<row halign="center">
				<cell><m>\uparrow</m></cell>
				<cell><m>\uparrow</m></cell>
				<cell/>
			</row>
			<row halign="center">
				<cell><em>characteristic equation!</em></cell>
				<cell><em>no solution</em></cell>
				<cell/>
			</row>
		</tabular>

		<p>
			Going through this process a few times should convince you that there is a simple relationship between the differential equation and its corresponding characteristic equation. Looking at the equations side-by-side shows that the derivatives of <m>y</m> map directly to the powers of <m>r</m>.
			<!-- <tabular>
				<row>
					<cell><m> a_n\ y^{(n)} + a_{n-1}\ y^{(n-1)} + \cdots + a_2\ y'' + a_1\ y' + a_0\ y = 0 </m></cell>
				</row>
				<row>
					<cell><m> a_n\ y^{(n)} + a_{n-1}\ y^{(n-1)} + \cdots + a_2\ y'' + a_1\ y' + a_0\ y = 0 </m></cell>
				</row>
				<row>
					<cell><m> a_n\ r^n + a_{n-1}\ r^{n-1} + \cdots + a_2\ r^2 + a_1\ r+ a_0\ = 0 </m></cell>
				</row>
			</tabular> -->

			<!-- a_n\ \underset{\downarrow}{	\underline{y^{(n)}}}	\amp + \cdots +	\amp a_2\ \underset{\downarrow}{\underline{y''}}	\amp + \amp	a_1\ \underset{\downarrow}{	\underline{y'}}	\amp + \amp	a_0\ \underset{\downarrow}{\underline{y}}	\amp =	\amp 0\\ -->
			
			<me>
				\begin{matrix}
					a_n\ \underline{y^{(n)}}	\amp + \cdots +	\amp a_2\ \underline{y''}	\amp +	\amp	a_1\ \underline{y'}		\amp +	\amp	a_0\ \underline{y}		\amp =\ 0	\\
						\ \ \ \downarrow		\amp			\amp    \ \ \ \downarrow	\amp 	\amp	   \ \ \ \downarrow		\amp 	\amp	   \ \ \ \downarrow		\amp	 	\\
					a_n\ \underline{r^n}		\amp + \cdots +	\amp a_2\ \underline{r^2}	\amp +	\amp	a_1\ \underline{r^1}	\amp +	\amp	a_0\ \underset{=\ 1}{\underline{r^0}}	\amp =\ 0
				\end{matrix}
			</me>

		</p>
		
		<definition xml:id="def-lhcc-ce">
			<statement>
				<p>
					The <term>characteristic equation</term> of an ? LHCC equation ? is given by
					<men xml:id="def-lhcc-ce-eqn">
						a_n\ r^{n} + \cdots + a_2\ r^2 + a_1\ r + a_0 = 0.
					</men>
				</p>
			</statement>
		</definition>

		<example>
			<p>
				Give the characteristic equation of the differential equation
				<me>
					y'' + 5y' - y = 0.
				</me>
			</p>

			<solution>
				<p>
					<me>
						r^2 + 5r - 1 = 0
					</me>
				</p>
			</solution>
	
		</example>

	</introduction>

	<introduction>

		<p>
			Once you have the characteristic equation of differential equation, you need to solve it. The equations you solve will be in the form
			<me>
				\overbrace{a_n\ r^{n} + \cdots + a_2\ r^2 + a_1\ r + a_0}^{ \large{\text{polynomial of degree } n} } = 0,
			</me>
			where <m>r</m> is the unknown. 
		</p>

		<p>
			Degree 2 characteristic equations have the familiar form
			<me>
				a\ r^2 + b\ r + c = 0,
			</me>
			and have two solutions, found by either factoring, 
			<md>
				<mrow>(r - r_1)(r - r_2) = 0,</mrow>
				<mrow>r = r_1,\ r_2 </mrow>
			</md>
			or, by applying the quadratic formula.
			<fn> 
				The solution to the equation 
				<me> 
					a\ x^2 + b\ x + c = 0, 
				</me> 
				is given by
				<me>
					\text{quadratic formula:} \quad x = \frac{b \pm \sqrt{b^2 - 4ac}}{2a}.
				</me>
			</fn>
			<!-- Since the values you get from either method are the same, we can technically write the factoring technique as
			<me>
				(r - r_1)(r - r_2) = 0,
			</me>
			where
			<me>
				r_1 = \frac{b + \sqrt{b^2 - 4ac}}{2a} \quad \text{ and } \quad r_2 = \frac{b - \sqrt{b^2 - 4ac}}{2a}.
			</me> -->
		</p>


		<paragraphs><title>	Characteristic Equations of Higher Degree </title><p/>

			<p>
				Higher degree characteristic equations, such as
				<md>
					<mrow> \text{degree 3:} \quad	\amp a\ r^3 + b\ r + c\ r + d = 0, </mrow>
					<mrow> \text{degree 4:} \quad	\amp a\ r^4 + b\ r^3 + c\ r^2 + d\ r + e  = 0, </mrow>
					<mrow> \text{degree 5:} \quad	\amp a\ r^5 + b\ r^4 + c\ r^3 + d\ r^2 + e\ r + f = 0, </mrow>
					<mrow> 							\amp \vdots </mrow>
				</md>
				can always be factored as
				<fn>
					This fact is known as the fundamental theorem of algebra.
				</fn>
				<md>
					<mrow> \text{degree 3:} \quad	\amp (r - r_1)(r - r_2)(r - r_3) = 0, </mrow>
					<mrow> \text{degree 4:} \quad	\amp (r - r_1)(r - r_2)(r - r_3)(r - r_4)  = 0, </mrow>
					<mrow> \text{degree 5:} \quad	\amp (r - r_1)(r - r_2)(r - r_3)(r - r_4)(r - r_5) = 0, </mrow>
					<mrow> 							\amp \vdots </mrow>
				</md>
				where <m> r_1, r_2, r_3, ... </m> are the solutions and could be real or complex.
				<aside>
					<p>
						A "complex" solution is one that is allowed to contain <m>\sqrt{-1}</m> (imaginary part).
					</p>
					<p>
						For example, the equation <m>x^2 = -4</m> has two complex solutions since 
						<md>
							<mrow> x	\amp= \pm \sqrt{-4} 				</mrow>
							<mrow>   	\amp= \pm \sqrt{4\cdot -1}			</mrow>
							<mrow>   	\amp= \pm \sqrt{4}\cdot \sqrt{-1}	</mrow>
							<mrow>   	\amp= \pm 2\ i						</mrow>
						</md>
					</p>
				</aside>
				The problem is that they are often difficult to factor. However, there are some cases where these equations can be factored fairly easily as the next example illustrates.
			</p>

			<example>
				<statement>
					<p>
						Completely factor and solve the following characteristic equations
						<ol>
							<li> <m> 4\ r^2 - 9 = 0 </m> </li>
							<li> <m> r^2 - 3 = 0 </m> </li>
							<li> <m> r^3 + 3\ r^2 - 4\ r = 0 </m> </li>
							<li> <m> r^5 + 10\ r^4 = 0 </m> </li>
							<li> <m> r^4 - 100\ r^2 = 0 </m> </li>
							<li> <m> r^5 - 4\ r^3 = 0 </m> </li>
							<li> <m> r^4 - 32 = 0 </m> </li>
						</ol>
					</p>
				</statement>
				<solution>
					<p>
						The degree of each equation tells you how many factors you should have.
						<ol>
							<li>
								<p>
									<tabular>
										<row>
											<cell><m> 4\ r^2 - 9 = 0 </m></cell>
											<cell/>
										</row>
										<row>
											<cell><m> (2\ r + 3)(2\ r - 3) = 0 </m></cell>
											<cell> <m>\leftarrow</m> difference of squares </cell>
										</row>
										<row>
											<cell><m> 2\ r + 3 = 0, \quad 2\ r - 3 = 0 </m></cell>
											<cell><m>\leftarrow</m> set each factor to 0 </cell>
										</row>
										<row>
											<cell><m> \displaystyle r_1 = -\frac32, \quad r_2 = \frac32 </m></cell>
											<cell><m>\leftarrow</m> solutions </cell>
										</row>
									</tabular>
								</p>
							</li>

							<li>
								<p>
									<tabular>
										<row>
											<cell><m> r^2 - 3 = 0 </m></cell>
											<cell/>
										</row>
										<row>
											<cell><m> (r + \sqrt{3})(r - \sqrt{3}) = 0 </m></cell>
											<cell> <m>\leftarrow</m> difference of squares </cell>
										</row>
										<row>
											<cell><m> \displaystyle r_1 = -\sqrt{3}, \quad r_2 = \sqrt{3} </m></cell>
											<cell><m>\leftarrow</m> solutions </cell>
										</row>
									</tabular>
								</p>
							</li>

							<li>
								<p>
									<tabular>
										<row>
											<cell><m> r^3 + 3\ r^2 - 4\ r = 0 </m></cell>
											<cell/>
										</row>
										<row>
											<cell><m> r\ (r^2 + 3\ r - 4) = 0 </m></cell>
											<cell> <m>\leftarrow</m> common factor </cell>
										</row>
										<row>
											<cell><m> r\ (r + 4)(r - 1) = 0 </m></cell>
											<cell> <m>\leftarrow</m> standard quadratic factoring </cell>
										</row>
										<row>
											<cell><m> \displaystyle r_1 = 0, \quad r_2 = -4, \quad r_3 = 1 </m></cell>
											<cell><m>\leftarrow</m> solutions </cell>
										</row>
									</tabular>
								</p>
							</li>
							
							<li>
								<p>
									<tabular>
										<row>
											<cell><m> r^5 + 10\ r^4 = 0 </m></cell>
											<cell/>
										</row>
										<row>
											<cell><m> r^4\ (r + 10) = 0 </m></cell>
											<cell> <m>\leftarrow</m> common factor </cell>
										</row>
										<row>
											<cell><m> \displaystyle r_1 = 0\ (\text{4 repeats}), \quad r_2 = -10 </m></cell>
											<cell><m>\leftarrow</m> solutions </cell>
										</row>
									</tabular>
								</p>
								<p>
									<em> Technically, <m>r^4 = (r-0)^4</m> and represents 4 repeated factors. </em>
								</p>
							</li>


							<li>
								<p>
									<tabular>
										<row>
											<cell><m> r^4 - 100\ r^2 = 0 </m></cell>
											<cell/>
										</row>
										<row>
											<cell><m> r^2\ (r^2 - 100) = 0 </m></cell>
											<cell> <m>\leftarrow</m> common factor </cell>
										</row>
										<row>
											<cell><m> r^2\ (r + 10)(r - 10) = 0 </m></cell>
											<cell> <m>\leftarrow</m> difference of squares </cell>
										</row>
										<row>
											<cell><m> \displaystyle r_1 = 0\ (\text{2 repeats}), \quad r_2 = -10, \quad r_3 = 10 </m></cell>
											<cell><m>\leftarrow</m> solutions </cell>
										</row>
									</tabular>
								</p>
							</li>

							<li>
								<p>
									<tabular>
										<row>
											<cell><m> r^5 - 4\ r^3 = 0 </m></cell>
											<cell/>
										</row>
										<row>
											<cell><m> r^3\ (r^2  - 4) = 0 </m></cell>
											<cell> <m>\leftarrow</m> common factor </cell>
										</row>
										<row>
											<cell><m> r^3\ (r + 2)(r - 2) = 0 </m></cell>
											<cell> <m>\leftarrow</m> difference of squares </cell>
										</row>
										<row>
											<cell><m> \displaystyle r_1 = 0\ (\text{3 repeats}), \quad r_2 = -2, \quad r_3 = 2 </m></cell>
											<cell><m>\leftarrow</m> solutions </cell>
										</row>
									</tabular>
								</p>
							</li>

							<li>
								<p>
									<tabular>
										<row>
											<cell><m> r^4 - 25 = 0 </m></cell>
											<cell/>
										</row>
										<row>
											<cell><m> (r^2 + 5)(r^2  - 5) = 0 </m></cell>
											<cell> <m>\leftarrow</m> difference of squares </cell>
										</row>
										<row>
											<cell><m> (r^2 + 5)(r - \sqrt{5})(r + \sqrt{5}) = 0 </m></cell>
											<cell> <m>\leftarrow</m> difference of squares </cell>
										</row>
										<row>
											<cell><m> r^2 + 5 = 0, \quad r - \sqrt{5} = 0, \quad r + \sqrt{5} = 0 </m></cell>
											<cell><m>\leftarrow</m> set each factor to 0 </cell>
										</row>
										<row>
											<cell><m> \displaystyle r_1 = -i\sqrt{5}, \quad r_2 = i\sqrt{5}, \quad r_3 = -\sqrt{5}, \quad r_4 = \sqrt{5} </m></cell>
											<cell><m>\leftarrow</m> solutions </cell>
										</row>
									</tabular>
								</p>
							</li>

						</ol>
					</p>
				</solution>
			</example>

		</paragraphs>

		<!-- <interactive xml:id="discont-function2" platform="sage" width="100%" aspect_ratio="1:1">
			<slate surface="sage">
				r = var('r')
				INI_func = 'r^2 - 2*r - 8'
				@interact
				def _(ce = input_box(INI_func, label="Characteristic Polynomial:", type=str, width=20)):

					ce_poly = sage_eval('lambda r: ' + ce)
					pretty_print( html( 'Factored Characteristic Equation:') )
					pretty_print( html( r'$ %s = 0 $'%latex(ce_poly(r) ) ) )
					pretty_print( html( r'$ %s = 0 $'%latex(ce_poly(r).factor()) ) )
			</slate>
		</interactive> -->

	</introduction>

	
	<xi:include href="./c3-s1-ss4-interactives.ptx" />

</subsection>