<section xmlns:xi="http://www.w3.org/2001/XInclude"><title> General Solutions </title>

	<p>
		Our goal is to solve <xref ref="def-lhcc" text="custom">LHCC equations</xref>. Before diving into the methods, let's develop some intuition about what the solutions should look like.
	</p>

	<p>
		Let's consider the simple first-order LHCC equation 
		<me> y' - 2 y = 0 </me>.
		You may remeber from algebra, the only type of terms that simplify to zero are like terms. For example, 
		<me>2x - 2x = 0 \quad \text{or} \quad 3w^2 - 3w^2 = 0</me>. 
		Therefore, this equation requires <m>y'</m> and <m>y</m> to be like terms. To see what kind of function might work let's try a few and see what happens.
	</p>

	<p>
		Consider <m>y = x^2</m>, <m>y = 2/x</m>, and <m>y = e^{2x}</m>. Plugging these in we see
		<sidebyside widths="30% 40% 30%">
			<p>
				<md>
					<mrow> \left[x^2\right]' - 2 \left[x^2\right] = 0 </mrow>
					<mrow> 2x - 2x^2 = 0 </mrow>
				</md>
			</p>
			<p>
				<md>
					<mrow> \left[\sin(2x)\right]' - 2 \sin(2x) = 0 </mrow>
					<mrow> 2\cos(2x) - 2\sin(2x) = 0 </mrow>
				</md>
			</p>
			<p>
				<md>
					<mrow> \left[e^{2x}\right]' - 2 \left[e^{2x}\right] = 0 </mrow>
					<mrow> 2e^{2x} - 2e^{2x} = 0 </mrow>
				</md>
			</p>
		</sidebyside>
		As you can see, the only function that is a like term with its derivative is <m>y = e^{2x}</m>. In general, the only functions with this property are exponential functions.
	</p>

	<p>
		Recall from calculus the function whose derivative is itself. If you thought of <m>e^x</m>, you're right! This can be framed as a differential equation: find the function <m>y</m> such that <m>y' = y</m>. The solution is <m>y = e^x</m>, but it's also true that <m>y = c e^x</m> for any constant <m>c</m>. Now, consider a function whose derivative is a multiple of itself, like <m>3y</m>. You might think of <m>y = e^{3x}</m>. If this isn't obvious, you can solve <m>y' = 3y</m> using separation of variables to find <m>y = c e^{3x}</m>.
	</p>


	<p>
		This leads us to an important concept:
		<assemblage><title> Property of the Exponential Function </title>
			<p>
				<ul marker="square">
					<li>
						<m>e^{rx}</m> is the only function whose derivative is a multiple of itself.
					</li>
					<li>
						<m>e^{rx}</m> and its derivatives are like terms that can be combined.
					</li>
				</ul>
			</p>
		</assemblage>
		Most functions change fundamentally when differentiated and do not yield like terms that can be combined. For example, the derivative of <m>x^8</m> is <m>8x^7</m>, which cannot be combined or simplified in the same way. However, <m>e^{3x}</m> and its derivative <m>3e^{3x}</m> can be added together as <m>e^{3x} + 3e^{3x} = 4e^{3x}</m>.
	</p>

	<p>
		Going back to the LHCC equation,
		<men xml:id="lhcc-equation-like-terms">
			\us{\text{must sum to } 0 \text{ after substituting } y}{\ub{
				a_n\ y^{(n)} + \cdots + a_2\ y'' + a_1\ y' + a_0\ y
			}}	= 0
		</men>,
		the right-hand side is zero, so the left-hand side must sum to zero after substituting <m>y</m>. This can only happen if the solution <m>y</m> and its derivatives combine to cancel each other out. However, the only possible functions that can be substituted for <m>y</m> are ones that contain <m>e^{rx}</m>.
	</p>

	<p>
		Let's look at a concrete example to illustrate why <m>e^{rx}</m> simplifies nicely in these equations, while other functions may not.
	</p>

	<example>
		<m>\ \ </m> Consider the LHCC equation:
		<me>
			y'' + 3y' - 4y = 0.
		</me>
		<p>
			Verify that <m>y = e^{4x}</m> is a solution, but <m>y = x^4</m> and <m>y = \sin(4x)</m> are not.
		</p>
		<solution>
			<p>
				Let's check each function:
			</p>
			<sidebyside>
				<p>
					<md>
						<mrow> 	[e^{4x}]'' + 3\left[e^{4x}\right]' - 4\left[e^{4x}\right]	=\amp\ 0	</mrow>
						<mrow> 	
							\us{\text{like terms simplify to }0}{\ub{
								16e^{4x} + 12e^{4x} - 4e^{4x}	
							}}
							=\amp\ 0	
						</mrow>
						<mrow> 	0	=\amp\ 0	\ \ ✅ </mrow>
					</md>
				</p>
				<p>
					<md>
						<mrow> 	[x^4]'' + 3\left[x^4\right]' - 4\left[x^4\right]	=\amp\ 0	</mrow>
						<mrow> 	
							\us{\text{not like terms, do not combine}}{\ub{
								24x^2 + 12x^3 - 4x^4	
							}}
							=\amp\ 0	\ \ ❌
						</mrow>
					</md>
				</p>
			</sidebyside>
			<p>
				<md>
					<mrow> 	[\sin(4x)]'' + 3\left[\sin(4x)\right]' - 4\left[\sin(4x)\right]	=\amp\ 0	</mrow>
					<mrow> 	
						\us{\text{not like terms}}{\ub{
							-16\sin(4x) + 12\cos(4x) - 4\sin(4x)	
						}}
						=\amp\ 0	\ \ ❌
					</mrow>
				</md>
			</p>
			<p>
				Of these three, only <m>y = e^{4x}</m> is a solution.
			</p>
		</solution>
	</example>

	<p>
		This example shows that <m>e^{rx}</m> is best suited for LHCC equations, but it doesn't tell the whole story. In some cases, if <m>e^{rx}</m> is a solution, then it is possible that <m>xe^{rx}</m> could also be a solution.
	</p>

	<p>
		The takeaway from this section should be that solutions to LHCC equations must involve <m>e^{rx}</m>, but not every value of <m>r</m> works. In the next section, we will see that the key to finding the general solution lies in finding the values of <m>r</m> that correspond to solutions.
	</p>

</section>
