<section xmlns:xi="http://www.w3.org/2001/XInclude"><title> General Solution Parts </title>
	
	<p>
		As discussed in the last section, every solution to a nonhomogeneous differential equation must account for the non-zero term on the right-hand side. However, hidden within these solutions could be terms that cancel out with each other instead of contributing to the term on the right-hand side.
	</p>

	<p>
		To see this, let's bring back the equation from the last section,
		<men xml:id="lncc-eqn1">
			y'' - 4y' + 3y = 9x
		</men>,
		which we know has <m>y=3x+4</m> as a solution. Would it still be a solution if we tossed another term, say <m>e^{3x}</m>, onto it so that <m>y=e^{3x} + 3x + 4</m>? To find out, we plug it in and track this new term (in blue), like so 
		<md>
			<mrow> 
				\left( {\color{blue} e^{3x}} + 3x + 4 \right)'' 
				-4\left( {\color{blue} e^{3x}} + 3x + 4 \right)' 
				+3\left( {\color{blue} e^{3x}} + 3x + 4 \right) =\ &amp; 9x 
			</mrow>
			<mrow> 
				\left( {\color{blue} e^{3x}} \right)'' + \left( 3x + 4 \right)''
				-4\left( {\color{blue} e^{3x}} \right)' - 4\left( 3x + 4 \right)'
				+3\left( {\color{blue} e^{3x}} \right) + 3\left( 3x + 4 \right) =\ &amp; 9x 
			</mrow>
			<mrow> 
				\us{\large e^{3x} \text{ in the LHS of } <xref ref="lncc-eqn1"/>}{\ub{
					\left( {\color{blue} e^{3x}} \right)'' 
					-4\left( {\color{blue} e^{3x}} \right)' 
					+3\left( {\color{blue} e^{3x}} \right)}
				} + 
				\us{\large 3x + 4 \text{ in the LHS of } <xref ref="lncc-eqn1"/>}{\ub{
					\left( 3x + 4 \right)'' 
					-4\left( 3x + 4 \right)' 
					+3\left( 3x + 4 \right)
				 }} =\ &amp; 9x 
			</mrow>
		</md>
		<!-- Before simplifying, notice that it looks like we plugged <m>e^{3x}</m> and <m>3x+4</m> separately into <xref ref="lncc-eqn1"/>. Now, let's finish simplifying to see if <m>y=e^{3x} + 3x + 4</m> is a solution. -->
		<md>
			<mrow> 
				\left( {\color{blue} 9e^{3x}} \right)
				-4\left( {\color{blue} 3e^{3x}} \right)
				+3\left( {\color{blue} e^{3x}} \right) + 
				0 -4\left( 3 \right) +3\left( 3x + 4 \right) =\ &amp; 9x 
			</mrow>
			<mrow> 
				{\color{blue} 9e^{3x} - 12e^{3x} + 3e^{3x}} - 12 + 9x + 12 =\ &amp; 9x 
			</mrow>
			<mrow> 
				{\color{blue} 0} + 9x =\ &amp; 9x 
			</mrow>
		</md>
		There is a lot built into this result, so let's carefully break it down. 
		<ul marker="square">
			<li>
				<p>
					First, <m>y=e^{3x} + 3x + 4</m> is a solution since it satisfies <xref ref="lncc-eqn1"/>.
				</p>
			</li>
			<li>
				<p>
					The solution contains the two parts
					<me>
						y=\us{(1)}{\ul{e^{3x}}} + \us{(2)}{\ul{3x + 4}}
					</me>,
					where part (1) contains the terms that simplifies to <m>0</m> and part (2) contains the terms that simplify to <m>9x</m> when plugged into <xref ref="lncc-eqn1"/>.
				</p>
			</li>
			<li>
				<p>
					The third step looks like <m>e^{3x}</m> and <m>3x+4</m> were separately plugged into <xref ref="lncc-eqn1"/>. As long as the equation is linear, this separation can happen.
				</p>
			</li>
		</ul>
	</p>

	<men xml:id="lncc-order2-gen-soln-parts">
		\underset{\text{terms that cancel}}{\underbrace{a_2 y_h'' + a_1 y_h' + a_0 y_h}} + 
		\underset{\text{terms that account for } f(x)}{\underbrace{a_2 y_p'' + a_1 y_p' + a_0 y_p}} = f(x)
	</men>

	<p>
		This example illustrates the following general principle of LNCC equations.
		
		<assemblage xml:id="lncc-general-solution-parts"><title>LNCC General Solution Parts</title>
			<p>
				The linear nonhomogeneous constant coefficient equation
			</p>

			<p>
				<men xml:id="lncc-general-equation">
					a_n y^{(n)} + \cdots + a_1 y' + a_0 y = f(x)
				</men>
				has a two-part general solution that can be written as
				<men xml:id="lncc-general-solution">
					y = y_h + y_p
				</men>.
				Plugging this into <xref ref="lncc-general-equation"/>, we can separate <m>y_h</m> and <m>y_p</m> like so
				<me>
					\us{\large \text{terms of } <xref ref="lncc-general-solution"/> \text{ that give } 0}{\ub{a_n y_h^{(n)} + \cdots + a_1 y_h' + a_0 y_h}} + 
					\us{\large \text{terms of } <xref ref="lncc-general-solution"/> \text{ that give } f(x)}{\ub{a_n y_p^{(n)} + \cdots + a_1 y_p' + a_0 y_p}} = f(x)
				</me>.
				We call <m>y_h</m> the <term>homogeneous part</term> of <xref ref="lncc-general-solution"/> and find it by solving
				<me>
					a_n y^{(n)} + \cdots + a_2 y'' + a_1 y' + a_0 y = 0
				</me>.
				The part, <m>y_p</m>, is the <term>particular solution</term> of <xref ref="lncc-general-solution"/>, which accounts for <m>f(x)</m>.
			</p>
		</assemblage>
	</p>

	<example>
		<statement>
			<p>
				Give the general solution to the differential equation
			</p>
			<me>
				y'' - 4y' + 3y = 9x
			</me>.
		</statement>
		<solution>
			<p>
				The general solution has the form 
				<me>
					y = y_h + y_p
				</me>
				where <m>y_p</m> is the particular solution that gives <m>9x</m>, is already known as
				<me>
					y_p = 3x + 4
				</me>.
				The homogeneous part, <m>y_h</m>, that gives <m>0</m>, is found by solving
				<me>
					y'' - 4y' + 3y = 0
				</me>
				using the characteristic equation, as follows 
				<me>
					r^2 - 4r + 3 = 0 \ \ \implies \ \ (r - 3)(r - 1) = 0 \ \ \implies \ \ r = 3, r = 1
				</me>.
				So the homogeneous part is
				<me>
					y_h = c_1e^{3x} + c_2e^x
				</me>
				and the general solution is given by
				<me>
					y = y_h + y_p = \us{\text{terms cancel}}{\ub{c_1e^{3x} + c_2e^x}} + \us{\text{terms give }9x}{\ub{3x + 4}}
				</me>
			</p>

		</solution>
	</example>

	<p>
		Before we can start solving these equations, we still need a strategy for finding the particular solution, <m>y_p</m>. This will be the focus of the next few sections.
	</p>

	<xi:include href="./p3-c2-s2-interactives.ptx" />

</section>