<section xmlns:xi="http://www.w3.org/2001/XInclude"><title> Additional Examples </title>

	<p>
		In this section, we will look at more advanced examples of the integrating factor method. These examples will demonstrate how the technique applies to a wider variety of differential equations, including those with more complex functions or integration techniques. Each example will follow the <xref ref="if-method" text="custom">four-step process</xref> outlined in the previous section.
	</p>

	<example>
		<m>\ \ </m> Solve the differential equation:
		<p> 
		  	<me>x^2 y' - y = 1, \quad x > 0</me>.
		</p>
	  
		<solution>

			<p>
				This is a first-order linear differential equation, so we can apply the integrating factor method.
			</p>
		
			<p>
				<xref ref="if-step-1" text="title"/>.
				<md>
					<mrow> y' + \us{P}{\boxed{-\frac{1}{x^2}}}\ y = \frac{1}{x^2}	</mrow>
				</md>
			</p>
		
			<p>
				<xref ref="if-step-2" text="title"/>.
				<md>
					<mrow> \mu(x) = e^{\large \int -\sfrac{1}{x^2} dx} = e^{1/x}	</mrow>
				</md>
			</p>
		
			<p>
				<xref ref="if-step-3" text="title"/>.
				<md>
					<mrow> e^{1/x}y' - \frac{e^{1/x}}{x^2} y	=\amp\ \frac{e^{1/x}}{x^2}	</mrow>
					<mrow> \frac{d}{dx}\left[e^{1/x} y\right]	=\amp\ \frac{e^{1/x}}{x^2}	</mrow>
				</md>
			</p>
		
			<p>
				<xref ref="if-step-4" text="title"/>.
				<md>
					<mrow> \int \frac{d}{dx}\left[e^{1/x} y\right] dx =\amp\ \int \frac{e^{1/x}}{x^2} dx \quad \left(u = \sfrac{1}{x}\right)	</mrow>
					<mrow> e^{1/x} y =\amp\ \int -e^u du	</mrow>
					<mrow> e^{1/x} y =\amp\ -e^u + c	</mrow>
					<mrow> e^{1/x} y =\amp\ -e^{1/x} + c	</mrow>
				</md>
				Now, we can solve for <m>y</m>:
				<md>
					<mrow> y = -1 + ce^{-1/x}	</mrow>
				</md>
			</p>
		
		</solution>
	  
	</example>

	<example>
		<m>\ \ </m> Solve the equation:
		<p> 
			<me> t^2 y' + 2ty = t^3 \ln t </me>.
		</p>

		<solution>

			<p>
				This is a linear equation, and we will solve it using the integrating factor method.
			</p>

			<p>
				<xref ref="if-step-1" text="title"/>.
				<md>
					<mrow> y' + \frac{2}{t} y = t \ln t </mrow>
				</md>
			</p>
+
			<p>
				<xref ref="if-step-2" text="title"/>.
				<md>
					<mrow> \mu(t) = e^{\large \int (\sfrac{2}{t})\, dt} = e^{2 \ln t} = t^2	</mrow>
				</md>
			</p>

			<p>
				<xref ref="if-step-3" text="title"/>.
				<md>
					<mrow> t^2 y' + 2t y					=\amp\ t^3 \ln t	</mrow>
					<mrow> \frac{d}{dt} \left[t^2 y\right]	=\amp\ t^3 \ln t	</mrow>
				</md>
			</p>

			<p>
				<xref ref="if-step-4" text="title"/>.
				<md>
					<mrow> \int \frac{d}{dt} \left[t^2 y\right] dt	=\amp\ \int t^3 \ln t\ dt	</mrow>
					<mrow> t^2 y									=\amp\ \int t^3 \ln t\ dt	</mrow>
				</md>
				Using <xref ref="ibp-formula" text="custom">integration by parts</xref> on the integral with
				<md>
					<mrow>u = \ln t,			\amp \quad v = \frac14t^4	</mrow>
					<mrow>du = \frac{1}{t}\ dt,	\amp \quad dv = t^3\ dt		</mrow>
				</md>
				gives us
				<md>
					<mrow> t^2 y	=\amp\ \frac14 t^4 \ln t - \int \frac14 t^4 \cdot \frac{1}{t}\ dt	</mrow>
					<mrow> t^2 y	=\amp\ \frac14 t^4 \ln t - \frac14 \int  t^3\ dt	</mrow>
					<mrow> t^2 y	=\amp\ \frac{t^4}{4} \ln t - \frac{t^4}{16} + c	</mrow>
					<mrow> y		=\amp\ \frac{t^2}{4} \ln t - \frac{t^2}{16} + c\,t^2	</mrow>
				</md>
			</p>

		</solution>

	</example>

	<example>

		<m>\ \ </m> Solve the initial value problem.
		<p> 
			<me>A = \sec\theta A' - \frac{\theta e^{\theta^2 + \sin\theta}}{\cos \theta}, \hspace{1cm} A(0) = -\frac{1}{2}</me>.
		</p>

		<solution>

			<p>
				Before applying the integration factor method, we note that the equation is first order and linear.
			</p>

			<p>
				<xref ref="if-step-1" text="title"/>.
				<md>
					<mrow>
						\sec\theta A' - A
							=\amp\ \frac{\theta e^{\theta^2 + \sin\theta}}{\cos \theta}	\qquad \text{Note: } \sec\theta = \frac{1}{\cos\theta}
					</mrow>
					<mrow>
						A' + \us{P}{\boxed{- \cos\theta}}\ A	
							=\amp\ \theta e^{\theta^2 + \sin\theta}
					</mrow>
				</md>
			</p>

			<p>
				<xref ref="if-step-2" text="title"/>.
				<md>
					<mrow> \mu = e^{\int -\cos\theta d\theta} = e^{-\sin\theta}	</mrow>
				</md>
			</p>

			<p>
				<xref ref="if-step-3" text="title"/>.
				<md>
					<mrow> e^{-\sin\theta}A' - \cos\theta e^{-\sin\theta}A = \theta e^{\theta^2 + \sin\theta}	</mrow>
					<mrow> \frac{d}{d\theta}\left[ e^{-\sin\theta}A \right] = \theta e^{\theta^2}	</mrow>
				</md>
			</p>

			<p>
				<xref ref="if-step-4" text="title"/>.
				<md>
					<mrow>
						\int \frac{d}{d\theta}\left[ e^{-\sin\theta}A \right] d\theta = \int \theta e^{\theta^2} d\theta
					</mrow>
					<mrow>
						e^{-\sin\theta}A = \frac{1}{2}e^{\theta^2} + c
					</mrow>
					<mrow>
						A = \frac{1}{2}e^{\theta^2 + \sin\theta} + ce^{\sin\theta}
					</mrow>
				</md>
			</p>

			<p>
				Finally, we apply the initial condition to determine the constant <m>c</m>.
				<md>
					<mrow> -\frac{1}{2} = A(0) = \frac{1}{2}e^{0^2 + \sin(0)} + ce^{\sin(0)} = \frac{1}{2}e^0 + ce^0= \frac{1}{2} + c	</mrow>
					<mrow> -1 = c	</mrow>
				</md>
			</p>

			<p>
				We can then write the particular solution to the initial value problem.
				<me>A(\theta) = \frac{1}{2}e^{\theta^2 + \sin\theta} - e^{\sin\theta}</me>
			</p>

		</solution>
		
	</example>

	<p>
		The integrating factor method is a versatile tool for solving first-order linear differential equations. By reducing the equation to a form that allows for direct integration, we can tackle a wide variety of problems with confidence. The examples in this chapter illustrate the broad applicability of this technique, and practice with a range of equations will solidify your understanding of how to use it effectively.
	</p>

	<xi:include href="./p2-c3-s4-interactives.ptx" />

</section>