<section xmlns:xi="http://www.w3.org/2001/XInclude"><title> Common Transforms </title>

	<introduction>
		<p>
			In this section, we will explore some of the most commonly encountered Laplace transforms. These functions frequently appear in differential equations, making their transforms especially valuable tools for solving such equations. Let's start with the Laplace transform of the exponential function, <m>e^{at}</m>, and gradually build up to more complex functions like power functions, sine, and cosine.
		</p>
	</introduction>

	<subsection><title> Constant Function, <m>1</m> </title>
		<example>

			<m>\ \ </m>Compute <m>\ds \lap{1}</m>.

			<solution><title> Solution </title>
				<p>
					By the definition above, we have the improper integral
					<men xml:id="lt-1-example-eqn-1"> 
						\lap{1} = \int_0^{\infty} e^{-st} \cdot 1\ dt = \lim_{b \to \infty} \ub{\int_0^b e^{-st}dt}_{I}
					</men>.
					To evaluate this, we treat <m>s</m> as a constant and integrate with respect to <m>t</m>.
					<md>
						<mrow>				
							I = \int_0^b e^{-st}dt
							=\amp\ -\frac{1}{s}e^{-st}\Big|_{t=0}^{t=b}
						</mrow>
						<mrow>			
							=\amp\ -\frac{1}{s}\left[ e^{-sb} - e^{-s\cdot 0} \right]
						</mrow>
						<mrow>			
							=\amp\ -\frac{1}{s}\left[ e^{-sb} - 1 \right]
						</mrow>
					</md>
					Now that we have <m>I</m>, we can plug it into the limit above.
					<md>
						<mrow> 
							\lim_{b \to \infty} -\frac{1}{s}\left[ e^{-sb} - 1 \right]
							=\amp\ -\frac{1}{s} \lim_{b \to \infty} \Big[ e^{-sb} - 1 \Big] 
							\qquad \leftarrow <xref text="custom" ref="reason-factor-out-s">why?</xref>
						</mrow>
						<mrow> 
								=\amp\ -\frac{1}{s} \Big[ \ub{\lim_{b \to \infty} e^{-sb}}_{L} - \us{=\ 1}{\ub{\lim_{b \to \infty} 1}} \Big] 
						</mrow>
					</md>
				</p>
		
				<p>
					The value of the remaining limit, <m>L</m>, depends on whether <m>s</m> is positive or negative. So we consider both cases:
					<ul>
						<li>
							<p>
								<line><m>s &lt; 0 \text{ (negative) and } b\to \infty \implies -sb \to \infty \implies e^{-sb} \to \infty</m></line>
							</p>
						</li>
						<li>
							<p>
								<line><m>s &gt; 0 \text{ (positive) and } b\to \infty \implies -sb \to -\infty \implies e^{-sb} \to 0</m></line>
							</p>
						</li>
					</ul>
					<!-- To visualize this, here is a <xref ref="compare-exp-graphs" text="custom">graph</xref> comparing <m>s=-1.2\ </m> versus <m>\, +1.2</m>. -->
				</p>
		
				<p>
					Therefore, when <m>s &gt; 0</m> the Laplace transform exists and evaluates to
					<me>\lap{1} = -\frac{1}{s} [0 - 1] = \frac{1}{s} \quad \text{for } s \gt 0.</me>
				</p>
			</solution>
		
		</example>

		<p>
			Now that we've worked through an example, here are a few key takeaways:
			<ul marker="square">
				<li>
				<p>
					The Laplace transform always results in a function of <m>s</m>. We typically denote the Laplace transform using the capitalized letter of the function we are transforming. For instance,
					<me> \lap{f(t)} = F(s) \quad \text{or} \quad \lap{q(t)} = Q(s).</me>
				</p>
				</li>
			
				<li>
				<p>
					The values of <m>s</m> for which the integral converges are crucial. While these values usually don't affect the solution to the differential equation, we will make a habit of noting them as we build our Laplace transform toolbox.
				</p>
				</li>
			
				<li>
				<p>
					The notation <m>\lap{}</m> includes curly braces to indicate the function being transformed.
				</p>
				</li>
			</ul>
		</p>
		
		<p>
			With this, we've introduced our first Laplace transform. In the next few sections, we will explore more of the common transforms that are used to solve differential equations.
		</p>

		<assemblage xml:id="lt-table-L1"><title>Common Laplace Transform <m>L_1</m></title>
			<p>
				<dl width="narrow">
					<li xml:id="L1"><title><m>{\LARGE \vphantom{\int}}L_1</m></title>
						<m>\ds \lap{ 1 } = \frac{1}{s}, \quad s &gt; 0 </m>
					</li>
				</dl>
			</p>
		</assemblage>

		<xi:include href="./p4-c1-s2-1-interactives.ptx" />
	</subsection>

	<subsection><title> Exponential Function, <m>e^{at}</m> </title>
		
		<p>
			The exponential function <m>e^{at}</m> is one of the most important functions in mathematics, especially in the context of differential equations. Let's explore how this works with a specific example. 
		</p>

		<example>

			<m>\ \ </m> Compute <m> \lap{ e^{7t}} </m>.
	
			<solution><title> Solution </title>
				<p>
					We begin by applying the definition of the Laplace transform:
					<md>
						<mrow> 
							\lap{ e^{7t} } 
							=\amp\ \int_0^{\infty} e^{-st} \cdot e^{7t}\ dt
						</mrow>
						<mrow> 
							=\amp\ \lim_{b \to \infty}\int_0^b e^{(-s+7)t}\ dt
						</mrow>
					</md>
					For this improper integral to converge, the exponent <m>-s+7</m> must be negative, meaning:
					<me> 
						-s+7 \lt 0 \hspace{0.5cm}\Rightarrow \hspace{0.5cm} -s \lt -7 \hspace{0.5cm}\Rightarrow \hspace{0.5cm} s \gt 7
					</me>.
					Thus, we proceed under the assumption that <m>s \gt 7</m>.
					<md>
						<mrow> 
							\lap{ e^{7t} } 
								=\amp\ \lim_{b \to \infty}\int_0^b e^{(-s+7)t}\, dt
						</mrow>
						<mrow> 
								=\amp\ \lim_{b \to \infty} \frac{1}{7-s} e^{(-s+7)t} \Bigg|_0^b
						</mrow>
						<mrow> 
								=\amp\ \frac{1}{-s+7} \left[ \lim_{b \to \infty} \left( e^{(-s+7)b} - e^{0} \right) \right]
						</mrow>
						<mrow> 
								=\amp\ \frac{1}{-s+7} \left[ \lim_{b \to \infty} e^{(-s+7)b} - 1 \right]
						</mrow>
						<mrow>
								=\amp\ \frac{1}{-s+7} \left[ 0 - 1 \right] \qquad \Big(e^{(\text{negative})b} \to 0\Big)
						</mrow>
						<mrow>
								=\amp\ -\frac{1}{-s+7} = \frac{1}{s-7}. \quad \text{for } s \gt 7
						</mrow>
					</md>
					Thus, the Laplace transform of <m>e^{7t}</m> is:
					<me>\ds \lap{e^{7t}} = \frac{1}{s - 7}, \quad s \gt 7.</me>
				</p>
			</solution>
	
		</example>
	
		<p>
			This result can be generalized for any constant <m>a</m>, giving us the Laplace transform of <m>e^{at}</m>. <xref ref="laplace-transform-of-exponential" text="custom">Here are the details.</xref>
		</p>
	
		<assemblage xml:id="lt-table-L2"><title>Common Laplace Transform (Exponential)</title>
			<p>
				<dl width="narrow">
					<li xml:id="L2"><title><m>L_2</m></title>
						<m>\ds \lap{ e^{at} } = \frac{1}{s - a}, \quad s \gt a, \quad <xref ref="laplace-transform-of-exponential" text="custom">\text{details}</xref></m>
					</li>
				</dl>
			</p>
		</assemblage>
	
		<xi:include href="./p4-c1-s2-2-interactives.ptx" />
	</subsection>

	<subsection><title> Power Function, <m>t^{n}</m> </title>
		<p>
			The power function <m>t^n</m> is another common function type found in differential equations. The Laplace transform of <m>t^n</m> follows a recursive pattern, which simplifies the computation for higher powers. We've already seen that <m>\ds\lap{1} = \sfrac{1}{s}</m>. Now, let's compute the transforms for <m>t</m> and <m>t^2</m>.
		</p>

		<example>

			<p>
				The Laplace transforms for <m>t</m> and <m>t^2</m> are as follows:
				<ul marker="square">
					<li>	
						<m> \ds \lap{t} 	= \frac{1}{s^2}, \quad s \gt 0 \quad </m> <xref ref="laplace-transform-of-t-power-1" text="custom">Details</xref>
					</li>
					<li>	
						<m> \ds \lap{t^2} = \frac{2}{s^3}, \quad s \gt 0 \quad </m> <xref ref="laplace-transform-of-t-power-2" text="custom">Details</xref>
					</li>
				</ul>
			</p>
		</example>

		<p>
			If you look in each solution, before computing <m>L = 0</m>, you'll notice a relationship between the Laplace transforms of powers that differ by one. Namely,
			<me>
				\lap{t} = \frac{1}{s}\lap{1} \quad \text{and} \quad \lap{t^2} = \frac{2}{s}\lap{t}
			</me>,
			and if you compute the Laplace transform of <m>t^3</m>, you'll find that
			<me>
				\lap{t^3} = \frac{3}{s}\lap{t^2}
			</me>.
			In general, this recursive pattern continues for any power <m>n</m> as
			<me>
				\lap{t^n} = \frac{n}{s}\lap{t^{n-1}}
			</me>.
			So if we wanted the Laplace transform of <m>t^4</m>, we could find it like so
			<md>
				<mrow> 
					\lap{t^4}
						=\amp\ \frac{4}{s}\lap{t^3}
				</mrow>
				<mrow> 				
						=\amp\ \frac{4}{s}\left[\frac{3}{s}\lap{t^2}\right] 
						= \frac{4\cdot 3}{s^2}\left[\frac{2}{s}\lap{t}\right] 
						= \frac{4\cdot 3\cdot 2}{s^3}\cdot\frac{1}{s^2} 
						= \ob{\frac{4\cdot 3\cdot 2\cdot 1}{s^5}}^{\text{factorial}}
				</mrow>
			</md>.
			This pattern is true for higher powers of <m>t</m>, leading to the next laplace transform rule which makes use of the <xref ref="factorial" text="title"/>.
		</p>

		<assemblage xml:id="lt-table-L3"><title>Common Laplace Transform (Power)</title>
			<p>
				<dl width="narrow">
					<li xml:id="L3"><title><m>{\LARGE \vphantom{\int}}L_3</m></title>
						<m>\ds \lap{ t^n } = \frac{n!}{s^{n+1}}, \quad s >0, \quad n = 1, 2, 3, \ldots </m>
					</li>
				</dl>
			</p>
		</assemblage>
	
		<xi:include href="./p4-c1-s2-3-interactives.ptx" />
	</subsection>

	<subsection><title> Sine and Cosine, <m>\sin(bt),\ \cos(bt)</m> </title>
		<p>
			Now, let's turn to the Laplace transforms of trigonometric functions, which frequently arise in systems involving oscillations or wave equations.
		</p>

		<example>
	
			<m>\ \ </m>Compute <m>\lap{\cos(3t)}</m>.
			
			<solution><title> Solution </title>
				<p>
					We start by applying the definition of the Laplace transform:
					<me>
						\lap{ \cos(3t)} = \int_0^{\infty} e^{-st} \cdot \cos(3t)\ dt 
					</me>.
					Rather than directly integrating, we will use a modified <xref ref="eulers-formula" text="title"></xref> to express cosine in terms of <m>e</m>
					<me>
						\cos(3t) = \frac12\left(e^{3it} + e^{-3it}\right).
					</me>
					Substituting this into the integral gives:
					<md>
						<mrow> 
							\lap{ \cos(3t)} 
							=\amp\ \frac12 \int_0^{\infty} e^{-st} \frac12\left(e^{3it} + e^{-3it}\right)\ dt 
						</mrow>
						<mrow>
							=\amp\ \frac12\left[\int_0^{\infty} e^{-st}\cdot e^{3it}\ dt + \int_0^{\infty} e^{-st}\cdot e^{-3it}\ dt\right]
						</mrow>
						<mrow>
							=\amp\ \frac{1}{2} \left[\lap{e^{3it}} + \lap{e^{-3it}}\right]
						</mrow>
						<mrow>
							=\amp\ \frac{1}{2} \left[\frac{1}{s - 3i} + \frac{1}{s + 3i}\right] \qquad (\text{by } <xref ref="L2" text="title"/>)
						</mrow>
						<mrow>
							=\amp\ \frac{1}{2} \left[\frac{s + 3i + s - 3i}{(s - 3i)(s + 3i)}\right]
						</mrow>
						<mrow>
							=\amp\ \frac{s}{s^2 + 9}.
						</mrow>
					</md>
					Therefore, the Laplace transform of <m>\cos(3t)</m> is:
					<me>
						\lap{\cos(3t)} = \frac{s}{s^2 + 9}.
					</me>
				</p>
			</solution>
		</example>

		<p>
			The sine function is handled in a similar way, as the next example shows.
		</p>

		<example>

			<m>\ \ </m>Compute <m>\lap{\sin(-4t)}</m>.
		
			<solution><title> Solution </title>
				<p>
					As with cosine, we begin with the definition of the Laplace transform,
					<me>
						\lap{ \sin(-4t)} = \int_0^{\infty} e^{-st} \cdot \sin(-4t)\ dt
					</me>
					and rewrite sine using Euler's formula,
					<me>
						\sin(-4t) = \frac{e^{-4it} - e^{4it}}{2i}.
					</me>
					Substituting this into the integral, we get:
					<md>
						<mrow> 
							\lap{ \sin(-4t)} 
							=\amp \frac{1}{2i} \int_0^{\infty} e^{-st} \left(e^{-4it} - e^{4it}\right)\, dt 
						</mrow>
						<mrow>
							=\amp \frac{1}{2i} \left[\int_0^{\infty} e^{-(s + 4i)t}\, dt - \int_0^{\infty} e^{-(s - 4i)t}\, dt\right]
						</mrow>
						<mrow>
							=\amp \frac{1}{2i} \left[\lap{e^{-4it}} - \lap{e^{4it}}\right].
						</mrow>
						<mrow>
							=\amp \frac{1}{2i} \left[\frac{1}{s + 4i} - \frac{1}{s - 4i}\right] \qquad (\text{by } <xref ref="L2" text="title"/>)
						</mrow>
						<mrow>
							=\amp \frac{1}{2i} \left[\frac{s - 4i - (s + 4i)}{(s + 4i)(s - 4i)}\right]
						</mrow>
						<mrow>
							=\amp \frac{4}{s^2 + 16}.
						</mrow>
					</md>
					Thus, the Laplace transform of <m>\sin(-4t)</m> is:
					<me>
						\lap{\sin(-4t)} = \frac{4}{s^2 + 16}.
					</me>
				</p>
			</solution>
		</example>

		<p>
			Both of these approaches can be generalized to show that the formula for the Laplace transforms of sine and cosine are given as follows:
		</p>

		<assemblage xml:id="lt-table-L4-L5"><title>Common Laplace Transform (Sine, Cosine)</title>
			<p>
				<dl width="narrow">
					<li xml:id="L4"><title><m>{\LARGE \vphantom{\int}}L_4</m></title>
						<m>\ds \lap{\sin(bt)} = \frac{b}{s^2+b^2}, \quad s \gt 0 </m>
					</li>
					<li xml:id="L5"><title><m>{\LARGE \vphantom{\int}}L_5</m></title>
						<m>\ds \lap{\cos(bt)} = \frac{s}{s^2+b^2}, \quad s \gt 0 </m>
					</li>
				</dl>
			</p>
		</assemblage>
	
		<xi:include href="./p4-c1-s2-4-interactives.ptx" />
	</subsection>

</section>