
<subsection xmlns:xi="http://www.w3.org/2001/XInclude"><title> Summary &amp; Exercises </title>

	<introduction>
		
		<p>
			<assemblage color="green"><title>Summary of the Key Ideas</title>
				<p>
					<term> <em> Method</em> </term>
					<p>
						
					</p>
				</p>
			</assemblage>
		</p>
		
	</introduction>

	<exercises>

		<exercisegroup cols="2"><title>Match the Sine Form</title>
		
			<introduction>
				<p>
					Rewrite each of the following into the form 
					<me>A \cdot \frac{b}{s^2 + b^2}</me>,
					by filling in the appropriate values in the boxes.
				</p>
			</introduction>
		
			<exercise> 
				
				<statement>
					<p>
						<m>\ds \frac{1}{s^2 + 49} = \fbox{\(\phantom{ \left|\frac{1}{7}\right|}\)} \cdot \frac{\fbox{\(\phantom{ |7| }\)}}{s^2 + \fbox{\(\phantom{ |7| }\)}^2}</m>
					</p>
				</statement>
				<answer>		
					<me>	
						\frac{1}{s^2 + 49} = \frac{1}{s^2 + 7^2} = \fbox{\(\frac{1}{7}\)} \cdot \frac{\fbox{\(7\)}}{s^2 + \fbox{\(7\)}^2}
					</me>
				</answer>

			</exercise>

			<exercise>
				<statement>
					<p>
						<m>\ds \frac{12}{s^2 + 16} = \fbox{\(\phantom{ \left|\frac{1}{4}\right|}\)} \cdot \frac{\fbox{\(\phantom{ |4| }\)}}{s^2 + \fbox{\(\phantom{ |4| }\)}^2}</m>
					</p>
				</statement>
				<answer>
					<me>
						\frac{12}{s^2 + 16} = 3 \cdot \frac{4}{s^2 + 4^2} = \fbox{\(3\)} \cdot \frac{\fbox{\(4\)}}{s^2 + \fbox{\(4\)}^2}
					</me>
				</answer>
			</exercise>

			<exercise>
				<statement>
					<p>
						<m>\ds \frac{3}{s^2 + 5} = \fbox{\(\phantom{ \frac{3}{\sqrt{5}}}\)} \cdot \frac{\fbox{\(\phantom{ \sqrt{5} }\)}}{s^2 + \fbox{\(\phantom{ \sqrt{5} }\)}^2}</m>
					</p>
				</statement>
				<answer>
					<me>
						\frac{3}{s^2 + 5} = \frac{3}{\sqrt{5}} \cdot \frac{\sqrt{5}}{s^2 + (\sqrt{5})^2} = \fbox{\(\frac{3}{\sqrt{5}}\)} \cdot \frac{\fbox{\(\sqrt{5}\)}}{s^2 + \fbox{\(\sqrt{5}\)}^2}
					</me>
				</answer>
			</exercise>

		</exercisegroup>

		<exercisegroup cols="2"><title>Match the Cosine Form</title>
		
			<introduction>
				<p>
					Rewrite each of the following into the form 
					<me>A \cdot \frac{s}{s^2 + b^2}</me>,
					by filling in the appropriate values in the boxes.
				</p>
			</introduction>

			<exercise>
				<statement>
					<p>
						<m>\ds \frac{4s}{s^2 + 9} = \fbox{\(\phantom{ \left|\frac{1}{3}\right|}\)} \cdot \frac{s}{s^2 + \fbox{\(\phantom{ |3| }\)}^2}</m>
					</p>
				</statement>
				<answer>
					<me>
						\frac{4s}{s^2 + 9} = 4 \cdot \frac{s}{s^2 + 3^2} = \fbox{\(4\)} \cdot \frac{s}{s^2 + \fbox{\(3\)}^2}
					</me>
				</answer>
			</exercise>

			<exercise>
				<statement>
					<p>
						<m>\ds \frac{s}{2s^2 + 8} = \fbox{\(\phantom{ \left|\frac{1}{2}\right|}\)} \cdot \frac{s}{s^2 + \fbox{\(\phantom{ |2| }\)}^2}</m>
					</p>
				</statement>
				<answer>
					<me>
						\frac{s}{2s^2 + 8} = \frac{1}{2} \cdot \frac{s}{s^2 + 2^2} = \fbox{\(\frac{1}{2}\)} \cdot \frac{s}{s^2 + \fbox{\(2\)}^2}
					</me>
				</answer>

			</exercise>

		</exercisegroup>

		<exercisegroup cols="2"><title>Match the Power Form</title>
		
			<introduction>
				<p>
					Rewrite each of the following into the form 
					<me>A \cdot \frac{n!}{s^{n+1}}</me>,
					by filling in the appropriate values in the boxes.
				</p>
			</introduction>

			<exercise>
				<statement>
					<p>
						<m>\ds \frac{1}{s^5} = \fbox{\(\phantom{ \frac{1}{24} }\)} \cdot \frac{\fbox{\(\phantom{ |4| }\)}\ {\large !}}{s\vphantom{S|}^{\fbox{\(\phantom{ 4\ }\)} + 1}}</m>
					</p>
				</statement>
				<answer>
					<me>
						\frac{1}{s^5} = \frac{1}{24} \cdot \frac{4!}{s^{4+1}} = \fbox{\(\frac{1}{24}\)} \cdot \frac{\fbox{\(4\)}!}{s^{\fbox{\(4\)}+1}}
					</me>
				</answer>
			</exercise>

			<exercise>
				<statement>
					<p>
						<m>\ds \frac{7}{s^3} = \fbox{\(\phantom{ \left|\frac{7}{2}\right| }\)} \cdot \frac{\fbox{\(\phantom{ |2| }\)}\ {\large !}}{s\vphantom{S|}^{\fbox{\(\phantom{ 2\ }\)} + 1}}</m>
					</p>
				</statement>
				<answer>
					<me>
						\frac{7}{s^3} = \frac{7}{2} \cdot \frac{2!}{s^{2+1}} = \fbox{\(\frac{7}{2}\)} \cdot \frac{\fbox{\(2\)}!}{s^{\fbox{\(2\)}+1}}
					</me>
				</answer>
			</exercise>

			<exercise>
				<statement>
					<p>
						<m>\ds \frac{2}{5s^4} = \fbox{\(\phantom{ \frac{1}{15} }\)} \cdot \frac{\fbox{\(\phantom{ |3| }\)}\ {\large !}}{s\vphantom{S|}^{\fbox{\(\phantom{ 3\ }\)} + 1}}</m>
					</p>
				</statement>
				<answer>
					<me>
						\frac{2}{5s^4} = \frac{1}{15} \cdot \frac{3!}{s^{3+1}} = \fbox{\(\frac{1}{15}\)} \cdot \frac{\fbox{\(3\)}!}{s^{\fbox{\(3\)}+1}}
					</me>
				</answer>
			</exercise>

		</exercisegroup>

		<exercisegroup><title>Backward Transforms- Level 1</title>

			<exercise> <!--== Problem 1 ==-->
				<statement>
					<m> \ds F(s) = \frac{6}{(s-1)^4} </m>
				</statement>
				<solution>
					<m> \ds F(s) = \frac{6}{(s-1)^4} </m>
				</solution>
				<answer>
					
				</answer>
			</exercise>
		
			<exercise> <!--== Problem 2 ==-->
				<statement>
					<m> \ds X(s) = \frac{1}{s^5} </m>
				</statement>
				<solution>
					<m> \ds X(s) = \frac{1}{s^5} </m>
				</solution>
				<answer>
					
				</answer>
			</exercise>
		
			<exercise> <!--== Problem 3 ==-->
				<statement>
					<m> \ds G(s) = \frac{4}{s^2 + 9} </m>
				</statement>
				<solution>
					<m> \ds G(s) = \frac{4}{s^2 + 9} </m>
				</solution>
				<answer>
					
				</answer>
			</exercise>
		
			<exercise> <!--== Problem 4 ==-->
				<statement>
					<m> \ds Y(s) = \frac{5s}{s^2 + 7} </m>
				</statement>
				<solution>
					<m> \ds Y(s) = \frac{5s}{s^2 + 7} </m>
				</solution>
				<answer>
					
				</answer>
			</exercise>
		
			<exercise> <!--== Problem 5 ==-->
				<statement>
					<m> \ds X(s) = \frac{21}{(s+2)^2 + 16} </m>
				</statement>
				<solution>
					<m> \ds X(s) = \frac{21}{(s+2)^2 + 16} </m>
				</solution>
				<answer>
					
				</answer>
			</exercise>
		
			<exercise> <!--== Problem 6 ==-->
				<statement>
					<m> \ds F(s) = \frac{10}{s-10} </m>
				</statement>
				<solution>
					<m> \ds F(s) = \frac{10}{s-10} </m>
				</solution>
				<answer>
					
				</answer>
			</exercise>
		
			<exercise> <!--== Problem 7 ==-->
				<statement>
					<m> \ds Q(s) = \frac{7s+7}{(s+1)^2 + 12} </m>
				</statement>
				<solution>
					<m> \ds Q(s) = \frac{7s+7}{(s+1)^2 + 12} </m>
				</solution>
				<answer>
					
				</answer>
			</exercise>
		
		</exercisegroup>
		
		<exercisegroup><title>Backward Transforms- Level 2</title>

			<exercise> <!--== Problem 8 ==-->
				<statement>
					<m> \ds G(s) = \frac{1}{s^2 + 4s + 8} </m>
				</statement>
				<solution>
					<m> \ds G(s) = \frac{1}{s^2 + 4s + 8} </m>
				</solution>
				<answer>
					
				</answer>
			</exercise>
		
			<exercise> <!--== Problem 9 ==-->
				<statement>
					<m> \ds F(s) = \frac{2s+16}{s^2 + 4s + 13} </m>
				</statement>
				<solution>
					<m> \ds F(s) = \frac{2s+16}{s^2 + 4s + 13} </m>
				</solution>
				<answer>
					
				</answer>
			</exercise>
		
			<exercise> <!--== Problem 10 ==-->
				<statement>
					<m> \ds Y(s) = \frac{3s-15}{2s^2 - 4s + 8} </m>
				</statement>
				<solution>
					<m> \ds Y(s) = \frac{3s-15}{2s^2 - 4s + 8} </m>
				</solution>
				<answer>
					
				</answer>
			</exercise>
		
			<exercise> <!--== Problem 11 ==-->
				<statement>
					<m> \ds Q(s) = \frac{1}{s^2 + 6s + 9} </m>
				</statement>
				<solution>
					<m> \ds Q(s) = \frac{1}{s^2 + 6s + 9} </m>
				</solution>
				<answer>
					
				</answer>
			</exercise>
		
			<exercise> <!--== Problem 12 ==-->
				<statement>
					<m> \ds H(s) = \frac{5}{s-6} - \frac{6s}{s^2 + 9} + \frac{3}{2s^2 + 8s + 10} </m>
				</statement>
				<solution>
					<m> \ds H(s) = \frac{5}{s-6} - \frac{6s}{s^2 + 9} + \frac{3}{2s^2 + 8s + 10} </m>
				</solution>
				<answer>
					
				</answer>
			</exercise>
		
			<exercise> <!--== Problem 13 ==-->
				<statement>
					<m> \ds X(s) = \frac{7s-4}{s^2 + 36} </m>
				</statement>
				<solution>
					<m> \ds X(s) = \frac{7s-4}{s^2 + 36} </m>
				</solution>
				<answer>
					
				</answer>
			</exercise>
		
			<exercise> <!--== Problem 14 ==-->
				<statement>
					<m> \ds G(s) = \frac{2s-19}{s^2 - 4s+13} + \frac{5}{s-1} </m>
				</statement>
				<solution>
					<m> \ds G(s) = \frac{2s-19}{s^2 - 4s+13} + \frac{5}{s-1} </m>
				</solution>
				<answer>
					
				</answer>
			</exercise>
		
			<exercise> <!--== Problem 15 ==-->
				<statement>
					<m> \ds F(s) = \frac{s}{s^2 + 6s + 11} </m> 
				</statement>
				<solution>
					<m> \ds F(s) = \frac{s}{s^2 + 6s + 11} </m> 
				</solution>
				<answer>
					
				</answer>
			</exercise>
		
		</exercisegroup>
		
		<exercisegroup><title>Backward Transforms- Level 3</title>
		
			<exercise> <!--== Problem 16 ==-->
				<statement>
					<m> \ds X(s) = \frac{90s^2 - 195s + 30}{s^3 - 7s^2 + 6s} </m>
				</statement>
				<solution>
					<m> \ds X(s) = \frac{90s^2 - 195s + 30}{s^3 - 7s^2 + 6s} </m>
				</solution>
				<answer>
					
				</answer>
			</exercise>
		
			<exercise> <!--== Problem 17 ==-->
				<statement>
					<m> \ds I(s) = \frac{5s^2 + 34s + 53}{(s+3)^2(s+1)} </m>
				</statement>
				<solution>
					<m> \ds I(s) = \frac{5s^2 + 34s + 53}{(s+3)^2(s+1)} </m>
				</solution>
				<answer>
					
				</answer>
			</exercise>
		
			<exercise> <!--== Problem 18 ==-->
				<statement>
					<m> \ds F(s) = \frac{7s^3 - 2s^2 - 3s + 6}{s^3(s-2)} </m> 
				</statement>
				<solution>
					<m> \ds F(s) = \frac{7s^3 - 2s^2 - 3s + 6}{s^3(s-2)} </m> 
				</solution>
				<answer>
					
				</answer>
			</exercise>
		
		</exercisegroup>
		
		<exercisegroup><title>Steps 3 &amp; 4</title>

			<exercise> <!--== Problem 19 ==-->
				<statement>
					<m> \ds s^2 F(s) - 4F(s) = \frac{60}{s+1} </m>
				</statement>
				<solution>
					<m> \ds s^2 F(s) - 4F(s) = \frac{60}{s+1} </m>
				</solution>
				<answer>
					
				</answer>
			</exercise>
		
			<exercise> <!--== Problem 20 ==-->
				<statement>
					<m> \ds \ds s^2 F(s) + sF(s) - 6F(s) = \frac{30s^2 + 120}{s^2 + s} </m>
				</statement>
				<solution>
					<m> \ds \ds s^2 F(s) + sF(s) - 6F(s) = \frac{30s^2 + 120}{s^2 + s} </m>
				</solution>
				<answer>
					
				</answer>
			</exercise>
		
		</exercisegroup>

		<exercisegroup><title>Inverse Laplace Transforms</title>
	
			<introduction>
				<p>
					Determine the original time-domain functions from the given Laplace-transformed functions.
				</p>
			</introduction>
	
			<exercise>
				<statement>
					<m>\ds Y(s) = \frac{2s + 7}{(s + 1)(s + 3)}</m>
				</statement>
				<solution>
					Decompose into partial fractions:
					<me>Y(s) = \frac{A}{s + 1} + \frac{B}{s + 3}</me>.
					Find <m>A</m> and <m>B</m>:
					<me>A = 1, B = \frac{1}{2}</me>.
					Use the inverse Laplace transform:
					<me>y(t) = e^{-t} + \frac{1}{2}e^{-3t}</me>.
				</solution>
				<answer>
					<m>\ds y(t) = e^{-t} + \frac{1}{2}e^{-3t}</m>
				</answer>
			</exercise>
	
			<exercise>
				<statement>
					<m>\ds F(s) = \frac{5}{s(s + 4)}</m>
				</statement>
				<solution>
					Decompose into partial fractions:
					<me>F(s) = \frac{A}{s} + \frac{B}{s + 4}</me>.
					Find <m>A</m> and <m>B</m>:
					<me>A = \frac{5}{4}, B = -\frac{5}{4}</me>.
					Use the inverse Laplace transform:
					<me>f(t) = \frac{5}{4}(1 - e^{-4t})</me>.
				</solution>
				<answer>
					<m>\ds f(t) = \frac{5}{4}(1 - e^{-4t})</m>
				</answer>
			</exercise>
	
		</exercisegroup>

	</exercises>

</subsection>