<exercises><title> Additional Exercises </title>

	<subsubsection><title> What's a Differential Equation </title>
		
	</subsubsection>

	<subsubsection><title> Variables, Terms, and Coefficients </title>
		
	</subsubsection>

	<subsubsection><title> Order &amp; Linearity </title>
		
	</subsubsection>

	<subsubsection><title> Solutions &amp; Initial Conditions </title>

		<p>
			<exercise>

				<statement>
					<p>
						To verify that the function <m>y = -3e^{x^2} + 3</m> is a particular solution to the initial-value problem
						<me>
							\frac{dy}{dx} = 2xy - 6x, \qquad y(0) = 0
						</me>,
						what two things must you show? Show them.
					</p>
				</statement>
				
				<solution>
					<p>
						To verify that the function <m>y = -3e^{x^2} + 3</m> is a particular solution to the initial-value problem
						<me>
							\frac{dy}{dx} = 2xy - 6x, \qquad y(0) = 0
						</me>,
						we must show the following two things:
					</p>

					<ul>
						<li>
							<p>
								<m>y = -3e^{x^2} + 3</m> satisfies the differential equation <m>\frac{dy}{dx} = 2xy - 6x</m>.
							</p>
						</li>
						<li>
							<p>
								<m>y = -3e^{x^2} + 3</m> satisfies the initial condition <m>y(0) = 0</m>.
							</p>
						</li>
					</ul>

					<p>
						Let's start by showing that the function <m>y = -3e^{x^2} + 3</m> satisfies the differential equation.
					</p>

					<p>
						<md>
							<mrow>							\frac{dy}{dx}	=\amp\ 2xy - 6x					</mrow>
							<mrow>	\frac{d}{dx}\left[-3e^{x^2} + 3\right]	=\amp\ 2x(-3e^{x^2} + 3) - 6x	</mrow>
							<mrow>	-3\frac{d}{dx}\left[e^{x^2}\right]+ 0	=\amp\ -6xe^{x^2} + 6x - 6x		</mrow>
							<mrow>			-3\left(e^{x^2} \cdot 2x\right)	=\amp\ -6xe^{x^2}				</mrow>
							<mrow>								-6xe^{x^2}	=\amp\ -6xe^{x^2}\quad✅		  </mrow>
						</md>
					</p>
					
					<p>
						Now, let's show that the function satisfies the initial condition <m>y(0) = 0</m>.
					</p>

					<p>
						<md>
							<mrow>	y(0)	=\amp\ -3e^{0^2} + 3	</mrow>
							<mrow>		0	=\amp\ -3e^0 + 3		</mrow>
							<mrow>		0	=\amp\ -3 + 3			</mrow>
							<mrow>		0	=\amp\ 0\quad✅		  </mrow>
						</md>
					</p>

				</solution>

			</exercise>
		</p>

	</subsubsection>

</exercises>