<section xmlns:xi="http://www.w3.org/2001/XInclude"><title> Verifying Solutions </title>

	<introduction>

		<p>
			It is worth pointing out that the following differential equations are identical:
			<me>
				y^\prime = 3y \quad \text{and} \quad y^\prime - 3y = 0
			</me>.
			This means that the solutions to both equations are the same and you are free to use either form when verifying solutions. For a beginner, it is often easier to verify solutions using the second form, as it is easier to see if the left-side of the equation simplifies to zero.
		</p>

		<assemblage xml:id="move-terms-when-verifying"><title> <em>TIP: Move Terms to the Left-Side before Verifying</em> </title>
			<p>
				Before verifying solutions, move all terms to the left-side of the equation using subtraction. This makes the right-side zero, simplifying the process.
			</p>
		</assemblage>

	</introduction>

	<p>
		<assemblage color="green" xml:id="solution-verification-steps"><title>Solution Verification Steps</title>
			<p>
				Verifying if a function is a solution to a differential equation involves checking if the function satisfies the equation, outlined as follows:
				<dl width="narrow">
					<li xml:id="solution-verification-step-1"><title>Move Terms</title>
						<p> 
							<xref ref="move-terms-when-verifying" text="custom">Move terms to the left-side of the equation</xref>.
						</p>
					</li>
					<li xml:id="solution-verification-step-2"><title>Compute Derivatives</title>
						<line> 
							Compute &amp; simplify derivatives appearing in the DE.
							<fn> This helps reduce errors by breaking the problem into more manageable steps. </fn>
						</line>
					</li>
					<li xml:id="solution-verification-step-3"><title>Plug-In &amp; Simplify</title>
						<p> 
							Substitute the function &amp; derivatives into the equation and simplify each side of the equation.
						</p>
					</li>
				</dl>
				If you end up with a true statement <m>\left(0 = 0\right)</m>, then the function is a solution.
			</p>
		</assemblage>
	</p>

	<p>
		Let's look at a few warm-up examples.
	</p>

	<example><title> <em>Solution Verification 1</em> </title>
		<p>
			Is <m>y= 2x^2</m> a solution to <m>\quad xy' - 2x^2 = y</m> ?
		</p>

		<solution>

			<p>
				Let's follow the steps outlined above.
			</p>

			<p>
				<xref ref="solution-verification-step-1" text="title"/>: <m>\quad xy' - 2x^2 - y = 0</m>
			</p>

			<p>
				<xref ref="solution-verification-step-2" text="title"/>: Find <m>y'</m> since it appears in the DE.
				<me>
					y	= 2x^2,	\quad	y' = 4x
				</me>
			</p>

			<p>
				<xref ref="solution-verification-step-3" text="title"/>: Plug <m>y</m> and <m>y'</m> into the DE and simplify.
				<md>
					<mrow> 									xy' - 2x^2 - y	\amp= 0									</mrow>
					<mrow> x\left(4x\right) - 2x^2 - \left( 2x^2 \right)	\amp= 0 								</mrow>
					<mrow> 								4x^2 - 2x^2 - 2x^2	\amp= 0									</mrow>
					<mrow> 												0	\amp= 0	\quad \leftarrow \text{true}	</mrow>
				</md>
				Therefore, <m>y= 2x^2</m> is a solution to <m>xy' - 2x^2 = y.</m>
			</p>

		</solution>

	</example>

	<example><title> <em>Solution Verification 2</em> </title>
		<p>
			Is <m>P = \sin t</m> a solution to <m>\quad 2P'' + P = \sin t</m> ?
		</p>

		<solution>

			<p>
				<xref ref="solution-verification-step-1" text="title"/>: <m>\quad 2P'' + P - \sin t = 0</m>
			</p>

			<p>
				<xref ref="solution-verification-step-2" text="title"/>. Find <m>P''</m> since it appears in the DE.
				<md>
					<mrow>	P	\amp= \sin t	</mrow>
					<mrow>	P'	\amp= \cos t	</mrow>
					<mrow>	P''	\amp= -\sin t	</mrow>
				</md>
			</p>

			<p>
				<xref ref="solution-verification-step-3" text="title"/>. Plug <m>P</m> and <m>P''</m> into the DE and simplify.
				<md>
					<mrow> 							2P'' + P - \sin t	\amp= 0									</mrow>
					<mrow> 2\left( -\sin t \right) + \sin t - \sin t	\amp= 0									</mrow>
					<mrow> -2\sin t + \cancel{\sin t} - \cancel{\sin t}	\amp= 0									</mrow>
					<mrow> 									-2\sin t	\amp= 0\quad \leftarrow \text{false}	</mrow>
				</md>
				Therefore, <m>P = \sin t</m> is <term> not a solution </term> to <m>2P'' + P = \sin t.</m>
			</p>

		</solution>

	</example>

	<example xml:id="de-two-solutions"><title> <em>Two Solutions for One DE</em> </title>
		<p>
			Verify that both <m>y= 2e^{-3t}</m> and <m>y= e^{4t}</m> are solutions to <m>\quad y'' - y' - 12y = 0</m> .
		</p>

		<solution><title><m>\quad y= 2e^{-3t}</m></title>
			<p>
				<xref ref="solution-verification-step-2" text="title"/>. Find <m>y'</m> and <m>y''</m> since they appear in the DE.
				<md>
					<mrow>	y	\amp=  2e^{-3t}									</mrow>
					<mrow>	y' 	\amp=  2e^{-3t}\left(-3\right)	=	-6e^{-3t}	</mrow>
					<mrow>	y'' \amp= -6e^{-3t}\left(-3\right)	=	18e^{-3t}	</mrow>
				</md>
			</p>

			<p>
				<xref ref="solution-verification-step-3" text="title"/>. Plug <m>y, y',</m> and <m>y''</m> into the DE and simplify.
				<md>
					<mrow> 													y'' - y' - 12y	\amp= 0									</mrow>
					<mrow> 18e^{-3t} - \left( -6e^{-3t} \right) - 12\left( 2e^{-3t} \right)	\amp= 0									</mrow>
					<mrow> 								18e^{-3t} + 6e^{-3t} - 24e^{-3t}	\amp= 0									</mrow>
					<mrow> 																0	\amp= 0	\quad \leftarrow \text{true}	</mrow>
				</md>
				Therefore, <m>y= 2e^{-3t}</m> is a solution to <m>y'' - y' - 12y = 0.</m>
			</p>

		</solution>

		<solution><title><m>\quad y= e^{4t}</m></title>
			<p>
				<xref ref="solution-verification-step-2" text="title"/>. Find <m>y'</m> and <m>y''</m> since they appear in the DE.
				<md>
					<mrow>	y	\amp=  e^{4t}							</mrow>
					<mrow>	y' 	\amp=  e^{4t}\left(4\right)	=	4e^{4t}	</mrow>
					<mrow>	y'' \amp= 4e^{4t}\left(4\right)	=	16e^{4t}</mrow>
				</md>
			</p>

			<p>
				<xref ref="solution-verification-step-3" text="title"/>. Plug <m>y, y',</m> and <m>y''</m> into the DE and simplify.
				<md>
					<mrow> 													y'' - y' - 12y	\amp= 0									</mrow>
					<mrow> 16e^{4t} - 4e^{4t} - 12\left( e^{4t} \right)	\amp= 0									</mrow>
					<mrow> 								16e^{4t} - 4e^{4t} - 12e^{4t}	\amp= 0									</mrow>
					<mrow> 																0	\amp= 0	\quad \leftarrow \text{true}	</mrow>
				</md>
				Therefore, <m>y= e^{4t}</m> is a solution to <m>y'' - y' - 12y = 0.</m>
			</p>

		</solution>

	</example>

	<example><title> <em>Solution Verification</em> </title>
		<p>
			Is <m>y= 3\sin(x^2)</m> a solution to the DE <m>\quad y' - xy'' = 12x^2\sin(x^2)</m>?
		</p>

		<solution>

			<p>
				<xref ref="solution-verification-step-1" text="title"/>: <m>\quad y' - xy'' - 12x^2\sin(x^2) = 0</m>
			</p>

			<p>
				<xref ref="solution-verification-step-2" text="title"/>. Find <m>y'</m> and <m>y''</m> since they appear in the DE.
				<md>
					<mrow>	y	\amp=  3\sin(x^2)									</mrow>
					<mrow>	y' 	\amp=  3\cos(x^2) \cdot 2x	=	6x\cos(x^2)	</mrow>
					<mrow>	y'' \amp= 6\cos(x^2) - 12x\sin(x^2)	=	6\cos(x^2) - 12x\sin(x^2)	</mrow>
				</md>
			</p>

			<p>
				<xref ref="solution-verification-step-3" text="title"/>. Plug <m>y, y',</m> and <m>y''</m> into the DE and simplify.
				<md>
					<mrow> 												y' - xy'' - 12x^2\sin(x^2) 	\amp= 0									</mrow>
					<mrow> 6x\cos(x^2) - x\left( 6\cos(x^2) - 12x\sin(x^2) \right) - 12x^2\sin(x^2)	\amp= 0									</mrow>
					<mrow> 				\cancel{6x\cos(x^2)} - \cancel{6x\cos(x^2)} - \cancel{12x^2\sin(x^2)} - \cancel{12x^2\sin(x^2)}	\amp= 0									</mrow>
					<mrow> 																		0	\amp= 0	</mrow>
				</md>
				Therefore, <m>y= 3\sin(x^2)</m> is a solution to <m>y' - 12x^2\sin(x^2) = xy''.</m>
			</p>

		</solution>

	</example>

	<xi:include href="./c1-s2-ss1-interactives.ptx" />

</section>