<section xmlns:xi="http://www.w3.org/2001/XInclude"><title> Method of Undetermined Coefficients </title>

	<p>
		When solving a non-homogeneous linear differential equation, selecting the correct form for the particular solution, <m>y_p</m>, is just the beginning. The next step is determining the values of its unknown coefficients, such as <m>A</m> and <m>B</m>. In this section, we'll explore how to compute these coefficients by substituting the guessed particular solution into the original equation.
	</p>

	<p>
		Let's revisit the example we discussed earlier. Consider the differential equation:
		<men xml:id="finding-yps-coefficients-de">
			y'' - 4y' + 3y = 9x
		</men>.
		We guessed that the particular solution would be linear, so we set
		<me>
			y_p = Ax + B
		</me>.
	</p>

	<p>
		Our goal now is to determine the values of <m>A</m> and <m>B</m>. To do this, we substitute <m>y_p = Ax + B</m> into the original differential equation. Here's how it works:
		<md>
			<mrow> y_p = Ax + B \quad \implies \quad y_p' = A \quad \implies \quad y_p'' = 0 </mrow>
		</md>
		Substituting <m>y_p</m>, <m>y_p'</m>, and <m>y_p''</m> into <xref ref="finding-yps-coefficients-de"/> results in:
		<md>
			<mrow> 0 - 4A + 3(Ax + B) =\amp\ 9x </mrow>
			<mrow> -4A + 3Ax + 3B =\amp\ 9x </mrow>
		</md>
		By matching the coefficients of like terms on opposite sides of the equation, 
		<image width="50%">
			<latex-image>
			
				\begin{tikzpicture}[join=round,rounded corners,&gt;=stealth,shorten &gt;=1pt,shorten &lt;=1pt,thick]
					\node (text1) 	at (1.4,0.5) 	{\scriptsize equal};
					\node (text2) 	at (3.4,0.7) 	{\scriptsize equal};
					
					\def\LA{0.1}
					\def\WA{0.64}
					\def\LB{1.27}
					\def\WB{1.65}
					\def\LC{3.33}
					\def\WC{0.3}
					\def\LD{4.2}
					\def\WD{0.28}

					\node[anchor=west] (eqn)	at (0,0)	{$\,3A\ x + \,- 4A + 3B\, = \ 9\ x + 0\ .$};
					\node (xterm1) at (\LA+\WA/2,0.1) {};
					\node (xterm2) at (\LC+\WC/2,0.1) {};
					\node (cterm1) at (\LB+\WB/2,0.1) {};
					\node (cterm2) at (\LD+\WD/2,0.1) {};
					
					\filldraw[fill=red!20,fill opacity=0.2,thin,draw=red]
						(\LA,-0.2)--(\WA,-0.2)--(\WA,0.2)--(\LA,0.2)--cycle;
					\filldraw[fill=blue!20,fill opacity=0.2,thin,draw=blue]
						(\LB,-0.2)--(\LB+\WB,-0.2)--(\LB+\WB,0.2)--(\LB,0.2)--cycle;
					\filldraw[fill=red!20,fill opacity=0.2,thin,draw=red]
						(\LC,-0.2)--(\LC+\WC,-0.2)--(\LC+\WC,0.2)--(\LC,0.2)--cycle;
					\filldraw[fill=blue!20,fill opacity=0.2,thin,draw=blue]
						(\LD,-0.2)--(\LD+\WD,-0.2)--(\LD+\WD,0.2)--(\LD,0.2)--cycle;
					
					\draw[-&gt;,thin] (text1.west)		--	+(-0.06,0.0) -| (xterm1);
					\draw[-&gt;,thin] (text1.east)		--	+(0.06,0.0) -| (xterm2);
					\draw[-&gt;,thin] (text2.west)		--	+(-0.06,0.0) -| (cterm1);
					\draw[-&gt;,thin] (text2.east)		--	+(0.06,0.0) -| (cterm2);
					
				\end{tikzpicture}
			</latex-image>
		</image>
		we solve:
		<md>
			<mrow>	3A		=\amp\ 9 \quad \implies \quad A = 3</mrow>
			<mrow> -4A + 3B	=\amp\ 0 \quad \implies \quad B = 4</mrow>
		</md>
		Thus, the particular solution is:
		<me>
			y_p = 3x + 4
		</me>.
	</p>

	<p>
		Regardless of <m>y_p</m>'s form, the process of finding the coefficients remains consistent:
		<ul marker="square">
			<li><p>Substitute the chosen <m>y_p</m> into the differential equation.</p></li>
			<li><p>Collect and match coefficients of like terms on both sides of the equation.</p></li>
			<li><p>Solve the resulting system to find <m>A, B, C, \ldots</m>.</p></li>
		</ul>
	</p>
	
	<p>
		This is why the method is called the "method of undetermined coefficients." and the complete process is summarized as follows.
	</p>

	<exploration xml:id="uc-method"><title> Undetermined Coefficients </title>
		<p>
			The linear nonhomogeneous equation with constant coefficients,
			<men xml:id="uc-method-lncc-de">
				a_n\ y^{(n)} + a_{n-1}\ y^{(n-1)} + \cdots + a_2\ y'' + a_1\ y' + a_0\ y = f(x),
			</men>
			has a general solution given by
			<men xml:id="uc-method-gen-soln">
				y = y_h + y_p,
			</men>
			where <m>y_h\ </m> is the solution to the homogeneous equation
			<men xml:id="uc-method-lhcc-de">
				a_n\ y^{(n)} + a_{n-1}\ y^{(n-1)} + \cdots + a_2\ y'' + a_1\ y' + a_0\ y = 0,
			</men>
			and <m>y_p</m> is the particular solution found through the following steps...
		</p>
		<dl width="narrow">
			<li xml:id="uc-step1"><title>Select Initial <m>y_p</m> </title>
				<p>
					Select the initial form of <m>y_p</m> that generalizes <m>f(x)</m>. 
				</p>
			</li>
			<li xml:id="uc-step2"><title>Adjust <m>y_p</m> </title>
				<p>
					If <m>y_p</m> shares terms with <m>y_h</m>, repeatedly multiply the terms by <m>x</m> until there are no terms in common.
				</p>
			</li>
			<li xml:id="uc-step3"><title>Find the Coefficients of <m>y_p</m> </title>
				<p>
					Plug <m>y_p</m> into <xref ref="uc-method-lncc-de"/> and match terms on each side to solve for the unknown coefficients of <m>y_p</m>.
				</p>
			</li>
		</dl>
	</exploration>

	<p>
		Now for a few examples to illustrate the complete application of the nndetermined coefficients method.
	</p>
	
	<example><title> <em>Find the general solution for each equation</em> </title>

		<solution><title> <m>y'' - 3y' + y = 2x^2 + 3x</m> </title>

			<p>
				Following the method of <xref ref="uc-method" text="title"/>, we first find <m>y_h</m> as
				<me> y_h = c_1 e^x + c_2 x e^x </me>.
				Next, we <xref ref="uc-step1" text="custom">select the initial form of <m>y_p</m></xref> as
				<md>
					<mrow> y_p = Ax^2 + Bx + C		</mrow>
				</md>
				and <xref ref="uc-step2" text="custom">adjust <m>y_p</m></xref>, if necessary. A quick check shows that <m>y_p</m> has no terms in common with <m>y_h</m>.
			</p>

			<p>
				Finally, we <xref ref="uc-step3" text="custom">find the coefficients of <m>y_p</m></xref>. To do this, let's compute <m>y_p'</m>, <m>y_p''</m>, plug these into the equation, and collect the <m>x^2</m>, <m>x</m>, and constant terms as follows:
				<me>y_p' = 2Ax + B \qquad y_p'' = 2A</me>
				<md>
					<mrow> 2A - 3(2Ax + B) + (Ax^2 + Bx + C) = 2x^2 + 3x </mrow>
					<mrow> 2A - 6Ax - 3B + Ax^2 + Bx + C = 2x^2 + 3x </mrow>
					<mrow> \us{1}{\ul{A}}x^2 + \us{2}{\ul{(- 6A + B)}}x + \us{3}{\ul{(2A - 3B + C)}} = \us{1}{\ul{2}}x^2 + \us{2}{\ul{3}}x + \us{3}{\ul{0}} </mrow>
				</md>.
				Matching the underlined coefficients leads to the following system of equations and solution for the coefficients <m>A</m>, <m>B</m>, and <m>C</m>:
				<sidebyside widths="15% 10% 30% 10% 10% 25%">
					<p/>
					<p>
						<md>
							<mrow>	\amp\ 1.	</mrow>
							<mrow>	\amp\ 2.	</mrow>
							<mrow>	\amp\ 3.	</mrow>
						</md>
					</p>
					<p>
						<md>
							<mrow> A			=\amp\ 2	</mrow>
							<mrow> -6A + B		=\amp\ 3	</mrow>
							<mrow> 2A - 3B + C	=\amp\ 0	</mrow>
						</md>
					</p>
					<p>
						<md>
							<mrow>				</mrow>
							<mrow>	\rightarrow	</mrow>
							<mrow>				</mrow>
						</md>
					</p>
					<p>
						<md>
							<mrow>	\amp\ A = 2  </mrow>
							<mrow>	\amp\ B = 9  </mrow>
							<mrow>	\amp\ C = 13 </mrow>
						</md>
					</p>
					<p/>
				</sidebyside>
				The general solution is then
				<me> y = y_h + y_p = c_1 e^x + c_2 x e^x + 2x^2 + 9x + 13 </me>.
			</p>
		</solution>

		<solution><title> <m>y'' + 3y' - 28y = 7t + e^{4t} - 1</m> </title>
			<p>
				Following the method of <xref ref="uc-method" text="title"/>, we find <m>y_h</m> as <m>\ds y_h = c_1 e^{4t} + c_2 e^{-7t} </m> and then find <m>y_p</m> through the steps that follow.
			</p>
			<p>
				<xref ref="uc-step1" text="title"/>. The initial form of <m>y_p</m> is
				<me> y_p = At + B + Ce^{4t}</me>,
			</p>
			<p>
				<xref ref="uc-step2" text="title"/>. Notice that <m>y_p</m> has an <m>e^{4t}</m> term, which overlaps with <m>y_h</m>. Therefore, we need to adjust <m>y_p</m> by multiplying the <m>e^{4t}</m> term by <m>t</m>,
				<me> y_p = At + B + Cte^{4t}</me>.
				Now that <m>y_p</m> and <m>y_h</m> are independent, we can proceed to find the coefficients <m>A</m>, <m>B</m>, and <m>C</m>. 
			</p>
			<p>
				<xref ref="uc-step3" text="title"/>. Before plugging in <m>y_p</m>, let's find <m>y_p'</m> and <m>y_p''</m>:
				<md>
					<mrow> y_p		=\amp\ At + B + Cte^{4t}		</mrow>
					<mrow> y_p'		=\amp\ A + Ce^{4t} + 4Cte^{4t}	</mrow>
					<mrow> y_p''	=\amp\ 8Ce^{4t} + 16Cte^{4t}	</mrow>
				</md>.
				Now, substituting these into the equation and collecting like terms, to get
				<md>
					<mrow> 
						8Ce^{4t} 
							+ 16 Cte^{4t} \amp\ + 3(A + Ce^{4t} + 4Cte^{4t}) 
					</mrow>
					<mrow> 
						\amp\ - 28(At + B + Cte^{4t}) = 7t + e^{4t} - 1
					</mrow>
					<mrow> 
						\us{1}{\ul{(11C)}}e^t + \us{2}{\ul{(-28A)}}\amp t + \us{3}{\ul{(3A-28B)}} = \us{1}{\ul{(1)}}e^{4t} + \us{2}{\ul{(7)}}t + \us{3}{\ul{(-1)}}
					</mrow>
				</md>,
				which leads to the following equations for <m>A</m>, <m>B</m>, and <m>C</m>:
				<sidebyside widths="15% 10% 30% 10% 10% 25%">
					<p/>
					<p>
						<md>
							<mrow>	\amp\ 1.	</mrow>
							<mrow>	\amp\ 2.	</mrow>
							<mrow>	\amp\ 3.	</mrow>
						</md>
					</p>
					<p>
						<md>
							<mrow> 11C		=\amp\ 1	</mrow>
							<mrow> -28A		=\amp\ 7	</mrow>
							<mrow> 3A - 28B	=\amp\ -1	</mrow>
						</md>
					</p>
					<p>
						<md>
							<mrow>				</mrow>
							<mrow>	\rightarrow	</mrow>
							<mrow>				</mrow>
						</md>
					</p>
					<p>
						<md>
							<mrow> \amp\ C = 1/11	</mrow>
							<mrow> \amp\ A = -1/4	</mrow>
							<mrow> \amp\ B = 1/112	</mrow>
						</md>
					</p>
					<p/>
				</sidebyside>
				Finally, the general solution is
				<me> y = y_h + y_p = c_1 e^{4t} + c_2 e^{-7t} - \frac{1}{4}t + \frac{1}{112} + \frac{1}{11}e^{4t} </me>.

			</p>

		</solution>

	</example>

	<!-- <assemblage><title>Tip: Identifying when things are Amiss</title>
		<p>
			Each coefficient should have exactly one solution. If you end up with conflicting values or unsolvable equations, it's a good idea to double-check your choice of <m>y_p</m> and computations.
		</p>
	</assemblage> -->

	<xi:include href="./p3-c2-s5-interactives.ptx" />

</section>