<section xmlns:xi="http://www.w3.org/2001/XInclude"><title> SOV Method </title>

	<p>
		We are now going to discuss the steps involved in the <em>separation of variables</em> method. In order to use this method, the differential equation must be first-order and be <xref ref="separable" text="custom">separable</xref>.
	</p>

	<p>
		Identifying a differential equation as first-order is as simple as observing the presence of a first derivative and no higher derivatives. In comparison, determining that an equation is separable is not always immediately apparent. Sometimes, it requires some algebra to rearrange the equation into a form where the method can be applied. 
	</p>

	<exploration xml:id="sov-method"><title> Separation of Variables </title>
		<p>
			If a differential equation can be written in the separable form
			<me xml:id="sov-method-de">
				\frac{dy}{dx} = f(x) \cdot g(y)
			</me>,
			then the general solution can be determined through the steps below.
		</p>
		<dl>
			<li xml:id="sov-step-1"><title> Step 1: Separate </title>
				<p>
					<m>\displaystyle \frac{1}{g(y)}\ dy = f(x)\ dx</m>
				</p>
			</li>
			<li xml:id="sov-step-2"><title> Step 2: Integrate </title>
				<p>
					<m>\displaystyle \int \frac{1}{g(y)}\ dy = \int f(x) \ dx</m>
				</p>
			</li>
			<li xml:id="sov-step-3"><title> Step 3: Finalize  </title>
				<p>
					Isolate <m>y</m> (if possible), and combine constants.
				</p>
			</li>
		</dl>
	</exploration> 

	<p>
		These problems serve as warm-up examples to familiarize you with the separation of variables method. You won't encounter any tricky algebra or calculus steps, allowing you to focus solely on the general steps needed to apply this technique. However, pay close attention to the new concept of "combining constants", as it will appear frequently throughout this course.
	</p>


	<example xml:id="sov-method-level-1-01"><title> SoV w/ no <m>y</m> variable </title>

		<statement><me> \frac{dy}{dx} = x^2 </me></statement>

		<solution>

			<p>
				You actually don't need separation of variables to solve for <m>y</m>. In fact, you might recognize that finding <m>y</m> is the same as finding the anti-derivative of <m>x^2</m>, which we know is <m>y = \frac13x^3 + C</m>. Nevertheless, let's apply separation of variables to make sure we get the same answer.
			</p>

			<p>
				The differential equation has order 1 and is separable since
				<me>\ds  \frac{dy}{dx} = \underset{f(x)}{\underset{\uparrow}{\big( x^2 \big)}} \cdot \underset{g(y)}{\underset{\uparrow}{\big( 1 \big)}}</me>
			</p>
	
			<p>
				<xref ref="sov-step-1" text="title" />
			</p>

			<p>
				We use algebra to move all the <m>y</m> terms to the left and all the <m>x</m> terms to the right, giving
				<me>\ds  \frac{1}{\underset{g(y)}{\underset{\uparrow}{ 1 }}} \frac{dy}{dx} = \underset{f(x)}{\underset{\uparrow}{ x^2 }}</me>
			</p>
	
			<p>
				<xref ref="sov-step-2" text="title" />
			</p>

			<p>
				We now integrate both sides with respect to <m>x</m>, like so
				<md>
					<mrow> \int 1 \underset{=\ dy}{\underbrace{\frac{dy}{dx}dx}} \amp = \int x^2\ dx</mrow>
					<mrow> \int 1\ dy \amp = \int x^2\ dx</mrow>
					<mrow> y + C_1    \amp = \frac13 x^3 + C_2. </mrow>
				</md>
			</p>

			<p>
				<xref ref="sov-step-3" text="title" />
			</p>
	
			<p>
				Finally, we isolate <m>y</m> and combine constants.
				<md>
				<mrow>  y \amp = \frac13 x^3 + C_2 - C_1 </mrow>
				</md>
			</p>
	
			<p>
				Since <m> C_2 - C_1 </m> is still a constant, we combine it into a single constant, <m>C</m>, and write our solution as
				<me>
				y = \frac13 x^3 + C
				</me>
			</p>

		</solution>

	</example>

	<p>
		Let's see how the solution changes if we replace <m>x^2</m> with <m>y^2</m>.
	</p>

	<example xml:id="sov-method-level-1-02"><title> SoV w/ no <m>x</m> variable </title>

		<statement><me> \frac{dy}{dx} = y^2 </me></statement>

		<solution>

			<p>
				The differential equation has order 1 and is separable since
				<me>
					\frac{dy}{dx} = \underset{f(x)}{\underset{\uparrow}{\big( 1 \big)}} \cdot \underset{g(y)}{\underset{\uparrow}{\big( y^2 \big)}}
				</me>
			</p>
	
			<p>
				<xref ref="sov-step-1" text="title" />
			</p>

			<p>
				We use algebra to move all the <m>y</m> terms to the left and all the <m>x</m> terms to the right, giving
				<me>
					\frac{1}{\underset{g(y)}{\underset{\uparrow}{ y^2 }}} \frac{dy}{dx} = \underset{f(x)}{\underset{\uparrow}{ 1 }}
				</me>
			</p>
	
			<p>
				<xref ref="sov-step-2" text="title" />
			</p>

			<p>
				We now integrate both sides with respect to <m>x</m>, like so
				<md>
					<mrow> \int 1\frac{1}{y^2} \underset{=\ dy}{\underbrace{\frac{dy}{dx}dx}} \amp = \int 1\ dx</mrow>
					<mrow> \int y^{-2}\ dy \amp = \int 1\ dx</mrow>
					<mrow> \frac{y^{-1}}{-1} + C_1    \amp = x + C_2. </mrow>
				</md>
			</p>

			<p>
				<xref ref="sov-step-3" text="title" />
			</p>
	
			<p>
				Finally, we isolate <m>y</m> and combine constants.
				<md>
					<mrow>  -\frac{1}{y} \amp = x + C_2 - C_1 </mrow>
					<mrow>  -\frac{1}{y} \amp = x - (C_2 - C_1) </mrow>
					<mrow>  \frac{1}{y} \amp = -x + C \quad \leftarrow \text{combined constant} </mrow>
					<mrow>  y \amp = \frac{1}{-x + C} </mrow>
				</md>
			</p>

		</solution>

	</example>

	<p>
		Here is a straight-forward example that includes both variables.
	</p>

	<example xml:id="sov-method-level-1-03"><title> SoV w/ simple integration </title>

		<statement><me> \frac{dy}{dx} + \frac{x}{y^2} = 0 </me></statement>

		<solution>

			<p>
				<me>
					\frac{dy}{dx} = - \frac{x}{y} = -x\left(\frac{1}{y^2}\right) \quad \leftarrow \text{separable}
				</me>
			</p>
	
			<p>
				<xref ref="sov-step-1" text="title" />
			</p>

			<p>
				<me>
					y^2\frac{dy}{dx} = -x
				</me>
			</p>
	
			<p>
				<xref ref="sov-step-2" text="title" />
			</p>

			<p>
				<md>
					<mrow> \int y^2 \underset{=\ dy}{\underbrace{\frac{dy}{dx}dx}}	\amp = \int -x\ dx</mrow>
					<mrow> 											\int y^2 \ dy 	\amp = \int -x\ dx</mrow>
					<mrow> 									\frac{y^{3}}{3} + C_1	\amp = -\frac{x^{2}}{2} + C_2. </mrow>
				</md>
			</p>

			<p>
				<xref ref="sov-step-3" text="title" />
			</p>
	
			<p>
				<md>
					<mrow> 	\frac{y^{3}}{3}	\amp = -\frac{x^{2}}{2} + \underset{=\ C_3}{\underbrace{C_2 - C_1}}  	</mrow>
					<mrow>  		y^{3}	\amp = -3\cdot\frac{x^{2}}{2} + \underset{=\ C}{\underbrace{3\cdot C_3}} 	</mrow>
					<mrow>  		y^{3}	\amp = -\frac32 x^2 + C 						</mrow>
					<mrow>  		y		\amp = \left(-\frac32 x^2 + C \right)^{1/3} 						</mrow>
				</md>
			</p>

		</solution>

	</example>

	<xi:include href="./p2-c2-s4-interactives.ptx" />
  
</section>