<section xmlns:xi="http://www.w3.org/2001/XInclude"><title> Characteristic Equation </title>

	<p>
        Our goal is to solve <xref ref="def-lhcc" text="custom">LHCC equations</xref>. Before we dive into specific solutions, let’s develop some intuition by looking at a familiar idea from calculus.
    </p>

    <p>
        You might recall the function whose derivative is itself: <m>e^x</m>. This can be framed as a differential equation, <m>y' = y</m>, with the solution <m>y = e^x</m>. Similarly, if we consider <m>y' = 3y</m>, the solution becomes <m>y = e^{3x}</m>. This is important because, for certain equations, the solutions involve functions like <m>e^{rx}</m>, where <m>r</m> is a constant that we need to figure out.
    </p>

    <p>
        So why is this relevant for LHCC equations? When we substitute <m>e^{rx}</m> and its derivatives into an LHCC equation, we often get terms that combine neatly and cancel out. For example, consider the LHCC equation:
    </p>

    <me> y'' + 3y' - 4y = 0 </me>

    <p>
        If we try substituting <m>y = e^{4x}</m> into this equation, we find that the terms simplify and cancel out to give <m>0 = 0</m>, meaning <m>y = e^{4x}</m> is a valid solution. However, if we try other functions, like <m>y = x^4</m> or <m>y = \sin(4x)</m>, they don’t work because their derivatives don’t combine in the same way. Only exponential functions <m>e^{rx}</m> seem to fit the bill.
    </p>

    <p>
        This brings us to a key concept: solutions to LHCC equations involve terms of the form <m>e^{rx}</m>, but not every value of <m>r</m> works. To find the correct values of <m>r</m>, we need a tool called the <term>characteristic equation</term>.
    </p>

    <p>
        The characteristic equation is a polynomial equation that gives us the values of <m>r</m> for which <m>e^{rx}</m> is a solution. Let’s see how this works with a simple example. Consider the first-order equation:
    </p>

    <me> y' - 5y = 0 </me>

    <p>
        To verify that <m>y = e^{rx}</m> is a solution, we substitute it into the equation:
    </p>

    <md>
        <mrow> \left[e^{rx}\right]' - 5 \left[e^{rx}\right] = 0 </mrow>
        <mrow> r e^{rx} - 5 e^{rx} = 0 </mrow>
        <mrow> (r - 5) e^{rx} = 0 </mrow>
    </md>

    <p>
        Since <m>e^{rx}</m> is never zero, we solve for <m>r</m> by setting <m>r - 5 = 0</m>, giving us <m>r = 5</m>. This means <m>y = e^{5x}</m> is a solution.
    </p>

    <p>
        Now let’s look at a second-order equation:
    </p>

    <me> y'' - 5y' + 6y = 0 </me>

    <p>
        Substituting <m>y = e^{rx}</m> into this equation gives:
    </p>

    <md>
        <mrow> \left[e^{rx}\right]'' - 5 \left[e^{rx}\right]' + 6 \left[e^{rx}\right] = 0 </mrow>
        <mrow> r^2 e^{rx} - 5r e^{rx} + 6 e^{rx} = 0 </mrow>
        <mrow> (r^2 - 5r + 6) e^{rx} = 0 </mrow>
    </md>

    <p>
        Again, since <m>e^{rx}</m> is never zero, we solve the quadratic equation <m>r^2 - 5r + 6 = 0</m>, which gives <m>r = 2</m> and <m>r = 3</m>. So, the solutions are <m>y = e^{2x}</m> and <m>y = e^{3x}</m>.
    </p>

    <p>
        In general, for any LHCC equation, substituting <m>y = e^{rx}</m> leads to a polynomial equation in terms of <m>r</m>. This polynomial is called the <em>characteristic equation</em>. To solve an LHCC equation, we first solve the characteristic equation to find the values of <m>r</m>, which then give us the solutions of the form <m>e^{rx}</m>.
    </p>

    <definition xml:id="def-characteristic-equation"><title>Characteristic Equation</title>
        <statement>
            <p>
                The <term>characteristic equation</term> of a linear homogeneous differential equation with constant coefficients (LHCC) is the polynomial equation:
            </p>
            <men xml:id="characteristic-equation"> 
                a_n\ r^n + a_{n-1}\ r^{n-1} + \cdots + a_1\ r + a_0 = 0
            </men>
        </statement>
    </definition>

    <p>
        The solutions to this equation provide the <m>r</m>-values needed to form the general solution of the LHCC equation.
    </p>

    <example>
        <p>
            Find the characteristic equation for the differential equation:
            <me> y'' + 5y' - y = 0 </me>
        </p>

        <solution>
            <p>
                The characteristic equation is obtained by substituting <m>y = e^{rx}</m> into the differential equation:
                <me> r^2 + 5r - 1 = 0 </me>.
                Solving this quadratic equation gives the <m>r</m>-values, which correspond to the solutions <m>e^{2x}</m> and <m>e^{3x}</m>.
            </p>
        </solution>
    </example>

	<xi:include href="./p3-c1-s2-interactives.ptx" />

</section>
