
<subsection xmlns:xi="http://www.w3.org/2001/XInclude"><title> Summary &amp; Exercises </title>

	<introduction>

		<p>
			This section covers the final step in solving differential equations using the Laplace Transform Method: finding the inverse Laplace transform. The focus is on converting the algebraic equation with unknown function <m>Y(s)</m> back to the original function <m>y(t)</m>. Several methods and techniques are introduced to handle different cases where direct computation isn't possible.
		</p>
		
		<p>
			<assemblage><title> Summary of the Key Ideas </title>
				<p>
						<term>Common Forms:</term> A table of common Laplace transforms is provided, which doubles as a reference for inverse transforms. The focus is on recognizing forms that match the table entries for functions like <m>\sin(bt), \cos(bt)</m>, and others.
					</p>

					<p>
						<term>Direct Computation:</term> When the function of <m>s</m> directly matches a form in the common Laplace transform table, the inverse Laplace transform can be easily computed.
					</p>
					
					<p>
						<term>Modifying Functions:</term> When a function doesn't match a known form, minor modifications, such as multiplying by missing constants or splitting fractions, can help.
					</p>
					
					<p>
						<term>Completing the Square:</term> When dealing with quadratic expressions in the denominator, especially when the discriminant is negative, completing the square can transform the expression into a form that matches known inverse Laplace transforms. Several examples demonstrate this technique.
					</p>

					<p>
						<term>Partial Fraction Decomposition:</term> For more complex rational functions, partial fraction decomposition breaks down the function into simpler fractions that match the common transform forms.
					</p>
			</assemblage>
		</p>
		
	</introduction>

	<exercises>

		<exercise><title> <em><m>\ds \ilap{\frac{1}{s - 1} - \frac{1}{s + 1} + \frac{4s + 3}{s^2 + 1}} = <fillin characters="10" /></m></em> </title>
			<statement/>
			<choices>
				<choice correct="yes">
					<statement><m>\ds e^{t} - e^{-t} + 4\cos(t) + 3\sin(t)</m></statement>
					<feedback>
						<p>
							Correct! The inverse Laplace transform matches the forms in the table.
						</p>
					</feedback>
				</choice>
				<choice>
					<statement><m>\ds e^{t} + e^{t} + \cos(t) + \sin(t)</m></statement>
					<feedback>
						<p>
							No, this does not match the correct inverse Laplace transform.
						</p>
					</feedback>
				</choice>
				<choice>
					<statement><m>\ds e^{-t} - e^{t} + \cos(t)</m></statement>
					<feedback>
						<p>
							Incorrect. This does not account for all terms in the inverse Laplace transform.
						</p>
					</feedback>
				</choice>
			</choices>
		</exercise>

		<exercise label="p4-c1-s1-1-rq11"><title> What is the Laplace transform of <m>e^{3t}</m>? </title>
			<statement/>
			<choices>
				<choice correct="yes">
					<statement><m>\ds\frac{1}{s-3}</m></statement>
				</choice>
				<choice>
					<statement><m>\ds\frac{1}{s+3}</m></statement>
				</choice>
				<choice>
					<statement><m>\ds\frac{1}{s-2}</m></statement>
				</choice>
				<choice>
					<statement><m>\ds\frac{1}{s}</m></statement>
				</choice>
			</choices>
		</exercise>
	
		<exercise label="p4-c1-s1-1-rq12"><title> In the equation <m>y'' + 4y = \cos(2t)</m>, what is the Laplace transform of the right-hand side? </title>
			<statement/>
			<choices>
				<choice correct="yes">
					<statement><m>\ds\frac{s}{s^2 + 4}</m></statement>
				</choice>
				<choice>
					<statement><m>\ds\frac{4}{s^2 + 4}</m></statement>
				</choice>
				<choice>
					<statement><m>\ds\frac{s}{s^2 + 1}</m></statement>
				</choice>
				<choice>
					<statement><m>\ds\frac{1}{s^2 + 4}</m></statement>
				</choice>
			</choices>
		</exercise>
	
		<exercise label="p4-c1-s1-1-rq13"><title> <em>The expression <m>\ds\frac{s-1}{(s-1)^2 + 4}</m> matches the form required to apply the inverse Laplace transform found in the common transform table</em> </title>
			<statement correct="yes"/>
			<feedback>
				<p>
					True. This expression matches the form in the table and can be directly transformed.
				</p>
			</feedback>
		</exercise>

		<exercisegroup cols="2"><title> Match the Sine Form </title>
		
			<introduction>
				<p>
					Rewrite each of the following into the form
					<me>A \cdot \frac{b}{s^2 + b^2}</me>,
					by filling in the appropriate values in the boxes.
				</p>
			</introduction>
		
			<exercise>
				
				<statement><m>\ds \frac{1}{s^2 + 49} = \boxed{\phantom{ \left|\frac{1}{7}\right|}} \cdot \frac{\boxed{\phantom{ |7| }}}{s^2 + \boxed{\phantom{ |7| }}^2}</m></statement>
				<answer>		
					<me>	
						\frac{1}{s^2 + 49} = \frac{1}{s^2 + 7^2} = \boxed{\frac{1}{7}} \cdot \frac{\boxed{7}}{s^2 + \boxed{7}^2}
					</me>
				</answer>

			</exercise>

			<exercise>
				<statement><m>\ds \frac{12}{s^2 + 16} = \boxed{\phantom{ \left|\frac{1}{4}\right|}} \cdot \frac{\boxed{\phantom{ |4| }}}{s^2 + \boxed{\phantom{ |4| }}^2}</m></statement>
				<answer>
					<p>
						<me>
						\frac{12}{s^2 + 16} = 3 \cdot \frac{4}{s^2 + 4^2} = \boxed{3} \cdot \frac{\boxed{4}}{s^2 + \boxed{4}^2}
					</me>
					</p>
				</answer>
			</exercise>

			<exercise>
				<statement><m>\ds \frac{3}{s^2 + 5} = \boxed{\phantom{ \frac{3}{\sqrt{5}}}} \cdot \frac{\boxed{\phantom{ \sqrt{5} }}}{s^2 + \boxed{\phantom{ \sqrt{5} }}^2}</m></statement>
				<answer>
					<p>
						<me>
						\frac{3}{s^2 + 5} = \frac{3}{\sqrt{5}} \cdot \frac{\sqrt{5}}{s^2 + (\sqrt{5})^2} = \boxed{\frac{3}{\sqrt{5}}} \cdot \frac{\boxed{\sqrt{5}}}{s^2 + \boxed{\sqrt{5}}^2}
					</me>
					</p>
				</answer>
			</exercise>

		</exercisegroup>

		<exercisegroup cols="2"><title> Match the Cosine Form </title>
		
			<introduction>
				<p>
					Rewrite each of the following into the form
					<me>A \cdot \frac{s}{s^2 + b^2}</me>,
					by filling in the appropriate values in the boxes.
				</p>
			</introduction>

			<exercise>
				<statement><m>\ds \frac{4s}{s^2 + 9} = \boxed{\phantom{ \left|\frac{1}{3}\right|}} \cdot \frac{s}{s^2 + \boxed{\phantom{ |3| }}^2}</m></statement>
				<answer>
					<p>
						<me>
						\frac{4s}{s^2 + 9} = 4 \cdot \frac{s}{s^2 + 3^2} = \boxed{4} \cdot \frac{s}{s^2 + \boxed{3}^2}
					</me>
					</p>
				</answer>
			</exercise>

			<exercise>
				<statement><m>\ds \frac{s}{2s^2 + 8} = \boxed{\phantom{ \left|\frac{1}{2}\right|}} \cdot \frac{s}{s^2 + \boxed{\phantom{ |2| }}^2}</m></statement>
				<answer>
					<p>
						<me>
						\frac{s}{2s^2 + 8} = \frac{1}{2} \cdot \frac{s}{s^2 + 2^2} = \boxed{\frac{1}{2}} \cdot \frac{s}{s^2 + \boxed{2}^2}
					</me>
					</p>
				</answer>

			</exercise>

		</exercisegroup>

		<exercisegroup cols="2"><title> Match the Power Form </title>
		
			<introduction>
				<p>
					Rewrite each of the following into the form
					<me>A \cdot \frac{n!}{s^{n+1}}</me>,
					by filling in the appropriate values in the boxes.
				</p>
			</introduction>

			<exercise>
				<statement><m>\ds \frac{1}{s^5} = \boxed{\phantom{ \frac{1}{24} }} \cdot \frac{\boxed{\phantom{ |4| }}\ {\large !}}{s\vphantom{S|}^{\boxed{\phantom{ 4\ }} + 1}}</m></statement>
				<answer>
					<p>
						<me>
						\frac{1}{s^5} = \frac{1}{24} \cdot \frac{4!}{s^{4+1}} = \boxed{\frac{1}{24}} \cdot \frac{\boxed{4}!}{s^{\boxed{4}+1}}
					</me>
					</p>
				</answer>
			</exercise>

			<exercise>
				<statement><m>\ds \frac{7}{s^3} = \boxed{\phantom{ \left|\frac{7}{2}\right| }} \cdot \frac{\boxed{\phantom{ |2| }}\ {\large !}}{s\vphantom{S|}^{\boxed{\phantom{ 2\ }} + 1}}</m></statement>
				<answer>
					<p>
						<me>
						\frac{7}{s^3} = \frac{7}{2} \cdot \frac{2!}{s^{2+1}} = \boxed{\frac{7}{2}} \cdot \frac{\boxed{2}!}{s^{\boxed{2}+1}}
					</me>
					</p>
				</answer>
			</exercise>

			<exercise>
				<statement><m>\ds \frac{2}{5s^4} = \boxed{\phantom{ \frac{1}{15} }} \cdot \frac{\boxed{\phantom{ |3| }}\ {\large !}}{s\vphantom{S|}^{\boxed{\phantom{ 3\ }} + 1}}</m></statement>
				<answer>
					<p>
						<me>
						\frac{2}{5s^4} = \frac{1}{15} \cdot \frac{3!}{s^{3+1}} = \boxed{\frac{1}{15}} \cdot \frac{\boxed{3}!}{s^{\boxed{3}+1}}
					</me>
					</p>
				</answer>
			</exercise>

		</exercisegroup>

		<exercisegroup><title> Backward Transforms- Level 1 </title>

			<exercise> <!--== Problem 1 ==-->
				<statement>
					<m> \ds F(s) = \frac{6}{(s-1)^4} </m>
				</statement>
				<solution>
					<p>
						<m> \ds F(s) = \frac{6}{(s-1)^4} </m>
					</p>
				</solution>
				<answer>
					<p>
						
					</p>
				</answer>
			</exercise>
		
			<exercise> <!--== Problem 2 ==-->
				<statement>
					<m> \ds X(s) = \frac{1}{s^5} </m>
				</statement>
				<solution>
					<p>
						<m> \ds X(s) = \frac{1}{s^5} </m>
					</p>
				</solution>
				<answer>
					<p>
						
					</p>
				</answer>
			</exercise>
		
			<exercise> <!--== Problem 3 ==-->
				<statement>
					<m> \ds G(s) = \frac{4}{s^2 + 9} </m>
				</statement>
				<solution>
					<p>
						<m> \ds G(s) = \frac{4}{s^2 + 9} </m>
					</p>
				</solution>
				<answer>
					<p>
						
					</p>
				</answer>
			</exercise>
		
			<exercise> <!--== Problem 4 ==-->
				<statement>
					<m> \ds Y(s) = \frac{5s}{s^2 + 7} </m>
				</statement>
				<solution>
					<p>
						<m> \ds Y(s) = \frac{5s}{s^2 + 7} </m>
					</p>
				</solution>
				<answer>
					<p>
						
					</p>
				</answer>
			</exercise>
		
			<exercise> <!--== Problem 5 ==-->
				<statement>
					<m> \ds X(s) = \frac{21}{(s+2)^2 + 16} </m>
				</statement>
				<solution>
					<p>
						<m> \ds X(s) = \frac{21}{(s+2)^2 + 16} </m>
					</p>
				</solution>
				<answer>
					<p>
						
					</p>
				</answer>
			</exercise>
		
			<exercise> <!--== Problem 6 ==-->
				<statement>
					<m> \ds F(s) = \frac{10}{s-10} </m>
				</statement>
				<solution>
					<p>
						<m> \ds F(s) = \frac{10}{s-10} </m>
					</p>
				</solution>
				<answer>
					<p>
						
					</p>
				</answer>
			</exercise>
		
			<exercise> <!--== Problem 7 ==-->
				<statement>
					<m> \ds Q(s) = \frac{7s+7}{(s+1)^2 + 12} </m>
				</statement>
				<solution>
					<p>
						<m> \ds Q(s) = \frac{7s+7}{(s+1)^2 + 12} </m>
					</p>
				</solution>
				<answer>
					<p>
						
					</p>
				</answer>
			</exercise>
		
		</exercisegroup>
		
		<exercisegroup><title> Backward Transforms- Level 2 </title>

			<exercise> <!--== Problem 8 ==-->
				<statement>
					<m> \ds G(s) = \frac{1}{s^2 + 4s + 8} </m>
				</statement>
				<solution>
					<p>
						<m> \ds G(s) = \frac{1}{s^2 + 4s + 8} </m>
					</p>
				</solution>
				<answer>
					<p>
						
					</p>
				</answer>
			</exercise>
		
			<exercise> <!--== Problem 9 ==-->
				<statement>
					<m> \ds F(s) = \frac{2s+16}{s^2 + 4s + 13} </m>
				</statement>
				<solution>
					<p>
						<m> \ds F(s) = \frac{2s+16}{s^2 + 4s + 13} </m>
					</p>
				</solution>
				<answer>
					<p>
						
					</p>
				</answer>
			</exercise>
		
			<exercise> <!--== Problem 10 ==-->
				<statement>
					<m> \ds Y(s) = \frac{3s-15}{2s^2 - 4s + 8} </m>
				</statement>
				<solution>
					<p>
						<m> \ds Y(s) = \frac{3s-15}{2s^2 - 4s + 8} </m>
					</p>
				</solution>
				<answer>
					<p>
						
					</p>
				</answer>
			</exercise>
		
			<exercise> <!--== Problem 11 ==-->
				<statement>
					<m> \ds Q(s) = \frac{1}{s^2 + 6s + 9} </m>
				</statement>
				<solution>
					<p>
						<m> \ds Q(s) = \frac{1}{s^2 + 6s + 9} </m>
					</p>
				</solution>
				<answer>
					<p>
						
					</p>
				</answer>
			</exercise>
		
			<exercise> <!--== Problem 12 ==-->
				<statement>
					<m> \ds H(s) = \frac{5}{s-6} - \frac{6s}{s^2 + 9} + \frac{3}{2s^2 + 8s + 10} </m>
				</statement>
				<solution>
					<p>
						<m> \ds H(s) = \frac{5}{s-6} - \frac{6s}{s^2 + 9} + \frac{3}{2s^2 + 8s + 10} </m>
					</p>
				</solution>
				<answer>
					<p>
						
					</p>
				</answer>
			</exercise>
		
			<exercise> <!--== Problem 13 ==-->
				<statement>
					<m> \ds X(s) = \frac{7s-4}{s^2 + 36} </m>
				</statement>
				<solution>
					<p>
						<m> \ds X(s) = \frac{7s-4}{s^2 + 36} </m>
					</p>
				</solution>
				<answer>
					<p>
						
					</p>
				</answer>
			</exercise>
		
			<exercise> <!--== Problem 14 ==-->
				<statement>
					<m> \ds G(s) = \frac{2s-19}{s^2 - 4s+13} + \frac{5}{s-1} </m>
				</statement>
				<solution>
					<p>
						<m> \ds G(s) = \frac{2s-19}{s^2 - 4s+13} + \frac{5}{s-1} </m>
					</p>
				</solution>
				<answer>
					<p>
						
					</p>
				</answer>
			</exercise>
		
			<exercise> <!--== Problem 15 ==-->
				<statement>
					<m> \ds F(s) = \frac{s}{s^2 + 6s + 11} </m>
				</statement>
				<solution>
					<p>
						<m> \ds F(s) = \frac{s}{s^2 + 6s + 11} </m>
					</p>
				</solution>
				<answer>
					<p>
						
					</p>
				</answer>
			</exercise>
		
		</exercisegroup>
		
		<exercisegroup><title> Backward Transforms- Level 3 </title>
		
			<exercise> <!--== Problem 16 ==-->
				<statement>
					<m> \ds X(s) = \frac{90s^2 - 195s + 30}{s^3 - 7s^2 + 6s} </m>
				</statement>
				<solution>
					<p>
						<m> \ds X(s) = \frac{90s^2 - 195s + 30}{s^3 - 7s^2 + 6s} </m>
					</p>
				</solution>
				<answer>
					<p>
						
					</p>
				</answer>
			</exercise>
		
			<exercise> <!--== Problem 17 ==-->
				<statement>
					<m> \ds I(s) = \frac{5s^2 + 34s + 53}{(s+3)^2(s+1)} </m>
				</statement>
				<solution>
					<p>
						<m> \ds I(s) = \frac{5s^2 + 34s + 53}{(s+3)^2(s+1)} </m>
					</p>
				</solution>
				<answer>
					<p>
						
					</p>
				</answer>
			</exercise>
		
			<exercise> <!--== Problem 18 ==-->
				<statement>
					<m> \ds F(s) = \frac{7s^3 - 2s^2 - 3s + 6}{s^3(s-2)} </m>
				</statement>
				<solution>
					<p>
						<m> \ds F(s) = \frac{7s^3 - 2s^2 - 3s + 6}{s^3(s-2)} </m>
					</p>
				</solution>
				<answer>
					<p>
						
					</p>
				</answer>
			</exercise>
		
		</exercisegroup>
		
		<exercisegroup><title> Steps 3 &amp; 4 </title>

			<exercise> <!--== Problem 19 ==-->
				<statement>
					<m> \ds s^2 F(s) - 4F(s) = \frac{60}{s+1} </m>
				</statement>
				<solution>
					<p>
						<m> \ds s^2 F(s) - 4F(s) = \frac{60}{s+1} </m>
					</p>
				</solution>
				<answer>
					<p>
						
					</p>
				</answer>
			</exercise>
		
			<exercise> <!--== Problem 20 ==-->
				<statement>
					<m> \ds \ds s^2 F(s) + sF(s) - 6F(s) = \frac{30s^2 + 120}{s^2 + s} </m>
				</statement>
				<solution>
					<p>
						<m> \ds \ds s^2 F(s) + sF(s) - 6F(s) = \frac{30s^2 + 120}{s^2 + s} </m>
					</p>
				</solution>
				<answer>
					<p>
						
					</p>
				</answer>
			</exercise>
		
		</exercisegroup>

		<exercisegroup><title> Inverse Laplace Transforms </title>
	
			<introduction>
				<p>
					Determine the original time-domain functions from the given Laplace-transformed functions.
				</p>
			</introduction>
	
			<exercise>
				<statement>
					<m>\ds Y(s) = \frac{2s + 7}{(s + 1)(s + 3)}</m>
				</statement>
				<solution>
					<p>
				Decompose into partial fractions:
					<me>Y(s) = \frac{A}{s + 1} + \frac{B}{s + 3}</me>.
					Find <m>A</m> and <m>B</m>:
					<me>A = 1, B = \frac{1}{2}</me>.
					Use the inverse Laplace transform:
					<me>y(t) = e^{-t} + \frac{1}{2}e^{-3t}</me>.
					</p>
				</solution>
				<answer>
					<p>
						<m>\ds y(t) = e^{-t} + \frac{1}{2}e^{-3t}</m>
					</p>
				</answer>
			</exercise>
	
			<exercise>
				<statement>
					<m>\ds F(s) = \frac{5}{s(s + 4)}</m>
				</statement>
				<solution>
					<p>
				Decompose into partial fractions:
					<me>F(s) = \frac{A}{s} + \frac{B}{s + 4}</me>.
					Find <m>A</m> and <m>B</m>:
					<me>A = \frac{5}{4}, B = -\frac{5}{4}</me>.
					Use the inverse Laplace transform:
					<me>f(t) = \frac{5}{4}(1 - e^{-4t})</me>.
					</p>
				</solution>
				<answer>
					<p>
						<m>\ds f(t) = \frac{5}{4}(1 - e^{-4t})</m>
					</p>
				</answer>
			</exercise>
	
		</exercisegroup>

		<exercisegroup>
		
			<introduction>
				<p>
					Find the inverse Laplace transforms of each function.
				</p>
			</introduction>
		
			<exercise>
				<statement><m>\ds R(s) = \frac{3s + 2}{s^2 + 4s + 4} </m></statement>
				<answer>
					<p>
						<p>
						<m>\ds r(t) = 3e^{-2t} + 2te^{-2t} </m>
					</p>
					</p>
				</answer>
			</exercise>

			<exercise>
				<statement><m>\ds  S(s) = \frac{4s + 1}{s^2 + 6s + 9} </m></statement>
				<answer>
					<p>
						<p>
						<m>\ds  s(t) = 4e^{-3t} + (t + 1)e^{-3t} </m>
					</p>
					</p>
				</answer>
			</exercise>
		
		</exercisegroup>

		<exercisegroup><title> Conceptual Questions </title>
	
			<exercise>
				<statement>
					<p>True or False: The inverse Laplace transform is always a unique function.</p>
				</statement>
				<answer>
					<p>
						<p>True</p>
					</p>
				</answer>
			</exercise>
	
			<exercise>
				<statement>
					<p>Which of the following is true about the inverse Laplace transform?</p>
					<choice>
						<li>It converts a function from the frequency domain to the time domain.</li>
						<li>It is a method to solve algebraic equations.</li>
						<li>It is used to differentiate a function with respect to time.</li>
						<li>It only works for polynomials.</li>
					</choice>
				</statement>
				<answer>
					<p>
						<p>It converts a function from the frequency domain to the time domain.</p>
					</p>
				</answer>
			</exercise>
	
			<exercise>
				<statement>
					<p>Explain the significance of completing the square in finding inverse Laplace transforms.</p>
				</statement>
				<answer>
					<p>
						<p>Completing the square is a technique used to transform quadratic expressions in the denominator into a form that matches known inverse Laplace transforms, particularly those involving sine and cosine functions.</p>
					</p>
				</answer>
			</exercise>
	
			<exercise>
				<statement>
					<p>Why is partial fraction decomposition helpful in finding inverse Laplace transforms?</p>
				</statement>
				<answer>
					<p>
						<p>Partial fraction decomposition breaks down complex rational functions into simpler fractions that correspond to known inverse Laplace transforms, making the transformation process easier.</p>
					</p>
				</answer>
			</exercise>
	
		</exercisegroup>
	
		<exercisegroup><title> Computational Problems </title>
	
			<exercise>
				<statement>
					<p>Find the inverse Laplace transform of <m>\ds \frac{5}{s^2 + 16}</m>.</p>
				</statement>
				<solution>
					<p>
						This expression matches the form <m>\ds \frac{b}{s^2 + b^2} </m> with <m>\ds b = 4 </m>, so the inverse Laplace transform is <m>\ds 5 \cdot \sin(4t) </m>.
					</p>
				</solution>
			</exercise>
	
			<exercise>
				<statement>
					<p>Compute the inverse Laplace transform of <m>\ds \frac{2s + 7}{(s + 3)^2 + 4} </m>.</p>
				</statement>
				<solution>
					<p>
						This expression can be split into two parts: <m>\ds \frac{2(s + 3)}{(s + 3)^2 + 4} </m> and <m>\ds \frac{7}{(s + 3)^2 + 4} </m>. The first part corresponds to <m>\ds e^{-3t} \cdot \cos(2t) </m> and the second part corresponds to <m>\ds e^{-3t} \cdot \sin(2t) </m>, so the inverse Laplace transform is <m>\ds 2e^{-3t} \cos(2t) + 7e^{-3t} \sin(2t) </m>.
					</p>
				</solution>
			</exercise>
	
			<exercise>
				<statement>
					<p>Use partial fraction decomposition to find the inverse Laplace transform of <m>\ds \frac{3s + 4}{s^2 + 2s + 1} </m>.</p>
				</statement>
				<solution>
					<p>
						First, factor the denominator as <m>\ds (s + 1)^2 </m>. Then, decompose the expression into <m>\ds \frac{A}{s + 1} + \frac{B}{(s + 1)^2} </m>. Solving for <m>\ds A </m> and <m>\ds B </m>, you get the inverse Laplace transform as <m>\ds 3e^{-t} + 4te^{-t} </m>.
					</p>
				</solution>
			</exercise>
	
		</exercisegroup>
	
		<exercisegroup><title> Application-Based Problems </title>
	
			<exercise>
				<statement>
					<p>Given the function <m>\ds Y(s) = \frac{7}{(s - 2)^2 + 9} </m>, describe the behavior of the corresponding time-domain function.</p>
				</statement>
				<solution>
					<p>
						The inverse Laplace transform is <m>\ds 7e^{2t} \sin(3t) </m>, which indicates a sinusoidal function modulated by an exponential growth factor.
					</p>
				</solution>
			</exercise>
	
			<exercise>
				<statement>
					<p>Find the inverse Laplace transform of the function <m>\ds F(s) = \frac{6s + 10}{(s + 4)(s^2 + 9)} </m> using partial fraction decomposition.</p>
				</statement>
				<solution>
					<p>
						Decompose the function into <m>\ds \frac{A}{s + 4} + \frac{Bs + C}{s^2 + 9} </m>. Solving for the constants <m> A </m>, <m> B </m>, and <m> C </m>, the inverse Laplace transform will be a combination of exponential and sinusoidal functions.
					</p>
				</solution>
			</exercise>
	
		</exercisegroup>

		<exercise><title> <em><m>\ds \ilap{\frac{4s^3 + 3s^2 - 2s + 1}{(s - 1)(s + 1)(s^2 + 1)}} = <fillin characters="6" /></m></em> </title>
			<statement/>
			<choices>
				<choice correct="yes">
					<statement><m>\ds e^{t} - e^{-t} + 4\cos(t) + 3\sin(t)</m></statement>
					<feedback>
						<p>
							Correct! The inverse Laplace transform is <m>e^{t} - e^{-t} + 4\cos(t) + 3\sin(t)</m>.
						</p>
					</feedback>
				</choice>
				<choice>
					<statement><m>\ds 1 + e^{-t} + \cos(t)</m></statement>
					<feedback>
						<p>
							Incorrect. This does not match the correct inverse Laplace transform.
						</p>
					</feedback>
				</choice>
				<choice>
					<statement><m>\ds 2\cos(t) + 3\sin(t)</m></statement>
					<feedback>
						<p>
							Incorrect. This does not include the full inverse Laplace transform.
						</p>
					</feedback>
				</choice>
			</choices>
		</exercise>

		<exercise><title> <em><m>\ds \ilap{\frac{s-1}{(s-1)^2 + 4}} = <fillin characters="6"/></m></em> </title>
			<statement/>
			<choices>
				<choice correct="yes">
					<statement><m>\ds e^{t}\cos(2t)</m></statement>
					<feedback>
						<p>
							Correct! The inverse Laplace transform of this expression is <m>e^{t}\cos(2t)</m>.
						</p>
					</feedback>
				</choice>
				<choice>
					<statement><m>\ds e^{-t}\sin(2t)</m></statement>
					<feedback>
						<p>
							Incorrect. The correct inverse Laplace transform is <m>e^{t}\cos(2t)</m>.
						</p>
					</feedback>
				</choice>
				<choice>
					<statement><m>\ds \cos(2t)</m></statement>
					<feedback>
						<p>
							Incorrect. The correct inverse Laplace transform is <m>e^{t}\cos(2t)</m>.
						</p>
					</feedback>
				</choice>
			</choices>
		</exercise>

		<exercise><title> <em><m>\ds \ilap{\frac{11}{(s - 3)^2 + 5}} = \frac{11}{\sqrt{5}}e^{3t}\sin(\sqrt{5}t)</m>, which matches the form in the table when <m>b = <fillin characters="1"/></m></em> </title>
			<statement/>
			<choices>
				<choice correct="yes">
					<statement><m>\sqrt{5}</m></statement>
					<feedback>
						<p>
							Correct! The correct value for <m>b</m> is <m>\sqrt{5}</m>.
						</p>
					</feedback>
				</choice>
				<choice>
					<statement><m>5</m></statement>
					<feedback>
						<p>
							Incorrect. The correct value is <m>\sqrt{5}</m>, not 5.
						</p>
					</feedback>
				</choice>
				<choice>
					<statement><m>3</m></statement>
					<feedback>
						<p>
							Incorrect. The correct value is <m>\sqrt{5}</m>, not 3.
						</p>
					</feedback>
				</choice>
			</choices>
		</exercise>

	</exercises>

</subsection>