<subsection xml:id="s-04-08-lt-lts-involving-unit-step-funcs" xmlns:xi="http://www.w3.org/2001/XInclude">
<title>Laplace Transforms Involving Unit Step Functions</title>
	

	<aside><p>Swap sections 4.8 and 4.9</p></aside>

	<p>
		We are now able to rewrite piecewise defined functions in terms of unit step functions. We now need to take Laplace transforms of piecewise defined functions, and then we will be
		ready to solve DEs involving piecewise defined functions. 
	</p>

	<example xml:id="ex_g_as_u">
		<p>
			Consider the function
			<me>
				g(t) = \left\{ 
				\begin{array}{ll}
					0,	\amp t \lt 2, \\
					6,	\amp 2 \le t \lt 5,\\
					-4,	\amp t \ge 5
				\end{array} \right.
			</me>

			<ol>
				<li>
					Write <m>g(t)</m> in terms of unit step functions.
					<me> g(t) = 6\ U(t-2) - 10\ U(t-5). </me>
				</li>
				<li>
					Find the Laplace transform of <m>g(t)</m> using the definition of the Laplace transform.
				</li>
				<li>
					Based on your answers to parts (a) and (b), hypothesize about a rule for taking the Laplace transform of a unit step function.
				</li>
			</ol>
		<p/>

		</p>
		<solution>
			<p>
				<ol>
					<li>
						The function changes behavior at <m>t = 2</m> and <m>t = 5.</m>  We can then assemble	the function as follows, thinking about turning the pieces 'on' and 'off' as described in the previous section.
						<md>
							<mrow>g(t)	=\amp\ 0 + (-0 + 6)\cdot U(t-2) + (-6 + -4) \cdot U(t-5)</mrow>
							<mrow>=\amp\ 6\ U(t-2) - 10\ U(t-5)</mrow>
						</md>
					</li>
					<li>
						We will use the definition of the Laplace transform and properties of integration, as follows.
						<md>
							<mrow>G(s)	=\amp\ \lap{ g(t) }</mrow>
							<mrow>=\amp\ \int_0^{\infty} e^{-st}g(t)dt</mrow>
							<mrow>=\amp\ \int_0^2 e^{-st}g(t)dt + \int_2^5 e^{-st}g(t)dt + \int_5^{\infty} e^{-st}g(t)dt</mrow>
							<mrow>=\amp\ \int_0^2 e^{-st}\cdot 0dt + \int_2^5 e^{-st}\cdot 6dt </mrow>
										+ \int_5^{\infty} e^{-st}\cdot (-4)dt
							<mrow>=\amp\ \int_0^2 e^{-st}\cdot 0dt + \int_2^5 e^{-st}\cdot 6dt </mrow>
										+ \int_5^{\infty} e^{-st}\cdot (-4)dt
							<mrow>=\amp\ 0 + 6\int_2^5 e^{-st}dt </mrow>
										- 4\lim_{b\to\infty}\int_5^b e^{-st}dt
							<mrow>=\amp\ -\frac{6}{s}e^{-st}\Big|_2^5 </mrow>
										- 4\lim_{b\to\infty}\int_5^b e^{-st}dt, 
										s gt 0
							<mrow>=\amp\ -\frac{6}{s}\left[e^{-s\cdot 5} - e^{-s\cdot 2}\right]</mrow>
									+ 4\lim_{b\to\infty}\frac{1}{s}e^{-st}\Big|_5^b,
									s gt 0	
							<mrow>=\amp\ -\frac{6e^{-5s}}{s} + \frac{6e^{-2s}}{s}</mrow>
									+ 4\lim_{b\to\infty}\frac{1}{s}\left[ e^{-s\cdot b} - e^{-s\cdot 5} \right],
									s gt 0	
							<mrow>=\amp\ -\frac{6e^{-5s}}{s} + \frac{6e^{-2s}}{s}</mrow>
									+ \frac{4}{s}\left[ \lim_{b\to\infty}e^{-sb} 
												- \lim_{b\to\infty}e^{-5s} \right],
									s gt 0	
							<mrow>=\amp\ -\frac{6e^{-5s}}{s} + \frac{6e^{-2s}}{s}</mrow>
									+ \frac{4}{s}\left[ 0 - e^{-5s} \right],
									s gt 0	
							<mrow>=\amp\ -\frac{6e^{-5s}}{s} + \frac{6e^{-2s}}{s} - \frac{4e^{-5s}}{s},</mrow>
									s gt 0	
							<mrow>=\amp\ \frac{6e^{-2s}}{s} - \frac{10e^{-5s}}{s},  s \gt 0	</mrow>
						</md>
					</li>
					<li>
						If we put together the results from the last two questions, we have
						<me> \lap{ 6\ U(t-2) - 10\ U(t-5) } = \frac{6e^{-2s}}{s} - \frac{10e^{-5s}}{s}. </me>
						Based on this, we can surmise the following property for Laplace transforms:
						<me> \lap{ U(t-a) } = \frac{e^{-as}}{s}. </me>
					</li>
				</ol>
			</p>
		</solution>
	</example>

	<p>
		We will add this property and a couple more to our table of Laplace transforms. These properties (<xref ref="LT-Table-L14-L16" text="custom"><m>L14</m> through <m>L16</m></xref>) will be added to the bottom of the table we used previously.
	</p>

	<p>
		<em> Table of Laplace Transforms</em> 
		<me>
			\begin{array}{|c|c|c|}
			\hline
								\amp f(t) 								\amp \lap{ f(t) } 	\amp 	\text{Condition/Notes}\\
			\hline
			\hline
			\text{L1}	\amp 1									\amp \ds \frac{1}{s}	\amp 	s>0\\
			\hline
			\text{L2}	\amp e^{at}								\amp \ds \frac{1}{s-a}	\amp 	s>a\\
			\hline
			\text{L3}	\amp t^n, \hspace{0.25cm}n = 1, 2, \ldots		\amp \ds \frac{n!}{s^{n+1}}	\amp 	s>0\\
			\hline
			\text{L4}	\amp \sin (bt)							\amp \ds \frac{b}{s^2 + b^2}	\amp 	s>0\\
			\hline
			\text{L5}	\amp \cos(bt)							\amp \ds \frac{s}{s^2 + b^2}	\amp 	s>0\\
			\hline
			\text{L6}	\amp t^n e^{at},  \hspace{0.25cm}n = 1, 2, \ldots	\amp \ds \frac{n!}{(s-a)^{n+1}}	\amp 	s>a\\
			\hline
			\text{L7}	\amp e^{at} \sin(bt)						\amp \ds \frac{b}{(s-a)^2 + b^2}	\amp 	s>a\\
			\hline
			\text{L8}	\amp e^{at} \cos(bt)						\amp \ds \frac{s-a}{(s-a)^2 + b^2}	\amp 	s>a\\
			\hline
			\text{L9}	\amp \alpha f(t) + \beta g(t)					\amp \ds \alpha \lap{ f(t) } + \beta \lap{ g(t) }	\amp 	 \alpha, \beta \text{ constant}\\
			\hline
			\text{L10}	\amp f'(t)								\amp s\lap{ f(t) } - f(0)	\amp 	\\
			\hline
			\text{L11}	\amp f''(t)								\amp s\lap{ f'(t) } - f'(0)	\amp 	\\
			\hline
			\text{L12}	\amp f^{(n)}(t)							\amp s\lap{ f^{(n-1)}(t) } - f^{(n-1)}(0)	\amp 	\\
			\hline
			\text{L13}	\amp t^n f(t)							\amp \ds (-1)^n\frac{d^n}{ds^n}\big( \lap{ f(t) } \big)	\amp 	\\
			\hline
			\text{L14.}	\amp U(t-a)								\amp \ds  \frac{e^{-as}}{s}\amp 	\\
			\hline
			\text{L15.}	\amp \ds f(t) U(t-a)						\amp \ds e^{-as} \lap{ f(t+a) }\amp 	\\
			\hline
			\text{L16.}	\amp \ds f(t-a)U(t-a)						\amp \ds e^{-as}F(s)\amp 	\\
			\hline
			\hline
			\end{array}
		</me>
	</p>

	<p>
		Let's practice using the new properties that have been added to the table for	Laplace transforms involving unit step functions.
	</p>

	<example xml:id="ex_lt_of_pw_func">
		<p>
			Find the Laplace transform of the function
			<me> q(t) = 3\ U(t-7) + t^2 U(t-4) </me>
		<p/>
		
		</p>
		<solution>
			<p>
				We will need to use linearity and then properties <xref ref="LT-Table-L14" text="custom"><m>L14</m></xref> and <xref ref="LT-Table-L15" text="custom"><m>L15</m></xref>.  We begin as	follows.
				<md>
					<mrow>Q(s)	=\amp\ \lap{ q(t) }</mrow>
					<mrow>=\amp\ \lap{  3\ U(t-7) + t^2 U(t-4) }</mrow>
					<mrow>=\amp\ 3\lap{ U(t-7) } + \lap{ t^2 U(t-4) }</mrow>
					<mrow>=\amp\ 3\cdot \frac{e^{-7s}}{s} + \lap{ t^2 U(t-4) }</mrow>
				</md>

			</p>

			<p>
				(Point out common mistake here??  In the margin??)
			</p>

			<p>
				For the second term, we need to use  <xref ref="LT-Table-L15" text="custom"><m>L15</m></xref>, with <m>f(t) = t^2</m> and <m>a = 4</m>. Then we have
				<md>
					<mrow>Q(s)	=\amp\ 3\cdot \frac{e^{-7s}}{s} + \lap{ t^2 U(t-4) },</mrow>
					<mrow>=\amp\ 3\cdot \frac{e^{-7s}}{s} + e^{-4s} \lap{ f(t+4) }.</mrow>
				</md>
			</p>

			<p>
				We aren't done yet, because we still need to evaluate <m>\lap{ f(t+4) }.</m>  First, since <m>f(t) = t^2,</m> then we know that 
				<md>
					<mrow>f(t+4)	=\amp\ (t+4)^2,</mrow>
					<mrow>=\amp\ t^2 + 8t + 16.</mrow>
				</md>
			</p>

			<p>
				We need to take the Laplace transform of this function; we will use linearity and properties <xref ref="LT-Table-L1" text="custom"><m>L1</m></xref> and <xref ref="LT-Table-L3" text="custom"><m>L3</m></xref>.  We continue below.
				<md>
					<mrow>Q(s)	=\amp\ 3\cdot \frac{e^{-7s}}{s} + e^{-4s} \lap{ f(t+4) }</mrow> 
					<mrow>=\amp\ 3\cdot \frac{e^{-7s}}{s} + e^{-4s} \lap{ t^2 + 8t + 16 } </mrow>
					<mrow>=\amp\ 3\cdot \frac{e^{-7s}}{s} + e^{-4s} \Big[ \lap{ t^2 } + 8\lap{ t } + 16\lap{ 1 } \Big]</mrow>
					<mrow>=\amp\ 3\cdot \frac{e^{-7s}}{s} + e^{-4s} \left[ \frac{2}{s^3} + \frac{8}{s^2} + \frac{16}{s} \right]</mrow>
				</md>
			</p>
		</solution>
	</example>

	<example xml:id="ex_lt_of_exp_times_u">
		<p>
			Evaluate <m>\lap{ e^{5t} U(t-6)}.</m>
		<p/>
		
		</p>
		<solution>
			<p>
				Here we will use  <xref ref="LT-Table-L15" text="custom"><m>L15</m></xref>, with <m>f(t) = e^{5t}</m> and <m>a = 6.</m>
				<md>
					<mrow>\lap{ e^{5t} U(t-6) }	=\amp\ e^{-6s}\lap{ f(t+6) }</mrow>
					<mrow>=\amp\ e^{-6s}\lap{ e^{5(t+6)} }</mrow>
					<mrow>=\amp\ e^{-6s}\lap{ e^{5t+30} }</mrow>
					<mrow>=\amp\ e^{-6s}\lap{ e^{5t}\cdot e^{30} }</mrow>
					<mrow>=\amp\ e^{-6s}e^{30}\lap{ e^{5t} }</mrow>
					<mrow>=\amp\ e^{-6s}e^{30}\cdot \frac{1}{s-5}</mrow>
					<mrow>=\amp\ \frac{e^{-6s + 30}}{s-5}</mrow>
				</md>
			</p>
		</solution>
	</example>

	<p>
		So far we have been taking Laplace transforms of functions involving unit step functions, and we have used properties <xref ref="LT-Table-L14" text="custom"><m>L14</m></xref> and <xref ref="LT-Table-L15" text="custom"><m>L15</m></xref>.  We will use  <xref ref="LT-Table-L16" text="custom"><m>L16</m></xref> for inverse Laplace transforms involving unit step functions.
	</p>

	<example xml:id="ex_ilt_of_exp_over_s_power">
		<p>
			Find the inverse Laplace transform of
			<me> X(s) = \frac{e^{-2s}}{s^3}. </me>
		<p/>
		
		</p>
		<solution>
			<p>
				We have a function of <m>s</m> that contains an exponential, and we want to find the inverse Laplace transform.  The presence of the exponential is a cue that we will be dealing with unit step functions.  In particular, we will use <xref ref="LT-Table-L16" text="custom"><m>L16</m></xref>. First it may be easier for us to rewrite <m>X(s)</m> as
				<md>
					<mrow>X(s)	=\amp\ e^{-2s}\cdot \frac{1}{s^3}</mrow>
					<mrow>=\amp\ e^{-2s}\cdot F(s)</mrow>
				</md>
			</p>

			<p>
				where <m>\ds F(s) = \frac{1}{s^3}.</m>  Now we can apply  <xref ref="LT-Table-L16" text="custom"><m>L16</m></xref> with  <m>a = 2</m>.
				<md>
					<mrow>x(t)	=\amp\ \lap^{-1}\left\{ X(s) \right\}</mrow>
					<mrow>=\amp\ \lap^{-1}\left\{ \frac{e^{-2s}}{s^3} \right\}</mrow>
					<mrow>=\amp\ \lap^{-1}\left\{ e^{-2s}\cdot \frac{1}{s^3} \right\}</mrow>
					<mrow>=\amp\ f(t-2)\cdot U(t-2)</mrow>
				</md>
			</p>

			<p>
				We know exactly what the function <m>U(t-2)</m> is; but we don't yet know what <m>f(t-2)</m> is.  We do know the function <m>F(s),</m> and therefore we need to take the inverse Laplace transform of <m>F(s)</m> to find the function <m>f(t).</m>
				<md>
					<mrow>f(t)	=\amp\ \lap^{-1}\left\{ F(s) \right\}</mrow>
					<mrow>=\amp\ \lap^{-1}\left\{ \frac{1}{s^3} \right\}</mrow>
					<mrow>=\amp\ \frac{1}{2} \lap^{-1}\left\{ \frac{2}{s^3} \right\}</mrow>
					<mrow>=\amp\ \frac{1}{2}t^2</mrow>
				</md>
			</p>

			<p>
				Now that we know the function <m>f(t),</m> we are prepared to finish assembling our answer.
				<md>
					<mrow>x(t)	=\amp\ f(t-2)\cdot U(t-2)</mrow>
					<mrow>=\amp\ \frac{1}{2}(t-2)^2 \cdot U(t-2)</mrow>
				</md>
			</p>
		</solution>
	</example>

	<example xml:id="ex_ilt_of_exp_over_sum_of_sqrs">
		<p>
			Find the inverse Laplace transform of
			<me> A(s) = \frac{e^{-3s}}{s^2 + 16}. </me>
		<p/>
		
		</p>
		<solution>
			<p>
				The cue that we need to use <xref ref="LT-Table-L16" text="custom"><m>L16</m></xref> when taking an inverse Laplace transform is the presence of an exponential.  We can rewrite <m>A(s)</m> as
				<md>
					<mrow>A(s)	=\amp\ e^{-3s}\cdot \frac{1}{s^2 + 16},</mrow>
					<mrow>=\amp\ e^{-3s}\cdot F(s),</mrow>
				</md>
			</p>

			<p>
				where <m>\ds F(s) = \frac{1}{s^2 + 16}.</m>  This form aligns with  <xref ref="LT-Table-L16" text="custom"><m>L16</m></xref>, using <m>a = 3</m>, and we can proceed to take the inverse Laplace transform as follows.
				<md>
					<mrow>a(t)	=\amp\ \lap^{-1}\left\{ A(s) \right\}</mrow>
					<mrow>=\amp\ \lap^{-1}\left\{ \frac{e^{-3s}}{s^2 + 16} \right\}</mrow>
					<mrow>=\amp\ \lap^{-1}\left\{ e^{-3s}\cdot \frac{1}{s^2 + 16} \right\}</mrow>
					<mrow>=\amp\ f(t - 3)\cdot U(t-3)</mrow>
				</md>
			</p>

			<p>
				We are not done yet; the function <m>U(t-3)</m> is well-defined, but we don't yet know what <m>f(t-3)</m> is.  Recall that <m>\ds F(s) = \frac{1}{s^2 + 16}.</m>  First we can find <m>f(t)</m> by taking the inverse Laplace transform of <m>F(s).</m>
				<md>
					<mrow>f(t)	=\amp\ \lap^{-1}\{ F(s) \}</mrow>
					<mrow>=\amp\ \lap^{-1}\{ \frac{1}{s^2 + 16} \}</mrow>
					<mrow>=\amp\ \lap^{-1}\{ \frac{1}{s^2 + 4^2} \}</mrow>
					<mrow>=\amp\ \frac{1}{4}\cdot \lap^{-1}\{ \frac{4}{s^2 + 4^2} \}</mrow>
					<mrow>=\amp\ \frac{1}{4}\sin(4t)</mrow>
				</md>
			</p>

			<p>
				Now that we know <m>f(t),</m> we are prepared to evaluate <m>f(t-3).</m>
				<md>
					<mrow>a(t)	=\amp\ f(t - 3)\cdot U(t-3)</mrow>
					<mrow>=\amp\ \frac{1}{4}\sin\big(4(t-3)\big) \cdot U(t-3)</mrow>
				</md>
			</p>
		</solution>
	</example>

	<example xml:id="ex_ilt_of_s_exp_over_quadratic">
		<p>
			Find the inverse LT of 
			<me> Y(s) = \frac{se^{-7s}}{s^2 + 4s + 5} </me>
		<p/>
		
		</p>
		<solution>
			<p>
				It may be easiest for us to rewrite <m>Y(s)</m> before we begin, as
				<md>
					<mrow>Y(s)	=\amp\  e^{-7s}\cdot \frac{s}{s^2 + 4s + 5},</mrow>
					<mrow>=\amp\ e^{-7s}F(s),</mrow>
				</md>
			</p>

			<p>
				where <m>F(s) = \ds  \frac{s}{s^2 + 4s + 5}.</m>  Since we have done several examples like this one, we know that we will need to find the inverse Laplace transform of <m>F(s),</m> so let's find that now.  This will require some algebraic manipulation as we saw in (name the section here).
				<md>
					<mrow>f(t)	=\amp\ \lap^{-1}\left\{ F(s) \right\}</mrow>
					<mrow>=\amp\ \lap^{-1}\left\{ \frac{s}{s^2 + 4s + 5} \right\}</mrow>
					<mrow>=\amp\ \lap^{-1}\left\{ \frac{s}{(s^2 + 4s + 4) + 5 - 4} \right\}</mrow>
					<mrow>=\amp\ \lap^{-1}\left\{ \frac{s}{(s+2)^2 + 1} \right\}</mrow>
					<mrow>=\amp\ \lap^{-1}\left\{ \frac{(s+2) - 2}{(s+2)^2 + 1^2} \right\}</mrow>
					<mrow>=\amp\ \lap^{-1}\left\{ \frac{s+2}{(s+2)^2 + 1^2} - 2\cdot \frac{1}{(s+2)^2 + 1^2}  \right\}</mrow>
					<mrow>=\amp\ \lap^{-1}\left\{ \frac{s+2}{(s+2)^2 + 1^2} \right\} - 2\cdot \lap^{-1}\left\{\frac{1}{(s+2)^2 + 1^2}  \right\}</mrow>
					<mrow>=\amp\ e^{-2t}\cos(t) - 2e^{-2t}\sin(t)</mrow>
				</md>
			</p>

			<p>
				Now we return to the question at hand: finding the inverse Laplace transform of <m>Y(s).</m>
				<md>
					<mrow>y(t)	=\amp\ \lap^{-1}\left\{ Y(s) \right\}</mrow>
					<mrow>=\amp\ \lap^{-1}\left\{ e^{-7s}F(s) \right\}</mrow>
					<mrow>=\amp\ f(t-7)\cdot U(t-7)</mrow>
					<mrow>=\amp\ \Big[e^{-2(t-7)}\cos(t-7) - 2e^{-2(t-7)}\sin(t-7)\Big]\cdot U(t-7)</mrow>
				</md>
			</p>
		</solution>
	</example>

	<xi:include href="./c4-s5-ss2-interactives.ptx" />

</subsection>