<section><title> Additional Examples </title>

    <introduction>
        <p>
            This is just a place to store extra examples which may or may not be used.
        </p>
    </introduction>

	<example xml:id="two-constant-solution-verification"><title> <em>Solution Verification with Two Constants</em> </title>
		<p>
			Verify that <m>y = \frac{1}{2}x^2 + c_1 x + c_2</m> is a solution to <m>\quad y'' = 1</m>.
		</p>
	
		<solution>

			<p>
				<xref ref="solution-verification-step-1" text="title"/>: <m>\quad y'' - 1 = 0</m>
			</p>
	
			<p>
				<xref ref="solution-verification-step-2" text="title"/>. Find <m>y''</m> since it appears in the DE.
				<md>
					<mrow>	y	\amp=  \frac{1}{2}x^2 + c_1 x + c_2									</mrow>
					<mrow>	y' 	\amp=  x + c_1													</mrow>
					<mrow>	y'' \amp=  1														</mrow>
				</md>
			</p>
			<p>
				<xref ref="solution-verification-step-3" text="title"/>. Plug <m>y''</m> into the DE and simplify.
				<md>
					<mrow> 	y'' - 1	\amp= 0	</mrow>
					<mrow> 	1 - 1	\amp= 0	</mrow>
					<mrow> 		0	\amp= 0	</mrow>
				</md>
				Therefore, <m>y = \frac{1}{2}x^2 + c_1 x + c_2</m> is a solution to <m>y'' = 1</m>. 
				<fn>
					In fact, it is the general solution, but we don't show that here. 
				</fn>
			</p>
	
		</solution>
	
	</example>

	<example>
	
		<p>
		Solve <me> y'' - y' - 12y = 0, \quad y(0) = 4, \quad y'(0) = -2. </me>
		</p>
	
		<solution>
	
		<p>
			The general solution to this DE was already found  to be
			<me>y = c_1e^{-3t} + c_2e^{4t}</me>.
			Notice that two initial conditions are provided in this example. This extra piece of information is needed since our general solution contains two constants.
		</p>
	
		<p>
			Since one initial condition involves the derivative, we will need to compute this before applying this condition.
			<me>y' = -3c_1e^{-3t} + 4c_2e^{4t}.</me>
		</p>
	
		<p>
			Now let's apply the initial conditions:
			<md>
			<mrow>y(0)	\amp= 4		\amp\Rightarrow \hspace{0.2cm} 	4
				\amp= c_1e^{-3\cdot 0} + c_2e^{4\cdot 0}</mrow>
			<mrow>			\amp	\amp	4
				\amp= c_1 + c_2		</mrow>
			<mrow>			\amp	\amp	\amp	</mrow>
			<mrow>y'(0)	\amp= -5	\amp\Rightarrow \hspace{0.2cm} 	-5
				\amp=-3c_1e^{-3\cdot} + 4c_2e^{4\cdot}	</mrow>
			<mrow>			\amp	\amp	-5	\amp= -3c_1 + 4c_2	</mrow>
			</md>
		</p>
	
		<p>
			We now have two equations and two unknowns,
			<md>
			<mrow>	 c_1 +  c_2	\amp=	4 	</mrow>
			<mrow> -3c_1 + 4c_2	\amp= -5 	</mrow>
			</md>
			There are multiple ways to solve this system of equations, and the reader is encouraged to verify that	<m>c_1 = 3</m> and <m>c_2 = 1</m>. Here is one
	
			<solution>
	
			We will solve for <m>c_2</m> in the first equation and then
			substitute into the second.
			<md>
				<mrow>4					\amp= c_1 + c_2										</mrow>
				<mrow>\Rightarrow c_2	\amp= 4 - c_1								</mrow>
				<mrow>					\amp															</mrow>
				<mrow>-5				\amp= -3c_1 + 4c_2								</mrow>
				<mrow>\Rightarrow -5	\amp= -3c_1 + 4(4 - c_1)		</mrow>
				<mrow>-5				\amp= -3c_1 + 16 - 4c_1						</mrow>
				<mrow>-21				\amp= -7c_1												</mrow>
				<mrow>3					\amp= c_1													</mrow>
				<mrow>					\amp															</mrow>
				<mrow>c_2				\amp=4 - c_1											</mrow>
				<mrow>					\amp= 4 - 3												</mrow>
				<mrow>					\amp= 1														</mrow>
			</md>
	
			</solution>
	
		</p>
	
		<p>
			Thus, the solution we that satisfies the DE and both of the provided initial conditions is	<me> y = 3e^{-3t} + e^{4t}. </me>
		</p>
	
		</solution>
	
	</example>

	<note><title> <em>Don't assume a function that satisfies a DE is a general solution!</em> </title>
		<p>
			A function that contains constants and satisfies a differential equation <em>does not mean it is the general solution</em> since it could be missing a term. For example, you could easily show that <m>y = \frac{1}{2}x^2 + c_1 x</m> is also a solution to 
			<me>\quad y'' = 1</me>, 
			but you already know from <xref ref="two-constant-solution-verification"/> that <m>y = \frac{1}{2}x^2 + c_1 x + c_2</m> is a solution, which is more general than <m>y = \frac{1}{2}x^2 + c_1 x</m>.
		</p>
	</note>
	
	<example>
	
		<p>
			Verify that <m>\DS y = Ce^{x^2} + 3</m>, where <m>C</m> is any constant, is a solution to the DE
			<me>\DS \frac{dy}{dx} = 2xy - 6x.</me>
		</p>
	
		<solution>
	
			<p>
				We'll approach this the same way we approached the algebraic equation in the example above: we will to substitute the function <m>\DS y = Ce^{x^2} + 3</m> in on the left and right hand sides of the equation
		
				<sidebyside widths="45% 55%" margins="auto" valign="top" halign="center">
					<p>
						<md>
						<mrow> \overset{LHS\vphantom{\Big|}}{\frac{dy}{dx}}
							\amp=\frac{d}{dx}\left( Ce^{x^2} + 3 \right)</mrow>
						<mrow> 	\amp= C\frac{d}{dx}\left( e^{x^2} \right) + \frac{d}{dx}\left( 3 \right)</mrow>
						<mrow> 	\amp= C \cdot e^{x^2} \cdot \frac{d}{dx}\left( x^2 \right) + 0</mrow>
						<mrow> 	\amp=  C \cdot e^{x^2} \cdot 2x</mrow>
						<mrow> 	\amp=  2Cxe^{x^2}</mrow>
						</md>
					</p>
					<p>
						<md>
						<mrow> 	\overset{RHS\vphantom{\Big|}}{2xy - 6x}
							\amp= 2x \left( Ce^{x^2} + 3 \right) - 6x</mrow>
						<mrow> 	\amp= 2Cxe^{x^2} + 6x - 6x</mrow>
						<mrow> 	\amp= 2Cxe^{x^2}</mrow>
						</md>
					</p>
				</sidebyside>
		
				Since both the <m>LHS</m> and <m>RHS</m> turn out to be	<m>2Cxe^{x^2}</m>, we have shown that <m>\DS y = Ce^{x^2} + 3</m> satisfies and is, thus, a	solution to	<m>\DS \frac{dy}{dx} = 2xy - 6x.</m>
			</p>
	
		</solution>
	
	</example>

	<note><title>Example Notes</title>
	
		<p>
			Since we used a generic constant <m>C</m>, we have shown that <m>\DS y = Ce^{x^2} + 3</m> is a solution for any value we like for the constant <m>C</m>. In particular,
			<ul>
			<li>for <m>C=-41, \quad y = -41e^{x^2} + 3 \quad</m> is a solution.</li>
			<li>for <m>C=199, \quad y = 199e^{x^2} + 3 \quad</m> is a solution.</li>
			<li>for <m>C=0, \quad y = 3 \quad</m> is a solution.</li>
			</ul>
			Since there is no limit to what <m>C</m> we can choose, this DE must have an infinite number of solutions. In the next section, we will describe this idea further.
		</p>
		
	</note>

	<example>
	
		<p>
			Determine if <m>y = c_1e^{-3t} + c_2e^{4t}</m> is a solution to the DE <m>y'' - y' - 12y = 0</m> where <m>c_1</m> and <m>c_2</m> are constants.
		</p>
	
		<solution>

			<p>
				Find <m>y, y', \text{ and } y''</m>.
				<md>
					<mrow>y		\amp= c_1e^{-3t} + c_2e^{4t} \hspace{-0.4cm}
						\amp\Rightarrow\hspace{0.1cm}
						y'	\amp= -3c_1e^{-3t} + 4c_2e^{4t} \hspace{-0.4cm}
						\amp\Rightarrow\hspace{0.1cm}
						y''	\amp= 9c_1e^{-3t} + 16c_2e^{4t}
					</mrow>
				</md>
			</p>
		
			<p>
				and substitute
				<md>
					<mrow>LHS	\amp= y'' - y' - 12y										</mrow>
					<mrow>		\amp= \left(9c_1e^{-3t} + 16c_2e^{4t}\right)
						- \left( -3c_1e^{-3t} + 4c_2e^{4t} \right)
						- 12\left( c_1e^{-3t} + c_2e^{4t} \right)				</mrow>
					<mrow>		\amp= 9c_1e^{-3t} + 16c_2e^{4t} + 3c_1e^{-3t}
						- 4c_2e^{4t} - 12c_1e^{-3t} - 12c_2e^{4t}			</mrow>
					<mrow>		\amp= \left( 9c_1e^{-3t} + 3c_1e^{-3t} - 12c_1e^{-3t} \right)
						+ \left( 16c_2e^{4t} - 4c_2e^{4t} - 12c_2e^{4t} \right)	</mrow>
					<mrow>		\amp = 0													</mrow>
					<mrow>		\amp= RHS													</mrow>
				</md>
				Which shows that <m>y = c_1e^{-3t} + c_2e^{4t}</m> is a solution to <m>y'' - y' - 12y = 0.</m>
			</p>
	
		</solution>
	
	</example>
	
	<note><title>Example Notes</title>
	
		<p>
			In this example, we showed that the function <m>y = c_1e^{-3t} + c_2e^{4t}</m> was a solution <m>y'' - y' - 12y = 0</m>.
		</p>
	
		<p>
			Notice that we were able to verify the solution, even though the constants, <m>c_1</m> and <m>c_2</m>, were not known. This suggests that you can substitute any values of <m>c_1</m> and <m>c_2</m> into the solution and it will still be a solution to the DE. <em> Try it! </em>
		</p>
	
		<p>
			Now, since there are infinitely many choices for <m>c_1</m> and <m>c_2</m>,	then, logically, there must be infinitely many solutions to the DE,	<m>y'' - y' - 12y = 0</m>.
		</p>
		
	</note>

	<example>
	
		<statement>
			<p>
				Verify that <m>y = Ce^{-5x^2} + \frac{3}{5}</m> is a solution to the DE
				<me>\frac{dy}{dx} = \big( 2x \big) \big( 3 - 5y \big)</me>
			</p>
		</statement>
	
		<solution>
			<p>
				Working out the left and right hand sides of this DE, we have:
	
				<sidebyside widths="45% 55%" margins="auto" valign="top" halign="center">
					<p>
						<md>
							<mrow> LHS: </mrow>
							<mrow> \frac{dy}{dx}
									\amp=\frac{d}{dx}\left( Ce^{-5x^2} + \frac{3}{5} \right)</mrow>
							<mrow> 	\amp= Ce^{-5x^2} \cdot \frac{d}{dx}(-5x^2) + 0</mrow>
							<mrow> 	\amp= Ce^{-5x^2} \cdot -10x</mrow>
							<mrow> 	\amp= -10Cxe^{-5x^2}</mrow>
						</md>
					</p>
					<p>
						<md>
							<mrow> RHS: </mrow>
							<mrow> 	\big(2x\big)\amp\big(3 - 5y\big)</mrow>
							<mrow> 	\amp= 2x \left[3 - 5\left(Ce^{-5x^2} + \frac{3}{5}\right) \right]</mrow>
							<mrow> 	\amp= 2x \left[ 3 - 5Ce^{-5x^2} - 3 \right]</mrow>
							<mrow> 	\amp= 2x \left[-5Ce^{-5x^2}\right]</mrow>
							<mrow> 	\amp= -10Cxe^{-5x^2}</mrow>
						</md>
					</p>
				</sidebyside>
			</p>
	
			<p>
				Since <m>LHS = RHS</m>, we have verified that
				<m>y = Ce^{-5x^2} + \frac{3}{5}</m> is a solution to
				<me>\frac{dy}{dx} = \big( 2x \big) \big( 3 - 5y \big)</me>
			</p>
			
		</solution>
	
	</example>

</section>