
	<section xmlns:xi="http://www.w3.org/2001/XInclude"><title> Summary &amp; Exercises </title>

	<introduction>
		<assemblage><title>Solving Initial Value Problems</title>
		<p>
			For most of the techniques in this book, solving an initial value problem requires two main steps:
			<ol marker="1.">
			<li>
				Solve for the general solution (with constants).
			</li>
			<li>
				Compute the constants in the general solution using the initial conditions.
			</li>
			</ol>
		</p>
		</assemblage>
		
		<p>
			In this section and in the exercises that follow, we will be only concerned with step 2. So don't worry if you do not understand where these general solutions come from. In chapter 2, we will look at our first technique for solving a differential equation.
		</p>

		<p>
			<assemblage color="green"><title>Summary of the Key Ideas</title>
				<p>
					<ul marker="">
						<li xml:id="summary-solution">
							<term> <em>Solution of a Differential Equation</em> </term>
							<ul marker="square">
								<li></li>
							</ul>
						</li>
						<li xml:id="summary-verifying-solutions"> 
							<term> <em>Verifying a function is a Solution</em> </term>
							<ul marker="square">
								<li></li>
							</ul>
						</li>
						<li xml:id="summary-types-of-solutions"> 
							<term> <em>Types of Solutions</em> </term>
							<ul marker="square">
								<li></li>
							</ul>
						</li>
						<li xml:id="summary-initial-conditions"> 
							<term> <em>Initial Conditions</em> </term>
							<ul marker="square">
								<li></li>
							</ul>
						</li>
					</ul>
				</p>
			</assemblage>
		</p>

		<p>
			To prepare you for this discussion, let's review a few important points of the previous section that will be useful in this section.
			<ul>
			<li>
				The general solution of a differential equation contains a certain number of constants.
			</li>
			<li>
				All different combinations of these constants give you the collection of possible solutions we called a family of solutions.
			</li>
			<li>
				Specific values for the constants produces a particular solution.
			</li>
			</ul>
		</p>
		
		
		<remark xml:id="sect-01-04-01-remark-01">
			<p>
			Typically, the number of constants present in the general solution is equal to the order of the differential equation<m>^{1}</m>.
			</p>
			<p>
			This is illustrated in ? since <m>y'' - y' - 12y = 0</m> is of 2nd order and the general solution, <m>y = c_1e^{-3t} + c_2e^{4t}</m>, has 2 constants, <m>c_1</m> and <m>c_2</m>.
			</p>
		</remark>
		
		<aside>
			<p>
			<m>^{1}</m> There are some exceptions when working with nonlinear DEs.
			</p>
		</aside>
		
	</introduction>

	<exercises>

		<exercise>
			<p>
				Discuss the difference between a general solution, family of solutions,
				and a particualr solution.
			</p>
		</exercise>
		
		<exercise>
			<p>
				Given the differential equation
					<me> y''-9y = 0 </me>
					determine if the following functions are solutions of this differential
				equation.
			</p>
			<p>
				<sidebyside width="30%">
					<p>
						<line> a. <m>\DS \,\, y = 3</m> </line>
						<line> b. <m>\DS \,\, y = 0</m> </line>
						<line> c. <m>\DS \,\, y = e^{3x}</m> </line>
					</p>
					<p>
						<line> d. <m>\DS \,\, y = 3x</m> </line>
						<line> e. <m>\DS \,\, y = 9e^x</m> </line>
						<line> f. <m>\DS \,\, y = x^9</m> </line>
					</p>
					<p>
						<line> g. <m>\DS \,\, y = 4e^{3x}</m> </line>
						<line> h. <m>\DS \,\, y = e^{-3x}</m> </line>
						<line> i. <m>\DS \,\, y = e^{3x} - 2e^{-3x}</m> </line>
					</p>
				</sidebyside>
			</p>

			<answer>
				<sidebyside width="30%">
					<p>
						<line> a. No </line>
						<line> b. Yes </line>
						<line> c. Yes </line>
					</p>
					<p>
						<line> d. No </line>
						<line> e. No </line>
						<line> f. No </line>
					</p>
					<p>
						<line> g. Yes </line>
						<line> h. Yes </line>
						<line> i. Yes </line>
					</p>
				</sidebyside>
			</answer>
		</exercise>
		
		<exercise>
			<p>
				Given the differential equation
				<me> y'' - 10y' + 25y = 0 </me>
				determine if the following functions are solutions of this differential	equation.
			</p>
			<p>
				<sidebyside width="30%">
					<p>
						<line> a. <m>\DS \,\, y = 0</m> </line>
						<line> b. <m>\DS \,\, y = x^2e^{5x}</m> </line>
						<line> c. <m>\DS \,\, y = e^{5x}</m> </line>
					</p>
					<p>
						<line> d. <m>\DS \,\, y = 5x</m> </line>
						<line> e. <m>\DS \,\, y = xe^{5x}</m> </line>
						<line> f. <m>\DS \,\, y = 5e^{5x}</m> </line>
					</p>
					<p>
						<line> g. <m>\DS \,\, y = 1/25</m> </line>
						<line> h. <m>\DS \,\, y = e^{-5x}</m> </line>
						<line> i. <m>\DS \,\, y = (1+x)e^{5x}</m> </line>
					</p>
				</sidebyside>
			</p>
		
			<answer>
				<p>
					<sidebyside width="30%">
						<p>
							<line> a. Yes </line>
							<line> b. No </line>
							<line> c. Yes </line>
						</p>
						<p>
							<line> d. No </line>
							<line> e. Yes </line>
							<line> f. Yes </line>
						</p>
						<p>
							<line> g. No </line>
							<line> h. No </line>
							<line> i. Yes </line>
						</p>
					</sidebyside>
				</p>
			</answer>
		</exercise>
		
		<exercise>
			<p>
				Match each function on the left with a DE on the right if this function is a solution (i.e. is in the family of solutions) for this DE.
			
				<sidebyside widths="40% 40%">
					<p>
						<ol marker="\(A.\)">
							<li> <m>y = 3x+x^2</m>	</li>
							<li> <m>y = e^{-8x}</m>	</li>
							<li> <m>y = \sin x</m>	</li>
							<li> <m>y = x^{1/2}</m>	</li>
							<li> <m>y = 6e^{8x}</m>	</li>
						</ol>
					</p>
					<p>
						<ul marker="">
							<li> <m>\fbox{\(\phantom{D}\)} \quad 2x^2y'' + 3xy' = y</m>				</li>
							<li> <m>\fbox{\(\phantom{B}\)} \quad y'' + 10 y' + 16 y = 0</m>			</li>
							<li> <m>\fbox{\(\phantom{E}\)} \quad y' = 8 y</m>						</li>
							<li> <m>\fbox{\(\phantom{C}\)} \quad y'' + y = 0</m>					</li>
							<li> <m>\fbox{\(\phantom{A}\)} \quad 3y'' - 2y + \frac{4}{x}y = 12</m>	</li>
						</ul>
					</p>
				</sidebyside>
			</p>
		
			<answer>
				<ul marker="">
					<li> <m>\fbox{\(D\)} \quad  2x^2y'' + 3xy' = y</m> 				</li>
					<li> <m>\fbox{\(B\)} \quad  y'' + 10 y' + 16 y = 0</m> 			</li>
					<li> <m>\fbox{\(E\)} \quad  y' = 8 y</m> 						</li>
					<li> <m>\fbox{\(C\)} \quad  y'' + y = 0</m> 					</li>
					<li> <m>\fbox{\(A\)} \quad  3y'' - 2y + \frac{4}{x}y = 12</m>	</li>
				</ul>
			</answer>
		</exercise>
		
		<exercise>
			<p>
				Find all values of <m>r</m> such that <m>y=e^{rx}</m> is a solution to
				<me>y''' - 10y'' + 24y' = 0</me>.
			</p>
			
			<answer>
				<m>r = 0, 6, 4</m>
			</answer>
		</exercise>
		
		<exercise>
			<p>
				Find all values of <m>r</m> such that <m>y = k e^{rx}</m> is a solution	to
				<me>y'' - 25y = 0</me>.
			</p>
		
			<answer>
					<m>r = -5, 5</m>
			</answer>
		</exercise>
		
		<exercise>
			<p>
				Find all values of <m>r</m> such that <m>y(x) = c_1 e^{r x} + c_2</m> is a solution to
				<me>7y'' = 8y</me>.
			</p>
		
			<answer>
					<m>r = 8/7</m>
			</answer>
		</exercise>
		
		<exercise>
			<p>
				Find all values of <m>r</m> such that <m>y = t^{r}</m> is a solution to
				<me>t^{2}y''- 11ty' + 32y = 0 \quad (t>0)</me>.
			</p>
		
			<answer>
					<m>r = 4, 8</m>
			</answer>
		</exercise>
		
		<exercise>
			<p>
				Find all values of <m>r</m> such that <m>y = rx^{2}</m> is a solution to
				<me>y' = 5x</me>.
			</p>
		
			<answer>
				<m>r = 2.5</m>
			</answer>
		</exercise>
		
		<exercise>
			<p>
				Find all values of <m>r</m> such that <m>y = \sin(rt)</m> is a solution to
				<me>y'' + 9y = 0</me>.
			</p>
		
			<answer>
				<m>r = 2.5</m>
			</answer>
		</exercise>
		
		<exercise>
			<p>
				Find the value of the constant <m>k</m> in order for the differential equation
				<me> \frac{d^2y}{dt^2} - 8 \frac{dy}{dt} + ky = 0</me>
				to have the solution <m>y = e^{3t}</m>.
			</p>
		
			<answer>
				<m>k = 15</m>
			</answer>
		</exercise>
		
		<exercise>
			<p>
				Is <m>\DS y = c_{1}e^{2x} + c_{2}xe^{2x}</m> a solution of the
				differential equation
				<me>\DS \frac{d^{2}y}{dx^{2}} - 4\frac{dy}{dx} + 4y = 0?</me>
			</p>
		
			<answer>
					Yes
			</answer>
		</exercise>
			
		<exercisegroup><title> Find the value of <m>r</m> </title>
		
			<introduction>
				<p>
					For each of the differential equations and function pairs, find all the possible values of <m>r</m> such that the function is a solution to the DE.
				</p>
			</introduction>
			<exercise>
				<m>y''' - 10y'' + 24y' = 0; \quad y=e^{rx}</m>
				<answer>
					<m>r = 0, 6, 4</m>
				</answer>
			</exercise>
		
			<exercise>
				<m>y'' - 25y = 0; \quad y = k e^{rx}</m>
				<answer>
					<m>r = -5, 5</m>
				</answer>
			</exercise>
			
			<exercise>
				<m>7y'' = 8y; \quad y(x) = c_1 e^{r x} + c_2</m>
				<answer>
					<m>r = 8/7</m>
				</answer>
			</exercise>
			
			<exercise>
				<m>t^{2}y''- 11ty' + 32y = 0; \quad y = t^{r} \quad (t>0)</m>
				<answer>
					<m>r = 4, 8</m>
				</answer>
			</exercise>
			
			<exercise>
				Let <m>y' = 5x; \quad y = rx^{2}</m>
				<answer>
					<m>r = 2.5</m>
				</answer>
			</exercise>
			
			<exercise>
				<m>y'' + 9y = 0; \quad y = \sin(rt)</m>
				<answer>
					<m>r = 2.5</m>
				</answer>
			</exercise>
		
		</exercisegroup>

		<exercise>
			<p>
				Explain the significance of initial condition(s) as they relate to the general solution of a differential equation.
			</p>
			<answer>
				<line>
				The initial condition(s) specify one or more points that the graph of the
				solution must pass through. This often allows one to solve for the
				constants in the general solution.
				</line>
				<line>
				Therefore, the initial condition(s) act to reduce the
				family of solutions down to a smaller set of solutions or, ideally, a
				single particular solution.
				</line>
			</answer>
		</exercise>

		<exercise>
			<p>
				Does an initial condition always give you a particular solution?
			</p>
			<answer>
				<line>When there is one constant in the general solution, yes.</line>
				<line>When there is more than one constant in the general solution, no.<m>^{1}</m></line>
				<aside>
				It does, however, limit the possible values of the constants.
				</aside>
			</answer>
		</exercise>

		<exercise>
			<p>
				Consider the differential equation
				<me>x^2y' + xy = 1</me>
			<ol>
				<li>
					Verify that the family of functions
					<me>y = \frac{\ln x + C}{x}</me>
					a solution to this differential equation.
				</li>
				<li>
					Find the particular solution that corresponds to the initial condition <m>y(9)=8</m>.
				</li>
			</ol>
			</p>
			<answer>
				<line>Yes</line>
				<line>
					<m>C = 72-\ln(9) \approx 69.803</m>, so
					<m>\DS y = \frac{\ln x + 69.803}{x} </m> is the particular solution
				</line>
			</answer>
		</exercise>

		<exercise>
			<p>
				Consider the differential equation
				<me>y^\prime = y-y^2</me>
				Which of the following is a family of solutions for this DE?
					<ol>
						<li> <m>\DS y=c\sin(-x)</m></li>
						<li> <m>\DS y=\frac{1}{1+ce^{-x}}</m></li>
						<li> <m>\DS y=\frac{1}{c+x^2}</m></li>
					</ol>
				Find the particular solution such that <m>y(0) = 7</m>.
			</p>
			<answer>
				<line>b. <m>\DS y=\frac{1}{1+ce^{-x}}</m></line>
				<line>
				<m>c = \frac{1}{7}-1 \approx -0.857</m>, so
				<m>\DS y = \frac{1}{1+(-0.857)e^{-x}} </m> is the particular solution
				</line>
			</answer>

			<solution>
				<line>Try <m>y=\frac{1}{c+x^2}</m> first.</line>
				<line>Compute</line>
				<line> <m>y^\prime = \frac{-4x}{(c+x^2)^2}</m> </line>
				<line> <m>y-y^2 = \frac{1}{c+x^2} - \frac{1}{(c+x^2)^2}
								= \frac{c+x^2}{(c+x^2)^2} - \frac{1}{(c+x^2)^2}
								= \frac{c+x^2-1}{(c+x^2)^2}</m></line>
				<line>So <m>y^\prime\neq y-y^2</m> for this function, it is not the solution.</line>
				<line>Now try <m>y=\frac{1}{1+ce^{-x}}</m>. Then</line>

				<line><m>y^\prime = \frac{ce^{-x}}{1+ce^{-x}}</m></line>
				<line>while</line>
				<line><m>y-y^2=\frac{1}{1+ce^{-x}}-\frac{1}{(1+ce^{-x})^2}
							=\frac{1+ce^{-x}}{(1+ce^{-x})^2}-\frac{1}{(1+ce^{-x})^2}
							=\frac{ce^{-x}}{(1+ce^{-x})^2}</m></line>
				<line>So this function is the solution</line>
				<line>Setting <m>y(0)=$y0</m> we get</line>
				<line><m>$y0 = \frac{1}{1+c}</m></line>
				<line>Solve for c, <m>c = \frac{1}{$y0}-1=$c</m></line>
				<line>So the solution for the IVP is <m>y = \frac{1}{1+(-0.857)e^{-x}}</m></line>
			</solution>
		</exercise>
		
		<exercisegroup><title> Understanding what it means to Solve a DE </title>
			<introduction>
				<p>
					We spend a lot of time solving equations, but do you even remember what it means to be a solution? Let's review what it means to be a solution to an algebraic equation (as in question <xref ref="alg_eqn_soln"/>), and then what it means to be a solution to a differential equation (as in question <xref ref="diff_eqn_soln"/>), and then we'll extend those ideas in questions <xref ref="soln_form1"/> and <xref ref="soln_form2"/>.
				</p>
			</introduction>

			<exercise>
				<p>
					Verify that <m>x = 3</m> is a solution to the equation 
					
					<men xml:id="alg_eqn_soln">2x^2 + 3 = 7x.</men>
				
				</p>
			
				<p>
					What confirms that <m>x = 3</m> is a solution? 
					<answer>
					the LHS = RHS after substituting <m>x = 3</m> into both sides of the equation.
					</answer>	
				</p>
			
				<p>	
					(<em> Note: Do not rearrange the equation to solve for <m>x</m>. That would be the
					process of finding a solution; you are asked to verify a solution.</em>)
				</p>

				<solution>
					We substitute <m>x = 3</m> into the left hand side (LHS) of the equation, 
					and then into the right hand side (RHS) of the equation:
					
					<md>
						<mrow>\text{LHS}	\amp= 2x^2 + 3										</mrow>
						<mrow>				\amp= 2(3)^2 + 3									</mrow>
						<mrow>				\amp= 18 + 3										</mrow>
						<mrow>				\amp= 21											</mrow>
						<mrow>				\amp 												</mrow>
						<mrow>\text{RHS}	\amp= 7x											</mrow>
						<mrow>				\amp= 7(3)											</mrow>
						<mrow>				\amp= 21											</mrow>	
					</md>
					
					Since we get the same result when we substitute the solution into the RHS and 
					into the LHS, we have confirmed that <m>x = 3</m> is a solution to the equation.
				</solution>

				<!-- Is this answer necessary? -->
				<answer>
					Since we get the same result (21) when we substitute the solution into the 
					RHS and into the LHS, we confirm that <m>x = 3</m> is a solution to the equation.
				</answer>
			
			</exercise>

			<exercise>
				<p>
					Verify that <m>y = c_1 \sin x + c_2 \cos x</m> is a solution to the DE 
					<men xml:id="diff_eqn_soln">\DS \frac{d^2y}{dx^2} + y = 0.</men>
				</p>
				
				<hint>
					Look back at the previous question and think about what it means to be a solution to a DE.
				</hint>
				<solution>
					We need to substitute into the DE. In order to substitute into the left hand side, we need to know the second derivative. So we begin by finding that.
					
					<md>
					<mrow>						y	\amp= c_1 \sin x + c_2 \cos x			</mrow>
					<mrow>	\Rightarrow \quad   y'	\amp= c_1 \cos x - c_2 \sin x			</mrow>
					<mrow>	\Rightarrow \quad   y''	\amp= -c_1 \sin x - c_2 \cos x			</mrow>	
					</md>
					
					Now we can substitute into the DE:
					
					<md>
					<mrow>\text{LHS}\amp= \frac{d^2y}{dx^2} + y								</mrow>
					<mrow>			\amp= \Big[ -c_1 \sin x - c_2 \cos x \Big] 
							+ \Big[ c_1 \sin x + c_2 \cos x \Big]		</mrow>
					<mrow>			\amp= 0													</mrow>
					<mrow>			\amp= \text{RHS}										</mrow>	
					</md>
					
					Since when we substitute in to the DE, we find that the LHS is equal to the RHS, we have verified that <m>y = c_1 \sin x + c_2 \cos x</m> is a solution to the DE <m>\DS \frac{d^2y}{dx^2} + y = 0.</m>
				</solution>

				<answer>
					Since we get the same result (0) when we substitute the solution into the RHS and into the LHS, we confirm that <m>y = c_1 \sin x + c_2 \cos x</m> is a solution to the DE.
				</answer>

			</exercise>
		
			<exercise> 
				<p>
					Consider the DE 
					<men xml:id="soln_form1">\DS \frac{d^2 y}{dx^2} + 6 \frac{dy}{dx} + 5y = 0.</men>
				</p>
				
				<p>		
					Find all values of <m>m</m> such that <m>y = e^{mx}</m> is a solution to the DE by taking derivatives and substituting into the DE, and then solving for <m>m</m>.
				</p>
					
				<hint>
					<m>e^{mx} \ne 0,</m> no matter the value of <m>x</m> or <m>m.</m> Therefore we might want to factor it out as it won't contribute to our answer.
				</hint>
				<solution>

					First we take derivatives so that we can substitute into the DE.
					<md>
					<mrow>						y	\amp= e^{mx}							</mrow>
					<mrow>	\Rightarrow \quad   y'	\amp= me^{mx}							</mrow>
					<mrow>	\Rightarrow \quad   y''	\amp= m^2 e^{mx}						</mrow>	
					</md> 
					Now we can substitute into the DE and solve for <m>m</m>:
					<md>
					<mrow>\frac{d^2 y}{dx^2} 
						+ 6 \frac{dy}{dx} + 5y	\amp= 0							</mrow>
					<mrow>\Big[ m^2 e^{mx} \Big] + 6\Big[ m e^{mx} \Big] 
						+ 5\Big[ e^{mx} \Big]	\amp= 0							</mrow>
					<mrow>	e^{mx} \Big[ m^2 + 6m + 5 Big]	\amp= 0							</mrow>
					<mrow>				e^{mx} (m+5)(m+1)	\amp= 0							</mrow>	
					</md>
					Recall that <m>e^{mx} \ne 0,</m> no matter the value of <m>x</m> or <m>m.</m>
					Thus we have:
					<md>
					<mrow>	m+5 = 0 \amp \text{ or } m+1 = 0								</mrow>
					<mrow>	m = -5,	\amp \text{ or } m = -1									</mrow>	
					</md>
					So the two solutions are <m>m = -5, -1.</m>

				</solution>

				<answer>
					<me> m = -5, -1 </me>
				</answer>

			</exercise>

			<exercise>
				<p>
					Now that you have (hopefully!) two values for <m>m,</m> choose one of the two values and then verify that <m>y = e^{mx}</m> is a solution for that value of <m>m.</m>
				</p>

				<solution>
					<p>
					The work here is for <m>m = -5,</m> and the work for <m>m = -1</m> is similar.
					</p>
					<p>
					First we take derivatives so that we can substitute into the DE.
					<md>
						<mrow>							y	\amp= e^{-5x}						</mrow>
						<mrow>		\Rightarrow \quad   y'	\amp= -5e^{-5x}						</mrow>
						<mrow>		\Rightarrow \quad 	y''	\amp= 25 e^{-5x}					</mrow>	
					</md> 	
					Now we can substitute into the DE:
					<md>
						<mrow>\text{LHS}\amp= \frac{d^2 y}{dx^2} + 6 \frac{dy}{dx} + 5y			</mrow>
						<mrow>			\amp= \Big[ 25e^{-5x} \Big] + 6\Big[ -5e^{-5x} \Big] 
								+ 5\Big[ e^{-5x} \Big]		</mrow>
						<mrow>			\amp= 25e^{-5x} - 30 e^{-5x} + 5e^{-5x}					</mrow>
						<mrow>			\amp= 0													</mrow>
						<mrow>			\amp= \text{RHS}										</mrow>	
					</md>
					Hence, we have shown that <m>y = e^{-5x}</m> is a solution to the DE 
					<m>\DS  \frac{d^2 y}{dx^2} + 6 \frac{dy}{dx} + 5y = 0.</m>
					</p>
				</solution>

				<answer>
					Since we get the same result (0) when we substitute the solution into the RHS and into the LHS, we confirm that <m>y = e^{-5x}</m> (or <m>y = e^{-x}</m>) is a solution to the DE.
				</answer>

			</exercise>

			<exercise> 
				<!-- Do we need this? -->
				<p>
					<em> Assuming the form of the solution of DE. </em>
				</p>
				
				
				<p>
					Find all values of <m>m</m> such that <m>y = x^m</m> is a solution of the DE 
					<men xml:id="soln_form2">\DS 3x^2 \frac{d^2y}{dx^2} = -11x \frac{dy}{dx} + 3y.</men>
				</p>

				<solution>
					<p>
					We proceed as in the previous question. First we take derivatives so that we can substitute into the DE.
					<md>
						<mrow>						y	\amp= x^m								</mrow>
						<mrow>	\Rightarrow \quad   y'	\amp= mx^{m-1}							</mrow>
						<mrow>	\Rightarrow \quad   y''	\amp= m(m-1)x^{m-2}						</mrow>	
					</md> 
					Now we can substitute into the DE:
					<md>
						<mrow>				3x^2 \frac{d^2y}{dx^2}	\amp= 
							-11x \frac{dy}{dx} + 3y						</mrow>
						<mrow>		3x^2\Big[ m(m-1)x^{m-2} \Big]	\amp= 
							-11x\Big[ mx^{m-1} \Big] + 3\Big[ x^m \Big]	</mrow>
						<mrow>					3m(m-1)x^2 x^{m-2}	\amp= 
							-11mx^1\cdot x^{m-1} + 3x^m					</mrow>
						<mrow>				(3m^2 - 3m)x^{2+(m-2)}	\amp= 
							-11m x^{1 + (m-1)} + 3x^m					</mrow>
						<mrow>					(3m^2 - 3m)x^{m}	\amp= -11m x^{m} + 3x^m		</mrow>
						<mrow>(3m^2 - 3m)x^{m} + 11m x^{m} - 3x^m	\amp= 0						</mrow>
						<mrow>			(3m^2 - 3m + 11m - 3)x^m	\amp= 0						</mrow>
						<mrow>					(3m^2 +8m - 3)x^m	\amp= 0						</mrow>
						<mrow>						(3m -1)(m+3)x^m	\amp= 0						</mrow>	
					</md>
					Note that there is no value of <m>m</m> that can guarantee that <m>x^m</m> is 0.
					Hence we have
					<md>
						<mrow>			3m-1 = 0 \amp \quad\text{or}\quad m+3 = 0				</mrow>
						<mrow>	m = \frac{1}{3}, \amp \quad\text{or}\quad m = -3				</mrow>	
					</md>
					So the two solutions are <m>m = -3, \frac{1}{3}.</m>
					</p>

				</solution>

				<answer>
					<me> m = -3, \frac{1}{3} </me>
				</answer>
			
			</exercise>

		</exercisegroup>
		
	</exercises>
		

	</section>