<?xml version="1.0" encoding="UTF-8" ?>

<!-- 11-DEsReview_limits -->

<subsection xml:id="r-01-11" xmlns:xi="http://www.w3.org/2001/XInclude">

<title>Limits at infinity</title>

<aside>I know. You thought your Calculus 1 instructor
was crazy for spending sooooooo long on limits, especially when you were convinced you
would never, ever use them, and now here they are again!
</aside>

<p>
In this section, we'll focus our attention on limits at infinity. If you want a refresher,
check out your Calculus 1 book (available online--just search for "APEX calculus".

<ol>
	<li>
	<p>
	Evaluate each of the following limits.
	<ol>
		<li><m>\ds \lim_{b\to \infty} \frac{1}{12}</m>		
		<solution>
			<p>
		The limit of a constant is the constant, so
		
			<me> \lim_{b\to \infty} \frac{1}{12} = \frac{1}{12}. </me>

			</p>
		</solution>
		<answer>
			<p>
				<m> \frac{1}{12} </m>
			</p>
		</answer>
		</li>
	
		<li><m>\ds \lim_{b\to \infty} \frac{1}{s},</m> where <m>s</m> is a constant			<solution>
				<p>
			The limit of a constant is the constant, so
	
			<me> \lim_{b\to \infty} \frac{1}{s} = \frac{1}{s}. </me>
		
			</p>
			</solution>
		<answer>
			<p>
				<m> \frac{1}{s} </m>
			</p>
		</answer>
		</li>
	
		<li><m>\ds \lim_{b\to \infty} e^{2b}</m>		
		<solution>
			<p>
		As <m>b</m> increases to large positive values, the value of <m>e^{2b}</m>
		also increases to large	positive values. Therefore
			
			<me> \lim_{b\to \infty} e^{2b} = \infty. </me>
			</p>
		</solution>
		<answer>
			<p>
				<m> \infty </m>
			</p>
		</answer>
		</li>
	
		<li><m>\ds \lim_{b\to \infty} e^{0.1b}</m>		
		<solution>
			<p>
		As <m>b</m> increases to large positive values, the value of <m>e^{0.1b}</m>
		also increases to large positive values. Therefore

			<me> \lim_{b\to \infty} e^{0.1b} = \infty. </me>
		
			</p>
		</solution>
		<answer>
			<p>
				<m> \infty </m>
			</p>
		</answer>
		</li>
	
		<li><m>\ds \lim_{b\to \infty} e^{-2b}</m>		
		<solution>
			<p>
		As <m>b</m> increases to large positive values, the value of <m>e^{-2b}</m>
		decreases to zero. Therefore
		
			<me> \lim_{b\to \infty} e^{-2b} = 0. </me>

			</p>
		</solution>
		<answer>
			<p>
				<m> 0 </m>
			</p>
		</answer>
		</li>
	</ol>
	</p>
	</li>	
	
	<li>For what values of <m>a</m> is the limit <m>\ds \lim_{b \to \infty}e^{ab}</m>
	finite?
	<solution>
		<p>
	Hopefully you thought a little bit about this as you answered the previous
	question. If you think about it for a little bit, you'll come to realize that:
	<ul marker="square">
		<li>
  		If <m>a=0,</m> then <m>e^{ab} = e^{0} = 1,</m> so
		<m>\ds \lim_{b \to \infty}e^{ab} = 1</m>.
		</li>
		<li>
		If <m>a</m> is negative, then as <m>b</m> increases to large positive values,
		the value of <m>e^{ab}</m> decreases to zero. Therefore
		<m>\ds \lim_{b\to \infty} e^{ab} = 0.</m>
		</li>
	</ul>
	Hence, the limit <m>\ds \lim_{b \to \infty}e^{ab}</m> finite when <m>a \le 0</m>.
		</p>
	</solution>
	<answer>
		<p>
			<m> a \le 0 </m>
		</p>
	</answer>
	</li>
	
	<li>
	<p>
	Evaluate each of the following limits.
  	<ol>
  		<li><m>\ds \lim_{b\to \infty} \left[ -\frac{1}{-3}e^{-3b}
															+ \frac{1}{-3} \right]</m>  		<solution>
			<p>
		<md>
			<mrow>\lim_{b\to \infty} \left[ -\frac{1}{-3}e^{-3b} + \frac{1}{-3} \right]
  						\amp = -\frac{1}{-3}\lim_{b\to \infty} \left[ e^{-3b}\right]
								+ \lim_{b\to \infty} \left[\frac{1}{-3} \right]		</mrow>
	  		<mrow>		\amp = -\frac{1}{-3}\cdot 0 + \frac{1}{-3}					</mrow>
  			<mrow>		\amp = 0 - \frac{1}{3}										</mrow>
  			<mrow>		\amp = -\frac{1}{3}											</mrow>
  		</md>
  			</p>
		</solution>
   		<answer>
			<p>
	  			<m>\ds -\frac{1}{3} </m>
   			</p>
		</answer>
  		</li>
  	
  		<li>
		<p>
		<m>\ds \lim_{b\to \infty} \left[ -\frac{1}{s}e^{-sb} + \frac{1}{s} \right]</m>
			
		<p/>
			
		where <m>s</m> is a constant and <m>s \gt 0</m>
   		<solution>
			<p>
		<md>
  			<mrow>\lim_{b\to \infty} \left[ -\frac{1}{s}e^{-sb} + \frac{1}{s} \right]
  						\amp = \lim_{b\to \infty} \left[ -\frac{1}{s}e^{-sb}\right]
									+ \lim_{b\to \infty} \left[\frac{1}{s} \right]	</mrow>
  			<mrow>		\amp = -\frac{1}{s}\lim_{b\to \infty} \left[ e^{-sb}\right]
									+ \frac{1}{s}									</mrow>
	  		<mrow>		\amp = -\frac{1}{s}\cdot 0 + \frac{1}{s}						</mrow>
  			<mrow>		\amp = \frac{1}{s}											</mrow>
  		</md>
   			</p>
		</solution>
  		<answer>
			<p>
	  			<m>\ds \frac{1}{s} </m>
	  		</p>
		</answer>
		</p>
		</li>
  	
  		<li>
		<p>
		<m>\ds \lim_{b\to \infty} \left[ -\frac{1}{s}e^{-sb}
																+ \frac{1}{s} \right]</m>
			
		<p/>
			
		where <m>s</m> is a constant and <m>s \lt 0</m>. 		
  		<solution>
			<p>
		<md>
	  		<mrow>\lim_{b\to \infty} \left[ -\frac{1}{s}e^{-sb} + \frac{1}{s} \right]
	  				\amp = \lim_{b\to \infty} \left[ -\frac{1}{s}e^{-sb}\right]
								+ \lim_{b\to \infty} \left[\frac{1}{s} \right]		</mrow>
  			<mrow>	\amp = -\frac{1}{s}\lim_{b\to \infty} \left[ e^{-sb}\right]
								+ \frac{1}{s}										</mrow>
  			<mrow>	\amp = -\frac{1}{s}\cdot \infty + \frac{1}{s}					</mrow>
  			<mrow>	\amp = \infty + \frac{1}{s}										</mrow>
	  		<mrow>	\amp = \infty													</mrow>
  		</md>
  			</p>
		</solution>
   		<answer>
			<p>
	  			<m> \infty </m>
   			</p>
		</answer>
		</p>
  		</li>
  	
  		<li>
		<p>
		<m>\ds \lim_{b\to \infty} \left[ \frac{1}{s^2}e^{-sb} \right]</m>
					
		<p/>
			
		where <m>s</m> is a constant and <m>s \gt 0</m>. 		
   		<solution>
			<p>
		<md>
	  		<mrow>\lim_{b\to \infty} \left[ \frac{1}{s^2}e^{-sb} \right]
	  					\amp = \frac{1}{s^2}\lim_{b\to \infty} \left[ e^{-sb} \right]</mrow>
	  		<mrow>		\amp = \frac{1}{s^2}\cdot 0									</mrow>
	  		<mrow>		\amp = 0														</mrow>
	  	</md>
   			</p>
		</solution>
  		<answer>
			<p>
	  			<m> 0 </m>
			</p>
		</answer>
		</p>
  		</li>
  	
  		<li>
		<p>
		<m>\ds \lim_{b\to\infty} \left[\frac{1}{s-3}e^{(3-s)b} + \frac{1}{3-s}\right]</m>
		
		<p/>
			
		where <m>s</m> is a constant and <m>s>3</m>		
  		<solution>
			<p>
		<md>
	  		<mrow>\lim_{b\to \infty} \left[ \frac{1}{s-3}e^{(3-s)b} + \frac{1}{3-s} \right]
	  					\amp = \lim_{b\to \infty} \left[ \frac{1}{s-3}e^{(3-s)b}\right]
								+ \lim_{b\to \infty} \left[ \frac{1}{3-s} \right]	</mrow>
	  		<mrow>		\amp = \frac{1}{s-3}\lim_{b\to \infty} \left[ e^{(3-s)b}\right]
								+ \frac{1}{3-s}										</mrow>
	  		<mrow>		\amp = \frac{1}{s-3}\cdot 0+ \frac{1}{3-s}					</mrow>
	  		<mrow>		\amp = \frac{1}{3-s}											</mrow>
	  	</md>
  		
	  		</p>
		</solution>
	  	<answer>
		<p>
		  		<m>\ds \frac{1}{3-s} </m>
	  		</p>
	</answer>
		</p>
  		</li>
  	
  		<li>
		<p>
		<m>\ds \lim_{b\to \infty} \left[ \frac{1}{s+7}e^{(-7-s)b}
															+ \frac{1}{-7-s} \right]</m>
		<p/>
			
		where <m>s</m> is a constant and <m>s \gt -7</m> 		
  		<solution>
			<p>
		<md>
	  		 <mrow>\lim_{b\to \infty} \left[ \frac{1}{s+7}e^{(-7-s)b}
		 														+ \frac{1}{-7-s} \right]
	  					\amp \lim_{b\to \infty} \left[ \frac{1}{s+7}e^{(-7-s)b}\right]
								+ \lim_{b\to \infty} \left[\frac{1}{-7-s} \right]	</mrow>
	  		<mrow>		\amp \frac{1}{s+7}\lim_{b\to \infty} \left[e^{(-7-s)b}\right]
								+ \frac{1}{-7-s}									</mrow>
	  		<mrow>		\amp = \frac{1}{s+7}\cdot 0 + \frac{1}{-7-s}					</mrow>
	  		<mrow>		\amp = \frac{1}{-7-s}										</mrow>
	  	</md>
	  		
	  		</p>
		</solution>
	  	<answer>
		<p>
		  		<m>\ds \frac{1}{-7-s} </m>
	  		</p>
	</answer>
		</p>
  		</li>
  	
  		<li>
		<p>
		<m>\ds \lim_{b\to \infty} \left[ \frac{1}{s-a}e^{(a-s)b}
																+ \frac{1}{a-s} \right]</m>
		<p/>
		
		where <m>s</m> is a constant and <m>s \lt a</m>. 		
	  	<solution>
		<p>
	<md>
	  		 <mrow>\lim_{b\to \infty} \left[ \frac{1}{s-a}e^{(a-s)b}
		 													+ \frac{1}{a-s} \right]
	  					\amp \lim_{b\to \infty} \left[ \frac{1}{s-a}e^{(a-s)b} \right]
								+ \lim_{b\to \infty} \left[\frac{1}{a-s} \right]	</mrow>
	  		<mrow>		\amp \frac{1}{s-a}\lim_{b\to \infty} \left[ e^{(a-s)b} \right]
								+ \frac{1}{a-s}										</mrow>
	  		<mrow>		\amp \frac{1}{s-a}\cdot 0 + \frac{1}{a-s}					</mrow>
	  		<mrow>		\amp = \frac{1}{a-s}											</mrow>
	  	</md>
	  		
	  		</p>
	</solution>
	  	<answer>
		<p>
		  		<m>\ds \frac{1}{a-s} </m>
	  		</p>
	</answer>
		</p>
  		</li>
	</ol>
	</p>
	</li>
	
</ol>
</p>
</subsection>
