<?xml version="1.0" encoding="UTF-8" ?>

<!-- 12-DEsReview_LHospital -->

<subsection xml:id="r-01-12" xmlns:xi="http://www.w3.org/2001/XInclude">

<title>L'Hospital's Rule</title>

<p>
If you prefer to see a video of this example,
<xref ref="video-lhospital" text="custom"> click here </xref>
</p>

<p>
Consider the following three limits.

	<me> 	(1)\quad\lim_{x\to\infty} \frac{x^2 + 4x}{x} \qquad
			(2)\quad\lim_{x\to\infty} \frac{x}{x^2 + 4x} \qquad
			(3)\quad\lim_{x\to\infty} \frac{x^2 + 4x}{x^2} 						</me>
		
Typically when we evaluate limits, we first attempt a direct substitution.
<em>Note that all three evaluate to the indeterminant form
<m>\ds\frac{\infty}{\infty}</m>. Since these are all rational functions, we have
some algebraic techniques we can try. Here's one way each can be evaluated. </em>

<md>
	<mrow>	(1)\quad\amp\lim_{x\to\infty} \frac{x^2 + 4x}{x}														= \lim_{x\to\infty} \frac{x(x + 4)}{x}
							= \lim_{x\to\infty} \left[ x+4 \right]
							= \infty											</mrow>
	<mrow/>
	<mrow>	(2)\quad\amp\lim_{x\to\infty} \frac{x}{x^2 + 4x}														= \lim_{x\to\infty} \frac{x}{x(x + 4)}
							= \lim_{x\to\infty} \frac{1}{x + 4}
							= 0													</mrow>
	<mrow/>
	<mrow>	(3)\quad\amp\lim_{x\to\infty} \frac{x^2 + 4x}{x^2}				
							= \lim_{x\to\infty} \left[ 1 + \frac{4}{x}\right]			
							= 1 + 0														
							= 1													</mrow>
</md>

Is this result surprising to you? Each had the same value, <m>\ds\frac{\infty}{\infty}</m>,
when we did direct substitution, but each has a different final answer. That's what
it means to be indeterminant. we can't tell what the answer is just based on knowing
that direct substitution yields <m>\ds\frac{\infty}{\infty}</m>.

</p>

<p>
We can do algebra when we have rational functions, but that doesn't work as well
when we have exponential and trig functions. One technique you might consider using when you have indeterminant forms like <m>\ds\frac{0}{0}</m> or <m>\ds\frac{\infty}{\infty}</m>
is L'Hospital's Rule. Here's a reminder.

<sidebyside widths="90%" margins="auto" valign="middle">
	<p>
	<em> L'Hospital's Rule. </em> Suppose <m>f</m> and <m>g</m> are
	differentiable functions and we want to evaluate

	<me> \lim_{x \to c} \frac{f(x)}{g(x)} </me>

	If direct substitution yields an indeterminant form <m>\ds\frac{0}{0}</m> or
	<m>\pm \frac{\infty}{\infty},</m> then
	
	<me> \lim_{x \to c} \frac{f(x)}{g(x)} = \lim_{x \to c} \frac{f'(x)}{g'(x)}, </me>

	assuming that the limit exists.
	</p>
</sidebyside>
</p>

<p>
Here's how it works for one of the limits above.

<md>	
	<mrow>\lim_{x\to\infty} \frac{x^2 + 4x}{x^2}	
			\amp = \lim_{x\to\infty} \frac{\DDX\big( x^2 + 4x \big)}{\DDX\big(x^2\big)}
									\text{ (by L'Hospital's Rule)} 				</mrow>
	<mrow>	\amp = \lim_{x\to\infty} \frac{2x + 4}{2x}							</mrow>
	<mrow>	\amp = \lim_{x\to\infty} \frac{\DDX\big( 2x + 4 \big)}{\DDX\big( 2x \big)}
									\text{ (by L'Hospital's Rule)}				</mrow>
	<mrow>	\amp = \lim_{x\to\infty} \frac{2+0}{2}								</mrow>
	<mrow>	\amp = \lim_{x\to\infty} 1											</mrow>
	<mrow>	\amp = 1																</mrow>
</md>
	
Recall that we MUST check to make sure that the limit is one of those indeterminant
forms before we use L'Hospital's Rule. (And note that we did get the same answer we
got before...which is good!)
</p>

<p>
If you want a more complete discussion and some examples, you can find more in
your Calculus 1 book, which is available for free online (just search for "APEX calculus").
</p>

<p>
<term>Evaluate each of the following limits. Use L'Hospital's Rule only if it
applies.</term>
<ol>
	<li> <m>\ds \lim_{b\to \infty} \frac{b}{e^b}</m>
	<solution>
		<p>
	<m>\ds \lim_{b\to \infty} \frac{b}{e^b}
		= \ub{\lim_{b\to \infty} \frac{1}{e^b}}_\left(= \frac{1}{\infty}\right) = 0	</m>
		
		</p>
	</solution>
	<answer>
		<p>
			<m> 0 </m>
		</p>
	</answer>
	</li>
	
	<li> <m>\ds\ds \lim_{b\to \infty} be^{-3b}</m>	
	<solution>
		<p>
	<m> \ds \lim_{b\to \infty} be^{-3b}
		= \ub{\lim_{b\to \infty} \frac{b}{e^{3b}}}_\left(= \frac{\infty}{\infty}\right)
		= \ub{\lim_{b\to \infty} \frac{1}{3e^{3b}}}_\left(= \frac{1}{\infty}\right)
		= 0																			</m>
		
		</p>
	</solution>
	<answer>
		<p>
			<m> 0 </m>
		</p>
	</answer>
	</li>

	<li> <m>\ds \lim_{b\to \infty} \left[ -\frac{1}{5}be^{-5b} - \frac{1}{25}e^{-5b} - \frac{1}{25} \right]</m>
			 		
	<solution>
		<p>
	<md>
		<mrow> \lim_{b\to \infty} \left[ -\frac{1}{5}be^{-5b} - \frac{1}{25}e^{-5b} - \frac{1}{25} \right]
		\amp = \lim_{b\to \infty} \left[ -\frac{1}{5}be^{-5b}\right] </mrow>
				- \lim_{b\to \infty} \left[\frac{1}{25}e^{-5b}\right]
					- \lim_{b\to \infty} \left[\frac{1}{25} \right]
		<mrow>\amp = -\frac{1}{5}\lim_{b\to \infty} \left[ be^{-5b}\right] </mrow>
				- \frac{1}{25}\lim_{b\to \infty} \left[e^{-5b}\right] - \frac{1}{25}
		<mrow>\amp = -\frac{1}{5}\lim_{b\to \infty} \left[ \frac{b}{e^{5b}}\right] </mrow>
				- \frac{1}{25}\cdot 0 - \frac{1}{25}
		<mrow>\amp = -\frac{1}{5}\lim_{b\to \infty} \left[ \frac{1}{5e^{5b}}\right]
				-0 - \frac{1}{25}</mrow>
		<mrow>\amp = -\frac{1}{5}\cdot 0 - \frac{1}{25}</mrow>
		<mrow>\amp = 0 - \frac{1}{25}</mrow>
		<mrow>\amp = - \frac{1}{25}</mrow>
	</md>
		
		</p>
	</solution>
	<answer>
		<p>
			<m>\ds - \frac{1}{25} </m>
		</p>
	</answer>
	</li>

	<li> <m>\ds \lim_{b\to \infty} \left[ -\frac{1}{s}be^{-sb} - \frac{1}{s^2}e^{-sb} - \frac{1}{s^2} \right],</m>
	where <m>s</m> is a constant and <m>s \gt 0</m>	
	<solution>
		<p>
	<md>
		<mrow> \lim_{b\to \infty} \left[ -\frac{1}{s}be^{-sb} - \frac{1}{s^2}e^{-sb} - \frac{1}{s^2} \right]
		\amp = \lim_{b\to \infty} \left[ -\frac{1}{s}be^{-sb}\right] </mrow>
				- \lim_{b\to \infty} \left[ \frac{1}{s^2}e^{-sb}\right]
					- \lim_{b\to \infty} \left[\frac{1}{s^2} \right]
		<mrow>\amp = -\frac{1}{s}\lim_{b\to \infty} \left[ \frac{b}{e^{sb}}\right] </mrow>
				- \frac{1}{s^2}\lim_{b\to \infty} \left[ e^{-sb}\right]
					- \frac{1}{s^2}
		<mrow>\amp = -\frac{1}{s}\lim_{b\to \infty} \left[ \frac{1}{se^{sb}}\right]
				- \frac{1}{s^2}\cdot 0
					- \frac{1}{s^2}</mrow>
		<mrow>\amp = -\frac{1}{s}\cdot 0 - \frac{1}{s^2}</mrow>
		<mrow>\amp = - \frac{1}{s^2}</mrow>
	</md>
		
		</p>
	</solution>
	<answer>
		<p>
			<m>\ds - \frac{1}{s^2} </m>
		</p>
	</answer>
	</li>
</ol>
</p>

</subsection>