<!-- LICENSING
  This file is part of the textbook "Exploring Differential Equations, An Interactive, Student-Centered Approach" by Geoffrey Cox.
  License: Creative Commons Attribution-ShareAlike 4.0 International (CC BY-SA 4.0)
  You are free to:
    • Share — copy and redistribute the material in any medium or format.
    • Adapt — remix, transform, and build upon the material for any purpose, even commercially.
  Under the following terms:
    • Attribution — You must give appropriate credit, provide a link to the license, and indicate if changes were made.
    • ShareAlike — If you remix, transform, or build upon the material, you must distribute your contributions under the same license.
  Full license text: https://creativecommons.org/licenses/by-sa/4.0/legalcode
  Recommended attribution: "Exploring Differential Equations" by Geoffrey Cox, licensed CC BY-SA 4.0"
-->
<section xml:id="r-01-02" xmlns:xi="http://www.w3.org/2001/XInclude">
<title><m>u</m>-substitution</title>

<p>
When an antiderivative is not immediately obvious, we sometimes use a substitution.
Substitution is a good choice when we have one part of the integrand "looks like" the derivative of another part of the integrand.
</p>
<aside>
Here, "looks like" means equal, except for a multiplication of a constant. For example, we might say
<sidebyside widths="90%" margins="auto" valign="middle">
<p>
<line><m>\succ 12x^2</m> "looks like" <m>x^2</m> or</line>
<line><m>\succ \cos x</m> "looks like" <m>.5\cos x</m></line>
</p>
</sidebyside>
</aside>

<p>
Let's look a a few examples
</p>

<example xml:id="r-01-02-usub_ex_01">
<title>Compute <m>\ds \int \, \cos x\sin x \ dx</m></title>
<p>
Since the derivative of <m>\cos x</m> is <m>-\sin x</m> which "looks like" <m>\sin x</m>, then <m>u</m>-substitution (with <m>u=\cos x</m>) works well. <em>Note, <m>u=\sin x</m> would also work.</em>
</p>

<sidebyside widths="40% 60%" margins="auto" valign="top">
<p>
<!--
step 1: <line>pick <m>u</m>, compute <m>du</m></line>
-->
<md>
	<mrow> u \amp = \cos x 					</mrow>
	<mrow> du \amp = -\sin x \, dx			</mrow>
	<mrow> -\frac{1}{\sin x}du \amp = dx	</mrow>
</md>
</p>
<p>
<!--
step 2: convert integral in terms of <m>u</m>
-->
<md>
	<mrow> \int \, \cos x\sin x \ dx	\amp = \int u \sin x \,
										\left[-\frac{1}{\sin x}du\right] 		</mrow>
	<mrow> 								\amp = -\int u \,du 					</mrow>
	<mrow> 								\amp = -\frac{u^2}{2} + C				</mrow>
	<mrow>								\amp = -\frac{1}{2}\cos^2 x + C			</mrow>
</md>
</p>
</sidebyside>
</example>


<example xml:id="r-01-02-usub_ex_02">
<title>Compute <m>\ds \int \frac{1}{x}\cdot \ln(15x) dx</m></title>


<p>
Substitution is a good choice here because we have a natural log function and we have
<m>\ds \frac{1}{x},</m> which is the derivative of natural log. So we would choose
</p>

<sidebyside widths="40% 60%" margins="auto" valign="top">
<p>
<md>
	<mrow>u 	\amp = \ln(15x)													</mrow>
	<mrow>du	\amp = \frac{d}{dx}\Big( \ln(15x) \Big)							</mrow>
	<mrow>		\amp = \frac{1}{15x}\cdot \frac{d}{dx}(15x)						</mrow>
	<mrow>		\amp = \frac{1}{15x}\cdot 15dx									</mrow>
	<mrow>		\amp = \frac{1}{x}du												</mrow>
</md>
</p>
<p>
<md>
	<mrow>\int \frac{1}{x}\cdot \ln(15x) dx	
				\amp =  \int \ub{\ln(15x)}_{u} \cdot \ub{\frac{1}{x} dx}_{du}	</mrow>
	<mrow>		\amp = \int udu													</mrow>
	<mrow> 						\amp = \frac{1}{2}u^2 + C						</mrow>
	<mrow>						\amp = \frac{1}{2}( \ln(15x))^2 + C				</mrow>
</md>
</p>
</sidebyside>

<p>
We usually pause to confirm that the new integral is simpler than the original.
In this case it certainly is, so we proceed to integrate and then change back to
the original variable, <m>x</m>.
</p>
</example>

<p>Now you try some.</p>

<p><term> Evaluate each of the following integrals. Use proper notation.</term>

<ol>
	<li><m>\ds  \int e^z \cos(e^z) dz \qquad</m>
		<solution>
			<p>
		We will choose <m>u = e^z.</m> Then <m>du = e^z dz.</m> Therefore we have:
		<md>
			<mrow>\int e^z \cos(e^z) dz	
					\amp = \int \cos(e^z) e^z dz									</mrow>
			<mrow>	\amp = \int \ub{\cos(e^z)}_{ss \cos (u)} \ub{e^z dz}_{ss du}	</mrow>
			<mrow>	\amp = \int \cos(u) du										</mrow>
			<mrow>	\amp = \sin(u) + C											</mrow>
			<mrow>	\amp = \sin(e^z) + C											</mrow>
		</md>
			</p>
		</solution>
		<answer>
			<p>
			<me> \sin(e^z) + C </me>
			</p>
		</answer>
	</li>
	<li><m>\ds \int t(t^2 - 12)^{57} dt \qquad</m>
		<solution>
			<p>
		We will choose <m>u = t^2 - 12.</m>  Then <m>du = 2tdt,</m> and therefore
		<m>\ds\frac{1}{2}du = tdt</m> Thus we have:
		<md>
			<mrow>\int t(t^2 - 12)^{57} dt	
							\amp = \int (t^2 - 12)^{57} tdt						</mrow>
			<mrow>			\amp = \int \ub{(t^2 - 12)^{57}}_{ss u^{57}}
												\ub{tdt}_{ss \frac{1}{2}du}		</mrow>
			<mrow>			\amp = \int u^{57}\cdot \frac{1}{2}du				</mrow>
			<mrow>			\amp = \frac{1}{2}\int u^{57}du						</mrow>
			<mrow>			\amp = \frac{1}{2}\cdot \frac{1}{58} u^{58} + C		</mrow>	
			<mrow>			\amp = \frac{1}{116}(t^2 - 12)^{58} + C				</mrow>
		</md>
			</p>
		</solution>
		<answer>
			<p>
			<me> \frac{1}{116}(t^2 - 12)^{58} + C </me>
			</p>
		</answer>
	</li>
	<li><m>\ds \int 5x^2 e^{(7x^3)} dx \qquad</m>
		<solution>
			<p>
		We will choose <m>u = 7x^3.</m>  Then <m>du = 21x^2dx,</m> and therefore
		<m>\ds\frac{1}{21}du = x^2dx</m> Thus we have:
		<md>
			<mrow>\int 5x^2 e^{(7x^3)} dx
							\amp = 5 \int e^{(7x^3)} x^2 dx						</mrow>
			<mrow>			\amp = 5\int \ub{e^{(7x^3)}}_{ss e^u}
										\ub{x^2 dx}_{ss \frac{1}{21}du}			</mrow>
			<mrow>			\amp = 5\int e^u\cdot \frac{1}{21}du					</mrow>
			<mrow>			\amp = \frac{5}{21}\int e^u du						</mrow>
			<mrow>			\amp = \frac{5}{21}e^u + C							</mrow>
			<mrow>			\amp = \frac{5}{21}e^{(7x^3)} + C 					</mrow>
		</md>
			</p>
		</solution>
		<answer>
			<p>
			<me> \frac{5}{21}e^{(7x^3)} + C </me>
			</p>
		</answer>
	</li>
</ol>
</p>
</section>