<!-- LICENSING
  This file is part of the textbook "Exploring Differential Equations, An Interactive, Student-Centered Approach" by Geoffrey Cox.
  License: Creative Commons Attribution-ShareAlike 4.0 International (CC BY-SA 4.0)
  You are free to:
    • Share — copy and redistribute the material in any medium or format.
    • Adapt — remix, transform, and build upon the material for any purpose, even commercially.
  Under the following terms:
    • Attribution — You must give appropriate credit, provide a link to the license, and indicate if changes were made.
    • ShareAlike — If you remix, transform, or build upon the material, you must distribute your contributions under the same license.
  Full license text: https://creativecommons.org/licenses/by-sa/4.0/legalcode
  Recommended attribution: "Exploring Differential Equations" by Geoffrey Cox, licensed CC BY-SA 4.0"
-->
<section xml:id="calculus-review-improper-integrals">
<title>Improper Integrals</title>

<p>
There are two types of improper integrals; the only type we'll be looking at in
differential equations are the type where the upper limit of the integral is infinity.
When we see improper integrals, we re-write the integral as a limit as follows.

	<me> \int_0^{\infty} f(x)dx = \lim_{b \to \infty} \int_0^b f(x) dx </me>

We don't have to use <m>b</m> for the placeholder in the limit, but we shouldn't use any
of the variables that is already in the integrand; in the above, we should not use
<m>x</m> or <m>f</m>. Once we've written the improper integral as a limit, we integrate
and use the fundamental theorem of calculus, keeping the limit as we go, and we evaluate
the limit at the very end. Here's an example.
</p>

<example xml:id="ex_improper_integral_01">
<title>Compute <m>\int_1^{\infty} \frac{1}{x^2}dx</m></title>
	
	<p>
	<md>
		<mrow>\int_1^{\infty} \frac{1}{x^2}dx	
					\amp = \lim_{b \to \infty} \int_1^b \frac{1}{x^2}dx			</mrow>
		<mrow>		\amp = \lim_{b \to \infty} \int_1^b x^{-2} dx				</mrow>
		<mrow>		\amp = \lim_{b \to \infty} \Bigg[ -x^{-1} \Bigg]_1^b			</mrow>
		<mrow>		\amp = \lim_{b \to \infty} \left[ -\frac{1}{x} \right]_1^b	</mrow>
		<mrow>		\amp = \lim_{b \to \infty} \left[ -\frac{1}{b}
											- \left(-\frac{1}{1}\right) \right]	</mrow>
		<mrow>		\amp = \lim_{b \to \infty} \left[ -\frac{1}{b} +1 \right]	</mrow>
		<mrow>		\amp = \lim_{b \to \infty} \left[ -\frac{1}{b}\right]
											+ \lim_{b \to \infty} 1				</mrow>
		<mrow>		\amp = 0 + 1													</mrow>
		<mrow>		\amp = 1														</mrow>
	</md>	
	</p>
</example>

<p>
If you want more of a refresher, check out your Calculus 2 book (available online--
just search for "APEX calculus").
</p>

<p>
<em>  Evaluate the following integrals. Use proper limit notation.</em>
<ol>
	<li> <m>\ds \int_0^{\infty}e^{-3t}dt \qquad</m>		
	<solution>
		<p>
	<md>
		<mrow>\int_0^{\infty}e^{-3t}dt	
				\amp = \lim_{b \to \infty}\int_0^b e^{-3t}dt						</mrow>
		<mrow>	\amp = \lim_{b \to \infty}\left[-\frac{1}{3}e^{-3t} \right]_0^b	</mrow>
		<mrow>	\amp = \lim_{b \to \infty}\left[-\frac{1}{3}e^{-3b}
								+ \frac{1}{3}e^{-3\cdot 0} \right]				</mrow>
		<mrow>	\amp = \lim_{b \to \infty}\left[-\frac{1}{3}e^{-3b}
								+ \frac{1}{3}\cdot 1 \right]					</mrow>
		<mrow>	\amp = \lim_{b \to \infty}\left[-\frac{1}{3}e^{-3b}\right]
								+ \lim_{b \to \infty}\left[\frac{1}{3} \right]	</mrow>
		<mrow>	\amp = -\frac{1}{3} \lim_{b \to \infty}\left[e^{-3b}\right]
								+ \frac{1}{3}									</mrow>
		<mrow>	\amp = -\frac{1}{3} \cdot 0+ \frac{1}{3}							</mrow>
		<mrow>	\amp = \frac{1}{3}												</mrow>
	</md>
		</p>
	</solution>
	<answer>
		<p>
			<m>\ds \frac{1}{3} </m>
		</p>
	</answer>
	</li>

	<li> <m>\ds \int_0^{\infty}e^{-st}dt</m>,
			where <m>s</m> is a constant and <m>s>0 \qquad</m>
	<solution>
		<p>
	<md>
		<mrow>\int_0^{\infty}e^{-st}dt	
				\amp = \lim_{b \to \infty}\int_0^b e^{-st}dt						</mrow>
		<mrow>	\amp = \lim_{b \to \infty}\left[-\frac{1}{s}e^{-st} \right]_0^b	</mrow>
		<mrow>	\amp = \lim_{b \to \infty}\left[-\frac{1}{s}e^{-sb}
								+ \frac{1}{s}e^{-s\cdot 0} \right]				</mrow>
		<mrow>	\amp = \lim_{b \to \infty}\left[-\frac{1}{s}e^{-sb}
								+ \frac{1}{s}\cdot 1 \right]					</mrow>
		<mrow>	\amp = \lim_{b \to \infty}\left[-\frac{1}{s}e^{-sb}\right]
								+ \lim_{b \to \infty}\left[\frac{1}{s} \right]	</mrow>
		<mrow>	\amp = -\frac{1}{s} \lim_{b \to \infty}\left[e^{-sb}\right]
								+ \frac{1}{s}									</mrow>
		<mrow>	\amp = -\frac{1}{s} \cdot 0+ \frac{1}{3}							</mrow>
		<mrow>	\amp = \frac{1}{s}												</mrow>
	</md>
		</p>
	</solution>
	<answer>
		<p>
			<m>\ds \frac{1}{s} </m>
		</p>
	</answer>
	</li>
</ol>
</p>
</section>