<section xmlns:xi="http://www.w3.org/2001/XInclude"><title>Forward Transforming Equations</title>
 
	<p>
		In the previous sections, we've focused on applying Laplace transforms to individual functions. Now, we shift our focus to solving differential equations by transforming the entire equation, along with its initial conditions. This process brings us back to the first step of the Laplace Transform Method roadmap.
	</p>

	<p>
		<image source="figures/Laplace-Roadmap-Step-1.png" width="100%">
			<shortdescription>Step 1: The Forward Laplace Transform</shortdescription>
		</image>
	</p>

	<p>
		To solve a differential equation using Laplace transforms, we apply the Laplace transform to both sides of the equation, leveraging the common transforms and properties we've discussed so far. Applying the transform to a function can be thought of as multiplying the function by <m>e^{-st}</m> and integrating with respect to <m>t</m>. However, instead of rewriting this process for each term, we simply apply the Laplace operator, <m>\laplacesym</m>, to both sides of the equation. Let's illustrate this with an example.
	</p>

	<example>
		<m>\ \ </m>Apply the Laplace Transform to the initial-value problem:
		<me>
			y'' + 3y' + 2y = -40e^{3t}, \quad y(0) = 0, \quad y'(0) = 1.
		</me>

		<solution><title> Solution </title>
			<p>
				First, we apply <m>\laplacesym</m> to both sides:
				<me>
					\lap{y'' + 3y' + 2y} = \lap{-40e^{3t}}.
				</me>
				Using the linearity property <xref ref="P1" text="custom">P<sub>1</sub></xref>, we break this into four separate transforms:
				<me>
					\ub{\lap{y''}}_{(1)} + 3\ub{\lap{y'}}_{(2)} + 2\ub{\lap{y}}_{(3)} = -40\ub{\lap{e^{3t}}}_{(4)}.
				</me>
			</p>

			<p>
				Now, let's compute each transform:
				<md>
					<mrow>
						(1):\quad \amp\ \lap{y''} = s^2Y - s\os{\large 0}{\os{\Large \shortparallel}{y(0)}} - \os{\large 1}{\os{\Large \shortparallel}{y'(0)}} = s^2Y - 1 \quad <xref ref="P4" text="title"/>.
					</mrow>
					<mrow>
						(2):\quad \amp\ \lap{y'} = sY - y(0) = sY \quad <xref ref="P3" text="title"/>.
					</mrow>
					<mrow>
						(3):\quad \amp\ \lap{y} = Y.
					</mrow>
					<mrow>
						(4):\quad \amp\ \lap{e^{3t}} = \frac{1}{s - 3} \quad <xref ref="L2" text="title"/>.
					</mrow>
				</md>
			</p>

			<p>
				Substituting these results back into the equation, we get:
				<md>
					<mrow>
						s^2Y - 1 + 3sY + 2Y =\amp\ \frac{-40}{s - 3}, \quad \text{or}
					</mrow>
					<mrow>
						s^2Y + 3sY + 2Y - 1 =\amp\ \frac{-40}{s - 3}.
					</mrow>
				</md>
			</p>
		</solution>
	</example>

	<p>
		Let's look at one more example for additional clarity.
	</p>

	<example>
		<m>\ \ </m>Apply the Laplace Transform to the initial-value problem:
		<me>
			y'' - 4y' + 6y = t^2, \quad y(0) = 2, \quad y'(0) = 0.
		</me>

		<solution><title> Solution </title>
			<p>
				Applying the Laplace transform to both sides:
				<md>
					<mrow>
						\lap{y'' - 4y' + 6y} =\amp\ \lap{t^2}, \\
						\lap{y''} - 4\lap{y'} + 6\lap{y} =\amp\ \lap{t^2}, \\
						s^2Y - s\os{\large 2}{\os{\Large \shortparallel}{y(0)}} - \os{\large 0}{\os{\Large \shortparallel}{y'(0)}} - 4(sY - \os{\large 2}{\os{\Large \shortparallel}{y(0)}}) + 6Y =\amp\ \frac{2}{s^3}, \\
						s^2Y - 2s - 4sY + 8 + 6Y =\amp\ \frac{2}{s^3}, \\
						s^2Y - 4sY + 6Y - 2s + 8 =\amp\ \frac{2}{s^3}.
					</mrow>
				</md>
			</p>
		</solution>
	</example>

	<p>
		In both examples, the differential equations have been transformed into algebraic equations. Solving for <m>Y(s)</m> is the next step in the Laplace Transform Roadmap.
	</p>

	<xi:include href="./p4-c1-s4-interactives.ptx" />
	
</section>
