<reading-questions><title> Check-Point Questions </title>

	<exercise label="p4-c1-s4-1-rq1"><title> <em>Applying the Laplace transform to a differential equation transforms the equation into an algebraic equation involving functions of <m>s</m></em> </title>
		<statement correct="yes"/>
		<feedback>
			<p>True. The Laplace transform converts a differential equation into an algebraic equation in <m>s</m>.</p>
		</feedback>
	</exercise>
	
	<exercise label="p4-c1-s4-1-rq2"><title> <em>Which of the following represents the correct Laplace transform of the equation <me>y'' + 3y' + 2y = -40e^{3t}, \quad y(0) = 1, \quad y'(0) = 0</me>?</em> </title>
		<statement/>
		<choices>
			<choice>
				<statement><m>\ds s^2Y + 3sY + 2Y = \frac{-40}{s-3}</m></statement>
				<feedback>
					<p>No, this is incorrect. Where are the initial conditions?</p>
				</feedback>
			</choice>
			<choice correct="yes">
				<statement><m>\ds s^2Y + 3sY + 2Y - s = \frac{-40}{s-3}</m></statement>
				<feedback>
					<p>Correct! This is the correct transformation of the given differential equation.</p>
				</feedback>
			</choice>
			<choice>
				<statement><m>\ds s^2Y + 3sY + 2Y + s = \frac{-40}{s - 3}</m></statement>
				<feedback>
					<p>No, this is close to the answer, but it is off by a sign.</p>
				</feedback>
			</choice>
			<choice>
				<statement><m>\ds s^2Y + 3sY + 2Y - 1 = \frac{-40}{s - 3}</m></statement>
				<feedback>
					<p>Incorrect, look closely at the initial conditions.</p>
				</feedback>
			</choice>
		</choices>
	</exercise>
	
	<exercise label="p4-c1-s4-1-rq3"><title> <em>Which of the following represents the correct Laplace transform of the equation <me>y'' - 4y' + 6y = t^2, \quad y(0) = 2, \quad y'(0) = -1</me>?</em> </title>
		<statement/>
		<choices>
			<choice>
				<statement><m>\ds s^2Y - 4sY + 6Y - 2s = \frac{1}{s^3}</m></statement>
				<feedback>
					<p>No, this is incorrect. You are missing a term.</p>
				</feedback>
			</choice>
			<choice>
				<statement><m>\ds s^2Y - 4sY + 6Y + 2s - 1 = \frac{2}{s^3}</m></statement>
				<feedback>
					<p>No, this is close to the answer. Double check the signs of the initial conditions.</p>
				</feedback>
			</choice>
			<choice>
				<statement><m>\ds s^2Y - 4sY + 6Y + 1 = \frac{1}{s^3}</m></statement>
				<feedback>
					<p>No, this is incorrect. You are missing a term.</p>
				</feedback>
			</choice>
			<choice correct="yes">
				<statement><m>\ds s^2Y - 4sY + 6Y - 2s + 1 = \frac{2}{s^3}</m></statement>
				<feedback>
					<p>Correct! This is the correct transformation using the Laplace transform and applying initial conditions.</p>
				</feedback>
			</choice>
		</choices>
	</exercise>
	
	<exercise label="p4-c1-s4-1-rq4"><title> <em>What is the Laplace transform of the initial-value problem <me>y'' - 4y' + 6y = \sin t, \quad y(0) = 2, \quad y'(0) = 0</me>?</em> </title>
		<statement/>
		<choices>
			<choice>
				<statement><m>s^2Y + 4sY + 6Y = \frac{1}{s^2 + 1}</m></statement>
				<feedback>
					<p>No, this is incorrect. Double-check the signs and the initial condition terms.</p>
				</feedback>
			</choice>
			<choice correct="yes">
				<statement><m>s^2Y - 4sY + 6Y - 2s + 8 = \frac{1}{s^2 + 1}</m></statement>
				<feedback>
					<p>Correct! This is the correct transformation of the initial-value problem.</p>
				</feedback>
			</choice>
			<choice>
				<statement><m>s^2Y - 4sY + 6Y = \frac{1}{s^2 + 1}</m></statement>
				<feedback>
					<p>No, this is incorrect. You are missing the initial condition terms on the left-hand side.</p>
				</feedback>
			</choice>
			<choice>
				<statement><m>Y = \frac{1}{s^2 + 1}</m></statement>
				<feedback>
					<p>No, this is incorrect. This only represents the transform of <m>t^2</m> and does not account for the left-hand side of the equation.</p>
				</feedback>
			</choice>
		</choices>
	</exercise>

</reading-questions>
