
	<section xmlns:xi="http://www.w3.org/2001/XInclude"><title> Summary &amp; Exercises </title>

	<introduction>

		<assemblage color="green"><title>Summary of the Key Ideas</title>
			<p>
				<ul marker="">
					<li xml:id="summary-solution">
						<term><em>What is a Solution?</em></term>
						<ul marker="square">
							<li>A solution to a differential equation is a function that, when substituted into the equation, satisfies the equation.</li>
						</ul>
					</li>
					<li xml:id="summary-verification">
						<term><em>Verifying Solutions</em></term>
						<ul marker="square">
							<li>Verification of a solution involves substituting the function into the equation and simplifying to check if a true statement is obtained.</li>
							<li>To verify a solution, all terms should ideally be moved to one side of the equation, simplifying the process.</li>
						</ul>
					</li>
					<li xml:id="summary-types-of-solutions">
						<term><em>Types of Solutions</em></term>
						<ul marker="square">
							<li>Differential equations can have different types of solutions: general and particular.</li>
							<li>The general solution includes arbitrary constants and represents a family of solutions.</li>
							<li>A particular solution is obtained by assigning specific values to these constants.</li>
						</ul>
					</li>
					<li xml:id="summary-initial-conditions">
						<term><em>Initial Conditions</em></term>
						<ul marker="square">
							<li>Initial conditions are values given for the solution or its derivatives at a specific point, often used to find a particular solution.</li>
							<li>They help specify which member of the general solution family is applicable in a specific context.</li>
						</ul>
					</li>
				</ul>
			</p>
		</assemblage>
		
	</introduction>

	<exercises>

		<exercise>
			<p>
				Discuss the difference between a general solution, family of solutions,
				and a particualr solution.
			</p>
		</exercise>
		
		<exercise>
			<p>
				Given the differential equation
					<me> y''-9y = 0 </me>
					determine if the following functions are solutions of this differential
				equation.
			</p>
			<p>
				<sidebyside width="30%">
					<p>
						<line> a. <m>\ds \,\, y = 3</m> </line>
						<line> b. <m>\ds \,\, y = 0</m> </line>
						<line> c. <m>\ds \,\, y = e^{3x}</m> </line>
					</p>
					<p>
						<line> d. <m>\ds \,\, y = 3x</m> </line>
						<line> e. <m>\ds \,\, y = 9e^x</m> </line>
						<line> f. <m>\ds \,\, y = x^9</m> </line>
					</p>
					<p>
						<line> g. <m>\ds \,\, y = 4e^{3x}</m> </line>
						<line> h. <m>\ds \,\, y = e^{-3x}</m> </line>
						<line> i. <m>\ds \,\, y = e^{3x} - 2e^{-3x}</m> </line>
					</p>
				</sidebyside>
			</p>

			<answer>
				<sidebyside width="30%">
					<p>
						<line> a. No </line>
						<line> b. Yes </line>
						<line> c. Yes </line>
					</p>
					<p>
						<line> d. No </line>
						<line> e. No </line>
						<line> f. No </line>
					</p>
					<p>
						<line> g. Yes </line>
						<line> h. Yes </line>
						<line> i. Yes </line>
					</p>
				</sidebyside>
			</answer>
		</exercise>
		
		<exercise>
			<p>
				Given the differential equation
				<me> y'' - 10y' + 25y = 0 </me>
				determine if the following functions are solutions of this differential	equation.
			</p>
			<p>
				<sidebyside width="30%">
					<p>
						<line> a. <m>\ds \,\, y = 0</m> </line>
						<line> b. <m>\ds \,\, y = x^2e^{5x}</m> </line>
						<line> c. <m>\ds \,\, y = e^{5x}</m> </line>
					</p>
					<p>
						<line> d. <m>\ds \,\, y = 5x</m> </line>
						<line> e. <m>\ds \,\, y = xe^{5x}</m> </line>
						<line> f. <m>\ds \,\, y = 5e^{5x}</m> </line>
					</p>
					<p>
						<line> g. <m>\ds \,\, y = 1/25</m> </line>
						<line> h. <m>\ds \,\, y = e^{-5x}</m> </line>
						<line> i. <m>\ds \,\, y = (1+x)e^{5x}</m> </line>
					</p>
				</sidebyside>
			</p>
		
			<answer>
				<p>
					<sidebyside width="30%">
						<p>
							<line> a. Yes </line>
							<line> b. No </line>
							<line> c. Yes </line>
						</p>
						<p>
							<line> d. No </line>
							<line> e. Yes </line>
							<line> f. Yes </line>
						</p>
						<p>
							<line> g. No </line>
							<line> h. No </line>
							<line> i. Yes </line>
						</p>
					</sidebyside>
				</p>
			</answer>
		</exercise>
		
		<exercise>
			<p>
				Match each function on the left with a DE on the right if this function is a solution (i.e. is in the family of solutions) for this DE.
			
				<sidebyside widths="40% 40%">
					<p>
						<ol marker="A.">
							<li> <m>y = 3x+x^2</m>	</li>
							<li> <m>y = e^{-8x}</m>	</li>
							<li> <m>y = \sin x</m>	</li>
							<li> <m>y = x^{1/2}</m>	</li>
							<li> <m>y = 6e^{8x}</m>	</li>
						</ol>
					</p>
					<p>
						<ul marker="">
							<li> <m>\fbox{\(\phantom{D}\)} \quad 2x^2y'' + 3xy' = y</m>				</li>
							<li> <m>\fbox{\(\phantom{B}\)} \quad y'' + 10 y' + 16 y = 0</m>			</li>
							<li> <m>\fbox{\(\phantom{E}\)} \quad y' = 8 y</m>						</li>
							<li> <m>\fbox{\(\phantom{C}\)} \quad y'' + y = 0</m>					</li>
							<li> <m>\fbox{\(\phantom{A}\)} \quad 3y'' - 2y + \frac{4}{x}y = 12</m>	</li>
						</ul>
					</p>
				</sidebyside>
			</p>
		
			<answer>
				<ul marker="">
					<li> <m>\fbox{\(D\)} \quad  2x^2y'' + 3xy' = y</m> 				</li>
					<li> <m>\fbox{\(B\)} \quad  y'' + 10 y' + 16 y = 0</m> 			</li>
					<li> <m>\fbox{\(E\)} \quad  y' = 8 y</m> 						</li>
					<li> <m>\fbox{\(C\)} \quad  y'' + y = 0</m> 					</li>
					<li> <m>\fbox{\(A\)} \quad  3y'' - 2y + \frac{4}{x}y = 12</m>	</li>
				</ul>
			</answer>
		</exercise>
		
		<exercise>
			<p>
				Find all values of <m>r</m> such that <m>y=e^{rx}</m> is a solution to
				<me>y''' - 10y'' + 24y' = 0</me>.
			</p>
			
			<answer>
				<m>r = 0, 6, 4</m>
			</answer>
		</exercise>
		
		<exercise>
			<p>
				Find all values of <m>r</m> such that <m>y = k e^{rx}</m> is a solution	to
				<me>y'' - 25y = 0</me>.
			</p>
		
			<answer>
					<m>r = -5, 5</m>
			</answer>
		</exercise>
		
		<exercise>
			<p>
				Find all values of <m>r</m> such that <m>y(x) = c_1 e^{r x} + c_2</m> is a solution to
				<me>7y'' = 8y</me>.
			</p>
		
			<answer>
					<m>r = 8/7</m>
			</answer>
		</exercise>
		
		<exercise>
			<p>
				Find all values of <m>r</m> such that <m>y = t^{r}</m> is a solution to
				<me>t^{2}y''- 11ty' + 32y = 0 \quad (t>0)</me>.
			</p>
		
			<answer>
					<m>r = 4, 8</m>
			</answer>
		</exercise>
		
		<exercise>
			<p>
				Find all values of <m>r</m> such that <m>y = rx^{2}</m> is a solution to
				<me>y' = 5x</me>.
			</p>
		
			<answer>
				<m>r = 2.5</m>
			</answer>
		</exercise>
		
		<exercise>
			<p>
				Find all values of <m>r</m> such that <m>y = \sin(rt)</m> is a solution to
				<me>y'' + 9y = 0</me>.
			</p>
		
			<answer>
				<m>r = 2.5</m>
			</answer>
		</exercise>
		
		<exercise>
			<p>
				Find the value of the constant <m>k</m> in order for the differential equation
				<me> \frac{d^2y}{dt^2} - 8 \frac{dy}{dt} + ky = 0</me>
				to have the solution <m>y = e^{3t}</m>.
			</p>
		
			<answer>
				<m>k = 15</m>
			</answer>
		</exercise>
		
		<exercise>
			<p>
				Is <m>\ds y = c_{1}e^{2x} + c_{2}xe^{2x}</m> a solution of the
				differential equation
				<me>\ds \frac{d^{2}y}{dx^{2}} - 4\frac{dy}{dx} + 4y = 0?</me>
			</p>
		
			<answer>
					Yes
			</answer>
		</exercise>
			
		<exercisegroup><title> Find the value of <m>r</m> </title>
		
			<introduction>
				<p>
					For each of the differential equations and function pairs, find all the possible values of <m>r</m> such that the function is a solution to the DE.
				</p>
			</introduction>
			<exercise>
				<m>y''' - 10y'' + 24y' = 0; \quad y=e^{rx}</m>
				<answer>
					<m>r = 0, 6, 4</m>
				</answer>
			</exercise>
		
			<exercise>
				<m>y'' - 25y = 0; \quad y = k e^{rx}</m>
				<answer>
					<m>r = -5, 5</m>
				</answer>
			</exercise>
			
			<exercise>
				<m>7y'' = 8y; \quad y(x) = c_1 e^{r x} + c_2</m>
				<answer>
					<m>r = 8/7</m>
				</answer>
			</exercise>
			
			<exercise>
				<m>t^{2}y''- 11ty' + 32y = 0; \quad y = t^{r} \quad (t>0)</m>
				<answer>
					<m>r = 4, 8</m>
				</answer>
			</exercise>
			
			<exercise>
				Let <m>y' = 5x; \quad y = rx^{2}</m>
				<answer>
					<m>r = 2.5</m>
				</answer>
			</exercise>
			
			<exercise>
				<m>y'' + 9y = 0; \quad y = \sin(rt)</m>
				<answer>
					<m>r = 2.5</m>
				</answer>
			</exercise>
		
		</exercisegroup>

		<exercise>
			<p>
				Explain the significance of initial condition(s) as they relate to the general solution of a differential equation.
			</p>
			<answer>
				<line>
				The initial condition(s) specify one or more points that the graph of the
				solution must pass through. This often allows one to solve for the
				constants in the general solution.
				</line>
				<line>
				Therefore, the initial condition(s) act to reduce the
				family of solutions down to a smaller set of solutions or, ideally, a
				single particular solution.
				</line>
			</answer>
		</exercise>

		<exercise>
			<p>
				Does an initial condition always give you a particular solution?
			</p>
			<answer>
				<line>When there is one constant in the general solution, yes.</line>
				<line>When there is more than one constant in the general solution, no.<m>^{1}</m></line>
				<aside>
				It does, however, limit the possible values of the constants.
				</aside>
			</answer>
		</exercise>

		<exercise>
			<p>
				Consider the differential equation
				<me>x^2y' + xy = 1</me>
			<ol>
				<li>
					Verify that the family of functions
					<me>y = \frac{\ln x + C}{x}</me>
					a solution to this differential equation.
				</li>
				<li>
					Find the particular solution that corresponds to the initial condition <m>y(9)=8</m>.
				</li>
			</ol>
			</p>
			<answer>
				<line>Yes</line>
				<line>
					<m>C = 72-\ln(9) \approx 69.803</m>, so
					<m>\ds y = \frac{\ln x + 69.803}{x} </m> is the particular solution
				</line>
			</answer>
		</exercise>

		<exercise>
			<p>
				Consider the differential equation
				<me>y^\prime = y-y^2</me>
				Which of the following is a family of solutions for this DE?
					<ol>
						<li> <m>\ds y=c\sin(-x)</m></li>
						<li> <m>\ds y=\frac{1}{1+ce^{-x}}</m></li>
						<li> <m>\ds y=\frac{1}{c+x^2}</m></li>
					</ol>
				Find the particular solution such that <m>y(0) = 7</m>.
			</p>
			<answer>
				<line>b. <m>\ds y=\frac{1}{1+ce^{-x}}</m></line>
				<line>
				<m>c = \frac{1}{7}-1 \approx -0.857</m>, so
				<m>\ds y = \frac{1}{1+(-0.857)e^{-x}} </m> is the particular solution
				</line>
			</answer>

			<solution>
				<line>Try <m>y=\frac{1}{c+x^2}</m> first.</line>
				<line>Compute</line>
				<line> <m>y^\prime = \frac{-4x}{(c+x^2)^2}</m> </line>
				<line> <m>y-y^2 = \frac{1}{c+x^2} - \frac{1}{(c+x^2)^2}
								= \frac{c+x^2}{(c+x^2)^2} - \frac{1}{(c+x^2)^2}
								= \frac{c+x^2-1}{(c+x^2)^2}</m></line>
				<line>So <m>y^\prime\neq y-y^2</m> for this function, it is not the solution.</line>
				<line>Now try <m>y=\frac{1}{1+ce^{-x}}</m>. Then</line>

				<line><m>y^\prime = \frac{ce^{-x}}{1+ce^{-x}}</m></line>
				<line>while</line>
				<line><m>y-y^2=\frac{1}{1+ce^{-x}}-\frac{1}{(1+ce^{-x})^2}
							=\frac{1+ce^{-x}}{(1+ce^{-x})^2}-\frac{1}{(1+ce^{-x})^2}
							=\frac{ce^{-x}}{(1+ce^{-x})^2}</m></line>
				<line>So this function is the solution</line>
				<line>Setting <m>y(0)=$y0</m> we get</line>
				<line><m>$y0 = \frac{1}{1+c}</m></line>
				<line>Solve for c, <m>c = \frac{1}{$y0}-1=$c</m></line>
				<line>So the solution for the IVP is <m>y = \frac{1}{1+(-0.857)e^{-x}}</m></line>
			</solution>
		</exercise>
		
		<exercisegroup><title> Understanding what it means to Solve a DE </title>
			<introduction>
				<p>
					We spend a lot of time solving equations, but do you even remember what it means to be a solution? Let's review what it means to be a solution to an algebraic equation (as in question <xref ref="alg_eqn_soln"/>), and then what it means to be a solution to a differential equation (as in question <xref ref="diff_eqn_soln"/>), and then we'll extend those ideas in questions <xref ref="soln_form1"/> and <xref ref="soln_form2"/>.
				</p>
			</introduction>

			<exercise>
				<p>
					Verify that <m>x = 3</m> is a solution to the equation 
					
					<men xml:id="alg_eqn_soln">2x^2 + 3 = 7x.</men>
				
				</p>
			
				<p>
					What confirms that <m>x = 3</m> is a solution? 
					<answer>
					the LHS = RHS after substituting <m>x = 3</m> into both sides of the equation.
					</answer>	
				</p>
			
				<p>	
					(<em> Note: Do not rearrange the equation to solve for <m>x</m>. That would be the
					process of finding a solution; you are asked to verify a solution.</em>)
				</p>

				<solution>
					We substitute <m>x = 3</m> into the left hand side (LHS) of the equation, 
					and then into the right hand side (RHS) of the equation:
					
					<md>
						<mrow>\text{LHS}	=\amp\ 2x^2 + 3										</mrow>
						<mrow>				=\amp\ 2(3)^2 + 3									</mrow>
						<mrow>				=\amp\ 18 + 3										</mrow>
						<mrow>				=\amp\ 21											</mrow>
						<mrow>				\amp 												</mrow>
						<mrow>\text{RHS}	=\amp\ 7x											</mrow>
						<mrow>				=\amp\ 7(3)											</mrow>
						<mrow>				=\amp\ 21											</mrow>	
					</md>
					
					Since we get the same result when we substitute the solution into the RHS and 
					into the LHS, we have confirmed that <m>x = 3</m> is a solution to the equation.
				</solution>

				<!-- Is this answer necessary? -->
				<answer>
					Since we get the same result (21) when we substitute the solution into the 
					RHS and into the LHS, we confirm that <m>x = 3</m> is a solution to the equation.
				</answer>
			
			</exercise>

			<exercise>
				<p>
					Verify that <m>y = c_1 \sin x + c_2 \cos x</m> is a solution to the DE 
					<men xml:id="diff_eqn_soln">\ds \frac{d^2y}{dx^2} + y = 0.</men>
				</p>
				
				<hint>
					Look back at the previous question and think about what it means to be a solution to a DE.
				</hint>
				<solution>
					We need to substitute into the DE. In order to substitute into the left hand side, we need to know the second derivative. So we begin by finding that.
					
					<md>
					<mrow>						y	=\amp\ c_1 \sin x + c_2 \cos x			</mrow>
					<mrow>	\Rightarrow \quad   y'	=\amp\ c_1 \cos x - c_2 \sin x			</mrow>
					<mrow>	\Rightarrow \quad   y''	=\amp\ -c_1 \sin x - c_2 \cos x			</mrow>	
					</md>
					
					Now we can substitute into the DE:
					
					<md>
					<mrow>\text{LHS}=\amp\ \frac{d^2y}{dx^2} + y								</mrow>
					<mrow>			=\amp\ \Big[ -c_1 \sin x - c_2 \cos x \Big] 
							+ \Big[ c_1 \sin x + c_2 \cos x \Big]		</mrow>
					<mrow>			=\amp\ 0													</mrow>
					<mrow>			=\amp\ \text{RHS}										</mrow>	
					</md>
					
					Since when we substitute in to the DE, we find that the LHS is equal to the RHS, we have verified that <m>y = c_1 \sin x + c_2 \cos x</m> is a solution to the DE <m>\ds \frac{d^2y}{dx^2} + y = 0.</m>
				</solution>

				<answer>
					Since we get the same result (0) when we substitute the solution into the RHS and into the LHS, we confirm that <m>y = c_1 \sin x + c_2 \cos x</m> is a solution to the DE.
				</answer>

			</exercise>
		
			<exercise> 
				<p>
					Consider the DE 
					<men xml:id="soln_form1">\ds \frac{d^2 y}{dx^2} + 6 \frac{dy}{dx} + 5y = 0.</men>
				</p>
				
				<p>		
					Find all values of <m>m</m> such that <m>y = e^{mx}</m> is a solution to the DE by taking derivatives and substituting into the DE, and then solving for <m>m</m>.
				</p>
					
				<hint>
					<m>e^{mx} \ne 0,</m> no matter the value of <m>x</m> or <m>m.</m> Therefore we might want to factor it out as it won't contribute to our answer.
				</hint>
				<solution>

					First we take derivatives so that we can substitute into the DE.
					<md>
					<mrow>						y	=\amp\ e^{mx}							</mrow>
					<mrow>	\Rightarrow \quad   y'	=\amp\ me^{mx}							</mrow>
					<mrow>	\Rightarrow \quad   y''	=\amp\ m^2 e^{mx}						</mrow>	
					</md> 
					Now we can substitute into the DE and solve for <m>m</m>:
					<md>
					<mrow>\frac{d^2 y}{dx^2} 
						+ 6 \frac{dy}{dx} + 5y	=\amp\ 0							</mrow>
					<mrow>\Big[ m^2 e^{mx} \Big] + 6\Big[ m e^{mx} \Big] 
						+ 5\Big[ e^{mx} \Big]	=\amp\ 0							</mrow>
					<mrow>	e^{mx} \Big[ m^2 + 6m + 5 Big]	=\amp\ 0							</mrow>
					<mrow>				e^{mx} (m+5)(m+1)	=\amp\ 0							</mrow>	
					</md>
					Recall that <m>e^{mx} \ne 0,</m> no matter the value of <m>x</m> or <m>m.</m>
					Thus we have:
					<md>
					<mrow>	m+5 = 0 \amp \text{ or } m+1 = 0								</mrow>
					<mrow>	m = -5,	\amp \text{ or } m = -1									</mrow>	
					</md>
					So the two solutions are <m>m = -5, -1.</m>

				</solution>

				<answer>
					<me> m = -5, -1 </me>
				</answer>

			</exercise>

			<exercise>
				<p>
					Now that you have (hopefully!) two values for <m>m,</m> choose one of the two values and then verify that <m>y = e^{mx}</m> is a solution for that value of <m>m.</m>
				</p>

				<solution>
					<p>
					The work here is for <m>m = -5,</m> and the work for <m>m = -1</m> is similar.
					</p>
					<p>
					First we take derivatives so that we can substitute into the DE.
					<md>
						<mrow>							y	=\amp\ e^{-5x}						</mrow>
						<mrow>		\Rightarrow \quad   y'	=\amp\ -5e^{-5x}						</mrow>
						<mrow>		\Rightarrow \quad 	y''	=\amp\ 25 e^{-5x}					</mrow>	
					</md> 	
					Now we can substitute into the DE:
					<md>
						<mrow>\text{LHS}=\amp\ \frac{d^2 y}{dx^2} + 6 \frac{dy}{dx} + 5y			</mrow>
						<mrow>			=\amp\ \Big[ 25e^{-5x} \Big] + 6\Big[ -5e^{-5x} \Big] 
								+ 5\Big[ e^{-5x} \Big]		</mrow>
						<mrow>			=\amp\ 25e^{-5x} - 30 e^{-5x} + 5e^{-5x}					</mrow>
						<mrow>			=\amp\ 0													</mrow>
						<mrow>			=\amp\ \text{RHS}										</mrow>	
					</md>
					Hence, we have shown that <m>y = e^{-5x}</m> is a solution to the DE 
					<m>\ds  \frac{d^2 y}{dx^2} + 6 \frac{dy}{dx} + 5y = 0.</m>
					</p>
				</solution>

				<answer>
					Since we get the same result (0) when we substitute the solution into the RHS and into the LHS, we confirm that <m>y = e^{-5x}</m> (or <m>y = e^{-x}</m>) is a solution to the DE.
				</answer>

			</exercise>

			<exercise> 
				<!-- Do we need this? -->
				<p>
					<em> Assuming the form of the solution of DE. </em>
				</p>
				
				
				<p>
					Find all values of <m>m</m> such that <m>y = x^m</m> is a solution of the DE 
					<men xml:id="soln_form2">\ds 3x^2 \frac{d^2y}{dx^2} = -11x \frac{dy}{dx} + 3y.</men>
				</p>

				<solution>
					<p>
					We proceed as in the previous question. First we take derivatives so that we can substitute into the DE.
					<md>
						<mrow>						y	=\amp\ x^m								</mrow>
						<mrow>	\Rightarrow \quad   y'	=\amp\ mx^{m-1}							</mrow>
						<mrow>	\Rightarrow \quad   y''	=\amp\ m(m-1)x^{m-2}						</mrow>	
					</md> 
					Now we can substitute into the DE:
					<md>
						<mrow>				3x^2 \frac{d^2y}{dx^2}	=\amp\ 
							-11x \frac{dy}{dx} + 3y						</mrow>
						<mrow>		3x^2\Big[ m(m-1)x^{m-2} \Big]	=\amp\ 
							-11x\Big[ mx^{m-1} \Big] + 3\Big[ x^m \Big]	</mrow>
						<mrow>					3m(m-1)x^2 x^{m-2}	=\amp\ 
							-11mx^1\cdot x^{m-1} + 3x^m					</mrow>
						<mrow>				(3m^2 - 3m)x^{2+(m-2)}	=\amp\ 
							-11m x^{1 + (m-1)} + 3x^m					</mrow>
						<mrow>					(3m^2 - 3m)x^{m}	=\amp\ -11m x^{m} + 3x^m		</mrow>
						<mrow>(3m^2 - 3m)x^{m} + 11m x^{m} - 3x^m	=\amp\ 0						</mrow>
						<mrow>			(3m^2 - 3m + 11m - 3)x^m	=\amp\ 0						</mrow>
						<mrow>					(3m^2 +8m - 3)x^m	=\amp\ 0						</mrow>
						<mrow>						(3m -1)(m+3)x^m	=\amp\ 0						</mrow>	
					</md>
					Note that there is no value of <m>m</m> that can guarantee that <m>x^m</m> is 0.
					Hence we have
					<md>
						<mrow>			3m-1 = 0 \amp \quad\text{or}\quad m+3 = 0				</mrow>
						<mrow>	m = \frac{1}{3}, \amp \quad\text{or}\quad m = -3				</mrow>	
					</md>
					So the two solutions are <m>m = -3, \frac{1}{3}.</m>
					</p>

				</solution>

				<answer>
					<me> m = -3, \frac{1}{3} </me>
				</answer>
			
			</exercise>

		</exercisegroup>
		
	</exercises>
		

	</section>