<section xmlns:xi="http://www.w3.org/2001/XInclude"><title> Finding Particular Solutions </title>

	<p>
		When solving a non-homogeneous linear differential equation, selecting the correct form for the particular solution, <m>y_p</m>, is just the beginning. The next important task is determining the values of its unknown coefficients, such as <m>A</m> and <m>B</m>. In this section, we'll explore how to compute these coefficients by plugging the guessed particular solution into the original equation.
	</p>

	<p>
		Let's revisit the example we discussed earlier. Consider the differential equation:
		<men xml:id="finding-yps-coefficients-de">
			y'' - 4y' + 3y = 9x
		</men>.
		We guessed that the particular solution would be linear, so we set
		<me>
			y_p = Ax + B
		</me>.
	</p>

	<p>
		Our goal now is to determine the values of <m>A</m> and <m>B</m>. To do this, we substitute <m>y_p = Ax + B</m> into the original differential equation. Here's how it works:
		<md>
			<mrow> y_p = Ax + B \quad \implies \quad y_p' = A \quad \implies \quad y_p'' = 0</mrow>
		</md>
		Substituting <m>y_p</m>, <m>y_p'</m>, and <m>y_p''</m> into <xref ref="finding-yps-coefficients-de"/> results in:
		<md>
			<mrow> 0 - 4A + 3(Ax + B) = 9x </mrow>
			<mrow> -4A + 3Ax + 3B = 9x </mrow>
		</md>
		The next step is to collect the like terms and compare the coefficients of <m>x</m> on both sides of the equation. For the left-hand side to equal the right-hand side, the coefficients of <m>x</m> must be the same, and the constant terms must also match, as follows:
		<image width="50%">
			<latex-image>
			
				\begin{tikzpicture}[join=round,rounded corners,&gt;=stealth,shorten &gt;=1pt,shorten &lt;=1pt,thick]
					\node (text1) 	at (1.4,0.5) 	{\scriptsize equal};
					\node (text2) 	at (3.4,0.7) 	{\scriptsize equal};
					
					\def\LA{0.1}
					\def\WA{0.64}
					\def\LB{1.27}
					\def\WB{1.65}
					\def\LC{3.33}
					\def\WC{0.3}
					\def\LD{4.2}
					\def\WD{0.28}

					\node[anchor=west] (eqn)	at (0,0)	{$\,3A\ x + \,- 4A + 3B\, = \ 9\ x + 0\ .$};
					\node (xterm1) at (\LA+\WA/2,0.1) {};
					\node (xterm2) at (\LC+\WC/2,0.1) {};
					\node (cterm1) at (\LB+\WB/2,0.1) {};
					\node (cterm2) at (\LD+\WD/2,0.1) {};
					
					\filldraw[fill=red!20,fill opacity=0.2,thin,draw=red]
						(\LA,-0.2)--(\WA,-0.2)--(\WA,0.2)--(\LA,0.2)--cycle;
					\filldraw[fill=blue!20,fill opacity=0.2,thin,draw=blue]
						(\LB,-0.2)--(\LB+\WB,-0.2)--(\LB+\WB,0.2)--(\LB,0.2)--cycle;
					\filldraw[fill=red!20,fill opacity=0.2,thin,draw=red]
						(\LC,-0.2)--(\LC+\WC,-0.2)--(\LC+\WC,0.2)--(\LC,0.2)--cycle;
					\filldraw[fill=blue!20,fill opacity=0.2,thin,draw=blue]
						(\LD,-0.2)--(\LD+\WD,-0.2)--(\LD+\WD,0.2)--(\LD,0.2)--cycle;
					
					\draw[-&gt;,thin] (text1.west)		--	+(-0.06,0.0) -| (xterm1);
					\draw[-&gt;,thin] (text1.east)		--	+(0.06,0.0) -| (xterm2);
					\draw[-&gt;,thin] (text2.west)		--	+(-0.06,0.0) -| (cterm1);
					\draw[-&gt;,thin] (text2.east)		--	+(0.06,0.0) -| (cterm2);
					
				\end{tikzpicture}
			</latex-image>
		</image>
		Setting the approriate terms equal, gives us the following system of equations:
		<md>
			<mrow>	3A		=\amp\ 9 \quad \implies \quad A = 3</mrow>
			<mrow> -4A + 3B	=\amp\ 0 \quad \implies \quad B = 4</mrow>
		</md>
		Therefore, the particular solution is:
		<me>
			y_p = 3x + 4
		</me>
	</p>

	<p>
		Regardless of <m>y_p</m>'s form, the process of finding the coefficients is the same. 
		<ul marker="square">
			<li>
				<p>
					Plug selected <m>y_p</m> into the differential equation.
				</p>
			</li>
			<li>
				<p>
					Collect and match the coefficients of the like terms on opposite sides of the equation.
				</p>
			</li>
			<li>
				<p>
					Solve the resulting system of equations to find <m>A, B, C, \ldots</m>.
				</p>
			</li>
		</ul>
	</p>

	<assemblage><title>Tip: Identifying when things are Amiss</title>
		<p>
			Each coefficient should have exactly one solution. If you end up with conflicting values or unsolvable equations, it's a good idea to double-check your choice of <m>y_p</m> and computations.
		</p>
	</assemblage>

	<xi:include href="./p3-c2-s3-interactives.ptx" />
	
	<example>

		<m>\ \ </m> Find the particular solution to the LNCC equation below.

		<p>
			<me> y'' + 3y' + 2y = 6e^{2x} </me>.
		</p>
			
		<solution>
			<p>
				Since the right-hand side is an exponential function, we set <m>y_p</m> below and compute the needed derivatives
				<md>
					<mrow> y_p		=\amp\ A e^{2x}		</mrow>
					<mrow> y_p'		=\amp\ 2A e^{2x}	</mrow>
					<mrow> y_p''	=\amp\ 4A e^{2x}	</mrow>
				</md>
			</p>
			<p>
				Substituting these into the equation and collecting like terms, we get
				<md>
					<mrow> 4A e^{2x} + 3(2A e^{2x}) + 2(A e^{2x}) = 6e^{2x} </mrow>
					<mrow> 4A e^{2x} + 6A e^{2x} + 2A e^{2x} = 6e^{2x} </mrow>
					<mrow> \ul{12A} e^{2x} = \ul{6} e^{2x} </mrow>
				</md>.
				Matching the underlined coefficients leads to an equation to find <m>A</m>
				<md>
					<mrow> 12A = 6 \quad \implies \quad A = \frac{1}{2} </mrow>
				</md>.
			</p>
			<p>
				Finally, we write the particular solution as
				<me> y_p = \frac{1}{2} e^{2x} </me>.
			</p>
		</solution>
	</example>
		
	<example>

		<m>\ \ </m> Find the particular solution to the LNCC equation below.

		<p>
			<me> y'' - 3y' + y = 2x^2 + 3x </me>.
		</p>
		
		<solution>

			<p>
				This time the right-hand side is a polynomial of degree 2, so we select <m>y_p</m> and compute its derivatives as follows:
				<md>
					<mrow> y_p = Ax^2 + Bx + C		</mrow>
					<mrow> y_p' = 2Ax + B, \quad y_p'' = 2A	</mrow>
				</md>
			</p>
			<p>
				Substituting these into the equation and collecting like terms, we get
				<md>
					<mrow> 2A - 3(2Ax + B) + (Ax^2 + Bx + C) = 2x^2 + 3x </mrow>
					<mrow> 2A - 6Ax - 3B + Ax^2 + Bx + C = 2x^2 + 3x </mrow>
					<mrow> \us{1}{\ul{A}}x^2 + \us{2}{\ul{(- 6A + B)}}x + \us{3}{\ul{(2A - 3B + C)}} = \us{[1]}{\ul{2}}x^2 + \us{[2]}{\ul{3}}x + \us{[3]}{\ul{0}} </mrow>
				</md>.
				Matching the underlined coefficients leads to an equation to find <m>A</m>
				<ol>
					<li><m>A = 2</m></li>
					<li><m>-6A + B = 3</m></li>
					<li><m>2A - 3B + C = 0</m></li>
				</ol>
				<md>
					<mrow> A = 2, \quad B = 9, \quad C = 13 </mrow>
				</md>.
			</p>
			<p>
				Finally, we write the particular solution as
				<me> y_p = 2x^2 + 9x + 13 </me>.
			</p>
		</solution>
	</example>
		
	<example>
		<statement>
			Solve the non-homogeneous differential equation:
			<me> y'' + y = 3 \cos x </me>. Find the particular solution.
		</statement>
		<solution>
			<p>
			Step 1: The right-hand side is trigonometric, so we guess:
			<me> y_p = A \cos x + B \sin x </me>.
			</p>
			<p>
			Step 2: Differentiate the guessed solution:
			<md>
				<mrow> y_p' = -A \sin x + B \cos x, \quad y_p'' = -A \cos x - B \sin x </mrow>
			</md>
			</p>
			<p>
			Step 3: Substitute into the original equation:
			<md>
				<mrow> (-A \cos x - B \sin x) + (A \cos x + B \sin x) = 3 \cos x </mrow>
				<mrow> 0A \sin x + 0B \cos x = 3 \cos x </mrow>
			</md>
			</p>
			<p>
			Step 4: Solve for <m> A </m> and <m> B </m>:
			<md>
				<mrow> A = 3, \quad B = 0 </mrow>
			</md>
			</p>
			<p>
			Step 5: Write the particular solution:
			<me> y_p = 3 \cos x </me>.
			</p>
		</solution>
	</example>

	<example>
		<statement> 
			Find a particular solution for the following differential equation.
			<me>y'' - 4y' - 12y = t{{\bf{e}}^{4t}}</me>
		</statement>
		  
		<solution>
			<p>
				You're probably getting tired of the opening comment, but again finding the homogeneous solution first really a good idea but again we've already done the work in the first example so we won't do it again here.  We promise that eventually you'll see why we keep using the same homogeneous problem and why we say it's a good idea to have the homogeneous solution in hand first.  At this point all we're trying to do is reinforce the habit of finding the homogeneous solution first.
			</p>
		  
			<p>
				Okay, let's start off by writing down the guesses for the individual pieces of the function.  The guess for the <me>t</me> would be
			</p>
			<me>At + B</me>
			  <p>while the guess for the exponential would be</p>
			<me>C{{\bf{e}}^{4t}}</me>
		  
			<p>Now, since we've got a product of two functions it seems like taking a product of the guesses for the individual pieces might work.  Doing this would give</p>
		  
			<me>C{{\bf{e}}^{4t}}\left( {At + B} \right)</me>
		  
			  <p>
				However, we will have problems with this.  As we will see, when we plug our guess into the differential equation we will only get two equations out of this.  The problem is that with this guess we've got three unknown constants.  With only two equations we won't be able to solve for all the constants.
			</p>
		  
			  <p>
				This is easy to fix however.  Let's notice that we could do the following
			</p>
		  
			<me>C{{\bf{e}}^{4t}}\left( {At + B} \right) = {{\bf{e}}^{4t}}\left( {ACt + BC} \right)</me>
		  
			  <p>
				If we multiply the <me>C</me> through, we can see that the guess can be written in such a way that there are really only two constants.  So, we will use the following for our guess.
			</p>
		  
			<me>{Y_P}\left( t \right) = {{\bf{e}}^{4t}}\left( {At + B} \right)</me>
		  
			  <p>Notice that this is nothing more than the guess for the <me>t</me> with an exponential tacked on for good measure.</p>
		  
			  <p>Now that we've got our guess, let's differentiate, plug into the differential equation and collect like terms.</p>
		  
			<md>
<mrow>{{\bf{e}}^{4t}}\left( {16At + 16B + 8A} \right) - 4\left( {{{\bf{e}}^{4t}}\left( {4At + 4B + A} \right)} \right) - 12\left( {{{\bf{e}}^{4t}}\left( {At + B} \right)} \right) <mrow> &amp;  = t{{\bf{e}}^{4t}}\\ \left( {16A - 16A - 12A} \right)t{{\bf{e}}^{4t}} + \left( {16B + 8A - 16B - 4A - 12B} \right){{\bf{e}}^{4t}} &amp; = t{{\bf{e}}^{4t}}</mrow> - 12At{{\bf{e}}^{4t}} + \left( {4A - 12B} \right){{\bf{e}}^{4t}} &amp; = t{{\bf{e}}^{4t}}</mrow>
</md>
		  
			  <p>Note that when we're collecting like terms we want the coefficient of each term to have only constants in it.  Following this rule we will get two terms when we collect like terms.  Now, set coefficients equal.</p>
		  
			<md> 
				<mrow> &amp;  t{{\bf{e}}^{4t}}\,: &amp; - 12A &amp; = 1 &amp; \Rightarrow  \hspace{0.25in}A &amp; =  - \frac{1}{{12}}</mrow>
				<mrow> &amp;  {{\bf{e}}^{4t}}\,: &amp;  4A - 12B &amp; = 0 &amp; \Rightarrow \hspace{0.25in}B &amp; =  - \frac{1}{{36}}</mrow>
			</md>
			<p>A particular solution for this differential equation is then</p>
			
				<me>{Y_P}\left( t \right) = {{\bf{e}}^{4t}}\left( { - \frac{t}{{12}} - \frac{1}{{36}}} \right) =  - \frac{1}{{36}}\left( {3t + 1} \right){{\bf{e}}^{4t}}</me>
		</solution>
	</example>

	<example>
		<statement> 
			Find a particular solution for the following differential equation.
			<me>y'' - 4y' - 12y = 3{{\bf{e}}^{5t}} + \sin \left( {2t} \right) + t{{\bf{e}}^{4t}}</me>
		</statement>
	  
		<solution>
			<p>This example is the reason that we've been using the same homogeneous differential equation for all the previous examples.  There is nothing to do with this problem.  All that we need to do it go back to the appropriate examples above and get the particular solution from that example and add them all together.</p>
			
			<p>Doing this gives</p>
			
				<me>{Y_P}\left( t \right) =  - \frac{3}{7}{{\bf{e}}^{5t}} + \frac{1}{{40}}\cos \left( {2t} \right) - \frac{1}{{20}}\sin \left( {2t} \right) - \frac{1}{{36}}\left( {3t + 1} \right){{\bf{e}}^{4t}}</me>
		</solution>
	</example>

</section>