<section xmlns:xi="http://www.w3.org/2001/XInclude"><title> Introduction </title>
	
	<p>
		Verifying that, say <m>y=e^{3x}+e^{4x}</m>, is a solution to the homogeneous equation
		<me>
			y'' - 4y' + 3y = 0
		</me>,
		involves plugging it into the left-hand side of the equation and simplifying. If it is a solution, then you would expect all the terms to cancel out, leaving you with zero so that the equation is satisfied. 
	</p>
	
	<p>
		In the case of a nonhomogeneous equation, 
		<me>
			y'' - 4y' + 3y = 9x
		</me>,
		you would instead expect the left side to simplify to <m>9x</m> after plugging in a solution. Let's brainstorm some functions that might simplify to <m>9x</m>. 
	</p>

	<p>
		<image width="75%">
			<latex-image>
			
				\begin{tikzpicture}[join=round,rounded corners,&gt;=stealth,shorten &gt;=1pt,shorten &lt;=1pt,thick]
					\node (text1) 	at (0.25,1.2) 	{\small 2 derivatives of \(y\)};
					\node (blank1) at (0.75,0.4) {};
					\filldraw[fill=blue!20,fill opacity=0.6]
						(0,0)--(1.5,0)--(1.5,0.5)--(0,0.5)--cycle;
					
					\node 			at (1.75,0.25)	{$-$};
					\node 			at (2.00,0.25)	{$4$};
					
					\node (text2) 	at (3.00,1.2) 	{\small 1 derivative of \(y\)};
					\node (blank2) at (3.00,0.4) {};
					\filldraw[fill=blue!20,fill opacity=0.6]
						(2.25,0)--(3.75,0)--(3.75,0.5)--(2.25,0.5)--cycle;
	
					\node 			at (4.00,0.25)	{$+$};
					\node 			at (4.25,0.25)	{$3$};
	
					\node (text3) 	at (5.25,1.2) 	{\small solution \(y\)};
					\node (blank3) at (5.25,0.4) {};
					\filldraw[fill=blue!20,fill opacity=0.6]
						(4.5,0)--(6.0,0)--(6.0,0.5)--(4.5,0.5)--cycle;
					\node 			at (6.25,0.25)	{$=$};
					\node 			at (6.70,0.25)	{$9x$};
					
					\draw[-&gt;,thick] (text1)		--	+(0,-0.3) -| (blank1); 
					\draw[-&gt;,thick] (text2)		--	+(0,-0.3) -| (blank2); 
					\draw[-&gt;,thick] (text3)		--	+(0,-0.3) -| (blank3); 
					
				\end{tikzpicture}
			</latex-image>
		</image>
	</p>

	<p>
		Since we need the left side to simplify to <m>9x</m>, it seems reasonable to consider functions that have <m>x</m> terms, such as polynomials. Let's try some below.
	</p>

	<p>
		<tabular top="minor" bottom="minor" right="minor" left="minor" halign="center">
			<col top="none" halign="center"/>
			<col halign="center"/>
			<col halign="right" right="none"/>
			<col halign="left"/>
			<col halign="center"/>
			<row left="none">
				<cell></cell>
				<cell><m>y</m></cell>
				<cell><m>y'' - 4y' + 3{\color{blue} y} =\!\!\!</m></cell>
				<cell>LHS</cell>
				<cell>LHS <m> \os{?}{=} 9x</m></cell>
			</row>

			<row>
				<cell>1</cell>
				<cell><m>3</m></cell>
				<cell><m>(3)'' - 4(3)' + 3({\color{blue} 3}) =\!\!\!</m></cell>
				<cell><m>{\color{blue} 9}</m></cell>
				<cell>No</cell>
			</row>

			<row>
				<cell>2</cell>
				<cell><m>3x</m></cell>
				<cell><m>(3x)'' - 4(3x)' + 3({\color{blue} 3x}) =\!\!\!</m></cell>
				<cell><m>-12 + {\color{blue} 9x}</m></cell>
				<cell>No</cell>
			</row>

			<row>
				<cell>3</cell>
				<cell><m>x^4</m></cell>
				<cell><m>(x^4)'' - 4(x^4)' + 3({\color{blue} x^4}) =\!\!\!</m></cell>
				<cell><m>12x^2 - 16x^3 + {\color{blue} 3x^4}</m></cell>
				<cell>No</cell>
			</row>

			<row>
				<cell>4</cell>
				<cell><m>x^2+3x</m></cell>
				<cell><m>(x^2+3x)'' - 4(x^2+3x)' + 3({\color{blue} x^2}+3x) =\!\!\!</m></cell>
				<cell><m>-10 + x + {\color{blue} 3x^2}</m></cell>
				<cell>No</cell>
			</row>

			<row>
				<cell>5</cell>
				<cell><m>3x-6</m></cell>
				<cell><m>(3x-6)'' - 4(3x-6)' + 3({\color{blue} 3x}-6) =\!\!\!</m></cell>
				<cell><m>-30+{\color{blue} 9x}</m></cell>
				<cell>No</cell>
			</row>

			<row>
				<cell>6</cell>
				<cell><m>3x+4</m></cell>
				<cell><m>(3x+4)'' - 4(3x+4)' + 3({\color{blue} 3x}+4) =\!\!\!</m></cell>
				<cell><m>{\color{blue} 9x}</m></cell>
				<cell>Yes</cell>
			</row>
		</tabular>
	</p>

	<p>
		Based on this table, we note that the correct solution is <m>y = 3x + 4</m> and
		<ul marker="square">
			<li>
				<p>
					Row 1 shows that a constant term alone could never produce an <m>x</m> term.
				</p>
			</li>
			<li>
				<p>
					Derivatives reduce the power of a polynomial, so the highest power term (highlighted in blue) comes from the <m>y</m> term.
					<fn>
						<m>y'' - 4y' + \os{\large y\text{ term}}{\boxed{3y}}</m>
					</fn>
				</p>
			</li>
			<li>
				<p>
					Rows 3 &amp; 4 illustrate the solution can't have a <m>x^2</m> or higher-degree term.
				</p>
			</li>
			<li>
				<p>
					Row 6 shows the solution (<m>3x+4</m>) needed an <m>x</m> term and constant term even though the right-hand side, <m>9x</m>, has only an <m>x</m> term.
				</p>
			</li>
		</ul>
	</p>

	<!-- <outcomes>
	
		<ul marker="square">
			<li>
				<p>
					Part of the general solution to an <xref ref="lncc-equation" text="custom">LNCC equation</xref> requires a specific function to account for the non-homogeneous term, <m>f(x)</m>. This part of the general solution is referred to as the <em>particular solution</em>.
				</p>
			</li>
			<li>
				<p>
					The <em>particular solution</em> often resembles the nonhomogeneous term, <m>f(x)</m>.
				</p>
			</li>
		</ul>
		
	</outcomes> -->
	
	<xi:include href="./p3-c2-s1-interactives.ptx" />

</section>