<!-- LICENSING
  This file is part of the textbook "Exploring Differential Equations, An Interactive, Student-Centered Approach" by Geoffrey Cox.
  License: Creative Commons Attribution-ShareAlike 4.0 International (CC BY-SA 4.0)
  You are free to:
    ‚Ä¢ Share ‚Äî copy and redistribute the material in any medium or format.
    ‚Ä¢ Adapt ‚Äî remix, transform, and build upon the material for any purpose, even commercially.
  Under the following terms:
    ‚Ä¢ Attribution ‚Äî You must give appropriate credit, provide a link to the license, and indicate if changes were made.
    ‚Ä¢ ShareAlike ‚Äî If you remix, transform, or build upon the material, you must distribute your contributions under the same license.
  Full license text: https://creativecommons.org/licenses/by-sa/4.0/legalcode
  Recommended attribution: "Exploring Differential Equations" by Geoffrey Cox, licensed CC BY-SA 4.0.
-->
<section label="showing-separability"> 
	<title>Showing Separability</title>

	<introduction>
		<p>
			Separable equations are often not presented in a <xref ref="separable" text="custom">separable form</xref>. In such cases, you'll need to rewrite the equation to verify it's separable. This process typically involves two main steps:
			<ol>
				<li>
					<p>
						<term>Isolate the derivative</term> on one side of the equation <m>\left(\dfrac{dy}{dx} = \ldots\right)</m>,
					</p>
				</li>
				<li>
					<p>
						Then form the product on the other side <m>\left(\dfrac{dy}{dx} = f(x) \cdot g(y)\right)</m>.
					</p>
				</li>
			</ol>
		</p>

		<p>
			Common algebra techniques to achieve this product include:
			<dl width="wide">
				<li xml:id="sums-to-products">
					<title>Sums <e component="emoji">‚ûú</e> Products</title>
					<m>\quad ab + ac = a \cdot (b + c)</m>
				</li>
				<li xml:id="exponents-to-products">
					<title>Exponents <e component="emoji">‚ûú</e> Products</title>
					<m>\quad a^{m + n} = a^m \cdot a^{n}</m>, <m>\quad a^{m - n} = \sfrac{a^m}{a^n}</m>
				</li>
				<li xml:id="fractions-to-products">
					<title>Fractions <e component="emoji">‚ûú</e> Products</title> 
					<m>\quad \dfrac{a}{b} = \dfrac{a}{1} \cdot \dfrac{1}{b}</m>,
					<m>\quad \dfrac{ab}{cd} = \dfrac{a}{c} \cdot \dfrac{b}{d}</m>
				</li>
			</dl>
		</p>

		<p>
			To illustrate this, consider the following warm-up examples.
		</p>
	</introduction>

	<subsection>
		<title>Warm-Up Examples</title>
		
		<p>
			Show that the differential equations are separable.
		</p>

		<example xml:id="example-show-separable-warmup-1">
			<statement><p><m>y' = y x^2 - y</m></p></statement>

			<solution>
				<p>
					To show this equation is separable, we convert <xref ref="sums-to-products" text="title"/> by factoring out the common <m>y</m>:
					<me>
						y' = \ub{y \cdot (x^2 - 1)}_{f(x)\ \cdot\ g(y)} \quad\leftarrow\text{separable}.
					</me>
				</p>
			</solution>
		</example>

		<example xml:id="example-show-separable-warmup-2">
			<statement><p><m>y' + 18xy = 6x</m></p></statement>

			<solution>
				<p>
					This time we isolate <m>y'</m> first, then factor out <m>x</m>:
					<me>
						y' = 6x - 18xy = 6x \cdot \left(1 - 3y\right) \quad\leftarrow\textit{separable}.
					</me>
				</p>
			</solution>
		</example>

		<example xml:id="example-show-separable-warmup-3">
			<statement><p><m>y y' - 1 = x</m></p></statement>

			<solution>
				<p>
					First, isolate <m>y'</m>:
					<me>
						yy' = x + 1 \quad \Rightarrow \quad y' = \frac{x + 1}{y},
					</me>
					then convert <xref ref="fractions-to-products" text="title"/>:
					<me>
						y' 
							= \frac{x + 1}{1} \cdot \frac{1}{y} 
							= \ub{(x+1) \cdot \frac{1}{y}}_{f(x)\ \cdot\ g(y)} \quad \leftarrow \text{separable}.
					</me>
				</p>
			</solution>
		</example>

		<example xml:id="example-show-separable-warmup-4">
			<statement><p><m>y' = {\large e^{x+y}}</m></p></statement>

			<solution>
				<p>
					At first glance, this doesn't look separable because of the <m>x+y</m>, but applying <xref ref="exponents-to-products" text="title"/> we get: 
					<me>
						{\large y' = e^{x+y} = \ub{e^x \cdot e^{y}}_{f(x)\ \cdot\ g(y)}} \quad\leftarrow\text{separable}.
					</me>
				</p>
			</solution>
		</example>

		<p>
			The next set of examples requires more work to demonstrate separability.
		</p>

	</subsection>

	<subsection>
		<title>Challenging Examples</title>

		<p>
			Show that the differential equations are separable.
		</p>

		<example xml:id="example-show-separable-1">
			<statement><p><m>P^2\dfrac{dP}{dt} + \dfrac{dP}{dt} = Pt</m></p></statement>

			<solution>
				<p>
					Since the variables in this equation are <m>t</m> and <m>P</m>, the separable form will look like
					<me>\dfrac{dP}{dt} = f(P) \cdot g(t)</me>.
				</p>

				<p>
					To get there, we isolate <m>dP/dt</m> first:
					<md>
						<mrow> P^2\dfrac{dP}{dt} + \dfrac{dP}{dt} \amp = Pt </mrow>
						<mrow> (1+P^2)\dfrac{dP}{dt} \amp = Pt </mrow>
						<mrow> \dfrac{dP}{dt} \amp = \dfrac{Pt}{1+P^2}. </mrow>
					</md>
				</p>

				<p>
					Now, we split the fraction so that <m>P</m> and <m>t</m> can be separated:
					<me>
						\dfrac{dP}{dt}
							= \dfrac{P\cdot t}{(P^2 + 1) \cdot (1)}
							= \ub{
								{\color{RoyalBlue}	\os{f(P)}{\os{\downarrow}{	\dfrac{P}{P^2 + 1}}}		} \cdot
								{\color{green}	\os{g(t)}{\os{\downarrow}{	\dfrac{t}{1}}}			}
							}_{\text{separable form}}.
					</me>
					So, the equation is <em>separable</em>.
				</p>
			</solution>
		</example>

		<!-- <example xml:id="example-show-separable-2">
			<statement><p><m>\normalsize\dfrac{dM}{d\omega} - 11e^{\omega + 3M} = 0</m></p></statement>

			<solution>
				<p>
					Isolating the derivative and applying <m>e^{A + B} = e^{A} \cdot e^{B}</m> leads to the separable form:
					<me>
						\dfrac{dM}{d\omega}
							= 11e^{\omega + 3M}
							= 11(e^{\omega} \cdot e^{3M})
							= \ub{
								{\color{RoyalBlue} \os{f(\omega)}{ \os{\downarrow}{ 11e^{\omega} }}	} \cdot
								{\color{green}\os{g(M)}{ \os{\downarrow}{ e^{3M} }}	}
							}_{\text{separable form}}.
					</me>
				</p>
			</solution>
		</example> -->

		<example xml:id="example-show-separable-3">
			<statement><p><m>y\dfrac{dy}{dx} + 8x^2e^{x + \cos y} = 6x^2e^x</m></p></statement>

			<solution>
				<p>
					This example uses a little of everything we discussed, so strap in.
				</p>

				<p>
					Noticing that the equation is first-order, we start by isolating <m>dy/dx</m>
					<md>
						<mrow>
							y\dfrac{dy}{dx} + 8x^2e^{x + \cos y} = 6x^2e^x
						</mrow>
						<mrow>
							\dfrac{dy}{dx} = \dfrac{6x^2e^x - 8x^2e^{x + \cos y}}{y}
						</mrow>
					</md>
				</p>

				<p>
					Next, we can rewrite the exponent in the numerator as a product
					<me>
						\dfrac{dy}{dx} = \dfrac{6x^2e^x - 8x^2e^{x}e^{\cos y}}{y}
					</me>
					and recognize that there is a common factor in the numerator
					<me>
						\dfrac{dy}{dx} = \dfrac{2x^2e^x(3 - 4e^{\cos y})}{y}
					</me>.
				</p>

				<p>
					From here, we write the result as a product of fractions,
					<me>
						\dfrac{dy}{dx} = \dfrac{2x^2e^x}{1} \cdot \dfrac{3 - 4e^{\cos y}}{y}
					</me>,
					and the equation is now clearly <em>separable</em>.
				</p>
			</solution>
		</example>

		<p>
			Learning to recognize when an equation is separable is the first step in applying the method of separation of variables, which we will discuss in the next section.
		</p>

		<exercise label="showing-separability-cyu-1">
			<task label="showing-separability-cyu-1-task-1">
				<title>Steps to Show Separable</title>

				<statement>
					<p>
						Suppose you want to show that the differential equation
						<me>\dfrac{dq}{dt} - 3qt^2 = 2q</me>
						is separable.
					</p>
					<p>
						Match the scrambled tasks (on the left) to the order in which they should be performed to show separability.
					</p>
				</statement>
				<cardsort>
					<match>
						<premise>check the equation is 1st-order</premise>					
						<response>The first task is to ...</response>
					</match>
					<match>
						<premise>move <m>3qt^2</m> to the left side via subtraction</premise>
						<response>Then, the second task is to ...</response>
					</match>
					<match>
						<premise>factor out a common factor of <m>q</m> on the left side</premise>
						<response>The final step is to ...</response>
					</match>
					<match>
						<premise>check the equation is linear</premise>					
						<premise>integrate both sides</premise>
						<premise>divide both sides by <m>3q</m></premise>
					</match>
				</cardsort>
			</task>

			<task label="showing-separability-cyu-1-task-2">
				<title><e component="emoji">üìñ‚ùì</e> Match the Needed Technique</title>

				<statement>
					<p>
						Match the technique required to demonstrate that each equation is separable.
					</p>
					<p>
						Drag the technique from the left to the equation on the right.
					</p>
				</statement>
				<feedback>
					<p>
						Review it
					</p>
				</feedback>
				<cardsort>
					<match>
						<premise>
							<p>
								<m>e^{A+B} = e^A \cdot e^B</m>
							</p>
						</premise>
						<response>
							<p>
								<m>\quad w' = w e^{t+w} </m>
							</p>
						</response>
					</match>
					<match>
						<premise>
							<p>
								<m>\quad\dfrac{A\cdot B}{C\cdot D} = \dfrac{A}{C} \cdot \dfrac{B}{D}</m>
							</p>
						</premise>
						<response>
							<p>
								<m>\quad\dfrac{dy}{d\theta} = \dfrac{3y}{(y+9)\theta} </m>
							</p>
						</response>
					</match>
					<match>
						<premise>
							<p>
								<m>\text{Isolate the derivative}</m>
							</p>
						</premise>
						<response>
							<p>
								<m>\quad xr' + 2r = 0 </m>
							</p>
						</response>
					</match>
					<match>
						<premise>
							<p>
								<m>\text{Take out a common factor}</m>
							</p>
						</premise>
						<response>
							<p>
								<m>\quad\dfrac{dP}{dt} = e^t P^2 - e^t </m>
							</p>
						</response>
					</match>
					<match>
						<premise>
							<p>
								<m>\text{No technique is needed}</m>
							</p>
						</premise>
						<response>
							<p>
								<m>\quad w' = e^Q e^{x}</m>
							</p>
						</response>
					</match>
				</cardsort>
			</task>

			<task label="showing-separability-cyu-1-task-3">
				<statement>
					<p>
						How can the equation, below, be rewritten to show it is separable?
						<me>
							\dfrac{dy}{dx} = \dfrac{y}{x+y}.
						</me>	
					</p>
				</statement>

				<choices>
					<choice>
						<statement>
							<p>
								<m>\quad\dfrac{dy}{dx} = y\left(\dfrac{1}{x} + \dfrac{1}{y}\right)</m>
							</p>
						</statement>
						<feedback>
							<p>
								Incorrect. This rewriting does not effectively separate the variables.
							</p>
						</feedback>
					</choice>
					<choice>
						<statement>
							<p>
								<m>\quad\dfrac{dy}{dx} = \dfrac{1}{x}\left(y + 1\right)</m>
							</p>
						</statement>
						<feedback>
							<p>
								Incorrect. This form still combines <m>x</m> and <m>y</m> terms in a way that is not separable.
							</p>
						</feedback>
					</choice>
					<choice>
						<statement>
							<p>
								<m>\quad\dfrac{dy}{dx} = \dfrac{1}{x}\cdot y - \dfrac{1}{x}</m>
							</p>
						</statement>
						<feedback>
							<p>
								Incorrect. This rewriting is not equivalent and does not separate the variables.
							</p>
						</feedback>
					</choice>
					<choice correct="yes">
						<statement>
							<p>
								This equation is not separable.
							</p>
						</statement>
						<feedback>
							<p>
								Correct! This equation is not separable, so it is impossible to write it in separable form.
							</p>
						</feedback>
					</choice>
				</choices>
			</task>

			<task label="showing-separability-cyu-1-task-4">
				<title><e component="emoji">ü§îüí≠</e> Find the Separable Equations</title>

				<statement>
					<p>
						Click on each of the separable differential equations below.
					</p>
				</statement>
				<areas>
					<tabular>
						<row><cell><m/></cell></row>
						<row>
							<cell><area correct="no">
								<m>\quad\dfrac{dy}{dx} = \dfrac{x + y}{xy}</m>
							</area></cell><cell/>
							<cell><area correct="yes">
								<m>\quad\dfrac{dy}{dx} = \dfrac{1}{x^2} + \dfrac{y}{x^2}</m>
							</area></cell>
						</row>
						<row><cell><m/></cell></row>
						<row>
							<cell><area correct="no">
								<m>\quad\dfrac{dy}{dx} = \dfrac{\sin(x+y)}{x}</m>
							</area></cell><cell/>
							<cell><area correct="yes">
								<m>\quad\dfrac{dy}{dx} = y \cdot e^{-x}</m>
							</area></cell>
						</row>
						<row><cell><m/></cell></row>
						<row>
							<cell><area correct="no">
								<m>\quad\dfrac{dy}{dx} = \dfrac{3}{x+y}</m>
							</area></cell><cell/>
							<cell><area correct="no">
								<m>\quad\dfrac{dy}{dx} = \cos(xy)</m>
							</area></cell>
						</row>
						<row><cell><m/></cell></row>
						<row>
							<cell><area correct="no">
								<m>\quad\dfrac{dy}{dx} = x - 3y</m>
							</area></cell><cell/>
							<cell><area correct="no">
								<m>\quad\dfrac{dy}{dx} = x^2 + y</m></area></cell>
						</row>
						<row><cell><m/></cell></row>
					</tabular>
				</areas>
				<feedback>
					<p>
						A differential equation is separable if you can rearrange it to express it as a product of functions involving only <m>x</m> and <m>y</m> separately. Look for equations that can be manipulated into this form, even if they do not initially appear separable.
					</p>
				</feedback>
			</task>
		</exercise>

		<example xml:id="example-non-separable-2">
			<statement>
				<p>
					Explain why the differential equations are NOT separable.
					<ol marker="A." cols="2">
						<li><m>\normalsize\dfrac{d^2y}{dx^2} = xy^2</m></li>
						<li><m>\normalsize\dfrac{dy}{dx} = -6x + 2y</m></li>
						<li><m>xy' + 3x = y</m></li>
						<li><m>y' = x^2y^2 + y</m></li>
						<li><m>y' = \cos(xy)</m></li>
					</ol>
				</p>
			</statement>

			<solution>
				<p>
					The first equation is a bit of a trick question to remind you of the first-order requirement of a separable equation. Since this equation is second-order, <em>separability does not apply</em>.
				</p>

				<p>
					This equation is first-order but not separable. To see this, we can rearrange the equation to isolate the derivative:
					<md>
						<mrow> xy' + 3x = y </mrow>
						<mrow> xy' = y - 3x </mrow>
						<mrow> y' = \dfrac{y - 3x}{x} </mrow>
					</md>.
					Since there is no common factor of <m>x</m> or <m>y</m> in the numerator, the variables cannot be separated, and the equation is not separable.
				</p>
			</solution>
		</example>

	</subsection>

</section>
