
<subsection xmlns:xi="http://www.w3.org/2001/XInclude"><title> Exercises </title>

	<xi:include href="./c4-exercises-conceptual.ptx" />

	<exercises><title> Solve the Differential Equations </title>
		
		<exercisegroup><title> Forward Product Rule </title>
	
			<introduction>
				Compute the derivative of each of the following functions.
			</introduction>

			<exercise>
				<statement>
					<m> \, \ds f(x) = \ln x\cos x </m>
				</statement>
				<answer>
					<p>
						<line><m> \ds f'(x)	= \left(\frac{1}{x}\right)\cos x + \ln x \left(-\sin x\right) = \frac{\cos x}{x} - \ln x \sin x</m></line>
					</p>
				</answer>
			</exercise>
	
		</exercisegroup>

		<exercisegroup><title> The Integrating Factor </title>
		
			<introduction>
				Find the integrating factor of each of the following differential equations.
			</introduction>

			<exercise>
				<statement>
					<m> \ds y' - 4y = x </m>
				</statement>
				<answer>
					<p>
						<line><m> \ds </m></line>
					</p>
				</answer>
			</exercise>
	
		</exercisegroup>
	
		<exercisegroup><title> General Solution </title>
		
			<introduction>
				Use an integrating factor to find the general solution to each equation.
			</introduction>
		
			<exercise>
				<statement>
					<m> \ds \frac{dy}{dx} - y = e^{3x} </m>
					<p/>
				</statement>
				<solution>
					<p>
				First we note that this DE is already in standard form for a first-order linear DE, <m> \ds \frac{dy}{dx} + P(x)y = f(x), </m> with <m> \ds P(x) = -1. </m>  Then we find the integrating factor <m> \ds z. </m>
					<md>
						<mrow>  z	 \amp =  e^{\Big(\mbox{an antiderivative of <m> \ds P(x) </m> }\Big)} </mrow>
						<mrow>   \amp =  e^{\Big(\mbox{an antiderivative of <m> \ds -1 </m> }\Big)} </mrow>
						<mrow>   \amp =  e^{-x} </mrow>

					</md>
					Now we multiply both sides of the DE by the integrating factor.
					<md>
						<mrow>  e^{-x}\cdot\frac{dy}{dx} - e^{-x}y	 \amp =  e^{-x}e^{3x} \nonumber </mrow>
						<mrow>  e^{-x}\cdot\frac{dy}{dx} - e^{-x}y	 \amp =  e^{2x}\nonumber  </mrow>
						<mrow>  \underbrace{e^{-x}}_{f}\cdot\underbrace{\frac{dy}{dx}}_{g'} + \underbrace{- e^{-x}}_{f'}\cdot\underbrace{y}_{g}  \amp =  e^{2x} \label{eq1}  </mrow>
					</md>
					Now we recall the product rule for derivatives: <m> \ds \frac{d}{dx}\Big( f\cdot g \Big) = f\cdot g' + f' \cdot g. </m> We note that the two terms on the left hand side of equation (\ref{eq1}) are the result of taking the derivative of the product.  Hence we can undo the product rule as follows: <m> \ds\frac{d}{dx}\Big(e^{-x}\cdot y \Big) = e^{2x}.</m> Now we can integrate both sides of the equation and then solve for the dependent variable.
					<md>
						<mrow>  \int \frac{d}{dx}\Big(e^{-x}\cdot y \Big)dx	 \amp =  \int e^{2x} dx </mrow>
						<mrow>  e^{-x}\cdot y	 \amp =  \frac{1}{2}e^{2x} + C </mrow>
						<mrow>  y	 \amp =  \frac{1}{2}\frac{e^{2x}}{e^{-x}} + \frac{C}{e^{-x}} </mrow>
						<mrow>   \amp =  \frac{1}{2}e^{2x}e^x + Ce^x </mrow>
						<mrow>   \amp =  \frac{1}{2}e^{3x} + Ce^x </mrow>

					</md>

					</p>
				</solution>
				<answer>
					<p>
						<m> \ds y = \frac{1}{2}e^{3x} + Ce^x </m>
					</p>
				</answer>
			</exercise>

			<exercise>
				<statement>
					<m> \ds \frac{dy}{dx} = \frac{y}{x} + 2x + 1 </m> , where <m> \ds x>0 </m>
					<p/>
				</statement>
				<solution>
					<p>
				First we put DE in standard form for a first-order linear DE <m> \ds \frac{dy}{dx} + P(x)y = f(x), </m> so we can identify <m> \ds P(x). </m>
					<md>
						<mrow>  \frac{dy}{dx}	 \amp =  \frac{y}{x} + 2x + 1 </mrow>
						<mrow>  \frac{dy}{dx} - \frac{y}{x}	 \amp =   2x + 1 </mrow>
						<mrow>  \frac{dy}{dx} + \left(- \frac{1}{x}\right)y	 \amp =   2x + 1 </mrow>

					</md>
					Thus, <m> \ds P(x) = - \frac{1}{x}. </m>  Then we find the integrating factor <m> \ds z. </m>
					<md>
						<mrow>  z	 \amp =  e^{\Big(\mbox{an antiderivative of <m> \ds P(x) </m> }\Big)} </mrow>
						<mrow>   \amp =  e^{\mbox{\Big(an antiderivative of <m> \ds -\frac{1}{x} </m> }\Big)} </mrow>
						<mrow>   \amp =  e^{-\ln|x|} </mrow>
						<mrow>   \amp =  e^{\ln (|x|^{-1})} </mrow>
						<mrow>   \amp =  |x|^{-1} </mrow>
						<mrow>   \amp =  \frac{1}{|x|} </mrow>
						<mrow>   \amp =  \frac{1}{x} \mbox{ (since <m> \ds x>0 </m> )}  </mrow>
					</md>
					Now we multiply both sides of the DE by the integrating factor.
					<md>
						<mrow>  \frac{1}{x}\cdot\frac{dy}{dx} + \frac{1}{x}\cdot \left(- \frac{1}{x}\right)y  \amp =  \frac{1}{x}(2x + 1) \nonumber </mrow>
						<mrow>  \frac{1}{x}\cdot\frac{dy}{dx} + \left(-\frac{1}{x^2}\right)\cdot y  \amp =  2 + \frac{1}{x} \nonumber </mrow>
						<mrow>  \underbrace{\frac{1}{x}}_{f}\cdot\underbrace{\frac{dy}{dx}}_{g'} + \underbrace{\left(-\frac{1}{x^2}\right)}_{f'}\cdot \underbrace{y}_{g}  \amp =  2 + \frac{1}{x} \label{eq2}  </mrow>
					</md>
					Now we recall the product rule for derivatives: <m> \ds \frac{d}{dx}\Big( f\cdot g \Big) = f\cdot g' + f' \cdot g. </m> We note that the two terms on the left hand side of equation (\ref{eq2}) are the result of taking the derivative of the product.  Hence we can undo the product rule as follows: <m> \ds\frac{d}{dx}\Big(\frac{1}{x}\cdot y \Big) = 2 + \frac{1}{x}.</m> Now we can integrate both sides of the equation and then solve for the dependent variable.
					<md>
						<mrow>  \int \frac{d}{dx}\Big(\frac{1}{x}\cdot y \Big)dx	 \amp =  \int \left(2 + \frac{1}{x} \right)dx </mrow>
						<mrow>  \frac{1}{x}\cdot y	 \amp =  2x + \ln|x| + C </mrow>
						<mrow>  \frac{1}{x}\cdot y	 \amp =  2x + \ln(x) + C \mbox{ (since <m> \ds x>0) </m> } </mrow>
						<mrow>  y	 \amp =  x \cdot (2x + \ln(x) + C) </mrow>
						<mrow>   \amp =  2x^2 + x\ln x + Cx </mrow>

					</md>

					</p>
				</solution>
				<answer>
					<p>
						<m> \ds y = 2x^2 + x\ln x + Cx </m>
					</p>
				</answer>
			</exercise>

			<exercise>
				<statement>
					<m> \ds \frac{dr}{d\theta} + r\tan \theta = \sec \theta, </m> where <m> \ds -\frac{\pi}{2} \le \theta \le \frac{\pi}{2} </m>
					<p/>
				</statement>
				<solution>
					<p>
				First we put DE in standard form for a first-order linear DE <m> \ds \frac{dy}{dx} + P(x)y = f(x), </m> so we can identify <m> \ds P(x). </m>  Notice that for this DE <m> \ds \theta </m> is the independent variable (i.e., it is like the <m> \ds x </m> ) and <m> \ds r </m> is the dependent variable (i.e., it is like the <m> \ds y </m> ).  Hence the standard form we will aim for is <m> \ds \frac{dr}{d\theta} + P(\theta)r = f(\theta), </m> and we want to identify <m> \ds P(\theta). </m>
					<md>
						<mrow>  \frac{dr}{d\theta} + r\tan \theta	 \amp =  \sec \theta </mrow>
						<mrow>  \frac{dr}{d\theta} + \tan \theta\cdot r	 \amp =  \sec \theta </mrow>

					</md>
					Thus, <m> \ds P(\theta) = \tan \theta. </m>  Then we find the integrating factor <m> \ds z. </m>
					<md>
						<mrow>  z	 \amp =  e^{\Big(\mbox{an antiderivative of <m> \ds P(\theta) </m> }\Big)} </mrow>
						<mrow>   \amp =  e^{\Big(\mbox{an antiderivative of <m> \ds \tan \theta </m> }\Big)} </mrow>
						<mrow>   \amp =  e^{-\ln|\cos \theta|} </mrow>
						<mrow>   \amp =  e^{\ln (|\cos \theta|^{-1})} </mrow>
						<mrow>   \amp =  |\cos \theta|^{-1} </mrow>
						<mrow>   \amp =  \frac{1}{|cos \theta|} </mrow>
						<mrow>   \amp =  \frac{1}{\cos \theta} \mbox{ (since <m> \ds -\frac{\pi}{2} \le \theta \le \frac{\pi}{2} </m> )} </mrow>
						<mrow>   \amp = \sec \theta </mrow>

					</md>
					Now we multiply both sides of the DE by the integrating factor.
					<md>
						<mrow>  \sec\theta \cdot\frac{dr}{d\theta} + \sec \theta\cdot \tan \theta\cdot r  \amp =  \sec\theta\cdot \sec \theta \nonumber </mrow>
						<mrow>  \sec\theta \cdot\frac{dr}{d\theta} + \sec \theta \tan \theta\cdot r  \amp =  \sec^2\theta \nonumber </mrow>
						<mrow>  \underbrace{\sec\theta}_{f} \cdot\underbrace{\frac{dr}{d\theta}}_{g'} + \underbrace{\sec \theta \tan \theta}_{f'}\cdot \underbrace{r}_{g}  \amp =  \sec^2\theta \label{eq3}  </mrow>
					</md>
					Now we recall the product rule for derivatives: <m> \ds \frac{d}{dx}\Big( f\cdot g \Big) = f\cdot g' + f' \cdot g. </m> We note that the two terms on the left hand side of equation (\ref{eq3}) are the result of taking the derivative of the product.  Hence we can undo the product rule as follows: <m> \ds\frac{d}{dx}\Big(\sec\theta\cdot r \Big) = \sec^2\theta.</m> Now we can integrate both sides of the equation and then solve for the dependent variable.
					<md>
						<mrow>  \int \frac{d}{dx}\Big(\sec\theta\cdot r \Big)d\theta	 \amp =  \int(\sec^2\theta) d\theta </mrow>
						<mrow>  \sec\theta\cdot r	 \amp =  \tan \theta + C </mrow>
						<mrow>  r	 \amp =  \frac{\tan \theta}{\sec\theta} + \frac{C}{\sec \theta} </mrow>
						<mrow>   \amp =  \tan\theta \cdot \cos \theta + C\cos\theta </mrow>
						<mrow>   \amp =  \frac{\sin\theta}{\cos\theta}\cdot \cos\theta + C\cos\theta </mrow>
						<mrow>   \amp =  \sin \theta + C\cos \theta </mrow>

					</md>

					</p>
				</solution>
				<answer>
					<p>
						<m> \ds r = \sin \theta + C\cos \theta </m>
					</p>
				</answer>
			</exercise>

			<exercise>
				<statement>
					<m> \ds y\frac{dx}{dy} + 2x = 5y^3 </m>
					<p/>
				</statement>
				<solution>
					<p>
				First we put DE in standard form for a first-order linear DE <m> \ds \frac{dy}{dx} + P(x)y = f(x), </m> so we can identify <m> \ds P(x). </m> ...EXCEPT for this DE, the roles of <m> \ds x </m> and <m> \ds y </m> are switched. Notice that here <m> \ds y </m> is the independent variable and <m> \ds x </m> is the dependent variable.  So we will aim for the standard for <m> \ds \frac{dx}{dy} + P(y)x = f(y), </m> and we want to identify <m> \ds P(y). </m>
					<md>
						<mrow>  y\frac{dx}{dy} + 2x	 \amp =  5y^3 </mrow>
						<mrow>  \frac{dx}{dy} + \frac{2}{y}x	 \amp =  5y^2 </mrow>

					</md>
					Thus, <m> \ds P(y) =  \frac{2}{y}. </m>  Then we find the integrating factor <m> \ds z. </m>
					<md>
						<mrow>  z	 \amp =  e^{\Big(\mbox{an antiderivative of <m> \ds P(y) </m> }\Big)} </mrow>
						<mrow>   \amp =  e^{\Big(\mbox{an antiderivative of <m> \ds \frac{2}{y} </m> }\Big)} </mrow>
						<mrow>   \amp =  e^{2\ln|y|} </mrow>
						<mrow>   \amp =  e^{\ln(|y|^2)} </mrow>
						<mrow>   \amp =  |y|^2 </mrow>
						<mrow>   \amp = y^2 </mrow>

					</md>
					Now we multiply both sides of the DE by the integrating factor.
					<md>
						<mrow>  y^2\cdot \frac{dx}{dy} + y^2\cdot \frac{2}{y}x	 \amp =  y^2\cdot 5y^2 \nonumber </mrow>
						<mrow>  y^2\cdot \frac{dx}{dy} + 2y\cdot x	 \amp =  5y^4 \nonumber </mrow>
						<mrow>  \underbrace{y^2}_{f} \cdot\underbrace{\frac{dx}{dy}}_{g'} + \underbrace{2y}_{f'}\cdot \underbrace{x}_{g}  \amp =  5y^4 \label{eq4}  </mrow>
					</md>
					Now we recall the product rule for derivatives: <m> \ds \frac{d}{dy}\Big( f\cdot g \Big) = f\cdot g' + f' \cdot g. </m> We note that the two terms on the left hand side of equation (\ref{eq4}) are the result of taking the derivative of the product.  Hence we can undo the product rule as follows: <m> \ds\frac{d}{dy}\Big(y^2\cdot x \Big) = 5y^4.</m> Now we can integrate both sides of the equation and then solve for the dependent variable.
					<md>
						<mrow>  \int \frac{d}{dy}\Big(y^2\cdot x \Big)dy	 \amp =  \int(5y^4) dy </mrow>
						<mrow>  y^2\cdot x	 \amp =  y^5 + C </mrow>
						<mrow>  x	 \amp =  \frac{y^5}{y^2} + \frac{C}{y^2} </mrow>
						<mrow>   \amp =  y^3 + \frac{C}{y^2} </mrow>

					</md>

					</p>
				</solution>
				<answer>
					<p>
						<m> \ds x = y^3 + \frac{C}{y^2} </m>
					</p>
				</answer>
			</exercise>
	
		</exercisegroup>
	
		<exercisegroup><title> Initial-Value Problems </title>
			<introduction>
				Solve each initial value problem
			</introduction>

			<exercise>
				<statement>
					<m> \ds \frac{dy}{dx} - \frac{y}{x} = xe^x, </m> where <m> \ds x>1 </m> and <m> \ds y(1) = e-1 </m>
					<p/>
				</statement>
				<solution>
					<p>
						<m> \ds \frac{dy}{dx} - \frac{y}{x} = xe^x, </m> where <m> \ds x>1 </m> and <m> \ds y(1) = e-1 </m>
					</p>
				</solution>
				<answer>
					<p>
	
					</p>
				</answer>
			</exercise>

			<exercise>
				<statement>
					<m> \ds e^t z' = 1 - 4e^t z, \hspace{0.5cm} \ds z(0) = \frac{4}{3} </m>
					<p/>
				</statement>
				<solution>
					<p>
						<m> \ds e^t z' = 1 - 4e^t z, \hspace{0.5cm} \ds z(0) = \frac{4}{3} </m>
					</p>
				</solution>
				<answer>
					<p>
	
					</p>
				</answer>
			</exercise>
	
		</exercisegroup>

		<exercise>
			<task label="rename-this"><title> <em>Multiple-Choice</em> </title>
				<statement>
					<em>What is the method used to solve the differential equation <me>\frac{d}{dx}[g(x,y)] = f(x)</me>?</em>
				</statement>
				<choices>
					<choice correct="yes">
						<statement>Direct integration.</statement>
						<feedback>Correct! The equation is solved by integrating both sides with respect to <m>x</m>.</feedback>
					</choice>
					<choice>
						<statement>Separation of variables.</statement>
						<feedback>Incorrect. Separation of variables is used when the variables can be separated, but here the equation is solved by direct integration.</feedback>
					</choice>
					<choice>
						<statement>Substitution.</statement>
						<feedback>Incorrect. Substitution is a different method. The correct method here is direct integration.</feedback>
					</choice>
					<choice>
						<statement>Partial fractions.</statement>
						<feedback>Incorrect. Partial fractions are used to simplify the integration process, but the primary method here is direct integration.</feedback>
					</choice>
				</choices>
			</task>
		</exercise>
	
	</exercises>

</subsection>