<section><title> Orphaned Content </title>

	<introduction>
		<p>
			This is just a place to put content that was written and may or not be used.
		</p>
	</introduction>

	<example><title> Verify our solution </title>

		<p>
			<p>
				Verify that
				<me>z = \tan(t+C)</me>
				is the particular solution to the initial value problem
				<me>z' - 1 = z^2, \quad z(4) = 9</me>
			</p>
		</p>
		
		<p>
			<solution>
				<p>
					As in the previous example, we don't have to check our answer, but one of the best parts about DEs is that we always can check, which means we can really know if we have the right solution. Let's check this one. We will substitute our solution back into the DE and verify that when we do, we get the same thing on both sides of the equation.
		
					<md>
						<mrow> LHS	\amp = z' -1</mrow>
						<mrow> \amp = \frac{d}{dt}\Big( \tan(t+C) \Big) - 1</mrow>
						<mrow> \amp = \sec^2(t+C)\cdot \frac{d}{dt}(t+C) - 1</mrow>
						<mrow> \amp = \sec^2(t+C)\cdot (1+0) - 1</mrow>
						<mrow> \amp = \sec^2(t+C) - 1</mrow>
					</md>
		
					<md>
						<mrow> RHS	\amp = z^2</mrow>
						<mrow> \amp = \Big( \tan(t+C) \Big)^2</mrow>
						<mrow> \amp = \tan^2(t+C)</mrow>
					</md>
		
				</p>
		
				<p>
					At first glance, it looks like we have different expressions on the left and right hand sides of the equation. However, if we recall the trigonometric identity
		
						<me>\tan^2 x = \sec^2 x - 1,</me>
		
					then we can see that these expressions are, in fact equivalent. Thus, we have verified that <m>z = \tan(t+C)</m>, where <m>C</m> is any constant, is a solution to the DE <m>z' -1 = z^2</m>.
				</p>
		
				<p>
					Now that we've practiced this solution technique a couple of times, let's summarize.
				</p>
			</solution>
		</p>

	</example>

</section>