<subsection xml:id="r-01-14" xmlns:xi="http://www.w3.org/2001/XInclude"><title> Completing the Square </title>

	<assemblage xml:id="completing-the-square"><title> ✳️ Completing the Square </title>
		<p>
			Completing the square is a tool to rewrite a quadratic expression like <m>x^2 + bx + c</m> into the form:
			<md>
				<mrow> \left(x - \frac{b}{2}\right)^2 + \text{a number} </mrow>
			</md>
		</p>

		<p>
			The strategy is as follows:
			<md>
				<mrow>
					x^2 + bx + c	
					=\amp\ \ub{x^2 + bx + \os{(\large \text{half of } b)^2}{\boxed{\left(\frac{b}{2}\right)^2}}}_{\Large \left(x - \frac{b}{2}\right)^2}
					- \ub{\os{(\large \text{half of } b)^2}{\boxed{\left(\frac{b}{2}\right)^2}} + c}_{\Large\text{a number}}
				</mrow>
			</md>
		</p>
	</assemblage>

	<p>
		<me>
			x^2 + bx = \ub{x^2 + bx + \left(\frac{b}{2}\right)^2}_{\left(x + \frac{b}{2}\right)^2} - \left(\frac{b}{2}\right)^2 = \left(x + \frac{b}{2}\right)^2 - \left(\frac{b}{2}\right)^2
		</me>.
	</p>
	

	<p>
		Let's walk through a few examples to illustrate how completing the square can simplify the inverse Laplace transform process.
	</p>

	<example><title> <em>Complete the Square of each Quadratic</em> </title>
		
		<solution><title> <m>x^2 + 6x + 10</m> </title>
			<p>
				Since <m>(\text{half of } b)^2 = (6/2)^2 = 9</m>, we add and substract <m>9</m>.
				<me>
					x^2 + 6x + 10 = x^2 + 6x + \boxed{9} - \boxed{9} + 10 = (x + 3)^2 + 1.
				</me>
			</p>
		</solution>

		<solution><title> <m>x^2 - 4x + 13</m> </title>
			<p>
				Since <m>(\text{half of } b)^2 = (4/2)^2 = 4</m>, we add and substract <m>4</m>.
				<me>
					x^2 - 4x + 13 = x^2 - 4x + \boxed{4} - \boxed{4} + 13 = (x - 2)^2 + 9.
				</me>
			</p>
		</solution>

		<solution><title> <m>x^2 + 8x + 20</m> </title>
			<p>
				Since <m>(\text{half of } b)^2 = (8/2)^2 = 16</m>, we add and substract <m>16</m>.
				<me>
					x^2 + 8x + 20 = x^2 + 8x + \boxed{16} - \boxed{16} + 20 = (x + 4)^2 + 4.
				</me>
			</p>
		</solution>

	</example>

	<p>
		<term> Complete the square for each of the following expressions. Verify by expanding
		your expression.</term>

		<ol>
			<li> <m>x^2 + 8x + 28 \qquad</m>		
				<solution>
					<p>
						<md>
							<mrow>x^2 + 8x + 28	=\amp\ (x^2 + 8x + 16) - 16 + 28						</mrow>
							<mrow>				=\amp\ (x+4)^2 - 16+28								</mrow>
							<mrow>				=\amp\ (x+4)^2 + 12									</mrow>
						</md>
					</p>
				</solution>
				<answer>
					<p>
						<m> (x+4)^2 + 12 </m>
					</p>
				</answer>
			</li>

			<li> <m>x^2 - 12x \qquad</m>		
			<solution>
				<p>
			<md>
				<mrow>x^2 - 12x	=\amp\ (x^2 - 12x + 36) - 36								</mrow>
				<mrow>			=\amp\ (x-6)^2 - 36										</mrow>
			</md>
				</p>
			</solution>
			<answer>
				<p>
					<m> (x-6)^2 - 36 </m>
				</p>
			</answer>
			</li>

			<li> <m>2x^2 - 8x - 7 \qquad</m>		
			<solution>
				<p>
			<md>
				<mrow>2x^2 - 8x - 7	=\amp\ (2x^2 - 8x) - 7								</mrow>
				<mrow>				=\amp\ 2(x^2 - 4x) - 7								</mrow>
				<mrow>				=\amp\ 2(x^2 - 4x + 4 - 4) - 7						</mrow>
				<mrow>				=\amp\ 2(x^2 - 4x + 4) - 8 - 7						</mrow>
				<mrow>				=\amp\ 2(x-2)^2 - 8 - 7								</mrow>
				<mrow>				=\amp\ 2(x-2)^2 - 15									</mrow>
			</md>
				</p>
			</solution>
			<answer>
				<p>
					<m> 2(x-2)^2 - 15 </m>
				</p>
			</answer>
			</li>
			
			<li> <m>4x^2  + 8x - 65 \qquad</m>
			<solution>
				<p>
			(Needs to be written)	
			<md>
				<mrow>		=\amp\ 														</mrow>
				<mrow>		=\amp\ 														</mrow>
				<mrow>		=\amp\ 														</mrow>
			</md>
				</p>
			</solution>
			<answer>
				<p>
					<m> 	 </m>
				</p>
			</answer>
			</li>
			
			<li> <m>-2x^2 + 20x -47 \qquad</m>
			<solution>
				<p>
			(Needs to be written)	
			<md>
				<mrow>		=\amp\ 														</mrow>
				<mrow>		=\amp\ 														</mrow>
				<mrow>		=\amp\ 														</mrow>
			</md>
				</p>
			</solution>
			<answer>
				<p>
					<m> 	 </m>
				</p>
			</answer>
			</li>
			
			<li> <m>-x^2 - 16x - 57 \qquad</m>		
			<solution>
				<p>
			<md>
				<mrow>-x^2 - 16x - 57	=\amp\ -(x^2 +16x) - 57							</mrow>
				<mrow>					=\amp\ -(x^2 +16x + 64 - 64) - 57				</mrow>
				<mrow>					=\amp\ -(x^2 + 16x + 64) + 64 -57				</mrow>
				<mrow>					=\amp\ -(x+8)^2 + 64 - 57						</mrow>
				<mrow>					=\amp\ -(x+8)^2 + 7								</mrow>
			</md>		
				</p>
			</solution>
			<answer>
				<p>
					<m> -(x+8)^2 + 7 </m>
				</p>
			</answer>
			</li>
		</ol>
	</p>
	
</subsection>