<subsection xml:id="r-01-21" xmlns:xi="http://www.w3.org/2001/XInclude">

<title> Interrelated functions </title>

{


<p>
In differential equations, we will encounter functions involving subscripts that are interrelated.  Let's
look at an example like that.

	<p>
	If you prefer to see a video of this example,
	<xref ref="video-interrelated_functions_01" text="custom"> click here </xref>
	</p>

	\begin{quote}
	<em> Example:</em>  Suppose:
		<md><mrow>	x_{n+1}	=\amp\ x_n + 0.5,</mrow>
		<mrow>y_{n+1}	=\amp\ [y_n\cdot (x_n)^2 + 1]x_{n+1} + y_n,</mrow>
		<mrow>x_0	=\amp\ 3, \mbox{ and}</mrow>
		<mrow>y_0	=\amp\ 2.</mrow>
	</md>
		Find the values of <m>y_1</m> and <m>y_2.</m>

	<answer>\it Answer:}
	
		First we would try to find <m>y_1.</m>  Notice that when we use the formula, we have
			<me> y_1 = [y_0\cdot (x_0)^2 + 1]x_1 + y_0. </me>
		While we do have the values of <m>x_0</m> and <m>y_0,</m> we don't yet have the value
		of <m>x_1.</m>  So we'll find that first:
		<md><mrow>	x_1	=\amp\ x_0 + 0.5</mrow>
		<mrow>=\amp\ 3 + 0.5</mrow>
		<mrow>=\amp\ 3.5</mrow>
	</md>
		
		Now we have all the information we need to find <m>y_1:</m>
		<md><mrow>	y_1	=\amp\ [y_0\cdot (x_0)^2 + 1]x_1 + y_0</mrow>
		<mrow>=\amp\ [2\cdot 3^2 + 1](3.5) + 2</mrow>
		<mrow>=\amp\ 68.5</mrow>
	</md>
		
		Now we proceed in the same manner.  First we find <m>x_2:</m>
		<md><mrow>	x_2	=\amp\ x_1 + 0.5</mrow>
		<mrow>=\amp\ 3.5 + 0.5</mrow>
		<mrow>=\amp\ 4</mrow>
	</md>
		
		Then we find <m>y_2:</m>
		<md><mrow>	y_2	=\amp\ [y_1\cdot (x_1)^2 + 1]x_2 + y_1</mrow>
		<mrow>=\amp\ [68.5\cdot 3.5^2 + 1](4) + 68.5</mrow>
		<mrow>=\amp\ 3429</mrow>
	</md>
		
	\end{quote}
	}
		</answer>
<ol>
	
		<li>
  Find <m>y_2</m> given the following information about <m>x_n</m> and <m>y_n.</m>
		<md><mrow>	x_{n+1}	=\amp\ x_n + 1,				\amp x_0 =\amp\ 2</mrow>
		<mrow>y_{n+1}	=\amp\ 3\cdot x_{n+1} + y_n		\amp y_0 =\amp\ -3</mrow>
	</md>
			
	<solution>
		<p>
	<md>
		<mrow>n = 0:  	x_1	=\amp\ x_0 +1</mrow>
		<mrow>=\amp\ 2 +1</mrow>
		<mrow>=\amp\ 3</mrow>
		<mrow>\amp</mrow>
		<mrow>y_1	=\amp\ 3\cdot x_1 + y_0</mrow>
		<mrow>=\amp\ 3\cdot 3 + (-3)</mrow>
		<mrow>=\amp\ 6</mrow>
		<mrow>\amp</mrow>
		<mrow>n = 1:  	x_2	=\amp\ x_1 + 1</mrow>
		<mrow>=\amp\ 3 +1</mrow>
		<mrow>=\amp\ 4</mrow>
		<mrow>\amp</mrow>
		<mrow>y_2	=\amp\ 3\cdot x_2 + y_1</mrow>
		<mrow>=\amp\ 3\cdot 4 + 6</mrow>
		<mrow>=\amp\ 18</mrow>
	</md>
		
		
		</p>
	</solution>
	<answer>
		<p>
			<me> y_2 = 18 </me>
		
		</p>
	</answer>

		
</li>
	
		<li>
  Find <m>y_2</m> given the following information about <m>x_n</m> and <m>y_n.</m>
		<md><mrow>	x_{n+1}	=\amp\ x_n + 1,							\amp x_0 = 0</mrow>
		<mrow>y_{n+1}	=\amp\ [x_n+y_n]^2\cdot[x_{n+1} - x_n] + y_n		\amp y_0 = 2</mrow>
	</md>
			
	<solution>
		<p>
	<md>
		<mrow>n = 0:  	x_1	=\amp\ x_0 +1</mrow>
		<mrow>=\amp\ 0 +1</mrow>
		<mrow>=\amp\ 1</mrow>
		<mrow>\amp</mrow>
		<mrow>y_1	=\amp\ [x_0+y_0]^2\cdot[x_1 - x_0] + y_0</mrow>
		<mrow>=\amp\ [0 + 2]^2\cdot[1 - 0] + 2</mrow>
		<mrow>=\amp\ 6</mrow>
		<mrow>\amp</mrow>
		<mrow>n = 1:  	x_2	=\amp\ x_1 + 1</mrow>
		<mrow>=\amp\ 1 +1</mrow>
		<mrow>=\amp\ 2</mrow>
		<mrow>\amp</mrow>
		<mrow>y_2	=\amp\ [x_1+y_1]^2\cdot[x_2 - x_1] + y_1</mrow>
		<mrow>=\amp\ [1+6]^2\cdot[2 - 1] + 6</mrow>
		<mrow>=\amp\ 55</mrow>
	</md>
		
		
		</p>
	</solution>
	<answer>
		<p>
			<me> y_2 = 55 </me>
		
		</p>
	</answer>

</li>
	
		<li>
  Find <m>y_2</m> given the following information about <m>x_n</m> and <m>y_n.</m>
		<md><mrow>	x_{n+1}	=\amp\ x_n + 2,					\amp x_0 = -1</mrow>
		<mrow>y_{n+1}	=\amp\ [3x_n - y_n^2]\cdot 2 + y_n		\amp y_0 = -6</mrow>
	</md>
			
	<solution>
		<p>
	<md>
		<mrow>n = 0:  	x_1	=\amp\ x_0 +2</mrow>
		<mrow>=\amp\ -1 +2</mrow>
		<mrow>=\amp\ 1</mrow>
		<mrow>\amp</mrow>
		<mrow>y_1	=\amp\ [3x_0 - y_0^2]\cdot 2 + y_0</mrow>
		<mrow>=\amp\ [3\cdot (-1) - (-6)^2]\cdot 2 + (-6)</mrow>
		<mrow>=\amp\ [-3-36]\cdot 2 - 6</mrow>
		<mrow>=\amp\ (-39)\cdot 2 - 6</mrow>
		<mrow>=\amp\ -78 - 6</mrow>
		<mrow>=\amp\ -84</mrow>
		<mrow>\amp</mrow>
		<mrow>n = 1:  	x_2	=\amp\ x_1 + 2</mrow>
		<mrow>=\amp\ 1 +2</mrow>
		<mrow>=\amp\ 3</mrow>
		<mrow>\amp</mrow>
		<mrow>y_2	=\amp\ [3x_1 - y_1^2]\cdot 2 + y_1</mrow>
		<mrow>=\amp\ [3\cdot1 - (-84)^2]\cdot 2 + (-84)</mrow>
		<mrow>=\amp\ [3 - 7056]\cdot 2 - 84</mrow>
		<mrow>=\amp\ (-7053)\cdot 2 - 84</mrow>
		<mrow>=\amp\ -14106 - 84</mrow>
		<mrow>=\amp\ -14190</mrow>
	</md>
		
		</p>
	</solution>
	<answer>
		<p>
			<me> y_2 = -14190 </me>
		
		</p>
	</answer>

		
	</li>
</ol></p>
</subsection>