<section label="laplace-piecewise-method">
	<title> Transforming Piecewise Functions </title>
	<introduction>
		<p>
			NEED AN INTRO
		</p>
	</introduction>

	<paragraphs>
		<title> General Strategy </title>
		<p>
			With all three step-function transform rules in place, we can now tackle full piecewise-defined functions.  
			The strategy is always the same:
		</p>

		<assemblage xml:id="piecewise-laplace-strategy">
			<title>üìú Strategy: Laplace Transform of a Piecewise Function </title>
			<p>
				To find <m>\lap{g(t)}</m> for a piecewise function:
				<ol>
					<li><xref ref="piecewise-to-unit-step" text="custom">Write <m>g(t)</m> using step functions.</xref></li>
					<li>Combine like <m>u_c(t)</m> terms.</li>
					<li>Apply <xref ref="lt-L9" text="custom">L<m>_9</m></xref> or <xref ref="lt-L10" text="custom">L<m>_{10}</m></xref> term-by-term.</li>
				</ol>
			</p>
		</assemblage>

		<p>
			<task label="prep-1-lap-piecewise"><title> Strategy Check: Laplace for Piecewise Functions </title>
				<statement correct="yes">
					<p>
						To take the Laplace transform of a piecewise function, you should first rewrite it in terms of unit step functions.
					</p>
				</statement>
				<feedback>
					<p>
						That's the foundation of this method! Once a piecewise function is rewritten using step functions, you can apply the shift rule to each piece.
					</p>
				</feedback>
			</task>

			<task label="prep-2-lap-piecewise"><title> Matching Each Interval to the Right Form </title>
			<statement>
				<p>
					Match each type of piecewise interval to the unit step expression that activates it.
				</p>
			</statement>
			<feedback>
				<p>
				These patterns should be second nature now, this matching is what allows us to build the step-based expression for the Laplace transform.
				</p>
			</feedback>
			<cardsort>
				<match>
				<premise><m>t \lt 3</m></premise>
				<response><m>1 - u_3(t)</m></response>
				</match>
				<match>
				<premise><m>3 \le t \lt 5</m></premise>
				<response><m>u_3(t) - u_5(t)</m></response>
				</match>
				<match>
				<premise><m>t \ge 5</m></premise>
				<response><m>u_5(t)</m></response>
				</match>
				<match>
				<premise><m>0 \le t \lt 2</m></premise>
				<response><m>u_0(t) - u_2(t)</m></response>
				</match>
			</cardsort>
			</task>
		</p>
	</paragraphs>

	<paragraphs>
		<title> Piecewise Functions in the Laplace Domain </title>

		<p>
			Let's apply this strategy to the forcing function of our nmodel problem, <m>g(t)</m>:
		</p>

		<p>
			1. <xref ref="piecewise-to-unit-step" text="custom">Write <m>g(t)</m> using step functions.</xref> The pieces, intervals and switches for <m>g</m> are:
		</p>

		<tabular halign="center">
			<col right="minor"/>
			<col right="minor"/>
			<row bottom="minor"> <cell>Piece</cell> <cell>Active Interval</cell> <cell>Step Function Switch</cell> </row>
			<row> <cell><me>2t</me></cell> <cell><me>0 \le t \lt 1		 </me></cell> <cell><me>u_0(t) - u_1(t)		</me></cell> </row>
			<row> <cell><me> 3</me></cell> <cell><me>1 \le t \lt 4 </me></cell> <cell><me>u_1(t) - u_4(t)	</me></cell> </row>
			<row> <cell><me> 0</me></cell> <cell><me>t \ge 4		 </me></cell> <cell><me>u_4(t)			</me></cell> </row>
		</tabular>

		<p>
			Multiplying each piece with its switch and summing them gives:
		</p>

		<me>
			g(t) = 2t\Big(u_0(t) - u_1(t)\Big) + 3\Big(u_1(t) - u_4(t)\Big) + 0\ u_4(t)
		</me>.

		<p>
			Combine like switch terms:
		</p>

		<me>
			g(t) = 2t\ u_0(t) + (3 - 2t)\ u_1(t) - 3\ u_4(t)
		</me>.

		<p>
			Now, we are ready to find the Laplace transform of <m>g</m>. Taking the Laplace transform of both sides and using linearity, we get <m>3</m> transforms:
			<me>
				\lap{g(t)} 
				= 2\ub{\lap{t\ u_0(t)}}_{\ds\text{1Ô∏è‚É£}} 
				+ \ub{\lap{(3 - 2t)\ u_1(t)}}_{\ds\text{2Ô∏è‚É£}} 
				- 3\ub{\lap{u_4(t)}}_{\ds\text{3Ô∏è‚É£}}
			</me>.
		</p>

		<p>
				1Ô∏è‚É£ Apply <xref ref="lt-L10" text="custom">L<m>_{10}</m></xref> with: <m>\quad c=0\quad</m> &amp; <m>\quad f(t) = t \quad\Rightarrow\quad f(t+0) = t</m>:
		</p>

		<md>
			<mrow>\lap{t\cdot u_0(t)} \amp = e^{-0s}\lap{f(t+0)} = \lap{t} = \frac1{s^2} </mrow>
		</md>

		<p>
				2Ô∏è‚É£ Apply <xref ref="lt-L10" text="custom">L<m>_{10}</m></xref> with: <m>\quad c=1\quad</m> &amp; <m>\quad f(t) = 3 - 2t \quad\Rightarrow\quad f(t+1) = 1-2t</m>:
		</p>

		<md>
			<mrow>\lap{(3 - 2t)\cdot u_1(t)} \amp = e^{-s}\lap{f(t+1)} = e^{-s}\lap{1-2t} = e^{-s}\left(\frac1{s} - \frac{2}{s^2}\right)</mrow>
		</md>

		<p>
				3Ô∏è‚É£ Apply <xref ref="lt-L9" text="custom">L<m>_{9}</m></xref> with: <m>\quad c=4</m>: <m>\quad\lap{u_4(t)} = \dfrac{e^{-4s}}{s}</m>
		</p>

		<p>
			Writing these together under one sum completes the Laplace transform:
		</p>

		<md>
			<mrow>\lap{g(t)} \amp =  \frac2{s^2} + \left(\frac1{s} - \frac{2}{s^2}\right)e^{-s} - \frac{3}{s}e^{-4s} </mrow>
		</md>

		<task label="chkpt-1-lap-piecewise"><title> Piecewise to Laplace </title>
			<statement>
				<p>
					A function is defined as:
					<me>
						f(t) = \left\{
						\begin{array}{ll}
							0, 		\amp t \lt 2 \\
							4, 		\amp 2 \le t \lt 5 \\
							t - 5,	\amp t \ge 5
						\end{array}
						\right.
					</me>
					What is <m>\lap{f(t)}</m> in terms of step functions and transforms?
				</p>
			</statement>
			<choices randomize="yes">
				<choice>
				<statement>
					<p>
					<m>\ds \lap{4\cdot (1 - u_2(t)) + (t - 5)\cdot u_5(t)}</m>
					</p>
				</statement>
				<feedback>
					<p>
					<m>1 - u_2(t)</m> is active before <m>t = 2</m>, but <m>f(t)</m> is zero there. That term doesn't match the interval.
					</p>
				</feedback>
				</choice>
				<choice>
				<statement>
					<p>
					<m>\ds \lap{4\cdot u_2(t) + (t - 5)\cdot u_5(t)}</m>
					</p>
				</statement>
				<feedback>
					<p>
					This expression turns <m>4</m> ON at <m>t = 2</m>, but never turns it OFF. We need an ON-window, not just a switch-on.
					</p>
				</feedback>
				</choice>
				<choice correct="yes">
				<statement>
					<p>
					<m>\ds \lap{4\cdot(u_2(t) - u_5(t)) + (t - 5)\cdot u_5(t)}</m>
					</p>
				</statement>
				<feedback>
					<p>
					Perfect. This captures <m>4</m> ON from <m>t = 2</m> to <m>t = 5</m> and <m>t - 5</m> turning ON at <m>t = 5</m>.
					</p>
				</feedback>
				</choice>
				<choice>
				<statement>
					<p>
					<m>\ds \lap{4\cdot(u_0(t) - u_2(t)) + (t - 5)\cdot u_2(t)}</m>
					</p>
				</statement>
				<feedback>
					<p>
					The function is 0 before <m>t = 2</m>, so the <m>u_0 - u_2</m> window doesn't apply here. Also, <m>t - 5</m> shouldn't turn ON at <m>t = 2</m>.
					</p>
				</feedback>
				</choice>
			</choices>
		</task>
	</paragraphs>

	<paragraphs>
		<title> Examples </title>
		<example><title> Transforming a 2-Part Piecewise Function </title>
			<statement>
				<p>
					Find the Laplace transform of the piecewise function:
					<me>
						g(t) = \left\{
						\begin{array}{ll}
							e^{-t},	\amp t \lt 1 \\
							3,		\amp t \ge 1
						\end{array}
						\right.
					</me>
				</p>
			</statement>
			<solution><title> <m>\rightarrow \lap{g(t)}</m> </title>
				<p>
					We begin by identifying the needed unit step functions.
					<me>
						g(t) =  \cdot
						\left\{
							\begin{array}{lll}
								e^{-t}, \amp t \lt 1 \quad \leftarrow (-\infty, 1): \amp 1-u_{1}(t)\\
								3,		\amp t \ge 1 \quad \leftarrow (1, \infty):	\amp u_{1}(t).
							\end{array}
						\right.
					</me>
				</p>

				<p>
					Then we can write <m>g(t)</m> as
					<me>
						g(t) = e^{-t} \cdot \left(1 - u_{1}(t)\right) + 3 \cdot u_{1}(t).
					</me>
				</p>

				<p>
					Combining like unit step function terms, we get
					<md>
						<mrow> 
							g(t) \amp 
							= e^{-t} - e^{-t} \cdot u_{1}(t) + 3 \cdot u_{1}(t)
						</mrow>
						<mrow>
							\amp 
							= e^{-t} + \left(-e^{-t} + 3\right) \cdot u_{1}(t)
						</mrow>,
					</md>
					and taking the Laplace transform of the last two terms separately.
					<me>
						\lap{g(t)} 
						= \us{\large\text{1Ô∏è‚É£}}{\ul{\lap{e^{-t}}}} 
						+ \us{\large\text{2Ô∏è‚É£}}{\ul{\lap{\left(3 - e^{-t}\right) \cdot u_{1}(t)}}}
					</me>
				</p>

				<sidebyside widths="5% 30% 65%" valign="middle">
					<p>1Ô∏è‚É£</p>
					<p><me>\lap{e^{-t}} = \frac{1}{s + 1}</me></p>
					<p/>
				</sidebyside>

				<p>
					<sidebyside widths="5% 60% 35%" valign="top">
						<p>2Ô∏è‚É£</p>
						<p>
							<md>
								<mrow> 
									\laplacesym \big\{\big({\DLO 3 }\ \amp {\DLO - e^{-t}}\big) \cdot u_{1}(t)\big\} 
								</mrow>
								<mrow> 
									\amp = e^{-s} \lap{{\DLO f(t + 1)}}
								</mrow>
								<mrow>				
									\amp = e^{-s} \lap{3 - e^{-t} \cdot e^{-1}}
								</mrow>
								<mrow> 
									\amp = e^{-s} \left(3\lap{1} - e^{-1}\lap{{e^{-t}}} \right)
								</mrow>
								<mrow> 
									\amp = e^{-s} \left(\frac{3}{s} - e^{-1} \cdot \frac{1}{s + 1}\right)
								</mrow>
							</md>
						</p>
						<p>
							<md>
								<mrow> \small\DLO f(t)\ 		\amp \small\DLO = 3 - e^{-t} </mrow>
								<mrow> \small\DLO f(t + 1)\ 	\amp \small\DLO = 3 - e^{-(t + 1)} </mrow>
								<mrow>						\amp \small\DLO = 3 - e^{-t} \cdot e^{-1} </mrow>
							</md>
						</p>
					</sidebyside>
				</p>

				<p>
					Combining 1Ô∏è‚É£ &amp; 2Ô∏è‚É£, we arrive at the Laplace transform
					<me>
						\lap{g(t)} 
						= \frac{1}{s + 1} + e^{-s} \left(\frac{3}{s} - \frac{e^{-1}}{s + 1}\right)
					</me>.
				</p>
			</solution>
			<solution>
				<title> Solution </title>
				<p>
					<term>Step 1:</term> Write <m>g(t)</m> using step functions.
					<me>
						g(t) = e^{-t}(1-u_1(t)) + 3u_1(t).
					</me>
				</p>
				<p>
					<term>Step 2:</term> Combine like terms where possible.
					<md>
						<mrow>
							g(t) \amp = e^{-t} - e^{-t}u_1(t) + 3u_1(t)
						</mrow>
						<mrow>
							\amp = e^{-t} + \big(3 - e^{-t}\big) u_1(t)
						</mrow>
					</md>
				</p>
				<p>
					<term>Step 3:</term> Take the Laplace transform term by term.
				</p>
				<ul marker="disc">
					<li><m>\lap{e^{-t}} = \frac{1}{s+1}</m></li>
					<li><m>\lap{(3 - e^{-t}) u_1(t)} = e^{-s} \lap{3 - e^{-(t+1)}} </m></li>
				</ul>
				<p>
					The second Laplace transform uses the rule <m>\lap{f(t) u_c(t)} = e^{-cs} \lap{f(t+c)}</m>.
				</p>
				<p>
					<term>Step 4:</term> Put it all together:
					<me>
						\lap{g(t)} = \frac{1}{s+1} + e^{-s}\left( \frac{3}{s} - \frac{e^{-1}}{s+1} \right).
					</me>
				</p>
			</solution>
		</example>

		<example><title> Forward Transform with Step Functions </title>
			<statement>
				<p>
					Apply the Laplace transform to both sides of the differential equation:
					<me>
						y'' + y = \left\{
						\begin{array}{ll}
							0,       \amp t \lt 1 \\
							3t,      \amp 1 \le t \lt 2 \\
							0,       \amp t \ge 2
						\end{array}
						\right., 
						\qquad
						y(0) = 0,\quad y'(0) = 0
					</me>
				</p>
			</statement>

			<solution><title> <m>\rightarrow</m> Laplace equation (Step 1) </title>
				<p>
					The forcing function is active only from <m>t = 1</m> to <m>t = 2</m>, so we rewrite it using a unit step window:
					<me>
						g(t) = 3t \cdot \left(u_1(t) - u_2(t)\right).
					</me>
				</p>

				<p>
					Apply the Laplace transform to both sides of the DE:
					<me>
						\lap{y'' + y} = \lap{3t \cdot (u_1(t) - u_2(t))}.
					</me>
					On the left-hand side, using <m>y(0) = y'(0) = 0</m>, we have:
					<me>
						s^2 Y(s) + Y(s).
					</me>
				</p>

				<p>
					On the right-hand side, distribute the Laplace transform:
					<me>
						\lap{3t \cdot (u_1(t) - u_2(t))} = 3\lap{t \cdot u_1(t)} - 3\lap{t \cdot u_2(t)}.
					</me>

					Use the shift rule for each term:
					<md>
						<mrow> \lap{t \cdot u_1(t)} = e^{-s} \lap{t + 1} = e^{-s} \cdot \lap{t + 1} </mrow>
						<mrow> \lap{t \cdot u_2(t)} = e^{-2s} \lap{t + 2} = e^{-2s} \cdot \lap{t + 2} </mrow>
					</md>

					Now apply linearity and known transforms:
					<md>
						<mrow> \lap{t + c} = \lap{t} + c\lap{1} = \frac{1}{s^2} + \frac{c}{s} </mrow>
					</md>

					So:
					<md>
						<mrow>
							\lap{3t \cdot (u_1 - u_2)} 
							\amp = 3e^{-s}\left(\frac{1}{s^2} + \frac{1}{s}\right) 
							- 3e^{-2s}\left(\frac{1}{s^2} + \frac{2}{s}\right)
						</mrow>
					</md>
				</p>

				<p>
					Combining both sides, we arrive at the Laplace equation:
					<me>
						(s^2 + 1)Y(s) = 3e^{-s}\left(\frac{1}{s^2} + \frac{1}{s}\right) 
						- 3e^{-2s}\left(\frac{1}{s^2} + \frac{2}{s}\right).
					</me>
					This completes Step 1.
				</p>
			</solution>
		</example>

		<p>
			These worked examples illustrate how the three step-function Laplace rules combine into one powerful method for handling any piecewise function you might encounter.
		</p>
	</paragraphs>

</section>