<section label="piecewise-worked-examples">
	<title> Worked Examples </title>
	<introduction>
		<p>
			Full examples showing the complete process from rewriting the forcing function, through the Laplace domain, and back to the time domain.
		</p>

		<p>
			These examples follow the same roadmap you've used all along: transform, solve, prepare, and invert. The only new ingredient is handling piecewise forcing functions with unit step notation. Once that's done, the method proceeds just as before, with a few exponential twists.
		</p>
	</introduction>

	<subsection><title> Worked Example 1 </title>

		<paragraphs>
			<title> The Model Equation </title>

			<p>
				We will walk through the Laplace Method by solving the following initial value problem with a piecewise forcing term:
			</p>

			<mdn>
				<mrow xml:id="lt-method-piecewise-model-eqn"> 
					\amp 
					\begin{array}{l}
						y'' + y = g(t) \\
						y(0) = 0,\ y'(0) = 0
					\end{array}
					\quad\text{where}\quad g(t) =
					\left\{
					\begin{array}{ll}
						2t, \amp 0 \le t \lt 1 \\
						3,  \amp 1 \le t \lt 4 \\
						0,  \amp t \ge 4
					\end{array}
					\right.
				</mrow>
			</mdn>

			<p>
				Summarize the differences...
			</p>
		</paragraphs>

		<paragraphs label="piecewise-forward">
			<title> Step 1 — Into the Laplace Domain </title>
			<p>
				Recall that our first step is to apply the Laplace transform of both sides of <xref provisional="lt-method-piecewise-model-eqn"/>:
				<me>
					\lap{y'' + y} = \lap{g(t)}
				</me>
			</p>

			<p>
				It's clear how to handle the left-side, but the right-side requires the transform of a piecewise function. Before we can use the rules we derived in this chapter, we first need to write <m>g(t)</m> in unit step form.
			</p>

			<p>
				Apply the Laplace transform to both sides of the differential equation:
				<me>
					y'' + y = \left\{
					\begin{array}{ll}
						0,       \amp t \lt 1 \\
						3t,      \amp 1 \le t \lt 2 \\
						0,       \amp t \ge 2
					\end{array}
					\right., 
					\qquad
					y(0) = 0,\quad y'(0) = 0
				</me>
			</p>

			<p>
				The forcing function is active only from <m>t = 1</m> to <m>t = 2</m>, so we rewrite it using a unit step window:
				<me>
					g(t) = 3t \cdot \left(u_1(t) - u_2(t)\right).
				</me>
			</p>

			<p>
				Apply the Laplace transform to both sides of the DE:
				<me>
					\lap{y'' + y} = \lap{3t \cdot (u_1(t) - u_2(t))}.
				</me>
				On the left-hand side, using <m>y(0) = y'(0) = 0</m>, we have:
				<me>
					s^2 Y(s) + Y(s).
				</me>
			</p>

			<p>
				On the right-hand side, distribute the Laplace transform:
				<me>
					\lap{3t \cdot (u_1(t) - u_2(t))} = 3\lap{t \cdot u_1(t)} - 3\lap{t \cdot u_2(t)}.
				</me>

				Use the shift rule for each term:
				<md>
					<mrow> \lap{t \cdot u_1(t)} = e^{-s} \lap{t + 1} = e^{-s} \cdot \lap{t + 1} </mrow>
					<mrow> \lap{t \cdot u_2(t)} = e^{-2s} \lap{t + 2} = e^{-2s} \cdot \lap{t + 2} </mrow>
				</md>

				Now apply linearity and known transforms:
				<md>
					<mrow> \lap{t + c} = \lap{t} + c\lap{1} = \frac{1}{s^2} + \frac{c}{s} </mrow>
				</md>

				So:
				<md>
					<mrow>
						\lap{3t \cdot (u_1 - u_2)} 
						\amp = 3e^{-s}\left(\frac{1}{s^2} + \frac{1}{s}\right) 
						- 3e^{-2s}\left(\frac{1}{s^2} + \frac{2}{s}\right)
					</mrow>
				</md>
			</p>

			<p>
				Combining both sides, we arrive at the Laplace equation:
				<me>
					(s^2 + 1)Y(s) = 3e^{-s}\left(\frac{1}{s^2} + \frac{1}{s}\right) 
					- 3e^{-2s}\left(\frac{1}{s^2} + \frac{2}{s}\right).
				</me>
				This completes Step 1.
			</p>

			<p>
				Now that we've built the Laplace equation, the remaining steps are familiar. We'll solve for <m>Y(s)</m>, simplify, and invert. But there's one twist: the presence of <m>e^{-cs}</m> terms means we'll need special care when taking the inverse Laplace transform. Let's explore that next.
			</p>
		</paragraphs>

		<paragraphs label="piecewise-laplace-domain">
			<title> Step 2 — Solving in the Laplace Domain </title>
			
		</paragraphs>

		<paragraphs label="piecewise-inverse">
			<title> Step 3 — Leaving the Laplace Domain </title>

			<p>
				Once we've solved for <m>Y(s)</m> in the Laplace domain, the final challenge is to take the inverse Laplace transform. When the forcing function was continuous, this step relied on partial fractions and matching terms from the Laplace table. That still works here, but now we'll also see terms involving exponentials like <m>e^{-cs}F(s)</m>.
			</p>

			<p>
				These exponentials come directly from transforming unit step expressions. To move back to the <m>t</m>-domain, we need a new tool: a rule that undoes the exponential shift.
			</p>

		</paragraphs>

	</subsection>

	<subsection><title> Worked Example 2 </title>

		<p>
			Solve the initial value problem:
			<me>
				2y' + y = g(t), \quad y(0) = 0,
				\qquad\text{where}\qquad
				g(t) =
				\left\{
				\begin{array}{ll}
					3,       \amp 0 \le t \lt 2 \\
					1,       \amp 2 \le t \lt 4 \\
					t - 4,   \amp t \ge 4
				\end{array}
				\right.
			</me>
		</p>

		<paragraphs><title>Step 1: Apply the Laplace Transform to Both Sides</title>
			<p>
				Apply the Laplace transform to both sides:
				<me>
					2\lap{y'} + \lap{y} = \lap{g(t)}
				</me>
			</p>

			<p>
				Using <xref ref="L9-eqn" text="custom"><m>L_{9}</m></xref> with the initial condition <m>y(0) = 1</m>, we get
				<me>
					2(sY(s) - 1) + Y(s) = \lap{g(t)}
				</me>
			</p>
				
			<p>
				To compute <m>\lap{g(t)}</m>, we first rewrite <m>g(t)</m> in terms of unit step functions:
			</p>

			<md>
				<mrow>
					g(t)\amp
					= 3\big(u_0(t)-u_2(t)\big) + 1\big(u_2(t) - u_4(t)\big) + (t - 4)u_4(t)
				</mrow>
				<mrow>
					\amp
					= 3u_0(t) - 2u_2(t) + (t - 4)u_4(t)
				</mrow> 
			</md>

			<p>
				and by rules <xref ref="L13-eqn" text="custom"><m>L_{13}</m></xref> and <xref ref="L14-eqn" text="custom"><m>L_{14}</m></xref>, we have:
				<md>
					<mrow>
						\lap{g(t)}\amp
						= 3\ob{\lap{u_0(t)}}^{\large 1/s} - 2\ob{\lap{u_2(t)}}^{\large e^{-2s}/s} + \ob{\lap{(t - 4)u_4(t)}}^{\large e^{-4s} \cdot \lap{t}}
					</mrow>
					<mrow>
						\amp
						= \frac{3}{s} - \frac{2e^{-2s}}{s} + e^{-4s}\cdot \frac{1}{s^2}
					</mrow>
				</md>
			</p>

			<p>
				Thus, the Laplace domain equation is:
				<me>
					2(sY(s) - 1) + Y(s) = \frac{3}{s} - \frac{2e^{-2s}}{s} + \frac{e^{-4s}}{s^2}
				</me>.
			</p>
		</paragraphs>

		<paragraphs><title>Step 2: Solve for <m>Y(s)</m></title>
			<p>
				Rearranging the equation so that all <m>Y(s)</m> terms are on one side:
				<me>
					2sY(s) + Y(s) = 2 + \frac{3}{s} - \frac{2e^{-2s}}{s} + \frac{e^{-4s}}{s^2}
				</me>.
				Factoring out <m>Y(s)</m>, on the left, and dividing by <m>2s + 1</m> completes step 2:
				<me>
					Y(s) = \frac{1}{2s + 1}\left(2 + \frac{3}{s} - \frac{2e^{-2s}}{s} + \frac{e^{-4s}}{s^2}\right)
				</me>
			</p>
		</paragraphs>

		<paragraphs><title>Step 3: Prepare <m>Y(s)</m> for an Inverse Transform</title>
			<p>
				We aim to write <m>Y(s)</m> as a sum of terms of the form <m>F_i(s)e^{-cs}</m>. Start by distributing:
				<me>
					Y(s) = \frac{2}{2s + 1} + \frac{3}{s(2s + 1)} - \frac{2e^{-2s}}{s(2s + 1)} + \frac{e^{-4s}}{s^2(2s + 1)}
				</me>
			</p>

			<p>
				Next, we separate and label each <em>different</em> rational part, <m>F_i(s)</m>:
			</p>

			<me>
				Y(s) 
				= \ub{\frac{2}{2s + 1}}_{\large F_1(s)} 
				+ 3\ub{\frac{1}{s(2s + 1)}}_{\large F_2(s)} 
				- 2\ub{\frac{1}{s(2s + 1)}}_{\large F_2(s)} \cdot e^{-2s}
				+ \ub{\frac{1}{s^2(2s + 1)}}_{\large F_3(s)} \cdot e^{-4s}
			</me>

			<aside>
				<p>
					Note: We doubled up on <m>F_2(s)</m> since it appears twice in <m>Y(s)</m>.
				</p>
			</aside>
			
			<p>
				So <m>Y(s)</m> is now in the form:
			</p>

			<me>
				Y(s) = F_1(s) + 3F_2(s) -2F_2(s)e^{-2s} + F_3(s)e^{-4s}
			</me>

			<p>
				<m>F_1(s)</m> is ready, but <m>F_2(s)</m> and <m>F_3(s)</m> need partial fraction decomposition for step 4:
			</p>

			<me>
				F_2(s) = \frac{1}{s} - \frac{2}{2s + 1},
				\qquad\text{and}\qquad
				F_3(s) = \frac{-2}{s} + \frac{1}{s^2} + \frac{4}{2s + 1}
			</me>

			<solution><title> Full Partial Fraction Decomposition Details of <m>F_2(s)</m> and <m>F_3(s)</m> </title>
				<p>
					For <m>F_2(s)</m>, the general form is:
					<me>
						\frac{1}{s(2s + 1)} = \frac{A}{s} + \frac{B}{2s + 1}
					</me>
					Multiplying through and grouping <m>s</m> terms:
					<md>
						<mrow> 1 \amp = A(2s + 1) + Bs</mrow> 
						<mrow> 1 \amp = 2As + A + Bs</mrow> 
						<mrow> 1 \amp = (2A + B)s + A</mrow> 
					</md>
					Leads to:
					<me>
						\begin{array}{l}
							2A + B = 0 \\
							A = 1
						\end{array}
						\qquad\Rightarrow\qquad
						\begin{array}{l}
							A = 1 \\
							B = -2
						\end{array}
					</me>

					Thus,
					<me>
						F_2 = \frac{1}{s} - \frac{2}{2s + 1}
					</me>

					<m>F_3(s)</m> can be found similarly:
					<me>
						F_3(s) = \frac{1}{s^2(2s + 1)} = \frac{A}{s} + \frac{B}{s^2} + \frac{C}{2s + 1}
					</me>
					Multiplying through and grouping <m>s</m> terms:
					<md>
						<mrow> 1 \amp = As(2s + 1) + B(2s + 1) + Cs^2</mrow> 
						<mrow> 1 \amp = 2As^2 + As + 2Bs + B + Cs^2</mrow>
						<mrow> 1 \amp = (2A + C)s^2 + (A + 2B)s + B</mrow>
					</md>
					Leads to:
					<me>
						\begin{array}{l}
							2A + C = 0 \\
							A + 2B = 0 \\
							B = 1
						\end{array}
						\qquad\Rightarrow\qquad
						\begin{array}{l}
							A = -2 \\
							B = 1 \\
							C = 4
						\end{array}
					</me>
					Thus,
					<me>
						F_3(s) = \frac{-2}{s} + \frac{1}{s^2} + \frac{4}{2s + 1}
					</me>
				</p>
			</solution>
		</paragraphs>

		<paragraphs><title> Step 4: Invert <m>Y(s)</m> to Recover <m>y(t)</m> </title>
			<p>
				We now compute the inverse transform:
				<me>
					y(t) = \ilap{F_1(s)} + 3\ilap{F_2(s)} -2\ilap{F_2(s)e^{-2s}} + \ilap{F_3(s)e^{-4s}}
				</me>
			</p>
			<p>
				Focusing on just the inverse transforms of the <m>F_i(s)</m> terms:
			</p>
			
			<md>
				<mrow>
					\succ\quad\ilap{F_1(s)}\amp
					= \ilap{\frac{2}{2s + 1}} = 2e^{-\frac{1}{2}t}
				</mrow>
				<mrow>
					\succ\quad\ilap{F_2(s)}\amp
					= \ilap{\frac{1}{s}} - \ilap{\frac{2}{2s + 1}} = {\DLBb 1 - 2e^{-\frac{1}{2}t} \quad\leftarrow f_2(t)}
				</mrow>
				<mrow>
					\succ\quad\ilap{F_3(s)}\amp
					= \ilap{\frac{-2}{s}} + \ilap{\frac{1}{s^2}} + \ilap{\frac{4}{2s + 1}}
				</mrow>
				<mrow>
					\amp
					= {\DLO -2 + t + 2e^{-\frac{1}{2}t} \quad\leftarrow f_3(t)}
				</mrow>
			</md>

			<p>
				Now, we can apply <xref ref="L15-eqn" text="custom"><m>L_{15}</m></xref> to get the other inverse transforms: 
			</p>

			<md>
				<mrow>
					\succ\quad\ilap{F_2(s)e^{-2s}} \amp
					= {\DLBb f_2(t - 2)}u_2(t)
					= \left({\DLBb 1 - 2e^{-\frac{1}{2}(t - 2)}}\right)u_2(t)
				</mrow>
				<mrow>
					\succ\quad\ilap{F_3(s)e^{-4s}} \amp
					= {\DLO f_3(t - 4)}u_4(t)
					= \left({\DLO (t - 4) - 2 + 2e^{-\frac{1}{2}(t - 4)}}\right)u_4(t)
				</mrow>
			</md>

			<p>
				Finally, putting everything together, the solution is:
			</p>

			<md>
				<mrow>
					y(t)
					= 2e^{-\frac{1}{2}t} + 3 - 6e^{-\frac{1}{2}t} - 2\amp\
					\left(1 - 2e^{-\frac{1}{2}(t - 2)}\right)u_2(t)
				</mrow>
				<mrow>
					+ \amp\
					\left((t - 4) - 2 + 2e^{-\frac{1}{2}(t - 4)}\right)u_4(t)
				</mrow>
			</md>
		</paragraphs>

	</subsection>

	<subsection><title> Worked Example 3 </title>

		<p>
			Solve the following differential equation:
			<me>
				\frac{d^2y}{dt^2} - 4\frac{dy}{dt} - 5y =
				\left\{
				\begin{array}{cl}
					e^{-t},	\amp 0 \le t \lt 1 \\
					1,	\amp t \ge 1
				\end{array}
				\right.
			</me>
			with initial conditions: <m>y(0) = 0</m> and <m>y'(0) = 0</m>.
		</p>

		<paragraphs><title>Step 1: Apply the Laplace Transform</title>
			<p>
				To take the transform of both sides of this equation, we first need to rewrite the piecewise forcing function using unit step functions:
				<me>
					\left\{
					\begin{array}{cl}
						e^{-t},	\amp 0 \le t \lt 1 \\
						1,	\amp t \ge 1
					\end{array}
					\right. \quad\rightarrow\quad
					e^{-t} \big(u_0(t) - u_1(t)\big) + 1 \cdot u_1(t)
				</me>
				Separating the <m>u_0</m> and <m>u_1</m> terms, the differential equation becomes:
				<me>
					\frac{d^2y}{dt^2} - 4\frac{dy}{dt} - 5y = e^{-t}u_0(t) + (1 - e^{-t})u_1(t)
				</me>
			</p>

			<p>
				Applying the Laplace transform to both sides gives:
				<me>
					\lap{y''} - 4\lap{y'} - 5\lap{y} = \lap{e^{-t}u_0(t)} + \lap{(1 - e^{-t})u_1(t)}
				</me>
			</p>

			<p>
				Using rules <xref ref="L9-eqn" text="custom"><m>L_{9}</m></xref> and <xref ref="L10-eqn" text="custom"><m>L_{10}</m></xref> on the left, and <xref ref="L14-eqn" text="custom"><m>L_{14}</m></xref> on the right, we have:
			</p>

			<md>
				<mrow>
					s^2Y(s) - 4sY(s) - 5Y(s) \amp
					= \lap{e^{-t}} + \lap{(1 - e^{-t})}e^{-s}
				</mrow>
			</md>

			<p>
				and the rules <xref ref="L1-eqn" text="custom"><m>L_{1}</m></xref> and <xref ref="L2-eqn" text="custom"><m>L_{2}</m></xref> give the transformed equation:
			</p>

			<me>
				s^2Y(s) - 4sY(s) - 5Y(s) =
				\frac{1}{s + 1} + \left(\frac{1}{s} - \frac{1}{s + 1}\right)e^{-s}
			</me>
		</paragraphs>

		<paragraphs><title>Step 2: Solve for <m>Y(s)</m> and Separate the Rational Parts </title>
			<p>
				Using a bit of algebra to isolate <m>Y(s)</m> yields the Laplace solution:
				<me>
					Y(s) 
					= \frac{1}{s^2 - 4s - 5} 
					\left[
						\frac{1}{s + 1} + \left(\frac{1}{s} - \frac{1}{s + 1}\right)e^{-s}
					\right]
				</me>
			</p>

			<p>
				Factoring <m>s^2 - 4s - 5</m> and combining the fractions next to <m>e^{-s}</m> gives:
			</p>

			<me>
				Y(s) 
				= \frac{1}{(s + 1)(s - 5)} 
				\left[
					\frac{1}{s + 1} + \frac{1}{s(s + 1)}e^{-s}
				\right]
			</me>
			
			<p>
				Then we distribute and label the rational parts, <m>F_i(s)</m>:
				<md>
					<mrow>
						Y(s) =
						\ub{\frac{1}{(s + 1)^2(s - 5)}}_{\large F_1(s)}
						+ \ub{\frac{1}{s(s + 1)^2(s - 5)}}_{\large F_2(s)} e^{-s}
					</mrow>
				</md>
			</p>

			<p>
				With this, the Laplace solution is now:
			</p>

			<me>
				Y(s) = F_1(s) + F_2(s)e^{-s}
			</me>
		</paragraphs>

		<paragraphs><title>Step 3: Prepare <m>Y(s)</m> for an Inverse Transform</title>

			<p>
				The partial fraction decomposition of <m>F_1</m> and <m>F_2</m> are given by:			
			</p>

			<ul marker="square">
				<li>
					<m>
						\ds F_1(s) = \frac{-\frac{1}{36}}{s + 1} - \frac{\frac{1}{6}}{(s + 1)^2} + \frac{\frac{1}{36}}{s - 5}
					</m>
				</li>
				<li>
					<m>
						\ds F_2(s) = \frac{-\frac{1}{5}}{s} + \frac{\frac{1}{6}}{s + 1} + \frac{\frac{2}{9}}{(s + 1)^2} + \frac{\frac{1}{180}}{s - 5}
					</m>
				</li>
			</ul>		

			<solution><title> Full Partial Fraction Decomposition Details of <m>F_2(s)</m> and <m>F_3(s)</m> </title>
				<p>
						For <m>F_1(s)</m>, the general form is:
						<me>
							\frac{1}{(s + 1)^2(s - 5)} = \frac{A}{s + 1} + \frac{B}{(s + 1)^2} + \frac{C}{s - 5}
						</me>
				</p>

				<p>
					Multiplying through:
					<md>
						<mrow> 1 \amp = A(s + 1)(s - 5) + B(s - 5) + C(s + 1)^2</mrow> 
					</md>
				</p>

				<p>
					Selecting values of <m>s</m> finds <m>A</m>, <m>B</m>, and <m>C</m>:
					<tabular>
						<col width="15%" halign="right"/>
						<col width="40%" halign="left"/>
						<col width="15%" halign="center"/>
						<col width="30%" halign="center"/>
						<row>
							<cell><p><m>s = -1:</m></p></cell>
							<cell><p><m>1 = A(0) + B(-6) + C(0)</m></p></cell>
							<cell><p><m>\implies</m></p></cell>
							<cell><p><m>B = -\frac16</m></p></cell>
						</row>
						<row>
							<cell><p><m>s = 5:</m></p></cell>
							<cell><p><m>1 = A(0) + B(0) + C(36)</m></p></cell>
							<cell><p><m>\implies</m></p></cell>
							<cell><p><m>C = \frac{1}{36}</m></p></cell>
						</row>
						<row>
							<cell><p><m>s = 0:</m></p></cell>
							<cell><p><m>1 = A(-5) + B(-5) + C(1)</m></p></cell>
							<cell><p><m>\implies</m></p></cell>
							<cell><p><m>1 = -5A + \frac56 + \frac{1}{36}</m></p></cell>
						</row>
						<row>
							<cell/>
							<cell/>
							<cell/>
							<cell><p><m> A = -\frac{1}{36}</m></p></cell>
						</row>
					</tabular>
				</p>

				<p>
					With these constants, we can write <m>F_1</m> as:
				</p>

				<me>
					F_1(s) = \frac{-\frac{1}{36}}{s + 1} - \frac{\frac{1}{6}}{(s + 1)^2} + \frac{\frac{1}{36}}{s - 5}
				</me>

				<p>
					Now, for <m>F_2(s)</m>, we have:
					<me>
						F_2(s) = \frac{1}{s(s + 1)^2(s - 5)} = \frac{A}{s} + \frac{B}{s + 1} + \frac{C}{(s + 1)^2} + \frac{D}{s - 5}
					</me>
				</p>

				<p>
					Multiplying through:
					<md>
						<mrow> 1 \amp = A(s + 1)^2(s - 5) + Bs(s + 1)(s - 5) + Cs(s - 5) + Ds(s + 1)^2</mrow> 
					</md>
				</p>

				<p>
					Selecting values of <m>s</m> finds <m>A</m>, <m>B</m>, <m>C</m>, and <m>D</m>:
					<tabular>
						<col width="10%" halign="right"/>
						<col width="44%" halign="left"/>
						<col width="10%" halign="center"/>
						<col width="36%" halign="center"/>
						<row>
							<cell><m>s = 0:</m></cell>
							<cell><m>1 = A(-5) + B(0) + C(0) + D(0)</m></cell>
							<cell><m>\implies</m></cell>
							<cell><m>A = -\frac{1}{5}</m></cell>
						</row>
						<row>
							<cell><m>s = -1:</m></cell>
							<cell><m>1 = A(0) + B(6) + C(0) + D(0)</m></cell>
							<cell><m>\implies</m></cell>
							<cell><m>B = \frac{1}{6}</m></cell>
						</row>
						<row>
							<cell><m>s = 5:</m></cell>
							<cell><m>1 = A(0) + B(0) + C(0) + D(180)</m></cell>
							<cell><m>\implies</m></cell>
							<cell><m>D = \frac{1}{180}</m></cell>
						</row>
						<row>
							<cell><m>s = 1:</m></cell>
							<cell><m>1 = A(-16) + B(-8) + C(-4) + D(4)</m></cell>
							<cell/>
							<cell/>
						</row>
					</tabular>
				</p>

				<p>
					To find <m>C</m>, we plug in the values of <m>A</m>, <m>B</m>, and <m>D</m>:
					<me>
						1 = \frac{16}{5} - \frac{4}{3} + C(-4) + \frac{1}{45} \implies
						C = \frac{2}{9}
					</me>
				</p>

				<p>
					With these constants, we can write <m>F_2</m> as:
				</p>

				<me>
					F_2(s) = \frac{-\frac{1}{5}}{s} + \frac{\frac{1}{6}}{s + 1} + \frac{\frac{2}{9}}{(s + 1)^2} + \frac{\frac{1}{180}}{s - 5}
				</me>
			</solution>
		</paragraphs>

		<paragraphs><title>Step 4: Invert <m>Y(s)</m> to Recover <m>y(t)</m></title>
			<p>
				Applying the inverse transform to each term of the Laplace Solution, <m>Y(s)</m>, we get
				<me>
					y(t) = \ilap{F_1(s)} + \ilap{F_2(s)e^{-s}}
				</me>
			</p>

			<p>
				Then using <xref ref="L15-eqn" text="custom"><m>L_{15}</m></xref>, we have
				<me>
					y(t) = f_1(t) + f_2(t - 1)u_1(t)
				</me>
			</p>

			<p>
				where
				<md>
					<mrow>
						f_1(t) \amp = \ilap{F_1(s)} = -\frac{1}{36}e^{-t} - \frac{1}{6}te^{-t} + \frac{1}{36}e^{5t}
					</mrow>
					<mrow>
						f_2(t) \amp = \ilap{F_2(s)} = -\frac{1}{5} + \frac{1}{6}e^{-t} + \frac{2}{9}te^{-t} + \frac{1}{180}e^{5t}
					</mrow>
				</md>
			</p>

			<p>
				Thus, the final solution is:
				<md>
					<mrow>
						y(t) =
						- \frac{1}{36}e^{-t} 
						\amp
						- \frac{1}{6}te^{-t} 
						+ \frac{1}{36}e^{5t} 
					</mrow>
					<mrow>
						\amp 
						+ \left(
							- \frac{1}{5}
							+ \frac{1}{6}e^{-(t - 1)}
							+ \frac{2}{9}(t - 1)e^{-(t - 1)}
							+ \frac{1}{180}e^{5(t - 1)}
						\right) u_1(t)
					</mrow>
				</md>
			</p>

			<p>
				This completes the setup and form of the solution. In a more advanced course, we would proceed to compute the inverse transforms explicitly using convolution or known transform pairs.
			</p>
		</paragraphs>

	</subsection>
</section>