<section><title> TEMPORARY REFERENCES </title>				
                
 		<p>               
                <md>
					<mrow xml:id="lt-L2">
						\text{L}_2:\quad\lap{e^{at}} = \frac{1}{s - a}, \quad s \gt a
					</mrow>.
		       	<mrow xml:id="lt-L10">
						\text{L}_{10}:\quad\lap{f(t) u_c(t)} = e^{-cs} \lap{f(t + c)}
					</mrow>.
                    					<mrow xml:id="lt-L11">
						\text{L}_{11}:\quad\lap{f(t-c) u_c(t)} = e^{-cs} F(s), \quad\text{where}\quad F(s) = \lap{f(t)}
					</mrow>.

                    					<mrow xml:id="lt-L9">
						\text{L}_9:\quad\lap{u_c(t)} = \frac{e^{-cs}}{s}, \qquad s \gt 0.
					</mrow>
				</md>
         </p>
		<p>
<assemblage xml:id="lt-roadmap-full">
			<title> Laplace Method Roadmap </title>
			<p>
				<sidebyside widths="32% 18% 42%" valign="middle">
					<p>
						<me>\ul{\quad\ \textbf{Original Domain}\ \quad}</me>
					</p>
					<p/>
					<p>
						<me>\DLBa\textbf{2Ô∏è‚É£  Laplace Domain}</me>
					</p>
				</sidebyside>
				<sidebyside widths="31% 18% 43%" valign="top">
					<p>
						<md>
							<mrow>\os{\vphantom{m}}{y'' - 9y = 10e^{2t}}</mrow>
							<mrow>y(0) = 1,\quad y'(0) = -7</mrow>
							<mrow>\os{\large üî∫ üî∫ üî∫ üî∫ üî∫}{\text{Differential Equation}}</mrow>
							<mrow/>
							<mrow/>
							<mrow>\us{\large üîª üîª üîª üîª üîª}{\text{Solution}}</mrow>
							<mrow> y = e^{3t} + 2e^{-3t} - 2e^{2t}</mrow>
						</md>
					</p>
					<p>
						<md>
							<mrow>\underrightarrow{\text{1Ô∏è‚É£ Forward}}</mrow>
							<mrow>\text{Apply}\ \laplacesym</mrow>
							<mrow/>
							<mrow/>
							<mrow/>
							<mrow/>
							<mrow>\text{Apply}\ \laplacesym^{-1}</mrow>
							<mrow>\overleftarrow{\text{3Ô∏è‚É£ Backward}}</mrow>
						</md>
					</p>
					<p>
						<assemblage>
							<p>
								<md>
									<mrow>\amp\DLBa s^2Y - 9Y - s + 7 = \frac{10}{s - 2}</mrow>
									<mrow>\amp\qquad\qquad {\Big\downarrow}\quad\text{Solve for}\ Y</mrow>
									<mrow>\amp\DLBa Y = \frac{1}{s^2 - 9}\left( \frac{10}{s - 2} + s - 7 \right)</mrow>
									<mrow>\amp\qquad\qquad {\Big\downarrow}\ \ \text{Prepare for Inverse}</mrow>
									<mrow>\amp\DLBa Y = \frac{1}{s - 3} + \frac{2}{s + 3} - \frac{2}{s - 2}</mrow>
								</md>
							</p>
						</assemblage>
					</p>
				</sidebyside>
			</p>
		</assemblage>
		</p>
		<p>
<assemblage xml:id="piecewise-to-unit-step">
			<title>üìú Converting Piecewise Form to Unit Step Form </title>
			<p>
				Here's a strategy for converting any piecewise function into step form:
				<ul marker="disc">
					<li>Find the intervals where each piece is active.</li>
					<li>
						Match the active interval for each piece to its step function switch:
						<tabular halign="center">
							<col right="minor"/>
							<col right="minor"/>
							<row bottom="minor"> <cell>Piece</cell> <cell>Active Interval</cell> <cell>Step Function Switch</cell> </row>
							<row> <cell><me>P(t)</me></cell> <cell><me>t \lt c		 </me></cell> <cell><me>1 - u_c(t)		</me></cell> </row>
							<row> <cell><me>Q(t)</me></cell> <cell><me>c \le t \lt d </me></cell> <cell><me>u_c(t) - u_d(t)	</me></cell> </row>
							<row> <cell><me>R(t)</me></cell> <cell><me>t \ge d		 </me></cell> <cell><me>u_d(t)			</me></cell> </row>
						</tabular>
					</li>
					<li>Multiply the piece by its switch, then add them all together.</li>
				</ul>
			</p>
		</assemblage>
		</p>
		<p>

<assemblage xml:id="laplace-ftc-uc"><title> Laplace Transform of <m>f(t - c)\cdot u_c(t)</m> </title>
					<p>
						When the function, <m>f(t)</m>, is also shifted by <m>c</m>, we get the Laplace transform
						<men xml:id="L15-eqn">
							\lap{f(t - c) \, u_c(t)} = e^{-cs} F(s), \quad\text{where}\quad F(s) = \lap{f(t)}
						</men>.
					</p>

					<p>
						<theorem><title> <m>\rightarrow \lap{f(t - c) \, u_c(t)}</m> </title>
							<p>
								To prove this, we start with the definition of the Laplace transform:
								<me>
									\lap{f(t - c) \cdot u_c(t)} = \int_0^\infty f(t - c) \cdot u_c(t) \cdot e^{-st} \, dt.
								</me>
							</p>

							<p>
								Since <m>u_c(t) = 0</m> for <m>t \lt c</m>, we can change the limits of integration to <m>c\le t\le\infty</m>.
							</p>

							<p>
								Using a <m>u</m>-substitution, we let <m>u = t - c</m>, so <m>t = u + c</m> and <m>dt = du</m>. The limits change to <m>u = 0</m> and <m>u \to \infty</m>.
							</p>

							<md>
								<mrow>
									\int_{t=c}^{t=\infty} f(t - c) e^{-st} \, dt 
									\amp = \int_{u=0}^{u=\infty} f(u) e^{-s(u + c)} \, du
								</mrow>
								<mrow>
									\amp = e^{-cs} \int_0^\infty f(u) e^{-su} \, du
								</mrow>
								<mrow>
									\amp = e^{-cs} \lap{f(t)} = e^{-cs} F(s)
								</mrow>
							</md>

							<p>
								This proves that the rule holds.
							</p>
						</theorem>
					</p>
				</assemblage>
		</p>
		<p>
			<md>
				<mrow xml:id="lt-R1">
					\text{R}_{1}:\quad
					\amp \lap{f'(t)} = sF(s) - f(0),
					\amp\amp s \gt 0
				</mrow>
				<mrow xml:id="lt-R2">
					\text{R}_{2}:\quad
					\amp \lap{f''(t)} = s^2F(s) - sf(0) - f'(0),
					\amp\amp s \gt 0
				</mrow>
				<mrow xml:id="lt-R3">
					\text{R}_{3}:\quad
					\amp \lap{f'''(t)} = s^3F(s) - s^2f(0) - sf'(0) - f''(0),
					\amp\amp s \gt 0
				</mrow>
			</md>
		</p>
</section>